@prefix : <https://w3id.org/netbeheer/IECCIM/TC57CIM/IEC62325/InfIEC62325/InfEnergyScheduling#> .
@prefix owl: <http://www.w3.org/2002/07/owl#> .
@prefix rdf: <http://www.w3.org/1999/02/22-rdf-syntax-ns#> .
@prefix xml: <http://www.w3.org/XML/1998/namespace> .
@prefix xsd: <http://www.w3.org/2001/XMLSchema#> .
@prefix rdfs: <http://www.w3.org/2000/01/rdf-schema#> .
@base <https://w3id.org/netbeheer/IECCIM/TC57CIM/IEC62325/InfIEC62325/InfEnergyScheduling#> .

<https://w3id.org/netbeheer/IECCIM/TC57CIM/IEC62325/InfIEC62325/InfEnergyScheduling#> rdf:type owl:Ontology .

#################################################################
#    Object Properties
#################################################################

###  https://w3id.org/netbeheer/IECCIM/TC57CIM/IEC62325/InfIEC62325/InfEnergyScheduling#AreaReserveSpec_lowerRegMarginReqt
:AreaReserveSpec_lowerRegMarginReqt rdf:type owl:ObjectProperty ;
                                    rdfs:domain :AreaReserveSpec ;
                                    rdfs:range <https://w3id.org/netbeheer/IECCIM/TC57CIM/IEC61970/Base/Domain#ActivePower> ;
                                    rdfs:comment """Lower regulating margin requirement in MW, the amount of generation that can be dropped by control in 10 minutes
""" .


###  https://w3id.org/netbeheer/IECCIM/TC57CIM/IEC62325/InfIEC62325/InfEnergyScheduling#AreaReserveSpec_opReserveReqt
:AreaReserveSpec_opReserveReqt rdf:type owl:ObjectProperty ;
                               rdfs:domain :AreaReserveSpec ;
                               rdfs:range <https://w3id.org/netbeheer/IECCIM/TC57CIM/IEC61970/Base/Domain#ActivePower> ;
                               rdfs:comment """Operating reserve requirement in MW, where operating reserve is the generating capability that is fully available within 30 minutes. Operating reserve is composed of primary reserve (t less than 10 min) and secondary reserve (10 less than t less than 30 min).
""" .


###  https://w3id.org/netbeheer/IECCIM/TC57CIM/IEC62325/InfIEC62325/InfEnergyScheduling#AreaReserveSpec_primaryReserveReqt
:AreaReserveSpec_primaryReserveReqt rdf:type owl:ObjectProperty ;
                                    rdfs:domain :AreaReserveSpec ;
                                    rdfs:range <https://w3id.org/netbeheer/IECCIM/TC57CIM/IEC61970/Base/Domain#ActivePower> ;
                                    rdfs:comment """Primary reserve requirement in MW, where primary reserve is generating capability that is fully available within 10 minutes. Primary reserve is composed of spinning reserve and quick-start reserve.
""" .


###  https://w3id.org/netbeheer/IECCIM/TC57CIM/IEC62325/InfIEC62325/InfEnergyScheduling#AreaReserveSpec_raiseRegMarginReqt
:AreaReserveSpec_raiseRegMarginReqt rdf:type owl:ObjectProperty ;
                                    rdfs:domain :AreaReserveSpec ;
                                    rdfs:range <https://w3id.org/netbeheer/IECCIM/TC57CIM/IEC61970/Base/Domain#ActivePower> ;
                                    rdfs:comment """Raise regulating margin requirement in MW, the amount of generation that can be picked up by control in 10 minutes
""" .


###  https://w3id.org/netbeheer/IECCIM/TC57CIM/IEC62325/InfIEC62325/InfEnergyScheduling#AreaReserveSpec_spinningReserveReqt
:AreaReserveSpec_spinningReserveReqt rdf:type owl:ObjectProperty ;
                                     rdfs:domain :AreaReserveSpec ;
                                     rdfs:range <https://w3id.org/netbeheer/IECCIM/TC57CIM/IEC61970/Base/Domain#ActivePower> ;
                                     rdfs:comment """Spinning reserve requirement in MW, spinning reserve is generating capability that is presently synchronized to the network and is fully available within 10 minutes
""" .


###  https://w3id.org/netbeheer/IECCIM/TC57CIM/IEC62325/InfIEC62325/InfEnergyScheduling#ControlAreaOperator_CAChildOf
:ControlAreaOperator_CAChildOf rdf:type owl:ObjectProperty ;
                               rdfs:domain <https://w3id.org/netbeheer/IECCIM/TC57CIM/IEC62325/InfIEC62325/InfFinancial#ControlAreaOperator> ;
                               rdfs:range :TieLine ;
                               rdfs:comment "A ControlAreaOperator has a collection of tie points that ring the ControlArea, called a TieLine.A ControlAreaOperator has a collection of tie points that ring the ControlArea, called a TieLine." .


###  https://w3id.org/netbeheer/IECCIM/TC57CIM/IEC62325/InfIEC62325/InfEnergyScheduling#CurrentEmergencyScheduledInterchange_InternalControlArea
:CurrentEmergencyScheduledInterchange_InternalControlArea rdf:type owl:ObjectProperty ;
                                                          rdfs:domain :CurrentEmergencyScheduledInterchange ;
                                                          rdfs:range :InternalControlArea ;
                                                          rdfs:comment "" .


###  https://w3id.org/netbeheer/IECCIM/TC57CIM/IEC62325/InfIEC62325/InfEnergyScheduling#CurrentScheduledInterchange_InternalControlArea
:CurrentScheduledInterchange_InternalControlArea rdf:type owl:ObjectProperty ;
                                                 rdfs:domain :CurrentScheduledInterchange ;
                                                 rdfs:range :InternalControlArea ;
                                                 rdfs:comment "" .


###  https://w3id.org/netbeheer/IECCIM/TC57CIM/IEC62325/InfIEC62325/InfEnergyScheduling#CustomerConsumer_CustChildOf
:CustomerConsumer_CustChildOf rdf:type owl:ObjectProperty ;
                              rdfs:domain <https://w3id.org/netbeheer/IECCIM/TC57CIM/IEC62325/InfIEC62325/InfFinancial#CustomerConsumer> ;
                              rdfs:range :TieLine ;
                              rdfs:comment "A CustomerConsumer may ring its perimeter with metering, which can create a unique SubControlArea at the collection of metering points, called a TieLine.A  ControlAreaOperator or CustomerConsumer may ring their perimeter with metering, which can create a unique SubControlArea at the collection of metering points, called a TieLine." .


###  https://w3id.org/netbeheer/IECCIM/TC57CIM/IEC62325/InfIEC62325/InfEnergyScheduling#EnergyProduct_GenerationProvider
:EnergyProduct_GenerationProvider rdf:type owl:ObjectProperty ;
                                  rdfs:domain :EnergyProduct ;
                                  rdfs:range <https://w3id.org/netbeheer/IECCIM/TC57CIM/IEC62325/InfIEC62325/InfFinancial#GenerationProvider> ;
                                  rdfs:comment "" .


###  https://w3id.org/netbeheer/IECCIM/TC57CIM/IEC62325/InfIEC62325/InfEnergyScheduling#EnergyProduct_ResoldBy_Marketer
:EnergyProduct_ResoldBy_Marketer rdf:type owl:ObjectProperty ;
                                 rdfs:domain :EnergyProduct ;
                                 rdfs:range <https://w3id.org/netbeheer/IECCIM/TC57CIM/IEC62325/InfIEC62325/InfFinancial#Marketer> ;
                                 rdfs:comment "A Marketer may resell an EnergyProduct.A Marketer may resell an EnergyProduct." .


###  https://w3id.org/netbeheer/IECCIM/TC57CIM/IEC62325/InfIEC62325/InfEnergyScheduling#EnergyProduct_TitleHeldBy_Marketer
:EnergyProduct_TitleHeldBy_Marketer rdf:type owl:ObjectProperty ;
                                    rdfs:domain :EnergyProduct ;
                                    rdfs:range <https://w3id.org/netbeheer/IECCIM/TC57CIM/IEC62325/InfIEC62325/InfFinancial#Marketer> ;
                                    rdfs:comment "A Marketer holds title to an EnergyProduct.A Marketer holds title to an EnergyProduct." .


###  https://w3id.org/netbeheer/IECCIM/TC57CIM/IEC62325/InfIEC62325/InfEnergyScheduling#GenerationProvider_ProvidedBy
:GenerationProvider_ProvidedBy rdf:type owl:ObjectProperty ;
                               owl:inverseOf :EnergyProduct_GenerationProvider ;
                               rdf:type owl:FunctionalProperty ;
                               rdfs:domain <https://w3id.org/netbeheer/IECCIM/TC57CIM/IEC62325/InfIEC62325/InfFinancial#GenerationProvider> ;
                               rdfs:range :EnergyProduct ;
                               rdfs:comment "" .


###  https://w3id.org/netbeheer/IECCIM/TC57CIM/IEC62325/InfIEC62325/InfEnergyScheduling#InternalControlArea_CurrentEmergencySI
:InternalControlArea_CurrentEmergencySI rdf:type owl:ObjectProperty ;
                                        owl:inverseOf :CurrentEmergencyScheduledInterchange_InternalControlArea ;
                                        rdf:type owl:FunctionalProperty ;
                                        rdfs:domain :InternalControlArea ;
                                        rdfs:range :CurrentEmergencyScheduledInterchange ;
                                        rdfs:comment "" .


###  https://w3id.org/netbeheer/IECCIM/TC57CIM/IEC62325/InfIEC62325/InfEnergyScheduling#InternalControlArea_CurrentScheduledInterchange
:InternalControlArea_CurrentScheduledInterchange rdf:type owl:ObjectProperty ;
                                                 owl:inverseOf :CurrentScheduledInterchange_InternalControlArea ;
                                                 rdf:type owl:FunctionalProperty ;
                                                 rdfs:domain :InternalControlArea ;
                                                 rdfs:range :CurrentScheduledInterchange ;
                                                 rdfs:comment "" .


###  https://w3id.org/netbeheer/IECCIM/TC57CIM/IEC62325/InfIEC62325/InfEnergyScheduling#LossProfile_HasLoss_
:LossProfile_HasLoss_ rdf:type owl:ObjectProperty ;
                      rdfs:domain :LossProfile ;
                      rdfs:range <https://w3id.org/netbeheer/IECCIM/TC57CIM/IEC62325/InfIEC62325/InfFinancial#TransmissionProvider> ;
                      rdfs:comment "Part of the LossProfile for an EnergyTransaction may be a loss for a TransmissionProvider. If so, the TransmissionProvider must be one of the participating entities in the EnergyTransaction.Part of the LossProfile for an EnergyTransaction may be a loss for a TransmissionProvider. If so, the TransmissionProvider must be one of the participating entities in the EnergyTransaction." .


###  https://w3id.org/netbeheer/IECCIM/TC57CIM/IEC62325/InfIEC62325/InfEnergyScheduling#Marketer_HoldsTitleTo_EnergyProducts
:Marketer_HoldsTitleTo_EnergyProducts rdf:type owl:ObjectProperty ;
                                      owl:inverseOf :EnergyProduct_TitleHeldBy_Marketer ;
                                      rdfs:domain <https://w3id.org/netbeheer/IECCIM/TC57CIM/IEC62325/InfIEC62325/InfFinancial#Marketer> ;
                                      rdfs:range :EnergyProduct ;
                                      rdfs:comment "A Marketer holds title to an EnergyProduct.A Marketer holds title to an EnergyProduct." .


###  https://w3id.org/netbeheer/IECCIM/TC57CIM/IEC62325/InfIEC62325/InfEnergyScheduling#Marketer_Resells_EnergyProduct
:Marketer_Resells_EnergyProduct rdf:type owl:ObjectProperty ;
                                owl:inverseOf :EnergyProduct_ResoldBy_Marketer ;
                                rdfs:domain <https://w3id.org/netbeheer/IECCIM/TC57CIM/IEC62325/InfIEC62325/InfFinancial#Marketer> ;
                                rdfs:range :EnergyProduct ;
                                rdfs:comment "A Marketer may resell an EnergyProduct.A Marketer may resell an EnergyProduct." .


###  https://w3id.org/netbeheer/IECCIM/TC57CIM/IEC62325/InfIEC62325/InfEnergyScheduling#TieLine_ParentOfA
:TieLine_ParentOfA rdf:type owl:ObjectProperty ;
                   owl:inverseOf :ControlAreaOperator_CAChildOf ;
                   rdfs:domain :TieLine ;
                   rdfs:range <https://w3id.org/netbeheer/IECCIM/TC57CIM/IEC62325/InfIEC62325/InfFinancial#ControlAreaOperator> ;
                   rdfs:comment "A ControlAreaOperator has a collection of tie points that ring the ControlArea, called a TieLine.A ControlAreaOperator has a collection of tie points that ring the ControlArea, called a TieLine." .


###  https://w3id.org/netbeheer/IECCIM/TC57CIM/IEC62325/InfIEC62325/InfEnergyScheduling#TieLine_ParentOfB
:TieLine_ParentOfB rdf:type owl:ObjectProperty ;
                   owl:inverseOf :CustomerConsumer_CustChildOf ;
                   rdfs:domain :TieLine ;
                   rdfs:range <https://w3id.org/netbeheer/IECCIM/TC57CIM/IEC62325/InfIEC62325/InfFinancial#CustomerConsumer> ;
                   rdfs:comment "A CustomerConsumer may ring its perimeter with metering, which can create a unique SubControlArea at the collection of metering points, called a TieLine.A  ControlAreaOperator or CustomerConsumer may ring their perimeter with metering, which can create a unique SubControlArea at the collection of metering points, called a TieLine." .


###  https://w3id.org/netbeheer/IECCIM/TC57CIM/IEC62325/InfIEC62325/InfEnergyScheduling#TransmissionCorridor_TransmissionRightOfWays
:TransmissionCorridor_TransmissionRightOfWays rdf:type owl:ObjectProperty ,
                                                       owl:FunctionalProperty ;
                                              rdfs:domain :TransmissionCorridor ;
                                              rdfs:range :TransmissionRightOfWay ;
                                              rdfs:comment "A transmission right-of-way is a member of a transmission corridorA transmission right-of-way is a member of a transmission corridor" .


###  https://w3id.org/netbeheer/IECCIM/TC57CIM/IEC62325/InfIEC62325/InfEnergyScheduling#TransmissionProvider_For
:TransmissionProvider_For rdf:type owl:ObjectProperty ;
                          owl:inverseOf :LossProfile_HasLoss_ ;
                          rdfs:domain <https://w3id.org/netbeheer/IECCIM/TC57CIM/IEC62325/InfIEC62325/InfFinancial#TransmissionProvider> ;
                          rdfs:range :LossProfile ;
                          rdfs:comment "Part of the LossProfile for an EnergyTransaction may be a loss for a TransmissionProvider. If so, the TransmissionProvider must be one of the participating entities in the EnergyTransaction.Part of the LossProfile for an EnergyTransaction may be a loss for a TransmissionProvider. If so, the TransmissionProvider must be one of the participating entities in the EnergyTransaction." .


###  https://w3id.org/netbeheer/IECCIM/TC57CIM/IEC62325/InfIEC62325/InfEnergyScheduling#TransmissionRightOfWay_TransmissionCorridor
:TransmissionRightOfWay_TransmissionCorridor rdf:type owl:ObjectProperty ;
                                             owl:inverseOf :TransmissionCorridor_TransmissionRightOfWays ;
                                             rdfs:domain :TransmissionRightOfWay ;
                                             rdfs:range :TransmissionCorridor ;
                                             rdfs:comment "A transmission right-of-way is a member of a transmission corridorA transmission right-of-way is a member of a transmission corridor" .


#################################################################
#    Data properties
#################################################################

###  https://w3id.org/netbeheer/IECCIM/TC57CIM/IEC62325/InfIEC62325/InfEnergyScheduling#AreaReserveSpec_Description
:AreaReserveSpec_Description rdf:type owl:DatatypeProperty ;
                             rdfs:domain :AreaReserveSpec ;
                             rdfs:range xsd:string ;
                             rdfs:comment """Description of the object or instance.
""" .


###  https://w3id.org/netbeheer/IECCIM/TC57CIM/IEC62325/InfIEC62325/InfEnergyScheduling#CurrentEmergencyScheduledInterchange_emergencyScheduleMW
:CurrentEmergencyScheduledInterchange_emergencyScheduleMW rdf:type owl:DatatypeProperty ;
                                                          rdfs:domain :CurrentEmergencyScheduledInterchange ;
                                                          rdfs:range xsd:float ;
                                                          rdfs:comment """Net tie MW. These are three entries, the current emergency schedule interchange and the two future schedules if they exist.
""" .


###  https://w3id.org/netbeheer/IECCIM/TC57CIM/IEC62325/InfIEC62325/InfEnergyScheduling#CurrentEmergencyScheduledInterchange_emergencyScheduleRampTime
:CurrentEmergencyScheduledInterchange_emergencyScheduleRampTime rdf:type owl:DatatypeProperty ;
                                                                rdfs:domain :CurrentEmergencyScheduledInterchange ;
                                                                rdfs:range xsd:nonNegativeInteger ;
                                                                rdfs:comment """Ramp time, the ramping time for a schedule. This is calculated as the remaining time to ramp if a schedule is ramping. Measured in seconds, but can be negattive.
""" .


###  https://w3id.org/netbeheer/IECCIM/TC57CIM/IEC62325/InfIEC62325/InfEnergyScheduling#CurrentEmergencyScheduledInterchange_emergencyScheduleStartTime
:CurrentEmergencyScheduledInterchange_emergencyScheduleStartTime rdf:type owl:DatatypeProperty ;
                                                                 rdfs:domain :CurrentEmergencyScheduledInterchange ;
                                                                 rdfs:range xsd:dateTime ;
                                                                 rdfs:comment """Net tie time,  the start time for a schedule. This is calculated as the current time if a schedule is ramping.
""" .


###  https://w3id.org/netbeheer/IECCIM/TC57CIM/IEC62325/InfIEC62325/InfEnergyScheduling#CurrentScheduledInterchange_currentNetTieMW
:CurrentScheduledInterchange_currentNetTieMW rdf:type owl:DatatypeProperty ;
                                             rdfs:domain :CurrentScheduledInterchange ;
                                             rdfs:range xsd:float ;
                                             rdfs:comment """Current control area net tie MW (the sum of the tie line flows, i.e the sum of flows into and out of the control area), the current instantaneous scheduled interchange.
""" .


###  https://w3id.org/netbeheer/IECCIM/TC57CIM/IEC62325/InfIEC62325/InfEnergyScheduling#CurrentScheduledInterchange_useEmergencySchedule
:CurrentScheduledInterchange_useEmergencySchedule rdf:type owl:DatatypeProperty ;
                                                  rdfs:domain :CurrentScheduledInterchange ;
                                                  rdfs:range xsd:boolean ;
                                                  rdfs:comment """Use Emergency Schedule 
Attribute Usage: Emergency use indicator, false = Emergency Schedular OFF, true = Emergency Schedular ON.
""" .


###  https://w3id.org/netbeheer/IECCIM/TC57CIM/IEC62325/InfIEC62325/InfEnergyScheduling#DynamicSchedule_dynSchedSignRev
:DynamicSchedule_dynSchedSignRev rdf:type owl:DatatypeProperty ;
                                 rdfs:domain :DynamicSchedule ;
                                 rdfs:range xsd:boolean ;
                                 rdfs:comment """Dynamic schedule sign reversal required (true/false)
""" .


###  https://w3id.org/netbeheer/IECCIM/TC57CIM/IEC62325/InfIEC62325/InfEnergyScheduling#DynamicSchedule_dynSchedStatus
:DynamicSchedule_dynSchedStatus rdf:type owl:DatatypeProperty ;
                                rdfs:domain :DynamicSchedule ;
                                rdfs:range xsd:string ;
                                rdfs:comment """The \"active\" or \"inactive\" status of the dynamic schedule
""" .


#################################################################
#    Classes
#################################################################

###  https://w3id.org/netbeheer/IECCIM/TC57CIM/IEC61968/Common#Agreement
<https://w3id.org/netbeheer/IECCIM/TC57CIM/IEC61968/Common#Agreement> rdf:type owl:Class .


###  https://w3id.org/netbeheer/IECCIM/TC57CIM/IEC61970/Base/Core#BasicIntervalSchedule
<https://w3id.org/netbeheer/IECCIM/TC57CIM/IEC61970/Base/Core#BasicIntervalSchedule> rdf:type owl:Class .


###  https://w3id.org/netbeheer/IECCIM/TC57CIM/IEC61970/Base/Core#IdentifiedObject
<https://w3id.org/netbeheer/IECCIM/TC57CIM/IEC61970/Base/Core#IdentifiedObject> rdf:type owl:Class .


###  https://w3id.org/netbeheer/IECCIM/TC57CIM/IEC61970/Base/Core#PowerSystemResource
<https://w3id.org/netbeheer/IECCIM/TC57CIM/IEC61970/Base/Core#PowerSystemResource> rdf:type owl:Class .


###  https://w3id.org/netbeheer/IECCIM/TC57CIM/IEC61970/Base/Domain#ActivePower
<https://w3id.org/netbeheer/IECCIM/TC57CIM/IEC61970/Base/Domain#ActivePower> rdf:type owl:Class .


###  https://w3id.org/netbeheer/IECCIM/TC57CIM/IEC62325/InfIEC62325/InfEnergyScheduling#AreaReserveSpec
:AreaReserveSpec rdf:type owl:Class ;
                 rdfs:subClassOf [ rdf:type owl:Restriction ;
                                   owl:onProperty :AreaReserveSpec_lowerRegMarginReqt ;
                                   owl:minQualifiedCardinality "0"^^xsd:nonNegativeInteger ;
                                   owl:onClass <https://w3id.org/netbeheer/IECCIM/TC57CIM/IEC61970/Base/Domain#ActivePower>
                                 ] ,
                                 [ rdf:type owl:Restriction ;
                                   owl:onProperty :AreaReserveSpec_opReserveReqt ;
                                   owl:minQualifiedCardinality "0"^^xsd:nonNegativeInteger ;
                                   owl:onClass <https://w3id.org/netbeheer/IECCIM/TC57CIM/IEC61970/Base/Domain#ActivePower>
                                 ] ,
                                 [ rdf:type owl:Restriction ;
                                   owl:onProperty :AreaReserveSpec_primaryReserveReqt ;
                                   owl:minQualifiedCardinality "0"^^xsd:nonNegativeInteger ;
                                   owl:onClass <https://w3id.org/netbeheer/IECCIM/TC57CIM/IEC61970/Base/Domain#ActivePower>
                                 ] ,
                                 [ rdf:type owl:Restriction ;
                                   owl:onProperty :AreaReserveSpec_raiseRegMarginReqt ;
                                   owl:minQualifiedCardinality "0"^^xsd:nonNegativeInteger ;
                                   owl:onClass <https://w3id.org/netbeheer/IECCIM/TC57CIM/IEC61970/Base/Domain#ActivePower>
                                 ] ,
                                 [ rdf:type owl:Restriction ;
                                   owl:onProperty :AreaReserveSpec_spinningReserveReqt ;
                                   owl:minQualifiedCardinality "0"^^xsd:nonNegativeInteger ;
                                   owl:onClass <https://w3id.org/netbeheer/IECCIM/TC57CIM/IEC61970/Base/Domain#ActivePower>
                                 ] ,
                                 [ rdf:type owl:Restriction ;
                                   owl:onProperty :AreaReserveSpec_lowerRegMarginReqt ;
                                   owl:maxQualifiedCardinality "1"^^xsd:nonNegativeInteger ;
                                   owl:onClass <https://w3id.org/netbeheer/IECCIM/TC57CIM/IEC61970/Base/Domain#ActivePower>
                                 ] ,
                                 [ rdf:type owl:Restriction ;
                                   owl:onProperty :AreaReserveSpec_opReserveReqt ;
                                   owl:maxQualifiedCardinality "1"^^xsd:nonNegativeInteger ;
                                   owl:onClass <https://w3id.org/netbeheer/IECCIM/TC57CIM/IEC61970/Base/Domain#ActivePower>
                                 ] ,
                                 [ rdf:type owl:Restriction ;
                                   owl:onProperty :AreaReserveSpec_primaryReserveReqt ;
                                   owl:maxQualifiedCardinality "1"^^xsd:nonNegativeInteger ;
                                   owl:onClass <https://w3id.org/netbeheer/IECCIM/TC57CIM/IEC61970/Base/Domain#ActivePower>
                                 ] ,
                                 [ rdf:type owl:Restriction ;
                                   owl:onProperty :AreaReserveSpec_raiseRegMarginReqt ;
                                   owl:maxQualifiedCardinality "1"^^xsd:nonNegativeInteger ;
                                   owl:onClass <https://w3id.org/netbeheer/IECCIM/TC57CIM/IEC61970/Base/Domain#ActivePower>
                                 ] ,
                                 [ rdf:type owl:Restriction ;
                                   owl:onProperty :AreaReserveSpec_spinningReserveReqt ;
                                   owl:maxQualifiedCardinality "1"^^xsd:nonNegativeInteger ;
                                   owl:onClass <https://w3id.org/netbeheer/IECCIM/TC57CIM/IEC61970/Base/Domain#ActivePower>
                                 ] ,
                                 [ rdf:type owl:Restriction ;
                                   owl:onProperty :AreaReserveSpec_Description ;
                                   owl:minQualifiedCardinality "0"^^xsd:nonNegativeInteger ;
                                   owl:onDataRange xsd:string
                                 ] ,
                                 [ rdf:type owl:Restriction ;
                                   owl:onProperty :AreaReserveSpec_Description ;
                                   owl:maxQualifiedCardinality "1"^^xsd:nonNegativeInteger ;
                                   owl:onDataRange xsd:string
                                 ] ;
                 rdfs:comment """The control area's reserve specification.
""" .


###  https://w3id.org/netbeheer/IECCIM/TC57CIM/IEC62325/InfIEC62325/InfEnergyScheduling#CurrentEmergencyScheduledInterchange
:CurrentEmergencyScheduledInterchange rdf:type owl:Class ;
                                      rdfs:subClassOf <https://w3id.org/netbeheer/IECCIM/TC57CIM/IEC61970/Base/Core#IdentifiedObject> ,
                                                      [ rdf:type owl:Restriction ;
                                                        owl:onProperty :CurrentEmergencyScheduledInterchange_InternalControlArea ;
                                                        owl:minQualifiedCardinality "0"^^xsd:nonNegativeInteger ;
                                                        owl:onClass :CurrentEmergencyScheduledInterchange
                                                      ] ,
                                                      [ rdf:type owl:Restriction ;
                                                        owl:onProperty :CurrentEmergencyScheduledInterchange_emergencyScheduleMW ;
                                                        owl:minQualifiedCardinality "0"^^xsd:nonNegativeInteger ;
                                                        owl:onDataRange xsd:float
                                                      ] ,
                                                      [ rdf:type owl:Restriction ;
                                                        owl:onProperty :CurrentEmergencyScheduledInterchange_emergencyScheduleRampTime ;
                                                        owl:minQualifiedCardinality "0"^^xsd:nonNegativeInteger ;
                                                        owl:onDataRange xsd:nonNegativeInteger
                                                      ] ,
                                                      [ rdf:type owl:Restriction ;
                                                        owl:onProperty :CurrentEmergencyScheduledInterchange_emergencyScheduleStartTime ;
                                                        owl:minQualifiedCardinality "0"^^xsd:nonNegativeInteger ;
                                                        owl:onDataRange xsd:dateTime
                                                      ] ,
                                                      [ rdf:type owl:Restriction ;
                                                        owl:onProperty :CurrentEmergencyScheduledInterchange_emergencyScheduleMW ;
                                                        owl:maxQualifiedCardinality "1"^^xsd:nonNegativeInteger ;
                                                        owl:onDataRange xsd:float
                                                      ] ,
                                                      [ rdf:type owl:Restriction ;
                                                        owl:onProperty :CurrentEmergencyScheduledInterchange_emergencyScheduleRampTime ;
                                                        owl:maxQualifiedCardinality "1"^^xsd:nonNegativeInteger ;
                                                        owl:onDataRange xsd:nonNegativeInteger
                                                      ] ,
                                                      [ rdf:type owl:Restriction ;
                                                        owl:onProperty :CurrentEmergencyScheduledInterchange_emergencyScheduleStartTime ;
                                                        owl:maxQualifiedCardinality "1"^^xsd:nonNegativeInteger ;
                                                        owl:onDataRange xsd:dateTime
                                                      ] ;
                                      rdfs:comment """Control area emergency schedules
""" .


###  https://w3id.org/netbeheer/IECCIM/TC57CIM/IEC62325/InfIEC62325/InfEnergyScheduling#CurrentScheduledInterchange
:CurrentScheduledInterchange rdf:type owl:Class ;
                             rdfs:subClassOf [ rdf:type owl:Restriction ;
                                               owl:onProperty :CurrentScheduledInterchange_InternalControlArea ;
                                               owl:minQualifiedCardinality "0"^^xsd:nonNegativeInteger ;
                                               owl:onClass :CurrentScheduledInterchange
                                             ] ,
                                             [ rdf:type owl:Restriction ;
                                               owl:onProperty :CurrentScheduledInterchange_InternalControlArea ;
                                               owl:maxQualifiedCardinality "1"^^xsd:nonNegativeInteger ;
                                               owl:onClass :CurrentScheduledInterchange
                                             ] ,
                                             [ rdf:type owl:Restriction ;
                                               owl:onProperty :CurrentScheduledInterchange_currentNetTieMW ;
                                               owl:minQualifiedCardinality "0"^^xsd:nonNegativeInteger ;
                                               owl:onDataRange xsd:float
                                             ] ,
                                             [ rdf:type owl:Restriction ;
                                               owl:onProperty :CurrentScheduledInterchange_useEmergencySchedule ;
                                               owl:minQualifiedCardinality "0"^^xsd:nonNegativeInteger ;
                                               owl:onDataRange xsd:boolean
                                             ] ,
                                             [ rdf:type owl:Restriction ;
                                               owl:onProperty :CurrentScheduledInterchange_currentNetTieMW ;
                                               owl:maxQualifiedCardinality "1"^^xsd:nonNegativeInteger ;
                                               owl:onDataRange xsd:float
                                             ] ,
                                             [ rdf:type owl:Restriction ;
                                               owl:onProperty :CurrentScheduledInterchange_useEmergencySchedule ;
                                               owl:maxQualifiedCardinality "1"^^xsd:nonNegativeInteger ;
                                               owl:onDataRange xsd:boolean
                                             ] ;
                             rdfs:comment """Control area current net tie (scheduled interchange) sent to real time dispatch.
""" .


###  https://w3id.org/netbeheer/IECCIM/TC57CIM/IEC62325/InfIEC62325/InfEnergyScheduling#CurtailmentProfile
:CurtailmentProfile rdf:type owl:Class ;
                    rdfs:subClassOf <https://w3id.org/netbeheer/IECCIM/TC57CIM/IEC62325/MarketOperations/MarketSystem/ExternalInputs#Profile> ;
                    rdfs:comment """Curtailing entity must be providing at least one service to the EnergyTransaction. The CurtailmentProfile must be completely contained within the EnergyProfile timeframe for this EnergyTransaction.
""" .


###  https://w3id.org/netbeheer/IECCIM/TC57CIM/IEC62325/InfIEC62325/InfEnergyScheduling#DynamicSchedule
:DynamicSchedule rdf:type owl:Class ;
                 rdfs:subClassOf <https://w3id.org/netbeheer/IECCIM/TC57CIM/IEC61970/Base/Core#BasicIntervalSchedule> ,
                                 [ rdf:type owl:Restriction ;
                                   owl:onProperty :DynamicSchedule_dynSchedSignRev ;
                                   owl:minQualifiedCardinality "0"^^xsd:nonNegativeInteger ;
                                   owl:onDataRange xsd:boolean
                                 ] ,
                                 [ rdf:type owl:Restriction ;
                                   owl:onProperty :DynamicSchedule_dynSchedStatus ;
                                   owl:minQualifiedCardinality "0"^^xsd:nonNegativeInteger ;
                                   owl:onDataRange xsd:string
                                 ] ,
                                 [ rdf:type owl:Restriction ;
                                   owl:onProperty :DynamicSchedule_dynSchedSignRev ;
                                   owl:maxQualifiedCardinality "1"^^xsd:nonNegativeInteger ;
                                   owl:onDataRange xsd:boolean
                                 ] ,
                                 [ rdf:type owl:Restriction ;
                                   owl:onProperty :DynamicSchedule_dynSchedStatus ;
                                   owl:maxQualifiedCardinality "1"^^xsd:nonNegativeInteger ;
                                   owl:onDataRange xsd:string
                                 ] ;
                 rdfs:comment """A continuously variable component of a control area's MW net interchange schedule. Dynamic schedules are sent and received by control areas.
""" .


###  https://w3id.org/netbeheer/IECCIM/TC57CIM/IEC62325/InfIEC62325/InfEnergyScheduling#EnergyProduct
:EnergyProduct rdf:type owl:Class ;
               rdfs:subClassOf <https://w3id.org/netbeheer/IECCIM/TC57CIM/IEC61968/Common#Agreement> ,
                               [ rdf:type owl:Restriction ;
                                 owl:onProperty :EnergyProduct_GenerationProvider ;
                                 owl:minQualifiedCardinality "1"^^xsd:nonNegativeInteger ;
                                 owl:onClass :EnergyProduct
                               ] ,
                               [ rdf:type owl:Restriction ;
                                 owl:onProperty :EnergyProduct_ResoldBy_Marketer ;
                                 owl:minQualifiedCardinality "0"^^xsd:nonNegativeInteger ;
                                 owl:onClass :EnergyProduct
                               ] ,
                               [ rdf:type owl:Restriction ;
                                 owl:onProperty :EnergyProduct_TitleHeldBy_Marketer ;
                                 owl:minQualifiedCardinality "0"^^xsd:nonNegativeInteger ;
                                 owl:onClass :EnergyProduct
                               ] ;
               rdfs:comment """An EnergyProduct is offered commercially as a ContractOrTariff.
""" .


###  https://w3id.org/netbeheer/IECCIM/TC57CIM/IEC62325/InfIEC62325/InfEnergyScheduling#InadvertentAccount
:InadvertentAccount rdf:type owl:Class ;
                    rdfs:comment """An account for tracking inadvertent interchange versus time for each control area. A control area may have more than one inadvertent account in order to track inadvertent over one or more specific tie points in addition to the usual overall net inadvertent. Separate accounts would also be used to track designated time periods, such as on-peak and off-peak.
""" .


###  https://w3id.org/netbeheer/IECCIM/TC57CIM/IEC62325/InfIEC62325/InfEnergyScheduling#InternalControlArea
:InternalControlArea rdf:type owl:Class ;
                     rdfs:subClassOf <https://w3id.org/netbeheer/IECCIM/TC57CIM/IEC61970/Base/Core#IdentifiedObject> ,
                                     [ rdf:type owl:Restriction ;
                                       owl:onProperty :InternalControlArea_CurrentEmergencySI ;
                                       owl:qualifiedCardinality "1"^^xsd:nonNegativeInteger ;
                                       owl:onClass :InternalControlArea
                                     ] ,
                                     [ rdf:type owl:Restriction ;
                                       owl:onProperty :InternalControlArea_CurrentScheduledInterchange ;
                                       owl:qualifiedCardinality "1"^^xsd:nonNegativeInteger ;
                                       owl:onClass :InternalControlArea
                                     ] ;
                     rdfs:comment """There is one internal control area in the system, which is the single control area in the primary network company. Real time generation control affects only the internal control area.
""" .


###  https://w3id.org/netbeheer/IECCIM/TC57CIM/IEC62325/InfIEC62325/InfEnergyScheduling#LossProfile
:LossProfile rdf:type owl:Class ;
             rdfs:subClassOf <https://w3id.org/netbeheer/IECCIM/TC57CIM/IEC62325/MarketOperations/MarketSystem/ExternalInputs#Profile> ,
                             [ rdf:type owl:Restriction ;
                               owl:onProperty :LossProfile_HasLoss_ ;
                               owl:minQualifiedCardinality "0"^^xsd:nonNegativeInteger ;
                               owl:onClass :LossProfile
                             ] ;
             rdfs:comment """LossProfile is associated with an EnerrgyTransaction and must be completely contained within the time frame of the EnergyProfile associated with this EnergyTransaction.
""" .


###  https://w3id.org/netbeheer/IECCIM/TC57CIM/IEC62325/InfIEC62325/InfEnergyScheduling#TieLine
:TieLine rdf:type owl:Class ;
         rdfs:subClassOf <https://w3id.org/netbeheer/IECCIM/TC57CIM/IEC61970/Base/Core#IdentifiedObject> ,
                         [ rdf:type owl:Restriction ;
                           owl:onProperty :TieLine_ParentOfA ;
                           owl:minQualifiedCardinality "0"^^xsd:nonNegativeInteger ;
                           owl:onClass :TieLine
                         ] ,
                         [ rdf:type owl:Restriction ;
                           owl:onProperty :TieLine_ParentOfB ;
                           owl:minQualifiedCardinality "0"^^xsd:nonNegativeInteger ;
                           owl:onClass :TieLine
                         ] .


###  https://w3id.org/netbeheer/IECCIM/TC57CIM/IEC62325/InfIEC62325/InfEnergyScheduling#TransmissionCorridor
:TransmissionCorridor rdf:type owl:Class ;
                      rdfs:subClassOf <https://w3id.org/netbeheer/IECCIM/TC57CIM/IEC61970/Base/Core#PowerSystemResource> ,
                                      [ rdf:type owl:Restriction ;
                                        owl:onProperty :TransmissionCorridor_TransmissionRightOfWays ;
                                        owl:qualifiedCardinality "1"^^xsd:nonNegativeInteger ;
                                        owl:onClass :TransmissionCorridor
                                      ] ;
                      rdfs:comment """A corridor containing one or more rights of way
""" .


###  https://w3id.org/netbeheer/IECCIM/TC57CIM/IEC62325/InfIEC62325/InfEnergyScheduling#TransmissionRightOfWay
:TransmissionRightOfWay rdf:type owl:Class ;
                        rdfs:subClassOf <https://w3id.org/netbeheer/IECCIM/TC57CIM/IEC61970/Base/Core#PowerSystemResource> ,
                                        [ rdf:type owl:Restriction ;
                                          owl:onProperty :TransmissionRightOfWay_TransmissionCorridor ;
                                          owl:minQualifiedCardinality "1"^^xsd:nonNegativeInteger ;
                                          owl:onClass :TransmissionRightOfWay
                                        ] ;
                        rdfs:comment """A collection of transmission lines that are close proximity to each other.
""" .


###  https://w3id.org/netbeheer/IECCIM/TC57CIM/IEC62325/InfIEC62325/InfFinancial#ControlAreaOperator
<https://w3id.org/netbeheer/IECCIM/TC57CIM/IEC62325/InfIEC62325/InfFinancial#ControlAreaOperator> rdf:type owl:Class ;
                                                                                                  rdfs:subClassOf [ rdf:type owl:Restriction ;
                                                                                                                    owl:onProperty :ControlAreaOperator_CAChildOf ;
                                                                                                                    owl:minQualifiedCardinality "0"^^xsd:nonNegativeInteger ;
                                                                                                                    owl:onClass <https://w3id.org/netbeheer/IECCIM/TC57CIM/IEC62325/InfIEC62325/InfFinancial#ControlAreaOperator>
                                                                                                                  ] .


###  https://w3id.org/netbeheer/IECCIM/TC57CIM/IEC62325/InfIEC62325/InfFinancial#CustomerConsumer
<https://w3id.org/netbeheer/IECCIM/TC57CIM/IEC62325/InfIEC62325/InfFinancial#CustomerConsumer> rdf:type owl:Class ;
                                                                                               rdfs:subClassOf [ rdf:type owl:Restriction ;
                                                                                                                 owl:onProperty :CustomerConsumer_CustChildOf ;
                                                                                                                 owl:minQualifiedCardinality "0"^^xsd:nonNegativeInteger ;
                                                                                                                 owl:onClass <https://w3id.org/netbeheer/IECCIM/TC57CIM/IEC62325/InfIEC62325/InfFinancial#CustomerConsumer>
                                                                                                               ] ,
                                                                                                               [ rdf:type owl:Restriction ;
                                                                                                                 owl:onProperty :CustomerConsumer_CustChildOf ;
                                                                                                                 owl:maxQualifiedCardinality "1"^^xsd:nonNegativeInteger ;
                                                                                                                 owl:onClass <https://w3id.org/netbeheer/IECCIM/TC57CIM/IEC62325/InfIEC62325/InfFinancial#CustomerConsumer>
                                                                                                               ] .


###  https://w3id.org/netbeheer/IECCIM/TC57CIM/IEC62325/InfIEC62325/InfFinancial#GenerationProvider
<https://w3id.org/netbeheer/IECCIM/TC57CIM/IEC62325/InfIEC62325/InfFinancial#GenerationProvider> rdf:type owl:Class ;
                                                                                                 rdfs:subClassOf [ rdf:type owl:Restriction ;
                                                                                                                   owl:onProperty :GenerationProvider_ProvidedBy ;
                                                                                                                   owl:qualifiedCardinality "1"^^xsd:nonNegativeInteger ;
                                                                                                                   owl:onClass <https://w3id.org/netbeheer/IECCIM/TC57CIM/IEC62325/InfIEC62325/InfFinancial#GenerationProvider>
                                                                                                                 ] .


###  https://w3id.org/netbeheer/IECCIM/TC57CIM/IEC62325/InfIEC62325/InfFinancial#Marketer
<https://w3id.org/netbeheer/IECCIM/TC57CIM/IEC62325/InfIEC62325/InfFinancial#Marketer> rdf:type owl:Class ;
                                                                                       rdfs:subClassOf [ rdf:type owl:Restriction ;
                                                                                                         owl:onProperty :Marketer_HoldsTitleTo_EnergyProducts ;
                                                                                                         owl:minQualifiedCardinality "0"^^xsd:nonNegativeInteger ;
                                                                                                         owl:onClass <https://w3id.org/netbeheer/IECCIM/TC57CIM/IEC62325/InfIEC62325/InfFinancial#Marketer>
                                                                                                       ] ,
                                                                                                       [ rdf:type owl:Restriction ;
                                                                                                         owl:onProperty :Marketer_Resells_EnergyProduct ;
                                                                                                         owl:minQualifiedCardinality "0"^^xsd:nonNegativeInteger ;
                                                                                                         owl:onClass <https://w3id.org/netbeheer/IECCIM/TC57CIM/IEC62325/InfIEC62325/InfFinancial#Marketer>
                                                                                                       ] ,
                                                                                                       [ rdf:type owl:Restriction ;
                                                                                                         owl:onProperty :Marketer_HoldsTitleTo_EnergyProducts ;
                                                                                                         owl:maxQualifiedCardinality "1"^^xsd:nonNegativeInteger ;
                                                                                                         owl:onClass <https://w3id.org/netbeheer/IECCIM/TC57CIM/IEC62325/InfIEC62325/InfFinancial#Marketer>
                                                                                                       ] .


###  https://w3id.org/netbeheer/IECCIM/TC57CIM/IEC62325/InfIEC62325/InfFinancial#TransmissionProvider
<https://w3id.org/netbeheer/IECCIM/TC57CIM/IEC62325/InfIEC62325/InfFinancial#TransmissionProvider> rdf:type owl:Class ;
                                                                                                   rdfs:subClassOf [ rdf:type owl:Restriction ;
                                                                                                                     owl:onProperty :TransmissionProvider_For ;
                                                                                                                     owl:minQualifiedCardinality "0"^^xsd:nonNegativeInteger ;
                                                                                                                     owl:onClass <https://w3id.org/netbeheer/IECCIM/TC57CIM/IEC62325/InfIEC62325/InfFinancial#TransmissionProvider>
                                                                                                                   ] ,
                                                                                                                   [ rdf:type owl:Restriction ;
                                                                                                                     owl:onProperty :TransmissionProvider_For ;
                                                                                                                     owl:maxQualifiedCardinality "1"^^xsd:nonNegativeInteger ;
                                                                                                                     owl:onClass <https://w3id.org/netbeheer/IECCIM/TC57CIM/IEC62325/InfIEC62325/InfFinancial#TransmissionProvider>
                                                                                                                   ] .


###  https://w3id.org/netbeheer/IECCIM/TC57CIM/IEC62325/MarketOperations/MarketSystem/ExternalInputs#Profile
<https://w3id.org/netbeheer/IECCIM/TC57CIM/IEC62325/MarketOperations/MarketSystem/ExternalInputs#Profile> rdf:type owl:Class .


###  Generated by the OWL API (version 5.1.10.2019-03-12T22:31:15Z) https://github.com/owlcs/owlapi/
