<?xml version="1.0"?>
<rdf:RDF xmlns="https://w3id.org/netbeheer/referentiemodellen/IECCIM/TC57CIM/PackageDependencies#"
     xml:base="https://w3id.org/netbeheer/referentiemodellen/IECCIM/TC57CIM/PackageDependencies"
     xmlns:owl="http://www.w3.org/2002/07/owl#"
     xmlns:rdf="http://www.w3.org/1999/02/22-rdf-syntax-ns#"
     xmlns:xml="http://www.w3.org/XML/1998/namespace"
     xmlns:xsd="http://www.w3.org/2001/XMLSchema#"
     xmlns:rdfs="http://www.w3.org/2000/01/rdf-schema#">
    <owl:Ontology rdf:about="https://w3id.org/netbeheer/referentiemodellen/IECCIM/TC57CIM/PackageDependencies#"/>
    


    <!-- 
    ///////////////////////////////////////////////////////////////////////////////////////
    //
    // Datatypes
    //
    ///////////////////////////////////////////////////////////////////////////////////////
     -->


    


    <!-- http://www.w3.org/2001/XMLSchema#date -->


    <rdfs:Datatype rdf:about="http://www.w3.org/2001/XMLSchema#date"/>
    


    <!-- 
    ///////////////////////////////////////////////////////////////////////////////////////
    //
    // Data properties
    //
    ///////////////////////////////////////////////////////////////////////////////////////
     -->


    


    <!-- PackageDependenciesCIMVersion_date -->


    <owl:DatatypeProperty rdf:about="PackageDependenciesCIMVersion_date">
        <rdfs:domain rdf:resource="https://w3id.org/netbeheer/referentiemodellen/IECCIM/TC57CIM/PackageDependencies#PackageDependenciesCIMVersion"/>
        <rdfs:range rdf:resource="http://www.w3.org/2001/XMLSchema#date"/>
        <rdfs:comment>Date of last change to the main package dependencies in format YYYY-MM-DD.   This is updated when the version attribute is updated.</rdfs:comment>
    </owl:DatatypeProperty>
    


    <!-- https://w3id.org/netbeheer/referentiemodellen/IECCIM/TC57CIM/PackageDependencies#PackageDependenciesCIMVersion_version -->


    <owl:DatatypeProperty rdf:about="https://w3id.org/netbeheer/referentiemodellen/IECCIM/TC57CIM/PackageDependencies#PackageDependenciesCIMVersion_version">
        <rdfs:domain rdf:resource="https://w3id.org/netbeheer/referentiemodellen/IECCIM/TC57CIM/PackageDependencies#PackageDependenciesCIMVersion"/>
        <rdfs:range rdf:resource="http://www.w3.org/2001/XMLSchema#string"/>
        <rdfs:comment>The version of the main subpackages of the combined CIM model.  The format is simply an integer.  The version (and date) initial values should be updated any time the dependencies in the model change and require an actual change to the diagrams within this package.</rdfs:comment>
    </owl:DatatypeProperty>
    


    <!-- 
    ///////////////////////////////////////////////////////////////////////////////////////
    //
    // Classes
    //
    ///////////////////////////////////////////////////////////////////////////////////////
     -->


    


    <!-- https://w3id.org/netbeheer/referentiemodellen/IECCIM/TC57CIM/PackageDependencies#PackageDependenciesCIMVersion -->


    <owl:Class rdf:about="https://w3id.org/netbeheer/referentiemodellen/IECCIM/TC57CIM/PackageDependencies#PackageDependenciesCIMVersion">
        <rdfs:subClassOf>
            <owl:Restriction>
                <owl:onProperty rdf:resource="PackageDependenciesCIMVersion_date"/>
                <owl:minQualifiedCardinality rdf:datatype="http://www.w3.org/2001/XMLSchema#nonNegativeInteger">0</owl:minQualifiedCardinality>
                <owl:onDataRange rdf:resource="http://www.w3.org/2001/XMLSchema#date"/>
            </owl:Restriction>
        </rdfs:subClassOf>
        <rdfs:subClassOf>
            <owl:Restriction>
                <owl:onProperty rdf:resource="https://w3id.org/netbeheer/referentiemodellen/IECCIM/TC57CIM/PackageDependencies#PackageDependenciesCIMVersion_version"/>
                <owl:minQualifiedCardinality rdf:datatype="http://www.w3.org/2001/XMLSchema#nonNegativeInteger">0</owl:minQualifiedCardinality>
                <owl:onDataRange rdf:resource="http://www.w3.org/2001/XMLSchema#string"/>
            </owl:Restriction>
        </rdfs:subClassOf>
        <rdfs:subClassOf>
            <owl:Restriction>
                <owl:onProperty rdf:resource="PackageDependenciesCIMVersion_date"/>
                <owl:maxQualifiedCardinality rdf:datatype="http://www.w3.org/2001/XMLSchema#nonNegativeInteger">1</owl:maxQualifiedCardinality>
                <owl:onDataRange rdf:resource="http://www.w3.org/2001/XMLSchema#date"/>
            </owl:Restriction>
        </rdfs:subClassOf>
        <rdfs:subClassOf>
            <owl:Restriction>
                <owl:onProperty rdf:resource="https://w3id.org/netbeheer/referentiemodellen/IECCIM/TC57CIM/PackageDependencies#PackageDependenciesCIMVersion_version"/>
                <owl:maxQualifiedCardinality rdf:datatype="http://www.w3.org/2001/XMLSchema#nonNegativeInteger">1</owl:maxQualifiedCardinality>
                <owl:onDataRange rdf:resource="http://www.w3.org/2001/XMLSchema#string"/>
            </owl:Restriction>
        </rdfs:subClassOf>
        <rdfs:comment>The version of dependencies description among top level subpackages of the combined CIM model.  This is not the same as the combined packages version.
</rdfs:comment>
    </owl:Class>
</rdf:RDF>



<!-- Generated by the OWL API (version 5.1.10.2019-03-12T22:31:15Z) https://github.com/owlcs/owlapi/ -->


