@prefix : <https://w3id.org/netbeheer/IECCIM/TC57CIM/PackageDependencies#> .
@prefix owl: <http://www.w3.org/2002/07/owl#> .
@prefix rdf: <http://www.w3.org/1999/02/22-rdf-syntax-ns#> .
@prefix xml: <http://www.w3.org/XML/1998/namespace> .
@prefix xsd: <http://www.w3.org/2001/XMLSchema#> .
@prefix rdfs: <http://www.w3.org/2000/01/rdf-schema#> .
@base <https://w3id.org/netbeheer/IECCIM/TC57CIM/PackageDependencies#> .

<https://w3id.org/netbeheer/IECCIM/TC57CIM/PackageDependencies#> rdf:type owl:Ontology .

#################################################################
#    Datatypes
#################################################################

###  http://www.w3.org/2001/XMLSchema#date
xsd:date rdf:type rdfs:Datatype .


#################################################################
#    Data properties
#################################################################

###  PackageDependenciesCIMVersion_date
<PackageDependenciesCIMVersion_date> rdf:type owl:DatatypeProperty ;
                                     rdfs:domain :PackageDependenciesCIMVersion ;
                                     rdfs:range xsd:date ;
                                     rdfs:comment "Date of last change to the main package dependencies in format YYYY-MM-DD.   This is updated when the version attribute is updated." .


###  https://w3id.org/netbeheer/IECCIM/TC57CIM/PackageDependencies#PackageDependenciesCIMVersion_version
:PackageDependenciesCIMVersion_version rdf:type owl:DatatypeProperty ;
                                       rdfs:domain :PackageDependenciesCIMVersion ;
                                       rdfs:range xsd:string ;
                                       rdfs:comment "The version of the main subpackages of the combined CIM model.  The format is simply an integer.  The version (and date) initial values should be updated any time the dependencies in the model change and require an actual change to the diagrams within this package." .


#################################################################
#    Classes
#################################################################

###  https://w3id.org/netbeheer/IECCIM/TC57CIM/PackageDependencies#PackageDependenciesCIMVersion
:PackageDependenciesCIMVersion rdf:type owl:Class ;
                               rdfs:subClassOf [ rdf:type owl:Restriction ;
                                                 owl:onProperty <PackageDependenciesCIMVersion_date> ;
                                                 owl:minQualifiedCardinality "0"^^xsd:nonNegativeInteger ;
                                                 owl:onDataRange xsd:date
                                               ] ,
                                               [ rdf:type owl:Restriction ;
                                                 owl:onProperty :PackageDependenciesCIMVersion_version ;
                                                 owl:minQualifiedCardinality "0"^^xsd:nonNegativeInteger ;
                                                 owl:onDataRange xsd:string
                                               ] ,
                                               [ rdf:type owl:Restriction ;
                                                 owl:onProperty <PackageDependenciesCIMVersion_date> ;
                                                 owl:maxQualifiedCardinality "1"^^xsd:nonNegativeInteger ;
                                                 owl:onDataRange xsd:date
                                               ] ,
                                               [ rdf:type owl:Restriction ;
                                                 owl:onProperty :PackageDependenciesCIMVersion_version ;
                                                 owl:maxQualifiedCardinality "1"^^xsd:nonNegativeInteger ;
                                                 owl:onDataRange xsd:string
                                               ] ;
                               rdfs:comment """The version of dependencies description among top level subpackages of the combined CIM model.  This is not the same as the combined packages version.
""" .


###  Generated by the OWL API (version 5.1.10.2019-03-12T22:31:15Z) https://github.com/owlcs/owlapi/
