<?xml version="1.0"?>
<rdf:RDF xmlns="https://w3id.org/netbeheer/referentiemodellen/IECCIM/TC57CIM/IEC62325/InfIEC62325/InfFinancial#"
     xml:base="https://w3id.org/netbeheer/referentiemodellen/IECCIM/TC57CIM/IEC62325/InfIEC62325/InfFinancial"
     xmlns:owl="http://www.w3.org/2002/07/owl#"
     xmlns:rdf="http://www.w3.org/1999/02/22-rdf-syntax-ns#"
     xmlns:xml="http://www.w3.org/XML/1998/namespace"
     xmlns:xsd="http://www.w3.org/2001/XMLSchema#"
     xmlns:rdfs="http://www.w3.org/2000/01/rdf-schema#">
    <owl:Ontology rdf:about="https://w3id.org/netbeheer/referentiemodellen/IECCIM/TC57CIM/IEC62325/InfIEC62325/InfFinancial#"/>
    


    <!-- 
    ///////////////////////////////////////////////////////////////////////////////////////
    //
    // Object Properties
    //
    ///////////////////////////////////////////////////////////////////////////////////////
     -->


    


    <!-- https://w3id.org/netbeheer/referentiemodellen/IECCIM/TC57CIM/IEC62325/InfIEC62325/InfFinancial#TransmissionProduct_TransmissionProvider -->


    <owl:ObjectProperty rdf:about="https://w3id.org/netbeheer/referentiemodellen/IECCIM/TC57CIM/IEC62325/InfIEC62325/InfFinancial#TransmissionProduct_TransmissionProvider">
        <rdfs:domain rdf:resource="https://w3id.org/netbeheer/referentiemodellen/IECCIM/TC57CIM/IEC62325/InfIEC62325/InfFinancial#TransmissionProduct"/>
        <rdfs:range rdf:resource="https://w3id.org/netbeheer/referentiemodellen/IECCIM/TC57CIM/IEC62325/InfIEC62325/InfFinancial#TransmissionProvider"/>
        <rdfs:comment>A TransmissionProvider offers a TransmissionProduct.A TransmissionProvider offers a TransmissionProduct.</rdfs:comment>
    </owl:ObjectProperty>
    


    <!-- https://w3id.org/netbeheer/referentiemodellen/IECCIM/TC57CIM/IEC62325/InfIEC62325/InfFinancial#TransmissionProvider_TransmissionProducts -->


    <owl:ObjectProperty rdf:about="https://w3id.org/netbeheer/referentiemodellen/IECCIM/TC57CIM/IEC62325/InfIEC62325/InfFinancial#TransmissionProvider_TransmissionProducts">
        <owl:inverseOf rdf:resource="https://w3id.org/netbeheer/referentiemodellen/IECCIM/TC57CIM/IEC62325/InfIEC62325/InfFinancial#TransmissionProduct_TransmissionProvider"/>
        <rdf:type rdf:resource="http://www.w3.org/2002/07/owl#FunctionalProperty"/>
        <rdfs:domain rdf:resource="https://w3id.org/netbeheer/referentiemodellen/IECCIM/TC57CIM/IEC62325/InfIEC62325/InfFinancial#TransmissionProvider"/>
        <rdfs:range rdf:resource="https://w3id.org/netbeheer/referentiemodellen/IECCIM/TC57CIM/IEC62325/InfIEC62325/InfFinancial#TransmissionProduct"/>
        <rdfs:comment>A TransmissionProvider offers a TransmissionProduct.A TransmissionProvider offers a TransmissionProduct.</rdfs:comment>
    </owl:ObjectProperty>
    


    <!-- 
    ///////////////////////////////////////////////////////////////////////////////////////
    //
    // Data properties
    //
    ///////////////////////////////////////////////////////////////////////////////////////
     -->


    


    <!-- https://w3id.org/netbeheer/referentiemodellen/IECCIM/TC57CIM/IEC62325/InfIEC62325/InfFinancial#IntSchedAgreement_defaultIntegrationMethod -->


    <owl:DatatypeProperty rdf:about="https://w3id.org/netbeheer/referentiemodellen/IECCIM/TC57CIM/IEC62325/InfIEC62325/InfFinancial#IntSchedAgreement_defaultIntegrationMethod">
        <rdfs:domain rdf:resource="https://w3id.org/netbeheer/referentiemodellen/IECCIM/TC57CIM/IEC62325/InfIEC62325/InfFinancial#IntSchedAgreement"/>
        <rdfs:range rdf:resource="http://www.w3.org/2001/XMLSchema#string"/>
        <rdfs:comment>The default method by which interchange schedules are to be integrated to obtain hourly MWh schedules for accounting. Method #1 is to integrate the instantaneous schedule between the hourly boundaries. Method #2 compensates for any up/down ramping that occurs across the hourly boundary (this is called block accounting).
</rdfs:comment>
    </owl:DatatypeProperty>
    


    <!-- https://w3id.org/netbeheer/referentiemodellen/IECCIM/TC57CIM/IEC62325/InfIEC62325/InfFinancial#TransmissionProduct_transmissionProductType -->


    <owl:DatatypeProperty rdf:about="https://w3id.org/netbeheer/referentiemodellen/IECCIM/TC57CIM/IEC62325/InfIEC62325/InfFinancial#TransmissionProduct_transmissionProductType">
        <rdfs:domain rdf:resource="https://w3id.org/netbeheer/referentiemodellen/IECCIM/TC57CIM/IEC62325/InfIEC62325/InfFinancial#TransmissionProduct"/>
        <rdfs:range rdf:resource="http://www.w3.org/2001/XMLSchema#string"/>
        <rdfs:comment>Type of the transmission product. This could be a transmission service class (firm, total transmission capability, or non-firm), transmission service period (on-peak, full-period, off-peak), transmission service increments (yearly extended, hourly fixed, monthly sliding, etc.), transmission service type (network, available transmission capability, or point-to-point, or a transmission service window (fixed hourly, sliding weekly, extended monthly, etc.).
</rdfs:comment>
    </owl:DatatypeProperty>
    


    <!-- 
    ///////////////////////////////////////////////////////////////////////////////////////
    //
    // Classes
    //
    ///////////////////////////////////////////////////////////////////////////////////////
     -->


    


    <!-- https://w3id.org/netbeheer/referentiemodellen/IECCIM/TC57CIM/IEC61968/Common#Agreement -->


    <owl:Class rdf:about="https://w3id.org/netbeheer/referentiemodellen/IECCIM/TC57CIM/IEC61968/Common#Agreement"/>
    


    <!-- https://w3id.org/netbeheer/referentiemodellen/IECCIM/TC57CIM/IEC61968/Common#Organisation -->


    <owl:Class rdf:about="https://w3id.org/netbeheer/referentiemodellen/IECCIM/TC57CIM/IEC61968/Common#Organisation"/>
    


    <!-- https://w3id.org/netbeheer/referentiemodellen/IECCIM/TC57CIM/IEC61970/Base/Core#IdentifiedObject -->


    <owl:Class rdf:about="https://w3id.org/netbeheer/referentiemodellen/IECCIM/TC57CIM/IEC61970/Base/Core#IdentifiedObject"/>
    


    <!-- https://w3id.org/netbeheer/referentiemodellen/IECCIM/TC57CIM/IEC62325/InfIEC62325/InfFinancial#ControlAreaOperator -->


    <owl:Class rdf:about="https://w3id.org/netbeheer/referentiemodellen/IECCIM/TC57CIM/IEC62325/InfIEC62325/InfFinancial#ControlAreaOperator">
        <rdfs:subClassOf rdf:resource="https://w3id.org/netbeheer/referentiemodellen/IECCIM/TC57CIM/IEC61968/Common#Organisation"/>
        <rdfs:comment>Operates the Control Area. Approves and implements energy transactions. Verifies both Inter-Control Area and Intra-Control Area transactions for the power system  before granting approval (and implementing) the transactions.
</rdfs:comment>
    </owl:Class>
    


    <!-- https://w3id.org/netbeheer/referentiemodellen/IECCIM/TC57CIM/IEC62325/InfIEC62325/InfFinancial#CustomerConsumer -->


    <owl:Class rdf:about="https://w3id.org/netbeheer/referentiemodellen/IECCIM/TC57CIM/IEC62325/InfIEC62325/InfFinancial#CustomerConsumer">
        <rdfs:subClassOf rdf:resource="https://w3id.org/netbeheer/referentiemodellen/IECCIM/TC57CIM/IEC61968/Common#Organisation"/>
        <rdfs:comment>The energy buyer in the energy marketplace.
</rdfs:comment>
    </owl:Class>
    


    <!-- https://w3id.org/netbeheer/referentiemodellen/IECCIM/TC57CIM/IEC62325/InfIEC62325/InfFinancial#GenerationProvider -->


    <owl:Class rdf:about="https://w3id.org/netbeheer/referentiemodellen/IECCIM/TC57CIM/IEC62325/InfIEC62325/InfFinancial#GenerationProvider">
        <rdfs:subClassOf rdf:resource="https://w3id.org/netbeheer/referentiemodellen/IECCIM/TC57CIM/IEC61968/Common#Organisation"/>
        <rdfs:comment>The energy seller in the energy marketplace.
</rdfs:comment>
    </owl:Class>
    


    <!-- https://w3id.org/netbeheer/referentiemodellen/IECCIM/TC57CIM/IEC62325/InfIEC62325/InfFinancial#IntSchedAgreement -->


    <owl:Class rdf:about="https://w3id.org/netbeheer/referentiemodellen/IECCIM/TC57CIM/IEC62325/InfIEC62325/InfFinancial#IntSchedAgreement">
        <rdfs:subClassOf rdf:resource="https://w3id.org/netbeheer/referentiemodellen/IECCIM/TC57CIM/IEC61968/Common#Agreement"/>
        <rdfs:subClassOf>
            <owl:Restriction>
                <owl:onProperty rdf:resource="https://w3id.org/netbeheer/referentiemodellen/IECCIM/TC57CIM/IEC62325/InfIEC62325/InfFinancial#IntSchedAgreement_defaultIntegrationMethod"/>
                <owl:minQualifiedCardinality rdf:datatype="http://www.w3.org/2001/XMLSchema#nonNegativeInteger">0</owl:minQualifiedCardinality>
                <owl:onDataRange rdf:resource="http://www.w3.org/2001/XMLSchema#string"/>
            </owl:Restriction>
        </rdfs:subClassOf>
        <rdfs:subClassOf>
            <owl:Restriction>
                <owl:onProperty rdf:resource="https://w3id.org/netbeheer/referentiemodellen/IECCIM/TC57CIM/IEC62325/InfIEC62325/InfFinancial#IntSchedAgreement_defaultIntegrationMethod"/>
                <owl:maxQualifiedCardinality rdf:datatype="http://www.w3.org/2001/XMLSchema#nonNegativeInteger">1</owl:maxQualifiedCardinality>
                <owl:onDataRange rdf:resource="http://www.w3.org/2001/XMLSchema#string"/>
            </owl:Restriction>
        </rdfs:subClassOf>
        <rdfs:comment>A type of agreement that provides the default method by which interchange schedules are to be integrated to obtain hourly MWh schedules for accounting. 
</rdfs:comment>
    </owl:Class>
    


    <!-- https://w3id.org/netbeheer/referentiemodellen/IECCIM/TC57CIM/IEC62325/InfIEC62325/InfFinancial#Marketer -->


    <owl:Class rdf:about="https://w3id.org/netbeheer/referentiemodellen/IECCIM/TC57CIM/IEC62325/InfIEC62325/InfFinancial#Marketer">
        <rdfs:subClassOf rdf:resource="https://w3id.org/netbeheer/referentiemodellen/IECCIM/TC57CIM/IEC61968/Common#Organisation"/>
        <rdfs:comment>Matches buyers and sellers, and secures transmission (and other ancillary services) needed to complete the energy transaction.
</rdfs:comment>
    </owl:Class>
    


    <!-- https://w3id.org/netbeheer/referentiemodellen/IECCIM/TC57CIM/IEC62325/InfIEC62325/InfFinancial#OpenAccessProduct -->


    <owl:Class rdf:about="https://w3id.org/netbeheer/referentiemodellen/IECCIM/TC57CIM/IEC62325/InfIEC62325/InfFinancial#OpenAccessProduct">
        <rdfs:subClassOf rdf:resource="https://w3id.org/netbeheer/referentiemodellen/IECCIM/TC57CIM/IEC61968/Common#Agreement"/>
        <rdfs:comment>Contracts for services offered commercially.
</rdfs:comment>
    </owl:Class>
    


    <!-- https://w3id.org/netbeheer/referentiemodellen/IECCIM/TC57CIM/IEC62325/InfIEC62325/InfFinancial#TransmissionProduct -->


    <owl:Class rdf:about="https://w3id.org/netbeheer/referentiemodellen/IECCIM/TC57CIM/IEC62325/InfIEC62325/InfFinancial#TransmissionProduct">
        <rdfs:subClassOf rdf:resource="https://w3id.org/netbeheer/referentiemodellen/IECCIM/TC57CIM/IEC61970/Base/Core#IdentifiedObject"/>
        <rdfs:subClassOf>
            <owl:Restriction>
                <owl:onProperty rdf:resource="https://w3id.org/netbeheer/referentiemodellen/IECCIM/TC57CIM/IEC62325/InfIEC62325/InfFinancial#TransmissionProduct_TransmissionProvider"/>
                <owl:minQualifiedCardinality rdf:datatype="http://www.w3.org/2001/XMLSchema#nonNegativeInteger">1</owl:minQualifiedCardinality>
                <owl:onClass rdf:resource="https://w3id.org/netbeheer/referentiemodellen/IECCIM/TC57CIM/IEC62325/InfIEC62325/InfFinancial#TransmissionProduct"/>
            </owl:Restriction>
        </rdfs:subClassOf>
        <rdfs:subClassOf>
            <owl:Restriction>
                <owl:onProperty rdf:resource="https://w3id.org/netbeheer/referentiemodellen/IECCIM/TC57CIM/IEC62325/InfIEC62325/InfFinancial#TransmissionProduct_transmissionProductType"/>
                <owl:minQualifiedCardinality rdf:datatype="http://www.w3.org/2001/XMLSchema#nonNegativeInteger">0</owl:minQualifiedCardinality>
                <owl:onDataRange rdf:resource="http://www.w3.org/2001/XMLSchema#string"/>
            </owl:Restriction>
        </rdfs:subClassOf>
        <rdfs:subClassOf>
            <owl:Restriction>
                <owl:onProperty rdf:resource="https://w3id.org/netbeheer/referentiemodellen/IECCIM/TC57CIM/IEC62325/InfIEC62325/InfFinancial#TransmissionProduct_transmissionProductType"/>
                <owl:maxQualifiedCardinality rdf:datatype="http://www.w3.org/2001/XMLSchema#nonNegativeInteger">1</owl:maxQualifiedCardinality>
                <owl:onDataRange rdf:resource="http://www.w3.org/2001/XMLSchema#string"/>
            </owl:Restriction>
        </rdfs:subClassOf>
    </owl:Class>
    


    <!-- https://w3id.org/netbeheer/referentiemodellen/IECCIM/TC57CIM/IEC62325/InfIEC62325/InfFinancial#TransmissionProvider -->


    <owl:Class rdf:about="https://w3id.org/netbeheer/referentiemodellen/IECCIM/TC57CIM/IEC62325/InfIEC62325/InfFinancial#TransmissionProvider">
        <rdfs:subClassOf rdf:resource="https://w3id.org/netbeheer/referentiemodellen/IECCIM/TC57CIM/IEC61968/Common#Organisation"/>
        <rdfs:subClassOf>
            <owl:Restriction>
                <owl:onProperty rdf:resource="https://w3id.org/netbeheer/referentiemodellen/IECCIM/TC57CIM/IEC62325/InfIEC62325/InfFinancial#TransmissionProvider_TransmissionProducts"/>
                <owl:qualifiedCardinality rdf:datatype="http://www.w3.org/2001/XMLSchema#nonNegativeInteger">1</owl:qualifiedCardinality>
                <owl:onClass rdf:resource="https://w3id.org/netbeheer/referentiemodellen/IECCIM/TC57CIM/IEC62325/InfIEC62325/InfFinancial#TransmissionProvider"/>
            </owl:Restriction>
        </rdfs:subClassOf>
        <rdfs:comment>Provider of  the transmission capacity (interconnecting wires between Generation and Consumption) required  to fulfill and Energy Transaction&apos;s energy exchange. Posts information for transmission paths and AvailableTransmissionCapacities  on a reservation node.  Buys and sells its products and services on the same reservation node.
</rdfs:comment>
    </owl:Class>
</rdf:RDF>



<!-- Generated by the OWL API (version 5.1.10.2019-03-12T22:31:15Z) https://github.com/owlcs/owlapi/ -->


