<?xml version="1.0"?>
<rdf:RDF xmlns="https://w3id.org/netbeheer/referentiemodellen/IECCIM/TC57CIM/IEC61970/Dynamics/StandardModels/AsynchronousMachineDynamics#"
     xml:base="https://w3id.org/netbeheer/referentiemodellen/IECCIM/TC57CIM/IEC61970/Dynamics/StandardModels/AsynchronousMachineDynamics"
     xmlns:owl="http://www.w3.org/2002/07/owl#"
     xmlns:rdf="http://www.w3.org/1999/02/22-rdf-syntax-ns#"
     xmlns:xml="http://www.w3.org/XML/1998/namespace"
     xmlns:xsd="http://www.w3.org/2001/XMLSchema#"
     xmlns:rdfs="http://www.w3.org/2000/01/rdf-schema#">
    <owl:Ontology rdf:about="https://w3id.org/netbeheer/referentiemodellen/IECCIM/TC57CIM/IEC61970/Dynamics/StandardModels/AsynchronousMachineDynamics#"/>
    


    <!-- 
    ///////////////////////////////////////////////////////////////////////////////////////
    //
    // Object Properties
    //
    ///////////////////////////////////////////////////////////////////////////////////////
     -->


    


    <!-- https://w3id.org/netbeheer/referentiemodellen/IECCIM/TC57CIM/IEC61970/Dynamics/StandardModels/AsynchronousMachineDynamics#AsynchronousMachineDynamics_MechanicalLoadDynamics -->


    <owl:ObjectProperty rdf:about="https://w3id.org/netbeheer/referentiemodellen/IECCIM/TC57CIM/IEC61970/Dynamics/StandardModels/AsynchronousMachineDynamics#AsynchronousMachineDynamics_MechanicalLoadDynamics">
        <owl:inverseOf rdf:resource="https://w3id.org/netbeheer/referentiemodellen/IECCIM/TC57CIM/IEC61970/Dynamics/StandardModels/AsynchronousMachineDynamics#MechanicalLoadDynamics_AsynchronousMachineDynamics"/>
        <rdfs:domain rdf:resource="https://w3id.org/netbeheer/referentiemodellen/IECCIM/TC57CIM/IEC61970/Dynamics/StandardModels/AsynchronousMachineDynamics#AsynchronousMachineDynamics"/>
        <rdfs:range rdf:resource="https://w3id.org/netbeheer/referentiemodellen/IECCIM/TC57CIM/IEC61970/Dynamics/StandardModels/MechanicalLoadDynamics#MechanicalLoadDynamics"/>
        <rdfs:comment>Mechanical load model associated with this asynchronous machine model.Asynchronous machine model with which this mechanical load model is associated.</rdfs:comment>
    </owl:ObjectProperty>
    


    <!-- https://w3id.org/netbeheer/referentiemodellen/IECCIM/TC57CIM/IEC61970/Dynamics/StandardModels/AsynchronousMachineDynamics#AsynchronousMachineDynamics_TurbineGovernorDynamics -->


    <owl:ObjectProperty rdf:about="https://w3id.org/netbeheer/referentiemodellen/IECCIM/TC57CIM/IEC61970/Dynamics/StandardModels/AsynchronousMachineDynamics#AsynchronousMachineDynamics_TurbineGovernorDynamics">
        <owl:inverseOf rdf:resource="https://w3id.org/netbeheer/referentiemodellen/IECCIM/TC57CIM/IEC61970/Dynamics/StandardModels/AsynchronousMachineDynamics#TurbineGovernorDynamics_AsynchronousMachineDynamics"/>
        <rdfs:domain rdf:resource="https://w3id.org/netbeheer/referentiemodellen/IECCIM/TC57CIM/IEC61970/Dynamics/StandardModels/AsynchronousMachineDynamics#AsynchronousMachineDynamics"/>
        <rdfs:range rdf:resource="https://w3id.org/netbeheer/referentiemodellen/IECCIM/TC57CIM/IEC61970/Dynamics/StandardModels/TurbineGovernorDynamics#TurbineGovernorDynamics"/>
        <rdfs:comment>Turbine-governor model associated with this asynchronous machine model.Asynchronous machine model with which this turbine-governor model is associated.</rdfs:comment>
    </owl:ObjectProperty>
    


    <!-- https://w3id.org/netbeheer/referentiemodellen/IECCIM/TC57CIM/IEC61970/Dynamics/StandardModels/AsynchronousMachineDynamics#AsynchronousMachineDynamics_WindTurbineType1or2Dynamics -->


    <owl:ObjectProperty rdf:about="https://w3id.org/netbeheer/referentiemodellen/IECCIM/TC57CIM/IEC61970/Dynamics/StandardModels/AsynchronousMachineDynamics#AsynchronousMachineDynamics_WindTurbineType1or2Dynamics">
        <owl:inverseOf rdf:resource="https://w3id.org/netbeheer/referentiemodellen/IECCIM/TC57CIM/IEC61970/Dynamics/StandardModels/AsynchronousMachineDynamics#WindTurbineType1or2Dynamics_AsynchronousMachineDynamics"/>
        <rdf:type rdf:resource="http://www.w3.org/2002/07/owl#FunctionalProperty"/>
        <rdfs:domain rdf:resource="https://w3id.org/netbeheer/referentiemodellen/IECCIM/TC57CIM/IEC61970/Dynamics/StandardModels/AsynchronousMachineDynamics#AsynchronousMachineDynamics"/>
        <rdfs:range rdf:resource="https://w3id.org/netbeheer/referentiemodellen/IECCIM/TC57CIM/IEC61970/Dynamics/StandardModels/WindDynamics#WindTurbineType1or2Dynamics"/>
        <rdfs:comment>Wind generator type 1 or 2 model associated with this asynchronous machine model.Asynchronous machine model with which this wind generator type 1 or 2 model is associated.</rdfs:comment>
    </owl:ObjectProperty>
    


    <!-- https://w3id.org/netbeheer/referentiemodellen/IECCIM/TC57CIM/IEC61970/Dynamics/StandardModels/AsynchronousMachineDynamics#AsynchronousMachineEquivalentCircuit_rr1 -->


    <owl:ObjectProperty rdf:about="https://w3id.org/netbeheer/referentiemodellen/IECCIM/TC57CIM/IEC61970/Dynamics/StandardModels/AsynchronousMachineDynamics#AsynchronousMachineEquivalentCircuit_rr1">
        <rdfs:domain rdf:resource="https://w3id.org/netbeheer/referentiemodellen/IECCIM/TC57CIM/IEC61970/Dynamics/StandardModels/AsynchronousMachineDynamics#AsynchronousMachineEquivalentCircuit"/>
        <rdfs:range rdf:resource="https://w3id.org/netbeheer/referentiemodellen/IECCIM/TC57CIM/IEC61970/Base/Domain#PU"/>
        <rdfs:comment>Damper 1 winding resistance.</rdfs:comment>
    </owl:ObjectProperty>
    


    <!-- https://w3id.org/netbeheer/referentiemodellen/IECCIM/TC57CIM/IEC61970/Dynamics/StandardModels/AsynchronousMachineDynamics#AsynchronousMachineEquivalentCircuit_rr2 -->


    <owl:ObjectProperty rdf:about="https://w3id.org/netbeheer/referentiemodellen/IECCIM/TC57CIM/IEC61970/Dynamics/StandardModels/AsynchronousMachineDynamics#AsynchronousMachineEquivalentCircuit_rr2">
        <rdfs:domain rdf:resource="https://w3id.org/netbeheer/referentiemodellen/IECCIM/TC57CIM/IEC61970/Dynamics/StandardModels/AsynchronousMachineDynamics#AsynchronousMachineEquivalentCircuit"/>
        <rdfs:range rdf:resource="https://w3id.org/netbeheer/referentiemodellen/IECCIM/TC57CIM/IEC61970/Base/Domain#PU"/>
        <rdfs:comment>Damper 2 winding resistance.</rdfs:comment>
    </owl:ObjectProperty>
    


    <!-- https://w3id.org/netbeheer/referentiemodellen/IECCIM/TC57CIM/IEC61970/Dynamics/StandardModels/AsynchronousMachineDynamics#AsynchronousMachineEquivalentCircuit_xlr1 -->


    <owl:ObjectProperty rdf:about="https://w3id.org/netbeheer/referentiemodellen/IECCIM/TC57CIM/IEC61970/Dynamics/StandardModels/AsynchronousMachineDynamics#AsynchronousMachineEquivalentCircuit_xlr1">
        <rdfs:domain rdf:resource="https://w3id.org/netbeheer/referentiemodellen/IECCIM/TC57CIM/IEC61970/Dynamics/StandardModels/AsynchronousMachineDynamics#AsynchronousMachineEquivalentCircuit"/>
        <rdfs:range rdf:resource="https://w3id.org/netbeheer/referentiemodellen/IECCIM/TC57CIM/IEC61970/Base/Domain#PU"/>
        <rdfs:comment>Damper 1 winding leakage reactance.</rdfs:comment>
    </owl:ObjectProperty>
    


    <!-- https://w3id.org/netbeheer/referentiemodellen/IECCIM/TC57CIM/IEC61970/Dynamics/StandardModels/AsynchronousMachineDynamics#AsynchronousMachineEquivalentCircuit_xlr2 -->


    <owl:ObjectProperty rdf:about="https://w3id.org/netbeheer/referentiemodellen/IECCIM/TC57CIM/IEC61970/Dynamics/StandardModels/AsynchronousMachineDynamics#AsynchronousMachineEquivalentCircuit_xlr2">
        <rdfs:domain rdf:resource="https://w3id.org/netbeheer/referentiemodellen/IECCIM/TC57CIM/IEC61970/Dynamics/StandardModels/AsynchronousMachineDynamics#AsynchronousMachineEquivalentCircuit"/>
        <rdfs:range rdf:resource="https://w3id.org/netbeheer/referentiemodellen/IECCIM/TC57CIM/IEC61970/Base/Domain#PU"/>
        <rdfs:comment>Damper 2 winding leakage reactance.</rdfs:comment>
    </owl:ObjectProperty>
    


    <!-- https://w3id.org/netbeheer/referentiemodellen/IECCIM/TC57CIM/IEC61970/Dynamics/StandardModels/AsynchronousMachineDynamics#AsynchronousMachineEquivalentCircuit_xm -->


    <owl:ObjectProperty rdf:about="https://w3id.org/netbeheer/referentiemodellen/IECCIM/TC57CIM/IEC61970/Dynamics/StandardModels/AsynchronousMachineDynamics#AsynchronousMachineEquivalentCircuit_xm">
        <rdfs:domain rdf:resource="https://w3id.org/netbeheer/referentiemodellen/IECCIM/TC57CIM/IEC61970/Dynamics/StandardModels/AsynchronousMachineDynamics#AsynchronousMachineEquivalentCircuit"/>
        <rdfs:range rdf:resource="https://w3id.org/netbeheer/referentiemodellen/IECCIM/TC57CIM/IEC61970/Base/Domain#PU"/>
        <rdfs:comment>Magnetizing reactance.</rdfs:comment>
    </owl:ObjectProperty>
    


    <!-- https://w3id.org/netbeheer/referentiemodellen/IECCIM/TC57CIM/IEC61970/Dynamics/StandardModels/AsynchronousMachineDynamics#AsynchronousMachineTimeConstantReactance_tpo -->


    <owl:ObjectProperty rdf:about="https://w3id.org/netbeheer/referentiemodellen/IECCIM/TC57CIM/IEC61970/Dynamics/StandardModels/AsynchronousMachineDynamics#AsynchronousMachineTimeConstantReactance_tpo">
        <rdfs:domain rdf:resource="https://w3id.org/netbeheer/referentiemodellen/IECCIM/TC57CIM/IEC61970/Dynamics/StandardModels/AsynchronousMachineDynamics#AsynchronousMachineTimeConstantReactance"/>
        <rdfs:range rdf:resource="https://w3id.org/netbeheer/referentiemodellen/IECCIM/TC57CIM/IEC61970/Base/Domain#Seconds"/>
        <rdfs:comment>Transient rotor time constant (T&apos;o) (&amp;gt; T&apos;&apos;o).  Typical Value = 5.</rdfs:comment>
    </owl:ObjectProperty>
    


    <!-- https://w3id.org/netbeheer/referentiemodellen/IECCIM/TC57CIM/IEC61970/Dynamics/StandardModels/AsynchronousMachineDynamics#AsynchronousMachineTimeConstantReactance_tppo -->


    <owl:ObjectProperty rdf:about="https://w3id.org/netbeheer/referentiemodellen/IECCIM/TC57CIM/IEC61970/Dynamics/StandardModels/AsynchronousMachineDynamics#AsynchronousMachineTimeConstantReactance_tppo">
        <rdfs:domain rdf:resource="https://w3id.org/netbeheer/referentiemodellen/IECCIM/TC57CIM/IEC61970/Dynamics/StandardModels/AsynchronousMachineDynamics#AsynchronousMachineTimeConstantReactance"/>
        <rdfs:range rdf:resource="https://w3id.org/netbeheer/referentiemodellen/IECCIM/TC57CIM/IEC61970/Base/Domain#Seconds"/>
        <rdfs:comment>Subtransient rotor time constant (T&apos;&apos;o) (&amp;gt; 0).  Typical Value = 0.03.</rdfs:comment>
    </owl:ObjectProperty>
    


    <!-- https://w3id.org/netbeheer/referentiemodellen/IECCIM/TC57CIM/IEC61970/Dynamics/StandardModels/AsynchronousMachineDynamics#AsynchronousMachineTimeConstantReactance_xp -->


    <owl:ObjectProperty rdf:about="https://w3id.org/netbeheer/referentiemodellen/IECCIM/TC57CIM/IEC61970/Dynamics/StandardModels/AsynchronousMachineDynamics#AsynchronousMachineTimeConstantReactance_xp">
        <rdfs:domain rdf:resource="https://w3id.org/netbeheer/referentiemodellen/IECCIM/TC57CIM/IEC61970/Dynamics/StandardModels/AsynchronousMachineDynamics#AsynchronousMachineTimeConstantReactance"/>
        <rdfs:range rdf:resource="https://w3id.org/netbeheer/referentiemodellen/IECCIM/TC57CIM/IEC61970/Base/Domain#PU"/>
        <rdfs:comment>Transient reactance (unsaturated) (X&apos;) (&amp;gt;=X&apos;&apos;).  Typical Value = 0.5.</rdfs:comment>
    </owl:ObjectProperty>
    


    <!-- https://w3id.org/netbeheer/referentiemodellen/IECCIM/TC57CIM/IEC61970/Dynamics/StandardModels/AsynchronousMachineDynamics#AsynchronousMachineTimeConstantReactance_xpp -->


    <owl:ObjectProperty rdf:about="https://w3id.org/netbeheer/referentiemodellen/IECCIM/TC57CIM/IEC61970/Dynamics/StandardModels/AsynchronousMachineDynamics#AsynchronousMachineTimeConstantReactance_xpp">
        <rdfs:domain rdf:resource="https://w3id.org/netbeheer/referentiemodellen/IECCIM/TC57CIM/IEC61970/Dynamics/StandardModels/AsynchronousMachineDynamics#AsynchronousMachineTimeConstantReactance"/>
        <rdfs:range rdf:resource="https://w3id.org/netbeheer/referentiemodellen/IECCIM/TC57CIM/IEC61970/Base/Domain#PU"/>
        <rdfs:comment>Subtransient reactance (unsaturated) (X&apos;&apos;) (&amp;gt; Xl).  Typical Value = 0.2.</rdfs:comment>
    </owl:ObjectProperty>
    


    <!-- https://w3id.org/netbeheer/referentiemodellen/IECCIM/TC57CIM/IEC61970/Dynamics/StandardModels/AsynchronousMachineDynamics#AsynchronousMachineTimeConstantReactance_xs -->


    <owl:ObjectProperty rdf:about="https://w3id.org/netbeheer/referentiemodellen/IECCIM/TC57CIM/IEC61970/Dynamics/StandardModels/AsynchronousMachineDynamics#AsynchronousMachineTimeConstantReactance_xs">
        <rdfs:domain rdf:resource="https://w3id.org/netbeheer/referentiemodellen/IECCIM/TC57CIM/IEC61970/Dynamics/StandardModels/AsynchronousMachineDynamics#AsynchronousMachineTimeConstantReactance"/>
        <rdfs:range rdf:resource="https://w3id.org/netbeheer/referentiemodellen/IECCIM/TC57CIM/IEC61970/Base/Domain#PU"/>
        <rdfs:comment>Synchronous reactance (Xs) (&amp;gt;= X&apos;).  Typical Value = 1.8.</rdfs:comment>
    </owl:ObjectProperty>
    


    <!-- https://w3id.org/netbeheer/referentiemodellen/IECCIM/TC57CIM/IEC61970/Dynamics/StandardModels/AsynchronousMachineDynamics#MechanicalLoadDynamics_AsynchronousMachineDynamics -->


    <owl:ObjectProperty rdf:about="https://w3id.org/netbeheer/referentiemodellen/IECCIM/TC57CIM/IEC61970/Dynamics/StandardModels/AsynchronousMachineDynamics#MechanicalLoadDynamics_AsynchronousMachineDynamics">
        <rdfs:domain rdf:resource="https://w3id.org/netbeheer/referentiemodellen/IECCIM/TC57CIM/IEC61970/Dynamics/StandardModels/MechanicalLoadDynamics#MechanicalLoadDynamics"/>
        <rdfs:range rdf:resource="https://w3id.org/netbeheer/referentiemodellen/IECCIM/TC57CIM/IEC61970/Dynamics/StandardModels/AsynchronousMachineDynamics#AsynchronousMachineDynamics"/>
        <rdfs:comment>Mechanical load model associated with this asynchronous machine model.Asynchronous machine model with which this mechanical load model is associated.</rdfs:comment>
    </owl:ObjectProperty>
    


    <!-- https://w3id.org/netbeheer/referentiemodellen/IECCIM/TC57CIM/IEC61970/Dynamics/StandardModels/AsynchronousMachineDynamics#TurbineGovernorDynamics_AsynchronousMachineDynamics -->


    <owl:ObjectProperty rdf:about="https://w3id.org/netbeheer/referentiemodellen/IECCIM/TC57CIM/IEC61970/Dynamics/StandardModels/AsynchronousMachineDynamics#TurbineGovernorDynamics_AsynchronousMachineDynamics">
        <rdfs:domain rdf:resource="https://w3id.org/netbeheer/referentiemodellen/IECCIM/TC57CIM/IEC61970/Dynamics/StandardModels/TurbineGovernorDynamics#TurbineGovernorDynamics"/>
        <rdfs:range rdf:resource="https://w3id.org/netbeheer/referentiemodellen/IECCIM/TC57CIM/IEC61970/Dynamics/StandardModels/AsynchronousMachineDynamics#AsynchronousMachineDynamics"/>
        <rdfs:comment>Turbine-governor model associated with this asynchronous machine model.Asynchronous machine model with which this turbine-governor model is associated.</rdfs:comment>
    </owl:ObjectProperty>
    


    <!-- https://w3id.org/netbeheer/referentiemodellen/IECCIM/TC57CIM/IEC61970/Dynamics/StandardModels/AsynchronousMachineDynamics#WindTurbineType1or2Dynamics_AsynchronousMachineDynamics -->


    <owl:ObjectProperty rdf:about="https://w3id.org/netbeheer/referentiemodellen/IECCIM/TC57CIM/IEC61970/Dynamics/StandardModels/AsynchronousMachineDynamics#WindTurbineType1or2Dynamics_AsynchronousMachineDynamics">
        <rdfs:domain rdf:resource="https://w3id.org/netbeheer/referentiemodellen/IECCIM/TC57CIM/IEC61970/Dynamics/StandardModels/WindDynamics#WindTurbineType1or2Dynamics"/>
        <rdfs:range rdf:resource="https://w3id.org/netbeheer/referentiemodellen/IECCIM/TC57CIM/IEC61970/Dynamics/StandardModels/AsynchronousMachineDynamics#AsynchronousMachineDynamics"/>
        <rdfs:comment>Wind generator type 1 or 2 model associated with this asynchronous machine model.Asynchronous machine model with which this wind generator type 1 or 2 model is associated.</rdfs:comment>
    </owl:ObjectProperty>
    


    <!-- 
    ///////////////////////////////////////////////////////////////////////////////////////
    //
    // Classes
    //
    ///////////////////////////////////////////////////////////////////////////////////////
     -->


    


    <!-- https://w3id.org/netbeheer/referentiemodellen/IECCIM/TC57CIM/IEC61970/Base/Domain#PU -->


    <owl:Class rdf:about="https://w3id.org/netbeheer/referentiemodellen/IECCIM/TC57CIM/IEC61970/Base/Domain#PU"/>
    


    <!-- https://w3id.org/netbeheer/referentiemodellen/IECCIM/TC57CIM/IEC61970/Base/Domain#Seconds -->


    <owl:Class rdf:about="https://w3id.org/netbeheer/referentiemodellen/IECCIM/TC57CIM/IEC61970/Base/Domain#Seconds"/>
    


    <!-- https://w3id.org/netbeheer/referentiemodellen/IECCIM/TC57CIM/IEC61970/Dynamics/StandardModels#RotatingMachineDynamics -->


    <owl:Class rdf:about="https://w3id.org/netbeheer/referentiemodellen/IECCIM/TC57CIM/IEC61970/Dynamics/StandardModels#RotatingMachineDynamics"/>
    


    <!-- https://w3id.org/netbeheer/referentiemodellen/IECCIM/TC57CIM/IEC61970/Dynamics/StandardModels/AsynchronousMachineDynamics#AsynchronousMachineDynamics -->


    <owl:Class rdf:about="https://w3id.org/netbeheer/referentiemodellen/IECCIM/TC57CIM/IEC61970/Dynamics/StandardModels/AsynchronousMachineDynamics#AsynchronousMachineDynamics">
        <rdfs:subClassOf rdf:resource="https://w3id.org/netbeheer/referentiemodellen/IECCIM/TC57CIM/IEC61970/Dynamics/StandardModels#RotatingMachineDynamics"/>
        <rdfs:subClassOf>
            <owl:Restriction>
                <owl:onProperty rdf:resource="https://w3id.org/netbeheer/referentiemodellen/IECCIM/TC57CIM/IEC61970/Dynamics/StandardModels/AsynchronousMachineDynamics#AsynchronousMachineDynamics_MechanicalLoadDynamics"/>
                <owl:minQualifiedCardinality rdf:datatype="http://www.w3.org/2001/XMLSchema#nonNegativeInteger">0</owl:minQualifiedCardinality>
                <owl:onClass rdf:resource="https://w3id.org/netbeheer/referentiemodellen/IECCIM/TC57CIM/IEC61970/Dynamics/StandardModels/AsynchronousMachineDynamics#AsynchronousMachineDynamics"/>
            </owl:Restriction>
        </rdfs:subClassOf>
        <rdfs:subClassOf>
            <owl:Restriction>
                <owl:onProperty rdf:resource="https://w3id.org/netbeheer/referentiemodellen/IECCIM/TC57CIM/IEC61970/Dynamics/StandardModels/AsynchronousMachineDynamics#AsynchronousMachineDynamics_TurbineGovernorDynamics"/>
                <owl:minQualifiedCardinality rdf:datatype="http://www.w3.org/2001/XMLSchema#nonNegativeInteger">0</owl:minQualifiedCardinality>
                <owl:onClass rdf:resource="https://w3id.org/netbeheer/referentiemodellen/IECCIM/TC57CIM/IEC61970/Dynamics/StandardModels/AsynchronousMachineDynamics#AsynchronousMachineDynamics"/>
            </owl:Restriction>
        </rdfs:subClassOf>
        <rdfs:subClassOf>
            <owl:Restriction>
                <owl:onProperty rdf:resource="https://w3id.org/netbeheer/referentiemodellen/IECCIM/TC57CIM/IEC61970/Dynamics/StandardModels/AsynchronousMachineDynamics#AsynchronousMachineDynamics_WindTurbineType1or2Dynamics"/>
                <owl:qualifiedCardinality rdf:datatype="http://www.w3.org/2001/XMLSchema#nonNegativeInteger">1</owl:qualifiedCardinality>
                <owl:onClass rdf:resource="https://w3id.org/netbeheer/referentiemodellen/IECCIM/TC57CIM/IEC61970/Dynamics/StandardModels/AsynchronousMachineDynamics#AsynchronousMachineDynamics"/>
            </owl:Restriction>
        </rdfs:subClassOf>
        <rdfs:subClassOf>
            <owl:Restriction>
                <owl:onProperty rdf:resource="https://w3id.org/netbeheer/referentiemodellen/IECCIM/TC57CIM/IEC61970/Dynamics/StandardModels/AsynchronousMachineDynamics#AsynchronousMachineDynamics_MechanicalLoadDynamics"/>
                <owl:maxQualifiedCardinality rdf:datatype="http://www.w3.org/2001/XMLSchema#nonNegativeInteger">1</owl:maxQualifiedCardinality>
                <owl:onClass rdf:resource="https://w3id.org/netbeheer/referentiemodellen/IECCIM/TC57CIM/IEC61970/Dynamics/StandardModels/AsynchronousMachineDynamics#AsynchronousMachineDynamics"/>
            </owl:Restriction>
        </rdfs:subClassOf>
        <rdfs:subClassOf>
            <owl:Restriction>
                <owl:onProperty rdf:resource="https://w3id.org/netbeheer/referentiemodellen/IECCIM/TC57CIM/IEC61970/Dynamics/StandardModels/AsynchronousMachineDynamics#AsynchronousMachineDynamics_TurbineGovernorDynamics"/>
                <owl:maxQualifiedCardinality rdf:datatype="http://www.w3.org/2001/XMLSchema#nonNegativeInteger">1</owl:maxQualifiedCardinality>
                <owl:onClass rdf:resource="https://w3id.org/netbeheer/referentiemodellen/IECCIM/TC57CIM/IEC61970/Dynamics/StandardModels/AsynchronousMachineDynamics#AsynchronousMachineDynamics"/>
            </owl:Restriction>
        </rdfs:subClassOf>
        <rdfs:comment>Asynchronous machine whose behaviour is described by reference to a standard model expressed in either time constant reactance form or equivalent circuit form &lt;font color=&quot;#0f0f0f&quot;&gt;or by definition of a user-defined model.&lt;/font&gt;

&lt;b&gt;Parameter Notes:&lt;/b&gt;
&lt;ol&gt;
 &lt;li&gt;Asynchronous machine parameters such as &lt;b&gt;Xl, Xs&lt;/b&gt; etc. are actually used as inductances (L) in the model, but are commonly referred to as reactances since, at nominal frequency, the per unit values are the same. However, some references use the symbol L instead of X. &lt;/li&gt;
&lt;/ol&gt;</rdfs:comment>
    </owl:Class>
    


    <!-- https://w3id.org/netbeheer/referentiemodellen/IECCIM/TC57CIM/IEC61970/Dynamics/StandardModels/AsynchronousMachineDynamics#AsynchronousMachineEquivalentCircuit -->


    <owl:Class rdf:about="https://w3id.org/netbeheer/referentiemodellen/IECCIM/TC57CIM/IEC61970/Dynamics/StandardModels/AsynchronousMachineDynamics#AsynchronousMachineEquivalentCircuit">
        <rdfs:subClassOf rdf:resource="https://w3id.org/netbeheer/referentiemodellen/IECCIM/TC57CIM/IEC61970/Dynamics/StandardModels/AsynchronousMachineDynamics#AsynchronousMachineDynamics"/>
        <rdfs:subClassOf>
            <owl:Restriction>
                <owl:onProperty rdf:resource="https://w3id.org/netbeheer/referentiemodellen/IECCIM/TC57CIM/IEC61970/Dynamics/StandardModels/AsynchronousMachineDynamics#AsynchronousMachineEquivalentCircuit_rr1"/>
                <owl:minQualifiedCardinality rdf:datatype="http://www.w3.org/2001/XMLSchema#nonNegativeInteger">0</owl:minQualifiedCardinality>
                <owl:onClass rdf:resource="https://w3id.org/netbeheer/referentiemodellen/IECCIM/TC57CIM/IEC61970/Base/Domain#PU"/>
            </owl:Restriction>
        </rdfs:subClassOf>
        <rdfs:subClassOf>
            <owl:Restriction>
                <owl:onProperty rdf:resource="https://w3id.org/netbeheer/referentiemodellen/IECCIM/TC57CIM/IEC61970/Dynamics/StandardModels/AsynchronousMachineDynamics#AsynchronousMachineEquivalentCircuit_rr2"/>
                <owl:minQualifiedCardinality rdf:datatype="http://www.w3.org/2001/XMLSchema#nonNegativeInteger">0</owl:minQualifiedCardinality>
                <owl:onClass rdf:resource="https://w3id.org/netbeheer/referentiemodellen/IECCIM/TC57CIM/IEC61970/Base/Domain#PU"/>
            </owl:Restriction>
        </rdfs:subClassOf>
        <rdfs:subClassOf>
            <owl:Restriction>
                <owl:onProperty rdf:resource="https://w3id.org/netbeheer/referentiemodellen/IECCIM/TC57CIM/IEC61970/Dynamics/StandardModels/AsynchronousMachineDynamics#AsynchronousMachineEquivalentCircuit_xlr1"/>
                <owl:minQualifiedCardinality rdf:datatype="http://www.w3.org/2001/XMLSchema#nonNegativeInteger">0</owl:minQualifiedCardinality>
                <owl:onClass rdf:resource="https://w3id.org/netbeheer/referentiemodellen/IECCIM/TC57CIM/IEC61970/Base/Domain#PU"/>
            </owl:Restriction>
        </rdfs:subClassOf>
        <rdfs:subClassOf>
            <owl:Restriction>
                <owl:onProperty rdf:resource="https://w3id.org/netbeheer/referentiemodellen/IECCIM/TC57CIM/IEC61970/Dynamics/StandardModels/AsynchronousMachineDynamics#AsynchronousMachineEquivalentCircuit_xlr2"/>
                <owl:minQualifiedCardinality rdf:datatype="http://www.w3.org/2001/XMLSchema#nonNegativeInteger">0</owl:minQualifiedCardinality>
                <owl:onClass rdf:resource="https://w3id.org/netbeheer/referentiemodellen/IECCIM/TC57CIM/IEC61970/Base/Domain#PU"/>
            </owl:Restriction>
        </rdfs:subClassOf>
        <rdfs:subClassOf>
            <owl:Restriction>
                <owl:onProperty rdf:resource="https://w3id.org/netbeheer/referentiemodellen/IECCIM/TC57CIM/IEC61970/Dynamics/StandardModels/AsynchronousMachineDynamics#AsynchronousMachineEquivalentCircuit_xm"/>
                <owl:minQualifiedCardinality rdf:datatype="http://www.w3.org/2001/XMLSchema#nonNegativeInteger">0</owl:minQualifiedCardinality>
                <owl:onClass rdf:resource="https://w3id.org/netbeheer/referentiemodellen/IECCIM/TC57CIM/IEC61970/Base/Domain#PU"/>
            </owl:Restriction>
        </rdfs:subClassOf>
        <rdfs:subClassOf>
            <owl:Restriction>
                <owl:onProperty rdf:resource="https://w3id.org/netbeheer/referentiemodellen/IECCIM/TC57CIM/IEC61970/Dynamics/StandardModels/AsynchronousMachineDynamics#AsynchronousMachineEquivalentCircuit_rr1"/>
                <owl:maxQualifiedCardinality rdf:datatype="http://www.w3.org/2001/XMLSchema#nonNegativeInteger">1</owl:maxQualifiedCardinality>
                <owl:onClass rdf:resource="https://w3id.org/netbeheer/referentiemodellen/IECCIM/TC57CIM/IEC61970/Base/Domain#PU"/>
            </owl:Restriction>
        </rdfs:subClassOf>
        <rdfs:subClassOf>
            <owl:Restriction>
                <owl:onProperty rdf:resource="https://w3id.org/netbeheer/referentiemodellen/IECCIM/TC57CIM/IEC61970/Dynamics/StandardModels/AsynchronousMachineDynamics#AsynchronousMachineEquivalentCircuit_rr2"/>
                <owl:maxQualifiedCardinality rdf:datatype="http://www.w3.org/2001/XMLSchema#nonNegativeInteger">1</owl:maxQualifiedCardinality>
                <owl:onClass rdf:resource="https://w3id.org/netbeheer/referentiemodellen/IECCIM/TC57CIM/IEC61970/Base/Domain#PU"/>
            </owl:Restriction>
        </rdfs:subClassOf>
        <rdfs:subClassOf>
            <owl:Restriction>
                <owl:onProperty rdf:resource="https://w3id.org/netbeheer/referentiemodellen/IECCIM/TC57CIM/IEC61970/Dynamics/StandardModels/AsynchronousMachineDynamics#AsynchronousMachineEquivalentCircuit_xlr1"/>
                <owl:maxQualifiedCardinality rdf:datatype="http://www.w3.org/2001/XMLSchema#nonNegativeInteger">1</owl:maxQualifiedCardinality>
                <owl:onClass rdf:resource="https://w3id.org/netbeheer/referentiemodellen/IECCIM/TC57CIM/IEC61970/Base/Domain#PU"/>
            </owl:Restriction>
        </rdfs:subClassOf>
        <rdfs:subClassOf>
            <owl:Restriction>
                <owl:onProperty rdf:resource="https://w3id.org/netbeheer/referentiemodellen/IECCIM/TC57CIM/IEC61970/Dynamics/StandardModels/AsynchronousMachineDynamics#AsynchronousMachineEquivalentCircuit_xlr2"/>
                <owl:maxQualifiedCardinality rdf:datatype="http://www.w3.org/2001/XMLSchema#nonNegativeInteger">1</owl:maxQualifiedCardinality>
                <owl:onClass rdf:resource="https://w3id.org/netbeheer/referentiemodellen/IECCIM/TC57CIM/IEC61970/Base/Domain#PU"/>
            </owl:Restriction>
        </rdfs:subClassOf>
        <rdfs:subClassOf>
            <owl:Restriction>
                <owl:onProperty rdf:resource="https://w3id.org/netbeheer/referentiemodellen/IECCIM/TC57CIM/IEC61970/Dynamics/StandardModels/AsynchronousMachineDynamics#AsynchronousMachineEquivalentCircuit_xm"/>
                <owl:maxQualifiedCardinality rdf:datatype="http://www.w3.org/2001/XMLSchema#nonNegativeInteger">1</owl:maxQualifiedCardinality>
                <owl:onClass rdf:resource="https://w3id.org/netbeheer/referentiemodellen/IECCIM/TC57CIM/IEC61970/Base/Domain#PU"/>
            </owl:Restriction>
        </rdfs:subClassOf>
        <rdfs:comment>The electrical equations of all variations of the asynchronous model are based on the AsynchronousEquivalentCircuit diagram for the direct and quadrature axes, with two equivalent rotor windings in each axis.  

&lt;b&gt;Equations for conversion between Equivalent Circuit and Time Constant Reactance forms:&lt;/b&gt;
&lt;b&gt;Xs&lt;/b&gt; = &lt;b&gt;Xm&lt;/b&gt; + &lt;b&gt;Xl&lt;/b&gt;
&lt;b&gt;X&apos;&lt;/b&gt; = &lt;b&gt;Xl&lt;/b&gt; + &lt;b&gt;Xm&lt;/b&gt; * &lt;b&gt;Xlr1&lt;/b&gt; / (&lt;b&gt;Xm&lt;/b&gt; + &lt;b&gt;Xlr1&lt;/b&gt;)
&lt;b&gt;X&apos;&apos;&lt;/b&gt; = &lt;b&gt;Xl&lt;/b&gt; + &lt;b&gt;Xm&lt;/b&gt; * &lt;b&gt;Xlr1&lt;/b&gt;* &lt;b&gt;Xlr2&lt;/b&gt; / (&lt;b&gt;Xm&lt;/b&gt; * &lt;b&gt;Xlr1&lt;/b&gt; + &lt;b&gt;Xm&lt;/b&gt; * &lt;b&gt;Xlr2&lt;/b&gt; + &lt;b&gt;Xlr1&lt;/b&gt; * &lt;b&gt;Xlr2&lt;/b&gt;)
&lt;b&gt;T&apos;o&lt;/b&gt; = (&lt;b&gt;Xm&lt;/b&gt; + &lt;b&gt;Xlr1&lt;/b&gt;) / (&lt;b&gt;omega&lt;/b&gt;&lt;b&gt;&lt;sub&gt;0&lt;/sub&gt;&lt;/b&gt; * &lt;b&gt;Rr1&lt;/b&gt;)
&lt;b&gt;T&apos;&apos;o&lt;/b&gt; = (&lt;b&gt;Xm&lt;/b&gt; * &lt;b&gt;Xlr1&lt;/b&gt; + &lt;b&gt;Xm&lt;/b&gt; * &lt;b&gt;Xlr2&lt;/b&gt; + &lt;b&gt;Xlr1&lt;/b&gt; * &lt;b&gt;Xlr2&lt;/b&gt;) / (&lt;b&gt;omega&lt;/b&gt;&lt;b&gt;&lt;sub&gt;0&lt;/sub&gt;&lt;/b&gt; * &lt;b&gt;Rr2&lt;/b&gt; * (&lt;b&gt;Xm &lt;/b&gt;+ &lt;b&gt;Xlr1&lt;/b&gt;)
&lt;b&gt;
&lt;/b&gt;Same equations using CIM attributes from AsynchronousMachineTimeConstantReactance class on left of = sign and AsynchronousMachineEquivalentCircuit class on right (except as noted):
xs = xm + RotatingMachineDynamics.statorLeakageReactance
xp = RotatingMachineDynamics.statorLeakageReactance + xm * xlr1 / (xm + xlr1)
xpp = RotatingMachineDynamics.statorLeakageReactance + xm * xlr1* xlr2 / (xm * xlr1 + xm * xlr2 + xlr1 * xlr2)
tpo = (xm + xlr1) / (2*pi*nominal frequency * rr1)
tppo = (xm * xlr1 + xm * xlr2 + xlr1 * xlr2) / (2*pi*nominal frequency * rr2 * (xm + xlr1).</rdfs:comment>
    </owl:Class>
    


    <!-- https://w3id.org/netbeheer/referentiemodellen/IECCIM/TC57CIM/IEC61970/Dynamics/StandardModels/AsynchronousMachineDynamics#AsynchronousMachineTimeConstantReactance -->


    <owl:Class rdf:about="https://w3id.org/netbeheer/referentiemodellen/IECCIM/TC57CIM/IEC61970/Dynamics/StandardModels/AsynchronousMachineDynamics#AsynchronousMachineTimeConstantReactance">
        <rdfs:subClassOf rdf:resource="https://w3id.org/netbeheer/referentiemodellen/IECCIM/TC57CIM/IEC61970/Dynamics/StandardModels/AsynchronousMachineDynamics#AsynchronousMachineDynamics"/>
        <rdfs:subClassOf>
            <owl:Restriction>
                <owl:onProperty rdf:resource="https://w3id.org/netbeheer/referentiemodellen/IECCIM/TC57CIM/IEC61970/Dynamics/StandardModels/AsynchronousMachineDynamics#AsynchronousMachineTimeConstantReactance_tpo"/>
                <owl:minQualifiedCardinality rdf:datatype="http://www.w3.org/2001/XMLSchema#nonNegativeInteger">0</owl:minQualifiedCardinality>
                <owl:onClass rdf:resource="https://w3id.org/netbeheer/referentiemodellen/IECCIM/TC57CIM/IEC61970/Base/Domain#Seconds"/>
            </owl:Restriction>
        </rdfs:subClassOf>
        <rdfs:subClassOf>
            <owl:Restriction>
                <owl:onProperty rdf:resource="https://w3id.org/netbeheer/referentiemodellen/IECCIM/TC57CIM/IEC61970/Dynamics/StandardModels/AsynchronousMachineDynamics#AsynchronousMachineTimeConstantReactance_tppo"/>
                <owl:minQualifiedCardinality rdf:datatype="http://www.w3.org/2001/XMLSchema#nonNegativeInteger">0</owl:minQualifiedCardinality>
                <owl:onClass rdf:resource="https://w3id.org/netbeheer/referentiemodellen/IECCIM/TC57CIM/IEC61970/Base/Domain#Seconds"/>
            </owl:Restriction>
        </rdfs:subClassOf>
        <rdfs:subClassOf>
            <owl:Restriction>
                <owl:onProperty rdf:resource="https://w3id.org/netbeheer/referentiemodellen/IECCIM/TC57CIM/IEC61970/Dynamics/StandardModels/AsynchronousMachineDynamics#AsynchronousMachineTimeConstantReactance_xp"/>
                <owl:minQualifiedCardinality rdf:datatype="http://www.w3.org/2001/XMLSchema#nonNegativeInteger">0</owl:minQualifiedCardinality>
                <owl:onClass rdf:resource="https://w3id.org/netbeheer/referentiemodellen/IECCIM/TC57CIM/IEC61970/Base/Domain#PU"/>
            </owl:Restriction>
        </rdfs:subClassOf>
        <rdfs:subClassOf>
            <owl:Restriction>
                <owl:onProperty rdf:resource="https://w3id.org/netbeheer/referentiemodellen/IECCIM/TC57CIM/IEC61970/Dynamics/StandardModels/AsynchronousMachineDynamics#AsynchronousMachineTimeConstantReactance_xpp"/>
                <owl:minQualifiedCardinality rdf:datatype="http://www.w3.org/2001/XMLSchema#nonNegativeInteger">0</owl:minQualifiedCardinality>
                <owl:onClass rdf:resource="https://w3id.org/netbeheer/referentiemodellen/IECCIM/TC57CIM/IEC61970/Base/Domain#PU"/>
            </owl:Restriction>
        </rdfs:subClassOf>
        <rdfs:subClassOf>
            <owl:Restriction>
                <owl:onProperty rdf:resource="https://w3id.org/netbeheer/referentiemodellen/IECCIM/TC57CIM/IEC61970/Dynamics/StandardModels/AsynchronousMachineDynamics#AsynchronousMachineTimeConstantReactance_xs"/>
                <owl:minQualifiedCardinality rdf:datatype="http://www.w3.org/2001/XMLSchema#nonNegativeInteger">0</owl:minQualifiedCardinality>
                <owl:onClass rdf:resource="https://w3id.org/netbeheer/referentiemodellen/IECCIM/TC57CIM/IEC61970/Base/Domain#PU"/>
            </owl:Restriction>
        </rdfs:subClassOf>
        <rdfs:subClassOf>
            <owl:Restriction>
                <owl:onProperty rdf:resource="https://w3id.org/netbeheer/referentiemodellen/IECCIM/TC57CIM/IEC61970/Dynamics/StandardModels/AsynchronousMachineDynamics#AsynchronousMachineTimeConstantReactance_tpo"/>
                <owl:maxQualifiedCardinality rdf:datatype="http://www.w3.org/2001/XMLSchema#nonNegativeInteger">1</owl:maxQualifiedCardinality>
                <owl:onClass rdf:resource="https://w3id.org/netbeheer/referentiemodellen/IECCIM/TC57CIM/IEC61970/Base/Domain#Seconds"/>
            </owl:Restriction>
        </rdfs:subClassOf>
        <rdfs:subClassOf>
            <owl:Restriction>
                <owl:onProperty rdf:resource="https://w3id.org/netbeheer/referentiemodellen/IECCIM/TC57CIM/IEC61970/Dynamics/StandardModels/AsynchronousMachineDynamics#AsynchronousMachineTimeConstantReactance_tppo"/>
                <owl:maxQualifiedCardinality rdf:datatype="http://www.w3.org/2001/XMLSchema#nonNegativeInteger">1</owl:maxQualifiedCardinality>
                <owl:onClass rdf:resource="https://w3id.org/netbeheer/referentiemodellen/IECCIM/TC57CIM/IEC61970/Base/Domain#Seconds"/>
            </owl:Restriction>
        </rdfs:subClassOf>
        <rdfs:subClassOf>
            <owl:Restriction>
                <owl:onProperty rdf:resource="https://w3id.org/netbeheer/referentiemodellen/IECCIM/TC57CIM/IEC61970/Dynamics/StandardModels/AsynchronousMachineDynamics#AsynchronousMachineTimeConstantReactance_xp"/>
                <owl:maxQualifiedCardinality rdf:datatype="http://www.w3.org/2001/XMLSchema#nonNegativeInteger">1</owl:maxQualifiedCardinality>
                <owl:onClass rdf:resource="https://w3id.org/netbeheer/referentiemodellen/IECCIM/TC57CIM/IEC61970/Base/Domain#PU"/>
            </owl:Restriction>
        </rdfs:subClassOf>
        <rdfs:subClassOf>
            <owl:Restriction>
                <owl:onProperty rdf:resource="https://w3id.org/netbeheer/referentiemodellen/IECCIM/TC57CIM/IEC61970/Dynamics/StandardModels/AsynchronousMachineDynamics#AsynchronousMachineTimeConstantReactance_xpp"/>
                <owl:maxQualifiedCardinality rdf:datatype="http://www.w3.org/2001/XMLSchema#nonNegativeInteger">1</owl:maxQualifiedCardinality>
                <owl:onClass rdf:resource="https://w3id.org/netbeheer/referentiemodellen/IECCIM/TC57CIM/IEC61970/Base/Domain#PU"/>
            </owl:Restriction>
        </rdfs:subClassOf>
        <rdfs:subClassOf>
            <owl:Restriction>
                <owl:onProperty rdf:resource="https://w3id.org/netbeheer/referentiemodellen/IECCIM/TC57CIM/IEC61970/Dynamics/StandardModels/AsynchronousMachineDynamics#AsynchronousMachineTimeConstantReactance_xs"/>
                <owl:maxQualifiedCardinality rdf:datatype="http://www.w3.org/2001/XMLSchema#nonNegativeInteger">1</owl:maxQualifiedCardinality>
                <owl:onClass rdf:resource="https://w3id.org/netbeheer/referentiemodellen/IECCIM/TC57CIM/IEC61970/Base/Domain#PU"/>
            </owl:Restriction>
        </rdfs:subClassOf>
        <rdfs:comment>&lt;b&gt;Parameter Notes:&lt;/b&gt;
&lt;ol&gt;
 &lt;li&gt;If &lt;b&gt;X&apos;&apos;&lt;/b&gt; = &lt;b&gt;X&apos;&lt;/b&gt;, a single cage (one equivalent rotor winding per axis) is modelled.&lt;/li&gt;
 &lt;li&gt;The “p” in the attribute names is a substitution for a “prime” in the usual parameter notation, e.g. tpo refers to T&apos;o.&lt;/li&gt;
&lt;/ol&gt;

The parameters used for models expressed in time constant reactance form include:
&lt;ul&gt;
 &lt;li&gt;RotatingMachine.ratedS (MVAbase)&lt;/li&gt;
 &lt;li&gt;RotatingMachineDynamics.damping (D)&lt;/li&gt;
 &lt;li&gt;RotatingMachineDynamics.inertia (H)&lt;/li&gt;
 &lt;li&gt;RotatingMachineDynamics.saturationFactor (S1)&lt;/li&gt;
 &lt;li&gt;RotatingMachineDynamics.saturationFactor120 (S12)&lt;/li&gt;
 &lt;li&gt;RotatingMachineDynamics.statorLeakageReactance (Xl)&lt;/li&gt;
 &lt;li&gt;RotatingMachineDynamics.statorResistance (Rs)&lt;/li&gt;
 &lt;li&gt;.xs (Xs)&lt;/li&gt;
 &lt;li&gt;.xp (X&apos;)&lt;/li&gt;
 &lt;li&gt;.xpp (X&apos;&apos;)&lt;/li&gt;
 &lt;li&gt;.tpo (T&apos;o)&lt;/li&gt;
 &lt;li&gt;.tppo (T&apos;&apos;o).&lt;/li&gt;
&lt;/ul&gt;</rdfs:comment>
    </owl:Class>
    


    <!-- https://w3id.org/netbeheer/referentiemodellen/IECCIM/TC57CIM/IEC61970/Dynamics/StandardModels/MechanicalLoadDynamics#MechanicalLoadDynamics -->


    <owl:Class rdf:about="https://w3id.org/netbeheer/referentiemodellen/IECCIM/TC57CIM/IEC61970/Dynamics/StandardModels/MechanicalLoadDynamics#MechanicalLoadDynamics">
        <rdfs:subClassOf>
            <owl:Restriction>
                <owl:onProperty rdf:resource="https://w3id.org/netbeheer/referentiemodellen/IECCIM/TC57CIM/IEC61970/Dynamics/StandardModels/AsynchronousMachineDynamics#MechanicalLoadDynamics_AsynchronousMachineDynamics"/>
                <owl:minQualifiedCardinality rdf:datatype="http://www.w3.org/2001/XMLSchema#nonNegativeInteger">0</owl:minQualifiedCardinality>
                <owl:onClass rdf:resource="https://w3id.org/netbeheer/referentiemodellen/IECCIM/TC57CIM/IEC61970/Dynamics/StandardModels/MechanicalLoadDynamics#MechanicalLoadDynamics"/>
            </owl:Restriction>
        </rdfs:subClassOf>
        <rdfs:subClassOf>
            <owl:Restriction>
                <owl:onProperty rdf:resource="https://w3id.org/netbeheer/referentiemodellen/IECCIM/TC57CIM/IEC61970/Dynamics/StandardModels/AsynchronousMachineDynamics#MechanicalLoadDynamics_AsynchronousMachineDynamics"/>
                <owl:maxQualifiedCardinality rdf:datatype="http://www.w3.org/2001/XMLSchema#nonNegativeInteger">1</owl:maxQualifiedCardinality>
                <owl:onClass rdf:resource="https://w3id.org/netbeheer/referentiemodellen/IECCIM/TC57CIM/IEC61970/Dynamics/StandardModels/MechanicalLoadDynamics#MechanicalLoadDynamics"/>
            </owl:Restriction>
        </rdfs:subClassOf>
    </owl:Class>
    


    <!-- https://w3id.org/netbeheer/referentiemodellen/IECCIM/TC57CIM/IEC61970/Dynamics/StandardModels/TurbineGovernorDynamics#TurbineGovernorDynamics -->


    <owl:Class rdf:about="https://w3id.org/netbeheer/referentiemodellen/IECCIM/TC57CIM/IEC61970/Dynamics/StandardModels/TurbineGovernorDynamics#TurbineGovernorDynamics">
        <rdfs:subClassOf>
            <owl:Restriction>
                <owl:onProperty rdf:resource="https://w3id.org/netbeheer/referentiemodellen/IECCIM/TC57CIM/IEC61970/Dynamics/StandardModels/AsynchronousMachineDynamics#TurbineGovernorDynamics_AsynchronousMachineDynamics"/>
                <owl:minQualifiedCardinality rdf:datatype="http://www.w3.org/2001/XMLSchema#nonNegativeInteger">0</owl:minQualifiedCardinality>
                <owl:onClass rdf:resource="https://w3id.org/netbeheer/referentiemodellen/IECCIM/TC57CIM/IEC61970/Dynamics/StandardModels/TurbineGovernorDynamics#TurbineGovernorDynamics"/>
            </owl:Restriction>
        </rdfs:subClassOf>
        <rdfs:subClassOf>
            <owl:Restriction>
                <owl:onProperty rdf:resource="https://w3id.org/netbeheer/referentiemodellen/IECCIM/TC57CIM/IEC61970/Dynamics/StandardModels/AsynchronousMachineDynamics#TurbineGovernorDynamics_AsynchronousMachineDynamics"/>
                <owl:maxQualifiedCardinality rdf:datatype="http://www.w3.org/2001/XMLSchema#nonNegativeInteger">1</owl:maxQualifiedCardinality>
                <owl:onClass rdf:resource="https://w3id.org/netbeheer/referentiemodellen/IECCIM/TC57CIM/IEC61970/Dynamics/StandardModels/TurbineGovernorDynamics#TurbineGovernorDynamics"/>
            </owl:Restriction>
        </rdfs:subClassOf>
    </owl:Class>
    


    <!-- https://w3id.org/netbeheer/referentiemodellen/IECCIM/TC57CIM/IEC61970/Dynamics/StandardModels/WindDynamics#WindTurbineType1or2Dynamics -->


    <owl:Class rdf:about="https://w3id.org/netbeheer/referentiemodellen/IECCIM/TC57CIM/IEC61970/Dynamics/StandardModels/WindDynamics#WindTurbineType1or2Dynamics">
        <rdfs:subClassOf>
            <owl:Restriction>
                <owl:onProperty rdf:resource="https://w3id.org/netbeheer/referentiemodellen/IECCIM/TC57CIM/IEC61970/Dynamics/StandardModels/AsynchronousMachineDynamics#WindTurbineType1or2Dynamics_AsynchronousMachineDynamics"/>
                <owl:minQualifiedCardinality rdf:datatype="http://www.w3.org/2001/XMLSchema#nonNegativeInteger">0</owl:minQualifiedCardinality>
                <owl:onClass rdf:resource="https://w3id.org/netbeheer/referentiemodellen/IECCIM/TC57CIM/IEC61970/Dynamics/StandardModels/WindDynamics#WindTurbineType1or2Dynamics"/>
            </owl:Restriction>
        </rdfs:subClassOf>
        <rdfs:subClassOf>
            <owl:Restriction>
                <owl:onProperty rdf:resource="https://w3id.org/netbeheer/referentiemodellen/IECCIM/TC57CIM/IEC61970/Dynamics/StandardModels/AsynchronousMachineDynamics#WindTurbineType1or2Dynamics_AsynchronousMachineDynamics"/>
                <owl:maxQualifiedCardinality rdf:datatype="http://www.w3.org/2001/XMLSchema#nonNegativeInteger">1</owl:maxQualifiedCardinality>
                <owl:onClass rdf:resource="https://w3id.org/netbeheer/referentiemodellen/IECCIM/TC57CIM/IEC61970/Dynamics/StandardModels/WindDynamics#WindTurbineType1or2Dynamics"/>
            </owl:Restriction>
        </rdfs:subClassOf>
    </owl:Class>
</rdf:RDF>



<!-- Generated by the OWL API (version 5.1.10.2019-03-12T22:31:15Z) https://github.com/owlcs/owlapi/ -->


