<?xml version="1.0"?>
<rdf:RDF xmlns="https://w3id.org/netbeheer/referentiemodellen/IECCIM/TC57CIM/IEC61970/Dynamics/StandardModels/VoltageCompensatorDynamics#"
     xml:base="https://w3id.org/netbeheer/referentiemodellen/IECCIM/TC57CIM/IEC61970/Dynamics/StandardModels/VoltageCompensatorDynamics"
     xmlns:owl="http://www.w3.org/2002/07/owl#"
     xmlns:rdf="http://www.w3.org/1999/02/22-rdf-syntax-ns#"
     xmlns:xml="http://www.w3.org/XML/1998/namespace"
     xmlns:xsd="http://www.w3.org/2001/XMLSchema#"
     xmlns:rdfs="http://www.w3.org/2000/01/rdf-schema#">
    <owl:Ontology rdf:about="https://w3id.org/netbeheer/referentiemodellen/IECCIM/TC57CIM/IEC61970/Dynamics/StandardModels/VoltageCompensatorDynamics#"/>
    


    <!-- 
    ///////////////////////////////////////////////////////////////////////////////////////
    //
    // Object Properties
    //
    ///////////////////////////////////////////////////////////////////////////////////////
     -->


    


    <!-- https://w3id.org/netbeheer/referentiemodellen/IECCIM/TC57CIM/IEC61970/Dynamics/StandardModels/VoltageCompensatorDynamics#GenICompensationForGenJ_VcompIEEEType2 -->


    <owl:ObjectProperty rdf:about="https://w3id.org/netbeheer/referentiemodellen/IECCIM/TC57CIM/IEC61970/Dynamics/StandardModels/VoltageCompensatorDynamics#GenICompensationForGenJ_VcompIEEEType2">
        <rdfs:domain rdf:resource="https://w3id.org/netbeheer/referentiemodellen/IECCIM/TC57CIM/IEC61970/Dynamics/StandardModels/VoltageCompensatorDynamics#GenICompensationForGenJ"/>
        <rdfs:range rdf:resource="https://w3id.org/netbeheer/referentiemodellen/IECCIM/TC57CIM/IEC61970/Dynamics/StandardModels/VoltageCompensatorDynamics#VCompIEEEType2"/>
        <rdfs:comment>Compensation of this voltage compensator&apos;s generator for current flow out of another generator.The standard IEEE Type 2 voltage compensator of this compensation.</rdfs:comment>
    </owl:ObjectProperty>
    


    <!-- https://w3id.org/netbeheer/referentiemodellen/IECCIM/TC57CIM/IEC61970/Dynamics/StandardModels/VoltageCompensatorDynamics#GenICompensationForGenJ_rcij -->


    <owl:ObjectProperty rdf:about="https://w3id.org/netbeheer/referentiemodellen/IECCIM/TC57CIM/IEC61970/Dynamics/StandardModels/VoltageCompensatorDynamics#GenICompensationForGenJ_rcij">
        <rdfs:domain rdf:resource="https://w3id.org/netbeheer/referentiemodellen/IECCIM/TC57CIM/IEC61970/Dynamics/StandardModels/VoltageCompensatorDynamics#GenICompensationForGenJ"/>
        <rdfs:range rdf:resource="https://w3id.org/netbeheer/referentiemodellen/IECCIM/TC57CIM/IEC61970/Base/Domain#PU"/>
        <rdfs:comment>&lt;font color=&quot;#0f0f0f&quot;&gt;Resistive component of compensation of generator associated with this IEEE Type 2 voltage compensator for current flow out of another generator (Rcij).&lt;/font&gt;</rdfs:comment>
    </owl:ObjectProperty>
    


    <!-- https://w3id.org/netbeheer/referentiemodellen/IECCIM/TC57CIM/IEC61970/Dynamics/StandardModels/VoltageCompensatorDynamics#GenICompensationForGenJ_xcij -->


    <owl:ObjectProperty rdf:about="https://w3id.org/netbeheer/referentiemodellen/IECCIM/TC57CIM/IEC61970/Dynamics/StandardModels/VoltageCompensatorDynamics#GenICompensationForGenJ_xcij">
        <rdfs:domain rdf:resource="https://w3id.org/netbeheer/referentiemodellen/IECCIM/TC57CIM/IEC61970/Dynamics/StandardModels/VoltageCompensatorDynamics#GenICompensationForGenJ"/>
        <rdfs:range rdf:resource="https://w3id.org/netbeheer/referentiemodellen/IECCIM/TC57CIM/IEC61970/Base/Domain#PU"/>
        <rdfs:comment>&lt;font color=&quot;#0f0f0f&quot;&gt;Reactive component of compensation of generator associated with this IEEE Type 2 voltage compensator for current flow out of another generator (Xcij).&lt;/font&gt;</rdfs:comment>
    </owl:ObjectProperty>
    


    <!-- https://w3id.org/netbeheer/referentiemodellen/IECCIM/TC57CIM/IEC61970/Dynamics/StandardModels/VoltageCompensatorDynamics#VCompIEEEType1_rc -->


    <owl:ObjectProperty rdf:about="https://w3id.org/netbeheer/referentiemodellen/IECCIM/TC57CIM/IEC61970/Dynamics/StandardModels/VoltageCompensatorDynamics#VCompIEEEType1_rc">
        <rdfs:domain rdf:resource="https://w3id.org/netbeheer/referentiemodellen/IECCIM/TC57CIM/IEC61970/Dynamics/StandardModels/VoltageCompensatorDynamics#VCompIEEEType1"/>
        <rdfs:range rdf:resource="https://w3id.org/netbeheer/referentiemodellen/IECCIM/TC57CIM/IEC61970/Base/Domain#PU"/>
        <rdfs:comment>&lt;font color=&quot;#0f0f0f&quot;&gt;Resistive component of compensation of a generator (Rc).&lt;/font&gt;</rdfs:comment>
    </owl:ObjectProperty>
    


    <!-- https://w3id.org/netbeheer/referentiemodellen/IECCIM/TC57CIM/IEC61970/Dynamics/StandardModels/VoltageCompensatorDynamics#VCompIEEEType1_tr -->


    <owl:ObjectProperty rdf:about="https://w3id.org/netbeheer/referentiemodellen/IECCIM/TC57CIM/IEC61970/Dynamics/StandardModels/VoltageCompensatorDynamics#VCompIEEEType1_tr">
        <rdfs:domain rdf:resource="https://w3id.org/netbeheer/referentiemodellen/IECCIM/TC57CIM/IEC61970/Dynamics/StandardModels/VoltageCompensatorDynamics#VCompIEEEType1"/>
        <rdfs:range rdf:resource="https://w3id.org/netbeheer/referentiemodellen/IECCIM/TC57CIM/IEC61970/Base/Domain#Seconds"/>
        <rdfs:comment>&lt;font color=&quot;#0f0f0f&quot;&gt;Time constant which is used for the combined voltage sensing and compensation signal (Tr).&lt;/font&gt;</rdfs:comment>
    </owl:ObjectProperty>
    


    <!-- https://w3id.org/netbeheer/referentiemodellen/IECCIM/TC57CIM/IEC61970/Dynamics/StandardModels/VoltageCompensatorDynamics#VCompIEEEType1_xc -->


    <owl:ObjectProperty rdf:about="https://w3id.org/netbeheer/referentiemodellen/IECCIM/TC57CIM/IEC61970/Dynamics/StandardModels/VoltageCompensatorDynamics#VCompIEEEType1_xc">
        <rdfs:domain rdf:resource="https://w3id.org/netbeheer/referentiemodellen/IECCIM/TC57CIM/IEC61970/Dynamics/StandardModels/VoltageCompensatorDynamics#VCompIEEEType1"/>
        <rdfs:range rdf:resource="https://w3id.org/netbeheer/referentiemodellen/IECCIM/TC57CIM/IEC61970/Base/Domain#PU"/>
        <rdfs:comment>&lt;font color=&quot;#0f0f0f&quot;&gt;Reactive component of compensation of a generator (Xc).&lt;/font&gt;</rdfs:comment>
    </owl:ObjectProperty>
    


    <!-- https://w3id.org/netbeheer/referentiemodellen/IECCIM/TC57CIM/IEC61970/Dynamics/StandardModels/VoltageCompensatorDynamics#VCompIEEEType2_GenICompensationForGenJ -->


    <owl:ObjectProperty rdf:about="https://w3id.org/netbeheer/referentiemodellen/IECCIM/TC57CIM/IEC61970/Dynamics/StandardModels/VoltageCompensatorDynamics#VCompIEEEType2_GenICompensationForGenJ">
        <owl:inverseOf rdf:resource="https://w3id.org/netbeheer/referentiemodellen/IECCIM/TC57CIM/IEC61970/Dynamics/StandardModels/VoltageCompensatorDynamics#GenICompensationForGenJ_VcompIEEEType2"/>
        <rdf:type rdf:resource="http://www.w3.org/2002/07/owl#FunctionalProperty"/>
        <rdfs:domain rdf:resource="https://w3id.org/netbeheer/referentiemodellen/IECCIM/TC57CIM/IEC61970/Dynamics/StandardModels/VoltageCompensatorDynamics#VCompIEEEType2"/>
        <rdfs:range rdf:resource="https://w3id.org/netbeheer/referentiemodellen/IECCIM/TC57CIM/IEC61970/Dynamics/StandardModels/VoltageCompensatorDynamics#GenICompensationForGenJ"/>
        <rdfs:comment>Compensation of this voltage compensator&apos;s generator for current flow out of another generator.The standard IEEE Type 2 voltage compensator of this compensation.</rdfs:comment>
    </owl:ObjectProperty>
    


    <!-- https://w3id.org/netbeheer/referentiemodellen/IECCIM/TC57CIM/IEC61970/Dynamics/StandardModels/VoltageCompensatorDynamics#VCompIEEEType2_tr -->


    <owl:ObjectProperty rdf:about="https://w3id.org/netbeheer/referentiemodellen/IECCIM/TC57CIM/IEC61970/Dynamics/StandardModels/VoltageCompensatorDynamics#VCompIEEEType2_tr">
        <rdfs:domain rdf:resource="https://w3id.org/netbeheer/referentiemodellen/IECCIM/TC57CIM/IEC61970/Dynamics/StandardModels/VoltageCompensatorDynamics#VCompIEEEType2"/>
        <rdfs:range rdf:resource="https://w3id.org/netbeheer/referentiemodellen/IECCIM/TC57CIM/IEC61970/Base/Domain#Seconds"/>
        <rdfs:comment>&lt;font color=&quot;#0f0f0f&quot;&gt;Time constant which is used for the combined voltage sensing and compensation signal (Tr).&lt;/font&gt;</rdfs:comment>
    </owl:ObjectProperty>
    


    <!-- 
    ///////////////////////////////////////////////////////////////////////////////////////
    //
    // Classes
    //
    ///////////////////////////////////////////////////////////////////////////////////////
     -->


    


    <!-- https://w3id.org/netbeheer/referentiemodellen/IECCIM/TC57CIM/IEC61970/Base/Core#IdentifiedObject -->


    <owl:Class rdf:about="https://w3id.org/netbeheer/referentiemodellen/IECCIM/TC57CIM/IEC61970/Base/Core#IdentifiedObject"/>
    


    <!-- https://w3id.org/netbeheer/referentiemodellen/IECCIM/TC57CIM/IEC61970/Base/Domain#PU -->


    <owl:Class rdf:about="https://w3id.org/netbeheer/referentiemodellen/IECCIM/TC57CIM/IEC61970/Base/Domain#PU"/>
    


    <!-- https://w3id.org/netbeheer/referentiemodellen/IECCIM/TC57CIM/IEC61970/Base/Domain#Seconds -->


    <owl:Class rdf:about="https://w3id.org/netbeheer/referentiemodellen/IECCIM/TC57CIM/IEC61970/Base/Domain#Seconds"/>
    


    <!-- https://w3id.org/netbeheer/referentiemodellen/IECCIM/TC57CIM/IEC61970/Dynamics/StandardModels#DynamicsFunctionBlock -->


    <owl:Class rdf:about="https://w3id.org/netbeheer/referentiemodellen/IECCIM/TC57CIM/IEC61970/Dynamics/StandardModels#DynamicsFunctionBlock"/>
    


    <!-- https://w3id.org/netbeheer/referentiemodellen/IECCIM/TC57CIM/IEC61970/Dynamics/StandardModels/VoltageCompensatorDynamics#GenICompensationForGenJ -->


    <owl:Class rdf:about="https://w3id.org/netbeheer/referentiemodellen/IECCIM/TC57CIM/IEC61970/Dynamics/StandardModels/VoltageCompensatorDynamics#GenICompensationForGenJ">
        <rdfs:subClassOf rdf:resource="https://w3id.org/netbeheer/referentiemodellen/IECCIM/TC57CIM/IEC61970/Base/Core#IdentifiedObject"/>
        <rdfs:subClassOf>
            <owl:Restriction>
                <owl:onProperty rdf:resource="https://w3id.org/netbeheer/referentiemodellen/IECCIM/TC57CIM/IEC61970/Dynamics/StandardModels/VoltageCompensatorDynamics#GenICompensationForGenJ_VcompIEEEType2"/>
                <owl:minQualifiedCardinality rdf:datatype="http://www.w3.org/2001/XMLSchema#nonNegativeInteger">2</owl:minQualifiedCardinality>
                <owl:onClass rdf:resource="https://w3id.org/netbeheer/referentiemodellen/IECCIM/TC57CIM/IEC61970/Dynamics/StandardModels/VoltageCompensatorDynamics#GenICompensationForGenJ"/>
            </owl:Restriction>
        </rdfs:subClassOf>
        <rdfs:subClassOf>
            <owl:Restriction>
                <owl:onProperty rdf:resource="https://w3id.org/netbeheer/referentiemodellen/IECCIM/TC57CIM/IEC61970/Dynamics/StandardModels/VoltageCompensatorDynamics#GenICompensationForGenJ_rcij"/>
                <owl:minQualifiedCardinality rdf:datatype="http://www.w3.org/2001/XMLSchema#nonNegativeInteger">0</owl:minQualifiedCardinality>
                <owl:onClass rdf:resource="https://w3id.org/netbeheer/referentiemodellen/IECCIM/TC57CIM/IEC61970/Base/Domain#PU"/>
            </owl:Restriction>
        </rdfs:subClassOf>
        <rdfs:subClassOf>
            <owl:Restriction>
                <owl:onProperty rdf:resource="https://w3id.org/netbeheer/referentiemodellen/IECCIM/TC57CIM/IEC61970/Dynamics/StandardModels/VoltageCompensatorDynamics#GenICompensationForGenJ_xcij"/>
                <owl:minQualifiedCardinality rdf:datatype="http://www.w3.org/2001/XMLSchema#nonNegativeInteger">0</owl:minQualifiedCardinality>
                <owl:onClass rdf:resource="https://w3id.org/netbeheer/referentiemodellen/IECCIM/TC57CIM/IEC61970/Base/Domain#PU"/>
            </owl:Restriction>
        </rdfs:subClassOf>
        <rdfs:subClassOf>
            <owl:Restriction>
                <owl:onProperty rdf:resource="https://w3id.org/netbeheer/referentiemodellen/IECCIM/TC57CIM/IEC61970/Dynamics/StandardModels/VoltageCompensatorDynamics#GenICompensationForGenJ_rcij"/>
                <owl:maxQualifiedCardinality rdf:datatype="http://www.w3.org/2001/XMLSchema#nonNegativeInteger">1</owl:maxQualifiedCardinality>
                <owl:onClass rdf:resource="https://w3id.org/netbeheer/referentiemodellen/IECCIM/TC57CIM/IEC61970/Base/Domain#PU"/>
            </owl:Restriction>
        </rdfs:subClassOf>
        <rdfs:subClassOf>
            <owl:Restriction>
                <owl:onProperty rdf:resource="https://w3id.org/netbeheer/referentiemodellen/IECCIM/TC57CIM/IEC61970/Dynamics/StandardModels/VoltageCompensatorDynamics#GenICompensationForGenJ_xcij"/>
                <owl:maxQualifiedCardinality rdf:datatype="http://www.w3.org/2001/XMLSchema#nonNegativeInteger">1</owl:maxQualifiedCardinality>
                <owl:onClass rdf:resource="https://w3id.org/netbeheer/referentiemodellen/IECCIM/TC57CIM/IEC61970/Base/Domain#PU"/>
            </owl:Restriction>
        </rdfs:subClassOf>
        <rdfs:comment>This class provides the resistive and reactive components of compensation for the generator associated with the IEEE Type 2 voltage compensator for current flow out of one of the other generators in the interconnection.</rdfs:comment>
    </owl:Class>
    


    <!-- https://w3id.org/netbeheer/referentiemodellen/IECCIM/TC57CIM/IEC61970/Dynamics/StandardModels/VoltageCompensatorDynamics#VCompIEEEType1 -->


    <owl:Class rdf:about="https://w3id.org/netbeheer/referentiemodellen/IECCIM/TC57CIM/IEC61970/Dynamics/StandardModels/VoltageCompensatorDynamics#VCompIEEEType1">
        <rdfs:subClassOf rdf:resource="https://w3id.org/netbeheer/referentiemodellen/IECCIM/TC57CIM/IEC61970/Dynamics/StandardModels/VoltageCompensatorDynamics#VoltageCompensatorDynamics"/>
        <rdfs:subClassOf>
            <owl:Restriction>
                <owl:onProperty rdf:resource="https://w3id.org/netbeheer/referentiemodellen/IECCIM/TC57CIM/IEC61970/Dynamics/StandardModels/VoltageCompensatorDynamics#VCompIEEEType1_rc"/>
                <owl:minQualifiedCardinality rdf:datatype="http://www.w3.org/2001/XMLSchema#nonNegativeInteger">0</owl:minQualifiedCardinality>
                <owl:onClass rdf:resource="https://w3id.org/netbeheer/referentiemodellen/IECCIM/TC57CIM/IEC61970/Base/Domain#PU"/>
            </owl:Restriction>
        </rdfs:subClassOf>
        <rdfs:subClassOf>
            <owl:Restriction>
                <owl:onProperty rdf:resource="https://w3id.org/netbeheer/referentiemodellen/IECCIM/TC57CIM/IEC61970/Dynamics/StandardModels/VoltageCompensatorDynamics#VCompIEEEType1_tr"/>
                <owl:minQualifiedCardinality rdf:datatype="http://www.w3.org/2001/XMLSchema#nonNegativeInteger">0</owl:minQualifiedCardinality>
                <owl:onClass rdf:resource="https://w3id.org/netbeheer/referentiemodellen/IECCIM/TC57CIM/IEC61970/Base/Domain#Seconds"/>
            </owl:Restriction>
        </rdfs:subClassOf>
        <rdfs:subClassOf>
            <owl:Restriction>
                <owl:onProperty rdf:resource="https://w3id.org/netbeheer/referentiemodellen/IECCIM/TC57CIM/IEC61970/Dynamics/StandardModels/VoltageCompensatorDynamics#VCompIEEEType1_xc"/>
                <owl:minQualifiedCardinality rdf:datatype="http://www.w3.org/2001/XMLSchema#nonNegativeInteger">0</owl:minQualifiedCardinality>
                <owl:onClass rdf:resource="https://w3id.org/netbeheer/referentiemodellen/IECCIM/TC57CIM/IEC61970/Base/Domain#PU"/>
            </owl:Restriction>
        </rdfs:subClassOf>
        <rdfs:subClassOf>
            <owl:Restriction>
                <owl:onProperty rdf:resource="https://w3id.org/netbeheer/referentiemodellen/IECCIM/TC57CIM/IEC61970/Dynamics/StandardModels/VoltageCompensatorDynamics#VCompIEEEType1_rc"/>
                <owl:maxQualifiedCardinality rdf:datatype="http://www.w3.org/2001/XMLSchema#nonNegativeInteger">1</owl:maxQualifiedCardinality>
                <owl:onClass rdf:resource="https://w3id.org/netbeheer/referentiemodellen/IECCIM/TC57CIM/IEC61970/Base/Domain#PU"/>
            </owl:Restriction>
        </rdfs:subClassOf>
        <rdfs:subClassOf>
            <owl:Restriction>
                <owl:onProperty rdf:resource="https://w3id.org/netbeheer/referentiemodellen/IECCIM/TC57CIM/IEC61970/Dynamics/StandardModels/VoltageCompensatorDynamics#VCompIEEEType1_tr"/>
                <owl:maxQualifiedCardinality rdf:datatype="http://www.w3.org/2001/XMLSchema#nonNegativeInteger">1</owl:maxQualifiedCardinality>
                <owl:onClass rdf:resource="https://w3id.org/netbeheer/referentiemodellen/IECCIM/TC57CIM/IEC61970/Base/Domain#Seconds"/>
            </owl:Restriction>
        </rdfs:subClassOf>
        <rdfs:subClassOf>
            <owl:Restriction>
                <owl:onProperty rdf:resource="https://w3id.org/netbeheer/referentiemodellen/IECCIM/TC57CIM/IEC61970/Dynamics/StandardModels/VoltageCompensatorDynamics#VCompIEEEType1_xc"/>
                <owl:maxQualifiedCardinality rdf:datatype="http://www.w3.org/2001/XMLSchema#nonNegativeInteger">1</owl:maxQualifiedCardinality>
                <owl:onClass rdf:resource="https://w3id.org/netbeheer/referentiemodellen/IECCIM/TC57CIM/IEC61970/Base/Domain#PU"/>
            </owl:Restriction>
        </rdfs:subClassOf>
        <rdfs:comment>&lt;font color=&quot;#0f0f0f&quot;&gt;The class represents the terminal voltage transducer and the load compensator as defined in the IEEE Std 421.5-2005, Section 4. This model is common to all excitation system models described in the IEEE Standard. &lt;/font&gt;

Reference: IEEE Standard 421.5-2005 Section 4. </rdfs:comment>
    </owl:Class>
    


    <!-- https://w3id.org/netbeheer/referentiemodellen/IECCIM/TC57CIM/IEC61970/Dynamics/StandardModels/VoltageCompensatorDynamics#VCompIEEEType2 -->


    <owl:Class rdf:about="https://w3id.org/netbeheer/referentiemodellen/IECCIM/TC57CIM/IEC61970/Dynamics/StandardModels/VoltageCompensatorDynamics#VCompIEEEType2">
        <rdfs:subClassOf rdf:resource="https://w3id.org/netbeheer/referentiemodellen/IECCIM/TC57CIM/IEC61970/Dynamics/StandardModels/VoltageCompensatorDynamics#VoltageCompensatorDynamics"/>
        <rdfs:subClassOf>
            <owl:Restriction>
                <owl:onProperty rdf:resource="https://w3id.org/netbeheer/referentiemodellen/IECCIM/TC57CIM/IEC61970/Dynamics/StandardModels/VoltageCompensatorDynamics#VCompIEEEType2_tr"/>
                <owl:minQualifiedCardinality rdf:datatype="http://www.w3.org/2001/XMLSchema#nonNegativeInteger">0</owl:minQualifiedCardinality>
                <owl:onClass rdf:resource="https://w3id.org/netbeheer/referentiemodellen/IECCIM/TC57CIM/IEC61970/Base/Domain#Seconds"/>
            </owl:Restriction>
        </rdfs:subClassOf>
        <rdfs:subClassOf>
            <owl:Restriction>
                <owl:onProperty rdf:resource="https://w3id.org/netbeheer/referentiemodellen/IECCIM/TC57CIM/IEC61970/Dynamics/StandardModels/VoltageCompensatorDynamics#VCompIEEEType2_GenICompensationForGenJ"/>
                <owl:qualifiedCardinality rdf:datatype="http://www.w3.org/2001/XMLSchema#nonNegativeInteger">1</owl:qualifiedCardinality>
                <owl:onClass rdf:resource="https://w3id.org/netbeheer/referentiemodellen/IECCIM/TC57CIM/IEC61970/Dynamics/StandardModels/VoltageCompensatorDynamics#VCompIEEEType2"/>
            </owl:Restriction>
        </rdfs:subClassOf>
        <rdfs:subClassOf>
            <owl:Restriction>
                <owl:onProperty rdf:resource="https://w3id.org/netbeheer/referentiemodellen/IECCIM/TC57CIM/IEC61970/Dynamics/StandardModels/VoltageCompensatorDynamics#VCompIEEEType2_tr"/>
                <owl:maxQualifiedCardinality rdf:datatype="http://www.w3.org/2001/XMLSchema#nonNegativeInteger">1</owl:maxQualifiedCardinality>
                <owl:onClass rdf:resource="https://w3id.org/netbeheer/referentiemodellen/IECCIM/TC57CIM/IEC61970/Base/Domain#Seconds"/>
            </owl:Restriction>
        </rdfs:subClassOf>
        <rdfs:comment>&lt;font color=&quot;#0f0f0f&quot;&gt;The class represents the terminal voltage transducer and the load compensator as defined in the IEEE Std 421.5-2005, Section 4. This model is designed to cover the following types of compensation: &lt;/font&gt;
&lt;ul&gt;
 &lt;li&gt;&lt;font color=&quot;#0f0f0f&quot;&gt;reactive droop&lt;/font&gt;&lt;/li&gt;
 &lt;li&gt;&lt;font color=&quot;#0f0f0f&quot;&gt;transformer-drop or line-drop compensation&lt;/font&gt;&lt;/li&gt;
 &lt;li&gt;&lt;font color=&quot;#0f0f0f&quot;&gt;reactive differential compensation known also as cross-current compensation.&lt;/font&gt;&lt;/li&gt;
&lt;/ul&gt;
&lt;font color=&quot;#0f0f0f&quot;&gt;
&lt;/font&gt;&lt;font color=&quot;#0f0f0f&quot;&gt;Reference: IEEE Standard 421.5-2005, Section 4.&lt;/font&gt;</rdfs:comment>
    </owl:Class>
    


    <!-- https://w3id.org/netbeheer/referentiemodellen/IECCIM/TC57CIM/IEC61970/Dynamics/StandardModels/VoltageCompensatorDynamics#VoltageCompensatorDynamics -->


    <owl:Class rdf:about="https://w3id.org/netbeheer/referentiemodellen/IECCIM/TC57CIM/IEC61970/Dynamics/StandardModels/VoltageCompensatorDynamics#VoltageCompensatorDynamics">
        <rdfs:subClassOf rdf:resource="https://w3id.org/netbeheer/referentiemodellen/IECCIM/TC57CIM/IEC61970/Dynamics/StandardModels#DynamicsFunctionBlock"/>
        <rdfs:comment>Voltage compensator function block whose behaviour is described by reference to a standard model &lt;font color=&quot;#0f0f0f&quot;&gt;or by definition of a user-defined model.&lt;/font&gt;</rdfs:comment>
    </owl:Class>
</rdf:RDF>



<!-- Generated by the OWL API (version 5.1.10.2019-03-12T22:31:15Z) https://github.com/owlcs/owlapi/ -->


