<?xml version="1.0"?>
<rdf:RDF xmlns="https://w3id.org/netbeheer/referentiemodellen/IECCIM/TC57CIM/IEC61970/Dynamics/StandardModels/WindDynamics#"
     xml:base="https://w3id.org/netbeheer/referentiemodellen/IECCIM/TC57CIM/IEC61970/Dynamics/StandardModels/WindDynamics"
     xmlns:owl="http://www.w3.org/2002/07/owl#"
     xmlns:rdf="http://www.w3.org/1999/02/22-rdf-syntax-ns#"
     xmlns:xml="http://www.w3.org/XML/1998/namespace"
     xmlns:xsd="http://www.w3.org/2001/XMLSchema#"
     xmlns:rdfs="http://www.w3.org/2000/01/rdf-schema#">
    <owl:Ontology rdf:about="https://w3id.org/netbeheer/referentiemodellen/IECCIM/TC57CIM/IEC61970/Dynamics/StandardModels/WindDynamics#"/>
    


    <!-- 
    ///////////////////////////////////////////////////////////////////////////////////////
    //
    // Datatypes
    //
    ///////////////////////////////////////////////////////////////////////////////////////
     -->


    


    <!-- https://w3id.org/netbeheer/referentiemodellen/IECCIM/TC57CIM/IEC61970/Dynamics/StandardModels/WindDynamics#WindLVRTQcontrolModesKind -->


    <rdfs:Datatype rdf:about="https://w3id.org/netbeheer/referentiemodellen/IECCIM/TC57CIM/IEC61970/Dynamics/StandardModels/WindDynamics#WindLVRTQcontrolModesKind">
        <owl:equivalentClass>
            <rdfs:Datatype>
                <owl:oneOf>
                    <rdf:Description>
                        <rdf:type rdf:resource="http://www.w3.org/1999/02/22-rdf-syntax-ns#List"/>
                        <rdf:first>mode1</rdf:first>
                        <rdf:rest>
                            <rdf:Description>
                                <rdf:type rdf:resource="http://www.w3.org/1999/02/22-rdf-syntax-ns#List"/>
                                <rdf:first>mode2</rdf:first>
                                <rdf:rest>
                                    <rdf:Description>
                                        <rdf:type rdf:resource="http://www.w3.org/1999/02/22-rdf-syntax-ns#List"/>
                                        <rdf:first>mode3</rdf:first>
                                        <rdf:rest rdf:resource="http://www.w3.org/1999/02/22-rdf-syntax-ns#nil"/>
                                    </rdf:Description>
                                </rdf:rest>
                            </rdf:Description>
                        </rdf:rest>
                    </rdf:Description>
                </owl:oneOf>
            </rdfs:Datatype>
        </owl:equivalentClass>
    </rdfs:Datatype>
    


    <!-- https://w3id.org/netbeheer/referentiemodellen/IECCIM/TC57CIM/IEC61970/Dynamics/StandardModels/WindDynamics#WindLookupTableFunctionKind -->


    <rdfs:Datatype rdf:about="https://w3id.org/netbeheer/referentiemodellen/IECCIM/TC57CIM/IEC61970/Dynamics/StandardModels/WindDynamics#WindLookupTableFunctionKind">
        <owl:equivalentClass>
            <rdfs:Datatype>
                <owl:oneOf>
                    <rdf:Description>
                        <rdf:type rdf:resource="http://www.w3.org/1999/02/22-rdf-syntax-ns#List"/>
                        <rdf:first>fdpf</rdf:first>
                        <rdf:rest>
                            <rdf:Description>
                                <rdf:type rdf:resource="http://www.w3.org/1999/02/22-rdf-syntax-ns#List"/>
                                <rdf:first>fpomega</rdf:first>
                                <rdf:rest>
                                    <rdf:Description>
                                        <rdf:type rdf:resource="http://www.w3.org/1999/02/22-rdf-syntax-ns#List"/>
                                        <rdf:first>fpslip</rdf:first>
                                        <rdf:rest>
                                            <rdf:Description>
                                                <rdf:type rdf:resource="http://www.w3.org/1999/02/22-rdf-syntax-ns#List"/>
                                                <rdf:first>ipvdl</rdf:first>
                                                <rdf:rest>
                                                    <rdf:Description>
                                                        <rdf:type rdf:resource="http://www.w3.org/1999/02/22-rdf-syntax-ns#List"/>
                                                        <rdf:first>iqvdl</rdf:first>
                                                        <rdf:rest rdf:resource="http://www.w3.org/1999/02/22-rdf-syntax-ns#nil"/>
                                                    </rdf:Description>
                                                </rdf:rest>
                                            </rdf:Description>
                                        </rdf:rest>
                                    </rdf:Description>
                                </rdf:rest>
                            </rdf:Description>
                        </rdf:rest>
                    </rdf:Description>
                </owl:oneOf>
            </rdfs:Datatype>
        </owl:equivalentClass>
    </rdfs:Datatype>
    


    <!-- https://w3id.org/netbeheer/referentiemodellen/IECCIM/TC57CIM/IEC61970/Dynamics/StandardModels/WindDynamics#WindQcontrolModesKind -->


    <rdfs:Datatype rdf:about="https://w3id.org/netbeheer/referentiemodellen/IECCIM/TC57CIM/IEC61970/Dynamics/StandardModels/WindDynamics#WindQcontrolModesKind">
        <owl:equivalentClass>
            <rdfs:Datatype>
                <owl:oneOf>
                    <rdf:Description>
                        <rdf:type rdf:resource="http://www.w3.org/1999/02/22-rdf-syntax-ns#List"/>
                        <rdf:first>openLoopReactivePower</rdf:first>
                        <rdf:rest>
                            <rdf:Description>
                                <rdf:type rdf:resource="http://www.w3.org/1999/02/22-rdf-syntax-ns#List"/>
                                <rdf:first>powerFactor</rdf:first>
                                <rdf:rest>
                                    <rdf:Description>
                                        <rdf:type rdf:resource="http://www.w3.org/1999/02/22-rdf-syntax-ns#List"/>
                                        <rdf:first>reactivePower</rdf:first>
                                        <rdf:rest>
                                            <rdf:Description>
                                                <rdf:type rdf:resource="http://www.w3.org/1999/02/22-rdf-syntax-ns#List"/>
                                                <rdf:first>voltage</rdf:first>
                                                <rdf:rest rdf:resource="http://www.w3.org/1999/02/22-rdf-syntax-ns#nil"/>
                                            </rdf:Description>
                                        </rdf:rest>
                                    </rdf:Description>
                                </rdf:rest>
                            </rdf:Description>
                        </rdf:rest>
                    </rdf:Description>
                </owl:oneOf>
            </rdfs:Datatype>
        </owl:equivalentClass>
    </rdfs:Datatype>
    


    <!-- 
    ///////////////////////////////////////////////////////////////////////////////////////
    //
    // Object Properties
    //
    ///////////////////////////////////////////////////////////////////////////////////////
     -->


    


    <!-- https://w3id.org/netbeheer/referentiemodellen/IECCIM/TC57CIM/IEC61970/Dynamics/StandardModels/WindDynamics#WindAeroConstIEC_WindGenTurbineType1IEC -->


    <owl:ObjectProperty rdf:about="https://w3id.org/netbeheer/referentiemodellen/IECCIM/TC57CIM/IEC61970/Dynamics/StandardModels/WindDynamics#WindAeroConstIEC_WindGenTurbineType1IEC">
        <rdf:type rdf:resource="http://www.w3.org/2002/07/owl#FunctionalProperty"/>
        <rdfs:domain rdf:resource="https://w3id.org/netbeheer/referentiemodellen/IECCIM/TC57CIM/IEC61970/Dynamics/StandardModels/WindDynamics#WindAeroConstIEC"/>
        <rdfs:range rdf:resource="https://w3id.org/netbeheer/referentiemodellen/IECCIM/TC57CIM/IEC61970/Dynamics/StandardModels/WindDynamics#WindGenTurbineType1IEC"/>
        <rdfs:comment>Wind aerodynamic model associated with this wind turbine type 1 model.Wind turbine type 1 model with which this wind aerodynamic model is associated.</rdfs:comment>
    </owl:ObjectProperty>
    


    <!-- https://w3id.org/netbeheer/referentiemodellen/IECCIM/TC57CIM/IEC61970/Dynamics/StandardModels/WindDynamics#WindAeroLinearIEC_WindGenTurbineType3IEC -->


    <owl:ObjectProperty rdf:about="https://w3id.org/netbeheer/referentiemodellen/IECCIM/TC57CIM/IEC61970/Dynamics/StandardModels/WindDynamics#WindAeroLinearIEC_WindGenTurbineType3IEC">
        <rdf:type rdf:resource="http://www.w3.org/2002/07/owl#FunctionalProperty"/>
        <rdfs:domain rdf:resource="https://w3id.org/netbeheer/referentiemodellen/IECCIM/TC57CIM/IEC61970/Dynamics/StandardModels/WindDynamics#WindAeroLinearIEC"/>
        <rdfs:range rdf:resource="https://w3id.org/netbeheer/referentiemodellen/IECCIM/TC57CIM/IEC61970/Dynamics/StandardModels/WindDynamics#WindGenTurbineType3IEC"/>
        <rdfs:comment>Wind aerodynamic model associated with this wind generator type 3 model.Wind generator type 3 model with which this wind aerodynamic model is associated.</rdfs:comment>
    </owl:ObjectProperty>
    


    <!-- https://w3id.org/netbeheer/referentiemodellen/IECCIM/TC57CIM/IEC61970/Dynamics/StandardModels/WindDynamics#WindAeroLinearIEC_dpomega -->


    <owl:ObjectProperty rdf:about="https://w3id.org/netbeheer/referentiemodellen/IECCIM/TC57CIM/IEC61970/Dynamics/StandardModels/WindDynamics#WindAeroLinearIEC_dpomega">
        <rdfs:domain rdf:resource="https://w3id.org/netbeheer/referentiemodellen/IECCIM/TC57CIM/IEC61970/Dynamics/StandardModels/WindDynamics#WindAeroLinearIEC"/>
        <rdfs:range rdf:resource="https://w3id.org/netbeheer/referentiemodellen/IECCIM/TC57CIM/IEC61970/Base/Domain#PU"/>
        <rdfs:comment>Partial derivative of aerodynamic power with respect to changes in WTR speed (&lt;i&gt;dp&lt;/i&gt;&lt;i&gt;&lt;sub&gt;omega&lt;/sub&gt;&lt;/i&gt;). It is case dependent parameter.</rdfs:comment>
    </owl:ObjectProperty>
    


    <!-- https://w3id.org/netbeheer/referentiemodellen/IECCIM/TC57CIM/IEC61970/Dynamics/StandardModels/WindDynamics#WindAeroLinearIEC_dptheta -->


    <owl:ObjectProperty rdf:about="https://w3id.org/netbeheer/referentiemodellen/IECCIM/TC57CIM/IEC61970/Dynamics/StandardModels/WindDynamics#WindAeroLinearIEC_dptheta">
        <rdfs:domain rdf:resource="https://w3id.org/netbeheer/referentiemodellen/IECCIM/TC57CIM/IEC61970/Dynamics/StandardModels/WindDynamics#WindAeroLinearIEC"/>
        <rdfs:range rdf:resource="https://w3id.org/netbeheer/referentiemodellen/IECCIM/TC57CIM/IEC61970/Base/Domain#PU"/>
        <rdfs:comment>Partial derivative of aerodynamic power with respect to changes in pitch angle (&lt;i&gt;dp&lt;/i&gt;&lt;i&gt;&lt;sub&gt;theta&lt;/sub&gt;&lt;/i&gt;). It is case dependent parameter.</rdfs:comment>
    </owl:ObjectProperty>
    


    <!-- https://w3id.org/netbeheer/referentiemodellen/IECCIM/TC57CIM/IEC61970/Dynamics/StandardModels/WindDynamics#WindAeroLinearIEC_omegazero -->


    <owl:ObjectProperty rdf:about="https://w3id.org/netbeheer/referentiemodellen/IECCIM/TC57CIM/IEC61970/Dynamics/StandardModels/WindDynamics#WindAeroLinearIEC_omegazero">
        <rdfs:domain rdf:resource="https://w3id.org/netbeheer/referentiemodellen/IECCIM/TC57CIM/IEC61970/Dynamics/StandardModels/WindDynamics#WindAeroLinearIEC"/>
        <rdfs:range rdf:resource="https://w3id.org/netbeheer/referentiemodellen/IECCIM/TC57CIM/IEC61970/Base/Domain#PU"/>
        <rdfs:comment>Rotor speed if the wind turbine is not derated (&lt;i&gt;omega&lt;/i&gt;&lt;i&gt;&lt;sub&gt;0&lt;/sub&gt;&lt;/i&gt;). It is case dependent parameter.</rdfs:comment>
    </owl:ObjectProperty>
    


    <!-- https://w3id.org/netbeheer/referentiemodellen/IECCIM/TC57CIM/IEC61970/Dynamics/StandardModels/WindDynamics#WindAeroLinearIEC_pavail -->


    <owl:ObjectProperty rdf:about="https://w3id.org/netbeheer/referentiemodellen/IECCIM/TC57CIM/IEC61970/Dynamics/StandardModels/WindDynamics#WindAeroLinearIEC_pavail">
        <rdfs:domain rdf:resource="https://w3id.org/netbeheer/referentiemodellen/IECCIM/TC57CIM/IEC61970/Dynamics/StandardModels/WindDynamics#WindAeroLinearIEC"/>
        <rdfs:range rdf:resource="https://w3id.org/netbeheer/referentiemodellen/IECCIM/TC57CIM/IEC61970/Base/Domain#PU"/>
        <rdfs:comment>Available aerodynamic power (&lt;i&gt;p&lt;/i&gt;&lt;sub&gt;avail&lt;/sub&gt;). It is case dependent parameter.</rdfs:comment>
    </owl:ObjectProperty>
    


    <!-- https://w3id.org/netbeheer/referentiemodellen/IECCIM/TC57CIM/IEC61970/Dynamics/StandardModels/WindDynamics#WindAeroLinearIEC_thetazero -->


    <owl:ObjectProperty rdf:about="https://w3id.org/netbeheer/referentiemodellen/IECCIM/TC57CIM/IEC61970/Dynamics/StandardModels/WindDynamics#WindAeroLinearIEC_thetazero">
        <rdfs:domain rdf:resource="https://w3id.org/netbeheer/referentiemodellen/IECCIM/TC57CIM/IEC61970/Dynamics/StandardModels/WindDynamics#WindAeroLinearIEC"/>
        <rdfs:range rdf:resource="https://w3id.org/netbeheer/referentiemodellen/IECCIM/TC57CIM/IEC61970/Base/Domain#AngleDegrees"/>
        <rdfs:comment>Pitch angle if the wind turbine is not derated (&lt;i&gt;theta&lt;/i&gt;&lt;i&gt;&lt;sub&gt;0&lt;/sub&gt;&lt;/i&gt;). It is case dependent parameter.</rdfs:comment>
    </owl:ObjectProperty>
    


    <!-- https://w3id.org/netbeheer/referentiemodellen/IECCIM/TC57CIM/IEC61970/Dynamics/StandardModels/WindDynamics#WindContCurrLimIEC_WindDynamicsLookupTable -->


    <owl:ObjectProperty rdf:about="https://w3id.org/netbeheer/referentiemodellen/IECCIM/TC57CIM/IEC61970/Dynamics/StandardModels/WindDynamics#WindContCurrLimIEC_WindDynamicsLookupTable">
        <owl:inverseOf rdf:resource="https://w3id.org/netbeheer/referentiemodellen/IECCIM/TC57CIM/IEC61970/Dynamics/StandardModels/WindDynamics#WindDynamicsLookupTable_WindContCurrLimIEC"/>
        <rdfs:domain rdf:resource="https://w3id.org/netbeheer/referentiemodellen/IECCIM/TC57CIM/IEC61970/Dynamics/StandardModels/WindDynamics#WindContCurrLimIEC"/>
        <rdfs:range rdf:resource="https://w3id.org/netbeheer/referentiemodellen/IECCIM/TC57CIM/IEC61970/Dynamics/StandardModels/WindDynamics#WindDynamicsLookupTable"/>
        <rdfs:comment>The wind dynamics lookup table associated with this current control limitation model.The current control limitation model with which this wind dynamics lookup table is associated.</rdfs:comment>
    </owl:ObjectProperty>
    


    <!-- https://w3id.org/netbeheer/referentiemodellen/IECCIM/TC57CIM/IEC61970/Dynamics/StandardModels/WindDynamics#WindContCurrLimIEC_WindTurbineType3or4IEC -->


    <owl:ObjectProperty rdf:about="https://w3id.org/netbeheer/referentiemodellen/IECCIM/TC57CIM/IEC61970/Dynamics/StandardModels/WindDynamics#WindContCurrLimIEC_WindTurbineType3or4IEC">
        <rdf:type rdf:resource="http://www.w3.org/2002/07/owl#FunctionalProperty"/>
        <rdfs:domain rdf:resource="https://w3id.org/netbeheer/referentiemodellen/IECCIM/TC57CIM/IEC61970/Dynamics/StandardModels/WindDynamics#WindContCurrLimIEC"/>
        <rdfs:range rdf:resource="https://w3id.org/netbeheer/referentiemodellen/IECCIM/TC57CIM/IEC61970/Dynamics/StandardModels/WindDynamics#WindTurbineType3or4IEC"/>
        <rdfs:comment>Wind control current limitation model associated with this wind turbine type 3 or 4 model.Wind turbine type 3 or 4 model with which this wind control current limitation model is associated.</rdfs:comment>
    </owl:ObjectProperty>
    


    <!-- https://w3id.org/netbeheer/referentiemodellen/IECCIM/TC57CIM/IEC61970/Dynamics/StandardModels/WindDynamics#WindContCurrLimIEC_imax -->


    <owl:ObjectProperty rdf:about="https://w3id.org/netbeheer/referentiemodellen/IECCIM/TC57CIM/IEC61970/Dynamics/StandardModels/WindDynamics#WindContCurrLimIEC_imax">
        <rdfs:domain rdf:resource="https://w3id.org/netbeheer/referentiemodellen/IECCIM/TC57CIM/IEC61970/Dynamics/StandardModels/WindDynamics#WindContCurrLimIEC"/>
        <rdfs:range rdf:resource="https://w3id.org/netbeheer/referentiemodellen/IECCIM/TC57CIM/IEC61970/Base/Domain#PU"/>
        <rdfs:comment>Maximum continuous current at the wind turbine terminals (&lt;i&gt;i&lt;/i&gt;&lt;sub&gt;max&lt;/sub&gt;). It is type dependent parameter.</rdfs:comment>
    </owl:ObjectProperty>
    


    <!-- https://w3id.org/netbeheer/referentiemodellen/IECCIM/TC57CIM/IEC61970/Dynamics/StandardModels/WindDynamics#WindContCurrLimIEC_imaxdip -->


    <owl:ObjectProperty rdf:about="https://w3id.org/netbeheer/referentiemodellen/IECCIM/TC57CIM/IEC61970/Dynamics/StandardModels/WindDynamics#WindContCurrLimIEC_imaxdip">
        <rdfs:domain rdf:resource="https://w3id.org/netbeheer/referentiemodellen/IECCIM/TC57CIM/IEC61970/Dynamics/StandardModels/WindDynamics#WindContCurrLimIEC"/>
        <rdfs:range rdf:resource="https://w3id.org/netbeheer/referentiemodellen/IECCIM/TC57CIM/IEC61970/Base/Domain#PU"/>
        <rdfs:comment>Maximum current during voltage dip at the wind turbine terminals (&lt;i&gt;i&lt;/i&gt;&lt;sub&gt;max,dip&lt;/sub&gt;). It is project dependent parameter.</rdfs:comment>
    </owl:ObjectProperty>
    


    <!-- https://w3id.org/netbeheer/referentiemodellen/IECCIM/TC57CIM/IEC61970/Dynamics/StandardModels/WindDynamics#WindContCurrLimIEC_tufilt -->


    <owl:ObjectProperty rdf:about="https://w3id.org/netbeheer/referentiemodellen/IECCIM/TC57CIM/IEC61970/Dynamics/StandardModels/WindDynamics#WindContCurrLimIEC_tufilt">
        <rdfs:domain rdf:resource="https://w3id.org/netbeheer/referentiemodellen/IECCIM/TC57CIM/IEC61970/Dynamics/StandardModels/WindDynamics#WindContCurrLimIEC"/>
        <rdfs:range rdf:resource="https://w3id.org/netbeheer/referentiemodellen/IECCIM/TC57CIM/IEC61970/Base/Domain#Seconds"/>
        <rdfs:comment>Voltage measurement filter time constant (&lt;i&gt;T&lt;/i&gt;&lt;sub&gt;ufilt&lt;/sub&gt;). It is type dependent parameter.</rdfs:comment>
    </owl:ObjectProperty>
    


    <!-- https://w3id.org/netbeheer/referentiemodellen/IECCIM/TC57CIM/IEC61970/Dynamics/StandardModels/WindDynamics#WindContPType3IEC_WindDynamicsLookupTable -->


    <owl:ObjectProperty rdf:about="https://w3id.org/netbeheer/referentiemodellen/IECCIM/TC57CIM/IEC61970/Dynamics/StandardModels/WindDynamics#WindContPType3IEC_WindDynamicsLookupTable">
        <owl:inverseOf rdf:resource="https://w3id.org/netbeheer/referentiemodellen/IECCIM/TC57CIM/IEC61970/Dynamics/StandardModels/WindDynamics#WindDynamicsLookupTable_WindContPType3IEC"/>
        <rdfs:domain rdf:resource="https://w3id.org/netbeheer/referentiemodellen/IECCIM/TC57CIM/IEC61970/Dynamics/StandardModels/WindDynamics#WindContPType3IEC"/>
        <rdfs:range rdf:resource="https://w3id.org/netbeheer/referentiemodellen/IECCIM/TC57CIM/IEC61970/Dynamics/StandardModels/WindDynamics#WindDynamicsLookupTable"/>
        <rdfs:comment>The wind dynamics lookup table associated with this P control type 3 model.The P control type 3 model with which this wind dynamics lookup table is associated.</rdfs:comment>
    </owl:ObjectProperty>
    


    <!-- https://w3id.org/netbeheer/referentiemodellen/IECCIM/TC57CIM/IEC61970/Dynamics/StandardModels/WindDynamics#WindContPType3IEC_WindGenTurbineType3IEC -->


    <owl:ObjectProperty rdf:about="https://w3id.org/netbeheer/referentiemodellen/IECCIM/TC57CIM/IEC61970/Dynamics/StandardModels/WindDynamics#WindContPType3IEC_WindGenTurbineType3IEC">
        <rdf:type rdf:resource="http://www.w3.org/2002/07/owl#FunctionalProperty"/>
        <rdfs:domain rdf:resource="https://w3id.org/netbeheer/referentiemodellen/IECCIM/TC57CIM/IEC61970/Dynamics/StandardModels/WindDynamics#WindContPType3IEC"/>
        <rdfs:range rdf:resource="https://w3id.org/netbeheer/referentiemodellen/IECCIM/TC57CIM/IEC61970/Dynamics/StandardModels/WindDynamics#WindGenTurbineType3IEC"/>
        <rdfs:comment>Wind control P type 3 model associated with this wind turbine type 3 model.Wind turbine type 3 model with which this Wind control P type 3 model is associated.</rdfs:comment>
    </owl:ObjectProperty>
    


    <!-- https://w3id.org/netbeheer/referentiemodellen/IECCIM/TC57CIM/IEC61970/Dynamics/StandardModels/WindDynamics#WindContPType3IEC_dpmax -->


    <owl:ObjectProperty rdf:about="https://w3id.org/netbeheer/referentiemodellen/IECCIM/TC57CIM/IEC61970/Dynamics/StandardModels/WindDynamics#WindContPType3IEC_dpmax">
        <rdfs:domain rdf:resource="https://w3id.org/netbeheer/referentiemodellen/IECCIM/TC57CIM/IEC61970/Dynamics/StandardModels/WindDynamics#WindContPType3IEC"/>
        <rdfs:range rdf:resource="https://w3id.org/netbeheer/referentiemodellen/IECCIM/TC57CIM/IEC61970/Base/Domain#PU"/>
        <rdfs:comment>Maximum wind turbine power ramp rate (&lt;i&gt;dp&lt;/i&gt;&lt;sub&gt;max&lt;/sub&gt;). It is project dependent parameter.</rdfs:comment>
    </owl:ObjectProperty>
    


    <!-- https://w3id.org/netbeheer/referentiemodellen/IECCIM/TC57CIM/IEC61970/Dynamics/StandardModels/WindDynamics#WindContPType3IEC_dtrisemaxlvrt -->


    <owl:ObjectProperty rdf:about="https://w3id.org/netbeheer/referentiemodellen/IECCIM/TC57CIM/IEC61970/Dynamics/StandardModels/WindDynamics#WindContPType3IEC_dtrisemaxlvrt">
        <rdfs:domain rdf:resource="https://w3id.org/netbeheer/referentiemodellen/IECCIM/TC57CIM/IEC61970/Dynamics/StandardModels/WindDynamics#WindContPType3IEC"/>
        <rdfs:range rdf:resource="https://w3id.org/netbeheer/referentiemodellen/IECCIM/TC57CIM/IEC61970/Base/Domain#PU"/>
        <rdfs:comment>Limitation of torque rise rate during LVRT for S&lt;sub&gt;1&lt;/sub&gt; (d&lt;i&gt;T&lt;/i&gt;&lt;sub&gt;risemaxLVRT&lt;/sub&gt;). It is project dependent parameter.</rdfs:comment>
    </owl:ObjectProperty>
    


    <!-- https://w3id.org/netbeheer/referentiemodellen/IECCIM/TC57CIM/IEC61970/Dynamics/StandardModels/WindDynamics#WindContPType3IEC_kdtd -->


    <owl:ObjectProperty rdf:about="https://w3id.org/netbeheer/referentiemodellen/IECCIM/TC57CIM/IEC61970/Dynamics/StandardModels/WindDynamics#WindContPType3IEC_kdtd">
        <rdfs:domain rdf:resource="https://w3id.org/netbeheer/referentiemodellen/IECCIM/TC57CIM/IEC61970/Dynamics/StandardModels/WindDynamics#WindContPType3IEC"/>
        <rdfs:range rdf:resource="https://w3id.org/netbeheer/referentiemodellen/IECCIM/TC57CIM/IEC61970/Base/Domain#PU"/>
        <rdfs:comment>Gain for active drive train damping (&lt;i&gt;K&lt;/i&gt;&lt;sub&gt;DTD&lt;/sub&gt;). It is type dependent parameter.</rdfs:comment>
    </owl:ObjectProperty>
    


    <!-- https://w3id.org/netbeheer/referentiemodellen/IECCIM/TC57CIM/IEC61970/Dynamics/StandardModels/WindDynamics#WindContPType3IEC_kip -->


    <owl:ObjectProperty rdf:about="https://w3id.org/netbeheer/referentiemodellen/IECCIM/TC57CIM/IEC61970/Dynamics/StandardModels/WindDynamics#WindContPType3IEC_kip">
        <rdfs:domain rdf:resource="https://w3id.org/netbeheer/referentiemodellen/IECCIM/TC57CIM/IEC61970/Dynamics/StandardModels/WindDynamics#WindContPType3IEC"/>
        <rdfs:range rdf:resource="https://w3id.org/netbeheer/referentiemodellen/IECCIM/TC57CIM/IEC61970/Base/Domain#PU"/>
        <rdfs:comment>PI controller integration parameter (&lt;i&gt;K&lt;/i&gt;&lt;sub&gt;Ip&lt;/sub&gt;). It is type dependent parameter.</rdfs:comment>
    </owl:ObjectProperty>
    


    <!-- https://w3id.org/netbeheer/referentiemodellen/IECCIM/TC57CIM/IEC61970/Dynamics/StandardModels/WindDynamics#WindContPType3IEC_kpp -->


    <owl:ObjectProperty rdf:about="https://w3id.org/netbeheer/referentiemodellen/IECCIM/TC57CIM/IEC61970/Dynamics/StandardModels/WindDynamics#WindContPType3IEC_kpp">
        <rdfs:domain rdf:resource="https://w3id.org/netbeheer/referentiemodellen/IECCIM/TC57CIM/IEC61970/Dynamics/StandardModels/WindDynamics#WindContPType3IEC"/>
        <rdfs:range rdf:resource="https://w3id.org/netbeheer/referentiemodellen/IECCIM/TC57CIM/IEC61970/Base/Domain#PU"/>
        <rdfs:comment>PI controller proportional gain (&lt;i&gt;K&lt;/i&gt;&lt;sub&gt;Pp&lt;/sub&gt;). It is type dependent parameter.</rdfs:comment>
    </owl:ObjectProperty>
    


    <!-- https://w3id.org/netbeheer/referentiemodellen/IECCIM/TC57CIM/IEC61970/Dynamics/StandardModels/WindDynamics#WindContPType3IEC_omegaoffset -->


    <owl:ObjectProperty rdf:about="https://w3id.org/netbeheer/referentiemodellen/IECCIM/TC57CIM/IEC61970/Dynamics/StandardModels/WindDynamics#WindContPType3IEC_omegaoffset">
        <rdfs:domain rdf:resource="https://w3id.org/netbeheer/referentiemodellen/IECCIM/TC57CIM/IEC61970/Dynamics/StandardModels/WindDynamics#WindContPType3IEC"/>
        <rdfs:range rdf:resource="https://w3id.org/netbeheer/referentiemodellen/IECCIM/TC57CIM/IEC61970/Base/Domain#PU"/>
        <rdfs:comment>Offset to reference value that limits controller action during rotor speed changes (omega&lt;sub&gt;offset&lt;/sub&gt;). It is case dependent parameter.</rdfs:comment>
    </owl:ObjectProperty>
    


    <!-- https://w3id.org/netbeheer/referentiemodellen/IECCIM/TC57CIM/IEC61970/Dynamics/StandardModels/WindDynamics#WindContPType3IEC_pdtdmax -->


    <owl:ObjectProperty rdf:about="https://w3id.org/netbeheer/referentiemodellen/IECCIM/TC57CIM/IEC61970/Dynamics/StandardModels/WindDynamics#WindContPType3IEC_pdtdmax">
        <rdfs:domain rdf:resource="https://w3id.org/netbeheer/referentiemodellen/IECCIM/TC57CIM/IEC61970/Dynamics/StandardModels/WindDynamics#WindContPType3IEC"/>
        <rdfs:range rdf:resource="https://w3id.org/netbeheer/referentiemodellen/IECCIM/TC57CIM/IEC61970/Base/Domain#PU"/>
        <rdfs:comment>Maximum active drive train damping power (&lt;i&gt;p&lt;/i&gt;&lt;sub&gt;DTDmax&lt;/sub&gt;). It is type dependent parameter.</rdfs:comment>
    </owl:ObjectProperty>
    


    <!-- https://w3id.org/netbeheer/referentiemodellen/IECCIM/TC57CIM/IEC61970/Dynamics/StandardModels/WindDynamics#WindContPType3IEC_rramp -->


    <owl:ObjectProperty rdf:about="https://w3id.org/netbeheer/referentiemodellen/IECCIM/TC57CIM/IEC61970/Dynamics/StandardModels/WindDynamics#WindContPType3IEC_rramp">
        <rdfs:domain rdf:resource="https://w3id.org/netbeheer/referentiemodellen/IECCIM/TC57CIM/IEC61970/Dynamics/StandardModels/WindDynamics#WindContPType3IEC"/>
        <rdfs:range rdf:resource="https://w3id.org/netbeheer/referentiemodellen/IECCIM/TC57CIM/IEC61970/Base/Domain#PU"/>
        <rdfs:comment>Ramp limitation of torque, required in some grid codes (&lt;i&gt;R&lt;/i&gt;&lt;sub&gt;ramp&lt;/sub&gt;). It is project dependent parameter.</rdfs:comment>
    </owl:ObjectProperty>
    


    <!-- https://w3id.org/netbeheer/referentiemodellen/IECCIM/TC57CIM/IEC61970/Dynamics/StandardModels/WindDynamics#WindContPType3IEC_tdvs -->


    <owl:ObjectProperty rdf:about="https://w3id.org/netbeheer/referentiemodellen/IECCIM/TC57CIM/IEC61970/Dynamics/StandardModels/WindDynamics#WindContPType3IEC_tdvs">
        <rdfs:domain rdf:resource="https://w3id.org/netbeheer/referentiemodellen/IECCIM/TC57CIM/IEC61970/Dynamics/StandardModels/WindDynamics#WindContPType3IEC"/>
        <rdfs:range rdf:resource="https://w3id.org/netbeheer/referentiemodellen/IECCIM/TC57CIM/IEC61970/Base/Domain#Seconds"/>
        <rdfs:comment>Time&lt;sub&gt; &lt;/sub&gt;delay after deep voltage sags (T&lt;sub&gt;DVS&lt;/sub&gt;). It is project dependent parameter.</rdfs:comment>
    </owl:ObjectProperty>
    


    <!-- https://w3id.org/netbeheer/referentiemodellen/IECCIM/TC57CIM/IEC61970/Dynamics/StandardModels/WindDynamics#WindContPType3IEC_temin -->


    <owl:ObjectProperty rdf:about="https://w3id.org/netbeheer/referentiemodellen/IECCIM/TC57CIM/IEC61970/Dynamics/StandardModels/WindDynamics#WindContPType3IEC_temin">
        <rdfs:domain rdf:resource="https://w3id.org/netbeheer/referentiemodellen/IECCIM/TC57CIM/IEC61970/Dynamics/StandardModels/WindDynamics#WindContPType3IEC"/>
        <rdfs:range rdf:resource="https://w3id.org/netbeheer/referentiemodellen/IECCIM/TC57CIM/IEC61970/Base/Domain#PU"/>
        <rdfs:comment>Minimum electrical generator torque (&lt;i&gt;T&lt;/i&gt;&lt;sub&gt;emin&lt;/sub&gt;). It is type dependent parameter.</rdfs:comment>
    </owl:ObjectProperty>
    


    <!-- https://w3id.org/netbeheer/referentiemodellen/IECCIM/TC57CIM/IEC61970/Dynamics/StandardModels/WindDynamics#WindContPType3IEC_tomegafilt -->


    <owl:ObjectProperty rdf:about="https://w3id.org/netbeheer/referentiemodellen/IECCIM/TC57CIM/IEC61970/Dynamics/StandardModels/WindDynamics#WindContPType3IEC_tomegafilt">
        <rdfs:domain rdf:resource="https://w3id.org/netbeheer/referentiemodellen/IECCIM/TC57CIM/IEC61970/Dynamics/StandardModels/WindDynamics#WindContPType3IEC"/>
        <rdfs:range rdf:resource="https://w3id.org/netbeheer/referentiemodellen/IECCIM/TC57CIM/IEC61970/Base/Domain#Seconds"/>
        <rdfs:comment>Filter time constant for generator speed measurement (&lt;i&gt;T&lt;/i&gt;&lt;sub&gt;omegafilt&lt;/sub&gt;). It is type dependent parameter.</rdfs:comment>
    </owl:ObjectProperty>
    


    <!-- https://w3id.org/netbeheer/referentiemodellen/IECCIM/TC57CIM/IEC61970/Dynamics/StandardModels/WindDynamics#WindContPType3IEC_tpfilt -->


    <owl:ObjectProperty rdf:about="https://w3id.org/netbeheer/referentiemodellen/IECCIM/TC57CIM/IEC61970/Dynamics/StandardModels/WindDynamics#WindContPType3IEC_tpfilt">
        <rdfs:domain rdf:resource="https://w3id.org/netbeheer/referentiemodellen/IECCIM/TC57CIM/IEC61970/Dynamics/StandardModels/WindDynamics#WindContPType3IEC"/>
        <rdfs:range rdf:resource="https://w3id.org/netbeheer/referentiemodellen/IECCIM/TC57CIM/IEC61970/Base/Domain#Seconds"/>
        <rdfs:comment>Filter time constant for power measurement (&lt;i&gt;T&lt;/i&gt;&lt;sub&gt;pfilt&lt;/sub&gt;). It is type dependent parameter.</rdfs:comment>
    </owl:ObjectProperty>
    


    <!-- https://w3id.org/netbeheer/referentiemodellen/IECCIM/TC57CIM/IEC61970/Dynamics/StandardModels/WindDynamics#WindContPType3IEC_tpord -->


    <owl:ObjectProperty rdf:about="https://w3id.org/netbeheer/referentiemodellen/IECCIM/TC57CIM/IEC61970/Dynamics/StandardModels/WindDynamics#WindContPType3IEC_tpord">
        <rdfs:domain rdf:resource="https://w3id.org/netbeheer/referentiemodellen/IECCIM/TC57CIM/IEC61970/Dynamics/StandardModels/WindDynamics#WindContPType3IEC"/>
        <rdfs:range rdf:resource="https://w3id.org/netbeheer/referentiemodellen/IECCIM/TC57CIM/IEC61970/Base/Domain#PU"/>
        <rdfs:comment>Time constant in power order lag (&lt;i&gt;T&lt;/i&gt;&lt;sub&gt;pord&lt;/sub&gt;). It is type dependent parameter.</rdfs:comment>
    </owl:ObjectProperty>
    


    <!-- https://w3id.org/netbeheer/referentiemodellen/IECCIM/TC57CIM/IEC61970/Dynamics/StandardModels/WindDynamics#WindContPType3IEC_tufilt -->


    <owl:ObjectProperty rdf:about="https://w3id.org/netbeheer/referentiemodellen/IECCIM/TC57CIM/IEC61970/Dynamics/StandardModels/WindDynamics#WindContPType3IEC_tufilt">
        <rdfs:domain rdf:resource="https://w3id.org/netbeheer/referentiemodellen/IECCIM/TC57CIM/IEC61970/Dynamics/StandardModels/WindDynamics#WindContPType3IEC"/>
        <rdfs:range rdf:resource="https://w3id.org/netbeheer/referentiemodellen/IECCIM/TC57CIM/IEC61970/Base/Domain#Seconds"/>
        <rdfs:comment>Filter time constant for voltage measurement (&lt;i&gt;T&lt;/i&gt;&lt;sub&gt;ufilt&lt;/sub&gt;). It is type dependent parameter.</rdfs:comment>
    </owl:ObjectProperty>
    


    <!-- https://w3id.org/netbeheer/referentiemodellen/IECCIM/TC57CIM/IEC61970/Dynamics/StandardModels/WindDynamics#WindContPType3IEC_tuscale -->


    <owl:ObjectProperty rdf:about="https://w3id.org/netbeheer/referentiemodellen/IECCIM/TC57CIM/IEC61970/Dynamics/StandardModels/WindDynamics#WindContPType3IEC_tuscale">
        <rdfs:domain rdf:resource="https://w3id.org/netbeheer/referentiemodellen/IECCIM/TC57CIM/IEC61970/Dynamics/StandardModels/WindDynamics#WindContPType3IEC"/>
        <rdfs:range rdf:resource="https://w3id.org/netbeheer/referentiemodellen/IECCIM/TC57CIM/IEC61970/Base/Domain#PU"/>
        <rdfs:comment>Voltage scaling factor of reset-torque (T&lt;sub&gt;uscale&lt;/sub&gt;). It is project dependent parameter.</rdfs:comment>
    </owl:ObjectProperty>
    


    <!-- https://w3id.org/netbeheer/referentiemodellen/IECCIM/TC57CIM/IEC61970/Dynamics/StandardModels/WindDynamics#WindContPType3IEC_twref -->


    <owl:ObjectProperty rdf:about="https://w3id.org/netbeheer/referentiemodellen/IECCIM/TC57CIM/IEC61970/Dynamics/StandardModels/WindDynamics#WindContPType3IEC_twref">
        <rdfs:domain rdf:resource="https://w3id.org/netbeheer/referentiemodellen/IECCIM/TC57CIM/IEC61970/Dynamics/StandardModels/WindDynamics#WindContPType3IEC"/>
        <rdfs:range rdf:resource="https://w3id.org/netbeheer/referentiemodellen/IECCIM/TC57CIM/IEC61970/Base/Domain#Seconds"/>
        <rdfs:comment>Time constant in speed reference filter (&lt;i&gt;T&lt;/i&gt;&lt;sub&gt;omega,ref&lt;/sub&gt;). It is type dependent parameter.</rdfs:comment>
    </owl:ObjectProperty>
    


    <!-- https://w3id.org/netbeheer/referentiemodellen/IECCIM/TC57CIM/IEC61970/Dynamics/StandardModels/WindDynamics#WindContPType3IEC_udvs -->


    <owl:ObjectProperty rdf:about="https://w3id.org/netbeheer/referentiemodellen/IECCIM/TC57CIM/IEC61970/Dynamics/StandardModels/WindDynamics#WindContPType3IEC_udvs">
        <rdfs:domain rdf:resource="https://w3id.org/netbeheer/referentiemodellen/IECCIM/TC57CIM/IEC61970/Dynamics/StandardModels/WindDynamics#WindContPType3IEC"/>
        <rdfs:range rdf:resource="https://w3id.org/netbeheer/referentiemodellen/IECCIM/TC57CIM/IEC61970/Base/Domain#PU"/>
        <rdfs:comment>Voltage limit for hold LVRT status after deep voltage sags (&lt;i&gt;u&lt;/i&gt;&lt;i&gt;&lt;sub&gt;DVS&lt;/sub&gt;&lt;/i&gt;). It is project dependent parameter.</rdfs:comment>
    </owl:ObjectProperty>
    


    <!-- https://w3id.org/netbeheer/referentiemodellen/IECCIM/TC57CIM/IEC61970/Dynamics/StandardModels/WindDynamics#WindContPType3IEC_updip -->


    <owl:ObjectProperty rdf:about="https://w3id.org/netbeheer/referentiemodellen/IECCIM/TC57CIM/IEC61970/Dynamics/StandardModels/WindDynamics#WindContPType3IEC_updip">
        <rdfs:domain rdf:resource="https://w3id.org/netbeheer/referentiemodellen/IECCIM/TC57CIM/IEC61970/Dynamics/StandardModels/WindDynamics#WindContPType3IEC"/>
        <rdfs:range rdf:resource="https://w3id.org/netbeheer/referentiemodellen/IECCIM/TC57CIM/IEC61970/Base/Domain#PU"/>
        <rdfs:comment>Voltage dip threshold for P-control (&lt;i&gt;u&lt;/i&gt;&lt;sub&gt;Pdip&lt;/sub&gt;).  Part of turbine control, often different (e.g 0.8) from converter thresholds. It is project dependent parameter.</rdfs:comment>
    </owl:ObjectProperty>
    


    <!-- https://w3id.org/netbeheer/referentiemodellen/IECCIM/TC57CIM/IEC61970/Dynamics/StandardModels/WindDynamics#WindContPType3IEC_wdtd -->


    <owl:ObjectProperty rdf:about="https://w3id.org/netbeheer/referentiemodellen/IECCIM/TC57CIM/IEC61970/Dynamics/StandardModels/WindDynamics#WindContPType3IEC_wdtd">
        <rdfs:domain rdf:resource="https://w3id.org/netbeheer/referentiemodellen/IECCIM/TC57CIM/IEC61970/Dynamics/StandardModels/WindDynamics#WindContPType3IEC"/>
        <rdfs:range rdf:resource="https://w3id.org/netbeheer/referentiemodellen/IECCIM/TC57CIM/IEC61970/Base/Domain#PU"/>
        <rdfs:comment>Active drive train damping frequency (omega&lt;sub&gt;DTD&lt;/sub&gt;). It can be calculated from two mass model parameters. It is type dependent parameter.</rdfs:comment>
    </owl:ObjectProperty>
    


    <!-- https://w3id.org/netbeheer/referentiemodellen/IECCIM/TC57CIM/IEC61970/Dynamics/StandardModels/WindDynamics#WindContPType4aIEC_WindTurbineType4aIEC -->


    <owl:ObjectProperty rdf:about="https://w3id.org/netbeheer/referentiemodellen/IECCIM/TC57CIM/IEC61970/Dynamics/StandardModels/WindDynamics#WindContPType4aIEC_WindTurbineType4aIEC">
        <rdf:type rdf:resource="http://www.w3.org/2002/07/owl#FunctionalProperty"/>
        <rdfs:domain rdf:resource="https://w3id.org/netbeheer/referentiemodellen/IECCIM/TC57CIM/IEC61970/Dynamics/StandardModels/WindDynamics#WindContPType4aIEC"/>
        <rdfs:range rdf:resource="https://w3id.org/netbeheer/referentiemodellen/IECCIM/TC57CIM/IEC61970/Dynamics/StandardModels/WindDynamics#WindTurbineType4aIEC"/>
        <rdfs:comment>Wind control P type 4A model associated with this wind turbine type 4A model. Wind turbine type 4A model with which this wind control P type 4A model is associated.</rdfs:comment>
    </owl:ObjectProperty>
    


    <!-- https://w3id.org/netbeheer/referentiemodellen/IECCIM/TC57CIM/IEC61970/Dynamics/StandardModels/WindDynamics#WindContPType4aIEC_dpmax -->


    <owl:ObjectProperty rdf:about="https://w3id.org/netbeheer/referentiemodellen/IECCIM/TC57CIM/IEC61970/Dynamics/StandardModels/WindDynamics#WindContPType4aIEC_dpmax">
        <rdfs:domain rdf:resource="https://w3id.org/netbeheer/referentiemodellen/IECCIM/TC57CIM/IEC61970/Dynamics/StandardModels/WindDynamics#WindContPType4aIEC"/>
        <rdfs:range rdf:resource="https://w3id.org/netbeheer/referentiemodellen/IECCIM/TC57CIM/IEC61970/Base/Domain#PU"/>
        <rdfs:comment>Maximum wind turbine power ramp rate (&lt;i&gt;dp&lt;/i&gt;&lt;sub&gt;max&lt;/sub&gt;). It is project dependent parameter.</rdfs:comment>
    </owl:ObjectProperty>
    


    <!-- https://w3id.org/netbeheer/referentiemodellen/IECCIM/TC57CIM/IEC61970/Dynamics/StandardModels/WindDynamics#WindContPType4aIEC_tpord -->


    <owl:ObjectProperty rdf:about="https://w3id.org/netbeheer/referentiemodellen/IECCIM/TC57CIM/IEC61970/Dynamics/StandardModels/WindDynamics#WindContPType4aIEC_tpord">
        <rdfs:domain rdf:resource="https://w3id.org/netbeheer/referentiemodellen/IECCIM/TC57CIM/IEC61970/Dynamics/StandardModels/WindDynamics#WindContPType4aIEC"/>
        <rdfs:range rdf:resource="https://w3id.org/netbeheer/referentiemodellen/IECCIM/TC57CIM/IEC61970/Base/Domain#Seconds"/>
        <rdfs:comment>Time constant in power order lag (&lt;i&gt;T&lt;/i&gt;&lt;sub&gt;pord&lt;/sub&gt;). It is type dependent parameter.</rdfs:comment>
    </owl:ObjectProperty>
    


    <!-- https://w3id.org/netbeheer/referentiemodellen/IECCIM/TC57CIM/IEC61970/Dynamics/StandardModels/WindDynamics#WindContPType4aIEC_tufilt -->


    <owl:ObjectProperty rdf:about="https://w3id.org/netbeheer/referentiemodellen/IECCIM/TC57CIM/IEC61970/Dynamics/StandardModels/WindDynamics#WindContPType4aIEC_tufilt">
        <rdfs:domain rdf:resource="https://w3id.org/netbeheer/referentiemodellen/IECCIM/TC57CIM/IEC61970/Dynamics/StandardModels/WindDynamics#WindContPType4aIEC"/>
        <rdfs:range rdf:resource="https://w3id.org/netbeheer/referentiemodellen/IECCIM/TC57CIM/IEC61970/Base/Domain#Seconds"/>
        <rdfs:comment>Voltage measurement filter time constant (&lt;i&gt;T&lt;/i&gt;&lt;sub&gt;ufilt&lt;/sub&gt;). It is type dependent parameter.</rdfs:comment>
    </owl:ObjectProperty>
    


    <!-- https://w3id.org/netbeheer/referentiemodellen/IECCIM/TC57CIM/IEC61970/Dynamics/StandardModels/WindDynamics#WindContPType4bIEC_WindTurbineType4bIEC -->


    <owl:ObjectProperty rdf:about="https://w3id.org/netbeheer/referentiemodellen/IECCIM/TC57CIM/IEC61970/Dynamics/StandardModels/WindDynamics#WindContPType4bIEC_WindTurbineType4bIEC">
        <rdf:type rdf:resource="http://www.w3.org/2002/07/owl#FunctionalProperty"/>
        <rdfs:domain rdf:resource="https://w3id.org/netbeheer/referentiemodellen/IECCIM/TC57CIM/IEC61970/Dynamics/StandardModels/WindDynamics#WindContPType4bIEC"/>
        <rdfs:range rdf:resource="https://w3id.org/netbeheer/referentiemodellen/IECCIM/TC57CIM/IEC61970/Dynamics/StandardModels/WindDynamics#WindTurbineType4bIEC"/>
        <rdfs:comment>Wind control P type 4B model associated with this wind turbine type 4B model.Wind turbine type 4B model with which this wind control P type 4B model is associated.</rdfs:comment>
    </owl:ObjectProperty>
    


    <!-- https://w3id.org/netbeheer/referentiemodellen/IECCIM/TC57CIM/IEC61970/Dynamics/StandardModels/WindDynamics#WindContPType4bIEC_dpmax -->


    <owl:ObjectProperty rdf:about="https://w3id.org/netbeheer/referentiemodellen/IECCIM/TC57CIM/IEC61970/Dynamics/StandardModels/WindDynamics#WindContPType4bIEC_dpmax">
        <rdfs:domain rdf:resource="https://w3id.org/netbeheer/referentiemodellen/IECCIM/TC57CIM/IEC61970/Dynamics/StandardModels/WindDynamics#WindContPType4bIEC"/>
        <rdfs:range rdf:resource="https://w3id.org/netbeheer/referentiemodellen/IECCIM/TC57CIM/IEC61970/Base/Domain#PU"/>
        <rdfs:comment>Maximum wind turbine power ramp rate (&lt;i&gt;dp&lt;/i&gt;&lt;sub&gt;max&lt;/sub&gt;). It is project dependent parameter.</rdfs:comment>
    </owl:ObjectProperty>
    


    <!-- https://w3id.org/netbeheer/referentiemodellen/IECCIM/TC57CIM/IEC61970/Dynamics/StandardModels/WindDynamics#WindContPType4bIEC_tpaero -->


    <owl:ObjectProperty rdf:about="https://w3id.org/netbeheer/referentiemodellen/IECCIM/TC57CIM/IEC61970/Dynamics/StandardModels/WindDynamics#WindContPType4bIEC_tpaero">
        <rdfs:domain rdf:resource="https://w3id.org/netbeheer/referentiemodellen/IECCIM/TC57CIM/IEC61970/Dynamics/StandardModels/WindDynamics#WindContPType4bIEC"/>
        <rdfs:range rdf:resource="https://w3id.org/netbeheer/referentiemodellen/IECCIM/TC57CIM/IEC61970/Base/Domain#Seconds"/>
        <rdfs:comment>Time constant in aerodynamic power response (&lt;i&gt;T&lt;/i&gt;&lt;sub&gt;paero&lt;/sub&gt;). It is type dependent parameter.</rdfs:comment>
    </owl:ObjectProperty>
    


    <!-- https://w3id.org/netbeheer/referentiemodellen/IECCIM/TC57CIM/IEC61970/Dynamics/StandardModels/WindDynamics#WindContPType4bIEC_tpord -->


    <owl:ObjectProperty rdf:about="https://w3id.org/netbeheer/referentiemodellen/IECCIM/TC57CIM/IEC61970/Dynamics/StandardModels/WindDynamics#WindContPType4bIEC_tpord">
        <rdfs:domain rdf:resource="https://w3id.org/netbeheer/referentiemodellen/IECCIM/TC57CIM/IEC61970/Dynamics/StandardModels/WindDynamics#WindContPType4bIEC"/>
        <rdfs:range rdf:resource="https://w3id.org/netbeheer/referentiemodellen/IECCIM/TC57CIM/IEC61970/Base/Domain#Seconds"/>
        <rdfs:comment>Time constant in power order lag (&lt;i&gt;T&lt;/i&gt;&lt;sub&gt;pord&lt;/sub&gt;). It is type dependent parameter.</rdfs:comment>
    </owl:ObjectProperty>
    


    <!-- https://w3id.org/netbeheer/referentiemodellen/IECCIM/TC57CIM/IEC61970/Dynamics/StandardModels/WindDynamics#WindContPType4bIEC_tufilt -->


    <owl:ObjectProperty rdf:about="https://w3id.org/netbeheer/referentiemodellen/IECCIM/TC57CIM/IEC61970/Dynamics/StandardModels/WindDynamics#WindContPType4bIEC_tufilt">
        <rdfs:domain rdf:resource="https://w3id.org/netbeheer/referentiemodellen/IECCIM/TC57CIM/IEC61970/Dynamics/StandardModels/WindDynamics#WindContPType4bIEC"/>
        <rdfs:range rdf:resource="https://w3id.org/netbeheer/referentiemodellen/IECCIM/TC57CIM/IEC61970/Base/Domain#Seconds"/>
        <rdfs:comment>Voltage measurement filter time constant (&lt;i&gt;T&lt;/i&gt;&lt;sub&gt;ufilt&lt;/sub&gt;). It is type dependent parameter.</rdfs:comment>
    </owl:ObjectProperty>
    


    <!-- https://w3id.org/netbeheer/referentiemodellen/IECCIM/TC57CIM/IEC61970/Dynamics/StandardModels/WindDynamics#WindContPitchAngleIEC_WindGenTurbineType3IEC -->


    <owl:ObjectProperty rdf:about="https://w3id.org/netbeheer/referentiemodellen/IECCIM/TC57CIM/IEC61970/Dynamics/StandardModels/WindDynamics#WindContPitchAngleIEC_WindGenTurbineType3IEC">
        <rdf:type rdf:resource="http://www.w3.org/2002/07/owl#FunctionalProperty"/>
        <rdfs:domain rdf:resource="https://w3id.org/netbeheer/referentiemodellen/IECCIM/TC57CIM/IEC61970/Dynamics/StandardModels/WindDynamics#WindContPitchAngleIEC"/>
        <rdfs:range rdf:resource="https://w3id.org/netbeheer/referentiemodellen/IECCIM/TC57CIM/IEC61970/Dynamics/StandardModels/WindDynamics#WindGenTurbineType3IEC"/>
        <rdfs:comment>Wind control pitch angle model associated with this wind turbine type 3.Wind turbine type 3 model with which this pitch control model is associated.</rdfs:comment>
    </owl:ObjectProperty>
    


    <!-- https://w3id.org/netbeheer/referentiemodellen/IECCIM/TC57CIM/IEC61970/Dynamics/StandardModels/WindDynamics#WindContPitchAngleIEC_kic -->


    <owl:ObjectProperty rdf:about="https://w3id.org/netbeheer/referentiemodellen/IECCIM/TC57CIM/IEC61970/Dynamics/StandardModels/WindDynamics#WindContPitchAngleIEC_kic">
        <rdfs:domain rdf:resource="https://w3id.org/netbeheer/referentiemodellen/IECCIM/TC57CIM/IEC61970/Dynamics/StandardModels/WindDynamics#WindContPitchAngleIEC"/>
        <rdfs:range rdf:resource="https://w3id.org/netbeheer/referentiemodellen/IECCIM/TC57CIM/IEC61970/Base/Domain#PU"/>
        <rdfs:comment>Power PI controller integration gain (&lt;i&gt;K&lt;/i&gt;&lt;sub&gt;Ic&lt;/sub&gt;). It is type dependent parameter.</rdfs:comment>
    </owl:ObjectProperty>
    


    <!-- https://w3id.org/netbeheer/referentiemodellen/IECCIM/TC57CIM/IEC61970/Dynamics/StandardModels/WindDynamics#WindContPitchAngleIEC_kiomega -->


    <owl:ObjectProperty rdf:about="https://w3id.org/netbeheer/referentiemodellen/IECCIM/TC57CIM/IEC61970/Dynamics/StandardModels/WindDynamics#WindContPitchAngleIEC_kiomega">
        <rdfs:domain rdf:resource="https://w3id.org/netbeheer/referentiemodellen/IECCIM/TC57CIM/IEC61970/Dynamics/StandardModels/WindDynamics#WindContPitchAngleIEC"/>
        <rdfs:range rdf:resource="https://w3id.org/netbeheer/referentiemodellen/IECCIM/TC57CIM/IEC61970/Base/Domain#PU"/>
        <rdfs:comment>Speed PI controller integration gain (&lt;i&gt;K&lt;/i&gt;&lt;sub&gt;Iomega&lt;/sub&gt;). It is type dependent parameter.</rdfs:comment>
    </owl:ObjectProperty>
    


    <!-- https://w3id.org/netbeheer/referentiemodellen/IECCIM/TC57CIM/IEC61970/Dynamics/StandardModels/WindDynamics#WindContPitchAngleIEC_kpc -->


    <owl:ObjectProperty rdf:about="https://w3id.org/netbeheer/referentiemodellen/IECCIM/TC57CIM/IEC61970/Dynamics/StandardModels/WindDynamics#WindContPitchAngleIEC_kpc">
        <rdfs:domain rdf:resource="https://w3id.org/netbeheer/referentiemodellen/IECCIM/TC57CIM/IEC61970/Dynamics/StandardModels/WindDynamics#WindContPitchAngleIEC"/>
        <rdfs:range rdf:resource="https://w3id.org/netbeheer/referentiemodellen/IECCIM/TC57CIM/IEC61970/Base/Domain#PU"/>
        <rdfs:comment>Power PI controller proportional gain (&lt;i&gt;K&lt;/i&gt;&lt;sub&gt;Pc&lt;/sub&gt;). It is type dependent parameter.</rdfs:comment>
    </owl:ObjectProperty>
    


    <!-- https://w3id.org/netbeheer/referentiemodellen/IECCIM/TC57CIM/IEC61970/Dynamics/StandardModels/WindDynamics#WindContPitchAngleIEC_kpomega -->


    <owl:ObjectProperty rdf:about="https://w3id.org/netbeheer/referentiemodellen/IECCIM/TC57CIM/IEC61970/Dynamics/StandardModels/WindDynamics#WindContPitchAngleIEC_kpomega">
        <rdfs:domain rdf:resource="https://w3id.org/netbeheer/referentiemodellen/IECCIM/TC57CIM/IEC61970/Dynamics/StandardModels/WindDynamics#WindContPitchAngleIEC"/>
        <rdfs:range rdf:resource="https://w3id.org/netbeheer/referentiemodellen/IECCIM/TC57CIM/IEC61970/Base/Domain#PU"/>
        <rdfs:comment>Speed PI controller proportional gain (&lt;i&gt;K&lt;/i&gt;&lt;sub&gt;Pomega&lt;/sub&gt;). It is type dependent parameter.</rdfs:comment>
    </owl:ObjectProperty>
    


    <!-- https://w3id.org/netbeheer/referentiemodellen/IECCIM/TC57CIM/IEC61970/Dynamics/StandardModels/WindDynamics#WindContPitchAngleIEC_kpx -->


    <owl:ObjectProperty rdf:about="https://w3id.org/netbeheer/referentiemodellen/IECCIM/TC57CIM/IEC61970/Dynamics/StandardModels/WindDynamics#WindContPitchAngleIEC_kpx">
        <rdfs:domain rdf:resource="https://w3id.org/netbeheer/referentiemodellen/IECCIM/TC57CIM/IEC61970/Dynamics/StandardModels/WindDynamics#WindContPitchAngleIEC"/>
        <rdfs:range rdf:resource="https://w3id.org/netbeheer/referentiemodellen/IECCIM/TC57CIM/IEC61970/Base/Domain#PU"/>
        <rdfs:comment>Pitch cross coupling gain (K&lt;sub&gt;PX&lt;/sub&gt;). It is type dependent parameter.</rdfs:comment>
    </owl:ObjectProperty>
    


    <!-- https://w3id.org/netbeheer/referentiemodellen/IECCIM/TC57CIM/IEC61970/Dynamics/StandardModels/WindDynamics#WindContPitchAngleIEC_thetamax -->


    <owl:ObjectProperty rdf:about="https://w3id.org/netbeheer/referentiemodellen/IECCIM/TC57CIM/IEC61970/Dynamics/StandardModels/WindDynamics#WindContPitchAngleIEC_thetamax">
        <rdfs:domain rdf:resource="https://w3id.org/netbeheer/referentiemodellen/IECCIM/TC57CIM/IEC61970/Dynamics/StandardModels/WindDynamics#WindContPitchAngleIEC"/>
        <rdfs:range rdf:resource="https://w3id.org/netbeheer/referentiemodellen/IECCIM/TC57CIM/IEC61970/Base/Domain#AngleDegrees"/>
        <rdfs:comment>Maximum pitch angle (&lt;i&gt;theta&lt;/i&gt;&lt;sub&gt;max&lt;/sub&gt;). It is type dependent parameter.</rdfs:comment>
    </owl:ObjectProperty>
    


    <!-- https://w3id.org/netbeheer/referentiemodellen/IECCIM/TC57CIM/IEC61970/Dynamics/StandardModels/WindDynamics#WindContPitchAngleIEC_thetamin -->


    <owl:ObjectProperty rdf:about="https://w3id.org/netbeheer/referentiemodellen/IECCIM/TC57CIM/IEC61970/Dynamics/StandardModels/WindDynamics#WindContPitchAngleIEC_thetamin">
        <rdfs:domain rdf:resource="https://w3id.org/netbeheer/referentiemodellen/IECCIM/TC57CIM/IEC61970/Dynamics/StandardModels/WindDynamics#WindContPitchAngleIEC"/>
        <rdfs:range rdf:resource="https://w3id.org/netbeheer/referentiemodellen/IECCIM/TC57CIM/IEC61970/Base/Domain#AngleDegrees"/>
        <rdfs:comment>Minimum pitch angle (&lt;i&gt;theta&lt;/i&gt;&lt;sub&gt;min&lt;/sub&gt;). It is type dependent parameter.</rdfs:comment>
    </owl:ObjectProperty>
    


    <!-- https://w3id.org/netbeheer/referentiemodellen/IECCIM/TC57CIM/IEC61970/Dynamics/StandardModels/WindDynamics#WindContPitchAngleIEC_ttheta -->


    <owl:ObjectProperty rdf:about="https://w3id.org/netbeheer/referentiemodellen/IECCIM/TC57CIM/IEC61970/Dynamics/StandardModels/WindDynamics#WindContPitchAngleIEC_ttheta">
        <rdfs:domain rdf:resource="https://w3id.org/netbeheer/referentiemodellen/IECCIM/TC57CIM/IEC61970/Dynamics/StandardModels/WindDynamics#WindContPitchAngleIEC"/>
        <rdfs:range rdf:resource="https://w3id.org/netbeheer/referentiemodellen/IECCIM/TC57CIM/IEC61970/Base/Domain#Seconds"/>
        <rdfs:comment>Pitch time constant (t&lt;i&gt;theta&lt;/i&gt;). It is type dependent parameter.</rdfs:comment>
    </owl:ObjectProperty>
    


    <!-- https://w3id.org/netbeheer/referentiemodellen/IECCIM/TC57CIM/IEC61970/Dynamics/StandardModels/WindDynamics#WindContQIEC_WindTurbineType3or4IEC -->


    <owl:ObjectProperty rdf:about="https://w3id.org/netbeheer/referentiemodellen/IECCIM/TC57CIM/IEC61970/Dynamics/StandardModels/WindDynamics#WindContQIEC_WindTurbineType3or4IEC">
        <rdf:type rdf:resource="http://www.w3.org/2002/07/owl#FunctionalProperty"/>
        <rdfs:domain rdf:resource="https://w3id.org/netbeheer/referentiemodellen/IECCIM/TC57CIM/IEC61970/Dynamics/StandardModels/WindDynamics#WindContQIEC"/>
        <rdfs:range rdf:resource="https://w3id.org/netbeheer/referentiemodellen/IECCIM/TC57CIM/IEC61970/Dynamics/StandardModels/WindDynamics#WindTurbineType3or4IEC"/>
        <rdfs:comment>Wind control Q model associated with this wind turbine type 3 or 4 model.Wind turbine type 3 or 4 model with which this reactive control mode is associated.</rdfs:comment>
    </owl:ObjectProperty>
    


    <!-- https://w3id.org/netbeheer/referentiemodellen/IECCIM/TC57CIM/IEC61970/Dynamics/StandardModels/WindDynamics#WindContQIEC_iqh1 -->


    <owl:ObjectProperty rdf:about="https://w3id.org/netbeheer/referentiemodellen/IECCIM/TC57CIM/IEC61970/Dynamics/StandardModels/WindDynamics#WindContQIEC_iqh1">
        <rdfs:domain rdf:resource="https://w3id.org/netbeheer/referentiemodellen/IECCIM/TC57CIM/IEC61970/Dynamics/StandardModels/WindDynamics#WindContQIEC"/>
        <rdfs:range rdf:resource="https://w3id.org/netbeheer/referentiemodellen/IECCIM/TC57CIM/IEC61970/Base/Domain#PU"/>
        <rdfs:comment>Maximum reactive current injection during dip (i&lt;sub&gt;qh1&lt;/sub&gt;). It is type dependent parameter.</rdfs:comment>
    </owl:ObjectProperty>
    


    <!-- https://w3id.org/netbeheer/referentiemodellen/IECCIM/TC57CIM/IEC61970/Dynamics/StandardModels/WindDynamics#WindContQIEC_iqmax -->


    <owl:ObjectProperty rdf:about="https://w3id.org/netbeheer/referentiemodellen/IECCIM/TC57CIM/IEC61970/Dynamics/StandardModels/WindDynamics#WindContQIEC_iqmax">
        <rdfs:domain rdf:resource="https://w3id.org/netbeheer/referentiemodellen/IECCIM/TC57CIM/IEC61970/Dynamics/StandardModels/WindDynamics#WindContQIEC"/>
        <rdfs:range rdf:resource="https://w3id.org/netbeheer/referentiemodellen/IECCIM/TC57CIM/IEC61970/Base/Domain#PU"/>
        <rdfs:comment>Maximum reactive current injection (i&lt;sub&gt;qmax&lt;/sub&gt;). It is type dependent parameter.</rdfs:comment>
    </owl:ObjectProperty>
    


    <!-- https://w3id.org/netbeheer/referentiemodellen/IECCIM/TC57CIM/IEC61970/Dynamics/StandardModels/WindDynamics#WindContQIEC_iqmin -->


    <owl:ObjectProperty rdf:about="https://w3id.org/netbeheer/referentiemodellen/IECCIM/TC57CIM/IEC61970/Dynamics/StandardModels/WindDynamics#WindContQIEC_iqmin">
        <rdfs:domain rdf:resource="https://w3id.org/netbeheer/referentiemodellen/IECCIM/TC57CIM/IEC61970/Dynamics/StandardModels/WindDynamics#WindContQIEC"/>
        <rdfs:range rdf:resource="https://w3id.org/netbeheer/referentiemodellen/IECCIM/TC57CIM/IEC61970/Base/Domain#PU"/>
        <rdfs:comment>Minimum reactive current injection (i&lt;sub&gt;qmin&lt;/sub&gt;). It is type dependent parameter.</rdfs:comment>
    </owl:ObjectProperty>
    


    <!-- https://w3id.org/netbeheer/referentiemodellen/IECCIM/TC57CIM/IEC61970/Dynamics/StandardModels/WindDynamics#WindContQIEC_iqpost -->


    <owl:ObjectProperty rdf:about="https://w3id.org/netbeheer/referentiemodellen/IECCIM/TC57CIM/IEC61970/Dynamics/StandardModels/WindDynamics#WindContQIEC_iqpost">
        <rdfs:domain rdf:resource="https://w3id.org/netbeheer/referentiemodellen/IECCIM/TC57CIM/IEC61970/Dynamics/StandardModels/WindDynamics#WindContQIEC"/>
        <rdfs:range rdf:resource="https://w3id.org/netbeheer/referentiemodellen/IECCIM/TC57CIM/IEC61970/Base/Domain#PU"/>
        <rdfs:comment>Post fault reactive current injection (&lt;i&gt;i&lt;/i&gt;&lt;sub&gt;qpost&lt;/sub&gt;). It is project dependent parameter.</rdfs:comment>
    </owl:ObjectProperty>
    


    <!-- https://w3id.org/netbeheer/referentiemodellen/IECCIM/TC57CIM/IEC61970/Dynamics/StandardModels/WindDynamics#WindContQIEC_kiq -->


    <owl:ObjectProperty rdf:about="https://w3id.org/netbeheer/referentiemodellen/IECCIM/TC57CIM/IEC61970/Dynamics/StandardModels/WindDynamics#WindContQIEC_kiq">
        <rdfs:domain rdf:resource="https://w3id.org/netbeheer/referentiemodellen/IECCIM/TC57CIM/IEC61970/Dynamics/StandardModels/WindDynamics#WindContQIEC"/>
        <rdfs:range rdf:resource="https://w3id.org/netbeheer/referentiemodellen/IECCIM/TC57CIM/IEC61970/Base/Domain#PU"/>
        <rdfs:comment>Reactive power PI controller integration gain (&lt;i&gt;K&lt;/i&gt;&lt;sub&gt;I,q&lt;/sub&gt;). It is type dependent parameter.</rdfs:comment>
    </owl:ObjectProperty>
    


    <!-- https://w3id.org/netbeheer/referentiemodellen/IECCIM/TC57CIM/IEC61970/Dynamics/StandardModels/WindDynamics#WindContQIEC_kiu -->


    <owl:ObjectProperty rdf:about="https://w3id.org/netbeheer/referentiemodellen/IECCIM/TC57CIM/IEC61970/Dynamics/StandardModels/WindDynamics#WindContQIEC_kiu">
        <rdfs:domain rdf:resource="https://w3id.org/netbeheer/referentiemodellen/IECCIM/TC57CIM/IEC61970/Dynamics/StandardModels/WindDynamics#WindContQIEC"/>
        <rdfs:range rdf:resource="https://w3id.org/netbeheer/referentiemodellen/IECCIM/TC57CIM/IEC61970/Base/Domain#PU"/>
        <rdfs:comment>Voltage PI controller integration gain (&lt;i&gt;K&lt;/i&gt;&lt;sub&gt;I,u&lt;/sub&gt;). It is type dependent parameter.</rdfs:comment>
    </owl:ObjectProperty>
    


    <!-- https://w3id.org/netbeheer/referentiemodellen/IECCIM/TC57CIM/IEC61970/Dynamics/StandardModels/WindDynamics#WindContQIEC_kpq -->


    <owl:ObjectProperty rdf:about="https://w3id.org/netbeheer/referentiemodellen/IECCIM/TC57CIM/IEC61970/Dynamics/StandardModels/WindDynamics#WindContQIEC_kpq">
        <rdfs:domain rdf:resource="https://w3id.org/netbeheer/referentiemodellen/IECCIM/TC57CIM/IEC61970/Dynamics/StandardModels/WindDynamics#WindContQIEC"/>
        <rdfs:range rdf:resource="https://w3id.org/netbeheer/referentiemodellen/IECCIM/TC57CIM/IEC61970/Base/Domain#PU"/>
        <rdfs:comment>Reactive power PI controller proportional gain (&lt;i&gt;K&lt;/i&gt;&lt;sub&gt;P,q&lt;/sub&gt;). It is type dependent parameter.</rdfs:comment>
    </owl:ObjectProperty>
    


    <!-- https://w3id.org/netbeheer/referentiemodellen/IECCIM/TC57CIM/IEC61970/Dynamics/StandardModels/WindDynamics#WindContQIEC_kpu -->


    <owl:ObjectProperty rdf:about="https://w3id.org/netbeheer/referentiemodellen/IECCIM/TC57CIM/IEC61970/Dynamics/StandardModels/WindDynamics#WindContQIEC_kpu">
        <rdfs:domain rdf:resource="https://w3id.org/netbeheer/referentiemodellen/IECCIM/TC57CIM/IEC61970/Dynamics/StandardModels/WindDynamics#WindContQIEC"/>
        <rdfs:range rdf:resource="https://w3id.org/netbeheer/referentiemodellen/IECCIM/TC57CIM/IEC61970/Base/Domain#PU"/>
        <rdfs:comment>Voltage PI controller proportional gain (&lt;i&gt;K&lt;/i&gt;&lt;sub&gt;P,u&lt;/sub&gt;). It is type dependent parameter.</rdfs:comment>
    </owl:ObjectProperty>
    


    <!-- https://w3id.org/netbeheer/referentiemodellen/IECCIM/TC57CIM/IEC61970/Dynamics/StandardModels/WindDynamics#WindContQIEC_kqv -->


    <owl:ObjectProperty rdf:about="https://w3id.org/netbeheer/referentiemodellen/IECCIM/TC57CIM/IEC61970/Dynamics/StandardModels/WindDynamics#WindContQIEC_kqv">
        <rdfs:domain rdf:resource="https://w3id.org/netbeheer/referentiemodellen/IECCIM/TC57CIM/IEC61970/Dynamics/StandardModels/WindDynamics#WindContQIEC"/>
        <rdfs:range rdf:resource="https://w3id.org/netbeheer/referentiemodellen/IECCIM/TC57CIM/IEC61970/Base/Domain#PU"/>
        <rdfs:comment>Voltage scaling factor for LVRT current (&lt;i&gt;K&lt;/i&gt;&lt;sub&gt;qv&lt;/sub&gt;). It is project dependent parameter.</rdfs:comment>
    </owl:ObjectProperty>
    


    <!-- https://w3id.org/netbeheer/referentiemodellen/IECCIM/TC57CIM/IEC61970/Dynamics/StandardModels/WindDynamics#WindContQIEC_qmax -->


    <owl:ObjectProperty rdf:about="https://w3id.org/netbeheer/referentiemodellen/IECCIM/TC57CIM/IEC61970/Dynamics/StandardModels/WindDynamics#WindContQIEC_qmax">
        <rdfs:domain rdf:resource="https://w3id.org/netbeheer/referentiemodellen/IECCIM/TC57CIM/IEC61970/Dynamics/StandardModels/WindDynamics#WindContQIEC"/>
        <rdfs:range rdf:resource="https://w3id.org/netbeheer/referentiemodellen/IECCIM/TC57CIM/IEC61970/Base/Domain#PU"/>
        <rdfs:comment>Maximum reactive power (q&lt;sub&gt;max&lt;/sub&gt;). It is type dependent parameter.</rdfs:comment>
    </owl:ObjectProperty>
    


    <!-- https://w3id.org/netbeheer/referentiemodellen/IECCIM/TC57CIM/IEC61970/Dynamics/StandardModels/WindDynamics#WindContQIEC_qmin -->


    <owl:ObjectProperty rdf:about="https://w3id.org/netbeheer/referentiemodellen/IECCIM/TC57CIM/IEC61970/Dynamics/StandardModels/WindDynamics#WindContQIEC_qmin">
        <rdfs:domain rdf:resource="https://w3id.org/netbeheer/referentiemodellen/IECCIM/TC57CIM/IEC61970/Dynamics/StandardModels/WindDynamics#WindContQIEC"/>
        <rdfs:range rdf:resource="https://w3id.org/netbeheer/referentiemodellen/IECCIM/TC57CIM/IEC61970/Base/Domain#PU"/>
        <rdfs:comment>Minimum reactive power (q&lt;sub&gt;min&lt;/sub&gt;). It is type dependent parameter.</rdfs:comment>
    </owl:ObjectProperty>
    


    <!-- https://w3id.org/netbeheer/referentiemodellen/IECCIM/TC57CIM/IEC61970/Dynamics/StandardModels/WindDynamics#WindContQIEC_rdroop -->


    <owl:ObjectProperty rdf:about="https://w3id.org/netbeheer/referentiemodellen/IECCIM/TC57CIM/IEC61970/Dynamics/StandardModels/WindDynamics#WindContQIEC_rdroop">
        <rdfs:domain rdf:resource="https://w3id.org/netbeheer/referentiemodellen/IECCIM/TC57CIM/IEC61970/Dynamics/StandardModels/WindDynamics#WindContQIEC"/>
        <rdfs:range rdf:resource="https://w3id.org/netbeheer/referentiemodellen/IECCIM/TC57CIM/IEC61970/Base/Domain#PU"/>
        <rdfs:comment>Resistive component of voltage drop impedance (&lt;i&gt;r&lt;/i&gt;&lt;sub&gt;droop&lt;/sub&gt;). It is project dependent parameter.</rdfs:comment>
    </owl:ObjectProperty>
    


    <!-- https://w3id.org/netbeheer/referentiemodellen/IECCIM/TC57CIM/IEC61970/Dynamics/StandardModels/WindDynamics#WindContQIEC_tiq -->


    <owl:ObjectProperty rdf:about="https://w3id.org/netbeheer/referentiemodellen/IECCIM/TC57CIM/IEC61970/Dynamics/StandardModels/WindDynamics#WindContQIEC_tiq">
        <rdfs:domain rdf:resource="https://w3id.org/netbeheer/referentiemodellen/IECCIM/TC57CIM/IEC61970/Dynamics/StandardModels/WindDynamics#WindContQIEC"/>
        <rdfs:range rdf:resource="https://w3id.org/netbeheer/referentiemodellen/IECCIM/TC57CIM/IEC61970/Base/Domain#Seconds"/>
        <rdfs:comment>Time constant in reactive current lag (T&lt;sub&gt;iq&lt;/sub&gt;). It is type dependent parameter.</rdfs:comment>
    </owl:ObjectProperty>
    


    <!-- https://w3id.org/netbeheer/referentiemodellen/IECCIM/TC57CIM/IEC61970/Dynamics/StandardModels/WindDynamics#WindContQIEC_tpfilt -->


    <owl:ObjectProperty rdf:about="https://w3id.org/netbeheer/referentiemodellen/IECCIM/TC57CIM/IEC61970/Dynamics/StandardModels/WindDynamics#WindContQIEC_tpfilt">
        <rdfs:domain rdf:resource="https://w3id.org/netbeheer/referentiemodellen/IECCIM/TC57CIM/IEC61970/Dynamics/StandardModels/WindDynamics#WindContQIEC"/>
        <rdfs:range rdf:resource="https://w3id.org/netbeheer/referentiemodellen/IECCIM/TC57CIM/IEC61970/Base/Domain#Seconds"/>
        <rdfs:comment>Power measurement filter time constant (&lt;i&gt;T&lt;/i&gt;&lt;sub&gt;pfilt&lt;/sub&gt;). It is type dependent parameter.</rdfs:comment>
    </owl:ObjectProperty>
    


    <!-- https://w3id.org/netbeheer/referentiemodellen/IECCIM/TC57CIM/IEC61970/Dynamics/StandardModels/WindDynamics#WindContQIEC_tpost -->


    <owl:ObjectProperty rdf:about="https://w3id.org/netbeheer/referentiemodellen/IECCIM/TC57CIM/IEC61970/Dynamics/StandardModels/WindDynamics#WindContQIEC_tpost">
        <rdfs:domain rdf:resource="https://w3id.org/netbeheer/referentiemodellen/IECCIM/TC57CIM/IEC61970/Dynamics/StandardModels/WindDynamics#WindContQIEC"/>
        <rdfs:range rdf:resource="https://w3id.org/netbeheer/referentiemodellen/IECCIM/TC57CIM/IEC61970/Base/Domain#Seconds"/>
        <rdfs:comment>Length of time period where post fault reactive power is injected (&lt;i&gt;T&lt;/i&gt;&lt;sub&gt;post&lt;/sub&gt;). It is project dependent parameter.</rdfs:comment>
    </owl:ObjectProperty>
    


    <!-- https://w3id.org/netbeheer/referentiemodellen/IECCIM/TC57CIM/IEC61970/Dynamics/StandardModels/WindDynamics#WindContQIEC_tqord -->


    <owl:ObjectProperty rdf:about="https://w3id.org/netbeheer/referentiemodellen/IECCIM/TC57CIM/IEC61970/Dynamics/StandardModels/WindDynamics#WindContQIEC_tqord">
        <rdfs:domain rdf:resource="https://w3id.org/netbeheer/referentiemodellen/IECCIM/TC57CIM/IEC61970/Dynamics/StandardModels/WindDynamics#WindContQIEC"/>
        <rdfs:range rdf:resource="https://w3id.org/netbeheer/referentiemodellen/IECCIM/TC57CIM/IEC61970/Base/Domain#Seconds"/>
        <rdfs:comment>Time constant in reactive power order lag (&lt;i&gt;T&lt;/i&gt;&lt;sub&gt;qord&lt;/sub&gt;). It is type dependent parameter.</rdfs:comment>
    </owl:ObjectProperty>
    


    <!-- https://w3id.org/netbeheer/referentiemodellen/IECCIM/TC57CIM/IEC61970/Dynamics/StandardModels/WindDynamics#WindContQIEC_tufilt -->


    <owl:ObjectProperty rdf:about="https://w3id.org/netbeheer/referentiemodellen/IECCIM/TC57CIM/IEC61970/Dynamics/StandardModels/WindDynamics#WindContQIEC_tufilt">
        <rdfs:domain rdf:resource="https://w3id.org/netbeheer/referentiemodellen/IECCIM/TC57CIM/IEC61970/Dynamics/StandardModels/WindDynamics#WindContQIEC"/>
        <rdfs:range rdf:resource="https://w3id.org/netbeheer/referentiemodellen/IECCIM/TC57CIM/IEC61970/Base/Domain#Seconds"/>
        <rdfs:comment>Voltage measurement filter time constant (&lt;i&gt;T&lt;/i&gt;&lt;sub&gt;ufilt&lt;/sub&gt;). It is type dependent parameter.</rdfs:comment>
    </owl:ObjectProperty>
    


    <!-- https://w3id.org/netbeheer/referentiemodellen/IECCIM/TC57CIM/IEC61970/Dynamics/StandardModels/WindDynamics#WindContQIEC_udb1 -->


    <owl:ObjectProperty rdf:about="https://w3id.org/netbeheer/referentiemodellen/IECCIM/TC57CIM/IEC61970/Dynamics/StandardModels/WindDynamics#WindContQIEC_udb1">
        <rdfs:domain rdf:resource="https://w3id.org/netbeheer/referentiemodellen/IECCIM/TC57CIM/IEC61970/Dynamics/StandardModels/WindDynamics#WindContQIEC"/>
        <rdfs:range rdf:resource="https://w3id.org/netbeheer/referentiemodellen/IECCIM/TC57CIM/IEC61970/Base/Domain#PU"/>
        <rdfs:comment>Voltage dead band lower limit (&lt;i&gt;u&lt;/i&gt;&lt;sub&gt;db1&lt;/sub&gt;). It is type dependent parameter.</rdfs:comment>
    </owl:ObjectProperty>
    


    <!-- https://w3id.org/netbeheer/referentiemodellen/IECCIM/TC57CIM/IEC61970/Dynamics/StandardModels/WindDynamics#WindContQIEC_udb2 -->


    <owl:ObjectProperty rdf:about="https://w3id.org/netbeheer/referentiemodellen/IECCIM/TC57CIM/IEC61970/Dynamics/StandardModels/WindDynamics#WindContQIEC_udb2">
        <rdfs:domain rdf:resource="https://w3id.org/netbeheer/referentiemodellen/IECCIM/TC57CIM/IEC61970/Dynamics/StandardModels/WindDynamics#WindContQIEC"/>
        <rdfs:range rdf:resource="https://w3id.org/netbeheer/referentiemodellen/IECCIM/TC57CIM/IEC61970/Base/Domain#PU"/>
        <rdfs:comment>Voltage dead band upper limit (&lt;i&gt;u&lt;/i&gt;&lt;sub&gt;db2&lt;/sub&gt;). It is type dependent parameter.</rdfs:comment>
    </owl:ObjectProperty>
    


    <!-- https://w3id.org/netbeheer/referentiemodellen/IECCIM/TC57CIM/IEC61970/Dynamics/StandardModels/WindDynamics#WindContQIEC_umax -->


    <owl:ObjectProperty rdf:about="https://w3id.org/netbeheer/referentiemodellen/IECCIM/TC57CIM/IEC61970/Dynamics/StandardModels/WindDynamics#WindContQIEC_umax">
        <rdfs:domain rdf:resource="https://w3id.org/netbeheer/referentiemodellen/IECCIM/TC57CIM/IEC61970/Dynamics/StandardModels/WindDynamics#WindContQIEC"/>
        <rdfs:range rdf:resource="https://w3id.org/netbeheer/referentiemodellen/IECCIM/TC57CIM/IEC61970/Base/Domain#PU"/>
        <rdfs:comment>Maximum voltage in voltage PI controller integral term (u&lt;sub&gt;max&lt;/sub&gt;). It is type dependent parameter.</rdfs:comment>
    </owl:ObjectProperty>
    


    <!-- https://w3id.org/netbeheer/referentiemodellen/IECCIM/TC57CIM/IEC61970/Dynamics/StandardModels/WindDynamics#WindContQIEC_umin -->


    <owl:ObjectProperty rdf:about="https://w3id.org/netbeheer/referentiemodellen/IECCIM/TC57CIM/IEC61970/Dynamics/StandardModels/WindDynamics#WindContQIEC_umin">
        <rdfs:domain rdf:resource="https://w3id.org/netbeheer/referentiemodellen/IECCIM/TC57CIM/IEC61970/Dynamics/StandardModels/WindDynamics#WindContQIEC"/>
        <rdfs:range rdf:resource="https://w3id.org/netbeheer/referentiemodellen/IECCIM/TC57CIM/IEC61970/Base/Domain#PU"/>
        <rdfs:comment>Minimum voltage in voltage PI controller integral term (u&lt;sub&gt;min&lt;/sub&gt;). It is type dependent parameter.</rdfs:comment>
    </owl:ObjectProperty>
    


    <!-- https://w3id.org/netbeheer/referentiemodellen/IECCIM/TC57CIM/IEC61970/Dynamics/StandardModels/WindDynamics#WindContQIEC_uqdip -->


    <owl:ObjectProperty rdf:about="https://w3id.org/netbeheer/referentiemodellen/IECCIM/TC57CIM/IEC61970/Dynamics/StandardModels/WindDynamics#WindContQIEC_uqdip">
        <rdfs:domain rdf:resource="https://w3id.org/netbeheer/referentiemodellen/IECCIM/TC57CIM/IEC61970/Dynamics/StandardModels/WindDynamics#WindContQIEC"/>
        <rdfs:range rdf:resource="https://w3id.org/netbeheer/referentiemodellen/IECCIM/TC57CIM/IEC61970/Base/Domain#PU"/>
        <rdfs:comment>Voltage threshold for LVRT detection in q control (&lt;i&gt;u&lt;/i&gt;&lt;sub&gt;qdip&lt;/sub&gt;). It is type dependent parameter.</rdfs:comment>
    </owl:ObjectProperty>
    


    <!-- https://w3id.org/netbeheer/referentiemodellen/IECCIM/TC57CIM/IEC61970/Dynamics/StandardModels/WindDynamics#WindContQIEC_uref0 -->


    <owl:ObjectProperty rdf:about="https://w3id.org/netbeheer/referentiemodellen/IECCIM/TC57CIM/IEC61970/Dynamics/StandardModels/WindDynamics#WindContQIEC_uref0">
        <rdfs:domain rdf:resource="https://w3id.org/netbeheer/referentiemodellen/IECCIM/TC57CIM/IEC61970/Dynamics/StandardModels/WindDynamics#WindContQIEC"/>
        <rdfs:range rdf:resource="https://w3id.org/netbeheer/referentiemodellen/IECCIM/TC57CIM/IEC61970/Base/Domain#PU"/>
        <rdfs:comment>User defined bias in voltage reference (&lt;i&gt;u&lt;/i&gt;&lt;sub&gt;ref0&lt;/sub&gt;), used when &lt;i&gt;M&lt;/i&gt;&lt;sub&gt;qG&lt;/sub&gt; =&lt;i&gt; M&lt;/i&gt;&lt;sub&gt;G,u&lt;/sub&gt;. It is case dependent parameter.</rdfs:comment>
    </owl:ObjectProperty>
    


    <!-- https://w3id.org/netbeheer/referentiemodellen/IECCIM/TC57CIM/IEC61970/Dynamics/StandardModels/WindDynamics#WindContQIEC_xdroop -->


    <owl:ObjectProperty rdf:about="https://w3id.org/netbeheer/referentiemodellen/IECCIM/TC57CIM/IEC61970/Dynamics/StandardModels/WindDynamics#WindContQIEC_xdroop">
        <rdfs:domain rdf:resource="https://w3id.org/netbeheer/referentiemodellen/IECCIM/TC57CIM/IEC61970/Dynamics/StandardModels/WindDynamics#WindContQIEC"/>
        <rdfs:range rdf:resource="https://w3id.org/netbeheer/referentiemodellen/IECCIM/TC57CIM/IEC61970/Base/Domain#PU"/>
        <rdfs:comment>Inductive component of voltage drop impedance (&lt;i&gt;x&lt;/i&gt;&lt;sub&gt;droop&lt;/sub&gt;). It is project dependent parameter.</rdfs:comment>
    </owl:ObjectProperty>
    


    <!-- https://w3id.org/netbeheer/referentiemodellen/IECCIM/TC57CIM/IEC61970/Dynamics/StandardModels/WindDynamics#WindContRotorRIEC_WindDynamicsLookupTable -->


    <owl:ObjectProperty rdf:about="https://w3id.org/netbeheer/referentiemodellen/IECCIM/TC57CIM/IEC61970/Dynamics/StandardModels/WindDynamics#WindContRotorRIEC_WindDynamicsLookupTable">
        <owl:inverseOf rdf:resource="https://w3id.org/netbeheer/referentiemodellen/IECCIM/TC57CIM/IEC61970/Dynamics/StandardModels/WindDynamics#WindDynamicsLookupTable_WindContRotorRIEC"/>
        <rdfs:domain rdf:resource="https://w3id.org/netbeheer/referentiemodellen/IECCIM/TC57CIM/IEC61970/Dynamics/StandardModels/WindDynamics#WindContRotorRIEC"/>
        <rdfs:range rdf:resource="https://w3id.org/netbeheer/referentiemodellen/IECCIM/TC57CIM/IEC61970/Dynamics/StandardModels/WindDynamics#WindDynamicsLookupTable"/>
        <rdfs:comment>The wind dynamics lookup table associated with this rotor resistance control model.The rotor resistance control model with which this wind dynamics lookup table is associated.</rdfs:comment>
    </owl:ObjectProperty>
    


    <!-- https://w3id.org/netbeheer/referentiemodellen/IECCIM/TC57CIM/IEC61970/Dynamics/StandardModels/WindDynamics#WindContRotorRIEC_WindGenTurbineType2IEC -->


    <owl:ObjectProperty rdf:about="https://w3id.org/netbeheer/referentiemodellen/IECCIM/TC57CIM/IEC61970/Dynamics/StandardModels/WindDynamics#WindContRotorRIEC_WindGenTurbineType2IEC">
        <rdf:type rdf:resource="http://www.w3.org/2002/07/owl#FunctionalProperty"/>
        <rdfs:domain rdf:resource="https://w3id.org/netbeheer/referentiemodellen/IECCIM/TC57CIM/IEC61970/Dynamics/StandardModels/WindDynamics#WindContRotorRIEC"/>
        <rdfs:range rdf:resource="https://w3id.org/netbeheer/referentiemodellen/IECCIM/TC57CIM/IEC61970/Dynamics/StandardModels/WindDynamics#WindGenTurbineType2IEC"/>
        <rdfs:comment>Wind control rotor resistance model associated with wind turbine type 2 model.Wind turbine type 2 model with whitch this wind control rotor resistance model is associated.</rdfs:comment>
    </owl:ObjectProperty>
    


    <!-- https://w3id.org/netbeheer/referentiemodellen/IECCIM/TC57CIM/IEC61970/Dynamics/StandardModels/WindDynamics#WindContRotorRIEC_kirr -->


    <owl:ObjectProperty rdf:about="https://w3id.org/netbeheer/referentiemodellen/IECCIM/TC57CIM/IEC61970/Dynamics/StandardModels/WindDynamics#WindContRotorRIEC_kirr">
        <rdfs:domain rdf:resource="https://w3id.org/netbeheer/referentiemodellen/IECCIM/TC57CIM/IEC61970/Dynamics/StandardModels/WindDynamics#WindContRotorRIEC"/>
        <rdfs:range rdf:resource="https://w3id.org/netbeheer/referentiemodellen/IECCIM/TC57CIM/IEC61970/Base/Domain#PU"/>
        <rdfs:comment>Integral gain in rotor resistance PI controller (&lt;i&gt;K&lt;/i&gt;&lt;sub&gt;Irr&lt;/sub&gt;). It is type dependent parameter.</rdfs:comment>
    </owl:ObjectProperty>
    


    <!-- https://w3id.org/netbeheer/referentiemodellen/IECCIM/TC57CIM/IEC61970/Dynamics/StandardModels/WindDynamics#WindContRotorRIEC_kprr -->


    <owl:ObjectProperty rdf:about="https://w3id.org/netbeheer/referentiemodellen/IECCIM/TC57CIM/IEC61970/Dynamics/StandardModels/WindDynamics#WindContRotorRIEC_kprr">
        <rdfs:domain rdf:resource="https://w3id.org/netbeheer/referentiemodellen/IECCIM/TC57CIM/IEC61970/Dynamics/StandardModels/WindDynamics#WindContRotorRIEC"/>
        <rdfs:range rdf:resource="https://w3id.org/netbeheer/referentiemodellen/IECCIM/TC57CIM/IEC61970/Base/Domain#PU"/>
        <rdfs:comment>Proportional gain in rotor resistance PI controller (&lt;i&gt;K&lt;/i&gt;&lt;sub&gt;Prr&lt;/sub&gt;). It is type dependent parameter.</rdfs:comment>
    </owl:ObjectProperty>
    


    <!-- https://w3id.org/netbeheer/referentiemodellen/IECCIM/TC57CIM/IEC61970/Dynamics/StandardModels/WindDynamics#WindContRotorRIEC_rmax -->


    <owl:ObjectProperty rdf:about="https://w3id.org/netbeheer/referentiemodellen/IECCIM/TC57CIM/IEC61970/Dynamics/StandardModels/WindDynamics#WindContRotorRIEC_rmax">
        <rdfs:domain rdf:resource="https://w3id.org/netbeheer/referentiemodellen/IECCIM/TC57CIM/IEC61970/Dynamics/StandardModels/WindDynamics#WindContRotorRIEC"/>
        <rdfs:range rdf:resource="https://w3id.org/netbeheer/referentiemodellen/IECCIM/TC57CIM/IEC61970/Base/Domain#PU"/>
        <rdfs:comment>Maximum rotor resistance (&lt;i&gt;r&lt;/i&gt;&lt;sub&gt;max&lt;/sub&gt;). It is type dependent parameter.</rdfs:comment>
    </owl:ObjectProperty>
    


    <!-- https://w3id.org/netbeheer/referentiemodellen/IECCIM/TC57CIM/IEC61970/Dynamics/StandardModels/WindDynamics#WindContRotorRIEC_rmin -->


    <owl:ObjectProperty rdf:about="https://w3id.org/netbeheer/referentiemodellen/IECCIM/TC57CIM/IEC61970/Dynamics/StandardModels/WindDynamics#WindContRotorRIEC_rmin">
        <rdfs:domain rdf:resource="https://w3id.org/netbeheer/referentiemodellen/IECCIM/TC57CIM/IEC61970/Dynamics/StandardModels/WindDynamics#WindContRotorRIEC"/>
        <rdfs:range rdf:resource="https://w3id.org/netbeheer/referentiemodellen/IECCIM/TC57CIM/IEC61970/Base/Domain#PU"/>
        <rdfs:comment>Minimum rotor resistance (&lt;i&gt;r&lt;/i&gt;&lt;sub&gt;min&lt;/sub&gt;). It is type dependent parameter.</rdfs:comment>
    </owl:ObjectProperty>
    


    <!-- https://w3id.org/netbeheer/referentiemodellen/IECCIM/TC57CIM/IEC61970/Dynamics/StandardModels/WindDynamics#WindContRotorRIEC_tomegafilt -->


    <owl:ObjectProperty rdf:about="https://w3id.org/netbeheer/referentiemodellen/IECCIM/TC57CIM/IEC61970/Dynamics/StandardModels/WindDynamics#WindContRotorRIEC_tomegafilt">
        <rdfs:domain rdf:resource="https://w3id.org/netbeheer/referentiemodellen/IECCIM/TC57CIM/IEC61970/Dynamics/StandardModels/WindDynamics#WindContRotorRIEC"/>
        <rdfs:range rdf:resource="https://w3id.org/netbeheer/referentiemodellen/IECCIM/TC57CIM/IEC61970/Base/Domain#Seconds"/>
        <rdfs:comment>Filter time constant for generator speed measurement (&lt;i&gt;T&lt;/i&gt;&lt;sub&gt;omegafilt&lt;/sub&gt;). It is type dependent parameter.</rdfs:comment>
    </owl:ObjectProperty>
    


    <!-- https://w3id.org/netbeheer/referentiemodellen/IECCIM/TC57CIM/IEC61970/Dynamics/StandardModels/WindDynamics#WindContRotorRIEC_tpfilt -->


    <owl:ObjectProperty rdf:about="https://w3id.org/netbeheer/referentiemodellen/IECCIM/TC57CIM/IEC61970/Dynamics/StandardModels/WindDynamics#WindContRotorRIEC_tpfilt">
        <rdfs:domain rdf:resource="https://w3id.org/netbeheer/referentiemodellen/IECCIM/TC57CIM/IEC61970/Dynamics/StandardModels/WindDynamics#WindContRotorRIEC"/>
        <rdfs:range rdf:resource="https://w3id.org/netbeheer/referentiemodellen/IECCIM/TC57CIM/IEC61970/Base/Domain#Seconds"/>
        <rdfs:comment>Filter time constant for power measurement (&lt;i&gt;T&lt;/i&gt;&lt;sub&gt;pfilt&lt;/sub&gt;). It is type dependent parameter.</rdfs:comment>
    </owl:ObjectProperty>
    


    <!-- https://w3id.org/netbeheer/referentiemodellen/IECCIM/TC57CIM/IEC61970/Dynamics/StandardModels/WindDynamics#WindDynamicsLookupTable_WindContCurrLimIEC -->


    <owl:ObjectProperty rdf:about="https://w3id.org/netbeheer/referentiemodellen/IECCIM/TC57CIM/IEC61970/Dynamics/StandardModels/WindDynamics#WindDynamicsLookupTable_WindContCurrLimIEC">
        <rdfs:domain rdf:resource="https://w3id.org/netbeheer/referentiemodellen/IECCIM/TC57CIM/IEC61970/Dynamics/StandardModels/WindDynamics#WindDynamicsLookupTable"/>
        <rdfs:range rdf:resource="https://w3id.org/netbeheer/referentiemodellen/IECCIM/TC57CIM/IEC61970/Dynamics/StandardModels/WindDynamics#WindContCurrLimIEC"/>
        <rdfs:comment>The wind dynamics lookup table associated with this current control limitation model.The current control limitation model with which this wind dynamics lookup table is associated.</rdfs:comment>
    </owl:ObjectProperty>
    


    <!-- https://w3id.org/netbeheer/referentiemodellen/IECCIM/TC57CIM/IEC61970/Dynamics/StandardModels/WindDynamics#WindDynamicsLookupTable_WindContPType3IEC -->


    <owl:ObjectProperty rdf:about="https://w3id.org/netbeheer/referentiemodellen/IECCIM/TC57CIM/IEC61970/Dynamics/StandardModels/WindDynamics#WindDynamicsLookupTable_WindContPType3IEC">
        <rdfs:domain rdf:resource="https://w3id.org/netbeheer/referentiemodellen/IECCIM/TC57CIM/IEC61970/Dynamics/StandardModels/WindDynamics#WindDynamicsLookupTable"/>
        <rdfs:range rdf:resource="https://w3id.org/netbeheer/referentiemodellen/IECCIM/TC57CIM/IEC61970/Dynamics/StandardModels/WindDynamics#WindContPType3IEC"/>
        <rdfs:comment>The wind dynamics lookup table associated with this P control type 3 model.The P control type 3 model with which this wind dynamics lookup table is associated.</rdfs:comment>
    </owl:ObjectProperty>
    


    <!-- https://w3id.org/netbeheer/referentiemodellen/IECCIM/TC57CIM/IEC61970/Dynamics/StandardModels/WindDynamics#WindDynamicsLookupTable_WindContRotorRIEC -->


    <owl:ObjectProperty rdf:about="https://w3id.org/netbeheer/referentiemodellen/IECCIM/TC57CIM/IEC61970/Dynamics/StandardModels/WindDynamics#WindDynamicsLookupTable_WindContRotorRIEC">
        <rdfs:domain rdf:resource="https://w3id.org/netbeheer/referentiemodellen/IECCIM/TC57CIM/IEC61970/Dynamics/StandardModels/WindDynamics#WindDynamicsLookupTable"/>
        <rdfs:range rdf:resource="https://w3id.org/netbeheer/referentiemodellen/IECCIM/TC57CIM/IEC61970/Dynamics/StandardModels/WindDynamics#WindContRotorRIEC"/>
        <rdfs:comment>The wind dynamics lookup table associated with this rotor resistance control model.The rotor resistance control model with which this wind dynamics lookup table is associated.</rdfs:comment>
    </owl:ObjectProperty>
    


    <!-- https://w3id.org/netbeheer/referentiemodellen/IECCIM/TC57CIM/IEC61970/Dynamics/StandardModels/WindDynamics#WindDynamicsLookupTable_WindPlantFreqPcontrolIEC -->


    <owl:ObjectProperty rdf:about="https://w3id.org/netbeheer/referentiemodellen/IECCIM/TC57CIM/IEC61970/Dynamics/StandardModels/WindDynamics#WindDynamicsLookupTable_WindPlantFreqPcontrolIEC">
        <rdfs:domain rdf:resource="https://w3id.org/netbeheer/referentiemodellen/IECCIM/TC57CIM/IEC61970/Dynamics/StandardModels/WindDynamics#WindDynamicsLookupTable"/>
        <rdfs:range rdf:resource="https://w3id.org/netbeheer/referentiemodellen/IECCIM/TC57CIM/IEC61970/Dynamics/StandardModels/WindDynamics#WindPlantFreqPcontrolIEC"/>
        <rdfs:comment>The wind dynamics lookup table associated with this frequency and active power wind plant model.The frequency and active power wind plant control model with which this wind dynamics lookup table is associated.</rdfs:comment>
    </owl:ObjectProperty>
    


    <!-- https://w3id.org/netbeheer/referentiemodellen/IECCIM/TC57CIM/IEC61970/Dynamics/StandardModels/WindDynamics#WindGenTurbineType1IEC_WindAeroConstIEC -->


    <owl:ObjectProperty rdf:about="https://w3id.org/netbeheer/referentiemodellen/IECCIM/TC57CIM/IEC61970/Dynamics/StandardModels/WindDynamics#WindGenTurbineType1IEC_WindAeroConstIEC">
        <owl:inverseOf rdf:resource="https://w3id.org/netbeheer/referentiemodellen/IECCIM/TC57CIM/IEC61970/Dynamics/StandardModels/WindDynamics#WindAeroConstIEC_WindGenTurbineType1IEC"/>
        <rdf:type rdf:resource="http://www.w3.org/2002/07/owl#FunctionalProperty"/>
        <rdfs:domain rdf:resource="https://w3id.org/netbeheer/referentiemodellen/IECCIM/TC57CIM/IEC61970/Dynamics/StandardModels/WindDynamics#WindGenTurbineType1IEC"/>
        <rdfs:range rdf:resource="https://w3id.org/netbeheer/referentiemodellen/IECCIM/TC57CIM/IEC61970/Dynamics/StandardModels/WindDynamics#WindAeroConstIEC"/>
        <rdfs:comment>Wind aerodynamic model associated with this wind turbine type 1 model.Wind turbine type 1 model with which this wind aerodynamic model is associated.</rdfs:comment>
    </owl:ObjectProperty>
    


    <!-- https://w3id.org/netbeheer/referentiemodellen/IECCIM/TC57CIM/IEC61970/Dynamics/StandardModels/WindDynamics#WindGenTurbineType2IEC_WindContRotorRIEC -->


    <owl:ObjectProperty rdf:about="https://w3id.org/netbeheer/referentiemodellen/IECCIM/TC57CIM/IEC61970/Dynamics/StandardModels/WindDynamics#WindGenTurbineType2IEC_WindContRotorRIEC">
        <owl:inverseOf rdf:resource="https://w3id.org/netbeheer/referentiemodellen/IECCIM/TC57CIM/IEC61970/Dynamics/StandardModels/WindDynamics#WindContRotorRIEC_WindGenTurbineType2IEC"/>
        <rdf:type rdf:resource="http://www.w3.org/2002/07/owl#FunctionalProperty"/>
        <rdfs:domain rdf:resource="https://w3id.org/netbeheer/referentiemodellen/IECCIM/TC57CIM/IEC61970/Dynamics/StandardModels/WindDynamics#WindGenTurbineType2IEC"/>
        <rdfs:range rdf:resource="https://w3id.org/netbeheer/referentiemodellen/IECCIM/TC57CIM/IEC61970/Dynamics/StandardModels/WindDynamics#WindContRotorRIEC"/>
        <rdfs:comment>Wind control rotor resistance model associated with wind turbine type 2 model.Wind turbine type 2 model with whitch this wind control rotor resistance model is associated.</rdfs:comment>
    </owl:ObjectProperty>
    


    <!-- https://w3id.org/netbeheer/referentiemodellen/IECCIM/TC57CIM/IEC61970/Dynamics/StandardModels/WindDynamics#WindGenTurbineType2IEC_WindPitchContEmulIEC -->


    <owl:ObjectProperty rdf:about="https://w3id.org/netbeheer/referentiemodellen/IECCIM/TC57CIM/IEC61970/Dynamics/StandardModels/WindDynamics#WindGenTurbineType2IEC_WindPitchContEmulIEC">
        <owl:inverseOf rdf:resource="https://w3id.org/netbeheer/referentiemodellen/IECCIM/TC57CIM/IEC61970/Dynamics/StandardModels/WindDynamics#WindPitchContEmulIEC_WindGenTurbineType2IEC"/>
        <rdf:type rdf:resource="http://www.w3.org/2002/07/owl#FunctionalProperty"/>
        <rdfs:domain rdf:resource="https://w3id.org/netbeheer/referentiemodellen/IECCIM/TC57CIM/IEC61970/Dynamics/StandardModels/WindDynamics#WindGenTurbineType2IEC"/>
        <rdfs:range rdf:resource="https://w3id.org/netbeheer/referentiemodellen/IECCIM/TC57CIM/IEC61970/Dynamics/StandardModels/WindDynamics#WindPitchContEmulIEC"/>
        <rdfs:comment>Pitch control emulator model associated with this wind turbine type 2 model.Wind turbine type 2 model with which this Pitch control emulator model is associated.</rdfs:comment>
    </owl:ObjectProperty>
    


    <!-- https://w3id.org/netbeheer/referentiemodellen/IECCIM/TC57CIM/IEC61970/Dynamics/StandardModels/WindDynamics#WindGenTurbineType3IEC_WindAeroLinearIEC -->


    <owl:ObjectProperty rdf:about="https://w3id.org/netbeheer/referentiemodellen/IECCIM/TC57CIM/IEC61970/Dynamics/StandardModels/WindDynamics#WindGenTurbineType3IEC_WindAeroLinearIEC">
        <owl:inverseOf rdf:resource="https://w3id.org/netbeheer/referentiemodellen/IECCIM/TC57CIM/IEC61970/Dynamics/StandardModels/WindDynamics#WindAeroLinearIEC_WindGenTurbineType3IEC"/>
        <rdf:type rdf:resource="http://www.w3.org/2002/07/owl#FunctionalProperty"/>
        <rdfs:domain rdf:resource="https://w3id.org/netbeheer/referentiemodellen/IECCIM/TC57CIM/IEC61970/Dynamics/StandardModels/WindDynamics#WindGenTurbineType3IEC"/>
        <rdfs:range rdf:resource="https://w3id.org/netbeheer/referentiemodellen/IECCIM/TC57CIM/IEC61970/Dynamics/StandardModels/WindDynamics#WindAeroLinearIEC"/>
        <rdfs:comment>Wind aerodynamic model associated with this wind generator type 3 model.Wind generator type 3 model with which this wind aerodynamic model is associated.</rdfs:comment>
    </owl:ObjectProperty>
    


    <!-- https://w3id.org/netbeheer/referentiemodellen/IECCIM/TC57CIM/IEC61970/Dynamics/StandardModels/WindDynamics#WindGenTurbineType3IEC_WindContPType3IEC -->


    <owl:ObjectProperty rdf:about="https://w3id.org/netbeheer/referentiemodellen/IECCIM/TC57CIM/IEC61970/Dynamics/StandardModels/WindDynamics#WindGenTurbineType3IEC_WindContPType3IEC">
        <owl:inverseOf rdf:resource="https://w3id.org/netbeheer/referentiemodellen/IECCIM/TC57CIM/IEC61970/Dynamics/StandardModels/WindDynamics#WindContPType3IEC_WindGenTurbineType3IEC"/>
        <rdf:type rdf:resource="http://www.w3.org/2002/07/owl#FunctionalProperty"/>
        <rdfs:domain rdf:resource="https://w3id.org/netbeheer/referentiemodellen/IECCIM/TC57CIM/IEC61970/Dynamics/StandardModels/WindDynamics#WindGenTurbineType3IEC"/>
        <rdfs:range rdf:resource="https://w3id.org/netbeheer/referentiemodellen/IECCIM/TC57CIM/IEC61970/Dynamics/StandardModels/WindDynamics#WindContPType3IEC"/>
        <rdfs:comment>Wind control P type 3 model associated with this wind turbine type 3 model.Wind turbine type 3 model with which this Wind control P type 3 model is associated.</rdfs:comment>
    </owl:ObjectProperty>
    


    <!-- https://w3id.org/netbeheer/referentiemodellen/IECCIM/TC57CIM/IEC61970/Dynamics/StandardModels/WindDynamics#WindGenTurbineType3IEC_WindContPitchAngleIEC -->


    <owl:ObjectProperty rdf:about="https://w3id.org/netbeheer/referentiemodellen/IECCIM/TC57CIM/IEC61970/Dynamics/StandardModels/WindDynamics#WindGenTurbineType3IEC_WindContPitchAngleIEC">
        <owl:inverseOf rdf:resource="https://w3id.org/netbeheer/referentiemodellen/IECCIM/TC57CIM/IEC61970/Dynamics/StandardModels/WindDynamics#WindContPitchAngleIEC_WindGenTurbineType3IEC"/>
        <rdf:type rdf:resource="http://www.w3.org/2002/07/owl#FunctionalProperty"/>
        <rdfs:domain rdf:resource="https://w3id.org/netbeheer/referentiemodellen/IECCIM/TC57CIM/IEC61970/Dynamics/StandardModels/WindDynamics#WindGenTurbineType3IEC"/>
        <rdfs:range rdf:resource="https://w3id.org/netbeheer/referentiemodellen/IECCIM/TC57CIM/IEC61970/Dynamics/StandardModels/WindDynamics#WindContPitchAngleIEC"/>
        <rdfs:comment>Wind control pitch angle model associated with this wind turbine type 3.Wind turbine type 3 model with which this pitch control model is associated.</rdfs:comment>
    </owl:ObjectProperty>
    


    <!-- https://w3id.org/netbeheer/referentiemodellen/IECCIM/TC57CIM/IEC61970/Dynamics/StandardModels/WindDynamics#WindGenTurbineType3IEC_WindMechIEC -->


    <owl:ObjectProperty rdf:about="https://w3id.org/netbeheer/referentiemodellen/IECCIM/TC57CIM/IEC61970/Dynamics/StandardModels/WindDynamics#WindGenTurbineType3IEC_WindMechIEC">
        <owl:inverseOf rdf:resource="https://w3id.org/netbeheer/referentiemodellen/IECCIM/TC57CIM/IEC61970/Dynamics/StandardModels/WindDynamics#WindMechIEC_WindGenTurbineType3IEC"/>
        <rdfs:domain rdf:resource="https://w3id.org/netbeheer/referentiemodellen/IECCIM/TC57CIM/IEC61970/Dynamics/StandardModels/WindDynamics#WindGenTurbineType3IEC"/>
        <rdfs:range rdf:resource="https://w3id.org/netbeheer/referentiemodellen/IECCIM/TC57CIM/IEC61970/Dynamics/StandardModels/WindDynamics#WindMechIEC"/>
        <rdfs:comment>Wind mechanical model associated with this wind turbine Type 3 model.Wind turbine Type 3 model with which this wind mechanical model is associated.</rdfs:comment>
    </owl:ObjectProperty>
    


    <!-- https://w3id.org/netbeheer/referentiemodellen/IECCIM/TC57CIM/IEC61970/Dynamics/StandardModels/WindDynamics#WindGenTurbineType3IEC_dipmax -->


    <owl:ObjectProperty rdf:about="https://w3id.org/netbeheer/referentiemodellen/IECCIM/TC57CIM/IEC61970/Dynamics/StandardModels/WindDynamics#WindGenTurbineType3IEC_dipmax">
        <rdfs:domain rdf:resource="https://w3id.org/netbeheer/referentiemodellen/IECCIM/TC57CIM/IEC61970/Dynamics/StandardModels/WindDynamics#WindGenTurbineType3IEC"/>
        <rdfs:range rdf:resource="https://w3id.org/netbeheer/referentiemodellen/IECCIM/TC57CIM/IEC61970/Base/Domain#PU"/>
        <rdfs:comment>Maximum active current ramp rate (di&lt;sub&gt;pmax&lt;/sub&gt;). It is project dependent parameter.</rdfs:comment>
    </owl:ObjectProperty>
    


    <!-- https://w3id.org/netbeheer/referentiemodellen/IECCIM/TC57CIM/IEC61970/Dynamics/StandardModels/WindDynamics#WindGenTurbineType3IEC_diqmax -->


    <owl:ObjectProperty rdf:about="https://w3id.org/netbeheer/referentiemodellen/IECCIM/TC57CIM/IEC61970/Dynamics/StandardModels/WindDynamics#WindGenTurbineType3IEC_diqmax">
        <rdfs:domain rdf:resource="https://w3id.org/netbeheer/referentiemodellen/IECCIM/TC57CIM/IEC61970/Dynamics/StandardModels/WindDynamics#WindGenTurbineType3IEC"/>
        <rdfs:range rdf:resource="https://w3id.org/netbeheer/referentiemodellen/IECCIM/TC57CIM/IEC61970/Base/Domain#PU"/>
        <rdfs:comment>Maximum reactive current ramp rate (di&lt;sub&gt;qmax&lt;/sub&gt;). It is project dependent parameter.</rdfs:comment>
    </owl:ObjectProperty>
    


    <!-- https://w3id.org/netbeheer/referentiemodellen/IECCIM/TC57CIM/IEC61970/Dynamics/StandardModels/WindDynamics#WindGenTurbineType3aIEC_tic -->


    <owl:ObjectProperty rdf:about="https://w3id.org/netbeheer/referentiemodellen/IECCIM/TC57CIM/IEC61970/Dynamics/StandardModels/WindDynamics#WindGenTurbineType3aIEC_tic">
        <rdfs:domain rdf:resource="https://w3id.org/netbeheer/referentiemodellen/IECCIM/TC57CIM/IEC61970/Dynamics/StandardModels/WindDynamics#WindGenTurbineType3aIEC"/>
        <rdfs:range rdf:resource="https://w3id.org/netbeheer/referentiemodellen/IECCIM/TC57CIM/IEC61970/Base/Domain#Seconds"/>
        <rdfs:comment>Current PI controller integration time constant (T&lt;sub&gt;Ic&lt;/sub&gt;). It is type dependent parameter.</rdfs:comment>
    </owl:ObjectProperty>
    


    <!-- https://w3id.org/netbeheer/referentiemodellen/IECCIM/TC57CIM/IEC61970/Dynamics/StandardModels/WindDynamics#WindGenTurbineType3aIEC_xs -->


    <owl:ObjectProperty rdf:about="https://w3id.org/netbeheer/referentiemodellen/IECCIM/TC57CIM/IEC61970/Dynamics/StandardModels/WindDynamics#WindGenTurbineType3aIEC_xs">
        <rdfs:domain rdf:resource="https://w3id.org/netbeheer/referentiemodellen/IECCIM/TC57CIM/IEC61970/Dynamics/StandardModels/WindDynamics#WindGenTurbineType3aIEC"/>
        <rdfs:range rdf:resource="https://w3id.org/netbeheer/referentiemodellen/IECCIM/TC57CIM/IEC61970/Base/Domain#PU"/>
        <rdfs:comment>Electromagnetic transient reactance (x&lt;sub&gt;S&lt;/sub&gt;). It is type dependent parameter.</rdfs:comment>
    </owl:ObjectProperty>
    


    <!-- https://w3id.org/netbeheer/referentiemodellen/IECCIM/TC57CIM/IEC61970/Dynamics/StandardModels/WindDynamics#WindGenTurbineType3bIEC_tg -->


    <owl:ObjectProperty rdf:about="https://w3id.org/netbeheer/referentiemodellen/IECCIM/TC57CIM/IEC61970/Dynamics/StandardModels/WindDynamics#WindGenTurbineType3bIEC_tg">
        <rdfs:domain rdf:resource="https://w3id.org/netbeheer/referentiemodellen/IECCIM/TC57CIM/IEC61970/Dynamics/StandardModels/WindDynamics#WindGenTurbineType3bIEC"/>
        <rdfs:range rdf:resource="https://w3id.org/netbeheer/referentiemodellen/IECCIM/TC57CIM/IEC61970/Base/Domain#Seconds"/>
        <rdfs:comment>Current generation Time constant (&lt;i&gt;T&lt;/i&gt;&lt;sub&gt;g&lt;/sub&gt;). It is type dependent parameter.</rdfs:comment>
    </owl:ObjectProperty>
    


    <!-- https://w3id.org/netbeheer/referentiemodellen/IECCIM/TC57CIM/IEC61970/Dynamics/StandardModels/WindDynamics#WindGenTurbineType3bIEC_two -->


    <owl:ObjectProperty rdf:about="https://w3id.org/netbeheer/referentiemodellen/IECCIM/TC57CIM/IEC61970/Dynamics/StandardModels/WindDynamics#WindGenTurbineType3bIEC_two">
        <rdfs:domain rdf:resource="https://w3id.org/netbeheer/referentiemodellen/IECCIM/TC57CIM/IEC61970/Dynamics/StandardModels/WindDynamics#WindGenTurbineType3bIEC"/>
        <rdfs:range rdf:resource="https://w3id.org/netbeheer/referentiemodellen/IECCIM/TC57CIM/IEC61970/Base/Domain#Seconds"/>
        <rdfs:comment>Time constant for crowbar washout filter (&lt;i&gt;T&lt;/i&gt;&lt;sub&gt;wo&lt;/sub&gt;). It is case dependent parameter.</rdfs:comment>
    </owl:ObjectProperty>
    


    <!-- https://w3id.org/netbeheer/referentiemodellen/IECCIM/TC57CIM/IEC61970/Dynamics/StandardModels/WindDynamics#WindGenTurbineType3bIEC_xs -->


    <owl:ObjectProperty rdf:about="https://w3id.org/netbeheer/referentiemodellen/IECCIM/TC57CIM/IEC61970/Dynamics/StandardModels/WindDynamics#WindGenTurbineType3bIEC_xs">
        <rdfs:domain rdf:resource="https://w3id.org/netbeheer/referentiemodellen/IECCIM/TC57CIM/IEC61970/Dynamics/StandardModels/WindDynamics#WindGenTurbineType3bIEC"/>
        <rdfs:range rdf:resource="https://w3id.org/netbeheer/referentiemodellen/IECCIM/TC57CIM/IEC61970/Base/Domain#PU"/>
        <rdfs:comment>Electromagnetic transient reactance (x&lt;sub&gt;S&lt;/sub&gt;). It is type dependent parameter.</rdfs:comment>
    </owl:ObjectProperty>
    


    <!-- https://w3id.org/netbeheer/referentiemodellen/IECCIM/TC57CIM/IEC61970/Dynamics/StandardModels/WindDynamics#WindGenType4IEC_dipmax -->


    <owl:ObjectProperty rdf:about="https://w3id.org/netbeheer/referentiemodellen/IECCIM/TC57CIM/IEC61970/Dynamics/StandardModels/WindDynamics#WindGenType4IEC_dipmax">
        <rdfs:domain rdf:resource="https://w3id.org/netbeheer/referentiemodellen/IECCIM/TC57CIM/IEC61970/Dynamics/StandardModels/WindDynamics#WindGenType4IEC"/>
        <rdfs:range rdf:resource="https://w3id.org/netbeheer/referentiemodellen/IECCIM/TC57CIM/IEC61970/Base/Domain#PU"/>
        <rdfs:comment>Maximum active current ramp rate (di&lt;sub&gt;pmax&lt;/sub&gt;). It is project dependent parameter.</rdfs:comment>
    </owl:ObjectProperty>
    


    <!-- https://w3id.org/netbeheer/referentiemodellen/IECCIM/TC57CIM/IEC61970/Dynamics/StandardModels/WindDynamics#WindGenType4IEC_diqmax -->


    <owl:ObjectProperty rdf:about="https://w3id.org/netbeheer/referentiemodellen/IECCIM/TC57CIM/IEC61970/Dynamics/StandardModels/WindDynamics#WindGenType4IEC_diqmax">
        <rdfs:domain rdf:resource="https://w3id.org/netbeheer/referentiemodellen/IECCIM/TC57CIM/IEC61970/Dynamics/StandardModels/WindDynamics#WindGenType4IEC"/>
        <rdfs:range rdf:resource="https://w3id.org/netbeheer/referentiemodellen/IECCIM/TC57CIM/IEC61970/Base/Domain#PU"/>
        <rdfs:comment>Maximum reactive current ramp rate (di&lt;sub&gt;qmax&lt;/sub&gt;). It is project dependent parameter.</rdfs:comment>
    </owl:ObjectProperty>
    


    <!-- https://w3id.org/netbeheer/referentiemodellen/IECCIM/TC57CIM/IEC61970/Dynamics/StandardModels/WindDynamics#WindGenType4IEC_diqmin -->


    <owl:ObjectProperty rdf:about="https://w3id.org/netbeheer/referentiemodellen/IECCIM/TC57CIM/IEC61970/Dynamics/StandardModels/WindDynamics#WindGenType4IEC_diqmin">
        <rdfs:domain rdf:resource="https://w3id.org/netbeheer/referentiemodellen/IECCIM/TC57CIM/IEC61970/Dynamics/StandardModels/WindDynamics#WindGenType4IEC"/>
        <rdfs:range rdf:resource="https://w3id.org/netbeheer/referentiemodellen/IECCIM/TC57CIM/IEC61970/Base/Domain#PU"/>
        <rdfs:comment>Minimum reactive current ramp rate (d&lt;i&gt;i&lt;/i&gt;&lt;sub&gt;qmin&lt;/sub&gt;). It is case dependent parameter.</rdfs:comment>
    </owl:ObjectProperty>
    


    <!-- https://w3id.org/netbeheer/referentiemodellen/IECCIM/TC57CIM/IEC61970/Dynamics/StandardModels/WindDynamics#WindGenType4IEC_tg -->


    <owl:ObjectProperty rdf:about="https://w3id.org/netbeheer/referentiemodellen/IECCIM/TC57CIM/IEC61970/Dynamics/StandardModels/WindDynamics#WindGenType4IEC_tg">
        <rdfs:domain rdf:resource="https://w3id.org/netbeheer/referentiemodellen/IECCIM/TC57CIM/IEC61970/Dynamics/StandardModels/WindDynamics#WindGenType4IEC"/>
        <rdfs:range rdf:resource="https://w3id.org/netbeheer/referentiemodellen/IECCIM/TC57CIM/IEC61970/Base/Domain#Seconds"/>
        <rdfs:comment>Time constant (T&lt;sub&gt;g&lt;/sub&gt;). It is type dependent parameter.</rdfs:comment>
    </owl:ObjectProperty>
    


    <!-- https://w3id.org/netbeheer/referentiemodellen/IECCIM/TC57CIM/IEC61970/Dynamics/StandardModels/WindDynamics#WindMechIEC_WindGenTurbineType3IEC -->


    <owl:ObjectProperty rdf:about="https://w3id.org/netbeheer/referentiemodellen/IECCIM/TC57CIM/IEC61970/Dynamics/StandardModels/WindDynamics#WindMechIEC_WindGenTurbineType3IEC">
        <rdf:type rdf:resource="http://www.w3.org/2002/07/owl#FunctionalProperty"/>
        <rdfs:domain rdf:resource="https://w3id.org/netbeheer/referentiemodellen/IECCIM/TC57CIM/IEC61970/Dynamics/StandardModels/WindDynamics#WindMechIEC"/>
        <rdfs:range rdf:resource="https://w3id.org/netbeheer/referentiemodellen/IECCIM/TC57CIM/IEC61970/Dynamics/StandardModels/WindDynamics#WindGenTurbineType3IEC"/>
        <rdfs:comment>Wind mechanical model associated with this wind turbine Type 3 model.Wind turbine Type 3 model with which this wind mechanical model is associated.</rdfs:comment>
    </owl:ObjectProperty>
    


    <!-- https://w3id.org/netbeheer/referentiemodellen/IECCIM/TC57CIM/IEC61970/Dynamics/StandardModels/WindDynamics#WindMechIEC_WindTurbineType1or2IEC -->


    <owl:ObjectProperty rdf:about="https://w3id.org/netbeheer/referentiemodellen/IECCIM/TC57CIM/IEC61970/Dynamics/StandardModels/WindDynamics#WindMechIEC_WindTurbineType1or2IEC">
        <rdf:type rdf:resource="http://www.w3.org/2002/07/owl#FunctionalProperty"/>
        <rdfs:domain rdf:resource="https://w3id.org/netbeheer/referentiemodellen/IECCIM/TC57CIM/IEC61970/Dynamics/StandardModels/WindDynamics#WindMechIEC"/>
        <rdfs:range rdf:resource="https://w3id.org/netbeheer/referentiemodellen/IECCIM/TC57CIM/IEC61970/Dynamics/StandardModels/WindDynamics#WindTurbineType1or2IEC"/>
        <rdfs:comment>Wind mechanical model associated with this wind generator type 1 or 2 model.Wind generator type 1 or 2 model with which this wind mechanical model is associated.</rdfs:comment>
    </owl:ObjectProperty>
    


    <!-- https://w3id.org/netbeheer/referentiemodellen/IECCIM/TC57CIM/IEC61970/Dynamics/StandardModels/WindDynamics#WindMechIEC_WindTurbineType4bIEC -->


    <owl:ObjectProperty rdf:about="https://w3id.org/netbeheer/referentiemodellen/IECCIM/TC57CIM/IEC61970/Dynamics/StandardModels/WindDynamics#WindMechIEC_WindTurbineType4bIEC">
        <rdf:type rdf:resource="http://www.w3.org/2002/07/owl#FunctionalProperty"/>
        <rdfs:domain rdf:resource="https://w3id.org/netbeheer/referentiemodellen/IECCIM/TC57CIM/IEC61970/Dynamics/StandardModels/WindDynamics#WindMechIEC"/>
        <rdfs:range rdf:resource="https://w3id.org/netbeheer/referentiemodellen/IECCIM/TC57CIM/IEC61970/Dynamics/StandardModels/WindDynamics#WindTurbineType4bIEC"/>
        <rdfs:comment>Wind mechanical model associated with this wind turbine Type 4B model.Wind turbine type 4B model with which this wind mechanical model is associated.</rdfs:comment>
    </owl:ObjectProperty>
    


    <!-- https://w3id.org/netbeheer/referentiemodellen/IECCIM/TC57CIM/IEC61970/Dynamics/StandardModels/WindDynamics#WindMechIEC_cdrt -->


    <owl:ObjectProperty rdf:about="https://w3id.org/netbeheer/referentiemodellen/IECCIM/TC57CIM/IEC61970/Dynamics/StandardModels/WindDynamics#WindMechIEC_cdrt">
        <rdfs:domain rdf:resource="https://w3id.org/netbeheer/referentiemodellen/IECCIM/TC57CIM/IEC61970/Dynamics/StandardModels/WindDynamics#WindMechIEC"/>
        <rdfs:range rdf:resource="https://w3id.org/netbeheer/referentiemodellen/IECCIM/TC57CIM/IEC61970/Base/Domain#PU"/>
        <rdfs:comment>Drive train damping (&lt;i&gt;c&lt;/i&gt;&lt;i&gt;&lt;sub&gt;drt&lt;/sub&gt;&lt;/i&gt;&lt;i&gt;)&lt;/i&gt;. It is type dependent parameter.</rdfs:comment>
    </owl:ObjectProperty>
    


    <!-- https://w3id.org/netbeheer/referentiemodellen/IECCIM/TC57CIM/IEC61970/Dynamics/StandardModels/WindDynamics#WindMechIEC_hgen -->


    <owl:ObjectProperty rdf:about="https://w3id.org/netbeheer/referentiemodellen/IECCIM/TC57CIM/IEC61970/Dynamics/StandardModels/WindDynamics#WindMechIEC_hgen">
        <rdfs:domain rdf:resource="https://w3id.org/netbeheer/referentiemodellen/IECCIM/TC57CIM/IEC61970/Dynamics/StandardModels/WindDynamics#WindMechIEC"/>
        <rdfs:range rdf:resource="https://w3id.org/netbeheer/referentiemodellen/IECCIM/TC57CIM/IEC61970/Base/Domain#Seconds"/>
        <rdfs:comment>Inertia constant of generator (&lt;i&gt;H&lt;/i&gt;&lt;sub&gt;gen&lt;/sub&gt;). It is type dependent parameter.</rdfs:comment>
    </owl:ObjectProperty>
    


    <!-- https://w3id.org/netbeheer/referentiemodellen/IECCIM/TC57CIM/IEC61970/Dynamics/StandardModels/WindDynamics#WindMechIEC_hwtr -->


    <owl:ObjectProperty rdf:about="https://w3id.org/netbeheer/referentiemodellen/IECCIM/TC57CIM/IEC61970/Dynamics/StandardModels/WindDynamics#WindMechIEC_hwtr">
        <rdfs:domain rdf:resource="https://w3id.org/netbeheer/referentiemodellen/IECCIM/TC57CIM/IEC61970/Dynamics/StandardModels/WindDynamics#WindMechIEC"/>
        <rdfs:range rdf:resource="https://w3id.org/netbeheer/referentiemodellen/IECCIM/TC57CIM/IEC61970/Base/Domain#Seconds"/>
        <rdfs:comment>Inertia constant of wind turbine rotor (&lt;i&gt;H&lt;/i&gt;&lt;sub&gt;WTR&lt;/sub&gt;). It is type dependent parameter.</rdfs:comment>
    </owl:ObjectProperty>
    


    <!-- https://w3id.org/netbeheer/referentiemodellen/IECCIM/TC57CIM/IEC61970/Dynamics/StandardModels/WindDynamics#WindMechIEC_kdrt -->


    <owl:ObjectProperty rdf:about="https://w3id.org/netbeheer/referentiemodellen/IECCIM/TC57CIM/IEC61970/Dynamics/StandardModels/WindDynamics#WindMechIEC_kdrt">
        <rdfs:domain rdf:resource="https://w3id.org/netbeheer/referentiemodellen/IECCIM/TC57CIM/IEC61970/Dynamics/StandardModels/WindDynamics#WindMechIEC"/>
        <rdfs:range rdf:resource="https://w3id.org/netbeheer/referentiemodellen/IECCIM/TC57CIM/IEC61970/Base/Domain#PU"/>
        <rdfs:comment>Drive train stiffness (&lt;i&gt;k&lt;/i&gt;&lt;i&gt;&lt;sub&gt;drt&lt;/sub&gt;&lt;/i&gt;). It is type dependent parameter.</rdfs:comment>
    </owl:ObjectProperty>
    


    <!-- https://w3id.org/netbeheer/referentiemodellen/IECCIM/TC57CIM/IEC61970/Dynamics/StandardModels/WindDynamics#WindPitchContEmulIEC_WindGenTurbineType2IEC -->


    <owl:ObjectProperty rdf:about="https://w3id.org/netbeheer/referentiemodellen/IECCIM/TC57CIM/IEC61970/Dynamics/StandardModels/WindDynamics#WindPitchContEmulIEC_WindGenTurbineType2IEC">
        <rdf:type rdf:resource="http://www.w3.org/2002/07/owl#FunctionalProperty"/>
        <rdfs:domain rdf:resource="https://w3id.org/netbeheer/referentiemodellen/IECCIM/TC57CIM/IEC61970/Dynamics/StandardModels/WindDynamics#WindPitchContEmulIEC"/>
        <rdfs:range rdf:resource="https://w3id.org/netbeheer/referentiemodellen/IECCIM/TC57CIM/IEC61970/Dynamics/StandardModels/WindDynamics#WindGenTurbineType2IEC"/>
        <rdfs:comment>Pitch control emulator model associated with this wind turbine type 2 model.Wind turbine type 2 model with which this Pitch control emulator model is associated.</rdfs:comment>
    </owl:ObjectProperty>
    


    <!-- https://w3id.org/netbeheer/referentiemodellen/IECCIM/TC57CIM/IEC61970/Dynamics/StandardModels/WindDynamics#WindPitchContEmulIEC_komegaaero -->


    <owl:ObjectProperty rdf:about="https://w3id.org/netbeheer/referentiemodellen/IECCIM/TC57CIM/IEC61970/Dynamics/StandardModels/WindDynamics#WindPitchContEmulIEC_komegaaero">
        <rdfs:domain rdf:resource="https://w3id.org/netbeheer/referentiemodellen/IECCIM/TC57CIM/IEC61970/Dynamics/StandardModels/WindDynamics#WindPitchContEmulIEC"/>
        <rdfs:range rdf:resource="https://w3id.org/netbeheer/referentiemodellen/IECCIM/TC57CIM/IEC61970/Base/Domain#PU"/>
        <rdfs:comment>Aerodynamic power change vs. omega&lt;sub&gt;WTR &lt;/sub&gt;change (&lt;i&gt;K&lt;/i&gt;&lt;sub&gt;omegaaero&lt;/sub&gt;). It is case dependent parameter.</rdfs:comment>
    </owl:ObjectProperty>
    


    <!-- https://w3id.org/netbeheer/referentiemodellen/IECCIM/TC57CIM/IEC61970/Dynamics/StandardModels/WindDynamics#WindPitchContEmulIEC_omegaref -->


    <owl:ObjectProperty rdf:about="https://w3id.org/netbeheer/referentiemodellen/IECCIM/TC57CIM/IEC61970/Dynamics/StandardModels/WindDynamics#WindPitchContEmulIEC_omegaref">
        <rdfs:domain rdf:resource="https://w3id.org/netbeheer/referentiemodellen/IECCIM/TC57CIM/IEC61970/Dynamics/StandardModels/WindDynamics#WindPitchContEmulIEC"/>
        <rdfs:range rdf:resource="https://w3id.org/netbeheer/referentiemodellen/IECCIM/TC57CIM/IEC61970/Base/Domain#PU"/>
        <rdfs:comment>Rotor speed in initial steady state (omega&lt;sub&gt;ref&lt;/sub&gt;). It is case dependent parameter.</rdfs:comment>
    </owl:ObjectProperty>
    


    <!-- https://w3id.org/netbeheer/referentiemodellen/IECCIM/TC57CIM/IEC61970/Dynamics/StandardModels/WindDynamics#WindPitchContEmulIEC_pimax -->


    <owl:ObjectProperty rdf:about="https://w3id.org/netbeheer/referentiemodellen/IECCIM/TC57CIM/IEC61970/Dynamics/StandardModels/WindDynamics#WindPitchContEmulIEC_pimax">
        <rdfs:domain rdf:resource="https://w3id.org/netbeheer/referentiemodellen/IECCIM/TC57CIM/IEC61970/Dynamics/StandardModels/WindDynamics#WindPitchContEmulIEC"/>
        <rdfs:range rdf:resource="https://w3id.org/netbeheer/referentiemodellen/IECCIM/TC57CIM/IEC61970/Base/Domain#PU"/>
        <rdfs:comment>Maximum steady state power (&lt;i&gt;p&lt;/i&gt;&lt;sub&gt;imax&lt;/sub&gt;). It is case dependent parameter.</rdfs:comment>
    </owl:ObjectProperty>
    


    <!-- https://w3id.org/netbeheer/referentiemodellen/IECCIM/TC57CIM/IEC61970/Dynamics/StandardModels/WindDynamics#WindPitchContEmulIEC_pimin -->


    <owl:ObjectProperty rdf:about="https://w3id.org/netbeheer/referentiemodellen/IECCIM/TC57CIM/IEC61970/Dynamics/StandardModels/WindDynamics#WindPitchContEmulIEC_pimin">
        <rdfs:domain rdf:resource="https://w3id.org/netbeheer/referentiemodellen/IECCIM/TC57CIM/IEC61970/Dynamics/StandardModels/WindDynamics#WindPitchContEmulIEC"/>
        <rdfs:range rdf:resource="https://w3id.org/netbeheer/referentiemodellen/IECCIM/TC57CIM/IEC61970/Base/Domain#PU"/>
        <rdfs:comment>Minimum steady state power (&lt;i&gt;p&lt;/i&gt;&lt;sub&gt;imin&lt;/sub&gt;). It is case dependent parameter.</rdfs:comment>
    </owl:ObjectProperty>
    


    <!-- https://w3id.org/netbeheer/referentiemodellen/IECCIM/TC57CIM/IEC61970/Dynamics/StandardModels/WindDynamics#WindPitchContEmulIEC_t1 -->


    <owl:ObjectProperty rdf:about="https://w3id.org/netbeheer/referentiemodellen/IECCIM/TC57CIM/IEC61970/Dynamics/StandardModels/WindDynamics#WindPitchContEmulIEC_t1">
        <rdfs:domain rdf:resource="https://w3id.org/netbeheer/referentiemodellen/IECCIM/TC57CIM/IEC61970/Dynamics/StandardModels/WindDynamics#WindPitchContEmulIEC"/>
        <rdfs:range rdf:resource="https://w3id.org/netbeheer/referentiemodellen/IECCIM/TC57CIM/IEC61970/Base/Domain#Seconds"/>
        <rdfs:comment>First time constant in pitch control lag (&lt;i&gt;T&lt;/i&gt;&lt;sub&gt;1&lt;/sub&gt;). It is type dependent parameter.</rdfs:comment>
    </owl:ObjectProperty>
    


    <!-- https://w3id.org/netbeheer/referentiemodellen/IECCIM/TC57CIM/IEC61970/Dynamics/StandardModels/WindDynamics#WindPitchContEmulIEC_t2 -->


    <owl:ObjectProperty rdf:about="https://w3id.org/netbeheer/referentiemodellen/IECCIM/TC57CIM/IEC61970/Dynamics/StandardModels/WindDynamics#WindPitchContEmulIEC_t2">
        <rdfs:domain rdf:resource="https://w3id.org/netbeheer/referentiemodellen/IECCIM/TC57CIM/IEC61970/Dynamics/StandardModels/WindDynamics#WindPitchContEmulIEC"/>
        <rdfs:range rdf:resource="https://w3id.org/netbeheer/referentiemodellen/IECCIM/TC57CIM/IEC61970/Base/Domain#Seconds"/>
        <rdfs:comment>Second time constant in pitch control lag (&lt;i&gt;T&lt;/i&gt;&lt;sub&gt;2&lt;/sub&gt;). It is type dependent parameter.</rdfs:comment>
    </owl:ObjectProperty>
    


    <!-- https://w3id.org/netbeheer/referentiemodellen/IECCIM/TC57CIM/IEC61970/Dynamics/StandardModels/WindDynamics#WindPitchContEmulIEC_tpe -->


    <owl:ObjectProperty rdf:about="https://w3id.org/netbeheer/referentiemodellen/IECCIM/TC57CIM/IEC61970/Dynamics/StandardModels/WindDynamics#WindPitchContEmulIEC_tpe">
        <rdfs:domain rdf:resource="https://w3id.org/netbeheer/referentiemodellen/IECCIM/TC57CIM/IEC61970/Dynamics/StandardModels/WindDynamics#WindPitchContEmulIEC"/>
        <rdfs:range rdf:resource="https://w3id.org/netbeheer/referentiemodellen/IECCIM/TC57CIM/IEC61970/Base/Domain#Seconds"/>
        <rdfs:comment>Time constant in generator air gap power lag (&lt;i&gt;T&lt;/i&gt;&lt;sub&gt;pe&lt;/sub&gt;). It is type dependent parameter.</rdfs:comment>
    </owl:ObjectProperty>
    


    <!-- https://w3id.org/netbeheer/referentiemodellen/IECCIM/TC57CIM/IEC61970/Dynamics/StandardModels/WindDynamics#WindPlantDynamics_WindTurbineType3or4Dynamics -->


    <owl:ObjectProperty rdf:about="https://w3id.org/netbeheer/referentiemodellen/IECCIM/TC57CIM/IEC61970/Dynamics/StandardModels/WindDynamics#WindPlantDynamics_WindTurbineType3or4Dynamics">
        <rdfs:domain rdf:resource="https://w3id.org/netbeheer/referentiemodellen/IECCIM/TC57CIM/IEC61970/Dynamics/StandardModels/WindDynamics#WindPlantDynamics"/>
        <rdfs:range rdf:resource="https://w3id.org/netbeheer/referentiemodellen/IECCIM/TC57CIM/IEC61970/Dynamics/StandardModels/WindDynamics#WindTurbineType3or4Dynamics"/>
        <rdfs:comment>The wind plant with which the wind turbines type 3 or 4 are associated.The wind turbine type 3 or 4 associated with this wind plant.</rdfs:comment>
    </owl:ObjectProperty>
    


    <!-- https://w3id.org/netbeheer/referentiemodellen/IECCIM/TC57CIM/IEC61970/Dynamics/StandardModels/WindDynamics#WindPlantFreqPcontrolIEC_WindDynamicsLookupTable -->


    <owl:ObjectProperty rdf:about="https://w3id.org/netbeheer/referentiemodellen/IECCIM/TC57CIM/IEC61970/Dynamics/StandardModels/WindDynamics#WindPlantFreqPcontrolIEC_WindDynamicsLookupTable">
        <owl:inverseOf rdf:resource="https://w3id.org/netbeheer/referentiemodellen/IECCIM/TC57CIM/IEC61970/Dynamics/StandardModels/WindDynamics#WindDynamicsLookupTable_WindPlantFreqPcontrolIEC"/>
        <rdfs:domain rdf:resource="https://w3id.org/netbeheer/referentiemodellen/IECCIM/TC57CIM/IEC61970/Dynamics/StandardModels/WindDynamics#WindPlantFreqPcontrolIEC"/>
        <rdfs:range rdf:resource="https://w3id.org/netbeheer/referentiemodellen/IECCIM/TC57CIM/IEC61970/Dynamics/StandardModels/WindDynamics#WindDynamicsLookupTable"/>
        <rdfs:comment>The wind dynamics lookup table associated with this frequency and active power wind plant model.The frequency and active power wind plant control model with which this wind dynamics lookup table is associated.</rdfs:comment>
    </owl:ObjectProperty>
    


    <!-- https://w3id.org/netbeheer/referentiemodellen/IECCIM/TC57CIM/IEC61970/Dynamics/StandardModels/WindDynamics#WindPlantFreqPcontrolIEC_WindPlantIEC -->


    <owl:ObjectProperty rdf:about="https://w3id.org/netbeheer/referentiemodellen/IECCIM/TC57CIM/IEC61970/Dynamics/StandardModels/WindDynamics#WindPlantFreqPcontrolIEC_WindPlantIEC">
        <rdf:type rdf:resource="http://www.w3.org/2002/07/owl#FunctionalProperty"/>
        <rdfs:domain rdf:resource="https://w3id.org/netbeheer/referentiemodellen/IECCIM/TC57CIM/IEC61970/Dynamics/StandardModels/WindDynamics#WindPlantFreqPcontrolIEC"/>
        <rdfs:range rdf:resource="https://w3id.org/netbeheer/referentiemodellen/IECCIM/TC57CIM/IEC61970/Dynamics/StandardModels/WindDynamics#WindPlantIEC"/>
        <rdfs:comment>Wind plant frequency and active power control model associated with this wind plant.Wind plant model with which this wind plant frequency and active power control is associated.</rdfs:comment>
    </owl:ObjectProperty>
    


    <!-- https://w3id.org/netbeheer/referentiemodellen/IECCIM/TC57CIM/IEC61970/Dynamics/StandardModels/WindDynamics#WindPlantFreqPcontrolIEC_dprefmax -->


    <owl:ObjectProperty rdf:about="https://w3id.org/netbeheer/referentiemodellen/IECCIM/TC57CIM/IEC61970/Dynamics/StandardModels/WindDynamics#WindPlantFreqPcontrolIEC_dprefmax">
        <rdfs:domain rdf:resource="https://w3id.org/netbeheer/referentiemodellen/IECCIM/TC57CIM/IEC61970/Dynamics/StandardModels/WindDynamics#WindPlantFreqPcontrolIEC"/>
        <rdfs:range rdf:resource="https://w3id.org/netbeheer/referentiemodellen/IECCIM/TC57CIM/IEC61970/Base/Domain#PU"/>
        <rdfs:comment>Maximum ramp rate of &lt;i&gt;p&lt;/i&gt;&lt;sub&gt;WTref&lt;/sub&gt; request from the plant controller to the wind turbines (&lt;i&gt;dp&lt;/i&gt;&lt;sub&gt;refmax&lt;/sub&gt;). It is project dependent parameter.</rdfs:comment>
    </owl:ObjectProperty>
    


    <!-- https://w3id.org/netbeheer/referentiemodellen/IECCIM/TC57CIM/IEC61970/Dynamics/StandardModels/WindDynamics#WindPlantFreqPcontrolIEC_dprefmin -->


    <owl:ObjectProperty rdf:about="https://w3id.org/netbeheer/referentiemodellen/IECCIM/TC57CIM/IEC61970/Dynamics/StandardModels/WindDynamics#WindPlantFreqPcontrolIEC_dprefmin">
        <rdfs:domain rdf:resource="https://w3id.org/netbeheer/referentiemodellen/IECCIM/TC57CIM/IEC61970/Dynamics/StandardModels/WindDynamics#WindPlantFreqPcontrolIEC"/>
        <rdfs:range rdf:resource="https://w3id.org/netbeheer/referentiemodellen/IECCIM/TC57CIM/IEC61970/Base/Domain#PU"/>
        <rdfs:comment>Minimum (negative) ramp rate of &lt;i&gt;p&lt;/i&gt;&lt;sub&gt;WTref&lt;/sub&gt; request from the plant controller to the wind turbines (&lt;i&gt;dp&lt;/i&gt;&lt;sub&gt;refmin&lt;/sub&gt;). It is project dependent parameter.</rdfs:comment>
    </owl:ObjectProperty>
    


    <!-- https://w3id.org/netbeheer/referentiemodellen/IECCIM/TC57CIM/IEC61970/Dynamics/StandardModels/WindDynamics#WindPlantFreqPcontrolIEC_prefmax -->


    <owl:ObjectProperty rdf:about="https://w3id.org/netbeheer/referentiemodellen/IECCIM/TC57CIM/IEC61970/Dynamics/StandardModels/WindDynamics#WindPlantFreqPcontrolIEC_prefmax">
        <rdfs:domain rdf:resource="https://w3id.org/netbeheer/referentiemodellen/IECCIM/TC57CIM/IEC61970/Dynamics/StandardModels/WindDynamics#WindPlantFreqPcontrolIEC"/>
        <rdfs:range rdf:resource="https://w3id.org/netbeheer/referentiemodellen/IECCIM/TC57CIM/IEC61970/Base/Domain#PU"/>
        <rdfs:comment>Maximum &lt;i&gt;p&lt;/i&gt;&lt;sub&gt;WTref&lt;/sub&gt; request from the plant controller to the wind turbines (&lt;i&gt;p&lt;/i&gt;&lt;sub&gt;refmax&lt;/sub&gt;). It is type dependent parameter.</rdfs:comment>
    </owl:ObjectProperty>
    


    <!-- https://w3id.org/netbeheer/referentiemodellen/IECCIM/TC57CIM/IEC61970/Dynamics/StandardModels/WindDynamics#WindPlantFreqPcontrolIEC_prefmin -->


    <owl:ObjectProperty rdf:about="https://w3id.org/netbeheer/referentiemodellen/IECCIM/TC57CIM/IEC61970/Dynamics/StandardModels/WindDynamics#WindPlantFreqPcontrolIEC_prefmin">
        <rdfs:domain rdf:resource="https://w3id.org/netbeheer/referentiemodellen/IECCIM/TC57CIM/IEC61970/Dynamics/StandardModels/WindDynamics#WindPlantFreqPcontrolIEC"/>
        <rdfs:range rdf:resource="https://w3id.org/netbeheer/referentiemodellen/IECCIM/TC57CIM/IEC61970/Base/Domain#PU"/>
        <rdfs:comment>Minimum &lt;i&gt;p&lt;/i&gt;&lt;sub&gt;WTref&lt;/sub&gt; request from the plant controller to the wind turbines (&lt;i&gt;p&lt;/i&gt;&lt;sub&gt;refmin&lt;/sub&gt;). It is type dependent parameter.</rdfs:comment>
    </owl:ObjectProperty>
    


    <!-- https://w3id.org/netbeheer/referentiemodellen/IECCIM/TC57CIM/IEC61970/Dynamics/StandardModels/WindDynamics#WindPlantFreqPcontrolIEC_tpft -->


    <owl:ObjectProperty rdf:about="https://w3id.org/netbeheer/referentiemodellen/IECCIM/TC57CIM/IEC61970/Dynamics/StandardModels/WindDynamics#WindPlantFreqPcontrolIEC_tpft">
        <rdfs:domain rdf:resource="https://w3id.org/netbeheer/referentiemodellen/IECCIM/TC57CIM/IEC61970/Dynamics/StandardModels/WindDynamics#WindPlantFreqPcontrolIEC"/>
        <rdfs:range rdf:resource="https://w3id.org/netbeheer/referentiemodellen/IECCIM/TC57CIM/IEC61970/Base/Domain#Seconds"/>
        <rdfs:comment>Lead time constant in reference value transfer function (&lt;i&gt;T&lt;/i&gt;&lt;sub&gt;pft&lt;/sub&gt;). It is type dependent parameter.</rdfs:comment>
    </owl:ObjectProperty>
    


    <!-- https://w3id.org/netbeheer/referentiemodellen/IECCIM/TC57CIM/IEC61970/Dynamics/StandardModels/WindDynamics#WindPlantFreqPcontrolIEC_tpfv -->


    <owl:ObjectProperty rdf:about="https://w3id.org/netbeheer/referentiemodellen/IECCIM/TC57CIM/IEC61970/Dynamics/StandardModels/WindDynamics#WindPlantFreqPcontrolIEC_tpfv">
        <rdfs:domain rdf:resource="https://w3id.org/netbeheer/referentiemodellen/IECCIM/TC57CIM/IEC61970/Dynamics/StandardModels/WindDynamics#WindPlantFreqPcontrolIEC"/>
        <rdfs:range rdf:resource="https://w3id.org/netbeheer/referentiemodellen/IECCIM/TC57CIM/IEC61970/Base/Domain#Seconds"/>
        <rdfs:comment>Lag time constant in reference value transfer function (&lt;i&gt;T&lt;/i&gt;&lt;sub&gt;pfv&lt;/sub&gt;). It is type dependent parameter.</rdfs:comment>
    </owl:ObjectProperty>
    


    <!-- https://w3id.org/netbeheer/referentiemodellen/IECCIM/TC57CIM/IEC61970/Dynamics/StandardModels/WindDynamics#WindPlantFreqPcontrolIEC_twpffilt -->


    <owl:ObjectProperty rdf:about="https://w3id.org/netbeheer/referentiemodellen/IECCIM/TC57CIM/IEC61970/Dynamics/StandardModels/WindDynamics#WindPlantFreqPcontrolIEC_twpffilt">
        <rdfs:domain rdf:resource="https://w3id.org/netbeheer/referentiemodellen/IECCIM/TC57CIM/IEC61970/Dynamics/StandardModels/WindDynamics#WindPlantFreqPcontrolIEC"/>
        <rdfs:range rdf:resource="https://w3id.org/netbeheer/referentiemodellen/IECCIM/TC57CIM/IEC61970/Base/Domain#Seconds"/>
        <rdfs:comment>Filter time constant for frequency measurement (&lt;i&gt;T&lt;/i&gt;&lt;sub&gt;WPffilt&lt;/sub&gt;). It is type dependent parameter.</rdfs:comment>
    </owl:ObjectProperty>
    


    <!-- https://w3id.org/netbeheer/referentiemodellen/IECCIM/TC57CIM/IEC61970/Dynamics/StandardModels/WindDynamics#WindPlantFreqPcontrolIEC_twppfilt -->


    <owl:ObjectProperty rdf:about="https://w3id.org/netbeheer/referentiemodellen/IECCIM/TC57CIM/IEC61970/Dynamics/StandardModels/WindDynamics#WindPlantFreqPcontrolIEC_twppfilt">
        <rdfs:domain rdf:resource="https://w3id.org/netbeheer/referentiemodellen/IECCIM/TC57CIM/IEC61970/Dynamics/StandardModels/WindDynamics#WindPlantFreqPcontrolIEC"/>
        <rdfs:range rdf:resource="https://w3id.org/netbeheer/referentiemodellen/IECCIM/TC57CIM/IEC61970/Base/Domain#Seconds"/>
        <rdfs:comment>Filter time constant for active power measurement (&lt;i&gt;T&lt;/i&gt;&lt;sub&gt;WPpfilt&lt;/sub&gt;). It is type dependent parameter.</rdfs:comment>
    </owl:ObjectProperty>
    


    <!-- https://w3id.org/netbeheer/referentiemodellen/IECCIM/TC57CIM/IEC61970/Dynamics/StandardModels/WindDynamics#WindPlantIEC_WindPlantFreqPcontrolIEC -->


    <owl:ObjectProperty rdf:about="https://w3id.org/netbeheer/referentiemodellen/IECCIM/TC57CIM/IEC61970/Dynamics/StandardModels/WindDynamics#WindPlantIEC_WindPlantFreqPcontrolIEC">
        <owl:inverseOf rdf:resource="https://w3id.org/netbeheer/referentiemodellen/IECCIM/TC57CIM/IEC61970/Dynamics/StandardModels/WindDynamics#WindPlantFreqPcontrolIEC_WindPlantIEC"/>
        <rdf:type rdf:resource="http://www.w3.org/2002/07/owl#FunctionalProperty"/>
        <rdfs:domain rdf:resource="https://w3id.org/netbeheer/referentiemodellen/IECCIM/TC57CIM/IEC61970/Dynamics/StandardModels/WindDynamics#WindPlantIEC"/>
        <rdfs:range rdf:resource="https://w3id.org/netbeheer/referentiemodellen/IECCIM/TC57CIM/IEC61970/Dynamics/StandardModels/WindDynamics#WindPlantFreqPcontrolIEC"/>
        <rdfs:comment>Wind plant frequency and active power control model associated with this wind plant.Wind plant model with which this wind plant frequency and active power control is associated.</rdfs:comment>
    </owl:ObjectProperty>
    


    <!-- https://w3id.org/netbeheer/referentiemodellen/IECCIM/TC57CIM/IEC61970/Dynamics/StandardModels/WindDynamics#WindPlantIEC_WindPlantReactiveControlIEC -->


    <owl:ObjectProperty rdf:about="https://w3id.org/netbeheer/referentiemodellen/IECCIM/TC57CIM/IEC61970/Dynamics/StandardModels/WindDynamics#WindPlantIEC_WindPlantReactiveControlIEC">
        <rdf:type rdf:resource="http://www.w3.org/2002/07/owl#FunctionalProperty"/>
        <rdfs:domain rdf:resource="https://w3id.org/netbeheer/referentiemodellen/IECCIM/TC57CIM/IEC61970/Dynamics/StandardModels/WindDynamics#WindPlantIEC"/>
        <rdfs:range rdf:resource="https://w3id.org/netbeheer/referentiemodellen/IECCIM/TC57CIM/IEC61970/Dynamics/StandardModels/WindDynamics#WindPlantReactiveControlIEC"/>
        <rdfs:comment>Wind plant reactive control model associated with this wind plant.Wind plant model with which this wind reactive control is associated.</rdfs:comment>
    </owl:ObjectProperty>
    


    <!-- https://w3id.org/netbeheer/referentiemodellen/IECCIM/TC57CIM/IEC61970/Dynamics/StandardModels/WindDynamics#WindPlantReactiveControlIEC_WindPlantIEC -->


    <owl:ObjectProperty rdf:about="https://w3id.org/netbeheer/referentiemodellen/IECCIM/TC57CIM/IEC61970/Dynamics/StandardModels/WindDynamics#WindPlantReactiveControlIEC_WindPlantIEC">
        <owl:inverseOf rdf:resource="https://w3id.org/netbeheer/referentiemodellen/IECCIM/TC57CIM/IEC61970/Dynamics/StandardModels/WindDynamics#WindPlantIEC_WindPlantReactiveControlIEC"/>
        <rdf:type rdf:resource="http://www.w3.org/2002/07/owl#FunctionalProperty"/>
        <rdfs:domain rdf:resource="https://w3id.org/netbeheer/referentiemodellen/IECCIM/TC57CIM/IEC61970/Dynamics/StandardModels/WindDynamics#WindPlantReactiveControlIEC"/>
        <rdfs:range rdf:resource="https://w3id.org/netbeheer/referentiemodellen/IECCIM/TC57CIM/IEC61970/Dynamics/StandardModels/WindDynamics#WindPlantIEC"/>
        <rdfs:comment>Wind plant reactive control model associated with this wind plant.Wind plant model with which this wind reactive control is associated.</rdfs:comment>
    </owl:ObjectProperty>
    


    <!-- https://w3id.org/netbeheer/referentiemodellen/IECCIM/TC57CIM/IEC61970/Dynamics/StandardModels/WindDynamics#WindPlantReactiveControlIEC_kwpqu -->


    <owl:ObjectProperty rdf:about="https://w3id.org/netbeheer/referentiemodellen/IECCIM/TC57CIM/IEC61970/Dynamics/StandardModels/WindDynamics#WindPlantReactiveControlIEC_kwpqu">
        <rdfs:domain rdf:resource="https://w3id.org/netbeheer/referentiemodellen/IECCIM/TC57CIM/IEC61970/Dynamics/StandardModels/WindDynamics#WindPlantReactiveControlIEC"/>
        <rdfs:range rdf:resource="https://w3id.org/netbeheer/referentiemodellen/IECCIM/TC57CIM/IEC61970/Base/Domain#PU"/>
        <rdfs:comment>Plant voltage control droop (&lt;i&gt;K&lt;/i&gt;&lt;sub&gt;WPqu&lt;/sub&gt;). It is project dependent parameter.</rdfs:comment>
    </owl:ObjectProperty>
    


    <!-- https://w3id.org/netbeheer/referentiemodellen/IECCIM/TC57CIM/IEC61970/Dynamics/StandardModels/WindDynamics#WindPlantReactiveControlIEC_twppfilt -->


    <owl:ObjectProperty rdf:about="https://w3id.org/netbeheer/referentiemodellen/IECCIM/TC57CIM/IEC61970/Dynamics/StandardModels/WindDynamics#WindPlantReactiveControlIEC_twppfilt">
        <rdfs:domain rdf:resource="https://w3id.org/netbeheer/referentiemodellen/IECCIM/TC57CIM/IEC61970/Dynamics/StandardModels/WindDynamics#WindPlantReactiveControlIEC"/>
        <rdfs:range rdf:resource="https://w3id.org/netbeheer/referentiemodellen/IECCIM/TC57CIM/IEC61970/Base/Domain#Seconds"/>
        <rdfs:comment>Filter time constant for active power measurement (&lt;i&gt;T&lt;/i&gt;&lt;sub&gt;WPpfilt&lt;/sub&gt;). It is type dependent parameter.</rdfs:comment>
    </owl:ObjectProperty>
    


    <!-- https://w3id.org/netbeheer/referentiemodellen/IECCIM/TC57CIM/IEC61970/Dynamics/StandardModels/WindDynamics#WindPlantReactiveControlIEC_twpqfilt -->


    <owl:ObjectProperty rdf:about="https://w3id.org/netbeheer/referentiemodellen/IECCIM/TC57CIM/IEC61970/Dynamics/StandardModels/WindDynamics#WindPlantReactiveControlIEC_twpqfilt">
        <rdfs:domain rdf:resource="https://w3id.org/netbeheer/referentiemodellen/IECCIM/TC57CIM/IEC61970/Dynamics/StandardModels/WindDynamics#WindPlantReactiveControlIEC"/>
        <rdfs:range rdf:resource="https://w3id.org/netbeheer/referentiemodellen/IECCIM/TC57CIM/IEC61970/Base/Domain#Seconds"/>
        <rdfs:comment>Filter time constant for reactive power measurement (&lt;i&gt;T&lt;/i&gt;&lt;sub&gt;WPqfilt&lt;/sub&gt;). It is type dependent parameter.</rdfs:comment>
    </owl:ObjectProperty>
    


    <!-- https://w3id.org/netbeheer/referentiemodellen/IECCIM/TC57CIM/IEC61970/Dynamics/StandardModels/WindDynamics#WindPlantReactiveControlIEC_twpufilt -->


    <owl:ObjectProperty rdf:about="https://w3id.org/netbeheer/referentiemodellen/IECCIM/TC57CIM/IEC61970/Dynamics/StandardModels/WindDynamics#WindPlantReactiveControlIEC_twpufilt">
        <rdfs:domain rdf:resource="https://w3id.org/netbeheer/referentiemodellen/IECCIM/TC57CIM/IEC61970/Dynamics/StandardModels/WindDynamics#WindPlantReactiveControlIEC"/>
        <rdfs:range rdf:resource="https://w3id.org/netbeheer/referentiemodellen/IECCIM/TC57CIM/IEC61970/Base/Domain#Seconds"/>
        <rdfs:comment>Filter time constant for voltage measurement (&lt;i&gt;T&lt;/i&gt;&lt;sub&gt;WPufilt&lt;/sub&gt;). It is type dependent parameter.</rdfs:comment>
    </owl:ObjectProperty>
    


    <!-- https://w3id.org/netbeheer/referentiemodellen/IECCIM/TC57CIM/IEC61970/Dynamics/StandardModels/WindDynamics#WindPlantReactiveControlIEC_txft -->


    <owl:ObjectProperty rdf:about="https://w3id.org/netbeheer/referentiemodellen/IECCIM/TC57CIM/IEC61970/Dynamics/StandardModels/WindDynamics#WindPlantReactiveControlIEC_txft">
        <rdfs:domain rdf:resource="https://w3id.org/netbeheer/referentiemodellen/IECCIM/TC57CIM/IEC61970/Dynamics/StandardModels/WindDynamics#WindPlantReactiveControlIEC"/>
        <rdfs:range rdf:resource="https://w3id.org/netbeheer/referentiemodellen/IECCIM/TC57CIM/IEC61970/Base/Domain#Seconds"/>
        <rdfs:comment>Lead time constant in reference value transfer function (&lt;i&gt;T&lt;/i&gt;&lt;sub&gt;xft&lt;/sub&gt;). It is type dependent parameter.</rdfs:comment>
    </owl:ObjectProperty>
    


    <!-- https://w3id.org/netbeheer/referentiemodellen/IECCIM/TC57CIM/IEC61970/Dynamics/StandardModels/WindDynamics#WindPlantReactiveControlIEC_txfv -->


    <owl:ObjectProperty rdf:about="https://w3id.org/netbeheer/referentiemodellen/IECCIM/TC57CIM/IEC61970/Dynamics/StandardModels/WindDynamics#WindPlantReactiveControlIEC_txfv">
        <rdfs:domain rdf:resource="https://w3id.org/netbeheer/referentiemodellen/IECCIM/TC57CIM/IEC61970/Dynamics/StandardModels/WindDynamics#WindPlantReactiveControlIEC"/>
        <rdfs:range rdf:resource="https://w3id.org/netbeheer/referentiemodellen/IECCIM/TC57CIM/IEC61970/Base/Domain#Seconds"/>
        <rdfs:comment>Lag time constant in reference value transfer function (&lt;i&gt;T&lt;/i&gt;&lt;sub&gt;xfv&lt;/sub&gt;). It is type dependent parameter.</rdfs:comment>
    </owl:ObjectProperty>
    


    <!-- https://w3id.org/netbeheer/referentiemodellen/IECCIM/TC57CIM/IEC61970/Dynamics/StandardModels/WindDynamics#WindPlantReactiveControlIEC_uwpqdip -->


    <owl:ObjectProperty rdf:about="https://w3id.org/netbeheer/referentiemodellen/IECCIM/TC57CIM/IEC61970/Dynamics/StandardModels/WindDynamics#WindPlantReactiveControlIEC_uwpqdip">
        <rdfs:domain rdf:resource="https://w3id.org/netbeheer/referentiemodellen/IECCIM/TC57CIM/IEC61970/Dynamics/StandardModels/WindDynamics#WindPlantReactiveControlIEC"/>
        <rdfs:range rdf:resource="https://w3id.org/netbeheer/referentiemodellen/IECCIM/TC57CIM/IEC61970/Base/Domain#PU"/>
        <rdfs:comment>Voltage threshold for LVRT detection in q control (&lt;i&gt;u&lt;/i&gt;&lt;sub&gt;WPqdip&lt;/sub&gt;). It is type dependent parameter.</rdfs:comment>
    </owl:ObjectProperty>
    


    <!-- https://w3id.org/netbeheer/referentiemodellen/IECCIM/TC57CIM/IEC61970/Dynamics/StandardModels/WindDynamics#WindPlantReactiveControlIEC_xrefmax -->


    <owl:ObjectProperty rdf:about="https://w3id.org/netbeheer/referentiemodellen/IECCIM/TC57CIM/IEC61970/Dynamics/StandardModels/WindDynamics#WindPlantReactiveControlIEC_xrefmax">
        <rdfs:domain rdf:resource="https://w3id.org/netbeheer/referentiemodellen/IECCIM/TC57CIM/IEC61970/Dynamics/StandardModels/WindDynamics#WindPlantReactiveControlIEC"/>
        <rdfs:range rdf:resource="https://w3id.org/netbeheer/referentiemodellen/IECCIM/TC57CIM/IEC61970/Base/Domain#PU"/>
        <rdfs:comment>Maximum &lt;i&gt;x&lt;/i&gt;&lt;sub&gt;WTref&lt;/sub&gt; (&lt;i&gt;q&lt;/i&gt;&lt;sub&gt;WTref&lt;/sub&gt; or delta &lt;i&gt;u&lt;/i&gt;&lt;sub&gt;WTref&lt;/sub&gt;) request from the plant controller (&lt;i&gt;x&lt;/i&gt;&lt;sub&gt;refmax&lt;/sub&gt;). It is project dependent parameter.</rdfs:comment>
    </owl:ObjectProperty>
    


    <!-- https://w3id.org/netbeheer/referentiemodellen/IECCIM/TC57CIM/IEC61970/Dynamics/StandardModels/WindDynamics#WindPlantReactiveControlIEC_xrefmin -->


    <owl:ObjectProperty rdf:about="https://w3id.org/netbeheer/referentiemodellen/IECCIM/TC57CIM/IEC61970/Dynamics/StandardModels/WindDynamics#WindPlantReactiveControlIEC_xrefmin">
        <rdfs:domain rdf:resource="https://w3id.org/netbeheer/referentiemodellen/IECCIM/TC57CIM/IEC61970/Dynamics/StandardModels/WindDynamics#WindPlantReactiveControlIEC"/>
        <rdfs:range rdf:resource="https://w3id.org/netbeheer/referentiemodellen/IECCIM/TC57CIM/IEC61970/Base/Domain#PU"/>
        <rdfs:comment>Minimum &lt;i&gt;x&lt;/i&gt;&lt;sub&gt;WTref&lt;/sub&gt; (&lt;i&gt;q&lt;/i&gt;&lt;sub&gt;WTref&lt;/sub&gt; or delta&lt;i&gt;u&lt;/i&gt;&lt;sub&gt;WTref&lt;/sub&gt;) request from the plant controller (&lt;i&gt;x&lt;/i&gt;&lt;sub&gt;refmin&lt;/sub&gt;). It is project dependent parameter.</rdfs:comment>
    </owl:ObjectProperty>
    


    <!-- https://w3id.org/netbeheer/referentiemodellen/IECCIM/TC57CIM/IEC61970/Dynamics/StandardModels/WindDynamics#WindProtectionIEC_WindTurbineType1or2IEC -->


    <owl:ObjectProperty rdf:about="https://w3id.org/netbeheer/referentiemodellen/IECCIM/TC57CIM/IEC61970/Dynamics/StandardModels/WindDynamics#WindProtectionIEC_WindTurbineType1or2IEC">
        <rdf:type rdf:resource="http://www.w3.org/2002/07/owl#FunctionalProperty"/>
        <rdfs:domain rdf:resource="https://w3id.org/netbeheer/referentiemodellen/IECCIM/TC57CIM/IEC61970/Dynamics/StandardModels/WindDynamics#WindProtectionIEC"/>
        <rdfs:range rdf:resource="https://w3id.org/netbeheer/referentiemodellen/IECCIM/TC57CIM/IEC61970/Dynamics/StandardModels/WindDynamics#WindTurbineType1or2IEC"/>
        <rdfs:comment>Wind turbune protection model associated with this wind generator type 1 or 2 model.Wind generator type 1 or 2 model with which this wind turbine protection model is associated.</rdfs:comment>
    </owl:ObjectProperty>
    


    <!-- https://w3id.org/netbeheer/referentiemodellen/IECCIM/TC57CIM/IEC61970/Dynamics/StandardModels/WindDynamics#WindProtectionIEC_WindTurbineType3or4IEC -->


    <owl:ObjectProperty rdf:about="https://w3id.org/netbeheer/referentiemodellen/IECCIM/TC57CIM/IEC61970/Dynamics/StandardModels/WindDynamics#WindProtectionIEC_WindTurbineType3or4IEC">
        <rdf:type rdf:resource="http://www.w3.org/2002/07/owl#FunctionalProperty"/>
        <rdfs:domain rdf:resource="https://w3id.org/netbeheer/referentiemodellen/IECCIM/TC57CIM/IEC61970/Dynamics/StandardModels/WindDynamics#WindProtectionIEC"/>
        <rdfs:range rdf:resource="https://w3id.org/netbeheer/referentiemodellen/IECCIM/TC57CIM/IEC61970/Dynamics/StandardModels/WindDynamics#WindTurbineType3or4IEC"/>
        <rdfs:comment>Wind turbune protection model associated with this wind generator type 3 or 4 model.Wind generator type 3 or 4 model with which this wind turbine protection model is associated.</rdfs:comment>
    </owl:ObjectProperty>
    


    <!-- https://w3id.org/netbeheer/referentiemodellen/IECCIM/TC57CIM/IEC61970/Dynamics/StandardModels/WindDynamics#WindProtectionIEC_fover -->


    <owl:ObjectProperty rdf:about="https://w3id.org/netbeheer/referentiemodellen/IECCIM/TC57CIM/IEC61970/Dynamics/StandardModels/WindDynamics#WindProtectionIEC_fover">
        <rdfs:domain rdf:resource="https://w3id.org/netbeheer/referentiemodellen/IECCIM/TC57CIM/IEC61970/Dynamics/StandardModels/WindDynamics#WindProtectionIEC"/>
        <rdfs:range rdf:resource="https://w3id.org/netbeheer/referentiemodellen/IECCIM/TC57CIM/IEC61970/Base/Domain#PU"/>
        <rdfs:comment>Set of wind turbine over frequency protection levels (&lt;i&gt;f&lt;/i&gt;&lt;i&gt;&lt;sub&gt;over&lt;/sub&gt;&lt;/i&gt;). It is project dependent parameter. </rdfs:comment>
    </owl:ObjectProperty>
    


    <!-- https://w3id.org/netbeheer/referentiemodellen/IECCIM/TC57CIM/IEC61970/Dynamics/StandardModels/WindDynamics#WindProtectionIEC_funder -->


    <owl:ObjectProperty rdf:about="https://w3id.org/netbeheer/referentiemodellen/IECCIM/TC57CIM/IEC61970/Dynamics/StandardModels/WindDynamics#WindProtectionIEC_funder">
        <rdfs:domain rdf:resource="https://w3id.org/netbeheer/referentiemodellen/IECCIM/TC57CIM/IEC61970/Dynamics/StandardModels/WindDynamics#WindProtectionIEC"/>
        <rdfs:range rdf:resource="https://w3id.org/netbeheer/referentiemodellen/IECCIM/TC57CIM/IEC61970/Base/Domain#PU"/>
        <rdfs:comment>Set of wind turbine under frequency protection levels (&lt;i&gt;f&lt;/i&gt;&lt;i&gt;&lt;sub&gt;under&lt;/sub&gt;&lt;/i&gt;). It is project dependent parameter.</rdfs:comment>
    </owl:ObjectProperty>
    


    <!-- https://w3id.org/netbeheer/referentiemodellen/IECCIM/TC57CIM/IEC61970/Dynamics/StandardModels/WindDynamics#WindProtectionIEC_tfover -->


    <owl:ObjectProperty rdf:about="https://w3id.org/netbeheer/referentiemodellen/IECCIM/TC57CIM/IEC61970/Dynamics/StandardModels/WindDynamics#WindProtectionIEC_tfover">
        <rdfs:domain rdf:resource="https://w3id.org/netbeheer/referentiemodellen/IECCIM/TC57CIM/IEC61970/Dynamics/StandardModels/WindDynamics#WindProtectionIEC"/>
        <rdfs:range rdf:resource="https://w3id.org/netbeheer/referentiemodellen/IECCIM/TC57CIM/IEC61970/Base/Domain#Seconds"/>
        <rdfs:comment>Set of corresponding wind turbine over frequency protection disconnection times (&lt;i&gt;T&lt;/i&gt;&lt;i&gt;&lt;sub&gt;fover&lt;/sub&gt;&lt;/i&gt;). It is project dependent parameter.</rdfs:comment>
    </owl:ObjectProperty>
    


    <!-- https://w3id.org/netbeheer/referentiemodellen/IECCIM/TC57CIM/IEC61970/Dynamics/StandardModels/WindDynamics#WindProtectionIEC_tfunder -->


    <owl:ObjectProperty rdf:about="https://w3id.org/netbeheer/referentiemodellen/IECCIM/TC57CIM/IEC61970/Dynamics/StandardModels/WindDynamics#WindProtectionIEC_tfunder">
        <rdfs:domain rdf:resource="https://w3id.org/netbeheer/referentiemodellen/IECCIM/TC57CIM/IEC61970/Dynamics/StandardModels/WindDynamics#WindProtectionIEC"/>
        <rdfs:range rdf:resource="https://w3id.org/netbeheer/referentiemodellen/IECCIM/TC57CIM/IEC61970/Base/Domain#Seconds"/>
        <rdfs:comment>Set of corresponding wind turbine under frequency protection disconnection times (&lt;i&gt;T&lt;/i&gt;&lt;i&gt;&lt;sub&gt;funder&lt;/sub&gt;&lt;/i&gt;). It is project dependent parameter.</rdfs:comment>
    </owl:ObjectProperty>
    


    <!-- https://w3id.org/netbeheer/referentiemodellen/IECCIM/TC57CIM/IEC61970/Dynamics/StandardModels/WindDynamics#WindProtectionIEC_tuover -->


    <owl:ObjectProperty rdf:about="https://w3id.org/netbeheer/referentiemodellen/IECCIM/TC57CIM/IEC61970/Dynamics/StandardModels/WindDynamics#WindProtectionIEC_tuover">
        <rdfs:domain rdf:resource="https://w3id.org/netbeheer/referentiemodellen/IECCIM/TC57CIM/IEC61970/Dynamics/StandardModels/WindDynamics#WindProtectionIEC"/>
        <rdfs:range rdf:resource="https://w3id.org/netbeheer/referentiemodellen/IECCIM/TC57CIM/IEC61970/Base/Domain#Seconds"/>
        <rdfs:comment>Set of corresponding wind turbine over voltage protection disconnection times (&lt;i&gt;T&lt;/i&gt;&lt;i&gt;&lt;sub&gt;uover&lt;/sub&gt;&lt;/i&gt;). It is project dependent parameter.</rdfs:comment>
    </owl:ObjectProperty>
    


    <!-- https://w3id.org/netbeheer/referentiemodellen/IECCIM/TC57CIM/IEC61970/Dynamics/StandardModels/WindDynamics#WindProtectionIEC_tuunder -->


    <owl:ObjectProperty rdf:about="https://w3id.org/netbeheer/referentiemodellen/IECCIM/TC57CIM/IEC61970/Dynamics/StandardModels/WindDynamics#WindProtectionIEC_tuunder">
        <rdfs:domain rdf:resource="https://w3id.org/netbeheer/referentiemodellen/IECCIM/TC57CIM/IEC61970/Dynamics/StandardModels/WindDynamics#WindProtectionIEC"/>
        <rdfs:range rdf:resource="https://w3id.org/netbeheer/referentiemodellen/IECCIM/TC57CIM/IEC61970/Base/Domain#Seconds"/>
        <rdfs:comment>Set of corresponding wind turbine under voltage protection disconnection times (&lt;i&gt;T&lt;/i&gt;&lt;i&gt;&lt;sub&gt;uunder&lt;/sub&gt;&lt;/i&gt;). It is project dependent parameter.</rdfs:comment>
    </owl:ObjectProperty>
    


    <!-- https://w3id.org/netbeheer/referentiemodellen/IECCIM/TC57CIM/IEC61970/Dynamics/StandardModels/WindDynamics#WindProtectionIEC_uover -->


    <owl:ObjectProperty rdf:about="https://w3id.org/netbeheer/referentiemodellen/IECCIM/TC57CIM/IEC61970/Dynamics/StandardModels/WindDynamics#WindProtectionIEC_uover">
        <rdfs:domain rdf:resource="https://w3id.org/netbeheer/referentiemodellen/IECCIM/TC57CIM/IEC61970/Dynamics/StandardModels/WindDynamics#WindProtectionIEC"/>
        <rdfs:range rdf:resource="https://w3id.org/netbeheer/referentiemodellen/IECCIM/TC57CIM/IEC61970/Base/Domain#PU"/>
        <rdfs:comment>Set of wind turbine over voltage protection levels (&lt;i&gt;u&lt;/i&gt;&lt;i&gt;&lt;sub&gt;over&lt;/sub&gt;&lt;/i&gt;). It is project dependent parameter.</rdfs:comment>
    </owl:ObjectProperty>
    


    <!-- https://w3id.org/netbeheer/referentiemodellen/IECCIM/TC57CIM/IEC61970/Dynamics/StandardModels/WindDynamics#WindProtectionIEC_uunder -->


    <owl:ObjectProperty rdf:about="https://w3id.org/netbeheer/referentiemodellen/IECCIM/TC57CIM/IEC61970/Dynamics/StandardModels/WindDynamics#WindProtectionIEC_uunder">
        <rdfs:domain rdf:resource="https://w3id.org/netbeheer/referentiemodellen/IECCIM/TC57CIM/IEC61970/Dynamics/StandardModels/WindDynamics#WindProtectionIEC"/>
        <rdfs:range rdf:resource="https://w3id.org/netbeheer/referentiemodellen/IECCIM/TC57CIM/IEC61970/Base/Domain#PU"/>
        <rdfs:comment>Set of wind turbine under voltage protection levels (&lt;i&gt;u&lt;/i&gt;&lt;i&gt;&lt;sub&gt;under&lt;/sub&gt;&lt;/i&gt;). It is project dependent parameter.</rdfs:comment>
    </owl:ObjectProperty>
    


    <!-- https://w3id.org/netbeheer/referentiemodellen/IECCIM/TC57CIM/IEC61970/Dynamics/StandardModels/WindDynamics#WindTurbineType1or2IEC_WindMechIEC -->


    <owl:ObjectProperty rdf:about="https://w3id.org/netbeheer/referentiemodellen/IECCIM/TC57CIM/IEC61970/Dynamics/StandardModels/WindDynamics#WindTurbineType1or2IEC_WindMechIEC">
        <owl:inverseOf rdf:resource="https://w3id.org/netbeheer/referentiemodellen/IECCIM/TC57CIM/IEC61970/Dynamics/StandardModels/WindDynamics#WindMechIEC_WindTurbineType1or2IEC"/>
        <rdfs:domain rdf:resource="https://w3id.org/netbeheer/referentiemodellen/IECCIM/TC57CIM/IEC61970/Dynamics/StandardModels/WindDynamics#WindTurbineType1or2IEC"/>
        <rdfs:range rdf:resource="https://w3id.org/netbeheer/referentiemodellen/IECCIM/TC57CIM/IEC61970/Dynamics/StandardModels/WindDynamics#WindMechIEC"/>
        <rdfs:comment>Wind mechanical model associated with this wind generator type 1 or 2 model.Wind generator type 1 or 2 model with which this wind mechanical model is associated.</rdfs:comment>
    </owl:ObjectProperty>
    


    <!-- https://w3id.org/netbeheer/referentiemodellen/IECCIM/TC57CIM/IEC61970/Dynamics/StandardModels/WindDynamics#WindTurbineType1or2IEC_WindProtectionIEC -->


    <owl:ObjectProperty rdf:about="https://w3id.org/netbeheer/referentiemodellen/IECCIM/TC57CIM/IEC61970/Dynamics/StandardModels/WindDynamics#WindTurbineType1or2IEC_WindProtectionIEC">
        <owl:inverseOf rdf:resource="https://w3id.org/netbeheer/referentiemodellen/IECCIM/TC57CIM/IEC61970/Dynamics/StandardModels/WindDynamics#WindProtectionIEC_WindTurbineType1or2IEC"/>
        <rdfs:domain rdf:resource="https://w3id.org/netbeheer/referentiemodellen/IECCIM/TC57CIM/IEC61970/Dynamics/StandardModels/WindDynamics#WindTurbineType1or2IEC"/>
        <rdfs:range rdf:resource="https://w3id.org/netbeheer/referentiemodellen/IECCIM/TC57CIM/IEC61970/Dynamics/StandardModels/WindDynamics#WindProtectionIEC"/>
        <rdfs:comment>Wind turbune protection model associated with this wind generator type 1 or 2 model.Wind generator type 1 or 2 model with which this wind turbine protection model is associated.</rdfs:comment>
    </owl:ObjectProperty>
    


    <!-- https://w3id.org/netbeheer/referentiemodellen/IECCIM/TC57CIM/IEC61970/Dynamics/StandardModels/WindDynamics#WindTurbineType3or4Dynamics_WindPlantDynamics -->


    <owl:ObjectProperty rdf:about="https://w3id.org/netbeheer/referentiemodellen/IECCIM/TC57CIM/IEC61970/Dynamics/StandardModels/WindDynamics#WindTurbineType3or4Dynamics_WindPlantDynamics">
        <owl:inverseOf rdf:resource="https://w3id.org/netbeheer/referentiemodellen/IECCIM/TC57CIM/IEC61970/Dynamics/StandardModels/WindDynamics#WindPlantDynamics_WindTurbineType3or4Dynamics"/>
        <rdfs:domain rdf:resource="https://w3id.org/netbeheer/referentiemodellen/IECCIM/TC57CIM/IEC61970/Dynamics/StandardModels/WindDynamics#WindTurbineType3or4Dynamics"/>
        <rdfs:range rdf:resource="https://w3id.org/netbeheer/referentiemodellen/IECCIM/TC57CIM/IEC61970/Dynamics/StandardModels/WindDynamics#WindPlantDynamics"/>
        <rdfs:comment>The wind plant with which the wind turbines type 3 or 4 are associated.The wind turbine type 3 or 4 associated with this wind plant.</rdfs:comment>
    </owl:ObjectProperty>
    


    <!-- https://w3id.org/netbeheer/referentiemodellen/IECCIM/TC57CIM/IEC61970/Dynamics/StandardModels/WindDynamics#WindTurbineType3or4IEC_WIndContQIEC -->


    <owl:ObjectProperty rdf:about="https://w3id.org/netbeheer/referentiemodellen/IECCIM/TC57CIM/IEC61970/Dynamics/StandardModels/WindDynamics#WindTurbineType3or4IEC_WIndContQIEC">
        <owl:inverseOf rdf:resource="https://w3id.org/netbeheer/referentiemodellen/IECCIM/TC57CIM/IEC61970/Dynamics/StandardModels/WindDynamics#WindContQIEC_WindTurbineType3or4IEC"/>
        <rdf:type rdf:resource="http://www.w3.org/2002/07/owl#FunctionalProperty"/>
        <rdfs:domain rdf:resource="https://w3id.org/netbeheer/referentiemodellen/IECCIM/TC57CIM/IEC61970/Dynamics/StandardModels/WindDynamics#WindTurbineType3or4IEC"/>
        <rdfs:range rdf:resource="https://w3id.org/netbeheer/referentiemodellen/IECCIM/TC57CIM/IEC61970/Dynamics/StandardModels/WindDynamics#WindContQIEC"/>
        <rdfs:comment>Wind control Q model associated with this wind turbine type 3 or 4 model.Wind turbine type 3 or 4 model with which this reactive control mode is associated.</rdfs:comment>
    </owl:ObjectProperty>
    


    <!-- https://w3id.org/netbeheer/referentiemodellen/IECCIM/TC57CIM/IEC61970/Dynamics/StandardModels/WindDynamics#WindTurbineType3or4IEC_WindContCurrLimIEC -->


    <owl:ObjectProperty rdf:about="https://w3id.org/netbeheer/referentiemodellen/IECCIM/TC57CIM/IEC61970/Dynamics/StandardModels/WindDynamics#WindTurbineType3or4IEC_WindContCurrLimIEC">
        <owl:inverseOf rdf:resource="https://w3id.org/netbeheer/referentiemodellen/IECCIM/TC57CIM/IEC61970/Dynamics/StandardModels/WindDynamics#WindContCurrLimIEC_WindTurbineType3or4IEC"/>
        <rdf:type rdf:resource="http://www.w3.org/2002/07/owl#FunctionalProperty"/>
        <rdfs:domain rdf:resource="https://w3id.org/netbeheer/referentiemodellen/IECCIM/TC57CIM/IEC61970/Dynamics/StandardModels/WindDynamics#WindTurbineType3or4IEC"/>
        <rdfs:range rdf:resource="https://w3id.org/netbeheer/referentiemodellen/IECCIM/TC57CIM/IEC61970/Dynamics/StandardModels/WindDynamics#WindContCurrLimIEC"/>
        <rdfs:comment>Wind control current limitation model associated with this wind turbine type 3 or 4 model.Wind turbine type 3 or 4 model with which this wind control current limitation model is associated.</rdfs:comment>
    </owl:ObjectProperty>
    


    <!-- https://w3id.org/netbeheer/referentiemodellen/IECCIM/TC57CIM/IEC61970/Dynamics/StandardModels/WindDynamics#WindTurbineType3or4IEC_WindProtectionIEC -->


    <owl:ObjectProperty rdf:about="https://w3id.org/netbeheer/referentiemodellen/IECCIM/TC57CIM/IEC61970/Dynamics/StandardModels/WindDynamics#WindTurbineType3or4IEC_WindProtectionIEC">
        <owl:inverseOf rdf:resource="https://w3id.org/netbeheer/referentiemodellen/IECCIM/TC57CIM/IEC61970/Dynamics/StandardModels/WindDynamics#WindProtectionIEC_WindTurbineType3or4IEC"/>
        <rdfs:domain rdf:resource="https://w3id.org/netbeheer/referentiemodellen/IECCIM/TC57CIM/IEC61970/Dynamics/StandardModels/WindDynamics#WindTurbineType3or4IEC"/>
        <rdfs:range rdf:resource="https://w3id.org/netbeheer/referentiemodellen/IECCIM/TC57CIM/IEC61970/Dynamics/StandardModels/WindDynamics#WindProtectionIEC"/>
        <rdfs:comment>Wind turbune protection model associated with this wind generator type 3 or 4 model.Wind generator type 3 or 4 model with which this wind turbine protection model is associated.</rdfs:comment>
    </owl:ObjectProperty>
    


    <!-- https://w3id.org/netbeheer/referentiemodellen/IECCIM/TC57CIM/IEC61970/Dynamics/StandardModels/WindDynamics#WindTurbineType4aIEC_WindContPType4aIEC -->


    <owl:ObjectProperty rdf:about="https://w3id.org/netbeheer/referentiemodellen/IECCIM/TC57CIM/IEC61970/Dynamics/StandardModels/WindDynamics#WindTurbineType4aIEC_WindContPType4aIEC">
        <owl:inverseOf rdf:resource="https://w3id.org/netbeheer/referentiemodellen/IECCIM/TC57CIM/IEC61970/Dynamics/StandardModels/WindDynamics#WindContPType4aIEC_WindTurbineType4aIEC"/>
        <rdf:type rdf:resource="http://www.w3.org/2002/07/owl#FunctionalProperty"/>
        <rdfs:domain rdf:resource="https://w3id.org/netbeheer/referentiemodellen/IECCIM/TC57CIM/IEC61970/Dynamics/StandardModels/WindDynamics#WindTurbineType4aIEC"/>
        <rdfs:range rdf:resource="https://w3id.org/netbeheer/referentiemodellen/IECCIM/TC57CIM/IEC61970/Dynamics/StandardModels/WindDynamics#WindContPType4aIEC"/>
        <rdfs:comment>Wind control P type 4A model associated with this wind turbine type 4A model. Wind turbine type 4A model with which this wind control P type 4A model is associated.</rdfs:comment>
    </owl:ObjectProperty>
    


    <!-- https://w3id.org/netbeheer/referentiemodellen/IECCIM/TC57CIM/IEC61970/Dynamics/StandardModels/WindDynamics#WindTurbineType4bIEC_WindContPType4bIEC -->


    <owl:ObjectProperty rdf:about="https://w3id.org/netbeheer/referentiemodellen/IECCIM/TC57CIM/IEC61970/Dynamics/StandardModels/WindDynamics#WindTurbineType4bIEC_WindContPType4bIEC">
        <owl:inverseOf rdf:resource="https://w3id.org/netbeheer/referentiemodellen/IECCIM/TC57CIM/IEC61970/Dynamics/StandardModels/WindDynamics#WindContPType4bIEC_WindTurbineType4bIEC"/>
        <rdf:type rdf:resource="http://www.w3.org/2002/07/owl#FunctionalProperty"/>
        <rdfs:domain rdf:resource="https://w3id.org/netbeheer/referentiemodellen/IECCIM/TC57CIM/IEC61970/Dynamics/StandardModels/WindDynamics#WindTurbineType4bIEC"/>
        <rdfs:range rdf:resource="https://w3id.org/netbeheer/referentiemodellen/IECCIM/TC57CIM/IEC61970/Dynamics/StandardModels/WindDynamics#WindContPType4bIEC"/>
        <rdfs:comment>Wind control P type 4B model associated with this wind turbine type 4B model.Wind turbine type 4B model with which this wind control P type 4B model is associated.</rdfs:comment>
    </owl:ObjectProperty>
    


    <!-- https://w3id.org/netbeheer/referentiemodellen/IECCIM/TC57CIM/IEC61970/Dynamics/StandardModels/WindDynamics#WindTurbineType4bIEC_WindMechIEC -->


    <owl:ObjectProperty rdf:about="https://w3id.org/netbeheer/referentiemodellen/IECCIM/TC57CIM/IEC61970/Dynamics/StandardModels/WindDynamics#WindTurbineType4bIEC_WindMechIEC">
        <owl:inverseOf rdf:resource="https://w3id.org/netbeheer/referentiemodellen/IECCIM/TC57CIM/IEC61970/Dynamics/StandardModels/WindDynamics#WindMechIEC_WindTurbineType4bIEC"/>
        <rdfs:domain rdf:resource="https://w3id.org/netbeheer/referentiemodellen/IECCIM/TC57CIM/IEC61970/Dynamics/StandardModels/WindDynamics#WindTurbineType4bIEC"/>
        <rdfs:range rdf:resource="https://w3id.org/netbeheer/referentiemodellen/IECCIM/TC57CIM/IEC61970/Dynamics/StandardModels/WindDynamics#WindMechIEC"/>
        <rdfs:comment>Wind mechanical model associated with this wind turbine Type 4B model.Wind turbine type 4B model with which this wind mechanical model is associated.</rdfs:comment>
    </owl:ObjectProperty>
    


    <!-- 
    ///////////////////////////////////////////////////////////////////////////////////////
    //
    // Data properties
    //
    ///////////////////////////////////////////////////////////////////////////////////////
     -->


    


    <!-- https://w3id.org/netbeheer/referentiemodellen/IECCIM/TC57CIM/IEC61970/Dynamics/StandardModels/WindDynamics#WindContCurrLimIEC_mdfslim -->


    <owl:DatatypeProperty rdf:about="https://w3id.org/netbeheer/referentiemodellen/IECCIM/TC57CIM/IEC61970/Dynamics/StandardModels/WindDynamics#WindContCurrLimIEC_mdfslim">
        <rdfs:domain rdf:resource="https://w3id.org/netbeheer/referentiemodellen/IECCIM/TC57CIM/IEC61970/Dynamics/StandardModels/WindDynamics#WindContCurrLimIEC"/>
        <rdfs:range rdf:resource="http://www.w3.org/2001/XMLSchema#boolean"/>
        <rdfs:comment>Limitation of type 3 stator current  (&lt;i&gt;M&lt;/i&gt;&lt;sub&gt;DFSLim&lt;/sub&gt;): 
- false=0: total current limitation, 
- true=1: stator current limitation).

It is type dependent parameter.</rdfs:comment>
    </owl:DatatypeProperty>
    


    <!-- https://w3id.org/netbeheer/referentiemodellen/IECCIM/TC57CIM/IEC61970/Dynamics/StandardModels/WindDynamics#WindContCurrLimIEC_mqpri -->


    <owl:DatatypeProperty rdf:about="https://w3id.org/netbeheer/referentiemodellen/IECCIM/TC57CIM/IEC61970/Dynamics/StandardModels/WindDynamics#WindContCurrLimIEC_mqpri">
        <rdfs:domain rdf:resource="https://w3id.org/netbeheer/referentiemodellen/IECCIM/TC57CIM/IEC61970/Dynamics/StandardModels/WindDynamics#WindContCurrLimIEC"/>
        <rdfs:range rdf:resource="http://www.w3.org/2001/XMLSchema#boolean"/>
        <rdfs:comment>Prioritisation of q control during LVRT (&lt;i&gt;M&lt;/i&gt;&lt;sub&gt;qpri&lt;/sub&gt;):
- true = 1: reactive power priority,
- false = 0: active power priority.

It is project dependent parameter.</rdfs:comment>
    </owl:DatatypeProperty>
    


    <!-- https://w3id.org/netbeheer/referentiemodellen/IECCIM/TC57CIM/IEC61970/Dynamics/StandardModels/WindDynamics#WindContPType3IEC_mplvrt -->


    <owl:DatatypeProperty rdf:about="https://w3id.org/netbeheer/referentiemodellen/IECCIM/TC57CIM/IEC61970/Dynamics/StandardModels/WindDynamics#WindContPType3IEC_mplvrt">
        <rdfs:domain rdf:resource="https://w3id.org/netbeheer/referentiemodellen/IECCIM/TC57CIM/IEC61970/Dynamics/StandardModels/WindDynamics#WindContPType3IEC"/>
        <rdfs:range rdf:resource="http://www.w3.org/2001/XMLSchema#boolean"/>
        <rdfs:comment>Enable LVRT power control mode (M&lt;sub&gt;pLVRT).&lt;/sub&gt;
true = 1: voltage control
false = 0: reactive power control.

It is project dependent parameter.</rdfs:comment>
    </owl:DatatypeProperty>
    


    <!-- https://w3id.org/netbeheer/referentiemodellen/IECCIM/TC57CIM/IEC61970/Dynamics/StandardModels/WindDynamics#WindContPType3IEC_zeta -->


    <owl:DatatypeProperty rdf:about="https://w3id.org/netbeheer/referentiemodellen/IECCIM/TC57CIM/IEC61970/Dynamics/StandardModels/WindDynamics#WindContPType3IEC_zeta">
        <rdfs:domain rdf:resource="https://w3id.org/netbeheer/referentiemodellen/IECCIM/TC57CIM/IEC61970/Dynamics/StandardModels/WindDynamics#WindContPType3IEC"/>
        <rdfs:range rdf:resource="http://www.w3.org/2001/XMLSchema#float"/>
        <rdfs:comment>Coefficient for active drive train damping (zeta). It is type dependent parameter.</rdfs:comment>
    </owl:DatatypeProperty>
    


    <!-- https://w3id.org/netbeheer/referentiemodellen/IECCIM/TC57CIM/IEC61970/Dynamics/StandardModels/WindDynamics#WindContPitchAngleIEC_dthetamax -->


    <owl:DatatypeProperty rdf:about="https://w3id.org/netbeheer/referentiemodellen/IECCIM/TC57CIM/IEC61970/Dynamics/StandardModels/WindDynamics#WindContPitchAngleIEC_dthetamax">
        <rdfs:domain rdf:resource="https://w3id.org/netbeheer/referentiemodellen/IECCIM/TC57CIM/IEC61970/Dynamics/StandardModels/WindDynamics#WindContPitchAngleIEC"/>
        <rdfs:range rdf:resource="http://www.w3.org/2001/XMLSchema#float"/>
        <rdfs:comment>Maximum pitch positive ramp rate (d&lt;i&gt;theta&lt;/i&gt;&lt;sub&gt;max&lt;/sub&gt;). It is type dependent parameter. Unit = degrees/sec. </rdfs:comment>
    </owl:DatatypeProperty>
    


    <!-- https://w3id.org/netbeheer/referentiemodellen/IECCIM/TC57CIM/IEC61970/Dynamics/StandardModels/WindDynamics#WindContPitchAngleIEC_dthetamin -->


    <owl:DatatypeProperty rdf:about="https://w3id.org/netbeheer/referentiemodellen/IECCIM/TC57CIM/IEC61970/Dynamics/StandardModels/WindDynamics#WindContPitchAngleIEC_dthetamin">
        <rdfs:domain rdf:resource="https://w3id.org/netbeheer/referentiemodellen/IECCIM/TC57CIM/IEC61970/Dynamics/StandardModels/WindDynamics#WindContPitchAngleIEC"/>
        <rdfs:range rdf:resource="http://www.w3.org/2001/XMLSchema#float"/>
        <rdfs:comment>Maximum pitch negative ramp rate (d&lt;i&gt;theta&lt;/i&gt;&lt;sub&gt;min&lt;/sub&gt;). It is type dependent parameter. Unit = degrees/sec. </rdfs:comment>
    </owl:DatatypeProperty>
    


    <!-- https://w3id.org/netbeheer/referentiemodellen/IECCIM/TC57CIM/IEC61970/Dynamics/StandardModels/WindDynamics#WindContQIEC_windLVRTQcontrolModesType -->


    <owl:DatatypeProperty rdf:about="https://w3id.org/netbeheer/referentiemodellen/IECCIM/TC57CIM/IEC61970/Dynamics/StandardModels/WindDynamics#WindContQIEC_windLVRTQcontrolModesType">
        <rdfs:domain rdf:resource="https://w3id.org/netbeheer/referentiemodellen/IECCIM/TC57CIM/IEC61970/Dynamics/StandardModels/WindDynamics#WindContQIEC"/>
        <rdfs:range rdf:resource="https://w3id.org/netbeheer/referentiemodellen/IECCIM/TC57CIM/IEC61970/Dynamics/StandardModels/WindDynamics#WindLVRTQcontrolModesKind"/>
        <rdfs:comment>Types of LVRT Q control modes (&lt;i&gt;M&lt;/i&gt;&lt;sub&gt;qLVRT&lt;/sub&gt;). It is project dependent parameter.</rdfs:comment>
    </owl:DatatypeProperty>
    


    <!-- https://w3id.org/netbeheer/referentiemodellen/IECCIM/TC57CIM/IEC61970/Dynamics/StandardModels/WindDynamics#WindContQIEC_windQcontrolModesType -->


    <owl:DatatypeProperty rdf:about="https://w3id.org/netbeheer/referentiemodellen/IECCIM/TC57CIM/IEC61970/Dynamics/StandardModels/WindDynamics#WindContQIEC_windQcontrolModesType">
        <rdfs:domain rdf:resource="https://w3id.org/netbeheer/referentiemodellen/IECCIM/TC57CIM/IEC61970/Dynamics/StandardModels/WindDynamics#WindContQIEC"/>
        <rdfs:range rdf:resource="https://w3id.org/netbeheer/referentiemodellen/IECCIM/TC57CIM/IEC61970/Dynamics/StandardModels/WindDynamics#WindQcontrolModesKind"/>
        <rdfs:comment>Types of general wind turbine Q control modes (&lt;i&gt;M&lt;/i&gt;&lt;sub&gt;qG&lt;/sub&gt;).  It is project dependent parameter.</rdfs:comment>
    </owl:DatatypeProperty>
    


    <!-- https://w3id.org/netbeheer/referentiemodellen/IECCIM/TC57CIM/IEC61970/Dynamics/StandardModels/WindDynamics#WindContRotorRIEC_komegafilt -->


    <owl:DatatypeProperty rdf:about="https://w3id.org/netbeheer/referentiemodellen/IECCIM/TC57CIM/IEC61970/Dynamics/StandardModels/WindDynamics#WindContRotorRIEC_komegafilt">
        <rdfs:domain rdf:resource="https://w3id.org/netbeheer/referentiemodellen/IECCIM/TC57CIM/IEC61970/Dynamics/StandardModels/WindDynamics#WindContRotorRIEC"/>
        <rdfs:range rdf:resource="http://www.w3.org/2001/XMLSchema#float"/>
        <rdfs:comment>Filter gain for generator speed measurement (K&lt;sub&gt;omegafilt&lt;/sub&gt;). It is type dependent parameter.</rdfs:comment>
    </owl:DatatypeProperty>
    


    <!-- https://w3id.org/netbeheer/referentiemodellen/IECCIM/TC57CIM/IEC61970/Dynamics/StandardModels/WindDynamics#WindContRotorRIEC_kpfilt -->


    <owl:DatatypeProperty rdf:about="https://w3id.org/netbeheer/referentiemodellen/IECCIM/TC57CIM/IEC61970/Dynamics/StandardModels/WindDynamics#WindContRotorRIEC_kpfilt">
        <rdfs:domain rdf:resource="https://w3id.org/netbeheer/referentiemodellen/IECCIM/TC57CIM/IEC61970/Dynamics/StandardModels/WindDynamics#WindContRotorRIEC"/>
        <rdfs:range rdf:resource="http://www.w3.org/2001/XMLSchema#float"/>
        <rdfs:comment>Filter gain for power measurement (&lt;i&gt;K&lt;/i&gt;&lt;sub&gt;pfilt&lt;/sub&gt;). It is type dependent parameter.</rdfs:comment>
    </owl:DatatypeProperty>
    


    <!-- https://w3id.org/netbeheer/referentiemodellen/IECCIM/TC57CIM/IEC61970/Dynamics/StandardModels/WindDynamics#WindDynamicsLookupTable_input -->


    <owl:DatatypeProperty rdf:about="https://w3id.org/netbeheer/referentiemodellen/IECCIM/TC57CIM/IEC61970/Dynamics/StandardModels/WindDynamics#WindDynamicsLookupTable_input">
        <rdfs:domain rdf:resource="https://w3id.org/netbeheer/referentiemodellen/IECCIM/TC57CIM/IEC61970/Dynamics/StandardModels/WindDynamics#WindDynamicsLookupTable"/>
        <rdfs:range rdf:resource="http://www.w3.org/2001/XMLSchema#float"/>
        <rdfs:comment>Input value (x) for the lookup table function.</rdfs:comment>
    </owl:DatatypeProperty>
    


    <!-- https://w3id.org/netbeheer/referentiemodellen/IECCIM/TC57CIM/IEC61970/Dynamics/StandardModels/WindDynamics#WindDynamicsLookupTable_lookupTableFunctionType -->


    <owl:DatatypeProperty rdf:about="https://w3id.org/netbeheer/referentiemodellen/IECCIM/TC57CIM/IEC61970/Dynamics/StandardModels/WindDynamics#WindDynamicsLookupTable_lookupTableFunctionType">
        <rdfs:domain rdf:resource="https://w3id.org/netbeheer/referentiemodellen/IECCIM/TC57CIM/IEC61970/Dynamics/StandardModels/WindDynamics#WindDynamicsLookupTable"/>
        <rdfs:range rdf:resource="https://w3id.org/netbeheer/referentiemodellen/IECCIM/TC57CIM/IEC61970/Dynamics/StandardModels/WindDynamics#WindLookupTableFunctionKind"/>
        <rdfs:comment>Type of the lookup table function.</rdfs:comment>
    </owl:DatatypeProperty>
    


    <!-- https://w3id.org/netbeheer/referentiemodellen/IECCIM/TC57CIM/IEC61970/Dynamics/StandardModels/WindDynamics#WindDynamicsLookupTable_output -->


    <owl:DatatypeProperty rdf:about="https://w3id.org/netbeheer/referentiemodellen/IECCIM/TC57CIM/IEC61970/Dynamics/StandardModels/WindDynamics#WindDynamicsLookupTable_output">
        <rdfs:domain rdf:resource="https://w3id.org/netbeheer/referentiemodellen/IECCIM/TC57CIM/IEC61970/Dynamics/StandardModels/WindDynamics#WindDynamicsLookupTable"/>
        <rdfs:range rdf:resource="http://www.w3.org/2001/XMLSchema#float"/>
        <rdfs:comment>Output value (y) for the lookup table function.</rdfs:comment>
    </owl:DatatypeProperty>
    


    <!-- https://w3id.org/netbeheer/referentiemodellen/IECCIM/TC57CIM/IEC61970/Dynamics/StandardModels/WindDynamics#WindDynamicsLookupTable_sequence -->


    <owl:DatatypeProperty rdf:about="https://w3id.org/netbeheer/referentiemodellen/IECCIM/TC57CIM/IEC61970/Dynamics/StandardModels/WindDynamics#WindDynamicsLookupTable_sequence">
        <rdfs:domain rdf:resource="https://w3id.org/netbeheer/referentiemodellen/IECCIM/TC57CIM/IEC61970/Dynamics/StandardModels/WindDynamics#WindDynamicsLookupTable"/>
        <rdfs:range rdf:resource="http://www.w3.org/2001/XMLSchema#nonNegativeInteger"/>
        <rdfs:comment>Sequence numbers of the pairs of the input (x) and the output (y) of the lookup table function.</rdfs:comment>
    </owl:DatatypeProperty>
    


    <!-- https://w3id.org/netbeheer/referentiemodellen/IECCIM/TC57CIM/IEC61970/Dynamics/StandardModels/WindDynamics#WindGenTurbineType3aIEC_kpc -->


    <owl:DatatypeProperty rdf:about="https://w3id.org/netbeheer/referentiemodellen/IECCIM/TC57CIM/IEC61970/Dynamics/StandardModels/WindDynamics#WindGenTurbineType3aIEC_kpc">
        <rdfs:domain rdf:resource="https://w3id.org/netbeheer/referentiemodellen/IECCIM/TC57CIM/IEC61970/Dynamics/StandardModels/WindDynamics#WindGenTurbineType3aIEC"/>
        <rdfs:range rdf:resource="http://www.w3.org/2001/XMLSchema#float"/>
        <rdfs:comment>Current PI controller proportional gain (K&lt;sub&gt;Pc&lt;/sub&gt;). It is type dependent parameter.</rdfs:comment>
    </owl:DatatypeProperty>
    


    <!-- https://w3id.org/netbeheer/referentiemodellen/IECCIM/TC57CIM/IEC61970/Dynamics/StandardModels/WindDynamics#WindGenTurbineType3bIEC_fducw -->


    <owl:DatatypeProperty rdf:about="https://w3id.org/netbeheer/referentiemodellen/IECCIM/TC57CIM/IEC61970/Dynamics/StandardModels/WindDynamics#WindGenTurbineType3bIEC_fducw">
        <rdfs:domain rdf:resource="https://w3id.org/netbeheer/referentiemodellen/IECCIM/TC57CIM/IEC61970/Dynamics/StandardModels/WindDynamics#WindGenTurbineType3bIEC"/>
        <rdfs:range rdf:resource="http://www.w3.org/2001/XMLSchema#float"/>
        <rdfs:comment>Crowbar duration versus voltage variation look-up table (f&lt;sub&gt;duCW&lt;/sub&gt;()). It is case dependent parameter.</rdfs:comment>
    </owl:DatatypeProperty>
    


    <!-- https://w3id.org/netbeheer/referentiemodellen/IECCIM/TC57CIM/IEC61970/Dynamics/StandardModels/WindDynamics#WindGenTurbineType3bIEC_mwtcwp -->


    <owl:DatatypeProperty rdf:about="https://w3id.org/netbeheer/referentiemodellen/IECCIM/TC57CIM/IEC61970/Dynamics/StandardModels/WindDynamics#WindGenTurbineType3bIEC_mwtcwp">
        <rdfs:domain rdf:resource="https://w3id.org/netbeheer/referentiemodellen/IECCIM/TC57CIM/IEC61970/Dynamics/StandardModels/WindDynamics#WindGenTurbineType3bIEC"/>
        <rdfs:range rdf:resource="http://www.w3.org/2001/XMLSchema#boolean"/>
        <rdfs:comment>Crowbar control mode (&lt;i&gt;M&lt;/i&gt;&lt;sub&gt;WTcwp&lt;/sub&gt;). 
&lt;ul&gt;
 &lt;li&gt;true = 1 in the model&lt;/li&gt;
 &lt;li&gt;false = 0 in the model.&lt;/li&gt;
&lt;/ul&gt;
The parameter is case dependent parameter.</rdfs:comment>
    </owl:DatatypeProperty>
    


    <!-- https://w3id.org/netbeheer/referentiemodellen/IECCIM/TC57CIM/IEC61970/Dynamics/StandardModels/WindDynamics#WindPitchContEmulIEC_kdroop -->


    <owl:DatatypeProperty rdf:about="https://w3id.org/netbeheer/referentiemodellen/IECCIM/TC57CIM/IEC61970/Dynamics/StandardModels/WindDynamics#WindPitchContEmulIEC_kdroop">
        <rdfs:domain rdf:resource="https://w3id.org/netbeheer/referentiemodellen/IECCIM/TC57CIM/IEC61970/Dynamics/StandardModels/WindDynamics#WindPitchContEmulIEC"/>
        <rdfs:range rdf:resource="http://www.w3.org/2001/XMLSchema#float"/>
        <rdfs:comment>Power error gain (&lt;i&gt;K&lt;/i&gt;&lt;sub&gt;droop&lt;/sub&gt;). It is case dependent parameter.</rdfs:comment>
    </owl:DatatypeProperty>
    


    <!-- https://w3id.org/netbeheer/referentiemodellen/IECCIM/TC57CIM/IEC61970/Dynamics/StandardModels/WindDynamics#WindPitchContEmulIEC_kipce -->


    <owl:DatatypeProperty rdf:about="https://w3id.org/netbeheer/referentiemodellen/IECCIM/TC57CIM/IEC61970/Dynamics/StandardModels/WindDynamics#WindPitchContEmulIEC_kipce">
        <rdfs:domain rdf:resource="https://w3id.org/netbeheer/referentiemodellen/IECCIM/TC57CIM/IEC61970/Dynamics/StandardModels/WindDynamics#WindPitchContEmulIEC"/>
        <rdfs:range rdf:resource="http://www.w3.org/2001/XMLSchema#float"/>
        <rdfs:comment>Pitch control emulator integral constant (&lt;i&gt;K&lt;/i&gt;&lt;sub&gt;I,pce&lt;/sub&gt;). It is type dependent parameter.</rdfs:comment>
    </owl:DatatypeProperty>
    


    <!-- https://w3id.org/netbeheer/referentiemodellen/IECCIM/TC57CIM/IEC61970/Dynamics/StandardModels/WindDynamics#WindPitchContEmulIEC_kppce -->


    <owl:DatatypeProperty rdf:about="https://w3id.org/netbeheer/referentiemodellen/IECCIM/TC57CIM/IEC61970/Dynamics/StandardModels/WindDynamics#WindPitchContEmulIEC_kppce">
        <rdfs:domain rdf:resource="https://w3id.org/netbeheer/referentiemodellen/IECCIM/TC57CIM/IEC61970/Dynamics/StandardModels/WindDynamics#WindPitchContEmulIEC"/>
        <rdfs:range rdf:resource="http://www.w3.org/2001/XMLSchema#float"/>
        <rdfs:comment>Pitch control emulator proportional constant (&lt;i&gt;K&lt;/i&gt;&lt;sub&gt;P,pce&lt;/sub&gt;). It is type dependent parameter.</rdfs:comment>
    </owl:DatatypeProperty>
    


    <!-- https://w3id.org/netbeheer/referentiemodellen/IECCIM/TC57CIM/IEC61970/Dynamics/StandardModels/WindDynamics#WindPlantFreqPcontrolIEC_kiwpp -->


    <owl:DatatypeProperty rdf:about="https://w3id.org/netbeheer/referentiemodellen/IECCIM/TC57CIM/IEC61970/Dynamics/StandardModels/WindDynamics#WindPlantFreqPcontrolIEC_kiwpp">
        <rdfs:domain rdf:resource="https://w3id.org/netbeheer/referentiemodellen/IECCIM/TC57CIM/IEC61970/Dynamics/StandardModels/WindDynamics#WindPlantFreqPcontrolIEC"/>
        <rdfs:range rdf:resource="http://www.w3.org/2001/XMLSchema#float"/>
        <rdfs:comment>Plant P controller integral gain (&lt;i&gt;K&lt;/i&gt;&lt;sub&gt;IWPp&lt;/sub&gt;). It is type dependent parameter.</rdfs:comment>
    </owl:DatatypeProperty>
    


    <!-- https://w3id.org/netbeheer/referentiemodellen/IECCIM/TC57CIM/IEC61970/Dynamics/StandardModels/WindDynamics#WindPlantFreqPcontrolIEC_kpwpp -->


    <owl:DatatypeProperty rdf:about="https://w3id.org/netbeheer/referentiemodellen/IECCIM/TC57CIM/IEC61970/Dynamics/StandardModels/WindDynamics#WindPlantFreqPcontrolIEC_kpwpp">
        <rdfs:domain rdf:resource="https://w3id.org/netbeheer/referentiemodellen/IECCIM/TC57CIM/IEC61970/Dynamics/StandardModels/WindDynamics#WindPlantFreqPcontrolIEC"/>
        <rdfs:range rdf:resource="http://www.w3.org/2001/XMLSchema#float"/>
        <rdfs:comment>Plant P controller proportional gain (&lt;i&gt;K&lt;/i&gt;&lt;sub&gt;PWPp&lt;/sub&gt;). It is type dependent parameter.</rdfs:comment>
    </owl:DatatypeProperty>
    


    <!-- https://w3id.org/netbeheer/referentiemodellen/IECCIM/TC57CIM/IEC61970/Dynamics/StandardModels/WindDynamics#WindPlantReactiveControlIEC_kiwpx -->


    <owl:DatatypeProperty rdf:about="https://w3id.org/netbeheer/referentiemodellen/IECCIM/TC57CIM/IEC61970/Dynamics/StandardModels/WindDynamics#WindPlantReactiveControlIEC_kiwpx">
        <rdfs:domain rdf:resource="https://w3id.org/netbeheer/referentiemodellen/IECCIM/TC57CIM/IEC61970/Dynamics/StandardModels/WindDynamics#WindPlantReactiveControlIEC"/>
        <rdfs:range rdf:resource="http://www.w3.org/2001/XMLSchema#float"/>
        <rdfs:comment>Plant Q controller integral gain (&lt;i&gt;K&lt;/i&gt;&lt;sub&gt;IWPx&lt;/sub&gt;). It is type dependent parameter.</rdfs:comment>
    </owl:DatatypeProperty>
    


    <!-- https://w3id.org/netbeheer/referentiemodellen/IECCIM/TC57CIM/IEC61970/Dynamics/StandardModels/WindDynamics#WindPlantReactiveControlIEC_kpwpx -->


    <owl:DatatypeProperty rdf:about="https://w3id.org/netbeheer/referentiemodellen/IECCIM/TC57CIM/IEC61970/Dynamics/StandardModels/WindDynamics#WindPlantReactiveControlIEC_kpwpx">
        <rdfs:domain rdf:resource="https://w3id.org/netbeheer/referentiemodellen/IECCIM/TC57CIM/IEC61970/Dynamics/StandardModels/WindDynamics#WindPlantReactiveControlIEC"/>
        <rdfs:range rdf:resource="http://www.w3.org/2001/XMLSchema#float"/>
        <rdfs:comment>Plant Q controller proportional gain (&lt;i&gt;K&lt;/i&gt;&lt;sub&gt;PWPx&lt;/sub&gt;). It is type dependent parameter.</rdfs:comment>
    </owl:DatatypeProperty>
    


    <!-- https://w3id.org/netbeheer/referentiemodellen/IECCIM/TC57CIM/IEC61970/Dynamics/StandardModels/WindDynamics#WindPlantReactiveControlIEC_mwppf -->


    <owl:DatatypeProperty rdf:about="https://w3id.org/netbeheer/referentiemodellen/IECCIM/TC57CIM/IEC61970/Dynamics/StandardModels/WindDynamics#WindPlantReactiveControlIEC_mwppf">
        <rdfs:domain rdf:resource="https://w3id.org/netbeheer/referentiemodellen/IECCIM/TC57CIM/IEC61970/Dynamics/StandardModels/WindDynamics#WindPlantReactiveControlIEC"/>
        <rdfs:range rdf:resource="http://www.w3.org/2001/XMLSchema#boolean"/>
        <rdfs:comment>Power factor control modes selector (&lt;i&gt;M&lt;/i&gt;&lt;sub&gt;WPpf&lt;/sub&gt;). Used only if mwpu is set to false.
true = 1: power factor control
false = 0: reactive power control.
It is project dependent parameter.</rdfs:comment>
    </owl:DatatypeProperty>
    


    <!-- https://w3id.org/netbeheer/referentiemodellen/IECCIM/TC57CIM/IEC61970/Dynamics/StandardModels/WindDynamics#WindPlantReactiveControlIEC_mwpu -->


    <owl:DatatypeProperty rdf:about="https://w3id.org/netbeheer/referentiemodellen/IECCIM/TC57CIM/IEC61970/Dynamics/StandardModels/WindDynamics#WindPlantReactiveControlIEC_mwpu">
        <rdfs:domain rdf:resource="https://w3id.org/netbeheer/referentiemodellen/IECCIM/TC57CIM/IEC61970/Dynamics/StandardModels/WindDynamics#WindPlantReactiveControlIEC"/>
        <rdfs:range rdf:resource="http://www.w3.org/2001/XMLSchema#boolean"/>
        <rdfs:comment>Reactive power control modes selector (&lt;i&gt;M&lt;/i&gt;&lt;sub&gt;WPu&lt;/sub&gt;).
true = 1: voltage control
false = 0: reactive power control.
It is project dependent parameter.</rdfs:comment>
    </owl:DatatypeProperty>
    


    <!-- 
    ///////////////////////////////////////////////////////////////////////////////////////
    //
    // Classes
    //
    ///////////////////////////////////////////////////////////////////////////////////////
     -->


    


    <!-- https://w3id.org/netbeheer/referentiemodellen/IECCIM/TC57CIM/IEC61970/Base/Core#IdentifiedObject -->


    <owl:Class rdf:about="https://w3id.org/netbeheer/referentiemodellen/IECCIM/TC57CIM/IEC61970/Base/Core#IdentifiedObject"/>
    


    <!-- https://w3id.org/netbeheer/referentiemodellen/IECCIM/TC57CIM/IEC61970/Base/Domain#AngleDegrees -->


    <owl:Class rdf:about="https://w3id.org/netbeheer/referentiemodellen/IECCIM/TC57CIM/IEC61970/Base/Domain#AngleDegrees"/>
    


    <!-- https://w3id.org/netbeheer/referentiemodellen/IECCIM/TC57CIM/IEC61970/Base/Domain#PU -->


    <owl:Class rdf:about="https://w3id.org/netbeheer/referentiemodellen/IECCIM/TC57CIM/IEC61970/Base/Domain#PU"/>
    


    <!-- https://w3id.org/netbeheer/referentiemodellen/IECCIM/TC57CIM/IEC61970/Base/Domain#Seconds -->


    <owl:Class rdf:about="https://w3id.org/netbeheer/referentiemodellen/IECCIM/TC57CIM/IEC61970/Base/Domain#Seconds"/>
    


    <!-- https://w3id.org/netbeheer/referentiemodellen/IECCIM/TC57CIM/IEC61970/Dynamics/StandardModels#DynamicsFunctionBlock -->


    <owl:Class rdf:about="https://w3id.org/netbeheer/referentiemodellen/IECCIM/TC57CIM/IEC61970/Dynamics/StandardModels#DynamicsFunctionBlock"/>
    


    <!-- https://w3id.org/netbeheer/referentiemodellen/IECCIM/TC57CIM/IEC61970/Dynamics/StandardModels/WindDynamics#WindAeroConstIEC -->


    <owl:Class rdf:about="https://w3id.org/netbeheer/referentiemodellen/IECCIM/TC57CIM/IEC61970/Dynamics/StandardModels/WindDynamics#WindAeroConstIEC">
        <rdfs:subClassOf rdf:resource="https://w3id.org/netbeheer/referentiemodellen/IECCIM/TC57CIM/IEC61970/Base/Core#IdentifiedObject"/>
        <rdfs:subClassOf>
            <owl:Restriction>
                <owl:onProperty rdf:resource="https://w3id.org/netbeheer/referentiemodellen/IECCIM/TC57CIM/IEC61970/Dynamics/StandardModels/WindDynamics#WindAeroConstIEC_WindGenTurbineType1IEC"/>
                <owl:qualifiedCardinality rdf:datatype="http://www.w3.org/2001/XMLSchema#nonNegativeInteger">1</owl:qualifiedCardinality>
                <owl:onClass rdf:resource="https://w3id.org/netbeheer/referentiemodellen/IECCIM/TC57CIM/IEC61970/Dynamics/StandardModels/WindDynamics#WindAeroConstIEC"/>
            </owl:Restriction>
        </rdfs:subClassOf>
        <rdfs:comment>The constant aerodynamic torque model assumes that the aerodynamic torque is constant.

Reference: IEC Standard 61400-27-1 Section 6.6.1.1.</rdfs:comment>
    </owl:Class>
    


    <!-- https://w3id.org/netbeheer/referentiemodellen/IECCIM/TC57CIM/IEC61970/Dynamics/StandardModels/WindDynamics#WindAeroLinearIEC -->


    <owl:Class rdf:about="https://w3id.org/netbeheer/referentiemodellen/IECCIM/TC57CIM/IEC61970/Dynamics/StandardModels/WindDynamics#WindAeroLinearIEC">
        <rdfs:subClassOf rdf:resource="https://w3id.org/netbeheer/referentiemodellen/IECCIM/TC57CIM/IEC61970/Base/Core#IdentifiedObject"/>
        <rdfs:subClassOf>
            <owl:Restriction>
                <owl:onProperty rdf:resource="https://w3id.org/netbeheer/referentiemodellen/IECCIM/TC57CIM/IEC61970/Dynamics/StandardModels/WindDynamics#WindAeroLinearIEC_dpomega"/>
                <owl:minQualifiedCardinality rdf:datatype="http://www.w3.org/2001/XMLSchema#nonNegativeInteger">0</owl:minQualifiedCardinality>
                <owl:onClass rdf:resource="https://w3id.org/netbeheer/referentiemodellen/IECCIM/TC57CIM/IEC61970/Base/Domain#PU"/>
            </owl:Restriction>
        </rdfs:subClassOf>
        <rdfs:subClassOf>
            <owl:Restriction>
                <owl:onProperty rdf:resource="https://w3id.org/netbeheer/referentiemodellen/IECCIM/TC57CIM/IEC61970/Dynamics/StandardModels/WindDynamics#WindAeroLinearIEC_dptheta"/>
                <owl:minQualifiedCardinality rdf:datatype="http://www.w3.org/2001/XMLSchema#nonNegativeInteger">0</owl:minQualifiedCardinality>
                <owl:onClass rdf:resource="https://w3id.org/netbeheer/referentiemodellen/IECCIM/TC57CIM/IEC61970/Base/Domain#PU"/>
            </owl:Restriction>
        </rdfs:subClassOf>
        <rdfs:subClassOf>
            <owl:Restriction>
                <owl:onProperty rdf:resource="https://w3id.org/netbeheer/referentiemodellen/IECCIM/TC57CIM/IEC61970/Dynamics/StandardModels/WindDynamics#WindAeroLinearIEC_omegazero"/>
                <owl:minQualifiedCardinality rdf:datatype="http://www.w3.org/2001/XMLSchema#nonNegativeInteger">0</owl:minQualifiedCardinality>
                <owl:onClass rdf:resource="https://w3id.org/netbeheer/referentiemodellen/IECCIM/TC57CIM/IEC61970/Base/Domain#PU"/>
            </owl:Restriction>
        </rdfs:subClassOf>
        <rdfs:subClassOf>
            <owl:Restriction>
                <owl:onProperty rdf:resource="https://w3id.org/netbeheer/referentiemodellen/IECCIM/TC57CIM/IEC61970/Dynamics/StandardModels/WindDynamics#WindAeroLinearIEC_pavail"/>
                <owl:minQualifiedCardinality rdf:datatype="http://www.w3.org/2001/XMLSchema#nonNegativeInteger">0</owl:minQualifiedCardinality>
                <owl:onClass rdf:resource="https://w3id.org/netbeheer/referentiemodellen/IECCIM/TC57CIM/IEC61970/Base/Domain#PU"/>
            </owl:Restriction>
        </rdfs:subClassOf>
        <rdfs:subClassOf>
            <owl:Restriction>
                <owl:onProperty rdf:resource="https://w3id.org/netbeheer/referentiemodellen/IECCIM/TC57CIM/IEC61970/Dynamics/StandardModels/WindDynamics#WindAeroLinearIEC_thetazero"/>
                <owl:minQualifiedCardinality rdf:datatype="http://www.w3.org/2001/XMLSchema#nonNegativeInteger">0</owl:minQualifiedCardinality>
                <owl:onClass rdf:resource="https://w3id.org/netbeheer/referentiemodellen/IECCIM/TC57CIM/IEC61970/Base/Domain#AngleDegrees"/>
            </owl:Restriction>
        </rdfs:subClassOf>
        <rdfs:subClassOf>
            <owl:Restriction>
                <owl:onProperty rdf:resource="https://w3id.org/netbeheer/referentiemodellen/IECCIM/TC57CIM/IEC61970/Dynamics/StandardModels/WindDynamics#WindAeroLinearIEC_WindGenTurbineType3IEC"/>
                <owl:qualifiedCardinality rdf:datatype="http://www.w3.org/2001/XMLSchema#nonNegativeInteger">1</owl:qualifiedCardinality>
                <owl:onClass rdf:resource="https://w3id.org/netbeheer/referentiemodellen/IECCIM/TC57CIM/IEC61970/Dynamics/StandardModels/WindDynamics#WindAeroLinearIEC"/>
            </owl:Restriction>
        </rdfs:subClassOf>
        <rdfs:subClassOf>
            <owl:Restriction>
                <owl:onProperty rdf:resource="https://w3id.org/netbeheer/referentiemodellen/IECCIM/TC57CIM/IEC61970/Dynamics/StandardModels/WindDynamics#WindAeroLinearIEC_dpomega"/>
                <owl:maxQualifiedCardinality rdf:datatype="http://www.w3.org/2001/XMLSchema#nonNegativeInteger">1</owl:maxQualifiedCardinality>
                <owl:onClass rdf:resource="https://w3id.org/netbeheer/referentiemodellen/IECCIM/TC57CIM/IEC61970/Base/Domain#PU"/>
            </owl:Restriction>
        </rdfs:subClassOf>
        <rdfs:subClassOf>
            <owl:Restriction>
                <owl:onProperty rdf:resource="https://w3id.org/netbeheer/referentiemodellen/IECCIM/TC57CIM/IEC61970/Dynamics/StandardModels/WindDynamics#WindAeroLinearIEC_dptheta"/>
                <owl:maxQualifiedCardinality rdf:datatype="http://www.w3.org/2001/XMLSchema#nonNegativeInteger">1</owl:maxQualifiedCardinality>
                <owl:onClass rdf:resource="https://w3id.org/netbeheer/referentiemodellen/IECCIM/TC57CIM/IEC61970/Base/Domain#PU"/>
            </owl:Restriction>
        </rdfs:subClassOf>
        <rdfs:subClassOf>
            <owl:Restriction>
                <owl:onProperty rdf:resource="https://w3id.org/netbeheer/referentiemodellen/IECCIM/TC57CIM/IEC61970/Dynamics/StandardModels/WindDynamics#WindAeroLinearIEC_omegazero"/>
                <owl:maxQualifiedCardinality rdf:datatype="http://www.w3.org/2001/XMLSchema#nonNegativeInteger">1</owl:maxQualifiedCardinality>
                <owl:onClass rdf:resource="https://w3id.org/netbeheer/referentiemodellen/IECCIM/TC57CIM/IEC61970/Base/Domain#PU"/>
            </owl:Restriction>
        </rdfs:subClassOf>
        <rdfs:subClassOf>
            <owl:Restriction>
                <owl:onProperty rdf:resource="https://w3id.org/netbeheer/referentiemodellen/IECCIM/TC57CIM/IEC61970/Dynamics/StandardModels/WindDynamics#WindAeroLinearIEC_pavail"/>
                <owl:maxQualifiedCardinality rdf:datatype="http://www.w3.org/2001/XMLSchema#nonNegativeInteger">1</owl:maxQualifiedCardinality>
                <owl:onClass rdf:resource="https://w3id.org/netbeheer/referentiemodellen/IECCIM/TC57CIM/IEC61970/Base/Domain#PU"/>
            </owl:Restriction>
        </rdfs:subClassOf>
        <rdfs:subClassOf>
            <owl:Restriction>
                <owl:onProperty rdf:resource="https://w3id.org/netbeheer/referentiemodellen/IECCIM/TC57CIM/IEC61970/Dynamics/StandardModels/WindDynamics#WindAeroLinearIEC_thetazero"/>
                <owl:maxQualifiedCardinality rdf:datatype="http://www.w3.org/2001/XMLSchema#nonNegativeInteger">1</owl:maxQualifiedCardinality>
                <owl:onClass rdf:resource="https://w3id.org/netbeheer/referentiemodellen/IECCIM/TC57CIM/IEC61970/Base/Domain#AngleDegrees"/>
            </owl:Restriction>
        </rdfs:subClassOf>
        <rdfs:comment>The linearised aerodynamic model.  

Reference: IEC Standard 614000-27-1 Section 6.6.1.2.</rdfs:comment>
    </owl:Class>
    


    <!-- https://w3id.org/netbeheer/referentiemodellen/IECCIM/TC57CIM/IEC61970/Dynamics/StandardModels/WindDynamics#WindContCurrLimIEC -->


    <owl:Class rdf:about="https://w3id.org/netbeheer/referentiemodellen/IECCIM/TC57CIM/IEC61970/Dynamics/StandardModels/WindDynamics#WindContCurrLimIEC">
        <rdfs:subClassOf rdf:resource="https://w3id.org/netbeheer/referentiemodellen/IECCIM/TC57CIM/IEC61970/Base/Core#IdentifiedObject"/>
        <rdfs:subClassOf>
            <owl:Restriction>
                <owl:onProperty rdf:resource="https://w3id.org/netbeheer/referentiemodellen/IECCIM/TC57CIM/IEC61970/Dynamics/StandardModels/WindDynamics#WindContCurrLimIEC_WindDynamicsLookupTable"/>
                <owl:minQualifiedCardinality rdf:datatype="http://www.w3.org/2001/XMLSchema#nonNegativeInteger">0</owl:minQualifiedCardinality>
                <owl:onClass rdf:resource="https://w3id.org/netbeheer/referentiemodellen/IECCIM/TC57CIM/IEC61970/Dynamics/StandardModels/WindDynamics#WindContCurrLimIEC"/>
            </owl:Restriction>
        </rdfs:subClassOf>
        <rdfs:subClassOf>
            <owl:Restriction>
                <owl:onProperty rdf:resource="https://w3id.org/netbeheer/referentiemodellen/IECCIM/TC57CIM/IEC61970/Dynamics/StandardModels/WindDynamics#WindContCurrLimIEC_imax"/>
                <owl:minQualifiedCardinality rdf:datatype="http://www.w3.org/2001/XMLSchema#nonNegativeInteger">0</owl:minQualifiedCardinality>
                <owl:onClass rdf:resource="https://w3id.org/netbeheer/referentiemodellen/IECCIM/TC57CIM/IEC61970/Base/Domain#PU"/>
            </owl:Restriction>
        </rdfs:subClassOf>
        <rdfs:subClassOf>
            <owl:Restriction>
                <owl:onProperty rdf:resource="https://w3id.org/netbeheer/referentiemodellen/IECCIM/TC57CIM/IEC61970/Dynamics/StandardModels/WindDynamics#WindContCurrLimIEC_imaxdip"/>
                <owl:minQualifiedCardinality rdf:datatype="http://www.w3.org/2001/XMLSchema#nonNegativeInteger">0</owl:minQualifiedCardinality>
                <owl:onClass rdf:resource="https://w3id.org/netbeheer/referentiemodellen/IECCIM/TC57CIM/IEC61970/Base/Domain#PU"/>
            </owl:Restriction>
        </rdfs:subClassOf>
        <rdfs:subClassOf>
            <owl:Restriction>
                <owl:onProperty rdf:resource="https://w3id.org/netbeheer/referentiemodellen/IECCIM/TC57CIM/IEC61970/Dynamics/StandardModels/WindDynamics#WindContCurrLimIEC_tufilt"/>
                <owl:minQualifiedCardinality rdf:datatype="http://www.w3.org/2001/XMLSchema#nonNegativeInteger">0</owl:minQualifiedCardinality>
                <owl:onClass rdf:resource="https://w3id.org/netbeheer/referentiemodellen/IECCIM/TC57CIM/IEC61970/Base/Domain#Seconds"/>
            </owl:Restriction>
        </rdfs:subClassOf>
        <rdfs:subClassOf>
            <owl:Restriction>
                <owl:onProperty rdf:resource="https://w3id.org/netbeheer/referentiemodellen/IECCIM/TC57CIM/IEC61970/Dynamics/StandardModels/WindDynamics#WindContCurrLimIEC_WindTurbineType3or4IEC"/>
                <owl:qualifiedCardinality rdf:datatype="http://www.w3.org/2001/XMLSchema#nonNegativeInteger">1</owl:qualifiedCardinality>
                <owl:onClass rdf:resource="https://w3id.org/netbeheer/referentiemodellen/IECCIM/TC57CIM/IEC61970/Dynamics/StandardModels/WindDynamics#WindContCurrLimIEC"/>
            </owl:Restriction>
        </rdfs:subClassOf>
        <rdfs:subClassOf>
            <owl:Restriction>
                <owl:onProperty rdf:resource="https://w3id.org/netbeheer/referentiemodellen/IECCIM/TC57CIM/IEC61970/Dynamics/StandardModels/WindDynamics#WindContCurrLimIEC_WindDynamicsLookupTable"/>
                <owl:maxQualifiedCardinality rdf:datatype="http://www.w3.org/2001/XMLSchema#nonNegativeInteger">1</owl:maxQualifiedCardinality>
                <owl:onClass rdf:resource="https://w3id.org/netbeheer/referentiemodellen/IECCIM/TC57CIM/IEC61970/Dynamics/StandardModels/WindDynamics#WindContCurrLimIEC"/>
            </owl:Restriction>
        </rdfs:subClassOf>
        <rdfs:subClassOf>
            <owl:Restriction>
                <owl:onProperty rdf:resource="https://w3id.org/netbeheer/referentiemodellen/IECCIM/TC57CIM/IEC61970/Dynamics/StandardModels/WindDynamics#WindContCurrLimIEC_imax"/>
                <owl:maxQualifiedCardinality rdf:datatype="http://www.w3.org/2001/XMLSchema#nonNegativeInteger">1</owl:maxQualifiedCardinality>
                <owl:onClass rdf:resource="https://w3id.org/netbeheer/referentiemodellen/IECCIM/TC57CIM/IEC61970/Base/Domain#PU"/>
            </owl:Restriction>
        </rdfs:subClassOf>
        <rdfs:subClassOf>
            <owl:Restriction>
                <owl:onProperty rdf:resource="https://w3id.org/netbeheer/referentiemodellen/IECCIM/TC57CIM/IEC61970/Dynamics/StandardModels/WindDynamics#WindContCurrLimIEC_imaxdip"/>
                <owl:maxQualifiedCardinality rdf:datatype="http://www.w3.org/2001/XMLSchema#nonNegativeInteger">1</owl:maxQualifiedCardinality>
                <owl:onClass rdf:resource="https://w3id.org/netbeheer/referentiemodellen/IECCIM/TC57CIM/IEC61970/Base/Domain#PU"/>
            </owl:Restriction>
        </rdfs:subClassOf>
        <rdfs:subClassOf>
            <owl:Restriction>
                <owl:onProperty rdf:resource="https://w3id.org/netbeheer/referentiemodellen/IECCIM/TC57CIM/IEC61970/Dynamics/StandardModels/WindDynamics#WindContCurrLimIEC_tufilt"/>
                <owl:maxQualifiedCardinality rdf:datatype="http://www.w3.org/2001/XMLSchema#nonNegativeInteger">1</owl:maxQualifiedCardinality>
                <owl:onClass rdf:resource="https://w3id.org/netbeheer/referentiemodellen/IECCIM/TC57CIM/IEC61970/Base/Domain#Seconds"/>
            </owl:Restriction>
        </rdfs:subClassOf>
        <rdfs:subClassOf>
            <owl:Restriction>
                <owl:onProperty rdf:resource="https://w3id.org/netbeheer/referentiemodellen/IECCIM/TC57CIM/IEC61970/Dynamics/StandardModels/WindDynamics#WindContCurrLimIEC_mdfslim"/>
                <owl:minQualifiedCardinality rdf:datatype="http://www.w3.org/2001/XMLSchema#nonNegativeInteger">0</owl:minQualifiedCardinality>
                <owl:onDataRange rdf:resource="http://www.w3.org/2001/XMLSchema#boolean"/>
            </owl:Restriction>
        </rdfs:subClassOf>
        <rdfs:subClassOf>
            <owl:Restriction>
                <owl:onProperty rdf:resource="https://w3id.org/netbeheer/referentiemodellen/IECCIM/TC57CIM/IEC61970/Dynamics/StandardModels/WindDynamics#WindContCurrLimIEC_mqpri"/>
                <owl:minQualifiedCardinality rdf:datatype="http://www.w3.org/2001/XMLSchema#nonNegativeInteger">0</owl:minQualifiedCardinality>
                <owl:onDataRange rdf:resource="http://www.w3.org/2001/XMLSchema#boolean"/>
            </owl:Restriction>
        </rdfs:subClassOf>
        <rdfs:subClassOf>
            <owl:Restriction>
                <owl:onProperty rdf:resource="https://w3id.org/netbeheer/referentiemodellen/IECCIM/TC57CIM/IEC61970/Dynamics/StandardModels/WindDynamics#WindContCurrLimIEC_mdfslim"/>
                <owl:maxQualifiedCardinality rdf:datatype="http://www.w3.org/2001/XMLSchema#nonNegativeInteger">1</owl:maxQualifiedCardinality>
                <owl:onDataRange rdf:resource="http://www.w3.org/2001/XMLSchema#boolean"/>
            </owl:Restriction>
        </rdfs:subClassOf>
        <rdfs:subClassOf>
            <owl:Restriction>
                <owl:onProperty rdf:resource="https://w3id.org/netbeheer/referentiemodellen/IECCIM/TC57CIM/IEC61970/Dynamics/StandardModels/WindDynamics#WindContCurrLimIEC_mqpri"/>
                <owl:maxQualifiedCardinality rdf:datatype="http://www.w3.org/2001/XMLSchema#nonNegativeInteger">1</owl:maxQualifiedCardinality>
                <owl:onDataRange rdf:resource="http://www.w3.org/2001/XMLSchema#boolean"/>
            </owl:Restriction>
        </rdfs:subClassOf>
        <rdfs:comment>Current limitation model.  The current limitation model combines the physical limits.

Reference: IEC Standard 61400-27-1 Section 6.6.5.7.</rdfs:comment>
    </owl:Class>
    


    <!-- https://w3id.org/netbeheer/referentiemodellen/IECCIM/TC57CIM/IEC61970/Dynamics/StandardModels/WindDynamics#WindContPType3IEC -->


    <owl:Class rdf:about="https://w3id.org/netbeheer/referentiemodellen/IECCIM/TC57CIM/IEC61970/Dynamics/StandardModels/WindDynamics#WindContPType3IEC">
        <rdfs:subClassOf rdf:resource="https://w3id.org/netbeheer/referentiemodellen/IECCIM/TC57CIM/IEC61970/Base/Core#IdentifiedObject"/>
        <rdfs:subClassOf>
            <owl:Restriction>
                <owl:onProperty rdf:resource="https://w3id.org/netbeheer/referentiemodellen/IECCIM/TC57CIM/IEC61970/Dynamics/StandardModels/WindDynamics#WindContPType3IEC_WindDynamicsLookupTable"/>
                <owl:minQualifiedCardinality rdf:datatype="http://www.w3.org/2001/XMLSchema#nonNegativeInteger">0</owl:minQualifiedCardinality>
                <owl:onClass rdf:resource="https://w3id.org/netbeheer/referentiemodellen/IECCIM/TC57CIM/IEC61970/Dynamics/StandardModels/WindDynamics#WindContPType3IEC"/>
            </owl:Restriction>
        </rdfs:subClassOf>
        <rdfs:subClassOf>
            <owl:Restriction>
                <owl:onProperty rdf:resource="https://w3id.org/netbeheer/referentiemodellen/IECCIM/TC57CIM/IEC61970/Dynamics/StandardModels/WindDynamics#WindContPType3IEC_dpmax"/>
                <owl:minQualifiedCardinality rdf:datatype="http://www.w3.org/2001/XMLSchema#nonNegativeInteger">0</owl:minQualifiedCardinality>
                <owl:onClass rdf:resource="https://w3id.org/netbeheer/referentiemodellen/IECCIM/TC57CIM/IEC61970/Base/Domain#PU"/>
            </owl:Restriction>
        </rdfs:subClassOf>
        <rdfs:subClassOf>
            <owl:Restriction>
                <owl:onProperty rdf:resource="https://w3id.org/netbeheer/referentiemodellen/IECCIM/TC57CIM/IEC61970/Dynamics/StandardModels/WindDynamics#WindContPType3IEC_dtrisemaxlvrt"/>
                <owl:minQualifiedCardinality rdf:datatype="http://www.w3.org/2001/XMLSchema#nonNegativeInteger">0</owl:minQualifiedCardinality>
                <owl:onClass rdf:resource="https://w3id.org/netbeheer/referentiemodellen/IECCIM/TC57CIM/IEC61970/Base/Domain#PU"/>
            </owl:Restriction>
        </rdfs:subClassOf>
        <rdfs:subClassOf>
            <owl:Restriction>
                <owl:onProperty rdf:resource="https://w3id.org/netbeheer/referentiemodellen/IECCIM/TC57CIM/IEC61970/Dynamics/StandardModels/WindDynamics#WindContPType3IEC_kdtd"/>
                <owl:minQualifiedCardinality rdf:datatype="http://www.w3.org/2001/XMLSchema#nonNegativeInteger">0</owl:minQualifiedCardinality>
                <owl:onClass rdf:resource="https://w3id.org/netbeheer/referentiemodellen/IECCIM/TC57CIM/IEC61970/Base/Domain#PU"/>
            </owl:Restriction>
        </rdfs:subClassOf>
        <rdfs:subClassOf>
            <owl:Restriction>
                <owl:onProperty rdf:resource="https://w3id.org/netbeheer/referentiemodellen/IECCIM/TC57CIM/IEC61970/Dynamics/StandardModels/WindDynamics#WindContPType3IEC_kip"/>
                <owl:minQualifiedCardinality rdf:datatype="http://www.w3.org/2001/XMLSchema#nonNegativeInteger">0</owl:minQualifiedCardinality>
                <owl:onClass rdf:resource="https://w3id.org/netbeheer/referentiemodellen/IECCIM/TC57CIM/IEC61970/Base/Domain#PU"/>
            </owl:Restriction>
        </rdfs:subClassOf>
        <rdfs:subClassOf>
            <owl:Restriction>
                <owl:onProperty rdf:resource="https://w3id.org/netbeheer/referentiemodellen/IECCIM/TC57CIM/IEC61970/Dynamics/StandardModels/WindDynamics#WindContPType3IEC_kpp"/>
                <owl:minQualifiedCardinality rdf:datatype="http://www.w3.org/2001/XMLSchema#nonNegativeInteger">0</owl:minQualifiedCardinality>
                <owl:onClass rdf:resource="https://w3id.org/netbeheer/referentiemodellen/IECCIM/TC57CIM/IEC61970/Base/Domain#PU"/>
            </owl:Restriction>
        </rdfs:subClassOf>
        <rdfs:subClassOf>
            <owl:Restriction>
                <owl:onProperty rdf:resource="https://w3id.org/netbeheer/referentiemodellen/IECCIM/TC57CIM/IEC61970/Dynamics/StandardModels/WindDynamics#WindContPType3IEC_omegaoffset"/>
                <owl:minQualifiedCardinality rdf:datatype="http://www.w3.org/2001/XMLSchema#nonNegativeInteger">0</owl:minQualifiedCardinality>
                <owl:onClass rdf:resource="https://w3id.org/netbeheer/referentiemodellen/IECCIM/TC57CIM/IEC61970/Base/Domain#PU"/>
            </owl:Restriction>
        </rdfs:subClassOf>
        <rdfs:subClassOf>
            <owl:Restriction>
                <owl:onProperty rdf:resource="https://w3id.org/netbeheer/referentiemodellen/IECCIM/TC57CIM/IEC61970/Dynamics/StandardModels/WindDynamics#WindContPType3IEC_pdtdmax"/>
                <owl:minQualifiedCardinality rdf:datatype="http://www.w3.org/2001/XMLSchema#nonNegativeInteger">0</owl:minQualifiedCardinality>
                <owl:onClass rdf:resource="https://w3id.org/netbeheer/referentiemodellen/IECCIM/TC57CIM/IEC61970/Base/Domain#PU"/>
            </owl:Restriction>
        </rdfs:subClassOf>
        <rdfs:subClassOf>
            <owl:Restriction>
                <owl:onProperty rdf:resource="https://w3id.org/netbeheer/referentiemodellen/IECCIM/TC57CIM/IEC61970/Dynamics/StandardModels/WindDynamics#WindContPType3IEC_rramp"/>
                <owl:minQualifiedCardinality rdf:datatype="http://www.w3.org/2001/XMLSchema#nonNegativeInteger">0</owl:minQualifiedCardinality>
                <owl:onClass rdf:resource="https://w3id.org/netbeheer/referentiemodellen/IECCIM/TC57CIM/IEC61970/Base/Domain#PU"/>
            </owl:Restriction>
        </rdfs:subClassOf>
        <rdfs:subClassOf>
            <owl:Restriction>
                <owl:onProperty rdf:resource="https://w3id.org/netbeheer/referentiemodellen/IECCIM/TC57CIM/IEC61970/Dynamics/StandardModels/WindDynamics#WindContPType3IEC_tdvs"/>
                <owl:minQualifiedCardinality rdf:datatype="http://www.w3.org/2001/XMLSchema#nonNegativeInteger">0</owl:minQualifiedCardinality>
                <owl:onClass rdf:resource="https://w3id.org/netbeheer/referentiemodellen/IECCIM/TC57CIM/IEC61970/Base/Domain#Seconds"/>
            </owl:Restriction>
        </rdfs:subClassOf>
        <rdfs:subClassOf>
            <owl:Restriction>
                <owl:onProperty rdf:resource="https://w3id.org/netbeheer/referentiemodellen/IECCIM/TC57CIM/IEC61970/Dynamics/StandardModels/WindDynamics#WindContPType3IEC_temin"/>
                <owl:minQualifiedCardinality rdf:datatype="http://www.w3.org/2001/XMLSchema#nonNegativeInteger">0</owl:minQualifiedCardinality>
                <owl:onClass rdf:resource="https://w3id.org/netbeheer/referentiemodellen/IECCIM/TC57CIM/IEC61970/Base/Domain#PU"/>
            </owl:Restriction>
        </rdfs:subClassOf>
        <rdfs:subClassOf>
            <owl:Restriction>
                <owl:onProperty rdf:resource="https://w3id.org/netbeheer/referentiemodellen/IECCIM/TC57CIM/IEC61970/Dynamics/StandardModels/WindDynamics#WindContPType3IEC_tomegafilt"/>
                <owl:minQualifiedCardinality rdf:datatype="http://www.w3.org/2001/XMLSchema#nonNegativeInteger">0</owl:minQualifiedCardinality>
                <owl:onClass rdf:resource="https://w3id.org/netbeheer/referentiemodellen/IECCIM/TC57CIM/IEC61970/Base/Domain#Seconds"/>
            </owl:Restriction>
        </rdfs:subClassOf>
        <rdfs:subClassOf>
            <owl:Restriction>
                <owl:onProperty rdf:resource="https://w3id.org/netbeheer/referentiemodellen/IECCIM/TC57CIM/IEC61970/Dynamics/StandardModels/WindDynamics#WindContPType3IEC_tpfilt"/>
                <owl:minQualifiedCardinality rdf:datatype="http://www.w3.org/2001/XMLSchema#nonNegativeInteger">0</owl:minQualifiedCardinality>
                <owl:onClass rdf:resource="https://w3id.org/netbeheer/referentiemodellen/IECCIM/TC57CIM/IEC61970/Base/Domain#Seconds"/>
            </owl:Restriction>
        </rdfs:subClassOf>
        <rdfs:subClassOf>
            <owl:Restriction>
                <owl:onProperty rdf:resource="https://w3id.org/netbeheer/referentiemodellen/IECCIM/TC57CIM/IEC61970/Dynamics/StandardModels/WindDynamics#WindContPType3IEC_tpord"/>
                <owl:minQualifiedCardinality rdf:datatype="http://www.w3.org/2001/XMLSchema#nonNegativeInteger">0</owl:minQualifiedCardinality>
                <owl:onClass rdf:resource="https://w3id.org/netbeheer/referentiemodellen/IECCIM/TC57CIM/IEC61970/Base/Domain#PU"/>
            </owl:Restriction>
        </rdfs:subClassOf>
        <rdfs:subClassOf>
            <owl:Restriction>
                <owl:onProperty rdf:resource="https://w3id.org/netbeheer/referentiemodellen/IECCIM/TC57CIM/IEC61970/Dynamics/StandardModels/WindDynamics#WindContPType3IEC_tufilt"/>
                <owl:minQualifiedCardinality rdf:datatype="http://www.w3.org/2001/XMLSchema#nonNegativeInteger">0</owl:minQualifiedCardinality>
                <owl:onClass rdf:resource="https://w3id.org/netbeheer/referentiemodellen/IECCIM/TC57CIM/IEC61970/Base/Domain#Seconds"/>
            </owl:Restriction>
        </rdfs:subClassOf>
        <rdfs:subClassOf>
            <owl:Restriction>
                <owl:onProperty rdf:resource="https://w3id.org/netbeheer/referentiemodellen/IECCIM/TC57CIM/IEC61970/Dynamics/StandardModels/WindDynamics#WindContPType3IEC_tuscale"/>
                <owl:minQualifiedCardinality rdf:datatype="http://www.w3.org/2001/XMLSchema#nonNegativeInteger">0</owl:minQualifiedCardinality>
                <owl:onClass rdf:resource="https://w3id.org/netbeheer/referentiemodellen/IECCIM/TC57CIM/IEC61970/Base/Domain#PU"/>
            </owl:Restriction>
        </rdfs:subClassOf>
        <rdfs:subClassOf>
            <owl:Restriction>
                <owl:onProperty rdf:resource="https://w3id.org/netbeheer/referentiemodellen/IECCIM/TC57CIM/IEC61970/Dynamics/StandardModels/WindDynamics#WindContPType3IEC_twref"/>
                <owl:minQualifiedCardinality rdf:datatype="http://www.w3.org/2001/XMLSchema#nonNegativeInteger">0</owl:minQualifiedCardinality>
                <owl:onClass rdf:resource="https://w3id.org/netbeheer/referentiemodellen/IECCIM/TC57CIM/IEC61970/Base/Domain#Seconds"/>
            </owl:Restriction>
        </rdfs:subClassOf>
        <rdfs:subClassOf>
            <owl:Restriction>
                <owl:onProperty rdf:resource="https://w3id.org/netbeheer/referentiemodellen/IECCIM/TC57CIM/IEC61970/Dynamics/StandardModels/WindDynamics#WindContPType3IEC_udvs"/>
                <owl:minQualifiedCardinality rdf:datatype="http://www.w3.org/2001/XMLSchema#nonNegativeInteger">0</owl:minQualifiedCardinality>
                <owl:onClass rdf:resource="https://w3id.org/netbeheer/referentiemodellen/IECCIM/TC57CIM/IEC61970/Base/Domain#PU"/>
            </owl:Restriction>
        </rdfs:subClassOf>
        <rdfs:subClassOf>
            <owl:Restriction>
                <owl:onProperty rdf:resource="https://w3id.org/netbeheer/referentiemodellen/IECCIM/TC57CIM/IEC61970/Dynamics/StandardModels/WindDynamics#WindContPType3IEC_updip"/>
                <owl:minQualifiedCardinality rdf:datatype="http://www.w3.org/2001/XMLSchema#nonNegativeInteger">0</owl:minQualifiedCardinality>
                <owl:onClass rdf:resource="https://w3id.org/netbeheer/referentiemodellen/IECCIM/TC57CIM/IEC61970/Base/Domain#PU"/>
            </owl:Restriction>
        </rdfs:subClassOf>
        <rdfs:subClassOf>
            <owl:Restriction>
                <owl:onProperty rdf:resource="https://w3id.org/netbeheer/referentiemodellen/IECCIM/TC57CIM/IEC61970/Dynamics/StandardModels/WindDynamics#WindContPType3IEC_wdtd"/>
                <owl:minQualifiedCardinality rdf:datatype="http://www.w3.org/2001/XMLSchema#nonNegativeInteger">0</owl:minQualifiedCardinality>
                <owl:onClass rdf:resource="https://w3id.org/netbeheer/referentiemodellen/IECCIM/TC57CIM/IEC61970/Base/Domain#PU"/>
            </owl:Restriction>
        </rdfs:subClassOf>
        <rdfs:subClassOf>
            <owl:Restriction>
                <owl:onProperty rdf:resource="https://w3id.org/netbeheer/referentiemodellen/IECCIM/TC57CIM/IEC61970/Dynamics/StandardModels/WindDynamics#WindContPType3IEC_WindGenTurbineType3IEC"/>
                <owl:qualifiedCardinality rdf:datatype="http://www.w3.org/2001/XMLSchema#nonNegativeInteger">1</owl:qualifiedCardinality>
                <owl:onClass rdf:resource="https://w3id.org/netbeheer/referentiemodellen/IECCIM/TC57CIM/IEC61970/Dynamics/StandardModels/WindDynamics#WindContPType3IEC"/>
            </owl:Restriction>
        </rdfs:subClassOf>
        <rdfs:subClassOf>
            <owl:Restriction>
                <owl:onProperty rdf:resource="https://w3id.org/netbeheer/referentiemodellen/IECCIM/TC57CIM/IEC61970/Dynamics/StandardModels/WindDynamics#WindContPType3IEC_WindDynamicsLookupTable"/>
                <owl:maxQualifiedCardinality rdf:datatype="http://www.w3.org/2001/XMLSchema#nonNegativeInteger">1</owl:maxQualifiedCardinality>
                <owl:onClass rdf:resource="https://w3id.org/netbeheer/referentiemodellen/IECCIM/TC57CIM/IEC61970/Dynamics/StandardModels/WindDynamics#WindContPType3IEC"/>
            </owl:Restriction>
        </rdfs:subClassOf>
        <rdfs:subClassOf>
            <owl:Restriction>
                <owl:onProperty rdf:resource="https://w3id.org/netbeheer/referentiemodellen/IECCIM/TC57CIM/IEC61970/Dynamics/StandardModels/WindDynamics#WindContPType3IEC_dpmax"/>
                <owl:maxQualifiedCardinality rdf:datatype="http://www.w3.org/2001/XMLSchema#nonNegativeInteger">1</owl:maxQualifiedCardinality>
                <owl:onClass rdf:resource="https://w3id.org/netbeheer/referentiemodellen/IECCIM/TC57CIM/IEC61970/Base/Domain#PU"/>
            </owl:Restriction>
        </rdfs:subClassOf>
        <rdfs:subClassOf>
            <owl:Restriction>
                <owl:onProperty rdf:resource="https://w3id.org/netbeheer/referentiemodellen/IECCIM/TC57CIM/IEC61970/Dynamics/StandardModels/WindDynamics#WindContPType3IEC_dtrisemaxlvrt"/>
                <owl:maxQualifiedCardinality rdf:datatype="http://www.w3.org/2001/XMLSchema#nonNegativeInteger">1</owl:maxQualifiedCardinality>
                <owl:onClass rdf:resource="https://w3id.org/netbeheer/referentiemodellen/IECCIM/TC57CIM/IEC61970/Base/Domain#PU"/>
            </owl:Restriction>
        </rdfs:subClassOf>
        <rdfs:subClassOf>
            <owl:Restriction>
                <owl:onProperty rdf:resource="https://w3id.org/netbeheer/referentiemodellen/IECCIM/TC57CIM/IEC61970/Dynamics/StandardModels/WindDynamics#WindContPType3IEC_kdtd"/>
                <owl:maxQualifiedCardinality rdf:datatype="http://www.w3.org/2001/XMLSchema#nonNegativeInteger">1</owl:maxQualifiedCardinality>
                <owl:onClass rdf:resource="https://w3id.org/netbeheer/referentiemodellen/IECCIM/TC57CIM/IEC61970/Base/Domain#PU"/>
            </owl:Restriction>
        </rdfs:subClassOf>
        <rdfs:subClassOf>
            <owl:Restriction>
                <owl:onProperty rdf:resource="https://w3id.org/netbeheer/referentiemodellen/IECCIM/TC57CIM/IEC61970/Dynamics/StandardModels/WindDynamics#WindContPType3IEC_kip"/>
                <owl:maxQualifiedCardinality rdf:datatype="http://www.w3.org/2001/XMLSchema#nonNegativeInteger">1</owl:maxQualifiedCardinality>
                <owl:onClass rdf:resource="https://w3id.org/netbeheer/referentiemodellen/IECCIM/TC57CIM/IEC61970/Base/Domain#PU"/>
            </owl:Restriction>
        </rdfs:subClassOf>
        <rdfs:subClassOf>
            <owl:Restriction>
                <owl:onProperty rdf:resource="https://w3id.org/netbeheer/referentiemodellen/IECCIM/TC57CIM/IEC61970/Dynamics/StandardModels/WindDynamics#WindContPType3IEC_kpp"/>
                <owl:maxQualifiedCardinality rdf:datatype="http://www.w3.org/2001/XMLSchema#nonNegativeInteger">1</owl:maxQualifiedCardinality>
                <owl:onClass rdf:resource="https://w3id.org/netbeheer/referentiemodellen/IECCIM/TC57CIM/IEC61970/Base/Domain#PU"/>
            </owl:Restriction>
        </rdfs:subClassOf>
        <rdfs:subClassOf>
            <owl:Restriction>
                <owl:onProperty rdf:resource="https://w3id.org/netbeheer/referentiemodellen/IECCIM/TC57CIM/IEC61970/Dynamics/StandardModels/WindDynamics#WindContPType3IEC_omegaoffset"/>
                <owl:maxQualifiedCardinality rdf:datatype="http://www.w3.org/2001/XMLSchema#nonNegativeInteger">1</owl:maxQualifiedCardinality>
                <owl:onClass rdf:resource="https://w3id.org/netbeheer/referentiemodellen/IECCIM/TC57CIM/IEC61970/Base/Domain#PU"/>
            </owl:Restriction>
        </rdfs:subClassOf>
        <rdfs:subClassOf>
            <owl:Restriction>
                <owl:onProperty rdf:resource="https://w3id.org/netbeheer/referentiemodellen/IECCIM/TC57CIM/IEC61970/Dynamics/StandardModels/WindDynamics#WindContPType3IEC_pdtdmax"/>
                <owl:maxQualifiedCardinality rdf:datatype="http://www.w3.org/2001/XMLSchema#nonNegativeInteger">1</owl:maxQualifiedCardinality>
                <owl:onClass rdf:resource="https://w3id.org/netbeheer/referentiemodellen/IECCIM/TC57CIM/IEC61970/Base/Domain#PU"/>
            </owl:Restriction>
        </rdfs:subClassOf>
        <rdfs:subClassOf>
            <owl:Restriction>
                <owl:onProperty rdf:resource="https://w3id.org/netbeheer/referentiemodellen/IECCIM/TC57CIM/IEC61970/Dynamics/StandardModels/WindDynamics#WindContPType3IEC_rramp"/>
                <owl:maxQualifiedCardinality rdf:datatype="http://www.w3.org/2001/XMLSchema#nonNegativeInteger">1</owl:maxQualifiedCardinality>
                <owl:onClass rdf:resource="https://w3id.org/netbeheer/referentiemodellen/IECCIM/TC57CIM/IEC61970/Base/Domain#PU"/>
            </owl:Restriction>
        </rdfs:subClassOf>
        <rdfs:subClassOf>
            <owl:Restriction>
                <owl:onProperty rdf:resource="https://w3id.org/netbeheer/referentiemodellen/IECCIM/TC57CIM/IEC61970/Dynamics/StandardModels/WindDynamics#WindContPType3IEC_tdvs"/>
                <owl:maxQualifiedCardinality rdf:datatype="http://www.w3.org/2001/XMLSchema#nonNegativeInteger">1</owl:maxQualifiedCardinality>
                <owl:onClass rdf:resource="https://w3id.org/netbeheer/referentiemodellen/IECCIM/TC57CIM/IEC61970/Base/Domain#Seconds"/>
            </owl:Restriction>
        </rdfs:subClassOf>
        <rdfs:subClassOf>
            <owl:Restriction>
                <owl:onProperty rdf:resource="https://w3id.org/netbeheer/referentiemodellen/IECCIM/TC57CIM/IEC61970/Dynamics/StandardModels/WindDynamics#WindContPType3IEC_temin"/>
                <owl:maxQualifiedCardinality rdf:datatype="http://www.w3.org/2001/XMLSchema#nonNegativeInteger">1</owl:maxQualifiedCardinality>
                <owl:onClass rdf:resource="https://w3id.org/netbeheer/referentiemodellen/IECCIM/TC57CIM/IEC61970/Base/Domain#PU"/>
            </owl:Restriction>
        </rdfs:subClassOf>
        <rdfs:subClassOf>
            <owl:Restriction>
                <owl:onProperty rdf:resource="https://w3id.org/netbeheer/referentiemodellen/IECCIM/TC57CIM/IEC61970/Dynamics/StandardModels/WindDynamics#WindContPType3IEC_tomegafilt"/>
                <owl:maxQualifiedCardinality rdf:datatype="http://www.w3.org/2001/XMLSchema#nonNegativeInteger">1</owl:maxQualifiedCardinality>
                <owl:onClass rdf:resource="https://w3id.org/netbeheer/referentiemodellen/IECCIM/TC57CIM/IEC61970/Base/Domain#Seconds"/>
            </owl:Restriction>
        </rdfs:subClassOf>
        <rdfs:subClassOf>
            <owl:Restriction>
                <owl:onProperty rdf:resource="https://w3id.org/netbeheer/referentiemodellen/IECCIM/TC57CIM/IEC61970/Dynamics/StandardModels/WindDynamics#WindContPType3IEC_tpfilt"/>
                <owl:maxQualifiedCardinality rdf:datatype="http://www.w3.org/2001/XMLSchema#nonNegativeInteger">1</owl:maxQualifiedCardinality>
                <owl:onClass rdf:resource="https://w3id.org/netbeheer/referentiemodellen/IECCIM/TC57CIM/IEC61970/Base/Domain#Seconds"/>
            </owl:Restriction>
        </rdfs:subClassOf>
        <rdfs:subClassOf>
            <owl:Restriction>
                <owl:onProperty rdf:resource="https://w3id.org/netbeheer/referentiemodellen/IECCIM/TC57CIM/IEC61970/Dynamics/StandardModels/WindDynamics#WindContPType3IEC_tpord"/>
                <owl:maxQualifiedCardinality rdf:datatype="http://www.w3.org/2001/XMLSchema#nonNegativeInteger">1</owl:maxQualifiedCardinality>
                <owl:onClass rdf:resource="https://w3id.org/netbeheer/referentiemodellen/IECCIM/TC57CIM/IEC61970/Base/Domain#PU"/>
            </owl:Restriction>
        </rdfs:subClassOf>
        <rdfs:subClassOf>
            <owl:Restriction>
                <owl:onProperty rdf:resource="https://w3id.org/netbeheer/referentiemodellen/IECCIM/TC57CIM/IEC61970/Dynamics/StandardModels/WindDynamics#WindContPType3IEC_tufilt"/>
                <owl:maxQualifiedCardinality rdf:datatype="http://www.w3.org/2001/XMLSchema#nonNegativeInteger">1</owl:maxQualifiedCardinality>
                <owl:onClass rdf:resource="https://w3id.org/netbeheer/referentiemodellen/IECCIM/TC57CIM/IEC61970/Base/Domain#Seconds"/>
            </owl:Restriction>
        </rdfs:subClassOf>
        <rdfs:subClassOf>
            <owl:Restriction>
                <owl:onProperty rdf:resource="https://w3id.org/netbeheer/referentiemodellen/IECCIM/TC57CIM/IEC61970/Dynamics/StandardModels/WindDynamics#WindContPType3IEC_tuscale"/>
                <owl:maxQualifiedCardinality rdf:datatype="http://www.w3.org/2001/XMLSchema#nonNegativeInteger">1</owl:maxQualifiedCardinality>
                <owl:onClass rdf:resource="https://w3id.org/netbeheer/referentiemodellen/IECCIM/TC57CIM/IEC61970/Base/Domain#PU"/>
            </owl:Restriction>
        </rdfs:subClassOf>
        <rdfs:subClassOf>
            <owl:Restriction>
                <owl:onProperty rdf:resource="https://w3id.org/netbeheer/referentiemodellen/IECCIM/TC57CIM/IEC61970/Dynamics/StandardModels/WindDynamics#WindContPType3IEC_twref"/>
                <owl:maxQualifiedCardinality rdf:datatype="http://www.w3.org/2001/XMLSchema#nonNegativeInteger">1</owl:maxQualifiedCardinality>
                <owl:onClass rdf:resource="https://w3id.org/netbeheer/referentiemodellen/IECCIM/TC57CIM/IEC61970/Base/Domain#Seconds"/>
            </owl:Restriction>
        </rdfs:subClassOf>
        <rdfs:subClassOf>
            <owl:Restriction>
                <owl:onProperty rdf:resource="https://w3id.org/netbeheer/referentiemodellen/IECCIM/TC57CIM/IEC61970/Dynamics/StandardModels/WindDynamics#WindContPType3IEC_udvs"/>
                <owl:maxQualifiedCardinality rdf:datatype="http://www.w3.org/2001/XMLSchema#nonNegativeInteger">1</owl:maxQualifiedCardinality>
                <owl:onClass rdf:resource="https://w3id.org/netbeheer/referentiemodellen/IECCIM/TC57CIM/IEC61970/Base/Domain#PU"/>
            </owl:Restriction>
        </rdfs:subClassOf>
        <rdfs:subClassOf>
            <owl:Restriction>
                <owl:onProperty rdf:resource="https://w3id.org/netbeheer/referentiemodellen/IECCIM/TC57CIM/IEC61970/Dynamics/StandardModels/WindDynamics#WindContPType3IEC_updip"/>
                <owl:maxQualifiedCardinality rdf:datatype="http://www.w3.org/2001/XMLSchema#nonNegativeInteger">1</owl:maxQualifiedCardinality>
                <owl:onClass rdf:resource="https://w3id.org/netbeheer/referentiemodellen/IECCIM/TC57CIM/IEC61970/Base/Domain#PU"/>
            </owl:Restriction>
        </rdfs:subClassOf>
        <rdfs:subClassOf>
            <owl:Restriction>
                <owl:onProperty rdf:resource="https://w3id.org/netbeheer/referentiemodellen/IECCIM/TC57CIM/IEC61970/Dynamics/StandardModels/WindDynamics#WindContPType3IEC_wdtd"/>
                <owl:maxQualifiedCardinality rdf:datatype="http://www.w3.org/2001/XMLSchema#nonNegativeInteger">1</owl:maxQualifiedCardinality>
                <owl:onClass rdf:resource="https://w3id.org/netbeheer/referentiemodellen/IECCIM/TC57CIM/IEC61970/Base/Domain#PU"/>
            </owl:Restriction>
        </rdfs:subClassOf>
        <rdfs:subClassOf>
            <owl:Restriction>
                <owl:onProperty rdf:resource="https://w3id.org/netbeheer/referentiemodellen/IECCIM/TC57CIM/IEC61970/Dynamics/StandardModels/WindDynamics#WindContPType3IEC_mplvrt"/>
                <owl:minQualifiedCardinality rdf:datatype="http://www.w3.org/2001/XMLSchema#nonNegativeInteger">0</owl:minQualifiedCardinality>
                <owl:onDataRange rdf:resource="http://www.w3.org/2001/XMLSchema#boolean"/>
            </owl:Restriction>
        </rdfs:subClassOf>
        <rdfs:subClassOf>
            <owl:Restriction>
                <owl:onProperty rdf:resource="https://w3id.org/netbeheer/referentiemodellen/IECCIM/TC57CIM/IEC61970/Dynamics/StandardModels/WindDynamics#WindContPType3IEC_zeta"/>
                <owl:minQualifiedCardinality rdf:datatype="http://www.w3.org/2001/XMLSchema#nonNegativeInteger">0</owl:minQualifiedCardinality>
                <owl:onDataRange rdf:resource="http://www.w3.org/2001/XMLSchema#float"/>
            </owl:Restriction>
        </rdfs:subClassOf>
        <rdfs:subClassOf>
            <owl:Restriction>
                <owl:onProperty rdf:resource="https://w3id.org/netbeheer/referentiemodellen/IECCIM/TC57CIM/IEC61970/Dynamics/StandardModels/WindDynamics#WindContPType3IEC_mplvrt"/>
                <owl:maxQualifiedCardinality rdf:datatype="http://www.w3.org/2001/XMLSchema#nonNegativeInteger">1</owl:maxQualifiedCardinality>
                <owl:onDataRange rdf:resource="http://www.w3.org/2001/XMLSchema#boolean"/>
            </owl:Restriction>
        </rdfs:subClassOf>
        <rdfs:subClassOf>
            <owl:Restriction>
                <owl:onProperty rdf:resource="https://w3id.org/netbeheer/referentiemodellen/IECCIM/TC57CIM/IEC61970/Dynamics/StandardModels/WindDynamics#WindContPType3IEC_zeta"/>
                <owl:maxQualifiedCardinality rdf:datatype="http://www.w3.org/2001/XMLSchema#nonNegativeInteger">1</owl:maxQualifiedCardinality>
                <owl:onDataRange rdf:resource="http://www.w3.org/2001/XMLSchema#float"/>
            </owl:Restriction>
        </rdfs:subClassOf>
        <rdfs:comment>P control model Type 3.

Reference: IEC Standard 61400-27-1 Section 6.6.5.3.</rdfs:comment>
    </owl:Class>
    


    <!-- https://w3id.org/netbeheer/referentiemodellen/IECCIM/TC57CIM/IEC61970/Dynamics/StandardModels/WindDynamics#WindContPType4aIEC -->


    <owl:Class rdf:about="https://w3id.org/netbeheer/referentiemodellen/IECCIM/TC57CIM/IEC61970/Dynamics/StandardModels/WindDynamics#WindContPType4aIEC">
        <rdfs:subClassOf rdf:resource="https://w3id.org/netbeheer/referentiemodellen/IECCIM/TC57CIM/IEC61970/Base/Core#IdentifiedObject"/>
        <rdfs:subClassOf>
            <owl:Restriction>
                <owl:onProperty rdf:resource="https://w3id.org/netbeheer/referentiemodellen/IECCIM/TC57CIM/IEC61970/Dynamics/StandardModels/WindDynamics#WindContPType4aIEC_dpmax"/>
                <owl:minQualifiedCardinality rdf:datatype="http://www.w3.org/2001/XMLSchema#nonNegativeInteger">0</owl:minQualifiedCardinality>
                <owl:onClass rdf:resource="https://w3id.org/netbeheer/referentiemodellen/IECCIM/TC57CIM/IEC61970/Base/Domain#PU"/>
            </owl:Restriction>
        </rdfs:subClassOf>
        <rdfs:subClassOf>
            <owl:Restriction>
                <owl:onProperty rdf:resource="https://w3id.org/netbeheer/referentiemodellen/IECCIM/TC57CIM/IEC61970/Dynamics/StandardModels/WindDynamics#WindContPType4aIEC_tpord"/>
                <owl:minQualifiedCardinality rdf:datatype="http://www.w3.org/2001/XMLSchema#nonNegativeInteger">0</owl:minQualifiedCardinality>
                <owl:onClass rdf:resource="https://w3id.org/netbeheer/referentiemodellen/IECCIM/TC57CIM/IEC61970/Base/Domain#Seconds"/>
            </owl:Restriction>
        </rdfs:subClassOf>
        <rdfs:subClassOf>
            <owl:Restriction>
                <owl:onProperty rdf:resource="https://w3id.org/netbeheer/referentiemodellen/IECCIM/TC57CIM/IEC61970/Dynamics/StandardModels/WindDynamics#WindContPType4aIEC_tufilt"/>
                <owl:minQualifiedCardinality rdf:datatype="http://www.w3.org/2001/XMLSchema#nonNegativeInteger">0</owl:minQualifiedCardinality>
                <owl:onClass rdf:resource="https://w3id.org/netbeheer/referentiemodellen/IECCIM/TC57CIM/IEC61970/Base/Domain#Seconds"/>
            </owl:Restriction>
        </rdfs:subClassOf>
        <rdfs:subClassOf>
            <owl:Restriction>
                <owl:onProperty rdf:resource="https://w3id.org/netbeheer/referentiemodellen/IECCIM/TC57CIM/IEC61970/Dynamics/StandardModels/WindDynamics#WindContPType4aIEC_WindTurbineType4aIEC"/>
                <owl:qualifiedCardinality rdf:datatype="http://www.w3.org/2001/XMLSchema#nonNegativeInteger">1</owl:qualifiedCardinality>
                <owl:onClass rdf:resource="https://w3id.org/netbeheer/referentiemodellen/IECCIM/TC57CIM/IEC61970/Dynamics/StandardModels/WindDynamics#WindContPType4aIEC"/>
            </owl:Restriction>
        </rdfs:subClassOf>
        <rdfs:subClassOf>
            <owl:Restriction>
                <owl:onProperty rdf:resource="https://w3id.org/netbeheer/referentiemodellen/IECCIM/TC57CIM/IEC61970/Dynamics/StandardModels/WindDynamics#WindContPType4aIEC_dpmax"/>
                <owl:maxQualifiedCardinality rdf:datatype="http://www.w3.org/2001/XMLSchema#nonNegativeInteger">1</owl:maxQualifiedCardinality>
                <owl:onClass rdf:resource="https://w3id.org/netbeheer/referentiemodellen/IECCIM/TC57CIM/IEC61970/Base/Domain#PU"/>
            </owl:Restriction>
        </rdfs:subClassOf>
        <rdfs:subClassOf>
            <owl:Restriction>
                <owl:onProperty rdf:resource="https://w3id.org/netbeheer/referentiemodellen/IECCIM/TC57CIM/IEC61970/Dynamics/StandardModels/WindDynamics#WindContPType4aIEC_tpord"/>
                <owl:maxQualifiedCardinality rdf:datatype="http://www.w3.org/2001/XMLSchema#nonNegativeInteger">1</owl:maxQualifiedCardinality>
                <owl:onClass rdf:resource="https://w3id.org/netbeheer/referentiemodellen/IECCIM/TC57CIM/IEC61970/Base/Domain#Seconds"/>
            </owl:Restriction>
        </rdfs:subClassOf>
        <rdfs:subClassOf>
            <owl:Restriction>
                <owl:onProperty rdf:resource="https://w3id.org/netbeheer/referentiemodellen/IECCIM/TC57CIM/IEC61970/Dynamics/StandardModels/WindDynamics#WindContPType4aIEC_tufilt"/>
                <owl:maxQualifiedCardinality rdf:datatype="http://www.w3.org/2001/XMLSchema#nonNegativeInteger">1</owl:maxQualifiedCardinality>
                <owl:onClass rdf:resource="https://w3id.org/netbeheer/referentiemodellen/IECCIM/TC57CIM/IEC61970/Base/Domain#Seconds"/>
            </owl:Restriction>
        </rdfs:subClassOf>
        <rdfs:comment>P control model Type 4A.

Reference: IEC Standard 61400-27-1 Section 6.6.5.4.</rdfs:comment>
    </owl:Class>
    


    <!-- https://w3id.org/netbeheer/referentiemodellen/IECCIM/TC57CIM/IEC61970/Dynamics/StandardModels/WindDynamics#WindContPType4bIEC -->


    <owl:Class rdf:about="https://w3id.org/netbeheer/referentiemodellen/IECCIM/TC57CIM/IEC61970/Dynamics/StandardModels/WindDynamics#WindContPType4bIEC">
        <rdfs:subClassOf rdf:resource="https://w3id.org/netbeheer/referentiemodellen/IECCIM/TC57CIM/IEC61970/Base/Core#IdentifiedObject"/>
        <rdfs:subClassOf>
            <owl:Restriction>
                <owl:onProperty rdf:resource="https://w3id.org/netbeheer/referentiemodellen/IECCIM/TC57CIM/IEC61970/Dynamics/StandardModels/WindDynamics#WindContPType4bIEC_dpmax"/>
                <owl:minQualifiedCardinality rdf:datatype="http://www.w3.org/2001/XMLSchema#nonNegativeInteger">0</owl:minQualifiedCardinality>
                <owl:onClass rdf:resource="https://w3id.org/netbeheer/referentiemodellen/IECCIM/TC57CIM/IEC61970/Base/Domain#PU"/>
            </owl:Restriction>
        </rdfs:subClassOf>
        <rdfs:subClassOf>
            <owl:Restriction>
                <owl:onProperty rdf:resource="https://w3id.org/netbeheer/referentiemodellen/IECCIM/TC57CIM/IEC61970/Dynamics/StandardModels/WindDynamics#WindContPType4bIEC_tpaero"/>
                <owl:minQualifiedCardinality rdf:datatype="http://www.w3.org/2001/XMLSchema#nonNegativeInteger">0</owl:minQualifiedCardinality>
                <owl:onClass rdf:resource="https://w3id.org/netbeheer/referentiemodellen/IECCIM/TC57CIM/IEC61970/Base/Domain#Seconds"/>
            </owl:Restriction>
        </rdfs:subClassOf>
        <rdfs:subClassOf>
            <owl:Restriction>
                <owl:onProperty rdf:resource="https://w3id.org/netbeheer/referentiemodellen/IECCIM/TC57CIM/IEC61970/Dynamics/StandardModels/WindDynamics#WindContPType4bIEC_tpord"/>
                <owl:minQualifiedCardinality rdf:datatype="http://www.w3.org/2001/XMLSchema#nonNegativeInteger">0</owl:minQualifiedCardinality>
                <owl:onClass rdf:resource="https://w3id.org/netbeheer/referentiemodellen/IECCIM/TC57CIM/IEC61970/Base/Domain#Seconds"/>
            </owl:Restriction>
        </rdfs:subClassOf>
        <rdfs:subClassOf>
            <owl:Restriction>
                <owl:onProperty rdf:resource="https://w3id.org/netbeheer/referentiemodellen/IECCIM/TC57CIM/IEC61970/Dynamics/StandardModels/WindDynamics#WindContPType4bIEC_tufilt"/>
                <owl:minQualifiedCardinality rdf:datatype="http://www.w3.org/2001/XMLSchema#nonNegativeInteger">0</owl:minQualifiedCardinality>
                <owl:onClass rdf:resource="https://w3id.org/netbeheer/referentiemodellen/IECCIM/TC57CIM/IEC61970/Base/Domain#Seconds"/>
            </owl:Restriction>
        </rdfs:subClassOf>
        <rdfs:subClassOf>
            <owl:Restriction>
                <owl:onProperty rdf:resource="https://w3id.org/netbeheer/referentiemodellen/IECCIM/TC57CIM/IEC61970/Dynamics/StandardModels/WindDynamics#WindContPType4bIEC_WindTurbineType4bIEC"/>
                <owl:qualifiedCardinality rdf:datatype="http://www.w3.org/2001/XMLSchema#nonNegativeInteger">1</owl:qualifiedCardinality>
                <owl:onClass rdf:resource="https://w3id.org/netbeheer/referentiemodellen/IECCIM/TC57CIM/IEC61970/Dynamics/StandardModels/WindDynamics#WindContPType4bIEC"/>
            </owl:Restriction>
        </rdfs:subClassOf>
        <rdfs:subClassOf>
            <owl:Restriction>
                <owl:onProperty rdf:resource="https://w3id.org/netbeheer/referentiemodellen/IECCIM/TC57CIM/IEC61970/Dynamics/StandardModels/WindDynamics#WindContPType4bIEC_dpmax"/>
                <owl:maxQualifiedCardinality rdf:datatype="http://www.w3.org/2001/XMLSchema#nonNegativeInteger">1</owl:maxQualifiedCardinality>
                <owl:onClass rdf:resource="https://w3id.org/netbeheer/referentiemodellen/IECCIM/TC57CIM/IEC61970/Base/Domain#PU"/>
            </owl:Restriction>
        </rdfs:subClassOf>
        <rdfs:subClassOf>
            <owl:Restriction>
                <owl:onProperty rdf:resource="https://w3id.org/netbeheer/referentiemodellen/IECCIM/TC57CIM/IEC61970/Dynamics/StandardModels/WindDynamics#WindContPType4bIEC_tpaero"/>
                <owl:maxQualifiedCardinality rdf:datatype="http://www.w3.org/2001/XMLSchema#nonNegativeInteger">1</owl:maxQualifiedCardinality>
                <owl:onClass rdf:resource="https://w3id.org/netbeheer/referentiemodellen/IECCIM/TC57CIM/IEC61970/Base/Domain#Seconds"/>
            </owl:Restriction>
        </rdfs:subClassOf>
        <rdfs:subClassOf>
            <owl:Restriction>
                <owl:onProperty rdf:resource="https://w3id.org/netbeheer/referentiemodellen/IECCIM/TC57CIM/IEC61970/Dynamics/StandardModels/WindDynamics#WindContPType4bIEC_tpord"/>
                <owl:maxQualifiedCardinality rdf:datatype="http://www.w3.org/2001/XMLSchema#nonNegativeInteger">1</owl:maxQualifiedCardinality>
                <owl:onClass rdf:resource="https://w3id.org/netbeheer/referentiemodellen/IECCIM/TC57CIM/IEC61970/Base/Domain#Seconds"/>
            </owl:Restriction>
        </rdfs:subClassOf>
        <rdfs:subClassOf>
            <owl:Restriction>
                <owl:onProperty rdf:resource="https://w3id.org/netbeheer/referentiemodellen/IECCIM/TC57CIM/IEC61970/Dynamics/StandardModels/WindDynamics#WindContPType4bIEC_tufilt"/>
                <owl:maxQualifiedCardinality rdf:datatype="http://www.w3.org/2001/XMLSchema#nonNegativeInteger">1</owl:maxQualifiedCardinality>
                <owl:onClass rdf:resource="https://w3id.org/netbeheer/referentiemodellen/IECCIM/TC57CIM/IEC61970/Base/Domain#Seconds"/>
            </owl:Restriction>
        </rdfs:subClassOf>
        <rdfs:comment>P control model Type 4B.

Reference: IEC Standard 61400-27-1 Section 6.6.5.5.</rdfs:comment>
    </owl:Class>
    


    <!-- https://w3id.org/netbeheer/referentiemodellen/IECCIM/TC57CIM/IEC61970/Dynamics/StandardModels/WindDynamics#WindContPitchAngleIEC -->


    <owl:Class rdf:about="https://w3id.org/netbeheer/referentiemodellen/IECCIM/TC57CIM/IEC61970/Dynamics/StandardModels/WindDynamics#WindContPitchAngleIEC">
        <rdfs:subClassOf rdf:resource="https://w3id.org/netbeheer/referentiemodellen/IECCIM/TC57CIM/IEC61970/Base/Core#IdentifiedObject"/>
        <rdfs:subClassOf>
            <owl:Restriction>
                <owl:onProperty rdf:resource="https://w3id.org/netbeheer/referentiemodellen/IECCIM/TC57CIM/IEC61970/Dynamics/StandardModels/WindDynamics#WindContPitchAngleIEC_kic"/>
                <owl:minQualifiedCardinality rdf:datatype="http://www.w3.org/2001/XMLSchema#nonNegativeInteger">0</owl:minQualifiedCardinality>
                <owl:onClass rdf:resource="https://w3id.org/netbeheer/referentiemodellen/IECCIM/TC57CIM/IEC61970/Base/Domain#PU"/>
            </owl:Restriction>
        </rdfs:subClassOf>
        <rdfs:subClassOf>
            <owl:Restriction>
                <owl:onProperty rdf:resource="https://w3id.org/netbeheer/referentiemodellen/IECCIM/TC57CIM/IEC61970/Dynamics/StandardModels/WindDynamics#WindContPitchAngleIEC_kiomega"/>
                <owl:minQualifiedCardinality rdf:datatype="http://www.w3.org/2001/XMLSchema#nonNegativeInteger">0</owl:minQualifiedCardinality>
                <owl:onClass rdf:resource="https://w3id.org/netbeheer/referentiemodellen/IECCIM/TC57CIM/IEC61970/Base/Domain#PU"/>
            </owl:Restriction>
        </rdfs:subClassOf>
        <rdfs:subClassOf>
            <owl:Restriction>
                <owl:onProperty rdf:resource="https://w3id.org/netbeheer/referentiemodellen/IECCIM/TC57CIM/IEC61970/Dynamics/StandardModels/WindDynamics#WindContPitchAngleIEC_kpc"/>
                <owl:minQualifiedCardinality rdf:datatype="http://www.w3.org/2001/XMLSchema#nonNegativeInteger">0</owl:minQualifiedCardinality>
                <owl:onClass rdf:resource="https://w3id.org/netbeheer/referentiemodellen/IECCIM/TC57CIM/IEC61970/Base/Domain#PU"/>
            </owl:Restriction>
        </rdfs:subClassOf>
        <rdfs:subClassOf>
            <owl:Restriction>
                <owl:onProperty rdf:resource="https://w3id.org/netbeheer/referentiemodellen/IECCIM/TC57CIM/IEC61970/Dynamics/StandardModels/WindDynamics#WindContPitchAngleIEC_kpomega"/>
                <owl:minQualifiedCardinality rdf:datatype="http://www.w3.org/2001/XMLSchema#nonNegativeInteger">0</owl:minQualifiedCardinality>
                <owl:onClass rdf:resource="https://w3id.org/netbeheer/referentiemodellen/IECCIM/TC57CIM/IEC61970/Base/Domain#PU"/>
            </owl:Restriction>
        </rdfs:subClassOf>
        <rdfs:subClassOf>
            <owl:Restriction>
                <owl:onProperty rdf:resource="https://w3id.org/netbeheer/referentiemodellen/IECCIM/TC57CIM/IEC61970/Dynamics/StandardModels/WindDynamics#WindContPitchAngleIEC_kpx"/>
                <owl:minQualifiedCardinality rdf:datatype="http://www.w3.org/2001/XMLSchema#nonNegativeInteger">0</owl:minQualifiedCardinality>
                <owl:onClass rdf:resource="https://w3id.org/netbeheer/referentiemodellen/IECCIM/TC57CIM/IEC61970/Base/Domain#PU"/>
            </owl:Restriction>
        </rdfs:subClassOf>
        <rdfs:subClassOf>
            <owl:Restriction>
                <owl:onProperty rdf:resource="https://w3id.org/netbeheer/referentiemodellen/IECCIM/TC57CIM/IEC61970/Dynamics/StandardModels/WindDynamics#WindContPitchAngleIEC_thetamax"/>
                <owl:minQualifiedCardinality rdf:datatype="http://www.w3.org/2001/XMLSchema#nonNegativeInteger">0</owl:minQualifiedCardinality>
                <owl:onClass rdf:resource="https://w3id.org/netbeheer/referentiemodellen/IECCIM/TC57CIM/IEC61970/Base/Domain#AngleDegrees"/>
            </owl:Restriction>
        </rdfs:subClassOf>
        <rdfs:subClassOf>
            <owl:Restriction>
                <owl:onProperty rdf:resource="https://w3id.org/netbeheer/referentiemodellen/IECCIM/TC57CIM/IEC61970/Dynamics/StandardModels/WindDynamics#WindContPitchAngleIEC_thetamin"/>
                <owl:minQualifiedCardinality rdf:datatype="http://www.w3.org/2001/XMLSchema#nonNegativeInteger">0</owl:minQualifiedCardinality>
                <owl:onClass rdf:resource="https://w3id.org/netbeheer/referentiemodellen/IECCIM/TC57CIM/IEC61970/Base/Domain#AngleDegrees"/>
            </owl:Restriction>
        </rdfs:subClassOf>
        <rdfs:subClassOf>
            <owl:Restriction>
                <owl:onProperty rdf:resource="https://w3id.org/netbeheer/referentiemodellen/IECCIM/TC57CIM/IEC61970/Dynamics/StandardModels/WindDynamics#WindContPitchAngleIEC_ttheta"/>
                <owl:minQualifiedCardinality rdf:datatype="http://www.w3.org/2001/XMLSchema#nonNegativeInteger">0</owl:minQualifiedCardinality>
                <owl:onClass rdf:resource="https://w3id.org/netbeheer/referentiemodellen/IECCIM/TC57CIM/IEC61970/Base/Domain#Seconds"/>
            </owl:Restriction>
        </rdfs:subClassOf>
        <rdfs:subClassOf>
            <owl:Restriction>
                <owl:onProperty rdf:resource="https://w3id.org/netbeheer/referentiemodellen/IECCIM/TC57CIM/IEC61970/Dynamics/StandardModels/WindDynamics#WindContPitchAngleIEC_WindGenTurbineType3IEC"/>
                <owl:qualifiedCardinality rdf:datatype="http://www.w3.org/2001/XMLSchema#nonNegativeInteger">1</owl:qualifiedCardinality>
                <owl:onClass rdf:resource="https://w3id.org/netbeheer/referentiemodellen/IECCIM/TC57CIM/IEC61970/Dynamics/StandardModels/WindDynamics#WindContPitchAngleIEC"/>
            </owl:Restriction>
        </rdfs:subClassOf>
        <rdfs:subClassOf>
            <owl:Restriction>
                <owl:onProperty rdf:resource="https://w3id.org/netbeheer/referentiemodellen/IECCIM/TC57CIM/IEC61970/Dynamics/StandardModels/WindDynamics#WindContPitchAngleIEC_kic"/>
                <owl:maxQualifiedCardinality rdf:datatype="http://www.w3.org/2001/XMLSchema#nonNegativeInteger">1</owl:maxQualifiedCardinality>
                <owl:onClass rdf:resource="https://w3id.org/netbeheer/referentiemodellen/IECCIM/TC57CIM/IEC61970/Base/Domain#PU"/>
            </owl:Restriction>
        </rdfs:subClassOf>
        <rdfs:subClassOf>
            <owl:Restriction>
                <owl:onProperty rdf:resource="https://w3id.org/netbeheer/referentiemodellen/IECCIM/TC57CIM/IEC61970/Dynamics/StandardModels/WindDynamics#WindContPitchAngleIEC_kiomega"/>
                <owl:maxQualifiedCardinality rdf:datatype="http://www.w3.org/2001/XMLSchema#nonNegativeInteger">1</owl:maxQualifiedCardinality>
                <owl:onClass rdf:resource="https://w3id.org/netbeheer/referentiemodellen/IECCIM/TC57CIM/IEC61970/Base/Domain#PU"/>
            </owl:Restriction>
        </rdfs:subClassOf>
        <rdfs:subClassOf>
            <owl:Restriction>
                <owl:onProperty rdf:resource="https://w3id.org/netbeheer/referentiemodellen/IECCIM/TC57CIM/IEC61970/Dynamics/StandardModels/WindDynamics#WindContPitchAngleIEC_kpc"/>
                <owl:maxQualifiedCardinality rdf:datatype="http://www.w3.org/2001/XMLSchema#nonNegativeInteger">1</owl:maxQualifiedCardinality>
                <owl:onClass rdf:resource="https://w3id.org/netbeheer/referentiemodellen/IECCIM/TC57CIM/IEC61970/Base/Domain#PU"/>
            </owl:Restriction>
        </rdfs:subClassOf>
        <rdfs:subClassOf>
            <owl:Restriction>
                <owl:onProperty rdf:resource="https://w3id.org/netbeheer/referentiemodellen/IECCIM/TC57CIM/IEC61970/Dynamics/StandardModels/WindDynamics#WindContPitchAngleIEC_kpomega"/>
                <owl:maxQualifiedCardinality rdf:datatype="http://www.w3.org/2001/XMLSchema#nonNegativeInteger">1</owl:maxQualifiedCardinality>
                <owl:onClass rdf:resource="https://w3id.org/netbeheer/referentiemodellen/IECCIM/TC57CIM/IEC61970/Base/Domain#PU"/>
            </owl:Restriction>
        </rdfs:subClassOf>
        <rdfs:subClassOf>
            <owl:Restriction>
                <owl:onProperty rdf:resource="https://w3id.org/netbeheer/referentiemodellen/IECCIM/TC57CIM/IEC61970/Dynamics/StandardModels/WindDynamics#WindContPitchAngleIEC_kpx"/>
                <owl:maxQualifiedCardinality rdf:datatype="http://www.w3.org/2001/XMLSchema#nonNegativeInteger">1</owl:maxQualifiedCardinality>
                <owl:onClass rdf:resource="https://w3id.org/netbeheer/referentiemodellen/IECCIM/TC57CIM/IEC61970/Base/Domain#PU"/>
            </owl:Restriction>
        </rdfs:subClassOf>
        <rdfs:subClassOf>
            <owl:Restriction>
                <owl:onProperty rdf:resource="https://w3id.org/netbeheer/referentiemodellen/IECCIM/TC57CIM/IEC61970/Dynamics/StandardModels/WindDynamics#WindContPitchAngleIEC_thetamax"/>
                <owl:maxQualifiedCardinality rdf:datatype="http://www.w3.org/2001/XMLSchema#nonNegativeInteger">1</owl:maxQualifiedCardinality>
                <owl:onClass rdf:resource="https://w3id.org/netbeheer/referentiemodellen/IECCIM/TC57CIM/IEC61970/Base/Domain#AngleDegrees"/>
            </owl:Restriction>
        </rdfs:subClassOf>
        <rdfs:subClassOf>
            <owl:Restriction>
                <owl:onProperty rdf:resource="https://w3id.org/netbeheer/referentiemodellen/IECCIM/TC57CIM/IEC61970/Dynamics/StandardModels/WindDynamics#WindContPitchAngleIEC_thetamin"/>
                <owl:maxQualifiedCardinality rdf:datatype="http://www.w3.org/2001/XMLSchema#nonNegativeInteger">1</owl:maxQualifiedCardinality>
                <owl:onClass rdf:resource="https://w3id.org/netbeheer/referentiemodellen/IECCIM/TC57CIM/IEC61970/Base/Domain#AngleDegrees"/>
            </owl:Restriction>
        </rdfs:subClassOf>
        <rdfs:subClassOf>
            <owl:Restriction>
                <owl:onProperty rdf:resource="https://w3id.org/netbeheer/referentiemodellen/IECCIM/TC57CIM/IEC61970/Dynamics/StandardModels/WindDynamics#WindContPitchAngleIEC_ttheta"/>
                <owl:maxQualifiedCardinality rdf:datatype="http://www.w3.org/2001/XMLSchema#nonNegativeInteger">1</owl:maxQualifiedCardinality>
                <owl:onClass rdf:resource="https://w3id.org/netbeheer/referentiemodellen/IECCIM/TC57CIM/IEC61970/Base/Domain#Seconds"/>
            </owl:Restriction>
        </rdfs:subClassOf>
        <rdfs:subClassOf>
            <owl:Restriction>
                <owl:onProperty rdf:resource="https://w3id.org/netbeheer/referentiemodellen/IECCIM/TC57CIM/IEC61970/Dynamics/StandardModels/WindDynamics#WindContPitchAngleIEC_dthetamax"/>
                <owl:minQualifiedCardinality rdf:datatype="http://www.w3.org/2001/XMLSchema#nonNegativeInteger">0</owl:minQualifiedCardinality>
                <owl:onDataRange rdf:resource="http://www.w3.org/2001/XMLSchema#float"/>
            </owl:Restriction>
        </rdfs:subClassOf>
        <rdfs:subClassOf>
            <owl:Restriction>
                <owl:onProperty rdf:resource="https://w3id.org/netbeheer/referentiemodellen/IECCIM/TC57CIM/IEC61970/Dynamics/StandardModels/WindDynamics#WindContPitchAngleIEC_dthetamin"/>
                <owl:minQualifiedCardinality rdf:datatype="http://www.w3.org/2001/XMLSchema#nonNegativeInteger">0</owl:minQualifiedCardinality>
                <owl:onDataRange rdf:resource="http://www.w3.org/2001/XMLSchema#float"/>
            </owl:Restriction>
        </rdfs:subClassOf>
        <rdfs:subClassOf>
            <owl:Restriction>
                <owl:onProperty rdf:resource="https://w3id.org/netbeheer/referentiemodellen/IECCIM/TC57CIM/IEC61970/Dynamics/StandardModels/WindDynamics#WindContPitchAngleIEC_dthetamax"/>
                <owl:maxQualifiedCardinality rdf:datatype="http://www.w3.org/2001/XMLSchema#nonNegativeInteger">1</owl:maxQualifiedCardinality>
                <owl:onDataRange rdf:resource="http://www.w3.org/2001/XMLSchema#float"/>
            </owl:Restriction>
        </rdfs:subClassOf>
        <rdfs:subClassOf>
            <owl:Restriction>
                <owl:onProperty rdf:resource="https://w3id.org/netbeheer/referentiemodellen/IECCIM/TC57CIM/IEC61970/Dynamics/StandardModels/WindDynamics#WindContPitchAngleIEC_dthetamin"/>
                <owl:maxQualifiedCardinality rdf:datatype="http://www.w3.org/2001/XMLSchema#nonNegativeInteger">1</owl:maxQualifiedCardinality>
                <owl:onDataRange rdf:resource="http://www.w3.org/2001/XMLSchema#float"/>
            </owl:Restriction>
        </rdfs:subClassOf>
        <rdfs:comment>Pitch angle control model.

Reference: IEC Standard 61400-27-1 Section 6.6.5.8.</rdfs:comment>
    </owl:Class>
    


    <!-- https://w3id.org/netbeheer/referentiemodellen/IECCIM/TC57CIM/IEC61970/Dynamics/StandardModels/WindDynamics#WindContQIEC -->


    <owl:Class rdf:about="https://w3id.org/netbeheer/referentiemodellen/IECCIM/TC57CIM/IEC61970/Dynamics/StandardModels/WindDynamics#WindContQIEC">
        <rdfs:subClassOf rdf:resource="https://w3id.org/netbeheer/referentiemodellen/IECCIM/TC57CIM/IEC61970/Base/Core#IdentifiedObject"/>
        <rdfs:subClassOf>
            <owl:Restriction>
                <owl:onProperty rdf:resource="https://w3id.org/netbeheer/referentiemodellen/IECCIM/TC57CIM/IEC61970/Dynamics/StandardModels/WindDynamics#WindContQIEC_iqh1"/>
                <owl:minQualifiedCardinality rdf:datatype="http://www.w3.org/2001/XMLSchema#nonNegativeInteger">0</owl:minQualifiedCardinality>
                <owl:onClass rdf:resource="https://w3id.org/netbeheer/referentiemodellen/IECCIM/TC57CIM/IEC61970/Base/Domain#PU"/>
            </owl:Restriction>
        </rdfs:subClassOf>
        <rdfs:subClassOf>
            <owl:Restriction>
                <owl:onProperty rdf:resource="https://w3id.org/netbeheer/referentiemodellen/IECCIM/TC57CIM/IEC61970/Dynamics/StandardModels/WindDynamics#WindContQIEC_iqmax"/>
                <owl:minQualifiedCardinality rdf:datatype="http://www.w3.org/2001/XMLSchema#nonNegativeInteger">0</owl:minQualifiedCardinality>
                <owl:onClass rdf:resource="https://w3id.org/netbeheer/referentiemodellen/IECCIM/TC57CIM/IEC61970/Base/Domain#PU"/>
            </owl:Restriction>
        </rdfs:subClassOf>
        <rdfs:subClassOf>
            <owl:Restriction>
                <owl:onProperty rdf:resource="https://w3id.org/netbeheer/referentiemodellen/IECCIM/TC57CIM/IEC61970/Dynamics/StandardModels/WindDynamics#WindContQIEC_iqmin"/>
                <owl:minQualifiedCardinality rdf:datatype="http://www.w3.org/2001/XMLSchema#nonNegativeInteger">0</owl:minQualifiedCardinality>
                <owl:onClass rdf:resource="https://w3id.org/netbeheer/referentiemodellen/IECCIM/TC57CIM/IEC61970/Base/Domain#PU"/>
            </owl:Restriction>
        </rdfs:subClassOf>
        <rdfs:subClassOf>
            <owl:Restriction>
                <owl:onProperty rdf:resource="https://w3id.org/netbeheer/referentiemodellen/IECCIM/TC57CIM/IEC61970/Dynamics/StandardModels/WindDynamics#WindContQIEC_iqpost"/>
                <owl:minQualifiedCardinality rdf:datatype="http://www.w3.org/2001/XMLSchema#nonNegativeInteger">0</owl:minQualifiedCardinality>
                <owl:onClass rdf:resource="https://w3id.org/netbeheer/referentiemodellen/IECCIM/TC57CIM/IEC61970/Base/Domain#PU"/>
            </owl:Restriction>
        </rdfs:subClassOf>
        <rdfs:subClassOf>
            <owl:Restriction>
                <owl:onProperty rdf:resource="https://w3id.org/netbeheer/referentiemodellen/IECCIM/TC57CIM/IEC61970/Dynamics/StandardModels/WindDynamics#WindContQIEC_kiq"/>
                <owl:minQualifiedCardinality rdf:datatype="http://www.w3.org/2001/XMLSchema#nonNegativeInteger">0</owl:minQualifiedCardinality>
                <owl:onClass rdf:resource="https://w3id.org/netbeheer/referentiemodellen/IECCIM/TC57CIM/IEC61970/Base/Domain#PU"/>
            </owl:Restriction>
        </rdfs:subClassOf>
        <rdfs:subClassOf>
            <owl:Restriction>
                <owl:onProperty rdf:resource="https://w3id.org/netbeheer/referentiemodellen/IECCIM/TC57CIM/IEC61970/Dynamics/StandardModels/WindDynamics#WindContQIEC_kiu"/>
                <owl:minQualifiedCardinality rdf:datatype="http://www.w3.org/2001/XMLSchema#nonNegativeInteger">0</owl:minQualifiedCardinality>
                <owl:onClass rdf:resource="https://w3id.org/netbeheer/referentiemodellen/IECCIM/TC57CIM/IEC61970/Base/Domain#PU"/>
            </owl:Restriction>
        </rdfs:subClassOf>
        <rdfs:subClassOf>
            <owl:Restriction>
                <owl:onProperty rdf:resource="https://w3id.org/netbeheer/referentiemodellen/IECCIM/TC57CIM/IEC61970/Dynamics/StandardModels/WindDynamics#WindContQIEC_kpq"/>
                <owl:minQualifiedCardinality rdf:datatype="http://www.w3.org/2001/XMLSchema#nonNegativeInteger">0</owl:minQualifiedCardinality>
                <owl:onClass rdf:resource="https://w3id.org/netbeheer/referentiemodellen/IECCIM/TC57CIM/IEC61970/Base/Domain#PU"/>
            </owl:Restriction>
        </rdfs:subClassOf>
        <rdfs:subClassOf>
            <owl:Restriction>
                <owl:onProperty rdf:resource="https://w3id.org/netbeheer/referentiemodellen/IECCIM/TC57CIM/IEC61970/Dynamics/StandardModels/WindDynamics#WindContQIEC_kpu"/>
                <owl:minQualifiedCardinality rdf:datatype="http://www.w3.org/2001/XMLSchema#nonNegativeInteger">0</owl:minQualifiedCardinality>
                <owl:onClass rdf:resource="https://w3id.org/netbeheer/referentiemodellen/IECCIM/TC57CIM/IEC61970/Base/Domain#PU"/>
            </owl:Restriction>
        </rdfs:subClassOf>
        <rdfs:subClassOf>
            <owl:Restriction>
                <owl:onProperty rdf:resource="https://w3id.org/netbeheer/referentiemodellen/IECCIM/TC57CIM/IEC61970/Dynamics/StandardModels/WindDynamics#WindContQIEC_kqv"/>
                <owl:minQualifiedCardinality rdf:datatype="http://www.w3.org/2001/XMLSchema#nonNegativeInteger">0</owl:minQualifiedCardinality>
                <owl:onClass rdf:resource="https://w3id.org/netbeheer/referentiemodellen/IECCIM/TC57CIM/IEC61970/Base/Domain#PU"/>
            </owl:Restriction>
        </rdfs:subClassOf>
        <rdfs:subClassOf>
            <owl:Restriction>
                <owl:onProperty rdf:resource="https://w3id.org/netbeheer/referentiemodellen/IECCIM/TC57CIM/IEC61970/Dynamics/StandardModels/WindDynamics#WindContQIEC_qmax"/>
                <owl:minQualifiedCardinality rdf:datatype="http://www.w3.org/2001/XMLSchema#nonNegativeInteger">0</owl:minQualifiedCardinality>
                <owl:onClass rdf:resource="https://w3id.org/netbeheer/referentiemodellen/IECCIM/TC57CIM/IEC61970/Base/Domain#PU"/>
            </owl:Restriction>
        </rdfs:subClassOf>
        <rdfs:subClassOf>
            <owl:Restriction>
                <owl:onProperty rdf:resource="https://w3id.org/netbeheer/referentiemodellen/IECCIM/TC57CIM/IEC61970/Dynamics/StandardModels/WindDynamics#WindContQIEC_qmin"/>
                <owl:minQualifiedCardinality rdf:datatype="http://www.w3.org/2001/XMLSchema#nonNegativeInteger">0</owl:minQualifiedCardinality>
                <owl:onClass rdf:resource="https://w3id.org/netbeheer/referentiemodellen/IECCIM/TC57CIM/IEC61970/Base/Domain#PU"/>
            </owl:Restriction>
        </rdfs:subClassOf>
        <rdfs:subClassOf>
            <owl:Restriction>
                <owl:onProperty rdf:resource="https://w3id.org/netbeheer/referentiemodellen/IECCIM/TC57CIM/IEC61970/Dynamics/StandardModels/WindDynamics#WindContQIEC_rdroop"/>
                <owl:minQualifiedCardinality rdf:datatype="http://www.w3.org/2001/XMLSchema#nonNegativeInteger">0</owl:minQualifiedCardinality>
                <owl:onClass rdf:resource="https://w3id.org/netbeheer/referentiemodellen/IECCIM/TC57CIM/IEC61970/Base/Domain#PU"/>
            </owl:Restriction>
        </rdfs:subClassOf>
        <rdfs:subClassOf>
            <owl:Restriction>
                <owl:onProperty rdf:resource="https://w3id.org/netbeheer/referentiemodellen/IECCIM/TC57CIM/IEC61970/Dynamics/StandardModels/WindDynamics#WindContQIEC_tiq"/>
                <owl:minQualifiedCardinality rdf:datatype="http://www.w3.org/2001/XMLSchema#nonNegativeInteger">0</owl:minQualifiedCardinality>
                <owl:onClass rdf:resource="https://w3id.org/netbeheer/referentiemodellen/IECCIM/TC57CIM/IEC61970/Base/Domain#Seconds"/>
            </owl:Restriction>
        </rdfs:subClassOf>
        <rdfs:subClassOf>
            <owl:Restriction>
                <owl:onProperty rdf:resource="https://w3id.org/netbeheer/referentiemodellen/IECCIM/TC57CIM/IEC61970/Dynamics/StandardModels/WindDynamics#WindContQIEC_tpfilt"/>
                <owl:minQualifiedCardinality rdf:datatype="http://www.w3.org/2001/XMLSchema#nonNegativeInteger">0</owl:minQualifiedCardinality>
                <owl:onClass rdf:resource="https://w3id.org/netbeheer/referentiemodellen/IECCIM/TC57CIM/IEC61970/Base/Domain#Seconds"/>
            </owl:Restriction>
        </rdfs:subClassOf>
        <rdfs:subClassOf>
            <owl:Restriction>
                <owl:onProperty rdf:resource="https://w3id.org/netbeheer/referentiemodellen/IECCIM/TC57CIM/IEC61970/Dynamics/StandardModels/WindDynamics#WindContQIEC_tpost"/>
                <owl:minQualifiedCardinality rdf:datatype="http://www.w3.org/2001/XMLSchema#nonNegativeInteger">0</owl:minQualifiedCardinality>
                <owl:onClass rdf:resource="https://w3id.org/netbeheer/referentiemodellen/IECCIM/TC57CIM/IEC61970/Base/Domain#Seconds"/>
            </owl:Restriction>
        </rdfs:subClassOf>
        <rdfs:subClassOf>
            <owl:Restriction>
                <owl:onProperty rdf:resource="https://w3id.org/netbeheer/referentiemodellen/IECCIM/TC57CIM/IEC61970/Dynamics/StandardModels/WindDynamics#WindContQIEC_tqord"/>
                <owl:minQualifiedCardinality rdf:datatype="http://www.w3.org/2001/XMLSchema#nonNegativeInteger">0</owl:minQualifiedCardinality>
                <owl:onClass rdf:resource="https://w3id.org/netbeheer/referentiemodellen/IECCIM/TC57CIM/IEC61970/Base/Domain#Seconds"/>
            </owl:Restriction>
        </rdfs:subClassOf>
        <rdfs:subClassOf>
            <owl:Restriction>
                <owl:onProperty rdf:resource="https://w3id.org/netbeheer/referentiemodellen/IECCIM/TC57CIM/IEC61970/Dynamics/StandardModels/WindDynamics#WindContQIEC_tufilt"/>
                <owl:minQualifiedCardinality rdf:datatype="http://www.w3.org/2001/XMLSchema#nonNegativeInteger">0</owl:minQualifiedCardinality>
                <owl:onClass rdf:resource="https://w3id.org/netbeheer/referentiemodellen/IECCIM/TC57CIM/IEC61970/Base/Domain#Seconds"/>
            </owl:Restriction>
        </rdfs:subClassOf>
        <rdfs:subClassOf>
            <owl:Restriction>
                <owl:onProperty rdf:resource="https://w3id.org/netbeheer/referentiemodellen/IECCIM/TC57CIM/IEC61970/Dynamics/StandardModels/WindDynamics#WindContQIEC_udb1"/>
                <owl:minQualifiedCardinality rdf:datatype="http://www.w3.org/2001/XMLSchema#nonNegativeInteger">0</owl:minQualifiedCardinality>
                <owl:onClass rdf:resource="https://w3id.org/netbeheer/referentiemodellen/IECCIM/TC57CIM/IEC61970/Base/Domain#PU"/>
            </owl:Restriction>
        </rdfs:subClassOf>
        <rdfs:subClassOf>
            <owl:Restriction>
                <owl:onProperty rdf:resource="https://w3id.org/netbeheer/referentiemodellen/IECCIM/TC57CIM/IEC61970/Dynamics/StandardModels/WindDynamics#WindContQIEC_udb2"/>
                <owl:minQualifiedCardinality rdf:datatype="http://www.w3.org/2001/XMLSchema#nonNegativeInteger">0</owl:minQualifiedCardinality>
                <owl:onClass rdf:resource="https://w3id.org/netbeheer/referentiemodellen/IECCIM/TC57CIM/IEC61970/Base/Domain#PU"/>
            </owl:Restriction>
        </rdfs:subClassOf>
        <rdfs:subClassOf>
            <owl:Restriction>
                <owl:onProperty rdf:resource="https://w3id.org/netbeheer/referentiemodellen/IECCIM/TC57CIM/IEC61970/Dynamics/StandardModels/WindDynamics#WindContQIEC_umax"/>
                <owl:minQualifiedCardinality rdf:datatype="http://www.w3.org/2001/XMLSchema#nonNegativeInteger">0</owl:minQualifiedCardinality>
                <owl:onClass rdf:resource="https://w3id.org/netbeheer/referentiemodellen/IECCIM/TC57CIM/IEC61970/Base/Domain#PU"/>
            </owl:Restriction>
        </rdfs:subClassOf>
        <rdfs:subClassOf>
            <owl:Restriction>
                <owl:onProperty rdf:resource="https://w3id.org/netbeheer/referentiemodellen/IECCIM/TC57CIM/IEC61970/Dynamics/StandardModels/WindDynamics#WindContQIEC_umin"/>
                <owl:minQualifiedCardinality rdf:datatype="http://www.w3.org/2001/XMLSchema#nonNegativeInteger">0</owl:minQualifiedCardinality>
                <owl:onClass rdf:resource="https://w3id.org/netbeheer/referentiemodellen/IECCIM/TC57CIM/IEC61970/Base/Domain#PU"/>
            </owl:Restriction>
        </rdfs:subClassOf>
        <rdfs:subClassOf>
            <owl:Restriction>
                <owl:onProperty rdf:resource="https://w3id.org/netbeheer/referentiemodellen/IECCIM/TC57CIM/IEC61970/Dynamics/StandardModels/WindDynamics#WindContQIEC_uqdip"/>
                <owl:minQualifiedCardinality rdf:datatype="http://www.w3.org/2001/XMLSchema#nonNegativeInteger">0</owl:minQualifiedCardinality>
                <owl:onClass rdf:resource="https://w3id.org/netbeheer/referentiemodellen/IECCIM/TC57CIM/IEC61970/Base/Domain#PU"/>
            </owl:Restriction>
        </rdfs:subClassOf>
        <rdfs:subClassOf>
            <owl:Restriction>
                <owl:onProperty rdf:resource="https://w3id.org/netbeheer/referentiemodellen/IECCIM/TC57CIM/IEC61970/Dynamics/StandardModels/WindDynamics#WindContQIEC_uref0"/>
                <owl:minQualifiedCardinality rdf:datatype="http://www.w3.org/2001/XMLSchema#nonNegativeInteger">0</owl:minQualifiedCardinality>
                <owl:onClass rdf:resource="https://w3id.org/netbeheer/referentiemodellen/IECCIM/TC57CIM/IEC61970/Base/Domain#PU"/>
            </owl:Restriction>
        </rdfs:subClassOf>
        <rdfs:subClassOf>
            <owl:Restriction>
                <owl:onProperty rdf:resource="https://w3id.org/netbeheer/referentiemodellen/IECCIM/TC57CIM/IEC61970/Dynamics/StandardModels/WindDynamics#WindContQIEC_xdroop"/>
                <owl:minQualifiedCardinality rdf:datatype="http://www.w3.org/2001/XMLSchema#nonNegativeInteger">0</owl:minQualifiedCardinality>
                <owl:onClass rdf:resource="https://w3id.org/netbeheer/referentiemodellen/IECCIM/TC57CIM/IEC61970/Base/Domain#PU"/>
            </owl:Restriction>
        </rdfs:subClassOf>
        <rdfs:subClassOf>
            <owl:Restriction>
                <owl:onProperty rdf:resource="https://w3id.org/netbeheer/referentiemodellen/IECCIM/TC57CIM/IEC61970/Dynamics/StandardModels/WindDynamics#WindContQIEC_WindTurbineType3or4IEC"/>
                <owl:qualifiedCardinality rdf:datatype="http://www.w3.org/2001/XMLSchema#nonNegativeInteger">1</owl:qualifiedCardinality>
                <owl:onClass rdf:resource="https://w3id.org/netbeheer/referentiemodellen/IECCIM/TC57CIM/IEC61970/Dynamics/StandardModels/WindDynamics#WindContQIEC"/>
            </owl:Restriction>
        </rdfs:subClassOf>
        <rdfs:subClassOf>
            <owl:Restriction>
                <owl:onProperty rdf:resource="https://w3id.org/netbeheer/referentiemodellen/IECCIM/TC57CIM/IEC61970/Dynamics/StandardModels/WindDynamics#WindContQIEC_iqh1"/>
                <owl:maxQualifiedCardinality rdf:datatype="http://www.w3.org/2001/XMLSchema#nonNegativeInteger">1</owl:maxQualifiedCardinality>
                <owl:onClass rdf:resource="https://w3id.org/netbeheer/referentiemodellen/IECCIM/TC57CIM/IEC61970/Base/Domain#PU"/>
            </owl:Restriction>
        </rdfs:subClassOf>
        <rdfs:subClassOf>
            <owl:Restriction>
                <owl:onProperty rdf:resource="https://w3id.org/netbeheer/referentiemodellen/IECCIM/TC57CIM/IEC61970/Dynamics/StandardModels/WindDynamics#WindContQIEC_iqmax"/>
                <owl:maxQualifiedCardinality rdf:datatype="http://www.w3.org/2001/XMLSchema#nonNegativeInteger">1</owl:maxQualifiedCardinality>
                <owl:onClass rdf:resource="https://w3id.org/netbeheer/referentiemodellen/IECCIM/TC57CIM/IEC61970/Base/Domain#PU"/>
            </owl:Restriction>
        </rdfs:subClassOf>
        <rdfs:subClassOf>
            <owl:Restriction>
                <owl:onProperty rdf:resource="https://w3id.org/netbeheer/referentiemodellen/IECCIM/TC57CIM/IEC61970/Dynamics/StandardModels/WindDynamics#WindContQIEC_iqmin"/>
                <owl:maxQualifiedCardinality rdf:datatype="http://www.w3.org/2001/XMLSchema#nonNegativeInteger">1</owl:maxQualifiedCardinality>
                <owl:onClass rdf:resource="https://w3id.org/netbeheer/referentiemodellen/IECCIM/TC57CIM/IEC61970/Base/Domain#PU"/>
            </owl:Restriction>
        </rdfs:subClassOf>
        <rdfs:subClassOf>
            <owl:Restriction>
                <owl:onProperty rdf:resource="https://w3id.org/netbeheer/referentiemodellen/IECCIM/TC57CIM/IEC61970/Dynamics/StandardModels/WindDynamics#WindContQIEC_iqpost"/>
                <owl:maxQualifiedCardinality rdf:datatype="http://www.w3.org/2001/XMLSchema#nonNegativeInteger">1</owl:maxQualifiedCardinality>
                <owl:onClass rdf:resource="https://w3id.org/netbeheer/referentiemodellen/IECCIM/TC57CIM/IEC61970/Base/Domain#PU"/>
            </owl:Restriction>
        </rdfs:subClassOf>
        <rdfs:subClassOf>
            <owl:Restriction>
                <owl:onProperty rdf:resource="https://w3id.org/netbeheer/referentiemodellen/IECCIM/TC57CIM/IEC61970/Dynamics/StandardModels/WindDynamics#WindContQIEC_kiq"/>
                <owl:maxQualifiedCardinality rdf:datatype="http://www.w3.org/2001/XMLSchema#nonNegativeInteger">1</owl:maxQualifiedCardinality>
                <owl:onClass rdf:resource="https://w3id.org/netbeheer/referentiemodellen/IECCIM/TC57CIM/IEC61970/Base/Domain#PU"/>
            </owl:Restriction>
        </rdfs:subClassOf>
        <rdfs:subClassOf>
            <owl:Restriction>
                <owl:onProperty rdf:resource="https://w3id.org/netbeheer/referentiemodellen/IECCIM/TC57CIM/IEC61970/Dynamics/StandardModels/WindDynamics#WindContQIEC_kiu"/>
                <owl:maxQualifiedCardinality rdf:datatype="http://www.w3.org/2001/XMLSchema#nonNegativeInteger">1</owl:maxQualifiedCardinality>
                <owl:onClass rdf:resource="https://w3id.org/netbeheer/referentiemodellen/IECCIM/TC57CIM/IEC61970/Base/Domain#PU"/>
            </owl:Restriction>
        </rdfs:subClassOf>
        <rdfs:subClassOf>
            <owl:Restriction>
                <owl:onProperty rdf:resource="https://w3id.org/netbeheer/referentiemodellen/IECCIM/TC57CIM/IEC61970/Dynamics/StandardModels/WindDynamics#WindContQIEC_kpq"/>
                <owl:maxQualifiedCardinality rdf:datatype="http://www.w3.org/2001/XMLSchema#nonNegativeInteger">1</owl:maxQualifiedCardinality>
                <owl:onClass rdf:resource="https://w3id.org/netbeheer/referentiemodellen/IECCIM/TC57CIM/IEC61970/Base/Domain#PU"/>
            </owl:Restriction>
        </rdfs:subClassOf>
        <rdfs:subClassOf>
            <owl:Restriction>
                <owl:onProperty rdf:resource="https://w3id.org/netbeheer/referentiemodellen/IECCIM/TC57CIM/IEC61970/Dynamics/StandardModels/WindDynamics#WindContQIEC_kpu"/>
                <owl:maxQualifiedCardinality rdf:datatype="http://www.w3.org/2001/XMLSchema#nonNegativeInteger">1</owl:maxQualifiedCardinality>
                <owl:onClass rdf:resource="https://w3id.org/netbeheer/referentiemodellen/IECCIM/TC57CIM/IEC61970/Base/Domain#PU"/>
            </owl:Restriction>
        </rdfs:subClassOf>
        <rdfs:subClassOf>
            <owl:Restriction>
                <owl:onProperty rdf:resource="https://w3id.org/netbeheer/referentiemodellen/IECCIM/TC57CIM/IEC61970/Dynamics/StandardModels/WindDynamics#WindContQIEC_kqv"/>
                <owl:maxQualifiedCardinality rdf:datatype="http://www.w3.org/2001/XMLSchema#nonNegativeInteger">1</owl:maxQualifiedCardinality>
                <owl:onClass rdf:resource="https://w3id.org/netbeheer/referentiemodellen/IECCIM/TC57CIM/IEC61970/Base/Domain#PU"/>
            </owl:Restriction>
        </rdfs:subClassOf>
        <rdfs:subClassOf>
            <owl:Restriction>
                <owl:onProperty rdf:resource="https://w3id.org/netbeheer/referentiemodellen/IECCIM/TC57CIM/IEC61970/Dynamics/StandardModels/WindDynamics#WindContQIEC_qmax"/>
                <owl:maxQualifiedCardinality rdf:datatype="http://www.w3.org/2001/XMLSchema#nonNegativeInteger">1</owl:maxQualifiedCardinality>
                <owl:onClass rdf:resource="https://w3id.org/netbeheer/referentiemodellen/IECCIM/TC57CIM/IEC61970/Base/Domain#PU"/>
            </owl:Restriction>
        </rdfs:subClassOf>
        <rdfs:subClassOf>
            <owl:Restriction>
                <owl:onProperty rdf:resource="https://w3id.org/netbeheer/referentiemodellen/IECCIM/TC57CIM/IEC61970/Dynamics/StandardModels/WindDynamics#WindContQIEC_qmin"/>
                <owl:maxQualifiedCardinality rdf:datatype="http://www.w3.org/2001/XMLSchema#nonNegativeInteger">1</owl:maxQualifiedCardinality>
                <owl:onClass rdf:resource="https://w3id.org/netbeheer/referentiemodellen/IECCIM/TC57CIM/IEC61970/Base/Domain#PU"/>
            </owl:Restriction>
        </rdfs:subClassOf>
        <rdfs:subClassOf>
            <owl:Restriction>
                <owl:onProperty rdf:resource="https://w3id.org/netbeheer/referentiemodellen/IECCIM/TC57CIM/IEC61970/Dynamics/StandardModels/WindDynamics#WindContQIEC_rdroop"/>
                <owl:maxQualifiedCardinality rdf:datatype="http://www.w3.org/2001/XMLSchema#nonNegativeInteger">1</owl:maxQualifiedCardinality>
                <owl:onClass rdf:resource="https://w3id.org/netbeheer/referentiemodellen/IECCIM/TC57CIM/IEC61970/Base/Domain#PU"/>
            </owl:Restriction>
        </rdfs:subClassOf>
        <rdfs:subClassOf>
            <owl:Restriction>
                <owl:onProperty rdf:resource="https://w3id.org/netbeheer/referentiemodellen/IECCIM/TC57CIM/IEC61970/Dynamics/StandardModels/WindDynamics#WindContQIEC_tiq"/>
                <owl:maxQualifiedCardinality rdf:datatype="http://www.w3.org/2001/XMLSchema#nonNegativeInteger">1</owl:maxQualifiedCardinality>
                <owl:onClass rdf:resource="https://w3id.org/netbeheer/referentiemodellen/IECCIM/TC57CIM/IEC61970/Base/Domain#Seconds"/>
            </owl:Restriction>
        </rdfs:subClassOf>
        <rdfs:subClassOf>
            <owl:Restriction>
                <owl:onProperty rdf:resource="https://w3id.org/netbeheer/referentiemodellen/IECCIM/TC57CIM/IEC61970/Dynamics/StandardModels/WindDynamics#WindContQIEC_tpfilt"/>
                <owl:maxQualifiedCardinality rdf:datatype="http://www.w3.org/2001/XMLSchema#nonNegativeInteger">1</owl:maxQualifiedCardinality>
                <owl:onClass rdf:resource="https://w3id.org/netbeheer/referentiemodellen/IECCIM/TC57CIM/IEC61970/Base/Domain#Seconds"/>
            </owl:Restriction>
        </rdfs:subClassOf>
        <rdfs:subClassOf>
            <owl:Restriction>
                <owl:onProperty rdf:resource="https://w3id.org/netbeheer/referentiemodellen/IECCIM/TC57CIM/IEC61970/Dynamics/StandardModels/WindDynamics#WindContQIEC_tpost"/>
                <owl:maxQualifiedCardinality rdf:datatype="http://www.w3.org/2001/XMLSchema#nonNegativeInteger">1</owl:maxQualifiedCardinality>
                <owl:onClass rdf:resource="https://w3id.org/netbeheer/referentiemodellen/IECCIM/TC57CIM/IEC61970/Base/Domain#Seconds"/>
            </owl:Restriction>
        </rdfs:subClassOf>
        <rdfs:subClassOf>
            <owl:Restriction>
                <owl:onProperty rdf:resource="https://w3id.org/netbeheer/referentiemodellen/IECCIM/TC57CIM/IEC61970/Dynamics/StandardModels/WindDynamics#WindContQIEC_tqord"/>
                <owl:maxQualifiedCardinality rdf:datatype="http://www.w3.org/2001/XMLSchema#nonNegativeInteger">1</owl:maxQualifiedCardinality>
                <owl:onClass rdf:resource="https://w3id.org/netbeheer/referentiemodellen/IECCIM/TC57CIM/IEC61970/Base/Domain#Seconds"/>
            </owl:Restriction>
        </rdfs:subClassOf>
        <rdfs:subClassOf>
            <owl:Restriction>
                <owl:onProperty rdf:resource="https://w3id.org/netbeheer/referentiemodellen/IECCIM/TC57CIM/IEC61970/Dynamics/StandardModels/WindDynamics#WindContQIEC_tufilt"/>
                <owl:maxQualifiedCardinality rdf:datatype="http://www.w3.org/2001/XMLSchema#nonNegativeInteger">1</owl:maxQualifiedCardinality>
                <owl:onClass rdf:resource="https://w3id.org/netbeheer/referentiemodellen/IECCIM/TC57CIM/IEC61970/Base/Domain#Seconds"/>
            </owl:Restriction>
        </rdfs:subClassOf>
        <rdfs:subClassOf>
            <owl:Restriction>
                <owl:onProperty rdf:resource="https://w3id.org/netbeheer/referentiemodellen/IECCIM/TC57CIM/IEC61970/Dynamics/StandardModels/WindDynamics#WindContQIEC_udb1"/>
                <owl:maxQualifiedCardinality rdf:datatype="http://www.w3.org/2001/XMLSchema#nonNegativeInteger">1</owl:maxQualifiedCardinality>
                <owl:onClass rdf:resource="https://w3id.org/netbeheer/referentiemodellen/IECCIM/TC57CIM/IEC61970/Base/Domain#PU"/>
            </owl:Restriction>
        </rdfs:subClassOf>
        <rdfs:subClassOf>
            <owl:Restriction>
                <owl:onProperty rdf:resource="https://w3id.org/netbeheer/referentiemodellen/IECCIM/TC57CIM/IEC61970/Dynamics/StandardModels/WindDynamics#WindContQIEC_udb2"/>
                <owl:maxQualifiedCardinality rdf:datatype="http://www.w3.org/2001/XMLSchema#nonNegativeInteger">1</owl:maxQualifiedCardinality>
                <owl:onClass rdf:resource="https://w3id.org/netbeheer/referentiemodellen/IECCIM/TC57CIM/IEC61970/Base/Domain#PU"/>
            </owl:Restriction>
        </rdfs:subClassOf>
        <rdfs:subClassOf>
            <owl:Restriction>
                <owl:onProperty rdf:resource="https://w3id.org/netbeheer/referentiemodellen/IECCIM/TC57CIM/IEC61970/Dynamics/StandardModels/WindDynamics#WindContQIEC_umax"/>
                <owl:maxQualifiedCardinality rdf:datatype="http://www.w3.org/2001/XMLSchema#nonNegativeInteger">1</owl:maxQualifiedCardinality>
                <owl:onClass rdf:resource="https://w3id.org/netbeheer/referentiemodellen/IECCIM/TC57CIM/IEC61970/Base/Domain#PU"/>
            </owl:Restriction>
        </rdfs:subClassOf>
        <rdfs:subClassOf>
            <owl:Restriction>
                <owl:onProperty rdf:resource="https://w3id.org/netbeheer/referentiemodellen/IECCIM/TC57CIM/IEC61970/Dynamics/StandardModels/WindDynamics#WindContQIEC_umin"/>
                <owl:maxQualifiedCardinality rdf:datatype="http://www.w3.org/2001/XMLSchema#nonNegativeInteger">1</owl:maxQualifiedCardinality>
                <owl:onClass rdf:resource="https://w3id.org/netbeheer/referentiemodellen/IECCIM/TC57CIM/IEC61970/Base/Domain#PU"/>
            </owl:Restriction>
        </rdfs:subClassOf>
        <rdfs:subClassOf>
            <owl:Restriction>
                <owl:onProperty rdf:resource="https://w3id.org/netbeheer/referentiemodellen/IECCIM/TC57CIM/IEC61970/Dynamics/StandardModels/WindDynamics#WindContQIEC_uqdip"/>
                <owl:maxQualifiedCardinality rdf:datatype="http://www.w3.org/2001/XMLSchema#nonNegativeInteger">1</owl:maxQualifiedCardinality>
                <owl:onClass rdf:resource="https://w3id.org/netbeheer/referentiemodellen/IECCIM/TC57CIM/IEC61970/Base/Domain#PU"/>
            </owl:Restriction>
        </rdfs:subClassOf>
        <rdfs:subClassOf>
            <owl:Restriction>
                <owl:onProperty rdf:resource="https://w3id.org/netbeheer/referentiemodellen/IECCIM/TC57CIM/IEC61970/Dynamics/StandardModels/WindDynamics#WindContQIEC_uref0"/>
                <owl:maxQualifiedCardinality rdf:datatype="http://www.w3.org/2001/XMLSchema#nonNegativeInteger">1</owl:maxQualifiedCardinality>
                <owl:onClass rdf:resource="https://w3id.org/netbeheer/referentiemodellen/IECCIM/TC57CIM/IEC61970/Base/Domain#PU"/>
            </owl:Restriction>
        </rdfs:subClassOf>
        <rdfs:subClassOf>
            <owl:Restriction>
                <owl:onProperty rdf:resource="https://w3id.org/netbeheer/referentiemodellen/IECCIM/TC57CIM/IEC61970/Dynamics/StandardModels/WindDynamics#WindContQIEC_xdroop"/>
                <owl:maxQualifiedCardinality rdf:datatype="http://www.w3.org/2001/XMLSchema#nonNegativeInteger">1</owl:maxQualifiedCardinality>
                <owl:onClass rdf:resource="https://w3id.org/netbeheer/referentiemodellen/IECCIM/TC57CIM/IEC61970/Base/Domain#PU"/>
            </owl:Restriction>
        </rdfs:subClassOf>
        <rdfs:subClassOf>
            <owl:Restriction>
                <owl:onProperty rdf:resource="https://w3id.org/netbeheer/referentiemodellen/IECCIM/TC57CIM/IEC61970/Dynamics/StandardModels/WindDynamics#WindContQIEC_windLVRTQcontrolModesType"/>
                <owl:minQualifiedCardinality rdf:datatype="http://www.w3.org/2001/XMLSchema#nonNegativeInteger">0</owl:minQualifiedCardinality>
                <owl:onDataRange rdf:resource="https://w3id.org/netbeheer/referentiemodellen/IECCIM/TC57CIM/IEC61970/Dynamics/StandardModels/WindDynamics#WindLVRTQcontrolModesKind"/>
            </owl:Restriction>
        </rdfs:subClassOf>
        <rdfs:subClassOf>
            <owl:Restriction>
                <owl:onProperty rdf:resource="https://w3id.org/netbeheer/referentiemodellen/IECCIM/TC57CIM/IEC61970/Dynamics/StandardModels/WindDynamics#WindContQIEC_windQcontrolModesType"/>
                <owl:minQualifiedCardinality rdf:datatype="http://www.w3.org/2001/XMLSchema#nonNegativeInteger">0</owl:minQualifiedCardinality>
                <owl:onDataRange rdf:resource="https://w3id.org/netbeheer/referentiemodellen/IECCIM/TC57CIM/IEC61970/Dynamics/StandardModels/WindDynamics#WindQcontrolModesKind"/>
            </owl:Restriction>
        </rdfs:subClassOf>
        <rdfs:subClassOf>
            <owl:Restriction>
                <owl:onProperty rdf:resource="https://w3id.org/netbeheer/referentiemodellen/IECCIM/TC57CIM/IEC61970/Dynamics/StandardModels/WindDynamics#WindContQIEC_windLVRTQcontrolModesType"/>
                <owl:maxQualifiedCardinality rdf:datatype="http://www.w3.org/2001/XMLSchema#nonNegativeInteger">1</owl:maxQualifiedCardinality>
                <owl:onDataRange rdf:resource="https://w3id.org/netbeheer/referentiemodellen/IECCIM/TC57CIM/IEC61970/Dynamics/StandardModels/WindDynamics#WindLVRTQcontrolModesKind"/>
            </owl:Restriction>
        </rdfs:subClassOf>
        <rdfs:subClassOf>
            <owl:Restriction>
                <owl:onProperty rdf:resource="https://w3id.org/netbeheer/referentiemodellen/IECCIM/TC57CIM/IEC61970/Dynamics/StandardModels/WindDynamics#WindContQIEC_windQcontrolModesType"/>
                <owl:maxQualifiedCardinality rdf:datatype="http://www.w3.org/2001/XMLSchema#nonNegativeInteger">1</owl:maxQualifiedCardinality>
                <owl:onDataRange rdf:resource="https://w3id.org/netbeheer/referentiemodellen/IECCIM/TC57CIM/IEC61970/Dynamics/StandardModels/WindDynamics#WindQcontrolModesKind"/>
            </owl:Restriction>
        </rdfs:subClassOf>
        <rdfs:comment>Q control model.

Reference: IEC Standard 61400-27-1 Section 6.6.5.6.</rdfs:comment>
    </owl:Class>
    


    <!-- https://w3id.org/netbeheer/referentiemodellen/IECCIM/TC57CIM/IEC61970/Dynamics/StandardModels/WindDynamics#WindContRotorRIEC -->


    <owl:Class rdf:about="https://w3id.org/netbeheer/referentiemodellen/IECCIM/TC57CIM/IEC61970/Dynamics/StandardModels/WindDynamics#WindContRotorRIEC">
        <rdfs:subClassOf rdf:resource="https://w3id.org/netbeheer/referentiemodellen/IECCIM/TC57CIM/IEC61970/Base/Core#IdentifiedObject"/>
        <rdfs:subClassOf>
            <owl:Restriction>
                <owl:onProperty rdf:resource="https://w3id.org/netbeheer/referentiemodellen/IECCIM/TC57CIM/IEC61970/Dynamics/StandardModels/WindDynamics#WindContRotorRIEC_WindDynamicsLookupTable"/>
                <owl:minQualifiedCardinality rdf:datatype="http://www.w3.org/2001/XMLSchema#nonNegativeInteger">0</owl:minQualifiedCardinality>
                <owl:onClass rdf:resource="https://w3id.org/netbeheer/referentiemodellen/IECCIM/TC57CIM/IEC61970/Dynamics/StandardModels/WindDynamics#WindContRotorRIEC"/>
            </owl:Restriction>
        </rdfs:subClassOf>
        <rdfs:subClassOf>
            <owl:Restriction>
                <owl:onProperty rdf:resource="https://w3id.org/netbeheer/referentiemodellen/IECCIM/TC57CIM/IEC61970/Dynamics/StandardModels/WindDynamics#WindContRotorRIEC_kirr"/>
                <owl:minQualifiedCardinality rdf:datatype="http://www.w3.org/2001/XMLSchema#nonNegativeInteger">0</owl:minQualifiedCardinality>
                <owl:onClass rdf:resource="https://w3id.org/netbeheer/referentiemodellen/IECCIM/TC57CIM/IEC61970/Base/Domain#PU"/>
            </owl:Restriction>
        </rdfs:subClassOf>
        <rdfs:subClassOf>
            <owl:Restriction>
                <owl:onProperty rdf:resource="https://w3id.org/netbeheer/referentiemodellen/IECCIM/TC57CIM/IEC61970/Dynamics/StandardModels/WindDynamics#WindContRotorRIEC_kprr"/>
                <owl:minQualifiedCardinality rdf:datatype="http://www.w3.org/2001/XMLSchema#nonNegativeInteger">0</owl:minQualifiedCardinality>
                <owl:onClass rdf:resource="https://w3id.org/netbeheer/referentiemodellen/IECCIM/TC57CIM/IEC61970/Base/Domain#PU"/>
            </owl:Restriction>
        </rdfs:subClassOf>
        <rdfs:subClassOf>
            <owl:Restriction>
                <owl:onProperty rdf:resource="https://w3id.org/netbeheer/referentiemodellen/IECCIM/TC57CIM/IEC61970/Dynamics/StandardModels/WindDynamics#WindContRotorRIEC_rmax"/>
                <owl:minQualifiedCardinality rdf:datatype="http://www.w3.org/2001/XMLSchema#nonNegativeInteger">0</owl:minQualifiedCardinality>
                <owl:onClass rdf:resource="https://w3id.org/netbeheer/referentiemodellen/IECCIM/TC57CIM/IEC61970/Base/Domain#PU"/>
            </owl:Restriction>
        </rdfs:subClassOf>
        <rdfs:subClassOf>
            <owl:Restriction>
                <owl:onProperty rdf:resource="https://w3id.org/netbeheer/referentiemodellen/IECCIM/TC57CIM/IEC61970/Dynamics/StandardModels/WindDynamics#WindContRotorRIEC_rmin"/>
                <owl:minQualifiedCardinality rdf:datatype="http://www.w3.org/2001/XMLSchema#nonNegativeInteger">0</owl:minQualifiedCardinality>
                <owl:onClass rdf:resource="https://w3id.org/netbeheer/referentiemodellen/IECCIM/TC57CIM/IEC61970/Base/Domain#PU"/>
            </owl:Restriction>
        </rdfs:subClassOf>
        <rdfs:subClassOf>
            <owl:Restriction>
                <owl:onProperty rdf:resource="https://w3id.org/netbeheer/referentiemodellen/IECCIM/TC57CIM/IEC61970/Dynamics/StandardModels/WindDynamics#WindContRotorRIEC_tomegafilt"/>
                <owl:minQualifiedCardinality rdf:datatype="http://www.w3.org/2001/XMLSchema#nonNegativeInteger">0</owl:minQualifiedCardinality>
                <owl:onClass rdf:resource="https://w3id.org/netbeheer/referentiemodellen/IECCIM/TC57CIM/IEC61970/Base/Domain#Seconds"/>
            </owl:Restriction>
        </rdfs:subClassOf>
        <rdfs:subClassOf>
            <owl:Restriction>
                <owl:onProperty rdf:resource="https://w3id.org/netbeheer/referentiemodellen/IECCIM/TC57CIM/IEC61970/Dynamics/StandardModels/WindDynamics#WindContRotorRIEC_tpfilt"/>
                <owl:minQualifiedCardinality rdf:datatype="http://www.w3.org/2001/XMLSchema#nonNegativeInteger">0</owl:minQualifiedCardinality>
                <owl:onClass rdf:resource="https://w3id.org/netbeheer/referentiemodellen/IECCIM/TC57CIM/IEC61970/Base/Domain#Seconds"/>
            </owl:Restriction>
        </rdfs:subClassOf>
        <rdfs:subClassOf>
            <owl:Restriction>
                <owl:onProperty rdf:resource="https://w3id.org/netbeheer/referentiemodellen/IECCIM/TC57CIM/IEC61970/Dynamics/StandardModels/WindDynamics#WindContRotorRIEC_WindGenTurbineType2IEC"/>
                <owl:qualifiedCardinality rdf:datatype="http://www.w3.org/2001/XMLSchema#nonNegativeInteger">1</owl:qualifiedCardinality>
                <owl:onClass rdf:resource="https://w3id.org/netbeheer/referentiemodellen/IECCIM/TC57CIM/IEC61970/Dynamics/StandardModels/WindDynamics#WindContRotorRIEC"/>
            </owl:Restriction>
        </rdfs:subClassOf>
        <rdfs:subClassOf>
            <owl:Restriction>
                <owl:onProperty rdf:resource="https://w3id.org/netbeheer/referentiemodellen/IECCIM/TC57CIM/IEC61970/Dynamics/StandardModels/WindDynamics#WindContRotorRIEC_WindDynamicsLookupTable"/>
                <owl:maxQualifiedCardinality rdf:datatype="http://www.w3.org/2001/XMLSchema#nonNegativeInteger">1</owl:maxQualifiedCardinality>
                <owl:onClass rdf:resource="https://w3id.org/netbeheer/referentiemodellen/IECCIM/TC57CIM/IEC61970/Dynamics/StandardModels/WindDynamics#WindContRotorRIEC"/>
            </owl:Restriction>
        </rdfs:subClassOf>
        <rdfs:subClassOf>
            <owl:Restriction>
                <owl:onProperty rdf:resource="https://w3id.org/netbeheer/referentiemodellen/IECCIM/TC57CIM/IEC61970/Dynamics/StandardModels/WindDynamics#WindContRotorRIEC_kirr"/>
                <owl:maxQualifiedCardinality rdf:datatype="http://www.w3.org/2001/XMLSchema#nonNegativeInteger">1</owl:maxQualifiedCardinality>
                <owl:onClass rdf:resource="https://w3id.org/netbeheer/referentiemodellen/IECCIM/TC57CIM/IEC61970/Base/Domain#PU"/>
            </owl:Restriction>
        </rdfs:subClassOf>
        <rdfs:subClassOf>
            <owl:Restriction>
                <owl:onProperty rdf:resource="https://w3id.org/netbeheer/referentiemodellen/IECCIM/TC57CIM/IEC61970/Dynamics/StandardModels/WindDynamics#WindContRotorRIEC_kprr"/>
                <owl:maxQualifiedCardinality rdf:datatype="http://www.w3.org/2001/XMLSchema#nonNegativeInteger">1</owl:maxQualifiedCardinality>
                <owl:onClass rdf:resource="https://w3id.org/netbeheer/referentiemodellen/IECCIM/TC57CIM/IEC61970/Base/Domain#PU"/>
            </owl:Restriction>
        </rdfs:subClassOf>
        <rdfs:subClassOf>
            <owl:Restriction>
                <owl:onProperty rdf:resource="https://w3id.org/netbeheer/referentiemodellen/IECCIM/TC57CIM/IEC61970/Dynamics/StandardModels/WindDynamics#WindContRotorRIEC_rmax"/>
                <owl:maxQualifiedCardinality rdf:datatype="http://www.w3.org/2001/XMLSchema#nonNegativeInteger">1</owl:maxQualifiedCardinality>
                <owl:onClass rdf:resource="https://w3id.org/netbeheer/referentiemodellen/IECCIM/TC57CIM/IEC61970/Base/Domain#PU"/>
            </owl:Restriction>
        </rdfs:subClassOf>
        <rdfs:subClassOf>
            <owl:Restriction>
                <owl:onProperty rdf:resource="https://w3id.org/netbeheer/referentiemodellen/IECCIM/TC57CIM/IEC61970/Dynamics/StandardModels/WindDynamics#WindContRotorRIEC_rmin"/>
                <owl:maxQualifiedCardinality rdf:datatype="http://www.w3.org/2001/XMLSchema#nonNegativeInteger">1</owl:maxQualifiedCardinality>
                <owl:onClass rdf:resource="https://w3id.org/netbeheer/referentiemodellen/IECCIM/TC57CIM/IEC61970/Base/Domain#PU"/>
            </owl:Restriction>
        </rdfs:subClassOf>
        <rdfs:subClassOf>
            <owl:Restriction>
                <owl:onProperty rdf:resource="https://w3id.org/netbeheer/referentiemodellen/IECCIM/TC57CIM/IEC61970/Dynamics/StandardModels/WindDynamics#WindContRotorRIEC_tomegafilt"/>
                <owl:maxQualifiedCardinality rdf:datatype="http://www.w3.org/2001/XMLSchema#nonNegativeInteger">1</owl:maxQualifiedCardinality>
                <owl:onClass rdf:resource="https://w3id.org/netbeheer/referentiemodellen/IECCIM/TC57CIM/IEC61970/Base/Domain#Seconds"/>
            </owl:Restriction>
        </rdfs:subClassOf>
        <rdfs:subClassOf>
            <owl:Restriction>
                <owl:onProperty rdf:resource="https://w3id.org/netbeheer/referentiemodellen/IECCIM/TC57CIM/IEC61970/Dynamics/StandardModels/WindDynamics#WindContRotorRIEC_tpfilt"/>
                <owl:maxQualifiedCardinality rdf:datatype="http://www.w3.org/2001/XMLSchema#nonNegativeInteger">1</owl:maxQualifiedCardinality>
                <owl:onClass rdf:resource="https://w3id.org/netbeheer/referentiemodellen/IECCIM/TC57CIM/IEC61970/Base/Domain#Seconds"/>
            </owl:Restriction>
        </rdfs:subClassOf>
        <rdfs:subClassOf>
            <owl:Restriction>
                <owl:onProperty rdf:resource="https://w3id.org/netbeheer/referentiemodellen/IECCIM/TC57CIM/IEC61970/Dynamics/StandardModels/WindDynamics#WindContRotorRIEC_komegafilt"/>
                <owl:minQualifiedCardinality rdf:datatype="http://www.w3.org/2001/XMLSchema#nonNegativeInteger">0</owl:minQualifiedCardinality>
                <owl:onDataRange rdf:resource="http://www.w3.org/2001/XMLSchema#float"/>
            </owl:Restriction>
        </rdfs:subClassOf>
        <rdfs:subClassOf>
            <owl:Restriction>
                <owl:onProperty rdf:resource="https://w3id.org/netbeheer/referentiemodellen/IECCIM/TC57CIM/IEC61970/Dynamics/StandardModels/WindDynamics#WindContRotorRIEC_kpfilt"/>
                <owl:minQualifiedCardinality rdf:datatype="http://www.w3.org/2001/XMLSchema#nonNegativeInteger">0</owl:minQualifiedCardinality>
                <owl:onDataRange rdf:resource="http://www.w3.org/2001/XMLSchema#float"/>
            </owl:Restriction>
        </rdfs:subClassOf>
        <rdfs:subClassOf>
            <owl:Restriction>
                <owl:onProperty rdf:resource="https://w3id.org/netbeheer/referentiemodellen/IECCIM/TC57CIM/IEC61970/Dynamics/StandardModels/WindDynamics#WindContRotorRIEC_komegafilt"/>
                <owl:maxQualifiedCardinality rdf:datatype="http://www.w3.org/2001/XMLSchema#nonNegativeInteger">1</owl:maxQualifiedCardinality>
                <owl:onDataRange rdf:resource="http://www.w3.org/2001/XMLSchema#float"/>
            </owl:Restriction>
        </rdfs:subClassOf>
        <rdfs:subClassOf>
            <owl:Restriction>
                <owl:onProperty rdf:resource="https://w3id.org/netbeheer/referentiemodellen/IECCIM/TC57CIM/IEC61970/Dynamics/StandardModels/WindDynamics#WindContRotorRIEC_kpfilt"/>
                <owl:maxQualifiedCardinality rdf:datatype="http://www.w3.org/2001/XMLSchema#nonNegativeInteger">1</owl:maxQualifiedCardinality>
                <owl:onDataRange rdf:resource="http://www.w3.org/2001/XMLSchema#float"/>
            </owl:Restriction>
        </rdfs:subClassOf>
        <rdfs:comment>Rotor resistance control model.

Reference: IEC Standard 61400-27-1 Section 6.6.5.2.</rdfs:comment>
    </owl:Class>
    


    <!-- https://w3id.org/netbeheer/referentiemodellen/IECCIM/TC57CIM/IEC61970/Dynamics/StandardModels/WindDynamics#WindDynamicsLookupTable -->


    <owl:Class rdf:about="https://w3id.org/netbeheer/referentiemodellen/IECCIM/TC57CIM/IEC61970/Dynamics/StandardModels/WindDynamics#WindDynamicsLookupTable">
        <rdfs:subClassOf rdf:resource="https://w3id.org/netbeheer/referentiemodellen/IECCIM/TC57CIM/IEC61970/Base/Core#IdentifiedObject"/>
        <rdfs:subClassOf>
            <owl:Restriction>
                <owl:onProperty rdf:resource="https://w3id.org/netbeheer/referentiemodellen/IECCIM/TC57CIM/IEC61970/Dynamics/StandardModels/WindDynamics#WindDynamicsLookupTable_WindContCurrLimIEC"/>
                <owl:minQualifiedCardinality rdf:datatype="http://www.w3.org/2001/XMLSchema#nonNegativeInteger">1</owl:minQualifiedCardinality>
                <owl:onClass rdf:resource="https://w3id.org/netbeheer/referentiemodellen/IECCIM/TC57CIM/IEC61970/Dynamics/StandardModels/WindDynamics#WindDynamicsLookupTable"/>
            </owl:Restriction>
        </rdfs:subClassOf>
        <rdfs:subClassOf>
            <owl:Restriction>
                <owl:onProperty rdf:resource="https://w3id.org/netbeheer/referentiemodellen/IECCIM/TC57CIM/IEC61970/Dynamics/StandardModels/WindDynamics#WindDynamicsLookupTable_WindContPType3IEC"/>
                <owl:minQualifiedCardinality rdf:datatype="http://www.w3.org/2001/XMLSchema#nonNegativeInteger">2</owl:minQualifiedCardinality>
                <owl:onClass rdf:resource="https://w3id.org/netbeheer/referentiemodellen/IECCIM/TC57CIM/IEC61970/Dynamics/StandardModels/WindDynamics#WindDynamicsLookupTable"/>
            </owl:Restriction>
        </rdfs:subClassOf>
        <rdfs:subClassOf>
            <owl:Restriction>
                <owl:onProperty rdf:resource="https://w3id.org/netbeheer/referentiemodellen/IECCIM/TC57CIM/IEC61970/Dynamics/StandardModels/WindDynamics#WindDynamicsLookupTable_WindContRotorRIEC"/>
                <owl:minQualifiedCardinality rdf:datatype="http://www.w3.org/2001/XMLSchema#nonNegativeInteger">1</owl:minQualifiedCardinality>
                <owl:onClass rdf:resource="https://w3id.org/netbeheer/referentiemodellen/IECCIM/TC57CIM/IEC61970/Dynamics/StandardModels/WindDynamics#WindDynamicsLookupTable"/>
            </owl:Restriction>
        </rdfs:subClassOf>
        <rdfs:subClassOf>
            <owl:Restriction>
                <owl:onProperty rdf:resource="https://w3id.org/netbeheer/referentiemodellen/IECCIM/TC57CIM/IEC61970/Dynamics/StandardModels/WindDynamics#WindDynamicsLookupTable_WindPlantFreqPcontrolIEC"/>
                <owl:minQualifiedCardinality rdf:datatype="http://www.w3.org/2001/XMLSchema#nonNegativeInteger">1</owl:minQualifiedCardinality>
                <owl:onClass rdf:resource="https://w3id.org/netbeheer/referentiemodellen/IECCIM/TC57CIM/IEC61970/Dynamics/StandardModels/WindDynamics#WindDynamicsLookupTable"/>
            </owl:Restriction>
        </rdfs:subClassOf>
        <rdfs:subClassOf>
            <owl:Restriction>
                <owl:onProperty rdf:resource="https://w3id.org/netbeheer/referentiemodellen/IECCIM/TC57CIM/IEC61970/Dynamics/StandardModels/WindDynamics#WindDynamicsLookupTable_input"/>
                <owl:minQualifiedCardinality rdf:datatype="http://www.w3.org/2001/XMLSchema#nonNegativeInteger">0</owl:minQualifiedCardinality>
                <owl:onDataRange rdf:resource="http://www.w3.org/2001/XMLSchema#float"/>
            </owl:Restriction>
        </rdfs:subClassOf>
        <rdfs:subClassOf>
            <owl:Restriction>
                <owl:onProperty rdf:resource="https://w3id.org/netbeheer/referentiemodellen/IECCIM/TC57CIM/IEC61970/Dynamics/StandardModels/WindDynamics#WindDynamicsLookupTable_lookupTableFunctionType"/>
                <owl:minQualifiedCardinality rdf:datatype="http://www.w3.org/2001/XMLSchema#nonNegativeInteger">0</owl:minQualifiedCardinality>
                <owl:onDataRange rdf:resource="https://w3id.org/netbeheer/referentiemodellen/IECCIM/TC57CIM/IEC61970/Dynamics/StandardModels/WindDynamics#WindLookupTableFunctionKind"/>
            </owl:Restriction>
        </rdfs:subClassOf>
        <rdfs:subClassOf>
            <owl:Restriction>
                <owl:onProperty rdf:resource="https://w3id.org/netbeheer/referentiemodellen/IECCIM/TC57CIM/IEC61970/Dynamics/StandardModels/WindDynamics#WindDynamicsLookupTable_output"/>
                <owl:minQualifiedCardinality rdf:datatype="http://www.w3.org/2001/XMLSchema#nonNegativeInteger">0</owl:minQualifiedCardinality>
                <owl:onDataRange rdf:resource="http://www.w3.org/2001/XMLSchema#float"/>
            </owl:Restriction>
        </rdfs:subClassOf>
        <rdfs:subClassOf>
            <owl:Restriction>
                <owl:onProperty rdf:resource="https://w3id.org/netbeheer/referentiemodellen/IECCIM/TC57CIM/IEC61970/Dynamics/StandardModels/WindDynamics#WindDynamicsLookupTable_sequence"/>
                <owl:minQualifiedCardinality rdf:datatype="http://www.w3.org/2001/XMLSchema#nonNegativeInteger">0</owl:minQualifiedCardinality>
                <owl:onDataRange rdf:resource="http://www.w3.org/2001/XMLSchema#nonNegativeInteger"/>
            </owl:Restriction>
        </rdfs:subClassOf>
        <rdfs:subClassOf>
            <owl:Restriction>
                <owl:onProperty rdf:resource="https://w3id.org/netbeheer/referentiemodellen/IECCIM/TC57CIM/IEC61970/Dynamics/StandardModels/WindDynamics#WindDynamicsLookupTable_input"/>
                <owl:maxQualifiedCardinality rdf:datatype="http://www.w3.org/2001/XMLSchema#nonNegativeInteger">1</owl:maxQualifiedCardinality>
                <owl:onDataRange rdf:resource="http://www.w3.org/2001/XMLSchema#float"/>
            </owl:Restriction>
        </rdfs:subClassOf>
        <rdfs:subClassOf>
            <owl:Restriction>
                <owl:onProperty rdf:resource="https://w3id.org/netbeheer/referentiemodellen/IECCIM/TC57CIM/IEC61970/Dynamics/StandardModels/WindDynamics#WindDynamicsLookupTable_lookupTableFunctionType"/>
                <owl:maxQualifiedCardinality rdf:datatype="http://www.w3.org/2001/XMLSchema#nonNegativeInteger">1</owl:maxQualifiedCardinality>
                <owl:onDataRange rdf:resource="https://w3id.org/netbeheer/referentiemodellen/IECCIM/TC57CIM/IEC61970/Dynamics/StandardModels/WindDynamics#WindLookupTableFunctionKind"/>
            </owl:Restriction>
        </rdfs:subClassOf>
        <rdfs:subClassOf>
            <owl:Restriction>
                <owl:onProperty rdf:resource="https://w3id.org/netbeheer/referentiemodellen/IECCIM/TC57CIM/IEC61970/Dynamics/StandardModels/WindDynamics#WindDynamicsLookupTable_output"/>
                <owl:maxQualifiedCardinality rdf:datatype="http://www.w3.org/2001/XMLSchema#nonNegativeInteger">1</owl:maxQualifiedCardinality>
                <owl:onDataRange rdf:resource="http://www.w3.org/2001/XMLSchema#float"/>
            </owl:Restriction>
        </rdfs:subClassOf>
        <rdfs:subClassOf>
            <owl:Restriction>
                <owl:onProperty rdf:resource="https://w3id.org/netbeheer/referentiemodellen/IECCIM/TC57CIM/IEC61970/Dynamics/StandardModels/WindDynamics#WindDynamicsLookupTable_sequence"/>
                <owl:maxQualifiedCardinality rdf:datatype="http://www.w3.org/2001/XMLSchema#nonNegativeInteger">1</owl:maxQualifiedCardinality>
                <owl:onDataRange rdf:resource="http://www.w3.org/2001/XMLSchema#nonNegativeInteger"/>
            </owl:Restriction>
        </rdfs:subClassOf>
        <rdfs:comment>The class models a look up table for the purpose of wind standard models.</rdfs:comment>
    </owl:Class>
    


    <!-- https://w3id.org/netbeheer/referentiemodellen/IECCIM/TC57CIM/IEC61970/Dynamics/StandardModels/WindDynamics#WindGenTurbineType1IEC -->


    <owl:Class rdf:about="https://w3id.org/netbeheer/referentiemodellen/IECCIM/TC57CIM/IEC61970/Dynamics/StandardModels/WindDynamics#WindGenTurbineType1IEC">
        <rdfs:subClassOf rdf:resource="https://w3id.org/netbeheer/referentiemodellen/IECCIM/TC57CIM/IEC61970/Dynamics/StandardModels/WindDynamics#WindTurbineType1or2IEC"/>
        <rdfs:subClassOf>
            <owl:Restriction>
                <owl:onProperty rdf:resource="https://w3id.org/netbeheer/referentiemodellen/IECCIM/TC57CIM/IEC61970/Dynamics/StandardModels/WindDynamics#WindGenTurbineType1IEC_WindAeroConstIEC"/>
                <owl:qualifiedCardinality rdf:datatype="http://www.w3.org/2001/XMLSchema#nonNegativeInteger">1</owl:qualifiedCardinality>
                <owl:onClass rdf:resource="https://w3id.org/netbeheer/referentiemodellen/IECCIM/TC57CIM/IEC61970/Dynamics/StandardModels/WindDynamics#WindGenTurbineType1IEC"/>
            </owl:Restriction>
        </rdfs:subClassOf>
        <rdfs:comment>Wind turbine IEC Type 1.

Reference: IEC Standard 61400-27-1, section 6.5.2.</rdfs:comment>
    </owl:Class>
    


    <!-- https://w3id.org/netbeheer/referentiemodellen/IECCIM/TC57CIM/IEC61970/Dynamics/StandardModels/WindDynamics#WindGenTurbineType2IEC -->


    <owl:Class rdf:about="https://w3id.org/netbeheer/referentiemodellen/IECCIM/TC57CIM/IEC61970/Dynamics/StandardModels/WindDynamics#WindGenTurbineType2IEC">
        <rdfs:subClassOf rdf:resource="https://w3id.org/netbeheer/referentiemodellen/IECCIM/TC57CIM/IEC61970/Dynamics/StandardModels/WindDynamics#WindTurbineType1or2IEC"/>
        <rdfs:subClassOf>
            <owl:Restriction>
                <owl:onProperty rdf:resource="https://w3id.org/netbeheer/referentiemodellen/IECCIM/TC57CIM/IEC61970/Dynamics/StandardModels/WindDynamics#WindGenTurbineType2IEC_WindContRotorRIEC"/>
                <owl:qualifiedCardinality rdf:datatype="http://www.w3.org/2001/XMLSchema#nonNegativeInteger">1</owl:qualifiedCardinality>
                <owl:onClass rdf:resource="https://w3id.org/netbeheer/referentiemodellen/IECCIM/TC57CIM/IEC61970/Dynamics/StandardModels/WindDynamics#WindGenTurbineType2IEC"/>
            </owl:Restriction>
        </rdfs:subClassOf>
        <rdfs:subClassOf>
            <owl:Restriction>
                <owl:onProperty rdf:resource="https://w3id.org/netbeheer/referentiemodellen/IECCIM/TC57CIM/IEC61970/Dynamics/StandardModels/WindDynamics#WindGenTurbineType2IEC_WindPitchContEmulIEC"/>
                <owl:qualifiedCardinality rdf:datatype="http://www.w3.org/2001/XMLSchema#nonNegativeInteger">1</owl:qualifiedCardinality>
                <owl:onClass rdf:resource="https://w3id.org/netbeheer/referentiemodellen/IECCIM/TC57CIM/IEC61970/Dynamics/StandardModels/WindDynamics#WindGenTurbineType2IEC"/>
            </owl:Restriction>
        </rdfs:subClassOf>
        <rdfs:comment>Wind turbine IEC Type 2.

Reference: IEC Standard 61400-27-1, section 6.5.3.</rdfs:comment>
    </owl:Class>
    


    <!-- https://w3id.org/netbeheer/referentiemodellen/IECCIM/TC57CIM/IEC61970/Dynamics/StandardModels/WindDynamics#WindGenTurbineType3IEC -->


    <owl:Class rdf:about="https://w3id.org/netbeheer/referentiemodellen/IECCIM/TC57CIM/IEC61970/Dynamics/StandardModels/WindDynamics#WindGenTurbineType3IEC">
        <rdfs:subClassOf rdf:resource="https://w3id.org/netbeheer/referentiemodellen/IECCIM/TC57CIM/IEC61970/Dynamics/StandardModels/WindDynamics#WindTurbineType3or4IEC"/>
        <rdfs:subClassOf>
            <owl:Restriction>
                <owl:onProperty rdf:resource="https://w3id.org/netbeheer/referentiemodellen/IECCIM/TC57CIM/IEC61970/Dynamics/StandardModels/WindDynamics#WindGenTurbineType3IEC_WindMechIEC"/>
                <owl:minQualifiedCardinality rdf:datatype="http://www.w3.org/2001/XMLSchema#nonNegativeInteger">0</owl:minQualifiedCardinality>
                <owl:onClass rdf:resource="https://w3id.org/netbeheer/referentiemodellen/IECCIM/TC57CIM/IEC61970/Dynamics/StandardModels/WindDynamics#WindGenTurbineType3IEC"/>
            </owl:Restriction>
        </rdfs:subClassOf>
        <rdfs:subClassOf>
            <owl:Restriction>
                <owl:onProperty rdf:resource="https://w3id.org/netbeheer/referentiemodellen/IECCIM/TC57CIM/IEC61970/Dynamics/StandardModels/WindDynamics#WindGenTurbineType3IEC_dipmax"/>
                <owl:minQualifiedCardinality rdf:datatype="http://www.w3.org/2001/XMLSchema#nonNegativeInteger">0</owl:minQualifiedCardinality>
                <owl:onClass rdf:resource="https://w3id.org/netbeheer/referentiemodellen/IECCIM/TC57CIM/IEC61970/Base/Domain#PU"/>
            </owl:Restriction>
        </rdfs:subClassOf>
        <rdfs:subClassOf>
            <owl:Restriction>
                <owl:onProperty rdf:resource="https://w3id.org/netbeheer/referentiemodellen/IECCIM/TC57CIM/IEC61970/Dynamics/StandardModels/WindDynamics#WindGenTurbineType3IEC_diqmax"/>
                <owl:minQualifiedCardinality rdf:datatype="http://www.w3.org/2001/XMLSchema#nonNegativeInteger">0</owl:minQualifiedCardinality>
                <owl:onClass rdf:resource="https://w3id.org/netbeheer/referentiemodellen/IECCIM/TC57CIM/IEC61970/Base/Domain#PU"/>
            </owl:Restriction>
        </rdfs:subClassOf>
        <rdfs:subClassOf>
            <owl:Restriction>
                <owl:onProperty rdf:resource="https://w3id.org/netbeheer/referentiemodellen/IECCIM/TC57CIM/IEC61970/Dynamics/StandardModels/WindDynamics#WindGenTurbineType3IEC_WindAeroLinearIEC"/>
                <owl:qualifiedCardinality rdf:datatype="http://www.w3.org/2001/XMLSchema#nonNegativeInteger">1</owl:qualifiedCardinality>
                <owl:onClass rdf:resource="https://w3id.org/netbeheer/referentiemodellen/IECCIM/TC57CIM/IEC61970/Dynamics/StandardModels/WindDynamics#WindGenTurbineType3IEC"/>
            </owl:Restriction>
        </rdfs:subClassOf>
        <rdfs:subClassOf>
            <owl:Restriction>
                <owl:onProperty rdf:resource="https://w3id.org/netbeheer/referentiemodellen/IECCIM/TC57CIM/IEC61970/Dynamics/StandardModels/WindDynamics#WindGenTurbineType3IEC_WindContPType3IEC"/>
                <owl:qualifiedCardinality rdf:datatype="http://www.w3.org/2001/XMLSchema#nonNegativeInteger">1</owl:qualifiedCardinality>
                <owl:onClass rdf:resource="https://w3id.org/netbeheer/referentiemodellen/IECCIM/TC57CIM/IEC61970/Dynamics/StandardModels/WindDynamics#WindGenTurbineType3IEC"/>
            </owl:Restriction>
        </rdfs:subClassOf>
        <rdfs:subClassOf>
            <owl:Restriction>
                <owl:onProperty rdf:resource="https://w3id.org/netbeheer/referentiemodellen/IECCIM/TC57CIM/IEC61970/Dynamics/StandardModels/WindDynamics#WindGenTurbineType3IEC_WindContPitchAngleIEC"/>
                <owl:qualifiedCardinality rdf:datatype="http://www.w3.org/2001/XMLSchema#nonNegativeInteger">1</owl:qualifiedCardinality>
                <owl:onClass rdf:resource="https://w3id.org/netbeheer/referentiemodellen/IECCIM/TC57CIM/IEC61970/Dynamics/StandardModels/WindDynamics#WindGenTurbineType3IEC"/>
            </owl:Restriction>
        </rdfs:subClassOf>
        <rdfs:subClassOf>
            <owl:Restriction>
                <owl:onProperty rdf:resource="https://w3id.org/netbeheer/referentiemodellen/IECCIM/TC57CIM/IEC61970/Dynamics/StandardModels/WindDynamics#WindGenTurbineType3IEC_WindMechIEC"/>
                <owl:maxQualifiedCardinality rdf:datatype="http://www.w3.org/2001/XMLSchema#nonNegativeInteger">1</owl:maxQualifiedCardinality>
                <owl:onClass rdf:resource="https://w3id.org/netbeheer/referentiemodellen/IECCIM/TC57CIM/IEC61970/Dynamics/StandardModels/WindDynamics#WindGenTurbineType3IEC"/>
            </owl:Restriction>
        </rdfs:subClassOf>
        <rdfs:subClassOf>
            <owl:Restriction>
                <owl:onProperty rdf:resource="https://w3id.org/netbeheer/referentiemodellen/IECCIM/TC57CIM/IEC61970/Dynamics/StandardModels/WindDynamics#WindGenTurbineType3IEC_dipmax"/>
                <owl:maxQualifiedCardinality rdf:datatype="http://www.w3.org/2001/XMLSchema#nonNegativeInteger">1</owl:maxQualifiedCardinality>
                <owl:onClass rdf:resource="https://w3id.org/netbeheer/referentiemodellen/IECCIM/TC57CIM/IEC61970/Base/Domain#PU"/>
            </owl:Restriction>
        </rdfs:subClassOf>
        <rdfs:subClassOf>
            <owl:Restriction>
                <owl:onProperty rdf:resource="https://w3id.org/netbeheer/referentiemodellen/IECCIM/TC57CIM/IEC61970/Dynamics/StandardModels/WindDynamics#WindGenTurbineType3IEC_diqmax"/>
                <owl:maxQualifiedCardinality rdf:datatype="http://www.w3.org/2001/XMLSchema#nonNegativeInteger">1</owl:maxQualifiedCardinality>
                <owl:onClass rdf:resource="https://w3id.org/netbeheer/referentiemodellen/IECCIM/TC57CIM/IEC61970/Base/Domain#PU"/>
            </owl:Restriction>
        </rdfs:subClassOf>
        <rdfs:comment>Generator model for wind turbines of IEC type 3A and 3B.</rdfs:comment>
    </owl:Class>
    


    <!-- https://w3id.org/netbeheer/referentiemodellen/IECCIM/TC57CIM/IEC61970/Dynamics/StandardModels/WindDynamics#WindGenTurbineType3aIEC -->


    <owl:Class rdf:about="https://w3id.org/netbeheer/referentiemodellen/IECCIM/TC57CIM/IEC61970/Dynamics/StandardModels/WindDynamics#WindGenTurbineType3aIEC">
        <rdfs:subClassOf rdf:resource="https://w3id.org/netbeheer/referentiemodellen/IECCIM/TC57CIM/IEC61970/Dynamics/StandardModels/WindDynamics#WindGenTurbineType3IEC"/>
        <rdfs:subClassOf>
            <owl:Restriction>
                <owl:onProperty rdf:resource="https://w3id.org/netbeheer/referentiemodellen/IECCIM/TC57CIM/IEC61970/Dynamics/StandardModels/WindDynamics#WindGenTurbineType3aIEC_tic"/>
                <owl:minQualifiedCardinality rdf:datatype="http://www.w3.org/2001/XMLSchema#nonNegativeInteger">0</owl:minQualifiedCardinality>
                <owl:onClass rdf:resource="https://w3id.org/netbeheer/referentiemodellen/IECCIM/TC57CIM/IEC61970/Base/Domain#Seconds"/>
            </owl:Restriction>
        </rdfs:subClassOf>
        <rdfs:subClassOf>
            <owl:Restriction>
                <owl:onProperty rdf:resource="https://w3id.org/netbeheer/referentiemodellen/IECCIM/TC57CIM/IEC61970/Dynamics/StandardModels/WindDynamics#WindGenTurbineType3aIEC_xs"/>
                <owl:minQualifiedCardinality rdf:datatype="http://www.w3.org/2001/XMLSchema#nonNegativeInteger">0</owl:minQualifiedCardinality>
                <owl:onClass rdf:resource="https://w3id.org/netbeheer/referentiemodellen/IECCIM/TC57CIM/IEC61970/Base/Domain#PU"/>
            </owl:Restriction>
        </rdfs:subClassOf>
        <rdfs:subClassOf>
            <owl:Restriction>
                <owl:onProperty rdf:resource="https://w3id.org/netbeheer/referentiemodellen/IECCIM/TC57CIM/IEC61970/Dynamics/StandardModels/WindDynamics#WindGenTurbineType3aIEC_tic"/>
                <owl:maxQualifiedCardinality rdf:datatype="http://www.w3.org/2001/XMLSchema#nonNegativeInteger">1</owl:maxQualifiedCardinality>
                <owl:onClass rdf:resource="https://w3id.org/netbeheer/referentiemodellen/IECCIM/TC57CIM/IEC61970/Base/Domain#Seconds"/>
            </owl:Restriction>
        </rdfs:subClassOf>
        <rdfs:subClassOf>
            <owl:Restriction>
                <owl:onProperty rdf:resource="https://w3id.org/netbeheer/referentiemodellen/IECCIM/TC57CIM/IEC61970/Dynamics/StandardModels/WindDynamics#WindGenTurbineType3aIEC_xs"/>
                <owl:maxQualifiedCardinality rdf:datatype="http://www.w3.org/2001/XMLSchema#nonNegativeInteger">1</owl:maxQualifiedCardinality>
                <owl:onClass rdf:resource="https://w3id.org/netbeheer/referentiemodellen/IECCIM/TC57CIM/IEC61970/Base/Domain#PU"/>
            </owl:Restriction>
        </rdfs:subClassOf>
        <rdfs:subClassOf>
            <owl:Restriction>
                <owl:onProperty rdf:resource="https://w3id.org/netbeheer/referentiemodellen/IECCIM/TC57CIM/IEC61970/Dynamics/StandardModels/WindDynamics#WindGenTurbineType3aIEC_kpc"/>
                <owl:minQualifiedCardinality rdf:datatype="http://www.w3.org/2001/XMLSchema#nonNegativeInteger">0</owl:minQualifiedCardinality>
                <owl:onDataRange rdf:resource="http://www.w3.org/2001/XMLSchema#float"/>
            </owl:Restriction>
        </rdfs:subClassOf>
        <rdfs:subClassOf>
            <owl:Restriction>
                <owl:onProperty rdf:resource="https://w3id.org/netbeheer/referentiemodellen/IECCIM/TC57CIM/IEC61970/Dynamics/StandardModels/WindDynamics#WindGenTurbineType3aIEC_kpc"/>
                <owl:maxQualifiedCardinality rdf:datatype="http://www.w3.org/2001/XMLSchema#nonNegativeInteger">1</owl:maxQualifiedCardinality>
                <owl:onDataRange rdf:resource="http://www.w3.org/2001/XMLSchema#float"/>
            </owl:Restriction>
        </rdfs:subClassOf>
        <rdfs:comment>IEC Type 3A generator set model.

Reference: IEC Standard 61400-27-1 Section 6.6.3.2.</rdfs:comment>
    </owl:Class>
    


    <!-- https://w3id.org/netbeheer/referentiemodellen/IECCIM/TC57CIM/IEC61970/Dynamics/StandardModels/WindDynamics#WindGenTurbineType3bIEC -->


    <owl:Class rdf:about="https://w3id.org/netbeheer/referentiemodellen/IECCIM/TC57CIM/IEC61970/Dynamics/StandardModels/WindDynamics#WindGenTurbineType3bIEC">
        <rdfs:subClassOf rdf:resource="https://w3id.org/netbeheer/referentiemodellen/IECCIM/TC57CIM/IEC61970/Dynamics/StandardModels/WindDynamics#WindGenTurbineType3IEC"/>
        <rdfs:subClassOf>
            <owl:Restriction>
                <owl:onProperty rdf:resource="https://w3id.org/netbeheer/referentiemodellen/IECCIM/TC57CIM/IEC61970/Dynamics/StandardModels/WindDynamics#WindGenTurbineType3bIEC_tg"/>
                <owl:minQualifiedCardinality rdf:datatype="http://www.w3.org/2001/XMLSchema#nonNegativeInteger">0</owl:minQualifiedCardinality>
                <owl:onClass rdf:resource="https://w3id.org/netbeheer/referentiemodellen/IECCIM/TC57CIM/IEC61970/Base/Domain#Seconds"/>
            </owl:Restriction>
        </rdfs:subClassOf>
        <rdfs:subClassOf>
            <owl:Restriction>
                <owl:onProperty rdf:resource="https://w3id.org/netbeheer/referentiemodellen/IECCIM/TC57CIM/IEC61970/Dynamics/StandardModels/WindDynamics#WindGenTurbineType3bIEC_two"/>
                <owl:minQualifiedCardinality rdf:datatype="http://www.w3.org/2001/XMLSchema#nonNegativeInteger">0</owl:minQualifiedCardinality>
                <owl:onClass rdf:resource="https://w3id.org/netbeheer/referentiemodellen/IECCIM/TC57CIM/IEC61970/Base/Domain#Seconds"/>
            </owl:Restriction>
        </rdfs:subClassOf>
        <rdfs:subClassOf>
            <owl:Restriction>
                <owl:onProperty rdf:resource="https://w3id.org/netbeheer/referentiemodellen/IECCIM/TC57CIM/IEC61970/Dynamics/StandardModels/WindDynamics#WindGenTurbineType3bIEC_xs"/>
                <owl:minQualifiedCardinality rdf:datatype="http://www.w3.org/2001/XMLSchema#nonNegativeInteger">0</owl:minQualifiedCardinality>
                <owl:onClass rdf:resource="https://w3id.org/netbeheer/referentiemodellen/IECCIM/TC57CIM/IEC61970/Base/Domain#PU"/>
            </owl:Restriction>
        </rdfs:subClassOf>
        <rdfs:subClassOf>
            <owl:Restriction>
                <owl:onProperty rdf:resource="https://w3id.org/netbeheer/referentiemodellen/IECCIM/TC57CIM/IEC61970/Dynamics/StandardModels/WindDynamics#WindGenTurbineType3bIEC_tg"/>
                <owl:maxQualifiedCardinality rdf:datatype="http://www.w3.org/2001/XMLSchema#nonNegativeInteger">1</owl:maxQualifiedCardinality>
                <owl:onClass rdf:resource="https://w3id.org/netbeheer/referentiemodellen/IECCIM/TC57CIM/IEC61970/Base/Domain#Seconds"/>
            </owl:Restriction>
        </rdfs:subClassOf>
        <rdfs:subClassOf>
            <owl:Restriction>
                <owl:onProperty rdf:resource="https://w3id.org/netbeheer/referentiemodellen/IECCIM/TC57CIM/IEC61970/Dynamics/StandardModels/WindDynamics#WindGenTurbineType3bIEC_two"/>
                <owl:maxQualifiedCardinality rdf:datatype="http://www.w3.org/2001/XMLSchema#nonNegativeInteger">1</owl:maxQualifiedCardinality>
                <owl:onClass rdf:resource="https://w3id.org/netbeheer/referentiemodellen/IECCIM/TC57CIM/IEC61970/Base/Domain#Seconds"/>
            </owl:Restriction>
        </rdfs:subClassOf>
        <rdfs:subClassOf>
            <owl:Restriction>
                <owl:onProperty rdf:resource="https://w3id.org/netbeheer/referentiemodellen/IECCIM/TC57CIM/IEC61970/Dynamics/StandardModels/WindDynamics#WindGenTurbineType3bIEC_xs"/>
                <owl:maxQualifiedCardinality rdf:datatype="http://www.w3.org/2001/XMLSchema#nonNegativeInteger">1</owl:maxQualifiedCardinality>
                <owl:onClass rdf:resource="https://w3id.org/netbeheer/referentiemodellen/IECCIM/TC57CIM/IEC61970/Base/Domain#PU"/>
            </owl:Restriction>
        </rdfs:subClassOf>
        <rdfs:subClassOf>
            <owl:Restriction>
                <owl:onProperty rdf:resource="https://w3id.org/netbeheer/referentiemodellen/IECCIM/TC57CIM/IEC61970/Dynamics/StandardModels/WindDynamics#WindGenTurbineType3bIEC_fducw"/>
                <owl:minQualifiedCardinality rdf:datatype="http://www.w3.org/2001/XMLSchema#nonNegativeInteger">0</owl:minQualifiedCardinality>
                <owl:onDataRange rdf:resource="http://www.w3.org/2001/XMLSchema#float"/>
            </owl:Restriction>
        </rdfs:subClassOf>
        <rdfs:subClassOf>
            <owl:Restriction>
                <owl:onProperty rdf:resource="https://w3id.org/netbeheer/referentiemodellen/IECCIM/TC57CIM/IEC61970/Dynamics/StandardModels/WindDynamics#WindGenTurbineType3bIEC_mwtcwp"/>
                <owl:minQualifiedCardinality rdf:datatype="http://www.w3.org/2001/XMLSchema#nonNegativeInteger">0</owl:minQualifiedCardinality>
                <owl:onDataRange rdf:resource="http://www.w3.org/2001/XMLSchema#boolean"/>
            </owl:Restriction>
        </rdfs:subClassOf>
        <rdfs:subClassOf>
            <owl:Restriction>
                <owl:onProperty rdf:resource="https://w3id.org/netbeheer/referentiemodellen/IECCIM/TC57CIM/IEC61970/Dynamics/StandardModels/WindDynamics#WindGenTurbineType3bIEC_fducw"/>
                <owl:maxQualifiedCardinality rdf:datatype="http://www.w3.org/2001/XMLSchema#nonNegativeInteger">1</owl:maxQualifiedCardinality>
                <owl:onDataRange rdf:resource="http://www.w3.org/2001/XMLSchema#float"/>
            </owl:Restriction>
        </rdfs:subClassOf>
        <rdfs:subClassOf>
            <owl:Restriction>
                <owl:onProperty rdf:resource="https://w3id.org/netbeheer/referentiemodellen/IECCIM/TC57CIM/IEC61970/Dynamics/StandardModels/WindDynamics#WindGenTurbineType3bIEC_mwtcwp"/>
                <owl:maxQualifiedCardinality rdf:datatype="http://www.w3.org/2001/XMLSchema#nonNegativeInteger">1</owl:maxQualifiedCardinality>
                <owl:onDataRange rdf:resource="http://www.w3.org/2001/XMLSchema#boolean"/>
            </owl:Restriction>
        </rdfs:subClassOf>
        <rdfs:comment>IEC Type 3B generator set model.

Reference: IEC Standard 61400-27-1 Section 6.6.3.3.</rdfs:comment>
    </owl:Class>
    


    <!-- https://w3id.org/netbeheer/referentiemodellen/IECCIM/TC57CIM/IEC61970/Dynamics/StandardModels/WindDynamics#WindGenType4IEC -->


    <owl:Class rdf:about="https://w3id.org/netbeheer/referentiemodellen/IECCIM/TC57CIM/IEC61970/Dynamics/StandardModels/WindDynamics#WindGenType4IEC">
        <rdfs:subClassOf rdf:resource="https://w3id.org/netbeheer/referentiemodellen/IECCIM/TC57CIM/IEC61970/Dynamics/StandardModels/WindDynamics#WindTurbineType3or4IEC"/>
        <rdfs:subClassOf>
            <owl:Restriction>
                <owl:onProperty rdf:resource="https://w3id.org/netbeheer/referentiemodellen/IECCIM/TC57CIM/IEC61970/Dynamics/StandardModels/WindDynamics#WindGenType4IEC_dipmax"/>
                <owl:minQualifiedCardinality rdf:datatype="http://www.w3.org/2001/XMLSchema#nonNegativeInteger">0</owl:minQualifiedCardinality>
                <owl:onClass rdf:resource="https://w3id.org/netbeheer/referentiemodellen/IECCIM/TC57CIM/IEC61970/Base/Domain#PU"/>
            </owl:Restriction>
        </rdfs:subClassOf>
        <rdfs:subClassOf>
            <owl:Restriction>
                <owl:onProperty rdf:resource="https://w3id.org/netbeheer/referentiemodellen/IECCIM/TC57CIM/IEC61970/Dynamics/StandardModels/WindDynamics#WindGenType4IEC_diqmax"/>
                <owl:minQualifiedCardinality rdf:datatype="http://www.w3.org/2001/XMLSchema#nonNegativeInteger">0</owl:minQualifiedCardinality>
                <owl:onClass rdf:resource="https://w3id.org/netbeheer/referentiemodellen/IECCIM/TC57CIM/IEC61970/Base/Domain#PU"/>
            </owl:Restriction>
        </rdfs:subClassOf>
        <rdfs:subClassOf>
            <owl:Restriction>
                <owl:onProperty rdf:resource="https://w3id.org/netbeheer/referentiemodellen/IECCIM/TC57CIM/IEC61970/Dynamics/StandardModels/WindDynamics#WindGenType4IEC_diqmin"/>
                <owl:minQualifiedCardinality rdf:datatype="http://www.w3.org/2001/XMLSchema#nonNegativeInteger">0</owl:minQualifiedCardinality>
                <owl:onClass rdf:resource="https://w3id.org/netbeheer/referentiemodellen/IECCIM/TC57CIM/IEC61970/Base/Domain#PU"/>
            </owl:Restriction>
        </rdfs:subClassOf>
        <rdfs:subClassOf>
            <owl:Restriction>
                <owl:onProperty rdf:resource="https://w3id.org/netbeheer/referentiemodellen/IECCIM/TC57CIM/IEC61970/Dynamics/StandardModels/WindDynamics#WindGenType4IEC_tg"/>
                <owl:minQualifiedCardinality rdf:datatype="http://www.w3.org/2001/XMLSchema#nonNegativeInteger">0</owl:minQualifiedCardinality>
                <owl:onClass rdf:resource="https://w3id.org/netbeheer/referentiemodellen/IECCIM/TC57CIM/IEC61970/Base/Domain#Seconds"/>
            </owl:Restriction>
        </rdfs:subClassOf>
        <rdfs:subClassOf>
            <owl:Restriction>
                <owl:onProperty rdf:resource="https://w3id.org/netbeheer/referentiemodellen/IECCIM/TC57CIM/IEC61970/Dynamics/StandardModels/WindDynamics#WindGenType4IEC_dipmax"/>
                <owl:maxQualifiedCardinality rdf:datatype="http://www.w3.org/2001/XMLSchema#nonNegativeInteger">1</owl:maxQualifiedCardinality>
                <owl:onClass rdf:resource="https://w3id.org/netbeheer/referentiemodellen/IECCIM/TC57CIM/IEC61970/Base/Domain#PU"/>
            </owl:Restriction>
        </rdfs:subClassOf>
        <rdfs:subClassOf>
            <owl:Restriction>
                <owl:onProperty rdf:resource="https://w3id.org/netbeheer/referentiemodellen/IECCIM/TC57CIM/IEC61970/Dynamics/StandardModels/WindDynamics#WindGenType4IEC_diqmax"/>
                <owl:maxQualifiedCardinality rdf:datatype="http://www.w3.org/2001/XMLSchema#nonNegativeInteger">1</owl:maxQualifiedCardinality>
                <owl:onClass rdf:resource="https://w3id.org/netbeheer/referentiemodellen/IECCIM/TC57CIM/IEC61970/Base/Domain#PU"/>
            </owl:Restriction>
        </rdfs:subClassOf>
        <rdfs:subClassOf>
            <owl:Restriction>
                <owl:onProperty rdf:resource="https://w3id.org/netbeheer/referentiemodellen/IECCIM/TC57CIM/IEC61970/Dynamics/StandardModels/WindDynamics#WindGenType4IEC_diqmin"/>
                <owl:maxQualifiedCardinality rdf:datatype="http://www.w3.org/2001/XMLSchema#nonNegativeInteger">1</owl:maxQualifiedCardinality>
                <owl:onClass rdf:resource="https://w3id.org/netbeheer/referentiemodellen/IECCIM/TC57CIM/IEC61970/Base/Domain#PU"/>
            </owl:Restriction>
        </rdfs:subClassOf>
        <rdfs:subClassOf>
            <owl:Restriction>
                <owl:onProperty rdf:resource="https://w3id.org/netbeheer/referentiemodellen/IECCIM/TC57CIM/IEC61970/Dynamics/StandardModels/WindDynamics#WindGenType4IEC_tg"/>
                <owl:maxQualifiedCardinality rdf:datatype="http://www.w3.org/2001/XMLSchema#nonNegativeInteger">1</owl:maxQualifiedCardinality>
                <owl:onClass rdf:resource="https://w3id.org/netbeheer/referentiemodellen/IECCIM/TC57CIM/IEC61970/Base/Domain#Seconds"/>
            </owl:Restriction>
        </rdfs:subClassOf>
        <rdfs:comment>IEC Type 4 generator set model.

Reference: IEC Standard 61400-27-1 Section 6.6.3.4.</rdfs:comment>
    </owl:Class>
    


    <!-- https://w3id.org/netbeheer/referentiemodellen/IECCIM/TC57CIM/IEC61970/Dynamics/StandardModels/WindDynamics#WindMechIEC -->


    <owl:Class rdf:about="https://w3id.org/netbeheer/referentiemodellen/IECCIM/TC57CIM/IEC61970/Dynamics/StandardModels/WindDynamics#WindMechIEC">
        <rdfs:subClassOf rdf:resource="https://w3id.org/netbeheer/referentiemodellen/IECCIM/TC57CIM/IEC61970/Base/Core#IdentifiedObject"/>
        <rdfs:subClassOf>
            <owl:Restriction>
                <owl:onProperty rdf:resource="https://w3id.org/netbeheer/referentiemodellen/IECCIM/TC57CIM/IEC61970/Dynamics/StandardModels/WindDynamics#WindMechIEC_cdrt"/>
                <owl:minQualifiedCardinality rdf:datatype="http://www.w3.org/2001/XMLSchema#nonNegativeInteger">0</owl:minQualifiedCardinality>
                <owl:onClass rdf:resource="https://w3id.org/netbeheer/referentiemodellen/IECCIM/TC57CIM/IEC61970/Base/Domain#PU"/>
            </owl:Restriction>
        </rdfs:subClassOf>
        <rdfs:subClassOf>
            <owl:Restriction>
                <owl:onProperty rdf:resource="https://w3id.org/netbeheer/referentiemodellen/IECCIM/TC57CIM/IEC61970/Dynamics/StandardModels/WindDynamics#WindMechIEC_hgen"/>
                <owl:minQualifiedCardinality rdf:datatype="http://www.w3.org/2001/XMLSchema#nonNegativeInteger">0</owl:minQualifiedCardinality>
                <owl:onClass rdf:resource="https://w3id.org/netbeheer/referentiemodellen/IECCIM/TC57CIM/IEC61970/Base/Domain#Seconds"/>
            </owl:Restriction>
        </rdfs:subClassOf>
        <rdfs:subClassOf>
            <owl:Restriction>
                <owl:onProperty rdf:resource="https://w3id.org/netbeheer/referentiemodellen/IECCIM/TC57CIM/IEC61970/Dynamics/StandardModels/WindDynamics#WindMechIEC_hwtr"/>
                <owl:minQualifiedCardinality rdf:datatype="http://www.w3.org/2001/XMLSchema#nonNegativeInteger">0</owl:minQualifiedCardinality>
                <owl:onClass rdf:resource="https://w3id.org/netbeheer/referentiemodellen/IECCIM/TC57CIM/IEC61970/Base/Domain#Seconds"/>
            </owl:Restriction>
        </rdfs:subClassOf>
        <rdfs:subClassOf>
            <owl:Restriction>
                <owl:onProperty rdf:resource="https://w3id.org/netbeheer/referentiemodellen/IECCIM/TC57CIM/IEC61970/Dynamics/StandardModels/WindDynamics#WindMechIEC_kdrt"/>
                <owl:minQualifiedCardinality rdf:datatype="http://www.w3.org/2001/XMLSchema#nonNegativeInteger">0</owl:minQualifiedCardinality>
                <owl:onClass rdf:resource="https://w3id.org/netbeheer/referentiemodellen/IECCIM/TC57CIM/IEC61970/Base/Domain#PU"/>
            </owl:Restriction>
        </rdfs:subClassOf>
        <rdfs:subClassOf>
            <owl:Restriction>
                <owl:onProperty rdf:resource="https://w3id.org/netbeheer/referentiemodellen/IECCIM/TC57CIM/IEC61970/Dynamics/StandardModels/WindDynamics#WindMechIEC_WindGenTurbineType3IEC"/>
                <owl:qualifiedCardinality rdf:datatype="http://www.w3.org/2001/XMLSchema#nonNegativeInteger">1</owl:qualifiedCardinality>
                <owl:onClass rdf:resource="https://w3id.org/netbeheer/referentiemodellen/IECCIM/TC57CIM/IEC61970/Dynamics/StandardModels/WindDynamics#WindMechIEC"/>
            </owl:Restriction>
        </rdfs:subClassOf>
        <rdfs:subClassOf>
            <owl:Restriction>
                <owl:onProperty rdf:resource="https://w3id.org/netbeheer/referentiemodellen/IECCIM/TC57CIM/IEC61970/Dynamics/StandardModels/WindDynamics#WindMechIEC_WindTurbineType1or2IEC"/>
                <owl:qualifiedCardinality rdf:datatype="http://www.w3.org/2001/XMLSchema#nonNegativeInteger">1</owl:qualifiedCardinality>
                <owl:onClass rdf:resource="https://w3id.org/netbeheer/referentiemodellen/IECCIM/TC57CIM/IEC61970/Dynamics/StandardModels/WindDynamics#WindMechIEC"/>
            </owl:Restriction>
        </rdfs:subClassOf>
        <rdfs:subClassOf>
            <owl:Restriction>
                <owl:onProperty rdf:resource="https://w3id.org/netbeheer/referentiemodellen/IECCIM/TC57CIM/IEC61970/Dynamics/StandardModels/WindDynamics#WindMechIEC_WindTurbineType4bIEC"/>
                <owl:qualifiedCardinality rdf:datatype="http://www.w3.org/2001/XMLSchema#nonNegativeInteger">1</owl:qualifiedCardinality>
                <owl:onClass rdf:resource="https://w3id.org/netbeheer/referentiemodellen/IECCIM/TC57CIM/IEC61970/Dynamics/StandardModels/WindDynamics#WindMechIEC"/>
            </owl:Restriction>
        </rdfs:subClassOf>
        <rdfs:subClassOf>
            <owl:Restriction>
                <owl:onProperty rdf:resource="https://w3id.org/netbeheer/referentiemodellen/IECCIM/TC57CIM/IEC61970/Dynamics/StandardModels/WindDynamics#WindMechIEC_cdrt"/>
                <owl:maxQualifiedCardinality rdf:datatype="http://www.w3.org/2001/XMLSchema#nonNegativeInteger">1</owl:maxQualifiedCardinality>
                <owl:onClass rdf:resource="https://w3id.org/netbeheer/referentiemodellen/IECCIM/TC57CIM/IEC61970/Base/Domain#PU"/>
            </owl:Restriction>
        </rdfs:subClassOf>
        <rdfs:subClassOf>
            <owl:Restriction>
                <owl:onProperty rdf:resource="https://w3id.org/netbeheer/referentiemodellen/IECCIM/TC57CIM/IEC61970/Dynamics/StandardModels/WindDynamics#WindMechIEC_hgen"/>
                <owl:maxQualifiedCardinality rdf:datatype="http://www.w3.org/2001/XMLSchema#nonNegativeInteger">1</owl:maxQualifiedCardinality>
                <owl:onClass rdf:resource="https://w3id.org/netbeheer/referentiemodellen/IECCIM/TC57CIM/IEC61970/Base/Domain#Seconds"/>
            </owl:Restriction>
        </rdfs:subClassOf>
        <rdfs:subClassOf>
            <owl:Restriction>
                <owl:onProperty rdf:resource="https://w3id.org/netbeheer/referentiemodellen/IECCIM/TC57CIM/IEC61970/Dynamics/StandardModels/WindDynamics#WindMechIEC_hwtr"/>
                <owl:maxQualifiedCardinality rdf:datatype="http://www.w3.org/2001/XMLSchema#nonNegativeInteger">1</owl:maxQualifiedCardinality>
                <owl:onClass rdf:resource="https://w3id.org/netbeheer/referentiemodellen/IECCIM/TC57CIM/IEC61970/Base/Domain#Seconds"/>
            </owl:Restriction>
        </rdfs:subClassOf>
        <rdfs:subClassOf>
            <owl:Restriction>
                <owl:onProperty rdf:resource="https://w3id.org/netbeheer/referentiemodellen/IECCIM/TC57CIM/IEC61970/Dynamics/StandardModels/WindDynamics#WindMechIEC_kdrt"/>
                <owl:maxQualifiedCardinality rdf:datatype="http://www.w3.org/2001/XMLSchema#nonNegativeInteger">1</owl:maxQualifiedCardinality>
                <owl:onClass rdf:resource="https://w3id.org/netbeheer/referentiemodellen/IECCIM/TC57CIM/IEC61970/Base/Domain#PU"/>
            </owl:Restriction>
        </rdfs:subClassOf>
        <rdfs:comment>Two mass model.

Reference: IEC Standard 61400-27-1 Section 6.6.2.1.</rdfs:comment>
    </owl:Class>
    


    <!-- https://w3id.org/netbeheer/referentiemodellen/IECCIM/TC57CIM/IEC61970/Dynamics/StandardModels/WindDynamics#WindPitchContEmulIEC -->


    <owl:Class rdf:about="https://w3id.org/netbeheer/referentiemodellen/IECCIM/TC57CIM/IEC61970/Dynamics/StandardModels/WindDynamics#WindPitchContEmulIEC">
        <rdfs:subClassOf rdf:resource="https://w3id.org/netbeheer/referentiemodellen/IECCIM/TC57CIM/IEC61970/Base/Core#IdentifiedObject"/>
        <rdfs:subClassOf>
            <owl:Restriction>
                <owl:onProperty rdf:resource="https://w3id.org/netbeheer/referentiemodellen/IECCIM/TC57CIM/IEC61970/Dynamics/StandardModels/WindDynamics#WindPitchContEmulIEC_komegaaero"/>
                <owl:minQualifiedCardinality rdf:datatype="http://www.w3.org/2001/XMLSchema#nonNegativeInteger">0</owl:minQualifiedCardinality>
                <owl:onClass rdf:resource="https://w3id.org/netbeheer/referentiemodellen/IECCIM/TC57CIM/IEC61970/Base/Domain#PU"/>
            </owl:Restriction>
        </rdfs:subClassOf>
        <rdfs:subClassOf>
            <owl:Restriction>
                <owl:onProperty rdf:resource="https://w3id.org/netbeheer/referentiemodellen/IECCIM/TC57CIM/IEC61970/Dynamics/StandardModels/WindDynamics#WindPitchContEmulIEC_omegaref"/>
                <owl:minQualifiedCardinality rdf:datatype="http://www.w3.org/2001/XMLSchema#nonNegativeInteger">0</owl:minQualifiedCardinality>
                <owl:onClass rdf:resource="https://w3id.org/netbeheer/referentiemodellen/IECCIM/TC57CIM/IEC61970/Base/Domain#PU"/>
            </owl:Restriction>
        </rdfs:subClassOf>
        <rdfs:subClassOf>
            <owl:Restriction>
                <owl:onProperty rdf:resource="https://w3id.org/netbeheer/referentiemodellen/IECCIM/TC57CIM/IEC61970/Dynamics/StandardModels/WindDynamics#WindPitchContEmulIEC_pimax"/>
                <owl:minQualifiedCardinality rdf:datatype="http://www.w3.org/2001/XMLSchema#nonNegativeInteger">0</owl:minQualifiedCardinality>
                <owl:onClass rdf:resource="https://w3id.org/netbeheer/referentiemodellen/IECCIM/TC57CIM/IEC61970/Base/Domain#PU"/>
            </owl:Restriction>
        </rdfs:subClassOf>
        <rdfs:subClassOf>
            <owl:Restriction>
                <owl:onProperty rdf:resource="https://w3id.org/netbeheer/referentiemodellen/IECCIM/TC57CIM/IEC61970/Dynamics/StandardModels/WindDynamics#WindPitchContEmulIEC_pimin"/>
                <owl:minQualifiedCardinality rdf:datatype="http://www.w3.org/2001/XMLSchema#nonNegativeInteger">0</owl:minQualifiedCardinality>
                <owl:onClass rdf:resource="https://w3id.org/netbeheer/referentiemodellen/IECCIM/TC57CIM/IEC61970/Base/Domain#PU"/>
            </owl:Restriction>
        </rdfs:subClassOf>
        <rdfs:subClassOf>
            <owl:Restriction>
                <owl:onProperty rdf:resource="https://w3id.org/netbeheer/referentiemodellen/IECCIM/TC57CIM/IEC61970/Dynamics/StandardModels/WindDynamics#WindPitchContEmulIEC_t1"/>
                <owl:minQualifiedCardinality rdf:datatype="http://www.w3.org/2001/XMLSchema#nonNegativeInteger">0</owl:minQualifiedCardinality>
                <owl:onClass rdf:resource="https://w3id.org/netbeheer/referentiemodellen/IECCIM/TC57CIM/IEC61970/Base/Domain#Seconds"/>
            </owl:Restriction>
        </rdfs:subClassOf>
        <rdfs:subClassOf>
            <owl:Restriction>
                <owl:onProperty rdf:resource="https://w3id.org/netbeheer/referentiemodellen/IECCIM/TC57CIM/IEC61970/Dynamics/StandardModels/WindDynamics#WindPitchContEmulIEC_t2"/>
                <owl:minQualifiedCardinality rdf:datatype="http://www.w3.org/2001/XMLSchema#nonNegativeInteger">0</owl:minQualifiedCardinality>
                <owl:onClass rdf:resource="https://w3id.org/netbeheer/referentiemodellen/IECCIM/TC57CIM/IEC61970/Base/Domain#Seconds"/>
            </owl:Restriction>
        </rdfs:subClassOf>
        <rdfs:subClassOf>
            <owl:Restriction>
                <owl:onProperty rdf:resource="https://w3id.org/netbeheer/referentiemodellen/IECCIM/TC57CIM/IEC61970/Dynamics/StandardModels/WindDynamics#WindPitchContEmulIEC_tpe"/>
                <owl:minQualifiedCardinality rdf:datatype="http://www.w3.org/2001/XMLSchema#nonNegativeInteger">0</owl:minQualifiedCardinality>
                <owl:onClass rdf:resource="https://w3id.org/netbeheer/referentiemodellen/IECCIM/TC57CIM/IEC61970/Base/Domain#Seconds"/>
            </owl:Restriction>
        </rdfs:subClassOf>
        <rdfs:subClassOf>
            <owl:Restriction>
                <owl:onProperty rdf:resource="https://w3id.org/netbeheer/referentiemodellen/IECCIM/TC57CIM/IEC61970/Dynamics/StandardModels/WindDynamics#WindPitchContEmulIEC_WindGenTurbineType2IEC"/>
                <owl:qualifiedCardinality rdf:datatype="http://www.w3.org/2001/XMLSchema#nonNegativeInteger">1</owl:qualifiedCardinality>
                <owl:onClass rdf:resource="https://w3id.org/netbeheer/referentiemodellen/IECCIM/TC57CIM/IEC61970/Dynamics/StandardModels/WindDynamics#WindPitchContEmulIEC"/>
            </owl:Restriction>
        </rdfs:subClassOf>
        <rdfs:subClassOf>
            <owl:Restriction>
                <owl:onProperty rdf:resource="https://w3id.org/netbeheer/referentiemodellen/IECCIM/TC57CIM/IEC61970/Dynamics/StandardModels/WindDynamics#WindPitchContEmulIEC_komegaaero"/>
                <owl:maxQualifiedCardinality rdf:datatype="http://www.w3.org/2001/XMLSchema#nonNegativeInteger">1</owl:maxQualifiedCardinality>
                <owl:onClass rdf:resource="https://w3id.org/netbeheer/referentiemodellen/IECCIM/TC57CIM/IEC61970/Base/Domain#PU"/>
            </owl:Restriction>
        </rdfs:subClassOf>
        <rdfs:subClassOf>
            <owl:Restriction>
                <owl:onProperty rdf:resource="https://w3id.org/netbeheer/referentiemodellen/IECCIM/TC57CIM/IEC61970/Dynamics/StandardModels/WindDynamics#WindPitchContEmulIEC_omegaref"/>
                <owl:maxQualifiedCardinality rdf:datatype="http://www.w3.org/2001/XMLSchema#nonNegativeInteger">1</owl:maxQualifiedCardinality>
                <owl:onClass rdf:resource="https://w3id.org/netbeheer/referentiemodellen/IECCIM/TC57CIM/IEC61970/Base/Domain#PU"/>
            </owl:Restriction>
        </rdfs:subClassOf>
        <rdfs:subClassOf>
            <owl:Restriction>
                <owl:onProperty rdf:resource="https://w3id.org/netbeheer/referentiemodellen/IECCIM/TC57CIM/IEC61970/Dynamics/StandardModels/WindDynamics#WindPitchContEmulIEC_pimax"/>
                <owl:maxQualifiedCardinality rdf:datatype="http://www.w3.org/2001/XMLSchema#nonNegativeInteger">1</owl:maxQualifiedCardinality>
                <owl:onClass rdf:resource="https://w3id.org/netbeheer/referentiemodellen/IECCIM/TC57CIM/IEC61970/Base/Domain#PU"/>
            </owl:Restriction>
        </rdfs:subClassOf>
        <rdfs:subClassOf>
            <owl:Restriction>
                <owl:onProperty rdf:resource="https://w3id.org/netbeheer/referentiemodellen/IECCIM/TC57CIM/IEC61970/Dynamics/StandardModels/WindDynamics#WindPitchContEmulIEC_pimin"/>
                <owl:maxQualifiedCardinality rdf:datatype="http://www.w3.org/2001/XMLSchema#nonNegativeInteger">1</owl:maxQualifiedCardinality>
                <owl:onClass rdf:resource="https://w3id.org/netbeheer/referentiemodellen/IECCIM/TC57CIM/IEC61970/Base/Domain#PU"/>
            </owl:Restriction>
        </rdfs:subClassOf>
        <rdfs:subClassOf>
            <owl:Restriction>
                <owl:onProperty rdf:resource="https://w3id.org/netbeheer/referentiemodellen/IECCIM/TC57CIM/IEC61970/Dynamics/StandardModels/WindDynamics#WindPitchContEmulIEC_t1"/>
                <owl:maxQualifiedCardinality rdf:datatype="http://www.w3.org/2001/XMLSchema#nonNegativeInteger">1</owl:maxQualifiedCardinality>
                <owl:onClass rdf:resource="https://w3id.org/netbeheer/referentiemodellen/IECCIM/TC57CIM/IEC61970/Base/Domain#Seconds"/>
            </owl:Restriction>
        </rdfs:subClassOf>
        <rdfs:subClassOf>
            <owl:Restriction>
                <owl:onProperty rdf:resource="https://w3id.org/netbeheer/referentiemodellen/IECCIM/TC57CIM/IEC61970/Dynamics/StandardModels/WindDynamics#WindPitchContEmulIEC_t2"/>
                <owl:maxQualifiedCardinality rdf:datatype="http://www.w3.org/2001/XMLSchema#nonNegativeInteger">1</owl:maxQualifiedCardinality>
                <owl:onClass rdf:resource="https://w3id.org/netbeheer/referentiemodellen/IECCIM/TC57CIM/IEC61970/Base/Domain#Seconds"/>
            </owl:Restriction>
        </rdfs:subClassOf>
        <rdfs:subClassOf>
            <owl:Restriction>
                <owl:onProperty rdf:resource="https://w3id.org/netbeheer/referentiemodellen/IECCIM/TC57CIM/IEC61970/Dynamics/StandardModels/WindDynamics#WindPitchContEmulIEC_tpe"/>
                <owl:maxQualifiedCardinality rdf:datatype="http://www.w3.org/2001/XMLSchema#nonNegativeInteger">1</owl:maxQualifiedCardinality>
                <owl:onClass rdf:resource="https://w3id.org/netbeheer/referentiemodellen/IECCIM/TC57CIM/IEC61970/Base/Domain#Seconds"/>
            </owl:Restriction>
        </rdfs:subClassOf>
        <rdfs:subClassOf>
            <owl:Restriction>
                <owl:onProperty rdf:resource="https://w3id.org/netbeheer/referentiemodellen/IECCIM/TC57CIM/IEC61970/Dynamics/StandardModels/WindDynamics#WindPitchContEmulIEC_kdroop"/>
                <owl:minQualifiedCardinality rdf:datatype="http://www.w3.org/2001/XMLSchema#nonNegativeInteger">0</owl:minQualifiedCardinality>
                <owl:onDataRange rdf:resource="http://www.w3.org/2001/XMLSchema#float"/>
            </owl:Restriction>
        </rdfs:subClassOf>
        <rdfs:subClassOf>
            <owl:Restriction>
                <owl:onProperty rdf:resource="https://w3id.org/netbeheer/referentiemodellen/IECCIM/TC57CIM/IEC61970/Dynamics/StandardModels/WindDynamics#WindPitchContEmulIEC_kipce"/>
                <owl:minQualifiedCardinality rdf:datatype="http://www.w3.org/2001/XMLSchema#nonNegativeInteger">0</owl:minQualifiedCardinality>
                <owl:onDataRange rdf:resource="http://www.w3.org/2001/XMLSchema#float"/>
            </owl:Restriction>
        </rdfs:subClassOf>
        <rdfs:subClassOf>
            <owl:Restriction>
                <owl:onProperty rdf:resource="https://w3id.org/netbeheer/referentiemodellen/IECCIM/TC57CIM/IEC61970/Dynamics/StandardModels/WindDynamics#WindPitchContEmulIEC_kppce"/>
                <owl:minQualifiedCardinality rdf:datatype="http://www.w3.org/2001/XMLSchema#nonNegativeInteger">0</owl:minQualifiedCardinality>
                <owl:onDataRange rdf:resource="http://www.w3.org/2001/XMLSchema#float"/>
            </owl:Restriction>
        </rdfs:subClassOf>
        <rdfs:subClassOf>
            <owl:Restriction>
                <owl:onProperty rdf:resource="https://w3id.org/netbeheer/referentiemodellen/IECCIM/TC57CIM/IEC61970/Dynamics/StandardModels/WindDynamics#WindPitchContEmulIEC_kdroop"/>
                <owl:maxQualifiedCardinality rdf:datatype="http://www.w3.org/2001/XMLSchema#nonNegativeInteger">1</owl:maxQualifiedCardinality>
                <owl:onDataRange rdf:resource="http://www.w3.org/2001/XMLSchema#float"/>
            </owl:Restriction>
        </rdfs:subClassOf>
        <rdfs:subClassOf>
            <owl:Restriction>
                <owl:onProperty rdf:resource="https://w3id.org/netbeheer/referentiemodellen/IECCIM/TC57CIM/IEC61970/Dynamics/StandardModels/WindDynamics#WindPitchContEmulIEC_kipce"/>
                <owl:maxQualifiedCardinality rdf:datatype="http://www.w3.org/2001/XMLSchema#nonNegativeInteger">1</owl:maxQualifiedCardinality>
                <owl:onDataRange rdf:resource="http://www.w3.org/2001/XMLSchema#float"/>
            </owl:Restriction>
        </rdfs:subClassOf>
        <rdfs:subClassOf>
            <owl:Restriction>
                <owl:onProperty rdf:resource="https://w3id.org/netbeheer/referentiemodellen/IECCIM/TC57CIM/IEC61970/Dynamics/StandardModels/WindDynamics#WindPitchContEmulIEC_kppce"/>
                <owl:maxQualifiedCardinality rdf:datatype="http://www.w3.org/2001/XMLSchema#nonNegativeInteger">1</owl:maxQualifiedCardinality>
                <owl:onDataRange rdf:resource="http://www.w3.org/2001/XMLSchema#float"/>
            </owl:Restriction>
        </rdfs:subClassOf>
        <rdfs:comment>Pitch control emulator model.

Reference: IEC Standard 61400-27-1 Section 6.6.5.1.</rdfs:comment>
    </owl:Class>
    


    <!-- https://w3id.org/netbeheer/referentiemodellen/IECCIM/TC57CIM/IEC61970/Dynamics/StandardModels/WindDynamics#WindPlantDynamics -->


    <owl:Class rdf:about="https://w3id.org/netbeheer/referentiemodellen/IECCIM/TC57CIM/IEC61970/Dynamics/StandardModels/WindDynamics#WindPlantDynamics">
        <rdfs:subClassOf rdf:resource="https://w3id.org/netbeheer/referentiemodellen/IECCIM/TC57CIM/IEC61970/Dynamics/StandardModels#DynamicsFunctionBlock"/>
        <rdfs:subClassOf>
            <owl:Restriction>
                <owl:onProperty rdf:resource="https://w3id.org/netbeheer/referentiemodellen/IECCIM/TC57CIM/IEC61970/Dynamics/StandardModels/WindDynamics#WindPlantDynamics_WindTurbineType3or4Dynamics"/>
                <owl:minQualifiedCardinality rdf:datatype="http://www.w3.org/2001/XMLSchema#nonNegativeInteger">0</owl:minQualifiedCardinality>
                <owl:onClass rdf:resource="https://w3id.org/netbeheer/referentiemodellen/IECCIM/TC57CIM/IEC61970/Dynamics/StandardModels/WindDynamics#WindPlantDynamics"/>
            </owl:Restriction>
        </rdfs:subClassOf>
        <rdfs:subClassOf>
            <owl:Restriction>
                <owl:onProperty rdf:resource="https://w3id.org/netbeheer/referentiemodellen/IECCIM/TC57CIM/IEC61970/Dynamics/StandardModels/WindDynamics#WindPlantDynamics_WindTurbineType3or4Dynamics"/>
                <owl:maxQualifiedCardinality rdf:datatype="http://www.w3.org/2001/XMLSchema#nonNegativeInteger">1</owl:maxQualifiedCardinality>
                <owl:onClass rdf:resource="https://w3id.org/netbeheer/referentiemodellen/IECCIM/TC57CIM/IEC61970/Dynamics/StandardModels/WindDynamics#WindPlantDynamics"/>
            </owl:Restriction>
        </rdfs:subClassOf>
        <rdfs:comment>Parent class supporting relationships to wind turbines Type 3 and 4 and wind plant IEC and user defined wind plants including their control models.</rdfs:comment>
    </owl:Class>
    


    <!-- https://w3id.org/netbeheer/referentiemodellen/IECCIM/TC57CIM/IEC61970/Dynamics/StandardModels/WindDynamics#WindPlantFreqPcontrolIEC -->


    <owl:Class rdf:about="https://w3id.org/netbeheer/referentiemodellen/IECCIM/TC57CIM/IEC61970/Dynamics/StandardModels/WindDynamics#WindPlantFreqPcontrolIEC">
        <rdfs:subClassOf rdf:resource="https://w3id.org/netbeheer/referentiemodellen/IECCIM/TC57CIM/IEC61970/Base/Core#IdentifiedObject"/>
        <rdfs:subClassOf>
            <owl:Restriction>
                <owl:onProperty rdf:resource="https://w3id.org/netbeheer/referentiemodellen/IECCIM/TC57CIM/IEC61970/Dynamics/StandardModels/WindDynamics#WindPlantFreqPcontrolIEC_WindDynamicsLookupTable"/>
                <owl:minQualifiedCardinality rdf:datatype="http://www.w3.org/2001/XMLSchema#nonNegativeInteger">0</owl:minQualifiedCardinality>
                <owl:onClass rdf:resource="https://w3id.org/netbeheer/referentiemodellen/IECCIM/TC57CIM/IEC61970/Dynamics/StandardModels/WindDynamics#WindPlantFreqPcontrolIEC"/>
            </owl:Restriction>
        </rdfs:subClassOf>
        <rdfs:subClassOf>
            <owl:Restriction>
                <owl:onProperty rdf:resource="https://w3id.org/netbeheer/referentiemodellen/IECCIM/TC57CIM/IEC61970/Dynamics/StandardModels/WindDynamics#WindPlantFreqPcontrolIEC_dprefmax"/>
                <owl:minQualifiedCardinality rdf:datatype="http://www.w3.org/2001/XMLSchema#nonNegativeInteger">0</owl:minQualifiedCardinality>
                <owl:onClass rdf:resource="https://w3id.org/netbeheer/referentiemodellen/IECCIM/TC57CIM/IEC61970/Base/Domain#PU"/>
            </owl:Restriction>
        </rdfs:subClassOf>
        <rdfs:subClassOf>
            <owl:Restriction>
                <owl:onProperty rdf:resource="https://w3id.org/netbeheer/referentiemodellen/IECCIM/TC57CIM/IEC61970/Dynamics/StandardModels/WindDynamics#WindPlantFreqPcontrolIEC_dprefmin"/>
                <owl:minQualifiedCardinality rdf:datatype="http://www.w3.org/2001/XMLSchema#nonNegativeInteger">0</owl:minQualifiedCardinality>
                <owl:onClass rdf:resource="https://w3id.org/netbeheer/referentiemodellen/IECCIM/TC57CIM/IEC61970/Base/Domain#PU"/>
            </owl:Restriction>
        </rdfs:subClassOf>
        <rdfs:subClassOf>
            <owl:Restriction>
                <owl:onProperty rdf:resource="https://w3id.org/netbeheer/referentiemodellen/IECCIM/TC57CIM/IEC61970/Dynamics/StandardModels/WindDynamics#WindPlantFreqPcontrolIEC_prefmax"/>
                <owl:minQualifiedCardinality rdf:datatype="http://www.w3.org/2001/XMLSchema#nonNegativeInteger">0</owl:minQualifiedCardinality>
                <owl:onClass rdf:resource="https://w3id.org/netbeheer/referentiemodellen/IECCIM/TC57CIM/IEC61970/Base/Domain#PU"/>
            </owl:Restriction>
        </rdfs:subClassOf>
        <rdfs:subClassOf>
            <owl:Restriction>
                <owl:onProperty rdf:resource="https://w3id.org/netbeheer/referentiemodellen/IECCIM/TC57CIM/IEC61970/Dynamics/StandardModels/WindDynamics#WindPlantFreqPcontrolIEC_prefmin"/>
                <owl:minQualifiedCardinality rdf:datatype="http://www.w3.org/2001/XMLSchema#nonNegativeInteger">0</owl:minQualifiedCardinality>
                <owl:onClass rdf:resource="https://w3id.org/netbeheer/referentiemodellen/IECCIM/TC57CIM/IEC61970/Base/Domain#PU"/>
            </owl:Restriction>
        </rdfs:subClassOf>
        <rdfs:subClassOf>
            <owl:Restriction>
                <owl:onProperty rdf:resource="https://w3id.org/netbeheer/referentiemodellen/IECCIM/TC57CIM/IEC61970/Dynamics/StandardModels/WindDynamics#WindPlantFreqPcontrolIEC_tpft"/>
                <owl:minQualifiedCardinality rdf:datatype="http://www.w3.org/2001/XMLSchema#nonNegativeInteger">0</owl:minQualifiedCardinality>
                <owl:onClass rdf:resource="https://w3id.org/netbeheer/referentiemodellen/IECCIM/TC57CIM/IEC61970/Base/Domain#Seconds"/>
            </owl:Restriction>
        </rdfs:subClassOf>
        <rdfs:subClassOf>
            <owl:Restriction>
                <owl:onProperty rdf:resource="https://w3id.org/netbeheer/referentiemodellen/IECCIM/TC57CIM/IEC61970/Dynamics/StandardModels/WindDynamics#WindPlantFreqPcontrolIEC_tpfv"/>
                <owl:minQualifiedCardinality rdf:datatype="http://www.w3.org/2001/XMLSchema#nonNegativeInteger">0</owl:minQualifiedCardinality>
                <owl:onClass rdf:resource="https://w3id.org/netbeheer/referentiemodellen/IECCIM/TC57CIM/IEC61970/Base/Domain#Seconds"/>
            </owl:Restriction>
        </rdfs:subClassOf>
        <rdfs:subClassOf>
            <owl:Restriction>
                <owl:onProperty rdf:resource="https://w3id.org/netbeheer/referentiemodellen/IECCIM/TC57CIM/IEC61970/Dynamics/StandardModels/WindDynamics#WindPlantFreqPcontrolIEC_twpffilt"/>
                <owl:minQualifiedCardinality rdf:datatype="http://www.w3.org/2001/XMLSchema#nonNegativeInteger">0</owl:minQualifiedCardinality>
                <owl:onClass rdf:resource="https://w3id.org/netbeheer/referentiemodellen/IECCIM/TC57CIM/IEC61970/Base/Domain#Seconds"/>
            </owl:Restriction>
        </rdfs:subClassOf>
        <rdfs:subClassOf>
            <owl:Restriction>
                <owl:onProperty rdf:resource="https://w3id.org/netbeheer/referentiemodellen/IECCIM/TC57CIM/IEC61970/Dynamics/StandardModels/WindDynamics#WindPlantFreqPcontrolIEC_twppfilt"/>
                <owl:minQualifiedCardinality rdf:datatype="http://www.w3.org/2001/XMLSchema#nonNegativeInteger">0</owl:minQualifiedCardinality>
                <owl:onClass rdf:resource="https://w3id.org/netbeheer/referentiemodellen/IECCIM/TC57CIM/IEC61970/Base/Domain#Seconds"/>
            </owl:Restriction>
        </rdfs:subClassOf>
        <rdfs:subClassOf>
            <owl:Restriction>
                <owl:onProperty rdf:resource="https://w3id.org/netbeheer/referentiemodellen/IECCIM/TC57CIM/IEC61970/Dynamics/StandardModels/WindDynamics#WindPlantFreqPcontrolIEC_WindPlantIEC"/>
                <owl:qualifiedCardinality rdf:datatype="http://www.w3.org/2001/XMLSchema#nonNegativeInteger">1</owl:qualifiedCardinality>
                <owl:onClass rdf:resource="https://w3id.org/netbeheer/referentiemodellen/IECCIM/TC57CIM/IEC61970/Dynamics/StandardModels/WindDynamics#WindPlantFreqPcontrolIEC"/>
            </owl:Restriction>
        </rdfs:subClassOf>
        <rdfs:subClassOf>
            <owl:Restriction>
                <owl:onProperty rdf:resource="https://w3id.org/netbeheer/referentiemodellen/IECCIM/TC57CIM/IEC61970/Dynamics/StandardModels/WindDynamics#WindPlantFreqPcontrolIEC_WindDynamicsLookupTable"/>
                <owl:maxQualifiedCardinality rdf:datatype="http://www.w3.org/2001/XMLSchema#nonNegativeInteger">1</owl:maxQualifiedCardinality>
                <owl:onClass rdf:resource="https://w3id.org/netbeheer/referentiemodellen/IECCIM/TC57CIM/IEC61970/Dynamics/StandardModels/WindDynamics#WindPlantFreqPcontrolIEC"/>
            </owl:Restriction>
        </rdfs:subClassOf>
        <rdfs:subClassOf>
            <owl:Restriction>
                <owl:onProperty rdf:resource="https://w3id.org/netbeheer/referentiemodellen/IECCIM/TC57CIM/IEC61970/Dynamics/StandardModels/WindDynamics#WindPlantFreqPcontrolIEC_dprefmax"/>
                <owl:maxQualifiedCardinality rdf:datatype="http://www.w3.org/2001/XMLSchema#nonNegativeInteger">1</owl:maxQualifiedCardinality>
                <owl:onClass rdf:resource="https://w3id.org/netbeheer/referentiemodellen/IECCIM/TC57CIM/IEC61970/Base/Domain#PU"/>
            </owl:Restriction>
        </rdfs:subClassOf>
        <rdfs:subClassOf>
            <owl:Restriction>
                <owl:onProperty rdf:resource="https://w3id.org/netbeheer/referentiemodellen/IECCIM/TC57CIM/IEC61970/Dynamics/StandardModels/WindDynamics#WindPlantFreqPcontrolIEC_dprefmin"/>
                <owl:maxQualifiedCardinality rdf:datatype="http://www.w3.org/2001/XMLSchema#nonNegativeInteger">1</owl:maxQualifiedCardinality>
                <owl:onClass rdf:resource="https://w3id.org/netbeheer/referentiemodellen/IECCIM/TC57CIM/IEC61970/Base/Domain#PU"/>
            </owl:Restriction>
        </rdfs:subClassOf>
        <rdfs:subClassOf>
            <owl:Restriction>
                <owl:onProperty rdf:resource="https://w3id.org/netbeheer/referentiemodellen/IECCIM/TC57CIM/IEC61970/Dynamics/StandardModels/WindDynamics#WindPlantFreqPcontrolIEC_prefmax"/>
                <owl:maxQualifiedCardinality rdf:datatype="http://www.w3.org/2001/XMLSchema#nonNegativeInteger">1</owl:maxQualifiedCardinality>
                <owl:onClass rdf:resource="https://w3id.org/netbeheer/referentiemodellen/IECCIM/TC57CIM/IEC61970/Base/Domain#PU"/>
            </owl:Restriction>
        </rdfs:subClassOf>
        <rdfs:subClassOf>
            <owl:Restriction>
                <owl:onProperty rdf:resource="https://w3id.org/netbeheer/referentiemodellen/IECCIM/TC57CIM/IEC61970/Dynamics/StandardModels/WindDynamics#WindPlantFreqPcontrolIEC_prefmin"/>
                <owl:maxQualifiedCardinality rdf:datatype="http://www.w3.org/2001/XMLSchema#nonNegativeInteger">1</owl:maxQualifiedCardinality>
                <owl:onClass rdf:resource="https://w3id.org/netbeheer/referentiemodellen/IECCIM/TC57CIM/IEC61970/Base/Domain#PU"/>
            </owl:Restriction>
        </rdfs:subClassOf>
        <rdfs:subClassOf>
            <owl:Restriction>
                <owl:onProperty rdf:resource="https://w3id.org/netbeheer/referentiemodellen/IECCIM/TC57CIM/IEC61970/Dynamics/StandardModels/WindDynamics#WindPlantFreqPcontrolIEC_tpft"/>
                <owl:maxQualifiedCardinality rdf:datatype="http://www.w3.org/2001/XMLSchema#nonNegativeInteger">1</owl:maxQualifiedCardinality>
                <owl:onClass rdf:resource="https://w3id.org/netbeheer/referentiemodellen/IECCIM/TC57CIM/IEC61970/Base/Domain#Seconds"/>
            </owl:Restriction>
        </rdfs:subClassOf>
        <rdfs:subClassOf>
            <owl:Restriction>
                <owl:onProperty rdf:resource="https://w3id.org/netbeheer/referentiemodellen/IECCIM/TC57CIM/IEC61970/Dynamics/StandardModels/WindDynamics#WindPlantFreqPcontrolIEC_tpfv"/>
                <owl:maxQualifiedCardinality rdf:datatype="http://www.w3.org/2001/XMLSchema#nonNegativeInteger">1</owl:maxQualifiedCardinality>
                <owl:onClass rdf:resource="https://w3id.org/netbeheer/referentiemodellen/IECCIM/TC57CIM/IEC61970/Base/Domain#Seconds"/>
            </owl:Restriction>
        </rdfs:subClassOf>
        <rdfs:subClassOf>
            <owl:Restriction>
                <owl:onProperty rdf:resource="https://w3id.org/netbeheer/referentiemodellen/IECCIM/TC57CIM/IEC61970/Dynamics/StandardModels/WindDynamics#WindPlantFreqPcontrolIEC_twpffilt"/>
                <owl:maxQualifiedCardinality rdf:datatype="http://www.w3.org/2001/XMLSchema#nonNegativeInteger">1</owl:maxQualifiedCardinality>
                <owl:onClass rdf:resource="https://w3id.org/netbeheer/referentiemodellen/IECCIM/TC57CIM/IEC61970/Base/Domain#Seconds"/>
            </owl:Restriction>
        </rdfs:subClassOf>
        <rdfs:subClassOf>
            <owl:Restriction>
                <owl:onProperty rdf:resource="https://w3id.org/netbeheer/referentiemodellen/IECCIM/TC57CIM/IEC61970/Dynamics/StandardModels/WindDynamics#WindPlantFreqPcontrolIEC_twppfilt"/>
                <owl:maxQualifiedCardinality rdf:datatype="http://www.w3.org/2001/XMLSchema#nonNegativeInteger">1</owl:maxQualifiedCardinality>
                <owl:onClass rdf:resource="https://w3id.org/netbeheer/referentiemodellen/IECCIM/TC57CIM/IEC61970/Base/Domain#Seconds"/>
            </owl:Restriction>
        </rdfs:subClassOf>
        <rdfs:subClassOf>
            <owl:Restriction>
                <owl:onProperty rdf:resource="https://w3id.org/netbeheer/referentiemodellen/IECCIM/TC57CIM/IEC61970/Dynamics/StandardModels/WindDynamics#WindPlantFreqPcontrolIEC_kiwpp"/>
                <owl:minQualifiedCardinality rdf:datatype="http://www.w3.org/2001/XMLSchema#nonNegativeInteger">0</owl:minQualifiedCardinality>
                <owl:onDataRange rdf:resource="http://www.w3.org/2001/XMLSchema#float"/>
            </owl:Restriction>
        </rdfs:subClassOf>
        <rdfs:subClassOf>
            <owl:Restriction>
                <owl:onProperty rdf:resource="https://w3id.org/netbeheer/referentiemodellen/IECCIM/TC57CIM/IEC61970/Dynamics/StandardModels/WindDynamics#WindPlantFreqPcontrolIEC_kpwpp"/>
                <owl:minQualifiedCardinality rdf:datatype="http://www.w3.org/2001/XMLSchema#nonNegativeInteger">0</owl:minQualifiedCardinality>
                <owl:onDataRange rdf:resource="http://www.w3.org/2001/XMLSchema#float"/>
            </owl:Restriction>
        </rdfs:subClassOf>
        <rdfs:subClassOf>
            <owl:Restriction>
                <owl:onProperty rdf:resource="https://w3id.org/netbeheer/referentiemodellen/IECCIM/TC57CIM/IEC61970/Dynamics/StandardModels/WindDynamics#WindPlantFreqPcontrolIEC_kiwpp"/>
                <owl:maxQualifiedCardinality rdf:datatype="http://www.w3.org/2001/XMLSchema#nonNegativeInteger">1</owl:maxQualifiedCardinality>
                <owl:onDataRange rdf:resource="http://www.w3.org/2001/XMLSchema#float"/>
            </owl:Restriction>
        </rdfs:subClassOf>
        <rdfs:subClassOf>
            <owl:Restriction>
                <owl:onProperty rdf:resource="https://w3id.org/netbeheer/referentiemodellen/IECCIM/TC57CIM/IEC61970/Dynamics/StandardModels/WindDynamics#WindPlantFreqPcontrolIEC_kpwpp"/>
                <owl:maxQualifiedCardinality rdf:datatype="http://www.w3.org/2001/XMLSchema#nonNegativeInteger">1</owl:maxQualifiedCardinality>
                <owl:onDataRange rdf:resource="http://www.w3.org/2001/XMLSchema#float"/>
            </owl:Restriction>
        </rdfs:subClassOf>
        <rdfs:comment>Frequency and active power controller model.

Reference: IEC Standard 61400-27-1 Annex E.</rdfs:comment>
    </owl:Class>
    


    <!-- https://w3id.org/netbeheer/referentiemodellen/IECCIM/TC57CIM/IEC61970/Dynamics/StandardModels/WindDynamics#WindPlantIEC -->


    <owl:Class rdf:about="https://w3id.org/netbeheer/referentiemodellen/IECCIM/TC57CIM/IEC61970/Dynamics/StandardModels/WindDynamics#WindPlantIEC">
        <rdfs:subClassOf rdf:resource="https://w3id.org/netbeheer/referentiemodellen/IECCIM/TC57CIM/IEC61970/Dynamics/StandardModels/WindDynamics#WindPlantDynamics"/>
        <rdfs:subClassOf>
            <owl:Restriction>
                <owl:onProperty rdf:resource="https://w3id.org/netbeheer/referentiemodellen/IECCIM/TC57CIM/IEC61970/Dynamics/StandardModels/WindDynamics#WindPlantIEC_WindPlantFreqPcontrolIEC"/>
                <owl:qualifiedCardinality rdf:datatype="http://www.w3.org/2001/XMLSchema#nonNegativeInteger">1</owl:qualifiedCardinality>
                <owl:onClass rdf:resource="https://w3id.org/netbeheer/referentiemodellen/IECCIM/TC57CIM/IEC61970/Dynamics/StandardModels/WindDynamics#WindPlantIEC"/>
            </owl:Restriction>
        </rdfs:subClassOf>
        <rdfs:subClassOf>
            <owl:Restriction>
                <owl:onProperty rdf:resource="https://w3id.org/netbeheer/referentiemodellen/IECCIM/TC57CIM/IEC61970/Dynamics/StandardModels/WindDynamics#WindPlantIEC_WindPlantReactiveControlIEC"/>
                <owl:qualifiedCardinality rdf:datatype="http://www.w3.org/2001/XMLSchema#nonNegativeInteger">1</owl:qualifiedCardinality>
                <owl:onClass rdf:resource="https://w3id.org/netbeheer/referentiemodellen/IECCIM/TC57CIM/IEC61970/Dynamics/StandardModels/WindDynamics#WindPlantIEC"/>
            </owl:Restriction>
        </rdfs:subClassOf>
        <rdfs:comment>Simplified IEC type plant level model. 

Reference: IEC 61400-27-1, AnnexE.</rdfs:comment>
    </owl:Class>
    


    <!-- https://w3id.org/netbeheer/referentiemodellen/IECCIM/TC57CIM/IEC61970/Dynamics/StandardModels/WindDynamics#WindPlantReactiveControlIEC -->


    <owl:Class rdf:about="https://w3id.org/netbeheer/referentiemodellen/IECCIM/TC57CIM/IEC61970/Dynamics/StandardModels/WindDynamics#WindPlantReactiveControlIEC">
        <rdfs:subClassOf rdf:resource="https://w3id.org/netbeheer/referentiemodellen/IECCIM/TC57CIM/IEC61970/Base/Core#IdentifiedObject"/>
        <rdfs:subClassOf>
            <owl:Restriction>
                <owl:onProperty rdf:resource="https://w3id.org/netbeheer/referentiemodellen/IECCIM/TC57CIM/IEC61970/Dynamics/StandardModels/WindDynamics#WindPlantReactiveControlIEC_kwpqu"/>
                <owl:minQualifiedCardinality rdf:datatype="http://www.w3.org/2001/XMLSchema#nonNegativeInteger">0</owl:minQualifiedCardinality>
                <owl:onClass rdf:resource="https://w3id.org/netbeheer/referentiemodellen/IECCIM/TC57CIM/IEC61970/Base/Domain#PU"/>
            </owl:Restriction>
        </rdfs:subClassOf>
        <rdfs:subClassOf>
            <owl:Restriction>
                <owl:onProperty rdf:resource="https://w3id.org/netbeheer/referentiemodellen/IECCIM/TC57CIM/IEC61970/Dynamics/StandardModels/WindDynamics#WindPlantReactiveControlIEC_twppfilt"/>
                <owl:minQualifiedCardinality rdf:datatype="http://www.w3.org/2001/XMLSchema#nonNegativeInteger">0</owl:minQualifiedCardinality>
                <owl:onClass rdf:resource="https://w3id.org/netbeheer/referentiemodellen/IECCIM/TC57CIM/IEC61970/Base/Domain#Seconds"/>
            </owl:Restriction>
        </rdfs:subClassOf>
        <rdfs:subClassOf>
            <owl:Restriction>
                <owl:onProperty rdf:resource="https://w3id.org/netbeheer/referentiemodellen/IECCIM/TC57CIM/IEC61970/Dynamics/StandardModels/WindDynamics#WindPlantReactiveControlIEC_twpqfilt"/>
                <owl:minQualifiedCardinality rdf:datatype="http://www.w3.org/2001/XMLSchema#nonNegativeInteger">0</owl:minQualifiedCardinality>
                <owl:onClass rdf:resource="https://w3id.org/netbeheer/referentiemodellen/IECCIM/TC57CIM/IEC61970/Base/Domain#Seconds"/>
            </owl:Restriction>
        </rdfs:subClassOf>
        <rdfs:subClassOf>
            <owl:Restriction>
                <owl:onProperty rdf:resource="https://w3id.org/netbeheer/referentiemodellen/IECCIM/TC57CIM/IEC61970/Dynamics/StandardModels/WindDynamics#WindPlantReactiveControlIEC_twpufilt"/>
                <owl:minQualifiedCardinality rdf:datatype="http://www.w3.org/2001/XMLSchema#nonNegativeInteger">0</owl:minQualifiedCardinality>
                <owl:onClass rdf:resource="https://w3id.org/netbeheer/referentiemodellen/IECCIM/TC57CIM/IEC61970/Base/Domain#Seconds"/>
            </owl:Restriction>
        </rdfs:subClassOf>
        <rdfs:subClassOf>
            <owl:Restriction>
                <owl:onProperty rdf:resource="https://w3id.org/netbeheer/referentiemodellen/IECCIM/TC57CIM/IEC61970/Dynamics/StandardModels/WindDynamics#WindPlantReactiveControlIEC_txft"/>
                <owl:minQualifiedCardinality rdf:datatype="http://www.w3.org/2001/XMLSchema#nonNegativeInteger">0</owl:minQualifiedCardinality>
                <owl:onClass rdf:resource="https://w3id.org/netbeheer/referentiemodellen/IECCIM/TC57CIM/IEC61970/Base/Domain#Seconds"/>
            </owl:Restriction>
        </rdfs:subClassOf>
        <rdfs:subClassOf>
            <owl:Restriction>
                <owl:onProperty rdf:resource="https://w3id.org/netbeheer/referentiemodellen/IECCIM/TC57CIM/IEC61970/Dynamics/StandardModels/WindDynamics#WindPlantReactiveControlIEC_txfv"/>
                <owl:minQualifiedCardinality rdf:datatype="http://www.w3.org/2001/XMLSchema#nonNegativeInteger">0</owl:minQualifiedCardinality>
                <owl:onClass rdf:resource="https://w3id.org/netbeheer/referentiemodellen/IECCIM/TC57CIM/IEC61970/Base/Domain#Seconds"/>
            </owl:Restriction>
        </rdfs:subClassOf>
        <rdfs:subClassOf>
            <owl:Restriction>
                <owl:onProperty rdf:resource="https://w3id.org/netbeheer/referentiemodellen/IECCIM/TC57CIM/IEC61970/Dynamics/StandardModels/WindDynamics#WindPlantReactiveControlIEC_uwpqdip"/>
                <owl:minQualifiedCardinality rdf:datatype="http://www.w3.org/2001/XMLSchema#nonNegativeInteger">0</owl:minQualifiedCardinality>
                <owl:onClass rdf:resource="https://w3id.org/netbeheer/referentiemodellen/IECCIM/TC57CIM/IEC61970/Base/Domain#PU"/>
            </owl:Restriction>
        </rdfs:subClassOf>
        <rdfs:subClassOf>
            <owl:Restriction>
                <owl:onProperty rdf:resource="https://w3id.org/netbeheer/referentiemodellen/IECCIM/TC57CIM/IEC61970/Dynamics/StandardModels/WindDynamics#WindPlantReactiveControlIEC_xrefmax"/>
                <owl:minQualifiedCardinality rdf:datatype="http://www.w3.org/2001/XMLSchema#nonNegativeInteger">0</owl:minQualifiedCardinality>
                <owl:onClass rdf:resource="https://w3id.org/netbeheer/referentiemodellen/IECCIM/TC57CIM/IEC61970/Base/Domain#PU"/>
            </owl:Restriction>
        </rdfs:subClassOf>
        <rdfs:subClassOf>
            <owl:Restriction>
                <owl:onProperty rdf:resource="https://w3id.org/netbeheer/referentiemodellen/IECCIM/TC57CIM/IEC61970/Dynamics/StandardModels/WindDynamics#WindPlantReactiveControlIEC_xrefmin"/>
                <owl:minQualifiedCardinality rdf:datatype="http://www.w3.org/2001/XMLSchema#nonNegativeInteger">0</owl:minQualifiedCardinality>
                <owl:onClass rdf:resource="https://w3id.org/netbeheer/referentiemodellen/IECCIM/TC57CIM/IEC61970/Base/Domain#PU"/>
            </owl:Restriction>
        </rdfs:subClassOf>
        <rdfs:subClassOf>
            <owl:Restriction>
                <owl:onProperty rdf:resource="https://w3id.org/netbeheer/referentiemodellen/IECCIM/TC57CIM/IEC61970/Dynamics/StandardModels/WindDynamics#WindPlantReactiveControlIEC_WindPlantIEC"/>
                <owl:qualifiedCardinality rdf:datatype="http://www.w3.org/2001/XMLSchema#nonNegativeInteger">1</owl:qualifiedCardinality>
                <owl:onClass rdf:resource="https://w3id.org/netbeheer/referentiemodellen/IECCIM/TC57CIM/IEC61970/Dynamics/StandardModels/WindDynamics#WindPlantReactiveControlIEC"/>
            </owl:Restriction>
        </rdfs:subClassOf>
        <rdfs:subClassOf>
            <owl:Restriction>
                <owl:onProperty rdf:resource="https://w3id.org/netbeheer/referentiemodellen/IECCIM/TC57CIM/IEC61970/Dynamics/StandardModels/WindDynamics#WindPlantReactiveControlIEC_kwpqu"/>
                <owl:maxQualifiedCardinality rdf:datatype="http://www.w3.org/2001/XMLSchema#nonNegativeInteger">1</owl:maxQualifiedCardinality>
                <owl:onClass rdf:resource="https://w3id.org/netbeheer/referentiemodellen/IECCIM/TC57CIM/IEC61970/Base/Domain#PU"/>
            </owl:Restriction>
        </rdfs:subClassOf>
        <rdfs:subClassOf>
            <owl:Restriction>
                <owl:onProperty rdf:resource="https://w3id.org/netbeheer/referentiemodellen/IECCIM/TC57CIM/IEC61970/Dynamics/StandardModels/WindDynamics#WindPlantReactiveControlIEC_twppfilt"/>
                <owl:maxQualifiedCardinality rdf:datatype="http://www.w3.org/2001/XMLSchema#nonNegativeInteger">1</owl:maxQualifiedCardinality>
                <owl:onClass rdf:resource="https://w3id.org/netbeheer/referentiemodellen/IECCIM/TC57CIM/IEC61970/Base/Domain#Seconds"/>
            </owl:Restriction>
        </rdfs:subClassOf>
        <rdfs:subClassOf>
            <owl:Restriction>
                <owl:onProperty rdf:resource="https://w3id.org/netbeheer/referentiemodellen/IECCIM/TC57CIM/IEC61970/Dynamics/StandardModels/WindDynamics#WindPlantReactiveControlIEC_twpqfilt"/>
                <owl:maxQualifiedCardinality rdf:datatype="http://www.w3.org/2001/XMLSchema#nonNegativeInteger">1</owl:maxQualifiedCardinality>
                <owl:onClass rdf:resource="https://w3id.org/netbeheer/referentiemodellen/IECCIM/TC57CIM/IEC61970/Base/Domain#Seconds"/>
            </owl:Restriction>
        </rdfs:subClassOf>
        <rdfs:subClassOf>
            <owl:Restriction>
                <owl:onProperty rdf:resource="https://w3id.org/netbeheer/referentiemodellen/IECCIM/TC57CIM/IEC61970/Dynamics/StandardModels/WindDynamics#WindPlantReactiveControlIEC_twpufilt"/>
                <owl:maxQualifiedCardinality rdf:datatype="http://www.w3.org/2001/XMLSchema#nonNegativeInteger">1</owl:maxQualifiedCardinality>
                <owl:onClass rdf:resource="https://w3id.org/netbeheer/referentiemodellen/IECCIM/TC57CIM/IEC61970/Base/Domain#Seconds"/>
            </owl:Restriction>
        </rdfs:subClassOf>
        <rdfs:subClassOf>
            <owl:Restriction>
                <owl:onProperty rdf:resource="https://w3id.org/netbeheer/referentiemodellen/IECCIM/TC57CIM/IEC61970/Dynamics/StandardModels/WindDynamics#WindPlantReactiveControlIEC_txft"/>
                <owl:maxQualifiedCardinality rdf:datatype="http://www.w3.org/2001/XMLSchema#nonNegativeInteger">1</owl:maxQualifiedCardinality>
                <owl:onClass rdf:resource="https://w3id.org/netbeheer/referentiemodellen/IECCIM/TC57CIM/IEC61970/Base/Domain#Seconds"/>
            </owl:Restriction>
        </rdfs:subClassOf>
        <rdfs:subClassOf>
            <owl:Restriction>
                <owl:onProperty rdf:resource="https://w3id.org/netbeheer/referentiemodellen/IECCIM/TC57CIM/IEC61970/Dynamics/StandardModels/WindDynamics#WindPlantReactiveControlIEC_txfv"/>
                <owl:maxQualifiedCardinality rdf:datatype="http://www.w3.org/2001/XMLSchema#nonNegativeInteger">1</owl:maxQualifiedCardinality>
                <owl:onClass rdf:resource="https://w3id.org/netbeheer/referentiemodellen/IECCIM/TC57CIM/IEC61970/Base/Domain#Seconds"/>
            </owl:Restriction>
        </rdfs:subClassOf>
        <rdfs:subClassOf>
            <owl:Restriction>
                <owl:onProperty rdf:resource="https://w3id.org/netbeheer/referentiemodellen/IECCIM/TC57CIM/IEC61970/Dynamics/StandardModels/WindDynamics#WindPlantReactiveControlIEC_uwpqdip"/>
                <owl:maxQualifiedCardinality rdf:datatype="http://www.w3.org/2001/XMLSchema#nonNegativeInteger">1</owl:maxQualifiedCardinality>
                <owl:onClass rdf:resource="https://w3id.org/netbeheer/referentiemodellen/IECCIM/TC57CIM/IEC61970/Base/Domain#PU"/>
            </owl:Restriction>
        </rdfs:subClassOf>
        <rdfs:subClassOf>
            <owl:Restriction>
                <owl:onProperty rdf:resource="https://w3id.org/netbeheer/referentiemodellen/IECCIM/TC57CIM/IEC61970/Dynamics/StandardModels/WindDynamics#WindPlantReactiveControlIEC_xrefmax"/>
                <owl:maxQualifiedCardinality rdf:datatype="http://www.w3.org/2001/XMLSchema#nonNegativeInteger">1</owl:maxQualifiedCardinality>
                <owl:onClass rdf:resource="https://w3id.org/netbeheer/referentiemodellen/IECCIM/TC57CIM/IEC61970/Base/Domain#PU"/>
            </owl:Restriction>
        </rdfs:subClassOf>
        <rdfs:subClassOf>
            <owl:Restriction>
                <owl:onProperty rdf:resource="https://w3id.org/netbeheer/referentiemodellen/IECCIM/TC57CIM/IEC61970/Dynamics/StandardModels/WindDynamics#WindPlantReactiveControlIEC_xrefmin"/>
                <owl:maxQualifiedCardinality rdf:datatype="http://www.w3.org/2001/XMLSchema#nonNegativeInteger">1</owl:maxQualifiedCardinality>
                <owl:onClass rdf:resource="https://w3id.org/netbeheer/referentiemodellen/IECCIM/TC57CIM/IEC61970/Base/Domain#PU"/>
            </owl:Restriction>
        </rdfs:subClassOf>
        <rdfs:subClassOf>
            <owl:Restriction>
                <owl:onProperty rdf:resource="https://w3id.org/netbeheer/referentiemodellen/IECCIM/TC57CIM/IEC61970/Dynamics/StandardModels/WindDynamics#WindPlantReactiveControlIEC_kiwpx"/>
                <owl:minQualifiedCardinality rdf:datatype="http://www.w3.org/2001/XMLSchema#nonNegativeInteger">0</owl:minQualifiedCardinality>
                <owl:onDataRange rdf:resource="http://www.w3.org/2001/XMLSchema#float"/>
            </owl:Restriction>
        </rdfs:subClassOf>
        <rdfs:subClassOf>
            <owl:Restriction>
                <owl:onProperty rdf:resource="https://w3id.org/netbeheer/referentiemodellen/IECCIM/TC57CIM/IEC61970/Dynamics/StandardModels/WindDynamics#WindPlantReactiveControlIEC_kpwpx"/>
                <owl:minQualifiedCardinality rdf:datatype="http://www.w3.org/2001/XMLSchema#nonNegativeInteger">0</owl:minQualifiedCardinality>
                <owl:onDataRange rdf:resource="http://www.w3.org/2001/XMLSchema#float"/>
            </owl:Restriction>
        </rdfs:subClassOf>
        <rdfs:subClassOf>
            <owl:Restriction>
                <owl:onProperty rdf:resource="https://w3id.org/netbeheer/referentiemodellen/IECCIM/TC57CIM/IEC61970/Dynamics/StandardModels/WindDynamics#WindPlantReactiveControlIEC_mwppf"/>
                <owl:minQualifiedCardinality rdf:datatype="http://www.w3.org/2001/XMLSchema#nonNegativeInteger">0</owl:minQualifiedCardinality>
                <owl:onDataRange rdf:resource="http://www.w3.org/2001/XMLSchema#boolean"/>
            </owl:Restriction>
        </rdfs:subClassOf>
        <rdfs:subClassOf>
            <owl:Restriction>
                <owl:onProperty rdf:resource="https://w3id.org/netbeheer/referentiemodellen/IECCIM/TC57CIM/IEC61970/Dynamics/StandardModels/WindDynamics#WindPlantReactiveControlIEC_mwpu"/>
                <owl:minQualifiedCardinality rdf:datatype="http://www.w3.org/2001/XMLSchema#nonNegativeInteger">0</owl:minQualifiedCardinality>
                <owl:onDataRange rdf:resource="http://www.w3.org/2001/XMLSchema#boolean"/>
            </owl:Restriction>
        </rdfs:subClassOf>
        <rdfs:subClassOf>
            <owl:Restriction>
                <owl:onProperty rdf:resource="https://w3id.org/netbeheer/referentiemodellen/IECCIM/TC57CIM/IEC61970/Dynamics/StandardModels/WindDynamics#WindPlantReactiveControlIEC_kiwpx"/>
                <owl:maxQualifiedCardinality rdf:datatype="http://www.w3.org/2001/XMLSchema#nonNegativeInteger">1</owl:maxQualifiedCardinality>
                <owl:onDataRange rdf:resource="http://www.w3.org/2001/XMLSchema#float"/>
            </owl:Restriction>
        </rdfs:subClassOf>
        <rdfs:subClassOf>
            <owl:Restriction>
                <owl:onProperty rdf:resource="https://w3id.org/netbeheer/referentiemodellen/IECCIM/TC57CIM/IEC61970/Dynamics/StandardModels/WindDynamics#WindPlantReactiveControlIEC_kpwpx"/>
                <owl:maxQualifiedCardinality rdf:datatype="http://www.w3.org/2001/XMLSchema#nonNegativeInteger">1</owl:maxQualifiedCardinality>
                <owl:onDataRange rdf:resource="http://www.w3.org/2001/XMLSchema#float"/>
            </owl:Restriction>
        </rdfs:subClassOf>
        <rdfs:subClassOf>
            <owl:Restriction>
                <owl:onProperty rdf:resource="https://w3id.org/netbeheer/referentiemodellen/IECCIM/TC57CIM/IEC61970/Dynamics/StandardModels/WindDynamics#WindPlantReactiveControlIEC_mwppf"/>
                <owl:maxQualifiedCardinality rdf:datatype="http://www.w3.org/2001/XMLSchema#nonNegativeInteger">1</owl:maxQualifiedCardinality>
                <owl:onDataRange rdf:resource="http://www.w3.org/2001/XMLSchema#boolean"/>
            </owl:Restriction>
        </rdfs:subClassOf>
        <rdfs:subClassOf>
            <owl:Restriction>
                <owl:onProperty rdf:resource="https://w3id.org/netbeheer/referentiemodellen/IECCIM/TC57CIM/IEC61970/Dynamics/StandardModels/WindDynamics#WindPlantReactiveControlIEC_mwpu"/>
                <owl:maxQualifiedCardinality rdf:datatype="http://www.w3.org/2001/XMLSchema#nonNegativeInteger">1</owl:maxQualifiedCardinality>
                <owl:onDataRange rdf:resource="http://www.w3.org/2001/XMLSchema#boolean"/>
            </owl:Restriction>
        </rdfs:subClassOf>
        <rdfs:comment>Simplified plant voltage and reactive power control model for use with type 3 and type 4 wind turbine models.

Reference: IEC Standard 61400-27-1 Annex E.</rdfs:comment>
    </owl:Class>
    


    <!-- https://w3id.org/netbeheer/referentiemodellen/IECCIM/TC57CIM/IEC61970/Dynamics/StandardModels/WindDynamics#WindProtectionIEC -->


    <owl:Class rdf:about="https://w3id.org/netbeheer/referentiemodellen/IECCIM/TC57CIM/IEC61970/Dynamics/StandardModels/WindDynamics#WindProtectionIEC">
        <rdfs:subClassOf rdf:resource="https://w3id.org/netbeheer/referentiemodellen/IECCIM/TC57CIM/IEC61970/Base/Core#IdentifiedObject"/>
        <rdfs:subClassOf>
            <owl:Restriction>
                <owl:onProperty rdf:resource="https://w3id.org/netbeheer/referentiemodellen/IECCIM/TC57CIM/IEC61970/Dynamics/StandardModels/WindDynamics#WindProtectionIEC_fover"/>
                <owl:minQualifiedCardinality rdf:datatype="http://www.w3.org/2001/XMLSchema#nonNegativeInteger">0</owl:minQualifiedCardinality>
                <owl:onClass rdf:resource="https://w3id.org/netbeheer/referentiemodellen/IECCIM/TC57CIM/IEC61970/Base/Domain#PU"/>
            </owl:Restriction>
        </rdfs:subClassOf>
        <rdfs:subClassOf>
            <owl:Restriction>
                <owl:onProperty rdf:resource="https://w3id.org/netbeheer/referentiemodellen/IECCIM/TC57CIM/IEC61970/Dynamics/StandardModels/WindDynamics#WindProtectionIEC_funder"/>
                <owl:minQualifiedCardinality rdf:datatype="http://www.w3.org/2001/XMLSchema#nonNegativeInteger">0</owl:minQualifiedCardinality>
                <owl:onClass rdf:resource="https://w3id.org/netbeheer/referentiemodellen/IECCIM/TC57CIM/IEC61970/Base/Domain#PU"/>
            </owl:Restriction>
        </rdfs:subClassOf>
        <rdfs:subClassOf>
            <owl:Restriction>
                <owl:onProperty rdf:resource="https://w3id.org/netbeheer/referentiemodellen/IECCIM/TC57CIM/IEC61970/Dynamics/StandardModels/WindDynamics#WindProtectionIEC_tfover"/>
                <owl:minQualifiedCardinality rdf:datatype="http://www.w3.org/2001/XMLSchema#nonNegativeInteger">0</owl:minQualifiedCardinality>
                <owl:onClass rdf:resource="https://w3id.org/netbeheer/referentiemodellen/IECCIM/TC57CIM/IEC61970/Base/Domain#Seconds"/>
            </owl:Restriction>
        </rdfs:subClassOf>
        <rdfs:subClassOf>
            <owl:Restriction>
                <owl:onProperty rdf:resource="https://w3id.org/netbeheer/referentiemodellen/IECCIM/TC57CIM/IEC61970/Dynamics/StandardModels/WindDynamics#WindProtectionIEC_tfunder"/>
                <owl:minQualifiedCardinality rdf:datatype="http://www.w3.org/2001/XMLSchema#nonNegativeInteger">0</owl:minQualifiedCardinality>
                <owl:onClass rdf:resource="https://w3id.org/netbeheer/referentiemodellen/IECCIM/TC57CIM/IEC61970/Base/Domain#Seconds"/>
            </owl:Restriction>
        </rdfs:subClassOf>
        <rdfs:subClassOf>
            <owl:Restriction>
                <owl:onProperty rdf:resource="https://w3id.org/netbeheer/referentiemodellen/IECCIM/TC57CIM/IEC61970/Dynamics/StandardModels/WindDynamics#WindProtectionIEC_tuover"/>
                <owl:minQualifiedCardinality rdf:datatype="http://www.w3.org/2001/XMLSchema#nonNegativeInteger">0</owl:minQualifiedCardinality>
                <owl:onClass rdf:resource="https://w3id.org/netbeheer/referentiemodellen/IECCIM/TC57CIM/IEC61970/Base/Domain#Seconds"/>
            </owl:Restriction>
        </rdfs:subClassOf>
        <rdfs:subClassOf>
            <owl:Restriction>
                <owl:onProperty rdf:resource="https://w3id.org/netbeheer/referentiemodellen/IECCIM/TC57CIM/IEC61970/Dynamics/StandardModels/WindDynamics#WindProtectionIEC_tuunder"/>
                <owl:minQualifiedCardinality rdf:datatype="http://www.w3.org/2001/XMLSchema#nonNegativeInteger">0</owl:minQualifiedCardinality>
                <owl:onClass rdf:resource="https://w3id.org/netbeheer/referentiemodellen/IECCIM/TC57CIM/IEC61970/Base/Domain#Seconds"/>
            </owl:Restriction>
        </rdfs:subClassOf>
        <rdfs:subClassOf>
            <owl:Restriction>
                <owl:onProperty rdf:resource="https://w3id.org/netbeheer/referentiemodellen/IECCIM/TC57CIM/IEC61970/Dynamics/StandardModels/WindDynamics#WindProtectionIEC_uover"/>
                <owl:minQualifiedCardinality rdf:datatype="http://www.w3.org/2001/XMLSchema#nonNegativeInteger">0</owl:minQualifiedCardinality>
                <owl:onClass rdf:resource="https://w3id.org/netbeheer/referentiemodellen/IECCIM/TC57CIM/IEC61970/Base/Domain#PU"/>
            </owl:Restriction>
        </rdfs:subClassOf>
        <rdfs:subClassOf>
            <owl:Restriction>
                <owl:onProperty rdf:resource="https://w3id.org/netbeheer/referentiemodellen/IECCIM/TC57CIM/IEC61970/Dynamics/StandardModels/WindDynamics#WindProtectionIEC_uunder"/>
                <owl:minQualifiedCardinality rdf:datatype="http://www.w3.org/2001/XMLSchema#nonNegativeInteger">0</owl:minQualifiedCardinality>
                <owl:onClass rdf:resource="https://w3id.org/netbeheer/referentiemodellen/IECCIM/TC57CIM/IEC61970/Base/Domain#PU"/>
            </owl:Restriction>
        </rdfs:subClassOf>
        <rdfs:subClassOf>
            <owl:Restriction>
                <owl:onProperty rdf:resource="https://w3id.org/netbeheer/referentiemodellen/IECCIM/TC57CIM/IEC61970/Dynamics/StandardModels/WindDynamics#WindProtectionIEC_WindTurbineType1or2IEC"/>
                <owl:qualifiedCardinality rdf:datatype="http://www.w3.org/2001/XMLSchema#nonNegativeInteger">1</owl:qualifiedCardinality>
                <owl:onClass rdf:resource="https://w3id.org/netbeheer/referentiemodellen/IECCIM/TC57CIM/IEC61970/Dynamics/StandardModels/WindDynamics#WindProtectionIEC"/>
            </owl:Restriction>
        </rdfs:subClassOf>
        <rdfs:subClassOf>
            <owl:Restriction>
                <owl:onProperty rdf:resource="https://w3id.org/netbeheer/referentiemodellen/IECCIM/TC57CIM/IEC61970/Dynamics/StandardModels/WindDynamics#WindProtectionIEC_WindTurbineType3or4IEC"/>
                <owl:qualifiedCardinality rdf:datatype="http://www.w3.org/2001/XMLSchema#nonNegativeInteger">1</owl:qualifiedCardinality>
                <owl:onClass rdf:resource="https://w3id.org/netbeheer/referentiemodellen/IECCIM/TC57CIM/IEC61970/Dynamics/StandardModels/WindDynamics#WindProtectionIEC"/>
            </owl:Restriction>
        </rdfs:subClassOf>
        <rdfs:subClassOf>
            <owl:Restriction>
                <owl:onProperty rdf:resource="https://w3id.org/netbeheer/referentiemodellen/IECCIM/TC57CIM/IEC61970/Dynamics/StandardModels/WindDynamics#WindProtectionIEC_fover"/>
                <owl:maxQualifiedCardinality rdf:datatype="http://www.w3.org/2001/XMLSchema#nonNegativeInteger">1</owl:maxQualifiedCardinality>
                <owl:onClass rdf:resource="https://w3id.org/netbeheer/referentiemodellen/IECCIM/TC57CIM/IEC61970/Base/Domain#PU"/>
            </owl:Restriction>
        </rdfs:subClassOf>
        <rdfs:subClassOf>
            <owl:Restriction>
                <owl:onProperty rdf:resource="https://w3id.org/netbeheer/referentiemodellen/IECCIM/TC57CIM/IEC61970/Dynamics/StandardModels/WindDynamics#WindProtectionIEC_funder"/>
                <owl:maxQualifiedCardinality rdf:datatype="http://www.w3.org/2001/XMLSchema#nonNegativeInteger">1</owl:maxQualifiedCardinality>
                <owl:onClass rdf:resource="https://w3id.org/netbeheer/referentiemodellen/IECCIM/TC57CIM/IEC61970/Base/Domain#PU"/>
            </owl:Restriction>
        </rdfs:subClassOf>
        <rdfs:subClassOf>
            <owl:Restriction>
                <owl:onProperty rdf:resource="https://w3id.org/netbeheer/referentiemodellen/IECCIM/TC57CIM/IEC61970/Dynamics/StandardModels/WindDynamics#WindProtectionIEC_tfover"/>
                <owl:maxQualifiedCardinality rdf:datatype="http://www.w3.org/2001/XMLSchema#nonNegativeInteger">1</owl:maxQualifiedCardinality>
                <owl:onClass rdf:resource="https://w3id.org/netbeheer/referentiemodellen/IECCIM/TC57CIM/IEC61970/Base/Domain#Seconds"/>
            </owl:Restriction>
        </rdfs:subClassOf>
        <rdfs:subClassOf>
            <owl:Restriction>
                <owl:onProperty rdf:resource="https://w3id.org/netbeheer/referentiemodellen/IECCIM/TC57CIM/IEC61970/Dynamics/StandardModels/WindDynamics#WindProtectionIEC_tfunder"/>
                <owl:maxQualifiedCardinality rdf:datatype="http://www.w3.org/2001/XMLSchema#nonNegativeInteger">1</owl:maxQualifiedCardinality>
                <owl:onClass rdf:resource="https://w3id.org/netbeheer/referentiemodellen/IECCIM/TC57CIM/IEC61970/Base/Domain#Seconds"/>
            </owl:Restriction>
        </rdfs:subClassOf>
        <rdfs:subClassOf>
            <owl:Restriction>
                <owl:onProperty rdf:resource="https://w3id.org/netbeheer/referentiemodellen/IECCIM/TC57CIM/IEC61970/Dynamics/StandardModels/WindDynamics#WindProtectionIEC_tuover"/>
                <owl:maxQualifiedCardinality rdf:datatype="http://www.w3.org/2001/XMLSchema#nonNegativeInteger">1</owl:maxQualifiedCardinality>
                <owl:onClass rdf:resource="https://w3id.org/netbeheer/referentiemodellen/IECCIM/TC57CIM/IEC61970/Base/Domain#Seconds"/>
            </owl:Restriction>
        </rdfs:subClassOf>
        <rdfs:subClassOf>
            <owl:Restriction>
                <owl:onProperty rdf:resource="https://w3id.org/netbeheer/referentiemodellen/IECCIM/TC57CIM/IEC61970/Dynamics/StandardModels/WindDynamics#WindProtectionIEC_tuunder"/>
                <owl:maxQualifiedCardinality rdf:datatype="http://www.w3.org/2001/XMLSchema#nonNegativeInteger">1</owl:maxQualifiedCardinality>
                <owl:onClass rdf:resource="https://w3id.org/netbeheer/referentiemodellen/IECCIM/TC57CIM/IEC61970/Base/Domain#Seconds"/>
            </owl:Restriction>
        </rdfs:subClassOf>
        <rdfs:subClassOf>
            <owl:Restriction>
                <owl:onProperty rdf:resource="https://w3id.org/netbeheer/referentiemodellen/IECCIM/TC57CIM/IEC61970/Dynamics/StandardModels/WindDynamics#WindProtectionIEC_uover"/>
                <owl:maxQualifiedCardinality rdf:datatype="http://www.w3.org/2001/XMLSchema#nonNegativeInteger">1</owl:maxQualifiedCardinality>
                <owl:onClass rdf:resource="https://w3id.org/netbeheer/referentiemodellen/IECCIM/TC57CIM/IEC61970/Base/Domain#PU"/>
            </owl:Restriction>
        </rdfs:subClassOf>
        <rdfs:subClassOf>
            <owl:Restriction>
                <owl:onProperty rdf:resource="https://w3id.org/netbeheer/referentiemodellen/IECCIM/TC57CIM/IEC61970/Dynamics/StandardModels/WindDynamics#WindProtectionIEC_uunder"/>
                <owl:maxQualifiedCardinality rdf:datatype="http://www.w3.org/2001/XMLSchema#nonNegativeInteger">1</owl:maxQualifiedCardinality>
                <owl:onClass rdf:resource="https://w3id.org/netbeheer/referentiemodellen/IECCIM/TC57CIM/IEC61970/Base/Domain#PU"/>
            </owl:Restriction>
        </rdfs:subClassOf>
        <rdfs:comment>The grid protection model includes protection against over and under voltage, and against over and under frequency.

Reference: IEC Standard 614000-27-1 Section 6.6.6.</rdfs:comment>
    </owl:Class>
    


    <!-- https://w3id.org/netbeheer/referentiemodellen/IECCIM/TC57CIM/IEC61970/Dynamics/StandardModels/WindDynamics#WindTurbineType1or2Dynamics -->


    <owl:Class rdf:about="https://w3id.org/netbeheer/referentiemodellen/IECCIM/TC57CIM/IEC61970/Dynamics/StandardModels/WindDynamics#WindTurbineType1or2Dynamics">
        <rdfs:subClassOf rdf:resource="https://w3id.org/netbeheer/referentiemodellen/IECCIM/TC57CIM/IEC61970/Dynamics/StandardModels#DynamicsFunctionBlock"/>
        <rdfs:comment>Parent class supporting relationships to wind turbines Type 1 and 2 and their control models.</rdfs:comment>
    </owl:Class>
    


    <!-- https://w3id.org/netbeheer/referentiemodellen/IECCIM/TC57CIM/IEC61970/Dynamics/StandardModels/WindDynamics#WindTurbineType1or2IEC -->


    <owl:Class rdf:about="https://w3id.org/netbeheer/referentiemodellen/IECCIM/TC57CIM/IEC61970/Dynamics/StandardModels/WindDynamics#WindTurbineType1or2IEC">
        <rdfs:subClassOf rdf:resource="https://w3id.org/netbeheer/referentiemodellen/IECCIM/TC57CIM/IEC61970/Dynamics/StandardModels/WindDynamics#WindTurbineType1or2Dynamics"/>
        <rdfs:subClassOf>
            <owl:Restriction>
                <owl:onProperty rdf:resource="https://w3id.org/netbeheer/referentiemodellen/IECCIM/TC57CIM/IEC61970/Dynamics/StandardModels/WindDynamics#WindTurbineType1or2IEC_WindMechIEC"/>
                <owl:minQualifiedCardinality rdf:datatype="http://www.w3.org/2001/XMLSchema#nonNegativeInteger">0</owl:minQualifiedCardinality>
                <owl:onClass rdf:resource="https://w3id.org/netbeheer/referentiemodellen/IECCIM/TC57CIM/IEC61970/Dynamics/StandardModels/WindDynamics#WindTurbineType1or2IEC"/>
            </owl:Restriction>
        </rdfs:subClassOf>
        <rdfs:subClassOf>
            <owl:Restriction>
                <owl:onProperty rdf:resource="https://w3id.org/netbeheer/referentiemodellen/IECCIM/TC57CIM/IEC61970/Dynamics/StandardModels/WindDynamics#WindTurbineType1or2IEC_WindProtectionIEC"/>
                <owl:minQualifiedCardinality rdf:datatype="http://www.w3.org/2001/XMLSchema#nonNegativeInteger">0</owl:minQualifiedCardinality>
                <owl:onClass rdf:resource="https://w3id.org/netbeheer/referentiemodellen/IECCIM/TC57CIM/IEC61970/Dynamics/StandardModels/WindDynamics#WindTurbineType1or2IEC"/>
            </owl:Restriction>
        </rdfs:subClassOf>
        <rdfs:subClassOf>
            <owl:Restriction>
                <owl:onProperty rdf:resource="https://w3id.org/netbeheer/referentiemodellen/IECCIM/TC57CIM/IEC61970/Dynamics/StandardModels/WindDynamics#WindTurbineType1or2IEC_WindMechIEC"/>
                <owl:maxQualifiedCardinality rdf:datatype="http://www.w3.org/2001/XMLSchema#nonNegativeInteger">1</owl:maxQualifiedCardinality>
                <owl:onClass rdf:resource="https://w3id.org/netbeheer/referentiemodellen/IECCIM/TC57CIM/IEC61970/Dynamics/StandardModels/WindDynamics#WindTurbineType1or2IEC"/>
            </owl:Restriction>
        </rdfs:subClassOf>
        <rdfs:subClassOf>
            <owl:Restriction>
                <owl:onProperty rdf:resource="https://w3id.org/netbeheer/referentiemodellen/IECCIM/TC57CIM/IEC61970/Dynamics/StandardModels/WindDynamics#WindTurbineType1or2IEC_WindProtectionIEC"/>
                <owl:maxQualifiedCardinality rdf:datatype="http://www.w3.org/2001/XMLSchema#nonNegativeInteger">1</owl:maxQualifiedCardinality>
                <owl:onClass rdf:resource="https://w3id.org/netbeheer/referentiemodellen/IECCIM/TC57CIM/IEC61970/Dynamics/StandardModels/WindDynamics#WindTurbineType1or2IEC"/>
            </owl:Restriction>
        </rdfs:subClassOf>
        <rdfs:comment>Generator model for wind turbine of IEC Type 1 or Type 2 is a standard asynchronous generator model.

Reference: IEC Standard 614000-27-1 Section 6.6.3.1.</rdfs:comment>
    </owl:Class>
    


    <!-- https://w3id.org/netbeheer/referentiemodellen/IECCIM/TC57CIM/IEC61970/Dynamics/StandardModels/WindDynamics#WindTurbineType3or4Dynamics -->


    <owl:Class rdf:about="https://w3id.org/netbeheer/referentiemodellen/IECCIM/TC57CIM/IEC61970/Dynamics/StandardModels/WindDynamics#WindTurbineType3or4Dynamics">
        <rdfs:subClassOf rdf:resource="https://w3id.org/netbeheer/referentiemodellen/IECCIM/TC57CIM/IEC61970/Dynamics/StandardModels#DynamicsFunctionBlock"/>
        <rdfs:subClassOf>
            <owl:Restriction>
                <owl:onProperty rdf:resource="https://w3id.org/netbeheer/referentiemodellen/IECCIM/TC57CIM/IEC61970/Dynamics/StandardModels/WindDynamics#WindTurbineType3or4Dynamics_WindPlantDynamics"/>
                <owl:minQualifiedCardinality rdf:datatype="http://www.w3.org/2001/XMLSchema#nonNegativeInteger">1</owl:minQualifiedCardinality>
                <owl:onClass rdf:resource="https://w3id.org/netbeheer/referentiemodellen/IECCIM/TC57CIM/IEC61970/Dynamics/StandardModels/WindDynamics#WindTurbineType3or4Dynamics"/>
            </owl:Restriction>
        </rdfs:subClassOf>
        <rdfs:comment>Parent class supporting relationships to wind turbines Type 3 and 4 and wind plant including their control models.</rdfs:comment>
    </owl:Class>
    


    <!-- https://w3id.org/netbeheer/referentiemodellen/IECCIM/TC57CIM/IEC61970/Dynamics/StandardModels/WindDynamics#WindTurbineType3or4IEC -->


    <owl:Class rdf:about="https://w3id.org/netbeheer/referentiemodellen/IECCIM/TC57CIM/IEC61970/Dynamics/StandardModels/WindDynamics#WindTurbineType3or4IEC">
        <rdfs:subClassOf rdf:resource="https://w3id.org/netbeheer/referentiemodellen/IECCIM/TC57CIM/IEC61970/Dynamics/StandardModels/WindDynamics#WindTurbineType3or4Dynamics"/>
        <rdfs:subClassOf>
            <owl:Restriction>
                <owl:onProperty rdf:resource="https://w3id.org/netbeheer/referentiemodellen/IECCIM/TC57CIM/IEC61970/Dynamics/StandardModels/WindDynamics#WindTurbineType3or4IEC_WindProtectionIEC"/>
                <owl:minQualifiedCardinality rdf:datatype="http://www.w3.org/2001/XMLSchema#nonNegativeInteger">0</owl:minQualifiedCardinality>
                <owl:onClass rdf:resource="https://w3id.org/netbeheer/referentiemodellen/IECCIM/TC57CIM/IEC61970/Dynamics/StandardModels/WindDynamics#WindTurbineType3or4IEC"/>
            </owl:Restriction>
        </rdfs:subClassOf>
        <rdfs:subClassOf>
            <owl:Restriction>
                <owl:onProperty rdf:resource="https://w3id.org/netbeheer/referentiemodellen/IECCIM/TC57CIM/IEC61970/Dynamics/StandardModels/WindDynamics#WindTurbineType3or4IEC_WIndContQIEC"/>
                <owl:qualifiedCardinality rdf:datatype="http://www.w3.org/2001/XMLSchema#nonNegativeInteger">1</owl:qualifiedCardinality>
                <owl:onClass rdf:resource="https://w3id.org/netbeheer/referentiemodellen/IECCIM/TC57CIM/IEC61970/Dynamics/StandardModels/WindDynamics#WindTurbineType3or4IEC"/>
            </owl:Restriction>
        </rdfs:subClassOf>
        <rdfs:subClassOf>
            <owl:Restriction>
                <owl:onProperty rdf:resource="https://w3id.org/netbeheer/referentiemodellen/IECCIM/TC57CIM/IEC61970/Dynamics/StandardModels/WindDynamics#WindTurbineType3or4IEC_WindContCurrLimIEC"/>
                <owl:qualifiedCardinality rdf:datatype="http://www.w3.org/2001/XMLSchema#nonNegativeInteger">1</owl:qualifiedCardinality>
                <owl:onClass rdf:resource="https://w3id.org/netbeheer/referentiemodellen/IECCIM/TC57CIM/IEC61970/Dynamics/StandardModels/WindDynamics#WindTurbineType3or4IEC"/>
            </owl:Restriction>
        </rdfs:subClassOf>
        <rdfs:subClassOf>
            <owl:Restriction>
                <owl:onProperty rdf:resource="https://w3id.org/netbeheer/referentiemodellen/IECCIM/TC57CIM/IEC61970/Dynamics/StandardModels/WindDynamics#WindTurbineType3or4IEC_WindProtectionIEC"/>
                <owl:maxQualifiedCardinality rdf:datatype="http://www.w3.org/2001/XMLSchema#nonNegativeInteger">1</owl:maxQualifiedCardinality>
                <owl:onClass rdf:resource="https://w3id.org/netbeheer/referentiemodellen/IECCIM/TC57CIM/IEC61970/Dynamics/StandardModels/WindDynamics#WindTurbineType3or4IEC"/>
            </owl:Restriction>
        </rdfs:subClassOf>
        <rdfs:comment>Parent class supporting relationships to IEC wind turbines Type 3 and 4 and wind plant including their control models.</rdfs:comment>
    </owl:Class>
    


    <!-- https://w3id.org/netbeheer/referentiemodellen/IECCIM/TC57CIM/IEC61970/Dynamics/StandardModels/WindDynamics#WindTurbineType4aIEC -->


    <owl:Class rdf:about="https://w3id.org/netbeheer/referentiemodellen/IECCIM/TC57CIM/IEC61970/Dynamics/StandardModels/WindDynamics#WindTurbineType4aIEC">
        <rdfs:subClassOf rdf:resource="https://w3id.org/netbeheer/referentiemodellen/IECCIM/TC57CIM/IEC61970/Dynamics/StandardModels/WindDynamics#WindGenType4IEC"/>
        <rdfs:subClassOf>
            <owl:Restriction>
                <owl:onProperty rdf:resource="https://w3id.org/netbeheer/referentiemodellen/IECCIM/TC57CIM/IEC61970/Dynamics/StandardModels/WindDynamics#WindTurbineType4aIEC_WindContPType4aIEC"/>
                <owl:qualifiedCardinality rdf:datatype="http://www.w3.org/2001/XMLSchema#nonNegativeInteger">1</owl:qualifiedCardinality>
                <owl:onClass rdf:resource="https://w3id.org/netbeheer/referentiemodellen/IECCIM/TC57CIM/IEC61970/Dynamics/StandardModels/WindDynamics#WindTurbineType4aIEC"/>
            </owl:Restriction>
        </rdfs:subClassOf>
        <rdfs:comment>Wind turbine IEC Type 4A.

Reference: IEC Standard 61400-27-1, section 6.5.5.2.</rdfs:comment>
    </owl:Class>
    


    <!-- https://w3id.org/netbeheer/referentiemodellen/IECCIM/TC57CIM/IEC61970/Dynamics/StandardModels/WindDynamics#WindTurbineType4bIEC -->


    <owl:Class rdf:about="https://w3id.org/netbeheer/referentiemodellen/IECCIM/TC57CIM/IEC61970/Dynamics/StandardModels/WindDynamics#WindTurbineType4bIEC">
        <rdfs:subClassOf rdf:resource="https://w3id.org/netbeheer/referentiemodellen/IECCIM/TC57CIM/IEC61970/Dynamics/StandardModels/WindDynamics#WindGenType4IEC"/>
        <rdfs:subClassOf>
            <owl:Restriction>
                <owl:onProperty rdf:resource="https://w3id.org/netbeheer/referentiemodellen/IECCIM/TC57CIM/IEC61970/Dynamics/StandardModels/WindDynamics#WindTurbineType4bIEC_WindMechIEC"/>
                <owl:minQualifiedCardinality rdf:datatype="http://www.w3.org/2001/XMLSchema#nonNegativeInteger">0</owl:minQualifiedCardinality>
                <owl:onClass rdf:resource="https://w3id.org/netbeheer/referentiemodellen/IECCIM/TC57CIM/IEC61970/Dynamics/StandardModels/WindDynamics#WindTurbineType4bIEC"/>
            </owl:Restriction>
        </rdfs:subClassOf>
        <rdfs:subClassOf>
            <owl:Restriction>
                <owl:onProperty rdf:resource="https://w3id.org/netbeheer/referentiemodellen/IECCIM/TC57CIM/IEC61970/Dynamics/StandardModels/WindDynamics#WindTurbineType4bIEC_WindContPType4bIEC"/>
                <owl:qualifiedCardinality rdf:datatype="http://www.w3.org/2001/XMLSchema#nonNegativeInteger">1</owl:qualifiedCardinality>
                <owl:onClass rdf:resource="https://w3id.org/netbeheer/referentiemodellen/IECCIM/TC57CIM/IEC61970/Dynamics/StandardModels/WindDynamics#WindTurbineType4bIEC"/>
            </owl:Restriction>
        </rdfs:subClassOf>
        <rdfs:subClassOf>
            <owl:Restriction>
                <owl:onProperty rdf:resource="https://w3id.org/netbeheer/referentiemodellen/IECCIM/TC57CIM/IEC61970/Dynamics/StandardModels/WindDynamics#WindTurbineType4bIEC_WindMechIEC"/>
                <owl:maxQualifiedCardinality rdf:datatype="http://www.w3.org/2001/XMLSchema#nonNegativeInteger">1</owl:maxQualifiedCardinality>
                <owl:onClass rdf:resource="https://w3id.org/netbeheer/referentiemodellen/IECCIM/TC57CIM/IEC61970/Dynamics/StandardModels/WindDynamics#WindTurbineType4bIEC"/>
            </owl:Restriction>
        </rdfs:subClassOf>
        <rdfs:comment>Wind turbine IEC Type 4A.

Reference: IEC Standard 61400-27-1, section 6.5.5.3.</rdfs:comment>
    </owl:Class>
</rdf:RDF>



<!-- Generated by the OWL API (version 5.1.10.2019-03-12T22:31:15Z) https://github.com/owlcs/owlapi/ -->


