<?xml version="1.0"?>
<rdf:RDF xmlns="https://w3id.org/netbeheer/referentiemodellen/IECCIM/TC57CIM/IEC61970/Dynamics/StandardModels#"
     xml:base="https://w3id.org/netbeheer/referentiemodellen/IECCIM/TC57CIM/IEC61970/Dynamics/StandardModels"
     xmlns:owl="http://www.w3.org/2002/07/owl#"
     xmlns:rdf="http://www.w3.org/1999/02/22-rdf-syntax-ns#"
     xmlns:xml="http://www.w3.org/XML/1998/namespace"
     xmlns:xsd="http://www.w3.org/2001/XMLSchema#"
     xmlns:rdfs="http://www.w3.org/2000/01/rdf-schema#">
    <owl:Ontology rdf:about="https://w3id.org/netbeheer/referentiemodellen/IECCIM/TC57CIM/IEC61970/Dynamics/StandardModels#"/>
    


    <!-- 
    ///////////////////////////////////////////////////////////////////////////////////////
    //
    // Object Properties
    //
    ///////////////////////////////////////////////////////////////////////////////////////
     -->


    


    <!-- https://w3id.org/netbeheer/referentiemodellen/IECCIM/TC57CIM/IEC61970/Dynamics/StandardModels#RotatingMachineDynamics_inertia -->


    <owl:ObjectProperty rdf:about="https://w3id.org/netbeheer/referentiemodellen/IECCIM/TC57CIM/IEC61970/Dynamics/StandardModels#RotatingMachineDynamics_inertia">
        <rdfs:domain rdf:resource="https://w3id.org/netbeheer/referentiemodellen/IECCIM/TC57CIM/IEC61970/Dynamics/StandardModels#RotatingMachineDynamics"/>
        <rdfs:range rdf:resource="https://w3id.org/netbeheer/referentiemodellen/IECCIM/TC57CIM/IEC61970/Base/Domain#Seconds"/>
        <rdfs:comment>Inertia constant of generator or motor and mechanical load (H) (&amp;gt;0).  This is the specification for the stored energy in the rotating mass when operating at rated speed.  For a generator, this includes the generator plus all other elements (turbine, exciter) on the same shaft and has units of MW*sec.  For a motor, it includes the motor plus its mechanical load. Conventional units are per unit on the generator MVA base, usually expressed as MW*second/MVA or just second.   This value is used in the accelerating power reference frame for operator training simulator solutions.  Typical Value = 3.</rdfs:comment>
    </owl:ObjectProperty>
    


    <!-- https://w3id.org/netbeheer/referentiemodellen/IECCIM/TC57CIM/IEC61970/Dynamics/StandardModels#RotatingMachineDynamics_statorLeakageReactance -->


    <owl:ObjectProperty rdf:about="https://w3id.org/netbeheer/referentiemodellen/IECCIM/TC57CIM/IEC61970/Dynamics/StandardModels#RotatingMachineDynamics_statorLeakageReactance">
        <rdfs:domain rdf:resource="https://w3id.org/netbeheer/referentiemodellen/IECCIM/TC57CIM/IEC61970/Dynamics/StandardModels#RotatingMachineDynamics"/>
        <rdfs:range rdf:resource="https://w3id.org/netbeheer/referentiemodellen/IECCIM/TC57CIM/IEC61970/Base/Domain#PU"/>
        <rdfs:comment>Stator leakage reactance (Xl) (&amp;gt; or =0). Typical Value = 0.15.</rdfs:comment>
    </owl:ObjectProperty>
    


    <!-- https://w3id.org/netbeheer/referentiemodellen/IECCIM/TC57CIM/IEC61970/Dynamics/StandardModels#RotatingMachineDynamics_statorResistance -->


    <owl:ObjectProperty rdf:about="https://w3id.org/netbeheer/referentiemodellen/IECCIM/TC57CIM/IEC61970/Dynamics/StandardModels#RotatingMachineDynamics_statorResistance">
        <rdfs:domain rdf:resource="https://w3id.org/netbeheer/referentiemodellen/IECCIM/TC57CIM/IEC61970/Dynamics/StandardModels#RotatingMachineDynamics"/>
        <rdfs:range rdf:resource="https://w3id.org/netbeheer/referentiemodellen/IECCIM/TC57CIM/IEC61970/Base/Domain#PU"/>
        <rdfs:comment>Stator (armature) resistance (Rs) (&amp;gt; or =0). Typical Value = 0.005.</rdfs:comment>
    </owl:ObjectProperty>
    


    <!-- 
    ///////////////////////////////////////////////////////////////////////////////////////
    //
    // Data properties
    //
    ///////////////////////////////////////////////////////////////////////////////////////
     -->


    


    <!-- https://w3id.org/netbeheer/referentiemodellen/IECCIM/TC57CIM/IEC61970/Dynamics/StandardModels#DynamicsFunctionBlock_enabled -->


    <owl:DatatypeProperty rdf:about="https://w3id.org/netbeheer/referentiemodellen/IECCIM/TC57CIM/IEC61970/Dynamics/StandardModels#DynamicsFunctionBlock_enabled">
        <rdfs:domain rdf:resource="https://w3id.org/netbeheer/referentiemodellen/IECCIM/TC57CIM/IEC61970/Dynamics/StandardModels#DynamicsFunctionBlock"/>
        <rdfs:range rdf:resource="http://www.w3.org/2001/XMLSchema#boolean"/>
        <rdfs:comment>Function block used indicator.
true = use of function block is enabled
false = use of function block is disabled.</rdfs:comment>
    </owl:DatatypeProperty>
    


    <!-- https://w3id.org/netbeheer/referentiemodellen/IECCIM/TC57CIM/IEC61970/Dynamics/StandardModels#RotatingMachineDynamics_damping -->


    <owl:DatatypeProperty rdf:about="https://w3id.org/netbeheer/referentiemodellen/IECCIM/TC57CIM/IEC61970/Dynamics/StandardModels#RotatingMachineDynamics_damping">
        <rdfs:domain rdf:resource="https://w3id.org/netbeheer/referentiemodellen/IECCIM/TC57CIM/IEC61970/Dynamics/StandardModels#RotatingMachineDynamics"/>
        <rdfs:range rdf:resource="http://www.w3.org/2001/XMLSchema#float"/>
        <rdfs:comment>Damping torque coefficient (D).  A proportionality constant that, when multiplied by the angular velocity of the rotor poles with respect to the magnetic field (frequency), results in the damping torque.  This value is often zero when the sources of damping torques (generator damper windings, load damping effects, etc.) are modelled in detail.  Typical Value = 0.</rdfs:comment>
    </owl:DatatypeProperty>
    


    <!-- https://w3id.org/netbeheer/referentiemodellen/IECCIM/TC57CIM/IEC61970/Dynamics/StandardModels#RotatingMachineDynamics_saturationFactor -->


    <owl:DatatypeProperty rdf:about="https://w3id.org/netbeheer/referentiemodellen/IECCIM/TC57CIM/IEC61970/Dynamics/StandardModels#RotatingMachineDynamics_saturationFactor">
        <rdfs:domain rdf:resource="https://w3id.org/netbeheer/referentiemodellen/IECCIM/TC57CIM/IEC61970/Dynamics/StandardModels#RotatingMachineDynamics"/>
        <rdfs:range rdf:resource="http://www.w3.org/2001/XMLSchema#float"/>
        <rdfs:comment>Saturation factor at rated terminal voltage (S1) (&amp;gt; or =0).  Not used by simplified model.  Defined by defined by S(E1) in the SynchronousMachineSaturationParameters diagram.  Typical Value = 0.02.</rdfs:comment>
    </owl:DatatypeProperty>
    


    <!-- https://w3id.org/netbeheer/referentiemodellen/IECCIM/TC57CIM/IEC61970/Dynamics/StandardModels#RotatingMachineDynamics_saturationFactor120 -->


    <owl:DatatypeProperty rdf:about="https://w3id.org/netbeheer/referentiemodellen/IECCIM/TC57CIM/IEC61970/Dynamics/StandardModels#RotatingMachineDynamics_saturationFactor120">
        <rdfs:domain rdf:resource="https://w3id.org/netbeheer/referentiemodellen/IECCIM/TC57CIM/IEC61970/Dynamics/StandardModels#RotatingMachineDynamics"/>
        <rdfs:range rdf:resource="http://www.w3.org/2001/XMLSchema#float"/>
        <rdfs:comment>Saturation factor at 120% of rated terminal voltage (S12) (&amp;gt; or =S1). Not used by the simplified model, defined by S(E2) in the SynchronousMachineSaturationParameters diagram.  Typical Value = 0.12.</rdfs:comment>
    </owl:DatatypeProperty>
    


    <!-- 
    ///////////////////////////////////////////////////////////////////////////////////////
    //
    // Classes
    //
    ///////////////////////////////////////////////////////////////////////////////////////
     -->


    


    <!-- https://w3id.org/netbeheer/referentiemodellen/IECCIM/TC57CIM/IEC61970/Base/Core#IdentifiedObject -->


    <owl:Class rdf:about="https://w3id.org/netbeheer/referentiemodellen/IECCIM/TC57CIM/IEC61970/Base/Core#IdentifiedObject"/>
    


    <!-- https://w3id.org/netbeheer/referentiemodellen/IECCIM/TC57CIM/IEC61970/Base/Domain#PU -->


    <owl:Class rdf:about="https://w3id.org/netbeheer/referentiemodellen/IECCIM/TC57CIM/IEC61970/Base/Domain#PU"/>
    


    <!-- https://w3id.org/netbeheer/referentiemodellen/IECCIM/TC57CIM/IEC61970/Base/Domain#Seconds -->


    <owl:Class rdf:about="https://w3id.org/netbeheer/referentiemodellen/IECCIM/TC57CIM/IEC61970/Base/Domain#Seconds"/>
    


    <!-- https://w3id.org/netbeheer/referentiemodellen/IECCIM/TC57CIM/IEC61970/Dynamics/StandardModels#DynamicsFunctionBlock -->


    <owl:Class rdf:about="https://w3id.org/netbeheer/referentiemodellen/IECCIM/TC57CIM/IEC61970/Dynamics/StandardModels#DynamicsFunctionBlock">
        <rdfs:subClassOf rdf:resource="https://w3id.org/netbeheer/referentiemodellen/IECCIM/TC57CIM/IEC61970/Base/Core#IdentifiedObject"/>
        <rdfs:subClassOf>
            <owl:Restriction>
                <owl:onProperty rdf:resource="https://w3id.org/netbeheer/referentiemodellen/IECCIM/TC57CIM/IEC61970/Dynamics/StandardModels#DynamicsFunctionBlock_enabled"/>
                <owl:minQualifiedCardinality rdf:datatype="http://www.w3.org/2001/XMLSchema#nonNegativeInteger">0</owl:minQualifiedCardinality>
                <owl:onDataRange rdf:resource="http://www.w3.org/2001/XMLSchema#boolean"/>
            </owl:Restriction>
        </rdfs:subClassOf>
        <rdfs:subClassOf>
            <owl:Restriction>
                <owl:onProperty rdf:resource="https://w3id.org/netbeheer/referentiemodellen/IECCIM/TC57CIM/IEC61970/Dynamics/StandardModels#DynamicsFunctionBlock_enabled"/>
                <owl:maxQualifiedCardinality rdf:datatype="http://www.w3.org/2001/XMLSchema#nonNegativeInteger">1</owl:maxQualifiedCardinality>
                <owl:onDataRange rdf:resource="http://www.w3.org/2001/XMLSchema#boolean"/>
            </owl:Restriction>
        </rdfs:subClassOf>
        <rdfs:comment>Abstract parent class for all Dynamics function blocks.</rdfs:comment>
    </owl:Class>
    


    <!-- https://w3id.org/netbeheer/referentiemodellen/IECCIM/TC57CIM/IEC61970/Dynamics/StandardModels#RotatingMachineDynamics -->


    <owl:Class rdf:about="https://w3id.org/netbeheer/referentiemodellen/IECCIM/TC57CIM/IEC61970/Dynamics/StandardModels#RotatingMachineDynamics">
        <rdfs:subClassOf rdf:resource="https://w3id.org/netbeheer/referentiemodellen/IECCIM/TC57CIM/IEC61970/Dynamics/StandardModels#DynamicsFunctionBlock"/>
        <rdfs:subClassOf>
            <owl:Restriction>
                <owl:onProperty rdf:resource="https://w3id.org/netbeheer/referentiemodellen/IECCIM/TC57CIM/IEC61970/Dynamics/StandardModels#RotatingMachineDynamics_inertia"/>
                <owl:minQualifiedCardinality rdf:datatype="http://www.w3.org/2001/XMLSchema#nonNegativeInteger">0</owl:minQualifiedCardinality>
                <owl:onClass rdf:resource="https://w3id.org/netbeheer/referentiemodellen/IECCIM/TC57CIM/IEC61970/Base/Domain#Seconds"/>
            </owl:Restriction>
        </rdfs:subClassOf>
        <rdfs:subClassOf>
            <owl:Restriction>
                <owl:onProperty rdf:resource="https://w3id.org/netbeheer/referentiemodellen/IECCIM/TC57CIM/IEC61970/Dynamics/StandardModels#RotatingMachineDynamics_statorLeakageReactance"/>
                <owl:minQualifiedCardinality rdf:datatype="http://www.w3.org/2001/XMLSchema#nonNegativeInteger">0</owl:minQualifiedCardinality>
                <owl:onClass rdf:resource="https://w3id.org/netbeheer/referentiemodellen/IECCIM/TC57CIM/IEC61970/Base/Domain#PU"/>
            </owl:Restriction>
        </rdfs:subClassOf>
        <rdfs:subClassOf>
            <owl:Restriction>
                <owl:onProperty rdf:resource="https://w3id.org/netbeheer/referentiemodellen/IECCIM/TC57CIM/IEC61970/Dynamics/StandardModels#RotatingMachineDynamics_statorResistance"/>
                <owl:minQualifiedCardinality rdf:datatype="http://www.w3.org/2001/XMLSchema#nonNegativeInteger">0</owl:minQualifiedCardinality>
                <owl:onClass rdf:resource="https://w3id.org/netbeheer/referentiemodellen/IECCIM/TC57CIM/IEC61970/Base/Domain#PU"/>
            </owl:Restriction>
        </rdfs:subClassOf>
        <rdfs:subClassOf>
            <owl:Restriction>
                <owl:onProperty rdf:resource="https://w3id.org/netbeheer/referentiemodellen/IECCIM/TC57CIM/IEC61970/Dynamics/StandardModels#RotatingMachineDynamics_inertia"/>
                <owl:maxQualifiedCardinality rdf:datatype="http://www.w3.org/2001/XMLSchema#nonNegativeInteger">1</owl:maxQualifiedCardinality>
                <owl:onClass rdf:resource="https://w3id.org/netbeheer/referentiemodellen/IECCIM/TC57CIM/IEC61970/Base/Domain#Seconds"/>
            </owl:Restriction>
        </rdfs:subClassOf>
        <rdfs:subClassOf>
            <owl:Restriction>
                <owl:onProperty rdf:resource="https://w3id.org/netbeheer/referentiemodellen/IECCIM/TC57CIM/IEC61970/Dynamics/StandardModels#RotatingMachineDynamics_statorLeakageReactance"/>
                <owl:maxQualifiedCardinality rdf:datatype="http://www.w3.org/2001/XMLSchema#nonNegativeInteger">1</owl:maxQualifiedCardinality>
                <owl:onClass rdf:resource="https://w3id.org/netbeheer/referentiemodellen/IECCIM/TC57CIM/IEC61970/Base/Domain#PU"/>
            </owl:Restriction>
        </rdfs:subClassOf>
        <rdfs:subClassOf>
            <owl:Restriction>
                <owl:onProperty rdf:resource="https://w3id.org/netbeheer/referentiemodellen/IECCIM/TC57CIM/IEC61970/Dynamics/StandardModels#RotatingMachineDynamics_statorResistance"/>
                <owl:maxQualifiedCardinality rdf:datatype="http://www.w3.org/2001/XMLSchema#nonNegativeInteger">1</owl:maxQualifiedCardinality>
                <owl:onClass rdf:resource="https://w3id.org/netbeheer/referentiemodellen/IECCIM/TC57CIM/IEC61970/Base/Domain#PU"/>
            </owl:Restriction>
        </rdfs:subClassOf>
        <rdfs:subClassOf>
            <owl:Restriction>
                <owl:onProperty rdf:resource="https://w3id.org/netbeheer/referentiemodellen/IECCIM/TC57CIM/IEC61970/Dynamics/StandardModels#RotatingMachineDynamics_damping"/>
                <owl:minQualifiedCardinality rdf:datatype="http://www.w3.org/2001/XMLSchema#nonNegativeInteger">0</owl:minQualifiedCardinality>
                <owl:onDataRange rdf:resource="http://www.w3.org/2001/XMLSchema#float"/>
            </owl:Restriction>
        </rdfs:subClassOf>
        <rdfs:subClassOf>
            <owl:Restriction>
                <owl:onProperty rdf:resource="https://w3id.org/netbeheer/referentiemodellen/IECCIM/TC57CIM/IEC61970/Dynamics/StandardModels#RotatingMachineDynamics_saturationFactor"/>
                <owl:minQualifiedCardinality rdf:datatype="http://www.w3.org/2001/XMLSchema#nonNegativeInteger">0</owl:minQualifiedCardinality>
                <owl:onDataRange rdf:resource="http://www.w3.org/2001/XMLSchema#float"/>
            </owl:Restriction>
        </rdfs:subClassOf>
        <rdfs:subClassOf>
            <owl:Restriction>
                <owl:onProperty rdf:resource="https://w3id.org/netbeheer/referentiemodellen/IECCIM/TC57CIM/IEC61970/Dynamics/StandardModels#RotatingMachineDynamics_saturationFactor120"/>
                <owl:minQualifiedCardinality rdf:datatype="http://www.w3.org/2001/XMLSchema#nonNegativeInteger">0</owl:minQualifiedCardinality>
                <owl:onDataRange rdf:resource="http://www.w3.org/2001/XMLSchema#float"/>
            </owl:Restriction>
        </rdfs:subClassOf>
        <rdfs:subClassOf>
            <owl:Restriction>
                <owl:onProperty rdf:resource="https://w3id.org/netbeheer/referentiemodellen/IECCIM/TC57CIM/IEC61970/Dynamics/StandardModels#RotatingMachineDynamics_damping"/>
                <owl:maxQualifiedCardinality rdf:datatype="http://www.w3.org/2001/XMLSchema#nonNegativeInteger">1</owl:maxQualifiedCardinality>
                <owl:onDataRange rdf:resource="http://www.w3.org/2001/XMLSchema#float"/>
            </owl:Restriction>
        </rdfs:subClassOf>
        <rdfs:subClassOf>
            <owl:Restriction>
                <owl:onProperty rdf:resource="https://w3id.org/netbeheer/referentiemodellen/IECCIM/TC57CIM/IEC61970/Dynamics/StandardModels#RotatingMachineDynamics_saturationFactor"/>
                <owl:maxQualifiedCardinality rdf:datatype="http://www.w3.org/2001/XMLSchema#nonNegativeInteger">1</owl:maxQualifiedCardinality>
                <owl:onDataRange rdf:resource="http://www.w3.org/2001/XMLSchema#float"/>
            </owl:Restriction>
        </rdfs:subClassOf>
        <rdfs:subClassOf>
            <owl:Restriction>
                <owl:onProperty rdf:resource="https://w3id.org/netbeheer/referentiemodellen/IECCIM/TC57CIM/IEC61970/Dynamics/StandardModels#RotatingMachineDynamics_saturationFactor120"/>
                <owl:maxQualifiedCardinality rdf:datatype="http://www.w3.org/2001/XMLSchema#nonNegativeInteger">1</owl:maxQualifiedCardinality>
                <owl:onDataRange rdf:resource="http://www.w3.org/2001/XMLSchema#float"/>
            </owl:Restriction>
        </rdfs:subClassOf>
        <rdfs:comment>Abstract parent class for all synchronous and asynchronous machine standard models.</rdfs:comment>
    </owl:Class>
</rdf:RDF>



<!-- Generated by the OWL API (version 5.1.10.2019-03-12T22:31:15Z) https://github.com/owlcs/owlapi/ -->


