<?xml version="1.0"?>
<rdf:RDF xmlns="https://w3id.org/netbeheer/referentiemodellen/IECCIM/TC57CIM/IEC61970/Base/ControlArea#"
     xml:base="https://w3id.org/netbeheer/referentiemodellen/IECCIM/TC57CIM/IEC61970/Base/ControlArea"
     xmlns:owl="http://www.w3.org/2002/07/owl#"
     xmlns:rdf="http://www.w3.org/1999/02/22-rdf-syntax-ns#"
     xmlns:xml="http://www.w3.org/XML/1998/namespace"
     xmlns:xsd="http://www.w3.org/2001/XMLSchema#"
     xmlns:rdfs="http://www.w3.org/2000/01/rdf-schema#">
    <owl:Ontology rdf:about="https://w3id.org/netbeheer/referentiemodellen/IECCIM/TC57CIM/IEC61970/Base/ControlArea#"/>
    


    <!-- 
    ///////////////////////////////////////////////////////////////////////////////////////
    //
    // Datatypes
    //
    ///////////////////////////////////////////////////////////////////////////////////////
     -->


    


    <!-- https://w3id.org/netbeheer/referentiemodellen/IECCIM/TC57CIM/IEC61970/Base/ControlArea#ControlAreaTypeKind -->


    <rdfs:Datatype rdf:about="https://w3id.org/netbeheer/referentiemodellen/IECCIM/TC57CIM/IEC61970/Base/ControlArea#ControlAreaTypeKind">
        <owl:equivalentClass>
            <rdfs:Datatype>
                <owl:oneOf>
                    <rdf:Description>
                        <rdf:type rdf:resource="http://www.w3.org/1999/02/22-rdf-syntax-ns#List"/>
                        <rdf:first>AGC</rdf:first>
                        <rdf:rest>
                            <rdf:Description>
                                <rdf:type rdf:resource="http://www.w3.org/1999/02/22-rdf-syntax-ns#List"/>
                                <rdf:first>Forecast</rdf:first>
                                <rdf:rest>
                                    <rdf:Description>
                                        <rdf:type rdf:resource="http://www.w3.org/1999/02/22-rdf-syntax-ns#List"/>
                                        <rdf:first>Interchange</rdf:first>
                                        <rdf:rest rdf:resource="http://www.w3.org/1999/02/22-rdf-syntax-ns#nil"/>
                                    </rdf:Description>
                                </rdf:rest>
                            </rdf:Description>
                        </rdf:rest>
                    </rdf:Description>
                </owl:oneOf>
            </rdfs:Datatype>
        </owl:equivalentClass>
    </rdfs:Datatype>
    


    <!-- 
    ///////////////////////////////////////////////////////////////////////////////////////
    //
    // Object Properties
    //
    ///////////////////////////////////////////////////////////////////////////////////////
     -->


    


    <!-- https://w3id.org/netbeheer/referentiemodellen/IECCIM/TC57CIM/IEC61970/Base/ControlArea#AltGeneratingUnitMeas.ControlAreaGeneratingUnit -->


    <owl:ObjectProperty rdf:about="https://w3id.org/netbeheer/referentiemodellen/IECCIM/TC57CIM/IEC61970/Base/ControlArea#AltGeneratingUnitMeas.ControlAreaGeneratingUnit">
        <rdfs:domain rdf:resource="https://w3id.org/netbeheer/referentiemodellen/IECCIM/TC57CIM/IEC61970/Base/ControlArea#AltGeneratingUnitMeas"/>
        <rdfs:range rdf:resource="https://w3id.org/netbeheer/referentiemodellen/IECCIM/TC57CIM/IEC61970/Base/ControlArea#ControlAreaGeneratingUnit"/>
        <rdfs:comment>The link to prioritized measurements for this GeneratingUnit.The control aread generating unit to which the prioritized measurement assignment is applied.</rdfs:comment>
    </owl:ObjectProperty>
    


    <!-- https://w3id.org/netbeheer/referentiemodellen/IECCIM/TC57CIM/IEC61970/Base/ControlArea#AltTieMeas.TieFlow -->


    <owl:ObjectProperty rdf:about="https://w3id.org/netbeheer/referentiemodellen/IECCIM/TC57CIM/IEC61970/Base/ControlArea#AltTieMeas.TieFlow">
        <rdfs:domain rdf:resource="https://w3id.org/netbeheer/referentiemodellen/IECCIM/TC57CIM/IEC61970/Base/ControlArea#AltTieMeas"/>
        <rdfs:range rdf:resource="https://w3id.org/netbeheer/referentiemodellen/IECCIM/TC57CIM/IEC61970/Base/ControlArea#TieFlow"/>
        <rdfs:comment>The primary and alternate tie flow measurements associated with the tie flow.The tie flow of the alternate measurements.</rdfs:comment>
    </owl:ObjectProperty>
    


    <!-- https://w3id.org/netbeheer/referentiemodellen/IECCIM/TC57CIM/IEC61970/Base/ControlArea#ControlArea.ControlAreaGeneratingUnit -->


    <owl:ObjectProperty rdf:about="https://w3id.org/netbeheer/referentiemodellen/IECCIM/TC57CIM/IEC61970/Base/ControlArea#ControlArea.ControlAreaGeneratingUnit">
        <owl:inverseOf rdf:resource="https://w3id.org/netbeheer/referentiemodellen/IECCIM/TC57CIM/IEC61970/Base/ControlArea#ControlAreaGeneratingUnit.ControlArea"/>
        <rdf:type rdf:resource="http://www.w3.org/2002/07/owl#FunctionalProperty"/>
        <rdfs:domain rdf:resource="https://w3id.org/netbeheer/referentiemodellen/IECCIM/TC57CIM/IEC61970/Base/ControlArea#ControlArea"/>
        <rdfs:range rdf:resource="https://w3id.org/netbeheer/referentiemodellen/IECCIM/TC57CIM/IEC61970/Base/ControlArea#ControlAreaGeneratingUnit"/>
        <rdfs:comment>The generating unit specificaitons for the control area.The parent control area for the generating unit specifications.</rdfs:comment>
    </owl:ObjectProperty>
    


    <!-- https://w3id.org/netbeheer/referentiemodellen/IECCIM/TC57CIM/IEC61970/Base/ControlArea#ControlArea.TieFlow -->


    <owl:ObjectProperty rdf:about="https://w3id.org/netbeheer/referentiemodellen/IECCIM/TC57CIM/IEC61970/Base/ControlArea#ControlArea.TieFlow">
        <owl:inverseOf rdf:resource="https://w3id.org/netbeheer/referentiemodellen/IECCIM/TC57CIM/IEC61970/Base/ControlArea#TieFlow.ControlArea"/>
        <rdf:type rdf:resource="http://www.w3.org/2002/07/owl#FunctionalProperty"/>
        <rdfs:domain rdf:resource="https://w3id.org/netbeheer/referentiemodellen/IECCIM/TC57CIM/IEC61970/Base/ControlArea#ControlArea"/>
        <rdfs:range rdf:resource="https://w3id.org/netbeheer/referentiemodellen/IECCIM/TC57CIM/IEC61970/Base/ControlArea#TieFlow"/>
        <rdfs:comment>The tie flows associated with the control area.The control area of the tie flows.</rdfs:comment>
    </owl:ObjectProperty>
    


    <!-- https://w3id.org/netbeheer/referentiemodellen/IECCIM/TC57CIM/IEC61970/Base/ControlArea#ControlArea.netInterchange -->


    <owl:ObjectProperty rdf:about="https://w3id.org/netbeheer/referentiemodellen/IECCIM/TC57CIM/IEC61970/Base/ControlArea#ControlArea.netInterchange">
        <rdfs:domain rdf:resource="https://w3id.org/netbeheer/referentiemodellen/IECCIM/TC57CIM/IEC61970/Base/ControlArea#ControlArea"/>
        <rdfs:range rdf:resource="https://w3id.org/netbeheer/referentiemodellen/IECCIM/TC57CIM/IEC61970/Base/Domain#ActivePower"/>
        <rdfs:comment>The specified positive net interchange into the control area, i.e. positive sign means flow in to the area.</rdfs:comment>
    </owl:ObjectProperty>
    


    <!-- https://w3id.org/netbeheer/referentiemodellen/IECCIM/TC57CIM/IEC61970/Base/ControlArea#ControlArea.pTolerance -->


    <owl:ObjectProperty rdf:about="https://w3id.org/netbeheer/referentiemodellen/IECCIM/TC57CIM/IEC61970/Base/ControlArea#ControlArea.pTolerance">
        <rdfs:domain rdf:resource="https://w3id.org/netbeheer/referentiemodellen/IECCIM/TC57CIM/IEC61970/Base/ControlArea#ControlArea"/>
        <rdfs:range rdf:resource="https://w3id.org/netbeheer/referentiemodellen/IECCIM/TC57CIM/IEC61970/Base/Domain#ActivePower"/>
        <rdfs:comment>Active power net interchange tolerance</rdfs:comment>
    </owl:ObjectProperty>
    


    <!-- https://w3id.org/netbeheer/referentiemodellen/IECCIM/TC57CIM/IEC61970/Base/ControlArea#ControlAreaGeneratingUnit.AltGeneratingUnitMeas -->


    <owl:ObjectProperty rdf:about="https://w3id.org/netbeheer/referentiemodellen/IECCIM/TC57CIM/IEC61970/Base/ControlArea#ControlAreaGeneratingUnit.AltGeneratingUnitMeas">
        <owl:inverseOf rdf:resource="https://w3id.org/netbeheer/referentiemodellen/IECCIM/TC57CIM/IEC61970/Base/ControlArea#AltGeneratingUnitMeas.ControlAreaGeneratingUnit"/>
        <rdf:type rdf:resource="http://www.w3.org/2002/07/owl#FunctionalProperty"/>
        <rdfs:domain rdf:resource="https://w3id.org/netbeheer/referentiemodellen/IECCIM/TC57CIM/IEC61970/Base/ControlArea#ControlAreaGeneratingUnit"/>
        <rdfs:range rdf:resource="https://w3id.org/netbeheer/referentiemodellen/IECCIM/TC57CIM/IEC61970/Base/ControlArea#AltGeneratingUnitMeas"/>
        <rdfs:comment>The link to prioritized measurements for this GeneratingUnit.The control aread generating unit to which the prioritized measurement assignment is applied.</rdfs:comment>
    </owl:ObjectProperty>
    


    <!-- https://w3id.org/netbeheer/referentiemodellen/IECCIM/TC57CIM/IEC61970/Base/ControlArea#ControlAreaGeneratingUnit.ControlArea -->


    <owl:ObjectProperty rdf:about="https://w3id.org/netbeheer/referentiemodellen/IECCIM/TC57CIM/IEC61970/Base/ControlArea#ControlAreaGeneratingUnit.ControlArea">
        <rdfs:domain rdf:resource="https://w3id.org/netbeheer/referentiemodellen/IECCIM/TC57CIM/IEC61970/Base/ControlArea#ControlAreaGeneratingUnit"/>
        <rdfs:range rdf:resource="https://w3id.org/netbeheer/referentiemodellen/IECCIM/TC57CIM/IEC61970/Base/ControlArea#ControlArea"/>
        <rdfs:comment>The generating unit specificaitons for the control area.The parent control area for the generating unit specifications.</rdfs:comment>
    </owl:ObjectProperty>
    


    <!-- https://w3id.org/netbeheer/referentiemodellen/IECCIM/TC57CIM/IEC61970/Base/ControlArea#TieFlow.AltTieMeas -->


    <owl:ObjectProperty rdf:about="https://w3id.org/netbeheer/referentiemodellen/IECCIM/TC57CIM/IEC61970/Base/ControlArea#TieFlow.AltTieMeas">
        <owl:inverseOf rdf:resource="https://w3id.org/netbeheer/referentiemodellen/IECCIM/TC57CIM/IEC61970/Base/ControlArea#AltTieMeas.TieFlow"/>
        <rdf:type rdf:resource="http://www.w3.org/2002/07/owl#FunctionalProperty"/>
        <rdfs:domain rdf:resource="https://w3id.org/netbeheer/referentiemodellen/IECCIM/TC57CIM/IEC61970/Base/ControlArea#TieFlow"/>
        <rdfs:range rdf:resource="https://w3id.org/netbeheer/referentiemodellen/IECCIM/TC57CIM/IEC61970/Base/ControlArea#AltTieMeas"/>
        <rdfs:comment>The primary and alternate tie flow measurements associated with the tie flow.The tie flow of the alternate measurements.</rdfs:comment>
    </owl:ObjectProperty>
    


    <!-- https://w3id.org/netbeheer/referentiemodellen/IECCIM/TC57CIM/IEC61970/Base/ControlArea#TieFlow.ControlArea -->


    <owl:ObjectProperty rdf:about="https://w3id.org/netbeheer/referentiemodellen/IECCIM/TC57CIM/IEC61970/Base/ControlArea#TieFlow.ControlArea">
        <rdfs:domain rdf:resource="https://w3id.org/netbeheer/referentiemodellen/IECCIM/TC57CIM/IEC61970/Base/ControlArea#TieFlow"/>
        <rdfs:range rdf:resource="https://w3id.org/netbeheer/referentiemodellen/IECCIM/TC57CIM/IEC61970/Base/ControlArea#ControlArea"/>
        <rdfs:comment>The tie flows associated with the control area.The control area of the tie flows.</rdfs:comment>
    </owl:ObjectProperty>
    


    <!-- 
    ///////////////////////////////////////////////////////////////////////////////////////
    //
    // Data properties
    //
    ///////////////////////////////////////////////////////////////////////////////////////
     -->


    


    <!-- https://w3id.org/netbeheer/referentiemodellen/IECCIM/TC57CIM/IEC61970/Base/ControlArea#AltGeneratingUnitMeas.priority -->


    <owl:DatatypeProperty rdf:about="https://w3id.org/netbeheer/referentiemodellen/IECCIM/TC57CIM/IEC61970/Base/ControlArea#AltGeneratingUnitMeas.priority">
        <rdfs:domain rdf:resource="https://w3id.org/netbeheer/referentiemodellen/IECCIM/TC57CIM/IEC61970/Base/ControlArea#AltGeneratingUnitMeas"/>
        <rdfs:range rdf:resource="http://www.w3.org/2001/XMLSchema#nonNegativeInteger"/>
        <rdfs:comment>Priority of a measurement usage.   Lower numbers have first priority.</rdfs:comment>
    </owl:DatatypeProperty>
    


    <!-- https://w3id.org/netbeheer/referentiemodellen/IECCIM/TC57CIM/IEC61970/Base/ControlArea#AltTieMeas.priority -->


    <owl:DatatypeProperty rdf:about="https://w3id.org/netbeheer/referentiemodellen/IECCIM/TC57CIM/IEC61970/Base/ControlArea#AltTieMeas.priority">
        <rdfs:domain rdf:resource="https://w3id.org/netbeheer/referentiemodellen/IECCIM/TC57CIM/IEC61970/Base/ControlArea#AltTieMeas"/>
        <rdfs:range rdf:resource="http://www.w3.org/2001/XMLSchema#nonNegativeInteger"/>
        <rdfs:comment>Priority of a measurement usage.   Lower numbers have first priority.</rdfs:comment>
    </owl:DatatypeProperty>
    


    <!-- https://w3id.org/netbeheer/referentiemodellen/IECCIM/TC57CIM/IEC61970/Base/ControlArea#ControlArea.type -->


    <owl:DatatypeProperty rdf:about="https://w3id.org/netbeheer/referentiemodellen/IECCIM/TC57CIM/IEC61970/Base/ControlArea#ControlArea.type">
        <rdfs:domain rdf:resource="https://w3id.org/netbeheer/referentiemodellen/IECCIM/TC57CIM/IEC61970/Base/ControlArea#ControlArea"/>
        <rdfs:range rdf:resource="https://w3id.org/netbeheer/referentiemodellen/IECCIM/TC57CIM/IEC61970/Base/ControlArea#ControlAreaTypeKind"/>
        <rdfs:comment>The primary type of control area definition used to determine if this is used for automatic generation control, for planning interchange control, or other purposes.   A control area specified with primary type of automatic generation control could still be forecast and used as an interchange area in power flow analysis.</rdfs:comment>
    </owl:DatatypeProperty>
    


    <!-- https://w3id.org/netbeheer/referentiemodellen/IECCIM/TC57CIM/IEC61970/Base/ControlArea#TieFlow.positiveFlowIn -->


    <owl:DatatypeProperty rdf:about="https://w3id.org/netbeheer/referentiemodellen/IECCIM/TC57CIM/IEC61970/Base/ControlArea#TieFlow.positiveFlowIn">
        <rdfs:domain rdf:resource="https://w3id.org/netbeheer/referentiemodellen/IECCIM/TC57CIM/IEC61970/Base/ControlArea#TieFlow"/>
        <rdfs:range rdf:resource="http://www.w3.org/2001/XMLSchema#boolean"/>
        <rdfs:comment>True if the flow into the terminal (load convention) is also flow into the control area.  For example, this attribute should be true if using the tie line terminal further away from the control area. For example to represent a tie to a shunt component (like a load or generator) in another area, this is the near end of a branch and this attribute would be specified as false.</rdfs:comment>
    </owl:DatatypeProperty>
    


    <!-- 
    ///////////////////////////////////////////////////////////////////////////////////////
    //
    // Classes
    //
    ///////////////////////////////////////////////////////////////////////////////////////
     -->


    


    <!-- https://w3id.org/netbeheer/referentiemodellen/IECCIM/TC57CIM/IEC61970/Base/ControlArea#AltGeneratingUnitMeas -->


    <owl:Class rdf:about="https://w3id.org/netbeheer/referentiemodellen/IECCIM/TC57CIM/IEC61970/Base/ControlArea#AltGeneratingUnitMeas">
        <rdfs:subClassOf>
            <owl:Restriction>
                <owl:onProperty rdf:resource="https://w3id.org/netbeheer/referentiemodellen/IECCIM/TC57CIM/IEC61970/Base/ControlArea#AltGeneratingUnitMeas.ControlAreaGeneratingUnit"/>
                <owl:minQualifiedCardinality rdf:datatype="http://www.w3.org/2001/XMLSchema#nonNegativeInteger">0</owl:minQualifiedCardinality>
                <owl:onClass rdf:resource="https://w3id.org/netbeheer/referentiemodellen/IECCIM/TC57CIM/IEC61970/Base/ControlArea#AltGeneratingUnitMeas"/>
            </owl:Restriction>
        </rdfs:subClassOf>
        <rdfs:subClassOf>
            <owl:Restriction>
                <owl:onProperty rdf:resource="https://w3id.org/netbeheer/referentiemodellen/IECCIM/TC57CIM/IEC61970/Base/ControlArea#AltGeneratingUnitMeas.priority"/>
                <owl:minQualifiedCardinality rdf:datatype="http://www.w3.org/2001/XMLSchema#nonNegativeInteger">0</owl:minQualifiedCardinality>
                <owl:onDataRange rdf:resource="http://www.w3.org/2001/XMLSchema#nonNegativeInteger"/>
            </owl:Restriction>
        </rdfs:subClassOf>
        <rdfs:subClassOf>
            <owl:Restriction>
                <owl:onProperty rdf:resource="https://w3id.org/netbeheer/referentiemodellen/IECCIM/TC57CIM/IEC61970/Base/ControlArea#AltGeneratingUnitMeas.priority"/>
                <owl:maxQualifiedCardinality rdf:datatype="http://www.w3.org/2001/XMLSchema#nonNegativeInteger">1</owl:maxQualifiedCardinality>
                <owl:onDataRange rdf:resource="http://www.w3.org/2001/XMLSchema#nonNegativeInteger"/>
            </owl:Restriction>
        </rdfs:subClassOf>
        <rdfs:comment>A prioritized measurement to be used for the generating unit in the control area specificaiton.</rdfs:comment>
    </owl:Class>
    


    <!-- https://w3id.org/netbeheer/referentiemodellen/IECCIM/TC57CIM/IEC61970/Base/ControlArea#AltTieMeas -->


    <owl:Class rdf:about="https://w3id.org/netbeheer/referentiemodellen/IECCIM/TC57CIM/IEC61970/Base/ControlArea#AltTieMeas">
        <rdfs:subClassOf>
            <owl:Restriction>
                <owl:onProperty rdf:resource="https://w3id.org/netbeheer/referentiemodellen/IECCIM/TC57CIM/IEC61970/Base/ControlArea#AltTieMeas.TieFlow"/>
                <owl:minQualifiedCardinality rdf:datatype="http://www.w3.org/2001/XMLSchema#nonNegativeInteger">0</owl:minQualifiedCardinality>
                <owl:onClass rdf:resource="https://w3id.org/netbeheer/referentiemodellen/IECCIM/TC57CIM/IEC61970/Base/ControlArea#AltTieMeas"/>
            </owl:Restriction>
        </rdfs:subClassOf>
        <rdfs:subClassOf>
            <owl:Restriction>
                <owl:onProperty rdf:resource="https://w3id.org/netbeheer/referentiemodellen/IECCIM/TC57CIM/IEC61970/Base/ControlArea#AltTieMeas.priority"/>
                <owl:minQualifiedCardinality rdf:datatype="http://www.w3.org/2001/XMLSchema#nonNegativeInteger">0</owl:minQualifiedCardinality>
                <owl:onDataRange rdf:resource="http://www.w3.org/2001/XMLSchema#nonNegativeInteger"/>
            </owl:Restriction>
        </rdfs:subClassOf>
        <rdfs:subClassOf>
            <owl:Restriction>
                <owl:onProperty rdf:resource="https://w3id.org/netbeheer/referentiemodellen/IECCIM/TC57CIM/IEC61970/Base/ControlArea#AltTieMeas.priority"/>
                <owl:maxQualifiedCardinality rdf:datatype="http://www.w3.org/2001/XMLSchema#nonNegativeInteger">1</owl:maxQualifiedCardinality>
                <owl:onDataRange rdf:resource="http://www.w3.org/2001/XMLSchema#nonNegativeInteger"/>
            </owl:Restriction>
        </rdfs:subClassOf>
        <rdfs:comment>A prioritized measurement to be used for the tie flow as part of the control area specification.</rdfs:comment>
    </owl:Class>
    


    <!-- https://w3id.org/netbeheer/referentiemodellen/IECCIM/TC57CIM/IEC61970/Base/ControlArea#ControlArea -->


    <owl:Class rdf:about="https://w3id.org/netbeheer/referentiemodellen/IECCIM/TC57CIM/IEC61970/Base/ControlArea#ControlArea">
        <rdfs:subClassOf rdf:resource="https://w3id.org/netbeheer/referentiemodellen/IECCIM/TC57CIM/IEC61970/Base/Core#PowerSystemResource"/>
        <rdfs:subClassOf>
            <owl:Restriction>
                <owl:onProperty rdf:resource="https://w3id.org/netbeheer/referentiemodellen/IECCIM/TC57CIM/IEC61970/Base/ControlArea#ControlArea.netInterchange"/>
                <owl:minQualifiedCardinality rdf:datatype="http://www.w3.org/2001/XMLSchema#nonNegativeInteger">0</owl:minQualifiedCardinality>
                <owl:onClass rdf:resource="https://w3id.org/netbeheer/referentiemodellen/IECCIM/TC57CIM/IEC61970/Base/Domain#ActivePower"/>
            </owl:Restriction>
        </rdfs:subClassOf>
        <rdfs:subClassOf>
            <owl:Restriction>
                <owl:onProperty rdf:resource="https://w3id.org/netbeheer/referentiemodellen/IECCIM/TC57CIM/IEC61970/Base/ControlArea#ControlArea.pTolerance"/>
                <owl:minQualifiedCardinality rdf:datatype="http://www.w3.org/2001/XMLSchema#nonNegativeInteger">0</owl:minQualifiedCardinality>
                <owl:onClass rdf:resource="https://w3id.org/netbeheer/referentiemodellen/IECCIM/TC57CIM/IEC61970/Base/Domain#ActivePower"/>
            </owl:Restriction>
        </rdfs:subClassOf>
        <rdfs:subClassOf>
            <owl:Restriction>
                <owl:onProperty rdf:resource="https://w3id.org/netbeheer/referentiemodellen/IECCIM/TC57CIM/IEC61970/Base/ControlArea#ControlArea.ControlAreaGeneratingUnit"/>
                <owl:qualifiedCardinality rdf:datatype="http://www.w3.org/2001/XMLSchema#nonNegativeInteger">1</owl:qualifiedCardinality>
                <owl:onClass rdf:resource="https://w3id.org/netbeheer/referentiemodellen/IECCIM/TC57CIM/IEC61970/Base/ControlArea#ControlArea"/>
            </owl:Restriction>
        </rdfs:subClassOf>
        <rdfs:subClassOf>
            <owl:Restriction>
                <owl:onProperty rdf:resource="https://w3id.org/netbeheer/referentiemodellen/IECCIM/TC57CIM/IEC61970/Base/ControlArea#ControlArea.TieFlow"/>
                <owl:qualifiedCardinality rdf:datatype="http://www.w3.org/2001/XMLSchema#nonNegativeInteger">1</owl:qualifiedCardinality>
                <owl:onClass rdf:resource="https://w3id.org/netbeheer/referentiemodellen/IECCIM/TC57CIM/IEC61970/Base/ControlArea#ControlArea"/>
            </owl:Restriction>
        </rdfs:subClassOf>
        <rdfs:subClassOf>
            <owl:Restriction>
                <owl:onProperty rdf:resource="https://w3id.org/netbeheer/referentiemodellen/IECCIM/TC57CIM/IEC61970/Base/ControlArea#ControlArea.netInterchange"/>
                <owl:maxQualifiedCardinality rdf:datatype="http://www.w3.org/2001/XMLSchema#nonNegativeInteger">1</owl:maxQualifiedCardinality>
                <owl:onClass rdf:resource="https://w3id.org/netbeheer/referentiemodellen/IECCIM/TC57CIM/IEC61970/Base/Domain#ActivePower"/>
            </owl:Restriction>
        </rdfs:subClassOf>
        <rdfs:subClassOf>
            <owl:Restriction>
                <owl:onProperty rdf:resource="https://w3id.org/netbeheer/referentiemodellen/IECCIM/TC57CIM/IEC61970/Base/ControlArea#ControlArea.pTolerance"/>
                <owl:maxQualifiedCardinality rdf:datatype="http://www.w3.org/2001/XMLSchema#nonNegativeInteger">1</owl:maxQualifiedCardinality>
                <owl:onClass rdf:resource="https://w3id.org/netbeheer/referentiemodellen/IECCIM/TC57CIM/IEC61970/Base/Domain#ActivePower"/>
            </owl:Restriction>
        </rdfs:subClassOf>
        <rdfs:subClassOf>
            <owl:Restriction>
                <owl:onProperty rdf:resource="https://w3id.org/netbeheer/referentiemodellen/IECCIM/TC57CIM/IEC61970/Base/ControlArea#ControlArea.type"/>
                <owl:minQualifiedCardinality rdf:datatype="http://www.w3.org/2001/XMLSchema#nonNegativeInteger">0</owl:minQualifiedCardinality>
                <owl:onDataRange rdf:resource="https://w3id.org/netbeheer/referentiemodellen/IECCIM/TC57CIM/IEC61970/Base/ControlArea#ControlAreaTypeKind"/>
            </owl:Restriction>
        </rdfs:subClassOf>
        <rdfs:subClassOf>
            <owl:Restriction>
                <owl:onProperty rdf:resource="https://w3id.org/netbeheer/referentiemodellen/IECCIM/TC57CIM/IEC61970/Base/ControlArea#ControlArea.type"/>
                <owl:maxQualifiedCardinality rdf:datatype="http://www.w3.org/2001/XMLSchema#nonNegativeInteger">1</owl:maxQualifiedCardinality>
                <owl:onDataRange rdf:resource="https://w3id.org/netbeheer/referentiemodellen/IECCIM/TC57CIM/IEC61970/Base/ControlArea#ControlAreaTypeKind"/>
            </owl:Restriction>
        </rdfs:subClassOf>
        <rdfs:comment>A control area is a grouping of generating units and/or loads and a cutset of tie lines (as terminals) which may be used for a variety of purposes including automatic generation control, powerflow solution area interchange control specification, and input to load forecasting.   Note that any number of overlapping control area specifications can be superimposed on the physical model.</rdfs:comment>
    </owl:Class>
    


    <!-- https://w3id.org/netbeheer/referentiemodellen/IECCIM/TC57CIM/IEC61970/Base/ControlArea#ControlAreaGeneratingUnit -->


    <owl:Class rdf:about="https://w3id.org/netbeheer/referentiemodellen/IECCIM/TC57CIM/IEC61970/Base/ControlArea#ControlAreaGeneratingUnit">
        <rdfs:subClassOf rdf:resource="https://w3id.org/netbeheer/referentiemodellen/IECCIM/TC57CIM/IEC61970/Base/Core#IdentifiedObject"/>
        <rdfs:subClassOf>
            <owl:Restriction>
                <owl:onProperty rdf:resource="https://w3id.org/netbeheer/referentiemodellen/IECCIM/TC57CIM/IEC61970/Base/ControlArea#ControlAreaGeneratingUnit.ControlArea"/>
                <owl:minQualifiedCardinality rdf:datatype="http://www.w3.org/2001/XMLSchema#nonNegativeInteger">0</owl:minQualifiedCardinality>
                <owl:onClass rdf:resource="https://w3id.org/netbeheer/referentiemodellen/IECCIM/TC57CIM/IEC61970/Base/ControlArea#ControlAreaGeneratingUnit"/>
            </owl:Restriction>
        </rdfs:subClassOf>
        <rdfs:subClassOf>
            <owl:Restriction>
                <owl:onProperty rdf:resource="https://w3id.org/netbeheer/referentiemodellen/IECCIM/TC57CIM/IEC61970/Base/ControlArea#ControlAreaGeneratingUnit.AltGeneratingUnitMeas"/>
                <owl:qualifiedCardinality rdf:datatype="http://www.w3.org/2001/XMLSchema#nonNegativeInteger">1</owl:qualifiedCardinality>
                <owl:onClass rdf:resource="https://w3id.org/netbeheer/referentiemodellen/IECCIM/TC57CIM/IEC61970/Base/ControlArea#ControlAreaGeneratingUnit"/>
            </owl:Restriction>
        </rdfs:subClassOf>
        <rdfs:comment>A control area generating unit. This class is needed so that alternate control area definitions may include the same generating unit.   Note only one instance within a control area should reference a specific generating unit.</rdfs:comment>
    </owl:Class>
    


    <!-- https://w3id.org/netbeheer/referentiemodellen/IECCIM/TC57CIM/IEC61970/Base/ControlArea#TieFlow -->


    <owl:Class rdf:about="https://w3id.org/netbeheer/referentiemodellen/IECCIM/TC57CIM/IEC61970/Base/ControlArea#TieFlow">
        <rdfs:subClassOf>
            <owl:Restriction>
                <owl:onProperty rdf:resource="https://w3id.org/netbeheer/referentiemodellen/IECCIM/TC57CIM/IEC61970/Base/ControlArea#TieFlow.ControlArea"/>
                <owl:minQualifiedCardinality rdf:datatype="http://www.w3.org/2001/XMLSchema#nonNegativeInteger">0</owl:minQualifiedCardinality>
                <owl:onClass rdf:resource="https://w3id.org/netbeheer/referentiemodellen/IECCIM/TC57CIM/IEC61970/Base/ControlArea#TieFlow"/>
            </owl:Restriction>
        </rdfs:subClassOf>
        <rdfs:subClassOf>
            <owl:Restriction>
                <owl:onProperty rdf:resource="https://w3id.org/netbeheer/referentiemodellen/IECCIM/TC57CIM/IEC61970/Base/ControlArea#TieFlow.AltTieMeas"/>
                <owl:qualifiedCardinality rdf:datatype="http://www.w3.org/2001/XMLSchema#nonNegativeInteger">1</owl:qualifiedCardinality>
                <owl:onClass rdf:resource="https://w3id.org/netbeheer/referentiemodellen/IECCIM/TC57CIM/IEC61970/Base/ControlArea#TieFlow"/>
            </owl:Restriction>
        </rdfs:subClassOf>
        <rdfs:subClassOf>
            <owl:Restriction>
                <owl:onProperty rdf:resource="https://w3id.org/netbeheer/referentiemodellen/IECCIM/TC57CIM/IEC61970/Base/ControlArea#TieFlow.positiveFlowIn"/>
                <owl:minQualifiedCardinality rdf:datatype="http://www.w3.org/2001/XMLSchema#nonNegativeInteger">0</owl:minQualifiedCardinality>
                <owl:onDataRange rdf:resource="http://www.w3.org/2001/XMLSchema#boolean"/>
            </owl:Restriction>
        </rdfs:subClassOf>
        <rdfs:subClassOf>
            <owl:Restriction>
                <owl:onProperty rdf:resource="https://w3id.org/netbeheer/referentiemodellen/IECCIM/TC57CIM/IEC61970/Base/ControlArea#TieFlow.positiveFlowIn"/>
                <owl:maxQualifiedCardinality rdf:datatype="http://www.w3.org/2001/XMLSchema#nonNegativeInteger">1</owl:maxQualifiedCardinality>
                <owl:onDataRange rdf:resource="http://www.w3.org/2001/XMLSchema#boolean"/>
            </owl:Restriction>
        </rdfs:subClassOf>
        <rdfs:comment>A flow specification in terms of location and direction for a control area.</rdfs:comment>
    </owl:Class>
    


    <!-- https://w3id.org/netbeheer/referentiemodellen/IECCIM/TC57CIM/IEC61970/Base/Core#IdentifiedObject -->


    <owl:Class rdf:about="https://w3id.org/netbeheer/referentiemodellen/IECCIM/TC57CIM/IEC61970/Base/Core#IdentifiedObject"/>
    


    <!-- https://w3id.org/netbeheer/referentiemodellen/IECCIM/TC57CIM/IEC61970/Base/Core#PowerSystemResource -->


    <owl:Class rdf:about="https://w3id.org/netbeheer/referentiemodellen/IECCIM/TC57CIM/IEC61970/Base/Core#PowerSystemResource"/>
    


    <!-- https://w3id.org/netbeheer/referentiemodellen/IECCIM/TC57CIM/IEC61970/Base/Domain#ActivePower -->


    <owl:Class rdf:about="https://w3id.org/netbeheer/referentiemodellen/IECCIM/TC57CIM/IEC61970/Base/Domain#ActivePower"/>
</rdf:RDF>



<!-- Generated by the OWL API (version 5.1.10.2019-03-12T22:31:15Z) https://github.com/owlcs/owlapi/ -->


