@prefix : <https://w3id.org/netbeheer/IECCIM/TC57CIM/IEC61970/Base/Core#> .
@prefix owl: <http://www.w3.org/2002/07/owl#> .
@prefix rdf: <http://www.w3.org/1999/02/22-rdf-syntax-ns#> .
@prefix xml: <http://www.w3.org/XML/1998/namespace> .
@prefix xsd: <http://www.w3.org/2001/XMLSchema#> .
@prefix rdfs: <http://www.w3.org/2000/01/rdf-schema#> .
@base <https://w3id.org/netbeheer/IECCIM/TC57CIM/IEC61970/Base/Core#> .

<https://w3id.org/netbeheer/IECCIM/TC57CIM/IEC61970/Base/Core#> rdf:type owl:Ontology .

#################################################################
#    Datatypes
#################################################################

###  https://w3id.org/netbeheer/IECCIM/TC57CIM/IEC61970/Base/Core#BreakerConfiguration
:BreakerConfiguration rdf:type rdfs:Datatype ;
                      owl:equivalentClass [ rdf:type rdfs:Datatype ;
                                            owl:oneOf [ rdf:type rdf:List ;
                                                        rdf:first "breakerAndAHalf" ;
                                                        rdf:rest [ rdf:type rdf:List ;
                                                                   rdf:first "doubleBreaker" ;
                                                                   rdf:rest [ rdf:type rdf:List ;
                                                                              rdf:first "noBreaker" ;
                                                                              rdf:rest [ rdf:type rdf:List ;
                                                                                         rdf:first "singleBreaker" ;
                                                                                         rdf:rest rdf:nil
                                                                                       ]
                                                                            ]
                                                                 ]
                                                      ]
                                          ] .


###  https://w3id.org/netbeheer/IECCIM/TC57CIM/IEC61970/Base/Core#BusbarConfiguration
:BusbarConfiguration rdf:type rdfs:Datatype ;
                     owl:equivalentClass [ rdf:type rdfs:Datatype ;
                                           owl:oneOf [ rdf:type rdf:List ;
                                                       rdf:first "doubleBus" ;
                                                       rdf:rest [ rdf:type rdf:List ;
                                                                  rdf:first "mainWithTransfer" ;
                                                                  rdf:rest [ rdf:type rdf:List ;
                                                                             rdf:first "ringBus" ;
                                                                             rdf:rest [ rdf:type rdf:List ;
                                                                                        rdf:first "singleBus" ;
                                                                                        rdf:rest rdf:nil
                                                                                      ]
                                                                           ]
                                                                ]
                                                     ]
                                         ] .


###  https://w3id.org/netbeheer/IECCIM/TC57CIM/IEC61970/Base/Core#CurveStyle
:CurveStyle rdf:type rdfs:Datatype ;
            owl:equivalentClass [ rdf:type rdfs:Datatype ;
                                  owl:oneOf [ rdf:type rdf:List ;
                                              rdf:first "constantYValue" ;
                                              rdf:rest [ rdf:type rdf:List ;
                                                         rdf:first "straightLineYValues" ;
                                                         rdf:rest rdf:nil
                                                       ]
                                            ]
                                ] .


###  https://w3id.org/netbeheer/IECCIM/TC57CIM/IEC61970/Base/Core#PhaseCode
:PhaseCode rdf:type rdfs:Datatype ;
           owl:equivalentClass [ rdf:type rdfs:Datatype ;
                                 owl:oneOf [ rdf:type rdf:List ;
                                             rdf:first "A" ;
                                             rdf:rest [ rdf:type rdf:List ;
                                                        rdf:first "AB" ;
                                                        rdf:rest [ rdf:type rdf:List ;
                                                                   rdf:first "ABC" ;
                                                                   rdf:rest [ rdf:type rdf:List ;
                                                                              rdf:first "ABCN" ;
                                                                              rdf:rest [ rdf:type rdf:List ;
                                                                                         rdf:first "ABN" ;
                                                                                         rdf:rest [ rdf:type rdf:List ;
                                                                                                    rdf:first "AC" ;
                                                                                                    rdf:rest [ rdf:type rdf:List ;
                                                                                                               rdf:first "ACN" ;
                                                                                                               rdf:rest [ rdf:type rdf:List ;
                                                                                                                          rdf:first "AN" ;
                                                                                                                          rdf:rest [ rdf:type rdf:List ;
                                                                                                                                     rdf:first "B" ;
                                                                                                                                     rdf:rest [ rdf:type rdf:List ;
                                                                                                                                                rdf:first "BC" ;
                                                                                                                                                rdf:rest [ rdf:type rdf:List ;
                                                                                                                                                           rdf:first "BCN" ;
                                                                                                                                                           rdf:rest [ rdf:type rdf:List ;
                                                                                                                                                                      rdf:first "BN" ;
                                                                                                                                                                      rdf:rest [ rdf:type rdf:List ;
                                                                                                                                                                                 rdf:first "C" ;
                                                                                                                                                                                 rdf:rest [ rdf:type rdf:List ;
                                                                                                                                                                                            rdf:first "CN" ;
                                                                                                                                                                                            rdf:rest [ rdf:type rdf:List ;
                                                                                                                                                                                                       rdf:first "N" ;
                                                                                                                                                                                                       rdf:rest [ rdf:type rdf:List ;
                                                                                                                                                                                                                  rdf:first "X" ;
                                                                                                                                                                                                                  rdf:rest [ rdf:type rdf:List ;
                                                                                                                                                                                                                             rdf:first "XN" ;
                                                                                                                                                                                                                             rdf:rest [ rdf:type rdf:List ;
                                                                                                                                                                                                                                        rdf:first "XY" ;
                                                                                                                                                                                                                                        rdf:rest [ rdf:type rdf:List ;
                                                                                                                                                                                                                                                   rdf:first "XYN" ;
                                                                                                                                                                                                                                                   rdf:rest [ rdf:type rdf:List ;
                                                                                                                                                                                                                                                              rdf:first "none" ;
                                                                                                                                                                                                                                                              rdf:rest [ rdf:type rdf:List ;
                                                                                                                                                                                                                                                                         rdf:first "s1" ;
                                                                                                                                                                                                                                                                         rdf:rest [ rdf:type rdf:List ;
                                                                                                                                                                                                                                                                                    rdf:first "s12" ;
                                                                                                                                                                                                                                                                                    rdf:rest [ rdf:type rdf:List ;
                                                                                                                                                                                                                                                                                               rdf:first "s12N" ;
                                                                                                                                                                                                                                                                                               rdf:rest [ rdf:type rdf:List ;
                                                                                                                                                                                                                                                                                                          rdf:first "s1N" ;
                                                                                                                                                                                                                                                                                                          rdf:rest [ rdf:type rdf:List ;
                                                                                                                                                                                                                                                                                                                     rdf:first "s2" ;
                                                                                                                                                                                                                                                                                                                     rdf:rest [ rdf:type rdf:List ;
                                                                                                                                                                                                                                                                                                                                rdf:first "s2N" ;
                                                                                                                                                                                                                                                                                                                                rdf:rest rdf:nil
                                                                                                                                                                                                                                                                                                                              ]
                                                                                                                                                                                                                                                                                                                   ]
                                                                                                                                                                                                                                                                                                        ]
                                                                                                                                                                                                                                                                                             ]
                                                                                                                                                                                                                                                                                  ]
                                                                                                                                                                                                                                                                       ]
                                                                                                                                                                                                                                                            ]
                                                                                                                                                                                                                                                 ]
                                                                                                                                                                                                                                      ]
                                                                                                                                                                                                                           ]
                                                                                                                                                                                                                ]
                                                                                                                                                                                                     ]
                                                                                                                                                                                          ]
                                                                                                                                                                               ]
                                                                                                                                                                    ]
                                                                                                                                                         ]
                                                                                                                                              ]
                                                                                                                                   ]
                                                                                                                        ]
                                                                                                             ]
                                                                                                  ]
                                                                                       ]
                                                                            ]
                                                                 ]
                                                      ]
                                           ]
                               ] .


###  https://w3id.org/netbeheer/IECCIM/TC57CIM/IEC61970/Base/Domain#UnitMultiplier
<https://w3id.org/netbeheer/IECCIM/TC57CIM/IEC61970/Base/Domain#UnitMultiplier> rdf:type rdfs:Datatype .


###  https://w3id.org/netbeheer/IECCIM/TC57CIM/IEC61970/Base/Domain#UnitSymbol
<https://w3id.org/netbeheer/IECCIM/TC57CIM/IEC61970/Base/Domain#UnitSymbol> rdf:type rdfs:Datatype .


#################################################################
#    Object Properties
#################################################################

###  https://w3id.org/netbeheer/IECCIM/TC57CIM/IEC61970/Base/Core#ACDCConverter_PccTerminal
:ACDCConverter_PccTerminal rdf:type owl:ObjectProperty ;
                           rdfs:domain <https://w3id.org/netbeheer/IECCIM/TC57CIM/IEC61970/Base/DC#ACDCConverter> ;
                           rdfs:range :Terminal ;
                           rdfs:comment "All converters' DC sides linked to this point of common coupling terminal.Point of common coupling terminal for this converter DC side. It is typically the terminal on the power transformer (or switch) closest to the AC network. The power flow measurement must be the sum of all flows into the transformer." .


###  https://w3id.org/netbeheer/IECCIM/TC57CIM/IEC61970/Base/Core#ACDCTerminal_BusNameMarker
:ACDCTerminal_BusNameMarker rdf:type owl:ObjectProperty ;
                            owl:inverseOf :BusNameMarker_Terminal ;
                            rdfs:domain :ACDCTerminal ;
                            rdfs:range <https://w3id.org/netbeheer/IECCIM/TC57CIM/IEC61970/Base/Topology#BusNameMarker> ;
                            rdfs:comment "The bus name marker used to name the bus (topological node).The terminals associated with this bus name marker." .


###  https://w3id.org/netbeheer/IECCIM/TC57CIM/IEC61970/Base/Core#ACDCTerminal_Measurements
:ACDCTerminal_Measurements rdf:type owl:ObjectProperty ;
                           owl:inverseOf :Measure_Terminal ;
                           rdfs:domain :ACDCTerminal ;
                           rdfs:range <https://w3id.org/netbeheer/IECCIM/TC57CIM/IEC61970/Base/Meas#Measure> ;
                           rdfs:comment "Measurements associated with this terminal defining  where the measurement is placed in the network topology.  It may be used, for instance, to capture the sensor position, such as a voltage transformer (PT) at a busbar or a current transformer (CT) at the bar between a breaker and an isolator.One or more measurements may be associated with a terminal in the network." .


###  https://w3id.org/netbeheer/IECCIM/TC57CIM/IEC61970/Base/Core#ACDCTerminal_OperationalLimitSet
:ACDCTerminal_OperationalLimitSet rdf:type owl:ObjectProperty ;
                                  owl:inverseOf :OperationalLimitSet_Terminal ;
                                  rdfs:domain :ACDCTerminal ;
                                  rdfs:range <https://w3id.org/netbeheer/IECCIM/TC57CIM/IEC61970/Base/OperationalLimits#OperationalLimitSet> ;
                                  rdfs:comment "" .


###  https://w3id.org/netbeheer/IECCIM/TC57CIM/IEC61970/Base/Core#AssetInfo_PowerSystemResources
:AssetInfo_PowerSystemResources rdf:type owl:ObjectProperty ;
                                rdfs:domain <https://w3id.org/netbeheer/IECCIM/TC57CIM/IEC61968/Assets#AssetInfo> ;
                                rdfs:range :PowerSystemResource ;
                                rdfs:comment "Datasheet information for this power system resource.All power system resources with this datasheet information." .


###  https://w3id.org/netbeheer/IECCIM/TC57CIM/IEC61970/Base/Core#Asset_PowerSystemResources
:Asset_PowerSystemResources rdf:type owl:ObjectProperty ;
                            rdfs:domain <https://w3id.org/netbeheer/IECCIM/TC57CIM/IEC61968/Assets#Asset> ;
                            rdfs:range :PowerSystemResource ;
                            rdfs:comment "All assets represented by this power system resource. For example, multiple conductor assets are electrically modelled as a single AC line segment.All power system resources used to electrically model this asset. For example, transformer asset is electrically modelled with a transformer and its windings and tap changer." .


###  https://w3id.org/netbeheer/IECCIM/TC57CIM/IEC61970/Base/Core#AuxiliaryEquipment_Terminal
:AuxiliaryEquipment_Terminal rdf:type owl:ObjectProperty ;
                             rdfs:domain <https://w3id.org/netbeheer/IECCIM/TC57CIM/IEC61970/Base/AuxiliaryEquipment#AuxiliaryEquipment> ;
                             rdfs:range :Terminal ;
                             rdfs:comment "The auxiliary equipment connected to the terminal.The Terminal at the equipment where the AuxiliaryEquipment is attached." .


###  https://w3id.org/netbeheer/IECCIM/TC57CIM/IEC61970/Base/Core#BaseFrequency_frequency
:BaseFrequency_frequency rdf:type owl:ObjectProperty ;
                         rdfs:domain :BaseFrequency ;
                         rdfs:range <https://w3id.org/netbeheer/IECCIM/TC57CIM/IEC61970/Base/Domain#Frequency> ;
                         rdfs:comment "The base frequency." .


###  https://w3id.org/netbeheer/IECCIM/TC57CIM/IEC61970/Base/Core#BasePower_basePower
:BasePower_basePower rdf:type owl:ObjectProperty ;
                     rdfs:domain :BasePower ;
                     rdfs:range <https://w3id.org/netbeheer/IECCIM/TC57CIM/IEC61970/Base/Domain#ApparentPower> ;
                     rdfs:comment """Value used as base power.
""" .


###  https://w3id.org/netbeheer/IECCIM/TC57CIM/IEC61970/Base/Core#BaseVoltage_ConductingEquipment
:BaseVoltage_ConductingEquipment rdf:type owl:ObjectProperty ;
                                 rdfs:domain :BaseVoltage ;
                                 rdfs:range :ConductingEquipment ;
                                 rdfs:comment "Base voltage of this conducting equipment.  Use only when there is no voltage level container used and only one base voltage applies.  For example, not used for transformers.All conducting equipment with this base voltage.  Use only when there is no voltage level container used and only one base voltage applies.  For example, not used for transformers." .


###  https://w3id.org/netbeheer/IECCIM/TC57CIM/IEC61970/Base/Core#BaseVoltage_TopologicalNode
:BaseVoltage_TopologicalNode rdf:type owl:ObjectProperty ;
                             owl:inverseOf :TopologicalNode_BaseVoltage ;
                             rdfs:domain :BaseVoltage ;
                             rdfs:range <https://w3id.org/netbeheer/IECCIM/TC57CIM/IEC61970/Base/Topology#TopologicalNode> ;
                             rdfs:comment "The topological nodes at the base voltage.The base voltage of the topologocial node." .


###  https://w3id.org/netbeheer/IECCIM/TC57CIM/IEC61970/Base/Core#BaseVoltage_TransformerEnds
:BaseVoltage_TransformerEnds rdf:type owl:ObjectProperty ;
                             owl:inverseOf :TransformerEnd_BaseVoltage ;
                             rdfs:domain :BaseVoltage ;
                             rdfs:range <https://w3id.org/netbeheer/IECCIM/TC57CIM/IEC61970/Base/Wires#TransformerEnd> ;
                             rdfs:comment "Transformer ends at the base voltage.  This is essential for PU calculation.Base voltage of the transformer end.  This is essential for PU calculation." .


###  https://w3id.org/netbeheer/IECCIM/TC57CIM/IEC61970/Base/Core#BaseVoltage_VoltageLevel
:BaseVoltage_VoltageLevel rdf:type owl:ObjectProperty ;
                          owl:inverseOf :VoltageLevel_BaseVoltage ;
                          rdf:type owl:FunctionalProperty ;
                          rdfs:domain :BaseVoltage ;
                          rdfs:range :VoltageLevel ;
                          rdfs:comment "The voltage levels having this base voltage.The base voltage used for all equipment within the voltage level." .


###  https://w3id.org/netbeheer/IECCIM/TC57CIM/IEC61970/Base/Core#BaseVoltage_nominalVoltage
:BaseVoltage_nominalVoltage rdf:type owl:ObjectProperty ;
                            rdfs:domain :BaseVoltage ;
                            rdfs:range <https://w3id.org/netbeheer/IECCIM/TC57CIM/IEC61970/Base/Domain#Voltage> ;
                            rdfs:comment """The power system resource's base voltage.
""" .


###  https://w3id.org/netbeheer/IECCIM/TC57CIM/IEC61970/Base/Core#Bay_Substation
:Bay_Substation rdf:type owl:ObjectProperty ;
                rdfs:domain :Bay ;
                rdfs:range :Substation ;
                rdfs:comment "Bays contained in the substation.Substation containing the bay." .


###  https://w3id.org/netbeheer/IECCIM/TC57CIM/IEC61970/Base/Core#Bay_VoltageLevel
:Bay_VoltageLevel rdf:type owl:ObjectProperty ;
                  owl:inverseOf :VoltageLevel_Bays ;
                  rdfs:domain :Bay ;
                  rdfs:range :VoltageLevel ;
                  rdfs:comment "The voltage level containing this bay.The bays within this voltage level." .


###  https://w3id.org/netbeheer/IECCIM/TC57CIM/IEC61970/Base/Core#BranchGroupTerminal_Terminal
:BranchGroupTerminal_Terminal rdf:type owl:ObjectProperty ;
                              rdfs:domain <https://w3id.org/netbeheer/IECCIM/TC57CIM/IEC61970/Base/OperationalLimits#BranchGroupTerminal> ;
                              rdfs:range :Terminal ;
                              rdfs:comment "The directed branch group terminals for which this terminal is monitored. The terminal to be summed." .


###  https://w3id.org/netbeheer/IECCIM/TC57CIM/IEC61970/Base/Core#BusNameMarker_ReportingGroup
:BusNameMarker_ReportingGroup rdf:type owl:ObjectProperty ;
                              rdfs:domain <https://w3id.org/netbeheer/IECCIM/TC57CIM/IEC61970/Base/Topology#BusNameMarker> ;
                              rdfs:range :ReportingGroup ;
                              rdfs:comment "The bus name markers that belong to this reporting group.The reporting group to which this bus name marker belongs." .


###  https://w3id.org/netbeheer/IECCIM/TC57CIM/IEC61970/Base/Core#BusNameMarker_Terminal
:BusNameMarker_Terminal rdf:type owl:ObjectProperty ;
                        rdfs:domain <https://w3id.org/netbeheer/IECCIM/TC57CIM/IEC61970/Base/Topology#BusNameMarker> ;
                        rdfs:range :ACDCTerminal ;
                        rdfs:comment "The bus name marker used to name the bus (topological node).The terminals associated with this bus name marker." .


###  https://w3id.org/netbeheer/IECCIM/TC57CIM/IEC61970/Base/Core#Bushing_Terminal
:Bushing_Terminal rdf:type owl:ObjectProperty ;
                  rdfs:domain <https://w3id.org/netbeheer/IECCIM/TC57CIM/IEC61968/InfIEC61968/InfAssets#Bushing> ;
                  rdfs:range :Terminal ;
                  rdfs:comment "" .


###  https://w3id.org/netbeheer/IECCIM/TC57CIM/IEC61970/Base/Core#CIMDataObject_PropertiesObject
:CIMDataObject_PropertiesObject rdf:type owl:ObjectProperty ;
                                rdfs:domain <https://w3id.org/netbeheer/IECCIM/TC57CIM/IEC61970/InfIEC61970/InfGenericDataset/CanonicalModel/GenericDatasetCore#CIMDataObject> ;
                                rdfs:range :IdentifiedObject ;
                                rdfs:comment "The single CIM data object in the appropriate dataset context.The CIM object holding the properties of this dataset context.   Sometimes properties are not required and only the reference to the registered object is required." .


###  https://w3id.org/netbeheer/IECCIM/TC57CIM/IEC61970/Base/Core#CIMDataObject_RegisteredObject
:CIMDataObject_RegisteredObject rdf:type owl:ObjectProperty ;
                                rdfs:domain <https://w3id.org/netbeheer/IECCIM/TC57CIM/IEC61970/InfIEC61970/InfGenericDataset/CanonicalModel/GenericDatasetCore#CIMDataObject> ;
                                rdfs:range :IdentifiedObject ;
                                rdfs:comment "Data objects registered.The registered CIM object." .


###  https://w3id.org/netbeheer/IECCIM/TC57CIM/IEC61970/Base/Core#ClearanceDocument_TaggedPSRs
:ClearanceDocument_TaggedPSRs rdf:type owl:ObjectProperty ;
                              rdfs:domain <https://w3id.org/netbeheer/IECCIM/TC57CIM/IEC61968/Operations#ClearanceDocument> ;
                              rdfs:range :PowerSystemResource ;
                              rdfs:comment "All clearances applicable to this power system resource.All power system resources tagged through this clearance." .


###  https://w3id.org/netbeheer/IECCIM/TC57CIM/IEC61970/Base/Core#ConductingEquipment_BaseVoltage
:ConductingEquipment_BaseVoltage rdf:type owl:ObjectProperty ;
                                 owl:inverseOf :BaseVoltage_ConductingEquipment ;
                                 rdfs:domain :ConductingEquipment ;
                                 rdfs:range :BaseVoltage ;
                                 rdfs:comment "Base voltage of this conducting equipment.  Use only when there is no voltage level container used and only one base voltage applies.  For example, not used for transformers.All conducting equipment with this base voltage.  Use only when there is no voltage level container used and only one base voltage applies.  For example, not used for transformers." .


###  https://w3id.org/netbeheer/IECCIM/TC57CIM/IEC61970/Base/Core#ConductingEquipment_GroundingAction
:ConductingEquipment_GroundingAction rdf:type owl:ObjectProperty ;
                                     owl:inverseOf :GroundAction_GroundedEquipment ;
                                     rdfs:domain :ConductingEquipment ;
                                     rdfs:range <https://w3id.org/netbeheer/IECCIM/TC57CIM/IEC61968/Operations#GroundAction> ;
                                     rdfs:comment "Action involving grounding operation on this conducting equipment.Equipment being grounded with this operation. In case of placing a ground anywhere along a line segment, you must use the clamp (to get the distance from one terminal), so use the explicit relation with line segment. In all other cases (including placing the ground at a line segment terminal), reference to one or more conducting equipment is sufficient." .


###  https://w3id.org/netbeheer/IECCIM/TC57CIM/IEC61970/Base/Core#ConductingEquipment_JumpingAction
:ConductingEquipment_JumpingAction rdf:type owl:ObjectProperty ;
                                   owl:inverseOf :JumperAction_JumpedEquipments ;
                                   rdfs:domain :ConductingEquipment ;
                                   rdfs:range <https://w3id.org/netbeheer/IECCIM/TC57CIM/IEC61968/Operations#JumperAction> ;
                                   rdfs:comment "Jumper action involving jumping operation on this conducting equipment.The conducting equipment that this jumper action will affect. In case of placing a jumper anywhere along a line segment, you must use the clamp (to get the distance from one terminal), so use the explicit relation with line segment. In all other cases (including placing the jumper at a line segment terminal), reference to one or more conducting equipment is sufficient." .


###  https://w3id.org/netbeheer/IECCIM/TC57CIM/IEC61970/Base/Core#ConductingEquipment_ProtectionEquipments
:ConductingEquipment_ProtectionEquipments rdf:type owl:ObjectProperty ;
                                          owl:inverseOf :ProtectionEquipment_ConductingEquipments ;
                                          rdfs:domain :ConductingEquipment ;
                                          rdfs:range <https://w3id.org/netbeheer/IECCIM/TC57CIM/IEC61970/Base/Protection#ProtectionEquipment> ;
                                          rdfs:comment "Protection equipment  used to protect specific conducting equipment. Protection equipment may be used to protect specific conducting equipment." .


###  https://w3id.org/netbeheer/IECCIM/TC57CIM/IEC61970/Base/Core#ConductingEquipment_ProtectiveActionAdjustment
:ConductingEquipment_ProtectiveActionAdjustment rdf:type owl:ObjectProperty ,
                                                         owl:FunctionalProperty ;
                                                rdfs:domain :ConductingEquipment ;
                                                rdfs:range <https://w3id.org/netbeheer/IECCIM/TC57CIM/IEC61970/InfIEC61970/InfSIPS#ProtectiveActionAdjustment> ;
                                                rdfs:comment "The operating condition to the Conducting Equipment is changed when protective action adjustment is activated. For Shunt Compensator or other conducting equipment that operates on discrete values (integer), the values given in float will be rounded. The operating condition to the Conducting Equipment is changed when protective action adjustment is activated. For Shunt Compensator or other conducting equipment that operates on discrete values (integer), the values given in float will be rounded. " .


###  https://w3id.org/netbeheer/IECCIM/TC57CIM/IEC61970/Base/Core#ConductingEquipment_SvStatus
:ConductingEquipment_SvStatus rdf:type owl:ObjectProperty ;
                              owl:inverseOf :SvStatus_ConductingEquipment ;
                              rdf:type owl:FunctionalProperty ;
                              rdfs:domain :ConductingEquipment ;
                              rdfs:range <https://w3id.org/netbeheer/IECCIM/TC57CIM/IEC61970/Base/StateVariables#SvStatus> ;
                              rdfs:comment "The status state variable associated with this conducting equipment.The conducting equipment associated with the status state variable." .


###  https://w3id.org/netbeheer/IECCIM/TC57CIM/IEC61970/Base/Core#ConductingEquipment_Terminals
:ConductingEquipment_Terminals rdf:type owl:ObjectProperty ;
                               owl:inverseOf :Terminal_ConductingEquipment ;
                               rdf:type owl:FunctionalProperty ;
                               rdfs:domain :ConductingEquipment ;
                               rdfs:range :Terminal ;
                               rdfs:comment "Conducting equipment have terminals that may be connected to other conducting equipment terminals via connectivity nodes or topological nodes.The conducting equipment of the terminal.  Conducting equipment have  terminals that may be connected to other conducting equipment terminals via connectivity nodes or topological nodes." .


###  https://w3id.org/netbeheer/IECCIM/TC57CIM/IEC61970/Base/Core#ConnectivityNodeContainer_ConnectivityNodes
:ConnectivityNodeContainer_ConnectivityNodes rdf:type owl:ObjectProperty ;
                                             owl:inverseOf :ConnectivityNode_ConnectivityNodeContainer ;
                                             rdf:type owl:FunctionalProperty ;
                                             rdfs:domain :ConnectivityNodeContainer ;
                                             rdfs:range :ConnectivityNode ;
                                             rdfs:comment "Connectivity nodes which belong to this connectivity node container.Container of this connectivity node." .


###  https://w3id.org/netbeheer/IECCIM/TC57CIM/IEC61970/Base/Core#ConnectivityNodeContainer_TopologicalNode
:ConnectivityNodeContainer_TopologicalNode rdf:type owl:ObjectProperty ;
                                           owl:inverseOf :TopologicalNode_ConnectivityNodeContainer ;
                                           rdfs:domain :ConnectivityNodeContainer ;
                                           rdfs:range <https://w3id.org/netbeheer/IECCIM/TC57CIM/IEC61970/Base/Topology#TopologicalNode> ;
                                           rdfs:comment "The topological nodes which belong to this connectivity node container.The connectivity node container to which the toplogical node belongs." .


###  https://w3id.org/netbeheer/IECCIM/TC57CIM/IEC61970/Base/Core#ConnectivityNode_ConnectivityNodeContainer
:ConnectivityNode_ConnectivityNodeContainer rdf:type owl:ObjectProperty ;
                                            rdfs:domain :ConnectivityNode ;
                                            rdfs:range :ConnectivityNodeContainer ;
                                            rdfs:comment "Connectivity nodes which belong to this connectivity node container.Container of this connectivity node." .


###  https://w3id.org/netbeheer/IECCIM/TC57CIM/IEC61970/Base/Core#ConnectivityNode_Terminals
:ConnectivityNode_Terminals rdf:type owl:ObjectProperty ;
                            owl:inverseOf :Terminal_ConnectivityNode ;
                            rdfs:domain :ConnectivityNode ;
                            rdfs:range :Terminal ;
                            rdfs:comment "Terminals interconnected with zero impedance at a this connectivity node. The connectivity node to which this terminal connects with zero impedance." .


###  https://w3id.org/netbeheer/IECCIM/TC57CIM/IEC61970/Base/Core#ConnectivityNode_TopologicalNode
:ConnectivityNode_TopologicalNode rdf:type owl:ObjectProperty ;
                                  rdfs:domain :ConnectivityNode ;
                                  rdfs:range <https://w3id.org/netbeheer/IECCIM/TC57CIM/IEC61970/Base/Topology#TopologicalNode> ;
                                  rdfs:comment "The connectivity nodes combine together to form this topological node.  May depend on the current state of switches in the network.The topological node to which this connectivity node is assigned.  May depend on the current state of switches in the network." .


###  https://w3id.org/netbeheer/IECCIM/TC57CIM/IEC61970/Base/Core#ContingencyEquipment_Equipment
:ContingencyEquipment_Equipment rdf:type owl:ObjectProperty ;
                                rdfs:domain <https://w3id.org/netbeheer/IECCIM/TC57CIM/IEC61970/Base/Contingency#ContingencyEquipment> ;
                                rdfs:range :Equipment ;
                                rdfs:comment "The contingency equipments in which this equipment participates.The single piece of equipment to which to apply the contingency." .


###  https://w3id.org/netbeheer/IECCIM/TC57CIM/IEC61970/Base/Core#Control_PowerSystemResource
:Control_PowerSystemResource rdf:type owl:ObjectProperty ;
                             owl:inverseOf :PowerSystemResource_Controls ;
                             rdfs:domain <https://w3id.org/netbeheer/IECCIM/TC57CIM/IEC61970/Base/Meas#Control> ;
                             rdfs:range :PowerSystemResource ;
                             rdfs:comment "Regulating device governed by this control output.The controller outputs used to actually govern a regulating device, e.g. the magnetization of a synchronous machine or capacitor bank breaker actuator." .


###  https://w3id.org/netbeheer/IECCIM/TC57CIM/IEC61970/Base/Core#CurveData_Curve
:CurveData_Curve rdf:type owl:ObjectProperty ;
                 rdfs:domain :CurveData ;
                 rdfs:range :Curve ;
                 rdfs:comment "The point data values that define this curve.The curve of  this curve data point." .


###  https://w3id.org/netbeheer/IECCIM/TC57CIM/IEC61970/Base/Core#Curve_CurveDatas
:Curve_CurveDatas rdf:type owl:ObjectProperty ;
                  owl:inverseOf :CurveData_Curve ;
                  rdf:type owl:FunctionalProperty ;
                  rdfs:domain :Curve ;
                  rdfs:range :CurveData ;
                  rdfs:comment "The point data values that define this curve.The curve of  this curve data point." .


###  https://w3id.org/netbeheer/IECCIM/TC57CIM/IEC61970/Base/Core#DCConverterUnit_Substation
:DCConverterUnit_Substation rdf:type owl:ObjectProperty ;
                            rdfs:domain <https://w3id.org/netbeheer/IECCIM/TC57CIM/IEC61970/Base/DC#DCConverterUnit> ;
                            rdfs:range :Substation ;
                            rdfs:comment "The DC converter unit belonging ot the substation.The containing substation of the DC converter unit." .


###  https://w3id.org/netbeheer/IECCIM/TC57CIM/IEC61970/Base/Core#DCLine_Region
:DCLine_Region rdf:type owl:ObjectProperty ;
               rdfs:domain <https://w3id.org/netbeheer/IECCIM/TC57CIM/IEC61970/Base/DC#DCLine> ;
               rdfs:range :SubGeographicalRegion ;
               rdfs:comment "" .


###  https://w3id.org/netbeheer/IECCIM/TC57CIM/IEC61970/Base/Core#DiagramObject_IdentifiedObject
:DiagramObject_IdentifiedObject rdf:type owl:ObjectProperty ;
                                owl:inverseOf :IdentifiedObject_DiagramObjects ;
                                rdfs:domain <https://w3id.org/netbeheer/IECCIM/TC57CIM/IEC61970/Base/DiagramLayout#DiagramObject> ;
                                rdfs:range :IdentifiedObject ;
                                rdfs:comment "The domain object to which this diagram object is associated.The diagram objects that are associated with the domain object." .


###  https://w3id.org/netbeheer/IECCIM/TC57CIM/IEC61970/Base/Core#EquipmentContainer_Equipments
:EquipmentContainer_Equipments rdf:type owl:ObjectProperty ;
                               rdfs:domain :EquipmentContainer ;
                               rdfs:range :Equipment ;
                               rdfs:comment "Container of this equipment.Contained equipment." .


###  https://w3id.org/netbeheer/IECCIM/TC57CIM/IEC61970/Base/Core#EquipmentLimitSeriesComponent_Equipment
:EquipmentLimitSeriesComponent_Equipment rdf:type owl:ObjectProperty ;
                                         rdfs:domain <https://w3id.org/netbeheer/IECCIM/TC57CIM/IEC61970/InfIEC61970/InfOperationalLimits#EquipmentLimitSeriesComponent> ;
                                         rdfs:range :Equipment ;
                                         rdfs:comment "Equipment limit series calculation component to which this equipment contributes.Equipment contributing toward the series limit.   The reference here is to Equipment rather than a specific limit on the equipment so the grouiping can be reused for multiple limits of different types on the same instance of equipment." .


###  https://w3id.org/netbeheer/IECCIM/TC57CIM/IEC61970/Base/Core#Equipment_ContingencyEquipment
:Equipment_ContingencyEquipment rdf:type owl:ObjectProperty ;
                                owl:inverseOf :ContingencyEquipment_Equipment ;
                                rdf:type owl:FunctionalProperty ;
                                rdfs:domain :Equipment ;
                                rdfs:range <https://w3id.org/netbeheer/IECCIM/TC57CIM/IEC61970/Base/Contingency#ContingencyEquipment> ;
                                rdfs:comment "The contingency equipments in which this equipment participates.The single piece of equipment to which to apply the contingency." .


###  https://w3id.org/netbeheer/IECCIM/TC57CIM/IEC61970/Base/Core#Equipment_EqiupmentLimitSeriesComponent
:Equipment_EqiupmentLimitSeriesComponent rdf:type owl:ObjectProperty ;
                                         owl:inverseOf :EquipmentLimitSeriesComponent_Equipment ;
                                         rdf:type owl:FunctionalProperty ;
                                         rdfs:domain :Equipment ;
                                         rdfs:range <https://w3id.org/netbeheer/IECCIM/TC57CIM/IEC61970/InfIEC61970/InfOperationalLimits#EquipmentLimitSeriesComponent> ;
                                         rdfs:comment "Equipment limit series calculation component to which this equipment contributes.Equipment contributing toward the series limit.   The reference here is to Equipment rather than a specific limit on the equipment so the grouiping can be reused for multiple limits of different types on the same instance of equipment." .


###  https://w3id.org/netbeheer/IECCIM/TC57CIM/IEC61970/Base/Core#Equipment_EquipmentContainer
:Equipment_EquipmentContainer rdf:type owl:ObjectProperty ;
                              owl:inverseOf :EquipmentContainer_Equipments ;
                              rdfs:domain :Equipment ;
                              rdfs:range :EquipmentContainer ;
                              rdfs:comment "Container of this equipment.Contained equipment." .


###  https://w3id.org/netbeheer/IECCIM/TC57CIM/IEC61970/Base/Core#Equipment_LimitDependencyModel
:Equipment_LimitDependencyModel rdf:type owl:ObjectProperty ;
                                owl:inverseOf :LimitDependency_Equipment ;
                                rdfs:domain :Equipment ;
                                rdfs:range <https://w3id.org/netbeheer/IECCIM/TC57CIM/IEC61970/InfIEC61970/InfOperationalLimits#LimitDependency> ;
                                rdfs:comment "Limit dependencymodels organized under this equipment as a means for organizing the model in a tree view.The equipment for which this limit dependency model is organized under." .


###  https://w3id.org/netbeheer/IECCIM/TC57CIM/IEC61970/Base/Core#Equipment_OperationalLimitSet
:Equipment_OperationalLimitSet rdf:type owl:ObjectProperty ;
                               owl:inverseOf :OperationalLimitSet_Equipment ;
                               rdfs:domain :Equipment ;
                               rdfs:range <https://w3id.org/netbeheer/IECCIM/TC57CIM/IEC61970/Base/OperationalLimits#OperationalLimitSet> ;
                               rdfs:comment "The operational limit sets associated with this equipment.The equipment to which the limit set applies." .


###  https://w3id.org/netbeheer/IECCIM/TC57CIM/IEC61970/Base/Core#Equipment_OperationalRestrictions
:Equipment_OperationalRestrictions rdf:type owl:ObjectProperty ;
                                   owl:inverseOf :OperationalRestriction_Equipments ;
                                   rdfs:domain :Equipment ;
                                   rdfs:range <https://w3id.org/netbeheer/IECCIM/TC57CIM/IEC61968/Operations#OperationalRestriction> ;
                                   rdfs:comment "All operational restrictions for this equipment.All equipments to which this restriction applies." .


###  https://w3id.org/netbeheer/IECCIM/TC57CIM/IEC61970/Base/Core#Equipment_Outages
:Equipment_Outages rdf:type owl:ObjectProperty ;
                   owl:inverseOf :Outage_Equipments ;
                   rdfs:domain :Equipment ;
                   rdfs:range <https://w3id.org/netbeheer/IECCIM/TC57CIM/IEC61968/Operations#Outage> ;
                   rdfs:comment "All outages in which this equipment is involved.All equipments associated with this outage." .


###  https://w3id.org/netbeheer/IECCIM/TC57CIM/IEC61970/Base/Core#Equipment_PinEquipment
:Equipment_PinEquipment rdf:type owl:ObjectProperty ;
                        owl:inverseOf :PinEquipment_Equipment ;
                        rdf:type owl:FunctionalProperty ;
                        rdfs:domain :Equipment ;
                        rdfs:range <https://w3id.org/netbeheer/IECCIM/TC57CIM/IEC61970/InfIEC61970/InfSIPS#PinEquipment> ;
                        rdfs:comment "" .


###  https://w3id.org/netbeheer/IECCIM/TC57CIM/IEC61970/Base/Core#Equipment_ProtectiveActionEquipment
:Equipment_ProtectiveActionEquipment rdf:type owl:ObjectProperty ;
                                     owl:inverseOf :ProtectiveActionEquipment_Equipment ;
                                     rdf:type owl:FunctionalProperty ;
                                     rdfs:domain :Equipment ;
                                     rdfs:range <https://w3id.org/netbeheer/IECCIM/TC57CIM/IEC61970/InfIEC61970/InfSIPS#ProtectiveActionEquipment> ;
                                     rdfs:comment "" .


###  https://w3id.org/netbeheer/IECCIM/TC57CIM/IEC61970/Base/Core#Equipment_UsagePoints
:Equipment_UsagePoints rdf:type owl:ObjectProperty ;
                       owl:inverseOf :UsagePoint_Equipments ;
                       rdfs:domain :Equipment ;
                       rdfs:range <https://w3id.org/netbeheer/IECCIM/TC57CIM/IEC61968/Metering#UsagePoint> ;
                       rdfs:comment "All usage points connected to the electrical grid through this equipment.All equipment connecting this usage point to the electrical grid." .


###  https://w3id.org/netbeheer/IECCIM/TC57CIM/IEC61970/Base/Core#Equipment_WeatherStation
:Equipment_WeatherStation rdf:type owl:ObjectProperty ;
                          rdfs:domain :Equipment ;
                          rdfs:range <https://w3id.org/netbeheer/IECCIM/TC57CIM/IEC61970/InfIEC61970/InfOperationalLimits#WeatherStation> ;
                          rdfs:comment "" .


###  https://w3id.org/netbeheer/IECCIM/TC57CIM/IEC61970/Base/Core#GeographicalRegion_Regions
:GeographicalRegion_Regions rdf:type owl:ObjectProperty ;
                            rdfs:domain :GeographicalRegion ;
                            rdfs:range :SubGeographicalRegion ;
                            rdfs:comment "The geographical region to which this sub-geographical region is within.All sub-geograhpical regions within this geographical region." .


###  https://w3id.org/netbeheer/IECCIM/TC57CIM/IEC61970/Base/Core#GroundAction_GroundedEquipment
:GroundAction_GroundedEquipment rdf:type owl:ObjectProperty ;
                                rdfs:domain <https://w3id.org/netbeheer/IECCIM/TC57CIM/IEC61968/Operations#GroundAction> ;
                                rdfs:range :ConductingEquipment ;
                                rdfs:comment "Action involving grounding operation on this conducting equipment.Equipment being grounded with this operation. In case of placing a ground anywhere along a line segment, you must use the clamp (to get the distance from one terminal), so use the explicit relation with line segment. In all other cases (including placing the ground at a line segment terminal), reference to one or more conducting equipment is sufficient." .


###  https://w3id.org/netbeheer/IECCIM/TC57CIM/IEC61970/Base/Core#IdentifiedObject_DiagramObjects
:IdentifiedObject_DiagramObjects rdf:type owl:ObjectProperty ;
                                 rdfs:domain :IdentifiedObject ;
                                 rdfs:range <https://w3id.org/netbeheer/IECCIM/TC57CIM/IEC61970/Base/DiagramLayout#DiagramObject> ;
                                 rdfs:comment "The domain object to which this diagram object is associated.The diagram objects that are associated with the domain object." .


###  https://w3id.org/netbeheer/IECCIM/TC57CIM/IEC61970/Base/Core#IdentifiedObject_Names
:IdentifiedObject_Names rdf:type owl:ObjectProperty ;
                        owl:inverseOf :Name_IdentifiedObject ;
                        rdf:type owl:FunctionalProperty ;
                        rdfs:domain :IdentifiedObject ;
                        rdfs:range :Name ;
                        rdfs:comment "All names of this identified object.Identified object that this name designates." .


###  https://w3id.org/netbeheer/IECCIM/TC57CIM/IEC61970/Base/Core#IdentifiedObject_PropertiesCIMDataObject
:IdentifiedObject_PropertiesCIMDataObject rdf:type owl:ObjectProperty ;
                                          owl:inverseOf :CIMDataObject_PropertiesObject ;
                                          rdfs:domain :IdentifiedObject ;
                                          rdfs:range <https://w3id.org/netbeheer/IECCIM/TC57CIM/IEC61970/InfIEC61970/InfGenericDataset/CanonicalModel/GenericDatasetCore#CIMDataObject> ;
                                          rdfs:comment "The single CIM data object in the appropriate dataset context.The CIM object holding the properties of this dataset context.   Sometimes properties are not required and only the reference to the registered object is required." .


###  https://w3id.org/netbeheer/IECCIM/TC57CIM/IEC61970/Base/Core#IdentifiedObject_RegisteredCIMDataObject
:IdentifiedObject_RegisteredCIMDataObject rdf:type owl:ObjectProperty ;
                                          owl:inverseOf :CIMDataObject_RegisteredObject ;
                                          rdf:type owl:FunctionalProperty ;
                                          rdfs:domain :IdentifiedObject ;
                                          rdfs:range <https://w3id.org/netbeheer/IECCIM/TC57CIM/IEC61970/InfIEC61970/InfGenericDataset/CanonicalModel/GenericDatasetCore#CIMDataObject> ;
                                          rdfs:comment "Data objects registered.The registered CIM object." .


###  https://w3id.org/netbeheer/IECCIM/TC57CIM/IEC61970/Base/Core#IrregularIntervalSchedule_TimePoints
:IrregularIntervalSchedule_TimePoints rdf:type owl:ObjectProperty ,
                                               owl:FunctionalProperty ;
                                      rdfs:domain :IrregularIntervalSchedule ;
                                      rdfs:range :IrregularTimePoint ;
                                      rdfs:comment "An IrregularTimePoint belongs to an IrregularIntervalSchedule.The point data values that define a curve." .


###  https://w3id.org/netbeheer/IECCIM/TC57CIM/IEC61970/Base/Core#IrregularTimePoint_IntervalSchedule
:IrregularTimePoint_IntervalSchedule rdf:type owl:ObjectProperty ;
                                     owl:inverseOf :IrregularIntervalSchedule_TimePoints ;
                                     rdfs:domain :IrregularTimePoint ;
                                     rdfs:range :IrregularIntervalSchedule ;
                                     rdfs:comment "An IrregularTimePoint belongs to an IrregularIntervalSchedule.The point data values that define a curve." .


###  https://w3id.org/netbeheer/IECCIM/TC57CIM/IEC61970/Base/Core#IrregularTimePoint_time
:IrregularTimePoint_time rdf:type owl:ObjectProperty ;
                         rdfs:domain :IrregularTimePoint ;
                         rdfs:range <https://w3id.org/netbeheer/IECCIM/TC57CIM/IEC61970/Base/Domain#Seconds> ;
                         rdfs:comment """The time is relative to the schedule starting time.

""" .


###  https://w3id.org/netbeheer/IECCIM/TC57CIM/IEC61970/Base/Core#JumperAction_JumpedEquipments
:JumperAction_JumpedEquipments rdf:type owl:ObjectProperty ;
                               rdfs:domain <https://w3id.org/netbeheer/IECCIM/TC57CIM/IEC61968/Operations#JumperAction> ;
                               rdfs:range :ConductingEquipment ;
                               rdfs:comment "Jumper action involving jumping operation on this conducting equipment.The conducting equipment that this jumper action will affect. In case of placing a jumper anywhere along a line segment, you must use the clamp (to get the distance from one terminal), so use the explicit relation with line segment. In all other cases (including placing the jumper at a line segment terminal), reference to one or more conducting equipment is sufficient." .


###  https://w3id.org/netbeheer/IECCIM/TC57CIM/IEC61970/Base/Core#LimitDependency_Equipment
:LimitDependency_Equipment rdf:type owl:ObjectProperty ;
                           rdfs:domain <https://w3id.org/netbeheer/IECCIM/TC57CIM/IEC61970/InfIEC61970/InfOperationalLimits#LimitDependency> ;
                           rdfs:range :Equipment ;
                           rdfs:comment "Limit dependencymodels organized under this equipment as a means for organizing the model in a tree view.The equipment for which this limit dependency model is organized under." .


###  https://w3id.org/netbeheer/IECCIM/TC57CIM/IEC61970/Base/Core#Line_Region
:Line_Region rdf:type owl:ObjectProperty ;
             owl:inverseOf :SubGeographicalRegion_Lines ;
             rdfs:domain <https://w3id.org/netbeheer/IECCIM/TC57CIM/IEC61970/Base/Wires#Line> ;
             rdfs:range :SubGeographicalRegion ;
             rdfs:comment "The sub-geographical region of the line.The lines within the sub-geographical region." .


###  https://w3id.org/netbeheer/IECCIM/TC57CIM/IEC61970/Base/Core#Location_PowerSystemResources
:Location_PowerSystemResources rdf:type owl:ObjectProperty ;
                               rdfs:domain <https://w3id.org/netbeheer/IECCIM/TC57CIM/IEC61968/Common#Location> ;
                               rdfs:range :PowerSystemResource ;
                               rdfs:comment "Location of this power system resource.All power system resources at this location." .


###  https://w3id.org/netbeheer/IECCIM/TC57CIM/IEC61970/Base/Core#Measure_PowerSystemResource
:Measure_PowerSystemResource rdf:type owl:ObjectProperty ;
                             owl:inverseOf :PowerSystemResource_Measurements ;
                             rdfs:domain <https://w3id.org/netbeheer/IECCIM/TC57CIM/IEC61970/Base/Meas#Measure> ;
                             rdfs:range :PowerSystemResource ;
                             rdfs:comment "The power system resource that contains the measurement.The measurements associated with this power system resource." .


###  https://w3id.org/netbeheer/IECCIM/TC57CIM/IEC61970/Base/Core#Measure_Terminal
:Measure_Terminal rdf:type owl:ObjectProperty ;
                  rdfs:domain <https://w3id.org/netbeheer/IECCIM/TC57CIM/IEC61970/Base/Meas#Measure> ;
                  rdfs:range :ACDCTerminal ;
                  rdfs:comment "Measurements associated with this terminal defining  where the measurement is placed in the network topology.  It may be used, for instance, to capture the sensor position, such as a voltage transformer (PT) at a busbar or a current transformer (CT) at the bar between a breaker and an isolator.One or more measurements may be associated with a terminal in the network." .


###  https://w3id.org/netbeheer/IECCIM/TC57CIM/IEC61970/Base/Core#MutualCoupling_First_Terminal
:MutualCoupling_First_Terminal rdf:type owl:ObjectProperty ;
                               rdfs:domain <https://w3id.org/netbeheer/IECCIM/TC57CIM/IEC61970/Base/Wires#MutualCoupling> ;
                               rdfs:range :Terminal ;
                               rdfs:comment "Mutual couplings associated with the branch as the first branch.The starting terminal for the calculation of distances along the first branch of the mutual coupling.  Normally MutualCoupling would only be used for terminals of AC line segments.  The first and second terminals of a mutual coupling should point to different AC line segments." .


###  https://w3id.org/netbeheer/IECCIM/TC57CIM/IEC61970/Base/Core#MutualCoupling_Second_Terminal
:MutualCoupling_Second_Terminal rdf:type owl:ObjectProperty ;
                                rdfs:domain <https://w3id.org/netbeheer/IECCIM/TC57CIM/IEC61970/Base/Wires#MutualCoupling> ;
                                rdfs:range :Terminal ;
                                rdfs:comment "Mutual couplings with the branch associated as the first branch.The starting terminal for the calculation of distances along the second branch of the mutual coupling." .


###  https://w3id.org/netbeheer/IECCIM/TC57CIM/IEC61970/Base/Core#NameTypeAuthority_NameTypes
:NameTypeAuthority_NameTypes rdf:type owl:ObjectProperty ;
                             owl:inverseOf :NameType_NameTypeAuthority ;
                             rdfs:domain :NameTypeAuthority ;
                             rdfs:range :NameType ;
                             rdfs:comment "All name types managed by this authority.Authority responsible for managing names of this type." .


###  https://w3id.org/netbeheer/IECCIM/TC57CIM/IEC61970/Base/Core#NameType_NameTypeAuthority
:NameType_NameTypeAuthority rdf:type owl:ObjectProperty ;
                            rdfs:domain :NameType ;
                            rdfs:range :NameTypeAuthority ;
                            rdfs:comment "All name types managed by this authority.Authority responsible for managing names of this type." .


###  https://w3id.org/netbeheer/IECCIM/TC57CIM/IEC61970/Base/Core#NameType_Names
:NameType_Names rdf:type owl:ObjectProperty ;
                owl:inverseOf :Name_NameType ;
                rdf:type owl:FunctionalProperty ;
                rdfs:domain :NameType ;
                rdfs:range :Name ;
                rdfs:comment "All names of this type.Type of this name." .


###  https://w3id.org/netbeheer/IECCIM/TC57CIM/IEC61970/Base/Core#Name_IdentifiedObject
:Name_IdentifiedObject rdf:type owl:ObjectProperty ;
                       rdfs:domain :Name ;
                       rdfs:range :IdentifiedObject ;
                       rdfs:comment "All names of this identified object.Identified object that this name designates." .


###  https://w3id.org/netbeheer/IECCIM/TC57CIM/IEC61970/Base/Core#Name_NameType
:Name_NameType rdf:type owl:ObjectProperty ;
               rdfs:domain :Name ;
               rdfs:range :NameType ;
               rdfs:comment "All names of this type.Type of this name." .


###  https://w3id.org/netbeheer/IECCIM/TC57CIM/IEC61970/Base/Core#OperatingParticipant_OperatingShare
:OperatingParticipant_OperatingShare rdf:type owl:ObjectProperty ;
                                     owl:inverseOf :OperatingShare_OperatingParticipant ;
                                     rdf:type owl:FunctionalProperty ;
                                     rdfs:domain :OperatingParticipant ;
                                     rdfs:range :OperatingShare ;
                                     rdfs:comment "The operating shares of this operating participant.  An operating participant can be resused for any number of power system resources.The operating participant having this share with the associated power system resource." .


###  https://w3id.org/netbeheer/IECCIM/TC57CIM/IEC61970/Base/Core#OperatingShare_OperatingParticipant
:OperatingShare_OperatingParticipant rdf:type owl:ObjectProperty ;
                                     rdfs:domain :OperatingShare ;
                                     rdfs:range :OperatingParticipant ;
                                     rdfs:comment "The operating shares of this operating participant.  An operating participant can be resused for any number of power system resources.The operating participant having this share with the associated power system resource." .


###  https://w3id.org/netbeheer/IECCIM/TC57CIM/IEC61970/Base/Core#OperatingShare_PowerSystemResource
:OperatingShare_PowerSystemResource rdf:type owl:ObjectProperty ;
                                    rdfs:domain :OperatingShare ;
                                    rdfs:range :PowerSystemResource ;
                                    rdfs:comment "The operating shares of this power system resource.The power system resource to which the share applies." .


###  https://w3id.org/netbeheer/IECCIM/TC57CIM/IEC61970/Base/Core#OperatingShare_percentage
:OperatingShare_percentage rdf:type owl:ObjectProperty ;
                           rdfs:domain :OperatingShare ;
                           rdfs:range <https://w3id.org/netbeheer/IECCIM/TC57CIM/IEC61970/Base/Domain#PerCent> ;
                           rdfs:comment """Percentage operational ownership between the pair (power system resource and operatging participant) associated with this share. The total percentage ownership for a power system resource should add to 100%.
""" .


###  https://w3id.org/netbeheer/IECCIM/TC57CIM/IEC61970/Base/Core#OperationalLimitSet_Equipment
:OperationalLimitSet_Equipment rdf:type owl:ObjectProperty ;
                               rdfs:domain <https://w3id.org/netbeheer/IECCIM/TC57CIM/IEC61970/Base/OperationalLimits#OperationalLimitSet> ;
                               rdfs:range :Equipment ;
                               rdfs:comment "The operational limit sets associated with this equipment.The equipment to which the limit set applies." .


###  https://w3id.org/netbeheer/IECCIM/TC57CIM/IEC61970/Base/Core#OperationalLimitSet_Terminal
:OperationalLimitSet_Terminal rdf:type owl:ObjectProperty ;
                              rdfs:domain <https://w3id.org/netbeheer/IECCIM/TC57CIM/IEC61970/Base/OperationalLimits#OperationalLimitSet> ;
                              rdfs:range :ACDCTerminal ;
                              rdfs:comment "" .


###  https://w3id.org/netbeheer/IECCIM/TC57CIM/IEC61970/Base/Core#OperationalRestriction_Equipments
:OperationalRestriction_Equipments rdf:type owl:ObjectProperty ;
                                   rdfs:domain <https://w3id.org/netbeheer/IECCIM/TC57CIM/IEC61968/Operations#OperationalRestriction> ;
                                   rdfs:range :Equipment ;
                                   rdfs:comment "All operational restrictions for this equipment.All equipments to which this restriction applies." .


###  https://w3id.org/netbeheer/IECCIM/TC57CIM/IEC61970/Base/Core#OperationalTag_PowerSystemResource
:OperationalTag_PowerSystemResource rdf:type owl:ObjectProperty ;
                                    rdfs:domain <https://w3id.org/netbeheer/IECCIM/TC57CIM/IEC61968/Operations#OperationalTag> ;
                                    rdfs:range :PowerSystemResource ;
                                    rdfs:comment "All operational tags placed on this power system resource.Power system resource on which this tag has been placed." .


###  https://w3id.org/netbeheer/IECCIM/TC57CIM/IEC61970/Base/Core#Outage_Equipments
:Outage_Equipments rdf:type owl:ObjectProperty ;
                   rdfs:domain <https://w3id.org/netbeheer/IECCIM/TC57CIM/IEC61968/Operations#Outage> ;
                   rdfs:range :Equipment ;
                   rdfs:comment "All outages in which this equipment is involved.All equipments associated with this outage." .


###  https://w3id.org/netbeheer/IECCIM/TC57CIM/IEC61970/Base/Core#PSREvent_PowerSystemResource
:PSREvent_PowerSystemResource rdf:type owl:ObjectProperty ;
                              rdfs:domain <https://w3id.org/netbeheer/IECCIM/TC57CIM/IEC61968/Operations#PSREvent> ;
                              rdfs:range :PowerSystemResource ;
                              rdfs:comment "All events associated with this power system resource.Power system resource that generated this event." .


###  https://w3id.org/netbeheer/IECCIM/TC57CIM/IEC61970/Base/Core#PSRType_PowerSystemResources
:PSRType_PowerSystemResources rdf:type owl:ObjectProperty ;
                              owl:inverseOf :PowerSystemResource_PSRType ;
                              rdfs:domain :PSRType ;
                              rdfs:range :PowerSystemResource ;
                              rdfs:comment "Power system resources classified with this power system resource type.Custom classification for this power system resource." .


###  https://w3id.org/netbeheer/IECCIM/TC57CIM/IEC61970/Base/Core#PinEquipment_Equipment
:PinEquipment_Equipment rdf:type owl:ObjectProperty ;
                        rdfs:domain <https://w3id.org/netbeheer/IECCIM/TC57CIM/IEC61970/InfIEC61970/InfSIPS#PinEquipment> ;
                        rdfs:range :Equipment ;
                        rdfs:comment "" .


###  https://w3id.org/netbeheer/IECCIM/TC57CIM/IEC61970/Base/Core#PinTerminal_Terminal
:PinTerminal_Terminal rdf:type owl:ObjectProperty ;
                      rdfs:domain <https://w3id.org/netbeheer/IECCIM/TC57CIM/IEC61970/InfIEC61970/InfSIPS#PinTerminal> ;
                      rdfs:range :Terminal ;
                      rdfs:comment "" .


###  https://w3id.org/netbeheer/IECCIM/TC57CIM/IEC61970/Base/Core#PowerSystemResource_AssetDatasheet
:PowerSystemResource_AssetDatasheet rdf:type owl:ObjectProperty ;
                                    owl:inverseOf :AssetInfo_PowerSystemResources ;
                                    rdfs:domain :PowerSystemResource ;
                                    rdfs:range <https://w3id.org/netbeheer/IECCIM/TC57CIM/IEC61968/Assets#AssetInfo> ;
                                    rdfs:comment "Datasheet information for this power system resource.All power system resources with this datasheet information." .


###  https://w3id.org/netbeheer/IECCIM/TC57CIM/IEC61970/Base/Core#PowerSystemResource_Assets
:PowerSystemResource_Assets rdf:type owl:ObjectProperty ;
                            owl:inverseOf :Asset_PowerSystemResources ;
                            rdfs:domain :PowerSystemResource ;
                            rdfs:range <https://w3id.org/netbeheer/IECCIM/TC57CIM/IEC61968/Assets#Asset> ;
                            rdfs:comment "All assets represented by this power system resource. For example, multiple conductor assets are electrically modelled as a single AC line segment.All power system resources used to electrically model this asset. For example, transformer asset is electrically modelled with a transformer and its windings and tap changer." .


###  https://w3id.org/netbeheer/IECCIM/TC57CIM/IEC61970/Base/Core#PowerSystemResource_Clearances
:PowerSystemResource_Clearances rdf:type owl:ObjectProperty ;
                                owl:inverseOf :ClearanceDocument_TaggedPSRs ;
                                rdfs:domain :PowerSystemResource ;
                                rdfs:range <https://w3id.org/netbeheer/IECCIM/TC57CIM/IEC61968/Operations#ClearanceDocument> ;
                                rdfs:comment "All clearances applicable to this power system resource.All power system resources tagged through this clearance." .


###  https://w3id.org/netbeheer/IECCIM/TC57CIM/IEC61970/Base/Core#PowerSystemResource_Controls
:PowerSystemResource_Controls rdf:type owl:ObjectProperty ;
                              rdfs:domain :PowerSystemResource ;
                              rdfs:range <https://w3id.org/netbeheer/IECCIM/TC57CIM/IEC61970/Base/Meas#Control> ;
                              rdfs:comment "Regulating device governed by this control output.The controller outputs used to actually govern a regulating device, e.g. the magnetization of a synchronous machine or capacitor bank breaker actuator." .


###  https://w3id.org/netbeheer/IECCIM/TC57CIM/IEC61970/Base/Core#PowerSystemResource_Location
:PowerSystemResource_Location rdf:type owl:ObjectProperty ;
                              owl:inverseOf :Location_PowerSystemResources ;
                              rdfs:domain :PowerSystemResource ;
                              rdfs:range <https://w3id.org/netbeheer/IECCIM/TC57CIM/IEC61968/Common#Location> ;
                              rdfs:comment "Location of this power system resource.All power system resources at this location." .


###  https://w3id.org/netbeheer/IECCIM/TC57CIM/IEC61970/Base/Core#PowerSystemResource_Measurements
:PowerSystemResource_Measurements rdf:type owl:ObjectProperty ;
                                  rdfs:domain :PowerSystemResource ;
                                  rdfs:range <https://w3id.org/netbeheer/IECCIM/TC57CIM/IEC61970/Base/Meas#Measure> ;
                                  rdfs:comment "The power system resource that contains the measurement.The measurements associated with this power system resource." .


###  https://w3id.org/netbeheer/IECCIM/TC57CIM/IEC61970/Base/Core#PowerSystemResource_OperatingShare
:PowerSystemResource_OperatingShare rdf:type owl:ObjectProperty ;
                                    owl:inverseOf :OperatingShare_PowerSystemResource ;
                                    rdf:type owl:FunctionalProperty ;
                                    rdfs:domain :PowerSystemResource ;
                                    rdfs:range :OperatingShare ;
                                    rdfs:comment "The operating shares of this power system resource.The power system resource to which the share applies." .


###  https://w3id.org/netbeheer/IECCIM/TC57CIM/IEC61970/Base/Core#PowerSystemResource_OperationalTags
:PowerSystemResource_OperationalTags rdf:type owl:ObjectProperty ;
                                     owl:inverseOf :OperationalTag_PowerSystemResource ;
                                     rdfs:domain :PowerSystemResource ;
                                     rdfs:range <https://w3id.org/netbeheer/IECCIM/TC57CIM/IEC61968/Operations#OperationalTag> ;
                                     rdfs:comment "All operational tags placed on this power system resource.Power system resource on which this tag has been placed." .


###  https://w3id.org/netbeheer/IECCIM/TC57CIM/IEC61970/Base/Core#PowerSystemResource_PSREvents
:PowerSystemResource_PSREvents rdf:type owl:ObjectProperty ;
                               owl:inverseOf :PSREvent_PowerSystemResource ;
                               rdfs:domain :PowerSystemResource ;
                               rdfs:range <https://w3id.org/netbeheer/IECCIM/TC57CIM/IEC61968/Operations#PSREvent> ;
                               rdfs:comment "All events associated with this power system resource.Power system resource that generated this event." .


###  https://w3id.org/netbeheer/IECCIM/TC57CIM/IEC61970/Base/Core#PowerSystemResource_PSRType
:PowerSystemResource_PSRType rdf:type owl:ObjectProperty ;
                             rdfs:domain :PowerSystemResource ;
                             rdfs:range :PSRType ;
                             rdfs:comment "Power system resources classified with this power system resource type.Custom classification for this power system resource." .


###  https://w3id.org/netbeheer/IECCIM/TC57CIM/IEC61970/Base/Core#PowerSystemResource_ReportingGroup
:PowerSystemResource_ReportingGroup rdf:type owl:ObjectProperty ;
                                    owl:inverseOf :ReportingGroup_PowerSystemResource ;
                                    rdfs:domain :PowerSystemResource ;
                                    rdfs:range :ReportingGroup ;
                                    rdfs:comment "Reporting groups to which this power system resource belongs.Power system resources which belong to this reporting group." .


###  https://w3id.org/netbeheer/IECCIM/TC57CIM/IEC61970/Base/Core#ProtectionEquipment_ConductingEquipments
:ProtectionEquipment_ConductingEquipments rdf:type owl:ObjectProperty ;
                                          rdfs:domain <https://w3id.org/netbeheer/IECCIM/TC57CIM/IEC61970/Base/Protection#ProtectionEquipment> ;
                                          rdfs:range :ConductingEquipment ;
                                          rdfs:comment "Protection equipment  used to protect specific conducting equipment. Protection equipment may be used to protect specific conducting equipment." .


###  https://w3id.org/netbeheer/IECCIM/TC57CIM/IEC61970/Base/Core#ProtectiveActionAdjustment_ConductingEquipment
:ProtectiveActionAdjustment_ConductingEquipment rdf:type owl:ObjectProperty ;
                                                owl:inverseOf :ConductingEquipment_ProtectiveActionAdjustment ;
                                                rdfs:domain <https://w3id.org/netbeheer/IECCIM/TC57CIM/IEC61970/InfIEC61970/InfSIPS#ProtectiveActionAdjustment> ;
                                                rdfs:range :ConductingEquipment ;
                                                rdfs:comment "The operating condition to the Conducting Equipment is changed when protective action adjustment is activated. For Shunt Compensator or other conducting equipment that operates on discrete values (integer), the values given in float will be rounded. The operating condition to the Conducting Equipment is changed when protective action adjustment is activated. For Shunt Compensator or other conducting equipment that operates on discrete values (integer), the values given in float will be rounded. " .


###  https://w3id.org/netbeheer/IECCIM/TC57CIM/IEC61970/Base/Core#ProtectiveActionEquipment_Equipment
:ProtectiveActionEquipment_Equipment rdf:type owl:ObjectProperty ;
                                     rdfs:domain <https://w3id.org/netbeheer/IECCIM/TC57CIM/IEC61970/InfIEC61970/InfSIPS#ProtectiveActionEquipment> ;
                                     rdfs:range :Equipment ;
                                     rdfs:comment "" .


###  https://w3id.org/netbeheer/IECCIM/TC57CIM/IEC61970/Base/Core#RegularIntervalSchedule_TimePoints
:RegularIntervalSchedule_TimePoints rdf:type owl:ObjectProperty ,
                                             owl:FunctionalProperty ;
                                    rdfs:domain :RegularIntervalSchedule ;
                                    rdfs:range :RegularTimePoint ;
                                    rdfs:comment "Regular interval schedule containing this time point.The regular interval time point data values that define this schedule." .


###  https://w3id.org/netbeheer/IECCIM/TC57CIM/IEC61970/Base/Core#RegularIntervalSchedule_timeStep
:RegularIntervalSchedule_timeStep rdf:type owl:ObjectProperty ;
                                  rdfs:domain :RegularIntervalSchedule ;
                                  rdfs:range <https://w3id.org/netbeheer/IECCIM/TC57CIM/IEC61970/Base/Domain#Seconds> ;
                                  rdfs:comment """The time between each pair of subsequent regular time points in sequence order.
""" .


###  https://w3id.org/netbeheer/IECCIM/TC57CIM/IEC61970/Base/Core#RegularTimePoint_IntervalSchedule
:RegularTimePoint_IntervalSchedule rdf:type owl:ObjectProperty ;
                                   owl:inverseOf :RegularIntervalSchedule_TimePoints ;
                                   rdfs:domain :RegularTimePoint ;
                                   rdfs:range :RegularIntervalSchedule ;
                                   rdfs:comment "Regular interval schedule containing this time point.The regular interval time point data values that define this schedule." .


###  https://w3id.org/netbeheer/IECCIM/TC57CIM/IEC61970/Base/Core#RegulatingControl_Terminal
:RegulatingControl_Terminal rdf:type owl:ObjectProperty ;
                            owl:inverseOf :Terminal_RegulatingControl ;
                            rdfs:domain <https://w3id.org/netbeheer/IECCIM/TC57CIM/IEC61970/Base/Wires#RegulatingControl> ;
                            rdfs:range :Terminal ;
                            rdfs:comment "The terminal associated with this regulating control.  The terminal is associated instead of a node, since the terminal could connect into either a topological node (bus in bus-branch model) or a connectivity node (detailed switch model).  Sometimes it is useful to model regulation at a terminal of a bus bar object since the bus bar can be present in both a bus-branch model or a model with switch detail.The controls regulating this terminal." .


###  https://w3id.org/netbeheer/IECCIM/TC57CIM/IEC61970/Base/Core#RemoteInputSignal_Terminal
:RemoteInputSignal_Terminal rdf:type owl:ObjectProperty ;
                            rdfs:domain <https://w3id.org/netbeheer/IECCIM/TC57CIM/IEC61970/Dynamics/StandardInterconnections#RemoteInputSignal> ;
                            rdfs:range :Terminal ;
                            rdfs:comment "Input signal coming from this terminal.Remote terminal with which this input signal is associated." .


###  https://w3id.org/netbeheer/IECCIM/TC57CIM/IEC61970/Base/Core#ReportingGroup_BusNameMarker
:ReportingGroup_BusNameMarker rdf:type owl:ObjectProperty ;
                              owl:inverseOf :BusNameMarker_ReportingGroup ;
                              rdfs:domain :ReportingGroup ;
                              rdfs:range <https://w3id.org/netbeheer/IECCIM/TC57CIM/IEC61970/Base/Topology#BusNameMarker> ;
                              rdfs:comment "The bus name markers that belong to this reporting group.The reporting group to which this bus name marker belongs." .


###  https://w3id.org/netbeheer/IECCIM/TC57CIM/IEC61970/Base/Core#ReportingGroup_PowerSystemResource
:ReportingGroup_PowerSystemResource rdf:type owl:ObjectProperty ;
                                    rdfs:domain :ReportingGroup ;
                                    rdfs:range :PowerSystemResource ;
                                    rdfs:comment "Reporting groups to which this power system resource belongs.Power system resources which belong to this reporting group." .


###  https://w3id.org/netbeheer/IECCIM/TC57CIM/IEC61970/Base/Core#ReportingGroup_ReportingSuperGroup
:ReportingGroup_ReportingSuperGroup rdf:type owl:ObjectProperty ;
                                    rdfs:domain :ReportingGroup ;
                                    rdfs:range :ReportingSuperGroup ;
                                    rdfs:comment "Reporting groups that are grouped under this super group.Reporting super group to which this reporting group belongs." .


###  https://w3id.org/netbeheer/IECCIM/TC57CIM/IEC61970/Base/Core#ReportingGroup_TopologicalNode
:ReportingGroup_TopologicalNode rdf:type owl:ObjectProperty ;
                                owl:inverseOf :TopologicalNode_ReportingGroup ;
                                rdfs:domain :ReportingGroup ;
                                rdfs:range <https://w3id.org/netbeheer/IECCIM/TC57CIM/IEC61970/Base/Topology#TopologicalNode> ;
                                rdfs:comment "The topological nodes that belong to the reporting group.The reporting group to which the topological node belongs." .


###  https://w3id.org/netbeheer/IECCIM/TC57CIM/IEC61970/Base/Core#ReportingSuperGroup_ReportingGroup
:ReportingSuperGroup_ReportingGroup rdf:type owl:ObjectProperty ;
                                    owl:inverseOf :ReportingGroup_ReportingSuperGroup ;
                                    rdfs:domain :ReportingSuperGroup ;
                                    rdfs:range :ReportingGroup ;
                                    rdfs:comment "Reporting groups that are grouped under this super group.Reporting super group to which this reporting group belongs." .


###  https://w3id.org/netbeheer/IECCIM/TC57CIM/IEC61970/Base/Core#SubGeographicalRegion_DCLines
:SubGeographicalRegion_DCLines rdf:type owl:ObjectProperty ;
                               owl:inverseOf :DCLine_Region ;
                               rdfs:domain :SubGeographicalRegion ;
                               rdfs:range <https://w3id.org/netbeheer/IECCIM/TC57CIM/IEC61970/Base/DC#DCLine> ;
                               rdfs:comment "" .


###  https://w3id.org/netbeheer/IECCIM/TC57CIM/IEC61970/Base/Core#SubGeographicalRegion_Lines
:SubGeographicalRegion_Lines rdf:type owl:ObjectProperty ;
                             rdfs:domain :SubGeographicalRegion ;
                             rdfs:range <https://w3id.org/netbeheer/IECCIM/TC57CIM/IEC61970/Base/Wires#Line> ;
                             rdfs:comment "The sub-geographical region of the line.The lines within the sub-geographical region." .


###  https://w3id.org/netbeheer/IECCIM/TC57CIM/IEC61970/Base/Core#SubGeographicalRegion_Region
:SubGeographicalRegion_Region rdf:type owl:ObjectProperty ;
                              owl:inverseOf :GeographicalRegion_Regions ;
                              rdfs:domain :SubGeographicalRegion ;
                              rdfs:range :GeographicalRegion ;
                              rdfs:comment "The geographical region to which this sub-geographical region is within.All sub-geograhpical regions within this geographical region." .


###  https://w3id.org/netbeheer/IECCIM/TC57CIM/IEC61970/Base/Core#SubGeographicalRegion_Substations
:SubGeographicalRegion_Substations rdf:type owl:ObjectProperty ;
                                   rdfs:domain :SubGeographicalRegion ;
                                   rdfs:range :Substation ;
                                   rdfs:comment "The SubGeographicalRegion containing the substation.The substations in this sub-geographical region." .


###  https://w3id.org/netbeheer/IECCIM/TC57CIM/IEC61970/Base/Core#Substation_Bays
:Substation_Bays rdf:type owl:ObjectProperty ;
                 owl:inverseOf :Bay_Substation ;
                 rdfs:domain :Substation ;
                 rdfs:range :Bay ;
                 rdfs:comment "Bays contained in the substation.Substation containing the bay." .


###  https://w3id.org/netbeheer/IECCIM/TC57CIM/IEC61970/Base/Core#Substation_DCConverterUnit
:Substation_DCConverterUnit rdf:type owl:ObjectProperty ;
                            owl:inverseOf :DCConverterUnit_Substation ;
                            rdfs:domain :Substation ;
                            rdfs:range <https://w3id.org/netbeheer/IECCIM/TC57CIM/IEC61970/Base/DC#DCConverterUnit> ;
                            rdfs:comment "The DC converter unit belonging ot the substation.The containing substation of the DC converter unit." .


###  https://w3id.org/netbeheer/IECCIM/TC57CIM/IEC61970/Base/Core#Substation_Region
:Substation_Region rdf:type owl:ObjectProperty ;
                   owl:inverseOf :SubGeographicalRegion_Substations ;
                   rdfs:domain :Substation ;
                   rdfs:range :SubGeographicalRegion ;
                   rdfs:comment "The SubGeographicalRegion containing the substation.The substations in this sub-geographical region." .


###  https://w3id.org/netbeheer/IECCIM/TC57CIM/IEC61970/Base/Core#Substation_VoltageLevels
:Substation_VoltageLevels rdf:type owl:ObjectProperty ,
                                   owl:FunctionalProperty ;
                          rdfs:domain :Substation ;
                          rdfs:range :VoltageLevel ;
                          rdfs:comment "The substation of the voltage level.The voltage levels within this substation." .


###  https://w3id.org/netbeheer/IECCIM/TC57CIM/IEC61970/Base/Core#SvPowerFlow_Terminal
:SvPowerFlow_Terminal rdf:type owl:ObjectProperty ;
                      rdfs:domain <https://w3id.org/netbeheer/IECCIM/TC57CIM/IEC61970/Base/StateVariables#SvPowerFlow> ;
                      rdfs:range :Terminal ;
                      rdfs:comment "The power flow state variable associated with the terminal.The terminal associated with the power flow state variable." .


###  https://w3id.org/netbeheer/IECCIM/TC57CIM/IEC61970/Base/Core#SvStatus_ConductingEquipment
:SvStatus_ConductingEquipment rdf:type owl:ObjectProperty ;
                              rdfs:domain <https://w3id.org/netbeheer/IECCIM/TC57CIM/IEC61970/Base/StateVariables#SvStatus> ;
                              rdfs:range :ConductingEquipment ;
                              rdfs:comment "The status state variable associated with this conducting equipment.The conducting equipment associated with the status state variable." .


###  https://w3id.org/netbeheer/IECCIM/TC57CIM/IEC61970/Base/Core#Terminal_AuxiliaryEquipment
:Terminal_AuxiliaryEquipment rdf:type owl:ObjectProperty ;
                             owl:inverseOf :AuxiliaryEquipment_Terminal ;
                             rdf:type owl:FunctionalProperty ;
                             rdfs:domain :Terminal ;
                             rdfs:range <https://w3id.org/netbeheer/IECCIM/TC57CIM/IEC61970/Base/AuxiliaryEquipment#AuxiliaryEquipment> ;
                             rdfs:comment "The auxiliary equipment connected to the terminal.The Terminal at the equipment where the AuxiliaryEquipment is attached." .


###  https://w3id.org/netbeheer/IECCIM/TC57CIM/IEC61970/Base/Core#Terminal_BranchGroupTerminal
:Terminal_BranchGroupTerminal rdf:type owl:ObjectProperty ;
                              owl:inverseOf :BranchGroupTerminal_Terminal ;
                              rdf:type owl:FunctionalProperty ;
                              rdfs:domain :Terminal ;
                              rdfs:range <https://w3id.org/netbeheer/IECCIM/TC57CIM/IEC61970/Base/OperationalLimits#BranchGroupTerminal> ;
                              rdfs:comment "The directed branch group terminals for which this terminal is monitored. The terminal to be summed." .


###  https://w3id.org/netbeheer/IECCIM/TC57CIM/IEC61970/Base/Core#Terminal_Bushing
:Terminal_Bushing rdf:type owl:ObjectProperty ;
                  owl:inverseOf :Bushing_Terminal ;
                  rdfs:domain :Terminal ;
                  rdfs:range <https://w3id.org/netbeheer/IECCIM/TC57CIM/IEC61968/InfIEC61968/InfAssets#Bushing> ;
                  rdfs:comment "" .


###  https://w3id.org/netbeheer/IECCIM/TC57CIM/IEC61970/Base/Core#Terminal_ConductingEquipment
:Terminal_ConductingEquipment rdf:type owl:ObjectProperty ;
                              rdfs:domain :Terminal ;
                              rdfs:range :ConductingEquipment ;
                              rdfs:comment "Conducting equipment have terminals that may be connected to other conducting equipment terminals via connectivity nodes or topological nodes.The conducting equipment of the terminal.  Conducting equipment have  terminals that may be connected to other conducting equipment terminals via connectivity nodes or topological nodes." .


###  https://w3id.org/netbeheer/IECCIM/TC57CIM/IEC61970/Base/Core#Terminal_ConnectivityNode
:Terminal_ConnectivityNode rdf:type owl:ObjectProperty ;
                           rdfs:domain :Terminal ;
                           rdfs:range :ConnectivityNode ;
                           rdfs:comment "Terminals interconnected with zero impedance at a this connectivity node. The connectivity node to which this terminal connects with zero impedance." .


###  https://w3id.org/netbeheer/IECCIM/TC57CIM/IEC61970/Base/Core#Terminal_ConverterDCSides
:Terminal_ConverterDCSides rdf:type owl:ObjectProperty ;
                           owl:inverseOf :ACDCConverter_PccTerminal ;
                           rdfs:domain :Terminal ;
                           rdfs:range <https://w3id.org/netbeheer/IECCIM/TC57CIM/IEC61970/Base/DC#ACDCConverter> ;
                           rdfs:comment "All converters' DC sides linked to this point of common coupling terminal.Point of common coupling terminal for this converter DC side. It is typically the terminal on the power transformer (or switch) closest to the AC network. The power flow measurement must be the sum of all flows into the transformer." .


###  https://w3id.org/netbeheer/IECCIM/TC57CIM/IEC61970/Base/Core#Terminal_HasFirstMutualCoupling
:Terminal_HasFirstMutualCoupling rdf:type owl:ObjectProperty ;
                                 owl:inverseOf :MutualCoupling_First_Terminal ;
                                 rdf:type owl:FunctionalProperty ;
                                 rdfs:domain :Terminal ;
                                 rdfs:range <https://w3id.org/netbeheer/IECCIM/TC57CIM/IEC61970/Base/Wires#MutualCoupling> ;
                                 rdfs:comment "Mutual couplings associated with the branch as the first branch.The starting terminal for the calculation of distances along the first branch of the mutual coupling.  Normally MutualCoupling would only be used for terminals of AC line segments.  The first and second terminals of a mutual coupling should point to different AC line segments." .


###  https://w3id.org/netbeheer/IECCIM/TC57CIM/IEC61970/Base/Core#Terminal_HasSecondMutualCoupling
:Terminal_HasSecondMutualCoupling rdf:type owl:ObjectProperty ;
                                  owl:inverseOf :MutualCoupling_Second_Terminal ;
                                  rdf:type owl:FunctionalProperty ;
                                  rdfs:domain :Terminal ;
                                  rdfs:range <https://w3id.org/netbeheer/IECCIM/TC57CIM/IEC61970/Base/Wires#MutualCoupling> ;
                                  rdfs:comment "Mutual couplings with the branch associated as the first branch.The starting terminal for the calculation of distances along the second branch of the mutual coupling." .


###  https://w3id.org/netbeheer/IECCIM/TC57CIM/IEC61970/Base/Core#Terminal_PinTerminal
:Terminal_PinTerminal rdf:type owl:ObjectProperty ;
                      owl:inverseOf :PinTerminal_Terminal ;
                      rdf:type owl:FunctionalProperty ;
                      rdfs:domain :Terminal ;
                      rdfs:range <https://w3id.org/netbeheer/IECCIM/TC57CIM/IEC61970/InfIEC61970/InfSIPS#PinTerminal> ;
                      rdfs:comment "" .


###  https://w3id.org/netbeheer/IECCIM/TC57CIM/IEC61970/Base/Core#Terminal_RegulatingControl
:Terminal_RegulatingControl rdf:type owl:ObjectProperty ;
                            rdfs:domain :Terminal ;
                            rdfs:range <https://w3id.org/netbeheer/IECCIM/TC57CIM/IEC61970/Base/Wires#RegulatingControl> ;
                            rdfs:comment "The terminal associated with this regulating control.  The terminal is associated instead of a node, since the terminal could connect into either a topological node (bus in bus-branch model) or a connectivity node (detailed switch model).  Sometimes it is useful to model regulation at a terminal of a bus bar object since the bus bar can be present in both a bus-branch model or a model with switch detail.The controls regulating this terminal." .


###  https://w3id.org/netbeheer/IECCIM/TC57CIM/IEC61970/Base/Core#Terminal_RemoteInputSignal
:Terminal_RemoteInputSignal rdf:type owl:ObjectProperty ;
                            owl:inverseOf :RemoteInputSignal_Terminal ;
                            rdf:type owl:FunctionalProperty ;
                            rdfs:domain :Terminal ;
                            rdfs:range <https://w3id.org/netbeheer/IECCIM/TC57CIM/IEC61970/Dynamics/StandardInterconnections#RemoteInputSignal> ;
                            rdfs:comment "Input signal coming from this terminal.Remote terminal with which this input signal is associated." .


###  https://w3id.org/netbeheer/IECCIM/TC57CIM/IEC61970/Base/Core#Terminal_SvPowerFlow
:Terminal_SvPowerFlow rdf:type owl:ObjectProperty ;
                      owl:inverseOf :SvPowerFlow_Terminal ;
                      rdf:type owl:FunctionalProperty ;
                      rdfs:domain :Terminal ;
                      rdfs:range <https://w3id.org/netbeheer/IECCIM/TC57CIM/IEC61970/Base/StateVariables#SvPowerFlow> ;
                      rdfs:comment "The power flow state variable associated with the terminal.The terminal associated with the power flow state variable." .


###  https://w3id.org/netbeheer/IECCIM/TC57CIM/IEC61970/Base/Core#Terminal_TieFlow
:Terminal_TieFlow rdf:type owl:ObjectProperty ;
                  owl:inverseOf :TieFlow_Terminal ;
                  rdf:type owl:FunctionalProperty ;
                  rdfs:domain :Terminal ;
                  rdfs:range <https://w3id.org/netbeheer/IECCIM/TC57CIM/IEC61970/Base/ControlArea#TieFlow> ;
                  rdfs:comment "The control area tie flows to which this terminal associates.The terminal to which this tie flow belongs." .


###  https://w3id.org/netbeheer/IECCIM/TC57CIM/IEC61970/Base/Core#Terminal_TopologicalNode
:Terminal_TopologicalNode rdf:type owl:ObjectProperty ;
                          rdfs:domain :Terminal ;
                          rdfs:range <https://w3id.org/netbeheer/IECCIM/TC57CIM/IEC61970/Base/Topology#TopologicalNode> ;
                          rdfs:comment "The terminals associated with the topological node.   This can be used as an alternative to the connectivity node path to terminal, thus making it unneccesary to model connectivity nodes in some cases.   Note that if connectivity nodes are in the model, this association would probably not be used as an input specification.The topological node associated with the terminal.   This can be used as an alternative to the connectivity node path to topological node, thus making it unneccesary to model connectivity nodes in some cases.   Note that the if connectivity nodes are in the model, this association would probably not be used as an input specification." .


###  https://w3id.org/netbeheer/IECCIM/TC57CIM/IEC61970/Base/Core#Terminal_TransformerEnd
:Terminal_TransformerEnd rdf:type owl:ObjectProperty ;
                         owl:inverseOf :TransformerEnd_Terminal ;
                         rdfs:domain :Terminal ;
                         rdfs:range <https://w3id.org/netbeheer/IECCIM/TC57CIM/IEC61970/Base/Wires#TransformerEnd> ;
                         rdfs:comment "All transformer ends connected at this terminal.Terminal of the power transformer to which this transformer end belongs." .


###  https://w3id.org/netbeheer/IECCIM/TC57CIM/IEC61970/Base/Core#TieFlow_Terminal
:TieFlow_Terminal rdf:type owl:ObjectProperty ;
                  rdfs:domain <https://w3id.org/netbeheer/IECCIM/TC57CIM/IEC61970/Base/ControlArea#TieFlow> ;
                  rdfs:range :Terminal ;
                  rdfs:comment "The control area tie flows to which this terminal associates.The terminal to which this tie flow belongs." .


###  https://w3id.org/netbeheer/IECCIM/TC57CIM/IEC61970/Base/Core#TopologicalNode_BaseVoltage
:TopologicalNode_BaseVoltage rdf:type owl:ObjectProperty ;
                             rdfs:domain <https://w3id.org/netbeheer/IECCIM/TC57CIM/IEC61970/Base/Topology#TopologicalNode> ;
                             rdfs:range :BaseVoltage ;
                             rdfs:comment "The topological nodes at the base voltage.The base voltage of the topologocial node." .


###  https://w3id.org/netbeheer/IECCIM/TC57CIM/IEC61970/Base/Core#TopologicalNode_ConnectivityNodeContainer
:TopologicalNode_ConnectivityNodeContainer rdf:type owl:ObjectProperty ;
                                           rdfs:domain <https://w3id.org/netbeheer/IECCIM/TC57CIM/IEC61970/Base/Topology#TopologicalNode> ;
                                           rdfs:range :ConnectivityNodeContainer ;
                                           rdfs:comment "The topological nodes which belong to this connectivity node container.The connectivity node container to which the toplogical node belongs." .


###  https://w3id.org/netbeheer/IECCIM/TC57CIM/IEC61970/Base/Core#TopologicalNode_ConnectivityNodes
:TopologicalNode_ConnectivityNodes rdf:type owl:ObjectProperty ;
                                   owl:inverseOf :ConnectivityNode_TopologicalNode ;
                                   rdfs:domain <https://w3id.org/netbeheer/IECCIM/TC57CIM/IEC61970/Base/Topology#TopologicalNode> ;
                                   rdfs:range :ConnectivityNode ;
                                   rdfs:comment "The connectivity nodes combine together to form this topological node.  May depend on the current state of switches in the network.The topological node to which this connectivity node is assigned.  May depend on the current state of switches in the network." .


###  https://w3id.org/netbeheer/IECCIM/TC57CIM/IEC61970/Base/Core#TopologicalNode_ReportingGroup
:TopologicalNode_ReportingGroup rdf:type owl:ObjectProperty ;
                                rdfs:domain <https://w3id.org/netbeheer/IECCIM/TC57CIM/IEC61970/Base/Topology#TopologicalNode> ;
                                rdfs:range :ReportingGroup ;
                                rdfs:comment "The topological nodes that belong to the reporting group.The reporting group to which the topological node belongs." .


###  https://w3id.org/netbeheer/IECCIM/TC57CIM/IEC61970/Base/Core#TopologicalNode_Terminal
:TopologicalNode_Terminal rdf:type owl:ObjectProperty ;
                          owl:inverseOf :Terminal_TopologicalNode ;
                          rdfs:domain <https://w3id.org/netbeheer/IECCIM/TC57CIM/IEC61970/Base/Topology#TopologicalNode> ;
                          rdfs:range :Terminal ;
                          rdfs:comment "The terminals associated with the topological node.   This can be used as an alternative to the connectivity node path to terminal, thus making it unneccesary to model connectivity nodes in some cases.   Note that if connectivity nodes are in the model, this association would probably not be used as an input specification.The topological node associated with the terminal.   This can be used as an alternative to the connectivity node path to topological node, thus making it unneccesary to model connectivity nodes in some cases.   Note that the if connectivity nodes are in the model, this association would probably not be used as an input specification." .


###  https://w3id.org/netbeheer/IECCIM/TC57CIM/IEC61970/Base/Core#TransformerEnd_BaseVoltage
:TransformerEnd_BaseVoltage rdf:type owl:ObjectProperty ;
                            rdfs:domain <https://w3id.org/netbeheer/IECCIM/TC57CIM/IEC61970/Base/Wires#TransformerEnd> ;
                            rdfs:range :BaseVoltage ;
                            rdfs:comment "Transformer ends at the base voltage.  This is essential for PU calculation.Base voltage of the transformer end.  This is essential for PU calculation." .


###  https://w3id.org/netbeheer/IECCIM/TC57CIM/IEC61970/Base/Core#TransformerEnd_Terminal
:TransformerEnd_Terminal rdf:type owl:ObjectProperty ;
                         rdfs:domain <https://w3id.org/netbeheer/IECCIM/TC57CIM/IEC61970/Base/Wires#TransformerEnd> ;
                         rdfs:range :Terminal ;
                         rdfs:comment "All transformer ends connected at this terminal.Terminal of the power transformer to which this transformer end belongs." .


###  https://w3id.org/netbeheer/IECCIM/TC57CIM/IEC61970/Base/Core#UsagePoint_Equipments
:UsagePoint_Equipments rdf:type owl:ObjectProperty ;
                       rdfs:domain <https://w3id.org/netbeheer/IECCIM/TC57CIM/IEC61968/Metering#UsagePoint> ;
                       rdfs:range :Equipment ;
                       rdfs:comment "All usage points connected to the electrical grid through this equipment.All equipment connecting this usage point to the electrical grid." .


###  https://w3id.org/netbeheer/IECCIM/TC57CIM/IEC61970/Base/Core#VoltageLevel_BaseVoltage
:VoltageLevel_BaseVoltage rdf:type owl:ObjectProperty ;
                          rdfs:domain :VoltageLevel ;
                          rdfs:range :BaseVoltage ;
                          rdfs:comment "The voltage levels having this base voltage.The base voltage used for all equipment within the voltage level." .


###  https://w3id.org/netbeheer/IECCIM/TC57CIM/IEC61970/Base/Core#VoltageLevel_Bays
:VoltageLevel_Bays rdf:type owl:ObjectProperty ;
                   rdfs:domain :VoltageLevel ;
                   rdfs:range :Bay ;
                   rdfs:comment "The voltage level containing this bay.The bays within this voltage level." .


###  https://w3id.org/netbeheer/IECCIM/TC57CIM/IEC61970/Base/Core#VoltageLevel_Substation
:VoltageLevel_Substation rdf:type owl:ObjectProperty ;
                         owl:inverseOf :Substation_VoltageLevels ;
                         rdfs:domain :VoltageLevel ;
                         rdfs:range :Substation ;
                         rdfs:comment "The substation of the voltage level.The voltage levels within this substation." .


###  https://w3id.org/netbeheer/IECCIM/TC57CIM/IEC61970/Base/Core#VoltageLevel_highVoltageLimit
:VoltageLevel_highVoltageLimit rdf:type owl:ObjectProperty ;
                               rdfs:domain :VoltageLevel ;
                               rdfs:range <https://w3id.org/netbeheer/IECCIM/TC57CIM/IEC61970/Base/Domain#Voltage> ;
                               rdfs:comment "The bus bar's high voltage limit" .


###  https://w3id.org/netbeheer/IECCIM/TC57CIM/IEC61970/Base/Core#VoltageLevel_lowVoltageLimit
:VoltageLevel_lowVoltageLimit rdf:type owl:ObjectProperty ;
                              rdfs:domain :VoltageLevel ;
                              rdfs:range <https://w3id.org/netbeheer/IECCIM/TC57CIM/IEC61970/Base/Domain#Voltage> ;
                              rdfs:comment "The bus bar's low voltage limit" .


###  https://w3id.org/netbeheer/IECCIM/TC57CIM/IEC61970/Base/Core#WeatherStation_Equipment
:WeatherStation_Equipment rdf:type owl:ObjectProperty ;
                          owl:inverseOf :Equipment_WeatherStation ;
                          rdfs:domain <https://w3id.org/netbeheer/IECCIM/TC57CIM/IEC61970/InfIEC61970/InfOperationalLimits#WeatherStation> ;
                          rdfs:range :Equipment ;
                          rdfs:comment "" .


#################################################################
#    Data properties
#################################################################

###  https://w3id.org/netbeheer/IECCIM/TC57CIM/IEC61970/Base/Core#ACDCTerminal_connected
:ACDCTerminal_connected rdf:type owl:DatatypeProperty ;
                        rdfs:domain :ACDCTerminal ;
                        rdfs:range xsd:boolean ;
                        rdfs:comment """The connected status is related to a bus-branch model and the topological node to terminal relation.  True implies the terminal is connected to the related topological node and false implies it is not. 
In a bus-branch model, the connected status is used to tell if equipment is disconnected without having to change the connectivity described by the topological node to terminal relation. A valid case is that conducting equipment can be connected in one end and open in the other. In particular for an AC line segment, where the reactive line charging can be significant, this is a relevant case.
""" .


###  https://w3id.org/netbeheer/IECCIM/TC57CIM/IEC61970/Base/Core#ACDCTerminal_sequenceNumber
:ACDCTerminal_sequenceNumber rdf:type owl:DatatypeProperty ;
                             rdfs:domain :ACDCTerminal ;
                             rdfs:range xsd:nonNegativeInteger ;
                             rdfs:comment """The orientation of the terminal connections for a multiple terminal conducting equipment.  The sequence numbering starts with 1 and additional terminals should follow in increasing order.   The first terminal is the \"starting point\" for a two terminal branch.
""" .


###  https://w3id.org/netbeheer/IECCIM/TC57CIM/IEC61970/Base/Core#BasicIntervalSchedule_startTime
:BasicIntervalSchedule_startTime rdf:type owl:DatatypeProperty ;
                                 rdfs:domain :BasicIntervalSchedule ;
                                 rdfs:range xsd:dateTime ;
                                 rdfs:comment "The time for the first time point." .


###  https://w3id.org/netbeheer/IECCIM/TC57CIM/IEC61970/Base/Core#BasicIntervalSchedule_value1Multiplier
:BasicIntervalSchedule_value1Multiplier rdf:type owl:DatatypeProperty ;
                                        rdfs:domain :BasicIntervalSchedule ;
                                        rdfs:range <https://w3id.org/netbeheer/IECCIM/TC57CIM/IEC61970/Base/Domain#UnitMultiplier> ;
                                        rdfs:comment "Multiplier for value1." .


###  https://w3id.org/netbeheer/IECCIM/TC57CIM/IEC61970/Base/Core#BasicIntervalSchedule_value1Unit
:BasicIntervalSchedule_value1Unit rdf:type owl:DatatypeProperty ;
                                  rdfs:domain :BasicIntervalSchedule ;
                                  rdfs:range <https://w3id.org/netbeheer/IECCIM/TC57CIM/IEC61970/Base/Domain#UnitSymbol> ;
                                  rdfs:comment "Value1 units of measure." .


###  https://w3id.org/netbeheer/IECCIM/TC57CIM/IEC61970/Base/Core#BasicIntervalSchedule_value2Multiplier
:BasicIntervalSchedule_value2Multiplier rdf:type owl:DatatypeProperty ;
                                        rdfs:domain :BasicIntervalSchedule ;
                                        rdfs:range <https://w3id.org/netbeheer/IECCIM/TC57CIM/IEC61970/Base/Domain#UnitMultiplier> ;
                                        rdfs:comment "Multiplier for value2." .


###  https://w3id.org/netbeheer/IECCIM/TC57CIM/IEC61970/Base/Core#BasicIntervalSchedule_value2Unit
:BasicIntervalSchedule_value2Unit rdf:type owl:DatatypeProperty ;
                                  rdfs:domain :BasicIntervalSchedule ;
                                  rdfs:range <https://w3id.org/netbeheer/IECCIM/TC57CIM/IEC61970/Base/Domain#UnitSymbol> ;
                                  rdfs:comment "Value2 units of measure." .


###  https://w3id.org/netbeheer/IECCIM/TC57CIM/IEC61970/Base/Core#Bay_bayEnergyMeasFlag
:Bay_bayEnergyMeasFlag rdf:type owl:DatatypeProperty ;
                       rdfs:domain :Bay ;
                       rdfs:range xsd:boolean ;
                       rdfs:comment "Indicates the presence/absence of energy measurements." .


###  https://w3id.org/netbeheer/IECCIM/TC57CIM/IEC61970/Base/Core#Bay_bayPowerMeasFlag
:Bay_bayPowerMeasFlag rdf:type owl:DatatypeProperty ;
                      rdfs:domain :Bay ;
                      rdfs:range xsd:boolean ;
                      rdfs:comment "Indicates the presence/absence of active/reactive power measurements." .


###  https://w3id.org/netbeheer/IECCIM/TC57CIM/IEC61970/Base/Core#Bay_breakerConfiguration
:Bay_breakerConfiguration rdf:type owl:DatatypeProperty ;
                          rdfs:domain :Bay ;
                          rdfs:range :BreakerConfiguration ;
                          rdfs:comment "Breaker configuration. " .


###  https://w3id.org/netbeheer/IECCIM/TC57CIM/IEC61970/Base/Core#Bay_busBarConfiguration
:Bay_busBarConfiguration rdf:type owl:DatatypeProperty ;
                         rdfs:domain :Bay ;
                         rdfs:range :BusbarConfiguration ;
                         rdfs:comment "Bus bar configuration." .


###  https://w3id.org/netbeheer/IECCIM/TC57CIM/IEC61970/Base/Core#CurveData_xvalue
:CurveData_xvalue rdf:type owl:DatatypeProperty ;
                  rdfs:domain :CurveData ;
                  rdfs:range xsd:float ;
                  rdfs:comment """The data value of the X-axis variable,  depending on the X-axis units.
""" .


###  https://w3id.org/netbeheer/IECCIM/TC57CIM/IEC61970/Base/Core#CurveData_y1value
:CurveData_y1value rdf:type owl:DatatypeProperty ;
                   rdfs:domain :CurveData ;
                   rdfs:range xsd:float ;
                   rdfs:comment """The data value of the  first Y-axis variable, depending on the Y-axis units.
""" .


###  https://w3id.org/netbeheer/IECCIM/TC57CIM/IEC61970/Base/Core#CurveData_y2value
:CurveData_y2value rdf:type owl:DatatypeProperty ;
                   rdfs:domain :CurveData ;
                   rdfs:range xsd:float ;
                   rdfs:comment """The data value of the second Y-axis variable (if present), depending on the Y-axis units.
""" .


###  https://w3id.org/netbeheer/IECCIM/TC57CIM/IEC61970/Base/Core#CurveData_y3value
:CurveData_y3value rdf:type owl:DatatypeProperty ;
                   rdfs:domain :CurveData ;
                   rdfs:range xsd:float ;
                   rdfs:comment """The data value of the third Y-axis variable (if present), depending on the Y-axis units.
""" .


###  https://w3id.org/netbeheer/IECCIM/TC57CIM/IEC61970/Base/Core#Curve_curveStyle
:Curve_curveStyle rdf:type owl:DatatypeProperty ;
                  rdfs:domain :Curve ;
                  rdfs:range :CurveStyle ;
                  rdfs:comment "The style or shape of the curve." .


###  https://w3id.org/netbeheer/IECCIM/TC57CIM/IEC61970/Base/Core#Curve_xMultiplier
:Curve_xMultiplier rdf:type owl:DatatypeProperty ;
                   rdfs:domain :Curve ;
                   rdfs:range <https://w3id.org/netbeheer/IECCIM/TC57CIM/IEC61970/Base/Domain#UnitMultiplier> ;
                   rdfs:comment "Multiplier for X-axis." .


###  https://w3id.org/netbeheer/IECCIM/TC57CIM/IEC61970/Base/Core#Curve_xUnit
:Curve_xUnit rdf:type owl:DatatypeProperty ;
             rdfs:domain :Curve ;
             rdfs:range <https://w3id.org/netbeheer/IECCIM/TC57CIM/IEC61970/Base/Domain#UnitSymbol> ;
             rdfs:comment "The X-axis units of measure." .


###  https://w3id.org/netbeheer/IECCIM/TC57CIM/IEC61970/Base/Core#Curve_y1Multiplier
:Curve_y1Multiplier rdf:type owl:DatatypeProperty ;
                    rdfs:domain :Curve ;
                    rdfs:range <https://w3id.org/netbeheer/IECCIM/TC57CIM/IEC61970/Base/Domain#UnitMultiplier> ;
                    rdfs:comment """Multiplier for Y1-axis.
""" .


###  https://w3id.org/netbeheer/IECCIM/TC57CIM/IEC61970/Base/Core#Curve_y1Unit
:Curve_y1Unit rdf:type owl:DatatypeProperty ;
              rdfs:domain :Curve ;
              rdfs:range <https://w3id.org/netbeheer/IECCIM/TC57CIM/IEC61970/Base/Domain#UnitSymbol> ;
              rdfs:comment "The Y1-axis units of measure." .


###  https://w3id.org/netbeheer/IECCIM/TC57CIM/IEC61970/Base/Core#Curve_y2Multiplier
:Curve_y2Multiplier rdf:type owl:DatatypeProperty ;
                    rdfs:domain :Curve ;
                    rdfs:range <https://w3id.org/netbeheer/IECCIM/TC57CIM/IEC61970/Base/Domain#UnitMultiplier> ;
                    rdfs:comment "Multiplier for Y2-axis." .


###  https://w3id.org/netbeheer/IECCIM/TC57CIM/IEC61970/Base/Core#Curve_y2Unit
:Curve_y2Unit rdf:type owl:DatatypeProperty ;
              rdfs:domain :Curve ;
              rdfs:range <https://w3id.org/netbeheer/IECCIM/TC57CIM/IEC61970/Base/Domain#UnitSymbol> ;
              rdfs:comment "The Y2-axis units of measure." .


###  https://w3id.org/netbeheer/IECCIM/TC57CIM/IEC61970/Base/Core#Curve_y3Multiplier
:Curve_y3Multiplier rdf:type owl:DatatypeProperty ;
                    rdfs:domain :Curve ;
                    rdfs:range <https://w3id.org/netbeheer/IECCIM/TC57CIM/IEC61970/Base/Domain#UnitMultiplier> ;
                    rdfs:comment "Multiplier for Y3-axis." .


###  https://w3id.org/netbeheer/IECCIM/TC57CIM/IEC61970/Base/Core#Curve_y3Unit
:Curve_y3Unit rdf:type owl:DatatypeProperty ;
              rdfs:domain :Curve ;
              rdfs:range <https://w3id.org/netbeheer/IECCIM/TC57CIM/IEC61970/Base/Domain#UnitSymbol> ;
              rdfs:comment "The Y3-axis units of measure." .


###  https://w3id.org/netbeheer/IECCIM/TC57CIM/IEC61970/Base/Core#Equipment_aggregate
:Equipment_aggregate rdf:type owl:DatatypeProperty ;
                     rdfs:domain :Equipment ;
                     rdfs:range xsd:boolean ;
                     rdfs:comment "The single instance of equipment represents multiple pieces of equipment that have been modeled together as an aggregate.  Examples would be power transformers or synchronous machines operating in parallel modeled as a single aggregate power transformer or aggregate synchronous machine.  This is not to be used to indicate equipment that is part of a group of interdependent equipment produced by a network production program.  " .


###  https://w3id.org/netbeheer/IECCIM/TC57CIM/IEC61970/Base/Core#Equipment_inService
:Equipment_inService rdf:type owl:DatatypeProperty ;
                     rdfs:domain :Equipment ;
                     rdfs:range xsd:boolean ;
                     rdfs:comment "If true, the equipment is in service." .


###  https://w3id.org/netbeheer/IECCIM/TC57CIM/IEC61970/Base/Core#Equipment_normallyInService
:Equipment_normallyInService rdf:type owl:DatatypeProperty ;
                             rdfs:domain :Equipment ;
                             rdfs:range xsd:boolean ;
                             rdfs:comment "If true, the equipment is normally in service." .


###  https://w3id.org/netbeheer/IECCIM/TC57CIM/IEC61970/Base/Core#IdentifiedObject_aliasName
:IdentifiedObject_aliasName rdf:type owl:DatatypeProperty ;
                            rdfs:domain :IdentifiedObject ;
                            rdfs:range xsd:string ;
                            rdfs:comment """The aliasName is free text human readable name of the object alternative to IdentifiedObject.name. It may be non unique and may not correlate to a naming hierarchy.
The attribute aliasName is retained because of backwards compatibility between CIM relases. It is however recommended to replace aliasName with the Name class as aliasName is planned for retirement at a future time.

""" .


###  https://w3id.org/netbeheer/IECCIM/TC57CIM/IEC61970/Base/Core#IdentifiedObject_description
:IdentifiedObject_description rdf:type owl:DatatypeProperty ;
                              rdfs:domain :IdentifiedObject ;
                              rdfs:range xsd:string ;
                              rdfs:comment "The description is a free human readable text describing or naming the object. It may be non unique and may not correlate to a naming hierarchy." .


###  https://w3id.org/netbeheer/IECCIM/TC57CIM/IEC61970/Base/Core#IdentifiedObject_mRID
:IdentifiedObject_mRID rdf:type owl:DatatypeProperty ;
                       rdfs:domain :IdentifiedObject ;
                       rdfs:range xsd:string ;
                       rdfs:comment """Master resource identifier issued by a model authority. The mRID is unique within an exchange context. Global uniqueness is easily achieved by using a UUID,  as specified in RFC 4122, for the mRID. The use of UUID is strongly recommended.
For CIMXML data files in RDF syntax conforming to IEC 61970-552 Edition 1, the mRID is mapped to rdf:ID or rdf:about attributes that identify CIM object elements.""" .


###  https://w3id.org/netbeheer/IECCIM/TC57CIM/IEC61970/Base/Core#IdentifiedObject_name
:IdentifiedObject_name rdf:type owl:DatatypeProperty ;
                       rdfs:domain :IdentifiedObject ;
                       rdfs:range xsd:string ;
                       rdfs:comment """The name is any free human readable and possibly non unique text naming the object.
""" .


###  https://w3id.org/netbeheer/IECCIM/TC57CIM/IEC61970/Base/Core#IrregularTimePoint_value1
:IrregularTimePoint_value1 rdf:type owl:DatatypeProperty ;
                           rdfs:domain :IrregularTimePoint ;
                           rdfs:range xsd:float ;
                           rdfs:comment """The first value at the time. The meaning of the value is defined by the derived type of the associated schedule.
""" .


###  https://w3id.org/netbeheer/IECCIM/TC57CIM/IEC61970/Base/Core#IrregularTimePoint_value2
:IrregularTimePoint_value2 rdf:type owl:DatatypeProperty ;
                           rdfs:domain :IrregularTimePoint ;
                           rdfs:range xsd:float ;
                           rdfs:comment """The second value at the time. The meaning of the value is defined by the derived type of the associated schedule.
""" .


###  https://w3id.org/netbeheer/IECCIM/TC57CIM/IEC61970/Base/Core#NameTypeAuthority_description
:NameTypeAuthority_description rdf:type owl:DatatypeProperty ;
                               rdfs:domain :NameTypeAuthority ;
                               rdfs:range xsd:string ;
                               rdfs:comment """Description of the name type authority.
""" .


###  https://w3id.org/netbeheer/IECCIM/TC57CIM/IEC61970/Base/Core#NameTypeAuthority_name
:NameTypeAuthority_name rdf:type owl:DatatypeProperty ;
                        rdfs:domain :NameTypeAuthority ;
                        rdfs:range xsd:string ;
                        rdfs:comment """Name of the name type authority.
""" .


###  https://w3id.org/netbeheer/IECCIM/TC57CIM/IEC61970/Base/Core#NameType_description
:NameType_description rdf:type owl:DatatypeProperty ;
                      rdfs:domain :NameType ;
                      rdfs:range xsd:string ;
                      rdfs:comment """Description of the name type.
""" .


###  https://w3id.org/netbeheer/IECCIM/TC57CIM/IEC61970/Base/Core#NameType_name
:NameType_name rdf:type owl:DatatypeProperty ;
               rdfs:domain :NameType ;
               rdfs:range xsd:string ;
               rdfs:comment """Name of the name type.
""" .


###  https://w3id.org/netbeheer/IECCIM/TC57CIM/IEC61970/Base/Core#Name_name
:Name_name rdf:type owl:DatatypeProperty ;
           rdfs:domain :Name ;
           rdfs:range xsd:string ;
           rdfs:comment """Any free text that name the object.
""" .


###  https://w3id.org/netbeheer/IECCIM/TC57CIM/IEC61970/Base/Core#RegularIntervalSchedule_endTime
:RegularIntervalSchedule_endTime rdf:type owl:DatatypeProperty ;
                                 rdfs:domain :RegularIntervalSchedule ;
                                 rdfs:range xsd:dateTime ;
                                 rdfs:comment "The time for the last time point." .


###  https://w3id.org/netbeheer/IECCIM/TC57CIM/IEC61970/Base/Core#RegularTimePoint_sequenceNumber
:RegularTimePoint_sequenceNumber rdf:type owl:DatatypeProperty ;
                                 rdfs:domain :RegularTimePoint ;
                                 rdfs:range xsd:nonNegativeInteger ;
                                 rdfs:comment """The position of the regular time point in the sequence. Note that time points don't have to be sequential, i.e. time points may be omitted. The actual time for a RegularTimePoint is computed by multiplying the associated regular interval schedule's time step with the regular time point sequence number and adding the associated schedules start time.
""" .


###  https://w3id.org/netbeheer/IECCIM/TC57CIM/IEC61970/Base/Core#RegularTimePoint_value1
:RegularTimePoint_value1 rdf:type owl:DatatypeProperty ;
                         rdfs:domain :RegularTimePoint ;
                         rdfs:range xsd:float ;
                         rdfs:comment """The first value at the time. The meaning of the value is defined by the derived type of the associated schedule.
""" .


###  https://w3id.org/netbeheer/IECCIM/TC57CIM/IEC61970/Base/Core#RegularTimePoint_value2
:RegularTimePoint_value2 rdf:type owl:DatatypeProperty ;
                         rdfs:domain :RegularTimePoint ;
                         rdfs:range xsd:float ;
                         rdfs:comment """The second value at the time. The meaning of the value is defined by the derived type of the associated schedule.

""" .


###  https://w3id.org/netbeheer/IECCIM/TC57CIM/IEC61970/Base/Core#Terminal_phases
:Terminal_phases rdf:type owl:DatatypeProperty ;
                 rdfs:domain :Terminal ;
                 rdfs:range :PhaseCode ;
                 rdfs:comment """Represents the normal network phasing condition.
If the attribute is missing three phases (ABC or ABCN) shall be assumed.""" .


#################################################################
#    Classes
#################################################################

###  https://w3id.org/netbeheer/IECCIM/TC57CIM/IEC61968/Assets#Asset
<https://w3id.org/netbeheer/IECCIM/TC57CIM/IEC61968/Assets#Asset> rdf:type owl:Class ;
                                                                  rdfs:subClassOf [ rdf:type owl:Restriction ;
                                                                                    owl:onProperty :Asset_PowerSystemResources ;
                                                                                    owl:minQualifiedCardinality "0"^^xsd:nonNegativeInteger ;
                                                                                    owl:onClass <https://w3id.org/netbeheer/IECCIM/TC57CIM/IEC61968/Assets#Asset>
                                                                                  ] .


###  https://w3id.org/netbeheer/IECCIM/TC57CIM/IEC61968/Assets#AssetInfo
<https://w3id.org/netbeheer/IECCIM/TC57CIM/IEC61968/Assets#AssetInfo> rdf:type owl:Class ;
                                                                      rdfs:subClassOf [ rdf:type owl:Restriction ;
                                                                                        owl:onProperty :AssetInfo_PowerSystemResources ;
                                                                                        owl:minQualifiedCardinality "0"^^xsd:nonNegativeInteger ;
                                                                                        owl:onClass <https://w3id.org/netbeheer/IECCIM/TC57CIM/IEC61968/Assets#AssetInfo>
                                                                                      ] ,
                                                                                      [ rdf:type owl:Restriction ;
                                                                                        owl:onProperty :AssetInfo_PowerSystemResources ;
                                                                                        owl:maxQualifiedCardinality "1"^^xsd:nonNegativeInteger ;
                                                                                        owl:onClass <https://w3id.org/netbeheer/IECCIM/TC57CIM/IEC61968/Assets#AssetInfo>
                                                                                      ] .


###  https://w3id.org/netbeheer/IECCIM/TC57CIM/IEC61968/Common#Location
<https://w3id.org/netbeheer/IECCIM/TC57CIM/IEC61968/Common#Location> rdf:type owl:Class ;
                                                                     rdfs:subClassOf [ rdf:type owl:Restriction ;
                                                                                       owl:onProperty :Location_PowerSystemResources ;
                                                                                       owl:minQualifiedCardinality "0"^^xsd:nonNegativeInteger ;
                                                                                       owl:onClass <https://w3id.org/netbeheer/IECCIM/TC57CIM/IEC61968/Common#Location>
                                                                                     ] ,
                                                                                     [ rdf:type owl:Restriction ;
                                                                                       owl:onProperty :Location_PowerSystemResources ;
                                                                                       owl:maxQualifiedCardinality "1"^^xsd:nonNegativeInteger ;
                                                                                       owl:onClass <https://w3id.org/netbeheer/IECCIM/TC57CIM/IEC61968/Common#Location>
                                                                                     ] .


###  https://w3id.org/netbeheer/IECCIM/TC57CIM/IEC61968/InfIEC61968/InfAssets#Bushing
<https://w3id.org/netbeheer/IECCIM/TC57CIM/IEC61968/InfIEC61968/InfAssets#Bushing> rdf:type owl:Class ;
                                                                                   rdfs:subClassOf [ rdf:type owl:Restriction ;
                                                                                                     owl:onProperty :Bushing_Terminal ;
                                                                                                     owl:minQualifiedCardinality "0"^^xsd:nonNegativeInteger ;
                                                                                                     owl:onClass <https://w3id.org/netbeheer/IECCIM/TC57CIM/IEC61968/InfIEC61968/InfAssets#Bushing>
                                                                                                   ] ,
                                                                                                   [ rdf:type owl:Restriction ;
                                                                                                     owl:onProperty :Bushing_Terminal ;
                                                                                                     owl:maxQualifiedCardinality "1"^^xsd:nonNegativeInteger ;
                                                                                                     owl:onClass <https://w3id.org/netbeheer/IECCIM/TC57CIM/IEC61968/InfIEC61968/InfAssets#Bushing>
                                                                                                   ] .


###  https://w3id.org/netbeheer/IECCIM/TC57CIM/IEC61968/Metering#UsagePoint
<https://w3id.org/netbeheer/IECCIM/TC57CIM/IEC61968/Metering#UsagePoint> rdf:type owl:Class ;
                                                                         rdfs:subClassOf [ rdf:type owl:Restriction ;
                                                                                           owl:onProperty :UsagePoint_Equipments ;
                                                                                           owl:minQualifiedCardinality "0"^^xsd:nonNegativeInteger ;
                                                                                           owl:onClass <https://w3id.org/netbeheer/IECCIM/TC57CIM/IEC61968/Metering#UsagePoint>
                                                                                         ] .


###  https://w3id.org/netbeheer/IECCIM/TC57CIM/IEC61968/Operations#ClearanceDocument
<https://w3id.org/netbeheer/IECCIM/TC57CIM/IEC61968/Operations#ClearanceDocument> rdf:type owl:Class ;
                                                                                  rdfs:subClassOf [ rdf:type owl:Restriction ;
                                                                                                    owl:onProperty :ClearanceDocument_TaggedPSRs ;
                                                                                                    owl:minQualifiedCardinality "0"^^xsd:nonNegativeInteger ;
                                                                                                    owl:onClass <https://w3id.org/netbeheer/IECCIM/TC57CIM/IEC61968/Operations#ClearanceDocument>
                                                                                                  ] .


###  https://w3id.org/netbeheer/IECCIM/TC57CIM/IEC61968/Operations#GroundAction
<https://w3id.org/netbeheer/IECCIM/TC57CIM/IEC61968/Operations#GroundAction> rdf:type owl:Class ;
                                                                             rdfs:subClassOf [ rdf:type owl:Restriction ;
                                                                                               owl:onProperty :GroundAction_GroundedEquipment ;
                                                                                               owl:minQualifiedCardinality "0"^^xsd:nonNegativeInteger ;
                                                                                               owl:onClass <https://w3id.org/netbeheer/IECCIM/TC57CIM/IEC61968/Operations#GroundAction>
                                                                                             ] ,
                                                                                             [ rdf:type owl:Restriction ;
                                                                                               owl:onProperty :GroundAction_GroundedEquipment ;
                                                                                               owl:maxQualifiedCardinality "1"^^xsd:nonNegativeInteger ;
                                                                                               owl:onClass <https://w3id.org/netbeheer/IECCIM/TC57CIM/IEC61968/Operations#GroundAction>
                                                                                             ] .


###  https://w3id.org/netbeheer/IECCIM/TC57CIM/IEC61968/Operations#JumperAction
<https://w3id.org/netbeheer/IECCIM/TC57CIM/IEC61968/Operations#JumperAction> rdf:type owl:Class ;
                                                                             rdfs:subClassOf [ rdf:type owl:Restriction ;
                                                                                               owl:onProperty :JumperAction_JumpedEquipments ;
                                                                                               owl:minQualifiedCardinality "0"^^xsd:nonNegativeInteger ;
                                                                                               owl:onClass <https://w3id.org/netbeheer/IECCIM/TC57CIM/IEC61968/Operations#JumperAction>
                                                                                             ] ,
                                                                                             [ rdf:type owl:Restriction ;
                                                                                               owl:onProperty :JumperAction_JumpedEquipments ;
                                                                                               owl:maxQualifiedCardinality "1"^^xsd:nonNegativeInteger ;
                                                                                               owl:onClass <https://w3id.org/netbeheer/IECCIM/TC57CIM/IEC61968/Operations#JumperAction>
                                                                                             ] .


###  https://w3id.org/netbeheer/IECCIM/TC57CIM/IEC61968/Operations#OperationalRestriction
<https://w3id.org/netbeheer/IECCIM/TC57CIM/IEC61968/Operations#OperationalRestriction> rdf:type owl:Class ;
                                                                                       rdfs:subClassOf [ rdf:type owl:Restriction ;
                                                                                                         owl:onProperty :OperationalRestriction_Equipments ;
                                                                                                         owl:minQualifiedCardinality "0"^^xsd:nonNegativeInteger ;
                                                                                                         owl:onClass <https://w3id.org/netbeheer/IECCIM/TC57CIM/IEC61968/Operations#OperationalRestriction>
                                                                                                       ] .


###  https://w3id.org/netbeheer/IECCIM/TC57CIM/IEC61968/Operations#OperationalTag
<https://w3id.org/netbeheer/IECCIM/TC57CIM/IEC61968/Operations#OperationalTag> rdf:type owl:Class ;
                                                                               rdfs:subClassOf [ rdf:type owl:Restriction ;
                                                                                                 owl:onProperty :OperationalTag_PowerSystemResource ;
                                                                                                 owl:minQualifiedCardinality "0"^^xsd:nonNegativeInteger ;
                                                                                                 owl:onClass <https://w3id.org/netbeheer/IECCIM/TC57CIM/IEC61968/Operations#OperationalTag>
                                                                                               ] .


###  https://w3id.org/netbeheer/IECCIM/TC57CIM/IEC61968/Operations#Outage
<https://w3id.org/netbeheer/IECCIM/TC57CIM/IEC61968/Operations#Outage> rdf:type owl:Class ;
                                                                       rdfs:subClassOf [ rdf:type owl:Restriction ;
                                                                                         owl:onProperty :Outage_Equipments ;
                                                                                         owl:minQualifiedCardinality "0"^^xsd:nonNegativeInteger ;
                                                                                         owl:onClass <https://w3id.org/netbeheer/IECCIM/TC57CIM/IEC61968/Operations#Outage>
                                                                                       ] .


###  https://w3id.org/netbeheer/IECCIM/TC57CIM/IEC61968/Operations#PSREvent
<https://w3id.org/netbeheer/IECCIM/TC57CIM/IEC61968/Operations#PSREvent> rdf:type owl:Class ;
                                                                         rdfs:subClassOf [ rdf:type owl:Restriction ;
                                                                                           owl:onProperty :PSREvent_PowerSystemResource ;
                                                                                           owl:minQualifiedCardinality "0"^^xsd:nonNegativeInteger ;
                                                                                           owl:onClass <https://w3id.org/netbeheer/IECCIM/TC57CIM/IEC61968/Operations#PSREvent>
                                                                                         ] .


###  https://w3id.org/netbeheer/IECCIM/TC57CIM/IEC61970/Base/AuxiliaryEquipment#AuxiliaryEquipment
<https://w3id.org/netbeheer/IECCIM/TC57CIM/IEC61970/Base/AuxiliaryEquipment#AuxiliaryEquipment> rdf:type owl:Class ;
                                                                                                rdfs:subClassOf [ rdf:type owl:Restriction ;
                                                                                                                  owl:onProperty :AuxiliaryEquipment_Terminal ;
                                                                                                                  owl:minQualifiedCardinality "0"^^xsd:nonNegativeInteger ;
                                                                                                                  owl:onClass <https://w3id.org/netbeheer/IECCIM/TC57CIM/IEC61970/Base/AuxiliaryEquipment#AuxiliaryEquipment>
                                                                                                                ] .


###  https://w3id.org/netbeheer/IECCIM/TC57CIM/IEC61970/Base/Contingency#ContingencyEquipment
<https://w3id.org/netbeheer/IECCIM/TC57CIM/IEC61970/Base/Contingency#ContingencyEquipment> rdf:type owl:Class ;
                                                                                           rdfs:subClassOf [ rdf:type owl:Restriction ;
                                                                                                             owl:onProperty :ContingencyEquipment_Equipment ;
                                                                                                             owl:minQualifiedCardinality "0"^^xsd:nonNegativeInteger ;
                                                                                                             owl:onClass <https://w3id.org/netbeheer/IECCIM/TC57CIM/IEC61970/Base/Contingency#ContingencyEquipment>
                                                                                                           ] .


###  https://w3id.org/netbeheer/IECCIM/TC57CIM/IEC61970/Base/ControlArea#TieFlow
<https://w3id.org/netbeheer/IECCIM/TC57CIM/IEC61970/Base/ControlArea#TieFlow> rdf:type owl:Class ;
                                                                              rdfs:subClassOf [ rdf:type owl:Restriction ;
                                                                                                owl:onProperty :TieFlow_Terminal ;
                                                                                                owl:minQualifiedCardinality "0"^^xsd:nonNegativeInteger ;
                                                                                                owl:onClass <https://w3id.org/netbeheer/IECCIM/TC57CIM/IEC61970/Base/ControlArea#TieFlow>
                                                                                              ] ,
                                                                                              [ rdf:type owl:Restriction ;
                                                                                                owl:onProperty :TieFlow_Terminal ;
                                                                                                owl:maxQualifiedCardinality "2"^^xsd:nonNegativeInteger ;
                                                                                                owl:onClass <https://w3id.org/netbeheer/IECCIM/TC57CIM/IEC61970/Base/ControlArea#TieFlow>
                                                                                              ] .


###  https://w3id.org/netbeheer/IECCIM/TC57CIM/IEC61970/Base/Core#ACDCTerminal
:ACDCTerminal rdf:type owl:Class ;
              rdfs:subClassOf :IdentifiedObject ,
                              [ rdf:type owl:Restriction ;
                                owl:onProperty :ACDCTerminal_BusNameMarker ;
                                owl:minQualifiedCardinality "1"^^xsd:nonNegativeInteger ;
                                owl:onClass :ACDCTerminal
                              ] ,
                              [ rdf:type owl:Restriction ;
                                owl:onProperty :ACDCTerminal_Measurements ;
                                owl:minQualifiedCardinality "0"^^xsd:nonNegativeInteger ;
                                owl:onClass :ACDCTerminal
                              ] ,
                              [ rdf:type owl:Restriction ;
                                owl:onProperty :ACDCTerminal_OperationalLimitSet ;
                                owl:minQualifiedCardinality "0"^^xsd:nonNegativeInteger ;
                                owl:onClass :ACDCTerminal
                              ] ,
                              [ rdf:type owl:Restriction ;
                                owl:onProperty :ACDCTerminal_Measurements ;
                                owl:maxQualifiedCardinality "1"^^xsd:nonNegativeInteger ;
                                owl:onClass :ACDCTerminal
                              ] ,
                              [ rdf:type owl:Restriction ;
                                owl:onProperty :ACDCTerminal_OperationalLimitSet ;
                                owl:maxQualifiedCardinality "1"^^xsd:nonNegativeInteger ;
                                owl:onClass :ACDCTerminal
                              ] ,
                              [ rdf:type owl:Restriction ;
                                owl:onProperty :ACDCTerminal_connected ;
                                owl:minQualifiedCardinality "0"^^xsd:nonNegativeInteger ;
                                owl:onDataRange xsd:boolean
                              ] ,
                              [ rdf:type owl:Restriction ;
                                owl:onProperty :ACDCTerminal_sequenceNumber ;
                                owl:minQualifiedCardinality "0"^^xsd:nonNegativeInteger ;
                                owl:onDataRange xsd:nonNegativeInteger
                              ] ,
                              [ rdf:type owl:Restriction ;
                                owl:onProperty :ACDCTerminal_connected ;
                                owl:maxQualifiedCardinality "1"^^xsd:nonNegativeInteger ;
                                owl:onDataRange xsd:boolean
                              ] ,
                              [ rdf:type owl:Restriction ;
                                owl:onProperty :ACDCTerminal_sequenceNumber ;
                                owl:maxQualifiedCardinality "1"^^xsd:nonNegativeInteger ;
                                owl:onDataRange xsd:nonNegativeInteger
                              ] ;
              rdfs:comment "An electrical connection point (AC or DC) to a piece of conducting equipment. Terminals are connected at physical connection points called connectivity nodes." .


###  https://w3id.org/netbeheer/IECCIM/TC57CIM/IEC61970/Base/Core#BaseFrequency
:BaseFrequency rdf:type owl:Class ;
               rdfs:subClassOf :IdentifiedObject ,
                               [ rdf:type owl:Restriction ;
                                 owl:onProperty :BaseFrequency_frequency ;
                                 owl:minQualifiedCardinality "0"^^xsd:nonNegativeInteger ;
                                 owl:onClass <https://w3id.org/netbeheer/IECCIM/TC57CIM/IEC61970/Base/Domain#Frequency>
                               ] ,
                               [ rdf:type owl:Restriction ;
                                 owl:onProperty :BaseFrequency_frequency ;
                                 owl:maxQualifiedCardinality "1"^^xsd:nonNegativeInteger ;
                                 owl:onClass <https://w3id.org/netbeheer/IECCIM/TC57CIM/IEC61970/Base/Domain#Frequency>
                               ] ;
               rdfs:comment "The class describe a base frequency for a power system network. In case of multiple power networks with different frequencies, e.g. 50 or 60 Hertz each network will have it's own base frequency class. Hence it is assumed that power system objects having different base frequencies appear in separate documents where each document has a single base frequency instance." .


###  https://w3id.org/netbeheer/IECCIM/TC57CIM/IEC61970/Base/Core#BasePower
:BasePower rdf:type owl:Class ;
           rdfs:subClassOf :IdentifiedObject ,
                           [ rdf:type owl:Restriction ;
                             owl:onProperty :BasePower_basePower ;
                             owl:minQualifiedCardinality "0"^^xsd:nonNegativeInteger ;
                             owl:onClass <https://w3id.org/netbeheer/IECCIM/TC57CIM/IEC61970/Base/Domain#ApparentPower>
                           ] ,
                           [ rdf:type owl:Restriction ;
                             owl:onProperty :BasePower_basePower ;
                             owl:maxQualifiedCardinality "1"^^xsd:nonNegativeInteger ;
                             owl:onClass <https://w3id.org/netbeheer/IECCIM/TC57CIM/IEC61970/Base/Domain#ApparentPower>
                           ] ;
           rdfs:comment "The BasePower class defines the base power used in the per unit calculations." .


###  https://w3id.org/netbeheer/IECCIM/TC57CIM/IEC61970/Base/Core#BaseVoltage
:BaseVoltage rdf:type owl:Class ;
             rdfs:subClassOf :IdentifiedObject ,
                             [ rdf:type owl:Restriction ;
                               owl:onProperty :BaseVoltage_ConductingEquipment ;
                               owl:minQualifiedCardinality "0"^^xsd:nonNegativeInteger ;
                               owl:onClass :BaseVoltage
                             ] ,
                             [ rdf:type owl:Restriction ;
                               owl:onProperty :BaseVoltage_TopologicalNode ;
                               owl:minQualifiedCardinality "0"^^xsd:nonNegativeInteger ;
                               owl:onClass :BaseVoltage
                             ] ,
                             [ rdf:type owl:Restriction ;
                               owl:onProperty :BaseVoltage_TransformerEnds ;
                               owl:minQualifiedCardinality "0"^^xsd:nonNegativeInteger ;
                               owl:onClass :BaseVoltage
                             ] ,
                             [ rdf:type owl:Restriction ;
                               owl:onProperty :BaseVoltage_nominalVoltage ;
                               owl:minQualifiedCardinality "0"^^xsd:nonNegativeInteger ;
                               owl:onClass <https://w3id.org/netbeheer/IECCIM/TC57CIM/IEC61970/Base/Domain#Voltage>
                             ] ,
                             [ rdf:type owl:Restriction ;
                               owl:onProperty :BaseVoltage_VoltageLevel ;
                               owl:qualifiedCardinality "1"^^xsd:nonNegativeInteger ;
                               owl:onClass :BaseVoltage
                             ] ,
                             [ rdf:type owl:Restriction ;
                               owl:onProperty :BaseVoltage_ConductingEquipment ;
                               owl:maxQualifiedCardinality "1"^^xsd:nonNegativeInteger ;
                               owl:onClass :BaseVoltage
                             ] ,
                             [ rdf:type owl:Restriction ;
                               owl:onProperty :BaseVoltage_TopologicalNode ;
                               owl:maxQualifiedCardinality "1"^^xsd:nonNegativeInteger ;
                               owl:onClass :BaseVoltage
                             ] ,
                             [ rdf:type owl:Restriction ;
                               owl:onProperty :BaseVoltage_TransformerEnds ;
                               owl:maxQualifiedCardinality "1"^^xsd:nonNegativeInteger ;
                               owl:onClass :BaseVoltage
                             ] ,
                             [ rdf:type owl:Restriction ;
                               owl:onProperty :BaseVoltage_nominalVoltage ;
                               owl:maxQualifiedCardinality "1"^^xsd:nonNegativeInteger ;
                               owl:onClass <https://w3id.org/netbeheer/IECCIM/TC57CIM/IEC61970/Base/Domain#Voltage>
                             ] ;
             rdfs:comment "Defines a system base voltage which is referenced. " .


###  https://w3id.org/netbeheer/IECCIM/TC57CIM/IEC61970/Base/Core#BasicIntervalSchedule
:BasicIntervalSchedule rdf:type owl:Class ;
                       rdfs:subClassOf :IdentifiedObject ,
                                       [ rdf:type owl:Restriction ;
                                         owl:onProperty :BasicIntervalSchedule_startTime ;
                                         owl:minQualifiedCardinality "0"^^xsd:nonNegativeInteger ;
                                         owl:onDataRange xsd:dateTime
                                       ] ,
                                       [ rdf:type owl:Restriction ;
                                         owl:onProperty :BasicIntervalSchedule_value1Multiplier ;
                                         owl:minQualifiedCardinality "0"^^xsd:nonNegativeInteger ;
                                         owl:onDataRange <https://w3id.org/netbeheer/IECCIM/TC57CIM/IEC61970/Base/Domain#UnitMultiplier>
                                       ] ,
                                       [ rdf:type owl:Restriction ;
                                         owl:onProperty :BasicIntervalSchedule_value1Unit ;
                                         owl:minQualifiedCardinality "0"^^xsd:nonNegativeInteger ;
                                         owl:onDataRange <https://w3id.org/netbeheer/IECCIM/TC57CIM/IEC61970/Base/Domain#UnitSymbol>
                                       ] ,
                                       [ rdf:type owl:Restriction ;
                                         owl:onProperty :BasicIntervalSchedule_value2Multiplier ;
                                         owl:minQualifiedCardinality "0"^^xsd:nonNegativeInteger ;
                                         owl:onDataRange <https://w3id.org/netbeheer/IECCIM/TC57CIM/IEC61970/Base/Domain#UnitMultiplier>
                                       ] ,
                                       [ rdf:type owl:Restriction ;
                                         owl:onProperty :BasicIntervalSchedule_value2Unit ;
                                         owl:minQualifiedCardinality "0"^^xsd:nonNegativeInteger ;
                                         owl:onDataRange <https://w3id.org/netbeheer/IECCIM/TC57CIM/IEC61970/Base/Domain#UnitSymbol>
                                       ] ,
                                       [ rdf:type owl:Restriction ;
                                         owl:onProperty :BasicIntervalSchedule_startTime ;
                                         owl:maxQualifiedCardinality "1"^^xsd:nonNegativeInteger ;
                                         owl:onDataRange xsd:dateTime
                                       ] ,
                                       [ rdf:type owl:Restriction ;
                                         owl:onProperty :BasicIntervalSchedule_value1Multiplier ;
                                         owl:maxQualifiedCardinality "1"^^xsd:nonNegativeInteger ;
                                         owl:onDataRange <https://w3id.org/netbeheer/IECCIM/TC57CIM/IEC61970/Base/Domain#UnitMultiplier>
                                       ] ,
                                       [ rdf:type owl:Restriction ;
                                         owl:onProperty :BasicIntervalSchedule_value1Unit ;
                                         owl:maxQualifiedCardinality "1"^^xsd:nonNegativeInteger ;
                                         owl:onDataRange <https://w3id.org/netbeheer/IECCIM/TC57CIM/IEC61970/Base/Domain#UnitSymbol>
                                       ] ,
                                       [ rdf:type owl:Restriction ;
                                         owl:onProperty :BasicIntervalSchedule_value2Multiplier ;
                                         owl:maxQualifiedCardinality "1"^^xsd:nonNegativeInteger ;
                                         owl:onDataRange <https://w3id.org/netbeheer/IECCIM/TC57CIM/IEC61970/Base/Domain#UnitMultiplier>
                                       ] ,
                                       [ rdf:type owl:Restriction ;
                                         owl:onProperty :BasicIntervalSchedule_value2Unit ;
                                         owl:maxQualifiedCardinality "1"^^xsd:nonNegativeInteger ;
                                         owl:onDataRange <https://w3id.org/netbeheer/IECCIM/TC57CIM/IEC61970/Base/Domain#UnitSymbol>
                                       ] ;
                       rdfs:comment "Schedule of values at points in time." .


###  https://w3id.org/netbeheer/IECCIM/TC57CIM/IEC61970/Base/Core#Bay
:Bay rdf:type owl:Class ;
     rdfs:subClassOf :EquipmentContainer ,
                     [ rdf:type owl:Restriction ;
                       owl:onProperty :Bay_Substation ;
                       owl:minQualifiedCardinality "0"^^xsd:nonNegativeInteger ;
                       owl:onClass :Bay
                     ] ,
                     [ rdf:type owl:Restriction ;
                       owl:onProperty :Bay_VoltageLevel ;
                       owl:minQualifiedCardinality "0"^^xsd:nonNegativeInteger ;
                       owl:onClass :Bay
                     ] ,
                     [ rdf:type owl:Restriction ;
                       owl:onProperty :Bay_bayEnergyMeasFlag ;
                       owl:minQualifiedCardinality "0"^^xsd:nonNegativeInteger ;
                       owl:onDataRange xsd:boolean
                     ] ,
                     [ rdf:type owl:Restriction ;
                       owl:onProperty :Bay_bayPowerMeasFlag ;
                       owl:minQualifiedCardinality "0"^^xsd:nonNegativeInteger ;
                       owl:onDataRange xsd:boolean
                     ] ,
                     [ rdf:type owl:Restriction ;
                       owl:onProperty :Bay_breakerConfiguration ;
                       owl:minQualifiedCardinality "0"^^xsd:nonNegativeInteger ;
                       owl:onDataRange :BreakerConfiguration
                     ] ,
                     [ rdf:type owl:Restriction ;
                       owl:onProperty :Bay_busBarConfiguration ;
                       owl:minQualifiedCardinality "0"^^xsd:nonNegativeInteger ;
                       owl:onDataRange :BusbarConfiguration
                     ] ,
                     [ rdf:type owl:Restriction ;
                       owl:onProperty :Bay_bayEnergyMeasFlag ;
                       owl:maxQualifiedCardinality "1"^^xsd:nonNegativeInteger ;
                       owl:onDataRange xsd:boolean
                     ] ,
                     [ rdf:type owl:Restriction ;
                       owl:onProperty :Bay_bayPowerMeasFlag ;
                       owl:maxQualifiedCardinality "1"^^xsd:nonNegativeInteger ;
                       owl:onDataRange xsd:boolean
                     ] ,
                     [ rdf:type owl:Restriction ;
                       owl:onProperty :Bay_breakerConfiguration ;
                       owl:maxQualifiedCardinality "1"^^xsd:nonNegativeInteger ;
                       owl:onDataRange :BreakerConfiguration
                     ] ,
                     [ rdf:type owl:Restriction ;
                       owl:onProperty :Bay_busBarConfiguration ;
                       owl:maxQualifiedCardinality "1"^^xsd:nonNegativeInteger ;
                       owl:onDataRange :BusbarConfiguration
                     ] ;
     rdfs:comment """A collection of power system resources (within a given substation) including conducting equipment, protection relays, measurements, and telemetry.  A bay typically represents a physical grouping related to modularization of equipment.
""" .


###  https://w3id.org/netbeheer/IECCIM/TC57CIM/IEC61970/Base/Core#ConductingEquipment
:ConductingEquipment rdf:type owl:Class ;
                     rdfs:subClassOf :Equipment ,
                                     [ rdf:type owl:Restriction ;
                                       owl:onProperty :ConductingEquipment_BaseVoltage ;
                                       owl:minQualifiedCardinality "0"^^xsd:nonNegativeInteger ;
                                       owl:onClass :ConductingEquipment
                                     ] ,
                                     [ rdf:type owl:Restriction ;
                                       owl:onProperty :ConductingEquipment_GroundingAction ;
                                       owl:minQualifiedCardinality "0"^^xsd:nonNegativeInteger ;
                                       owl:onClass :ConductingEquipment
                                     ] ,
                                     [ rdf:type owl:Restriction ;
                                       owl:onProperty :ConductingEquipment_JumpingAction ;
                                       owl:minQualifiedCardinality "0"^^xsd:nonNegativeInteger ;
                                       owl:onClass :ConductingEquipment
                                     ] ,
                                     [ rdf:type owl:Restriction ;
                                       owl:onProperty :ConductingEquipment_ProtectionEquipments ;
                                       owl:minQualifiedCardinality "0"^^xsd:nonNegativeInteger ;
                                       owl:onClass :ConductingEquipment
                                     ] ,
                                     [ rdf:type owl:Restriction ;
                                       owl:onProperty :ConductingEquipment_ProtectiveActionAdjustment ;
                                       owl:qualifiedCardinality "1"^^xsd:nonNegativeInteger ;
                                       owl:onClass :ConductingEquipment
                                     ] ,
                                     [ rdf:type owl:Restriction ;
                                       owl:onProperty :ConductingEquipment_SvStatus ;
                                       owl:qualifiedCardinality "1"^^xsd:nonNegativeInteger ;
                                       owl:onClass :ConductingEquipment
                                     ] ,
                                     [ rdf:type owl:Restriction ;
                                       owl:onProperty :ConductingEquipment_Terminals ;
                                       owl:qualifiedCardinality "1"^^xsd:nonNegativeInteger ;
                                       owl:onClass :ConductingEquipment
                                     ] ,
                                     [ rdf:type owl:Restriction ;
                                       owl:onProperty :ConductingEquipment_GroundingAction ;
                                       owl:maxQualifiedCardinality "1"^^xsd:nonNegativeInteger ;
                                       owl:onClass :ConductingEquipment
                                     ] ;
                     rdfs:comment "The parts of the AC power system that are designed to carry current or that are conductively connected through terminals." .


###  https://w3id.org/netbeheer/IECCIM/TC57CIM/IEC61970/Base/Core#ConnectivityNode
:ConnectivityNode rdf:type owl:Class ;
                  rdfs:subClassOf :IdentifiedObject ,
                                  [ rdf:type owl:Restriction ;
                                    owl:onProperty :ConnectivityNode_ConnectivityNodeContainer ;
                                    owl:minQualifiedCardinality "0"^^xsd:nonNegativeInteger ;
                                    owl:onClass :ConnectivityNode
                                  ] ,
                                  [ rdf:type owl:Restriction ;
                                    owl:onProperty :ConnectivityNode_Terminals ;
                                    owl:minQualifiedCardinality "0"^^xsd:nonNegativeInteger ;
                                    owl:onClass :ConnectivityNode
                                  ] ,
                                  [ rdf:type owl:Restriction ;
                                    owl:onProperty :ConnectivityNode_TopologicalNode ;
                                    owl:minQualifiedCardinality "0"^^xsd:nonNegativeInteger ;
                                    owl:onClass :ConnectivityNode
                                  ] ,
                                  [ rdf:type owl:Restriction ;
                                    owl:onProperty :ConnectivityNode_Terminals ;
                                    owl:maxQualifiedCardinality "1"^^xsd:nonNegativeInteger ;
                                    owl:onClass :ConnectivityNode
                                  ] ;
                  rdfs:comment "Connectivity nodes are points where terminals of AC conducting equipment are connected together with zero impedance." .


###  https://w3id.org/netbeheer/IECCIM/TC57CIM/IEC61970/Base/Core#ConnectivityNodeContainer
:ConnectivityNodeContainer rdf:type owl:Class ;
                           rdfs:subClassOf :PowerSystemResource ,
                                           [ rdf:type owl:Restriction ;
                                             owl:onProperty :ConnectivityNodeContainer_TopologicalNode ;
                                             owl:minQualifiedCardinality "0"^^xsd:nonNegativeInteger ;
                                             owl:onClass :ConnectivityNodeContainer
                                           ] ,
                                           [ rdf:type owl:Restriction ;
                                             owl:onProperty :ConnectivityNodeContainer_ConnectivityNodes ;
                                             owl:qualifiedCardinality "1"^^xsd:nonNegativeInteger ;
                                             owl:onClass :ConnectivityNodeContainer
                                           ] ,
                                           [ rdf:type owl:Restriction ;
                                             owl:onProperty :ConnectivityNodeContainer_TopologicalNode ;
                                             owl:maxQualifiedCardinality "1"^^xsd:nonNegativeInteger ;
                                             owl:onClass :ConnectivityNodeContainer
                                           ] ;
                           rdfs:comment """A base class for all objects that may contain connectivity nodes or topological nodes.
""" .


###  https://w3id.org/netbeheer/IECCIM/TC57CIM/IEC61970/Base/Core#Curve
:Curve rdf:type owl:Class ;
       rdfs:subClassOf :IdentifiedObject ,
                       [ rdf:type owl:Restriction ;
                         owl:onProperty :Curve_CurveDatas ;
                         owl:qualifiedCardinality "1"^^xsd:nonNegativeInteger ;
                         owl:onClass :Curve
                       ] ,
                       [ rdf:type owl:Restriction ;
                         owl:onProperty :Curve_curveStyle ;
                         owl:minQualifiedCardinality "0"^^xsd:nonNegativeInteger ;
                         owl:onDataRange :CurveStyle
                       ] ,
                       [ rdf:type owl:Restriction ;
                         owl:onProperty :Curve_xMultiplier ;
                         owl:minQualifiedCardinality "0"^^xsd:nonNegativeInteger ;
                         owl:onDataRange <https://w3id.org/netbeheer/IECCIM/TC57CIM/IEC61970/Base/Domain#UnitMultiplier>
                       ] ,
                       [ rdf:type owl:Restriction ;
                         owl:onProperty :Curve_xUnit ;
                         owl:minQualifiedCardinality "0"^^xsd:nonNegativeInteger ;
                         owl:onDataRange <https://w3id.org/netbeheer/IECCIM/TC57CIM/IEC61970/Base/Domain#UnitSymbol>
                       ] ,
                       [ rdf:type owl:Restriction ;
                         owl:onProperty :Curve_y1Multiplier ;
                         owl:minQualifiedCardinality "0"^^xsd:nonNegativeInteger ;
                         owl:onDataRange <https://w3id.org/netbeheer/IECCIM/TC57CIM/IEC61970/Base/Domain#UnitMultiplier>
                       ] ,
                       [ rdf:type owl:Restriction ;
                         owl:onProperty :Curve_y1Unit ;
                         owl:minQualifiedCardinality "0"^^xsd:nonNegativeInteger ;
                         owl:onDataRange <https://w3id.org/netbeheer/IECCIM/TC57CIM/IEC61970/Base/Domain#UnitSymbol>
                       ] ,
                       [ rdf:type owl:Restriction ;
                         owl:onProperty :Curve_y2Multiplier ;
                         owl:minQualifiedCardinality "0"^^xsd:nonNegativeInteger ;
                         owl:onDataRange <https://w3id.org/netbeheer/IECCIM/TC57CIM/IEC61970/Base/Domain#UnitMultiplier>
                       ] ,
                       [ rdf:type owl:Restriction ;
                         owl:onProperty :Curve_y2Unit ;
                         owl:minQualifiedCardinality "0"^^xsd:nonNegativeInteger ;
                         owl:onDataRange <https://w3id.org/netbeheer/IECCIM/TC57CIM/IEC61970/Base/Domain#UnitSymbol>
                       ] ,
                       [ rdf:type owl:Restriction ;
                         owl:onProperty :Curve_y3Multiplier ;
                         owl:minQualifiedCardinality "0"^^xsd:nonNegativeInteger ;
                         owl:onDataRange <https://w3id.org/netbeheer/IECCIM/TC57CIM/IEC61970/Base/Domain#UnitMultiplier>
                       ] ,
                       [ rdf:type owl:Restriction ;
                         owl:onProperty :Curve_y3Unit ;
                         owl:minQualifiedCardinality "0"^^xsd:nonNegativeInteger ;
                         owl:onDataRange <https://w3id.org/netbeheer/IECCIM/TC57CIM/IEC61970/Base/Domain#UnitSymbol>
                       ] ,
                       [ rdf:type owl:Restriction ;
                         owl:onProperty :Curve_curveStyle ;
                         owl:maxQualifiedCardinality "1"^^xsd:nonNegativeInteger ;
                         owl:onDataRange :CurveStyle
                       ] ,
                       [ rdf:type owl:Restriction ;
                         owl:onProperty :Curve_xMultiplier ;
                         owl:maxQualifiedCardinality "1"^^xsd:nonNegativeInteger ;
                         owl:onDataRange <https://w3id.org/netbeheer/IECCIM/TC57CIM/IEC61970/Base/Domain#UnitMultiplier>
                       ] ,
                       [ rdf:type owl:Restriction ;
                         owl:onProperty :Curve_xUnit ;
                         owl:maxQualifiedCardinality "1"^^xsd:nonNegativeInteger ;
                         owl:onDataRange <https://w3id.org/netbeheer/IECCIM/TC57CIM/IEC61970/Base/Domain#UnitSymbol>
                       ] ,
                       [ rdf:type owl:Restriction ;
                         owl:onProperty :Curve_y1Multiplier ;
                         owl:maxQualifiedCardinality "1"^^xsd:nonNegativeInteger ;
                         owl:onDataRange <https://w3id.org/netbeheer/IECCIM/TC57CIM/IEC61970/Base/Domain#UnitMultiplier>
                       ] ,
                       [ rdf:type owl:Restriction ;
                         owl:onProperty :Curve_y1Unit ;
                         owl:maxQualifiedCardinality "1"^^xsd:nonNegativeInteger ;
                         owl:onDataRange <https://w3id.org/netbeheer/IECCIM/TC57CIM/IEC61970/Base/Domain#UnitSymbol>
                       ] ,
                       [ rdf:type owl:Restriction ;
                         owl:onProperty :Curve_y2Multiplier ;
                         owl:maxQualifiedCardinality "1"^^xsd:nonNegativeInteger ;
                         owl:onDataRange <https://w3id.org/netbeheer/IECCIM/TC57CIM/IEC61970/Base/Domain#UnitMultiplier>
                       ] ,
                       [ rdf:type owl:Restriction ;
                         owl:onProperty :Curve_y2Unit ;
                         owl:maxQualifiedCardinality "1"^^xsd:nonNegativeInteger ;
                         owl:onDataRange <https://w3id.org/netbeheer/IECCIM/TC57CIM/IEC61970/Base/Domain#UnitSymbol>
                       ] ,
                       [ rdf:type owl:Restriction ;
                         owl:onProperty :Curve_y3Multiplier ;
                         owl:maxQualifiedCardinality "1"^^xsd:nonNegativeInteger ;
                         owl:onDataRange <https://w3id.org/netbeheer/IECCIM/TC57CIM/IEC61970/Base/Domain#UnitMultiplier>
                       ] ,
                       [ rdf:type owl:Restriction ;
                         owl:onProperty :Curve_y3Unit ;
                         owl:maxQualifiedCardinality "1"^^xsd:nonNegativeInteger ;
                         owl:onDataRange <https://w3id.org/netbeheer/IECCIM/TC57CIM/IEC61970/Base/Domain#UnitSymbol>
                       ] ;
       rdfs:comment """A multi-purpose curve or functional relationship between an independent variable (X-axis) and dependent (Y-axis) variables. 
""" .


###  https://w3id.org/netbeheer/IECCIM/TC57CIM/IEC61970/Base/Core#CurveData
:CurveData rdf:type owl:Class ;
           rdfs:subClassOf [ rdf:type owl:Restriction ;
                             owl:onProperty :CurveData_Curve ;
                             owl:minQualifiedCardinality "0"^^xsd:nonNegativeInteger ;
                             owl:onClass :CurveData
                           ] ,
                           [ rdf:type owl:Restriction ;
                             owl:onProperty :CurveData_xvalue ;
                             owl:minQualifiedCardinality "0"^^xsd:nonNegativeInteger ;
                             owl:onDataRange xsd:float
                           ] ,
                           [ rdf:type owl:Restriction ;
                             owl:onProperty :CurveData_y1value ;
                             owl:minQualifiedCardinality "0"^^xsd:nonNegativeInteger ;
                             owl:onDataRange xsd:float
                           ] ,
                           [ rdf:type owl:Restriction ;
                             owl:onProperty :CurveData_y2value ;
                             owl:minQualifiedCardinality "0"^^xsd:nonNegativeInteger ;
                             owl:onDataRange xsd:float
                           ] ,
                           [ rdf:type owl:Restriction ;
                             owl:onProperty :CurveData_y3value ;
                             owl:minQualifiedCardinality "0"^^xsd:nonNegativeInteger ;
                             owl:onDataRange xsd:float
                           ] ,
                           [ rdf:type owl:Restriction ;
                             owl:onProperty :CurveData_xvalue ;
                             owl:maxQualifiedCardinality "1"^^xsd:nonNegativeInteger ;
                             owl:onDataRange xsd:float
                           ] ,
                           [ rdf:type owl:Restriction ;
                             owl:onProperty :CurveData_y1value ;
                             owl:maxQualifiedCardinality "1"^^xsd:nonNegativeInteger ;
                             owl:onDataRange xsd:float
                           ] ,
                           [ rdf:type owl:Restriction ;
                             owl:onProperty :CurveData_y2value ;
                             owl:maxQualifiedCardinality "1"^^xsd:nonNegativeInteger ;
                             owl:onDataRange xsd:float
                           ] ,
                           [ rdf:type owl:Restriction ;
                             owl:onProperty :CurveData_y3value ;
                             owl:maxQualifiedCardinality "1"^^xsd:nonNegativeInteger ;
                             owl:onDataRange xsd:float
                           ] ;
           rdfs:comment """Multi-purpose data points for defining a curve.  The use of this generic class is discouraged if a more specific class  can be used to specify the x and y axis values along with their specific data types.
""" .


###  https://w3id.org/netbeheer/IECCIM/TC57CIM/IEC61970/Base/Core#Equipment
:Equipment rdf:type owl:Class ;
           rdfs:subClassOf :PowerSystemResource ,
                           [ rdf:type owl:Restriction ;
                             owl:onProperty :Equipment_EquipmentContainer ;
                             owl:minQualifiedCardinality "0"^^xsd:nonNegativeInteger ;
                             owl:onClass :Equipment
                           ] ,
                           [ rdf:type owl:Restriction ;
                             owl:onProperty :Equipment_LimitDependencyModel ;
                             owl:minQualifiedCardinality "0"^^xsd:nonNegativeInteger ;
                             owl:onClass :Equipment
                           ] ,
                           [ rdf:type owl:Restriction ;
                             owl:onProperty :Equipment_OperationalLimitSet ;
                             owl:minQualifiedCardinality "0"^^xsd:nonNegativeInteger ;
                             owl:onClass :Equipment
                           ] ,
                           [ rdf:type owl:Restriction ;
                             owl:onProperty :Equipment_OperationalRestrictions ;
                             owl:minQualifiedCardinality "0"^^xsd:nonNegativeInteger ;
                             owl:onClass :Equipment
                           ] ,
                           [ rdf:type owl:Restriction ;
                             owl:onProperty :Equipment_Outages ;
                             owl:minQualifiedCardinality "0"^^xsd:nonNegativeInteger ;
                             owl:onClass :Equipment
                           ] ,
                           [ rdf:type owl:Restriction ;
                             owl:onProperty :Equipment_UsagePoints ;
                             owl:minQualifiedCardinality "0"^^xsd:nonNegativeInteger ;
                             owl:onClass :Equipment
                           ] ,
                           [ rdf:type owl:Restriction ;
                             owl:onProperty :Equipment_WeatherStation ;
                             owl:minQualifiedCardinality "0"^^xsd:nonNegativeInteger ;
                             owl:onClass :Equipment
                           ] ,
                           [ rdf:type owl:Restriction ;
                             owl:onProperty :Equipment_ContingencyEquipment ;
                             owl:qualifiedCardinality "1"^^xsd:nonNegativeInteger ;
                             owl:onClass :Equipment
                           ] ,
                           [ rdf:type owl:Restriction ;
                             owl:onProperty :Equipment_EqiupmentLimitSeriesComponent ;
                             owl:qualifiedCardinality "1"^^xsd:nonNegativeInteger ;
                             owl:onClass :Equipment
                           ] ,
                           [ rdf:type owl:Restriction ;
                             owl:onProperty :Equipment_PinEquipment ;
                             owl:qualifiedCardinality "1"^^xsd:nonNegativeInteger ;
                             owl:onClass :Equipment
                           ] ,
                           [ rdf:type owl:Restriction ;
                             owl:onProperty :Equipment_ProtectiveActionEquipment ;
                             owl:qualifiedCardinality "1"^^xsd:nonNegativeInteger ;
                             owl:onClass :Equipment
                           ] ,
                           [ rdf:type owl:Restriction ;
                             owl:onProperty :Equipment_LimitDependencyModel ;
                             owl:maxQualifiedCardinality "1"^^xsd:nonNegativeInteger ;
                             owl:onClass :Equipment
                           ] ,
                           [ rdf:type owl:Restriction ;
                             owl:onProperty :Equipment_OperationalLimitSet ;
                             owl:maxQualifiedCardinality "1"^^xsd:nonNegativeInteger ;
                             owl:onClass :Equipment
                           ] ,
                           [ rdf:type owl:Restriction ;
                             owl:onProperty :Equipment_aggregate ;
                             owl:minQualifiedCardinality "0"^^xsd:nonNegativeInteger ;
                             owl:onDataRange xsd:boolean
                           ] ,
                           [ rdf:type owl:Restriction ;
                             owl:onProperty :Equipment_inService ;
                             owl:minQualifiedCardinality "0"^^xsd:nonNegativeInteger ;
                             owl:onDataRange xsd:boolean
                           ] ,
                           [ rdf:type owl:Restriction ;
                             owl:onProperty :Equipment_normallyInService ;
                             owl:minQualifiedCardinality "0"^^xsd:nonNegativeInteger ;
                             owl:onDataRange xsd:boolean
                           ] ,
                           [ rdf:type owl:Restriction ;
                             owl:onProperty :Equipment_aggregate ;
                             owl:maxQualifiedCardinality "1"^^xsd:nonNegativeInteger ;
                             owl:onDataRange xsd:boolean
                           ] ,
                           [ rdf:type owl:Restriction ;
                             owl:onProperty :Equipment_inService ;
                             owl:maxQualifiedCardinality "1"^^xsd:nonNegativeInteger ;
                             owl:onDataRange xsd:boolean
                           ] ,
                           [ rdf:type owl:Restriction ;
                             owl:onProperty :Equipment_normallyInService ;
                             owl:maxQualifiedCardinality "1"^^xsd:nonNegativeInteger ;
                             owl:onDataRange xsd:boolean
                           ] ;
           rdfs:comment "The parts of a power system that are physical devices, electronic or mechanical." .


###  https://w3id.org/netbeheer/IECCIM/TC57CIM/IEC61970/Base/Core#EquipmentContainer
:EquipmentContainer rdf:type owl:Class ;
                    rdfs:subClassOf :ConnectivityNodeContainer ,
                                    [ rdf:type owl:Restriction ;
                                      owl:onProperty :EquipmentContainer_Equipments ;
                                      owl:minQualifiedCardinality "0"^^xsd:nonNegativeInteger ;
                                      owl:onClass :EquipmentContainer
                                    ] ,
                                    [ rdf:type owl:Restriction ;
                                      owl:onProperty :EquipmentContainer_Equipments ;
                                      owl:maxQualifiedCardinality "1"^^xsd:nonNegativeInteger ;
                                      owl:onClass :EquipmentContainer
                                    ] ;
                    rdfs:comment "A modeling construct to provide a root class for containing equipment. " .


###  https://w3id.org/netbeheer/IECCIM/TC57CIM/IEC61970/Base/Core#GeographicalRegion
:GeographicalRegion rdf:type owl:Class ;
                    rdfs:subClassOf :IdentifiedObject ,
                                    [ rdf:type owl:Restriction ;
                                      owl:onProperty :GeographicalRegion_Regions ;
                                      owl:minQualifiedCardinality "0"^^xsd:nonNegativeInteger ;
                                      owl:onClass :GeographicalRegion
                                    ] ,
                                    [ rdf:type owl:Restriction ;
                                      owl:onProperty :GeographicalRegion_Regions ;
                                      owl:maxQualifiedCardinality "1"^^xsd:nonNegativeInteger ;
                                      owl:onClass :GeographicalRegion
                                    ] ;
                    rdfs:comment """A geographical region of a power system network model.
""" .


###  https://w3id.org/netbeheer/IECCIM/TC57CIM/IEC61970/Base/Core#IdentifiedObject
:IdentifiedObject rdf:type owl:Class ;
                  rdfs:subClassOf [ rdf:type owl:Restriction ;
                                    owl:onProperty :IdentifiedObject_DiagramObjects ;
                                    owl:minQualifiedCardinality "0"^^xsd:nonNegativeInteger ;
                                    owl:onClass :IdentifiedObject
                                  ] ,
                                  [ rdf:type owl:Restriction ;
                                    owl:onProperty :IdentifiedObject_PropertiesCIMDataObject ;
                                    owl:minQualifiedCardinality "0"^^xsd:nonNegativeInteger ;
                                    owl:onClass :IdentifiedObject
                                  ] ,
                                  [ rdf:type owl:Restriction ;
                                    owl:onProperty :IdentifiedObject_Names ;
                                    owl:qualifiedCardinality "1"^^xsd:nonNegativeInteger ;
                                    owl:onClass :IdentifiedObject
                                  ] ,
                                  [ rdf:type owl:Restriction ;
                                    owl:onProperty :IdentifiedObject_RegisteredCIMDataObject ;
                                    owl:qualifiedCardinality "1"^^xsd:nonNegativeInteger ;
                                    owl:onClass :IdentifiedObject
                                  ] ,
                                  [ rdf:type owl:Restriction ;
                                    owl:onProperty :IdentifiedObject_DiagramObjects ;
                                    owl:maxQualifiedCardinality "1"^^xsd:nonNegativeInteger ;
                                    owl:onClass :IdentifiedObject
                                  ] ,
                                  [ rdf:type owl:Restriction ;
                                    owl:onProperty :IdentifiedObject_PropertiesCIMDataObject ;
                                    owl:maxQualifiedCardinality "1"^^xsd:nonNegativeInteger ;
                                    owl:onClass :IdentifiedObject
                                  ] ,
                                  [ rdf:type owl:Restriction ;
                                    owl:onProperty :IdentifiedObject_aliasName ;
                                    owl:minQualifiedCardinality "0"^^xsd:nonNegativeInteger ;
                                    owl:onDataRange xsd:string
                                  ] ,
                                  [ rdf:type owl:Restriction ;
                                    owl:onProperty :IdentifiedObject_description ;
                                    owl:minQualifiedCardinality "0"^^xsd:nonNegativeInteger ;
                                    owl:onDataRange xsd:string
                                  ] ,
                                  [ rdf:type owl:Restriction ;
                                    owl:onProperty :IdentifiedObject_mRID ;
                                    owl:minQualifiedCardinality "0"^^xsd:nonNegativeInteger ;
                                    owl:onDataRange xsd:string
                                  ] ,
                                  [ rdf:type owl:Restriction ;
                                    owl:onProperty :IdentifiedObject_name ;
                                    owl:minQualifiedCardinality "0"^^xsd:nonNegativeInteger ;
                                    owl:onDataRange xsd:string
                                  ] ,
                                  [ rdf:type owl:Restriction ;
                                    owl:onProperty :IdentifiedObject_aliasName ;
                                    owl:maxQualifiedCardinality "1"^^xsd:nonNegativeInteger ;
                                    owl:onDataRange xsd:string
                                  ] ,
                                  [ rdf:type owl:Restriction ;
                                    owl:onProperty :IdentifiedObject_description ;
                                    owl:maxQualifiedCardinality "1"^^xsd:nonNegativeInteger ;
                                    owl:onDataRange xsd:string
                                  ] ,
                                  [ rdf:type owl:Restriction ;
                                    owl:onProperty :IdentifiedObject_mRID ;
                                    owl:maxQualifiedCardinality "1"^^xsd:nonNegativeInteger ;
                                    owl:onDataRange xsd:string
                                  ] ,
                                  [ rdf:type owl:Restriction ;
                                    owl:onProperty :IdentifiedObject_name ;
                                    owl:maxQualifiedCardinality "1"^^xsd:nonNegativeInteger ;
                                    owl:onDataRange xsd:string
                                  ] ;
                  rdfs:comment "This is a root class to provide common identification for all classes needing identification and naming attributes." .


###  https://w3id.org/netbeheer/IECCIM/TC57CIM/IEC61970/Base/Core#IrregularIntervalSchedule
:IrregularIntervalSchedule rdf:type owl:Class ;
                           rdfs:subClassOf :BasicIntervalSchedule ,
                                           [ rdf:type owl:Restriction ;
                                             owl:onProperty :IrregularIntervalSchedule_TimePoints ;
                                             owl:qualifiedCardinality "1"^^xsd:nonNegativeInteger ;
                                             owl:onClass :IrregularIntervalSchedule
                                           ] ;
                           rdfs:comment """The schedule has time points where the time between them varies.
""" .


###  https://w3id.org/netbeheer/IECCIM/TC57CIM/IEC61970/Base/Core#IrregularTimePoint
:IrregularTimePoint rdf:type owl:Class ;
                    rdfs:subClassOf [ rdf:type owl:Restriction ;
                                      owl:onProperty :IrregularTimePoint_IntervalSchedule ;
                                      owl:minQualifiedCardinality "1"^^xsd:nonNegativeInteger ;
                                      owl:onClass :IrregularTimePoint
                                    ] ,
                                    [ rdf:type owl:Restriction ;
                                      owl:onProperty :IrregularTimePoint_time ;
                                      owl:minQualifiedCardinality "0"^^xsd:nonNegativeInteger ;
                                      owl:onClass <https://w3id.org/netbeheer/IECCIM/TC57CIM/IEC61970/Base/Domain#Seconds>
                                    ] ,
                                    [ rdf:type owl:Restriction ;
                                      owl:onProperty :IrregularTimePoint_time ;
                                      owl:maxQualifiedCardinality "1"^^xsd:nonNegativeInteger ;
                                      owl:onClass <https://w3id.org/netbeheer/IECCIM/TC57CIM/IEC61970/Base/Domain#Seconds>
                                    ] ,
                                    [ rdf:type owl:Restriction ;
                                      owl:onProperty :IrregularTimePoint_value1 ;
                                      owl:minQualifiedCardinality "0"^^xsd:nonNegativeInteger ;
                                      owl:onDataRange xsd:float
                                    ] ,
                                    [ rdf:type owl:Restriction ;
                                      owl:onProperty :IrregularTimePoint_value2 ;
                                      owl:minQualifiedCardinality "0"^^xsd:nonNegativeInteger ;
                                      owl:onDataRange xsd:float
                                    ] ,
                                    [ rdf:type owl:Restriction ;
                                      owl:onProperty :IrregularTimePoint_value1 ;
                                      owl:maxQualifiedCardinality "1"^^xsd:nonNegativeInteger ;
                                      owl:onDataRange xsd:float
                                    ] ,
                                    [ rdf:type owl:Restriction ;
                                      owl:onProperty :IrregularTimePoint_value2 ;
                                      owl:maxQualifiedCardinality "1"^^xsd:nonNegativeInteger ;
                                      owl:onDataRange xsd:float
                                    ] ;
                    rdfs:comment """TimePoints for a schedule where the time between the points varies.
""" .


###  https://w3id.org/netbeheer/IECCIM/TC57CIM/IEC61970/Base/Core#Name
:Name rdf:type owl:Class ;
      rdfs:subClassOf [ rdf:type owl:Restriction ;
                        owl:onProperty :Name_IdentifiedObject ;
                        owl:minQualifiedCardinality "0"^^xsd:nonNegativeInteger ;
                        owl:onClass :Name
                      ] ,
                      [ rdf:type owl:Restriction ;
                        owl:onProperty :Name_NameType ;
                        owl:minQualifiedCardinality "0"^^xsd:nonNegativeInteger ;
                        owl:onClass :Name
                      ] ,
                      [ rdf:type owl:Restriction ;
                        owl:onProperty :Name_name ;
                        owl:minQualifiedCardinality "0"^^xsd:nonNegativeInteger ;
                        owl:onDataRange xsd:string
                      ] ,
                      [ rdf:type owl:Restriction ;
                        owl:onProperty :Name_name ;
                        owl:maxQualifiedCardinality "1"^^xsd:nonNegativeInteger ;
                        owl:onDataRange xsd:string
                      ] ;
      rdfs:comment """The Name class provides the means to define any number of human readable  names for an object. A name is <b>not</b> to be used for defining inter-object relationships. For inter-object relationships instead use the object identification 'mRID'.
""" .


###  https://w3id.org/netbeheer/IECCIM/TC57CIM/IEC61970/Base/Core#NameType
:NameType rdf:type owl:Class ;
          rdfs:subClassOf [ rdf:type owl:Restriction ;
                            owl:onProperty :NameType_NameTypeAuthority ;
                            owl:minQualifiedCardinality "0"^^xsd:nonNegativeInteger ;
                            owl:onClass :NameType
                          ] ,
                          [ rdf:type owl:Restriction ;
                            owl:onProperty :NameType_Names ;
                            owl:qualifiedCardinality "1"^^xsd:nonNegativeInteger ;
                            owl:onClass :NameType
                          ] ,
                          [ rdf:type owl:Restriction ;
                            owl:onProperty :NameType_description ;
                            owl:minQualifiedCardinality "0"^^xsd:nonNegativeInteger ;
                            owl:onDataRange xsd:string
                          ] ,
                          [ rdf:type owl:Restriction ;
                            owl:onProperty :NameType_name ;
                            owl:minQualifiedCardinality "0"^^xsd:nonNegativeInteger ;
                            owl:onDataRange xsd:string
                          ] ,
                          [ rdf:type owl:Restriction ;
                            owl:onProperty :NameType_description ;
                            owl:maxQualifiedCardinality "1"^^xsd:nonNegativeInteger ;
                            owl:onDataRange xsd:string
                          ] ,
                          [ rdf:type owl:Restriction ;
                            owl:onProperty :NameType_name ;
                            owl:maxQualifiedCardinality "1"^^xsd:nonNegativeInteger ;
                            owl:onDataRange xsd:string
                          ] ;
          rdfs:comment """Type of name. Possible values for attribute 'name' are implementation dependent but standard profiles may specify types. An enterprise may have multiple IT systems each having its own local name for the same object, e.g. a planning system may have different names from an EMS. An object may also have different names within the same IT system, e.g. localName as defined in CIM version 14. The definition from CIM14 is:
The localName is a human readable name of the object. It is a free text name local to a node in a naming hierarchy similar to a file directory structure. A power system related naming hierarchy may be: Substation, VoltageLevel, Equipment etc. Children of the same parent in such a hierarchy have names that typically are unique among them.
""" .


###  https://w3id.org/netbeheer/IECCIM/TC57CIM/IEC61970/Base/Core#NameTypeAuthority
:NameTypeAuthority rdf:type owl:Class ;
                   rdfs:subClassOf [ rdf:type owl:Restriction ;
                                     owl:onProperty :NameTypeAuthority_NameTypes ;
                                     owl:minQualifiedCardinality "0"^^xsd:nonNegativeInteger ;
                                     owl:onClass :NameTypeAuthority
                                   ] ,
                                   [ rdf:type owl:Restriction ;
                                     owl:onProperty :NameTypeAuthority_NameTypes ;
                                     owl:maxQualifiedCardinality "1"^^xsd:nonNegativeInteger ;
                                     owl:onClass :NameTypeAuthority
                                   ] ,
                                   [ rdf:type owl:Restriction ;
                                     owl:onProperty :NameTypeAuthority_description ;
                                     owl:minQualifiedCardinality "0"^^xsd:nonNegativeInteger ;
                                     owl:onDataRange xsd:string
                                   ] ,
                                   [ rdf:type owl:Restriction ;
                                     owl:onProperty :NameTypeAuthority_name ;
                                     owl:minQualifiedCardinality "0"^^xsd:nonNegativeInteger ;
                                     owl:onDataRange xsd:string
                                   ] ,
                                   [ rdf:type owl:Restriction ;
                                     owl:onProperty :NameTypeAuthority_description ;
                                     owl:maxQualifiedCardinality "1"^^xsd:nonNegativeInteger ;
                                     owl:onDataRange xsd:string
                                   ] ,
                                   [ rdf:type owl:Restriction ;
                                     owl:onProperty :NameTypeAuthority_name ;
                                     owl:maxQualifiedCardinality "1"^^xsd:nonNegativeInteger ;
                                     owl:onDataRange xsd:string
                                   ] ;
                   rdfs:comment """Authority responsible for creation and management of names of a given type; typically an organization or an enterprise system.
""" .


###  https://w3id.org/netbeheer/IECCIM/TC57CIM/IEC61970/Base/Core#OperatingParticipant
:OperatingParticipant rdf:type owl:Class ;
                      rdfs:subClassOf :IdentifiedObject ,
                                      [ rdf:type owl:Restriction ;
                                        owl:onProperty :OperatingParticipant_OperatingShare ;
                                        owl:qualifiedCardinality "1"^^xsd:nonNegativeInteger ;
                                        owl:onClass :OperatingParticipant
                                      ] ;
                      rdfs:comment """An operator of multiple power system resource objects. Note multple operating participants may operate the same power system resource object.   This can be used for modeling jointly owned units where each owner operates as a contractual share.
""" .


###  https://w3id.org/netbeheer/IECCIM/TC57CIM/IEC61970/Base/Core#OperatingShare
:OperatingShare rdf:type owl:Class ;
                rdfs:subClassOf [ rdf:type owl:Restriction ;
                                  owl:onProperty :OperatingShare_OperatingParticipant ;
                                  owl:minQualifiedCardinality "0"^^xsd:nonNegativeInteger ;
                                  owl:onClass :OperatingShare
                                ] ,
                                [ rdf:type owl:Restriction ;
                                  owl:onProperty :OperatingShare_PowerSystemResource ;
                                  owl:minQualifiedCardinality "0"^^xsd:nonNegativeInteger ;
                                  owl:onClass :OperatingShare
                                ] ,
                                [ rdf:type owl:Restriction ;
                                  owl:onProperty :OperatingShare_percentage ;
                                  owl:minQualifiedCardinality "0"^^xsd:nonNegativeInteger ;
                                  owl:onClass <https://w3id.org/netbeheer/IECCIM/TC57CIM/IEC61970/Base/Domain#PerCent>
                                ] ,
                                [ rdf:type owl:Restriction ;
                                  owl:onProperty :OperatingShare_percentage ;
                                  owl:maxQualifiedCardinality "1"^^xsd:nonNegativeInteger ;
                                  owl:onClass <https://w3id.org/netbeheer/IECCIM/TC57CIM/IEC61970/Base/Domain#PerCent>
                                ] ;
                rdfs:comment """Specifies the operations contract relationship between a power system resource and a contract participant.
""" .


###  https://w3id.org/netbeheer/IECCIM/TC57CIM/IEC61970/Base/Core#PSRType
:PSRType rdf:type owl:Class ;
         rdfs:subClassOf :IdentifiedObject ,
                         [ rdf:type owl:Restriction ;
                           owl:onProperty :PSRType_PowerSystemResources ;
                           owl:minQualifiedCardinality "0"^^xsd:nonNegativeInteger ;
                           owl:onClass :PSRType
                         ] ,
                         [ rdf:type owl:Restriction ;
                           owl:onProperty :PSRType_PowerSystemResources ;
                           owl:maxQualifiedCardinality "1"^^xsd:nonNegativeInteger ;
                           owl:onClass :PSRType
                         ] ;
         rdfs:comment """Classifying instances of the same class, e.g. overhead and underground ACLineSegments. This classification mechanism is intended to provide flexibility outside the scope of this standard, i.e. provide customisation that is non standard.
""" .


###  https://w3id.org/netbeheer/IECCIM/TC57CIM/IEC61970/Base/Core#PowerSystemResource
:PowerSystemResource rdf:type owl:Class ;
                     rdfs:subClassOf :IdentifiedObject ,
                                     [ rdf:type owl:Restriction ;
                                       owl:onProperty :PowerSystemResource_AssetDatasheet ;
                                       owl:minQualifiedCardinality "0"^^xsd:nonNegativeInteger ;
                                       owl:onClass :PowerSystemResource
                                     ] ,
                                     [ rdf:type owl:Restriction ;
                                       owl:onProperty :PowerSystemResource_Assets ;
                                       owl:minQualifiedCardinality "0"^^xsd:nonNegativeInteger ;
                                       owl:onClass :PowerSystemResource
                                     ] ,
                                     [ rdf:type owl:Restriction ;
                                       owl:onProperty :PowerSystemResource_Clearances ;
                                       owl:minQualifiedCardinality "0"^^xsd:nonNegativeInteger ;
                                       owl:onClass :PowerSystemResource
                                     ] ,
                                     [ rdf:type owl:Restriction ;
                                       owl:onProperty :PowerSystemResource_Controls ;
                                       owl:minQualifiedCardinality "0"^^xsd:nonNegativeInteger ;
                                       owl:onClass :PowerSystemResource
                                     ] ,
                                     [ rdf:type owl:Restriction ;
                                       owl:onProperty :PowerSystemResource_Location ;
                                       owl:minQualifiedCardinality "0"^^xsd:nonNegativeInteger ;
                                       owl:onClass :PowerSystemResource
                                     ] ,
                                     [ rdf:type owl:Restriction ;
                                       owl:onProperty :PowerSystemResource_Measurements ;
                                       owl:minQualifiedCardinality "0"^^xsd:nonNegativeInteger ;
                                       owl:onClass :PowerSystemResource
                                     ] ,
                                     [ rdf:type owl:Restriction ;
                                       owl:onProperty :PowerSystemResource_OperationalTags ;
                                       owl:minQualifiedCardinality "0"^^xsd:nonNegativeInteger ;
                                       owl:onClass :PowerSystemResource
                                     ] ,
                                     [ rdf:type owl:Restriction ;
                                       owl:onProperty :PowerSystemResource_PSREvents ;
                                       owl:minQualifiedCardinality "0"^^xsd:nonNegativeInteger ;
                                       owl:onClass :PowerSystemResource
                                     ] ,
                                     [ rdf:type owl:Restriction ;
                                       owl:onProperty :PowerSystemResource_PSRType ;
                                       owl:minQualifiedCardinality "0"^^xsd:nonNegativeInteger ;
                                       owl:onClass :PowerSystemResource
                                     ] ,
                                     [ rdf:type owl:Restriction ;
                                       owl:onProperty :PowerSystemResource_ReportingGroup ;
                                       owl:minQualifiedCardinality "0"^^xsd:nonNegativeInteger ;
                                       owl:onClass :PowerSystemResource
                                     ] ,
                                     [ rdf:type owl:Restriction ;
                                       owl:onProperty :PowerSystemResource_OperatingShare ;
                                       owl:qualifiedCardinality "1"^^xsd:nonNegativeInteger ;
                                       owl:onClass :PowerSystemResource
                                     ] ,
                                     [ rdf:type owl:Restriction ;
                                       owl:onProperty :PowerSystemResource_Controls ;
                                       owl:maxQualifiedCardinality "1"^^xsd:nonNegativeInteger ;
                                       owl:onClass :PowerSystemResource
                                     ] ,
                                     [ rdf:type owl:Restriction ;
                                       owl:onProperty :PowerSystemResource_Measurements ;
                                       owl:maxQualifiedCardinality "1"^^xsd:nonNegativeInteger ;
                                       owl:onClass :PowerSystemResource
                                     ] ,
                                     [ rdf:type owl:Restriction ;
                                       owl:onProperty :PowerSystemResource_OperationalTags ;
                                       owl:maxQualifiedCardinality "1"^^xsd:nonNegativeInteger ;
                                       owl:onClass :PowerSystemResource
                                     ] ,
                                     [ rdf:type owl:Restriction ;
                                       owl:onProperty :PowerSystemResource_PSREvents ;
                                       owl:maxQualifiedCardinality "1"^^xsd:nonNegativeInteger ;
                                       owl:onClass :PowerSystemResource
                                     ] ;
                     rdfs:comment """A power system resource can be an item of equipment such as a switch, an equipment container containing many individual items of equipment such as a substation, or an organisational entity such as sub-control area. Power system resources can have measurements associated.
""" .


###  https://w3id.org/netbeheer/IECCIM/TC57CIM/IEC61970/Base/Core#RegularIntervalSchedule
:RegularIntervalSchedule rdf:type owl:Class ;
                         rdfs:subClassOf :BasicIntervalSchedule ,
                                         [ rdf:type owl:Restriction ;
                                           owl:onProperty :RegularIntervalSchedule_timeStep ;
                                           owl:minQualifiedCardinality "0"^^xsd:nonNegativeInteger ;
                                           owl:onClass <https://w3id.org/netbeheer/IECCIM/TC57CIM/IEC61970/Base/Domain#Seconds>
                                         ] ,
                                         [ rdf:type owl:Restriction ;
                                           owl:onProperty :RegularIntervalSchedule_TimePoints ;
                                           owl:qualifiedCardinality "1"^^xsd:nonNegativeInteger ;
                                           owl:onClass :RegularIntervalSchedule
                                         ] ,
                                         [ rdf:type owl:Restriction ;
                                           owl:onProperty :RegularIntervalSchedule_timeStep ;
                                           owl:maxQualifiedCardinality "1"^^xsd:nonNegativeInteger ;
                                           owl:onClass <https://w3id.org/netbeheer/IECCIM/TC57CIM/IEC61970/Base/Domain#Seconds>
                                         ] ,
                                         [ rdf:type owl:Restriction ;
                                           owl:onProperty :RegularIntervalSchedule_endTime ;
                                           owl:minQualifiedCardinality "0"^^xsd:nonNegativeInteger ;
                                           owl:onDataRange xsd:dateTime
                                         ] ,
                                         [ rdf:type owl:Restriction ;
                                           owl:onProperty :RegularIntervalSchedule_endTime ;
                                           owl:maxQualifiedCardinality "1"^^xsd:nonNegativeInteger ;
                                           owl:onDataRange xsd:dateTime
                                         ] ;
                         rdfs:comment """The schedule has time points where the time between them is constant.
""" .


###  https://w3id.org/netbeheer/IECCIM/TC57CIM/IEC61970/Base/Core#RegularTimePoint
:RegularTimePoint rdf:type owl:Class ;
                  rdfs:subClassOf [ rdf:type owl:Restriction ;
                                    owl:onProperty :RegularTimePoint_IntervalSchedule ;
                                    owl:minQualifiedCardinality "1"^^xsd:nonNegativeInteger ;
                                    owl:onClass :RegularTimePoint
                                  ] ,
                                  [ rdf:type owl:Restriction ;
                                    owl:onProperty :RegularTimePoint_sequenceNumber ;
                                    owl:minQualifiedCardinality "0"^^xsd:nonNegativeInteger ;
                                    owl:onDataRange xsd:nonNegativeInteger
                                  ] ,
                                  [ rdf:type owl:Restriction ;
                                    owl:onProperty :RegularTimePoint_value1 ;
                                    owl:minQualifiedCardinality "0"^^xsd:nonNegativeInteger ;
                                    owl:onDataRange xsd:float
                                  ] ,
                                  [ rdf:type owl:Restriction ;
                                    owl:onProperty :RegularTimePoint_value2 ;
                                    owl:minQualifiedCardinality "0"^^xsd:nonNegativeInteger ;
                                    owl:onDataRange xsd:float
                                  ] ,
                                  [ rdf:type owl:Restriction ;
                                    owl:onProperty :RegularTimePoint_sequenceNumber ;
                                    owl:maxQualifiedCardinality "1"^^xsd:nonNegativeInteger ;
                                    owl:onDataRange xsd:nonNegativeInteger
                                  ] ,
                                  [ rdf:type owl:Restriction ;
                                    owl:onProperty :RegularTimePoint_value1 ;
                                    owl:maxQualifiedCardinality "1"^^xsd:nonNegativeInteger ;
                                    owl:onDataRange xsd:float
                                  ] ,
                                  [ rdf:type owl:Restriction ;
                                    owl:onProperty :RegularTimePoint_value2 ;
                                    owl:maxQualifiedCardinality "1"^^xsd:nonNegativeInteger ;
                                    owl:onDataRange xsd:float
                                  ] ;
                  rdfs:comment """Time point for a schedule where the time between the consecutive points is constant.
""" .


###  https://w3id.org/netbeheer/IECCIM/TC57CIM/IEC61970/Base/Core#ReportingGroup
:ReportingGroup rdf:type owl:Class ;
                rdfs:subClassOf :IdentifiedObject ,
                                [ rdf:type owl:Restriction ;
                                  owl:onProperty :ReportingGroup_BusNameMarker ;
                                  owl:minQualifiedCardinality "0"^^xsd:nonNegativeInteger ;
                                  owl:onClass :ReportingGroup
                                ] ,
                                [ rdf:type owl:Restriction ;
                                  owl:onProperty :ReportingGroup_PowerSystemResource ;
                                  owl:minQualifiedCardinality "0"^^xsd:nonNegativeInteger ;
                                  owl:onClass :ReportingGroup
                                ] ,
                                [ rdf:type owl:Restriction ;
                                  owl:onProperty :ReportingGroup_ReportingSuperGroup ;
                                  owl:minQualifiedCardinality "0"^^xsd:nonNegativeInteger ;
                                  owl:onClass :ReportingGroup
                                ] ,
                                [ rdf:type owl:Restriction ;
                                  owl:onProperty :ReportingGroup_TopologicalNode ;
                                  owl:minQualifiedCardinality "0"^^xsd:nonNegativeInteger ;
                                  owl:onClass :ReportingGroup
                                ] ,
                                [ rdf:type owl:Restriction ;
                                  owl:onProperty :ReportingGroup_BusNameMarker ;
                                  owl:maxQualifiedCardinality "1"^^xsd:nonNegativeInteger ;
                                  owl:onClass :ReportingGroup
                                ] ,
                                [ rdf:type owl:Restriction ;
                                  owl:onProperty :ReportingGroup_TopologicalNode ;
                                  owl:maxQualifiedCardinality "1"^^xsd:nonNegativeInteger ;
                                  owl:onClass :ReportingGroup
                                ] ;
                rdfs:comment """A reporting group is used for various ad-hoc groupings used for reporting.
""" .


###  https://w3id.org/netbeheer/IECCIM/TC57CIM/IEC61970/Base/Core#ReportingSuperGroup
:ReportingSuperGroup rdf:type owl:Class ;
                     rdfs:subClassOf :IdentifiedObject ,
                                     [ rdf:type owl:Restriction ;
                                       owl:onProperty :ReportingSuperGroup_ReportingGroup ;
                                       owl:minQualifiedCardinality "0"^^xsd:nonNegativeInteger ;
                                       owl:onClass :ReportingSuperGroup
                                     ] ,
                                     [ rdf:type owl:Restriction ;
                                       owl:onProperty :ReportingSuperGroup_ReportingGroup ;
                                       owl:maxQualifiedCardinality "1"^^xsd:nonNegativeInteger ;
                                       owl:onClass :ReportingSuperGroup
                                     ] ;
                     rdfs:comment "A reporting super group, groups reporting groups for a higher level report." .


###  https://w3id.org/netbeheer/IECCIM/TC57CIM/IEC61970/Base/Core#SubGeographicalRegion
:SubGeographicalRegion rdf:type owl:Class ;
                       rdfs:subClassOf :IdentifiedObject ,
                                       [ rdf:type owl:Restriction ;
                                         owl:onProperty :SubGeographicalRegion_DCLines ;
                                         owl:minQualifiedCardinality "0"^^xsd:nonNegativeInteger ;
                                         owl:onClass :SubGeographicalRegion
                                       ] ,
                                       [ rdf:type owl:Restriction ;
                                         owl:onProperty :SubGeographicalRegion_Lines ;
                                         owl:minQualifiedCardinality "0"^^xsd:nonNegativeInteger ;
                                         owl:onClass :SubGeographicalRegion
                                       ] ,
                                       [ rdf:type owl:Restriction ;
                                         owl:onProperty :SubGeographicalRegion_Region ;
                                         owl:minQualifiedCardinality "0"^^xsd:nonNegativeInteger ;
                                         owl:onClass :SubGeographicalRegion
                                       ] ,
                                       [ rdf:type owl:Restriction ;
                                         owl:onProperty :SubGeographicalRegion_Substations ;
                                         owl:minQualifiedCardinality "0"^^xsd:nonNegativeInteger ;
                                         owl:onClass :SubGeographicalRegion
                                       ] ,
                                       [ rdf:type owl:Restriction ;
                                         owl:onProperty :SubGeographicalRegion_DCLines ;
                                         owl:maxQualifiedCardinality "1"^^xsd:nonNegativeInteger ;
                                         owl:onClass :SubGeographicalRegion
                                       ] ,
                                       [ rdf:type owl:Restriction ;
                                         owl:onProperty :SubGeographicalRegion_Lines ;
                                         owl:maxQualifiedCardinality "1"^^xsd:nonNegativeInteger ;
                                         owl:onClass :SubGeographicalRegion
                                       ] ,
                                       [ rdf:type owl:Restriction ;
                                         owl:onProperty :SubGeographicalRegion_Substations ;
                                         owl:maxQualifiedCardinality "1"^^xsd:nonNegativeInteger ;
                                         owl:onClass :SubGeographicalRegion
                                       ] ;
                       rdfs:comment """A subset of a geographical region of a power system network model.
""" .


###  https://w3id.org/netbeheer/IECCIM/TC57CIM/IEC61970/Base/Core#Substation
:Substation rdf:type owl:Class ;
            rdfs:subClassOf :EquipmentContainer ,
                            [ rdf:type owl:Restriction ;
                              owl:onProperty :Substation_Bays ;
                              owl:minQualifiedCardinality "0"^^xsd:nonNegativeInteger ;
                              owl:onClass :Substation
                            ] ,
                            [ rdf:type owl:Restriction ;
                              owl:onProperty :Substation_DCConverterUnit ;
                              owl:minQualifiedCardinality "0"^^xsd:nonNegativeInteger ;
                              owl:onClass :Substation
                            ] ,
                            [ rdf:type owl:Restriction ;
                              owl:onProperty :Substation_Region ;
                              owl:minQualifiedCardinality "0"^^xsd:nonNegativeInteger ;
                              owl:onClass :Substation
                            ] ,
                            [ rdf:type owl:Restriction ;
                              owl:onProperty :Substation_VoltageLevels ;
                              owl:qualifiedCardinality "1"^^xsd:nonNegativeInteger ;
                              owl:onClass :Substation
                            ] ,
                            [ rdf:type owl:Restriction ;
                              owl:onProperty :Substation_Bays ;
                              owl:maxQualifiedCardinality "1"^^xsd:nonNegativeInteger ;
                              owl:onClass :Substation
                            ] ,
                            [ rdf:type owl:Restriction ;
                              owl:onProperty :Substation_DCConverterUnit ;
                              owl:maxQualifiedCardinality "1"^^xsd:nonNegativeInteger ;
                              owl:onClass :Substation
                            ] ;
            rdfs:comment """A collection of equipment for purposes other than generation or utilization, through which electric energy in bulk is passed for the purposes of switching or modifying its characteristics. 
""" .


###  https://w3id.org/netbeheer/IECCIM/TC57CIM/IEC61970/Base/Core#Terminal
:Terminal rdf:type owl:Class ;
          rdfs:subClassOf :ACDCTerminal ,
                          [ rdf:type owl:Restriction ;
                            owl:onProperty :Terminal_Bushing ;
                            owl:minQualifiedCardinality "0"^^xsd:nonNegativeInteger ;
                            owl:onClass :Terminal
                          ] ,
                          [ rdf:type owl:Restriction ;
                            owl:onProperty :Terminal_ConductingEquipment ;
                            owl:minQualifiedCardinality "0"^^xsd:nonNegativeInteger ;
                            owl:onClass :Terminal
                          ] ,
                          [ rdf:type owl:Restriction ;
                            owl:onProperty :Terminal_ConnectivityNode ;
                            owl:minQualifiedCardinality "0"^^xsd:nonNegativeInteger ;
                            owl:onClass :Terminal
                          ] ,
                          [ rdf:type owl:Restriction ;
                            owl:onProperty :Terminal_ConverterDCSides ;
                            owl:minQualifiedCardinality "0"^^xsd:nonNegativeInteger ;
                            owl:onClass :Terminal
                          ] ,
                          [ rdf:type owl:Restriction ;
                            owl:onProperty :Terminal_RegulatingControl ;
                            owl:minQualifiedCardinality "0"^^xsd:nonNegativeInteger ;
                            owl:onClass :Terminal
                          ] ,
                          [ rdf:type owl:Restriction ;
                            owl:onProperty :Terminal_TopologicalNode ;
                            owl:minQualifiedCardinality "0"^^xsd:nonNegativeInteger ;
                            owl:onClass :Terminal
                          ] ,
                          [ rdf:type owl:Restriction ;
                            owl:onProperty :Terminal_TransformerEnd ;
                            owl:minQualifiedCardinality "0"^^xsd:nonNegativeInteger ;
                            owl:onClass :Terminal
                          ] ,
                          [ rdf:type owl:Restriction ;
                            owl:onProperty :Terminal_AuxiliaryEquipment ;
                            owl:qualifiedCardinality "1"^^xsd:nonNegativeInteger ;
                            owl:onClass :Terminal
                          ] ,
                          [ rdf:type owl:Restriction ;
                            owl:onProperty :Terminal_BranchGroupTerminal ;
                            owl:qualifiedCardinality "1"^^xsd:nonNegativeInteger ;
                            owl:onClass :Terminal
                          ] ,
                          [ rdf:type owl:Restriction ;
                            owl:onProperty :Terminal_HasFirstMutualCoupling ;
                            owl:qualifiedCardinality "1"^^xsd:nonNegativeInteger ;
                            owl:onClass :Terminal
                          ] ,
                          [ rdf:type owl:Restriction ;
                            owl:onProperty :Terminal_HasSecondMutualCoupling ;
                            owl:qualifiedCardinality "1"^^xsd:nonNegativeInteger ;
                            owl:onClass :Terminal
                          ] ,
                          [ rdf:type owl:Restriction ;
                            owl:onProperty :Terminal_PinTerminal ;
                            owl:qualifiedCardinality "1"^^xsd:nonNegativeInteger ;
                            owl:onClass :Terminal
                          ] ,
                          [ rdf:type owl:Restriction ;
                            owl:onProperty :Terminal_RemoteInputSignal ;
                            owl:qualifiedCardinality "1"^^xsd:nonNegativeInteger ;
                            owl:onClass :Terminal
                          ] ,
                          [ rdf:type owl:Restriction ;
                            owl:onProperty :Terminal_SvPowerFlow ;
                            owl:qualifiedCardinality "1"^^xsd:nonNegativeInteger ;
                            owl:onClass :Terminal
                          ] ,
                          [ rdf:type owl:Restriction ;
                            owl:onProperty :Terminal_TieFlow ;
                            owl:qualifiedCardinality "1"^^xsd:nonNegativeInteger ;
                            owl:onClass :Terminal
                          ] ,
                          [ rdf:type owl:Restriction ;
                            owl:onProperty :Terminal_Bushing ;
                            owl:maxQualifiedCardinality "1"^^xsd:nonNegativeInteger ;
                            owl:onClass :Terminal
                          ] ,
                          [ rdf:type owl:Restriction ;
                            owl:onProperty :Terminal_ConverterDCSides ;
                            owl:maxQualifiedCardinality "1"^^xsd:nonNegativeInteger ;
                            owl:onClass :Terminal
                          ] ,
                          [ rdf:type owl:Restriction ;
                            owl:onProperty :Terminal_RegulatingControl ;
                            owl:maxQualifiedCardinality "1"^^xsd:nonNegativeInteger ;
                            owl:onClass :Terminal
                          ] ,
                          [ rdf:type owl:Restriction ;
                            owl:onProperty :Terminal_TransformerEnd ;
                            owl:maxQualifiedCardinality "1"^^xsd:nonNegativeInteger ;
                            owl:onClass :Terminal
                          ] ,
                          [ rdf:type owl:Restriction ;
                            owl:onProperty :Terminal_phases ;
                            owl:minQualifiedCardinality "0"^^xsd:nonNegativeInteger ;
                            owl:onDataRange :PhaseCode
                          ] ,
                          [ rdf:type owl:Restriction ;
                            owl:onProperty :Terminal_phases ;
                            owl:maxQualifiedCardinality "1"^^xsd:nonNegativeInteger ;
                            owl:onDataRange :PhaseCode
                          ] ;
          rdfs:comment "An AC electrical connection point to a piece of conducting equipment. Terminals are connected at physical connection points called connectivity nodes." .


###  https://w3id.org/netbeheer/IECCIM/TC57CIM/IEC61970/Base/Core#VoltageLevel
:VoltageLevel rdf:type owl:Class ;
              rdfs:subClassOf :EquipmentContainer ,
                              [ rdf:type owl:Restriction ;
                                owl:onProperty :VoltageLevel_BaseVoltage ;
                                owl:minQualifiedCardinality "0"^^xsd:nonNegativeInteger ;
                                owl:onClass :VoltageLevel
                              ] ,
                              [ rdf:type owl:Restriction ;
                                owl:onProperty :VoltageLevel_Bays ;
                                owl:minQualifiedCardinality "0"^^xsd:nonNegativeInteger ;
                                owl:onClass :VoltageLevel
                              ] ,
                              [ rdf:type owl:Restriction ;
                                owl:onProperty :VoltageLevel_Substation ;
                                owl:minQualifiedCardinality "0"^^xsd:nonNegativeInteger ;
                                owl:onClass :VoltageLevel
                              ] ,
                              [ rdf:type owl:Restriction ;
                                owl:onProperty :VoltageLevel_highVoltageLimit ;
                                owl:minQualifiedCardinality "0"^^xsd:nonNegativeInteger ;
                                owl:onClass <https://w3id.org/netbeheer/IECCIM/TC57CIM/IEC61970/Base/Domain#Voltage>
                              ] ,
                              [ rdf:type owl:Restriction ;
                                owl:onProperty :VoltageLevel_lowVoltageLimit ;
                                owl:minQualifiedCardinality "0"^^xsd:nonNegativeInteger ;
                                owl:onClass <https://w3id.org/netbeheer/IECCIM/TC57CIM/IEC61970/Base/Domain#Voltage>
                              ] ,
                              [ rdf:type owl:Restriction ;
                                owl:onProperty :VoltageLevel_Bays ;
                                owl:maxQualifiedCardinality "1"^^xsd:nonNegativeInteger ;
                                owl:onClass :VoltageLevel
                              ] ,
                              [ rdf:type owl:Restriction ;
                                owl:onProperty :VoltageLevel_highVoltageLimit ;
                                owl:maxQualifiedCardinality "1"^^xsd:nonNegativeInteger ;
                                owl:onClass <https://w3id.org/netbeheer/IECCIM/TC57CIM/IEC61970/Base/Domain#Voltage>
                              ] ,
                              [ rdf:type owl:Restriction ;
                                owl:onProperty :VoltageLevel_lowVoltageLimit ;
                                owl:maxQualifiedCardinality "1"^^xsd:nonNegativeInteger ;
                                owl:onClass <https://w3id.org/netbeheer/IECCIM/TC57CIM/IEC61970/Base/Domain#Voltage>
                              ] ;
              rdfs:comment """A collection of equipment at one common system voltage forming a switchgear. The equipment typically consist of breakers, busbars, instrumentation, control, regulation and protection devices as well as assemblies of all these.
""" .


###  https://w3id.org/netbeheer/IECCIM/TC57CIM/IEC61970/Base/DC#ACDCConverter
<https://w3id.org/netbeheer/IECCIM/TC57CIM/IEC61970/Base/DC#ACDCConverter> rdf:type owl:Class ;
                                                                           rdfs:subClassOf [ rdf:type owl:Restriction ;
                                                                                             owl:onProperty :ACDCConverter_PccTerminal ;
                                                                                             owl:minQualifiedCardinality "0"^^xsd:nonNegativeInteger ;
                                                                                             owl:onClass <https://w3id.org/netbeheer/IECCIM/TC57CIM/IEC61970/Base/DC#ACDCConverter>
                                                                                           ] .


###  https://w3id.org/netbeheer/IECCIM/TC57CIM/IEC61970/Base/DC#DCConverterUnit
<https://w3id.org/netbeheer/IECCIM/TC57CIM/IEC61970/Base/DC#DCConverterUnit> rdf:type owl:Class ;
                                                                             rdfs:subClassOf [ rdf:type owl:Restriction ;
                                                                                               owl:onProperty :DCConverterUnit_Substation ;
                                                                                               owl:minQualifiedCardinality "0"^^xsd:nonNegativeInteger ;
                                                                                               owl:onClass <https://w3id.org/netbeheer/IECCIM/TC57CIM/IEC61970/Base/DC#DCConverterUnit>
                                                                                             ] .


###  https://w3id.org/netbeheer/IECCIM/TC57CIM/IEC61970/Base/DC#DCLine
<https://w3id.org/netbeheer/IECCIM/TC57CIM/IEC61970/Base/DC#DCLine> rdf:type owl:Class ;
                                                                    rdfs:subClassOf [ rdf:type owl:Restriction ;
                                                                                      owl:onProperty :DCLine_Region ;
                                                                                      owl:minQualifiedCardinality "0"^^xsd:nonNegativeInteger ;
                                                                                      owl:onClass <https://w3id.org/netbeheer/IECCIM/TC57CIM/IEC61970/Base/DC#DCLine>
                                                                                    ] .


###  https://w3id.org/netbeheer/IECCIM/TC57CIM/IEC61970/Base/DiagramLayout#DiagramObject
<https://w3id.org/netbeheer/IECCIM/TC57CIM/IEC61970/Base/DiagramLayout#DiagramObject> rdf:type owl:Class ;
                                                                                      rdfs:subClassOf [ rdf:type owl:Restriction ;
                                                                                                        owl:onProperty :DiagramObject_IdentifiedObject ;
                                                                                                        owl:minQualifiedCardinality "0"^^xsd:nonNegativeInteger ;
                                                                                                        owl:onClass <https://w3id.org/netbeheer/IECCIM/TC57CIM/IEC61970/Base/DiagramLayout#DiagramObject>
                                                                                                      ] .


###  https://w3id.org/netbeheer/IECCIM/TC57CIM/IEC61970/Base/Domain#ApparentPower
<https://w3id.org/netbeheer/IECCIM/TC57CIM/IEC61970/Base/Domain#ApparentPower> rdf:type owl:Class .


###  https://w3id.org/netbeheer/IECCIM/TC57CIM/IEC61970/Base/Domain#Frequency
<https://w3id.org/netbeheer/IECCIM/TC57CIM/IEC61970/Base/Domain#Frequency> rdf:type owl:Class .


###  https://w3id.org/netbeheer/IECCIM/TC57CIM/IEC61970/Base/Domain#PerCent
<https://w3id.org/netbeheer/IECCIM/TC57CIM/IEC61970/Base/Domain#PerCent> rdf:type owl:Class .


###  https://w3id.org/netbeheer/IECCIM/TC57CIM/IEC61970/Base/Domain#Seconds
<https://w3id.org/netbeheer/IECCIM/TC57CIM/IEC61970/Base/Domain#Seconds> rdf:type owl:Class .


###  https://w3id.org/netbeheer/IECCIM/TC57CIM/IEC61970/Base/Domain#Voltage
<https://w3id.org/netbeheer/IECCIM/TC57CIM/IEC61970/Base/Domain#Voltage> rdf:type owl:Class .


###  https://w3id.org/netbeheer/IECCIM/TC57CIM/IEC61970/Base/Meas#Control
<https://w3id.org/netbeheer/IECCIM/TC57CIM/IEC61970/Base/Meas#Control> rdf:type owl:Class ;
                                                                       rdfs:subClassOf [ rdf:type owl:Restriction ;
                                                                                         owl:onProperty :Control_PowerSystemResource ;
                                                                                         owl:minQualifiedCardinality "0"^^xsd:nonNegativeInteger ;
                                                                                         owl:onClass <https://w3id.org/netbeheer/IECCIM/TC57CIM/IEC61970/Base/Meas#Control>
                                                                                       ] .


###  https://w3id.org/netbeheer/IECCIM/TC57CIM/IEC61970/Base/Meas#Measure
<https://w3id.org/netbeheer/IECCIM/TC57CIM/IEC61970/Base/Meas#Measure> rdf:type owl:Class ;
                                                                       rdfs:subClassOf [ rdf:type owl:Restriction ;
                                                                                         owl:onProperty :Measure_PowerSystemResource ;
                                                                                         owl:minQualifiedCardinality "0"^^xsd:nonNegativeInteger ;
                                                                                         owl:onClass <https://w3id.org/netbeheer/IECCIM/TC57CIM/IEC61970/Base/Meas#Measure>
                                                                                       ] ,
                                                                                       [ rdf:type owl:Restriction ;
                                                                                         owl:onProperty :Measure_Terminal ;
                                                                                         owl:minQualifiedCardinality "0"^^xsd:nonNegativeInteger ;
                                                                                         owl:onClass <https://w3id.org/netbeheer/IECCIM/TC57CIM/IEC61970/Base/Meas#Measure>
                                                                                       ] .


###  https://w3id.org/netbeheer/IECCIM/TC57CIM/IEC61970/Base/OperationalLimits#BranchGroupTerminal
<https://w3id.org/netbeheer/IECCIM/TC57CIM/IEC61970/Base/OperationalLimits#BranchGroupTerminal> rdf:type owl:Class ;
                                                                                                rdfs:subClassOf [ rdf:type owl:Restriction ;
                                                                                                                  owl:onProperty :BranchGroupTerminal_Terminal ;
                                                                                                                  owl:minQualifiedCardinality "0"^^xsd:nonNegativeInteger ;
                                                                                                                  owl:onClass <https://w3id.org/netbeheer/IECCIM/TC57CIM/IEC61970/Base/OperationalLimits#BranchGroupTerminal>
                                                                                                                ] .


###  https://w3id.org/netbeheer/IECCIM/TC57CIM/IEC61970/Base/OperationalLimits#OperationalLimitSet
<https://w3id.org/netbeheer/IECCIM/TC57CIM/IEC61970/Base/OperationalLimits#OperationalLimitSet> rdf:type owl:Class ;
                                                                                                rdfs:subClassOf [ rdf:type owl:Restriction ;
                                                                                                                  owl:onProperty :OperationalLimitSet_Equipment ;
                                                                                                                  owl:minQualifiedCardinality "0"^^xsd:nonNegativeInteger ;
                                                                                                                  owl:onClass <https://w3id.org/netbeheer/IECCIM/TC57CIM/IEC61970/Base/OperationalLimits#OperationalLimitSet>
                                                                                                                ] ,
                                                                                                                [ rdf:type owl:Restriction ;
                                                                                                                  owl:onProperty :OperationalLimitSet_Terminal ;
                                                                                                                  owl:minQualifiedCardinality "0"^^xsd:nonNegativeInteger ;
                                                                                                                  owl:onClass <https://w3id.org/netbeheer/IECCIM/TC57CIM/IEC61970/Base/OperationalLimits#OperationalLimitSet>
                                                                                                                ] .


###  https://w3id.org/netbeheer/IECCIM/TC57CIM/IEC61970/Base/Protection#ProtectionEquipment
<https://w3id.org/netbeheer/IECCIM/TC57CIM/IEC61970/Base/Protection#ProtectionEquipment> rdf:type owl:Class ;
                                                                                         rdfs:subClassOf [ rdf:type owl:Restriction ;
                                                                                                           owl:onProperty :ProtectionEquipment_ConductingEquipments ;
                                                                                                           owl:minQualifiedCardinality "0"^^xsd:nonNegativeInteger ;
                                                                                                           owl:onClass <https://w3id.org/netbeheer/IECCIM/TC57CIM/IEC61970/Base/Protection#ProtectionEquipment>
                                                                                                         ] .


###  https://w3id.org/netbeheer/IECCIM/TC57CIM/IEC61970/Base/StateVariables#SvPowerFlow
<https://w3id.org/netbeheer/IECCIM/TC57CIM/IEC61970/Base/StateVariables#SvPowerFlow> rdf:type owl:Class ;
                                                                                     rdfs:subClassOf [ rdf:type owl:Restriction ;
                                                                                                       owl:onProperty :SvPowerFlow_Terminal ;
                                                                                                       owl:minQualifiedCardinality "0"^^xsd:nonNegativeInteger ;
                                                                                                       owl:onClass <https://w3id.org/netbeheer/IECCIM/TC57CIM/IEC61970/Base/StateVariables#SvPowerFlow>
                                                                                                     ] .


###  https://w3id.org/netbeheer/IECCIM/TC57CIM/IEC61970/Base/StateVariables#SvStatus
<https://w3id.org/netbeheer/IECCIM/TC57CIM/IEC61970/Base/StateVariables#SvStatus> rdf:type owl:Class ;
                                                                                  rdfs:subClassOf [ rdf:type owl:Restriction ;
                                                                                                    owl:onProperty :SvStatus_ConductingEquipment ;
                                                                                                    owl:minQualifiedCardinality "0"^^xsd:nonNegativeInteger ;
                                                                                                    owl:onClass <https://w3id.org/netbeheer/IECCIM/TC57CIM/IEC61970/Base/StateVariables#SvStatus>
                                                                                                  ] .


###  https://w3id.org/netbeheer/IECCIM/TC57CIM/IEC61970/Base/Topology#BusNameMarker
<https://w3id.org/netbeheer/IECCIM/TC57CIM/IEC61970/Base/Topology#BusNameMarker> rdf:type owl:Class ;
                                                                                 rdfs:subClassOf [ rdf:type owl:Restriction ;
                                                                                                   owl:onProperty :BusNameMarker_ReportingGroup ;
                                                                                                   owl:minQualifiedCardinality "0"^^xsd:nonNegativeInteger ;
                                                                                                   owl:onClass <https://w3id.org/netbeheer/IECCIM/TC57CIM/IEC61970/Base/Topology#BusNameMarker>
                                                                                                 ] ,
                                                                                                 [ rdf:type owl:Restriction ;
                                                                                                   owl:onProperty :BusNameMarker_Terminal ;
                                                                                                   owl:minQualifiedCardinality "0"^^xsd:nonNegativeInteger ;
                                                                                                   owl:onClass <https://w3id.org/netbeheer/IECCIM/TC57CIM/IEC61970/Base/Topology#BusNameMarker>
                                                                                                 ] ,
                                                                                                 [ rdf:type owl:Restriction ;
                                                                                                   owl:onProperty :BusNameMarker_Terminal ;
                                                                                                   owl:maxQualifiedCardinality "1"^^xsd:nonNegativeInteger ;
                                                                                                   owl:onClass <https://w3id.org/netbeheer/IECCIM/TC57CIM/IEC61970/Base/Topology#BusNameMarker>
                                                                                                 ] .


###  https://w3id.org/netbeheer/IECCIM/TC57CIM/IEC61970/Base/Topology#TopologicalNode
<https://w3id.org/netbeheer/IECCIM/TC57CIM/IEC61970/Base/Topology#TopologicalNode> rdf:type owl:Class ;
                                                                                   rdfs:subClassOf [ rdf:type owl:Restriction ;
                                                                                                     owl:onProperty :TopologicalNode_BaseVoltage ;
                                                                                                     owl:minQualifiedCardinality "0"^^xsd:nonNegativeInteger ;
                                                                                                     owl:onClass <https://w3id.org/netbeheer/IECCIM/TC57CIM/IEC61970/Base/Topology#TopologicalNode>
                                                                                                   ] ,
                                                                                                   [ rdf:type owl:Restriction ;
                                                                                                     owl:onProperty :TopologicalNode_ConnectivityNodeContainer ;
                                                                                                     owl:minQualifiedCardinality "0"^^xsd:nonNegativeInteger ;
                                                                                                     owl:onClass <https://w3id.org/netbeheer/IECCIM/TC57CIM/IEC61970/Base/Topology#TopologicalNode>
                                                                                                   ] ,
                                                                                                   [ rdf:type owl:Restriction ;
                                                                                                     owl:onProperty :TopologicalNode_ConnectivityNodes ;
                                                                                                     owl:minQualifiedCardinality "0"^^xsd:nonNegativeInteger ;
                                                                                                     owl:onClass <https://w3id.org/netbeheer/IECCIM/TC57CIM/IEC61970/Base/Topology#TopologicalNode>
                                                                                                   ] ,
                                                                                                   [ rdf:type owl:Restriction ;
                                                                                                     owl:onProperty :TopologicalNode_ReportingGroup ;
                                                                                                     owl:minQualifiedCardinality "0"^^xsd:nonNegativeInteger ;
                                                                                                     owl:onClass <https://w3id.org/netbeheer/IECCIM/TC57CIM/IEC61970/Base/Topology#TopologicalNode>
                                                                                                   ] ,
                                                                                                   [ rdf:type owl:Restriction ;
                                                                                                     owl:onProperty :TopologicalNode_Terminal ;
                                                                                                     owl:minQualifiedCardinality "0"^^xsd:nonNegativeInteger ;
                                                                                                     owl:onClass <https://w3id.org/netbeheer/IECCIM/TC57CIM/IEC61970/Base/Topology#TopologicalNode>
                                                                                                   ] ,
                                                                                                   [ rdf:type owl:Restriction ;
                                                                                                     owl:onProperty :TopologicalNode_ConnectivityNodes ;
                                                                                                     owl:maxQualifiedCardinality "1"^^xsd:nonNegativeInteger ;
                                                                                                     owl:onClass <https://w3id.org/netbeheer/IECCIM/TC57CIM/IEC61970/Base/Topology#TopologicalNode>
                                                                                                   ] ,
                                                                                                   [ rdf:type owl:Restriction ;
                                                                                                     owl:onProperty :TopologicalNode_Terminal ;
                                                                                                     owl:maxQualifiedCardinality "1"^^xsd:nonNegativeInteger ;
                                                                                                     owl:onClass <https://w3id.org/netbeheer/IECCIM/TC57CIM/IEC61970/Base/Topology#TopologicalNode>
                                                                                                   ] .


###  https://w3id.org/netbeheer/IECCIM/TC57CIM/IEC61970/Base/Wires#Line
<https://w3id.org/netbeheer/IECCIM/TC57CIM/IEC61970/Base/Wires#Line> rdf:type owl:Class ;
                                                                     rdfs:subClassOf [ rdf:type owl:Restriction ;
                                                                                       owl:onProperty :Line_Region ;
                                                                                       owl:minQualifiedCardinality "0"^^xsd:nonNegativeInteger ;
                                                                                       owl:onClass <https://w3id.org/netbeheer/IECCIM/TC57CIM/IEC61970/Base/Wires#Line>
                                                                                     ] .


###  https://w3id.org/netbeheer/IECCIM/TC57CIM/IEC61970/Base/Wires#MutualCoupling
<https://w3id.org/netbeheer/IECCIM/TC57CIM/IEC61970/Base/Wires#MutualCoupling> rdf:type owl:Class ;
                                                                               rdfs:subClassOf [ rdf:type owl:Restriction ;
                                                                                                 owl:onProperty :MutualCoupling_First_Terminal ;
                                                                                                 owl:minQualifiedCardinality "0"^^xsd:nonNegativeInteger ;
                                                                                                 owl:onClass <https://w3id.org/netbeheer/IECCIM/TC57CIM/IEC61970/Base/Wires#MutualCoupling>
                                                                                               ] ,
                                                                                               [ rdf:type owl:Restriction ;
                                                                                                 owl:onProperty :MutualCoupling_Second_Terminal ;
                                                                                                 owl:minQualifiedCardinality "0"^^xsd:nonNegativeInteger ;
                                                                                                 owl:onClass <https://w3id.org/netbeheer/IECCIM/TC57CIM/IEC61970/Base/Wires#MutualCoupling>
                                                                                               ] .


###  https://w3id.org/netbeheer/IECCIM/TC57CIM/IEC61970/Base/Wires#RegulatingControl
<https://w3id.org/netbeheer/IECCIM/TC57CIM/IEC61970/Base/Wires#RegulatingControl> rdf:type owl:Class ;
                                                                                  rdfs:subClassOf [ rdf:type owl:Restriction ;
                                                                                                    owl:onProperty :RegulatingControl_Terminal ;
                                                                                                    owl:minQualifiedCardinality "0"^^xsd:nonNegativeInteger ;
                                                                                                    owl:onClass <https://w3id.org/netbeheer/IECCIM/TC57CIM/IEC61970/Base/Wires#RegulatingControl>
                                                                                                  ] .


###  https://w3id.org/netbeheer/IECCIM/TC57CIM/IEC61970/Base/Wires#TransformerEnd
<https://w3id.org/netbeheer/IECCIM/TC57CIM/IEC61970/Base/Wires#TransformerEnd> rdf:type owl:Class ;
                                                                               rdfs:subClassOf [ rdf:type owl:Restriction ;
                                                                                                 owl:onProperty :TransformerEnd_BaseVoltage ;
                                                                                                 owl:minQualifiedCardinality "0"^^xsd:nonNegativeInteger ;
                                                                                                 owl:onClass <https://w3id.org/netbeheer/IECCIM/TC57CIM/IEC61970/Base/Wires#TransformerEnd>
                                                                                               ] ,
                                                                                               [ rdf:type owl:Restriction ;
                                                                                                 owl:onProperty :TransformerEnd_Terminal ;
                                                                                                 owl:minQualifiedCardinality "0"^^xsd:nonNegativeInteger ;
                                                                                                 owl:onClass <https://w3id.org/netbeheer/IECCIM/TC57CIM/IEC61970/Base/Wires#TransformerEnd>
                                                                                               ] .


###  https://w3id.org/netbeheer/IECCIM/TC57CIM/IEC61970/Dynamics/StandardInterconnections#RemoteInputSignal
<https://w3id.org/netbeheer/IECCIM/TC57CIM/IEC61970/Dynamics/StandardInterconnections#RemoteInputSignal> rdf:type owl:Class ;
                                                                                                         rdfs:subClassOf [ rdf:type owl:Restriction ;
                                                                                                                           owl:onProperty :RemoteInputSignal_Terminal ;
                                                                                                                           owl:minQualifiedCardinality "0"^^xsd:nonNegativeInteger ;
                                                                                                                           owl:onClass <https://w3id.org/netbeheer/IECCIM/TC57CIM/IEC61970/Dynamics/StandardInterconnections#RemoteInputSignal>
                                                                                                                         ] .


###  https://w3id.org/netbeheer/IECCIM/TC57CIM/IEC61970/InfIEC61970/InfGenericDataset/CanonicalModel/GenericDatasetCore#CIMDataObject
<https://w3id.org/netbeheer/IECCIM/TC57CIM/IEC61970/InfIEC61970/InfGenericDataset/CanonicalModel/GenericDatasetCore#CIMDataObject> rdf:type owl:Class ;
                                                                                                                                   rdfs:subClassOf [ rdf:type owl:Restriction ;
                                                                                                                                                     owl:onProperty :CIMDataObject_PropertiesObject ;
                                                                                                                                                     owl:minQualifiedCardinality "0"^^xsd:nonNegativeInteger ;
                                                                                                                                                     owl:onClass <https://w3id.org/netbeheer/IECCIM/TC57CIM/IEC61970/InfIEC61970/InfGenericDataset/CanonicalModel/GenericDatasetCore#CIMDataObject>
                                                                                                                                                   ] ,
                                                                                                                                                   [ rdf:type owl:Restriction ;
                                                                                                                                                     owl:onProperty :CIMDataObject_RegisteredObject ;
                                                                                                                                                     owl:minQualifiedCardinality "0"^^xsd:nonNegativeInteger ;
                                                                                                                                                     owl:onClass <https://w3id.org/netbeheer/IECCIM/TC57CIM/IEC61970/InfIEC61970/InfGenericDataset/CanonicalModel/GenericDatasetCore#CIMDataObject>
                                                                                                                                                   ] ,
                                                                                                                                                   [ rdf:type owl:Restriction ;
                                                                                                                                                     owl:onProperty :CIMDataObject_PropertiesObject ;
                                                                                                                                                     owl:maxQualifiedCardinality "1"^^xsd:nonNegativeInteger ;
                                                                                                                                                     owl:onClass <https://w3id.org/netbeheer/IECCIM/TC57CIM/IEC61970/InfIEC61970/InfGenericDataset/CanonicalModel/GenericDatasetCore#CIMDataObject>
                                                                                                                                                   ] .


###  https://w3id.org/netbeheer/IECCIM/TC57CIM/IEC61970/InfIEC61970/InfOperationalLimits#EquipmentLimitSeriesComponent
<https://w3id.org/netbeheer/IECCIM/TC57CIM/IEC61970/InfIEC61970/InfOperationalLimits#EquipmentLimitSeriesComponent> rdf:type owl:Class ;
                                                                                                                    rdfs:subClassOf [ rdf:type owl:Restriction ;
                                                                                                                                      owl:onProperty :EquipmentLimitSeriesComponent_Equipment ;
                                                                                                                                      owl:minQualifiedCardinality "0"^^xsd:nonNegativeInteger ;
                                                                                                                                      owl:onClass <https://w3id.org/netbeheer/IECCIM/TC57CIM/IEC61970/InfIEC61970/InfOperationalLimits#EquipmentLimitSeriesComponent>
                                                                                                                                    ] .


###  https://w3id.org/netbeheer/IECCIM/TC57CIM/IEC61970/InfIEC61970/InfOperationalLimits#LimitDependency
<https://w3id.org/netbeheer/IECCIM/TC57CIM/IEC61970/InfIEC61970/InfOperationalLimits#LimitDependency> rdf:type owl:Class ;
                                                                                                      rdfs:subClassOf [ rdf:type owl:Restriction ;
                                                                                                                        owl:onProperty :LimitDependency_Equipment ;
                                                                                                                        owl:minQualifiedCardinality "0"^^xsd:nonNegativeInteger ;
                                                                                                                        owl:onClass <https://w3id.org/netbeheer/IECCIM/TC57CIM/IEC61970/InfIEC61970/InfOperationalLimits#LimitDependency>
                                                                                                                      ] .


###  https://w3id.org/netbeheer/IECCIM/TC57CIM/IEC61970/InfIEC61970/InfOperationalLimits#WeatherStation
<https://w3id.org/netbeheer/IECCIM/TC57CIM/IEC61970/InfIEC61970/InfOperationalLimits#WeatherStation> rdf:type owl:Class ;
                                                                                                     rdfs:subClassOf [ rdf:type owl:Restriction ;
                                                                                                                       owl:onProperty :WeatherStation_Equipment ;
                                                                                                                       owl:minQualifiedCardinality "0"^^xsd:nonNegativeInteger ;
                                                                                                                       owl:onClass <https://w3id.org/netbeheer/IECCIM/TC57CIM/IEC61970/InfIEC61970/InfOperationalLimits#WeatherStation>
                                                                                                                     ] .


###  https://w3id.org/netbeheer/IECCIM/TC57CIM/IEC61970/InfIEC61970/InfSIPS#PinEquipment
<https://w3id.org/netbeheer/IECCIM/TC57CIM/IEC61970/InfIEC61970/InfSIPS#PinEquipment> rdf:type owl:Class ;
                                                                                      rdfs:subClassOf [ rdf:type owl:Restriction ;
                                                                                                        owl:onProperty :PinEquipment_Equipment ;
                                                                                                        owl:minQualifiedCardinality "0"^^xsd:nonNegativeInteger ;
                                                                                                        owl:onClass <https://w3id.org/netbeheer/IECCIM/TC57CIM/IEC61970/InfIEC61970/InfSIPS#PinEquipment>
                                                                                                      ] .


###  https://w3id.org/netbeheer/IECCIM/TC57CIM/IEC61970/InfIEC61970/InfSIPS#PinTerminal
<https://w3id.org/netbeheer/IECCIM/TC57CIM/IEC61970/InfIEC61970/InfSIPS#PinTerminal> rdf:type owl:Class ;
                                                                                     rdfs:subClassOf [ rdf:type owl:Restriction ;
                                                                                                       owl:onProperty :PinTerminal_Terminal ;
                                                                                                       owl:minQualifiedCardinality "0"^^xsd:nonNegativeInteger ;
                                                                                                       owl:onClass <https://w3id.org/netbeheer/IECCIM/TC57CIM/IEC61970/InfIEC61970/InfSIPS#PinTerminal>
                                                                                                     ] .


###  https://w3id.org/netbeheer/IECCIM/TC57CIM/IEC61970/InfIEC61970/InfSIPS#ProtectiveActionAdjustment
<https://w3id.org/netbeheer/IECCIM/TC57CIM/IEC61970/InfIEC61970/InfSIPS#ProtectiveActionAdjustment> rdf:type owl:Class ;
                                                                                                    rdfs:subClassOf [ rdf:type owl:Restriction ;
                                                                                                                      owl:onProperty :ProtectiveActionAdjustment_ConductingEquipment ;
                                                                                                                      owl:minQualifiedCardinality "0"^^xsd:nonNegativeInteger ;
                                                                                                                      owl:onClass <https://w3id.org/netbeheer/IECCIM/TC57CIM/IEC61970/InfIEC61970/InfSIPS#ProtectiveActionAdjustment>
                                                                                                                    ] .


###  https://w3id.org/netbeheer/IECCIM/TC57CIM/IEC61970/InfIEC61970/InfSIPS#ProtectiveActionEquipment
<https://w3id.org/netbeheer/IECCIM/TC57CIM/IEC61970/InfIEC61970/InfSIPS#ProtectiveActionEquipment> rdf:type owl:Class ;
                                                                                                   rdfs:subClassOf [ rdf:type owl:Restriction ;
                                                                                                                     owl:onProperty :ProtectiveActionEquipment_Equipment ;
                                                                                                                     owl:minQualifiedCardinality "0"^^xsd:nonNegativeInteger ;
                                                                                                                     owl:onClass <https://w3id.org/netbeheer/IECCIM/TC57CIM/IEC61970/InfIEC61970/InfSIPS#ProtectiveActionEquipment>
                                                                                                                   ] .


###  Generated by the OWL API (version 5.1.10.2019-03-12T22:31:15Z) https://github.com/owlcs/owlapi/
