@prefix : <https://w3id.org/netbeheer/IECCIM/TC57CIM/IEC61970/Base/Core#> .
@prefix owl: <http://www.w3.org/2002/07/owl#> .
@prefix rdf: <http://www.w3.org/1999/02/22-rdf-syntax-ns#> .
@prefix xml: <http://www.w3.org/XML/1998/namespace> .
@prefix xsd: <http://www.w3.org/2001/XMLSchema#> .
@prefix rdfs: <http://www.w3.org/2000/01/rdf-schema#> .

<https://w3id.org/netbeheer/IECCIM/TC57CIM/IEC61970/Base/Core#> a owl:Ontology .
# 
# 
# #################################################################
# #
# #    Datatypes
# #
# #################################################################
# 
# 
# https://w3id.org/netbeheer/IECCIM/TC57CIM/IEC61970/Base/Core#BreakerConfiguration

:BreakerConfiguration a rdfs:Datatype ;
	owl:equivalentClass _:genid1 .

_:genid1 a rdfs:Datatype ;
	owl:oneOf _:genid9 .

_:genid9 a rdf:List ;
	rdf:first "breakerAndAHalf" ;
	rdf:rest _:genid8 .

_:genid8 a rdf:List ;
	rdf:first "doubleBreaker" ;
	rdf:rest _:genid7 .

_:genid7 a rdf:List ;
	rdf:first "noBreaker" ;
	rdf:rest _:genid6 .

_:genid6 a rdf:List ;
	rdf:first "singleBreaker" ;
	rdf:rest rdf:nil .
# 
# https://w3id.org/netbeheer/IECCIM/TC57CIM/IEC61970/Base/Core#BusbarConfiguration

:BusbarConfiguration a rdfs:Datatype ;
	owl:equivalentClass _:genid10 .

_:genid10 a rdfs:Datatype ;
	owl:oneOf _:genid18 .

_:genid18 a rdf:List ;
	rdf:first "doubleBus" ;
	rdf:rest _:genid17 .

_:genid17 a rdf:List ;
	rdf:first "mainWithTransfer" ;
	rdf:rest _:genid16 .

_:genid16 a rdf:List ;
	rdf:first "ringBus" ;
	rdf:rest _:genid15 .

_:genid15 a rdf:List ;
	rdf:first "singleBus" ;
	rdf:rest rdf:nil .
# 
# https://w3id.org/netbeheer/IECCIM/TC57CIM/IEC61970/Base/Core#CurveStyle

:CurveStyle a rdfs:Datatype ;
	owl:equivalentClass _:genid19 .

_:genid19 a rdfs:Datatype ;
	owl:oneOf _:genid23 .

_:genid23 a rdf:List ;
	rdf:first "constantYValue" ;
	rdf:rest _:genid22 .

_:genid22 a rdf:List ;
	rdf:first "straightLineYValues" ;
	rdf:rest rdf:nil .
# 
# https://w3id.org/netbeheer/IECCIM/TC57CIM/IEC61970/Base/Core#PhaseCode

:PhaseCode a rdfs:Datatype ;
	owl:equivalentClass _:genid24 .

_:genid24 a rdfs:Datatype ;
	owl:oneOf _:genid76 .

_:genid76 a rdf:List ;
	rdf:first "A" ;
	rdf:rest _:genid75 .

_:genid75 a rdf:List ;
	rdf:first "AB" ;
	rdf:rest _:genid74 .

_:genid74 a rdf:List ;
	rdf:first "ABC" ;
	rdf:rest _:genid73 .

_:genid73 a rdf:List ;
	rdf:first "ABCN" ;
	rdf:rest _:genid72 .

_:genid72 a rdf:List ;
	rdf:first "ABN" ;
	rdf:rest _:genid71 .

_:genid71 a rdf:List ;
	rdf:first "AC" ;
	rdf:rest _:genid70 .

_:genid70 a rdf:List ;
	rdf:first "ACN" ;
	rdf:rest _:genid69 .

_:genid69 a rdf:List ;
	rdf:first "AN" ;
	rdf:rest _:genid68 .

_:genid68 a rdf:List ;
	rdf:first "B" ;
	rdf:rest _:genid67 .

_:genid67 a rdf:List ;
	rdf:first "BC" ;
	rdf:rest _:genid66 .

_:genid66 a rdf:List ;
	rdf:first "BCN" ;
	rdf:rest _:genid65 .

_:genid65 a rdf:List ;
	rdf:first "BN" ;
	rdf:rest _:genid64 .

_:genid64 a rdf:List ;
	rdf:first "C" ;
	rdf:rest _:genid63 .

_:genid63 a rdf:List ;
	rdf:first "CN" ;
	rdf:rest _:genid62 .

_:genid62 a rdf:List ;
	rdf:first "N" ;
	rdf:rest _:genid61 .

_:genid61 a rdf:List ;
	rdf:first "X" ;
	rdf:rest _:genid60 .

_:genid60 a rdf:List ;
	rdf:first "XN" ;
	rdf:rest _:genid59 .

_:genid59 a rdf:List ;
	rdf:first "XY" ;
	rdf:rest _:genid58 .

_:genid58 a rdf:List ;
	rdf:first "XYN" ;
	rdf:rest _:genid57 .

_:genid57 a rdf:List ;
	rdf:first "none" ;
	rdf:rest _:genid56 .

_:genid56 a rdf:List ;
	rdf:first "s1" ;
	rdf:rest _:genid55 .

_:genid55 a rdf:List ;
	rdf:first "s12" ;
	rdf:rest _:genid54 .

_:genid54 a rdf:List ;
	rdf:first "s12N" ;
	rdf:rest _:genid53 .

_:genid53 a rdf:List ;
	rdf:first "s1N" ;
	rdf:rest _:genid52 .

_:genid52 a rdf:List ;
	rdf:first "s2" ;
	rdf:rest _:genid51 .

_:genid51 a rdf:List ;
	rdf:first "s2N" ;
	rdf:rest rdf:nil .
# 
# https://w3id.org/netbeheer/IECCIM/TC57CIM/IEC61970/Base/Domain#UnitMultiplier

<https://w3id.org/netbeheer/IECCIM/TC57CIM/IEC61970/Base/Domain#UnitMultiplier> a rdfs:Datatype .
# 
# https://w3id.org/netbeheer/IECCIM/TC57CIM/IEC61970/Base/Domain#UnitSymbol

<https://w3id.org/netbeheer/IECCIM/TC57CIM/IEC61970/Base/Domain#UnitSymbol> a rdfs:Datatype .
# 
# 
# 
# #################################################################
# #
# #    Object Properties
# #
# #################################################################
# 
# 
# https://w3id.org/netbeheer/IECCIM/TC57CIM/IEC61970/Base/Core#ACDCConverter_PccTerminal

:ACDCConverter_PccTerminal a owl:ObjectProperty ;
	owl:inverseOf :Terminal_ConverterDCSides ;
	rdfs:domain <https://w3id.org/netbeheer/IECCIM/TC57CIM/IEC61970/Base/DC#ACDCConverter> ;
	rdfs:range :Terminal ;
	rdfs:comment "All converters' DC sides linked to this point of common coupling terminal.Point of common coupling terminal for this converter DC side. It is typically the terminal on the power transformer (or switch) closest to the AC network. The power flow measurement must be the sum of all flows into the transformer." .
# 
# https://w3id.org/netbeheer/IECCIM/TC57CIM/IEC61970/Base/Core#ACDCTerminal_BusNameMarker

:ACDCTerminal_BusNameMarker a owl:ObjectProperty ;
	owl:inverseOf :BusNameMarker_Terminal ;
	rdfs:domain :ACDCTerminal ;
	rdfs:range <https://w3id.org/netbeheer/IECCIM/TC57CIM/IEC61970/Base/Topology#BusNameMarker> ;
	rdfs:comment "The bus name marker used to name the bus (topological node).The terminals associated with this bus name marker." .
# 
# https://w3id.org/netbeheer/IECCIM/TC57CIM/IEC61970/Base/Core#ACDCTerminal_Measurements

:ACDCTerminal_Measurements a owl:ObjectProperty ;
	owl:inverseOf :Measure_Terminal ;
	rdfs:domain :ACDCTerminal ;
	rdfs:range <https://w3id.org/netbeheer/IECCIM/TC57CIM/IEC61970/Base/Meas#Measure> ;
	rdfs:comment "Measurements associated with this terminal defining  where the measurement is placed in the network topology.  It may be used, for instance, to capture the sensor position, such as a voltage transformer (PT) at a busbar or a current transformer (CT) at the bar between a breaker and an isolator.One or more measurements may be associated with a terminal in the network." .
# 
# https://w3id.org/netbeheer/IECCIM/TC57CIM/IEC61970/Base/Core#ACDCTerminal_OperationalLimitSet

:ACDCTerminal_OperationalLimitSet a owl:ObjectProperty ;
	owl:inverseOf :OperationalLimitSet_Terminal ;
	rdfs:domain :ACDCTerminal ;
	rdfs:range <https://w3id.org/netbeheer/IECCIM/TC57CIM/IEC61970/Base/OperationalLimits#OperationalLimitSet> ;
	rdfs:comment "" .
# 
# https://w3id.org/netbeheer/IECCIM/TC57CIM/IEC61970/Base/Core#AssetInfo_PowerSystemResources

:AssetInfo_PowerSystemResources a owl:ObjectProperty ;
	owl:inverseOf :PowerSystemResource_AssetDatasheet ;
	rdfs:domain <https://w3id.org/netbeheer/IECCIM/TC57CIM/IEC61968/Assets#AssetInfo> ;
	rdfs:range :PowerSystemResource ;
	rdfs:comment "Datasheet information for this power system resource.All power system resources with this datasheet information." .
# 
# https://w3id.org/netbeheer/IECCIM/TC57CIM/IEC61970/Base/Core#Asset_PowerSystemResources

:Asset_PowerSystemResources a owl:ObjectProperty ;
	owl:inverseOf :PowerSystemResource_Assets ;
	rdfs:domain <https://w3id.org/netbeheer/IECCIM/TC57CIM/IEC61968/Assets#Asset> ;
	rdfs:range :PowerSystemResource ;
	rdfs:comment "All assets represented by this power system resource. For example, multiple conductor assets are electrically modelled as a single AC line segment.All power system resources used to electrically model this asset. For example, transformer asset is electrically modelled with a transformer and its windings and tap changer." .
# 
# https://w3id.org/netbeheer/IECCIM/TC57CIM/IEC61970/Base/Core#AuxiliaryEquipment_Terminal

:AuxiliaryEquipment_Terminal a owl:ObjectProperty ;
	owl:inverseOf :Terminal_AuxiliaryEquipment ;
	rdfs:domain <https://w3id.org/netbeheer/IECCIM/TC57CIM/IEC61970/Base/AuxiliaryEquipment#AuxiliaryEquipment> ;
	rdfs:range :Terminal ;
	rdfs:comment "The auxiliary equipment connected to the terminal.The Terminal at the equipment where the AuxiliaryEquipment is attached." .
# 
# https://w3id.org/netbeheer/IECCIM/TC57CIM/IEC61970/Base/Core#BaseFrequency_frequency

:BaseFrequency_frequency a owl:ObjectProperty ;
	rdfs:domain :BaseFrequency ;
	rdfs:range <https://w3id.org/netbeheer/IECCIM/TC57CIM/IEC61970/Base/Domain#Frequency> ;
	rdfs:comment "The base frequency." .
# 
# https://w3id.org/netbeheer/IECCIM/TC57CIM/IEC61970/Base/Core#BasePower_basePower

:BasePower_basePower a owl:ObjectProperty ;
	rdfs:domain :BasePower ;
	rdfs:range <https://w3id.org/netbeheer/IECCIM/TC57CIM/IEC61970/Base/Domain#ApparentPower> ;
	rdfs:comment """Value used as base power.
""" .
# 
# https://w3id.org/netbeheer/IECCIM/TC57CIM/IEC61970/Base/Core#BaseVoltage_ConductingEquipment

:BaseVoltage_ConductingEquipment a owl:ObjectProperty ;
	owl:inverseOf :ConductingEquipment_BaseVoltage ;
	rdfs:domain :BaseVoltage ;
	rdfs:range :ConductingEquipment ;
	rdfs:comment "Base voltage of this conducting equipment.  Use only when there is no voltage level container used and only one base voltage applies.  For example, not used for transformers.All conducting equipment with this base voltage.  Use only when there is no voltage level container used and only one base voltage applies.  For example, not used for transformers." .
# 
# https://w3id.org/netbeheer/IECCIM/TC57CIM/IEC61970/Base/Core#BaseVoltage_TopologicalNode

:BaseVoltage_TopologicalNode a owl:ObjectProperty ;
	owl:inverseOf :TopologicalNode_BaseVoltage ;
	rdfs:domain :BaseVoltage ;
	rdfs:range <https://w3id.org/netbeheer/IECCIM/TC57CIM/IEC61970/Base/Topology#TopologicalNode> ;
	rdfs:comment "The topological nodes at the base voltage.The base voltage of the topologocial node." .
# 
# https://w3id.org/netbeheer/IECCIM/TC57CIM/IEC61970/Base/Core#BaseVoltage_TransformerEnds

:BaseVoltage_TransformerEnds a owl:ObjectProperty ;
	owl:inverseOf :TransformerEnd_BaseVoltage ;
	rdfs:domain :BaseVoltage ;
	rdfs:range <https://w3id.org/netbeheer/IECCIM/TC57CIM/IEC61970/Base/Wires#TransformerEnd> ;
	rdfs:comment "Transformer ends at the base voltage.  This is essential for PU calculation.Base voltage of the transformer end.  This is essential for PU calculation." .
# 
# https://w3id.org/netbeheer/IECCIM/TC57CIM/IEC61970/Base/Core#BaseVoltage_VoltageLevel

:BaseVoltage_VoltageLevel a owl:ObjectProperty ;
	owl:inverseOf :VoltageLevel_BaseVoltage ;
	a owl:FunctionalProperty ;
	rdfs:domain :BaseVoltage ;
	rdfs:range :VoltageLevel ;
	rdfs:comment "The voltage levels having this base voltage.The base voltage used for all equipment within the voltage level." .
# 
# https://w3id.org/netbeheer/IECCIM/TC57CIM/IEC61970/Base/Core#BaseVoltage_nominalVoltage

:BaseVoltage_nominalVoltage a owl:ObjectProperty ;
	rdfs:domain :BaseVoltage ;
	rdfs:range <https://w3id.org/netbeheer/IECCIM/TC57CIM/IEC61970/Base/Domain#Voltage> ;
	rdfs:comment """The power system resource's base voltage.
""" .
# 
# https://w3id.org/netbeheer/IECCIM/TC57CIM/IEC61970/Base/Core#Bay_Substation

:Bay_Substation a owl:ObjectProperty ;
	owl:inverseOf :Substation_Bays ;
	rdfs:domain :Bay ;
	rdfs:range :Substation ;
	rdfs:comment "Bays contained in the substation.Substation containing the bay." .
# 
# https://w3id.org/netbeheer/IECCIM/TC57CIM/IEC61970/Base/Core#Bay_VoltageLevel

:Bay_VoltageLevel a owl:ObjectProperty ;
	owl:inverseOf :VoltageLevel_Bays ;
	rdfs:domain :Bay ;
	rdfs:range :VoltageLevel ;
	rdfs:comment "The voltage level containing this bay.The bays within this voltage level." .
# 
# https://w3id.org/netbeheer/IECCIM/TC57CIM/IEC61970/Base/Core#BranchGroupTerminal_Terminal

:BranchGroupTerminal_Terminal a owl:ObjectProperty ;
	owl:inverseOf :Terminal_BranchGroupTerminal ;
	rdfs:domain <https://w3id.org/netbeheer/IECCIM/TC57CIM/IEC61970/Base/OperationalLimits#BranchGroupTerminal> ;
	rdfs:range :Terminal ;
	rdfs:comment "The directed branch group terminals for which this terminal is monitored. The terminal to be summed." .
# 
# https://w3id.org/netbeheer/IECCIM/TC57CIM/IEC61970/Base/Core#BusNameMarker_ReportingGroup

:BusNameMarker_ReportingGroup a owl:ObjectProperty ;
	owl:inverseOf :ReportingGroup_BusNameMarker ;
	rdfs:domain <https://w3id.org/netbeheer/IECCIM/TC57CIM/IEC61970/Base/Topology#BusNameMarker> ;
	rdfs:range :ReportingGroup ;
	rdfs:comment "The bus name markers that belong to this reporting group.The reporting group to which this bus name marker belongs." .
# 
# https://w3id.org/netbeheer/IECCIM/TC57CIM/IEC61970/Base/Core#BusNameMarker_Terminal

:BusNameMarker_Terminal a owl:ObjectProperty ;
	rdfs:domain <https://w3id.org/netbeheer/IECCIM/TC57CIM/IEC61970/Base/Topology#BusNameMarker> ;
	rdfs:range :ACDCTerminal ;
	rdfs:comment "The bus name marker used to name the bus (topological node).The terminals associated with this bus name marker." .
# 
# https://w3id.org/netbeheer/IECCIM/TC57CIM/IEC61970/Base/Core#Bushing_Terminal

:Bushing_Terminal a owl:ObjectProperty ;
	owl:inverseOf :Terminal_Bushing ;
	rdfs:domain <https://w3id.org/netbeheer/IECCIM/TC57CIM/IEC61968/InfIEC61968/InfAssets#Bushing> ;
	rdfs:range :Terminal ;
	rdfs:comment "" .
# 
# https://w3id.org/netbeheer/IECCIM/TC57CIM/IEC61970/Base/Core#CIMDataObject_PropertiesObject

:CIMDataObject_PropertiesObject a owl:ObjectProperty ;
	owl:inverseOf :IdentifiedObject_PropertiesCIMDataObject ;
	rdfs:domain <https://w3id.org/netbeheer/IECCIM/TC57CIM/IEC61970/InfIEC61970/InfGenericDataset/CanonicalModel/GenericDatasetCore#CIMDataObject> ;
	rdfs:range :IdentifiedObject ;
	rdfs:comment "The single CIM data object in the appropriate dataset context.The CIM object holding the properties of this dataset context.   Sometimes properties are not required and only the reference to the registered object is required." .
# 
# https://w3id.org/netbeheer/IECCIM/TC57CIM/IEC61970/Base/Core#CIMDataObject_RegisteredObject

:CIMDataObject_RegisteredObject a owl:ObjectProperty ;
	owl:inverseOf :IdentifiedObject_RegisteredCIMDataObject ;
	rdfs:domain <https://w3id.org/netbeheer/IECCIM/TC57CIM/IEC61970/InfIEC61970/InfGenericDataset/CanonicalModel/GenericDatasetCore#CIMDataObject> ;
	rdfs:range :IdentifiedObject ;
	rdfs:comment "Data objects registered.The registered CIM object." .
# 
# https://w3id.org/netbeheer/IECCIM/TC57CIM/IEC61970/Base/Core#ClearanceDocument_TaggedPSRs

:ClearanceDocument_TaggedPSRs a owl:ObjectProperty ;
	owl:inverseOf :PowerSystemResource_Clearances ;
	rdfs:domain <https://w3id.org/netbeheer/IECCIM/TC57CIM/IEC61968/Operations#ClearanceDocument> ;
	rdfs:range :PowerSystemResource ;
	rdfs:comment "All clearances applicable to this power system resource.All power system resources tagged through this clearance." .
# 
# https://w3id.org/netbeheer/IECCIM/TC57CIM/IEC61970/Base/Core#ConductingEquipment_BaseVoltage

:ConductingEquipment_BaseVoltage a owl:ObjectProperty ;
	rdfs:domain :ConductingEquipment ;
	rdfs:range :BaseVoltage ;
	rdfs:comment "Base voltage of this conducting equipment.  Use only when there is no voltage level container used and only one base voltage applies.  For example, not used for transformers.All conducting equipment with this base voltage.  Use only when there is no voltage level container used and only one base voltage applies.  For example, not used for transformers." .
# 
# https://w3id.org/netbeheer/IECCIM/TC57CIM/IEC61970/Base/Core#ConductingEquipment_GroundingAction

:ConductingEquipment_GroundingAction a owl:ObjectProperty ;
	owl:inverseOf :GroundAction_GroundedEquipment ;
	rdfs:domain :ConductingEquipment ;
	rdfs:range <https://w3id.org/netbeheer/IECCIM/TC57CIM/IEC61968/Operations#GroundAction> ;
	rdfs:comment "Action involving grounding operation on this conducting equipment.Equipment being grounded with this operation. In case of placing a ground anywhere along a line segment, you must use the clamp (to get the distance from one terminal), so use the explicit relation with line segment. In all other cases (including placing the ground at a line segment terminal), reference to one or more conducting equipment is sufficient." .
# 
# https://w3id.org/netbeheer/IECCIM/TC57CIM/IEC61970/Base/Core#ConductingEquipment_JumpingAction

:ConductingEquipment_JumpingAction a owl:ObjectProperty ;
	owl:inverseOf :JumperAction_JumpedEquipments ;
	rdfs:domain :ConductingEquipment ;
	rdfs:range <https://w3id.org/netbeheer/IECCIM/TC57CIM/IEC61968/Operations#JumperAction> ;
	rdfs:comment "Jumper action involving jumping operation on this conducting equipment.The conducting equipment that this jumper action will affect. In case of placing a jumper anywhere along a line segment, you must use the clamp (to get the distance from one terminal), so use the explicit relation with line segment. In all other cases (including placing the jumper at a line segment terminal), reference to one or more conducting equipment is sufficient." .
# 
# https://w3id.org/netbeheer/IECCIM/TC57CIM/IEC61970/Base/Core#ConductingEquipment_ProtectionEquipments

:ConductingEquipment_ProtectionEquipments a owl:ObjectProperty ;
	owl:inverseOf :ProtectionEquipment_ConductingEquipments ;
	rdfs:domain :ConductingEquipment ;
	rdfs:range <https://w3id.org/netbeheer/IECCIM/TC57CIM/IEC61970/Base/Protection#ProtectionEquipment> ;
	rdfs:comment "Protection equipment  used to protect specific conducting equipment. Protection equipment may be used to protect specific conducting equipment." .
# 
# https://w3id.org/netbeheer/IECCIM/TC57CIM/IEC61970/Base/Core#ConductingEquipment_ProtectiveActionAdjustment

:ConductingEquipment_ProtectiveActionAdjustment a owl:ObjectProperty ;
	owl:inverseOf :ProtectiveActionAdjustment_ConductingEquipment ;
	a owl:FunctionalProperty ;
	rdfs:domain :ConductingEquipment ;
	rdfs:range <https://w3id.org/netbeheer/IECCIM/TC57CIM/IEC61970/InfIEC61970/InfSIPS#ProtectiveActionAdjustment> ;
	rdfs:comment "The operating condition to the Conducting Equipment is changed when protective action adjustment is activated. For Shunt Compensator or other conducting equipment that operates on discrete values (integer), the values given in float will be rounded. The operating condition to the Conducting Equipment is changed when protective action adjustment is activated. For Shunt Compensator or other conducting equipment that operates on discrete values (integer), the values given in float will be rounded. " .
# 
# https://w3id.org/netbeheer/IECCIM/TC57CIM/IEC61970/Base/Core#ConductingEquipment_SvStatus

:ConductingEquipment_SvStatus a owl:ObjectProperty ;
	owl:inverseOf :SvStatus_ConductingEquipment ;
	a owl:FunctionalProperty ;
	rdfs:domain :ConductingEquipment ;
	rdfs:range <https://w3id.org/netbeheer/IECCIM/TC57CIM/IEC61970/Base/StateVariables#SvStatus> ;
	rdfs:comment "The status state variable associated with this conducting equipment.The conducting equipment associated with the status state variable." .
# 
# https://w3id.org/netbeheer/IECCIM/TC57CIM/IEC61970/Base/Core#ConductingEquipment_Terminals

:ConductingEquipment_Terminals a owl:ObjectProperty ;
	owl:inverseOf :Terminal_ConductingEquipment ;
	a owl:FunctionalProperty ;
	rdfs:domain :ConductingEquipment ;
	rdfs:range :Terminal ;
	rdfs:comment "Conducting equipment have terminals that may be connected to other conducting equipment terminals via connectivity nodes or topological nodes.The conducting equipment of the terminal.  Conducting equipment have  terminals that may be connected to other conducting equipment terminals via connectivity nodes or topological nodes." .
# 
# https://w3id.org/netbeheer/IECCIM/TC57CIM/IEC61970/Base/Core#ConnectivityNodeContainer_ConnectivityNodes

:ConnectivityNodeContainer_ConnectivityNodes a owl:ObjectProperty ;
	owl:inverseOf :ConnectivityNode_ConnectivityNodeContainer ;
	a owl:FunctionalProperty ;
	rdfs:domain :ConnectivityNodeContainer ;
	rdfs:range :ConnectivityNode ;
	rdfs:comment "Connectivity nodes which belong to this connectivity node container.Container of this connectivity node." .
# 
# https://w3id.org/netbeheer/IECCIM/TC57CIM/IEC61970/Base/Core#ConnectivityNodeContainer_TopologicalNode

:ConnectivityNodeContainer_TopologicalNode a owl:ObjectProperty ;
	owl:inverseOf :TopologicalNode_ConnectivityNodeContainer ;
	rdfs:domain :ConnectivityNodeContainer ;
	rdfs:range <https://w3id.org/netbeheer/IECCIM/TC57CIM/IEC61970/Base/Topology#TopologicalNode> ;
	rdfs:comment "The topological nodes which belong to this connectivity node container.The connectivity node container to which the toplogical node belongs." .
# 
# https://w3id.org/netbeheer/IECCIM/TC57CIM/IEC61970/Base/Core#ConnectivityNode_ConnectivityNodeContainer

:ConnectivityNode_ConnectivityNodeContainer a owl:ObjectProperty ;
	rdfs:domain :ConnectivityNode ;
	rdfs:range :ConnectivityNodeContainer ;
	rdfs:comment "Connectivity nodes which belong to this connectivity node container.Container of this connectivity node." .
# 
# https://w3id.org/netbeheer/IECCIM/TC57CIM/IEC61970/Base/Core#ConnectivityNode_Terminals

:ConnectivityNode_Terminals a owl:ObjectProperty ;
	owl:inverseOf :Terminal_ConnectivityNode ;
	rdfs:domain :ConnectivityNode ;
	rdfs:range :Terminal ;
	rdfs:comment "Terminals interconnected with zero impedance at a this connectivity node. The connectivity node to which this terminal connects with zero impedance." .
# 
# https://w3id.org/netbeheer/IECCIM/TC57CIM/IEC61970/Base/Core#ConnectivityNode_TopologicalNode

:ConnectivityNode_TopologicalNode a owl:ObjectProperty ;
	owl:inverseOf :TopologicalNode_ConnectivityNodes ;
	rdfs:domain :ConnectivityNode ;
	rdfs:range <https://w3id.org/netbeheer/IECCIM/TC57CIM/IEC61970/Base/Topology#TopologicalNode> ;
	rdfs:comment "The connectivity nodes combine together to form this topological node.  May depend on the current state of switches in the network.The topological node to which this connectivity node is assigned.  May depend on the current state of switches in the network." .
# 
# https://w3id.org/netbeheer/IECCIM/TC57CIM/IEC61970/Base/Core#ContingencyEquipment_Equipment

:ContingencyEquipment_Equipment a owl:ObjectProperty ;
	owl:inverseOf :Equipment_ContingencyEquipment ;
	rdfs:domain <https://w3id.org/netbeheer/IECCIM/TC57CIM/IEC61970/Base/Contingency#ContingencyEquipment> ;
	rdfs:range :Equipment ;
	rdfs:comment "The contingency equipments in which this equipment participates.The single piece of equipment to which to apply the contingency." .
# 
# https://w3id.org/netbeheer/IECCIM/TC57CIM/IEC61970/Base/Core#Control_PowerSystemResource

:Control_PowerSystemResource a owl:ObjectProperty ;
	owl:inverseOf :PowerSystemResource_Controls ;
	rdfs:domain <https://w3id.org/netbeheer/IECCIM/TC57CIM/IEC61970/Base/Meas#Control> ;
	rdfs:range :PowerSystemResource ;
	rdfs:comment "Regulating device governed by this control output.The controller outputs used to actually govern a regulating device, e.g. the magnetization of a synchronous machine or capacitor bank breaker actuator." .
# 
# https://w3id.org/netbeheer/IECCIM/TC57CIM/IEC61970/Base/Core#CurveData_Curve

:CurveData_Curve a owl:ObjectProperty ;
	owl:inverseOf :Curve_CurveDatas ;
	rdfs:domain :CurveData ;
	rdfs:range :Curve ;
	rdfs:comment "The point data values that define this curve.The curve of  this curve data point." .
# 
# https://w3id.org/netbeheer/IECCIM/TC57CIM/IEC61970/Base/Core#Curve_CurveDatas

:Curve_CurveDatas a owl:ObjectProperty , owl:FunctionalProperty ;
	rdfs:domain :Curve ;
	rdfs:range :CurveData ;
	rdfs:comment "The point data values that define this curve.The curve of  this curve data point." .
# 
# https://w3id.org/netbeheer/IECCIM/TC57CIM/IEC61970/Base/Core#DCConverterUnit_Substation

:DCConverterUnit_Substation a owl:ObjectProperty ;
	owl:inverseOf :Substation_DCConverterUnit ;
	rdfs:domain <https://w3id.org/netbeheer/IECCIM/TC57CIM/IEC61970/Base/DC#DCConverterUnit> ;
	rdfs:range :Substation ;
	rdfs:comment "The DC converter unit belonging ot the substation.The containing substation of the DC converter unit." .
# 
# https://w3id.org/netbeheer/IECCIM/TC57CIM/IEC61970/Base/Core#DCLine_Region

:DCLine_Region a owl:ObjectProperty ;
	owl:inverseOf :SubGeographicalRegion_DCLines ;
	rdfs:domain <https://w3id.org/netbeheer/IECCIM/TC57CIM/IEC61970/Base/DC#DCLine> ;
	rdfs:range :SubGeographicalRegion ;
	rdfs:comment "" .
# 
# https://w3id.org/netbeheer/IECCIM/TC57CIM/IEC61970/Base/Core#DiagramObject_IdentifiedObject

:DiagramObject_IdentifiedObject a owl:ObjectProperty ;
	owl:inverseOf :IdentifiedObject_DiagramObjects ;
	rdfs:domain <https://w3id.org/netbeheer/IECCIM/TC57CIM/IEC61970/Base/DiagramLayout#DiagramObject> ;
	rdfs:range :IdentifiedObject ;
	rdfs:comment "The domain object to which this diagram object is associated.The diagram objects that are associated with the domain object." .
# 
# https://w3id.org/netbeheer/IECCIM/TC57CIM/IEC61970/Base/Core#EquipmentContainer_Equipments

:EquipmentContainer_Equipments a owl:ObjectProperty ;
	owl:inverseOf :Equipment_EquipmentContainer ;
	rdfs:domain :EquipmentContainer ;
	rdfs:range :Equipment ;
	rdfs:comment "Container of this equipment.Contained equipment." .
# 
# https://w3id.org/netbeheer/IECCIM/TC57CIM/IEC61970/Base/Core#EquipmentLimitSeriesComponent_Equipment

:EquipmentLimitSeriesComponent_Equipment a owl:ObjectProperty ;
	owl:inverseOf :Equipment_EqiupmentLimitSeriesComponent ;
	rdfs:domain <https://w3id.org/netbeheer/IECCIM/TC57CIM/IEC61970/InfIEC61970/InfOperationalLimits#EquipmentLimitSeriesComponent> ;
	rdfs:range :Equipment ;
	rdfs:comment "Equipment limit series calculation component to which this equipment contributes.Equipment contributing toward the series limit.   The reference here is to Equipment rather than a specific limit on the equipment so the grouiping can be reused for multiple limits of different types on the same instance of equipment." .
# 
# https://w3id.org/netbeheer/IECCIM/TC57CIM/IEC61970/Base/Core#Equipment_ContingencyEquipment

:Equipment_ContingencyEquipment a owl:ObjectProperty , owl:FunctionalProperty ;
	rdfs:domain :Equipment ;
	rdfs:range <https://w3id.org/netbeheer/IECCIM/TC57CIM/IEC61970/Base/Contingency#ContingencyEquipment> ;
	rdfs:comment "The contingency equipments in which this equipment participates.The single piece of equipment to which to apply the contingency." .
# 
# https://w3id.org/netbeheer/IECCIM/TC57CIM/IEC61970/Base/Core#Equipment_EqiupmentLimitSeriesComponent

:Equipment_EqiupmentLimitSeriesComponent a owl:ObjectProperty , owl:FunctionalProperty ;
	rdfs:domain :Equipment ;
	rdfs:range <https://w3id.org/netbeheer/IECCIM/TC57CIM/IEC61970/InfIEC61970/InfOperationalLimits#EquipmentLimitSeriesComponent> ;
	rdfs:comment "Equipment limit series calculation component to which this equipment contributes.Equipment contributing toward the series limit.   The reference here is to Equipment rather than a specific limit on the equipment so the grouiping can be reused for multiple limits of different types on the same instance of equipment." .
# 
# https://w3id.org/netbeheer/IECCIM/TC57CIM/IEC61970/Base/Core#Equipment_EquipmentContainer

:Equipment_EquipmentContainer a owl:ObjectProperty ;
	rdfs:domain :Equipment ;
	rdfs:range :EquipmentContainer ;
	rdfs:comment "Container of this equipment.Contained equipment." .
# 
# https://w3id.org/netbeheer/IECCIM/TC57CIM/IEC61970/Base/Core#Equipment_LimitDependencyModel

:Equipment_LimitDependencyModel a owl:ObjectProperty ;
	owl:inverseOf :LimitDependency_Equipment ;
	rdfs:domain :Equipment ;
	rdfs:range <https://w3id.org/netbeheer/IECCIM/TC57CIM/IEC61970/InfIEC61970/InfOperationalLimits#LimitDependency> ;
	rdfs:comment "Limit dependencymodels organized under this equipment as a means for organizing the model in a tree view.The equipment for which this limit dependency model is organized under." .
# 
# https://w3id.org/netbeheer/IECCIM/TC57CIM/IEC61970/Base/Core#Equipment_OperationalLimitSet

:Equipment_OperationalLimitSet a owl:ObjectProperty ;
	owl:inverseOf :OperationalLimitSet_Equipment ;
	rdfs:domain :Equipment ;
	rdfs:range <https://w3id.org/netbeheer/IECCIM/TC57CIM/IEC61970/Base/OperationalLimits#OperationalLimitSet> ;
	rdfs:comment "The operational limit sets associated with this equipment.The equipment to which the limit set applies." .
# 
# https://w3id.org/netbeheer/IECCIM/TC57CIM/IEC61970/Base/Core#Equipment_OperationalRestrictions

:Equipment_OperationalRestrictions a owl:ObjectProperty ;
	owl:inverseOf :OperationalRestriction_Equipments ;
	rdfs:domain :Equipment ;
	rdfs:range <https://w3id.org/netbeheer/IECCIM/TC57CIM/IEC61968/Operations#OperationalRestriction> ;
	rdfs:comment "All operational restrictions for this equipment.All equipments to which this restriction applies." .
# 
# https://w3id.org/netbeheer/IECCIM/TC57CIM/IEC61970/Base/Core#Equipment_Outages

:Equipment_Outages a owl:ObjectProperty ;
	owl:inverseOf :Outage_Equipments ;
	rdfs:domain :Equipment ;
	rdfs:range <https://w3id.org/netbeheer/IECCIM/TC57CIM/IEC61968/Operations#Outage> ;
	rdfs:comment "All outages in which this equipment is involved.All equipments associated with this outage." .
# 
# https://w3id.org/netbeheer/IECCIM/TC57CIM/IEC61970/Base/Core#Equipment_PinEquipment

:Equipment_PinEquipment a owl:ObjectProperty ;
	owl:inverseOf :PinEquipment_Equipment ;
	a owl:FunctionalProperty ;
	rdfs:domain :Equipment ;
	rdfs:range <https://w3id.org/netbeheer/IECCIM/TC57CIM/IEC61970/InfIEC61970/InfSIPS#PinEquipment> ;
	rdfs:comment "" .
# 
# https://w3id.org/netbeheer/IECCIM/TC57CIM/IEC61970/Base/Core#Equipment_ProtectiveActionEquipment

:Equipment_ProtectiveActionEquipment a owl:ObjectProperty ;
	owl:inverseOf :ProtectiveActionEquipment_Equipment ;
	a owl:FunctionalProperty ;
	rdfs:domain :Equipment ;
	rdfs:range <https://w3id.org/netbeheer/IECCIM/TC57CIM/IEC61970/InfIEC61970/InfSIPS#ProtectiveActionEquipment> ;
	rdfs:comment "" .
# 
# https://w3id.org/netbeheer/IECCIM/TC57CIM/IEC61970/Base/Core#Equipment_UsagePoints

:Equipment_UsagePoints a owl:ObjectProperty ;
	owl:inverseOf :UsagePoint_Equipments ;
	rdfs:domain :Equipment ;
	rdfs:range <https://w3id.org/netbeheer/IECCIM/TC57CIM/IEC61968/Metering#UsagePoint> ;
	rdfs:comment "All usage points connected to the electrical grid through this equipment.All equipment connecting this usage point to the electrical grid." .
# 
# https://w3id.org/netbeheer/IECCIM/TC57CIM/IEC61970/Base/Core#Equipment_WeatherStation

:Equipment_WeatherStation a owl:ObjectProperty ;
	owl:inverseOf :WeatherStation_Equipment ;
	rdfs:domain :Equipment ;
	rdfs:range <https://w3id.org/netbeheer/IECCIM/TC57CIM/IEC61970/InfIEC61970/InfOperationalLimits#WeatherStation> ;
	rdfs:comment "" .
# 
# https://w3id.org/netbeheer/IECCIM/TC57CIM/IEC61970/Base/Core#GeographicalRegion_Regions

:GeographicalRegion_Regions a owl:ObjectProperty ;
	owl:inverseOf :SubGeographicalRegion_Region ;
	rdfs:domain :GeographicalRegion ;
	rdfs:range :SubGeographicalRegion ;
	rdfs:comment "The geographical region to which this sub-geographical region is within.All sub-geograhpical regions within this geographical region." .
# 
# https://w3id.org/netbeheer/IECCIM/TC57CIM/IEC61970/Base/Core#GroundAction_GroundedEquipment

:GroundAction_GroundedEquipment a owl:ObjectProperty ;
	rdfs:domain <https://w3id.org/netbeheer/IECCIM/TC57CIM/IEC61968/Operations#GroundAction> ;
	rdfs:range :ConductingEquipment ;
	rdfs:comment "Action involving grounding operation on this conducting equipment.Equipment being grounded with this operation. In case of placing a ground anywhere along a line segment, you must use the clamp (to get the distance from one terminal), so use the explicit relation with line segment. In all other cases (including placing the ground at a line segment terminal), reference to one or more conducting equipment is sufficient." .
# 
# https://w3id.org/netbeheer/IECCIM/TC57CIM/IEC61970/Base/Core#IdentifiedObject_DiagramObjects

:IdentifiedObject_DiagramObjects a owl:ObjectProperty ;
	rdfs:domain :IdentifiedObject ;
	rdfs:range <https://w3id.org/netbeheer/IECCIM/TC57CIM/IEC61970/Base/DiagramLayout#DiagramObject> ;
	rdfs:comment "The domain object to which this diagram object is associated.The diagram objects that are associated with the domain object." .
# 
# https://w3id.org/netbeheer/IECCIM/TC57CIM/IEC61970/Base/Core#IdentifiedObject_Names

:IdentifiedObject_Names a owl:ObjectProperty ;
	owl:inverseOf :Name_IdentifiedObject ;
	a owl:FunctionalProperty ;
	rdfs:domain :IdentifiedObject ;
	rdfs:range :Name ;
	rdfs:comment "All names of this identified object.Identified object that this name designates." .
# 
# https://w3id.org/netbeheer/IECCIM/TC57CIM/IEC61970/Base/Core#IdentifiedObject_PropertiesCIMDataObject

:IdentifiedObject_PropertiesCIMDataObject a owl:ObjectProperty ;
	rdfs:domain :IdentifiedObject ;
	rdfs:range <https://w3id.org/netbeheer/IECCIM/TC57CIM/IEC61970/InfIEC61970/InfGenericDataset/CanonicalModel/GenericDatasetCore#CIMDataObject> ;
	rdfs:comment "The single CIM data object in the appropriate dataset context.The CIM object holding the properties of this dataset context.   Sometimes properties are not required and only the reference to the registered object is required." .
# 
# https://w3id.org/netbeheer/IECCIM/TC57CIM/IEC61970/Base/Core#IdentifiedObject_RegisteredCIMDataObject

:IdentifiedObject_RegisteredCIMDataObject a owl:ObjectProperty , owl:FunctionalProperty ;
	rdfs:domain :IdentifiedObject ;
	rdfs:range <https://w3id.org/netbeheer/IECCIM/TC57CIM/IEC61970/InfIEC61970/InfGenericDataset/CanonicalModel/GenericDatasetCore#CIMDataObject> ;
	rdfs:comment "Data objects registered.The registered CIM object." .
# 
# https://w3id.org/netbeheer/IECCIM/TC57CIM/IEC61970/Base/Core#IrregularIntervalSchedule_TimePoints

:IrregularIntervalSchedule_TimePoints a owl:ObjectProperty ;
	owl:inverseOf :IrregularTimePoint_IntervalSchedule ;
	a owl:FunctionalProperty ;
	rdfs:domain :IrregularIntervalSchedule ;
	rdfs:range :IrregularTimePoint ;
	rdfs:comment "An IrregularTimePoint belongs to an IrregularIntervalSchedule.The point data values that define a curve." .
# 
# https://w3id.org/netbeheer/IECCIM/TC57CIM/IEC61970/Base/Core#IrregularTimePoint_IntervalSchedule

:IrregularTimePoint_IntervalSchedule a owl:ObjectProperty ;
	rdfs:domain :IrregularTimePoint ;
	rdfs:range :IrregularIntervalSchedule ;
	rdfs:comment "An IrregularTimePoint belongs to an IrregularIntervalSchedule.The point data values that define a curve." .
# 
# https://w3id.org/netbeheer/IECCIM/TC57CIM/IEC61970/Base/Core#IrregularTimePoint_time

:IrregularTimePoint_time a owl:ObjectProperty ;
	rdfs:domain :IrregularTimePoint ;
	rdfs:range <https://w3id.org/netbeheer/IECCIM/TC57CIM/IEC61970/Base/Domain#Seconds> ;
	rdfs:comment """The time is relative to the schedule starting time.

""" .
# 
# https://w3id.org/netbeheer/IECCIM/TC57CIM/IEC61970/Base/Core#JumperAction_JumpedEquipments

:JumperAction_JumpedEquipments a owl:ObjectProperty ;
	rdfs:domain <https://w3id.org/netbeheer/IECCIM/TC57CIM/IEC61968/Operations#JumperAction> ;
	rdfs:range :ConductingEquipment ;
	rdfs:comment "Jumper action involving jumping operation on this conducting equipment.The conducting equipment that this jumper action will affect. In case of placing a jumper anywhere along a line segment, you must use the clamp (to get the distance from one terminal), so use the explicit relation with line segment. In all other cases (including placing the jumper at a line segment terminal), reference to one or more conducting equipment is sufficient." .
# 
# https://w3id.org/netbeheer/IECCIM/TC57CIM/IEC61970/Base/Core#LimitDependency_Equipment

:LimitDependency_Equipment a owl:ObjectProperty ;
	rdfs:domain <https://w3id.org/netbeheer/IECCIM/TC57CIM/IEC61970/InfIEC61970/InfOperationalLimits#LimitDependency> ;
	rdfs:range :Equipment ;
	rdfs:comment "Limit dependencymodels organized under this equipment as a means for organizing the model in a tree view.The equipment for which this limit dependency model is organized under." .
# 
# https://w3id.org/netbeheer/IECCIM/TC57CIM/IEC61970/Base/Core#Line_Region

:Line_Region a owl:ObjectProperty ;
	owl:inverseOf :SubGeographicalRegion_Lines ;
	rdfs:domain <https://w3id.org/netbeheer/IECCIM/TC57CIM/IEC61970/Base/Wires#Line> ;
	rdfs:range :SubGeographicalRegion ;
	rdfs:comment "The sub-geographical region of the line.The lines within the sub-geographical region." .
# 
# https://w3id.org/netbeheer/IECCIM/TC57CIM/IEC61970/Base/Core#Location_PowerSystemResources

:Location_PowerSystemResources a owl:ObjectProperty ;
	owl:inverseOf :PowerSystemResource_Location ;
	rdfs:domain <https://w3id.org/netbeheer/IECCIM/TC57CIM/IEC61968/Common#Location> ;
	rdfs:range :PowerSystemResource ;
	rdfs:comment "Location of this power system resource.All power system resources at this location." .
# 
# https://w3id.org/netbeheer/IECCIM/TC57CIM/IEC61970/Base/Core#Measure_PowerSystemResource

:Measure_PowerSystemResource a owl:ObjectProperty ;
	owl:inverseOf :PowerSystemResource_Measurements ;
	rdfs:domain <https://w3id.org/netbeheer/IECCIM/TC57CIM/IEC61970/Base/Meas#Measure> ;
	rdfs:range :PowerSystemResource ;
	rdfs:comment "The power system resource that contains the measurement.The measurements associated with this power system resource." .
# 
# https://w3id.org/netbeheer/IECCIM/TC57CIM/IEC61970/Base/Core#Measure_Terminal

:Measure_Terminal a owl:ObjectProperty ;
	rdfs:domain <https://w3id.org/netbeheer/IECCIM/TC57CIM/IEC61970/Base/Meas#Measure> ;
	rdfs:range :ACDCTerminal ;
	rdfs:comment "Measurements associated with this terminal defining  where the measurement is placed in the network topology.  It may be used, for instance, to capture the sensor position, such as a voltage transformer (PT) at a busbar or a current transformer (CT) at the bar between a breaker and an isolator.One or more measurements may be associated with a terminal in the network." .
# 
# https://w3id.org/netbeheer/IECCIM/TC57CIM/IEC61970/Base/Core#MutualCoupling_First_Terminal

:MutualCoupling_First_Terminal a owl:ObjectProperty ;
	owl:inverseOf :Terminal_HasFirstMutualCoupling ;
	rdfs:domain <https://w3id.org/netbeheer/IECCIM/TC57CIM/IEC61970/Base/Wires#MutualCoupling> ;
	rdfs:range :Terminal ;
	rdfs:comment "Mutual couplings associated with the branch as the first branch.The starting terminal for the calculation of distances along the first branch of the mutual coupling.  Normally MutualCoupling would only be used for terminals of AC line segments.  The first and second terminals of a mutual coupling should point to different AC line segments." .
# 
# https://w3id.org/netbeheer/IECCIM/TC57CIM/IEC61970/Base/Core#MutualCoupling_Second_Terminal

:MutualCoupling_Second_Terminal a owl:ObjectProperty ;
	owl:inverseOf :Terminal_HasSecondMutualCoupling ;
	rdfs:domain <https://w3id.org/netbeheer/IECCIM/TC57CIM/IEC61970/Base/Wires#MutualCoupling> ;
	rdfs:range :Terminal ;
	rdfs:comment "Mutual couplings with the branch associated as the first branch.The starting terminal for the calculation of distances along the second branch of the mutual coupling." .
# 
# https://w3id.org/netbeheer/IECCIM/TC57CIM/IEC61970/Base/Core#NameTypeAuthority_NameTypes

:NameTypeAuthority_NameTypes a owl:ObjectProperty ;
	owl:inverseOf :NameType_NameTypeAuthority ;
	rdfs:domain :NameTypeAuthority ;
	rdfs:range :NameType ;
	rdfs:comment "All name types managed by this authority.Authority responsible for managing names of this type." .
# 
# https://w3id.org/netbeheer/IECCIM/TC57CIM/IEC61970/Base/Core#NameType_NameTypeAuthority

:NameType_NameTypeAuthority a owl:ObjectProperty ;
	rdfs:domain :NameType ;
	rdfs:range :NameTypeAuthority ;
	rdfs:comment "All name types managed by this authority.Authority responsible for managing names of this type." .
# 
# https://w3id.org/netbeheer/IECCIM/TC57CIM/IEC61970/Base/Core#NameType_Names

:NameType_Names a owl:ObjectProperty ;
	owl:inverseOf :Name_NameType ;
	a owl:FunctionalProperty ;
	rdfs:domain :NameType ;
	rdfs:range :Name ;
	rdfs:comment "All names of this type.Type of this name." .
# 
# https://w3id.org/netbeheer/IECCIM/TC57CIM/IEC61970/Base/Core#Name_IdentifiedObject

:Name_IdentifiedObject a owl:ObjectProperty ;
	rdfs:domain :Name ;
	rdfs:range :IdentifiedObject ;
	rdfs:comment "All names of this identified object.Identified object that this name designates." .
# 
# https://w3id.org/netbeheer/IECCIM/TC57CIM/IEC61970/Base/Core#Name_NameType

:Name_NameType a owl:ObjectProperty ;
	rdfs:domain :Name ;
	rdfs:range :NameType ;
	rdfs:comment "All names of this type.Type of this name." .
# 
# https://w3id.org/netbeheer/IECCIM/TC57CIM/IEC61970/Base/Core#OperatingParticipant_OperatingShare

:OperatingParticipant_OperatingShare a owl:ObjectProperty ;
	owl:inverseOf :OperatingShare_OperatingParticipant ;
	a owl:FunctionalProperty ;
	rdfs:domain :OperatingParticipant ;
	rdfs:range :OperatingShare ;
	rdfs:comment "The operating shares of this operating participant.  An operating participant can be resused for any number of power system resources.The operating participant having this share with the associated power system resource." .
# 
# https://w3id.org/netbeheer/IECCIM/TC57CIM/IEC61970/Base/Core#OperatingShare_OperatingParticipant

:OperatingShare_OperatingParticipant a owl:ObjectProperty ;
	rdfs:domain :OperatingShare ;
	rdfs:range :OperatingParticipant ;
	rdfs:comment "The operating shares of this operating participant.  An operating participant can be resused for any number of power system resources.The operating participant having this share with the associated power system resource." .
# 
# https://w3id.org/netbeheer/IECCIM/TC57CIM/IEC61970/Base/Core#OperatingShare_PowerSystemResource

:OperatingShare_PowerSystemResource a owl:ObjectProperty ;
	owl:inverseOf :PowerSystemResource_OperatingShare ;
	rdfs:domain :OperatingShare ;
	rdfs:range :PowerSystemResource ;
	rdfs:comment "The operating shares of this power system resource.The power system resource to which the share applies." .
# 
# https://w3id.org/netbeheer/IECCIM/TC57CIM/IEC61970/Base/Core#OperatingShare_percentage

:OperatingShare_percentage a owl:ObjectProperty ;
	rdfs:domain :OperatingShare ;
	rdfs:range <https://w3id.org/netbeheer/IECCIM/TC57CIM/IEC61970/Base/Domain#PerCent> ;
	rdfs:comment """Percentage operational ownership between the pair (power system resource and operatging participant) associated with this share. The total percentage ownership for a power system resource should add to 100%.
""" .
# 
# https://w3id.org/netbeheer/IECCIM/TC57CIM/IEC61970/Base/Core#OperationalLimitSet_Equipment

:OperationalLimitSet_Equipment a owl:ObjectProperty ;
	rdfs:domain <https://w3id.org/netbeheer/IECCIM/TC57CIM/IEC61970/Base/OperationalLimits#OperationalLimitSet> ;
	rdfs:range :Equipment ;
	rdfs:comment "The operational limit sets associated with this equipment.The equipment to which the limit set applies." .
# 
# https://w3id.org/netbeheer/IECCIM/TC57CIM/IEC61970/Base/Core#OperationalLimitSet_Terminal

:OperationalLimitSet_Terminal a owl:ObjectProperty ;
	rdfs:domain <https://w3id.org/netbeheer/IECCIM/TC57CIM/IEC61970/Base/OperationalLimits#OperationalLimitSet> ;
	rdfs:range :ACDCTerminal ;
	rdfs:comment "" .
# 
# https://w3id.org/netbeheer/IECCIM/TC57CIM/IEC61970/Base/Core#OperationalRestriction_Equipments

:OperationalRestriction_Equipments a owl:ObjectProperty ;
	rdfs:domain <https://w3id.org/netbeheer/IECCIM/TC57CIM/IEC61968/Operations#OperationalRestriction> ;
	rdfs:range :Equipment ;
	rdfs:comment "All operational restrictions for this equipment.All equipments to which this restriction applies." .
# 
# https://w3id.org/netbeheer/IECCIM/TC57CIM/IEC61970/Base/Core#OperationalTag_PowerSystemResource

:OperationalTag_PowerSystemResource a owl:ObjectProperty ;
	owl:inverseOf :PowerSystemResource_OperationalTags ;
	rdfs:domain <https://w3id.org/netbeheer/IECCIM/TC57CIM/IEC61968/Operations#OperationalTag> ;
	rdfs:range :PowerSystemResource ;
	rdfs:comment "All operational tags placed on this power system resource.Power system resource on which this tag has been placed." .
# 
# https://w3id.org/netbeheer/IECCIM/TC57CIM/IEC61970/Base/Core#Outage_Equipments

:Outage_Equipments a owl:ObjectProperty ;
	rdfs:domain <https://w3id.org/netbeheer/IECCIM/TC57CIM/IEC61968/Operations#Outage> ;
	rdfs:range :Equipment ;
	rdfs:comment "All outages in which this equipment is involved.All equipments associated with this outage." .
# 
# https://w3id.org/netbeheer/IECCIM/TC57CIM/IEC61970/Base/Core#PSREvent_PowerSystemResource

:PSREvent_PowerSystemResource a owl:ObjectProperty ;
	owl:inverseOf :PowerSystemResource_PSREvents ;
	rdfs:domain <https://w3id.org/netbeheer/IECCIM/TC57CIM/IEC61968/Operations#PSREvent> ;
	rdfs:range :PowerSystemResource ;
	rdfs:comment "All events associated with this power system resource.Power system resource that generated this event." .
# 
# https://w3id.org/netbeheer/IECCIM/TC57CIM/IEC61970/Base/Core#PSRType_PowerSystemResources

:PSRType_PowerSystemResources a owl:ObjectProperty ;
	owl:inverseOf :PowerSystemResource_PSRType ;
	rdfs:domain :PSRType ;
	rdfs:range :PowerSystemResource ;
	rdfs:comment "Power system resources classified with this power system resource type.Custom classification for this power system resource." .
# 
# https://w3id.org/netbeheer/IECCIM/TC57CIM/IEC61970/Base/Core#PinEquipment_Equipment

:PinEquipment_Equipment a owl:ObjectProperty ;
	rdfs:domain <https://w3id.org/netbeheer/IECCIM/TC57CIM/IEC61970/InfIEC61970/InfSIPS#PinEquipment> ;
	rdfs:range :Equipment ;
	rdfs:comment "" .
# 
# https://w3id.org/netbeheer/IECCIM/TC57CIM/IEC61970/Base/Core#PinTerminal_Terminal

:PinTerminal_Terminal a owl:ObjectProperty ;
	owl:inverseOf :Terminal_PinTerminal ;
	rdfs:domain <https://w3id.org/netbeheer/IECCIM/TC57CIM/IEC61970/InfIEC61970/InfSIPS#PinTerminal> ;
	rdfs:range :Terminal ;
	rdfs:comment "" .
# 
# https://w3id.org/netbeheer/IECCIM/TC57CIM/IEC61970/Base/Core#PowerSystemResource_AssetDatasheet

:PowerSystemResource_AssetDatasheet a owl:ObjectProperty ;
	rdfs:domain :PowerSystemResource ;
	rdfs:range <https://w3id.org/netbeheer/IECCIM/TC57CIM/IEC61968/Assets#AssetInfo> ;
	rdfs:comment "Datasheet information for this power system resource.All power system resources with this datasheet information." .
# 
# https://w3id.org/netbeheer/IECCIM/TC57CIM/IEC61970/Base/Core#PowerSystemResource_Assets

:PowerSystemResource_Assets a owl:ObjectProperty ;
	rdfs:domain :PowerSystemResource ;
	rdfs:range <https://w3id.org/netbeheer/IECCIM/TC57CIM/IEC61968/Assets#Asset> ;
	rdfs:comment "All assets represented by this power system resource. For example, multiple conductor assets are electrically modelled as a single AC line segment.All power system resources used to electrically model this asset. For example, transformer asset is electrically modelled with a transformer and its windings and tap changer." .
# 
# https://w3id.org/netbeheer/IECCIM/TC57CIM/IEC61970/Base/Core#PowerSystemResource_Clearances

:PowerSystemResource_Clearances a owl:ObjectProperty ;
	rdfs:domain :PowerSystemResource ;
	rdfs:range <https://w3id.org/netbeheer/IECCIM/TC57CIM/IEC61968/Operations#ClearanceDocument> ;
	rdfs:comment "All clearances applicable to this power system resource.All power system resources tagged through this clearance." .
# 
# https://w3id.org/netbeheer/IECCIM/TC57CIM/IEC61970/Base/Core#PowerSystemResource_Controls

:PowerSystemResource_Controls a owl:ObjectProperty ;
	rdfs:domain :PowerSystemResource ;
	rdfs:range <https://w3id.org/netbeheer/IECCIM/TC57CIM/IEC61970/Base/Meas#Control> ;
	rdfs:comment "Regulating device governed by this control output.The controller outputs used to actually govern a regulating device, e.g. the magnetization of a synchronous machine or capacitor bank breaker actuator." .
# 
# https://w3id.org/netbeheer/IECCIM/TC57CIM/IEC61970/Base/Core#PowerSystemResource_Location

:PowerSystemResource_Location a owl:ObjectProperty ;
	rdfs:domain :PowerSystemResource ;
	rdfs:range <https://w3id.org/netbeheer/IECCIM/TC57CIM/IEC61968/Common#Location> ;
	rdfs:comment "Location of this power system resource.All power system resources at this location." .
# 
# https://w3id.org/netbeheer/IECCIM/TC57CIM/IEC61970/Base/Core#PowerSystemResource_Measurements

:PowerSystemResource_Measurements a owl:ObjectProperty ;
	rdfs:domain :PowerSystemResource ;
	rdfs:range <https://w3id.org/netbeheer/IECCIM/TC57CIM/IEC61970/Base/Meas#Measure> ;
	rdfs:comment "The power system resource that contains the measurement.The measurements associated with this power system resource." .
# 
# https://w3id.org/netbeheer/IECCIM/TC57CIM/IEC61970/Base/Core#PowerSystemResource_OperatingShare

:PowerSystemResource_OperatingShare a owl:ObjectProperty , owl:FunctionalProperty ;
	rdfs:domain :PowerSystemResource ;
	rdfs:range :OperatingShare ;
	rdfs:comment "The operating shares of this power system resource.The power system resource to which the share applies." .
# 
# https://w3id.org/netbeheer/IECCIM/TC57CIM/IEC61970/Base/Core#PowerSystemResource_OperationalTags

:PowerSystemResource_OperationalTags a owl:ObjectProperty ;
	rdfs:domain :PowerSystemResource ;
	rdfs:range <https://w3id.org/netbeheer/IECCIM/TC57CIM/IEC61968/Operations#OperationalTag> ;
	rdfs:comment "All operational tags placed on this power system resource.Power system resource on which this tag has been placed." .
# 
# https://w3id.org/netbeheer/IECCIM/TC57CIM/IEC61970/Base/Core#PowerSystemResource_PSREvents

:PowerSystemResource_PSREvents a owl:ObjectProperty ;
	rdfs:domain :PowerSystemResource ;
	rdfs:range <https://w3id.org/netbeheer/IECCIM/TC57CIM/IEC61968/Operations#PSREvent> ;
	rdfs:comment "All events associated with this power system resource.Power system resource that generated this event." .
# 
# https://w3id.org/netbeheer/IECCIM/TC57CIM/IEC61970/Base/Core#PowerSystemResource_PSRType

:PowerSystemResource_PSRType a owl:ObjectProperty ;
	rdfs:domain :PowerSystemResource ;
	rdfs:range :PSRType ;
	rdfs:comment "Power system resources classified with this power system resource type.Custom classification for this power system resource." .
# 
# https://w3id.org/netbeheer/IECCIM/TC57CIM/IEC61970/Base/Core#PowerSystemResource_ReportingGroup

:PowerSystemResource_ReportingGroup a owl:ObjectProperty ;
	owl:inverseOf :ReportingGroup_PowerSystemResource ;
	rdfs:domain :PowerSystemResource ;
	rdfs:range :ReportingGroup ;
	rdfs:comment "Reporting groups to which this power system resource belongs.Power system resources which belong to this reporting group." .
# 
# https://w3id.org/netbeheer/IECCIM/TC57CIM/IEC61970/Base/Core#ProtectionEquipment_ConductingEquipments

:ProtectionEquipment_ConductingEquipments a owl:ObjectProperty ;
	rdfs:domain <https://w3id.org/netbeheer/IECCIM/TC57CIM/IEC61970/Base/Protection#ProtectionEquipment> ;
	rdfs:range :ConductingEquipment ;
	rdfs:comment "Protection equipment  used to protect specific conducting equipment. Protection equipment may be used to protect specific conducting equipment." .
# 
# https://w3id.org/netbeheer/IECCIM/TC57CIM/IEC61970/Base/Core#ProtectiveActionAdjustment_ConductingEquipment

:ProtectiveActionAdjustment_ConductingEquipment a owl:ObjectProperty ;
	rdfs:domain <https://w3id.org/netbeheer/IECCIM/TC57CIM/IEC61970/InfIEC61970/InfSIPS#ProtectiveActionAdjustment> ;
	rdfs:range :ConductingEquipment ;
	rdfs:comment "The operating condition to the Conducting Equipment is changed when protective action adjustment is activated. For Shunt Compensator or other conducting equipment that operates on discrete values (integer), the values given in float will be rounded. The operating condition to the Conducting Equipment is changed when protective action adjustment is activated. For Shunt Compensator or other conducting equipment that operates on discrete values (integer), the values given in float will be rounded. " .
# 
# https://w3id.org/netbeheer/IECCIM/TC57CIM/IEC61970/Base/Core#ProtectiveActionEquipment_Equipment

:ProtectiveActionEquipment_Equipment a owl:ObjectProperty ;
	rdfs:domain <https://w3id.org/netbeheer/IECCIM/TC57CIM/IEC61970/InfIEC61970/InfSIPS#ProtectiveActionEquipment> ;
	rdfs:range :Equipment ;
	rdfs:comment "" .
# 
# https://w3id.org/netbeheer/IECCIM/TC57CIM/IEC61970/Base/Core#RegularIntervalSchedule_TimePoints

:RegularIntervalSchedule_TimePoints a owl:ObjectProperty ;
	owl:inverseOf :RegularTimePoint_IntervalSchedule ;
	a owl:FunctionalProperty ;
	rdfs:domain :RegularIntervalSchedule ;
	rdfs:range :RegularTimePoint ;
	rdfs:comment "Regular interval schedule containing this time point.The regular interval time point data values that define this schedule." .
# 
# https://w3id.org/netbeheer/IECCIM/TC57CIM/IEC61970/Base/Core#RegularIntervalSchedule_timeStep

:RegularIntervalSchedule_timeStep a owl:ObjectProperty ;
	rdfs:domain :RegularIntervalSchedule ;
	rdfs:range <https://w3id.org/netbeheer/IECCIM/TC57CIM/IEC61970/Base/Domain#Seconds> ;
	rdfs:comment """The time between each pair of subsequent regular time points in sequence order.
""" .
# 
# https://w3id.org/netbeheer/IECCIM/TC57CIM/IEC61970/Base/Core#RegularTimePoint_IntervalSchedule

:RegularTimePoint_IntervalSchedule a owl:ObjectProperty ;
	rdfs:domain :RegularTimePoint ;
	rdfs:range :RegularIntervalSchedule ;
	rdfs:comment "Regular interval schedule containing this time point.The regular interval time point data values that define this schedule." .
# 
# https://w3id.org/netbeheer/IECCIM/TC57CIM/IEC61970/Base/Core#RegulatingControl_Terminal

:RegulatingControl_Terminal a owl:ObjectProperty ;
	owl:inverseOf :Terminal_RegulatingControl ;
	rdfs:domain <https://w3id.org/netbeheer/IECCIM/TC57CIM/IEC61970/Base/Wires#RegulatingControl> ;
	rdfs:range :Terminal ;
	rdfs:comment "The terminal associated with this regulating control.  The terminal is associated instead of a node, since the terminal could connect into either a topological node (bus in bus-branch model) or a connectivity node (detailed switch model).  Sometimes it is useful to model regulation at a terminal of a bus bar object since the bus bar can be present in both a bus-branch model or a model with switch detail.The controls regulating this terminal." .
# 
# https://w3id.org/netbeheer/IECCIM/TC57CIM/IEC61970/Base/Core#RemoteInputSignal_Terminal

:RemoteInputSignal_Terminal a owl:ObjectProperty ;
	owl:inverseOf :Terminal_RemoteInputSignal ;
	rdfs:domain <https://w3id.org/netbeheer/IECCIM/TC57CIM/IEC61970/Dynamics/StandardInterconnections#RemoteInputSignal> ;
	rdfs:range :Terminal ;
	rdfs:comment "Input signal coming from this terminal.Remote terminal with which this input signal is associated." .
# 
# https://w3id.org/netbeheer/IECCIM/TC57CIM/IEC61970/Base/Core#ReportingGroup_BusNameMarker

:ReportingGroup_BusNameMarker a owl:ObjectProperty ;
	rdfs:domain :ReportingGroup ;
	rdfs:range <https://w3id.org/netbeheer/IECCIM/TC57CIM/IEC61970/Base/Topology#BusNameMarker> ;
	rdfs:comment "The bus name markers that belong to this reporting group.The reporting group to which this bus name marker belongs." .
# 
# https://w3id.org/netbeheer/IECCIM/TC57CIM/IEC61970/Base/Core#ReportingGroup_PowerSystemResource

:ReportingGroup_PowerSystemResource a owl:ObjectProperty ;
	rdfs:domain :ReportingGroup ;
	rdfs:range :PowerSystemResource ;
	rdfs:comment "Reporting groups to which this power system resource belongs.Power system resources which belong to this reporting group." .
# 
# https://w3id.org/netbeheer/IECCIM/TC57CIM/IEC61970/Base/Core#ReportingGroup_ReportingSuperGroup

:ReportingGroup_ReportingSuperGroup a owl:ObjectProperty ;
	owl:inverseOf :ReportingSuperGroup_ReportingGroup ;
	rdfs:domain :ReportingGroup ;
	rdfs:range :ReportingSuperGroup ;
	rdfs:comment "Reporting groups that are grouped under this super group.Reporting super group to which this reporting group belongs." .
# 
# https://w3id.org/netbeheer/IECCIM/TC57CIM/IEC61970/Base/Core#ReportingGroup_TopologicalNode

:ReportingGroup_TopologicalNode a owl:ObjectProperty ;
	owl:inverseOf :TopologicalNode_ReportingGroup ;
	rdfs:domain :ReportingGroup ;
	rdfs:range <https://w3id.org/netbeheer/IECCIM/TC57CIM/IEC61970/Base/Topology#TopologicalNode> ;
	rdfs:comment "The topological nodes that belong to the reporting group.The reporting group to which the topological node belongs." .
# 
# https://w3id.org/netbeheer/IECCIM/TC57CIM/IEC61970/Base/Core#ReportingSuperGroup_ReportingGroup

:ReportingSuperGroup_ReportingGroup a owl:ObjectProperty ;
	rdfs:domain :ReportingSuperGroup ;
	rdfs:range :ReportingGroup ;
	rdfs:comment "Reporting groups that are grouped under this super group.Reporting super group to which this reporting group belongs." .
# 
# https://w3id.org/netbeheer/IECCIM/TC57CIM/IEC61970/Base/Core#SubGeographicalRegion_DCLines

:SubGeographicalRegion_DCLines a owl:ObjectProperty ;
	rdfs:domain :SubGeographicalRegion ;
	rdfs:range <https://w3id.org/netbeheer/IECCIM/TC57CIM/IEC61970/Base/DC#DCLine> ;
	rdfs:comment "" .
# 
# https://w3id.org/netbeheer/IECCIM/TC57CIM/IEC61970/Base/Core#SubGeographicalRegion_Lines

:SubGeographicalRegion_Lines a owl:ObjectProperty ;
	rdfs:domain :SubGeographicalRegion ;
	rdfs:range <https://w3id.org/netbeheer/IECCIM/TC57CIM/IEC61970/Base/Wires#Line> ;
	rdfs:comment "The sub-geographical region of the line.The lines within the sub-geographical region." .
# 
# https://w3id.org/netbeheer/IECCIM/TC57CIM/IEC61970/Base/Core#SubGeographicalRegion_Region

:SubGeographicalRegion_Region a owl:ObjectProperty ;
	rdfs:domain :SubGeographicalRegion ;
	rdfs:range :GeographicalRegion ;
	rdfs:comment "The geographical region to which this sub-geographical region is within.All sub-geograhpical regions within this geographical region." .
# 
# https://w3id.org/netbeheer/IECCIM/TC57CIM/IEC61970/Base/Core#SubGeographicalRegion_Substations

:SubGeographicalRegion_Substations a owl:ObjectProperty ;
	owl:inverseOf :Substation_Region ;
	rdfs:domain :SubGeographicalRegion ;
	rdfs:range :Substation ;
	rdfs:comment "The SubGeographicalRegion containing the substation.The substations in this sub-geographical region." .
# 
# https://w3id.org/netbeheer/IECCIM/TC57CIM/IEC61970/Base/Core#Substation_Bays

:Substation_Bays a owl:ObjectProperty ;
	rdfs:domain :Substation ;
	rdfs:range :Bay ;
	rdfs:comment "Bays contained in the substation.Substation containing the bay." .
# 
# https://w3id.org/netbeheer/IECCIM/TC57CIM/IEC61970/Base/Core#Substation_DCConverterUnit

:Substation_DCConverterUnit a owl:ObjectProperty ;
	rdfs:domain :Substation ;
	rdfs:range <https://w3id.org/netbeheer/IECCIM/TC57CIM/IEC61970/Base/DC#DCConverterUnit> ;
	rdfs:comment "The DC converter unit belonging ot the substation.The containing substation of the DC converter unit." .
# 
# https://w3id.org/netbeheer/IECCIM/TC57CIM/IEC61970/Base/Core#Substation_Region

:Substation_Region a owl:ObjectProperty ;
	rdfs:domain :Substation ;
	rdfs:range :SubGeographicalRegion ;
	rdfs:comment "The SubGeographicalRegion containing the substation.The substations in this sub-geographical region." .
# 
# https://w3id.org/netbeheer/IECCIM/TC57CIM/IEC61970/Base/Core#Substation_VoltageLevels

:Substation_VoltageLevels a owl:ObjectProperty ;
	owl:inverseOf :VoltageLevel_Substation ;
	a owl:FunctionalProperty ;
	rdfs:domain :Substation ;
	rdfs:range :VoltageLevel ;
	rdfs:comment "The substation of the voltage level.The voltage levels within this substation." .
# 
# https://w3id.org/netbeheer/IECCIM/TC57CIM/IEC61970/Base/Core#SvPowerFlow_Terminal

:SvPowerFlow_Terminal a owl:ObjectProperty ;
	owl:inverseOf :Terminal_SvPowerFlow ;
	rdfs:domain <https://w3id.org/netbeheer/IECCIM/TC57CIM/IEC61970/Base/StateVariables#SvPowerFlow> ;
	rdfs:range :Terminal ;
	rdfs:comment "The power flow state variable associated with the terminal.The terminal associated with the power flow state variable." .
# 
# https://w3id.org/netbeheer/IECCIM/TC57CIM/IEC61970/Base/Core#SvStatus_ConductingEquipment

:SvStatus_ConductingEquipment a owl:ObjectProperty ;
	rdfs:domain <https://w3id.org/netbeheer/IECCIM/TC57CIM/IEC61970/Base/StateVariables#SvStatus> ;
	rdfs:range :ConductingEquipment ;
	rdfs:comment "The status state variable associated with this conducting equipment.The conducting equipment associated with the status state variable." .
# 
# https://w3id.org/netbeheer/IECCIM/TC57CIM/IEC61970/Base/Core#Terminal_AuxiliaryEquipment

:Terminal_AuxiliaryEquipment a owl:ObjectProperty , owl:FunctionalProperty ;
	rdfs:domain :Terminal ;
	rdfs:range <https://w3id.org/netbeheer/IECCIM/TC57CIM/IEC61970/Base/AuxiliaryEquipment#AuxiliaryEquipment> ;
	rdfs:comment "The auxiliary equipment connected to the terminal.The Terminal at the equipment where the AuxiliaryEquipment is attached." .
# 
# https://w3id.org/netbeheer/IECCIM/TC57CIM/IEC61970/Base/Core#Terminal_BranchGroupTerminal

:Terminal_BranchGroupTerminal a owl:ObjectProperty , owl:FunctionalProperty ;
	rdfs:domain :Terminal ;
	rdfs:range <https://w3id.org/netbeheer/IECCIM/TC57CIM/IEC61970/Base/OperationalLimits#BranchGroupTerminal> ;
	rdfs:comment "The directed branch group terminals for which this terminal is monitored. The terminal to be summed." .
# 
# https://w3id.org/netbeheer/IECCIM/TC57CIM/IEC61970/Base/Core#Terminal_Bushing

:Terminal_Bushing a owl:ObjectProperty ;
	rdfs:domain :Terminal ;
	rdfs:range <https://w3id.org/netbeheer/IECCIM/TC57CIM/IEC61968/InfIEC61968/InfAssets#Bushing> ;
	rdfs:comment "" .
# 
# https://w3id.org/netbeheer/IECCIM/TC57CIM/IEC61970/Base/Core#Terminal_ConductingEquipment

:Terminal_ConductingEquipment a owl:ObjectProperty ;
	rdfs:domain :Terminal ;
	rdfs:range :ConductingEquipment ;
	rdfs:comment "Conducting equipment have terminals that may be connected to other conducting equipment terminals via connectivity nodes or topological nodes.The conducting equipment of the terminal.  Conducting equipment have  terminals that may be connected to other conducting equipment terminals via connectivity nodes or topological nodes." .
# 
# https://w3id.org/netbeheer/IECCIM/TC57CIM/IEC61970/Base/Core#Terminal_ConnectivityNode

:Terminal_ConnectivityNode a owl:ObjectProperty ;
	rdfs:domain :Terminal ;
	rdfs:range :ConnectivityNode ;
	rdfs:comment "Terminals interconnected with zero impedance at a this connectivity node. The connectivity node to which this terminal connects with zero impedance." .
# 
# https://w3id.org/netbeheer/IECCIM/TC57CIM/IEC61970/Base/Core#Terminal_ConverterDCSides

:Terminal_ConverterDCSides a owl:ObjectProperty ;
	rdfs:domain :Terminal ;
	rdfs:range <https://w3id.org/netbeheer/IECCIM/TC57CIM/IEC61970/Base/DC#ACDCConverter> ;
	rdfs:comment "All converters' DC sides linked to this point of common coupling terminal.Point of common coupling terminal for this converter DC side. It is typically the terminal on the power transformer (or switch) closest to the AC network. The power flow measurement must be the sum of all flows into the transformer." .
# 
# https://w3id.org/netbeheer/IECCIM/TC57CIM/IEC61970/Base/Core#Terminal_HasFirstMutualCoupling

:Terminal_HasFirstMutualCoupling a owl:ObjectProperty , owl:FunctionalProperty ;
	rdfs:domain :Terminal ;
	rdfs:range <https://w3id.org/netbeheer/IECCIM/TC57CIM/IEC61970/Base/Wires#MutualCoupling> ;
	rdfs:comment "Mutual couplings associated with the branch as the first branch.The starting terminal for the calculation of distances along the first branch of the mutual coupling.  Normally MutualCoupling would only be used for terminals of AC line segments.  The first and second terminals of a mutual coupling should point to different AC line segments." .
# 
# https://w3id.org/netbeheer/IECCIM/TC57CIM/IEC61970/Base/Core#Terminal_HasSecondMutualCoupling

:Terminal_HasSecondMutualCoupling a owl:ObjectProperty , owl:FunctionalProperty ;
	rdfs:domain :Terminal ;
	rdfs:range <https://w3id.org/netbeheer/IECCIM/TC57CIM/IEC61970/Base/Wires#MutualCoupling> ;
	rdfs:comment "Mutual couplings with the branch associated as the first branch.The starting terminal for the calculation of distances along the second branch of the mutual coupling." .
# 
# https://w3id.org/netbeheer/IECCIM/TC57CIM/IEC61970/Base/Core#Terminal_PinTerminal

:Terminal_PinTerminal a owl:ObjectProperty , owl:FunctionalProperty ;
	rdfs:domain :Terminal ;
	rdfs:range <https://w3id.org/netbeheer/IECCIM/TC57CIM/IEC61970/InfIEC61970/InfSIPS#PinTerminal> ;
	rdfs:comment "" .
# 
# https://w3id.org/netbeheer/IECCIM/TC57CIM/IEC61970/Base/Core#Terminal_RegulatingControl

:Terminal_RegulatingControl a owl:ObjectProperty ;
	rdfs:domain :Terminal ;
	rdfs:range <https://w3id.org/netbeheer/IECCIM/TC57CIM/IEC61970/Base/Wires#RegulatingControl> ;
	rdfs:comment "The terminal associated with this regulating control.  The terminal is associated instead of a node, since the terminal could connect into either a topological node (bus in bus-branch model) or a connectivity node (detailed switch model).  Sometimes it is useful to model regulation at a terminal of a bus bar object since the bus bar can be present in both a bus-branch model or a model with switch detail.The controls regulating this terminal." .
# 
# https://w3id.org/netbeheer/IECCIM/TC57CIM/IEC61970/Base/Core#Terminal_RemoteInputSignal

:Terminal_RemoteInputSignal a owl:ObjectProperty , owl:FunctionalProperty ;
	rdfs:domain :Terminal ;
	rdfs:range <https://w3id.org/netbeheer/IECCIM/TC57CIM/IEC61970/Dynamics/StandardInterconnections#RemoteInputSignal> ;
	rdfs:comment "Input signal coming from this terminal.Remote terminal with which this input signal is associated." .
# 
# https://w3id.org/netbeheer/IECCIM/TC57CIM/IEC61970/Base/Core#Terminal_SvPowerFlow

:Terminal_SvPowerFlow a owl:ObjectProperty , owl:FunctionalProperty ;
	rdfs:domain :Terminal ;
	rdfs:range <https://w3id.org/netbeheer/IECCIM/TC57CIM/IEC61970/Base/StateVariables#SvPowerFlow> ;
	rdfs:comment "The power flow state variable associated with the terminal.The terminal associated with the power flow state variable." .
# 
# https://w3id.org/netbeheer/IECCIM/TC57CIM/IEC61970/Base/Core#Terminal_TieFlow

:Terminal_TieFlow a owl:ObjectProperty ;
	owl:inverseOf :TieFlow_Terminal ;
	a owl:FunctionalProperty ;
	rdfs:domain :Terminal ;
	rdfs:range <https://w3id.org/netbeheer/IECCIM/TC57CIM/IEC61970/Base/ControlArea#TieFlow> ;
	rdfs:comment "The control area tie flows to which this terminal associates.The terminal to which this tie flow belongs." .
# 
# https://w3id.org/netbeheer/IECCIM/TC57CIM/IEC61970/Base/Core#Terminal_TopologicalNode

:Terminal_TopologicalNode a owl:ObjectProperty ;
	owl:inverseOf :TopologicalNode_Terminal ;
	rdfs:domain :Terminal ;
	rdfs:range <https://w3id.org/netbeheer/IECCIM/TC57CIM/IEC61970/Base/Topology#TopologicalNode> ;
	rdfs:comment "The terminals associated with the topological node.   This can be used as an alternative to the connectivity node path to terminal, thus making it unneccesary to model connectivity nodes in some cases.   Note that if connectivity nodes are in the model, this association would probably not be used as an input specification.The topological node associated with the terminal.   This can be used as an alternative to the connectivity node path to topological node, thus making it unneccesary to model connectivity nodes in some cases.   Note that the if connectivity nodes are in the model, this association would probably not be used as an input specification." .
# 
# https://w3id.org/netbeheer/IECCIM/TC57CIM/IEC61970/Base/Core#Terminal_TransformerEnd

:Terminal_TransformerEnd a owl:ObjectProperty ;
	owl:inverseOf :TransformerEnd_Terminal ;
	rdfs:domain :Terminal ;
	rdfs:range <https://w3id.org/netbeheer/IECCIM/TC57CIM/IEC61970/Base/Wires#TransformerEnd> ;
	rdfs:comment "All transformer ends connected at this terminal.Terminal of the power transformer to which this transformer end belongs." .
# 
# https://w3id.org/netbeheer/IECCIM/TC57CIM/IEC61970/Base/Core#TieFlow_Terminal

:TieFlow_Terminal a owl:ObjectProperty ;
	rdfs:domain <https://w3id.org/netbeheer/IECCIM/TC57CIM/IEC61970/Base/ControlArea#TieFlow> ;
	rdfs:range :Terminal ;
	rdfs:comment "The control area tie flows to which this terminal associates.The terminal to which this tie flow belongs." .
# 
# https://w3id.org/netbeheer/IECCIM/TC57CIM/IEC61970/Base/Core#TopologicalNode_BaseVoltage

:TopologicalNode_BaseVoltage a owl:ObjectProperty ;
	rdfs:domain <https://w3id.org/netbeheer/IECCIM/TC57CIM/IEC61970/Base/Topology#TopologicalNode> ;
	rdfs:range :BaseVoltage ;
	rdfs:comment "The topological nodes at the base voltage.The base voltage of the topologocial node." .
# 
# https://w3id.org/netbeheer/IECCIM/TC57CIM/IEC61970/Base/Core#TopologicalNode_ConnectivityNodeContainer

:TopologicalNode_ConnectivityNodeContainer a owl:ObjectProperty ;
	rdfs:domain <https://w3id.org/netbeheer/IECCIM/TC57CIM/IEC61970/Base/Topology#TopologicalNode> ;
	rdfs:range :ConnectivityNodeContainer ;
	rdfs:comment "The topological nodes which belong to this connectivity node container.The connectivity node container to which the toplogical node belongs." .
# 
# https://w3id.org/netbeheer/IECCIM/TC57CIM/IEC61970/Base/Core#TopologicalNode_ConnectivityNodes

:TopologicalNode_ConnectivityNodes a owl:ObjectProperty ;
	rdfs:domain <https://w3id.org/netbeheer/IECCIM/TC57CIM/IEC61970/Base/Topology#TopologicalNode> ;
	rdfs:range :ConnectivityNode ;
	rdfs:comment "The connectivity nodes combine together to form this topological node.  May depend on the current state of switches in the network.The topological node to which this connectivity node is assigned.  May depend on the current state of switches in the network." .
# 
# https://w3id.org/netbeheer/IECCIM/TC57CIM/IEC61970/Base/Core#TopologicalNode_ReportingGroup

:TopologicalNode_ReportingGroup a owl:ObjectProperty ;
	rdfs:domain <https://w3id.org/netbeheer/IECCIM/TC57CIM/IEC61970/Base/Topology#TopologicalNode> ;
	rdfs:range :ReportingGroup ;
	rdfs:comment "The topological nodes that belong to the reporting group.The reporting group to which the topological node belongs." .
# 
# https://w3id.org/netbeheer/IECCIM/TC57CIM/IEC61970/Base/Core#TopologicalNode_Terminal

:TopologicalNode_Terminal a owl:ObjectProperty ;
	rdfs:domain <https://w3id.org/netbeheer/IECCIM/TC57CIM/IEC61970/Base/Topology#TopologicalNode> ;
	rdfs:range :Terminal ;
	rdfs:comment "The terminals associated with the topological node.   This can be used as an alternative to the connectivity node path to terminal, thus making it unneccesary to model connectivity nodes in some cases.   Note that if connectivity nodes are in the model, this association would probably not be used as an input specification.The topological node associated with the terminal.   This can be used as an alternative to the connectivity node path to topological node, thus making it unneccesary to model connectivity nodes in some cases.   Note that the if connectivity nodes are in the model, this association would probably not be used as an input specification." .
# 
# https://w3id.org/netbeheer/IECCIM/TC57CIM/IEC61970/Base/Core#TransformerEnd_BaseVoltage

:TransformerEnd_BaseVoltage a owl:ObjectProperty ;
	rdfs:domain <https://w3id.org/netbeheer/IECCIM/TC57CIM/IEC61970/Base/Wires#TransformerEnd> ;
	rdfs:range :BaseVoltage ;
	rdfs:comment "Transformer ends at the base voltage.  This is essential for PU calculation.Base voltage of the transformer end.  This is essential for PU calculation." .
# 
# https://w3id.org/netbeheer/IECCIM/TC57CIM/IEC61970/Base/Core#TransformerEnd_Terminal

:TransformerEnd_Terminal a owl:ObjectProperty ;
	rdfs:domain <https://w3id.org/netbeheer/IECCIM/TC57CIM/IEC61970/Base/Wires#TransformerEnd> ;
	rdfs:range :Terminal ;
	rdfs:comment "All transformer ends connected at this terminal.Terminal of the power transformer to which this transformer end belongs." .
# 
# https://w3id.org/netbeheer/IECCIM/TC57CIM/IEC61970/Base/Core#UsagePoint_Equipments

:UsagePoint_Equipments a owl:ObjectProperty ;
	rdfs:domain <https://w3id.org/netbeheer/IECCIM/TC57CIM/IEC61968/Metering#UsagePoint> ;
	rdfs:range :Equipment ;
	rdfs:comment "All usage points connected to the electrical grid through this equipment.All equipment connecting this usage point to the electrical grid." .
# 
# https://w3id.org/netbeheer/IECCIM/TC57CIM/IEC61970/Base/Core#VoltageLevel_BaseVoltage

:VoltageLevel_BaseVoltage a owl:ObjectProperty ;
	rdfs:domain :VoltageLevel ;
	rdfs:range :BaseVoltage ;
	rdfs:comment "The voltage levels having this base voltage.The base voltage used for all equipment within the voltage level." .
# 
# https://w3id.org/netbeheer/IECCIM/TC57CIM/IEC61970/Base/Core#VoltageLevel_Bays

:VoltageLevel_Bays a owl:ObjectProperty ;
	rdfs:domain :VoltageLevel ;
	rdfs:range :Bay ;
	rdfs:comment "The voltage level containing this bay.The bays within this voltage level." .
# 
# https://w3id.org/netbeheer/IECCIM/TC57CIM/IEC61970/Base/Core#VoltageLevel_Substation

:VoltageLevel_Substation a owl:ObjectProperty ;
	rdfs:domain :VoltageLevel ;
	rdfs:range :Substation ;
	rdfs:comment "The substation of the voltage level.The voltage levels within this substation." .
# 
# https://w3id.org/netbeheer/IECCIM/TC57CIM/IEC61970/Base/Core#VoltageLevel_highVoltageLimit

:VoltageLevel_highVoltageLimit a owl:ObjectProperty ;
	rdfs:domain :VoltageLevel ;
	rdfs:range <https://w3id.org/netbeheer/IECCIM/TC57CIM/IEC61970/Base/Domain#Voltage> ;
	rdfs:comment "The bus bar's high voltage limit" .
# 
# https://w3id.org/netbeheer/IECCIM/TC57CIM/IEC61970/Base/Core#VoltageLevel_lowVoltageLimit

:VoltageLevel_lowVoltageLimit a owl:ObjectProperty ;
	rdfs:domain :VoltageLevel ;
	rdfs:range <https://w3id.org/netbeheer/IECCIM/TC57CIM/IEC61970/Base/Domain#Voltage> ;
	rdfs:comment "The bus bar's low voltage limit" .
# 
# https://w3id.org/netbeheer/IECCIM/TC57CIM/IEC61970/Base/Core#WeatherStation_Equipment

:WeatherStation_Equipment a owl:ObjectProperty ;
	rdfs:domain <https://w3id.org/netbeheer/IECCIM/TC57CIM/IEC61970/InfIEC61970/InfOperationalLimits#WeatherStation> ;
	rdfs:range :Equipment ;
	rdfs:comment "" .
# 
# 
# 
# #################################################################
# #
# #    Data properties
# #
# #################################################################
# 
# 
# https://w3id.org/netbeheer/IECCIM/TC57CIM/IEC61970/Base/Core#ACDCTerminal_connected

:ACDCTerminal_connected a owl:DatatypeProperty ;
	rdfs:domain :ACDCTerminal ;
	rdfs:range xsd:boolean ;
	rdfs:comment """The connected status is related to a bus-branch model and the topological node to terminal relation.  True implies the terminal is connected to the related topological node and false implies it is not. 
In a bus-branch model, the connected status is used to tell if equipment is disconnected without having to change the connectivity described by the topological node to terminal relation. A valid case is that conducting equipment can be connected in one end and open in the other. In particular for an AC line segment, where the reactive line charging can be significant, this is a relevant case.
""" .
# 
# https://w3id.org/netbeheer/IECCIM/TC57CIM/IEC61970/Base/Core#ACDCTerminal_sequenceNumber

:ACDCTerminal_sequenceNumber a owl:DatatypeProperty ;
	rdfs:domain :ACDCTerminal ;
	rdfs:range xsd:nonNegativeInteger ;
	rdfs:comment """The orientation of the terminal connections for a multiple terminal conducting equipment.  The sequence numbering starts with 1 and additional terminals should follow in increasing order.   The first terminal is the \"starting point\" for a two terminal branch.
""" .
# 
# https://w3id.org/netbeheer/IECCIM/TC57CIM/IEC61970/Base/Core#BasicIntervalSchedule_startTime

:BasicIntervalSchedule_startTime a owl:DatatypeProperty ;
	rdfs:domain :BasicIntervalSchedule ;
	rdfs:range xsd:dateTime ;
	rdfs:comment "The time for the first time point." .
# 
# https://w3id.org/netbeheer/IECCIM/TC57CIM/IEC61970/Base/Core#BasicIntervalSchedule_value1Multiplier

:BasicIntervalSchedule_value1Multiplier a owl:DatatypeProperty ;
	rdfs:domain :BasicIntervalSchedule ;
	rdfs:range <https://w3id.org/netbeheer/IECCIM/TC57CIM/IEC61970/Base/Domain#UnitMultiplier> ;
	rdfs:comment "Multiplier for value1." .
# 
# https://w3id.org/netbeheer/IECCIM/TC57CIM/IEC61970/Base/Core#BasicIntervalSchedule_value1Unit

:BasicIntervalSchedule_value1Unit a owl:DatatypeProperty ;
	rdfs:domain :BasicIntervalSchedule ;
	rdfs:range <https://w3id.org/netbeheer/IECCIM/TC57CIM/IEC61970/Base/Domain#UnitSymbol> ;
	rdfs:comment "Value1 units of measure." .
# 
# https://w3id.org/netbeheer/IECCIM/TC57CIM/IEC61970/Base/Core#BasicIntervalSchedule_value2Multiplier

:BasicIntervalSchedule_value2Multiplier a owl:DatatypeProperty ;
	rdfs:domain :BasicIntervalSchedule ;
	rdfs:range <https://w3id.org/netbeheer/IECCIM/TC57CIM/IEC61970/Base/Domain#UnitMultiplier> ;
	rdfs:comment "Multiplier for value2." .
# 
# https://w3id.org/netbeheer/IECCIM/TC57CIM/IEC61970/Base/Core#BasicIntervalSchedule_value2Unit

:BasicIntervalSchedule_value2Unit a owl:DatatypeProperty ;
	rdfs:domain :BasicIntervalSchedule ;
	rdfs:range <https://w3id.org/netbeheer/IECCIM/TC57CIM/IEC61970/Base/Domain#UnitSymbol> ;
	rdfs:comment "Value2 units of measure." .
# 
# https://w3id.org/netbeheer/IECCIM/TC57CIM/IEC61970/Base/Core#Bay_bayEnergyMeasFlag

:Bay_bayEnergyMeasFlag a owl:DatatypeProperty ;
	rdfs:domain :Bay ;
	rdfs:range xsd:boolean ;
	rdfs:comment "Indicates the presence/absence of energy measurements." .
# 
# https://w3id.org/netbeheer/IECCIM/TC57CIM/IEC61970/Base/Core#Bay_bayPowerMeasFlag

:Bay_bayPowerMeasFlag a owl:DatatypeProperty ;
	rdfs:domain :Bay ;
	rdfs:range xsd:boolean ;
	rdfs:comment "Indicates the presence/absence of active/reactive power measurements." .
# 
# https://w3id.org/netbeheer/IECCIM/TC57CIM/IEC61970/Base/Core#Bay_breakerConfiguration

:Bay_breakerConfiguration a owl:DatatypeProperty ;
	rdfs:domain :Bay ;
	rdfs:range :BreakerConfiguration ;
	rdfs:comment "Breaker configuration. " .
# 
# https://w3id.org/netbeheer/IECCIM/TC57CIM/IEC61970/Base/Core#Bay_busBarConfiguration

:Bay_busBarConfiguration a owl:DatatypeProperty ;
	rdfs:domain :Bay ;
	rdfs:range :BusbarConfiguration ;
	rdfs:comment "Bus bar configuration." .
# 
# https://w3id.org/netbeheer/IECCIM/TC57CIM/IEC61970/Base/Core#CurveData_xvalue

:CurveData_xvalue a owl:DatatypeProperty ;
	rdfs:domain :CurveData ;
	rdfs:range xsd:float ;
	rdfs:comment """The data value of the X-axis variable,  depending on the X-axis units.
""" .
# 
# https://w3id.org/netbeheer/IECCIM/TC57CIM/IEC61970/Base/Core#CurveData_y1value

:CurveData_y1value a owl:DatatypeProperty ;
	rdfs:domain :CurveData ;
	rdfs:range xsd:float ;
	rdfs:comment """The data value of the  first Y-axis variable, depending on the Y-axis units.
""" .
# 
# https://w3id.org/netbeheer/IECCIM/TC57CIM/IEC61970/Base/Core#CurveData_y2value

:CurveData_y2value a owl:DatatypeProperty ;
	rdfs:domain :CurveData ;
	rdfs:range xsd:float ;
	rdfs:comment """The data value of the second Y-axis variable (if present), depending on the Y-axis units.
""" .
# 
# https://w3id.org/netbeheer/IECCIM/TC57CIM/IEC61970/Base/Core#CurveData_y3value

:CurveData_y3value a owl:DatatypeProperty ;
	rdfs:domain :CurveData ;
	rdfs:range xsd:float ;
	rdfs:comment """The data value of the third Y-axis variable (if present), depending on the Y-axis units.
""" .
# 
# https://w3id.org/netbeheer/IECCIM/TC57CIM/IEC61970/Base/Core#Curve_curveStyle

:Curve_curveStyle a owl:DatatypeProperty ;
	rdfs:domain :Curve ;
	rdfs:range :CurveStyle ;
	rdfs:comment "The style or shape of the curve." .
# 
# https://w3id.org/netbeheer/IECCIM/TC57CIM/IEC61970/Base/Core#Curve_xMultiplier

:Curve_xMultiplier a owl:DatatypeProperty ;
	rdfs:domain :Curve ;
	rdfs:range <https://w3id.org/netbeheer/IECCIM/TC57CIM/IEC61970/Base/Domain#UnitMultiplier> ;
	rdfs:comment "Multiplier for X-axis." .
# 
# https://w3id.org/netbeheer/IECCIM/TC57CIM/IEC61970/Base/Core#Curve_xUnit

:Curve_xUnit a owl:DatatypeProperty ;
	rdfs:domain :Curve ;
	rdfs:range <https://w3id.org/netbeheer/IECCIM/TC57CIM/IEC61970/Base/Domain#UnitSymbol> ;
	rdfs:comment "The X-axis units of measure." .
# 
# https://w3id.org/netbeheer/IECCIM/TC57CIM/IEC61970/Base/Core#Curve_y1Multiplier

:Curve_y1Multiplier a owl:DatatypeProperty ;
	rdfs:domain :Curve ;
	rdfs:range <https://w3id.org/netbeheer/IECCIM/TC57CIM/IEC61970/Base/Domain#UnitMultiplier> ;
	rdfs:comment """Multiplier for Y1-axis.
""" .
# 
# https://w3id.org/netbeheer/IECCIM/TC57CIM/IEC61970/Base/Core#Curve_y1Unit

:Curve_y1Unit a owl:DatatypeProperty ;
	rdfs:domain :Curve ;
	rdfs:range <https://w3id.org/netbeheer/IECCIM/TC57CIM/IEC61970/Base/Domain#UnitSymbol> ;
	rdfs:comment "The Y1-axis units of measure." .
# 
# https://w3id.org/netbeheer/IECCIM/TC57CIM/IEC61970/Base/Core#Curve_y2Multiplier

:Curve_y2Multiplier a owl:DatatypeProperty ;
	rdfs:domain :Curve ;
	rdfs:range <https://w3id.org/netbeheer/IECCIM/TC57CIM/IEC61970/Base/Domain#UnitMultiplier> ;
	rdfs:comment "Multiplier for Y2-axis." .
# 
# https://w3id.org/netbeheer/IECCIM/TC57CIM/IEC61970/Base/Core#Curve_y2Unit

:Curve_y2Unit a owl:DatatypeProperty ;
	rdfs:domain :Curve ;
	rdfs:range <https://w3id.org/netbeheer/IECCIM/TC57CIM/IEC61970/Base/Domain#UnitSymbol> ;
	rdfs:comment "The Y2-axis units of measure." .
# 
# https://w3id.org/netbeheer/IECCIM/TC57CIM/IEC61970/Base/Core#Curve_y3Multiplier

:Curve_y3Multiplier a owl:DatatypeProperty ;
	rdfs:domain :Curve ;
	rdfs:range <https://w3id.org/netbeheer/IECCIM/TC57CIM/IEC61970/Base/Domain#UnitMultiplier> ;
	rdfs:comment "Multiplier for Y3-axis." .
# 
# https://w3id.org/netbeheer/IECCIM/TC57CIM/IEC61970/Base/Core#Curve_y3Unit

:Curve_y3Unit a owl:DatatypeProperty ;
	rdfs:domain :Curve ;
	rdfs:range <https://w3id.org/netbeheer/IECCIM/TC57CIM/IEC61970/Base/Domain#UnitSymbol> ;
	rdfs:comment "The Y3-axis units of measure." .
# 
# https://w3id.org/netbeheer/IECCIM/TC57CIM/IEC61970/Base/Core#Equipment_aggregate

:Equipment_aggregate a owl:DatatypeProperty ;
	rdfs:domain :Equipment ;
	rdfs:range xsd:boolean ;
	rdfs:comment "The single instance of equipment represents multiple pieces of equipment that have been modeled together as an aggregate.  Examples would be power transformers or synchronous machines operating in parallel modeled as a single aggregate power transformer or aggregate synchronous machine.  This is not to be used to indicate equipment that is part of a group of interdependent equipment produced by a network production program.  " .
# 
# https://w3id.org/netbeheer/IECCIM/TC57CIM/IEC61970/Base/Core#Equipment_inService

:Equipment_inService a owl:DatatypeProperty ;
	rdfs:domain :Equipment ;
	rdfs:range xsd:boolean ;
	rdfs:comment "If true, the equipment is in service." .
# 
# https://w3id.org/netbeheer/IECCIM/TC57CIM/IEC61970/Base/Core#Equipment_normallyInService

:Equipment_normallyInService a owl:DatatypeProperty ;
	rdfs:domain :Equipment ;
	rdfs:range xsd:boolean ;
	rdfs:comment "If true, the equipment is normally in service." .
# 
# https://w3id.org/netbeheer/IECCIM/TC57CIM/IEC61970/Base/Core#IdentifiedObject_aliasName

:IdentifiedObject_aliasName a owl:DatatypeProperty ;
	rdfs:domain :IdentifiedObject ;
	rdfs:range xsd:string ;
	rdfs:comment """The aliasName is free text human readable name of the object alternative to IdentifiedObject.name. It may be non unique and may not correlate to a naming hierarchy.
The attribute aliasName is retained because of backwards compatibility between CIM relases. It is however recommended to replace aliasName with the Name class as aliasName is planned for retirement at a future time.

""" .
# 
# https://w3id.org/netbeheer/IECCIM/TC57CIM/IEC61970/Base/Core#IdentifiedObject_description

:IdentifiedObject_description a owl:DatatypeProperty ;
	rdfs:domain :IdentifiedObject ;
	rdfs:range xsd:string ;
	rdfs:comment "The description is a free human readable text describing or naming the object. It may be non unique and may not correlate to a naming hierarchy." .
# 
# https://w3id.org/netbeheer/IECCIM/TC57CIM/IEC61970/Base/Core#IdentifiedObject_mRID

:IdentifiedObject_mRID a owl:DatatypeProperty ;
	rdfs:domain :IdentifiedObject ;
	rdfs:range xsd:string ;
	rdfs:comment """Master resource identifier issued by a model authority. The mRID is unique within an exchange context. Global uniqueness is easily achieved by using a UUID,  as specified in RFC 4122, for the mRID. The use of UUID is strongly recommended.
For CIMXML data files in RDF syntax conforming to IEC 61970-552 Edition 1, the mRID is mapped to rdf:ID or rdf:about attributes that identify CIM object elements.""" .
# 
# https://w3id.org/netbeheer/IECCIM/TC57CIM/IEC61970/Base/Core#IdentifiedObject_name

:IdentifiedObject_name a owl:DatatypeProperty ;
	rdfs:domain :IdentifiedObject ;
	rdfs:range xsd:string ;
	rdfs:comment """The name is any free human readable and possibly non unique text naming the object.
""" .
# 
# https://w3id.org/netbeheer/IECCIM/TC57CIM/IEC61970/Base/Core#IrregularTimePoint_value1

:IrregularTimePoint_value1 a owl:DatatypeProperty ;
	rdfs:domain :IrregularTimePoint ;
	rdfs:range xsd:float ;
	rdfs:comment """The first value at the time. The meaning of the value is defined by the derived type of the associated schedule.
""" .
# 
# https://w3id.org/netbeheer/IECCIM/TC57CIM/IEC61970/Base/Core#IrregularTimePoint_value2

:IrregularTimePoint_value2 a owl:DatatypeProperty ;
	rdfs:domain :IrregularTimePoint ;
	rdfs:range xsd:float ;
	rdfs:comment """The second value at the time. The meaning of the value is defined by the derived type of the associated schedule.
""" .
# 
# https://w3id.org/netbeheer/IECCIM/TC57CIM/IEC61970/Base/Core#NameTypeAuthority_description

:NameTypeAuthority_description a owl:DatatypeProperty ;
	rdfs:domain :NameTypeAuthority ;
	rdfs:range xsd:string ;
	rdfs:comment """Description of the name type authority.
""" .
# 
# https://w3id.org/netbeheer/IECCIM/TC57CIM/IEC61970/Base/Core#NameTypeAuthority_name

:NameTypeAuthority_name a owl:DatatypeProperty ;
	rdfs:domain :NameTypeAuthority ;
	rdfs:range xsd:string ;
	rdfs:comment """Name of the name type authority.
""" .
# 
# https://w3id.org/netbeheer/IECCIM/TC57CIM/IEC61970/Base/Core#NameType_description

:NameType_description a owl:DatatypeProperty ;
	rdfs:domain :NameType ;
	rdfs:range xsd:string ;
	rdfs:comment """Description of the name type.
""" .
# 
# https://w3id.org/netbeheer/IECCIM/TC57CIM/IEC61970/Base/Core#NameType_name

:NameType_name a owl:DatatypeProperty ;
	rdfs:domain :NameType ;
	rdfs:range xsd:string ;
	rdfs:comment """Name of the name type.
""" .
# 
# https://w3id.org/netbeheer/IECCIM/TC57CIM/IEC61970/Base/Core#Name_name

:Name_name a owl:DatatypeProperty ;
	rdfs:domain :Name ;
	rdfs:range xsd:string ;
	rdfs:comment """Any free text that name the object.
""" .
# 
# https://w3id.org/netbeheer/IECCIM/TC57CIM/IEC61970/Base/Core#RegularIntervalSchedule_endTime

:RegularIntervalSchedule_endTime a owl:DatatypeProperty ;
	rdfs:domain :RegularIntervalSchedule ;
	rdfs:range xsd:dateTime ;
	rdfs:comment "The time for the last time point." .
# 
# https://w3id.org/netbeheer/IECCIM/TC57CIM/IEC61970/Base/Core#RegularTimePoint_sequenceNumber

:RegularTimePoint_sequenceNumber a owl:DatatypeProperty ;
	rdfs:domain :RegularTimePoint ;
	rdfs:range xsd:nonNegativeInteger ;
	rdfs:comment """The position of the regular time point in the sequence. Note that time points don't have to be sequential, i.e. time points may be omitted. The actual time for a RegularTimePoint is computed by multiplying the associated regular interval schedule's time step with the regular time point sequence number and adding the associated schedules start time.
""" .
# 
# https://w3id.org/netbeheer/IECCIM/TC57CIM/IEC61970/Base/Core#RegularTimePoint_value1

:RegularTimePoint_value1 a owl:DatatypeProperty ;
	rdfs:domain :RegularTimePoint ;
	rdfs:range xsd:float ;
	rdfs:comment """The first value at the time. The meaning of the value is defined by the derived type of the associated schedule.
""" .
# 
# https://w3id.org/netbeheer/IECCIM/TC57CIM/IEC61970/Base/Core#RegularTimePoint_value2

:RegularTimePoint_value2 a owl:DatatypeProperty ;
	rdfs:domain :RegularTimePoint ;
	rdfs:range xsd:float ;
	rdfs:comment """The second value at the time. The meaning of the value is defined by the derived type of the associated schedule.

""" .
# 
# https://w3id.org/netbeheer/IECCIM/TC57CIM/IEC61970/Base/Core#Terminal_phases

:Terminal_phases a owl:DatatypeProperty ;
	rdfs:domain :Terminal ;
	rdfs:range :PhaseCode ;
	rdfs:comment """Represents the normal network phasing condition.
If the attribute is missing three phases (ABC or ABCN) shall be assumed.""" .
# 
# 
# 
# #################################################################
# #
# #    Classes
# #
# #################################################################
# 
# 
# https://w3id.org/netbeheer/IECCIM/TC57CIM/IEC61968/Assets#Asset

<https://w3id.org/netbeheer/IECCIM/TC57CIM/IEC61968/Assets#Asset> a owl:Class ;
	rdfs:subClassOf _:genid77 .

_:genid77 a owl:Restriction ;
	owl:onProperty :Asset_PowerSystemResources ;
	owl:minQualifiedCardinality "0"^^xsd:nonNegativeInteger ;
	owl:onClass <https://w3id.org/netbeheer/IECCIM/TC57CIM/IEC61968/Assets#Asset> .
# 
# https://w3id.org/netbeheer/IECCIM/TC57CIM/IEC61968/Assets#AssetInfo

<https://w3id.org/netbeheer/IECCIM/TC57CIM/IEC61968/Assets#AssetInfo> a owl:Class ;
	rdfs:subClassOf _:genid78 .

_:genid78 a owl:Restriction ;
	owl:onProperty :AssetInfo_PowerSystemResources ;
	owl:minQualifiedCardinality "0"^^xsd:nonNegativeInteger ;
	owl:onClass <https://w3id.org/netbeheer/IECCIM/TC57CIM/IEC61968/Assets#AssetInfo> .

<https://w3id.org/netbeheer/IECCIM/TC57CIM/IEC61968/Assets#AssetInfo> rdfs:subClassOf _:genid79 .

_:genid79 a owl:Restriction ;
	owl:onProperty :AssetInfo_PowerSystemResources ;
	owl:maxQualifiedCardinality "1"^^xsd:nonNegativeInteger ;
	owl:onClass <https://w3id.org/netbeheer/IECCIM/TC57CIM/IEC61968/Assets#AssetInfo> .
# 
# https://w3id.org/netbeheer/IECCIM/TC57CIM/IEC61968/Common#Location

<https://w3id.org/netbeheer/IECCIM/TC57CIM/IEC61968/Common#Location> a owl:Class ;
	rdfs:subClassOf _:genid80 .

_:genid80 a owl:Restriction ;
	owl:onProperty :Location_PowerSystemResources ;
	owl:minQualifiedCardinality "0"^^xsd:nonNegativeInteger ;
	owl:onClass <https://w3id.org/netbeheer/IECCIM/TC57CIM/IEC61968/Common#Location> .

<https://w3id.org/netbeheer/IECCIM/TC57CIM/IEC61968/Common#Location> rdfs:subClassOf _:genid81 .

_:genid81 a owl:Restriction ;
	owl:onProperty :Location_PowerSystemResources ;
	owl:maxQualifiedCardinality "1"^^xsd:nonNegativeInteger ;
	owl:onClass <https://w3id.org/netbeheer/IECCIM/TC57CIM/IEC61968/Common#Location> .
# 
# https://w3id.org/netbeheer/IECCIM/TC57CIM/IEC61968/InfIEC61968/InfAssets#Bushing

<https://w3id.org/netbeheer/IECCIM/TC57CIM/IEC61968/InfIEC61968/InfAssets#Bushing> a owl:Class ;
	rdfs:subClassOf _:genid82 .

_:genid82 a owl:Restriction ;
	owl:onProperty :Bushing_Terminal ;
	owl:minQualifiedCardinality "0"^^xsd:nonNegativeInteger ;
	owl:onClass <https://w3id.org/netbeheer/IECCIM/TC57CIM/IEC61968/InfIEC61968/InfAssets#Bushing> .

<https://w3id.org/netbeheer/IECCIM/TC57CIM/IEC61968/InfIEC61968/InfAssets#Bushing> rdfs:subClassOf _:genid83 .

_:genid83 a owl:Restriction ;
	owl:onProperty :Bushing_Terminal ;
	owl:maxQualifiedCardinality "1"^^xsd:nonNegativeInteger ;
	owl:onClass <https://w3id.org/netbeheer/IECCIM/TC57CIM/IEC61968/InfIEC61968/InfAssets#Bushing> .
# 
# https://w3id.org/netbeheer/IECCIM/TC57CIM/IEC61968/Metering#UsagePoint

<https://w3id.org/netbeheer/IECCIM/TC57CIM/IEC61968/Metering#UsagePoint> a owl:Class ;
	rdfs:subClassOf _:genid84 .

_:genid84 a owl:Restriction ;
	owl:onProperty :UsagePoint_Equipments ;
	owl:minQualifiedCardinality "0"^^xsd:nonNegativeInteger ;
	owl:onClass <https://w3id.org/netbeheer/IECCIM/TC57CIM/IEC61968/Metering#UsagePoint> .
# 
# https://w3id.org/netbeheer/IECCIM/TC57CIM/IEC61968/Operations#ClearanceDocument

<https://w3id.org/netbeheer/IECCIM/TC57CIM/IEC61968/Operations#ClearanceDocument> a owl:Class ;
	rdfs:subClassOf _:genid85 .

_:genid85 a owl:Restriction ;
	owl:onProperty :ClearanceDocument_TaggedPSRs ;
	owl:minQualifiedCardinality "0"^^xsd:nonNegativeInteger ;
	owl:onClass <https://w3id.org/netbeheer/IECCIM/TC57CIM/IEC61968/Operations#ClearanceDocument> .
# 
# https://w3id.org/netbeheer/IECCIM/TC57CIM/IEC61968/Operations#GroundAction

<https://w3id.org/netbeheer/IECCIM/TC57CIM/IEC61968/Operations#GroundAction> a owl:Class ;
	rdfs:subClassOf _:genid86 .

_:genid86 a owl:Restriction ;
	owl:onProperty :GroundAction_GroundedEquipment ;
	owl:minQualifiedCardinality "0"^^xsd:nonNegativeInteger ;
	owl:onClass <https://w3id.org/netbeheer/IECCIM/TC57CIM/IEC61968/Operations#GroundAction> .

<https://w3id.org/netbeheer/IECCIM/TC57CIM/IEC61968/Operations#GroundAction> rdfs:subClassOf _:genid87 .

_:genid87 a owl:Restriction ;
	owl:onProperty :GroundAction_GroundedEquipment ;
	owl:maxQualifiedCardinality "1"^^xsd:nonNegativeInteger ;
	owl:onClass <https://w3id.org/netbeheer/IECCIM/TC57CIM/IEC61968/Operations#GroundAction> .
# 
# https://w3id.org/netbeheer/IECCIM/TC57CIM/IEC61968/Operations#JumperAction

<https://w3id.org/netbeheer/IECCIM/TC57CIM/IEC61968/Operations#JumperAction> a owl:Class ;
	rdfs:subClassOf _:genid88 .

_:genid88 a owl:Restriction ;
	owl:onProperty :JumperAction_JumpedEquipments ;
	owl:minQualifiedCardinality "0"^^xsd:nonNegativeInteger ;
	owl:onClass <https://w3id.org/netbeheer/IECCIM/TC57CIM/IEC61968/Operations#JumperAction> .

<https://w3id.org/netbeheer/IECCIM/TC57CIM/IEC61968/Operations#JumperAction> rdfs:subClassOf _:genid89 .

_:genid89 a owl:Restriction ;
	owl:onProperty :JumperAction_JumpedEquipments ;
	owl:maxQualifiedCardinality "1"^^xsd:nonNegativeInteger ;
	owl:onClass <https://w3id.org/netbeheer/IECCIM/TC57CIM/IEC61968/Operations#JumperAction> .
# 
# https://w3id.org/netbeheer/IECCIM/TC57CIM/IEC61968/Operations#OperationalRestriction

<https://w3id.org/netbeheer/IECCIM/TC57CIM/IEC61968/Operations#OperationalRestriction> a owl:Class ;
	rdfs:subClassOf _:genid90 .

_:genid90 a owl:Restriction ;
	owl:onProperty :OperationalRestriction_Equipments ;
	owl:minQualifiedCardinality "0"^^xsd:nonNegativeInteger ;
	owl:onClass <https://w3id.org/netbeheer/IECCIM/TC57CIM/IEC61968/Operations#OperationalRestriction> .
# 
# https://w3id.org/netbeheer/IECCIM/TC57CIM/IEC61968/Operations#OperationalTag

<https://w3id.org/netbeheer/IECCIM/TC57CIM/IEC61968/Operations#OperationalTag> a owl:Class ;
	rdfs:subClassOf _:genid91 .

_:genid91 a owl:Restriction ;
	owl:onProperty :OperationalTag_PowerSystemResource ;
	owl:minQualifiedCardinality "0"^^xsd:nonNegativeInteger ;
	owl:onClass <https://w3id.org/netbeheer/IECCIM/TC57CIM/IEC61968/Operations#OperationalTag> .
# 
# https://w3id.org/netbeheer/IECCIM/TC57CIM/IEC61968/Operations#Outage

<https://w3id.org/netbeheer/IECCIM/TC57CIM/IEC61968/Operations#Outage> a owl:Class ;
	rdfs:subClassOf _:genid92 .

_:genid92 a owl:Restriction ;
	owl:onProperty :Outage_Equipments ;
	owl:minQualifiedCardinality "0"^^xsd:nonNegativeInteger ;
	owl:onClass <https://w3id.org/netbeheer/IECCIM/TC57CIM/IEC61968/Operations#Outage> .
# 
# https://w3id.org/netbeheer/IECCIM/TC57CIM/IEC61968/Operations#PSREvent

<https://w3id.org/netbeheer/IECCIM/TC57CIM/IEC61968/Operations#PSREvent> a owl:Class ;
	rdfs:subClassOf _:genid93 .

_:genid93 a owl:Restriction ;
	owl:onProperty :PSREvent_PowerSystemResource ;
	owl:minQualifiedCardinality "0"^^xsd:nonNegativeInteger ;
	owl:onClass <https://w3id.org/netbeheer/IECCIM/TC57CIM/IEC61968/Operations#PSREvent> .
# 
# https://w3id.org/netbeheer/IECCIM/TC57CIM/IEC61970/Base/AuxiliaryEquipment#AuxiliaryEquipment

<https://w3id.org/netbeheer/IECCIM/TC57CIM/IEC61970/Base/AuxiliaryEquipment#AuxiliaryEquipment> a owl:Class ;
	rdfs:subClassOf _:genid94 .

_:genid94 a owl:Restriction ;
	owl:onProperty :AuxiliaryEquipment_Terminal ;
	owl:minQualifiedCardinality "0"^^xsd:nonNegativeInteger ;
	owl:onClass <https://w3id.org/netbeheer/IECCIM/TC57CIM/IEC61970/Base/AuxiliaryEquipment#AuxiliaryEquipment> .
# 
# https://w3id.org/netbeheer/IECCIM/TC57CIM/IEC61970/Base/Contingency#ContingencyEquipment

<https://w3id.org/netbeheer/IECCIM/TC57CIM/IEC61970/Base/Contingency#ContingencyEquipment> a owl:Class ;
	rdfs:subClassOf _:genid95 .

_:genid95 a owl:Restriction ;
	owl:onProperty :ContingencyEquipment_Equipment ;
	owl:minQualifiedCardinality "0"^^xsd:nonNegativeInteger ;
	owl:onClass <https://w3id.org/netbeheer/IECCIM/TC57CIM/IEC61970/Base/Contingency#ContingencyEquipment> .
# 
# https://w3id.org/netbeheer/IECCIM/TC57CIM/IEC61970/Base/ControlArea#TieFlow

<https://w3id.org/netbeheer/IECCIM/TC57CIM/IEC61970/Base/ControlArea#TieFlow> a owl:Class ;
	rdfs:subClassOf _:genid96 .

_:genid96 a owl:Restriction ;
	owl:onProperty :TieFlow_Terminal ;
	owl:minQualifiedCardinality "0"^^xsd:nonNegativeInteger ;
	owl:onClass <https://w3id.org/netbeheer/IECCIM/TC57CIM/IEC61970/Base/ControlArea#TieFlow> .

<https://w3id.org/netbeheer/IECCIM/TC57CIM/IEC61970/Base/ControlArea#TieFlow> rdfs:subClassOf _:genid97 .

_:genid97 a owl:Restriction ;
	owl:onProperty :TieFlow_Terminal ;
	owl:maxQualifiedCardinality "2"^^xsd:nonNegativeInteger ;
	owl:onClass <https://w3id.org/netbeheer/IECCIM/TC57CIM/IEC61970/Base/ControlArea#TieFlow> .
# 
# https://w3id.org/netbeheer/IECCIM/TC57CIM/IEC61970/Base/Core#ACDCTerminal

:ACDCTerminal a owl:Class ;
	rdfs:subClassOf :IdentifiedObject , _:genid98 .

_:genid98 a owl:Restriction ;
	owl:onProperty :ACDCTerminal_BusNameMarker ;
	owl:minQualifiedCardinality "1"^^xsd:nonNegativeInteger ;
	owl:onClass :ACDCTerminal .

:ACDCTerminal rdfs:subClassOf _:genid99 .

_:genid99 a owl:Restriction ;
	owl:onProperty :ACDCTerminal_Measurements ;
	owl:minQualifiedCardinality "0"^^xsd:nonNegativeInteger ;
	owl:onClass :ACDCTerminal .

:ACDCTerminal rdfs:subClassOf _:genid100 .

_:genid100 a owl:Restriction ;
	owl:onProperty :ACDCTerminal_OperationalLimitSet ;
	owl:minQualifiedCardinality "0"^^xsd:nonNegativeInteger ;
	owl:onClass :ACDCTerminal .

:ACDCTerminal rdfs:subClassOf _:genid101 .

_:genid101 a owl:Restriction ;
	owl:onProperty :ACDCTerminal_Measurements ;
	owl:maxQualifiedCardinality "1"^^xsd:nonNegativeInteger ;
	owl:onClass :ACDCTerminal .

:ACDCTerminal rdfs:subClassOf _:genid102 .

_:genid102 a owl:Restriction ;
	owl:onProperty :ACDCTerminal_OperationalLimitSet ;
	owl:maxQualifiedCardinality "1"^^xsd:nonNegativeInteger ;
	owl:onClass :ACDCTerminal .

:ACDCTerminal rdfs:subClassOf _:genid103 .

_:genid103 a owl:Restriction ;
	owl:onProperty :ACDCTerminal_connected ;
	owl:minQualifiedCardinality "0"^^xsd:nonNegativeInteger ;
	owl:onDataRange xsd:boolean .

:ACDCTerminal rdfs:subClassOf _:genid104 .

_:genid104 a owl:Restriction ;
	owl:onProperty :ACDCTerminal_sequenceNumber ;
	owl:minQualifiedCardinality "0"^^xsd:nonNegativeInteger ;
	owl:onDataRange xsd:nonNegativeInteger .

:ACDCTerminal rdfs:subClassOf _:genid105 .

_:genid105 a owl:Restriction ;
	owl:onProperty :ACDCTerminal_connected ;
	owl:maxQualifiedCardinality "1"^^xsd:nonNegativeInteger ;
	owl:onDataRange xsd:boolean .

:ACDCTerminal rdfs:subClassOf _:genid106 .

_:genid106 a owl:Restriction ;
	owl:onProperty :ACDCTerminal_sequenceNumber ;
	owl:maxQualifiedCardinality "1"^^xsd:nonNegativeInteger ;
	owl:onDataRange xsd:nonNegativeInteger .

:ACDCTerminal rdfs:comment "An electrical connection point (AC or DC) to a piece of conducting equipment. Terminals are connected at physical connection points called connectivity nodes." .
# 
# https://w3id.org/netbeheer/IECCIM/TC57CIM/IEC61970/Base/Core#BaseFrequency

:BaseFrequency a owl:Class ;
	rdfs:subClassOf :IdentifiedObject , _:genid107 .

_:genid107 a owl:Restriction ;
	owl:onProperty :BaseFrequency_frequency ;
	owl:minQualifiedCardinality "0"^^xsd:nonNegativeInteger ;
	owl:onClass <https://w3id.org/netbeheer/IECCIM/TC57CIM/IEC61970/Base/Domain#Frequency> .

:BaseFrequency rdfs:subClassOf _:genid108 .

_:genid108 a owl:Restriction ;
	owl:onProperty :BaseFrequency_frequency ;
	owl:maxQualifiedCardinality "1"^^xsd:nonNegativeInteger ;
	owl:onClass <https://w3id.org/netbeheer/IECCIM/TC57CIM/IEC61970/Base/Domain#Frequency> .

:BaseFrequency rdfs:comment "The class describe a base frequency for a power system network. In case of multiple power networks with different frequencies, e.g. 50 or 60 Hertz each network will have it's own base frequency class. Hence it is assumed that power system objects having different base frequencies appear in separate documents where each document has a single base frequency instance." .
# 
# https://w3id.org/netbeheer/IECCIM/TC57CIM/IEC61970/Base/Core#BasePower

:BasePower a owl:Class ;
	rdfs:subClassOf :IdentifiedObject , _:genid109 .

_:genid109 a owl:Restriction ;
	owl:onProperty :BasePower_basePower ;
	owl:minQualifiedCardinality "0"^^xsd:nonNegativeInteger ;
	owl:onClass <https://w3id.org/netbeheer/IECCIM/TC57CIM/IEC61970/Base/Domain#ApparentPower> .

:BasePower rdfs:subClassOf _:genid110 .

_:genid110 a owl:Restriction ;
	owl:onProperty :BasePower_basePower ;
	owl:maxQualifiedCardinality "1"^^xsd:nonNegativeInteger ;
	owl:onClass <https://w3id.org/netbeheer/IECCIM/TC57CIM/IEC61970/Base/Domain#ApparentPower> .

:BasePower rdfs:comment "The BasePower class defines the base power used in the per unit calculations." .
# 
# https://w3id.org/netbeheer/IECCIM/TC57CIM/IEC61970/Base/Core#BaseVoltage

:BaseVoltage a owl:Class ;
	rdfs:subClassOf :IdentifiedObject , _:genid111 .

_:genid111 a owl:Restriction ;
	owl:onProperty :BaseVoltage_ConductingEquipment ;
	owl:minQualifiedCardinality "0"^^xsd:nonNegativeInteger ;
	owl:onClass :BaseVoltage .

:BaseVoltage rdfs:subClassOf _:genid112 .

_:genid112 a owl:Restriction ;
	owl:onProperty :BaseVoltage_TopologicalNode ;
	owl:minQualifiedCardinality "0"^^xsd:nonNegativeInteger ;
	owl:onClass :BaseVoltage .

:BaseVoltage rdfs:subClassOf _:genid113 .

_:genid113 a owl:Restriction ;
	owl:onProperty :BaseVoltage_TransformerEnds ;
	owl:minQualifiedCardinality "0"^^xsd:nonNegativeInteger ;
	owl:onClass :BaseVoltage .

:BaseVoltage rdfs:subClassOf _:genid114 .

_:genid114 a owl:Restriction ;
	owl:onProperty :BaseVoltage_nominalVoltage ;
	owl:minQualifiedCardinality "0"^^xsd:nonNegativeInteger ;
	owl:onClass <https://w3id.org/netbeheer/IECCIM/TC57CIM/IEC61970/Base/Domain#Voltage> .

:BaseVoltage rdfs:subClassOf _:genid115 .

_:genid115 a owl:Restriction ;
	owl:onProperty :BaseVoltage_VoltageLevel ;
	owl:qualifiedCardinality "1"^^xsd:nonNegativeInteger ;
	owl:onClass :BaseVoltage .

:BaseVoltage rdfs:subClassOf _:genid116 .

_:genid116 a owl:Restriction ;
	owl:onProperty :BaseVoltage_ConductingEquipment ;
	owl:maxQualifiedCardinality "1"^^xsd:nonNegativeInteger ;
	owl:onClass :BaseVoltage .

:BaseVoltage rdfs:subClassOf _:genid117 .

_:genid117 a owl:Restriction ;
	owl:onProperty :BaseVoltage_TopologicalNode ;
	owl:maxQualifiedCardinality "1"^^xsd:nonNegativeInteger ;
	owl:onClass :BaseVoltage .

:BaseVoltage rdfs:subClassOf _:genid118 .

_:genid118 a owl:Restriction ;
	owl:onProperty :BaseVoltage_TransformerEnds ;
	owl:maxQualifiedCardinality "1"^^xsd:nonNegativeInteger ;
	owl:onClass :BaseVoltage .

:BaseVoltage rdfs:subClassOf _:genid119 .

_:genid119 a owl:Restriction ;
	owl:onProperty :BaseVoltage_nominalVoltage ;
	owl:maxQualifiedCardinality "1"^^xsd:nonNegativeInteger ;
	owl:onClass <https://w3id.org/netbeheer/IECCIM/TC57CIM/IEC61970/Base/Domain#Voltage> .

:BaseVoltage rdfs:comment "Defines a system base voltage which is referenced. " .
# 
# https://w3id.org/netbeheer/IECCIM/TC57CIM/IEC61970/Base/Core#BasicIntervalSchedule

:BasicIntervalSchedule a owl:Class ;
	rdfs:subClassOf :IdentifiedObject , _:genid120 .

_:genid120 a owl:Restriction ;
	owl:onProperty :BasicIntervalSchedule_startTime ;
	owl:minQualifiedCardinality "0"^^xsd:nonNegativeInteger ;
	owl:onDataRange xsd:dateTime .

:BasicIntervalSchedule rdfs:subClassOf _:genid121 .

_:genid121 a owl:Restriction ;
	owl:onProperty :BasicIntervalSchedule_value1Multiplier ;
	owl:minQualifiedCardinality "0"^^xsd:nonNegativeInteger ;
	owl:onDataRange <https://w3id.org/netbeheer/IECCIM/TC57CIM/IEC61970/Base/Domain#UnitMultiplier> .

:BasicIntervalSchedule rdfs:subClassOf _:genid122 .

_:genid122 a owl:Restriction ;
	owl:onProperty :BasicIntervalSchedule_value1Unit ;
	owl:minQualifiedCardinality "0"^^xsd:nonNegativeInteger ;
	owl:onDataRange <https://w3id.org/netbeheer/IECCIM/TC57CIM/IEC61970/Base/Domain#UnitSymbol> .

:BasicIntervalSchedule rdfs:subClassOf _:genid123 .

_:genid123 a owl:Restriction ;
	owl:onProperty :BasicIntervalSchedule_value2Multiplier ;
	owl:minQualifiedCardinality "0"^^xsd:nonNegativeInteger ;
	owl:onDataRange <https://w3id.org/netbeheer/IECCIM/TC57CIM/IEC61970/Base/Domain#UnitMultiplier> .

:BasicIntervalSchedule rdfs:subClassOf _:genid124 .

_:genid124 a owl:Restriction ;
	owl:onProperty :BasicIntervalSchedule_value2Unit ;
	owl:minQualifiedCardinality "0"^^xsd:nonNegativeInteger ;
	owl:onDataRange <https://w3id.org/netbeheer/IECCIM/TC57CIM/IEC61970/Base/Domain#UnitSymbol> .

:BasicIntervalSchedule rdfs:subClassOf _:genid125 .

_:genid125 a owl:Restriction ;
	owl:onProperty :BasicIntervalSchedule_startTime ;
	owl:maxQualifiedCardinality "1"^^xsd:nonNegativeInteger ;
	owl:onDataRange xsd:dateTime .

:BasicIntervalSchedule rdfs:subClassOf _:genid126 .

_:genid126 a owl:Restriction ;
	owl:onProperty :BasicIntervalSchedule_value1Multiplier ;
	owl:maxQualifiedCardinality "1"^^xsd:nonNegativeInteger ;
	owl:onDataRange <https://w3id.org/netbeheer/IECCIM/TC57CIM/IEC61970/Base/Domain#UnitMultiplier> .

:BasicIntervalSchedule rdfs:subClassOf _:genid127 .

_:genid127 a owl:Restriction ;
	owl:onProperty :BasicIntervalSchedule_value1Unit ;
	owl:maxQualifiedCardinality "1"^^xsd:nonNegativeInteger ;
	owl:onDataRange <https://w3id.org/netbeheer/IECCIM/TC57CIM/IEC61970/Base/Domain#UnitSymbol> .

:BasicIntervalSchedule rdfs:subClassOf _:genid128 .

_:genid128 a owl:Restriction ;
	owl:onProperty :BasicIntervalSchedule_value2Multiplier ;
	owl:maxQualifiedCardinality "1"^^xsd:nonNegativeInteger ;
	owl:onDataRange <https://w3id.org/netbeheer/IECCIM/TC57CIM/IEC61970/Base/Domain#UnitMultiplier> .

:BasicIntervalSchedule rdfs:subClassOf _:genid129 .

_:genid129 a owl:Restriction ;
	owl:onProperty :BasicIntervalSchedule_value2Unit ;
	owl:maxQualifiedCardinality "1"^^xsd:nonNegativeInteger ;
	owl:onDataRange <https://w3id.org/netbeheer/IECCIM/TC57CIM/IEC61970/Base/Domain#UnitSymbol> .

:BasicIntervalSchedule rdfs:comment "Schedule of values at points in time." .
# 
# https://w3id.org/netbeheer/IECCIM/TC57CIM/IEC61970/Base/Core#Bay

:Bay a owl:Class ;
	rdfs:subClassOf :EquipmentContainer , _:genid130 .

_:genid130 a owl:Restriction ;
	owl:onProperty :Bay_Substation ;
	owl:minQualifiedCardinality "0"^^xsd:nonNegativeInteger ;
	owl:onClass :Bay .

:Bay rdfs:subClassOf _:genid131 .

_:genid131 a owl:Restriction ;
	owl:onProperty :Bay_VoltageLevel ;
	owl:minQualifiedCardinality "0"^^xsd:nonNegativeInteger ;
	owl:onClass :Bay .

:Bay rdfs:subClassOf _:genid132 .

_:genid132 a owl:Restriction ;
	owl:onProperty :Bay_bayEnergyMeasFlag ;
	owl:minQualifiedCardinality "0"^^xsd:nonNegativeInteger ;
	owl:onDataRange xsd:boolean .

:Bay rdfs:subClassOf _:genid133 .

_:genid133 a owl:Restriction ;
	owl:onProperty :Bay_bayPowerMeasFlag ;
	owl:minQualifiedCardinality "0"^^xsd:nonNegativeInteger ;
	owl:onDataRange xsd:boolean .

:Bay rdfs:subClassOf _:genid134 .

_:genid134 a owl:Restriction ;
	owl:onProperty :Bay_breakerConfiguration ;
	owl:minQualifiedCardinality "0"^^xsd:nonNegativeInteger ;
	owl:onDataRange :BreakerConfiguration .

:Bay rdfs:subClassOf _:genid135 .

_:genid135 a owl:Restriction ;
	owl:onProperty :Bay_busBarConfiguration ;
	owl:minQualifiedCardinality "0"^^xsd:nonNegativeInteger ;
	owl:onDataRange :BusbarConfiguration .

:Bay rdfs:subClassOf _:genid136 .

_:genid136 a owl:Restriction ;
	owl:onProperty :Bay_bayEnergyMeasFlag ;
	owl:maxQualifiedCardinality "1"^^xsd:nonNegativeInteger ;
	owl:onDataRange xsd:boolean .

:Bay rdfs:subClassOf _:genid137 .

_:genid137 a owl:Restriction ;
	owl:onProperty :Bay_bayPowerMeasFlag ;
	owl:maxQualifiedCardinality "1"^^xsd:nonNegativeInteger ;
	owl:onDataRange xsd:boolean .

:Bay rdfs:subClassOf _:genid138 .

_:genid138 a owl:Restriction ;
	owl:onProperty :Bay_breakerConfiguration ;
	owl:maxQualifiedCardinality "1"^^xsd:nonNegativeInteger ;
	owl:onDataRange :BreakerConfiguration .

:Bay rdfs:subClassOf _:genid139 .

_:genid139 a owl:Restriction ;
	owl:onProperty :Bay_busBarConfiguration ;
	owl:maxQualifiedCardinality "1"^^xsd:nonNegativeInteger ;
	owl:onDataRange :BusbarConfiguration .

:Bay rdfs:comment """A collection of power system resources (within a given substation) including conducting equipment, protection relays, measurements, and telemetry.  A bay typically represents a physical grouping related to modularization of equipment.
""" .
# 
# https://w3id.org/netbeheer/IECCIM/TC57CIM/IEC61970/Base/Core#ConductingEquipment

:ConductingEquipment a owl:Class ;
	rdfs:subClassOf :Equipment , _:genid140 .

_:genid140 a owl:Restriction ;
	owl:onProperty :ConductingEquipment_BaseVoltage ;
	owl:minQualifiedCardinality "0"^^xsd:nonNegativeInteger ;
	owl:onClass :ConductingEquipment .

:ConductingEquipment rdfs:subClassOf _:genid141 .

_:genid141 a owl:Restriction ;
	owl:onProperty :ConductingEquipment_GroundingAction ;
	owl:minQualifiedCardinality "0"^^xsd:nonNegativeInteger ;
	owl:onClass :ConductingEquipment .

:ConductingEquipment rdfs:subClassOf _:genid142 .

_:genid142 a owl:Restriction ;
	owl:onProperty :ConductingEquipment_JumpingAction ;
	owl:minQualifiedCardinality "0"^^xsd:nonNegativeInteger ;
	owl:onClass :ConductingEquipment .

:ConductingEquipment rdfs:subClassOf _:genid143 .

_:genid143 a owl:Restriction ;
	owl:onProperty :ConductingEquipment_ProtectionEquipments ;
	owl:minQualifiedCardinality "0"^^xsd:nonNegativeInteger ;
	owl:onClass :ConductingEquipment .

:ConductingEquipment rdfs:subClassOf _:genid144 .

_:genid144 a owl:Restriction ;
	owl:onProperty :ConductingEquipment_ProtectiveActionAdjustment ;
	owl:qualifiedCardinality "1"^^xsd:nonNegativeInteger ;
	owl:onClass :ConductingEquipment .

:ConductingEquipment rdfs:subClassOf _:genid145 .

_:genid145 a owl:Restriction ;
	owl:onProperty :ConductingEquipment_SvStatus ;
	owl:qualifiedCardinality "1"^^xsd:nonNegativeInteger ;
	owl:onClass :ConductingEquipment .

:ConductingEquipment rdfs:subClassOf _:genid146 .

_:genid146 a owl:Restriction ;
	owl:onProperty :ConductingEquipment_Terminals ;
	owl:qualifiedCardinality "1"^^xsd:nonNegativeInteger ;
	owl:onClass :ConductingEquipment .

:ConductingEquipment rdfs:subClassOf _:genid147 .

_:genid147 a owl:Restriction ;
	owl:onProperty :ConductingEquipment_GroundingAction ;
	owl:maxQualifiedCardinality "1"^^xsd:nonNegativeInteger ;
	owl:onClass :ConductingEquipment .

:ConductingEquipment rdfs:comment "The parts of the AC power system that are designed to carry current or that are conductively connected through terminals." .
# 
# https://w3id.org/netbeheer/IECCIM/TC57CIM/IEC61970/Base/Core#ConnectivityNode

:ConnectivityNode a owl:Class ;
	rdfs:subClassOf :IdentifiedObject , _:genid148 .

_:genid148 a owl:Restriction ;
	owl:onProperty :ConnectivityNode_ConnectivityNodeContainer ;
	owl:minQualifiedCardinality "0"^^xsd:nonNegativeInteger ;
	owl:onClass :ConnectivityNode .

:ConnectivityNode rdfs:subClassOf _:genid149 .

_:genid149 a owl:Restriction ;
	owl:onProperty :ConnectivityNode_Terminals ;
	owl:minQualifiedCardinality "0"^^xsd:nonNegativeInteger ;
	owl:onClass :ConnectivityNode .

:ConnectivityNode rdfs:subClassOf _:genid150 .

_:genid150 a owl:Restriction ;
	owl:onProperty :ConnectivityNode_TopologicalNode ;
	owl:minQualifiedCardinality "0"^^xsd:nonNegativeInteger ;
	owl:onClass :ConnectivityNode .

:ConnectivityNode rdfs:subClassOf _:genid151 .

_:genid151 a owl:Restriction ;
	owl:onProperty :ConnectivityNode_Terminals ;
	owl:maxQualifiedCardinality "1"^^xsd:nonNegativeInteger ;
	owl:onClass :ConnectivityNode .

:ConnectivityNode rdfs:comment "Connectivity nodes are points where terminals of AC conducting equipment are connected together with zero impedance." .
# 
# https://w3id.org/netbeheer/IECCIM/TC57CIM/IEC61970/Base/Core#ConnectivityNodeContainer

:ConnectivityNodeContainer a owl:Class ;
	rdfs:subClassOf :PowerSystemResource , _:genid152 .

_:genid152 a owl:Restriction ;
	owl:onProperty :ConnectivityNodeContainer_TopologicalNode ;
	owl:minQualifiedCardinality "0"^^xsd:nonNegativeInteger ;
	owl:onClass :ConnectivityNodeContainer .

:ConnectivityNodeContainer rdfs:subClassOf _:genid153 .

_:genid153 a owl:Restriction ;
	owl:onProperty :ConnectivityNodeContainer_ConnectivityNodes ;
	owl:qualifiedCardinality "1"^^xsd:nonNegativeInteger ;
	owl:onClass :ConnectivityNodeContainer .

:ConnectivityNodeContainer rdfs:subClassOf _:genid154 .

_:genid154 a owl:Restriction ;
	owl:onProperty :ConnectivityNodeContainer_TopologicalNode ;
	owl:maxQualifiedCardinality "1"^^xsd:nonNegativeInteger ;
	owl:onClass :ConnectivityNodeContainer .

:ConnectivityNodeContainer rdfs:comment """A base class for all objects that may contain connectivity nodes or topological nodes.
""" .
# 
# https://w3id.org/netbeheer/IECCIM/TC57CIM/IEC61970/Base/Core#Curve

:Curve a owl:Class ;
	rdfs:subClassOf :IdentifiedObject , _:genid155 .

_:genid155 a owl:Restriction ;
	owl:onProperty :Curve_CurveDatas ;
	owl:qualifiedCardinality "1"^^xsd:nonNegativeInteger ;
	owl:onClass :Curve .

:Curve rdfs:subClassOf _:genid156 .

_:genid156 a owl:Restriction ;
	owl:onProperty :Curve_curveStyle ;
	owl:minQualifiedCardinality "0"^^xsd:nonNegativeInteger ;
	owl:onDataRange :CurveStyle .

:Curve rdfs:subClassOf _:genid157 .

_:genid157 a owl:Restriction ;
	owl:onProperty :Curve_xMultiplier ;
	owl:minQualifiedCardinality "0"^^xsd:nonNegativeInteger ;
	owl:onDataRange <https://w3id.org/netbeheer/IECCIM/TC57CIM/IEC61970/Base/Domain#UnitMultiplier> .

:Curve rdfs:subClassOf _:genid158 .

_:genid158 a owl:Restriction ;
	owl:onProperty :Curve_xUnit ;
	owl:minQualifiedCardinality "0"^^xsd:nonNegativeInteger ;
	owl:onDataRange <https://w3id.org/netbeheer/IECCIM/TC57CIM/IEC61970/Base/Domain#UnitSymbol> .

:Curve rdfs:subClassOf _:genid159 .

_:genid159 a owl:Restriction ;
	owl:onProperty :Curve_y1Multiplier ;
	owl:minQualifiedCardinality "0"^^xsd:nonNegativeInteger ;
	owl:onDataRange <https://w3id.org/netbeheer/IECCIM/TC57CIM/IEC61970/Base/Domain#UnitMultiplier> .

:Curve rdfs:subClassOf _:genid160 .

_:genid160 a owl:Restriction ;
	owl:onProperty :Curve_y1Unit ;
	owl:minQualifiedCardinality "0"^^xsd:nonNegativeInteger ;
	owl:onDataRange <https://w3id.org/netbeheer/IECCIM/TC57CIM/IEC61970/Base/Domain#UnitSymbol> .

:Curve rdfs:subClassOf _:genid161 .

_:genid161 a owl:Restriction ;
	owl:onProperty :Curve_y2Multiplier ;
	owl:minQualifiedCardinality "0"^^xsd:nonNegativeInteger ;
	owl:onDataRange <https://w3id.org/netbeheer/IECCIM/TC57CIM/IEC61970/Base/Domain#UnitMultiplier> .

:Curve rdfs:subClassOf _:genid162 .

_:genid162 a owl:Restriction ;
	owl:onProperty :Curve_y2Unit ;
	owl:minQualifiedCardinality "0"^^xsd:nonNegativeInteger ;
	owl:onDataRange <https://w3id.org/netbeheer/IECCIM/TC57CIM/IEC61970/Base/Domain#UnitSymbol> .

:Curve rdfs:subClassOf _:genid163 .

_:genid163 a owl:Restriction ;
	owl:onProperty :Curve_y3Multiplier ;
	owl:minQualifiedCardinality "0"^^xsd:nonNegativeInteger ;
	owl:onDataRange <https://w3id.org/netbeheer/IECCIM/TC57CIM/IEC61970/Base/Domain#UnitMultiplier> .

:Curve rdfs:subClassOf _:genid164 .

_:genid164 a owl:Restriction ;
	owl:onProperty :Curve_y3Unit ;
	owl:minQualifiedCardinality "0"^^xsd:nonNegativeInteger ;
	owl:onDataRange <https://w3id.org/netbeheer/IECCIM/TC57CIM/IEC61970/Base/Domain#UnitSymbol> .

:Curve rdfs:subClassOf _:genid165 .

_:genid165 a owl:Restriction ;
	owl:onProperty :Curve_curveStyle ;
	owl:maxQualifiedCardinality "1"^^xsd:nonNegativeInteger ;
	owl:onDataRange :CurveStyle .

:Curve rdfs:subClassOf _:genid166 .

_:genid166 a owl:Restriction ;
	owl:onProperty :Curve_xMultiplier ;
	owl:maxQualifiedCardinality "1"^^xsd:nonNegativeInteger ;
	owl:onDataRange <https://w3id.org/netbeheer/IECCIM/TC57CIM/IEC61970/Base/Domain#UnitMultiplier> .

:Curve rdfs:subClassOf _:genid167 .

_:genid167 a owl:Restriction ;
	owl:onProperty :Curve_xUnit ;
	owl:maxQualifiedCardinality "1"^^xsd:nonNegativeInteger ;
	owl:onDataRange <https://w3id.org/netbeheer/IECCIM/TC57CIM/IEC61970/Base/Domain#UnitSymbol> .

:Curve rdfs:subClassOf _:genid168 .

_:genid168 a owl:Restriction ;
	owl:onProperty :Curve_y1Multiplier ;
	owl:maxQualifiedCardinality "1"^^xsd:nonNegativeInteger ;
	owl:onDataRange <https://w3id.org/netbeheer/IECCIM/TC57CIM/IEC61970/Base/Domain#UnitMultiplier> .

:Curve rdfs:subClassOf _:genid169 .

_:genid169 a owl:Restriction ;
	owl:onProperty :Curve_y1Unit ;
	owl:maxQualifiedCardinality "1"^^xsd:nonNegativeInteger ;
	owl:onDataRange <https://w3id.org/netbeheer/IECCIM/TC57CIM/IEC61970/Base/Domain#UnitSymbol> .

:Curve rdfs:subClassOf _:genid170 .

_:genid170 a owl:Restriction ;
	owl:onProperty :Curve_y2Multiplier ;
	owl:maxQualifiedCardinality "1"^^xsd:nonNegativeInteger ;
	owl:onDataRange <https://w3id.org/netbeheer/IECCIM/TC57CIM/IEC61970/Base/Domain#UnitMultiplier> .

:Curve rdfs:subClassOf _:genid171 .

_:genid171 a owl:Restriction ;
	owl:onProperty :Curve_y2Unit ;
	owl:maxQualifiedCardinality "1"^^xsd:nonNegativeInteger ;
	owl:onDataRange <https://w3id.org/netbeheer/IECCIM/TC57CIM/IEC61970/Base/Domain#UnitSymbol> .

:Curve rdfs:subClassOf _:genid172 .

_:genid172 a owl:Restriction ;
	owl:onProperty :Curve_y3Multiplier ;
	owl:maxQualifiedCardinality "1"^^xsd:nonNegativeInteger ;
	owl:onDataRange <https://w3id.org/netbeheer/IECCIM/TC57CIM/IEC61970/Base/Domain#UnitMultiplier> .

:Curve rdfs:subClassOf _:genid173 .

_:genid173 a owl:Restriction ;
	owl:onProperty :Curve_y3Unit ;
	owl:maxQualifiedCardinality "1"^^xsd:nonNegativeInteger ;
	owl:onDataRange <https://w3id.org/netbeheer/IECCIM/TC57CIM/IEC61970/Base/Domain#UnitSymbol> .

:Curve rdfs:comment """A multi-purpose curve or functional relationship between an independent variable (X-axis) and dependent (Y-axis) variables. 
""" .
# 
# https://w3id.org/netbeheer/IECCIM/TC57CIM/IEC61970/Base/Core#CurveData

:CurveData a owl:Class ;
	rdfs:subClassOf _:genid174 .

_:genid174 a owl:Restriction ;
	owl:onProperty :CurveData_Curve ;
	owl:minQualifiedCardinality "0"^^xsd:nonNegativeInteger ;
	owl:onClass :CurveData .

:CurveData rdfs:subClassOf _:genid175 .

_:genid175 a owl:Restriction ;
	owl:onProperty :CurveData_xvalue ;
	owl:minQualifiedCardinality "0"^^xsd:nonNegativeInteger ;
	owl:onDataRange xsd:float .

:CurveData rdfs:subClassOf _:genid176 .

_:genid176 a owl:Restriction ;
	owl:onProperty :CurveData_y1value ;
	owl:minQualifiedCardinality "0"^^xsd:nonNegativeInteger ;
	owl:onDataRange xsd:float .

:CurveData rdfs:subClassOf _:genid177 .

_:genid177 a owl:Restriction ;
	owl:onProperty :CurveData_y2value ;
	owl:minQualifiedCardinality "0"^^xsd:nonNegativeInteger ;
	owl:onDataRange xsd:float .

:CurveData rdfs:subClassOf _:genid178 .

_:genid178 a owl:Restriction ;
	owl:onProperty :CurveData_y3value ;
	owl:minQualifiedCardinality "0"^^xsd:nonNegativeInteger ;
	owl:onDataRange xsd:float .

:CurveData rdfs:subClassOf _:genid179 .

_:genid179 a owl:Restriction ;
	owl:onProperty :CurveData_xvalue ;
	owl:maxQualifiedCardinality "1"^^xsd:nonNegativeInteger ;
	owl:onDataRange xsd:float .

:CurveData rdfs:subClassOf _:genid180 .

_:genid180 a owl:Restriction ;
	owl:onProperty :CurveData_y1value ;
	owl:maxQualifiedCardinality "1"^^xsd:nonNegativeInteger ;
	owl:onDataRange xsd:float .

:CurveData rdfs:subClassOf _:genid181 .

_:genid181 a owl:Restriction ;
	owl:onProperty :CurveData_y2value ;
	owl:maxQualifiedCardinality "1"^^xsd:nonNegativeInteger ;
	owl:onDataRange xsd:float .

:CurveData rdfs:subClassOf _:genid182 .

_:genid182 a owl:Restriction ;
	owl:onProperty :CurveData_y3value ;
	owl:maxQualifiedCardinality "1"^^xsd:nonNegativeInteger ;
	owl:onDataRange xsd:float .

:CurveData rdfs:comment """Multi-purpose data points for defining a curve.  The use of this generic class is discouraged if a more specific class  can be used to specify the x and y axis values along with their specific data types.
""" .
# 
# https://w3id.org/netbeheer/IECCIM/TC57CIM/IEC61970/Base/Core#Equipment

:Equipment a owl:Class ;
	rdfs:subClassOf :PowerSystemResource , _:genid183 .

_:genid183 a owl:Restriction ;
	owl:onProperty :Equipment_EquipmentContainer ;
	owl:minQualifiedCardinality "0"^^xsd:nonNegativeInteger ;
	owl:onClass :Equipment .

:Equipment rdfs:subClassOf _:genid184 .

_:genid184 a owl:Restriction ;
	owl:onProperty :Equipment_LimitDependencyModel ;
	owl:minQualifiedCardinality "0"^^xsd:nonNegativeInteger ;
	owl:onClass :Equipment .

:Equipment rdfs:subClassOf _:genid185 .

_:genid185 a owl:Restriction ;
	owl:onProperty :Equipment_OperationalLimitSet ;
	owl:minQualifiedCardinality "0"^^xsd:nonNegativeInteger ;
	owl:onClass :Equipment .

:Equipment rdfs:subClassOf _:genid186 .

_:genid186 a owl:Restriction ;
	owl:onProperty :Equipment_OperationalRestrictions ;
	owl:minQualifiedCardinality "0"^^xsd:nonNegativeInteger ;
	owl:onClass :Equipment .

:Equipment rdfs:subClassOf _:genid187 .

_:genid187 a owl:Restriction ;
	owl:onProperty :Equipment_Outages ;
	owl:minQualifiedCardinality "0"^^xsd:nonNegativeInteger ;
	owl:onClass :Equipment .

:Equipment rdfs:subClassOf _:genid188 .

_:genid188 a owl:Restriction ;
	owl:onProperty :Equipment_UsagePoints ;
	owl:minQualifiedCardinality "0"^^xsd:nonNegativeInteger ;
	owl:onClass :Equipment .

:Equipment rdfs:subClassOf _:genid189 .

_:genid189 a owl:Restriction ;
	owl:onProperty :Equipment_WeatherStation ;
	owl:minQualifiedCardinality "0"^^xsd:nonNegativeInteger ;
	owl:onClass :Equipment .

:Equipment rdfs:subClassOf _:genid190 .

_:genid190 a owl:Restriction ;
	owl:onProperty :Equipment_ContingencyEquipment ;
	owl:qualifiedCardinality "1"^^xsd:nonNegativeInteger ;
	owl:onClass :Equipment .

:Equipment rdfs:subClassOf _:genid191 .

_:genid191 a owl:Restriction ;
	owl:onProperty :Equipment_EqiupmentLimitSeriesComponent ;
	owl:qualifiedCardinality "1"^^xsd:nonNegativeInteger ;
	owl:onClass :Equipment .

:Equipment rdfs:subClassOf _:genid192 .

_:genid192 a owl:Restriction ;
	owl:onProperty :Equipment_PinEquipment ;
	owl:qualifiedCardinality "1"^^xsd:nonNegativeInteger ;
	owl:onClass :Equipment .

:Equipment rdfs:subClassOf _:genid193 .

_:genid193 a owl:Restriction ;
	owl:onProperty :Equipment_ProtectiveActionEquipment ;
	owl:qualifiedCardinality "1"^^xsd:nonNegativeInteger ;
	owl:onClass :Equipment .

:Equipment rdfs:subClassOf _:genid194 .

_:genid194 a owl:Restriction ;
	owl:onProperty :Equipment_LimitDependencyModel ;
	owl:maxQualifiedCardinality "1"^^xsd:nonNegativeInteger ;
	owl:onClass :Equipment .

:Equipment rdfs:subClassOf _:genid195 .

_:genid195 a owl:Restriction ;
	owl:onProperty :Equipment_OperationalLimitSet ;
	owl:maxQualifiedCardinality "1"^^xsd:nonNegativeInteger ;
	owl:onClass :Equipment .

:Equipment rdfs:subClassOf _:genid196 .

_:genid196 a owl:Restriction ;
	owl:onProperty :Equipment_aggregate ;
	owl:minQualifiedCardinality "0"^^xsd:nonNegativeInteger ;
	owl:onDataRange xsd:boolean .

:Equipment rdfs:subClassOf _:genid197 .

_:genid197 a owl:Restriction ;
	owl:onProperty :Equipment_inService ;
	owl:minQualifiedCardinality "0"^^xsd:nonNegativeInteger ;
	owl:onDataRange xsd:boolean .

:Equipment rdfs:subClassOf _:genid198 .

_:genid198 a owl:Restriction ;
	owl:onProperty :Equipment_normallyInService ;
	owl:minQualifiedCardinality "0"^^xsd:nonNegativeInteger ;
	owl:onDataRange xsd:boolean .

:Equipment rdfs:subClassOf _:genid199 .

_:genid199 a owl:Restriction ;
	owl:onProperty :Equipment_aggregate ;
	owl:maxQualifiedCardinality "1"^^xsd:nonNegativeInteger ;
	owl:onDataRange xsd:boolean .

:Equipment rdfs:subClassOf _:genid200 .

_:genid200 a owl:Restriction ;
	owl:onProperty :Equipment_inService ;
	owl:maxQualifiedCardinality "1"^^xsd:nonNegativeInteger ;
	owl:onDataRange xsd:boolean .

:Equipment rdfs:subClassOf _:genid201 .

_:genid201 a owl:Restriction ;
	owl:onProperty :Equipment_normallyInService ;
	owl:maxQualifiedCardinality "1"^^xsd:nonNegativeInteger ;
	owl:onDataRange xsd:boolean .

:Equipment rdfs:comment "The parts of a power system that are physical devices, electronic or mechanical." .
# 
# https://w3id.org/netbeheer/IECCIM/TC57CIM/IEC61970/Base/Core#EquipmentContainer

:EquipmentContainer a owl:Class ;
	rdfs:subClassOf :ConnectivityNodeContainer , _:genid202 .

_:genid202 a owl:Restriction ;
	owl:onProperty :EquipmentContainer_Equipments ;
	owl:minQualifiedCardinality "0"^^xsd:nonNegativeInteger ;
	owl:onClass :EquipmentContainer .

:EquipmentContainer rdfs:subClassOf _:genid203 .

_:genid203 a owl:Restriction ;
	owl:onProperty :EquipmentContainer_Equipments ;
	owl:maxQualifiedCardinality "1"^^xsd:nonNegativeInteger ;
	owl:onClass :EquipmentContainer .

:EquipmentContainer rdfs:comment "A modeling construct to provide a root class for containing equipment. " .
# 
# https://w3id.org/netbeheer/IECCIM/TC57CIM/IEC61970/Base/Core#GeographicalRegion

:GeographicalRegion a owl:Class ;
	rdfs:subClassOf :IdentifiedObject , _:genid204 .

_:genid204 a owl:Restriction ;
	owl:onProperty :GeographicalRegion_Regions ;
	owl:minQualifiedCardinality "0"^^xsd:nonNegativeInteger ;
	owl:onClass :GeographicalRegion .

:GeographicalRegion rdfs:subClassOf _:genid205 .

_:genid205 a owl:Restriction ;
	owl:onProperty :GeographicalRegion_Regions ;
	owl:maxQualifiedCardinality "1"^^xsd:nonNegativeInteger ;
	owl:onClass :GeographicalRegion .

:GeographicalRegion rdfs:comment """A geographical region of a power system network model.
""" .
# 
# https://w3id.org/netbeheer/IECCIM/TC57CIM/IEC61970/Base/Core#IdentifiedObject

:IdentifiedObject a owl:Class ;
	rdfs:subClassOf _:genid206 .

_:genid206 a owl:Restriction ;
	owl:onProperty :IdentifiedObject_DiagramObjects ;
	owl:minQualifiedCardinality "0"^^xsd:nonNegativeInteger ;
	owl:onClass :IdentifiedObject .

:IdentifiedObject rdfs:subClassOf _:genid207 .

_:genid207 a owl:Restriction ;
	owl:onProperty :IdentifiedObject_PropertiesCIMDataObject ;
	owl:minQualifiedCardinality "0"^^xsd:nonNegativeInteger ;
	owl:onClass :IdentifiedObject .

:IdentifiedObject rdfs:subClassOf _:genid208 .

_:genid208 a owl:Restriction ;
	owl:onProperty :IdentifiedObject_Names ;
	owl:qualifiedCardinality "1"^^xsd:nonNegativeInteger ;
	owl:onClass :IdentifiedObject .

:IdentifiedObject rdfs:subClassOf _:genid209 .

_:genid209 a owl:Restriction ;
	owl:onProperty :IdentifiedObject_RegisteredCIMDataObject ;
	owl:qualifiedCardinality "1"^^xsd:nonNegativeInteger ;
	owl:onClass :IdentifiedObject .

:IdentifiedObject rdfs:subClassOf _:genid210 .

_:genid210 a owl:Restriction ;
	owl:onProperty :IdentifiedObject_DiagramObjects ;
	owl:maxQualifiedCardinality "1"^^xsd:nonNegativeInteger ;
	owl:onClass :IdentifiedObject .

:IdentifiedObject rdfs:subClassOf _:genid211 .

_:genid211 a owl:Restriction ;
	owl:onProperty :IdentifiedObject_PropertiesCIMDataObject ;
	owl:maxQualifiedCardinality "1"^^xsd:nonNegativeInteger ;
	owl:onClass :IdentifiedObject .

:IdentifiedObject rdfs:subClassOf _:genid212 .

_:genid212 a owl:Restriction ;
	owl:onProperty :IdentifiedObject_aliasName ;
	owl:minQualifiedCardinality "0"^^xsd:nonNegativeInteger ;
	owl:onDataRange xsd:string .

:IdentifiedObject rdfs:subClassOf _:genid213 .

_:genid213 a owl:Restriction ;
	owl:onProperty :IdentifiedObject_description ;
	owl:minQualifiedCardinality "0"^^xsd:nonNegativeInteger ;
	owl:onDataRange xsd:string .

:IdentifiedObject rdfs:subClassOf _:genid214 .

_:genid214 a owl:Restriction ;
	owl:onProperty :IdentifiedObject_mRID ;
	owl:minQualifiedCardinality "0"^^xsd:nonNegativeInteger ;
	owl:onDataRange xsd:string .

:IdentifiedObject rdfs:subClassOf _:genid215 .

_:genid215 a owl:Restriction ;
	owl:onProperty :IdentifiedObject_name ;
	owl:minQualifiedCardinality "0"^^xsd:nonNegativeInteger ;
	owl:onDataRange xsd:string .

:IdentifiedObject rdfs:subClassOf _:genid216 .

_:genid216 a owl:Restriction ;
	owl:onProperty :IdentifiedObject_aliasName ;
	owl:maxQualifiedCardinality "1"^^xsd:nonNegativeInteger ;
	owl:onDataRange xsd:string .

:IdentifiedObject rdfs:subClassOf _:genid217 .

_:genid217 a owl:Restriction ;
	owl:onProperty :IdentifiedObject_description ;
	owl:maxQualifiedCardinality "1"^^xsd:nonNegativeInteger ;
	owl:onDataRange xsd:string .

:IdentifiedObject rdfs:subClassOf _:genid218 .

_:genid218 a owl:Restriction ;
	owl:onProperty :IdentifiedObject_mRID ;
	owl:maxQualifiedCardinality "1"^^xsd:nonNegativeInteger ;
	owl:onDataRange xsd:string .

:IdentifiedObject rdfs:subClassOf _:genid219 .

_:genid219 a owl:Restriction ;
	owl:onProperty :IdentifiedObject_name ;
	owl:maxQualifiedCardinality "1"^^xsd:nonNegativeInteger ;
	owl:onDataRange xsd:string .

:IdentifiedObject rdfs:comment "This is a root class to provide common identification for all classes needing identification and naming attributes." .
# 
# https://w3id.org/netbeheer/IECCIM/TC57CIM/IEC61970/Base/Core#IrregularIntervalSchedule

:IrregularIntervalSchedule a owl:Class ;
	rdfs:subClassOf :BasicIntervalSchedule , _:genid220 .

_:genid220 a owl:Restriction ;
	owl:onProperty :IrregularIntervalSchedule_TimePoints ;
	owl:qualifiedCardinality "1"^^xsd:nonNegativeInteger ;
	owl:onClass :IrregularIntervalSchedule .

:IrregularIntervalSchedule rdfs:comment """The schedule has time points where the time between them varies.
""" .
# 
# https://w3id.org/netbeheer/IECCIM/TC57CIM/IEC61970/Base/Core#IrregularTimePoint

:IrregularTimePoint a owl:Class ;
	rdfs:subClassOf _:genid221 .

_:genid221 a owl:Restriction ;
	owl:onProperty :IrregularTimePoint_IntervalSchedule ;
	owl:minQualifiedCardinality "1"^^xsd:nonNegativeInteger ;
	owl:onClass :IrregularTimePoint .

:IrregularTimePoint rdfs:subClassOf _:genid222 .

_:genid222 a owl:Restriction ;
	owl:onProperty :IrregularTimePoint_time ;
	owl:minQualifiedCardinality "0"^^xsd:nonNegativeInteger ;
	owl:onClass <https://w3id.org/netbeheer/IECCIM/TC57CIM/IEC61970/Base/Domain#Seconds> .

:IrregularTimePoint rdfs:subClassOf _:genid223 .

_:genid223 a owl:Restriction ;
	owl:onProperty :IrregularTimePoint_time ;
	owl:maxQualifiedCardinality "1"^^xsd:nonNegativeInteger ;
	owl:onClass <https://w3id.org/netbeheer/IECCIM/TC57CIM/IEC61970/Base/Domain#Seconds> .

:IrregularTimePoint rdfs:subClassOf _:genid224 .

_:genid224 a owl:Restriction ;
	owl:onProperty :IrregularTimePoint_value1 ;
	owl:minQualifiedCardinality "0"^^xsd:nonNegativeInteger ;
	owl:onDataRange xsd:float .

:IrregularTimePoint rdfs:subClassOf _:genid225 .

_:genid225 a owl:Restriction ;
	owl:onProperty :IrregularTimePoint_value2 ;
	owl:minQualifiedCardinality "0"^^xsd:nonNegativeInteger ;
	owl:onDataRange xsd:float .

:IrregularTimePoint rdfs:subClassOf _:genid226 .

_:genid226 a owl:Restriction ;
	owl:onProperty :IrregularTimePoint_value1 ;
	owl:maxQualifiedCardinality "1"^^xsd:nonNegativeInteger ;
	owl:onDataRange xsd:float .

:IrregularTimePoint rdfs:subClassOf _:genid227 .

_:genid227 a owl:Restriction ;
	owl:onProperty :IrregularTimePoint_value2 ;
	owl:maxQualifiedCardinality "1"^^xsd:nonNegativeInteger ;
	owl:onDataRange xsd:float .

:IrregularTimePoint rdfs:comment """TimePoints for a schedule where the time between the points varies.
""" .
# 
# https://w3id.org/netbeheer/IECCIM/TC57CIM/IEC61970/Base/Core#Name

:Name a owl:Class ;
	rdfs:subClassOf _:genid228 .

_:genid228 a owl:Restriction ;
	owl:onProperty :Name_IdentifiedObject ;
	owl:minQualifiedCardinality "0"^^xsd:nonNegativeInteger ;
	owl:onClass :Name .

:Name rdfs:subClassOf _:genid229 .

_:genid229 a owl:Restriction ;
	owl:onProperty :Name_NameType ;
	owl:minQualifiedCardinality "0"^^xsd:nonNegativeInteger ;
	owl:onClass :Name .

:Name rdfs:subClassOf _:genid230 .

_:genid230 a owl:Restriction ;
	owl:onProperty :Name_name ;
	owl:minQualifiedCardinality "0"^^xsd:nonNegativeInteger ;
	owl:onDataRange xsd:string .

:Name rdfs:subClassOf _:genid231 .

_:genid231 a owl:Restriction ;
	owl:onProperty :Name_name ;
	owl:maxQualifiedCardinality "1"^^xsd:nonNegativeInteger ;
	owl:onDataRange xsd:string .

:Name rdfs:comment """The Name class provides the means to define any number of human readable  names for an object. A name is <b>not</b> to be used for defining inter-object relationships. For inter-object relationships instead use the object identification 'mRID'.
""" .
# 
# https://w3id.org/netbeheer/IECCIM/TC57CIM/IEC61970/Base/Core#NameType

:NameType a owl:Class ;
	rdfs:subClassOf _:genid232 .

_:genid232 a owl:Restriction ;
	owl:onProperty :NameType_NameTypeAuthority ;
	owl:minQualifiedCardinality "0"^^xsd:nonNegativeInteger ;
	owl:onClass :NameType .

:NameType rdfs:subClassOf _:genid233 .

_:genid233 a owl:Restriction ;
	owl:onProperty :NameType_Names ;
	owl:qualifiedCardinality "1"^^xsd:nonNegativeInteger ;
	owl:onClass :NameType .

:NameType rdfs:subClassOf _:genid234 .

_:genid234 a owl:Restriction ;
	owl:onProperty :NameType_description ;
	owl:minQualifiedCardinality "0"^^xsd:nonNegativeInteger ;
	owl:onDataRange xsd:string .

:NameType rdfs:subClassOf _:genid235 .

_:genid235 a owl:Restriction ;
	owl:onProperty :NameType_name ;
	owl:minQualifiedCardinality "0"^^xsd:nonNegativeInteger ;
	owl:onDataRange xsd:string .

:NameType rdfs:subClassOf _:genid236 .

_:genid236 a owl:Restriction ;
	owl:onProperty :NameType_description ;
	owl:maxQualifiedCardinality "1"^^xsd:nonNegativeInteger ;
	owl:onDataRange xsd:string .

:NameType rdfs:subClassOf _:genid237 .

_:genid237 a owl:Restriction ;
	owl:onProperty :NameType_name ;
	owl:maxQualifiedCardinality "1"^^xsd:nonNegativeInteger ;
	owl:onDataRange xsd:string .

:NameType rdfs:comment """Type of name. Possible values for attribute 'name' are implementation dependent but standard profiles may specify types. An enterprise may have multiple IT systems each having its own local name for the same object, e.g. a planning system may have different names from an EMS. An object may also have different names within the same IT system, e.g. localName as defined in CIM version 14. The definition from CIM14 is:
The localName is a human readable name of the object. It is a free text name local to a node in a naming hierarchy similar to a file directory structure. A power system related naming hierarchy may be: Substation, VoltageLevel, Equipment etc. Children of the same parent in such a hierarchy have names that typically are unique among them.
""" .
# 
# https://w3id.org/netbeheer/IECCIM/TC57CIM/IEC61970/Base/Core#NameTypeAuthority

:NameTypeAuthority a owl:Class ;
	rdfs:subClassOf _:genid238 .

_:genid238 a owl:Restriction ;
	owl:onProperty :NameTypeAuthority_NameTypes ;
	owl:minQualifiedCardinality "0"^^xsd:nonNegativeInteger ;
	owl:onClass :NameTypeAuthority .

:NameTypeAuthority rdfs:subClassOf _:genid239 .

_:genid239 a owl:Restriction ;
	owl:onProperty :NameTypeAuthority_NameTypes ;
	owl:maxQualifiedCardinality "1"^^xsd:nonNegativeInteger ;
	owl:onClass :NameTypeAuthority .

:NameTypeAuthority rdfs:subClassOf _:genid240 .

_:genid240 a owl:Restriction ;
	owl:onProperty :NameTypeAuthority_description ;
	owl:minQualifiedCardinality "0"^^xsd:nonNegativeInteger ;
	owl:onDataRange xsd:string .

:NameTypeAuthority rdfs:subClassOf _:genid241 .

_:genid241 a owl:Restriction ;
	owl:onProperty :NameTypeAuthority_name ;
	owl:minQualifiedCardinality "0"^^xsd:nonNegativeInteger ;
	owl:onDataRange xsd:string .

:NameTypeAuthority rdfs:subClassOf _:genid242 .

_:genid242 a owl:Restriction ;
	owl:onProperty :NameTypeAuthority_description ;
	owl:maxQualifiedCardinality "1"^^xsd:nonNegativeInteger ;
	owl:onDataRange xsd:string .

:NameTypeAuthority rdfs:subClassOf _:genid243 .

_:genid243 a owl:Restriction ;
	owl:onProperty :NameTypeAuthority_name ;
	owl:maxQualifiedCardinality "1"^^xsd:nonNegativeInteger ;
	owl:onDataRange xsd:string .

:NameTypeAuthority rdfs:comment """Authority responsible for creation and management of names of a given type; typically an organization or an enterprise system.
""" .
# 
# https://w3id.org/netbeheer/IECCIM/TC57CIM/IEC61970/Base/Core#OperatingParticipant

:OperatingParticipant a owl:Class ;
	rdfs:subClassOf :IdentifiedObject , _:genid244 .

_:genid244 a owl:Restriction ;
	owl:onProperty :OperatingParticipant_OperatingShare ;
	owl:qualifiedCardinality "1"^^xsd:nonNegativeInteger ;
	owl:onClass :OperatingParticipant .

:OperatingParticipant rdfs:comment """An operator of multiple power system resource objects. Note multple operating participants may operate the same power system resource object.   This can be used for modeling jointly owned units where each owner operates as a contractual share.
""" .
# 
# https://w3id.org/netbeheer/IECCIM/TC57CIM/IEC61970/Base/Core#OperatingShare

:OperatingShare a owl:Class ;
	rdfs:subClassOf _:genid245 .

_:genid245 a owl:Restriction ;
	owl:onProperty :OperatingShare_OperatingParticipant ;
	owl:minQualifiedCardinality "0"^^xsd:nonNegativeInteger ;
	owl:onClass :OperatingShare .

:OperatingShare rdfs:subClassOf _:genid246 .

_:genid246 a owl:Restriction ;
	owl:onProperty :OperatingShare_PowerSystemResource ;
	owl:minQualifiedCardinality "0"^^xsd:nonNegativeInteger ;
	owl:onClass :OperatingShare .

:OperatingShare rdfs:subClassOf _:genid247 .

_:genid247 a owl:Restriction ;
	owl:onProperty :OperatingShare_percentage ;
	owl:minQualifiedCardinality "0"^^xsd:nonNegativeInteger ;
	owl:onClass <https://w3id.org/netbeheer/IECCIM/TC57CIM/IEC61970/Base/Domain#PerCent> .

:OperatingShare rdfs:subClassOf _:genid248 .

_:genid248 a owl:Restriction ;
	owl:onProperty :OperatingShare_percentage ;
	owl:maxQualifiedCardinality "1"^^xsd:nonNegativeInteger ;
	owl:onClass <https://w3id.org/netbeheer/IECCIM/TC57CIM/IEC61970/Base/Domain#PerCent> .

:OperatingShare rdfs:comment """Specifies the operations contract relationship between a power system resource and a contract participant.
""" .
# 
# https://w3id.org/netbeheer/IECCIM/TC57CIM/IEC61970/Base/Core#PSRType

:PSRType a owl:Class ;
	rdfs:subClassOf :IdentifiedObject , _:genid249 .

_:genid249 a owl:Restriction ;
	owl:onProperty :PSRType_PowerSystemResources ;
	owl:minQualifiedCardinality "0"^^xsd:nonNegativeInteger ;
	owl:onClass :PSRType .

:PSRType rdfs:subClassOf _:genid250 .

_:genid250 a owl:Restriction ;
	owl:onProperty :PSRType_PowerSystemResources ;
	owl:maxQualifiedCardinality "1"^^xsd:nonNegativeInteger ;
	owl:onClass :PSRType .

:PSRType rdfs:comment """Classifying instances of the same class, e.g. overhead and underground ACLineSegments. This classification mechanism is intended to provide flexibility outside the scope of this standard, i.e. provide customisation that is non standard.
""" .
# 
# https://w3id.org/netbeheer/IECCIM/TC57CIM/IEC61970/Base/Core#PowerSystemResource

:PowerSystemResource a owl:Class ;
	rdfs:subClassOf :IdentifiedObject , _:genid251 .

_:genid251 a owl:Restriction ;
	owl:onProperty :PowerSystemResource_AssetDatasheet ;
	owl:minQualifiedCardinality "0"^^xsd:nonNegativeInteger ;
	owl:onClass :PowerSystemResource .

:PowerSystemResource rdfs:subClassOf _:genid252 .

_:genid252 a owl:Restriction ;
	owl:onProperty :PowerSystemResource_Assets ;
	owl:minQualifiedCardinality "0"^^xsd:nonNegativeInteger ;
	owl:onClass :PowerSystemResource .

:PowerSystemResource rdfs:subClassOf _:genid253 .

_:genid253 a owl:Restriction ;
	owl:onProperty :PowerSystemResource_Clearances ;
	owl:minQualifiedCardinality "0"^^xsd:nonNegativeInteger ;
	owl:onClass :PowerSystemResource .

:PowerSystemResource rdfs:subClassOf _:genid254 .

_:genid254 a owl:Restriction ;
	owl:onProperty :PowerSystemResource_Controls ;
	owl:minQualifiedCardinality "0"^^xsd:nonNegativeInteger ;
	owl:onClass :PowerSystemResource .

:PowerSystemResource rdfs:subClassOf _:genid255 .

_:genid255 a owl:Restriction ;
	owl:onProperty :PowerSystemResource_Location ;
	owl:minQualifiedCardinality "0"^^xsd:nonNegativeInteger ;
	owl:onClass :PowerSystemResource .

:PowerSystemResource rdfs:subClassOf _:genid256 .

_:genid256 a owl:Restriction ;
	owl:onProperty :PowerSystemResource_Measurements ;
	owl:minQualifiedCardinality "0"^^xsd:nonNegativeInteger ;
	owl:onClass :PowerSystemResource .

:PowerSystemResource rdfs:subClassOf _:genid257 .

_:genid257 a owl:Restriction ;
	owl:onProperty :PowerSystemResource_OperationalTags ;
	owl:minQualifiedCardinality "0"^^xsd:nonNegativeInteger ;
	owl:onClass :PowerSystemResource .

:PowerSystemResource rdfs:subClassOf _:genid258 .

_:genid258 a owl:Restriction ;
	owl:onProperty :PowerSystemResource_PSREvents ;
	owl:minQualifiedCardinality "0"^^xsd:nonNegativeInteger ;
	owl:onClass :PowerSystemResource .

:PowerSystemResource rdfs:subClassOf _:genid259 .

_:genid259 a owl:Restriction ;
	owl:onProperty :PowerSystemResource_PSRType ;
	owl:minQualifiedCardinality "0"^^xsd:nonNegativeInteger ;
	owl:onClass :PowerSystemResource .

:PowerSystemResource rdfs:subClassOf _:genid260 .

_:genid260 a owl:Restriction ;
	owl:onProperty :PowerSystemResource_ReportingGroup ;
	owl:minQualifiedCardinality "0"^^xsd:nonNegativeInteger ;
	owl:onClass :PowerSystemResource .

:PowerSystemResource rdfs:subClassOf _:genid261 .

_:genid261 a owl:Restriction ;
	owl:onProperty :PowerSystemResource_OperatingShare ;
	owl:qualifiedCardinality "1"^^xsd:nonNegativeInteger ;
	owl:onClass :PowerSystemResource .

:PowerSystemResource rdfs:subClassOf _:genid262 .

_:genid262 a owl:Restriction ;
	owl:onProperty :PowerSystemResource_Controls ;
	owl:maxQualifiedCardinality "1"^^xsd:nonNegativeInteger ;
	owl:onClass :PowerSystemResource .

:PowerSystemResource rdfs:subClassOf _:genid263 .

_:genid263 a owl:Restriction ;
	owl:onProperty :PowerSystemResource_Measurements ;
	owl:maxQualifiedCardinality "1"^^xsd:nonNegativeInteger ;
	owl:onClass :PowerSystemResource .

:PowerSystemResource rdfs:subClassOf _:genid264 .

_:genid264 a owl:Restriction ;
	owl:onProperty :PowerSystemResource_OperationalTags ;
	owl:maxQualifiedCardinality "1"^^xsd:nonNegativeInteger ;
	owl:onClass :PowerSystemResource .

:PowerSystemResource rdfs:subClassOf _:genid265 .

_:genid265 a owl:Restriction ;
	owl:onProperty :PowerSystemResource_PSREvents ;
	owl:maxQualifiedCardinality "1"^^xsd:nonNegativeInteger ;
	owl:onClass :PowerSystemResource .

:PowerSystemResource rdfs:comment """A power system resource can be an item of equipment such as a switch, an equipment container containing many individual items of equipment such as a substation, or an organisational entity such as sub-control area. Power system resources can have measurements associated.
""" .
# 
# https://w3id.org/netbeheer/IECCIM/TC57CIM/IEC61970/Base/Core#RegularIntervalSchedule

:RegularIntervalSchedule a owl:Class ;
	rdfs:subClassOf :BasicIntervalSchedule , _:genid266 .

_:genid266 a owl:Restriction ;
	owl:onProperty :RegularIntervalSchedule_timeStep ;
	owl:minQualifiedCardinality "0"^^xsd:nonNegativeInteger ;
	owl:onClass <https://w3id.org/netbeheer/IECCIM/TC57CIM/IEC61970/Base/Domain#Seconds> .

:RegularIntervalSchedule rdfs:subClassOf _:genid267 .

_:genid267 a owl:Restriction ;
	owl:onProperty :RegularIntervalSchedule_TimePoints ;
	owl:qualifiedCardinality "1"^^xsd:nonNegativeInteger ;
	owl:onClass :RegularIntervalSchedule .

:RegularIntervalSchedule rdfs:subClassOf _:genid268 .

_:genid268 a owl:Restriction ;
	owl:onProperty :RegularIntervalSchedule_timeStep ;
	owl:maxQualifiedCardinality "1"^^xsd:nonNegativeInteger ;
	owl:onClass <https://w3id.org/netbeheer/IECCIM/TC57CIM/IEC61970/Base/Domain#Seconds> .

:RegularIntervalSchedule rdfs:subClassOf _:genid269 .

_:genid269 a owl:Restriction ;
	owl:onProperty :RegularIntervalSchedule_endTime ;
	owl:minQualifiedCardinality "0"^^xsd:nonNegativeInteger ;
	owl:onDataRange xsd:dateTime .

:RegularIntervalSchedule rdfs:subClassOf _:genid270 .

_:genid270 a owl:Restriction ;
	owl:onProperty :RegularIntervalSchedule_endTime ;
	owl:maxQualifiedCardinality "1"^^xsd:nonNegativeInteger ;
	owl:onDataRange xsd:dateTime .

:RegularIntervalSchedule rdfs:comment """The schedule has time points where the time between them is constant.
""" .
# 
# https://w3id.org/netbeheer/IECCIM/TC57CIM/IEC61970/Base/Core#RegularTimePoint

:RegularTimePoint a owl:Class ;
	rdfs:subClassOf _:genid271 .

_:genid271 a owl:Restriction ;
	owl:onProperty :RegularTimePoint_IntervalSchedule ;
	owl:minQualifiedCardinality "1"^^xsd:nonNegativeInteger ;
	owl:onClass :RegularTimePoint .

:RegularTimePoint rdfs:subClassOf _:genid272 .

_:genid272 a owl:Restriction ;
	owl:onProperty :RegularTimePoint_sequenceNumber ;
	owl:minQualifiedCardinality "0"^^xsd:nonNegativeInteger ;
	owl:onDataRange xsd:nonNegativeInteger .

:RegularTimePoint rdfs:subClassOf _:genid273 .

_:genid273 a owl:Restriction ;
	owl:onProperty :RegularTimePoint_value1 ;
	owl:minQualifiedCardinality "0"^^xsd:nonNegativeInteger ;
	owl:onDataRange xsd:float .

:RegularTimePoint rdfs:subClassOf _:genid274 .

_:genid274 a owl:Restriction ;
	owl:onProperty :RegularTimePoint_value2 ;
	owl:minQualifiedCardinality "0"^^xsd:nonNegativeInteger ;
	owl:onDataRange xsd:float .

:RegularTimePoint rdfs:subClassOf _:genid275 .

_:genid275 a owl:Restriction ;
	owl:onProperty :RegularTimePoint_sequenceNumber ;
	owl:maxQualifiedCardinality "1"^^xsd:nonNegativeInteger ;
	owl:onDataRange xsd:nonNegativeInteger .

:RegularTimePoint rdfs:subClassOf _:genid276 .

_:genid276 a owl:Restriction ;
	owl:onProperty :RegularTimePoint_value1 ;
	owl:maxQualifiedCardinality "1"^^xsd:nonNegativeInteger ;
	owl:onDataRange xsd:float .

:RegularTimePoint rdfs:subClassOf _:genid277 .

_:genid277 a owl:Restriction ;
	owl:onProperty :RegularTimePoint_value2 ;
	owl:maxQualifiedCardinality "1"^^xsd:nonNegativeInteger ;
	owl:onDataRange xsd:float .

:RegularTimePoint rdfs:comment """Time point for a schedule where the time between the consecutive points is constant.
""" .
# 
# https://w3id.org/netbeheer/IECCIM/TC57CIM/IEC61970/Base/Core#ReportingGroup

:ReportingGroup a owl:Class ;
	rdfs:subClassOf :IdentifiedObject , _:genid278 .

_:genid278 a owl:Restriction ;
	owl:onProperty :ReportingGroup_BusNameMarker ;
	owl:minQualifiedCardinality "0"^^xsd:nonNegativeInteger ;
	owl:onClass :ReportingGroup .

:ReportingGroup rdfs:subClassOf _:genid279 .

_:genid279 a owl:Restriction ;
	owl:onProperty :ReportingGroup_PowerSystemResource ;
	owl:minQualifiedCardinality "0"^^xsd:nonNegativeInteger ;
	owl:onClass :ReportingGroup .

:ReportingGroup rdfs:subClassOf _:genid280 .

_:genid280 a owl:Restriction ;
	owl:onProperty :ReportingGroup_ReportingSuperGroup ;
	owl:minQualifiedCardinality "0"^^xsd:nonNegativeInteger ;
	owl:onClass :ReportingGroup .

:ReportingGroup rdfs:subClassOf _:genid281 .

_:genid281 a owl:Restriction ;
	owl:onProperty :ReportingGroup_TopologicalNode ;
	owl:minQualifiedCardinality "0"^^xsd:nonNegativeInteger ;
	owl:onClass :ReportingGroup .

:ReportingGroup rdfs:subClassOf _:genid282 .

_:genid282 a owl:Restriction ;
	owl:onProperty :ReportingGroup_BusNameMarker ;
	owl:maxQualifiedCardinality "1"^^xsd:nonNegativeInteger ;
	owl:onClass :ReportingGroup .

:ReportingGroup rdfs:subClassOf _:genid283 .

_:genid283 a owl:Restriction ;
	owl:onProperty :ReportingGroup_TopologicalNode ;
	owl:maxQualifiedCardinality "1"^^xsd:nonNegativeInteger ;
	owl:onClass :ReportingGroup .

:ReportingGroup rdfs:comment """A reporting group is used for various ad-hoc groupings used for reporting.
""" .
# 
# https://w3id.org/netbeheer/IECCIM/TC57CIM/IEC61970/Base/Core#ReportingSuperGroup

:ReportingSuperGroup a owl:Class ;
	rdfs:subClassOf :IdentifiedObject , _:genid284 .

_:genid284 a owl:Restriction ;
	owl:onProperty :ReportingSuperGroup_ReportingGroup ;
	owl:minQualifiedCardinality "0"^^xsd:nonNegativeInteger ;
	owl:onClass :ReportingSuperGroup .

:ReportingSuperGroup rdfs:subClassOf _:genid285 .

_:genid285 a owl:Restriction ;
	owl:onProperty :ReportingSuperGroup_ReportingGroup ;
	owl:maxQualifiedCardinality "1"^^xsd:nonNegativeInteger ;
	owl:onClass :ReportingSuperGroup .

:ReportingSuperGroup rdfs:comment "A reporting super group, groups reporting groups for a higher level report." .
# 
# https://w3id.org/netbeheer/IECCIM/TC57CIM/IEC61970/Base/Core#SubGeographicalRegion

:SubGeographicalRegion a owl:Class ;
	rdfs:subClassOf :IdentifiedObject , _:genid286 .

_:genid286 a owl:Restriction ;
	owl:onProperty :SubGeographicalRegion_DCLines ;
	owl:minQualifiedCardinality "0"^^xsd:nonNegativeInteger ;
	owl:onClass :SubGeographicalRegion .

:SubGeographicalRegion rdfs:subClassOf _:genid287 .

_:genid287 a owl:Restriction ;
	owl:onProperty :SubGeographicalRegion_Lines ;
	owl:minQualifiedCardinality "0"^^xsd:nonNegativeInteger ;
	owl:onClass :SubGeographicalRegion .

:SubGeographicalRegion rdfs:subClassOf _:genid288 .

_:genid288 a owl:Restriction ;
	owl:onProperty :SubGeographicalRegion_Region ;
	owl:minQualifiedCardinality "0"^^xsd:nonNegativeInteger ;
	owl:onClass :SubGeographicalRegion .

:SubGeographicalRegion rdfs:subClassOf _:genid289 .

_:genid289 a owl:Restriction ;
	owl:onProperty :SubGeographicalRegion_Substations ;
	owl:minQualifiedCardinality "0"^^xsd:nonNegativeInteger ;
	owl:onClass :SubGeographicalRegion .

:SubGeographicalRegion rdfs:subClassOf _:genid290 .

_:genid290 a owl:Restriction ;
	owl:onProperty :SubGeographicalRegion_DCLines ;
	owl:maxQualifiedCardinality "1"^^xsd:nonNegativeInteger ;
	owl:onClass :SubGeographicalRegion .

:SubGeographicalRegion rdfs:subClassOf _:genid291 .

_:genid291 a owl:Restriction ;
	owl:onProperty :SubGeographicalRegion_Lines ;
	owl:maxQualifiedCardinality "1"^^xsd:nonNegativeInteger ;
	owl:onClass :SubGeographicalRegion .

:SubGeographicalRegion rdfs:subClassOf _:genid292 .

_:genid292 a owl:Restriction ;
	owl:onProperty :SubGeographicalRegion_Substations ;
	owl:maxQualifiedCardinality "1"^^xsd:nonNegativeInteger ;
	owl:onClass :SubGeographicalRegion .

:SubGeographicalRegion rdfs:comment """A subset of a geographical region of a power system network model.
""" .
# 
# https://w3id.org/netbeheer/IECCIM/TC57CIM/IEC61970/Base/Core#Substation

:Substation a owl:Class ;
	rdfs:subClassOf :EquipmentContainer , _:genid293 .

_:genid293 a owl:Restriction ;
	owl:onProperty :Substation_Bays ;
	owl:minQualifiedCardinality "0"^^xsd:nonNegativeInteger ;
	owl:onClass :Substation .

:Substation rdfs:subClassOf _:genid294 .

_:genid294 a owl:Restriction ;
	owl:onProperty :Substation_DCConverterUnit ;
	owl:minQualifiedCardinality "0"^^xsd:nonNegativeInteger ;
	owl:onClass :Substation .

:Substation rdfs:subClassOf _:genid295 .

_:genid295 a owl:Restriction ;
	owl:onProperty :Substation_Region ;
	owl:minQualifiedCardinality "0"^^xsd:nonNegativeInteger ;
	owl:onClass :Substation .

:Substation rdfs:subClassOf _:genid296 .

_:genid296 a owl:Restriction ;
	owl:onProperty :Substation_VoltageLevels ;
	owl:qualifiedCardinality "1"^^xsd:nonNegativeInteger ;
	owl:onClass :Substation .

:Substation rdfs:subClassOf _:genid297 .

_:genid297 a owl:Restriction ;
	owl:onProperty :Substation_Bays ;
	owl:maxQualifiedCardinality "1"^^xsd:nonNegativeInteger ;
	owl:onClass :Substation .

:Substation rdfs:subClassOf _:genid298 .

_:genid298 a owl:Restriction ;
	owl:onProperty :Substation_DCConverterUnit ;
	owl:maxQualifiedCardinality "1"^^xsd:nonNegativeInteger ;
	owl:onClass :Substation .

:Substation rdfs:comment """A collection of equipment for purposes other than generation or utilization, through which electric energy in bulk is passed for the purposes of switching or modifying its characteristics. 
""" .
# 
# https://w3id.org/netbeheer/IECCIM/TC57CIM/IEC61970/Base/Core#Terminal

:Terminal a owl:Class ;
	rdfs:subClassOf :ACDCTerminal , _:genid299 .

_:genid299 a owl:Restriction ;
	owl:onProperty :Terminal_Bushing ;
	owl:minQualifiedCardinality "0"^^xsd:nonNegativeInteger ;
	owl:onClass :Terminal .

:Terminal rdfs:subClassOf _:genid300 .

_:genid300 a owl:Restriction ;
	owl:onProperty :Terminal_ConductingEquipment ;
	owl:minQualifiedCardinality "0"^^xsd:nonNegativeInteger ;
	owl:onClass :Terminal .

:Terminal rdfs:subClassOf _:genid301 .

_:genid301 a owl:Restriction ;
	owl:onProperty :Terminal_ConnectivityNode ;
	owl:minQualifiedCardinality "0"^^xsd:nonNegativeInteger ;
	owl:onClass :Terminal .

:Terminal rdfs:subClassOf _:genid302 .

_:genid302 a owl:Restriction ;
	owl:onProperty :Terminal_ConverterDCSides ;
	owl:minQualifiedCardinality "0"^^xsd:nonNegativeInteger ;
	owl:onClass :Terminal .

:Terminal rdfs:subClassOf _:genid303 .

_:genid303 a owl:Restriction ;
	owl:onProperty :Terminal_RegulatingControl ;
	owl:minQualifiedCardinality "0"^^xsd:nonNegativeInteger ;
	owl:onClass :Terminal .

:Terminal rdfs:subClassOf _:genid304 .

_:genid304 a owl:Restriction ;
	owl:onProperty :Terminal_TopologicalNode ;
	owl:minQualifiedCardinality "0"^^xsd:nonNegativeInteger ;
	owl:onClass :Terminal .

:Terminal rdfs:subClassOf _:genid305 .

_:genid305 a owl:Restriction ;
	owl:onProperty :Terminal_TransformerEnd ;
	owl:minQualifiedCardinality "0"^^xsd:nonNegativeInteger ;
	owl:onClass :Terminal .

:Terminal rdfs:subClassOf _:genid306 .

_:genid306 a owl:Restriction ;
	owl:onProperty :Terminal_AuxiliaryEquipment ;
	owl:qualifiedCardinality "1"^^xsd:nonNegativeInteger ;
	owl:onClass :Terminal .

:Terminal rdfs:subClassOf _:genid307 .

_:genid307 a owl:Restriction ;
	owl:onProperty :Terminal_BranchGroupTerminal ;
	owl:qualifiedCardinality "1"^^xsd:nonNegativeInteger ;
	owl:onClass :Terminal .

:Terminal rdfs:subClassOf _:genid308 .

_:genid308 a owl:Restriction ;
	owl:onProperty :Terminal_HasFirstMutualCoupling ;
	owl:qualifiedCardinality "1"^^xsd:nonNegativeInteger ;
	owl:onClass :Terminal .

:Terminal rdfs:subClassOf _:genid309 .

_:genid309 a owl:Restriction ;
	owl:onProperty :Terminal_HasSecondMutualCoupling ;
	owl:qualifiedCardinality "1"^^xsd:nonNegativeInteger ;
	owl:onClass :Terminal .

:Terminal rdfs:subClassOf _:genid310 .

_:genid310 a owl:Restriction ;
	owl:onProperty :Terminal_PinTerminal ;
	owl:qualifiedCardinality "1"^^xsd:nonNegativeInteger ;
	owl:onClass :Terminal .

:Terminal rdfs:subClassOf _:genid311 .

_:genid311 a owl:Restriction ;
	owl:onProperty :Terminal_RemoteInputSignal ;
	owl:qualifiedCardinality "1"^^xsd:nonNegativeInteger ;
	owl:onClass :Terminal .

:Terminal rdfs:subClassOf _:genid312 .

_:genid312 a owl:Restriction ;
	owl:onProperty :Terminal_SvPowerFlow ;
	owl:qualifiedCardinality "1"^^xsd:nonNegativeInteger ;
	owl:onClass :Terminal .

:Terminal rdfs:subClassOf _:genid313 .

_:genid313 a owl:Restriction ;
	owl:onProperty :Terminal_TieFlow ;
	owl:qualifiedCardinality "1"^^xsd:nonNegativeInteger ;
	owl:onClass :Terminal .

:Terminal rdfs:subClassOf _:genid314 .

_:genid314 a owl:Restriction ;
	owl:onProperty :Terminal_Bushing ;
	owl:maxQualifiedCardinality "1"^^xsd:nonNegativeInteger ;
	owl:onClass :Terminal .

:Terminal rdfs:subClassOf _:genid315 .

_:genid315 a owl:Restriction ;
	owl:onProperty :Terminal_ConverterDCSides ;
	owl:maxQualifiedCardinality "1"^^xsd:nonNegativeInteger ;
	owl:onClass :Terminal .

:Terminal rdfs:subClassOf _:genid316 .

_:genid316 a owl:Restriction ;
	owl:onProperty :Terminal_RegulatingControl ;
	owl:maxQualifiedCardinality "1"^^xsd:nonNegativeInteger ;
	owl:onClass :Terminal .

:Terminal rdfs:subClassOf _:genid317 .

_:genid317 a owl:Restriction ;
	owl:onProperty :Terminal_TransformerEnd ;
	owl:maxQualifiedCardinality "1"^^xsd:nonNegativeInteger ;
	owl:onClass :Terminal .

:Terminal rdfs:subClassOf _:genid318 .

_:genid318 a owl:Restriction ;
	owl:onProperty :Terminal_phases ;
	owl:minQualifiedCardinality "0"^^xsd:nonNegativeInteger ;
	owl:onDataRange :PhaseCode .

:Terminal rdfs:subClassOf _:genid319 .

_:genid319 a owl:Restriction ;
	owl:onProperty :Terminal_phases ;
	owl:maxQualifiedCardinality "1"^^xsd:nonNegativeInteger ;
	owl:onDataRange :PhaseCode .

:Terminal rdfs:comment "An AC electrical connection point to a piece of conducting equipment. Terminals are connected at physical connection points called connectivity nodes." .
# 
# https://w3id.org/netbeheer/IECCIM/TC57CIM/IEC61970/Base/Core#VoltageLevel

:VoltageLevel a owl:Class ;
	rdfs:subClassOf :EquipmentContainer , _:genid320 .

_:genid320 a owl:Restriction ;
	owl:onProperty :VoltageLevel_BaseVoltage ;
	owl:minQualifiedCardinality "0"^^xsd:nonNegativeInteger ;
	owl:onClass :VoltageLevel .

:VoltageLevel rdfs:subClassOf _:genid321 .

_:genid321 a owl:Restriction ;
	owl:onProperty :VoltageLevel_Bays ;
	owl:minQualifiedCardinality "0"^^xsd:nonNegativeInteger ;
	owl:onClass :VoltageLevel .

:VoltageLevel rdfs:subClassOf _:genid322 .

_:genid322 a owl:Restriction ;
	owl:onProperty :VoltageLevel_Substation ;
	owl:minQualifiedCardinality "0"^^xsd:nonNegativeInteger ;
	owl:onClass :VoltageLevel .

:VoltageLevel rdfs:subClassOf _:genid323 .

_:genid323 a owl:Restriction ;
	owl:onProperty :VoltageLevel_highVoltageLimit ;
	owl:minQualifiedCardinality "0"^^xsd:nonNegativeInteger ;
	owl:onClass <https://w3id.org/netbeheer/IECCIM/TC57CIM/IEC61970/Base/Domain#Voltage> .

:VoltageLevel rdfs:subClassOf _:genid324 .

_:genid324 a owl:Restriction ;
	owl:onProperty :VoltageLevel_lowVoltageLimit ;
	owl:minQualifiedCardinality "0"^^xsd:nonNegativeInteger ;
	owl:onClass <https://w3id.org/netbeheer/IECCIM/TC57CIM/IEC61970/Base/Domain#Voltage> .

:VoltageLevel rdfs:subClassOf _:genid325 .

_:genid325 a owl:Restriction ;
	owl:onProperty :VoltageLevel_Bays ;
	owl:maxQualifiedCardinality "1"^^xsd:nonNegativeInteger ;
	owl:onClass :VoltageLevel .

:VoltageLevel rdfs:subClassOf _:genid326 .

_:genid326 a owl:Restriction ;
	owl:onProperty :VoltageLevel_highVoltageLimit ;
	owl:maxQualifiedCardinality "1"^^xsd:nonNegativeInteger ;
	owl:onClass <https://w3id.org/netbeheer/IECCIM/TC57CIM/IEC61970/Base/Domain#Voltage> .

:VoltageLevel rdfs:subClassOf _:genid327 .

_:genid327 a owl:Restriction ;
	owl:onProperty :VoltageLevel_lowVoltageLimit ;
	owl:maxQualifiedCardinality "1"^^xsd:nonNegativeInteger ;
	owl:onClass <https://w3id.org/netbeheer/IECCIM/TC57CIM/IEC61970/Base/Domain#Voltage> .

:VoltageLevel rdfs:comment """A collection of equipment at one common system voltage forming a switchgear. The equipment typically consist of breakers, busbars, instrumentation, control, regulation and protection devices as well as assemblies of all these.
""" .
# 
# https://w3id.org/netbeheer/IECCIM/TC57CIM/IEC61970/Base/DC#ACDCConverter

<https://w3id.org/netbeheer/IECCIM/TC57CIM/IEC61970/Base/DC#ACDCConverter> a owl:Class ;
	rdfs:subClassOf _:genid328 .

_:genid328 a owl:Restriction ;
	owl:onProperty :ACDCConverter_PccTerminal ;
	owl:minQualifiedCardinality "0"^^xsd:nonNegativeInteger ;
	owl:onClass <https://w3id.org/netbeheer/IECCIM/TC57CIM/IEC61970/Base/DC#ACDCConverter> .
# 
# https://w3id.org/netbeheer/IECCIM/TC57CIM/IEC61970/Base/DC#DCConverterUnit

<https://w3id.org/netbeheer/IECCIM/TC57CIM/IEC61970/Base/DC#DCConverterUnit> a owl:Class ;
	rdfs:subClassOf _:genid329 .

_:genid329 a owl:Restriction ;
	owl:onProperty :DCConverterUnit_Substation ;
	owl:minQualifiedCardinality "0"^^xsd:nonNegativeInteger ;
	owl:onClass <https://w3id.org/netbeheer/IECCIM/TC57CIM/IEC61970/Base/DC#DCConverterUnit> .
# 
# https://w3id.org/netbeheer/IECCIM/TC57CIM/IEC61970/Base/DC#DCLine

<https://w3id.org/netbeheer/IECCIM/TC57CIM/IEC61970/Base/DC#DCLine> a owl:Class ;
	rdfs:subClassOf _:genid330 .

_:genid330 a owl:Restriction ;
	owl:onProperty :DCLine_Region ;
	owl:minQualifiedCardinality "0"^^xsd:nonNegativeInteger ;
	owl:onClass <https://w3id.org/netbeheer/IECCIM/TC57CIM/IEC61970/Base/DC#DCLine> .
# 
# https://w3id.org/netbeheer/IECCIM/TC57CIM/IEC61970/Base/DiagramLayout#DiagramObject

<https://w3id.org/netbeheer/IECCIM/TC57CIM/IEC61970/Base/DiagramLayout#DiagramObject> a owl:Class ;
	rdfs:subClassOf _:genid331 .

_:genid331 a owl:Restriction ;
	owl:onProperty :DiagramObject_IdentifiedObject ;
	owl:minQualifiedCardinality "0"^^xsd:nonNegativeInteger ;
	owl:onClass <https://w3id.org/netbeheer/IECCIM/TC57CIM/IEC61970/Base/DiagramLayout#DiagramObject> .
# 
# https://w3id.org/netbeheer/IECCIM/TC57CIM/IEC61970/Base/Domain#ApparentPower

<https://w3id.org/netbeheer/IECCIM/TC57CIM/IEC61970/Base/Domain#ApparentPower> a owl:Class .
# 
# https://w3id.org/netbeheer/IECCIM/TC57CIM/IEC61970/Base/Domain#Frequency

<https://w3id.org/netbeheer/IECCIM/TC57CIM/IEC61970/Base/Domain#Frequency> a owl:Class .
# 
# https://w3id.org/netbeheer/IECCIM/TC57CIM/IEC61970/Base/Domain#PerCent

<https://w3id.org/netbeheer/IECCIM/TC57CIM/IEC61970/Base/Domain#PerCent> a owl:Class .
# 
# https://w3id.org/netbeheer/IECCIM/TC57CIM/IEC61970/Base/Domain#Seconds

<https://w3id.org/netbeheer/IECCIM/TC57CIM/IEC61970/Base/Domain#Seconds> a owl:Class .
# 
# https://w3id.org/netbeheer/IECCIM/TC57CIM/IEC61970/Base/Domain#Voltage

<https://w3id.org/netbeheer/IECCIM/TC57CIM/IEC61970/Base/Domain#Voltage> a owl:Class .
# 
# https://w3id.org/netbeheer/IECCIM/TC57CIM/IEC61970/Base/Meas#Control

<https://w3id.org/netbeheer/IECCIM/TC57CIM/IEC61970/Base/Meas#Control> a owl:Class ;
	rdfs:subClassOf _:genid332 .

_:genid332 a owl:Restriction ;
	owl:onProperty :Control_PowerSystemResource ;
	owl:minQualifiedCardinality "0"^^xsd:nonNegativeInteger ;
	owl:onClass <https://w3id.org/netbeheer/IECCIM/TC57CIM/IEC61970/Base/Meas#Control> .
# 
# https://w3id.org/netbeheer/IECCIM/TC57CIM/IEC61970/Base/Meas#Measure

<https://w3id.org/netbeheer/IECCIM/TC57CIM/IEC61970/Base/Meas#Measure> a owl:Class ;
	rdfs:subClassOf _:genid333 .

_:genid333 a owl:Restriction ;
	owl:onProperty :Measure_PowerSystemResource ;
	owl:minQualifiedCardinality "0"^^xsd:nonNegativeInteger ;
	owl:onClass <https://w3id.org/netbeheer/IECCIM/TC57CIM/IEC61970/Base/Meas#Measure> .

<https://w3id.org/netbeheer/IECCIM/TC57CIM/IEC61970/Base/Meas#Measure> rdfs:subClassOf _:genid334 .

_:genid334 a owl:Restriction ;
	owl:onProperty :Measure_Terminal ;
	owl:minQualifiedCardinality "0"^^xsd:nonNegativeInteger ;
	owl:onClass <https://w3id.org/netbeheer/IECCIM/TC57CIM/IEC61970/Base/Meas#Measure> .
# 
# https://w3id.org/netbeheer/IECCIM/TC57CIM/IEC61970/Base/OperationalLimits#BranchGroupTerminal

<https://w3id.org/netbeheer/IECCIM/TC57CIM/IEC61970/Base/OperationalLimits#BranchGroupTerminal> a owl:Class ;
	rdfs:subClassOf _:genid335 .

_:genid335 a owl:Restriction ;
	owl:onProperty :BranchGroupTerminal_Terminal ;
	owl:minQualifiedCardinality "0"^^xsd:nonNegativeInteger ;
	owl:onClass <https://w3id.org/netbeheer/IECCIM/TC57CIM/IEC61970/Base/OperationalLimits#BranchGroupTerminal> .
# 
# https://w3id.org/netbeheer/IECCIM/TC57CIM/IEC61970/Base/OperationalLimits#OperationalLimitSet

<https://w3id.org/netbeheer/IECCIM/TC57CIM/IEC61970/Base/OperationalLimits#OperationalLimitSet> a owl:Class ;
	rdfs:subClassOf _:genid336 .

_:genid336 a owl:Restriction ;
	owl:onProperty :OperationalLimitSet_Equipment ;
	owl:minQualifiedCardinality "0"^^xsd:nonNegativeInteger ;
	owl:onClass <https://w3id.org/netbeheer/IECCIM/TC57CIM/IEC61970/Base/OperationalLimits#OperationalLimitSet> .

<https://w3id.org/netbeheer/IECCIM/TC57CIM/IEC61970/Base/OperationalLimits#OperationalLimitSet> rdfs:subClassOf _:genid337 .

_:genid337 a owl:Restriction ;
	owl:onProperty :OperationalLimitSet_Terminal ;
	owl:minQualifiedCardinality "0"^^xsd:nonNegativeInteger ;
	owl:onClass <https://w3id.org/netbeheer/IECCIM/TC57CIM/IEC61970/Base/OperationalLimits#OperationalLimitSet> .
# 
# https://w3id.org/netbeheer/IECCIM/TC57CIM/IEC61970/Base/Protection#ProtectionEquipment

<https://w3id.org/netbeheer/IECCIM/TC57CIM/IEC61970/Base/Protection#ProtectionEquipment> a owl:Class ;
	rdfs:subClassOf _:genid338 .

_:genid338 a owl:Restriction ;
	owl:onProperty :ProtectionEquipment_ConductingEquipments ;
	owl:minQualifiedCardinality "0"^^xsd:nonNegativeInteger ;
	owl:onClass <https://w3id.org/netbeheer/IECCIM/TC57CIM/IEC61970/Base/Protection#ProtectionEquipment> .
# 
# https://w3id.org/netbeheer/IECCIM/TC57CIM/IEC61970/Base/StateVariables#SvPowerFlow

<https://w3id.org/netbeheer/IECCIM/TC57CIM/IEC61970/Base/StateVariables#SvPowerFlow> a owl:Class ;
	rdfs:subClassOf _:genid339 .

_:genid339 a owl:Restriction ;
	owl:onProperty :SvPowerFlow_Terminal ;
	owl:minQualifiedCardinality "0"^^xsd:nonNegativeInteger ;
	owl:onClass <https://w3id.org/netbeheer/IECCIM/TC57CIM/IEC61970/Base/StateVariables#SvPowerFlow> .
# 
# https://w3id.org/netbeheer/IECCIM/TC57CIM/IEC61970/Base/StateVariables#SvStatus

<https://w3id.org/netbeheer/IECCIM/TC57CIM/IEC61970/Base/StateVariables#SvStatus> a owl:Class ;
	rdfs:subClassOf _:genid340 .

_:genid340 a owl:Restriction ;
	owl:onProperty :SvStatus_ConductingEquipment ;
	owl:minQualifiedCardinality "0"^^xsd:nonNegativeInteger ;
	owl:onClass <https://w3id.org/netbeheer/IECCIM/TC57CIM/IEC61970/Base/StateVariables#SvStatus> .
# 
# https://w3id.org/netbeheer/IECCIM/TC57CIM/IEC61970/Base/Topology#BusNameMarker

<https://w3id.org/netbeheer/IECCIM/TC57CIM/IEC61970/Base/Topology#BusNameMarker> a owl:Class ;
	rdfs:subClassOf _:genid341 .

_:genid341 a owl:Restriction ;
	owl:onProperty :BusNameMarker_ReportingGroup ;
	owl:minQualifiedCardinality "0"^^xsd:nonNegativeInteger ;
	owl:onClass <https://w3id.org/netbeheer/IECCIM/TC57CIM/IEC61970/Base/Topology#BusNameMarker> .

<https://w3id.org/netbeheer/IECCIM/TC57CIM/IEC61970/Base/Topology#BusNameMarker> rdfs:subClassOf _:genid342 .

_:genid342 a owl:Restriction ;
	owl:onProperty :BusNameMarker_Terminal ;
	owl:minQualifiedCardinality "0"^^xsd:nonNegativeInteger ;
	owl:onClass <https://w3id.org/netbeheer/IECCIM/TC57CIM/IEC61970/Base/Topology#BusNameMarker> .

<https://w3id.org/netbeheer/IECCIM/TC57CIM/IEC61970/Base/Topology#BusNameMarker> rdfs:subClassOf _:genid343 .

_:genid343 a owl:Restriction ;
	owl:onProperty :BusNameMarker_Terminal ;
	owl:maxQualifiedCardinality "1"^^xsd:nonNegativeInteger ;
	owl:onClass <https://w3id.org/netbeheer/IECCIM/TC57CIM/IEC61970/Base/Topology#BusNameMarker> .
# 
# https://w3id.org/netbeheer/IECCIM/TC57CIM/IEC61970/Base/Topology#TopologicalNode

<https://w3id.org/netbeheer/IECCIM/TC57CIM/IEC61970/Base/Topology#TopologicalNode> a owl:Class ;
	rdfs:subClassOf _:genid344 .

_:genid344 a owl:Restriction ;
	owl:onProperty :TopologicalNode_BaseVoltage ;
	owl:minQualifiedCardinality "0"^^xsd:nonNegativeInteger ;
	owl:onClass <https://w3id.org/netbeheer/IECCIM/TC57CIM/IEC61970/Base/Topology#TopologicalNode> .

<https://w3id.org/netbeheer/IECCIM/TC57CIM/IEC61970/Base/Topology#TopologicalNode> rdfs:subClassOf _:genid345 .

_:genid345 a owl:Restriction ;
	owl:onProperty :TopologicalNode_ConnectivityNodeContainer ;
	owl:minQualifiedCardinality "0"^^xsd:nonNegativeInteger ;
	owl:onClass <https://w3id.org/netbeheer/IECCIM/TC57CIM/IEC61970/Base/Topology#TopologicalNode> .

<https://w3id.org/netbeheer/IECCIM/TC57CIM/IEC61970/Base/Topology#TopologicalNode> rdfs:subClassOf _:genid346 .

_:genid346 a owl:Restriction ;
	owl:onProperty :TopologicalNode_ConnectivityNodes ;
	owl:minQualifiedCardinality "0"^^xsd:nonNegativeInteger ;
	owl:onClass <https://w3id.org/netbeheer/IECCIM/TC57CIM/IEC61970/Base/Topology#TopologicalNode> .

<https://w3id.org/netbeheer/IECCIM/TC57CIM/IEC61970/Base/Topology#TopologicalNode> rdfs:subClassOf _:genid347 .

_:genid347 a owl:Restriction ;
	owl:onProperty :TopologicalNode_ReportingGroup ;
	owl:minQualifiedCardinality "0"^^xsd:nonNegativeInteger ;
	owl:onClass <https://w3id.org/netbeheer/IECCIM/TC57CIM/IEC61970/Base/Topology#TopologicalNode> .

<https://w3id.org/netbeheer/IECCIM/TC57CIM/IEC61970/Base/Topology#TopologicalNode> rdfs:subClassOf _:genid348 .

_:genid348 a owl:Restriction ;
	owl:onProperty :TopologicalNode_Terminal ;
	owl:minQualifiedCardinality "0"^^xsd:nonNegativeInteger ;
	owl:onClass <https://w3id.org/netbeheer/IECCIM/TC57CIM/IEC61970/Base/Topology#TopologicalNode> .

<https://w3id.org/netbeheer/IECCIM/TC57CIM/IEC61970/Base/Topology#TopologicalNode> rdfs:subClassOf _:genid349 .

_:genid349 a owl:Restriction ;
	owl:onProperty :TopologicalNode_ConnectivityNodes ;
	owl:maxQualifiedCardinality "1"^^xsd:nonNegativeInteger ;
	owl:onClass <https://w3id.org/netbeheer/IECCIM/TC57CIM/IEC61970/Base/Topology#TopologicalNode> .

<https://w3id.org/netbeheer/IECCIM/TC57CIM/IEC61970/Base/Topology#TopologicalNode> rdfs:subClassOf _:genid350 .

_:genid350 a owl:Restriction ;
	owl:onProperty :TopologicalNode_Terminal ;
	owl:maxQualifiedCardinality "1"^^xsd:nonNegativeInteger ;
	owl:onClass <https://w3id.org/netbeheer/IECCIM/TC57CIM/IEC61970/Base/Topology#TopologicalNode> .
# 
# https://w3id.org/netbeheer/IECCIM/TC57CIM/IEC61970/Base/Wires#Line

<https://w3id.org/netbeheer/IECCIM/TC57CIM/IEC61970/Base/Wires#Line> a owl:Class ;
	rdfs:subClassOf _:genid351 .

_:genid351 a owl:Restriction ;
	owl:onProperty :Line_Region ;
	owl:minQualifiedCardinality "0"^^xsd:nonNegativeInteger ;
	owl:onClass <https://w3id.org/netbeheer/IECCIM/TC57CIM/IEC61970/Base/Wires#Line> .
# 
# https://w3id.org/netbeheer/IECCIM/TC57CIM/IEC61970/Base/Wires#MutualCoupling

<https://w3id.org/netbeheer/IECCIM/TC57CIM/IEC61970/Base/Wires#MutualCoupling> a owl:Class ;
	rdfs:subClassOf _:genid352 .

_:genid352 a owl:Restriction ;
	owl:onProperty :MutualCoupling_First_Terminal ;
	owl:minQualifiedCardinality "0"^^xsd:nonNegativeInteger ;
	owl:onClass <https://w3id.org/netbeheer/IECCIM/TC57CIM/IEC61970/Base/Wires#MutualCoupling> .

<https://w3id.org/netbeheer/IECCIM/TC57CIM/IEC61970/Base/Wires#MutualCoupling> rdfs:subClassOf _:genid353 .

_:genid353 a owl:Restriction ;
	owl:onProperty :MutualCoupling_Second_Terminal ;
	owl:minQualifiedCardinality "0"^^xsd:nonNegativeInteger ;
	owl:onClass <https://w3id.org/netbeheer/IECCIM/TC57CIM/IEC61970/Base/Wires#MutualCoupling> .
# 
# https://w3id.org/netbeheer/IECCIM/TC57CIM/IEC61970/Base/Wires#RegulatingControl

<https://w3id.org/netbeheer/IECCIM/TC57CIM/IEC61970/Base/Wires#RegulatingControl> a owl:Class ;
	rdfs:subClassOf _:genid354 .

_:genid354 a owl:Restriction ;
	owl:onProperty :RegulatingControl_Terminal ;
	owl:minQualifiedCardinality "0"^^xsd:nonNegativeInteger ;
	owl:onClass <https://w3id.org/netbeheer/IECCIM/TC57CIM/IEC61970/Base/Wires#RegulatingControl> .
# 
# https://w3id.org/netbeheer/IECCIM/TC57CIM/IEC61970/Base/Wires#TransformerEnd

<https://w3id.org/netbeheer/IECCIM/TC57CIM/IEC61970/Base/Wires#TransformerEnd> a owl:Class ;
	rdfs:subClassOf _:genid355 .

_:genid355 a owl:Restriction ;
	owl:onProperty :TransformerEnd_BaseVoltage ;
	owl:minQualifiedCardinality "0"^^xsd:nonNegativeInteger ;
	owl:onClass <https://w3id.org/netbeheer/IECCIM/TC57CIM/IEC61970/Base/Wires#TransformerEnd> .

<https://w3id.org/netbeheer/IECCIM/TC57CIM/IEC61970/Base/Wires#TransformerEnd> rdfs:subClassOf _:genid356 .

_:genid356 a owl:Restriction ;
	owl:onProperty :TransformerEnd_Terminal ;
	owl:minQualifiedCardinality "0"^^xsd:nonNegativeInteger ;
	owl:onClass <https://w3id.org/netbeheer/IECCIM/TC57CIM/IEC61970/Base/Wires#TransformerEnd> .
# 
# https://w3id.org/netbeheer/IECCIM/TC57CIM/IEC61970/Dynamics/StandardInterconnections#RemoteInputSignal

<https://w3id.org/netbeheer/IECCIM/TC57CIM/IEC61970/Dynamics/StandardInterconnections#RemoteInputSignal> a owl:Class ;
	rdfs:subClassOf _:genid357 .

_:genid357 a owl:Restriction ;
	owl:onProperty :RemoteInputSignal_Terminal ;
	owl:minQualifiedCardinality "0"^^xsd:nonNegativeInteger ;
	owl:onClass <https://w3id.org/netbeheer/IECCIM/TC57CIM/IEC61970/Dynamics/StandardInterconnections#RemoteInputSignal> .
# 
# https://w3id.org/netbeheer/IECCIM/TC57CIM/IEC61970/InfIEC61970/InfGenericDataset/CanonicalModel/GenericDatasetCore#CIMDataObject

<https://w3id.org/netbeheer/IECCIM/TC57CIM/IEC61970/InfIEC61970/InfGenericDataset/CanonicalModel/GenericDatasetCore#CIMDataObject> a owl:Class ;
	rdfs:subClassOf _:genid358 .

_:genid358 a owl:Restriction ;
	owl:onProperty :CIMDataObject_PropertiesObject ;
	owl:minQualifiedCardinality "0"^^xsd:nonNegativeInteger ;
	owl:onClass <https://w3id.org/netbeheer/IECCIM/TC57CIM/IEC61970/InfIEC61970/InfGenericDataset/CanonicalModel/GenericDatasetCore#CIMDataObject> .

<https://w3id.org/netbeheer/IECCIM/TC57CIM/IEC61970/InfIEC61970/InfGenericDataset/CanonicalModel/GenericDatasetCore#CIMDataObject> rdfs:subClassOf _:genid359 .

_:genid359 a owl:Restriction ;
	owl:onProperty :CIMDataObject_RegisteredObject ;
	owl:minQualifiedCardinality "0"^^xsd:nonNegativeInteger ;
	owl:onClass <https://w3id.org/netbeheer/IECCIM/TC57CIM/IEC61970/InfIEC61970/InfGenericDataset/CanonicalModel/GenericDatasetCore#CIMDataObject> .

<https://w3id.org/netbeheer/IECCIM/TC57CIM/IEC61970/InfIEC61970/InfGenericDataset/CanonicalModel/GenericDatasetCore#CIMDataObject> rdfs:subClassOf _:genid360 .

_:genid360 a owl:Restriction ;
	owl:onProperty :CIMDataObject_PropertiesObject ;
	owl:maxQualifiedCardinality "1"^^xsd:nonNegativeInteger ;
	owl:onClass <https://w3id.org/netbeheer/IECCIM/TC57CIM/IEC61970/InfIEC61970/InfGenericDataset/CanonicalModel/GenericDatasetCore#CIMDataObject> .
# 
# https://w3id.org/netbeheer/IECCIM/TC57CIM/IEC61970/InfIEC61970/InfOperationalLimits#EquipmentLimitSeriesComponent

<https://w3id.org/netbeheer/IECCIM/TC57CIM/IEC61970/InfIEC61970/InfOperationalLimits#EquipmentLimitSeriesComponent> a owl:Class ;
	rdfs:subClassOf _:genid361 .

_:genid361 a owl:Restriction ;
	owl:onProperty :EquipmentLimitSeriesComponent_Equipment ;
	owl:minQualifiedCardinality "0"^^xsd:nonNegativeInteger ;
	owl:onClass <https://w3id.org/netbeheer/IECCIM/TC57CIM/IEC61970/InfIEC61970/InfOperationalLimits#EquipmentLimitSeriesComponent> .
# 
# https://w3id.org/netbeheer/IECCIM/TC57CIM/IEC61970/InfIEC61970/InfOperationalLimits#LimitDependency

<https://w3id.org/netbeheer/IECCIM/TC57CIM/IEC61970/InfIEC61970/InfOperationalLimits#LimitDependency> a owl:Class ;
	rdfs:subClassOf _:genid362 .

_:genid362 a owl:Restriction ;
	owl:onProperty :LimitDependency_Equipment ;
	owl:minQualifiedCardinality "0"^^xsd:nonNegativeInteger ;
	owl:onClass <https://w3id.org/netbeheer/IECCIM/TC57CIM/IEC61970/InfIEC61970/InfOperationalLimits#LimitDependency> .
# 
# https://w3id.org/netbeheer/IECCIM/TC57CIM/IEC61970/InfIEC61970/InfOperationalLimits#WeatherStation

<https://w3id.org/netbeheer/IECCIM/TC57CIM/IEC61970/InfIEC61970/InfOperationalLimits#WeatherStation> a owl:Class ;
	rdfs:subClassOf _:genid363 .

_:genid363 a owl:Restriction ;
	owl:onProperty :WeatherStation_Equipment ;
	owl:minQualifiedCardinality "0"^^xsd:nonNegativeInteger ;
	owl:onClass <https://w3id.org/netbeheer/IECCIM/TC57CIM/IEC61970/InfIEC61970/InfOperationalLimits#WeatherStation> .
# 
# https://w3id.org/netbeheer/IECCIM/TC57CIM/IEC61970/InfIEC61970/InfSIPS#PinEquipment

<https://w3id.org/netbeheer/IECCIM/TC57CIM/IEC61970/InfIEC61970/InfSIPS#PinEquipment> a owl:Class ;
	rdfs:subClassOf _:genid364 .

_:genid364 a owl:Restriction ;
	owl:onProperty :PinEquipment_Equipment ;
	owl:minQualifiedCardinality "0"^^xsd:nonNegativeInteger ;
	owl:onClass <https://w3id.org/netbeheer/IECCIM/TC57CIM/IEC61970/InfIEC61970/InfSIPS#PinEquipment> .
# 
# https://w3id.org/netbeheer/IECCIM/TC57CIM/IEC61970/InfIEC61970/InfSIPS#PinTerminal

<https://w3id.org/netbeheer/IECCIM/TC57CIM/IEC61970/InfIEC61970/InfSIPS#PinTerminal> a owl:Class ;
	rdfs:subClassOf _:genid365 .

_:genid365 a owl:Restriction ;
	owl:onProperty :PinTerminal_Terminal ;
	owl:minQualifiedCardinality "0"^^xsd:nonNegativeInteger ;
	owl:onClass <https://w3id.org/netbeheer/IECCIM/TC57CIM/IEC61970/InfIEC61970/InfSIPS#PinTerminal> .
# 
# https://w3id.org/netbeheer/IECCIM/TC57CIM/IEC61970/InfIEC61970/InfSIPS#ProtectiveActionAdjustment

<https://w3id.org/netbeheer/IECCIM/TC57CIM/IEC61970/InfIEC61970/InfSIPS#ProtectiveActionAdjustment> a owl:Class ;
	rdfs:subClassOf _:genid366 .

_:genid366 a owl:Restriction ;
	owl:onProperty :ProtectiveActionAdjustment_ConductingEquipment ;
	owl:minQualifiedCardinality "0"^^xsd:nonNegativeInteger ;
	owl:onClass <https://w3id.org/netbeheer/IECCIM/TC57CIM/IEC61970/InfIEC61970/InfSIPS#ProtectiveActionAdjustment> .
# 
# https://w3id.org/netbeheer/IECCIM/TC57CIM/IEC61970/InfIEC61970/InfSIPS#ProtectiveActionEquipment

<https://w3id.org/netbeheer/IECCIM/TC57CIM/IEC61970/InfIEC61970/InfSIPS#ProtectiveActionEquipment> a owl:Class ;
	rdfs:subClassOf _:genid367 .

_:genid367 a owl:Restriction ;
	owl:onProperty :ProtectiveActionEquipment_Equipment ;
	owl:minQualifiedCardinality "0"^^xsd:nonNegativeInteger ;
	owl:onClass <https://w3id.org/netbeheer/IECCIM/TC57CIM/IEC61970/InfIEC61970/InfSIPS#ProtectiveActionEquipment> .
# 
# Generated by the OWL API (version 4.5.9.2019-02-01T07:24:44Z) https://github.com/owlcs/owlapi
