@prefix : <https://w3id.org/netbeheer/IECCIM/TC57CIM/IEC61970/Base/Wires#> .
@prefix owl: <http://www.w3.org/2002/07/owl#> .
@prefix rdf: <http://www.w3.org/1999/02/22-rdf-syntax-ns#> .
@prefix xml: <http://www.w3.org/XML/1998/namespace> .
@prefix xsd: <http://www.w3.org/2001/XMLSchema#> .
@prefix rdfs: <http://www.w3.org/2000/01/rdf-schema#> .
@base <https://w3id.org/netbeheer/IECCIM/TC57CIM/IEC61970/Base/Wires#> .

<https://w3id.org/netbeheer/IECCIM/TC57CIM/IEC61970/Base/Wires#> rdf:type owl:Ontology .

#################################################################
#    Datatypes
#################################################################

###  https://w3id.org/netbeheer/IECCIM/TC57CIM/IEC61970/Base/Core#PhaseCode
<https://w3id.org/netbeheer/IECCIM/TC57CIM/IEC61970/Base/Core#PhaseCode> rdf:type rdfs:Datatype .


###  https://w3id.org/netbeheer/IECCIM/TC57CIM/IEC61970/Base/Domain#UnitMultiplier
<https://w3id.org/netbeheer/IECCIM/TC57CIM/IEC61970/Base/Domain#UnitMultiplier> rdf:type rdfs:Datatype .


###  https://w3id.org/netbeheer/IECCIM/TC57CIM/IEC61970/Base/Wires#AsynchronousMachineKind
:AsynchronousMachineKind rdf:type rdfs:Datatype ;
                         owl:equivalentClass [ rdf:type rdfs:Datatype ;
                                               owl:oneOf [ rdf:type rdf:List ;
                                                           rdf:first "generator" ;
                                                           rdf:rest [ rdf:type rdf:List ;
                                                                      rdf:first "motor" ;
                                                                      rdf:rest rdf:nil
                                                                    ]
                                                         ]
                                             ] .


###  https://w3id.org/netbeheer/IECCIM/TC57CIM/IEC61970/Base/Wires#CoolantType
:CoolantType rdf:type rdfs:Datatype ;
             owl:equivalentClass [ rdf:type rdfs:Datatype ;
                                   owl:oneOf [ rdf:type rdf:List ;
                                               rdf:first "air" ;
                                               rdf:rest [ rdf:type rdf:List ;
                                                          rdf:first "hydrogenGas" ;
                                                          rdf:rest [ rdf:type rdf:List ;
                                                                     rdf:first "water" ;
                                                                     rdf:rest rdf:nil
                                                                   ]
                                                        ]
                                             ]
                                 ] .


###  https://w3id.org/netbeheer/IECCIM/TC57CIM/IEC61970/Base/Wires#PetersenCoilModeKind
:PetersenCoilModeKind rdf:type rdfs:Datatype ;
                      owl:equivalentClass [ rdf:type rdfs:Datatype ;
                                            owl:oneOf [ rdf:type rdf:List ;
                                                        rdf:first "automaticPositioning" ;
                                                        rdf:rest [ rdf:type rdf:List ;
                                                                   rdf:first "fixed" ;
                                                                   rdf:rest [ rdf:type rdf:List ;
                                                                              rdf:first "manual" ;
                                                                              rdf:rest rdf:nil
                                                                            ]
                                                                 ]
                                                      ]
                                          ] .


###  https://w3id.org/netbeheer/IECCIM/TC57CIM/IEC61970/Base/Wires#PhaseShuntConnectionKind
:PhaseShuntConnectionKind rdf:type rdfs:Datatype ;
                          owl:equivalentClass [ rdf:type rdfs:Datatype ;
                                                owl:oneOf [ rdf:type rdf:List ;
                                                            rdf:first "D" ;
                                                            rdf:rest [ rdf:type rdf:List ;
                                                                       rdf:first "G" ;
                                                                       rdf:rest [ rdf:type rdf:List ;
                                                                                  rdf:first "I" ;
                                                                                  rdf:rest [ rdf:type rdf:List ;
                                                                                             rdf:first "Y" ;
                                                                                             rdf:rest [ rdf:type rdf:List ;
                                                                                                        rdf:first "Yn" ;
                                                                                                        rdf:rest rdf:nil
                                                                                                      ]
                                                                                           ]
                                                                                ]
                                                                     ]
                                                          ]
                                              ] .


###  https://w3id.org/netbeheer/IECCIM/TC57CIM/IEC61970/Base/Wires#RegulatingControlModeKind
:RegulatingControlModeKind rdf:type rdfs:Datatype ;
                           owl:equivalentClass [ rdf:type rdfs:Datatype ;
                                                 owl:oneOf [ rdf:type rdf:List ;
                                                             rdf:first "activePower" ;
                                                             rdf:rest [ rdf:type rdf:List ;
                                                                        rdf:first "admittance" ;
                                                                        rdf:rest [ rdf:type rdf:List ;
                                                                                   rdf:first "currentFlow" ;
                                                                                   rdf:rest [ rdf:type rdf:List ;
                                                                                              rdf:first "powerFactor" ;
                                                                                              rdf:rest [ rdf:type rdf:List ;
                                                                                                         rdf:first "reactivePower" ;
                                                                                                         rdf:rest [ rdf:type rdf:List ;
                                                                                                                    rdf:first "temperature" ;
                                                                                                                    rdf:rest [ rdf:type rdf:List ;
                                                                                                                               rdf:first "timeScheduled" ;
                                                                                                                               rdf:rest [ rdf:type rdf:List ;
                                                                                                                                          rdf:first "voltage" ;
                                                                                                                                          rdf:rest rdf:nil
                                                                                                                                        ]
                                                                                                                             ]
                                                                                                                  ]
                                                                                                       ]
                                                                                            ]
                                                                                 ]
                                                                      ]
                                                           ]
                                               ] .


###  https://w3id.org/netbeheer/IECCIM/TC57CIM/IEC61970/Base/Wires#SVCControlMode
:SVCControlMode rdf:type rdfs:Datatype ;
                owl:equivalentClass [ rdf:type rdfs:Datatype ;
                                      owl:oneOf [ rdf:type rdf:List ;
                                                  rdf:first "reactivePower" ;
                                                  rdf:rest [ rdf:type rdf:List ;
                                                             rdf:first "voltage" ;
                                                             rdf:rest rdf:nil
                                                           ]
                                                ]
                                    ] .


###  https://w3id.org/netbeheer/IECCIM/TC57CIM/IEC61970/Base/Wires#ShortCircuitRotorKind
:ShortCircuitRotorKind rdf:type rdfs:Datatype ;
                       owl:equivalentClass [ rdf:type rdfs:Datatype ;
                                             owl:oneOf [ rdf:type rdf:List ;
                                                         rdf:first "salientPole1" ;
                                                         rdf:rest [ rdf:type rdf:List ;
                                                                    rdf:first "salientPole2" ;
                                                                    rdf:rest [ rdf:type rdf:List ;
                                                                               rdf:first "turboSeries1" ;
                                                                               rdf:rest [ rdf:type rdf:List ;
                                                                                          rdf:first "turboSeries2" ;
                                                                                          rdf:rest rdf:nil
                                                                                        ]
                                                                             ]
                                                                  ]
                                                       ]
                                           ] .


###  https://w3id.org/netbeheer/IECCIM/TC57CIM/IEC61970/Base/Wires#SinglePhaseKind
:SinglePhaseKind rdf:type rdfs:Datatype ;
                 owl:equivalentClass [ rdf:type rdfs:Datatype ;
                                       owl:oneOf [ rdf:type rdf:List ;
                                                   rdf:first "A" ;
                                                   rdf:rest [ rdf:type rdf:List ;
                                                              rdf:first "B" ;
                                                              rdf:rest [ rdf:type rdf:List ;
                                                                         rdf:first "C" ;
                                                                         rdf:rest [ rdf:type rdf:List ;
                                                                                    rdf:first "N" ;
                                                                                    rdf:rest [ rdf:type rdf:List ;
                                                                                               rdf:first "s1" ;
                                                                                               rdf:rest [ rdf:type rdf:List ;
                                                                                                          rdf:first "s2" ;
                                                                                                          rdf:rest rdf:nil
                                                                                                        ]
                                                                                             ]
                                                                                  ]
                                                                       ]
                                                            ]
                                                 ]
                                     ] .


###  https://w3id.org/netbeheer/IECCIM/TC57CIM/IEC61970/Base/Wires#SynchronousMachineKind
:SynchronousMachineKind rdf:type rdfs:Datatype ;
                        owl:equivalentClass [ rdf:type rdfs:Datatype ;
                                              owl:oneOf [ rdf:type rdf:List ;
                                                          rdf:first "condenser" ;
                                                          rdf:rest [ rdf:type rdf:List ;
                                                                     rdf:first "generator" ;
                                                                     rdf:rest [ rdf:type rdf:List ;
                                                                                rdf:first "generatorOrCondenser" ;
                                                                                rdf:rest [ rdf:type rdf:List ;
                                                                                           rdf:first "generatorOrCondenserOrMotor" ;
                                                                                           rdf:rest [ rdf:type rdf:List ;
                                                                                                      rdf:first "generatorOrMotor" ;
                                                                                                      rdf:rest [ rdf:type rdf:List ;
                                                                                                                 rdf:first "motor" ;
                                                                                                                 rdf:rest [ rdf:type rdf:List ;
                                                                                                                            rdf:first "motorOrCondenser" ;
                                                                                                                            rdf:rest rdf:nil
                                                                                                                          ]
                                                                                                               ]
                                                                                                    ]
                                                                                         ]
                                                                              ]
                                                                   ]
                                                        ]
                                            ] .


###  https://w3id.org/netbeheer/IECCIM/TC57CIM/IEC61970/Base/Wires#SynchronousMachineOperatingMode
:SynchronousMachineOperatingMode rdf:type rdfs:Datatype ;
                                 owl:equivalentClass [ rdf:type rdfs:Datatype ;
                                                       owl:oneOf [ rdf:type rdf:List ;
                                                                   rdf:first "condenser" ;
                                                                   rdf:rest [ rdf:type rdf:List ;
                                                                              rdf:first "generator" ;
                                                                              rdf:rest [ rdf:type rdf:List ;
                                                                                         rdf:first "motor" ;
                                                                                         rdf:rest rdf:nil
                                                                                       ]
                                                                            ]
                                                                 ]
                                                     ] .


###  https://w3id.org/netbeheer/IECCIM/TC57CIM/IEC61970/Base/Wires#TransformerControlMode
:TransformerControlMode rdf:type rdfs:Datatype ;
                        owl:equivalentClass [ rdf:type rdfs:Datatype ;
                                              owl:oneOf [ rdf:type rdf:List ;
                                                          rdf:first "reactive" ;
                                                          rdf:rest [ rdf:type rdf:List ;
                                                                     rdf:first "volt" ;
                                                                     rdf:rest rdf:nil
                                                                   ]
                                                        ]
                                            ] .


###  https://w3id.org/netbeheer/IECCIM/TC57CIM/IEC61970/Base/Wires#WindingConnection
:WindingConnection rdf:type rdfs:Datatype ;
                   owl:equivalentClass [ rdf:type rdfs:Datatype ;
                                         owl:oneOf [ rdf:type rdf:List ;
                                                     rdf:first "A" ;
                                                     rdf:rest [ rdf:type rdf:List ;
                                                                rdf:first "D" ;
                                                                rdf:rest [ rdf:type rdf:List ;
                                                                           rdf:first "I" ;
                                                                           rdf:rest [ rdf:type rdf:List ;
                                                                                      rdf:first "Y" ;
                                                                                      rdf:rest [ rdf:type rdf:List ;
                                                                                                 rdf:first "Yn" ;
                                                                                                 rdf:rest [ rdf:type rdf:List ;
                                                                                                            rdf:first "Z" ;
                                                                                                            rdf:rest [ rdf:type rdf:List ;
                                                                                                                       rdf:first "Zn" ;
                                                                                                                       rdf:rest rdf:nil
                                                                                                                     ]
                                                                                                          ]
                                                                                               ]
                                                                                    ]
                                                                         ]
                                                              ]
                                                   ]
                                       ] .


#################################################################
#    Object Properties
#################################################################

###  https://w3id.org/netbeheer/IECCIM/TC57CIM/IEC61970/Base/Wires#ACLineSegmentPhase_ACLineSegment
:ACLineSegmentPhase_ACLineSegment rdf:type owl:ObjectProperty ;
                                  rdfs:domain :ACLineSegmentPhase ;
                                  rdfs:range :ACLineSegment ;
                                  rdfs:comment "The line segment phases which belong to the line segment.The line segment to which the phase belongs." .


###  https://w3id.org/netbeheer/IECCIM/TC57CIM/IEC61970/Base/Wires#ACLineSegment_ACLineSegmentPhases
:ACLineSegment_ACLineSegmentPhases rdf:type owl:ObjectProperty ;
                                   owl:inverseOf :ACLineSegmentPhase_ACLineSegment ;
                                   rdf:type owl:FunctionalProperty ;
                                   rdfs:domain :ACLineSegment ;
                                   rdfs:range :ACLineSegmentPhase ;
                                   rdfs:comment "The line segment phases which belong to the line segment.The line segment to which the phase belongs." .


###  https://w3id.org/netbeheer/IECCIM/TC57CIM/IEC61970/Base/Wires#ACLineSegment_Clamp
:ACLineSegment_Clamp rdf:type owl:ObjectProperty ,
                              owl:FunctionalProperty ;
                     rdfs:domain :ACLineSegment ;
                     rdfs:range :Clamp ;
                     rdfs:comment "The line segment to which the clamp is connected.The clamps connected to the line segment." .


###  https://w3id.org/netbeheer/IECCIM/TC57CIM/IEC61970/Base/Wires#ACLineSegment_Cut
:ACLineSegment_Cut rdf:type owl:ObjectProperty ;
                   owl:inverseOf :Cut_ACLineSegment ;
                   rdf:type owl:FunctionalProperty ;
                   rdfs:domain :ACLineSegment ;
                   rdfs:range :Cut ;
                   rdfs:comment "Cuts applied to the line segment.The line segment to which the cut is applied." .


###  https://w3id.org/netbeheer/IECCIM/TC57CIM/IEC61970/Base/Wires#ACLineSegment_LineGroundingAction
:ACLineSegment_LineGroundingAction rdf:type owl:ObjectProperty ;
                                   owl:inverseOf :GroundAction_AlongACLineSegment ;
                                   rdfs:domain :ACLineSegment ;
                                   rdfs:range <https://w3id.org/netbeheer/IECCIM/TC57CIM/IEC61968/Operations#GroundAction> ;
                                   rdfs:comment "Ground action involving clamp usage (for the case when the ground is applied along the line segment instead of at its terminals).The line segment that this ground action will affect. This is the only way to access relationship to clamp in case the ground needs to be placed along the line segment." .


###  https://w3id.org/netbeheer/IECCIM/TC57CIM/IEC61970/Base/Wires#ACLineSegment_LineJumpingAction
:ACLineSegment_LineJumpingAction rdf:type owl:ObjectProperty ;
                                 owl:inverseOf :JumperAction_AlongACLineSegments ;
                                 rdfs:domain :ACLineSegment ;
                                 rdfs:range <https://w3id.org/netbeheer/IECCIM/TC57CIM/IEC61968/Operations#JumperAction> ;
                                 rdfs:comment "Jumper action involving clamp usage (for the case when the jumper is applied along the line segment instead of at its terminals).The line segment that this jumper action will affect. This is the only way to access relationship to clamp in case the jumper needs to connect along the line segment." .


###  https://w3id.org/netbeheer/IECCIM/TC57CIM/IEC61970/Base/Wires#ACLineSegment_PerLengthImpedance
:ACLineSegment_PerLengthImpedance rdf:type owl:ObjectProperty ;
                                  owl:inverseOf :PerLengthImpedance_ACLineSegments ;
                                  rdfs:domain :ACLineSegment ;
                                  rdfs:range :PerLengthImpedance ;
                                  rdfs:comment "Per-length impedance of this line segment.All line segments described by this per-length impedance." .


###  https://w3id.org/netbeheer/IECCIM/TC57CIM/IEC61970/Base/Wires#ACLineSegment_WireSpacing
:ACLineSegment_WireSpacing rdf:type owl:ObjectProperty ;
                           owl:inverseOf :WireSpacing_ACLineSegments ;
                           rdfs:domain :ACLineSegment ;
                           rdfs:range <https://w3id.org/netbeheer/IECCIM/TC57CIM/IEC61968/AssetInfo#WireSpacing> ;
                           rdfs:comment "Wire spacing configuration for this line segment.All line segments described with this wire spacing configuration." .


###  https://w3id.org/netbeheer/IECCIM/TC57CIM/IEC61970/Base/Wires#ACLineSegment_b0ch
:ACLineSegment_b0ch rdf:type owl:ObjectProperty ;
                    rdfs:domain :ACLineSegment ;
                    rdfs:range <https://w3id.org/netbeheer/IECCIM/TC57CIM/IEC61970/Base/Domain#Susceptance> ;
                    rdfs:comment "Zero sequence shunt (charging) susceptance, uniformly distributed, of the entire line section." .


###  https://w3id.org/netbeheer/IECCIM/TC57CIM/IEC61970/Base/Wires#ACLineSegment_bch
:ACLineSegment_bch rdf:type owl:ObjectProperty ;
                   rdfs:domain :ACLineSegment ;
                   rdfs:range <https://w3id.org/netbeheer/IECCIM/TC57CIM/IEC61970/Base/Domain#Susceptance> ;
                   rdfs:comment "Positive sequence shunt (charging) susceptance, uniformly distributed, of the entire line section.  This value represents the full charging over the full length of the line." .


###  https://w3id.org/netbeheer/IECCIM/TC57CIM/IEC61970/Base/Wires#ACLineSegment_g0ch
:ACLineSegment_g0ch rdf:type owl:ObjectProperty ;
                    rdfs:domain :ACLineSegment ;
                    rdfs:range <https://w3id.org/netbeheer/IECCIM/TC57CIM/IEC61970/Base/Domain#Conductance> ;
                    rdfs:comment "Zero sequence shunt (charging) conductance, uniformly distributed, of the entire line section." .


###  https://w3id.org/netbeheer/IECCIM/TC57CIM/IEC61970/Base/Wires#ACLineSegment_gch
:ACLineSegment_gch rdf:type owl:ObjectProperty ;
                   rdfs:domain :ACLineSegment ;
                   rdfs:range <https://w3id.org/netbeheer/IECCIM/TC57CIM/IEC61970/Base/Domain#Conductance> ;
                   rdfs:comment "Positive sequence shunt (charging) conductance, uniformly distributed, of the entire line section." .


###  https://w3id.org/netbeheer/IECCIM/TC57CIM/IEC61970/Base/Wires#ACLineSegment_r
:ACLineSegment_r rdf:type owl:ObjectProperty ;
                 rdfs:domain :ACLineSegment ;
                 rdfs:range <https://w3id.org/netbeheer/IECCIM/TC57CIM/IEC61970/Base/Domain#Resistance> ;
                 rdfs:comment "Positive sequence series resistance of the entire line section." .


###  https://w3id.org/netbeheer/IECCIM/TC57CIM/IEC61970/Base/Wires#ACLineSegment_r0
:ACLineSegment_r0 rdf:type owl:ObjectProperty ;
                  rdfs:domain :ACLineSegment ;
                  rdfs:range <https://w3id.org/netbeheer/IECCIM/TC57CIM/IEC61970/Base/Domain#Resistance> ;
                  rdfs:comment "Zero sequence series resistance of the entire line section." .


###  https://w3id.org/netbeheer/IECCIM/TC57CIM/IEC61970/Base/Wires#ACLineSegment_shortCircuitEndTemperature
:ACLineSegment_shortCircuitEndTemperature rdf:type owl:ObjectProperty ;
                                          rdfs:domain :ACLineSegment ;
                                          rdfs:range <https://w3id.org/netbeheer/IECCIM/TC57CIM/IEC61970/Base/Domain#Temperature> ;
                                          rdfs:comment "Maximum permitted temperature at the end of SC for the calculation of minimum short-circuit currents. Used for short circuit data exchange according to IEC 60909" .


###  https://w3id.org/netbeheer/IECCIM/TC57CIM/IEC61970/Base/Wires#ACLineSegment_x
:ACLineSegment_x rdf:type owl:ObjectProperty ;
                 rdfs:domain :ACLineSegment ;
                 rdfs:range <https://w3id.org/netbeheer/IECCIM/TC57CIM/IEC61970/Base/Domain#Reactance> ;
                 rdfs:comment "Positive sequence series reactance of the entire line section." .


###  https://w3id.org/netbeheer/IECCIM/TC57CIM/IEC61970/Base/Wires#ACLineSegment_x0
:ACLineSegment_x0 rdf:type owl:ObjectProperty ;
                  rdfs:domain :ACLineSegment ;
                  rdfs:range <https://w3id.org/netbeheer/IECCIM/TC57CIM/IEC61970/Base/Domain#Reactance> ;
                  rdfs:comment "Zero sequence series reactance of the entire line section." .


###  https://w3id.org/netbeheer/IECCIM/TC57CIM/IEC61970/Base/Wires#AsynchronousMachineDynamics_AsynchronousMachine
:AsynchronousMachineDynamics_AsynchronousMachine rdf:type owl:ObjectProperty ;
                                                 rdfs:domain <https://w3id.org/netbeheer/IECCIM/TC57CIM/IEC61970/Dynamics/StandardModels/AsynchronousMachineDynamics#AsynchronousMachineDynamics> ;
                                                 rdfs:range :AsynchronousMachine ;
                                                 rdfs:comment "Asynchronous machine dynamics model used to describe dynamic behavior of this asynchronous machine.Asynchronous machine to which this asynchronous machine dynamics model applies." .


###  https://w3id.org/netbeheer/IECCIM/TC57CIM/IEC61970/Base/Wires#AsynchronousMachine_AsynchronousMachineDynamics
:AsynchronousMachine_AsynchronousMachineDynamics rdf:type owl:ObjectProperty ;
                                                 owl:inverseOf :AsynchronousMachineDynamics_AsynchronousMachine ;
                                                 rdf:type owl:FunctionalProperty ;
                                                 rdfs:domain :AsynchronousMachine ;
                                                 rdfs:range <https://w3id.org/netbeheer/IECCIM/TC57CIM/IEC61970/Dynamics/StandardModels/AsynchronousMachineDynamics#AsynchronousMachineDynamics> ;
                                                 rdfs:comment "Asynchronous machine dynamics model used to describe dynamic behavior of this asynchronous machine.Asynchronous machine to which this asynchronous machine dynamics model applies." .


###  https://w3id.org/netbeheer/IECCIM/TC57CIM/IEC61970/Base/Wires#AsynchronousMachine_efficiency
:AsynchronousMachine_efficiency rdf:type owl:ObjectProperty ;
                                rdfs:domain :AsynchronousMachine ;
                                rdfs:range <https://w3id.org/netbeheer/IECCIM/TC57CIM/IEC61970/Base/Domain#PerCent> ;
                                rdfs:comment "Efficiency of the asynchronous machine at nominal operation in percent. Indicator for converter drive motors. Used for short circuit data exchange according to IEC 60909" .


###  https://w3id.org/netbeheer/IECCIM/TC57CIM/IEC61970/Base/Wires#AsynchronousMachine_nominalFrequency
:AsynchronousMachine_nominalFrequency rdf:type owl:ObjectProperty ;
                                      rdfs:domain :AsynchronousMachine ;
                                      rdfs:range <https://w3id.org/netbeheer/IECCIM/TC57CIM/IEC61970/Base/Domain#Frequency> ;
                                      rdfs:comment "Nameplate data indicates if the machine is 50 or 60 Hz." .


###  https://w3id.org/netbeheer/IECCIM/TC57CIM/IEC61970/Base/Wires#AsynchronousMachine_nominalSpeed
:AsynchronousMachine_nominalSpeed rdf:type owl:ObjectProperty ;
                                  rdfs:domain :AsynchronousMachine ;
                                  rdfs:range <https://w3id.org/netbeheer/IECCIM/TC57CIM/IEC61970/Base/Domain#RotationSpeed> ;
                                  rdfs:comment "Nameplate data.  Depends on the slip and number of pole pairs." .


###  https://w3id.org/netbeheer/IECCIM/TC57CIM/IEC61970/Base/Wires#AsynchronousMachine_ratedMechanicalPower
:AsynchronousMachine_ratedMechanicalPower rdf:type owl:ObjectProperty ;
                                          rdfs:domain :AsynchronousMachine ;
                                          rdfs:range <https://w3id.org/netbeheer/IECCIM/TC57CIM/IEC61970/Base/Domain#ActivePower> ;
                                          rdfs:comment "Rated mechanical power (Pr in the IEC 60909-0). Used for short circuit data exchange according to IEC 60909." .


###  https://w3id.org/netbeheer/IECCIM/TC57CIM/IEC61970/Base/Wires#AsynchronousMachine_rr1
:AsynchronousMachine_rr1 rdf:type owl:ObjectProperty ;
                         rdfs:domain :AsynchronousMachine ;
                         rdfs:range <https://w3id.org/netbeheer/IECCIM/TC57CIM/IEC61970/Base/Domain#Resistance> ;
                         rdfs:comment """Damper 1 winding resistance.
""" .


###  https://w3id.org/netbeheer/IECCIM/TC57CIM/IEC61970/Base/Wires#AsynchronousMachine_rr2
:AsynchronousMachine_rr2 rdf:type owl:ObjectProperty ;
                         rdfs:domain :AsynchronousMachine ;
                         rdfs:range <https://w3id.org/netbeheer/IECCIM/TC57CIM/IEC61970/Base/Domain#Resistance> ;
                         rdfs:comment """Damper 2 winding resistance.
""" .


###  https://w3id.org/netbeheer/IECCIM/TC57CIM/IEC61970/Base/Wires#AsynchronousMachine_tpo
:AsynchronousMachine_tpo rdf:type owl:ObjectProperty ;
                         rdfs:domain :AsynchronousMachine ;
                         rdfs:range <https://w3id.org/netbeheer/IECCIM/TC57CIM/IEC61970/Base/Domain#Seconds> ;
                         rdfs:comment "Transient rotor time constant (greater than tppo)." .


###  https://w3id.org/netbeheer/IECCIM/TC57CIM/IEC61970/Base/Wires#AsynchronousMachine_tppo
:AsynchronousMachine_tppo rdf:type owl:ObjectProperty ;
                          rdfs:domain :AsynchronousMachine ;
                          rdfs:range <https://w3id.org/netbeheer/IECCIM/TC57CIM/IEC61970/Base/Domain#Seconds> ;
                          rdfs:comment """Sub-transient rotor time constant (greater than 0).
""" .


###  https://w3id.org/netbeheer/IECCIM/TC57CIM/IEC61970/Base/Wires#AsynchronousMachine_xlr1
:AsynchronousMachine_xlr1 rdf:type owl:ObjectProperty ;
                          rdfs:domain :AsynchronousMachine ;
                          rdfs:range <https://w3id.org/netbeheer/IECCIM/TC57CIM/IEC61970/Base/Domain#Reactance> ;
                          rdfs:comment """Damper 1 winding leakage reactance.
""" .


###  https://w3id.org/netbeheer/IECCIM/TC57CIM/IEC61970/Base/Wires#AsynchronousMachine_xlr2
:AsynchronousMachine_xlr2 rdf:type owl:ObjectProperty ;
                          rdfs:domain :AsynchronousMachine ;
                          rdfs:range <https://w3id.org/netbeheer/IECCIM/TC57CIM/IEC61970/Base/Domain#Reactance> ;
                          rdfs:comment """Damper 2 winding leakage reactance.
""" .


###  https://w3id.org/netbeheer/IECCIM/TC57CIM/IEC61970/Base/Wires#AsynchronousMachine_xm
:AsynchronousMachine_xm rdf:type owl:ObjectProperty ;
                        rdfs:domain :AsynchronousMachine ;
                        rdfs:range <https://w3id.org/netbeheer/IECCIM/TC57CIM/IEC61970/Base/Domain#Reactance> ;
                        rdfs:comment """Magnetizing reactance.
""" .


###  https://w3id.org/netbeheer/IECCIM/TC57CIM/IEC61970/Base/Wires#AsynchronousMachine_xp
:AsynchronousMachine_xp rdf:type owl:ObjectProperty ;
                        rdfs:domain :AsynchronousMachine ;
                        rdfs:range <https://w3id.org/netbeheer/IECCIM/TC57CIM/IEC61970/Base/Domain#Reactance> ;
                        rdfs:comment """Transient reactance (unsaturated) (greater than or equal to xpp).
""" .


###  https://w3id.org/netbeheer/IECCIM/TC57CIM/IEC61970/Base/Wires#AsynchronousMachine_xpp
:AsynchronousMachine_xpp rdf:type owl:ObjectProperty ;
                         rdfs:domain :AsynchronousMachine ;
                         rdfs:range <https://w3id.org/netbeheer/IECCIM/TC57CIM/IEC61970/Base/Domain#Reactance> ;
                         rdfs:comment """Sub-transient reactance (unsaturated) (greather than Xl).
""" .


###  https://w3id.org/netbeheer/IECCIM/TC57CIM/IEC61970/Base/Wires#AsynchronousMachine_xs
:AsynchronousMachine_xs rdf:type owl:ObjectProperty ;
                        rdfs:domain :AsynchronousMachine ;
                        rdfs:range <https://w3id.org/netbeheer/IECCIM/TC57CIM/IEC61970/Base/Domain#Reactance> ;
                        rdfs:comment """Synchronous reactance (greather than xp).
""" .


###  https://w3id.org/netbeheer/IECCIM/TC57CIM/IEC61970/Base/Wires#Breaker_inTransitTime
:Breaker_inTransitTime rdf:type owl:ObjectProperty ;
                       rdfs:domain :Breaker ;
                       rdfs:range <https://w3id.org/netbeheer/IECCIM/TC57CIM/IEC61970/Base/Domain#Seconds> ;
                       rdfs:comment """The transition time from open to close.
""" .


###  https://w3id.org/netbeheer/IECCIM/TC57CIM/IEC61970/Base/Wires#BusbarSection_VoltageControlZone
:BusbarSection_VoltageControlZone rdf:type owl:ObjectProperty ,
                                           owl:FunctionalProperty ;
                                  rdfs:domain :BusbarSection ;
                                  rdfs:range :VoltageControlZone ;
                                  rdfs:comment "A VoltageControlZone is controlled by a designated BusbarSection.A VoltageControlZone is controlled by a designated BusbarSection." .


###  https://w3id.org/netbeheer/IECCIM/TC57CIM/IEC61970/Base/Wires#BusbarSection_ipMax
:BusbarSection_ipMax rdf:type owl:ObjectProperty ;
                     rdfs:domain :BusbarSection ;
                     rdfs:range <https://w3id.org/netbeheer/IECCIM/TC57CIM/IEC61970/Base/Domain#CurrentFlow> ;
                     rdfs:comment """Maximum allowable peak short-circuit current of busbar (Ipmax in the IEC 60909-0). 
Mechanical limit of the busbar in the substation itself. Used for short circuit data exchange according to IEC 60909""" .


###  https://w3id.org/netbeheer/IECCIM/TC57CIM/IEC61970/Base/Wires#Clamp_ACLineSegment
:Clamp_ACLineSegment rdf:type owl:ObjectProperty ;
                     owl:inverseOf :ACLineSegment_Clamp ;
                     rdfs:domain :Clamp ;
                     rdfs:range :ACLineSegment ;
                     rdfs:comment "The line segment to which the clamp is connected.The clamps connected to the line segment." .


###  https://w3id.org/netbeheer/IECCIM/TC57CIM/IEC61970/Base/Wires#Clamp_lengthFromTerminal1
:Clamp_lengthFromTerminal1 rdf:type owl:ObjectProperty ;
                           rdfs:domain :Clamp ;
                           rdfs:range <https://w3id.org/netbeheer/IECCIM/TC57CIM/IEC61970/Base/Domain#Length> ;
                           rdfs:comment """The length to the place where the clamp is located starting from side one of the line segment, i.e. the line segment terminal with sequence number equal to 1.
""" .


###  https://w3id.org/netbeheer/IECCIM/TC57CIM/IEC61970/Base/Wires#CompositeSwitch_Switches
:CompositeSwitch_Switches rdf:type owl:ObjectProperty ;
                          rdfs:domain :CompositeSwitch ;
                          rdfs:range :Switch ;
                          rdfs:comment "Composite switch to which this Switch belongs.Switches contained in this Composite switch." .


###  https://w3id.org/netbeheer/IECCIM/TC57CIM/IEC61970/Base/Wires#Conductor_length
:Conductor_length rdf:type owl:ObjectProperty ;
                  rdfs:domain :Conductor ;
                  rdfs:range <https://w3id.org/netbeheer/IECCIM/TC57CIM/IEC61970/Base/Domain#Length> ;
                  rdfs:comment "Segment length for calculating line section capabilities" .


###  https://w3id.org/netbeheer/IECCIM/TC57CIM/IEC61970/Base/Wires#ConnectDisconnectFunction_Switches
:ConnectDisconnectFunction_Switches rdf:type owl:ObjectProperty ;
                                    rdfs:domain <https://w3id.org/netbeheer/IECCIM/TC57CIM/IEC61968/LoadControl#ConnectDisconnectFunction> ;
                                    rdfs:range :Switch ;
                                    rdfs:comment "" .


###  https://w3id.org/netbeheer/IECCIM/TC57CIM/IEC61970/Base/Wires#CutAction_Cut
:CutAction_Cut rdf:type owl:ObjectProperty ;
               rdfs:domain <https://w3id.org/netbeheer/IECCIM/TC57CIM/IEC61968/Operations#CutAction> ;
               rdfs:range :Cut ;
               rdfs:comment "Action taken with this cut.Cut on which this action is taken." .


###  https://w3id.org/netbeheer/IECCIM/TC57CIM/IEC61970/Base/Wires#Cut_ACLineSegment
:Cut_ACLineSegment rdf:type owl:ObjectProperty ;
                   rdfs:domain :Cut ;
                   rdfs:range :ACLineSegment ;
                   rdfs:comment "Cuts applied to the line segment.The line segment to which the cut is applied." .


###  https://w3id.org/netbeheer/IECCIM/TC57CIM/IEC61970/Base/Wires#Cut_CutAction
:Cut_CutAction rdf:type owl:ObjectProperty ;
               owl:inverseOf :CutAction_Cut ;
               rdfs:domain :Cut ;
               rdfs:range <https://w3id.org/netbeheer/IECCIM/TC57CIM/IEC61968/Operations#CutAction> ;
               rdfs:comment "Action taken with this cut.Cut on which this action is taken." .


###  https://w3id.org/netbeheer/IECCIM/TC57CIM/IEC61970/Base/Wires#Cut_lengthFromTerminal1
:Cut_lengthFromTerminal1 rdf:type owl:ObjectProperty ;
                         rdfs:domain :Cut ;
                         rdfs:range <https://w3id.org/netbeheer/IECCIM/TC57CIM/IEC61970/Base/Domain#Length> ;
                         rdfs:comment """The length to the place where the cut is located starting from side one of the cut line segment, i.e. the line segment Terminal with sequenceNumber equal to 1.
""" .


###  https://w3id.org/netbeheer/IECCIM/TC57CIM/IEC61970/Base/Wires#EarthFaultCompensator_r
:EarthFaultCompensator_r rdf:type owl:ObjectProperty ;
                         rdfs:domain :EarthFaultCompensator ;
                         rdfs:range <https://w3id.org/netbeheer/IECCIM/TC57CIM/IEC61970/Base/Domain#Resistance> ;
                         rdfs:comment "Nominal resistance of device." .


###  https://w3id.org/netbeheer/IECCIM/TC57CIM/IEC61970/Base/Wires#EnergyConsumerPhase_EnergyConsumer
:EnergyConsumerPhase_EnergyConsumer rdf:type owl:ObjectProperty ;
                                    owl:inverseOf :EnergyConsumer_EnergyConsumerPhase ;
                                    rdfs:domain :EnergyConsumerPhase ;
                                    rdfs:range :EnergyConsumer ;
                                    rdfs:comment "The energy consumer to which this phase belongs.The individual phase models for this energy consumer." .


###  https://w3id.org/netbeheer/IECCIM/TC57CIM/IEC61970/Base/Wires#EnergyConsumerPhase_pfixed
:EnergyConsumerPhase_pfixed rdf:type owl:ObjectProperty ;
                            rdfs:domain :EnergyConsumerPhase ;
                            rdfs:range <https://w3id.org/netbeheer/IECCIM/TC57CIM/IEC61970/Base/Domain#ActivePower> ;
                            rdfs:comment """Active power of the load that is a fixed quantity. Load sign convention is used, i.e. positive sign means flow out from a node.
""" .


###  https://w3id.org/netbeheer/IECCIM/TC57CIM/IEC61970/Base/Wires#EnergyConsumerPhase_pfixedPct
:EnergyConsumerPhase_pfixedPct rdf:type owl:ObjectProperty ;
                               rdfs:domain :EnergyConsumerPhase ;
                               rdfs:range <https://w3id.org/netbeheer/IECCIM/TC57CIM/IEC61970/Base/Domain#PerCent> ;
                               rdfs:comment """Fixed active power as per cent of load group fixed active power. Load sign convention is used, i.e. positive sign means flow out from a node.
""" .


###  https://w3id.org/netbeheer/IECCIM/TC57CIM/IEC61970/Base/Wires#EnergyConsumerPhase_qfixed
:EnergyConsumerPhase_qfixed rdf:type owl:ObjectProperty ;
                            rdfs:domain :EnergyConsumerPhase ;
                            rdfs:range <https://w3id.org/netbeheer/IECCIM/TC57CIM/IEC61970/Base/Domain#ReactivePower> ;
                            rdfs:comment """Reactive power of the load that is a fixed quantity. Load sign convention is used, i.e. positive sign means flow out from a node.
""" .


###  https://w3id.org/netbeheer/IECCIM/TC57CIM/IEC61970/Base/Wires#EnergyConsumerPhase_qfixedPct
:EnergyConsumerPhase_qfixedPct rdf:type owl:ObjectProperty ;
                               rdfs:domain :EnergyConsumerPhase ;
                               rdfs:range <https://w3id.org/netbeheer/IECCIM/TC57CIM/IEC61970/Base/Domain#PerCent> ;
                               rdfs:comment """Fixed reactive power as per cent of load group fixed reactive power. Load sign convention is used, i.e. positive sign means flow out from a node.
""" .


###  https://w3id.org/netbeheer/IECCIM/TC57CIM/IEC61970/Base/Wires#EnergyConsumer_EnergyConsumerPhase
:EnergyConsumer_EnergyConsumerPhase rdf:type owl:ObjectProperty ,
                                             owl:FunctionalProperty ;
                                    rdfs:domain :EnergyConsumer ;
                                    rdfs:range :EnergyConsumerPhase ;
                                    rdfs:comment "The energy consumer to which this phase belongs.The individual phase models for this energy consumer." .


###  https://w3id.org/netbeheer/IECCIM/TC57CIM/IEC61970/Base/Wires#EnergyConsumer_LoadDynamics
:EnergyConsumer_LoadDynamics rdf:type owl:ObjectProperty ;
                             owl:inverseOf :LoadDynamics_EnergyConsumer ;
                             rdfs:domain :EnergyConsumer ;
                             rdfs:range <https://w3id.org/netbeheer/IECCIM/TC57CIM/IEC61970/Dynamics/StandardModels/LoadDynamics#LoadDynamics> ;
                             rdfs:comment "Load dynamics model used to describe dynamic behavior of this energy consumer.Energy consumer to which this dynamics load model applies." .


###  https://w3id.org/netbeheer/IECCIM/TC57CIM/IEC61970/Base/Wires#EnergyConsumer_LoadResponse
:EnergyConsumer_LoadResponse rdf:type owl:ObjectProperty ;
                             rdfs:domain :EnergyConsumer ;
                             rdfs:range <https://w3id.org/netbeheer/IECCIM/TC57CIM/IEC61970/Base/LoadModel#LoadResponseCharacteristic> ;
                             rdfs:comment "The set of loads that have the response characteristics.The load response characteristic of this load.  If missing, this load is assumed to be constant power." .


###  https://w3id.org/netbeheer/IECCIM/TC57CIM/IEC61970/Base/Wires#EnergyConsumer_PowerCutZone
:EnergyConsumer_PowerCutZone rdf:type owl:ObjectProperty ;
                             owl:inverseOf :PowerCutZone_EnergyConsumers ;
                             rdfs:domain :EnergyConsumer ;
                             rdfs:range <https://w3id.org/netbeheer/IECCIM/TC57CIM/IEC61970/Base/LoadModel#PowerCutZone> ;
                             rdfs:comment "The  energy consumer is assigned to this power cut zone.Energy consumer is assigned to the power cut zone." .


###  https://w3id.org/netbeheer/IECCIM/TC57CIM/IEC61970/Base/Wires#EnergyConsumer_p
:EnergyConsumer_p rdf:type owl:ObjectProperty ;
                  rdfs:domain :EnergyConsumer ;
                  rdfs:range <https://w3id.org/netbeheer/IECCIM/TC57CIM/IEC61970/Base/Domain#ActivePower> ;
                  rdfs:comment """Active power of the load. Load sign convention is used, i.e. positive sign means flow out from a node.
For voltage dependent loads the value is at rated voltage.
Starting value for a steady state solution.""" .


###  https://w3id.org/netbeheer/IECCIM/TC57CIM/IEC61970/Base/Wires#EnergyConsumer_pfixed
:EnergyConsumer_pfixed rdf:type owl:ObjectProperty ;
                       rdfs:domain :EnergyConsumer ;
                       rdfs:range <https://w3id.org/netbeheer/IECCIM/TC57CIM/IEC61970/Base/Domain#ActivePower> ;
                       rdfs:comment """Active power of the load that is a fixed quantity. Load sign convention is used, i.e. positive sign means flow out from a node.
""" .


###  https://w3id.org/netbeheer/IECCIM/TC57CIM/IEC61970/Base/Wires#EnergyConsumer_pfixedPct
:EnergyConsumer_pfixedPct rdf:type owl:ObjectProperty ;
                          rdfs:domain :EnergyConsumer ;
                          rdfs:range <https://w3id.org/netbeheer/IECCIM/TC57CIM/IEC61970/Base/Domain#PerCent> ;
                          rdfs:comment """Fixed active power as per cent of load group fixed active power. Load sign convention is used, i.e. positive sign means flow out from a node.
""" .


###  https://w3id.org/netbeheer/IECCIM/TC57CIM/IEC61970/Base/Wires#EnergyConsumer_q
:EnergyConsumer_q rdf:type owl:ObjectProperty ;
                  rdfs:domain :EnergyConsumer ;
                  rdfs:range <https://w3id.org/netbeheer/IECCIM/TC57CIM/IEC61970/Base/Domain#ReactivePower> ;
                  rdfs:comment """Reactive power of the load. Load sign convention is used, i.e. positive sign means flow out from a node.
For voltage dependent loads the value is at rated voltage.
Starting value for a steady state solution.""" .


###  https://w3id.org/netbeheer/IECCIM/TC57CIM/IEC61970/Base/Wires#EnergyConsumer_qfixed
:EnergyConsumer_qfixed rdf:type owl:ObjectProperty ;
                       rdfs:domain :EnergyConsumer ;
                       rdfs:range <https://w3id.org/netbeheer/IECCIM/TC57CIM/IEC61970/Base/Domain#ReactivePower> ;
                       rdfs:comment """Reactive power of the load that is a fixed quantity. Load sign convention is used, i.e. positive sign means flow out from a node.
""" .


###  https://w3id.org/netbeheer/IECCIM/TC57CIM/IEC61970/Base/Wires#EnergyConsumer_qfixedPct
:EnergyConsumer_qfixedPct rdf:type owl:ObjectProperty ;
                          rdfs:domain :EnergyConsumer ;
                          rdfs:range <https://w3id.org/netbeheer/IECCIM/TC57CIM/IEC61970/Base/Domain#PerCent> ;
                          rdfs:comment """Fixed reactive power as per cent of load group fixed reactive power. Load sign convention is used, i.e. positive sign means flow out from a node.
""" .


###  https://w3id.org/netbeheer/IECCIM/TC57CIM/IEC61970/Base/Wires#EnergySchedulingType_EnergySource
:EnergySchedulingType_EnergySource rdf:type owl:ObjectProperty ;
                                   owl:inverseOf :EnergySource_EnergySchedulingType ;
                                   rdfs:domain <https://w3id.org/netbeheer/IECCIM/TC57CIM/IEC61970/InfIEC61970/InfEnergySource#EnergySchedulingType> ;
                                   rdfs:range :EnergySource ;
                                   rdfs:comment "Energy Source of a particular Energy Scheduling TypeEnergy Scheduling Type of an Energy Source" .


###  https://w3id.org/netbeheer/IECCIM/TC57CIM/IEC61970/Base/Wires#EnergySourceAction_EnergySource
:EnergySourceAction_EnergySource rdf:type owl:ObjectProperty ;
                                 rdfs:domain <https://w3id.org/netbeheer/IECCIM/TC57CIM/IEC61968/Operations#EnergySourceAction> ;
                                 rdfs:range :EnergySource ;
                                 rdfs:comment "Action taken with this energy source.Energy source on which this action is taken." .


###  https://w3id.org/netbeheer/IECCIM/TC57CIM/IEC61970/Base/Wires#EnergySourcePhase_EnergySource
:EnergySourcePhase_EnergySource rdf:type owl:ObjectProperty ;
                                rdfs:domain :EnergySourcePhase ;
                                rdfs:range :EnergySource ;
                                rdfs:comment "The individual phase information of the energy source.The energy sourceto which the phase belongs." .


###  https://w3id.org/netbeheer/IECCIM/TC57CIM/IEC61970/Base/Wires#EnergySource_EnergySchedulingType
:EnergySource_EnergySchedulingType rdf:type owl:ObjectProperty ;
                                   rdfs:domain :EnergySource ;
                                   rdfs:range <https://w3id.org/netbeheer/IECCIM/TC57CIM/IEC61970/InfIEC61970/InfEnergySource#EnergySchedulingType> ;
                                   rdfs:comment "Energy Source of a particular Energy Scheduling TypeEnergy Scheduling Type of an Energy Source" .


###  https://w3id.org/netbeheer/IECCIM/TC57CIM/IEC61970/Base/Wires#EnergySource_EnergySourceAction
:EnergySource_EnergySourceAction rdf:type owl:ObjectProperty ;
                                 owl:inverseOf :EnergySourceAction_EnergySource ;
                                 rdfs:domain :EnergySource ;
                                 rdfs:range <https://w3id.org/netbeheer/IECCIM/TC57CIM/IEC61968/Operations#EnergySourceAction> ;
                                 rdfs:comment "Action taken with this energy source.Energy source on which this action is taken." .


###  https://w3id.org/netbeheer/IECCIM/TC57CIM/IEC61970/Base/Wires#EnergySource_EnergySourcePhase
:EnergySource_EnergySourcePhase rdf:type owl:ObjectProperty ;
                                owl:inverseOf :EnergySourcePhase_EnergySource ;
                                rdf:type owl:FunctionalProperty ;
                                rdfs:domain :EnergySource ;
                                rdfs:range :EnergySourcePhase ;
                                rdfs:comment "The individual phase information of the energy source.The energy sourceto which the phase belongs." .


###  https://w3id.org/netbeheer/IECCIM/TC57CIM/IEC61970/Base/Wires#EnergySource_WindTurbineType3or4Dynamics
:EnergySource_WindTurbineType3or4Dynamics rdf:type owl:ObjectProperty ;
                                          owl:inverseOf :WindTurbineType3or4Dynamics_EnergySource ;
                                          rdf:type owl:FunctionalProperty ;
                                          rdfs:domain :EnergySource ;
                                          rdfs:range <https://w3id.org/netbeheer/IECCIM/TC57CIM/IEC61970/Dynamics/StandardModels/WindDynamics#WindTurbineType3or4Dynamics> ;
                                          rdfs:comment "Wind generator Type 3 or 4 dynamics model associated with this energy source.Energy Source (current source) with which this wind Type 3 or 4 dynamics model is asoociated." .


###  https://w3id.org/netbeheer/IECCIM/TC57CIM/IEC61970/Base/Wires#EnergySource_activePower
:EnergySource_activePower rdf:type owl:ObjectProperty ;
                          rdfs:domain :EnergySource ;
                          rdfs:range <https://w3id.org/netbeheer/IECCIM/TC57CIM/IEC61970/Base/Domain#ActivePower> ;
                          rdfs:comment """High voltage source active injection. Load sign convention is used, i.e. positive sign means flow out from a node.
Starting value for steady state solutions.""" .


###  https://w3id.org/netbeheer/IECCIM/TC57CIM/IEC61970/Base/Wires#EnergySource_nominalVoltage
:EnergySource_nominalVoltage rdf:type owl:ObjectProperty ;
                             rdfs:domain :EnergySource ;
                             rdfs:range <https://w3id.org/netbeheer/IECCIM/TC57CIM/IEC61970/Base/Domain#Voltage> ;
                             rdfs:comment "Phase-to-phase nominal voltage." .


###  https://w3id.org/netbeheer/IECCIM/TC57CIM/IEC61970/Base/Wires#EnergySource_r
:EnergySource_r rdf:type owl:ObjectProperty ;
                rdfs:domain :EnergySource ;
                rdfs:range <https://w3id.org/netbeheer/IECCIM/TC57CIM/IEC61970/Base/Domain#Resistance> ;
                rdfs:comment "Positive sequence Thevenin resistance." .


###  https://w3id.org/netbeheer/IECCIM/TC57CIM/IEC61970/Base/Wires#EnergySource_r0
:EnergySource_r0 rdf:type owl:ObjectProperty ;
                 rdfs:domain :EnergySource ;
                 rdfs:range <https://w3id.org/netbeheer/IECCIM/TC57CIM/IEC61970/Base/Domain#Resistance> ;
                 rdfs:comment "Zero sequence Thevenin resistance." .


###  https://w3id.org/netbeheer/IECCIM/TC57CIM/IEC61970/Base/Wires#EnergySource_reactivePower
:EnergySource_reactivePower rdf:type owl:ObjectProperty ;
                            rdfs:domain :EnergySource ;
                            rdfs:range <https://w3id.org/netbeheer/IECCIM/TC57CIM/IEC61970/Base/Domain#ReactivePower> ;
                            rdfs:comment """High voltage source reactive injection. Load sign convention is used, i.e. positive sign means flow out from a node.
Starting value for steady state solutions.""" .


###  https://w3id.org/netbeheer/IECCIM/TC57CIM/IEC61970/Base/Wires#EnergySource_rn
:EnergySource_rn rdf:type owl:ObjectProperty ;
                 rdfs:domain :EnergySource ;
                 rdfs:range <https://w3id.org/netbeheer/IECCIM/TC57CIM/IEC61970/Base/Domain#Resistance> ;
                 rdfs:comment "Negative sequence Thevenin resistance." .


###  https://w3id.org/netbeheer/IECCIM/TC57CIM/IEC61970/Base/Wires#EnergySource_voltageAngle
:EnergySource_voltageAngle rdf:type owl:ObjectProperty ;
                           rdfs:domain :EnergySource ;
                           rdfs:range <https://w3id.org/netbeheer/IECCIM/TC57CIM/IEC61970/Base/Domain#AngleRadians> ;
                           rdfs:comment "Phase angle of a-phase open circuit." .


###  https://w3id.org/netbeheer/IECCIM/TC57CIM/IEC61970/Base/Wires#EnergySource_voltageMagnitude
:EnergySource_voltageMagnitude rdf:type owl:ObjectProperty ;
                               rdfs:domain :EnergySource ;
                               rdfs:range <https://w3id.org/netbeheer/IECCIM/TC57CIM/IEC61970/Base/Domain#Voltage> ;
                               rdfs:comment "Phase-to-phase open circuit voltage magnitude." .


###  https://w3id.org/netbeheer/IECCIM/TC57CIM/IEC61970/Base/Wires#EnergySource_x
:EnergySource_x rdf:type owl:ObjectProperty ;
                rdfs:domain :EnergySource ;
                rdfs:range <https://w3id.org/netbeheer/IECCIM/TC57CIM/IEC61970/Base/Domain#Reactance> ;
                rdfs:comment "Positive sequence Thevenin reactance." .


###  https://w3id.org/netbeheer/IECCIM/TC57CIM/IEC61970/Base/Wires#EnergySource_x0
:EnergySource_x0 rdf:type owl:ObjectProperty ;
                 rdfs:domain :EnergySource ;
                 rdfs:range <https://w3id.org/netbeheer/IECCIM/TC57CIM/IEC61970/Base/Domain#Reactance> ;
                 rdfs:comment "Zero sequence Thevenin reactance." .


###  https://w3id.org/netbeheer/IECCIM/TC57CIM/IEC61970/Base/Wires#EnergySource_xn
:EnergySource_xn rdf:type owl:ObjectProperty ;
                 rdfs:domain :EnergySource ;
                 rdfs:range <https://w3id.org/netbeheer/IECCIM/TC57CIM/IEC61970/Base/Domain#Reactance> ;
                 rdfs:comment "Negative sequence Thevenin reactance." .


###  https://w3id.org/netbeheer/IECCIM/TC57CIM/IEC61970/Base/Wires#EquivalentInjection_ReactiveCapabilityCurve
:EquivalentInjection_ReactiveCapabilityCurve rdf:type owl:ObjectProperty ;
                                             owl:inverseOf :ReactiveCapabilityCurve_EquivalentInjection ;
                                             rdfs:domain <https://w3id.org/netbeheer/IECCIM/TC57CIM/IEC61970/Base/Equivalents#EquivalentInjection> ;
                                             rdfs:range :ReactiveCapabilityCurve ;
                                             rdfs:comment "The reactive capability curve used by this equivalent injection.The equivalent injection using this reactive capability curve." .


###  https://w3id.org/netbeheer/IECCIM/TC57CIM/IEC61970/Base/Wires#ExternalNetworkInjection_governorSCD
:ExternalNetworkInjection_governorSCD rdf:type owl:ObjectProperty ;
                                      rdfs:domain :ExternalNetworkInjection ;
                                      rdfs:range <https://w3id.org/netbeheer/IECCIM/TC57CIM/IEC61970/Base/Domain#ActivePowerPerFrequency> ;
                                      rdfs:comment "Power Frequency Bias. This is the change in power injection divided by the change in frequency and negated.  A positive value of the power frequency bias provides additional power injection upon a drop in frequency." .


###  https://w3id.org/netbeheer/IECCIM/TC57CIM/IEC61970/Base/Wires#ExternalNetworkInjection_maxInitialSymShCCurrent
:ExternalNetworkInjection_maxInitialSymShCCurrent rdf:type owl:ObjectProperty ;
                                                  rdfs:domain :ExternalNetworkInjection ;
                                                  rdfs:range <https://w3id.org/netbeheer/IECCIM/TC57CIM/IEC61970/Base/Domain#CurrentFlow> ;
                                                  rdfs:comment """  Maximum initial symmetrical short-circuit currents (Ik\" max) in A (Ik\" = Sk\"/(SQRT(3) Un)). Used for short circuit data exchange according to IEC 60909
""" .


###  https://w3id.org/netbeheer/IECCIM/TC57CIM/IEC61970/Base/Wires#ExternalNetworkInjection_maxP
:ExternalNetworkInjection_maxP rdf:type owl:ObjectProperty ;
                               rdfs:domain :ExternalNetworkInjection ;
                               rdfs:range <https://w3id.org/netbeheer/IECCIM/TC57CIM/IEC61970/Base/Domain#ActivePower> ;
                               rdfs:comment "Maximum active power of the injection." .


###  https://w3id.org/netbeheer/IECCIM/TC57CIM/IEC61970/Base/Wires#ExternalNetworkInjection_maxQ
:ExternalNetworkInjection_maxQ rdf:type owl:ObjectProperty ;
                               rdfs:domain :ExternalNetworkInjection ;
                               rdfs:range <https://w3id.org/netbeheer/IECCIM/TC57CIM/IEC61970/Base/Domain#ReactivePower> ;
                               rdfs:comment """Not for short circuit modelling; It is used for modelling of infeed for load flow exchange. If maxQ and minQ are not used ReactiveCapabilityCurve can be used 
""" .


###  https://w3id.org/netbeheer/IECCIM/TC57CIM/IEC61970/Base/Wires#ExternalNetworkInjection_minInitialSymShCCurrent
:ExternalNetworkInjection_minInitialSymShCCurrent rdf:type owl:ObjectProperty ;
                                                  rdfs:domain :ExternalNetworkInjection ;
                                                  rdfs:range <https://w3id.org/netbeheer/IECCIM/TC57CIM/IEC61970/Base/Domain#CurrentFlow> ;
                                                  rdfs:comment """Minimum initial symmetrical short-circuit currents (Ik\" min) in A (Ik\" = Sk\"/(SQRT(3) Un)). Used for short circuit data exchange according to IEC 60909
""" .


###  https://w3id.org/netbeheer/IECCIM/TC57CIM/IEC61970/Base/Wires#ExternalNetworkInjection_minP
:ExternalNetworkInjection_minP rdf:type owl:ObjectProperty ;
                               rdfs:domain :ExternalNetworkInjection ;
                               rdfs:range <https://w3id.org/netbeheer/IECCIM/TC57CIM/IEC61970/Base/Domain#ActivePower> ;
                               rdfs:comment "Minimum active power of the injection." .


###  https://w3id.org/netbeheer/IECCIM/TC57CIM/IEC61970/Base/Wires#ExternalNetworkInjection_minQ
:ExternalNetworkInjection_minQ rdf:type owl:ObjectProperty ;
                               rdfs:domain :ExternalNetworkInjection ;
                               rdfs:range <https://w3id.org/netbeheer/IECCIM/TC57CIM/IEC61970/Base/Domain#ReactivePower> ;
                               rdfs:comment """Not for short circuit modelling; It is used for modelling of infeed for load flow exchange. If maxQ and minQ are not used ReactiveCapabilityCurve can be used
""" .


###  https://w3id.org/netbeheer/IECCIM/TC57CIM/IEC61970/Base/Wires#ExternalNetworkInjection_p
:ExternalNetworkInjection_p rdf:type owl:ObjectProperty ;
                            rdfs:domain :ExternalNetworkInjection ;
                            rdfs:range <https://w3id.org/netbeheer/IECCIM/TC57CIM/IEC61970/Base/Domain#ActivePower> ;
                            rdfs:comment """Active power injection. Load sign convention is used, i.e. positive sign means flow out from a node.
Starting value for steady state solutions.""" .


###  https://w3id.org/netbeheer/IECCIM/TC57CIM/IEC61970/Base/Wires#ExternalNetworkInjection_q
:ExternalNetworkInjection_q rdf:type owl:ObjectProperty ;
                            rdfs:domain :ExternalNetworkInjection ;
                            rdfs:range <https://w3id.org/netbeheer/IECCIM/TC57CIM/IEC61970/Base/Domain#ReactivePower> ;
                            rdfs:comment """Reactive power injection. Load sign convention is used, i.e. positive sign means flow out from a node.
Starting value for steady state solutions.""" .


###  https://w3id.org/netbeheer/IECCIM/TC57CIM/IEC61970/Base/Wires#ExternalNetworkInjection_voltageFactor
:ExternalNetworkInjection_voltageFactor rdf:type owl:ObjectProperty ;
                                        rdfs:domain :ExternalNetworkInjection ;
                                        rdfs:range <https://w3id.org/netbeheer/IECCIM/TC57CIM/IEC61970/Base/Domain#PU> ;
                                        rdfs:comment """Voltage factor in pu, which was used to calculate short-circuit current Ik\" and power Sk\".
""" .


###  https://w3id.org/netbeheer/IECCIM/TC57CIM/IEC61970/Base/Wires#FrequencyConverter_frequency
:FrequencyConverter_frequency rdf:type owl:ObjectProperty ;
                              rdfs:domain :FrequencyConverter ;
                              rdfs:range <https://w3id.org/netbeheer/IECCIM/TC57CIM/IEC61970/Base/Domain#Frequency> ;
                              rdfs:comment "Frequency on the AC side." .


###  https://w3id.org/netbeheer/IECCIM/TC57CIM/IEC61970/Base/Wires#FrequencyConverter_maxP
:FrequencyConverter_maxP rdf:type owl:ObjectProperty ;
                         rdfs:domain :FrequencyConverter ;
                         rdfs:range <https://w3id.org/netbeheer/IECCIM/TC57CIM/IEC61970/Base/Domain#ActivePower> ;
                         rdfs:comment "The maximum active power on the DC side at which the frequence converter should operate." .


###  https://w3id.org/netbeheer/IECCIM/TC57CIM/IEC61970/Base/Wires#FrequencyConverter_maxU
:FrequencyConverter_maxU rdf:type owl:ObjectProperty ;
                         rdfs:domain :FrequencyConverter ;
                         rdfs:range <https://w3id.org/netbeheer/IECCIM/TC57CIM/IEC61970/Base/Domain#Voltage> ;
                         rdfs:comment "The maximum voltage on the DC side at which the frequency converter should operate." .


###  https://w3id.org/netbeheer/IECCIM/TC57CIM/IEC61970/Base/Wires#FrequencyConverter_minP
:FrequencyConverter_minP rdf:type owl:ObjectProperty ;
                         rdfs:domain :FrequencyConverter ;
                         rdfs:range <https://w3id.org/netbeheer/IECCIM/TC57CIM/IEC61970/Base/Domain#ActivePower> ;
                         rdfs:comment "The minimum active power on the DC side at which the frequence converter should operate." .


###  https://w3id.org/netbeheer/IECCIM/TC57CIM/IEC61970/Base/Wires#FrequencyConverter_minU
:FrequencyConverter_minU rdf:type owl:ObjectProperty ;
                         rdfs:domain :FrequencyConverter ;
                         rdfs:range <https://w3id.org/netbeheer/IECCIM/TC57CIM/IEC61970/Base/Domain#Voltage> ;
                         rdfs:comment "The minimum voltage on the DC side at which the frequency converter should operate." .


###  https://w3id.org/netbeheer/IECCIM/TC57CIM/IEC61970/Base/Wires#GeneratingUnit_RotatingMachine
:GeneratingUnit_RotatingMachine rdf:type owl:ObjectProperty ;
                                rdfs:domain <https://w3id.org/netbeheer/IECCIM/TC57CIM/IEC61970/Base/Generation/Production#GeneratingUnit> ;
                                rdfs:range :RotatingMachine ;
                                rdfs:comment "A synchronous machine may operate as a generator and as such becomes a member of a generating unit.A synchronous machine may operate as a generator and as such becomes a member of a generating unit." .


###  https://w3id.org/netbeheer/IECCIM/TC57CIM/IEC61970/Base/Wires#GroundAction_AlongACLineSegment
:GroundAction_AlongACLineSegment rdf:type owl:ObjectProperty ;
                                 rdfs:domain <https://w3id.org/netbeheer/IECCIM/TC57CIM/IEC61968/Operations#GroundAction> ;
                                 rdfs:range :ACLineSegment ;
                                 rdfs:comment "Ground action involving clamp usage (for the case when the ground is applied along the line segment instead of at its terminals).The line segment that this ground action will affect. This is the only way to access relationship to clamp in case the ground needs to be placed along the line segment." .


###  https://w3id.org/netbeheer/IECCIM/TC57CIM/IEC61970/Base/Wires#GroundAction_Ground
:GroundAction_Ground rdf:type owl:ObjectProperty ;
                     rdfs:domain <https://w3id.org/netbeheer/IECCIM/TC57CIM/IEC61968/Operations#GroundAction> ;
                     rdfs:range :Ground ;
                     rdfs:comment "Action taken with this ground.Ground on which this action is taken." .


###  https://w3id.org/netbeheer/IECCIM/TC57CIM/IEC61970/Base/Wires#Ground_GroundAction
:Ground_GroundAction rdf:type owl:ObjectProperty ;
                     owl:inverseOf :GroundAction_Ground ;
                     rdfs:domain :Ground ;
                     rdfs:range <https://w3id.org/netbeheer/IECCIM/TC57CIM/IEC61968/Operations#GroundAction> ;
                     rdfs:comment "Action taken with this ground.Ground on which this action is taken." .


###  https://w3id.org/netbeheer/IECCIM/TC57CIM/IEC61970/Base/Wires#GroundingImpedance_x
:GroundingImpedance_x rdf:type owl:ObjectProperty ;
                      rdfs:domain :GroundingImpedance ;
                      rdfs:range <https://w3id.org/netbeheer/IECCIM/TC57CIM/IEC61970/Base/Domain#Reactance> ;
                      rdfs:comment "Reactance of device." .


###  https://w3id.org/netbeheer/IECCIM/TC57CIM/IEC61970/Base/Wires#HydroPump_RotatingMachine
:HydroPump_RotatingMachine rdf:type owl:ObjectProperty ;
                           owl:inverseOf :RotatingMachine_HydroPump ;
                           rdfs:domain <https://w3id.org/netbeheer/IECCIM/TC57CIM/IEC61970/Base/Generation/Production#HydroPump> ;
                           rdfs:range :RotatingMachine ;
                           rdfs:comment "The synchronous machine drives the turbine which moves the water from a low elevation to a higher elevation. The direction of machine rotation for pumping may or may not be the same as for generating.The synchronous machine drives the turbine which moves the water from a low elevation to a higher elevation. The direction of machine rotation for pumping may or may not be the same as for generating." .


###  https://w3id.org/netbeheer/IECCIM/TC57CIM/IEC61970/Base/Wires#JumperAction_AlongACLineSegments
:JumperAction_AlongACLineSegments rdf:type owl:ObjectProperty ;
                                  rdfs:domain <https://w3id.org/netbeheer/IECCIM/TC57CIM/IEC61968/Operations#JumperAction> ;
                                  rdfs:range :ACLineSegment ;
                                  rdfs:comment "Jumper action involving clamp usage (for the case when the jumper is applied along the line segment instead of at its terminals).The line segment that this jumper action will affect. This is the only way to access relationship to clamp in case the jumper needs to connect along the line segment." .


###  https://w3id.org/netbeheer/IECCIM/TC57CIM/IEC61970/Base/Wires#JumperAction_Jumper
:JumperAction_Jumper rdf:type owl:ObjectProperty ;
                     rdfs:domain <https://w3id.org/netbeheer/IECCIM/TC57CIM/IEC61968/Operations#JumperAction> ;
                     rdfs:range :Jumper ;
                     rdfs:comment "Action taken with this jumper.Jumper on which this action is taken." .


###  https://w3id.org/netbeheer/IECCIM/TC57CIM/IEC61970/Base/Wires#Jumper_JumperAction
:Jumper_JumperAction rdf:type owl:ObjectProperty ;
                     owl:inverseOf :JumperAction_Jumper ;
                     rdfs:domain :Jumper ;
                     rdfs:range <https://w3id.org/netbeheer/IECCIM/TC57CIM/IEC61968/Operations#JumperAction> ;
                     rdfs:comment "Action taken with this jumper.Jumper on which this action is taken." .


###  https://w3id.org/netbeheer/IECCIM/TC57CIM/IEC61970/Base/Wires#LinearShuntCompensatorPhase_bPerSection
:LinearShuntCompensatorPhase_bPerSection rdf:type owl:ObjectProperty ;
                                         rdfs:domain :LinearShuntCompensatorPhase ;
                                         rdfs:range <https://w3id.org/netbeheer/IECCIM/TC57CIM/IEC61970/Base/Domain#Susceptance> ;
                                         rdfs:comment """Susceptance per section of the phase if shunt compensator is wye connected.   Susceptance per section phase to phase if shunt compensator is delta connected.
""" .


###  https://w3id.org/netbeheer/IECCIM/TC57CIM/IEC61970/Base/Wires#LinearShuntCompensatorPhase_gPerSection
:LinearShuntCompensatorPhase_gPerSection rdf:type owl:ObjectProperty ;
                                         rdfs:domain :LinearShuntCompensatorPhase ;
                                         rdfs:range <https://w3id.org/netbeheer/IECCIM/TC57CIM/IEC61970/Base/Domain#Conductance> ;
                                         rdfs:comment """Conductance per section for this phase if shunt compensator is wye connected.  Conductance per section phase to phase if shunt compensator is delta connected.
""" .


###  https://w3id.org/netbeheer/IECCIM/TC57CIM/IEC61970/Base/Wires#LinearShuntCompensator_b0PerSection
:LinearShuntCompensator_b0PerSection rdf:type owl:ObjectProperty ;
                                     rdfs:domain :LinearShuntCompensator ;
                                     rdfs:range <https://w3id.org/netbeheer/IECCIM/TC57CIM/IEC61970/Base/Domain#Susceptance> ;
                                     rdfs:comment "Zero sequence shunt (charging) susceptance per section" .


###  https://w3id.org/netbeheer/IECCIM/TC57CIM/IEC61970/Base/Wires#LinearShuntCompensator_bPerSection
:LinearShuntCompensator_bPerSection rdf:type owl:ObjectProperty ;
                                    rdfs:domain :LinearShuntCompensator ;
                                    rdfs:range <https://w3id.org/netbeheer/IECCIM/TC57CIM/IEC61970/Base/Domain#Susceptance> ;
                                    rdfs:comment "Positive sequence shunt (charging) susceptance per section" .


###  https://w3id.org/netbeheer/IECCIM/TC57CIM/IEC61970/Base/Wires#LinearShuntCompensator_g0PerSection
:LinearShuntCompensator_g0PerSection rdf:type owl:ObjectProperty ;
                                     rdfs:domain :LinearShuntCompensator ;
                                     rdfs:range <https://w3id.org/netbeheer/IECCIM/TC57CIM/IEC61970/Base/Domain#Conductance> ;
                                     rdfs:comment "Zero sequence shunt (charging) conductance per section" .


###  https://w3id.org/netbeheer/IECCIM/TC57CIM/IEC61970/Base/Wires#LinearShuntCompensator_gPerSection
:LinearShuntCompensator_gPerSection rdf:type owl:ObjectProperty ;
                                    rdfs:domain :LinearShuntCompensator ;
                                    rdfs:range <https://w3id.org/netbeheer/IECCIM/TC57CIM/IEC61970/Base/Domain#Conductance> ;
                                    rdfs:comment "Positive sequence shunt (charging) conductance per section" .


###  https://w3id.org/netbeheer/IECCIM/TC57CIM/IEC61970/Base/Wires#LoadDynamics_EnergyConsumer
:LoadDynamics_EnergyConsumer rdf:type owl:ObjectProperty ;
                             rdfs:domain <https://w3id.org/netbeheer/IECCIM/TC57CIM/IEC61970/Dynamics/StandardModels/LoadDynamics#LoadDynamics> ;
                             rdfs:range :EnergyConsumer ;
                             rdfs:comment "Load dynamics model used to describe dynamic behavior of this energy consumer.Energy consumer to which this dynamics load model applies." .


###  https://w3id.org/netbeheer/IECCIM/TC57CIM/IEC61970/Base/Wires#LoadResponseCharacteristic_EnergyConsumer
:LoadResponseCharacteristic_EnergyConsumer rdf:type owl:ObjectProperty ;
                                           owl:inverseOf :EnergyConsumer_LoadResponse ;
                                           rdfs:domain <https://w3id.org/netbeheer/IECCIM/TC57CIM/IEC61970/Base/LoadModel#LoadResponseCharacteristic> ;
                                           rdfs:range :EnergyConsumer ;
                                           rdfs:comment "The set of loads that have the response characteristics.The load response characteristic of this load.  If missing, this load is assumed to be constant power." .


###  https://w3id.org/netbeheer/IECCIM/TC57CIM/IEC61970/Base/Wires#MutualCoupling_b0ch
:MutualCoupling_b0ch rdf:type owl:ObjectProperty ;
                     rdfs:domain :MutualCoupling ;
                     rdfs:range <https://w3id.org/netbeheer/IECCIM/TC57CIM/IEC61970/Base/Domain#Susceptance> ;
                     rdfs:comment "Zero sequence mutual coupling shunt (charging) susceptance, uniformly distributed, of the entire line section." .


###  https://w3id.org/netbeheer/IECCIM/TC57CIM/IEC61970/Base/Wires#MutualCoupling_distance11
:MutualCoupling_distance11 rdf:type owl:ObjectProperty ;
                           rdfs:domain :MutualCoupling ;
                           rdfs:range <https://w3id.org/netbeheer/IECCIM/TC57CIM/IEC61970/Base/Domain#Length> ;
                           rdfs:comment """Distance to the start of the coupled region from the first line's terminal having sequence number equal to 1.
""" .


###  https://w3id.org/netbeheer/IECCIM/TC57CIM/IEC61970/Base/Wires#MutualCoupling_distance12
:MutualCoupling_distance12 rdf:type owl:ObjectProperty ;
                           rdfs:domain :MutualCoupling ;
                           rdfs:range <https://w3id.org/netbeheer/IECCIM/TC57CIM/IEC61970/Base/Domain#Length> ;
                           rdfs:comment """Distance to the end of the coupled region from the first line's terminal with sequence number equal to 1.
""" .


###  https://w3id.org/netbeheer/IECCIM/TC57CIM/IEC61970/Base/Wires#MutualCoupling_distance21
:MutualCoupling_distance21 rdf:type owl:ObjectProperty ;
                           rdfs:domain :MutualCoupling ;
                           rdfs:range <https://w3id.org/netbeheer/IECCIM/TC57CIM/IEC61970/Base/Domain#Length> ;
                           rdfs:comment """Distance to the start of coupled region from the second line's terminal with sequence number equal to 1.
""" .


###  https://w3id.org/netbeheer/IECCIM/TC57CIM/IEC61970/Base/Wires#MutualCoupling_distance22
:MutualCoupling_distance22 rdf:type owl:ObjectProperty ;
                           rdfs:domain :MutualCoupling ;
                           rdfs:range <https://w3id.org/netbeheer/IECCIM/TC57CIM/IEC61970/Base/Domain#Length> ;
                           rdfs:comment "Distance to the end of coupled region from the second line's terminal with sequence number equal to 1." .


###  https://w3id.org/netbeheer/IECCIM/TC57CIM/IEC61970/Base/Wires#MutualCoupling_g0ch
:MutualCoupling_g0ch rdf:type owl:ObjectProperty ;
                     rdfs:domain :MutualCoupling ;
                     rdfs:range <https://w3id.org/netbeheer/IECCIM/TC57CIM/IEC61970/Base/Domain#Conductance> ;
                     rdfs:comment "Zero sequence mutual coupling shunt (charging) conductance, uniformly distributed, of the entire line section." .


###  https://w3id.org/netbeheer/IECCIM/TC57CIM/IEC61970/Base/Wires#MutualCoupling_r0
:MutualCoupling_r0 rdf:type owl:ObjectProperty ;
                   rdfs:domain :MutualCoupling ;
                   rdfs:range <https://w3id.org/netbeheer/IECCIM/TC57CIM/IEC61970/Base/Domain#Resistance> ;
                   rdfs:comment """Zero sequence branch-to-branch mutual impedance coupling, resistance.
""" .


###  https://w3id.org/netbeheer/IECCIM/TC57CIM/IEC61970/Base/Wires#MutualCoupling_x0
:MutualCoupling_x0 rdf:type owl:ObjectProperty ;
                   rdfs:domain :MutualCoupling ;
                   rdfs:range <https://w3id.org/netbeheer/IECCIM/TC57CIM/IEC61970/Base/Domain#Reactance> ;
                   rdfs:comment """Zero sequence branch-to-branch mutual impedance coupling, reactance.
""" .


###  https://w3id.org/netbeheer/IECCIM/TC57CIM/IEC61970/Base/Wires#NonlinearShuntCompensatorPhasePoint_NonlinearShuntCompensatorPhase
:NonlinearShuntCompensatorPhasePoint_NonlinearShuntCompensatorPhase rdf:type owl:ObjectProperty ;
                                                                    rdfs:domain :NonlinearShuntCompensatorPhasePoint ;
                                                                    rdfs:range :NonlinearShuntCompensatorPhase ;
                                                                    rdfs:comment "All points of the non-linear shunt compensator phase.Non-linear shunt compensator phase owning this point." .


###  https://w3id.org/netbeheer/IECCIM/TC57CIM/IEC61970/Base/Wires#NonlinearShuntCompensatorPhasePoint_b
:NonlinearShuntCompensatorPhasePoint_b rdf:type owl:ObjectProperty ;
                                       rdfs:domain :NonlinearShuntCompensatorPhasePoint ;
                                       rdfs:range <https://w3id.org/netbeheer/IECCIM/TC57CIM/IEC61970/Base/Domain#Susceptance> ;
                                       rdfs:comment "Positive sequence shunt (charging) susceptance per section" .


###  https://w3id.org/netbeheer/IECCIM/TC57CIM/IEC61970/Base/Wires#NonlinearShuntCompensatorPhasePoint_g
:NonlinearShuntCompensatorPhasePoint_g rdf:type owl:ObjectProperty ;
                                       rdfs:domain :NonlinearShuntCompensatorPhasePoint ;
                                       rdfs:range <https://w3id.org/netbeheer/IECCIM/TC57CIM/IEC61970/Base/Domain#Conductance> ;
                                       rdfs:comment "Positive sequence shunt (charging) conductance per section" .


###  https://w3id.org/netbeheer/IECCIM/TC57CIM/IEC61970/Base/Wires#NonlinearShuntCompensatorPhase_NonlinearShuntCompensatorPhasePoints
:NonlinearShuntCompensatorPhase_NonlinearShuntCompensatorPhasePoints rdf:type owl:ObjectProperty ;
                                                                     owl:inverseOf :NonlinearShuntCompensatorPhasePoint_NonlinearShuntCompensatorPhase ;
                                                                     rdf:type owl:FunctionalProperty ;
                                                                     rdfs:domain :NonlinearShuntCompensatorPhase ;
                                                                     rdfs:range :NonlinearShuntCompensatorPhasePoint ;
                                                                     rdfs:comment "All points of the non-linear shunt compensator phase.Non-linear shunt compensator phase owning this point." .


###  https://w3id.org/netbeheer/IECCIM/TC57CIM/IEC61970/Base/Wires#NonlinearShuntCompensatorPoint_NonlinearShuntCompensator
:NonlinearShuntCompensatorPoint_NonlinearShuntCompensator rdf:type owl:ObjectProperty ;
                                                          rdfs:domain :NonlinearShuntCompensatorPoint ;
                                                          rdfs:range :NonlinearShuntCompensator ;
                                                          rdfs:comment "All points of the non-linear shunt compensator.Non-linear shunt compensator owning this point." .


###  https://w3id.org/netbeheer/IECCIM/TC57CIM/IEC61970/Base/Wires#NonlinearShuntCompensatorPoint_b
:NonlinearShuntCompensatorPoint_b rdf:type owl:ObjectProperty ;
                                  rdfs:domain :NonlinearShuntCompensatorPoint ;
                                  rdfs:range <https://w3id.org/netbeheer/IECCIM/TC57CIM/IEC61970/Base/Domain#Susceptance> ;
                                  rdfs:comment "Positive sequence shunt (charging) susceptance per section" .


###  https://w3id.org/netbeheer/IECCIM/TC57CIM/IEC61970/Base/Wires#NonlinearShuntCompensatorPoint_b0
:NonlinearShuntCompensatorPoint_b0 rdf:type owl:ObjectProperty ;
                                   rdfs:domain :NonlinearShuntCompensatorPoint ;
                                   rdfs:range <https://w3id.org/netbeheer/IECCIM/TC57CIM/IEC61970/Base/Domain#Susceptance> ;
                                   rdfs:comment "Zero sequence shunt (charging) susceptance per section" .


###  https://w3id.org/netbeheer/IECCIM/TC57CIM/IEC61970/Base/Wires#NonlinearShuntCompensatorPoint_g
:NonlinearShuntCompensatorPoint_g rdf:type owl:ObjectProperty ;
                                  rdfs:domain :NonlinearShuntCompensatorPoint ;
                                  rdfs:range <https://w3id.org/netbeheer/IECCIM/TC57CIM/IEC61970/Base/Domain#Conductance> ;
                                  rdfs:comment "Positive sequence shunt (charging) conductance per section" .


###  https://w3id.org/netbeheer/IECCIM/TC57CIM/IEC61970/Base/Wires#NonlinearShuntCompensatorPoint_g0
:NonlinearShuntCompensatorPoint_g0 rdf:type owl:ObjectProperty ;
                                   rdfs:domain :NonlinearShuntCompensatorPoint ;
                                   rdfs:range <https://w3id.org/netbeheer/IECCIM/TC57CIM/IEC61970/Base/Domain#Conductance> ;
                                   rdfs:comment "Zero sequence shunt (charging) conductance per section" .


###  https://w3id.org/netbeheer/IECCIM/TC57CIM/IEC61970/Base/Wires#NonlinearShuntCompensator_NonlinearShuntCompensatorPoints
:NonlinearShuntCompensator_NonlinearShuntCompensatorPoints rdf:type owl:ObjectProperty ;
                                                           owl:inverseOf :NonlinearShuntCompensatorPoint_NonlinearShuntCompensator ;
                                                           rdf:type owl:FunctionalProperty ;
                                                           rdfs:domain :NonlinearShuntCompensator ;
                                                           rdfs:range :NonlinearShuntCompensatorPoint ;
                                                           rdfs:comment "All points of the non-linear shunt compensator.Non-linear shunt compensator owning this point." .


###  https://w3id.org/netbeheer/IECCIM/TC57CIM/IEC61970/Base/Wires#Outage_OpenedSwitches
:Outage_OpenedSwitches rdf:type owl:ObjectProperty ;
                       rdfs:domain <https://w3id.org/netbeheer/IECCIM/TC57CIM/IEC61968/Operations#Outage> ;
                       rdfs:range :Switch ;
                       rdfs:comment "Current outage of this protective device.All potentially open switches causing this outage. This realationship is meant to be used as \"indication\" for initiation of outage-related business processes, whereas for actual actions of switches, SwitchAction-Switch relationship should be used." .


###  https://w3id.org/netbeheer/IECCIM/TC57CIM/IEC61970/Base/Wires#PerLengthImpedance_ACLineSegments
:PerLengthImpedance_ACLineSegments rdf:type owl:ObjectProperty ;
                                   rdfs:domain :PerLengthImpedance ;
                                   rdfs:range :ACLineSegment ;
                                   rdfs:comment "Per-length impedance of this line segment.All line segments described by this per-length impedance." .


###  https://w3id.org/netbeheer/IECCIM/TC57CIM/IEC61970/Base/Wires#PerLengthLineParameter_WireInfos
:PerLengthLineParameter_WireInfos rdf:type owl:ObjectProperty ;
                                  owl:inverseOf :WireInfo_PerLengthParameters ;
                                  rdfs:domain :PerLengthLineParameter ;
                                  rdfs:range <https://w3id.org/netbeheer/IECCIM/TC57CIM/IEC61968/AssetInfo#WireInfo> ;
                                  rdfs:comment "All wire datasheets used to calculate this per-length parameter.All per-length parameters calculated from this wire datasheet." .


###  https://w3id.org/netbeheer/IECCIM/TC57CIM/IEC61970/Base/Wires#PerLengthLineParameter_WireSpacingInfo
:PerLengthLineParameter_WireSpacingInfo rdf:type owl:ObjectProperty ;
                                        owl:inverseOf :WireSpacing_PerLengthParameters ;
                                        rdfs:domain :PerLengthLineParameter ;
                                        rdfs:range <https://w3id.org/netbeheer/IECCIM/TC57CIM/IEC61968/AssetInfo#WireSpacing> ;
                                        rdfs:comment "Wire spacing datasheet used to calculate this per-length parameter.All per-length parameters calculated from this wire spacing datasheet." .


###  https://w3id.org/netbeheer/IECCIM/TC57CIM/IEC61970/Base/Wires#PerLengthPhaseImpedance_PhaseImpedanceData
:PerLengthPhaseImpedance_PhaseImpedanceData rdf:type owl:ObjectProperty ,
                                                     owl:FunctionalProperty ;
                                            rdfs:domain :PerLengthPhaseImpedance ;
                                            rdfs:range :PhaseImpedanceData ;
                                            rdfs:comment "Conductor phase impedance to which this data belongs.All data that belong to this conductor phase impedance." .


###  https://w3id.org/netbeheer/IECCIM/TC57CIM/IEC61970/Base/Wires#PerLengthSequenceImpedance_b0ch
:PerLengthSequenceImpedance_b0ch rdf:type owl:ObjectProperty ;
                                 rdfs:domain :PerLengthSequenceImpedance ;
                                 rdfs:range <https://w3id.org/netbeheer/IECCIM/TC57CIM/IEC61970/Base/Domain#SusceptancePerLength> ;
                                 rdfs:comment """Zero sequence shunt (charging) susceptance, per unit of length.
""" .


###  https://w3id.org/netbeheer/IECCIM/TC57CIM/IEC61970/Base/Wires#PerLengthSequenceImpedance_bch
:PerLengthSequenceImpedance_bch rdf:type owl:ObjectProperty ;
                                rdfs:domain :PerLengthSequenceImpedance ;
                                rdfs:range <https://w3id.org/netbeheer/IECCIM/TC57CIM/IEC61970/Base/Domain#SusceptancePerLength> ;
                                rdfs:comment """Positive sequence shunt (charging) susceptance, per unit of length.
""" .


###  https://w3id.org/netbeheer/IECCIM/TC57CIM/IEC61970/Base/Wires#PerLengthSequenceImpedance_g0ch
:PerLengthSequenceImpedance_g0ch rdf:type owl:ObjectProperty ;
                                 rdfs:domain :PerLengthSequenceImpedance ;
                                 rdfs:range <https://w3id.org/netbeheer/IECCIM/TC57CIM/IEC61970/Base/Domain#ConductancePerLength> ;
                                 rdfs:comment """Zero sequence shunt (charging) conductance, per unit of length.
""" .


###  https://w3id.org/netbeheer/IECCIM/TC57CIM/IEC61970/Base/Wires#PerLengthSequenceImpedance_gch
:PerLengthSequenceImpedance_gch rdf:type owl:ObjectProperty ;
                                rdfs:domain :PerLengthSequenceImpedance ;
                                rdfs:range <https://w3id.org/netbeheer/IECCIM/TC57CIM/IEC61970/Base/Domain#ConductancePerLength> ;
                                rdfs:comment """Positive sequence shunt (charging) conductance, per unit of length.
""" .


###  https://w3id.org/netbeheer/IECCIM/TC57CIM/IEC61970/Base/Wires#PerLengthSequenceImpedance_r
:PerLengthSequenceImpedance_r rdf:type owl:ObjectProperty ;
                              rdfs:domain :PerLengthSequenceImpedance ;
                              rdfs:range <https://w3id.org/netbeheer/IECCIM/TC57CIM/IEC61970/Base/Domain#ResistancePerLength> ;
                              rdfs:comment """Positive sequence series resistance, per unit of length.
""" .


###  https://w3id.org/netbeheer/IECCIM/TC57CIM/IEC61970/Base/Wires#PerLengthSequenceImpedance_r0
:PerLengthSequenceImpedance_r0 rdf:type owl:ObjectProperty ;
                               rdfs:domain :PerLengthSequenceImpedance ;
                               rdfs:range <https://w3id.org/netbeheer/IECCIM/TC57CIM/IEC61970/Base/Domain#ResistancePerLength> ;
                               rdfs:comment """Zero sequence series resistance, per unit of length.
""" .


###  https://w3id.org/netbeheer/IECCIM/TC57CIM/IEC61970/Base/Wires#PerLengthSequenceImpedance_x
:PerLengthSequenceImpedance_x rdf:type owl:ObjectProperty ;
                              rdfs:domain :PerLengthSequenceImpedance ;
                              rdfs:range <https://w3id.org/netbeheer/IECCIM/TC57CIM/IEC61970/Base/Domain#ReactancePerLength> ;
                              rdfs:comment """Positive sequence series reactance, per unit of length.
""" .


###  https://w3id.org/netbeheer/IECCIM/TC57CIM/IEC61970/Base/Wires#PerLengthSequenceImpedance_x0
:PerLengthSequenceImpedance_x0 rdf:type owl:ObjectProperty ;
                               rdfs:domain :PerLengthSequenceImpedance ;
                               rdfs:range <https://w3id.org/netbeheer/IECCIM/TC57CIM/IEC61970/Base/Domain#ReactancePerLength> ;
                               rdfs:comment """Zero sequence series reactance, per unit of length.
""" .


###  https://w3id.org/netbeheer/IECCIM/TC57CIM/IEC61970/Base/Wires#PetersenCoil_nominalU
:PetersenCoil_nominalU rdf:type owl:ObjectProperty ;
                       rdfs:domain :PetersenCoil ;
                       rdfs:range <https://w3id.org/netbeheer/IECCIM/TC57CIM/IEC61970/Base/Domain#Voltage> ;
                       rdfs:comment "The nominal voltage for which the coil is designed." .


###  https://w3id.org/netbeheer/IECCIM/TC57CIM/IEC61970/Base/Wires#PetersenCoil_offsetCurrent
:PetersenCoil_offsetCurrent rdf:type owl:ObjectProperty ;
                            rdfs:domain :PetersenCoil ;
                            rdfs:range <https://w3id.org/netbeheer/IECCIM/TC57CIM/IEC61970/Base/Domain#CurrentFlow> ;
                            rdfs:comment "The offset current that the Petersen coil controller is operating from the resonant point.  This is normally a fixed amount for which the controller is configured and could be positive or negative.  Typically 0 to 60 Amperes depending on voltage and resonance conditions." .


###  https://w3id.org/netbeheer/IECCIM/TC57CIM/IEC61970/Base/Wires#PetersenCoil_positionCurrent
:PetersenCoil_positionCurrent rdf:type owl:ObjectProperty ;
                              rdfs:domain :PetersenCoil ;
                              rdfs:range <https://w3id.org/netbeheer/IECCIM/TC57CIM/IEC61970/Base/Domain#CurrentFlow> ;
                              rdfs:comment "The control current used to control the Petersen coil also known as the position current.  Typically in the range of 20-200mA." .


###  https://w3id.org/netbeheer/IECCIM/TC57CIM/IEC61970/Base/Wires#PetersenCoil_xGroundMax
:PetersenCoil_xGroundMax rdf:type owl:ObjectProperty ;
                         rdfs:domain :PetersenCoil ;
                         rdfs:range <https://w3id.org/netbeheer/IECCIM/TC57CIM/IEC61970/Base/Domain#Reactance> ;
                         rdfs:comment "The maximum reactance. " .


###  https://w3id.org/netbeheer/IECCIM/TC57CIM/IEC61970/Base/Wires#PetersenCoil_xGroundMin
:PetersenCoil_xGroundMin rdf:type owl:ObjectProperty ;
                         rdfs:domain :PetersenCoil ;
                         rdfs:range <https://w3id.org/netbeheer/IECCIM/TC57CIM/IEC61970/Base/Domain#Reactance> ;
                         rdfs:comment "The minimum reactance." .


###  https://w3id.org/netbeheer/IECCIM/TC57CIM/IEC61970/Base/Wires#PetersenCoil_xGroundNominal
:PetersenCoil_xGroundNominal rdf:type owl:ObjectProperty ;
                             rdfs:domain :PetersenCoil ;
                             rdfs:range <https://w3id.org/netbeheer/IECCIM/TC57CIM/IEC61970/Base/Domain#Reactance> ;
                             rdfs:comment "The nominal reactance.  This is the operating point (normally over compensation) that is defined based on the resonance point in the healthy network condition.  The impedance is calculated based on nominal voltage divided by position current." .


###  https://w3id.org/netbeheer/IECCIM/TC57CIM/IEC61970/Base/Wires#PhaseImpedanceData_PhaseImpedance
:PhaseImpedanceData_PhaseImpedance rdf:type owl:ObjectProperty ;
                                   owl:inverseOf :PerLengthPhaseImpedance_PhaseImpedanceData ;
                                   rdfs:domain :PhaseImpedanceData ;
                                   rdfs:range :PerLengthPhaseImpedance ;
                                   rdfs:comment "Conductor phase impedance to which this data belongs.All data that belong to this conductor phase impedance." .


###  https://w3id.org/netbeheer/IECCIM/TC57CIM/IEC61970/Base/Wires#PhaseImpedanceData_b
:PhaseImpedanceData_b rdf:type owl:ObjectProperty ;
                      rdfs:domain :PhaseImpedanceData ;
                      rdfs:range <https://w3id.org/netbeheer/IECCIM/TC57CIM/IEC61970/Base/Domain#SusceptancePerLength> ;
                      rdfs:comment """Susceptance matrix element value, per length of unit.
""" .


###  https://w3id.org/netbeheer/IECCIM/TC57CIM/IEC61970/Base/Wires#PhaseImpedanceData_r
:PhaseImpedanceData_r rdf:type owl:ObjectProperty ;
                      rdfs:domain :PhaseImpedanceData ;
                      rdfs:range <https://w3id.org/netbeheer/IECCIM/TC57CIM/IEC61970/Base/Domain#ResistancePerLength> ;
                      rdfs:comment """Resistance matrix element value, per length of unit.
""" .


###  https://w3id.org/netbeheer/IECCIM/TC57CIM/IEC61970/Base/Wires#PhaseImpedanceData_x
:PhaseImpedanceData_x rdf:type owl:ObjectProperty ;
                      rdfs:domain :PhaseImpedanceData ;
                      rdfs:range <https://w3id.org/netbeheer/IECCIM/TC57CIM/IEC61970/Base/Domain#ReactancePerLength> ;
                      rdfs:comment """Reactance matrix element value, per length of unit.
""" .


###  https://w3id.org/netbeheer/IECCIM/TC57CIM/IEC61970/Base/Wires#PhaseTapChangerAsymmetrical_windingConnectionAngle
:PhaseTapChangerAsymmetrical_windingConnectionAngle rdf:type owl:ObjectProperty ;
                                                    rdfs:domain :PhaseTapChangerAsymmetrical ;
                                                    rdfs:range <https://w3id.org/netbeheer/IECCIM/TC57CIM/IEC61970/Base/Domain#AngleDegrees> ;
                                                    rdfs:comment """The phase angle between the in-phase winding and the out-of -phase winding used for creating phase shift. The out-of-phase winding produces what is known as the difference voltage.  Setting this angle to 90 degrees is not the same as a symmemtrical transformer.
""" .


###  https://w3id.org/netbeheer/IECCIM/TC57CIM/IEC61970/Base/Wires#PhaseTapChangerLinear_stepPhaseShiftIncrement
:PhaseTapChangerLinear_stepPhaseShiftIncrement rdf:type owl:ObjectProperty ;
                                               rdfs:domain :PhaseTapChangerLinear ;
                                               rdfs:range <https://w3id.org/netbeheer/IECCIM/TC57CIM/IEC61970/Base/Domain#AngleDegrees> ;
                                               rdfs:comment """Phase shift per step position. A positive value indicates a positive phase shift from the winding where the tap is located to the other winding (for a two-winding transformer).
The actual phase shift increment might be more accurately computed from the symmetrical or asymmetrical models or a tap step table lookup if those are available.""" .


###  https://w3id.org/netbeheer/IECCIM/TC57CIM/IEC61970/Base/Wires#PhaseTapChangerLinear_xMax
:PhaseTapChangerLinear_xMax rdf:type owl:ObjectProperty ;
                            rdfs:domain :PhaseTapChangerLinear ;
                            rdfs:range <https://w3id.org/netbeheer/IECCIM/TC57CIM/IEC61970/Base/Domain#Reactance> ;
                            rdfs:comment "The reactance depend on the tap position according to a \"u\" shaped curve. The maximum reactance (xMax) appear at the low and high tap positions." .


###  https://w3id.org/netbeheer/IECCIM/TC57CIM/IEC61970/Base/Wires#PhaseTapChangerLinear_xMin
:PhaseTapChangerLinear_xMin rdf:type owl:ObjectProperty ;
                            rdfs:domain :PhaseTapChangerLinear ;
                            rdfs:range <https://w3id.org/netbeheer/IECCIM/TC57CIM/IEC61970/Base/Domain#Reactance> ;
                            rdfs:comment "The reactance depend on the tap position according to a \"u\" shaped curve. The minimum reactance (xMin) appear at the mid tap position." .


###  https://w3id.org/netbeheer/IECCIM/TC57CIM/IEC61970/Base/Wires#PhaseTapChangerNonLinear_voltageStepIncrement
:PhaseTapChangerNonLinear_voltageStepIncrement rdf:type owl:ObjectProperty ;
                                               rdfs:domain :PhaseTapChangerNonLinear ;
                                               rdfs:range <https://w3id.org/netbeheer/IECCIM/TC57CIM/IEC61970/Base/Domain#PerCent> ;
                                               rdfs:comment """The voltage step increment on the out of phase winding specified in percent of nominal voltage of the transformer end.
""" .


###  https://w3id.org/netbeheer/IECCIM/TC57CIM/IEC61970/Base/Wires#PhaseTapChangerNonLinear_xMax
:PhaseTapChangerNonLinear_xMax rdf:type owl:ObjectProperty ;
                               rdfs:domain :PhaseTapChangerNonLinear ;
                               rdfs:range <https://w3id.org/netbeheer/IECCIM/TC57CIM/IEC61970/Base/Domain#Reactance> ;
                               rdfs:comment "The reactance depend on the tap position according to a \"u\" shaped curve. The maximum reactance (xMax) appear at the low and high tap positions." .


###  https://w3id.org/netbeheer/IECCIM/TC57CIM/IEC61970/Base/Wires#PhaseTapChangerNonLinear_xMin
:PhaseTapChangerNonLinear_xMin rdf:type owl:ObjectProperty ;
                               rdfs:domain :PhaseTapChangerNonLinear ;
                               rdfs:range <https://w3id.org/netbeheer/IECCIM/TC57CIM/IEC61970/Base/Domain#Reactance> ;
                               rdfs:comment "The reactance depend on the tap position according to a \"u\" shaped curve. The minimum reactance (xMin) appear at the mid tap position." .


###  https://w3id.org/netbeheer/IECCIM/TC57CIM/IEC61970/Base/Wires#PhaseTapChangerTablePoint_PhaseTapChangerTable
:PhaseTapChangerTablePoint_PhaseTapChangerTable rdf:type owl:ObjectProperty ;
                                                rdfs:domain :PhaseTapChangerTablePoint ;
                                                rdfs:range :PhaseTapChangerTable ;
                                                rdfs:comment "The points of this table.The table of this point." .


###  https://w3id.org/netbeheer/IECCIM/TC57CIM/IEC61970/Base/Wires#PhaseTapChangerTablePoint_angle
:PhaseTapChangerTablePoint_angle rdf:type owl:ObjectProperty ;
                                 rdfs:domain :PhaseTapChangerTablePoint ;
                                 rdfs:range <https://w3id.org/netbeheer/IECCIM/TC57CIM/IEC61970/Base/Domain#AngleDegrees> ;
                                 rdfs:comment """The angle difference in degrees.
""" .


###  https://w3id.org/netbeheer/IECCIM/TC57CIM/IEC61970/Base/Wires#PhaseTapChangerTable_PhaseTapChangerTablePoint
:PhaseTapChangerTable_PhaseTapChangerTablePoint rdf:type owl:ObjectProperty ;
                                                owl:inverseOf :PhaseTapChangerTablePoint_PhaseTapChangerTable ;
                                                rdf:type owl:FunctionalProperty ;
                                                rdfs:domain :PhaseTapChangerTable ;
                                                rdfs:range :PhaseTapChangerTablePoint ;
                                                rdfs:comment "The points of this table.The table of this point." .


###  https://w3id.org/netbeheer/IECCIM/TC57CIM/IEC61970/Base/Wires#PhaseTapChangerTable_PhaseTapChangerTabular
:PhaseTapChangerTable_PhaseTapChangerTabular rdf:type owl:ObjectProperty ;
                                             rdfs:domain :PhaseTapChangerTable ;
                                             rdfs:range :PhaseTapChangerTabular ;
                                             rdfs:comment "The phase tap changer table for this phase tap changer.The phase tap changers to which this phase tap table applies." .


###  https://w3id.org/netbeheer/IECCIM/TC57CIM/IEC61970/Base/Wires#PhaseTapChangerTabular_PhaseTapChangerTable
:PhaseTapChangerTabular_PhaseTapChangerTable rdf:type owl:ObjectProperty ;
                                             owl:inverseOf :PhaseTapChangerTable_PhaseTapChangerTabular ;
                                             rdfs:domain :PhaseTapChangerTabular ;
                                             rdfs:range :PhaseTapChangerTable ;
                                             rdfs:comment "The phase tap changer table for this phase tap changer.The phase tap changers to which this phase tap table applies." .


###  https://w3id.org/netbeheer/IECCIM/TC57CIM/IEC61970/Base/Wires#PhaseTapChanger_TransformerEnd
:PhaseTapChanger_TransformerEnd rdf:type owl:ObjectProperty ;
                                owl:inverseOf :TransformerEnd_PhaseTapChanger ;
                                rdfs:domain :PhaseTapChanger ;
                                rdfs:range :TransformerEnd ;
                                rdfs:comment "Transformer end to which this phase tap changer belongs.Phase tap changer associated with this transformer end." .


###  https://w3id.org/netbeheer/IECCIM/TC57CIM/IEC61970/Base/Wires#PowerCutZone_EnergyConsumers
:PowerCutZone_EnergyConsumers rdf:type owl:ObjectProperty ;
                              rdfs:domain <https://w3id.org/netbeheer/IECCIM/TC57CIM/IEC61970/Base/LoadModel#PowerCutZone> ;
                              rdfs:range :EnergyConsumer ;
                              rdfs:comment "The  energy consumer is assigned to this power cut zone.Energy consumer is assigned to the power cut zone." .


###  https://w3id.org/netbeheer/IECCIM/TC57CIM/IEC61970/Base/Wires#PowerTransformerEnd_PowerTransformer
:PowerTransformerEnd_PowerTransformer rdf:type owl:ObjectProperty ;
                                      owl:inverseOf :PowerTransformer_PowerTransformerEnd ;
                                      rdfs:domain :PowerTransformerEnd ;
                                      rdfs:range :PowerTransformer ;
                                      rdfs:comment "The power transformer of this power transformer end.The ends of this power transformer." .


###  https://w3id.org/netbeheer/IECCIM/TC57CIM/IEC61970/Base/Wires#PowerTransformerEnd_b
:PowerTransformerEnd_b rdf:type owl:ObjectProperty ;
                       rdfs:domain :PowerTransformerEnd ;
                       rdfs:range <https://w3id.org/netbeheer/IECCIM/TC57CIM/IEC61970/Base/Domain#Susceptance> ;
                       rdfs:comment """Magnetizing branch susceptance (B mag).  The value can be positive or negative.
""" .


###  https://w3id.org/netbeheer/IECCIM/TC57CIM/IEC61970/Base/Wires#PowerTransformerEnd_b0
:PowerTransformerEnd_b0 rdf:type owl:ObjectProperty ;
                        rdfs:domain :PowerTransformerEnd ;
                        rdfs:range <https://w3id.org/netbeheer/IECCIM/TC57CIM/IEC61970/Base/Domain#Susceptance> ;
                        rdfs:comment """Zero sequence magnetizing branch susceptance.
""" .


###  https://w3id.org/netbeheer/IECCIM/TC57CIM/IEC61970/Base/Wires#PowerTransformerEnd_g
:PowerTransformerEnd_g rdf:type owl:ObjectProperty ;
                       rdfs:domain :PowerTransformerEnd ;
                       rdfs:range <https://w3id.org/netbeheer/IECCIM/TC57CIM/IEC61970/Base/Domain#Conductance> ;
                       rdfs:comment """Magnetizing branch conductance.
""" .


###  https://w3id.org/netbeheer/IECCIM/TC57CIM/IEC61970/Base/Wires#PowerTransformerEnd_g0
:PowerTransformerEnd_g0 rdf:type owl:ObjectProperty ;
                        rdfs:domain :PowerTransformerEnd ;
                        rdfs:range <https://w3id.org/netbeheer/IECCIM/TC57CIM/IEC61970/Base/Domain#Conductance> ;
                        rdfs:comment """Zero sequence magnetizing branch conductance (star-model).
""" .


###  https://w3id.org/netbeheer/IECCIM/TC57CIM/IEC61970/Base/Wires#PowerTransformerEnd_r
:PowerTransformerEnd_r rdf:type owl:ObjectProperty ;
                       rdfs:domain :PowerTransformerEnd ;
                       rdfs:range <https://w3id.org/netbeheer/IECCIM/TC57CIM/IEC61970/Base/Domain#Resistance> ;
                       rdfs:comment """Resistance (star-model) of the transformer end.
The attribute shall be equal or greater than zero for non-equivalent transformers.""" .


###  https://w3id.org/netbeheer/IECCIM/TC57CIM/IEC61970/Base/Wires#PowerTransformerEnd_r0
:PowerTransformerEnd_r0 rdf:type owl:ObjectProperty ;
                        rdfs:domain :PowerTransformerEnd ;
                        rdfs:range <https://w3id.org/netbeheer/IECCIM/TC57CIM/IEC61970/Base/Domain#Resistance> ;
                        rdfs:comment """Zero sequence series resistance (star-model) of the transformer end.
""" .


###  https://w3id.org/netbeheer/IECCIM/TC57CIM/IEC61970/Base/Wires#PowerTransformerEnd_ratedS
:PowerTransformerEnd_ratedS rdf:type owl:ObjectProperty ;
                            rdfs:domain :PowerTransformerEnd ;
                            rdfs:range <https://w3id.org/netbeheer/IECCIM/TC57CIM/IEC61970/Base/Domain#ApparentPower> ;
                            rdfs:comment """Normal apparent power rating.
The attribute shall be a positive value. For a two-winding transformer the values for the high and low voltage sides shall be identical. """ .


###  https://w3id.org/netbeheer/IECCIM/TC57CIM/IEC61970/Base/Wires#PowerTransformerEnd_ratedU
:PowerTransformerEnd_ratedU rdf:type owl:ObjectProperty ;
                            rdfs:domain :PowerTransformerEnd ;
                            rdfs:range <https://w3id.org/netbeheer/IECCIM/TC57CIM/IEC61970/Base/Domain#Voltage> ;
                            rdfs:comment """Rated voltage: phase-phase for three-phase windings, and either phase-phase or phase-neutral for single-phase windings.
A high voltage side, as given by TransformerEnd.endNumber, shall have a ratedU that is greater or equal than ratedU for the lower voltage sides.""" .


###  https://w3id.org/netbeheer/IECCIM/TC57CIM/IEC61970/Base/Wires#PowerTransformerEnd_x
:PowerTransformerEnd_x rdf:type owl:ObjectProperty ;
                       rdfs:domain :PowerTransformerEnd ;
                       rdfs:range <https://w3id.org/netbeheer/IECCIM/TC57CIM/IEC61970/Base/Domain#Reactance> ;
                       rdfs:comment """Positive sequence series reactance (star-model) of the transformer end.
""" .


###  https://w3id.org/netbeheer/IECCIM/TC57CIM/IEC61970/Base/Wires#PowerTransformerEnd_x0
:PowerTransformerEnd_x0 rdf:type owl:ObjectProperty ;
                        rdfs:domain :PowerTransformerEnd ;
                        rdfs:range <https://w3id.org/netbeheer/IECCIM/TC57CIM/IEC61970/Base/Domain#Reactance> ;
                        rdfs:comment """Zero sequence series reactance of the transformer end.
""" .


###  https://w3id.org/netbeheer/IECCIM/TC57CIM/IEC61970/Base/Wires#PowerTransformer_PowerTransformerEnd
:PowerTransformer_PowerTransformerEnd rdf:type owl:ObjectProperty ;
                                      rdfs:domain :PowerTransformer ;
                                      rdfs:range :PowerTransformerEnd ;
                                      rdfs:comment "The power transformer of this power transformer end.The ends of this power transformer." .


###  https://w3id.org/netbeheer/IECCIM/TC57CIM/IEC61970/Base/Wires#PowerTransformer_TransformerTanks
:PowerTransformer_TransformerTanks rdf:type owl:ObjectProperty ;
                                   owl:inverseOf :TransformerTank_PowerTransformer ;
                                   rdfs:domain :PowerTransformer ;
                                   rdfs:range :TransformerTank ;
                                   rdfs:comment "All transformers that belong to this bank.Bank this transformer belongs to." .


###  https://w3id.org/netbeheer/IECCIM/TC57CIM/IEC61970/Base/Wires#PowerTransformer_beforeShCircuitHighestOperatingCurrent
:PowerTransformer_beforeShCircuitHighestOperatingCurrent rdf:type owl:ObjectProperty ;
                                                         rdfs:domain :PowerTransformer ;
                                                         rdfs:range <https://w3id.org/netbeheer/IECCIM/TC57CIM/IEC61970/Base/Domain#CurrentFlow> ;
                                                         rdfs:comment "The highest operating current (Ib in the IEC 60909-0) before short circuit (depends on network configuration and relevant reliability philosophy). It is used for calculation of the impedance correction factor KT defined in IEC 60909-0." .


###  https://w3id.org/netbeheer/IECCIM/TC57CIM/IEC61970/Base/Wires#PowerTransformer_beforeShCircuitHighestOperatingVoltage
:PowerTransformer_beforeShCircuitHighestOperatingVoltage rdf:type owl:ObjectProperty ;
                                                         rdfs:domain :PowerTransformer ;
                                                         rdfs:range <https://w3id.org/netbeheer/IECCIM/TC57CIM/IEC61970/Base/Domain#Voltage> ;
                                                         rdfs:comment "The highest operating voltage (Ub in the IEC 60909-0) before short circuit. It is used for calculation of the impedance correction factor KT defined in IEC 60909-0. This is worst case voltage on the low side winding (Section 3.7.1 in the standard). Used to define operating conditions." .


###  https://w3id.org/netbeheer/IECCIM/TC57CIM/IEC61970/Base/Wires#PowerTransformer_beforeShortCircuitAnglePf
:PowerTransformer_beforeShortCircuitAnglePf rdf:type owl:ObjectProperty ;
                                            rdfs:domain :PowerTransformer ;
                                            rdfs:range <https://w3id.org/netbeheer/IECCIM/TC57CIM/IEC61970/Base/Domain#AngleDegrees> ;
                                            rdfs:comment "The angle of power factor before short circuit (phib in the IEC 60909-0). It is used for calculation of the impedance correction factor KT defined in IEC 60909-0. This is the worst case power factor. Used to define operating conditions." .


###  https://w3id.org/netbeheer/IECCIM/TC57CIM/IEC61970/Base/Wires#PowerTransformer_highSideMinOperatingU
:PowerTransformer_highSideMinOperatingU rdf:type owl:ObjectProperty ;
                                        rdfs:domain :PowerTransformer ;
                                        rdfs:range <https://w3id.org/netbeheer/IECCIM/TC57CIM/IEC61970/Base/Domain#Voltage> ;
                                        rdfs:comment "The minimum operating voltage (uQmin in the IEC 60909-0) at the high voltage side (Q side) of the unit transformer of the power station unit. A value well established from long-term operating experience of the system. It is used for calculation of the impedance correction factor KG defined in IEC 60909-0" .


###  https://w3id.org/netbeheer/IECCIM/TC57CIM/IEC61970/Base/Wires#PrimeMover_SynchronousMachines
:PrimeMover_SynchronousMachines rdf:type owl:ObjectProperty ;
                                rdfs:domain <https://w3id.org/netbeheer/IECCIM/TC57CIM/IEC61970/Base/Generation/GenerationTrainingSimulation#PrimeMover> ;
                                rdfs:range :SynchronousMachine ;
                                rdfs:comment "Prime movers that drive this SynchronousMachine.Synchronous machines this Prime mover drives." .


###  https://w3id.org/netbeheer/IECCIM/TC57CIM/IEC61970/Base/Wires#ProtectedSwitch_OperatedByProtectionEquipment
:ProtectedSwitch_OperatedByProtectionEquipment rdf:type owl:ObjectProperty ;
                                               owl:inverseOf :ProtectionEquipment_ProtectedSwitches ;
                                               rdfs:domain :ProtectedSwitch ;
                                               rdfs:range <https://w3id.org/netbeheer/IECCIM/TC57CIM/IEC61970/Base/Protection#ProtectionEquipment> ;
                                               rdfs:comment "Protection equipments that operate this ProtectedSwitch.Protected switches operated by this ProtectionEquipment." .


###  https://w3id.org/netbeheer/IECCIM/TC57CIM/IEC61970/Base/Wires#ProtectedSwitch_RecloseSequences
:ProtectedSwitch_RecloseSequences rdf:type owl:ObjectProperty ;
                                  owl:inverseOf :RecloseSequence_ProtectedSwitch ;
                                  rdf:type owl:FunctionalProperty ;
                                  rdfs:domain :ProtectedSwitch ;
                                  rdfs:range <https://w3id.org/netbeheer/IECCIM/TC57CIM/IEC61970/Base/Protection#RecloseSequence> ;
                                  rdfs:comment "A breaker may have zero or more automatic reclosures after a trip occurs.A breaker may have zero or more automatic reclosures after a trip occurs." .


###  https://w3id.org/netbeheer/IECCIM/TC57CIM/IEC61970/Base/Wires#ProtectedSwitch_breakingCapacity
:ProtectedSwitch_breakingCapacity rdf:type owl:ObjectProperty ;
                                  rdfs:domain :ProtectedSwitch ;
                                  rdfs:range <https://w3id.org/netbeheer/IECCIM/TC57CIM/IEC61970/Base/Domain#CurrentFlow> ;
                                  rdfs:comment """The maximum fault current a breaking device can break safely under prescribed conditions of use.
""" .


###  https://w3id.org/netbeheer/IECCIM/TC57CIM/IEC61970/Base/Wires#ProtectionEquipment_ProtectedSwitches
:ProtectionEquipment_ProtectedSwitches rdf:type owl:ObjectProperty ;
                                       rdfs:domain <https://w3id.org/netbeheer/IECCIM/TC57CIM/IEC61970/Base/Protection#ProtectionEquipment> ;
                                       rdfs:range :ProtectedSwitch ;
                                       rdfs:comment "Protection equipments that operate this ProtectedSwitch.Protected switches operated by this ProtectionEquipment." .


###  https://w3id.org/netbeheer/IECCIM/TC57CIM/IEC61970/Base/Wires#ProtectiveActionRegulation_RegulatingControl
:ProtectiveActionRegulation_RegulatingControl rdf:type owl:ObjectProperty ;
                                              rdfs:domain <https://w3id.org/netbeheer/IECCIM/TC57CIM/IEC61970/InfIEC61970/InfSIPS#ProtectiveActionRegulation> ;
                                              rdfs:range :RegulatingControl ;
                                              rdfs:comment "" .


###  https://w3id.org/netbeheer/IECCIM/TC57CIM/IEC61970/Base/Wires#RatioTapChangerTablePoint_RatioTapChangerTable
:RatioTapChangerTablePoint_RatioTapChangerTable rdf:type owl:ObjectProperty ;
                                                rdfs:domain :RatioTapChangerTablePoint ;
                                                rdfs:range :RatioTapChangerTable ;
                                                rdfs:comment "Points of this table.Table of this point." .


###  https://w3id.org/netbeheer/IECCIM/TC57CIM/IEC61970/Base/Wires#RatioTapChangerTable_RatioTapChanger
:RatioTapChangerTable_RatioTapChanger rdf:type owl:ObjectProperty ;
                                      owl:inverseOf :RatioTapChanger_RatioTapChangerTable ;
                                      rdfs:domain :RatioTapChangerTable ;
                                      rdfs:range :RatioTapChanger ;
                                      rdfs:comment "The ratio tap changer of this tap ratio table.The tap ratio table for this ratio  tap changer." .


###  https://w3id.org/netbeheer/IECCIM/TC57CIM/IEC61970/Base/Wires#RatioTapChangerTable_RatioTapChangerTablePoint
:RatioTapChangerTable_RatioTapChangerTablePoint rdf:type owl:ObjectProperty ;
                                                owl:inverseOf :RatioTapChangerTablePoint_RatioTapChangerTable ;
                                                rdf:type owl:FunctionalProperty ;
                                                rdfs:domain :RatioTapChangerTable ;
                                                rdfs:range :RatioTapChangerTablePoint ;
                                                rdfs:comment "Points of this table.Table of this point." .


###  https://w3id.org/netbeheer/IECCIM/TC57CIM/IEC61970/Base/Wires#RatioTapChanger_RatioTapChangerTable
:RatioTapChanger_RatioTapChangerTable rdf:type owl:ObjectProperty ;
                                      rdfs:domain :RatioTapChanger ;
                                      rdfs:range :RatioTapChangerTable ;
                                      rdfs:comment "The ratio tap changer of this tap ratio table.The tap ratio table for this ratio  tap changer." .


###  https://w3id.org/netbeheer/IECCIM/TC57CIM/IEC61970/Base/Wires#RatioTapChanger_TransformerEnd
:RatioTapChanger_TransformerEnd rdf:type owl:ObjectProperty ;
                                owl:inverseOf :TransformerEnd_RatioTapChanger ;
                                rdfs:domain :RatioTapChanger ;
                                rdfs:range :TransformerEnd ;
                                rdfs:comment "Transformer end to which this ratio tap changer belongs.Ratio tap changer associated with this transformer end." .


###  https://w3id.org/netbeheer/IECCIM/TC57CIM/IEC61970/Base/Wires#RatioTapChanger_stepVoltageIncrement
:RatioTapChanger_stepVoltageIncrement rdf:type owl:ObjectProperty ;
                                      rdfs:domain :RatioTapChanger ;
                                      rdfs:range <https://w3id.org/netbeheer/IECCIM/TC57CIM/IEC61970/Base/Domain#PerCent> ;
                                      rdfs:comment """Tap step increment, in per cent of nominal voltage, per step position.
""" .


###  https://w3id.org/netbeheer/IECCIM/TC57CIM/IEC61970/Base/Wires#ReactiveCapabilityCurve_EquivalentInjection
:ReactiveCapabilityCurve_EquivalentInjection rdf:type owl:ObjectProperty ;
                                             rdfs:domain :ReactiveCapabilityCurve ;
                                             rdfs:range <https://w3id.org/netbeheer/IECCIM/TC57CIM/IEC61970/Base/Equivalents#EquivalentInjection> ;
                                             rdfs:comment "The reactive capability curve used by this equivalent injection.The equivalent injection using this reactive capability curve." .


###  https://w3id.org/netbeheer/IECCIM/TC57CIM/IEC61970/Base/Wires#ReactiveCapabilityCurve_InitiallyUsedBySynchronousMachines
:ReactiveCapabilityCurve_InitiallyUsedBySynchronousMachines rdf:type owl:ObjectProperty ;
                                                            rdfs:domain :ReactiveCapabilityCurve ;
                                                            rdfs:range :SynchronousMachine ;
                                                            rdfs:comment "The default reactive capability curve for use by a synchronous machine.Synchronous machines using this curve as default." .


###  https://w3id.org/netbeheer/IECCIM/TC57CIM/IEC61970/Base/Wires#ReactiveCapabilityCurve_SynchronousMachines
:ReactiveCapabilityCurve_SynchronousMachines rdf:type owl:ObjectProperty ;
                                             rdfs:domain :ReactiveCapabilityCurve ;
                                             rdfs:range :SynchronousMachine ;
                                             rdfs:comment "All available reactive capability curves for this synchronous machine.Synchronous machines using this curve." .


###  https://w3id.org/netbeheer/IECCIM/TC57CIM/IEC61970/Base/Wires#ReactiveCapabilityCurve_coolantTemperature
:ReactiveCapabilityCurve_coolantTemperature rdf:type owl:ObjectProperty ;
                                            rdfs:domain :ReactiveCapabilityCurve ;
                                            rdfs:range <https://w3id.org/netbeheer/IECCIM/TC57CIM/IEC61970/Base/Domain#Temperature> ;
                                            rdfs:comment "The machine's coolant temperature (e.g., ambient air or stator circulating water)." .


###  https://w3id.org/netbeheer/IECCIM/TC57CIM/IEC61970/Base/Wires#ReactiveCapabilityCurve_hydrogenPressure
:ReactiveCapabilityCurve_hydrogenPressure rdf:type owl:ObjectProperty ;
                                          rdfs:domain :ReactiveCapabilityCurve ;
                                          rdfs:range <https://w3id.org/netbeheer/IECCIM/TC57CIM/IEC61970/Base/Domain#Pressure> ;
                                          rdfs:comment "The hydrogen coolant pressure" .


###  https://w3id.org/netbeheer/IECCIM/TC57CIM/IEC61970/Base/Wires#RecloseSequence_ProtectedSwitch
:RecloseSequence_ProtectedSwitch rdf:type owl:ObjectProperty ;
                                 rdfs:domain <https://w3id.org/netbeheer/IECCIM/TC57CIM/IEC61970/Base/Protection#RecloseSequence> ;
                                 rdfs:range :ProtectedSwitch ;
                                 rdfs:comment "A breaker may have zero or more automatic reclosures after a trip occurs.A breaker may have zero or more automatic reclosures after a trip occurs." .


###  https://w3id.org/netbeheer/IECCIM/TC57CIM/IEC61970/Base/Wires#RegulatingCondEq_RegulatingControl
:RegulatingCondEq_RegulatingControl rdf:type owl:ObjectProperty ;
                                    rdfs:domain :RegulatingCondEq ;
                                    rdfs:range :RegulatingControl ;
                                    rdfs:comment "The equipment that participates in this regulating control scheme.The regulating control scheme in which this equipment participates." .


###  https://w3id.org/netbeheer/IECCIM/TC57CIM/IEC61970/Base/Wires#RegulatingControl_ProtectiveActionRegulation
:RegulatingControl_ProtectiveActionRegulation rdf:type owl:ObjectProperty ;
                                              owl:inverseOf :ProtectiveActionRegulation_RegulatingControl ;
                                              rdf:type owl:FunctionalProperty ;
                                              rdfs:domain :RegulatingControl ;
                                              rdfs:range <https://w3id.org/netbeheer/IECCIM/TC57CIM/IEC61970/InfIEC61970/InfSIPS#ProtectiveActionRegulation> ;
                                              rdfs:comment "" .


###  https://w3id.org/netbeheer/IECCIM/TC57CIM/IEC61970/Base/Wires#RegulatingControl_RegulatingCondEq
:RegulatingControl_RegulatingCondEq rdf:type owl:ObjectProperty ;
                                    owl:inverseOf :RegulatingCondEq_RegulatingControl ;
                                    rdfs:domain :RegulatingControl ;
                                    rdfs:range :RegulatingCondEq ;
                                    rdfs:comment "The equipment that participates in this regulating control scheme.The regulating control scheme in which this equipment participates." .


###  https://w3id.org/netbeheer/IECCIM/TC57CIM/IEC61970/Base/Wires#RegulatingControl_RegulationSchedule
:RegulatingControl_RegulationSchedule rdf:type owl:ObjectProperty ;
                                      owl:inverseOf :RegulationSchedule_RegulatingControl ;
                                      rdf:type owl:FunctionalProperty ;
                                      rdfs:domain :RegulatingControl ;
                                      rdfs:range :RegulationSchedule ;
                                      rdfs:comment "Schedule for this Regulating regulating control.Regulating controls that have this Schedule." .


###  https://w3id.org/netbeheer/IECCIM/TC57CIM/IEC61970/Base/Wires#RegulationSchedule_RegulatingControl
:RegulationSchedule_RegulatingControl rdf:type owl:ObjectProperty ;
                                      rdfs:domain :RegulationSchedule ;
                                      rdfs:range :RegulatingControl ;
                                      rdfs:comment "Schedule for this Regulating regulating control.Regulating controls that have this Schedule." .


###  https://w3id.org/netbeheer/IECCIM/TC57CIM/IEC61970/Base/Wires#RegulationSchedule_VoltageControlZones
:RegulationSchedule_VoltageControlZones rdf:type owl:ObjectProperty ;
                                        rdfs:domain :RegulationSchedule ;
                                        rdfs:range :VoltageControlZone ;
                                        rdfs:comment "A VoltageControlZone may have a  voltage regulation schedule.A VoltageControlZone may have a  voltage regulation schedule." .


###  https://w3id.org/netbeheer/IECCIM/TC57CIM/IEC61970/Base/Wires#RotatingMachine_GeneratingUnit
:RotatingMachine_GeneratingUnit rdf:type owl:ObjectProperty ;
                                owl:inverseOf :GeneratingUnit_RotatingMachine ;
                                rdfs:domain :RotatingMachine ;
                                rdfs:range <https://w3id.org/netbeheer/IECCIM/TC57CIM/IEC61970/Base/Generation/Production#GeneratingUnit> ;
                                rdfs:comment "A synchronous machine may operate as a generator and as such becomes a member of a generating unit.A synchronous machine may operate as a generator and as such becomes a member of a generating unit." .


###  https://w3id.org/netbeheer/IECCIM/TC57CIM/IEC61970/Base/Wires#RotatingMachine_HydroPump
:RotatingMachine_HydroPump rdf:type owl:ObjectProperty ,
                                    owl:FunctionalProperty ;
                           rdfs:domain :RotatingMachine ;
                           rdfs:range <https://w3id.org/netbeheer/IECCIM/TC57CIM/IEC61970/Base/Generation/Production#HydroPump> ;
                           rdfs:comment "The synchronous machine drives the turbine which moves the water from a low elevation to a higher elevation. The direction of machine rotation for pumping may or may not be the same as for generating.The synchronous machine drives the turbine which moves the water from a low elevation to a higher elevation. The direction of machine rotation for pumping may or may not be the same as for generating." .


###  https://w3id.org/netbeheer/IECCIM/TC57CIM/IEC61970/Base/Wires#RotatingMachine_p
:RotatingMachine_p rdf:type owl:ObjectProperty ;
                   rdfs:domain :RotatingMachine ;
                   rdfs:range <https://w3id.org/netbeheer/IECCIM/TC57CIM/IEC61970/Base/Domain#ActivePower> ;
                   rdfs:comment """Active power injection. Load sign convention is used, i.e. positive sign means flow out from a node.
Starting value for a steady state solution.""" .


###  https://w3id.org/netbeheer/IECCIM/TC57CIM/IEC61970/Base/Wires#RotatingMachine_q
:RotatingMachine_q rdf:type owl:ObjectProperty ;
                   rdfs:domain :RotatingMachine ;
                   rdfs:range <https://w3id.org/netbeheer/IECCIM/TC57CIM/IEC61970/Base/Domain#ReactivePower> ;
                   rdfs:comment """Reactive power injection. Load sign convention is used, i.e. positive sign means flow out from a node.
Starting value for a steady state solution.""" .


###  https://w3id.org/netbeheer/IECCIM/TC57CIM/IEC61970/Base/Wires#RotatingMachine_ratedS
:RotatingMachine_ratedS rdf:type owl:ObjectProperty ;
                        rdfs:domain :RotatingMachine ;
                        rdfs:range <https://w3id.org/netbeheer/IECCIM/TC57CIM/IEC61970/Base/Domain#ApparentPower> ;
                        rdfs:comment """Nameplate apparent power rating for the unit.
The attribute shall have a positive value.""" .


###  https://w3id.org/netbeheer/IECCIM/TC57CIM/IEC61970/Base/Wires#RotatingMachine_ratedU
:RotatingMachine_ratedU rdf:type owl:ObjectProperty ;
                        rdfs:domain :RotatingMachine ;
                        rdfs:range <https://w3id.org/netbeheer/IECCIM/TC57CIM/IEC61970/Base/Domain#Voltage> ;
                        rdfs:comment "Rated voltage (nameplate data, Ur in IEC 60909-0). It is primarily used for short circuit data exchange according to IEC 60909." .


###  https://w3id.org/netbeheer/IECCIM/TC57CIM/IEC61970/Base/Wires#SeriesCompensator_r
:SeriesCompensator_r rdf:type owl:ObjectProperty ;
                     rdfs:domain :SeriesCompensator ;
                     rdfs:range <https://w3id.org/netbeheer/IECCIM/TC57CIM/IEC61970/Base/Domain#Resistance> ;
                     rdfs:comment "Positive sequence resistance." .


###  https://w3id.org/netbeheer/IECCIM/TC57CIM/IEC61970/Base/Wires#SeriesCompensator_r0
:SeriesCompensator_r0 rdf:type owl:ObjectProperty ;
                      rdfs:domain :SeriesCompensator ;
                      rdfs:range <https://w3id.org/netbeheer/IECCIM/TC57CIM/IEC61970/Base/Domain#Resistance> ;
                      rdfs:comment """Zero sequence resistance.
""" .


###  https://w3id.org/netbeheer/IECCIM/TC57CIM/IEC61970/Base/Wires#SeriesCompensator_varistorRatedCurrent
:SeriesCompensator_varistorRatedCurrent rdf:type owl:ObjectProperty ;
                                        rdfs:domain :SeriesCompensator ;
                                        rdfs:range <https://w3id.org/netbeheer/IECCIM/TC57CIM/IEC61970/Base/Domain#CurrentFlow> ;
                                        rdfs:comment "The maximum current the varistor is designed to handle at specified duration." .


###  https://w3id.org/netbeheer/IECCIM/TC57CIM/IEC61970/Base/Wires#SeriesCompensator_varistorVoltageThreshold
:SeriesCompensator_varistorVoltageThreshold rdf:type owl:ObjectProperty ;
                                            rdfs:domain :SeriesCompensator ;
                                            rdfs:range <https://w3id.org/netbeheer/IECCIM/TC57CIM/IEC61970/Base/Domain#Voltage> ;
                                            rdfs:comment "The dc voltage at which the varistor start conducting." .


###  https://w3id.org/netbeheer/IECCIM/TC57CIM/IEC61970/Base/Wires#SeriesCompensator_x
:SeriesCompensator_x rdf:type owl:ObjectProperty ;
                     rdfs:domain :SeriesCompensator ;
                     rdfs:range <https://w3id.org/netbeheer/IECCIM/TC57CIM/IEC61970/Base/Domain#Reactance> ;
                     rdfs:comment "Positive sequence reactance." .


###  https://w3id.org/netbeheer/IECCIM/TC57CIM/IEC61970/Base/Wires#SeriesCompensator_x0
:SeriesCompensator_x0 rdf:type owl:ObjectProperty ;
                      rdfs:domain :SeriesCompensator ;
                      rdfs:range <https://w3id.org/netbeheer/IECCIM/TC57CIM/IEC61970/Base/Domain#Reactance> ;
                      rdfs:comment """Zero sequence reactance.
""" .


###  https://w3id.org/netbeheer/IECCIM/TC57CIM/IEC61970/Base/Wires#ShuntCompensatorPhase_ShuntCompensator
:ShuntCompensatorPhase_ShuntCompensator rdf:type owl:ObjectProperty ;
                                        owl:inverseOf :ShuntCompensator_ShuntCompensatorPhase ;
                                        rdfs:domain :ShuntCompensatorPhase ;
                                        rdfs:range :ShuntCompensator ;
                                        rdfs:comment "Shunt compensator of this shunt compensator phase.The individual phases models for the shunt compensator." .


###  https://w3id.org/netbeheer/IECCIM/TC57CIM/IEC61970/Base/Wires#ShuntCompensator_ShuntCompensatorPhase
:ShuntCompensator_ShuntCompensatorPhase rdf:type owl:ObjectProperty ,
                                                 owl:FunctionalProperty ;
                                        rdfs:domain :ShuntCompensator ;
                                        rdfs:range :ShuntCompensatorPhase ;
                                        rdfs:comment "Shunt compensator of this shunt compensator phase.The individual phases models for the shunt compensator." .


###  https://w3id.org/netbeheer/IECCIM/TC57CIM/IEC61970/Base/Wires#ShuntCompensator_SvShuntCompensatorSections
:ShuntCompensator_SvShuntCompensatorSections rdf:type owl:ObjectProperty ;
                                             owl:inverseOf :SvShuntCompensatorSections_ShuntCompensator ;
                                             rdf:type owl:FunctionalProperty ;
                                             rdfs:domain :ShuntCompensator ;
                                             rdfs:range <https://w3id.org/netbeheer/IECCIM/TC57CIM/IEC61970/Base/StateVariables#SvShuntCompensatorSections> ;
                                             rdfs:comment "The state for the number of shunt compensator sections in service.The shunt compensator for which the state applies." .


###  https://w3id.org/netbeheer/IECCIM/TC57CIM/IEC61970/Base/Wires#ShuntCompensator_aVRDelay
:ShuntCompensator_aVRDelay rdf:type owl:ObjectProperty ;
                           rdfs:domain :ShuntCompensator ;
                           rdfs:range <https://w3id.org/netbeheer/IECCIM/TC57CIM/IEC61970/Base/Domain#Seconds> ;
                           rdfs:comment "Time delay required for the device to be connected or disconnected by automatic voltage regulation (AVR)." .


###  https://w3id.org/netbeheer/IECCIM/TC57CIM/IEC61970/Base/Wires#ShuntCompensator_nomU
:ShuntCompensator_nomU rdf:type owl:ObjectProperty ;
                       rdfs:domain :ShuntCompensator ;
                       rdfs:range <https://w3id.org/netbeheer/IECCIM/TC57CIM/IEC61970/Base/Domain#Voltage> ;
                       rdfs:comment """The voltage at which the nominal reactive power may be calculated. This should normally be within 10% of the voltage at which the capacitor is connected to the network.
""" .


###  https://w3id.org/netbeheer/IECCIM/TC57CIM/IEC61970/Base/Wires#ShuntCompensator_voltageSensitivity
:ShuntCompensator_voltageSensitivity rdf:type owl:ObjectProperty ;
                                     rdfs:domain :ShuntCompensator ;
                                     rdfs:range <https://w3id.org/netbeheer/IECCIM/TC57CIM/IEC61970/Base/Domain#VoltagePerReactivePower> ;
                                     rdfs:comment "Voltage sensitivity required for the device to regulate the bus voltage, in voltage/reactive power." .


###  https://w3id.org/netbeheer/IECCIM/TC57CIM/IEC61970/Base/Wires#StaticVarCompensator_capacitiveRating
:StaticVarCompensator_capacitiveRating rdf:type owl:ObjectProperty ;
                                       rdfs:domain :StaticVarCompensator ;
                                       rdfs:range <https://w3id.org/netbeheer/IECCIM/TC57CIM/IEC61970/Base/Domain#Reactance> ;
                                       rdfs:comment """Maximum available capacitive reactance.
""" .


###  https://w3id.org/netbeheer/IECCIM/TC57CIM/IEC61970/Base/Wires#StaticVarCompensator_inductiveRating
:StaticVarCompensator_inductiveRating rdf:type owl:ObjectProperty ;
                                      rdfs:domain :StaticVarCompensator ;
                                      rdfs:range <https://w3id.org/netbeheer/IECCIM/TC57CIM/IEC61970/Base/Domain#Reactance> ;
                                      rdfs:comment """Maximum available inductive reactance.
""" .


###  https://w3id.org/netbeheer/IECCIM/TC57CIM/IEC61970/Base/Wires#StaticVarCompensator_q
:StaticVarCompensator_q rdf:type owl:ObjectProperty ;
                        rdfs:domain :StaticVarCompensator ;
                        rdfs:range <https://w3id.org/netbeheer/IECCIM/TC57CIM/IEC61970/Base/Domain#ReactivePower> ;
                        rdfs:comment """Reactive power injection. Load sign convention is used, i.e. positive sign means flow out from a node.
Starting value for a steady state solution.""" .


###  https://w3id.org/netbeheer/IECCIM/TC57CIM/IEC61970/Base/Wires#StaticVarCompensator_slope
:StaticVarCompensator_slope rdf:type owl:ObjectProperty ;
                            rdfs:domain :StaticVarCompensator ;
                            rdfs:range <https://w3id.org/netbeheer/IECCIM/TC57CIM/IEC61970/Base/Domain#VoltagePerReactivePower> ;
                            rdfs:comment "The characteristics slope of an SVC defines how the reactive power output changes in proportion to the difference between the regulated bus voltage and the voltage setpoint." .


###  https://w3id.org/netbeheer/IECCIM/TC57CIM/IEC61970/Base/Wires#StaticVarCompensator_voltageSetPoint
:StaticVarCompensator_voltageSetPoint rdf:type owl:ObjectProperty ;
                                      rdfs:domain :StaticVarCompensator ;
                                      rdfs:range <https://w3id.org/netbeheer/IECCIM/TC57CIM/IEC61970/Base/Domain#Voltage> ;
                                      rdfs:comment "The reactive power output of the SVC is proportional to the difference between the voltage at the regulated bus and the voltage setpoint.  When the regulated bus voltage is equal to the voltage setpoint, the reactive power output is zero." .


###  https://w3id.org/netbeheer/IECCIM/TC57CIM/IEC61970/Base/Wires#SvShuntCompensatorSections_ShuntCompensator
:SvShuntCompensatorSections_ShuntCompensator rdf:type owl:ObjectProperty ;
                                             rdfs:domain <https://w3id.org/netbeheer/IECCIM/TC57CIM/IEC61970/Base/StateVariables#SvShuntCompensatorSections> ;
                                             rdfs:range :ShuntCompensator ;
                                             rdfs:comment "The state for the number of shunt compensator sections in service.The shunt compensator for which the state applies." .


###  https://w3id.org/netbeheer/IECCIM/TC57CIM/IEC61970/Base/Wires#SvTapStep_TapChanger
:SvTapStep_TapChanger rdf:type owl:ObjectProperty ;
                      rdfs:domain <https://w3id.org/netbeheer/IECCIM/TC57CIM/IEC61970/Base/StateVariables#SvTapStep> ;
                      rdfs:range :TapChanger ;
                      rdfs:comment "The tap step state associated with the tap changer.The tap changer associated with the tap step state." .


###  https://w3id.org/netbeheer/IECCIM/TC57CIM/IEC61970/Base/Wires#SwitchAction_OperatedSwitch
:SwitchAction_OperatedSwitch rdf:type owl:ObjectProperty ;
                             rdfs:domain <https://w3id.org/netbeheer/IECCIM/TC57CIM/IEC61968/Operations#SwitchAction> ;
                             rdfs:range :Switch ;
                             rdfs:comment "Action changing status of this switch.Switch that is the object of this switch action." .


###  https://w3id.org/netbeheer/IECCIM/TC57CIM/IEC61970/Base/Wires#SwitchPhase_Switch
:SwitchPhase_Switch rdf:type owl:ObjectProperty ;
                    owl:inverseOf :Switch_SwitchPhase ;
                    rdfs:domain :SwitchPhase ;
                    rdfs:range :Switch ;
                    rdfs:comment "The switch of the switch phase.The individual switch phases for the switch." .


###  https://w3id.org/netbeheer/IECCIM/TC57CIM/IEC61970/Base/Wires#SwitchSchedule_Switch
:SwitchSchedule_Switch rdf:type owl:ObjectProperty ;
                       owl:inverseOf :Switch_SwitchSchedules ;
                       rdfs:domain :SwitchSchedule ;
                       rdfs:range :Switch ;
                       rdfs:comment "A SwitchSchedule is associated with a Switch.A Switch can be associated with SwitchSchedules." .


###  https://w3id.org/netbeheer/IECCIM/TC57CIM/IEC61970/Base/Wires#Switch_CompositeSwitch
:Switch_CompositeSwitch rdf:type owl:ObjectProperty ;
                        owl:inverseOf :CompositeSwitch_Switches ;
                        rdfs:domain :Switch ;
                        rdfs:range :CompositeSwitch ;
                        rdfs:comment "Composite switch to which this Switch belongs.Switches contained in this Composite switch." .


###  https://w3id.org/netbeheer/IECCIM/TC57CIM/IEC61970/Base/Wires#Switch_ConnectDisconnectFunctions
:Switch_ConnectDisconnectFunctions rdf:type owl:ObjectProperty ;
                                   owl:inverseOf :ConnectDisconnectFunction_Switches ;
                                   rdfs:domain :Switch ;
                                   rdfs:range <https://w3id.org/netbeheer/IECCIM/TC57CIM/IEC61968/LoadControl#ConnectDisconnectFunction> ;
                                   rdfs:comment "" .


###  https://w3id.org/netbeheer/IECCIM/TC57CIM/IEC61970/Base/Wires#Switch_Outage
:Switch_Outage rdf:type owl:ObjectProperty ;
               owl:inverseOf :Outage_OpenedSwitches ;
               rdfs:domain :Switch ;
               rdfs:range <https://w3id.org/netbeheer/IECCIM/TC57CIM/IEC61968/Operations#Outage> ;
               rdfs:comment "Current outage of this protective device.All potentially open switches causing this outage. This realationship is meant to be used as \"indication\" for initiation of outage-related business processes, whereas for actual actions of switches, SwitchAction-Switch relationship should be used." .


###  https://w3id.org/netbeheer/IECCIM/TC57CIM/IEC61970/Base/Wires#Switch_SwitchAction
:Switch_SwitchAction rdf:type owl:ObjectProperty ;
                     owl:inverseOf :SwitchAction_OperatedSwitch ;
                     rdfs:domain :Switch ;
                     rdfs:range <https://w3id.org/netbeheer/IECCIM/TC57CIM/IEC61968/Operations#SwitchAction> ;
                     rdfs:comment "Action changing status of this switch.Switch that is the object of this switch action." .


###  https://w3id.org/netbeheer/IECCIM/TC57CIM/IEC61970/Base/Wires#Switch_SwitchPhase
:Switch_SwitchPhase rdf:type owl:ObjectProperty ,
                             owl:FunctionalProperty ;
                    rdfs:domain :Switch ;
                    rdfs:range :SwitchPhase ;
                    rdfs:comment "The switch of the switch phase.The individual switch phases for the switch." .


###  https://w3id.org/netbeheer/IECCIM/TC57CIM/IEC61970/Base/Wires#Switch_SwitchSchedules
:Switch_SwitchSchedules rdf:type owl:ObjectProperty ,
                                 owl:FunctionalProperty ;
                        rdfs:domain :Switch ;
                        rdfs:range :SwitchSchedule ;
                        rdfs:comment "A SwitchSchedule is associated with a Switch.A Switch can be associated with SwitchSchedules." .


###  https://w3id.org/netbeheer/IECCIM/TC57CIM/IEC61970/Base/Wires#Switch_ratedCurrent
:Switch_ratedCurrent rdf:type owl:ObjectProperty ;
                     rdfs:domain :Switch ;
                     rdfs:range <https://w3id.org/netbeheer/IECCIM/TC57CIM/IEC61970/Base/Domain#CurrentFlow> ;
                     rdfs:comment """The maximum continuous current carrying capacity in amps governed by the device material and construction.
""" .


###  https://w3id.org/netbeheer/IECCIM/TC57CIM/IEC61970/Base/Wires#SynchronousMachineDynamics_SynchronousMachine
:SynchronousMachineDynamics_SynchronousMachine rdf:type owl:ObjectProperty ;
                                               rdfs:domain <https://w3id.org/netbeheer/IECCIM/TC57CIM/IEC61970/Dynamics/StandardModels/SynchronousMachineDynamics#SynchronousMachineDynamics> ;
                                               rdfs:range :SynchronousMachine ;
                                               rdfs:comment "Synchronous machine dynamics model used to describe dynamic behavior of this synchronous machine.Synchronous machine to which synchronous machine dynamics model applies." .


###  https://w3id.org/netbeheer/IECCIM/TC57CIM/IEC61970/Base/Wires#SynchronousMachine_InitialReactiveCapabilityCurve
:SynchronousMachine_InitialReactiveCapabilityCurve rdf:type owl:ObjectProperty ;
                                                   owl:inverseOf :ReactiveCapabilityCurve_InitiallyUsedBySynchronousMachines ;
                                                   rdfs:domain :SynchronousMachine ;
                                                   rdfs:range :ReactiveCapabilityCurve ;
                                                   rdfs:comment "The default reactive capability curve for use by a synchronous machine.Synchronous machines using this curve as default." .


###  https://w3id.org/netbeheer/IECCIM/TC57CIM/IEC61970/Base/Wires#SynchronousMachine_PrimeMovers
:SynchronousMachine_PrimeMovers rdf:type owl:ObjectProperty ;
                                owl:inverseOf :PrimeMover_SynchronousMachines ;
                                rdfs:domain :SynchronousMachine ;
                                rdfs:range <https://w3id.org/netbeheer/IECCIM/TC57CIM/IEC61970/Base/Generation/GenerationTrainingSimulation#PrimeMover> ;
                                rdfs:comment "Prime movers that drive this SynchronousMachine.Synchronous machines this Prime mover drives." .


###  https://w3id.org/netbeheer/IECCIM/TC57CIM/IEC61970/Base/Wires#SynchronousMachine_ReactiveCapabilityCurves
:SynchronousMachine_ReactiveCapabilityCurves rdf:type owl:ObjectProperty ;
                                             owl:inverseOf :ReactiveCapabilityCurve_SynchronousMachines ;
                                             rdfs:domain :SynchronousMachine ;
                                             rdfs:range :ReactiveCapabilityCurve ;
                                             rdfs:comment "All available reactive capability curves for this synchronous machine.Synchronous machines using this curve." .


###  https://w3id.org/netbeheer/IECCIM/TC57CIM/IEC61970/Base/Wires#SynchronousMachine_SynchronousMachineDynamics
:SynchronousMachine_SynchronousMachineDynamics rdf:type owl:ObjectProperty ;
                                               owl:inverseOf :SynchronousMachineDynamics_SynchronousMachine ;
                                               rdf:type owl:FunctionalProperty ;
                                               rdfs:domain :SynchronousMachine ;
                                               rdfs:range <https://w3id.org/netbeheer/IECCIM/TC57CIM/IEC61970/Dynamics/StandardModels/SynchronousMachineDynamics#SynchronousMachineDynamics> ;
                                               rdfs:comment "Synchronous machine dynamics model used to describe dynamic behavior of this synchronous machine.Synchronous machine to which synchronous machine dynamics model applies." .


###  https://w3id.org/netbeheer/IECCIM/TC57CIM/IEC61970/Base/Wires#SynchronousMachine_aVRToManualLag
:SynchronousMachine_aVRToManualLag rdf:type owl:ObjectProperty ;
                                   rdfs:domain :SynchronousMachine ;
                                   rdfs:range <https://w3id.org/netbeheer/IECCIM/TC57CIM/IEC61970/Base/Domain#Seconds> ;
                                   rdfs:comment "Time delay required when switching from Automatic Voltage Regulation (AVR) to Manual for a lagging MVAr violation." .


###  https://w3id.org/netbeheer/IECCIM/TC57CIM/IEC61970/Base/Wires#SynchronousMachine_aVRToManualLead
:SynchronousMachine_aVRToManualLead rdf:type owl:ObjectProperty ;
                                    rdfs:domain :SynchronousMachine ;
                                    rdfs:range <https://w3id.org/netbeheer/IECCIM/TC57CIM/IEC61970/Base/Domain#Seconds> ;
                                    rdfs:comment "Time delay required when switching from Automatic Voltage Regulation (AVR) to Manual for a leading MVAr violation." .


###  https://w3id.org/netbeheer/IECCIM/TC57CIM/IEC61970/Base/Wires#SynchronousMachine_baseQ
:SynchronousMachine_baseQ rdf:type owl:ObjectProperty ;
                          rdfs:domain :SynchronousMachine ;
                          rdfs:range <https://w3id.org/netbeheer/IECCIM/TC57CIM/IEC61970/Base/Domain#ReactivePower> ;
                          rdfs:comment "Default base reactive power value. This value represents the initial reactive power that can be used by any application function." .


###  https://w3id.org/netbeheer/IECCIM/TC57CIM/IEC61970/Base/Wires#SynchronousMachine_condenserP
:SynchronousMachine_condenserP rdf:type owl:ObjectProperty ;
                               rdfs:domain :SynchronousMachine ;
                               rdfs:range <https://w3id.org/netbeheer/IECCIM/TC57CIM/IEC61970/Base/Domain#ActivePower> ;
                               rdfs:comment "Active power consumed when in condenser mode operation." .


###  https://w3id.org/netbeheer/IECCIM/TC57CIM/IEC61970/Base/Wires#SynchronousMachine_earthingStarPointR
:SynchronousMachine_earthingStarPointR rdf:type owl:ObjectProperty ;
                                       rdfs:domain :SynchronousMachine ;
                                       rdfs:range <https://w3id.org/netbeheer/IECCIM/TC57CIM/IEC61970/Base/Domain#Resistance> ;
                                       rdfs:comment "Generator star point earthing resistance (Re). Used for short circuit data exchange according to IEC 60909" .


###  https://w3id.org/netbeheer/IECCIM/TC57CIM/IEC61970/Base/Wires#SynchronousMachine_earthingStarPointX
:SynchronousMachine_earthingStarPointX rdf:type owl:ObjectProperty ;
                                       rdfs:domain :SynchronousMachine ;
                                       rdfs:range <https://w3id.org/netbeheer/IECCIM/TC57CIM/IEC61970/Base/Domain#Reactance> ;
                                       rdfs:comment "Generator star point earthing reactance (Xe). Used for short circuit data exchange according to IEC 60909" .


###  https://w3id.org/netbeheer/IECCIM/TC57CIM/IEC61970/Base/Wires#SynchronousMachine_ikk
:SynchronousMachine_ikk rdf:type owl:ObjectProperty ;
                        rdfs:domain :SynchronousMachine ;
                        rdfs:range <https://w3id.org/netbeheer/IECCIM/TC57CIM/IEC61970/Base/Domain#CurrentFlow> ;
                        rdfs:comment """Steady-state short-circuit current (in A for the profile) of generator with compound excitation during 3-phase short circuit.
- Ikk=0: Generator with no compound excitation.
- Ikk?0: Generator with compound excitation.
Ikk is used to calculate the minimum steady-state short-circuit current for generators with compound excitation
(Section 4.6.1.2 in the IEC 60909-0)
Used only for single fed short circuit on a generator. (Section 4.3.4.2. in the IEC 60909-0)""" .


###  https://w3id.org/netbeheer/IECCIM/TC57CIM/IEC61970/Base/Wires#SynchronousMachine_manualToAVR
:SynchronousMachine_manualToAVR rdf:type owl:ObjectProperty ;
                                rdfs:domain :SynchronousMachine ;
                                rdfs:range <https://w3id.org/netbeheer/IECCIM/TC57CIM/IEC61970/Base/Domain#Seconds> ;
                                rdfs:comment "Time delay required when switching from Manual to Automatic Voltage Regulation. This value is used in the accelerating power reference frame for powerflow solutions" .


###  https://w3id.org/netbeheer/IECCIM/TC57CIM/IEC61970/Base/Wires#SynchronousMachine_maxQ
:SynchronousMachine_maxQ rdf:type owl:ObjectProperty ;
                         rdfs:domain :SynchronousMachine ;
                         rdfs:range <https://w3id.org/netbeheer/IECCIM/TC57CIM/IEC61970/Base/Domain#ReactivePower> ;
                         rdfs:comment "Maximum reactive power limit. This is the maximum (nameplate) limit for the unit." .


###  https://w3id.org/netbeheer/IECCIM/TC57CIM/IEC61970/Base/Wires#SynchronousMachine_maxU
:SynchronousMachine_maxU rdf:type owl:ObjectProperty ;
                         rdfs:domain :SynchronousMachine ;
                         rdfs:range <https://w3id.org/netbeheer/IECCIM/TC57CIM/IEC61970/Base/Domain#Voltage> ;
                         rdfs:comment "Maximum voltage limit for the unit." .


###  https://w3id.org/netbeheer/IECCIM/TC57CIM/IEC61970/Base/Wires#SynchronousMachine_minQ
:SynchronousMachine_minQ rdf:type owl:ObjectProperty ;
                         rdfs:domain :SynchronousMachine ;
                         rdfs:range <https://w3id.org/netbeheer/IECCIM/TC57CIM/IEC61970/Base/Domain#ReactivePower> ;
                         rdfs:comment "Minimum reactive power limit for the unit." .


###  https://w3id.org/netbeheer/IECCIM/TC57CIM/IEC61970/Base/Wires#SynchronousMachine_minU
:SynchronousMachine_minU rdf:type owl:ObjectProperty ;
                         rdfs:domain :SynchronousMachine ;
                         rdfs:range <https://w3id.org/netbeheer/IECCIM/TC57CIM/IEC61970/Base/Domain#Voltage> ;
                         rdfs:comment "Minimum voltage  limit for the unit." .


###  https://w3id.org/netbeheer/IECCIM/TC57CIM/IEC61970/Base/Wires#SynchronousMachine_qPercent
:SynchronousMachine_qPercent rdf:type owl:ObjectProperty ;
                             rdfs:domain :SynchronousMachine ;
                             rdfs:range <https://w3id.org/netbeheer/IECCIM/TC57CIM/IEC61970/Base/Domain#PerCent> ;
                             rdfs:comment "Percent of the coordinated reactive control that comes from this machine." .


###  https://w3id.org/netbeheer/IECCIM/TC57CIM/IEC61970/Base/Wires#SynchronousMachine_r
:SynchronousMachine_r rdf:type owl:ObjectProperty ;
                      rdfs:domain :SynchronousMachine ;
                      rdfs:range <https://w3id.org/netbeheer/IECCIM/TC57CIM/IEC61970/Base/Domain#Resistance> ;
                      rdfs:comment "Equivalent resistance (RG) of generator. RG is considered for the calculation of all currents, except for the calculation of the peak current ip. Used for short circuit data exchange according to IEC 60909" .


###  https://w3id.org/netbeheer/IECCIM/TC57CIM/IEC61970/Base/Wires#SynchronousMachine_r0
:SynchronousMachine_r0 rdf:type owl:ObjectProperty ;
                       rdfs:domain :SynchronousMachine ;
                       rdfs:range <https://w3id.org/netbeheer/IECCIM/TC57CIM/IEC61970/Base/Domain#Resistance> ;
                       rdfs:comment "Zero sequence resistance of the synchronous machine." .


###  https://w3id.org/netbeheer/IECCIM/TC57CIM/IEC61970/Base/Wires#SynchronousMachine_r2
:SynchronousMachine_r2 rdf:type owl:ObjectProperty ;
                       rdfs:domain :SynchronousMachine ;
                       rdfs:range <https://w3id.org/netbeheer/IECCIM/TC57CIM/IEC61970/Base/Domain#Resistance> ;
                       rdfs:comment "Negative sequence resistance." .


###  https://w3id.org/netbeheer/IECCIM/TC57CIM/IEC61970/Base/Wires#SynchronousMachine_satDirectSubtransX
:SynchronousMachine_satDirectSubtransX rdf:type owl:ObjectProperty ;
                                       rdfs:domain :SynchronousMachine ;
                                       rdfs:range <https://w3id.org/netbeheer/IECCIM/TC57CIM/IEC61970/Base/Domain#PU> ;
                                       rdfs:comment "Direct-axis subtransient reactance saturated, also known as Xd\"sat." .


###  https://w3id.org/netbeheer/IECCIM/TC57CIM/IEC61970/Base/Wires#SynchronousMachine_satDirectSyncX
:SynchronousMachine_satDirectSyncX rdf:type owl:ObjectProperty ;
                                   rdfs:domain :SynchronousMachine ;
                                   rdfs:range <https://w3id.org/netbeheer/IECCIM/TC57CIM/IEC61970/Base/Domain#PU> ;
                                   rdfs:comment "Direct-axes saturated synchronous reactance (xdsat); reciprocal of short-circuit ration. Used for short circuit data exchange, only for single fed short circuit on a generator. (Section 4.3.4.2. in the IEC 60909-0)." .


###  https://w3id.org/netbeheer/IECCIM/TC57CIM/IEC61970/Base/Wires#SynchronousMachine_satDirectTransX
:SynchronousMachine_satDirectTransX rdf:type owl:ObjectProperty ;
                                    rdfs:domain :SynchronousMachine ;
                                    rdfs:range <https://w3id.org/netbeheer/IECCIM/TC57CIM/IEC61970/Base/Domain#PU> ;
                                    rdfs:comment "Saturated Direct-axis transient reactance. The attribute is primarily used for short circuit calculations according to ANSI." .


###  https://w3id.org/netbeheer/IECCIM/TC57CIM/IEC61970/Base/Wires#SynchronousMachine_voltageRegulationRange
:SynchronousMachine_voltageRegulationRange rdf:type owl:ObjectProperty ;
                                           rdfs:domain :SynchronousMachine ;
                                           rdfs:range <https://w3id.org/netbeheer/IECCIM/TC57CIM/IEC61970/Base/Domain#PerCent> ;
                                           rdfs:comment """Range of generator voltage regulation (PG in the IEC 60909-0) used for calculation of the impedance correction factor KG defined in IEC 60909-0
This attribute is used to describe the operating voltage of the generating unit.""" .


###  https://w3id.org/netbeheer/IECCIM/TC57CIM/IEC61970/Base/Wires#SynchronousMachine_x0
:SynchronousMachine_x0 rdf:type owl:ObjectProperty ;
                       rdfs:domain :SynchronousMachine ;
                       rdfs:range <https://w3id.org/netbeheer/IECCIM/TC57CIM/IEC61970/Base/Domain#Reactance> ;
                       rdfs:comment "Zero sequence reactance of the synchronous machine." .


###  https://w3id.org/netbeheer/IECCIM/TC57CIM/IEC61970/Base/Wires#SynchronousMachine_x2
:SynchronousMachine_x2 rdf:type owl:ObjectProperty ;
                       rdfs:domain :SynchronousMachine ;
                       rdfs:range <https://w3id.org/netbeheer/IECCIM/TC57CIM/IEC61970/Base/Domain#Reactance> ;
                       rdfs:comment "Negative sequence reactance." .


###  https://w3id.org/netbeheer/IECCIM/TC57CIM/IEC61970/Base/Wires#TapChangerControl_TapChanger
:TapChangerControl_TapChanger rdf:type owl:ObjectProperty ;
                              owl:inverseOf :TapChanger_TapChangerControl ;
                              rdfs:domain :TapChangerControl ;
                              rdfs:range :TapChanger ;
                              rdfs:comment "The tap changers that participates in this regulating tap control scheme.The regulating control scheme in which this tap changer participates." .


###  https://w3id.org/netbeheer/IECCIM/TC57CIM/IEC61970/Base/Wires#TapChangerControl_limitVoltage
:TapChangerControl_limitVoltage rdf:type owl:ObjectProperty ;
                                rdfs:domain :TapChangerControl ;
                                rdfs:range <https://w3id.org/netbeheer/IECCIM/TC57CIM/IEC61970/Base/Domain#Voltage> ;
                                rdfs:comment """Maximum allowed regulated voltage on the PT secondary, regardless of line drop compensation. Sometimes referred to as first-house protection.
""" .


###  https://w3id.org/netbeheer/IECCIM/TC57CIM/IEC61970/Base/Wires#TapChangerControl_lineDropR
:TapChangerControl_lineDropR rdf:type owl:ObjectProperty ;
                             rdfs:domain :TapChangerControl ;
                             rdfs:range <https://w3id.org/netbeheer/IECCIM/TC57CIM/IEC61970/Base/Domain#Resistance> ;
                             rdfs:comment "Line drop compensator resistance setting for normal (forward) power flow." .


###  https://w3id.org/netbeheer/IECCIM/TC57CIM/IEC61970/Base/Wires#TapChangerControl_lineDropX
:TapChangerControl_lineDropX rdf:type owl:ObjectProperty ;
                             rdfs:domain :TapChangerControl ;
                             rdfs:range <https://w3id.org/netbeheer/IECCIM/TC57CIM/IEC61970/Base/Domain#Reactance> ;
                             rdfs:comment "Line drop compensator reactance setting for normal (forward) power flow." .


###  https://w3id.org/netbeheer/IECCIM/TC57CIM/IEC61970/Base/Wires#TapChangerControl_reverseLineDropR
:TapChangerControl_reverseLineDropR rdf:type owl:ObjectProperty ;
                                    rdfs:domain :TapChangerControl ;
                                    rdfs:range <https://w3id.org/netbeheer/IECCIM/TC57CIM/IEC61970/Base/Domain#Resistance> ;
                                    rdfs:comment "Line drop compensator resistance setting for reverse power flow." .


###  https://w3id.org/netbeheer/IECCIM/TC57CIM/IEC61970/Base/Wires#TapChangerControl_reverseLineDropX
:TapChangerControl_reverseLineDropX rdf:type owl:ObjectProperty ;
                                    rdfs:domain :TapChangerControl ;
                                    rdfs:range <https://w3id.org/netbeheer/IECCIM/TC57CIM/IEC61970/Base/Domain#Reactance> ;
                                    rdfs:comment "Line drop compensator reactance setting for reverse power flow." .


###  https://w3id.org/netbeheer/IECCIM/TC57CIM/IEC61970/Base/Wires#TapChangerTablePoint_b
:TapChangerTablePoint_b rdf:type owl:ObjectProperty ;
                        rdfs:domain :TapChangerTablePoint ;
                        rdfs:range <https://w3id.org/netbeheer/IECCIM/TC57CIM/IEC61970/Base/Domain#PerCent> ;
                        rdfs:comment """The magnetizing branch susceptance deviation in percent of nominal value. The actual susceptance is calculated as follows:
calculated magnetizing susceptance = b(nominal) * (1 + b(from this class)/100).   The b(nominal) is defined as the static magnetizing susceptance on the associated power transformer end or ends.  This model assumes the star impedance (pi model) form.
""" .


###  https://w3id.org/netbeheer/IECCIM/TC57CIM/IEC61970/Base/Wires#TapChangerTablePoint_g
:TapChangerTablePoint_g rdf:type owl:ObjectProperty ;
                        rdfs:domain :TapChangerTablePoint ;
                        rdfs:range <https://w3id.org/netbeheer/IECCIM/TC57CIM/IEC61970/Base/Domain#PerCent> ;
                        rdfs:comment """The magnetizing branch conductance deviation in percent of nominal value. The actual conductance is calculated as follows:
calculated magnetizing conductance = g(nominal) * (1 + g(from this class)/100).   The g(nominal) is defined as the static magnetizing conductance on the associated power transformer end or ends.  This model assumes the star impedance (pi model) form.
""" .


###  https://w3id.org/netbeheer/IECCIM/TC57CIM/IEC61970/Base/Wires#TapChangerTablePoint_r
:TapChangerTablePoint_r rdf:type owl:ObjectProperty ;
                        rdfs:domain :TapChangerTablePoint ;
                        rdfs:range <https://w3id.org/netbeheer/IECCIM/TC57CIM/IEC61970/Base/Domain#PerCent> ;
                        rdfs:comment """The resistance deviation in percent of nominal value. The actual reactance is calculated as follows:
calculated resistance = r(nominal) * (1 + r(from this class)/100).   The r(nominal) is defined as the static resistance on the associated power transformer end or ends.  This model assumes the star impedance (pi model) form.
""" .


###  https://w3id.org/netbeheer/IECCIM/TC57CIM/IEC61970/Base/Wires#TapChangerTablePoint_x
:TapChangerTablePoint_x rdf:type owl:ObjectProperty ;
                        rdfs:domain :TapChangerTablePoint ;
                        rdfs:range <https://w3id.org/netbeheer/IECCIM/TC57CIM/IEC61970/Base/Domain#PerCent> ;
                        rdfs:comment """The series reactance deviation in percent of nominal value. The actual reactance is calculated as follows:
calculated reactance = x(nominal) * (1 + x(from this class)/100).   The x(nominal) is defined as the static series reactance on the associated power transformer end or ends.  This model assumes the star impedance (pi model) form.
""" .


###  https://w3id.org/netbeheer/IECCIM/TC57CIM/IEC61970/Base/Wires#TapChanger_SvTapStep
:TapChanger_SvTapStep rdf:type owl:ObjectProperty ;
                      owl:inverseOf :SvTapStep_TapChanger ;
                      rdf:type owl:FunctionalProperty ;
                      rdfs:domain :TapChanger ;
                      rdfs:range <https://w3id.org/netbeheer/IECCIM/TC57CIM/IEC61970/Base/StateVariables#SvTapStep> ;
                      rdfs:comment "The tap step state associated with the tap changer.The tap changer associated with the tap step state." .


###  https://w3id.org/netbeheer/IECCIM/TC57CIM/IEC61970/Base/Wires#TapChanger_TapChangerControl
:TapChanger_TapChangerControl rdf:type owl:ObjectProperty ;
                              rdfs:domain :TapChanger ;
                              rdfs:range :TapChangerControl ;
                              rdfs:comment "The tap changers that participates in this regulating tap control scheme.The regulating control scheme in which this tap changer participates." .


###  https://w3id.org/netbeheer/IECCIM/TC57CIM/IEC61970/Base/Wires#TapChanger_TapSchedules
:TapChanger_TapSchedules rdf:type owl:ObjectProperty ;
                         owl:inverseOf :TapSchedule_TapChanger ;
                         rdf:type owl:FunctionalProperty ;
                         rdfs:domain :TapChanger ;
                         rdfs:range :TapSchedule ;
                         rdfs:comment "A TapChanger can have TapSchedules.A TapSchedule is associated with a TapChanger." .


###  https://w3id.org/netbeheer/IECCIM/TC57CIM/IEC61970/Base/Wires#TapChanger_initialDelay
:TapChanger_initialDelay rdf:type owl:ObjectProperty ;
                         rdfs:domain :TapChanger ;
                         rdfs:range <https://w3id.org/netbeheer/IECCIM/TC57CIM/IEC61970/Base/Domain#Seconds> ;
                         rdfs:comment "For an LTC, the delay for initial tap changer operation (first step change)" .


###  https://w3id.org/netbeheer/IECCIM/TC57CIM/IEC61970/Base/Wires#TapChanger_neutralU
:TapChanger_neutralU rdf:type owl:ObjectProperty ;
                     rdfs:domain :TapChanger ;
                     rdfs:range <https://w3id.org/netbeheer/IECCIM/TC57CIM/IEC61970/Base/Domain#Voltage> ;
                     rdfs:comment "Voltage at which the winding operates at the neutral tap setting." .


###  https://w3id.org/netbeheer/IECCIM/TC57CIM/IEC61970/Base/Wires#TapChanger_subsequentDelay
:TapChanger_subsequentDelay rdf:type owl:ObjectProperty ;
                            rdfs:domain :TapChanger ;
                            rdfs:range <https://w3id.org/netbeheer/IECCIM/TC57CIM/IEC61970/Base/Domain#Seconds> ;
                            rdfs:comment "For an LTC, the delay for subsequent tap changer operation (second and later step changes)" .


###  https://w3id.org/netbeheer/IECCIM/TC57CIM/IEC61970/Base/Wires#TapSchedule_TapChanger
:TapSchedule_TapChanger rdf:type owl:ObjectProperty ;
                        rdfs:domain :TapSchedule ;
                        rdfs:range :TapChanger ;
                        rdfs:comment "A TapChanger can have TapSchedules.A TapSchedule is associated with a TapChanger." .


###  https://w3id.org/netbeheer/IECCIM/TC57CIM/IEC61970/Base/Wires#TransformerCoreAdmittance_TransformerEnd
:TransformerCoreAdmittance_TransformerEnd rdf:type owl:ObjectProperty ;
                                          rdfs:domain :TransformerCoreAdmittance ;
                                          rdfs:range :TransformerEnd ;
                                          rdfs:comment "Core admittance of this transformer end, representing magnetising current and core losses. The full values of the transformer should be supplied for one transformer end only.All transformer ends having this core admittance." .


###  https://w3id.org/netbeheer/IECCIM/TC57CIM/IEC61970/Base/Wires#TransformerCoreAdmittance_TransformerEndInfo
:TransformerCoreAdmittance_TransformerEndInfo rdf:type owl:ObjectProperty ;
                                              owl:inverseOf :TransformerEndInfo_CoreAdmittance ;
                                              rdfs:domain :TransformerCoreAdmittance ;
                                              rdfs:range <https://w3id.org/netbeheer/IECCIM/TC57CIM/IEC61968/AssetInfo#TransformerEndInfo> ;
                                              rdfs:comment "Transformer end datasheet used to calculate this core admittance.Core admittance calculated from this transformer end datasheet, representing magnetising current and core losses. The full values of the transformer should be supplied for one transformer end info only." .


###  https://w3id.org/netbeheer/IECCIM/TC57CIM/IEC61970/Base/Wires#TransformerCoreAdmittance_b
:TransformerCoreAdmittance_b rdf:type owl:ObjectProperty ;
                             rdfs:domain :TransformerCoreAdmittance ;
                             rdfs:range <https://w3id.org/netbeheer/IECCIM/TC57CIM/IEC61970/Base/Domain#Susceptance> ;
                             rdfs:comment """Magnetizing branch susceptance (B mag).  The value can be positive or negative.
""" .


###  https://w3id.org/netbeheer/IECCIM/TC57CIM/IEC61970/Base/Wires#TransformerCoreAdmittance_b0
:TransformerCoreAdmittance_b0 rdf:type owl:ObjectProperty ;
                              rdfs:domain :TransformerCoreAdmittance ;
                              rdfs:range <https://w3id.org/netbeheer/IECCIM/TC57CIM/IEC61970/Base/Domain#Susceptance> ;
                              rdfs:comment """Zero sequence magnetizing branch susceptance.
""" .


###  https://w3id.org/netbeheer/IECCIM/TC57CIM/IEC61970/Base/Wires#TransformerCoreAdmittance_g
:TransformerCoreAdmittance_g rdf:type owl:ObjectProperty ;
                             rdfs:domain :TransformerCoreAdmittance ;
                             rdfs:range <https://w3id.org/netbeheer/IECCIM/TC57CIM/IEC61970/Base/Domain#Conductance> ;
                             rdfs:comment """Magnetizing branch conductance (G mag).
""" .


###  https://w3id.org/netbeheer/IECCIM/TC57CIM/IEC61970/Base/Wires#TransformerCoreAdmittance_g0
:TransformerCoreAdmittance_g0 rdf:type owl:ObjectProperty ;
                              rdfs:domain :TransformerCoreAdmittance ;
                              rdfs:range <https://w3id.org/netbeheer/IECCIM/TC57CIM/IEC61970/Base/Domain#Conductance> ;
                              rdfs:comment """Zero sequence magnetizing branch conductance.
""" .


###  https://w3id.org/netbeheer/IECCIM/TC57CIM/IEC61970/Base/Wires#TransformerEndInfo_CoreAdmittance
:TransformerEndInfo_CoreAdmittance rdf:type owl:ObjectProperty ;
                                   rdfs:domain <https://w3id.org/netbeheer/IECCIM/TC57CIM/IEC61968/AssetInfo#TransformerEndInfo> ;
                                   rdfs:range :TransformerCoreAdmittance ;
                                   rdfs:comment "Transformer end datasheet used to calculate this core admittance.Core admittance calculated from this transformer end datasheet, representing magnetising current and core losses. The full values of the transformer should be supplied for one transformer end info only." .


###  https://w3id.org/netbeheer/IECCIM/TC57CIM/IEC61970/Base/Wires#TransformerEndInfo_FromMeshImpedances
:TransformerEndInfo_FromMeshImpedances rdf:type owl:ObjectProperty ;
                                       rdfs:domain <https://w3id.org/netbeheer/IECCIM/TC57CIM/IEC61968/AssetInfo#TransformerEndInfo> ;
                                       rdfs:range :TransformerMeshImpedance ;
                                       rdfs:comment "'from' transformer end datasheet this mesh impedance is calculated from. It determines the voltage reference.All mesh impedances between this 'to' and other 'from' transformer ends." .


###  https://w3id.org/netbeheer/IECCIM/TC57CIM/IEC61970/Base/Wires#TransformerEndInfo_ToMeshImpedances
:TransformerEndInfo_ToMeshImpedances rdf:type owl:ObjectProperty ;
                                     rdfs:domain <https://w3id.org/netbeheer/IECCIM/TC57CIM/IEC61968/AssetInfo#TransformerEndInfo> ;
                                     rdfs:range :TransformerMeshImpedance ;
                                     rdfs:comment "All 'to' transformer end datasheets this mesh impedance for 'from' transformer end is calculated from.All mesh impedances between this 'from' and other 'to' transformer ends." .


###  https://w3id.org/netbeheer/IECCIM/TC57CIM/IEC61970/Base/Wires#TransformerEndInfo_TransformerStarImpedance
:TransformerEndInfo_TransformerStarImpedance rdf:type owl:ObjectProperty ;
                                             rdfs:domain <https://w3id.org/netbeheer/IECCIM/TC57CIM/IEC61968/AssetInfo#TransformerEndInfo> ;
                                             rdfs:range :TransformerStarImpedance ;
                                             rdfs:comment "Transformer end datasheet used to calculate this transformer star impedance.Transformer star impedance calculated from this transformer end datasheet." .


###  https://w3id.org/netbeheer/IECCIM/TC57CIM/IEC61970/Base/Wires#TransformerEnd_CoreAdmittance
:TransformerEnd_CoreAdmittance rdf:type owl:ObjectProperty ;
                               owl:inverseOf :TransformerCoreAdmittance_TransformerEnd ;
                               rdfs:domain :TransformerEnd ;
                               rdfs:range :TransformerCoreAdmittance ;
                               rdfs:comment "Core admittance of this transformer end, representing magnetising current and core losses. The full values of the transformer should be supplied for one transformer end only.All transformer ends having this core admittance." .


###  https://w3id.org/netbeheer/IECCIM/TC57CIM/IEC61970/Base/Wires#TransformerEnd_FromMeshImpedance
:TransformerEnd_FromMeshImpedance rdf:type owl:ObjectProperty ;
                                  owl:inverseOf :TransformerMeshImpedance_FromTransformerEnd ;
                                  rdf:type owl:FunctionalProperty ;
                                  rdfs:domain :TransformerEnd ;
                                  rdfs:range :TransformerMeshImpedance ;
                                  rdfs:comment "All mesh impedances between this 'to' and other 'from' transformer ends.From end this mesh impedance is connected to. It determines the voltage reference." .


###  https://w3id.org/netbeheer/IECCIM/TC57CIM/IEC61970/Base/Wires#TransformerEnd_FromWindingInsulations
:TransformerEnd_FromWindingInsulations rdf:type owl:ObjectProperty ;
                                       owl:inverseOf :WindingInsulation_FromWinding ;
                                       rdf:type owl:FunctionalProperty ;
                                       rdfs:domain :TransformerEnd ;
                                       rdfs:range <https://w3id.org/netbeheer/IECCIM/TC57CIM/IEC61968/InfIEC61968/InfAssets#WindingInsulation> ;
                                       rdfs:comment "" .


###  https://w3id.org/netbeheer/IECCIM/TC57CIM/IEC61970/Base/Wires#TransformerEnd_PhaseTapChanger
:TransformerEnd_PhaseTapChanger rdf:type owl:ObjectProperty ,
                                         owl:FunctionalProperty ;
                                rdfs:domain :TransformerEnd ;
                                rdfs:range :PhaseTapChanger ;
                                rdfs:comment "Transformer end to which this phase tap changer belongs.Phase tap changer associated with this transformer end." .


###  https://w3id.org/netbeheer/IECCIM/TC57CIM/IEC61970/Base/Wires#TransformerEnd_RatioTapChanger
:TransformerEnd_RatioTapChanger rdf:type owl:ObjectProperty ,
                                         owl:FunctionalProperty ;
                                rdfs:domain :TransformerEnd ;
                                rdfs:range :RatioTapChanger ;
                                rdfs:comment "Transformer end to which this ratio tap changer belongs.Ratio tap changer associated with this transformer end." .


###  https://w3id.org/netbeheer/IECCIM/TC57CIM/IEC61970/Base/Wires#TransformerEnd_StarImpedance
:TransformerEnd_StarImpedance rdf:type owl:ObjectProperty ;
                              rdfs:domain :TransformerEnd ;
                              rdfs:range :TransformerStarImpedance ;
                              rdfs:comment "All transformer ends having this star impedance.(accurate for 2- or 3-winding transformers only) Pi-model impedances of this transformer end. By convention, for a two winding transformer, the full values of the transformer should be entered on the high voltage end (endNumber=1)." .


###  https://w3id.org/netbeheer/IECCIM/TC57CIM/IEC61970/Base/Wires#TransformerEnd_ToMeshImpedance
:TransformerEnd_ToMeshImpedance rdf:type owl:ObjectProperty ;
                                owl:inverseOf :TransformerMeshImpedance_ToTransformerEnd ;
                                rdfs:domain :TransformerEnd ;
                                rdfs:range :TransformerMeshImpedance ;
                                rdfs:comment "All mesh impedances between this 'from' and other 'to' transformer ends.All transformer ends this mesh impedance is connected to." .


###  https://w3id.org/netbeheer/IECCIM/TC57CIM/IEC61970/Base/Wires#TransformerEnd_ToWindingInsulations
:TransformerEnd_ToWindingInsulations rdf:type owl:ObjectProperty ;
                                     owl:inverseOf :WindingInsulation_ToWinding ;
                                     rdf:type owl:FunctionalProperty ;
                                     rdfs:domain :TransformerEnd ;
                                     rdfs:range <https://w3id.org/netbeheer/IECCIM/TC57CIM/IEC61968/InfIEC61968/InfAssets#WindingInsulation> ;
                                     rdfs:comment "" .


###  https://w3id.org/netbeheer/IECCIM/TC57CIM/IEC61970/Base/Wires#TransformerEnd_bmagSat
:TransformerEnd_bmagSat rdf:type owl:ObjectProperty ;
                        rdfs:domain :TransformerEnd ;
                        rdfs:range <https://w3id.org/netbeheer/IECCIM/TC57CIM/IEC61970/Base/Domain#PerCent> ;
                        rdfs:comment """Core shunt magnetizing susceptance in the saturation region.
""" .


###  https://w3id.org/netbeheer/IECCIM/TC57CIM/IEC61970/Base/Wires#TransformerEnd_magBaseU
:TransformerEnd_magBaseU rdf:type owl:ObjectProperty ;
                         rdfs:domain :TransformerEnd ;
                         rdfs:range <https://w3id.org/netbeheer/IECCIM/TC57CIM/IEC61970/Base/Domain#Voltage> ;
                         rdfs:comment """The reference voltage at which the magnetizing saturation measurements were made
""" .


###  https://w3id.org/netbeheer/IECCIM/TC57CIM/IEC61970/Base/Wires#TransformerEnd_magSatFlux
:TransformerEnd_magSatFlux rdf:type owl:ObjectProperty ;
                           rdfs:domain :TransformerEnd ;
                           rdfs:range <https://w3id.org/netbeheer/IECCIM/TC57CIM/IEC61970/Base/Domain#PerCent> ;
                           rdfs:comment """Core magnetizing saturation curve knee flux level.
""" .


###  https://w3id.org/netbeheer/IECCIM/TC57CIM/IEC61970/Base/Wires#TransformerEnd_rground
:TransformerEnd_rground rdf:type owl:ObjectProperty ;
                        rdfs:domain :TransformerEnd ;
                        rdfs:range <https://w3id.org/netbeheer/IECCIM/TC57CIM/IEC61970/Base/Domain#Resistance> ;
                        rdfs:comment "(for Yn and Zn connections) Resistance part of neutral impedance where 'grounded' is true." .


###  https://w3id.org/netbeheer/IECCIM/TC57CIM/IEC61970/Base/Wires#TransformerEnd_xground
:TransformerEnd_xground rdf:type owl:ObjectProperty ;
                        rdfs:domain :TransformerEnd ;
                        rdfs:range <https://w3id.org/netbeheer/IECCIM/TC57CIM/IEC61970/Base/Domain#Reactance> ;
                        rdfs:comment "(for Yn and Zn connections) Reactive part of neutral impedance where 'grounded' is true." .


###  https://w3id.org/netbeheer/IECCIM/TC57CIM/IEC61970/Base/Wires#TransformerMeshImpedance_FromTransformerEnd
:TransformerMeshImpedance_FromTransformerEnd rdf:type owl:ObjectProperty ;
                                             rdfs:domain :TransformerMeshImpedance ;
                                             rdfs:range :TransformerEnd ;
                                             rdfs:comment "All mesh impedances between this 'to' and other 'from' transformer ends.From end this mesh impedance is connected to. It determines the voltage reference." .


###  https://w3id.org/netbeheer/IECCIM/TC57CIM/IEC61970/Base/Wires#TransformerMeshImpedance_FromTransformerEndInfo
:TransformerMeshImpedance_FromTransformerEndInfo rdf:type owl:ObjectProperty ;
                                                 owl:inverseOf :TransformerEndInfo_FromMeshImpedances ;
                                                 rdfs:domain :TransformerMeshImpedance ;
                                                 rdfs:range <https://w3id.org/netbeheer/IECCIM/TC57CIM/IEC61968/AssetInfo#TransformerEndInfo> ;
                                                 rdfs:comment "'from' transformer end datasheet this mesh impedance is calculated from. It determines the voltage reference.All mesh impedances between this 'to' and other 'from' transformer ends." .


###  https://w3id.org/netbeheer/IECCIM/TC57CIM/IEC61970/Base/Wires#TransformerMeshImpedance_ToTransformerEnd
:TransformerMeshImpedance_ToTransformerEnd rdf:type owl:ObjectProperty ;
                                           rdfs:domain :TransformerMeshImpedance ;
                                           rdfs:range :TransformerEnd ;
                                           rdfs:comment "All mesh impedances between this 'from' and other 'to' transformer ends.All transformer ends this mesh impedance is connected to." .


###  https://w3id.org/netbeheer/IECCIM/TC57CIM/IEC61970/Base/Wires#TransformerMeshImpedance_ToTransformerEndInfos
:TransformerMeshImpedance_ToTransformerEndInfos rdf:type owl:ObjectProperty ;
                                                owl:inverseOf :TransformerEndInfo_ToMeshImpedances ;
                                                rdfs:domain :TransformerMeshImpedance ;
                                                rdfs:range <https://w3id.org/netbeheer/IECCIM/TC57CIM/IEC61968/AssetInfo#TransformerEndInfo> ;
                                                rdfs:comment "All 'to' transformer end datasheets this mesh impedance for 'from' transformer end is calculated from.All mesh impedances between this 'from' and other 'to' transformer ends." .


###  https://w3id.org/netbeheer/IECCIM/TC57CIM/IEC61970/Base/Wires#TransformerMeshImpedance_r
:TransformerMeshImpedance_r rdf:type owl:ObjectProperty ;
                            rdfs:domain :TransformerMeshImpedance ;
                            rdfs:range <https://w3id.org/netbeheer/IECCIM/TC57CIM/IEC61970/Base/Domain#Resistance> ;
                            rdfs:comment """Resistance between the 'from' and the 'to' end, seen from the 'from' end.
""" .


###  https://w3id.org/netbeheer/IECCIM/TC57CIM/IEC61970/Base/Wires#TransformerMeshImpedance_r0
:TransformerMeshImpedance_r0 rdf:type owl:ObjectProperty ;
                             rdfs:domain :TransformerMeshImpedance ;
                             rdfs:range <https://w3id.org/netbeheer/IECCIM/TC57CIM/IEC61970/Base/Domain#Resistance> ;
                             rdfs:comment """Zero-sequence resistance between the 'from' and the 'to' end, seen from the 'from' end.
""" .


###  https://w3id.org/netbeheer/IECCIM/TC57CIM/IEC61970/Base/Wires#TransformerMeshImpedance_x
:TransformerMeshImpedance_x rdf:type owl:ObjectProperty ;
                            rdfs:domain :TransformerMeshImpedance ;
                            rdfs:range <https://w3id.org/netbeheer/IECCIM/TC57CIM/IEC61970/Base/Domain#Reactance> ;
                            rdfs:comment """Reactance between the 'from' and the 'to' end, seen from the 'from' end.
""" .


###  https://w3id.org/netbeheer/IECCIM/TC57CIM/IEC61970/Base/Wires#TransformerMeshImpedance_x0
:TransformerMeshImpedance_x0 rdf:type owl:ObjectProperty ;
                             rdfs:domain :TransformerMeshImpedance ;
                             rdfs:range <https://w3id.org/netbeheer/IECCIM/TC57CIM/IEC61970/Base/Domain#Reactance> ;
                             rdfs:comment """Zero-sequence reactance between the 'from' and the 'to' end, seen from the 'from' end.
""" .


###  https://w3id.org/netbeheer/IECCIM/TC57CIM/IEC61970/Base/Wires#TransformerObservation_Transformer
:TransformerObservation_Transformer rdf:type owl:ObjectProperty ;
                                    rdfs:domain <https://w3id.org/netbeheer/IECCIM/TC57CIM/IEC61968/InfIEC61968/InfAssets#TransformerObservation> ;
                                    rdfs:range :TransformerTank ;
                                    rdfs:comment "" .


###  https://w3id.org/netbeheer/IECCIM/TC57CIM/IEC61970/Base/Wires#TransformerStarImpedance_TransformerEnd
:TransformerStarImpedance_TransformerEnd rdf:type owl:ObjectProperty ;
                                         owl:inverseOf :TransformerEnd_StarImpedance ;
                                         rdfs:domain :TransformerStarImpedance ;
                                         rdfs:range :TransformerEnd ;
                                         rdfs:comment "All transformer ends having this star impedance.(accurate for 2- or 3-winding transformers only) Pi-model impedances of this transformer end. By convention, for a two winding transformer, the full values of the transformer should be entered on the high voltage end (endNumber=1)." .


###  https://w3id.org/netbeheer/IECCIM/TC57CIM/IEC61970/Base/Wires#TransformerStarImpedance_TransformerEndInfo
:TransformerStarImpedance_TransformerEndInfo rdf:type owl:ObjectProperty ;
                                             owl:inverseOf :TransformerEndInfo_TransformerStarImpedance ;
                                             rdfs:domain :TransformerStarImpedance ;
                                             rdfs:range <https://w3id.org/netbeheer/IECCIM/TC57CIM/IEC61968/AssetInfo#TransformerEndInfo> ;
                                             rdfs:comment "Transformer end datasheet used to calculate this transformer star impedance.Transformer star impedance calculated from this transformer end datasheet." .


###  https://w3id.org/netbeheer/IECCIM/TC57CIM/IEC61970/Base/Wires#TransformerStarImpedance_r
:TransformerStarImpedance_r rdf:type owl:ObjectProperty ;
                            rdfs:domain :TransformerStarImpedance ;
                            rdfs:range <https://w3id.org/netbeheer/IECCIM/TC57CIM/IEC61970/Base/Domain#Resistance> ;
                            rdfs:comment """Resistance of the transformer end.
""" .


###  https://w3id.org/netbeheer/IECCIM/TC57CIM/IEC61970/Base/Wires#TransformerStarImpedance_r0
:TransformerStarImpedance_r0 rdf:type owl:ObjectProperty ;
                             rdfs:domain :TransformerStarImpedance ;
                             rdfs:range <https://w3id.org/netbeheer/IECCIM/TC57CIM/IEC61970/Base/Domain#Resistance> ;
                             rdfs:comment """Zero sequence series resistance of the transformer end.
""" .


###  https://w3id.org/netbeheer/IECCIM/TC57CIM/IEC61970/Base/Wires#TransformerStarImpedance_x
:TransformerStarImpedance_x rdf:type owl:ObjectProperty ;
                            rdfs:domain :TransformerStarImpedance ;
                            rdfs:range <https://w3id.org/netbeheer/IECCIM/TC57CIM/IEC61970/Base/Domain#Reactance> ;
                            rdfs:comment """Positive sequence series reactance of the transformer end.
""" .


###  https://w3id.org/netbeheer/IECCIM/TC57CIM/IEC61970/Base/Wires#TransformerStarImpedance_x0
:TransformerStarImpedance_x0 rdf:type owl:ObjectProperty ;
                             rdfs:domain :TransformerStarImpedance ;
                             rdfs:range <https://w3id.org/netbeheer/IECCIM/TC57CIM/IEC61970/Base/Domain#Reactance> ;
                             rdfs:comment """Zero sequence series reactance of the transformer end.
""" .


###  https://w3id.org/netbeheer/IECCIM/TC57CIM/IEC61970/Base/Wires#TransformerTankEnd_TransformerTank
:TransformerTankEnd_TransformerTank rdf:type owl:ObjectProperty ;
                                    rdfs:domain :TransformerTankEnd ;
                                    rdfs:range :TransformerTank ;
                                    rdfs:comment "All windings of this transformer.Transformer this winding belongs to." .


###  https://w3id.org/netbeheer/IECCIM/TC57CIM/IEC61970/Base/Wires#TransformerTank_PowerTransformer
:TransformerTank_PowerTransformer rdf:type owl:ObjectProperty ;
                                  rdfs:domain :TransformerTank ;
                                  rdfs:range :PowerTransformer ;
                                  rdfs:comment "All transformers that belong to this bank.Bank this transformer belongs to." .


###  https://w3id.org/netbeheer/IECCIM/TC57CIM/IEC61970/Base/Wires#TransformerTank_TransformerObservations
:TransformerTank_TransformerObservations rdf:type owl:ObjectProperty ;
                                         owl:inverseOf :TransformerObservation_Transformer ;
                                         rdfs:domain :TransformerTank ;
                                         rdfs:range <https://w3id.org/netbeheer/IECCIM/TC57CIM/IEC61968/InfIEC61968/InfAssets#TransformerObservation> ;
                                         rdfs:comment "" .


###  https://w3id.org/netbeheer/IECCIM/TC57CIM/IEC61970/Base/Wires#TransformerTank_TransformerTankEnds
:TransformerTank_TransformerTankEnds rdf:type owl:ObjectProperty ;
                                     owl:inverseOf :TransformerTankEnd_TransformerTank ;
                                     rdfs:domain :TransformerTank ;
                                     rdfs:range :TransformerTankEnd ;
                                     rdfs:comment "All windings of this transformer.Transformer this winding belongs to." .


###  https://w3id.org/netbeheer/IECCIM/TC57CIM/IEC61970/Base/Wires#VoltageControlZone_BusbarSection
:VoltageControlZone_BusbarSection rdf:type owl:ObjectProperty ;
                                  owl:inverseOf :BusbarSection_VoltageControlZone ;
                                  rdfs:domain :VoltageControlZone ;
                                  rdfs:range :BusbarSection ;
                                  rdfs:comment "A VoltageControlZone is controlled by a designated BusbarSection.A VoltageControlZone is controlled by a designated BusbarSection." .


###  https://w3id.org/netbeheer/IECCIM/TC57CIM/IEC61970/Base/Wires#VoltageControlZone_RegulationSchedule
:VoltageControlZone_RegulationSchedule rdf:type owl:ObjectProperty ;
                                       owl:inverseOf :RegulationSchedule_VoltageControlZones ;
                                       rdfs:domain :VoltageControlZone ;
                                       rdfs:range :RegulationSchedule ;
                                       rdfs:comment "A VoltageControlZone may have a  voltage regulation schedule.A VoltageControlZone may have a  voltage regulation schedule." .


###  https://w3id.org/netbeheer/IECCIM/TC57CIM/IEC61970/Base/Wires#WindTurbineType3or4Dynamics_EnergySource
:WindTurbineType3or4Dynamics_EnergySource rdf:type owl:ObjectProperty ;
                                          rdfs:domain <https://w3id.org/netbeheer/IECCIM/TC57CIM/IEC61970/Dynamics/StandardModels/WindDynamics#WindTurbineType3or4Dynamics> ;
                                          rdfs:range :EnergySource ;
                                          rdfs:comment "Wind generator Type 3 or 4 dynamics model associated with this energy source.Energy Source (current source) with which this wind Type 3 or 4 dynamics model is asoociated." .


###  https://w3id.org/netbeheer/IECCIM/TC57CIM/IEC61970/Base/Wires#WindingInsulation_FromWinding
:WindingInsulation_FromWinding rdf:type owl:ObjectProperty ;
                               rdfs:domain <https://w3id.org/netbeheer/IECCIM/TC57CIM/IEC61968/InfIEC61968/InfAssets#WindingInsulation> ;
                               rdfs:range :TransformerEnd ;
                               rdfs:comment "" .


###  https://w3id.org/netbeheer/IECCIM/TC57CIM/IEC61970/Base/Wires#WindingInsulation_ToWinding
:WindingInsulation_ToWinding rdf:type owl:ObjectProperty ;
                             rdfs:domain <https://w3id.org/netbeheer/IECCIM/TC57CIM/IEC61968/InfIEC61968/InfAssets#WindingInsulation> ;
                             rdfs:range :TransformerEnd ;
                             rdfs:comment "" .


###  https://w3id.org/netbeheer/IECCIM/TC57CIM/IEC61970/Base/Wires#WireInfo_PerLengthParameters
:WireInfo_PerLengthParameters rdf:type owl:ObjectProperty ;
                              rdfs:domain <https://w3id.org/netbeheer/IECCIM/TC57CIM/IEC61968/AssetInfo#WireInfo> ;
                              rdfs:range :PerLengthLineParameter ;
                              rdfs:comment "All wire datasheets used to calculate this per-length parameter.All per-length parameters calculated from this wire datasheet." .


###  https://w3id.org/netbeheer/IECCIM/TC57CIM/IEC61970/Base/Wires#WireSpacing_ACLineSegments
:WireSpacing_ACLineSegments rdf:type owl:ObjectProperty ;
                            rdfs:domain <https://w3id.org/netbeheer/IECCIM/TC57CIM/IEC61968/AssetInfo#WireSpacing> ;
                            rdfs:range :ACLineSegment ;
                            rdfs:comment "Wire spacing configuration for this line segment.All line segments described with this wire spacing configuration." .


###  https://w3id.org/netbeheer/IECCIM/TC57CIM/IEC61970/Base/Wires#WireSpacing_PerLengthParameters
:WireSpacing_PerLengthParameters rdf:type owl:ObjectProperty ;
                                 rdfs:domain <https://w3id.org/netbeheer/IECCIM/TC57CIM/IEC61968/AssetInfo#WireSpacing> ;
                                 rdfs:range :PerLengthLineParameter ;
                                 rdfs:comment "Wire spacing datasheet used to calculate this per-length parameter.All per-length parameters calculated from this wire spacing datasheet." .


#################################################################
#    Data properties
#################################################################

###  https://w3id.org/netbeheer/IECCIM/TC57CIM/IEC61970/Base/Wires#ACLineSegmentPhase_phase
:ACLineSegmentPhase_phase rdf:type owl:DatatypeProperty ;
                          rdfs:domain :ACLineSegmentPhase ;
                          rdfs:range :SinglePhaseKind ;
                          rdfs:comment """The phase connection of the wire at both ends.
""" .


###  https://w3id.org/netbeheer/IECCIM/TC57CIM/IEC61970/Base/Wires#ACLineSegmentPhase_sequenceNumber
:ACLineSegmentPhase_sequenceNumber rdf:type owl:DatatypeProperty ;
                                   rdfs:domain :ACLineSegmentPhase ;
                                   rdfs:range xsd:nonNegativeInteger ;
                                   rdfs:comment "Number designation for this line segment phase. Each line segment phase within a line segment should have a unique sequence number. This is useful for unbalanced modeling to bind the mathematical model (PhaseImpedanceData of PerLengthPhaseImpedance) with the connectivity model (this class) and the physical model (WirePosition) without tight coupling." .


###  https://w3id.org/netbeheer/IECCIM/TC57CIM/IEC61970/Base/Wires#AsynchronousMachine_asynchronousMachineType
:AsynchronousMachine_asynchronousMachineType rdf:type owl:DatatypeProperty ;
                                             rdfs:domain :AsynchronousMachine ;
                                             rdfs:range :AsynchronousMachineKind ;
                                             rdfs:comment "Indicates the type of Asynchronous Machine (motor or generator)." .


###  https://w3id.org/netbeheer/IECCIM/TC57CIM/IEC61970/Base/Wires#AsynchronousMachine_converterFedDrive
:AsynchronousMachine_converterFedDrive rdf:type owl:DatatypeProperty ;
                                       rdfs:domain :AsynchronousMachine ;
                                       rdfs:range xsd:boolean ;
                                       rdfs:comment "Indicates whether the machine is a converter fed drive. Used for short circuit data exchange according to IEC 60909" .


###  https://w3id.org/netbeheer/IECCIM/TC57CIM/IEC61970/Base/Wires#AsynchronousMachine_iaIrRatio
:AsynchronousMachine_iaIrRatio rdf:type owl:DatatypeProperty ;
                               rdfs:domain :AsynchronousMachine ;
                               rdfs:range xsd:float ;
                               rdfs:comment "Ratio of locked-rotor current to the rated current of the motor (Ia/Ir). Used for short circuit data exchange according to IEC 60909" .


###  https://w3id.org/netbeheer/IECCIM/TC57CIM/IEC61970/Base/Wires#AsynchronousMachine_polePairNumber
:AsynchronousMachine_polePairNumber rdf:type owl:DatatypeProperty ;
                                    rdfs:domain :AsynchronousMachine ;
                                    rdfs:range xsd:nonNegativeInteger ;
                                    rdfs:comment "Number of pole pairs of stator. Used for short circuit data exchange according to IEC 60909" .


###  https://w3id.org/netbeheer/IECCIM/TC57CIM/IEC61970/Base/Wires#AsynchronousMachine_reversible
:AsynchronousMachine_reversible rdf:type owl:DatatypeProperty ;
                                rdfs:domain :AsynchronousMachine ;
                                rdfs:range xsd:boolean ;
                                rdfs:comment "Indicates for converter drive motors if the power can be reversible. Used for short circuit data exchange according to IEC 60909" .


###  https://w3id.org/netbeheer/IECCIM/TC57CIM/IEC61970/Base/Wires#AsynchronousMachine_rxLockedRotorRatio
:AsynchronousMachine_rxLockedRotorRatio rdf:type owl:DatatypeProperty ;
                                        rdfs:domain :AsynchronousMachine ;
                                        rdfs:range xsd:float ;
                                        rdfs:comment "Locked rotor ratio (R/X). Used for short circuit data exchange according to IEC 60909" .


###  https://w3id.org/netbeheer/IECCIM/TC57CIM/IEC61970/Base/Wires#CompositeSwitch_compositeSwitchType
:CompositeSwitch_compositeSwitchType rdf:type owl:DatatypeProperty ;
                                     rdfs:domain :CompositeSwitch ;
                                     rdfs:range xsd:string ;
                                     rdfs:comment "An alphanumeric code that can be used as a reference to extra information such as the description of the interlocking scheme if any." .


###  https://w3id.org/netbeheer/IECCIM/TC57CIM/IEC61970/Base/Wires#EnergyConsumerPhase_phase
:EnergyConsumerPhase_phase rdf:type owl:DatatypeProperty ;
                           rdfs:domain :EnergyConsumerPhase ;
                           rdfs:range :SinglePhaseKind ;
                           rdfs:comment """Phase of this energy consumer component.   If the energy consumer is wye connected, the connection is from the indicated phase to the central ground or neutral point.  If the energy consumer is delta connected, the phase indicates an energy consumer connected from the indicated phase to the next logical non-neutral phase.
""" .


###  https://w3id.org/netbeheer/IECCIM/TC57CIM/IEC61970/Base/Wires#EnergyConsumer_customerCount
:EnergyConsumer_customerCount rdf:type owl:DatatypeProperty ;
                              rdfs:domain :EnergyConsumer ;
                              rdfs:range xsd:nonNegativeInteger ;
                              rdfs:comment """Number of individual customers represented by this demand.
""" .


###  https://w3id.org/netbeheer/IECCIM/TC57CIM/IEC61970/Base/Wires#EnergyConsumer_grounded
:EnergyConsumer_grounded rdf:type owl:DatatypeProperty ;
                         rdfs:domain :EnergyConsumer ;
                         rdfs:range xsd:boolean ;
                         rdfs:comment "Used for Yn and Zn connections. True if the neutral is solidly grounded." .


###  https://w3id.org/netbeheer/IECCIM/TC57CIM/IEC61970/Base/Wires#EnergyConsumer_phaseConnection
:EnergyConsumer_phaseConnection rdf:type owl:DatatypeProperty ;
                                rdfs:domain :EnergyConsumer ;
                                rdfs:range :PhaseShuntConnectionKind ;
                                rdfs:comment """The type of phase connection, such as wye or delta.
""" .


###  https://w3id.org/netbeheer/IECCIM/TC57CIM/IEC61970/Base/Wires#EnergySourcePhase_phase
:EnergySourcePhase_phase rdf:type owl:DatatypeProperty ;
                         rdfs:domain :EnergySourcePhase ;
                         rdfs:range :SinglePhaseKind ;
                         rdfs:comment "Phase of this energy source component.   If the energy source wye connected, the connection is from the indicated phase to the central ground or neutral point.  If the energy source is delta connected, the phase indicates an energy source connected from the indicated phase to the next logical non-neutral phase." .


###  https://w3id.org/netbeheer/IECCIM/TC57CIM/IEC61970/Base/Wires#ExternalNetworkInjection_ikSecond
:ExternalNetworkInjection_ikSecond rdf:type owl:DatatypeProperty ;
                                   rdfs:domain :ExternalNetworkInjection ;
                                   rdfs:range xsd:boolean ;
                                   rdfs:comment """Indicates whether initial symmetrical short-circuit current and power have been calculated according to IEC (Ik\").
""" .


###  https://w3id.org/netbeheer/IECCIM/TC57CIM/IEC61970/Base/Wires#ExternalNetworkInjection_maxR0ToX0Ratio
:ExternalNetworkInjection_maxR0ToX0Ratio rdf:type owl:DatatypeProperty ;
                                         rdfs:domain :ExternalNetworkInjection ;
                                         rdfs:range xsd:float ;
                                         rdfs:comment """Maximum ratio of zero sequence resistance of Network Feeder to its zero sequence reactance (R(0)/X(0) max). Used for short circuit data exchange according to IEC 60909
""" .


###  https://w3id.org/netbeheer/IECCIM/TC57CIM/IEC61970/Base/Wires#ExternalNetworkInjection_maxR1ToX1Ratio
:ExternalNetworkInjection_maxR1ToX1Ratio rdf:type owl:DatatypeProperty ;
                                         rdfs:domain :ExternalNetworkInjection ;
                                         rdfs:range xsd:float ;
                                         rdfs:comment """Maximum ratio of positive sequence resistance of Network Feeder to its positive sequence reactance (R(1)/X(1) max). Used for short circuit data exchange according to IEC 60909
""" .


###  https://w3id.org/netbeheer/IECCIM/TC57CIM/IEC61970/Base/Wires#ExternalNetworkInjection_maxZ0ToZ1Ratio
:ExternalNetworkInjection_maxZ0ToZ1Ratio rdf:type owl:DatatypeProperty ;
                                         rdfs:domain :ExternalNetworkInjection ;
                                         rdfs:range xsd:float ;
                                         rdfs:comment """Maximum ratio of zero sequence impedance to its positive sequence impedance (Z(0)/Z(1) max). Used for short circuit data exchange according to IEC 60909
""" .


###  https://w3id.org/netbeheer/IECCIM/TC57CIM/IEC61970/Base/Wires#ExternalNetworkInjection_minR0ToX0Ratio
:ExternalNetworkInjection_minR0ToX0Ratio rdf:type owl:DatatypeProperty ;
                                         rdfs:domain :ExternalNetworkInjection ;
                                         rdfs:range xsd:float ;
                                         rdfs:comment """Indicates whether initial symmetrical short-circuit current and power have been calculated according to IEC (Ik\"). Used for short circuit data exchange according to IEC 6090
""" .


###  https://w3id.org/netbeheer/IECCIM/TC57CIM/IEC61970/Base/Wires#ExternalNetworkInjection_minR1ToX1Ratio
:ExternalNetworkInjection_minR1ToX1Ratio rdf:type owl:DatatypeProperty ;
                                         rdfs:domain :ExternalNetworkInjection ;
                                         rdfs:range xsd:float ;
                                         rdfs:comment """Minimum ratio of positive sequence resistance of Network Feeder to its positive sequence reactance (R(1)/X(1) min). Used for short circuit data exchange according to IEC 60909
""" .


###  https://w3id.org/netbeheer/IECCIM/TC57CIM/IEC61970/Base/Wires#ExternalNetworkInjection_minZ0ToZ1Ratio
:ExternalNetworkInjection_minZ0ToZ1Ratio rdf:type owl:DatatypeProperty ;
                                         rdfs:domain :ExternalNetworkInjection ;
                                         rdfs:range xsd:float ;
                                         rdfs:comment """Minimum ratio of zero sequence impedance to its positive sequence impedance (Z(0)/Z(1) min). Used for short circuit data exchange according to IEC 60909
""" .


###  https://w3id.org/netbeheer/IECCIM/TC57CIM/IEC61970/Base/Wires#ExternalNetworkInjection_referencePriority
:ExternalNetworkInjection_referencePriority rdf:type owl:DatatypeProperty ;
                                            rdfs:domain :ExternalNetworkInjection ;
                                            rdfs:range xsd:nonNegativeInteger ;
                                            rdfs:comment """Priority of unit for use as powerflow voltage phase angle reference bus selection. 0 = don t care (default) 1 = highest priority. 2 is less than 1 and so on.
""" .


###  https://w3id.org/netbeheer/IECCIM/TC57CIM/IEC61970/Base/Wires#NonlinearShuntCompensatorPhasePoint_sectionNumber
:NonlinearShuntCompensatorPhasePoint_sectionNumber rdf:type owl:DatatypeProperty ;
                                                   rdfs:domain :NonlinearShuntCompensatorPhasePoint ;
                                                   rdfs:range xsd:nonNegativeInteger ;
                                                   rdfs:comment "The number of the section." .


###  https://w3id.org/netbeheer/IECCIM/TC57CIM/IEC61970/Base/Wires#NonlinearShuntCompensatorPoint_sectionNumber
:NonlinearShuntCompensatorPoint_sectionNumber rdf:type owl:DatatypeProperty ;
                                              rdfs:domain :NonlinearShuntCompensatorPoint ;
                                              rdfs:range xsd:nonNegativeInteger ;
                                              rdfs:comment "The number of the section." .


###  https://w3id.org/netbeheer/IECCIM/TC57CIM/IEC61970/Base/Wires#PerLengthPhaseImpedance_conductorCount
:PerLengthPhaseImpedance_conductorCount rdf:type owl:DatatypeProperty ;
                                        rdfs:domain :PerLengthPhaseImpedance ;
                                        rdfs:range xsd:nonNegativeInteger ;
                                        rdfs:comment "Number of phase, neutral, and other wires retained. Constrains the number of matrix elements and the phase codes that can be used with this matrix." .


###  https://w3id.org/netbeheer/IECCIM/TC57CIM/IEC61970/Base/Wires#PetersenCoil_mode
:PetersenCoil_mode rdf:type owl:DatatypeProperty ;
                   rdfs:domain :PetersenCoil ;
                   rdfs:range :PetersenCoilModeKind ;
                   rdfs:comment "The mode of operation of the Petersen coil." .


###  https://w3id.org/netbeheer/IECCIM/TC57CIM/IEC61970/Base/Wires#PhaseImpedanceData_sequenceNumber
:PhaseImpedanceData_sequenceNumber rdf:type owl:DatatypeProperty ;
                                   rdfs:domain :PhaseImpedanceData ;
                                   rdfs:range xsd:nonNegativeInteger ;
                                   rdfs:comment "Column-wise element index, assuming a symmetrical matrix. Ranges from 1 to N + N*(N-1)/2, where N is the number of phases possibly including neutral.    For instance, with N=4, column 1 = [1 2 3 4 ], column 2 = [- 5 6 7 ], column 3 = [- - 8 9], column 4 = [- - - 10]." .


###  https://w3id.org/netbeheer/IECCIM/TC57CIM/IEC61970/Base/Wires#PowerTransformerEnd_connectionKind
:PowerTransformerEnd_connectionKind rdf:type owl:DatatypeProperty ;
                                    rdfs:domain :PowerTransformerEnd ;
                                    rdfs:range :WindingConnection ;
                                    rdfs:comment """Kind of connection.
""" .


###  https://w3id.org/netbeheer/IECCIM/TC57CIM/IEC61970/Base/Wires#PowerTransformerEnd_phaseAngleClock
:PowerTransformerEnd_phaseAngleClock rdf:type owl:DatatypeProperty ;
                                     rdfs:domain :PowerTransformerEnd ;
                                     rdfs:range xsd:nonNegativeInteger ;
                                     rdfs:comment """Terminal voltage phase angle displacement where 360 degrees are represented with clock hours. The valid values are 0 to 11. For example, for the secondary side end of a transformer with vector group code of 'Dyn11', specify the connection kind as wye with neutral and specify the phase angle of the clock as 11.  The clock value of the transformer end number specified as 1, is assumed to be zero.  Note the transformer end number is not assumed to be the same as the terminal sequence number.
""" .


###  https://w3id.org/netbeheer/IECCIM/TC57CIM/IEC61970/Base/Wires#PowerTransformer_isPartOfGeneratorUnit
:PowerTransformer_isPartOfGeneratorUnit rdf:type owl:DatatypeProperty ;
                                        rdfs:domain :PowerTransformer ;
                                        rdfs:range xsd:boolean ;
                                        rdfs:comment "Indicates whether the machine is part of a power station unit. Used for short circuit data exchange according to IEC 60909" .


###  https://w3id.org/netbeheer/IECCIM/TC57CIM/IEC61970/Base/Wires#PowerTransformer_operationalValuesConsidered
:PowerTransformer_operationalValuesConsidered rdf:type owl:DatatypeProperty ;
                                              rdfs:domain :PowerTransformer ;
                                              rdfs:range xsd:boolean ;
                                              rdfs:comment "It is used to define if the data (other attributes related to short circuit data exchange) defines long term operational conditions or not. Used for short circuit data exchange according to IEC 60909." .


###  https://w3id.org/netbeheer/IECCIM/TC57CIM/IEC61970/Base/Wires#PowerTransformer_vectorGroup
:PowerTransformer_vectorGroup rdf:type owl:DatatypeProperty ;
                              rdfs:domain :PowerTransformer ;
                              rdfs:range xsd:string ;
                              rdfs:comment """Vector group of the transformer for protective relaying, e.g., Dyn1. For unbalanced transformers, this may not be simply determined from the constituent winding connections and phase angle dispacements.

The vectorGroup string consists of the following components in the order listed: high voltage winding connection, mid voltage winding connection (for three winding transformers), phase displacement clock number from 0 to 11,  low voltage winding connection 
phase displacement clock number from 0 to 11.   The winding connections are D (delta), Y (wye), YN (wye with neutral), Z (zigzag), ZN (zigzag with neutral), A (auto transformer). Upper case means the high voltage, lower case mid or low. The high voltage winding always has clock postion 0 and is not included in the vector group string.  Some examples: YNy0 (two winding wye to wye with no phase displacement), YNd11 (two winding wye to delta with 330 degrees phase displacement), YNyn0d5 (three winding transformer wye with neutral high voltgage, wye with neutral mid voltgage and no phase displacement, delta low voltage with 150 degrees displacement).

Phase displacement is defined as the angular difference between the phasors representing the voltages between the neutral point (real or imaginary) and the corresponding terminals of two windings, a positive sequence voltage system being applied to the high-voltage terminals, following each other in alphabetical sequence if they are lettered, or in numerical sequence if they are numbered: the phasors are assumed to rotate in a counter-clockwise sense.
""" .


###  https://w3id.org/netbeheer/IECCIM/TC57CIM/IEC61970/Base/Wires#RatioTapChanger_tculControlMode
:RatioTapChanger_tculControlMode rdf:type owl:DatatypeProperty ;
                                 rdfs:domain :RatioTapChanger ;
                                 rdfs:range :TransformerControlMode ;
                                 rdfs:comment "Specifies the regulation control mode (voltage or reactive) of the RatioTapChanger." .


###  https://w3id.org/netbeheer/IECCIM/TC57CIM/IEC61970/Base/Wires#RegulatingCondEq_controlEnabled
:RegulatingCondEq_controlEnabled rdf:type owl:DatatypeProperty ;
                                 rdfs:domain :RegulatingCondEq ;
                                 rdfs:range xsd:boolean ;
                                 rdfs:comment "Specifies the regulation status of the equipment.  True is regulating, false is not regulating." .


###  https://w3id.org/netbeheer/IECCIM/TC57CIM/IEC61970/Base/Wires#RegulatingControl_discrete
:RegulatingControl_discrete rdf:type owl:DatatypeProperty ;
                            rdfs:domain :RegulatingControl ;
                            rdfs:range xsd:boolean ;
                            rdfs:comment "The regulation is performed in a discrete mode. This applies to equipment with discrete controls, e.g. tap changers and shunt compensators." .


###  https://w3id.org/netbeheer/IECCIM/TC57CIM/IEC61970/Base/Wires#RegulatingControl_enabled
:RegulatingControl_enabled rdf:type owl:DatatypeProperty ;
                           rdfs:domain :RegulatingControl ;
                           rdfs:range xsd:boolean ;
                           rdfs:comment "The flag tells if regulation is enabled." .


###  https://w3id.org/netbeheer/IECCIM/TC57CIM/IEC61970/Base/Wires#RegulatingControl_mode
:RegulatingControl_mode rdf:type owl:DatatypeProperty ;
                        rdfs:domain :RegulatingControl ;
                        rdfs:range :RegulatingControlModeKind ;
                        rdfs:comment "The regulating control mode presently available.  This specification allows for determining the kind of regulation without need for obtaining the units from a schedule." .


###  https://w3id.org/netbeheer/IECCIM/TC57CIM/IEC61970/Base/Wires#RegulatingControl_monitoredPhase
:RegulatingControl_monitoredPhase rdf:type owl:DatatypeProperty ;
                                  rdfs:domain :RegulatingControl ;
                                  rdfs:range <https://w3id.org/netbeheer/IECCIM/TC57CIM/IEC61970/Base/Core#PhaseCode> ;
                                  rdfs:comment "Phase voltage controlling this regulator, measured at regulator location." .


###  https://w3id.org/netbeheer/IECCIM/TC57CIM/IEC61970/Base/Wires#RegulatingControl_targetDeadband
:RegulatingControl_targetDeadband rdf:type owl:DatatypeProperty ;
                                  rdfs:domain :RegulatingControl ;
                                  rdfs:range xsd:float ;
                                  rdfs:comment """This is a deadband used with discrete control to avoid excessive update of controls like tap changers and shunt compensator banks while regulating.
The units of those appropriate for the mode.""" .


###  https://w3id.org/netbeheer/IECCIM/TC57CIM/IEC61970/Base/Wires#RegulatingControl_targetValue
:RegulatingControl_targetValue rdf:type owl:DatatypeProperty ;
                               rdfs:domain :RegulatingControl ;
                               rdfs:range xsd:float ;
                               rdfs:comment "The target value specified for case input.   This value can be used for the target value without the use of schedules. The value has the units appropriate to the mode attribute." .


###  https://w3id.org/netbeheer/IECCIM/TC57CIM/IEC61970/Base/Wires#RegulatingControl_targetValueUnitMultiplier
:RegulatingControl_targetValueUnitMultiplier rdf:type owl:DatatypeProperty ;
                                             rdfs:domain :RegulatingControl ;
                                             rdfs:range <https://w3id.org/netbeheer/IECCIM/TC57CIM/IEC61970/Base/Domain#UnitMultiplier> ;
                                             rdfs:comment "Specify the multiplier for used for the targetValue." .


###  https://w3id.org/netbeheer/IECCIM/TC57CIM/IEC61970/Base/Wires#RotatingMachine_ratedPowerFactor
:RotatingMachine_ratedPowerFactor rdf:type owl:DatatypeProperty ;
                                  rdfs:domain :RotatingMachine ;
                                  rdfs:range xsd:float ;
                                  rdfs:comment "Power factor (nameplate data). It is primarily used for short circuit data exchange according to IEC 60909." .


###  https://w3id.org/netbeheer/IECCIM/TC57CIM/IEC61970/Base/Wires#SeriesCompensator_varistorPresent
:SeriesCompensator_varistorPresent rdf:type owl:DatatypeProperty ;
                                   rdfs:domain :SeriesCompensator ;
                                   rdfs:range xsd:boolean ;
                                   rdfs:comment "Describe if a metal oxide varistor (mov) for over voltage protection is configured at the series compensator." .


###  https://w3id.org/netbeheer/IECCIM/TC57CIM/IEC61970/Base/Wires#ShuntCompensatorPhase_maximumSections
:ShuntCompensatorPhase_maximumSections rdf:type owl:DatatypeProperty ;
                                       rdfs:domain :ShuntCompensatorPhase ;
                                       rdfs:range xsd:nonNegativeInteger ;
                                       rdfs:comment """The maximum number of sections that may be switched in for this phase. 
""" .


###  https://w3id.org/netbeheer/IECCIM/TC57CIM/IEC61970/Base/Wires#ShuntCompensatorPhase_normalSections
:ShuntCompensatorPhase_normalSections rdf:type owl:DatatypeProperty ;
                                      rdfs:domain :ShuntCompensatorPhase ;
                                      rdfs:range xsd:nonNegativeInteger ;
                                      rdfs:comment """For the capacitor phase, the normal number of sections switched in.
""" .


###  https://w3id.org/netbeheer/IECCIM/TC57CIM/IEC61970/Base/Wires#ShuntCompensatorPhase_phase
:ShuntCompensatorPhase_phase rdf:type owl:DatatypeProperty ;
                             rdfs:domain :ShuntCompensatorPhase ;
                             rdfs:range :SinglePhaseKind ;
                             rdfs:comment """Phase of this shunt compensator component.   If the shunt compensator is wye connected, the connection is from the indicated phase to the central ground or neutral point.  If the shunt compensator is delta connected, the phase indicates a shunt compensator connected from the indicated phase to the next logical non-neutral phase.
""" .


###  https://w3id.org/netbeheer/IECCIM/TC57CIM/IEC61970/Base/Wires#ShuntCompensator_grounded
:ShuntCompensator_grounded rdf:type owl:DatatypeProperty ;
                           rdfs:domain :ShuntCompensator ;
                           rdfs:range xsd:boolean ;
                           rdfs:comment "Used for Yn and Zn connections. True if the neutral is solidly grounded." .


###  https://w3id.org/netbeheer/IECCIM/TC57CIM/IEC61970/Base/Wires#ShuntCompensator_maximumSections
:ShuntCompensator_maximumSections rdf:type owl:DatatypeProperty ;
                                  rdfs:domain :ShuntCompensator ;
                                  rdfs:range xsd:nonNegativeInteger ;
                                  rdfs:comment """The maximum number of sections that may be switched in. 
""" .


###  https://w3id.org/netbeheer/IECCIM/TC57CIM/IEC61970/Base/Wires#ShuntCompensator_normalSections
:ShuntCompensator_normalSections rdf:type owl:DatatypeProperty ;
                                 rdfs:domain :ShuntCompensator ;
                                 rdfs:range xsd:nonNegativeInteger ;
                                 rdfs:comment """The normal number of sections switched in.
""" .


###  https://w3id.org/netbeheer/IECCIM/TC57CIM/IEC61970/Base/Wires#ShuntCompensator_phaseConnection
:ShuntCompensator_phaseConnection rdf:type owl:DatatypeProperty ;
                                  rdfs:domain :ShuntCompensator ;
                                  rdfs:range :PhaseShuntConnectionKind ;
                                  rdfs:comment """The type of phase connection, such as wye or delta.
""" .


###  https://w3id.org/netbeheer/IECCIM/TC57CIM/IEC61970/Base/Wires#ShuntCompensator_sections
:ShuntCompensator_sections rdf:type owl:DatatypeProperty ;
                           rdfs:domain :ShuntCompensator ;
                           rdfs:range xsd:float ;
                           rdfs:comment """Shunt compensator sections in use.
Starting value for steady state solution. Non integer values are allowed to support continuous variables. The reasons for continuous value are to support study cases where no discrete shunt compensators has yet been designed, a solutions where a narrow voltage band force the sections to oscillate or accommodate for a continuous solution as input.""" .


###  https://w3id.org/netbeheer/IECCIM/TC57CIM/IEC61970/Base/Wires#ShuntCompensator_switchOnCount
:ShuntCompensator_switchOnCount rdf:type owl:DatatypeProperty ;
                                rdfs:domain :ShuntCompensator ;
                                rdfs:range xsd:nonNegativeInteger ;
                                rdfs:comment "The switch on count since the capacitor count was last reset or initialized." .


###  https://w3id.org/netbeheer/IECCIM/TC57CIM/IEC61970/Base/Wires#ShuntCompensator_switchOnDate
:ShuntCompensator_switchOnDate rdf:type owl:DatatypeProperty ;
                               rdfs:domain :ShuntCompensator ;
                               rdfs:range xsd:dateTime ;
                               rdfs:comment "The date and time when the capacitor bank was last switched on." .


###  https://w3id.org/netbeheer/IECCIM/TC57CIM/IEC61970/Base/Wires#StaticVarCompensator_sVCControlMode
:StaticVarCompensator_sVCControlMode rdf:type owl:DatatypeProperty ;
                                     rdfs:domain :StaticVarCompensator ;
                                     rdfs:range :SVCControlMode ;
                                     rdfs:comment "SVC control mode." .


###  https://w3id.org/netbeheer/IECCIM/TC57CIM/IEC61970/Base/Wires#SwitchPhase_closed
:SwitchPhase_closed rdf:type owl:DatatypeProperty ;
                    rdfs:domain :SwitchPhase ;
                    rdfs:range xsd:boolean ;
                    rdfs:comment "The attribute tells if the switch is considered closed when used as input to topology processing." .


###  https://w3id.org/netbeheer/IECCIM/TC57CIM/IEC61970/Base/Wires#SwitchPhase_normalOpen
:SwitchPhase_normalOpen rdf:type owl:DatatypeProperty ;
                        rdfs:domain :SwitchPhase ;
                        rdfs:range xsd:boolean ;
                        rdfs:comment """Used in cases when no Measurement for the status value is present. If the SwitchPhase has a status measurement the Discrete.normalValue is expected to match with this value.
""" .


###  https://w3id.org/netbeheer/IECCIM/TC57CIM/IEC61970/Base/Wires#SwitchPhase_phaseSide1
:SwitchPhase_phaseSide1 rdf:type owl:DatatypeProperty ;
                        rdfs:domain :SwitchPhase ;
                        rdfs:range :SinglePhaseKind ;
                        rdfs:comment """Phase of this SwitchPhase on the side with terminal sequence number equal 1. Should be a phase contained in that terminal&rsquo;s phases attribute.
""" .


###  https://w3id.org/netbeheer/IECCIM/TC57CIM/IEC61970/Base/Wires#SwitchPhase_phaseSide2
:SwitchPhase_phaseSide2 rdf:type owl:DatatypeProperty ;
                        rdfs:domain :SwitchPhase ;
                        rdfs:range :SinglePhaseKind ;
                        rdfs:comment """Phase of this SwitchPhase on the side with terminal sequence number equal 2.  Should be a phase contained in that terminal&rsquo;s Terminal.phases attribute.
""" .


###  https://w3id.org/netbeheer/IECCIM/TC57CIM/IEC61970/Base/Wires#Switch_normalOpen
:Switch_normalOpen rdf:type owl:DatatypeProperty ;
                   rdfs:domain :Switch ;
                   rdfs:range xsd:boolean ;
                   rdfs:comment "The attribute is used in cases when no Measurement for the status value is present. If the Switch has a status measurement the Discrete.normalValue is expected to match with the Switch.normalOpen." .


###  https://w3id.org/netbeheer/IECCIM/TC57CIM/IEC61970/Base/Wires#Switch_open
:Switch_open rdf:type owl:DatatypeProperty ;
             rdfs:domain :Switch ;
             rdfs:range xsd:boolean ;
             rdfs:comment "The attribute tells if the switch is considered open when used as input to topology processing." .


###  https://w3id.org/netbeheer/IECCIM/TC57CIM/IEC61970/Base/Wires#Switch_retained
:Switch_retained rdf:type owl:DatatypeProperty ;
                 rdfs:domain :Switch ;
                 rdfs:range xsd:boolean ;
                 rdfs:comment "Branch is retained in a bus branch model.  The flow through retained switches will normally be calculated in power flow." .


###  https://w3id.org/netbeheer/IECCIM/TC57CIM/IEC61970/Base/Wires#Switch_switchOnCount
:Switch_switchOnCount rdf:type owl:DatatypeProperty ;
                      rdfs:domain :Switch ;
                      rdfs:range xsd:nonNegativeInteger ;
                      rdfs:comment "The switch on count since the switch was last reset or initialized." .


###  https://w3id.org/netbeheer/IECCIM/TC57CIM/IEC61970/Base/Wires#Switch_switchOnDate
:Switch_switchOnDate rdf:type owl:DatatypeProperty ;
                     rdfs:domain :Switch ;
                     rdfs:range xsd:dateTime ;
                     rdfs:comment "The date and time when the switch was last switched on." .


###  https://w3id.org/netbeheer/IECCIM/TC57CIM/IEC61970/Base/Wires#SynchronousMachine_coolantCondition
:SynchronousMachine_coolantCondition rdf:type owl:DatatypeProperty ;
                                     rdfs:domain :SynchronousMachine ;
                                     rdfs:range xsd:float ;
                                     rdfs:comment "Temperature or pressure of coolant medium" .


###  https://w3id.org/netbeheer/IECCIM/TC57CIM/IEC61970/Base/Wires#SynchronousMachine_coolantType
:SynchronousMachine_coolantType rdf:type owl:DatatypeProperty ;
                                rdfs:domain :SynchronousMachine ;
                                rdfs:range :CoolantType ;
                                rdfs:comment "Method of cooling the machine." .


###  https://w3id.org/netbeheer/IECCIM/TC57CIM/IEC61970/Base/Wires#SynchronousMachine_earthing
:SynchronousMachine_earthing rdf:type owl:DatatypeProperty ;
                             rdfs:domain :SynchronousMachine ;
                             rdfs:range xsd:boolean ;
                             rdfs:comment "Indicates whether or not the generator is earthed. Used for short circuit data exchange according to IEC 60909" .


###  https://w3id.org/netbeheer/IECCIM/TC57CIM/IEC61970/Base/Wires#SynchronousMachine_mu
:SynchronousMachine_mu rdf:type owl:DatatypeProperty ;
                       rdfs:domain :SynchronousMachine ;
                       rdfs:range xsd:float ;
                       rdfs:comment """Factor to calculate the breaking current (Section 4.5.2.1 in the IEC 60909-0).
Used only for single fed short circuit on a generator (Section 4.3.4.2. in the IEC 60909-0).""" .


###  https://w3id.org/netbeheer/IECCIM/TC57CIM/IEC61970/Base/Wires#SynchronousMachine_operatingMode
:SynchronousMachine_operatingMode rdf:type owl:DatatypeProperty ;
                                  rdfs:domain :SynchronousMachine ;
                                  rdfs:range :SynchronousMachineOperatingMode ;
                                  rdfs:comment "Current mode of operation." .


###  https://w3id.org/netbeheer/IECCIM/TC57CIM/IEC61970/Base/Wires#SynchronousMachine_referencePriority
:SynchronousMachine_referencePriority rdf:type owl:DatatypeProperty ;
                                      rdfs:domain :SynchronousMachine ;
                                      rdfs:range xsd:nonNegativeInteger ;
                                      rdfs:comment """Priority of unit for use as powerflow voltage phase angle reference bus selection. 0 = don t care (default) 1 = highest priority. 2 is less than 1 and so on.
""" .


###  https://w3id.org/netbeheer/IECCIM/TC57CIM/IEC61970/Base/Wires#SynchronousMachine_shortCircuitRotorType
:SynchronousMachine_shortCircuitRotorType rdf:type owl:DatatypeProperty ;
                                          rdfs:domain :SynchronousMachine ;
                                          rdfs:range :ShortCircuitRotorKind ;
                                          rdfs:comment "Type of rotor, used by short circuit applications, only for single fed short circuit according to IEC 60909." .


###  https://w3id.org/netbeheer/IECCIM/TC57CIM/IEC61970/Base/Wires#SynchronousMachine_type
:SynchronousMachine_type rdf:type owl:DatatypeProperty ;
                         rdfs:domain :SynchronousMachine ;
                         rdfs:range :SynchronousMachineKind ;
                         rdfs:comment "Modes that this synchronous machine can operate in." .


###  https://w3id.org/netbeheer/IECCIM/TC57CIM/IEC61970/Base/Wires#TapChangerControl_lineDropCompensation
:TapChangerControl_lineDropCompensation rdf:type owl:DatatypeProperty ;
                                        rdfs:domain :TapChangerControl ;
                                        rdfs:range xsd:boolean ;
                                        rdfs:comment "If true, the line drop compensation is to be applied." .


###  https://w3id.org/netbeheer/IECCIM/TC57CIM/IEC61970/Base/Wires#TapChangerTablePoint_ratio
:TapChangerTablePoint_ratio rdf:type owl:DatatypeProperty ;
                            rdfs:domain :TapChangerTablePoint ;
                            rdfs:range xsd:float ;
                            rdfs:comment """The voltage ratio in per unit. Hence this is a value close to one.
""" .


###  https://w3id.org/netbeheer/IECCIM/TC57CIM/IEC61970/Base/Wires#TapChangerTablePoint_step
:TapChangerTablePoint_step rdf:type owl:DatatypeProperty ;
                           rdfs:domain :TapChangerTablePoint ;
                           rdfs:range xsd:nonNegativeInteger ;
                           rdfs:comment """The tap step.
""" .


###  https://w3id.org/netbeheer/IECCIM/TC57CIM/IEC61970/Base/Wires#TapChanger_controlEnabled
:TapChanger_controlEnabled rdf:type owl:DatatypeProperty ;
                           rdfs:domain :TapChanger ;
                           rdfs:range xsd:boolean ;
                           rdfs:comment "Specifies the regulation status of the equipment.  True is regulating, false is not regulating." .


###  https://w3id.org/netbeheer/IECCIM/TC57CIM/IEC61970/Base/Wires#TapChanger_highStep
:TapChanger_highStep rdf:type owl:DatatypeProperty ;
                     rdfs:domain :TapChanger ;
                     rdfs:range xsd:nonNegativeInteger ;
                     rdfs:comment """Highest possible tap step position, advance from neutral.
The attribute shall be greater than lowStep.""" .


###  https://w3id.org/netbeheer/IECCIM/TC57CIM/IEC61970/Base/Wires#TapChanger_lowStep
:TapChanger_lowStep rdf:type owl:DatatypeProperty ;
                    rdfs:domain :TapChanger ;
                    rdfs:range xsd:nonNegativeInteger ;
                    rdfs:comment "Lowest possible tap step position, retard from neutral" .


###  https://w3id.org/netbeheer/IECCIM/TC57CIM/IEC61970/Base/Wires#TapChanger_ltcFlag
:TapChanger_ltcFlag rdf:type owl:DatatypeProperty ;
                    rdfs:domain :TapChanger ;
                    rdfs:range xsd:boolean ;
                    rdfs:comment "Specifies whether or not a TapChanger has load tap changing capabilities." .


###  https://w3id.org/netbeheer/IECCIM/TC57CIM/IEC61970/Base/Wires#TapChanger_neutralStep
:TapChanger_neutralStep rdf:type owl:DatatypeProperty ;
                        rdfs:domain :TapChanger ;
                        rdfs:range xsd:nonNegativeInteger ;
                        rdfs:comment """The neutral tap step position for this winding.
The attribute shall be equal or greater than lowStep and equal or less than highStep.""" .


###  https://w3id.org/netbeheer/IECCIM/TC57CIM/IEC61970/Base/Wires#TapChanger_normalStep
:TapChanger_normalStep rdf:type owl:DatatypeProperty ;
                       rdfs:domain :TapChanger ;
                       rdfs:range xsd:nonNegativeInteger ;
                       rdfs:comment """The tap step position used in \"normal\" network operation for this winding. For a \"Fixed\" tap changer indicates the current physical tap setting.
The attribute shall be equal or greater than lowStep and equal or less than highStep.""" .


###  https://w3id.org/netbeheer/IECCIM/TC57CIM/IEC61970/Base/Wires#TapChanger_step
:TapChanger_step rdf:type owl:DatatypeProperty ;
                 rdfs:domain :TapChanger ;
                 rdfs:range xsd:float ;
                 rdfs:comment """Tap changer position.
Starting step for a steady state solution. Non integer values are allowed to support continuous tap variables. The reasons for continuous value are to support study cases where no discrete tap changers has yet been designed, a solutions where a narrow voltage band force the tap step to oscillate or accommodate for a continuous solution as input.
The attribute shall be equal or greater than lowStep and equal or less than highStep.""" .


###  https://w3id.org/netbeheer/IECCIM/TC57CIM/IEC61970/Base/Wires#TransformerEnd_endNumber
:TransformerEnd_endNumber rdf:type owl:DatatypeProperty ;
                          rdfs:domain :TransformerEnd ;
                          rdfs:range xsd:nonNegativeInteger ;
                          rdfs:comment """Number for this transformer end, corresponding to the end's order in the power transformer vector group or phase angle clock number.  Highest voltage winding should be 1.  Each end within a power transformer should have a unique subsequent end number.   Note the transformer end number need not match the terminal sequence number.
""" .


###  https://w3id.org/netbeheer/IECCIM/TC57CIM/IEC61970/Base/Wires#TransformerEnd_grounded
:TransformerEnd_grounded rdf:type owl:DatatypeProperty ;
                         rdfs:domain :TransformerEnd ;
                         rdfs:range xsd:boolean ;
                         rdfs:comment "(for Yn and Zn connections) True if the neutral is solidly grounded." .


###  https://w3id.org/netbeheer/IECCIM/TC57CIM/IEC61970/Base/Wires#TransformerTankEnd_phases
:TransformerTankEnd_phases rdf:type owl:DatatypeProperty ;
                           rdfs:domain :TransformerTankEnd ;
                           rdfs:range <https://w3id.org/netbeheer/IECCIM/TC57CIM/IEC61970/Base/Core#PhaseCode> ;
                           rdfs:comment "Describes the phases carried by a conducting equipment." .


#################################################################
#    Classes
#################################################################

###  https://w3id.org/netbeheer/IECCIM/TC57CIM/IEC61968/AssetInfo#TransformerEndInfo
<https://w3id.org/netbeheer/IECCIM/TC57CIM/IEC61968/AssetInfo#TransformerEndInfo> rdf:type owl:Class ;
                                                                                  rdfs:subClassOf [ rdf:type owl:Restriction ;
                                                                                                    owl:onProperty :TransformerEndInfo_CoreAdmittance ;
                                                                                                    owl:minQualifiedCardinality "0"^^xsd:nonNegativeInteger ;
                                                                                                    owl:onClass <https://w3id.org/netbeheer/IECCIM/TC57CIM/IEC61968/AssetInfo#TransformerEndInfo>
                                                                                                  ] ,
                                                                                                  [ rdf:type owl:Restriction ;
                                                                                                    owl:onProperty :TransformerEndInfo_FromMeshImpedances ;
                                                                                                    owl:minQualifiedCardinality "0"^^xsd:nonNegativeInteger ;
                                                                                                    owl:onClass <https://w3id.org/netbeheer/IECCIM/TC57CIM/IEC61968/AssetInfo#TransformerEndInfo>
                                                                                                  ] ,
                                                                                                  [ rdf:type owl:Restriction ;
                                                                                                    owl:onProperty :TransformerEndInfo_ToMeshImpedances ;
                                                                                                    owl:minQualifiedCardinality "0"^^xsd:nonNegativeInteger ;
                                                                                                    owl:onClass <https://w3id.org/netbeheer/IECCIM/TC57CIM/IEC61968/AssetInfo#TransformerEndInfo>
                                                                                                  ] ,
                                                                                                  [ rdf:type owl:Restriction ;
                                                                                                    owl:onProperty :TransformerEndInfo_TransformerStarImpedance ;
                                                                                                    owl:minQualifiedCardinality "0"^^xsd:nonNegativeInteger ;
                                                                                                    owl:onClass <https://w3id.org/netbeheer/IECCIM/TC57CIM/IEC61968/AssetInfo#TransformerEndInfo>
                                                                                                  ] ,
                                                                                                  [ rdf:type owl:Restriction ;
                                                                                                    owl:onProperty :TransformerEndInfo_CoreAdmittance ;
                                                                                                    owl:maxQualifiedCardinality "1"^^xsd:nonNegativeInteger ;
                                                                                                    owl:onClass <https://w3id.org/netbeheer/IECCIM/TC57CIM/IEC61968/AssetInfo#TransformerEndInfo>
                                                                                                  ] ,
                                                                                                  [ rdf:type owl:Restriction ;
                                                                                                    owl:onProperty :TransformerEndInfo_FromMeshImpedances ;
                                                                                                    owl:maxQualifiedCardinality "1"^^xsd:nonNegativeInteger ;
                                                                                                    owl:onClass <https://w3id.org/netbeheer/IECCIM/TC57CIM/IEC61968/AssetInfo#TransformerEndInfo>
                                                                                                  ] ,
                                                                                                  [ rdf:type owl:Restriction ;
                                                                                                    owl:onProperty :TransformerEndInfo_TransformerStarImpedance ;
                                                                                                    owl:maxQualifiedCardinality "1"^^xsd:nonNegativeInteger ;
                                                                                                    owl:onClass <https://w3id.org/netbeheer/IECCIM/TC57CIM/IEC61968/AssetInfo#TransformerEndInfo>
                                                                                                  ] .


###  https://w3id.org/netbeheer/IECCIM/TC57CIM/IEC61968/AssetInfo#WireInfo
<https://w3id.org/netbeheer/IECCIM/TC57CIM/IEC61968/AssetInfo#WireInfo> rdf:type owl:Class ;
                                                                        rdfs:subClassOf [ rdf:type owl:Restriction ;
                                                                                          owl:onProperty :WireInfo_PerLengthParameters ;
                                                                                          owl:minQualifiedCardinality "0"^^xsd:nonNegativeInteger ;
                                                                                          owl:onClass <https://w3id.org/netbeheer/IECCIM/TC57CIM/IEC61968/AssetInfo#WireInfo>
                                                                                        ] .


###  https://w3id.org/netbeheer/IECCIM/TC57CIM/IEC61968/AssetInfo#WireSpacing
<https://w3id.org/netbeheer/IECCIM/TC57CIM/IEC61968/AssetInfo#WireSpacing> rdf:type owl:Class ;
                                                                           rdfs:subClassOf [ rdf:type owl:Restriction ;
                                                                                             owl:onProperty :WireSpacing_ACLineSegments ;
                                                                                             owl:minQualifiedCardinality "0"^^xsd:nonNegativeInteger ;
                                                                                             owl:onClass <https://w3id.org/netbeheer/IECCIM/TC57CIM/IEC61968/AssetInfo#WireSpacing>
                                                                                           ] ,
                                                                                           [ rdf:type owl:Restriction ;
                                                                                             owl:onProperty :WireSpacing_PerLengthParameters ;
                                                                                             owl:minQualifiedCardinality "0"^^xsd:nonNegativeInteger ;
                                                                                             owl:onClass <https://w3id.org/netbeheer/IECCIM/TC57CIM/IEC61968/AssetInfo#WireSpacing>
                                                                                           ] ,
                                                                                           [ rdf:type owl:Restriction ;
                                                                                             owl:onProperty :WireSpacing_ACLineSegments ;
                                                                                             owl:maxQualifiedCardinality "1"^^xsd:nonNegativeInteger ;
                                                                                             owl:onClass <https://w3id.org/netbeheer/IECCIM/TC57CIM/IEC61968/AssetInfo#WireSpacing>
                                                                                           ] ,
                                                                                           [ rdf:type owl:Restriction ;
                                                                                             owl:onProperty :WireSpacing_PerLengthParameters ;
                                                                                             owl:maxQualifiedCardinality "1"^^xsd:nonNegativeInteger ;
                                                                                             owl:onClass <https://w3id.org/netbeheer/IECCIM/TC57CIM/IEC61968/AssetInfo#WireSpacing>
                                                                                           ] .


###  https://w3id.org/netbeheer/IECCIM/TC57CIM/IEC61968/InfIEC61968/InfAssets#TransformerObservation
<https://w3id.org/netbeheer/IECCIM/TC57CIM/IEC61968/InfIEC61968/InfAssets#TransformerObservation> rdf:type owl:Class ;
                                                                                                  rdfs:subClassOf [ rdf:type owl:Restriction ;
                                                                                                                    owl:onProperty :TransformerObservation_Transformer ;
                                                                                                                    owl:minQualifiedCardinality "0"^^xsd:nonNegativeInteger ;
                                                                                                                    owl:onClass <https://w3id.org/netbeheer/IECCIM/TC57CIM/IEC61968/InfIEC61968/InfAssets#TransformerObservation>
                                                                                                                  ] .


###  https://w3id.org/netbeheer/IECCIM/TC57CIM/IEC61968/InfIEC61968/InfAssets#WindingInsulation
<https://w3id.org/netbeheer/IECCIM/TC57CIM/IEC61968/InfIEC61968/InfAssets#WindingInsulation> rdf:type owl:Class ;
                                                                                             rdfs:subClassOf [ rdf:type owl:Restriction ;
                                                                                                               owl:onProperty :WindingInsulation_FromWinding ;
                                                                                                               owl:minQualifiedCardinality "0"^^xsd:nonNegativeInteger ;
                                                                                                               owl:onClass <https://w3id.org/netbeheer/IECCIM/TC57CIM/IEC61968/InfIEC61968/InfAssets#WindingInsulation>
                                                                                                             ] ,
                                                                                                             [ rdf:type owl:Restriction ;
                                                                                                               owl:onProperty :WindingInsulation_ToWinding ;
                                                                                                               owl:minQualifiedCardinality "0"^^xsd:nonNegativeInteger ;
                                                                                                               owl:onClass <https://w3id.org/netbeheer/IECCIM/TC57CIM/IEC61968/InfIEC61968/InfAssets#WindingInsulation>
                                                                                                             ] .


###  https://w3id.org/netbeheer/IECCIM/TC57CIM/IEC61968/LoadControl#ConnectDisconnectFunction
<https://w3id.org/netbeheer/IECCIM/TC57CIM/IEC61968/LoadControl#ConnectDisconnectFunction> rdf:type owl:Class ;
                                                                                           rdfs:subClassOf [ rdf:type owl:Restriction ;
                                                                                                             owl:onProperty :ConnectDisconnectFunction_Switches ;
                                                                                                             owl:minQualifiedCardinality "0"^^xsd:nonNegativeInteger ;
                                                                                                             owl:onClass <https://w3id.org/netbeheer/IECCIM/TC57CIM/IEC61968/LoadControl#ConnectDisconnectFunction>
                                                                                                           ] .


###  https://w3id.org/netbeheer/IECCIM/TC57CIM/IEC61968/Operations#CutAction
<https://w3id.org/netbeheer/IECCIM/TC57CIM/IEC61968/Operations#CutAction> rdf:type owl:Class ;
                                                                          rdfs:subClassOf [ rdf:type owl:Restriction ;
                                                                                            owl:onProperty :CutAction_Cut ;
                                                                                            owl:minQualifiedCardinality "0"^^xsd:nonNegativeInteger ;
                                                                                            owl:onClass <https://w3id.org/netbeheer/IECCIM/TC57CIM/IEC61968/Operations#CutAction>
                                                                                          ] ,
                                                                                          [ rdf:type owl:Restriction ;
                                                                                            owl:onProperty :CutAction_Cut ;
                                                                                            owl:maxQualifiedCardinality "1"^^xsd:nonNegativeInteger ;
                                                                                            owl:onClass <https://w3id.org/netbeheer/IECCIM/TC57CIM/IEC61968/Operations#CutAction>
                                                                                          ] .


###  https://w3id.org/netbeheer/IECCIM/TC57CIM/IEC61968/Operations#EnergySourceAction
<https://w3id.org/netbeheer/IECCIM/TC57CIM/IEC61968/Operations#EnergySourceAction> rdf:type owl:Class ;
                                                                                   rdfs:subClassOf [ rdf:type owl:Restriction ;
                                                                                                     owl:onProperty :EnergySourceAction_EnergySource ;
                                                                                                     owl:minQualifiedCardinality "0"^^xsd:nonNegativeInteger ;
                                                                                                     owl:onClass <https://w3id.org/netbeheer/IECCIM/TC57CIM/IEC61968/Operations#EnergySourceAction>
                                                                                                   ] ,
                                                                                                   [ rdf:type owl:Restriction ;
                                                                                                     owl:onProperty :EnergySourceAction_EnergySource ;
                                                                                                     owl:maxQualifiedCardinality "1"^^xsd:nonNegativeInteger ;
                                                                                                     owl:onClass <https://w3id.org/netbeheer/IECCIM/TC57CIM/IEC61968/Operations#EnergySourceAction>
                                                                                                   ] .


###  https://w3id.org/netbeheer/IECCIM/TC57CIM/IEC61968/Operations#GroundAction
<https://w3id.org/netbeheer/IECCIM/TC57CIM/IEC61968/Operations#GroundAction> rdf:type owl:Class ;
                                                                             rdfs:subClassOf [ rdf:type owl:Restriction ;
                                                                                               owl:onProperty :GroundAction_AlongACLineSegment ;
                                                                                               owl:minQualifiedCardinality "0"^^xsd:nonNegativeInteger ;
                                                                                               owl:onClass <https://w3id.org/netbeheer/IECCIM/TC57CIM/IEC61968/Operations#GroundAction>
                                                                                             ] ,
                                                                                             [ rdf:type owl:Restriction ;
                                                                                               owl:onProperty :GroundAction_Ground ;
                                                                                               owl:minQualifiedCardinality "0"^^xsd:nonNegativeInteger ;
                                                                                               owl:onClass <https://w3id.org/netbeheer/IECCIM/TC57CIM/IEC61968/Operations#GroundAction>
                                                                                             ] ,
                                                                                             [ rdf:type owl:Restriction ;
                                                                                               owl:onProperty :GroundAction_AlongACLineSegment ;
                                                                                               owl:maxQualifiedCardinality "1"^^xsd:nonNegativeInteger ;
                                                                                               owl:onClass <https://w3id.org/netbeheer/IECCIM/TC57CIM/IEC61968/Operations#GroundAction>
                                                                                             ] ,
                                                                                             [ rdf:type owl:Restriction ;
                                                                                               owl:onProperty :GroundAction_Ground ;
                                                                                               owl:maxQualifiedCardinality "1"^^xsd:nonNegativeInteger ;
                                                                                               owl:onClass <https://w3id.org/netbeheer/IECCIM/TC57CIM/IEC61968/Operations#GroundAction>
                                                                                             ] .


###  https://w3id.org/netbeheer/IECCIM/TC57CIM/IEC61968/Operations#JumperAction
<https://w3id.org/netbeheer/IECCIM/TC57CIM/IEC61968/Operations#JumperAction> rdf:type owl:Class ;
                                                                             rdfs:subClassOf [ rdf:type owl:Restriction ;
                                                                                               owl:onProperty :JumperAction_AlongACLineSegments ;
                                                                                               owl:minQualifiedCardinality "0"^^xsd:nonNegativeInteger ;
                                                                                               owl:onClass <https://w3id.org/netbeheer/IECCIM/TC57CIM/IEC61968/Operations#JumperAction>
                                                                                             ] ,
                                                                                             [ rdf:type owl:Restriction ;
                                                                                               owl:onProperty :JumperAction_Jumper ;
                                                                                               owl:minQualifiedCardinality "0"^^xsd:nonNegativeInteger ;
                                                                                               owl:onClass <https://w3id.org/netbeheer/IECCIM/TC57CIM/IEC61968/Operations#JumperAction>
                                                                                             ] ,
                                                                                             [ rdf:type owl:Restriction ;
                                                                                               owl:onProperty :JumperAction_AlongACLineSegments ;
                                                                                               owl:maxQualifiedCardinality "1"^^xsd:nonNegativeInteger ;
                                                                                               owl:onClass <https://w3id.org/netbeheer/IECCIM/TC57CIM/IEC61968/Operations#JumperAction>
                                                                                             ] ,
                                                                                             [ rdf:type owl:Restriction ;
                                                                                               owl:onProperty :JumperAction_Jumper ;
                                                                                               owl:maxQualifiedCardinality "1"^^xsd:nonNegativeInteger ;
                                                                                               owl:onClass <https://w3id.org/netbeheer/IECCIM/TC57CIM/IEC61968/Operations#JumperAction>
                                                                                             ] .


###  https://w3id.org/netbeheer/IECCIM/TC57CIM/IEC61968/Operations#Outage
<https://w3id.org/netbeheer/IECCIM/TC57CIM/IEC61968/Operations#Outage> rdf:type owl:Class ;
                                                                       rdfs:subClassOf [ rdf:type owl:Restriction ;
                                                                                         owl:onProperty :Outage_OpenedSwitches ;
                                                                                         owl:minQualifiedCardinality "0"^^xsd:nonNegativeInteger ;
                                                                                         owl:onClass <https://w3id.org/netbeheer/IECCIM/TC57CIM/IEC61968/Operations#Outage>
                                                                                       ] ,
                                                                                       [ rdf:type owl:Restriction ;
                                                                                         owl:onProperty :Outage_OpenedSwitches ;
                                                                                         owl:maxQualifiedCardinality "1"^^xsd:nonNegativeInteger ;
                                                                                         owl:onClass <https://w3id.org/netbeheer/IECCIM/TC57CIM/IEC61968/Operations#Outage>
                                                                                       ] .


###  https://w3id.org/netbeheer/IECCIM/TC57CIM/IEC61968/Operations#SwitchAction
<https://w3id.org/netbeheer/IECCIM/TC57CIM/IEC61968/Operations#SwitchAction> rdf:type owl:Class ;
                                                                             rdfs:subClassOf [ rdf:type owl:Restriction ;
                                                                                               owl:onProperty :SwitchAction_OperatedSwitch ;
                                                                                               owl:minQualifiedCardinality "0"^^xsd:nonNegativeInteger ;
                                                                                               owl:onClass <https://w3id.org/netbeheer/IECCIM/TC57CIM/IEC61968/Operations#SwitchAction>
                                                                                             ] ,
                                                                                             [ rdf:type owl:Restriction ;
                                                                                               owl:onProperty :SwitchAction_OperatedSwitch ;
                                                                                               owl:maxQualifiedCardinality "1"^^xsd:nonNegativeInteger ;
                                                                                               owl:onClass <https://w3id.org/netbeheer/IECCIM/TC57CIM/IEC61968/Operations#SwitchAction>
                                                                                             ] .


###  https://w3id.org/netbeheer/IECCIM/TC57CIM/IEC61970/Base/Core#ConductingEquipment
<https://w3id.org/netbeheer/IECCIM/TC57CIM/IEC61970/Base/Core#ConductingEquipment> rdf:type owl:Class .


###  https://w3id.org/netbeheer/IECCIM/TC57CIM/IEC61970/Base/Core#Curve
<https://w3id.org/netbeheer/IECCIM/TC57CIM/IEC61970/Base/Core#Curve> rdf:type owl:Class .


###  https://w3id.org/netbeheer/IECCIM/TC57CIM/IEC61970/Base/Core#Equipment
<https://w3id.org/netbeheer/IECCIM/TC57CIM/IEC61970/Base/Core#Equipment> rdf:type owl:Class .


###  https://w3id.org/netbeheer/IECCIM/TC57CIM/IEC61970/Base/Core#EquipmentContainer
<https://w3id.org/netbeheer/IECCIM/TC57CIM/IEC61970/Base/Core#EquipmentContainer> rdf:type owl:Class .


###  https://w3id.org/netbeheer/IECCIM/TC57CIM/IEC61970/Base/Core#IdentifiedObject
<https://w3id.org/netbeheer/IECCIM/TC57CIM/IEC61970/Base/Core#IdentifiedObject> rdf:type owl:Class .


###  https://w3id.org/netbeheer/IECCIM/TC57CIM/IEC61970/Base/Core#PowerSystemResource
<https://w3id.org/netbeheer/IECCIM/TC57CIM/IEC61970/Base/Core#PowerSystemResource> rdf:type owl:Class .


###  https://w3id.org/netbeheer/IECCIM/TC57CIM/IEC61970/Base/Domain#ActivePower
<https://w3id.org/netbeheer/IECCIM/TC57CIM/IEC61970/Base/Domain#ActivePower> rdf:type owl:Class .


###  https://w3id.org/netbeheer/IECCIM/TC57CIM/IEC61970/Base/Domain#ActivePowerPerFrequency
<https://w3id.org/netbeheer/IECCIM/TC57CIM/IEC61970/Base/Domain#ActivePowerPerFrequency> rdf:type owl:Class .


###  https://w3id.org/netbeheer/IECCIM/TC57CIM/IEC61970/Base/Domain#AngleDegrees
<https://w3id.org/netbeheer/IECCIM/TC57CIM/IEC61970/Base/Domain#AngleDegrees> rdf:type owl:Class .


###  https://w3id.org/netbeheer/IECCIM/TC57CIM/IEC61970/Base/Domain#AngleRadians
<https://w3id.org/netbeheer/IECCIM/TC57CIM/IEC61970/Base/Domain#AngleRadians> rdf:type owl:Class .


###  https://w3id.org/netbeheer/IECCIM/TC57CIM/IEC61970/Base/Domain#ApparentPower
<https://w3id.org/netbeheer/IECCIM/TC57CIM/IEC61970/Base/Domain#ApparentPower> rdf:type owl:Class .


###  https://w3id.org/netbeheer/IECCIM/TC57CIM/IEC61970/Base/Domain#Conductance
<https://w3id.org/netbeheer/IECCIM/TC57CIM/IEC61970/Base/Domain#Conductance> rdf:type owl:Class .


###  https://w3id.org/netbeheer/IECCIM/TC57CIM/IEC61970/Base/Domain#ConductancePerLength
<https://w3id.org/netbeheer/IECCIM/TC57CIM/IEC61970/Base/Domain#ConductancePerLength> rdf:type owl:Class .


###  https://w3id.org/netbeheer/IECCIM/TC57CIM/IEC61970/Base/Domain#CurrentFlow
<https://w3id.org/netbeheer/IECCIM/TC57CIM/IEC61970/Base/Domain#CurrentFlow> rdf:type owl:Class .


###  https://w3id.org/netbeheer/IECCIM/TC57CIM/IEC61970/Base/Domain#Frequency
<https://w3id.org/netbeheer/IECCIM/TC57CIM/IEC61970/Base/Domain#Frequency> rdf:type owl:Class .


###  https://w3id.org/netbeheer/IECCIM/TC57CIM/IEC61970/Base/Domain#Length
<https://w3id.org/netbeheer/IECCIM/TC57CIM/IEC61970/Base/Domain#Length> rdf:type owl:Class .


###  https://w3id.org/netbeheer/IECCIM/TC57CIM/IEC61970/Base/Domain#PU
<https://w3id.org/netbeheer/IECCIM/TC57CIM/IEC61970/Base/Domain#PU> rdf:type owl:Class .


###  https://w3id.org/netbeheer/IECCIM/TC57CIM/IEC61970/Base/Domain#PerCent
<https://w3id.org/netbeheer/IECCIM/TC57CIM/IEC61970/Base/Domain#PerCent> rdf:type owl:Class .


###  https://w3id.org/netbeheer/IECCIM/TC57CIM/IEC61970/Base/Domain#Pressure
<https://w3id.org/netbeheer/IECCIM/TC57CIM/IEC61970/Base/Domain#Pressure> rdf:type owl:Class .


###  https://w3id.org/netbeheer/IECCIM/TC57CIM/IEC61970/Base/Domain#Reactance
<https://w3id.org/netbeheer/IECCIM/TC57CIM/IEC61970/Base/Domain#Reactance> rdf:type owl:Class .


###  https://w3id.org/netbeheer/IECCIM/TC57CIM/IEC61970/Base/Domain#ReactancePerLength
<https://w3id.org/netbeheer/IECCIM/TC57CIM/IEC61970/Base/Domain#ReactancePerLength> rdf:type owl:Class .


###  https://w3id.org/netbeheer/IECCIM/TC57CIM/IEC61970/Base/Domain#ReactivePower
<https://w3id.org/netbeheer/IECCIM/TC57CIM/IEC61970/Base/Domain#ReactivePower> rdf:type owl:Class .


###  https://w3id.org/netbeheer/IECCIM/TC57CIM/IEC61970/Base/Domain#Resistance
<https://w3id.org/netbeheer/IECCIM/TC57CIM/IEC61970/Base/Domain#Resistance> rdf:type owl:Class .


###  https://w3id.org/netbeheer/IECCIM/TC57CIM/IEC61970/Base/Domain#ResistancePerLength
<https://w3id.org/netbeheer/IECCIM/TC57CIM/IEC61970/Base/Domain#ResistancePerLength> rdf:type owl:Class .


###  https://w3id.org/netbeheer/IECCIM/TC57CIM/IEC61970/Base/Domain#RotationSpeed
<https://w3id.org/netbeheer/IECCIM/TC57CIM/IEC61970/Base/Domain#RotationSpeed> rdf:type owl:Class .


###  https://w3id.org/netbeheer/IECCIM/TC57CIM/IEC61970/Base/Domain#Seconds
<https://w3id.org/netbeheer/IECCIM/TC57CIM/IEC61970/Base/Domain#Seconds> rdf:type owl:Class .


###  https://w3id.org/netbeheer/IECCIM/TC57CIM/IEC61970/Base/Domain#Susceptance
<https://w3id.org/netbeheer/IECCIM/TC57CIM/IEC61970/Base/Domain#Susceptance> rdf:type owl:Class .


###  https://w3id.org/netbeheer/IECCIM/TC57CIM/IEC61970/Base/Domain#SusceptancePerLength
<https://w3id.org/netbeheer/IECCIM/TC57CIM/IEC61970/Base/Domain#SusceptancePerLength> rdf:type owl:Class .


###  https://w3id.org/netbeheer/IECCIM/TC57CIM/IEC61970/Base/Domain#Temperature
<https://w3id.org/netbeheer/IECCIM/TC57CIM/IEC61970/Base/Domain#Temperature> rdf:type owl:Class .


###  https://w3id.org/netbeheer/IECCIM/TC57CIM/IEC61970/Base/Domain#Voltage
<https://w3id.org/netbeheer/IECCIM/TC57CIM/IEC61970/Base/Domain#Voltage> rdf:type owl:Class .


###  https://w3id.org/netbeheer/IECCIM/TC57CIM/IEC61970/Base/Domain#VoltagePerReactivePower
<https://w3id.org/netbeheer/IECCIM/TC57CIM/IEC61970/Base/Domain#VoltagePerReactivePower> rdf:type owl:Class .


###  https://w3id.org/netbeheer/IECCIM/TC57CIM/IEC61970/Base/Equivalents#EquivalentInjection
<https://w3id.org/netbeheer/IECCIM/TC57CIM/IEC61970/Base/Equivalents#EquivalentInjection> rdf:type owl:Class ;
                                                                                          rdfs:subClassOf [ rdf:type owl:Restriction ;
                                                                                                            owl:onProperty :EquivalentInjection_ReactiveCapabilityCurve ;
                                                                                                            owl:minQualifiedCardinality "0"^^xsd:nonNegativeInteger ;
                                                                                                            owl:onClass <https://w3id.org/netbeheer/IECCIM/TC57CIM/IEC61970/Base/Equivalents#EquivalentInjection>
                                                                                                          ] .


###  https://w3id.org/netbeheer/IECCIM/TC57CIM/IEC61970/Base/Generation/GenerationTrainingSimulation#PrimeMover
<https://w3id.org/netbeheer/IECCIM/TC57CIM/IEC61970/Base/Generation/GenerationTrainingSimulation#PrimeMover> rdf:type owl:Class ;
                                                                                                             rdfs:subClassOf [ rdf:type owl:Restriction ;
                                                                                                                               owl:onProperty :PrimeMover_SynchronousMachines ;
                                                                                                                               owl:minQualifiedCardinality "0"^^xsd:nonNegativeInteger ;
                                                                                                                               owl:onClass <https://w3id.org/netbeheer/IECCIM/TC57CIM/IEC61970/Base/Generation/GenerationTrainingSimulation#PrimeMover>
                                                                                                                             ] .


###  https://w3id.org/netbeheer/IECCIM/TC57CIM/IEC61970/Base/Generation/Production#GeneratingUnit
<https://w3id.org/netbeheer/IECCIM/TC57CIM/IEC61970/Base/Generation/Production#GeneratingUnit> rdf:type owl:Class ;
                                                                                               rdfs:subClassOf [ rdf:type owl:Restriction ;
                                                                                                                 owl:onProperty :GeneratingUnit_RotatingMachine ;
                                                                                                                 owl:minQualifiedCardinality "0"^^xsd:nonNegativeInteger ;
                                                                                                                 owl:onClass <https://w3id.org/netbeheer/IECCIM/TC57CIM/IEC61970/Base/Generation/Production#GeneratingUnit>
                                                                                                               ] ,
                                                                                                               [ rdf:type owl:Restriction ;
                                                                                                                 owl:onProperty :GeneratingUnit_RotatingMachine ;
                                                                                                                 owl:maxQualifiedCardinality "1"^^xsd:nonNegativeInteger ;
                                                                                                                 owl:onClass <https://w3id.org/netbeheer/IECCIM/TC57CIM/IEC61970/Base/Generation/Production#GeneratingUnit>
                                                                                                               ] .


###  https://w3id.org/netbeheer/IECCIM/TC57CIM/IEC61970/Base/Generation/Production#HydroPump
<https://w3id.org/netbeheer/IECCIM/TC57CIM/IEC61970/Base/Generation/Production#HydroPump> rdf:type owl:Class ;
                                                                                          rdfs:subClassOf [ rdf:type owl:Restriction ;
                                                                                                            owl:onProperty :HydroPump_RotatingMachine ;
                                                                                                            owl:minQualifiedCardinality "0"^^xsd:nonNegativeInteger ;
                                                                                                            owl:onClass <https://w3id.org/netbeheer/IECCIM/TC57CIM/IEC61970/Base/Generation/Production#HydroPump>
                                                                                                          ] ,
                                                                                                          [ rdf:type owl:Restriction ;
                                                                                                            owl:onProperty :HydroPump_RotatingMachine ;
                                                                                                            owl:maxQualifiedCardinality "1"^^xsd:nonNegativeInteger ;
                                                                                                            owl:onClass <https://w3id.org/netbeheer/IECCIM/TC57CIM/IEC61970/Base/Generation/Production#HydroPump>
                                                                                                          ] .


###  https://w3id.org/netbeheer/IECCIM/TC57CIM/IEC61970/Base/LoadModel#LoadResponseCharacteristic
<https://w3id.org/netbeheer/IECCIM/TC57CIM/IEC61970/Base/LoadModel#LoadResponseCharacteristic> rdf:type owl:Class ;
                                                                                               rdfs:subClassOf [ rdf:type owl:Restriction ;
                                                                                                                 owl:onProperty :LoadResponseCharacteristic_EnergyConsumer ;
                                                                                                                 owl:minQualifiedCardinality "0"^^xsd:nonNegativeInteger ;
                                                                                                                 owl:onClass <https://w3id.org/netbeheer/IECCIM/TC57CIM/IEC61970/Base/LoadModel#LoadResponseCharacteristic>
                                                                                                               ] ,
                                                                                                               [ rdf:type owl:Restriction ;
                                                                                                                 owl:onProperty :LoadResponseCharacteristic_EnergyConsumer ;
                                                                                                                 owl:maxQualifiedCardinality "1"^^xsd:nonNegativeInteger ;
                                                                                                                 owl:onClass <https://w3id.org/netbeheer/IECCIM/TC57CIM/IEC61970/Base/LoadModel#LoadResponseCharacteristic>
                                                                                                               ] .


###  https://w3id.org/netbeheer/IECCIM/TC57CIM/IEC61970/Base/LoadModel#PowerCutZone
<https://w3id.org/netbeheer/IECCIM/TC57CIM/IEC61970/Base/LoadModel#PowerCutZone> rdf:type owl:Class ;
                                                                                 rdfs:subClassOf [ rdf:type owl:Restriction ;
                                                                                                   owl:onProperty :PowerCutZone_EnergyConsumers ;
                                                                                                   owl:minQualifiedCardinality "0"^^xsd:nonNegativeInteger ;
                                                                                                   owl:onClass <https://w3id.org/netbeheer/IECCIM/TC57CIM/IEC61970/Base/LoadModel#PowerCutZone>
                                                                                                 ] ,
                                                                                                 [ rdf:type owl:Restriction ;
                                                                                                   owl:onProperty :PowerCutZone_EnergyConsumers ;
                                                                                                   owl:maxQualifiedCardinality "1"^^xsd:nonNegativeInteger ;
                                                                                                   owl:onClass <https://w3id.org/netbeheer/IECCIM/TC57CIM/IEC61970/Base/LoadModel#PowerCutZone>
                                                                                                 ] .


###  https://w3id.org/netbeheer/IECCIM/TC57CIM/IEC61970/Base/LoadModel#SeasonDayTypeSchedule
<https://w3id.org/netbeheer/IECCIM/TC57CIM/IEC61970/Base/LoadModel#SeasonDayTypeSchedule> rdf:type owl:Class .


###  https://w3id.org/netbeheer/IECCIM/TC57CIM/IEC61970/Base/Protection#ProtectionEquipment
<https://w3id.org/netbeheer/IECCIM/TC57CIM/IEC61970/Base/Protection#ProtectionEquipment> rdf:type owl:Class ;
                                                                                         rdfs:subClassOf [ rdf:type owl:Restriction ;
                                                                                                           owl:onProperty :ProtectionEquipment_ProtectedSwitches ;
                                                                                                           owl:minQualifiedCardinality "0"^^xsd:nonNegativeInteger ;
                                                                                                           owl:onClass <https://w3id.org/netbeheer/IECCIM/TC57CIM/IEC61970/Base/Protection#ProtectionEquipment>
                                                                                                         ] .


###  https://w3id.org/netbeheer/IECCIM/TC57CIM/IEC61970/Base/Protection#RecloseSequence
<https://w3id.org/netbeheer/IECCIM/TC57CIM/IEC61970/Base/Protection#RecloseSequence> rdf:type owl:Class ;
                                                                                     rdfs:subClassOf [ rdf:type owl:Restriction ;
                                                                                                       owl:onProperty :RecloseSequence_ProtectedSwitch ;
                                                                                                       owl:minQualifiedCardinality "0"^^xsd:nonNegativeInteger ;
                                                                                                       owl:onClass <https://w3id.org/netbeheer/IECCIM/TC57CIM/IEC61970/Base/Protection#RecloseSequence>
                                                                                                     ] .


###  https://w3id.org/netbeheer/IECCIM/TC57CIM/IEC61970/Base/StateVariables#SvShuntCompensatorSections
<https://w3id.org/netbeheer/IECCIM/TC57CIM/IEC61970/Base/StateVariables#SvShuntCompensatorSections> rdf:type owl:Class ;
                                                                                                    rdfs:subClassOf [ rdf:type owl:Restriction ;
                                                                                                                      owl:onProperty :SvShuntCompensatorSections_ShuntCompensator ;
                                                                                                                      owl:minQualifiedCardinality "0"^^xsd:nonNegativeInteger ;
                                                                                                                      owl:onClass <https://w3id.org/netbeheer/IECCIM/TC57CIM/IEC61970/Base/StateVariables#SvShuntCompensatorSections>
                                                                                                                    ] ,
                                                                                                                    [ rdf:type owl:Restriction ;
                                                                                                                      owl:onProperty :SvShuntCompensatorSections_ShuntCompensator ;
                                                                                                                      owl:maxQualifiedCardinality "1"^^xsd:nonNegativeInteger ;
                                                                                                                      owl:onClass <https://w3id.org/netbeheer/IECCIM/TC57CIM/IEC61970/Base/StateVariables#SvShuntCompensatorSections>
                                                                                                                    ] .


###  https://w3id.org/netbeheer/IECCIM/TC57CIM/IEC61970/Base/StateVariables#SvTapStep
<https://w3id.org/netbeheer/IECCIM/TC57CIM/IEC61970/Base/StateVariables#SvTapStep> rdf:type owl:Class ;
                                                                                   rdfs:subClassOf [ rdf:type owl:Restriction ;
                                                                                                     owl:onProperty :SvTapStep_TapChanger ;
                                                                                                     owl:minQualifiedCardinality "0"^^xsd:nonNegativeInteger ;
                                                                                                     owl:onClass <https://w3id.org/netbeheer/IECCIM/TC57CIM/IEC61970/Base/StateVariables#SvTapStep>
                                                                                                   ] ,
                                                                                                   [ rdf:type owl:Restriction ;
                                                                                                     owl:onProperty :SvTapStep_TapChanger ;
                                                                                                     owl:maxQualifiedCardinality "1"^^xsd:nonNegativeInteger ;
                                                                                                     owl:onClass <https://w3id.org/netbeheer/IECCIM/TC57CIM/IEC61970/Base/StateVariables#SvTapStep>
                                                                                                   ] .


###  https://w3id.org/netbeheer/IECCIM/TC57CIM/IEC61970/Base/Wires#ACLineSegment
:ACLineSegment rdf:type owl:Class ;
               rdfs:subClassOf :Conductor ,
                               [ rdf:type owl:Restriction ;
                                 owl:onProperty :ACLineSegment_LineGroundingAction ;
                                 owl:minQualifiedCardinality "0"^^xsd:nonNegativeInteger ;
                                 owl:onClass :ACLineSegment
                               ] ,
                               [ rdf:type owl:Restriction ;
                                 owl:onProperty :ACLineSegment_LineJumpingAction ;
                                 owl:minQualifiedCardinality "0"^^xsd:nonNegativeInteger ;
                                 owl:onClass :ACLineSegment
                               ] ,
                               [ rdf:type owl:Restriction ;
                                 owl:onProperty :ACLineSegment_PerLengthImpedance ;
                                 owl:minQualifiedCardinality "0"^^xsd:nonNegativeInteger ;
                                 owl:onClass :ACLineSegment
                               ] ,
                               [ rdf:type owl:Restriction ;
                                 owl:onProperty :ACLineSegment_WireSpacing ;
                                 owl:minQualifiedCardinality "0"^^xsd:nonNegativeInteger ;
                                 owl:onClass :ACLineSegment
                               ] ,
                               [ rdf:type owl:Restriction ;
                                 owl:onProperty :ACLineSegment_b0ch ;
                                 owl:minQualifiedCardinality "0"^^xsd:nonNegativeInteger ;
                                 owl:onClass <https://w3id.org/netbeheer/IECCIM/TC57CIM/IEC61970/Base/Domain#Susceptance>
                               ] ,
                               [ rdf:type owl:Restriction ;
                                 owl:onProperty :ACLineSegment_bch ;
                                 owl:minQualifiedCardinality "0"^^xsd:nonNegativeInteger ;
                                 owl:onClass <https://w3id.org/netbeheer/IECCIM/TC57CIM/IEC61970/Base/Domain#Susceptance>
                               ] ,
                               [ rdf:type owl:Restriction ;
                                 owl:onProperty :ACLineSegment_g0ch ;
                                 owl:minQualifiedCardinality "0"^^xsd:nonNegativeInteger ;
                                 owl:onClass <https://w3id.org/netbeheer/IECCIM/TC57CIM/IEC61970/Base/Domain#Conductance>
                               ] ,
                               [ rdf:type owl:Restriction ;
                                 owl:onProperty :ACLineSegment_gch ;
                                 owl:minQualifiedCardinality "0"^^xsd:nonNegativeInteger ;
                                 owl:onClass <https://w3id.org/netbeheer/IECCIM/TC57CIM/IEC61970/Base/Domain#Conductance>
                               ] ,
                               [ rdf:type owl:Restriction ;
                                 owl:onProperty :ACLineSegment_r ;
                                 owl:minQualifiedCardinality "0"^^xsd:nonNegativeInteger ;
                                 owl:onClass <https://w3id.org/netbeheer/IECCIM/TC57CIM/IEC61970/Base/Domain#Resistance>
                               ] ,
                               [ rdf:type owl:Restriction ;
                                 owl:onProperty :ACLineSegment_r0 ;
                                 owl:minQualifiedCardinality "0"^^xsd:nonNegativeInteger ;
                                 owl:onClass <https://w3id.org/netbeheer/IECCIM/TC57CIM/IEC61970/Base/Domain#Resistance>
                               ] ,
                               [ rdf:type owl:Restriction ;
                                 owl:onProperty :ACLineSegment_shortCircuitEndTemperature ;
                                 owl:minQualifiedCardinality "0"^^xsd:nonNegativeInteger ;
                                 owl:onClass <https://w3id.org/netbeheer/IECCIM/TC57CIM/IEC61970/Base/Domain#Temperature>
                               ] ,
                               [ rdf:type owl:Restriction ;
                                 owl:onProperty :ACLineSegment_x ;
                                 owl:minQualifiedCardinality "0"^^xsd:nonNegativeInteger ;
                                 owl:onClass <https://w3id.org/netbeheer/IECCIM/TC57CIM/IEC61970/Base/Domain#Reactance>
                               ] ,
                               [ rdf:type owl:Restriction ;
                                 owl:onProperty :ACLineSegment_x0 ;
                                 owl:minQualifiedCardinality "0"^^xsd:nonNegativeInteger ;
                                 owl:onClass <https://w3id.org/netbeheer/IECCIM/TC57CIM/IEC61970/Base/Domain#Reactance>
                               ] ,
                               [ rdf:type owl:Restriction ;
                                 owl:onProperty :ACLineSegment_ACLineSegmentPhases ;
                                 owl:qualifiedCardinality "1"^^xsd:nonNegativeInteger ;
                                 owl:onClass :ACLineSegment
                               ] ,
                               [ rdf:type owl:Restriction ;
                                 owl:onProperty :ACLineSegment_Clamp ;
                                 owl:qualifiedCardinality "1"^^xsd:nonNegativeInteger ;
                                 owl:onClass :ACLineSegment
                               ] ,
                               [ rdf:type owl:Restriction ;
                                 owl:onProperty :ACLineSegment_Cut ;
                                 owl:qualifiedCardinality "1"^^xsd:nonNegativeInteger ;
                                 owl:onClass :ACLineSegment
                               ] ,
                               [ rdf:type owl:Restriction ;
                                 owl:onProperty :ACLineSegment_LineGroundingAction ;
                                 owl:maxQualifiedCardinality "1"^^xsd:nonNegativeInteger ;
                                 owl:onClass :ACLineSegment
                               ] ,
                               [ rdf:type owl:Restriction ;
                                 owl:onProperty :ACLineSegment_b0ch ;
                                 owl:maxQualifiedCardinality "1"^^xsd:nonNegativeInteger ;
                                 owl:onClass <https://w3id.org/netbeheer/IECCIM/TC57CIM/IEC61970/Base/Domain#Susceptance>
                               ] ,
                               [ rdf:type owl:Restriction ;
                                 owl:onProperty :ACLineSegment_bch ;
                                 owl:maxQualifiedCardinality "1"^^xsd:nonNegativeInteger ;
                                 owl:onClass <https://w3id.org/netbeheer/IECCIM/TC57CIM/IEC61970/Base/Domain#Susceptance>
                               ] ,
                               [ rdf:type owl:Restriction ;
                                 owl:onProperty :ACLineSegment_g0ch ;
                                 owl:maxQualifiedCardinality "1"^^xsd:nonNegativeInteger ;
                                 owl:onClass <https://w3id.org/netbeheer/IECCIM/TC57CIM/IEC61970/Base/Domain#Conductance>
                               ] ,
                               [ rdf:type owl:Restriction ;
                                 owl:onProperty :ACLineSegment_gch ;
                                 owl:maxQualifiedCardinality "1"^^xsd:nonNegativeInteger ;
                                 owl:onClass <https://w3id.org/netbeheer/IECCIM/TC57CIM/IEC61970/Base/Domain#Conductance>
                               ] ,
                               [ rdf:type owl:Restriction ;
                                 owl:onProperty :ACLineSegment_r ;
                                 owl:maxQualifiedCardinality "1"^^xsd:nonNegativeInteger ;
                                 owl:onClass <https://w3id.org/netbeheer/IECCIM/TC57CIM/IEC61970/Base/Domain#Resistance>
                               ] ,
                               [ rdf:type owl:Restriction ;
                                 owl:onProperty :ACLineSegment_r0 ;
                                 owl:maxQualifiedCardinality "1"^^xsd:nonNegativeInteger ;
                                 owl:onClass <https://w3id.org/netbeheer/IECCIM/TC57CIM/IEC61970/Base/Domain#Resistance>
                               ] ,
                               [ rdf:type owl:Restriction ;
                                 owl:onProperty :ACLineSegment_shortCircuitEndTemperature ;
                                 owl:maxQualifiedCardinality "1"^^xsd:nonNegativeInteger ;
                                 owl:onClass <https://w3id.org/netbeheer/IECCIM/TC57CIM/IEC61970/Base/Domain#Temperature>
                               ] ,
                               [ rdf:type owl:Restriction ;
                                 owl:onProperty :ACLineSegment_x ;
                                 owl:maxQualifiedCardinality "1"^^xsd:nonNegativeInteger ;
                                 owl:onClass <https://w3id.org/netbeheer/IECCIM/TC57CIM/IEC61970/Base/Domain#Reactance>
                               ] ,
                               [ rdf:type owl:Restriction ;
                                 owl:onProperty :ACLineSegment_x0 ;
                                 owl:maxQualifiedCardinality "1"^^xsd:nonNegativeInteger ;
                                 owl:onClass <https://w3id.org/netbeheer/IECCIM/TC57CIM/IEC61970/Base/Domain#Reactance>
                               ] ;
               rdfs:comment """A wire or combination of wires, with consistent electrical characteristics, building a single electrical system, used to carry alternating current between points in the power system.
For symmetrical, transposed 3ph lines, it is sufficient to use  attributes of the line segment, which describe impedances and admittances for the entire length of the segment.  Additionally impedances can be computed by using length and associated per length impedances.
The BaseVoltage at the two ends of ACLineSegments in a Line shall have the same BaseVoltage.nominalVoltage. However, boundary lines  may have slightly different BaseVoltage.nominalVoltages and  variation is allowed. Larger voltage difference in general requires use of an equivalent branch.""" .


###  https://w3id.org/netbeheer/IECCIM/TC57CIM/IEC61970/Base/Wires#ACLineSegmentPhase
:ACLineSegmentPhase rdf:type owl:Class ;
                    rdfs:subClassOf <https://w3id.org/netbeheer/IECCIM/TC57CIM/IEC61970/Base/Core#PowerSystemResource> ,
                                    [ rdf:type owl:Restriction ;
                                      owl:onProperty :ACLineSegmentPhase_ACLineSegment ;
                                      owl:minQualifiedCardinality "0"^^xsd:nonNegativeInteger ;
                                      owl:onClass :ACLineSegmentPhase
                                    ] ,
                                    [ rdf:type owl:Restriction ;
                                      owl:onProperty :ACLineSegmentPhase_phase ;
                                      owl:minQualifiedCardinality "0"^^xsd:nonNegativeInteger ;
                                      owl:onDataRange :SinglePhaseKind
                                    ] ,
                                    [ rdf:type owl:Restriction ;
                                      owl:onProperty :ACLineSegmentPhase_sequenceNumber ;
                                      owl:minQualifiedCardinality "0"^^xsd:nonNegativeInteger ;
                                      owl:onDataRange xsd:nonNegativeInteger
                                    ] ,
                                    [ rdf:type owl:Restriction ;
                                      owl:onProperty :ACLineSegmentPhase_phase ;
                                      owl:maxQualifiedCardinality "1"^^xsd:nonNegativeInteger ;
                                      owl:onDataRange :SinglePhaseKind
                                    ] ,
                                    [ rdf:type owl:Restriction ;
                                      owl:onProperty :ACLineSegmentPhase_sequenceNumber ;
                                      owl:maxQualifiedCardinality "1"^^xsd:nonNegativeInteger ;
                                      owl:onDataRange xsd:nonNegativeInteger
                                    ] ;
                    rdfs:comment """Represents a single wire of an alternating current line segment.
""" .


###  https://w3id.org/netbeheer/IECCIM/TC57CIM/IEC61970/Base/Wires#AsynchronousMachine
:AsynchronousMachine rdf:type owl:Class ;
                     rdfs:subClassOf :RotatingMachine ,
                                     [ rdf:type owl:Restriction ;
                                       owl:onProperty :AsynchronousMachine_efficiency ;
                                       owl:minQualifiedCardinality "0"^^xsd:nonNegativeInteger ;
                                       owl:onClass <https://w3id.org/netbeheer/IECCIM/TC57CIM/IEC61970/Base/Domain#PerCent>
                                     ] ,
                                     [ rdf:type owl:Restriction ;
                                       owl:onProperty :AsynchronousMachine_nominalFrequency ;
                                       owl:minQualifiedCardinality "0"^^xsd:nonNegativeInteger ;
                                       owl:onClass <https://w3id.org/netbeheer/IECCIM/TC57CIM/IEC61970/Base/Domain#Frequency>
                                     ] ,
                                     [ rdf:type owl:Restriction ;
                                       owl:onProperty :AsynchronousMachine_nominalSpeed ;
                                       owl:minQualifiedCardinality "0"^^xsd:nonNegativeInteger ;
                                       owl:onClass <https://w3id.org/netbeheer/IECCIM/TC57CIM/IEC61970/Base/Domain#RotationSpeed>
                                     ] ,
                                     [ rdf:type owl:Restriction ;
                                       owl:onProperty :AsynchronousMachine_ratedMechanicalPower ;
                                       owl:minQualifiedCardinality "0"^^xsd:nonNegativeInteger ;
                                       owl:onClass <https://w3id.org/netbeheer/IECCIM/TC57CIM/IEC61970/Base/Domain#ActivePower>
                                     ] ,
                                     [ rdf:type owl:Restriction ;
                                       owl:onProperty :AsynchronousMachine_rr1 ;
                                       owl:minQualifiedCardinality "0"^^xsd:nonNegativeInteger ;
                                       owl:onClass <https://w3id.org/netbeheer/IECCIM/TC57CIM/IEC61970/Base/Domain#Resistance>
                                     ] ,
                                     [ rdf:type owl:Restriction ;
                                       owl:onProperty :AsynchronousMachine_rr2 ;
                                       owl:minQualifiedCardinality "0"^^xsd:nonNegativeInteger ;
                                       owl:onClass <https://w3id.org/netbeheer/IECCIM/TC57CIM/IEC61970/Base/Domain#Resistance>
                                     ] ,
                                     [ rdf:type owl:Restriction ;
                                       owl:onProperty :AsynchronousMachine_tpo ;
                                       owl:minQualifiedCardinality "0"^^xsd:nonNegativeInteger ;
                                       owl:onClass <https://w3id.org/netbeheer/IECCIM/TC57CIM/IEC61970/Base/Domain#Seconds>
                                     ] ,
                                     [ rdf:type owl:Restriction ;
                                       owl:onProperty :AsynchronousMachine_tppo ;
                                       owl:minQualifiedCardinality "0"^^xsd:nonNegativeInteger ;
                                       owl:onClass <https://w3id.org/netbeheer/IECCIM/TC57CIM/IEC61970/Base/Domain#Seconds>
                                     ] ,
                                     [ rdf:type owl:Restriction ;
                                       owl:onProperty :AsynchronousMachine_xlr1 ;
                                       owl:minQualifiedCardinality "0"^^xsd:nonNegativeInteger ;
                                       owl:onClass <https://w3id.org/netbeheer/IECCIM/TC57CIM/IEC61970/Base/Domain#Reactance>
                                     ] ,
                                     [ rdf:type owl:Restriction ;
                                       owl:onProperty :AsynchronousMachine_xlr2 ;
                                       owl:minQualifiedCardinality "0"^^xsd:nonNegativeInteger ;
                                       owl:onClass <https://w3id.org/netbeheer/IECCIM/TC57CIM/IEC61970/Base/Domain#Reactance>
                                     ] ,
                                     [ rdf:type owl:Restriction ;
                                       owl:onProperty :AsynchronousMachine_xm ;
                                       owl:minQualifiedCardinality "0"^^xsd:nonNegativeInteger ;
                                       owl:onClass <https://w3id.org/netbeheer/IECCIM/TC57CIM/IEC61970/Base/Domain#Reactance>
                                     ] ,
                                     [ rdf:type owl:Restriction ;
                                       owl:onProperty :AsynchronousMachine_xp ;
                                       owl:minQualifiedCardinality "0"^^xsd:nonNegativeInteger ;
                                       owl:onClass <https://w3id.org/netbeheer/IECCIM/TC57CIM/IEC61970/Base/Domain#Reactance>
                                     ] ,
                                     [ rdf:type owl:Restriction ;
                                       owl:onProperty :AsynchronousMachine_xpp ;
                                       owl:minQualifiedCardinality "0"^^xsd:nonNegativeInteger ;
                                       owl:onClass <https://w3id.org/netbeheer/IECCIM/TC57CIM/IEC61970/Base/Domain#Reactance>
                                     ] ,
                                     [ rdf:type owl:Restriction ;
                                       owl:onProperty :AsynchronousMachine_xs ;
                                       owl:minQualifiedCardinality "0"^^xsd:nonNegativeInteger ;
                                       owl:onClass <https://w3id.org/netbeheer/IECCIM/TC57CIM/IEC61970/Base/Domain#Reactance>
                                     ] ,
                                     [ rdf:type owl:Restriction ;
                                       owl:onProperty :AsynchronousMachine_AsynchronousMachineDynamics ;
                                       owl:qualifiedCardinality "1"^^xsd:nonNegativeInteger ;
                                       owl:onClass :AsynchronousMachine
                                     ] ,
                                     [ rdf:type owl:Restriction ;
                                       owl:onProperty :AsynchronousMachine_efficiency ;
                                       owl:maxQualifiedCardinality "1"^^xsd:nonNegativeInteger ;
                                       owl:onClass <https://w3id.org/netbeheer/IECCIM/TC57CIM/IEC61970/Base/Domain#PerCent>
                                     ] ,
                                     [ rdf:type owl:Restriction ;
                                       owl:onProperty :AsynchronousMachine_nominalFrequency ;
                                       owl:maxQualifiedCardinality "1"^^xsd:nonNegativeInteger ;
                                       owl:onClass <https://w3id.org/netbeheer/IECCIM/TC57CIM/IEC61970/Base/Domain#Frequency>
                                     ] ,
                                     [ rdf:type owl:Restriction ;
                                       owl:onProperty :AsynchronousMachine_nominalSpeed ;
                                       owl:maxQualifiedCardinality "1"^^xsd:nonNegativeInteger ;
                                       owl:onClass <https://w3id.org/netbeheer/IECCIM/TC57CIM/IEC61970/Base/Domain#RotationSpeed>
                                     ] ,
                                     [ rdf:type owl:Restriction ;
                                       owl:onProperty :AsynchronousMachine_ratedMechanicalPower ;
                                       owl:maxQualifiedCardinality "1"^^xsd:nonNegativeInteger ;
                                       owl:onClass <https://w3id.org/netbeheer/IECCIM/TC57CIM/IEC61970/Base/Domain#ActivePower>
                                     ] ,
                                     [ rdf:type owl:Restriction ;
                                       owl:onProperty :AsynchronousMachine_rr1 ;
                                       owl:maxQualifiedCardinality "1"^^xsd:nonNegativeInteger ;
                                       owl:onClass <https://w3id.org/netbeheer/IECCIM/TC57CIM/IEC61970/Base/Domain#Resistance>
                                     ] ,
                                     [ rdf:type owl:Restriction ;
                                       owl:onProperty :AsynchronousMachine_rr2 ;
                                       owl:maxQualifiedCardinality "1"^^xsd:nonNegativeInteger ;
                                       owl:onClass <https://w3id.org/netbeheer/IECCIM/TC57CIM/IEC61970/Base/Domain#Resistance>
                                     ] ,
                                     [ rdf:type owl:Restriction ;
                                       owl:onProperty :AsynchronousMachine_tpo ;
                                       owl:maxQualifiedCardinality "1"^^xsd:nonNegativeInteger ;
                                       owl:onClass <https://w3id.org/netbeheer/IECCIM/TC57CIM/IEC61970/Base/Domain#Seconds>
                                     ] ,
                                     [ rdf:type owl:Restriction ;
                                       owl:onProperty :AsynchronousMachine_tppo ;
                                       owl:maxQualifiedCardinality "1"^^xsd:nonNegativeInteger ;
                                       owl:onClass <https://w3id.org/netbeheer/IECCIM/TC57CIM/IEC61970/Base/Domain#Seconds>
                                     ] ,
                                     [ rdf:type owl:Restriction ;
                                       owl:onProperty :AsynchronousMachine_xlr1 ;
                                       owl:maxQualifiedCardinality "1"^^xsd:nonNegativeInteger ;
                                       owl:onClass <https://w3id.org/netbeheer/IECCIM/TC57CIM/IEC61970/Base/Domain#Reactance>
                                     ] ,
                                     [ rdf:type owl:Restriction ;
                                       owl:onProperty :AsynchronousMachine_xlr2 ;
                                       owl:maxQualifiedCardinality "1"^^xsd:nonNegativeInteger ;
                                       owl:onClass <https://w3id.org/netbeheer/IECCIM/TC57CIM/IEC61970/Base/Domain#Reactance>
                                     ] ,
                                     [ rdf:type owl:Restriction ;
                                       owl:onProperty :AsynchronousMachine_xm ;
                                       owl:maxQualifiedCardinality "1"^^xsd:nonNegativeInteger ;
                                       owl:onClass <https://w3id.org/netbeheer/IECCIM/TC57CIM/IEC61970/Base/Domain#Reactance>
                                     ] ,
                                     [ rdf:type owl:Restriction ;
                                       owl:onProperty :AsynchronousMachine_xp ;
                                       owl:maxQualifiedCardinality "1"^^xsd:nonNegativeInteger ;
                                       owl:onClass <https://w3id.org/netbeheer/IECCIM/TC57CIM/IEC61970/Base/Domain#Reactance>
                                     ] ,
                                     [ rdf:type owl:Restriction ;
                                       owl:onProperty :AsynchronousMachine_xpp ;
                                       owl:maxQualifiedCardinality "1"^^xsd:nonNegativeInteger ;
                                       owl:onClass <https://w3id.org/netbeheer/IECCIM/TC57CIM/IEC61970/Base/Domain#Reactance>
                                     ] ,
                                     [ rdf:type owl:Restriction ;
                                       owl:onProperty :AsynchronousMachine_xs ;
                                       owl:maxQualifiedCardinality "1"^^xsd:nonNegativeInteger ;
                                       owl:onClass <https://w3id.org/netbeheer/IECCIM/TC57CIM/IEC61970/Base/Domain#Reactance>
                                     ] ,
                                     [ rdf:type owl:Restriction ;
                                       owl:onProperty :AsynchronousMachine_asynchronousMachineType ;
                                       owl:minQualifiedCardinality "0"^^xsd:nonNegativeInteger ;
                                       owl:onDataRange :AsynchronousMachineKind
                                     ] ,
                                     [ rdf:type owl:Restriction ;
                                       owl:onProperty :AsynchronousMachine_converterFedDrive ;
                                       owl:minQualifiedCardinality "0"^^xsd:nonNegativeInteger ;
                                       owl:onDataRange xsd:boolean
                                     ] ,
                                     [ rdf:type owl:Restriction ;
                                       owl:onProperty :AsynchronousMachine_iaIrRatio ;
                                       owl:minQualifiedCardinality "0"^^xsd:nonNegativeInteger ;
                                       owl:onDataRange xsd:float
                                     ] ,
                                     [ rdf:type owl:Restriction ;
                                       owl:onProperty :AsynchronousMachine_polePairNumber ;
                                       owl:minQualifiedCardinality "0"^^xsd:nonNegativeInteger ;
                                       owl:onDataRange xsd:nonNegativeInteger
                                     ] ,
                                     [ rdf:type owl:Restriction ;
                                       owl:onProperty :AsynchronousMachine_reversible ;
                                       owl:minQualifiedCardinality "0"^^xsd:nonNegativeInteger ;
                                       owl:onDataRange xsd:boolean
                                     ] ,
                                     [ rdf:type owl:Restriction ;
                                       owl:onProperty :AsynchronousMachine_rxLockedRotorRatio ;
                                       owl:minQualifiedCardinality "0"^^xsd:nonNegativeInteger ;
                                       owl:onDataRange xsd:float
                                     ] ,
                                     [ rdf:type owl:Restriction ;
                                       owl:onProperty :AsynchronousMachine_asynchronousMachineType ;
                                       owl:maxQualifiedCardinality "1"^^xsd:nonNegativeInteger ;
                                       owl:onDataRange :AsynchronousMachineKind
                                     ] ,
                                     [ rdf:type owl:Restriction ;
                                       owl:onProperty :AsynchronousMachine_converterFedDrive ;
                                       owl:maxQualifiedCardinality "1"^^xsd:nonNegativeInteger ;
                                       owl:onDataRange xsd:boolean
                                     ] ,
                                     [ rdf:type owl:Restriction ;
                                       owl:onProperty :AsynchronousMachine_iaIrRatio ;
                                       owl:maxQualifiedCardinality "1"^^xsd:nonNegativeInteger ;
                                       owl:onDataRange xsd:float
                                     ] ,
                                     [ rdf:type owl:Restriction ;
                                       owl:onProperty :AsynchronousMachine_polePairNumber ;
                                       owl:maxQualifiedCardinality "1"^^xsd:nonNegativeInteger ;
                                       owl:onDataRange xsd:nonNegativeInteger
                                     ] ,
                                     [ rdf:type owl:Restriction ;
                                       owl:onProperty :AsynchronousMachine_reversible ;
                                       owl:maxQualifiedCardinality "1"^^xsd:nonNegativeInteger ;
                                       owl:onDataRange xsd:boolean
                                     ] ,
                                     [ rdf:type owl:Restriction ;
                                       owl:onProperty :AsynchronousMachine_rxLockedRotorRatio ;
                                       owl:maxQualifiedCardinality "1"^^xsd:nonNegativeInteger ;
                                       owl:onDataRange xsd:float
                                     ] ;
                     rdfs:comment "A rotating machine whose shaft rotates asynchronously with the electrical field.  Also known as an induction machine with no external connection to the rotor windings, e.g squirrel-cage induction machine." .


###  https://w3id.org/netbeheer/IECCIM/TC57CIM/IEC61970/Base/Wires#Breaker
:Breaker rdf:type owl:Class ;
         rdfs:subClassOf :ProtectedSwitch ,
                         [ rdf:type owl:Restriction ;
                           owl:onProperty :Breaker_inTransitTime ;
                           owl:minQualifiedCardinality "0"^^xsd:nonNegativeInteger ;
                           owl:onClass <https://w3id.org/netbeheer/IECCIM/TC57CIM/IEC61970/Base/Domain#Seconds>
                         ] ,
                         [ rdf:type owl:Restriction ;
                           owl:onProperty :Breaker_inTransitTime ;
                           owl:maxQualifiedCardinality "1"^^xsd:nonNegativeInteger ;
                           owl:onClass <https://w3id.org/netbeheer/IECCIM/TC57CIM/IEC61970/Base/Domain#Seconds>
                         ] ;
         rdfs:comment "A mechanical switching device capable of making, carrying, and breaking currents under normal circuit conditions and also making, carrying for a specified time, and breaking currents under specified abnormal circuit conditions e.g.  those of short circuit." .


###  https://w3id.org/netbeheer/IECCIM/TC57CIM/IEC61970/Base/Wires#BusbarSection
:BusbarSection rdf:type owl:Class ;
               rdfs:subClassOf :Connector ,
                               [ rdf:type owl:Restriction ;
                                 owl:onProperty :BusbarSection_ipMax ;
                                 owl:minQualifiedCardinality "0"^^xsd:nonNegativeInteger ;
                                 owl:onClass <https://w3id.org/netbeheer/IECCIM/TC57CIM/IEC61970/Base/Domain#CurrentFlow>
                               ] ,
                               [ rdf:type owl:Restriction ;
                                 owl:onProperty :BusbarSection_VoltageControlZone ;
                                 owl:qualifiedCardinality "1"^^xsd:nonNegativeInteger ;
                                 owl:onClass :BusbarSection
                               ] ,
                               [ rdf:type owl:Restriction ;
                                 owl:onProperty :BusbarSection_ipMax ;
                                 owl:maxQualifiedCardinality "1"^^xsd:nonNegativeInteger ;
                                 owl:onClass <https://w3id.org/netbeheer/IECCIM/TC57CIM/IEC61970/Base/Domain#CurrentFlow>
                               ] ;
               rdfs:comment """A conductor, or group of conductors, with negligible impedance, that serve to connect other conducting equipment within a single substation. 
Voltage measurements are typically obtained from VoltageTransformers that are connected to busbar sections. A bus bar section may have many physical terminals but for analysis is modelled with exactly one logical terminal.""" .


###  https://w3id.org/netbeheer/IECCIM/TC57CIM/IEC61970/Base/Wires#Clamp
:Clamp rdf:type owl:Class ;
       rdfs:subClassOf <https://w3id.org/netbeheer/IECCIM/TC57CIM/IEC61970/Base/Core#ConductingEquipment> ,
                       [ rdf:type owl:Restriction ;
                         owl:onProperty :Clamp_ACLineSegment ;
                         owl:minQualifiedCardinality "0"^^xsd:nonNegativeInteger ;
                         owl:onClass :Clamp
                       ] ,
                       [ rdf:type owl:Restriction ;
                         owl:onProperty :Clamp_lengthFromTerminal1 ;
                         owl:minQualifiedCardinality "0"^^xsd:nonNegativeInteger ;
                         owl:onClass <https://w3id.org/netbeheer/IECCIM/TC57CIM/IEC61970/Base/Domain#Length>
                       ] ,
                       [ rdf:type owl:Restriction ;
                         owl:onProperty :Clamp_lengthFromTerminal1 ;
                         owl:maxQualifiedCardinality "1"^^xsd:nonNegativeInteger ;
                         owl:onClass <https://w3id.org/netbeheer/IECCIM/TC57CIM/IEC61970/Base/Domain#Length>
                       ] ;
       rdfs:comment """A Clamp is a galvanic connection at a line segment where other equipment is connected. A Clamp does not cut the line segment. 
A Clamp is ConductingEquipment and has one Terminal with an associated ConnectivityNode. Any other ConductingEquipment can be connected to the Clamp ConnectivityNode.
""" .


###  https://w3id.org/netbeheer/IECCIM/TC57CIM/IEC61970/Base/Wires#CompositeSwitch
:CompositeSwitch rdf:type owl:Class ;
                 rdfs:subClassOf <https://w3id.org/netbeheer/IECCIM/TC57CIM/IEC61970/Base/Core#Equipment> ,
                                 [ rdf:type owl:Restriction ;
                                   owl:onProperty :CompositeSwitch_Switches ;
                                   owl:minQualifiedCardinality "0"^^xsd:nonNegativeInteger ;
                                   owl:onClass :CompositeSwitch
                                 ] ,
                                 [ rdf:type owl:Restriction ;
                                   owl:onProperty :CompositeSwitch_Switches ;
                                   owl:maxQualifiedCardinality "1"^^xsd:nonNegativeInteger ;
                                   owl:onClass :CompositeSwitch
                                 ] ,
                                 [ rdf:type owl:Restriction ;
                                   owl:onProperty :CompositeSwitch_compositeSwitchType ;
                                   owl:minQualifiedCardinality "0"^^xsd:nonNegativeInteger ;
                                   owl:onDataRange xsd:string
                                 ] ,
                                 [ rdf:type owl:Restriction ;
                                   owl:onProperty :CompositeSwitch_compositeSwitchType ;
                                   owl:maxQualifiedCardinality "1"^^xsd:nonNegativeInteger ;
                                   owl:onDataRange xsd:string
                                 ] ;
                 rdfs:comment """A model of a set of individual Switches normally enclosed within the same cabinet and possibly with interlocks that restrict the combination of switch positions. These are typically found in medium voltage distribution networks. 
A CompositeSwitch could represent a Ring-Main-Unit (RMU), or pad-mounted switchgear, with primitive internal devices such as an internal bus-bar plus 3 or 4 internal switches each of which may individually be open or closed. A CompositeSwitch and a set of contained Switches can also be used to represent a multi-position switch e.g. a switch that can connect a circuit to Ground, Open or Busbar.""" .


###  https://w3id.org/netbeheer/IECCIM/TC57CIM/IEC61970/Base/Wires#Conductor
:Conductor rdf:type owl:Class ;
           rdfs:subClassOf <https://w3id.org/netbeheer/IECCIM/TC57CIM/IEC61970/Base/Core#ConductingEquipment> ,
                           [ rdf:type owl:Restriction ;
                             owl:onProperty :Conductor_length ;
                             owl:minQualifiedCardinality "0"^^xsd:nonNegativeInteger ;
                             owl:onClass <https://w3id.org/netbeheer/IECCIM/TC57CIM/IEC61970/Base/Domain#Length>
                           ] ,
                           [ rdf:type owl:Restriction ;
                             owl:onProperty :Conductor_length ;
                             owl:maxQualifiedCardinality "1"^^xsd:nonNegativeInteger ;
                             owl:onClass <https://w3id.org/netbeheer/IECCIM/TC57CIM/IEC61970/Base/Domain#Length>
                           ] ;
           rdfs:comment "Combination of conducting material with consistent electrical characteristics, building a single electrical system, used to carry current between points in the power system.  " .


###  https://w3id.org/netbeheer/IECCIM/TC57CIM/IEC61970/Base/Wires#Connector
:Connector rdf:type owl:Class ;
           rdfs:subClassOf <https://w3id.org/netbeheer/IECCIM/TC57CIM/IEC61970/Base/Core#ConductingEquipment> ;
           rdfs:comment "A conductor, or group of conductors, with negligible impedance, that serve to connect other conducting equipment within a single substation and are modelled with a single logical terminal." .


###  https://w3id.org/netbeheer/IECCIM/TC57CIM/IEC61970/Base/Wires#Cut
:Cut rdf:type owl:Class ;
     rdfs:subClassOf :Switch ,
                     [ rdf:type owl:Restriction ;
                       owl:onProperty :Cut_ACLineSegment ;
                       owl:minQualifiedCardinality "0"^^xsd:nonNegativeInteger ;
                       owl:onClass :Cut
                     ] ,
                     [ rdf:type owl:Restriction ;
                       owl:onProperty :Cut_CutAction ;
                       owl:minQualifiedCardinality "0"^^xsd:nonNegativeInteger ;
                       owl:onClass :Cut
                     ] ,
                     [ rdf:type owl:Restriction ;
                       owl:onProperty :Cut_lengthFromTerminal1 ;
                       owl:minQualifiedCardinality "0"^^xsd:nonNegativeInteger ;
                       owl:onClass <https://w3id.org/netbeheer/IECCIM/TC57CIM/IEC61970/Base/Domain#Length>
                     ] ,
                     [ rdf:type owl:Restriction ;
                       owl:onProperty :Cut_CutAction ;
                       owl:maxQualifiedCardinality "1"^^xsd:nonNegativeInteger ;
                       owl:onClass :Cut
                     ] ,
                     [ rdf:type owl:Restriction ;
                       owl:onProperty :Cut_lengthFromTerminal1 ;
                       owl:maxQualifiedCardinality "1"^^xsd:nonNegativeInteger ;
                       owl:onClass <https://w3id.org/netbeheer/IECCIM/TC57CIM/IEC61970/Base/Domain#Length>
                     ] ;
     rdfs:comment """A cut separates a line segment into two parts. The cut appears as a switch inserted between these two parts and connects them together. As the cut is normally open there is no galvanic connection between the two line segment parts. But it is possible to close the cut to get galvanic connection.
The cut terminals are oriented towards the line segment terminals with the same sequence number. Hence the cut terminal with sequence number equal to 1 is oriented to the line segment's terminal with sequence number equal to 1.
The cut terminals also act as connection points for jumpers and other equipment, e.g. a mobile generator. To enable this, connectivity nodes are placed at the cut terminals. Once the connectivity nodes are in place any conducting equipment can be connected at them.
""" .


###  https://w3id.org/netbeheer/IECCIM/TC57CIM/IEC61970/Base/Wires#Disconnector
:Disconnector rdf:type owl:Class ;
              rdfs:subClassOf :Switch ;
              rdfs:comment "A manually operated or motor operated mechanical switching device used for changing the connections in a circuit, or for isolating a circuit or equipment from a source of power. It is required to open or close circuits when negligible current is broken or made. " .


###  https://w3id.org/netbeheer/IECCIM/TC57CIM/IEC61970/Base/Wires#EarthFaultCompensator
:EarthFaultCompensator rdf:type owl:Class ;
                       rdfs:subClassOf <https://w3id.org/netbeheer/IECCIM/TC57CIM/IEC61970/Base/Core#ConductingEquipment> ,
                                       [ rdf:type owl:Restriction ;
                                         owl:onProperty :EarthFaultCompensator_r ;
                                         owl:minQualifiedCardinality "0"^^xsd:nonNegativeInteger ;
                                         owl:onClass <https://w3id.org/netbeheer/IECCIM/TC57CIM/IEC61970/Base/Domain#Resistance>
                                       ] ,
                                       [ rdf:type owl:Restriction ;
                                         owl:onProperty :EarthFaultCompensator_r ;
                                         owl:maxQualifiedCardinality "1"^^xsd:nonNegativeInteger ;
                                         owl:onClass <https://w3id.org/netbeheer/IECCIM/TC57CIM/IEC61970/Base/Domain#Resistance>
                                       ] ;
                       rdfs:comment "A conducting equipment used to represent a connection to ground which is typically used to compensate earth faults..   An earth fault compensator device modeled with a single terminal implies a second terminal solidly connected to ground.  If two terminals are modeled, the ground is not assumed and normal connection rules apply." .


###  https://w3id.org/netbeheer/IECCIM/TC57CIM/IEC61970/Base/Wires#EnergyConsumer
:EnergyConsumer rdf:type owl:Class ;
                rdfs:subClassOf <https://w3id.org/netbeheer/IECCIM/TC57CIM/IEC61970/Base/Core#ConductingEquipment> ,
                                [ rdf:type owl:Restriction ;
                                  owl:onProperty :EnergyConsumer_LoadDynamics ;
                                  owl:minQualifiedCardinality "0"^^xsd:nonNegativeInteger ;
                                  owl:onClass :EnergyConsumer
                                ] ,
                                [ rdf:type owl:Restriction ;
                                  owl:onProperty :EnergyConsumer_LoadResponse ;
                                  owl:minQualifiedCardinality "0"^^xsd:nonNegativeInteger ;
                                  owl:onClass :EnergyConsumer
                                ] ,
                                [ rdf:type owl:Restriction ;
                                  owl:onProperty :EnergyConsumer_PowerCutZone ;
                                  owl:minQualifiedCardinality "1"^^xsd:nonNegativeInteger ;
                                  owl:onClass :EnergyConsumer
                                ] ,
                                [ rdf:type owl:Restriction ;
                                  owl:onProperty :EnergyConsumer_p ;
                                  owl:minQualifiedCardinality "0"^^xsd:nonNegativeInteger ;
                                  owl:onClass <https://w3id.org/netbeheer/IECCIM/TC57CIM/IEC61970/Base/Domain#ActivePower>
                                ] ,
                                [ rdf:type owl:Restriction ;
                                  owl:onProperty :EnergyConsumer_pfixed ;
                                  owl:minQualifiedCardinality "0"^^xsd:nonNegativeInteger ;
                                  owl:onClass <https://w3id.org/netbeheer/IECCIM/TC57CIM/IEC61970/Base/Domain#ActivePower>
                                ] ,
                                [ rdf:type owl:Restriction ;
                                  owl:onProperty :EnergyConsumer_pfixedPct ;
                                  owl:minQualifiedCardinality "0"^^xsd:nonNegativeInteger ;
                                  owl:onClass <https://w3id.org/netbeheer/IECCIM/TC57CIM/IEC61970/Base/Domain#PerCent>
                                ] ,
                                [ rdf:type owl:Restriction ;
                                  owl:onProperty :EnergyConsumer_q ;
                                  owl:minQualifiedCardinality "0"^^xsd:nonNegativeInteger ;
                                  owl:onClass <https://w3id.org/netbeheer/IECCIM/TC57CIM/IEC61970/Base/Domain#ReactivePower>
                                ] ,
                                [ rdf:type owl:Restriction ;
                                  owl:onProperty :EnergyConsumer_qfixed ;
                                  owl:minQualifiedCardinality "0"^^xsd:nonNegativeInteger ;
                                  owl:onClass <https://w3id.org/netbeheer/IECCIM/TC57CIM/IEC61970/Base/Domain#ReactivePower>
                                ] ,
                                [ rdf:type owl:Restriction ;
                                  owl:onProperty :EnergyConsumer_qfixedPct ;
                                  owl:minQualifiedCardinality "0"^^xsd:nonNegativeInteger ;
                                  owl:onClass <https://w3id.org/netbeheer/IECCIM/TC57CIM/IEC61970/Base/Domain#PerCent>
                                ] ,
                                [ rdf:type owl:Restriction ;
                                  owl:onProperty :EnergyConsumer_EnergyConsumerPhase ;
                                  owl:qualifiedCardinality "1"^^xsd:nonNegativeInteger ;
                                  owl:onClass :EnergyConsumer
                                ] ,
                                [ rdf:type owl:Restriction ;
                                  owl:onProperty :EnergyConsumer_p ;
                                  owl:maxQualifiedCardinality "1"^^xsd:nonNegativeInteger ;
                                  owl:onClass <https://w3id.org/netbeheer/IECCIM/TC57CIM/IEC61970/Base/Domain#ActivePower>
                                ] ,
                                [ rdf:type owl:Restriction ;
                                  owl:onProperty :EnergyConsumer_pfixed ;
                                  owl:maxQualifiedCardinality "1"^^xsd:nonNegativeInteger ;
                                  owl:onClass <https://w3id.org/netbeheer/IECCIM/TC57CIM/IEC61970/Base/Domain#ActivePower>
                                ] ,
                                [ rdf:type owl:Restriction ;
                                  owl:onProperty :EnergyConsumer_pfixedPct ;
                                  owl:maxQualifiedCardinality "1"^^xsd:nonNegativeInteger ;
                                  owl:onClass <https://w3id.org/netbeheer/IECCIM/TC57CIM/IEC61970/Base/Domain#PerCent>
                                ] ,
                                [ rdf:type owl:Restriction ;
                                  owl:onProperty :EnergyConsumer_q ;
                                  owl:maxQualifiedCardinality "1"^^xsd:nonNegativeInteger ;
                                  owl:onClass <https://w3id.org/netbeheer/IECCIM/TC57CIM/IEC61970/Base/Domain#ReactivePower>
                                ] ,
                                [ rdf:type owl:Restriction ;
                                  owl:onProperty :EnergyConsumer_qfixed ;
                                  owl:maxQualifiedCardinality "1"^^xsd:nonNegativeInteger ;
                                  owl:onClass <https://w3id.org/netbeheer/IECCIM/TC57CIM/IEC61970/Base/Domain#ReactivePower>
                                ] ,
                                [ rdf:type owl:Restriction ;
                                  owl:onProperty :EnergyConsumer_qfixedPct ;
                                  owl:maxQualifiedCardinality "1"^^xsd:nonNegativeInteger ;
                                  owl:onClass <https://w3id.org/netbeheer/IECCIM/TC57CIM/IEC61970/Base/Domain#PerCent>
                                ] ,
                                [ rdf:type owl:Restriction ;
                                  owl:onProperty :EnergyConsumer_customerCount ;
                                  owl:minQualifiedCardinality "0"^^xsd:nonNegativeInteger ;
                                  owl:onDataRange xsd:nonNegativeInteger
                                ] ,
                                [ rdf:type owl:Restriction ;
                                  owl:onProperty :EnergyConsumer_grounded ;
                                  owl:minQualifiedCardinality "0"^^xsd:nonNegativeInteger ;
                                  owl:onDataRange xsd:boolean
                                ] ,
                                [ rdf:type owl:Restriction ;
                                  owl:onProperty :EnergyConsumer_phaseConnection ;
                                  owl:minQualifiedCardinality "0"^^xsd:nonNegativeInteger ;
                                  owl:onDataRange :PhaseShuntConnectionKind
                                ] ,
                                [ rdf:type owl:Restriction ;
                                  owl:onProperty :EnergyConsumer_customerCount ;
                                  owl:maxQualifiedCardinality "1"^^xsd:nonNegativeInteger ;
                                  owl:onDataRange xsd:nonNegativeInteger
                                ] ,
                                [ rdf:type owl:Restriction ;
                                  owl:onProperty :EnergyConsumer_grounded ;
                                  owl:maxQualifiedCardinality "1"^^xsd:nonNegativeInteger ;
                                  owl:onDataRange xsd:boolean
                                ] ,
                                [ rdf:type owl:Restriction ;
                                  owl:onProperty :EnergyConsumer_phaseConnection ;
                                  owl:maxQualifiedCardinality "1"^^xsd:nonNegativeInteger ;
                                  owl:onDataRange :PhaseShuntConnectionKind
                                ] ;
                rdfs:comment "Generic user of energy - a  point of consumption on the power system model." .


###  https://w3id.org/netbeheer/IECCIM/TC57CIM/IEC61970/Base/Wires#EnergyConsumerPhase
:EnergyConsumerPhase rdf:type owl:Class ;
                     rdfs:subClassOf <https://w3id.org/netbeheer/IECCIM/TC57CIM/IEC61970/Base/Core#PowerSystemResource> ,
                                     [ rdf:type owl:Restriction ;
                                       owl:onProperty :EnergyConsumerPhase_EnergyConsumer ;
                                       owl:minQualifiedCardinality "0"^^xsd:nonNegativeInteger ;
                                       owl:onClass :EnergyConsumerPhase
                                     ] ,
                                     [ rdf:type owl:Restriction ;
                                       owl:onProperty :EnergyConsumerPhase_pfixed ;
                                       owl:minQualifiedCardinality "0"^^xsd:nonNegativeInteger ;
                                       owl:onClass <https://w3id.org/netbeheer/IECCIM/TC57CIM/IEC61970/Base/Domain#ActivePower>
                                     ] ,
                                     [ rdf:type owl:Restriction ;
                                       owl:onProperty :EnergyConsumerPhase_pfixedPct ;
                                       owl:minQualifiedCardinality "0"^^xsd:nonNegativeInteger ;
                                       owl:onClass <https://w3id.org/netbeheer/IECCIM/TC57CIM/IEC61970/Base/Domain#PerCent>
                                     ] ,
                                     [ rdf:type owl:Restriction ;
                                       owl:onProperty :EnergyConsumerPhase_qfixed ;
                                       owl:minQualifiedCardinality "0"^^xsd:nonNegativeInteger ;
                                       owl:onClass <https://w3id.org/netbeheer/IECCIM/TC57CIM/IEC61970/Base/Domain#ReactivePower>
                                     ] ,
                                     [ rdf:type owl:Restriction ;
                                       owl:onProperty :EnergyConsumerPhase_qfixedPct ;
                                       owl:minQualifiedCardinality "0"^^xsd:nonNegativeInteger ;
                                       owl:onClass <https://w3id.org/netbeheer/IECCIM/TC57CIM/IEC61970/Base/Domain#PerCent>
                                     ] ,
                                     [ rdf:type owl:Restriction ;
                                       owl:onProperty :EnergyConsumerPhase_pfixed ;
                                       owl:maxQualifiedCardinality "1"^^xsd:nonNegativeInteger ;
                                       owl:onClass <https://w3id.org/netbeheer/IECCIM/TC57CIM/IEC61970/Base/Domain#ActivePower>
                                     ] ,
                                     [ rdf:type owl:Restriction ;
                                       owl:onProperty :EnergyConsumerPhase_pfixedPct ;
                                       owl:maxQualifiedCardinality "1"^^xsd:nonNegativeInteger ;
                                       owl:onClass <https://w3id.org/netbeheer/IECCIM/TC57CIM/IEC61970/Base/Domain#PerCent>
                                     ] ,
                                     [ rdf:type owl:Restriction ;
                                       owl:onProperty :EnergyConsumerPhase_qfixed ;
                                       owl:maxQualifiedCardinality "1"^^xsd:nonNegativeInteger ;
                                       owl:onClass <https://w3id.org/netbeheer/IECCIM/TC57CIM/IEC61970/Base/Domain#ReactivePower>
                                     ] ,
                                     [ rdf:type owl:Restriction ;
                                       owl:onProperty :EnergyConsumerPhase_qfixedPct ;
                                       owl:maxQualifiedCardinality "1"^^xsd:nonNegativeInteger ;
                                       owl:onClass <https://w3id.org/netbeheer/IECCIM/TC57CIM/IEC61970/Base/Domain#PerCent>
                                     ] ,
                                     [ rdf:type owl:Restriction ;
                                       owl:onProperty :EnergyConsumerPhase_phase ;
                                       owl:minQualifiedCardinality "0"^^xsd:nonNegativeInteger ;
                                       owl:onDataRange :SinglePhaseKind
                                     ] ,
                                     [ rdf:type owl:Restriction ;
                                       owl:onProperty :EnergyConsumerPhase_phase ;
                                       owl:maxQualifiedCardinality "1"^^xsd:nonNegativeInteger ;
                                       owl:onDataRange :SinglePhaseKind
                                     ] ;
                     rdfs:comment """A single phase of an energy consumer.
""" .


###  https://w3id.org/netbeheer/IECCIM/TC57CIM/IEC61970/Base/Wires#EnergySource
:EnergySource rdf:type owl:Class ;
              rdfs:subClassOf <https://w3id.org/netbeheer/IECCIM/TC57CIM/IEC61970/Base/Core#ConductingEquipment> ,
                              [ rdf:type owl:Restriction ;
                                owl:onProperty :EnergySource_EnergySchedulingType ;
                                owl:minQualifiedCardinality "0"^^xsd:nonNegativeInteger ;
                                owl:onClass :EnergySource
                              ] ,
                              [ rdf:type owl:Restriction ;
                                owl:onProperty :EnergySource_EnergySourceAction ;
                                owl:minQualifiedCardinality "0"^^xsd:nonNegativeInteger ;
                                owl:onClass :EnergySource
                              ] ,
                              [ rdf:type owl:Restriction ;
                                owl:onProperty :EnergySource_activePower ;
                                owl:minQualifiedCardinality "0"^^xsd:nonNegativeInteger ;
                                owl:onClass <https://w3id.org/netbeheer/IECCIM/TC57CIM/IEC61970/Base/Domain#ActivePower>
                              ] ,
                              [ rdf:type owl:Restriction ;
                                owl:onProperty :EnergySource_nominalVoltage ;
                                owl:minQualifiedCardinality "0"^^xsd:nonNegativeInteger ;
                                owl:onClass <https://w3id.org/netbeheer/IECCIM/TC57CIM/IEC61970/Base/Domain#Voltage>
                              ] ,
                              [ rdf:type owl:Restriction ;
                                owl:onProperty :EnergySource_r ;
                                owl:minQualifiedCardinality "0"^^xsd:nonNegativeInteger ;
                                owl:onClass <https://w3id.org/netbeheer/IECCIM/TC57CIM/IEC61970/Base/Domain#Resistance>
                              ] ,
                              [ rdf:type owl:Restriction ;
                                owl:onProperty :EnergySource_r0 ;
                                owl:minQualifiedCardinality "0"^^xsd:nonNegativeInteger ;
                                owl:onClass <https://w3id.org/netbeheer/IECCIM/TC57CIM/IEC61970/Base/Domain#Resistance>
                              ] ,
                              [ rdf:type owl:Restriction ;
                                owl:onProperty :EnergySource_reactivePower ;
                                owl:minQualifiedCardinality "0"^^xsd:nonNegativeInteger ;
                                owl:onClass <https://w3id.org/netbeheer/IECCIM/TC57CIM/IEC61970/Base/Domain#ReactivePower>
                              ] ,
                              [ rdf:type owl:Restriction ;
                                owl:onProperty :EnergySource_rn ;
                                owl:minQualifiedCardinality "0"^^xsd:nonNegativeInteger ;
                                owl:onClass <https://w3id.org/netbeheer/IECCIM/TC57CIM/IEC61970/Base/Domain#Resistance>
                              ] ,
                              [ rdf:type owl:Restriction ;
                                owl:onProperty :EnergySource_voltageAngle ;
                                owl:minQualifiedCardinality "0"^^xsd:nonNegativeInteger ;
                                owl:onClass <https://w3id.org/netbeheer/IECCIM/TC57CIM/IEC61970/Base/Domain#AngleRadians>
                              ] ,
                              [ rdf:type owl:Restriction ;
                                owl:onProperty :EnergySource_voltageMagnitude ;
                                owl:minQualifiedCardinality "0"^^xsd:nonNegativeInteger ;
                                owl:onClass <https://w3id.org/netbeheer/IECCIM/TC57CIM/IEC61970/Base/Domain#Voltage>
                              ] ,
                              [ rdf:type owl:Restriction ;
                                owl:onProperty :EnergySource_x ;
                                owl:minQualifiedCardinality "0"^^xsd:nonNegativeInteger ;
                                owl:onClass <https://w3id.org/netbeheer/IECCIM/TC57CIM/IEC61970/Base/Domain#Reactance>
                              ] ,
                              [ rdf:type owl:Restriction ;
                                owl:onProperty :EnergySource_x0 ;
                                owl:minQualifiedCardinality "0"^^xsd:nonNegativeInteger ;
                                owl:onClass <https://w3id.org/netbeheer/IECCIM/TC57CIM/IEC61970/Base/Domain#Reactance>
                              ] ,
                              [ rdf:type owl:Restriction ;
                                owl:onProperty :EnergySource_xn ;
                                owl:minQualifiedCardinality "0"^^xsd:nonNegativeInteger ;
                                owl:onClass <https://w3id.org/netbeheer/IECCIM/TC57CIM/IEC61970/Base/Domain#Reactance>
                              ] ,
                              [ rdf:type owl:Restriction ;
                                owl:onProperty :EnergySource_EnergySourcePhase ;
                                owl:qualifiedCardinality "1"^^xsd:nonNegativeInteger ;
                                owl:onClass :EnergySource
                              ] ,
                              [ rdf:type owl:Restriction ;
                                owl:onProperty :EnergySource_WindTurbineType3or4Dynamics ;
                                owl:qualifiedCardinality "1"^^xsd:nonNegativeInteger ;
                                owl:onClass :EnergySource
                              ] ,
                              [ rdf:type owl:Restriction ;
                                owl:onProperty :EnergySource_EnergySourceAction ;
                                owl:maxQualifiedCardinality "1"^^xsd:nonNegativeInteger ;
                                owl:onClass :EnergySource
                              ] ,
                              [ rdf:type owl:Restriction ;
                                owl:onProperty :EnergySource_activePower ;
                                owl:maxQualifiedCardinality "1"^^xsd:nonNegativeInteger ;
                                owl:onClass <https://w3id.org/netbeheer/IECCIM/TC57CIM/IEC61970/Base/Domain#ActivePower>
                              ] ,
                              [ rdf:type owl:Restriction ;
                                owl:onProperty :EnergySource_nominalVoltage ;
                                owl:maxQualifiedCardinality "1"^^xsd:nonNegativeInteger ;
                                owl:onClass <https://w3id.org/netbeheer/IECCIM/TC57CIM/IEC61970/Base/Domain#Voltage>
                              ] ,
                              [ rdf:type owl:Restriction ;
                                owl:onProperty :EnergySource_r ;
                                owl:maxQualifiedCardinality "1"^^xsd:nonNegativeInteger ;
                                owl:onClass <https://w3id.org/netbeheer/IECCIM/TC57CIM/IEC61970/Base/Domain#Resistance>
                              ] ,
                              [ rdf:type owl:Restriction ;
                                owl:onProperty :EnergySource_r0 ;
                                owl:maxQualifiedCardinality "1"^^xsd:nonNegativeInteger ;
                                owl:onClass <https://w3id.org/netbeheer/IECCIM/TC57CIM/IEC61970/Base/Domain#Resistance>
                              ] ,
                              [ rdf:type owl:Restriction ;
                                owl:onProperty :EnergySource_reactivePower ;
                                owl:maxQualifiedCardinality "1"^^xsd:nonNegativeInteger ;
                                owl:onClass <https://w3id.org/netbeheer/IECCIM/TC57CIM/IEC61970/Base/Domain#ReactivePower>
                              ] ,
                              [ rdf:type owl:Restriction ;
                                owl:onProperty :EnergySource_rn ;
                                owl:maxQualifiedCardinality "1"^^xsd:nonNegativeInteger ;
                                owl:onClass <https://w3id.org/netbeheer/IECCIM/TC57CIM/IEC61970/Base/Domain#Resistance>
                              ] ,
                              [ rdf:type owl:Restriction ;
                                owl:onProperty :EnergySource_voltageAngle ;
                                owl:maxQualifiedCardinality "1"^^xsd:nonNegativeInteger ;
                                owl:onClass <https://w3id.org/netbeheer/IECCIM/TC57CIM/IEC61970/Base/Domain#AngleRadians>
                              ] ,
                              [ rdf:type owl:Restriction ;
                                owl:onProperty :EnergySource_voltageMagnitude ;
                                owl:maxQualifiedCardinality "1"^^xsd:nonNegativeInteger ;
                                owl:onClass <https://w3id.org/netbeheer/IECCIM/TC57CIM/IEC61970/Base/Domain#Voltage>
                              ] ,
                              [ rdf:type owl:Restriction ;
                                owl:onProperty :EnergySource_x ;
                                owl:maxQualifiedCardinality "1"^^xsd:nonNegativeInteger ;
                                owl:onClass <https://w3id.org/netbeheer/IECCIM/TC57CIM/IEC61970/Base/Domain#Reactance>
                              ] ,
                              [ rdf:type owl:Restriction ;
                                owl:onProperty :EnergySource_x0 ;
                                owl:maxQualifiedCardinality "1"^^xsd:nonNegativeInteger ;
                                owl:onClass <https://w3id.org/netbeheer/IECCIM/TC57CIM/IEC61970/Base/Domain#Reactance>
                              ] ,
                              [ rdf:type owl:Restriction ;
                                owl:onProperty :EnergySource_xn ;
                                owl:maxQualifiedCardinality "1"^^xsd:nonNegativeInteger ;
                                owl:onClass <https://w3id.org/netbeheer/IECCIM/TC57CIM/IEC61970/Base/Domain#Reactance>
                              ] ;
              rdfs:comment "A generic equivalent for an energy supplier on a transmission or distribution voltage level." .


###  https://w3id.org/netbeheer/IECCIM/TC57CIM/IEC61970/Base/Wires#EnergySourcePhase
:EnergySourcePhase rdf:type owl:Class ;
                   rdfs:subClassOf <https://w3id.org/netbeheer/IECCIM/TC57CIM/IEC61970/Base/Core#PowerSystemResource> ,
                                   [ rdf:type owl:Restriction ;
                                     owl:onProperty :EnergySourcePhase_EnergySource ;
                                     owl:minQualifiedCardinality "0"^^xsd:nonNegativeInteger ;
                                     owl:onClass :EnergySourcePhase
                                   ] ,
                                   [ rdf:type owl:Restriction ;
                                     owl:onProperty :EnergySourcePhase_phase ;
                                     owl:minQualifiedCardinality "0"^^xsd:nonNegativeInteger ;
                                     owl:onDataRange :SinglePhaseKind
                                   ] ,
                                   [ rdf:type owl:Restriction ;
                                     owl:onProperty :EnergySourcePhase_phase ;
                                     owl:maxQualifiedCardinality "1"^^xsd:nonNegativeInteger ;
                                     owl:onDataRange :SinglePhaseKind
                                   ] ;
                   rdfs:comment "Represents the single phase information of an unbalanced energy source." .


###  https://w3id.org/netbeheer/IECCIM/TC57CIM/IEC61970/Base/Wires#ExternalNetworkInjection
:ExternalNetworkInjection rdf:type owl:Class ;
                          rdfs:subClassOf :RegulatingCondEq ,
                                          [ rdf:type owl:Restriction ;
                                            owl:onProperty :ExternalNetworkInjection_governorSCD ;
                                            owl:minQualifiedCardinality "0"^^xsd:nonNegativeInteger ;
                                            owl:onClass <https://w3id.org/netbeheer/IECCIM/TC57CIM/IEC61970/Base/Domain#ActivePowerPerFrequency>
                                          ] ,
                                          [ rdf:type owl:Restriction ;
                                            owl:onProperty :ExternalNetworkInjection_maxInitialSymShCCurrent ;
                                            owl:minQualifiedCardinality "0"^^xsd:nonNegativeInteger ;
                                            owl:onClass <https://w3id.org/netbeheer/IECCIM/TC57CIM/IEC61970/Base/Domain#CurrentFlow>
                                          ] ,
                                          [ rdf:type owl:Restriction ;
                                            owl:onProperty :ExternalNetworkInjection_maxP ;
                                            owl:minQualifiedCardinality "0"^^xsd:nonNegativeInteger ;
                                            owl:onClass <https://w3id.org/netbeheer/IECCIM/TC57CIM/IEC61970/Base/Domain#ActivePower>
                                          ] ,
                                          [ rdf:type owl:Restriction ;
                                            owl:onProperty :ExternalNetworkInjection_maxQ ;
                                            owl:minQualifiedCardinality "0"^^xsd:nonNegativeInteger ;
                                            owl:onClass <https://w3id.org/netbeheer/IECCIM/TC57CIM/IEC61970/Base/Domain#ReactivePower>
                                          ] ,
                                          [ rdf:type owl:Restriction ;
                                            owl:onProperty :ExternalNetworkInjection_minInitialSymShCCurrent ;
                                            owl:minQualifiedCardinality "0"^^xsd:nonNegativeInteger ;
                                            owl:onClass <https://w3id.org/netbeheer/IECCIM/TC57CIM/IEC61970/Base/Domain#CurrentFlow>
                                          ] ,
                                          [ rdf:type owl:Restriction ;
                                            owl:onProperty :ExternalNetworkInjection_minP ;
                                            owl:minQualifiedCardinality "0"^^xsd:nonNegativeInteger ;
                                            owl:onClass <https://w3id.org/netbeheer/IECCIM/TC57CIM/IEC61970/Base/Domain#ActivePower>
                                          ] ,
                                          [ rdf:type owl:Restriction ;
                                            owl:onProperty :ExternalNetworkInjection_minQ ;
                                            owl:minQualifiedCardinality "0"^^xsd:nonNegativeInteger ;
                                            owl:onClass <https://w3id.org/netbeheer/IECCIM/TC57CIM/IEC61970/Base/Domain#ReactivePower>
                                          ] ,
                                          [ rdf:type owl:Restriction ;
                                            owl:onProperty :ExternalNetworkInjection_p ;
                                            owl:minQualifiedCardinality "0"^^xsd:nonNegativeInteger ;
                                            owl:onClass <https://w3id.org/netbeheer/IECCIM/TC57CIM/IEC61970/Base/Domain#ActivePower>
                                          ] ,
                                          [ rdf:type owl:Restriction ;
                                            owl:onProperty :ExternalNetworkInjection_q ;
                                            owl:minQualifiedCardinality "0"^^xsd:nonNegativeInteger ;
                                            owl:onClass <https://w3id.org/netbeheer/IECCIM/TC57CIM/IEC61970/Base/Domain#ReactivePower>
                                          ] ,
                                          [ rdf:type owl:Restriction ;
                                            owl:onProperty :ExternalNetworkInjection_voltageFactor ;
                                            owl:minQualifiedCardinality "0"^^xsd:nonNegativeInteger ;
                                            owl:onClass <https://w3id.org/netbeheer/IECCIM/TC57CIM/IEC61970/Base/Domain#PU>
                                          ] ,
                                          [ rdf:type owl:Restriction ;
                                            owl:onProperty :ExternalNetworkInjection_governorSCD ;
                                            owl:maxQualifiedCardinality "1"^^xsd:nonNegativeInteger ;
                                            owl:onClass <https://w3id.org/netbeheer/IECCIM/TC57CIM/IEC61970/Base/Domain#ActivePowerPerFrequency>
                                          ] ,
                                          [ rdf:type owl:Restriction ;
                                            owl:onProperty :ExternalNetworkInjection_maxInitialSymShCCurrent ;
                                            owl:maxQualifiedCardinality "1"^^xsd:nonNegativeInteger ;
                                            owl:onClass <https://w3id.org/netbeheer/IECCIM/TC57CIM/IEC61970/Base/Domain#CurrentFlow>
                                          ] ,
                                          [ rdf:type owl:Restriction ;
                                            owl:onProperty :ExternalNetworkInjection_maxP ;
                                            owl:maxQualifiedCardinality "1"^^xsd:nonNegativeInteger ;
                                            owl:onClass <https://w3id.org/netbeheer/IECCIM/TC57CIM/IEC61970/Base/Domain#ActivePower>
                                          ] ,
                                          [ rdf:type owl:Restriction ;
                                            owl:onProperty :ExternalNetworkInjection_maxQ ;
                                            owl:maxQualifiedCardinality "1"^^xsd:nonNegativeInteger ;
                                            owl:onClass <https://w3id.org/netbeheer/IECCIM/TC57CIM/IEC61970/Base/Domain#ReactivePower>
                                          ] ,
                                          [ rdf:type owl:Restriction ;
                                            owl:onProperty :ExternalNetworkInjection_minInitialSymShCCurrent ;
                                            owl:maxQualifiedCardinality "1"^^xsd:nonNegativeInteger ;
                                            owl:onClass <https://w3id.org/netbeheer/IECCIM/TC57CIM/IEC61970/Base/Domain#CurrentFlow>
                                          ] ,
                                          [ rdf:type owl:Restriction ;
                                            owl:onProperty :ExternalNetworkInjection_minP ;
                                            owl:maxQualifiedCardinality "1"^^xsd:nonNegativeInteger ;
                                            owl:onClass <https://w3id.org/netbeheer/IECCIM/TC57CIM/IEC61970/Base/Domain#ActivePower>
                                          ] ,
                                          [ rdf:type owl:Restriction ;
                                            owl:onProperty :ExternalNetworkInjection_minQ ;
                                            owl:maxQualifiedCardinality "1"^^xsd:nonNegativeInteger ;
                                            owl:onClass <https://w3id.org/netbeheer/IECCIM/TC57CIM/IEC61970/Base/Domain#ReactivePower>
                                          ] ,
                                          [ rdf:type owl:Restriction ;
                                            owl:onProperty :ExternalNetworkInjection_p ;
                                            owl:maxQualifiedCardinality "1"^^xsd:nonNegativeInteger ;
                                            owl:onClass <https://w3id.org/netbeheer/IECCIM/TC57CIM/IEC61970/Base/Domain#ActivePower>
                                          ] ,
                                          [ rdf:type owl:Restriction ;
                                            owl:onProperty :ExternalNetworkInjection_q ;
                                            owl:maxQualifiedCardinality "1"^^xsd:nonNegativeInteger ;
                                            owl:onClass <https://w3id.org/netbeheer/IECCIM/TC57CIM/IEC61970/Base/Domain#ReactivePower>
                                          ] ,
                                          [ rdf:type owl:Restriction ;
                                            owl:onProperty :ExternalNetworkInjection_voltageFactor ;
                                            owl:maxQualifiedCardinality "1"^^xsd:nonNegativeInteger ;
                                            owl:onClass <https://w3id.org/netbeheer/IECCIM/TC57CIM/IEC61970/Base/Domain#PU>
                                          ] ,
                                          [ rdf:type owl:Restriction ;
                                            owl:onProperty :ExternalNetworkInjection_ikSecond ;
                                            owl:minQualifiedCardinality "0"^^xsd:nonNegativeInteger ;
                                            owl:onDataRange xsd:boolean
                                          ] ,
                                          [ rdf:type owl:Restriction ;
                                            owl:onProperty :ExternalNetworkInjection_maxR0ToX0Ratio ;
                                            owl:minQualifiedCardinality "0"^^xsd:nonNegativeInteger ;
                                            owl:onDataRange xsd:float
                                          ] ,
                                          [ rdf:type owl:Restriction ;
                                            owl:onProperty :ExternalNetworkInjection_maxR1ToX1Ratio ;
                                            owl:minQualifiedCardinality "0"^^xsd:nonNegativeInteger ;
                                            owl:onDataRange xsd:float
                                          ] ,
                                          [ rdf:type owl:Restriction ;
                                            owl:onProperty :ExternalNetworkInjection_maxZ0ToZ1Ratio ;
                                            owl:minQualifiedCardinality "0"^^xsd:nonNegativeInteger ;
                                            owl:onDataRange xsd:float
                                          ] ,
                                          [ rdf:type owl:Restriction ;
                                            owl:onProperty :ExternalNetworkInjection_minR0ToX0Ratio ;
                                            owl:minQualifiedCardinality "0"^^xsd:nonNegativeInteger ;
                                            owl:onDataRange xsd:float
                                          ] ,
                                          [ rdf:type owl:Restriction ;
                                            owl:onProperty :ExternalNetworkInjection_minR1ToX1Ratio ;
                                            owl:minQualifiedCardinality "0"^^xsd:nonNegativeInteger ;
                                            owl:onDataRange xsd:float
                                          ] ,
                                          [ rdf:type owl:Restriction ;
                                            owl:onProperty :ExternalNetworkInjection_minZ0ToZ1Ratio ;
                                            owl:minQualifiedCardinality "0"^^xsd:nonNegativeInteger ;
                                            owl:onDataRange xsd:float
                                          ] ,
                                          [ rdf:type owl:Restriction ;
                                            owl:onProperty :ExternalNetworkInjection_referencePriority ;
                                            owl:minQualifiedCardinality "0"^^xsd:nonNegativeInteger ;
                                            owl:onDataRange xsd:nonNegativeInteger
                                          ] ,
                                          [ rdf:type owl:Restriction ;
                                            owl:onProperty :ExternalNetworkInjection_ikSecond ;
                                            owl:maxQualifiedCardinality "1"^^xsd:nonNegativeInteger ;
                                            owl:onDataRange xsd:boolean
                                          ] ,
                                          [ rdf:type owl:Restriction ;
                                            owl:onProperty :ExternalNetworkInjection_maxR0ToX0Ratio ;
                                            owl:maxQualifiedCardinality "1"^^xsd:nonNegativeInteger ;
                                            owl:onDataRange xsd:float
                                          ] ,
                                          [ rdf:type owl:Restriction ;
                                            owl:onProperty :ExternalNetworkInjection_maxR1ToX1Ratio ;
                                            owl:maxQualifiedCardinality "1"^^xsd:nonNegativeInteger ;
                                            owl:onDataRange xsd:float
                                          ] ,
                                          [ rdf:type owl:Restriction ;
                                            owl:onProperty :ExternalNetworkInjection_maxZ0ToZ1Ratio ;
                                            owl:maxQualifiedCardinality "1"^^xsd:nonNegativeInteger ;
                                            owl:onDataRange xsd:float
                                          ] ,
                                          [ rdf:type owl:Restriction ;
                                            owl:onProperty :ExternalNetworkInjection_minR0ToX0Ratio ;
                                            owl:maxQualifiedCardinality "1"^^xsd:nonNegativeInteger ;
                                            owl:onDataRange xsd:float
                                          ] ,
                                          [ rdf:type owl:Restriction ;
                                            owl:onProperty :ExternalNetworkInjection_minR1ToX1Ratio ;
                                            owl:maxQualifiedCardinality "1"^^xsd:nonNegativeInteger ;
                                            owl:onDataRange xsd:float
                                          ] ,
                                          [ rdf:type owl:Restriction ;
                                            owl:onProperty :ExternalNetworkInjection_minZ0ToZ1Ratio ;
                                            owl:maxQualifiedCardinality "1"^^xsd:nonNegativeInteger ;
                                            owl:onDataRange xsd:float
                                          ] ,
                                          [ rdf:type owl:Restriction ;
                                            owl:onProperty :ExternalNetworkInjection_referencePriority ;
                                            owl:maxQualifiedCardinality "1"^^xsd:nonNegativeInteger ;
                                            owl:onDataRange xsd:nonNegativeInteger
                                          ] ;
                          rdfs:comment "This class represents external network and it is used for IEC 60909 calculations." .


###  https://w3id.org/netbeheer/IECCIM/TC57CIM/IEC61970/Base/Wires#FrequencyConverter
:FrequencyConverter rdf:type owl:Class ;
                    rdfs:subClassOf :RegulatingCondEq ,
                                    [ rdf:type owl:Restriction ;
                                      owl:onProperty :FrequencyConverter_frequency ;
                                      owl:minQualifiedCardinality "0"^^xsd:nonNegativeInteger ;
                                      owl:onClass <https://w3id.org/netbeheer/IECCIM/TC57CIM/IEC61970/Base/Domain#Frequency>
                                    ] ,
                                    [ rdf:type owl:Restriction ;
                                      owl:onProperty :FrequencyConverter_maxP ;
                                      owl:minQualifiedCardinality "0"^^xsd:nonNegativeInteger ;
                                      owl:onClass <https://w3id.org/netbeheer/IECCIM/TC57CIM/IEC61970/Base/Domain#ActivePower>
                                    ] ,
                                    [ rdf:type owl:Restriction ;
                                      owl:onProperty :FrequencyConverter_maxU ;
                                      owl:minQualifiedCardinality "0"^^xsd:nonNegativeInteger ;
                                      owl:onClass <https://w3id.org/netbeheer/IECCIM/TC57CIM/IEC61970/Base/Domain#Voltage>
                                    ] ,
                                    [ rdf:type owl:Restriction ;
                                      owl:onProperty :FrequencyConverter_minP ;
                                      owl:minQualifiedCardinality "0"^^xsd:nonNegativeInteger ;
                                      owl:onClass <https://w3id.org/netbeheer/IECCIM/TC57CIM/IEC61970/Base/Domain#ActivePower>
                                    ] ,
                                    [ rdf:type owl:Restriction ;
                                      owl:onProperty :FrequencyConverter_minU ;
                                      owl:minQualifiedCardinality "0"^^xsd:nonNegativeInteger ;
                                      owl:onClass <https://w3id.org/netbeheer/IECCIM/TC57CIM/IEC61970/Base/Domain#Voltage>
                                    ] ,
                                    [ rdf:type owl:Restriction ;
                                      owl:onProperty :FrequencyConverter_frequency ;
                                      owl:maxQualifiedCardinality "1"^^xsd:nonNegativeInteger ;
                                      owl:onClass <https://w3id.org/netbeheer/IECCIM/TC57CIM/IEC61970/Base/Domain#Frequency>
                                    ] ,
                                    [ rdf:type owl:Restriction ;
                                      owl:onProperty :FrequencyConverter_maxP ;
                                      owl:maxQualifiedCardinality "1"^^xsd:nonNegativeInteger ;
                                      owl:onClass <https://w3id.org/netbeheer/IECCIM/TC57CIM/IEC61970/Base/Domain#ActivePower>
                                    ] ,
                                    [ rdf:type owl:Restriction ;
                                      owl:onProperty :FrequencyConverter_maxU ;
                                      owl:maxQualifiedCardinality "1"^^xsd:nonNegativeInteger ;
                                      owl:onClass <https://w3id.org/netbeheer/IECCIM/TC57CIM/IEC61970/Base/Domain#Voltage>
                                    ] ,
                                    [ rdf:type owl:Restriction ;
                                      owl:onProperty :FrequencyConverter_minP ;
                                      owl:maxQualifiedCardinality "1"^^xsd:nonNegativeInteger ;
                                      owl:onClass <https://w3id.org/netbeheer/IECCIM/TC57CIM/IEC61970/Base/Domain#ActivePower>
                                    ] ,
                                    [ rdf:type owl:Restriction ;
                                      owl:onProperty :FrequencyConverter_minU ;
                                      owl:maxQualifiedCardinality "1"^^xsd:nonNegativeInteger ;
                                      owl:onClass <https://w3id.org/netbeheer/IECCIM/TC57CIM/IEC61970/Base/Domain#Voltage>
                                    ] ;
                    rdfs:comment "A device to convert from one frequency to another (e.g., frequency F1 to F2) comprises a pair of FrequencyConverter instances. One converts from F1 to DC, the other converts the DC to F2." .


###  https://w3id.org/netbeheer/IECCIM/TC57CIM/IEC61970/Base/Wires#Fuse
:Fuse rdf:type owl:Class ;
      rdfs:subClassOf :Switch ;
      rdfs:comment "An overcurrent protective device with a circuit opening fusible part that is heated and severed by the passage of overcurrent through it. A fuse is considered a switching device because it breaks current." .


###  https://w3id.org/netbeheer/IECCIM/TC57CIM/IEC61970/Base/Wires#Ground
:Ground rdf:type owl:Class ;
        rdfs:subClassOf <https://w3id.org/netbeheer/IECCIM/TC57CIM/IEC61970/Base/Core#ConductingEquipment> ,
                        [ rdf:type owl:Restriction ;
                          owl:onProperty :Ground_GroundAction ;
                          owl:minQualifiedCardinality "0"^^xsd:nonNegativeInteger ;
                          owl:onClass :Ground
                        ] ,
                        [ rdf:type owl:Restriction ;
                          owl:onProperty :Ground_GroundAction ;
                          owl:maxQualifiedCardinality "1"^^xsd:nonNegativeInteger ;
                          owl:onClass :Ground
                        ] ;
        rdfs:comment "A point where the system is grounded used for connecting conducting equipment to ground. The power system model can have any number of grounds." .


###  https://w3id.org/netbeheer/IECCIM/TC57CIM/IEC61970/Base/Wires#GroundDisconnector
:GroundDisconnector rdf:type owl:Class ;
                    rdfs:subClassOf :Switch ;
                    rdfs:comment "A manually operated or motor operated mechanical switching device used for isolating a circuit or equipment from ground." .


###  https://w3id.org/netbeheer/IECCIM/TC57CIM/IEC61970/Base/Wires#GroundingImpedance
:GroundingImpedance rdf:type owl:Class ;
                    rdfs:subClassOf :EarthFaultCompensator ,
                                    [ rdf:type owl:Restriction ;
                                      owl:onProperty :GroundingImpedance_x ;
                                      owl:minQualifiedCardinality "0"^^xsd:nonNegativeInteger ;
                                      owl:onClass <https://w3id.org/netbeheer/IECCIM/TC57CIM/IEC61970/Base/Domain#Reactance>
                                    ] ,
                                    [ rdf:type owl:Restriction ;
                                      owl:onProperty :GroundingImpedance_x ;
                                      owl:maxQualifiedCardinality "1"^^xsd:nonNegativeInteger ;
                                      owl:onClass <https://w3id.org/netbeheer/IECCIM/TC57CIM/IEC61970/Base/Domain#Reactance>
                                    ] ;
                    rdfs:comment "A fixed impedance device used for grounding." .


###  https://w3id.org/netbeheer/IECCIM/TC57CIM/IEC61970/Base/Wires#Jumper
:Jumper rdf:type owl:Class ;
        rdfs:subClassOf :Switch ,
                        [ rdf:type owl:Restriction ;
                          owl:onProperty :Jumper_JumperAction ;
                          owl:minQualifiedCardinality "0"^^xsd:nonNegativeInteger ;
                          owl:onClass :Jumper
                        ] ,
                        [ rdf:type owl:Restriction ;
                          owl:onProperty :Jumper_JumperAction ;
                          owl:maxQualifiedCardinality "1"^^xsd:nonNegativeInteger ;
                          owl:onClass :Jumper
                        ] ;
        rdfs:comment """A short section of conductor with negligible impedance which can be manually removed and replaced if the circuit is de-energized. Note that zero-impedance branches can potentially be modeled by other equipment types.
""" .


###  https://w3id.org/netbeheer/IECCIM/TC57CIM/IEC61970/Base/Wires#Junction
:Junction rdf:type owl:Class ;
          rdfs:subClassOf :Connector ;
          rdfs:comment "A point where one or more conducting equipments are connected with zero resistance." .


###  https://w3id.org/netbeheer/IECCIM/TC57CIM/IEC61970/Base/Wires#Line
:Line rdf:type owl:Class ;
      rdfs:subClassOf <https://w3id.org/netbeheer/IECCIM/TC57CIM/IEC61970/Base/Core#EquipmentContainer> ;
      rdfs:comment "Contains equipment beyond a substation belonging to a power transmission line. " .


###  https://w3id.org/netbeheer/IECCIM/TC57CIM/IEC61970/Base/Wires#LinearShuntCompensator
:LinearShuntCompensator rdf:type owl:Class ;
                        rdfs:subClassOf :ShuntCompensator ,
                                        [ rdf:type owl:Restriction ;
                                          owl:onProperty :LinearShuntCompensator_b0PerSection ;
                                          owl:minQualifiedCardinality "0"^^xsd:nonNegativeInteger ;
                                          owl:onClass <https://w3id.org/netbeheer/IECCIM/TC57CIM/IEC61970/Base/Domain#Susceptance>
                                        ] ,
                                        [ rdf:type owl:Restriction ;
                                          owl:onProperty :LinearShuntCompensator_bPerSection ;
                                          owl:minQualifiedCardinality "0"^^xsd:nonNegativeInteger ;
                                          owl:onClass <https://w3id.org/netbeheer/IECCIM/TC57CIM/IEC61970/Base/Domain#Susceptance>
                                        ] ,
                                        [ rdf:type owl:Restriction ;
                                          owl:onProperty :LinearShuntCompensator_g0PerSection ;
                                          owl:minQualifiedCardinality "0"^^xsd:nonNegativeInteger ;
                                          owl:onClass <https://w3id.org/netbeheer/IECCIM/TC57CIM/IEC61970/Base/Domain#Conductance>
                                        ] ,
                                        [ rdf:type owl:Restriction ;
                                          owl:onProperty :LinearShuntCompensator_gPerSection ;
                                          owl:minQualifiedCardinality "0"^^xsd:nonNegativeInteger ;
                                          owl:onClass <https://w3id.org/netbeheer/IECCIM/TC57CIM/IEC61970/Base/Domain#Conductance>
                                        ] ,
                                        [ rdf:type owl:Restriction ;
                                          owl:onProperty :LinearShuntCompensator_b0PerSection ;
                                          owl:maxQualifiedCardinality "1"^^xsd:nonNegativeInteger ;
                                          owl:onClass <https://w3id.org/netbeheer/IECCIM/TC57CIM/IEC61970/Base/Domain#Susceptance>
                                        ] ,
                                        [ rdf:type owl:Restriction ;
                                          owl:onProperty :LinearShuntCompensator_bPerSection ;
                                          owl:maxQualifiedCardinality "1"^^xsd:nonNegativeInteger ;
                                          owl:onClass <https://w3id.org/netbeheer/IECCIM/TC57CIM/IEC61970/Base/Domain#Susceptance>
                                        ] ,
                                        [ rdf:type owl:Restriction ;
                                          owl:onProperty :LinearShuntCompensator_g0PerSection ;
                                          owl:maxQualifiedCardinality "1"^^xsd:nonNegativeInteger ;
                                          owl:onClass <https://w3id.org/netbeheer/IECCIM/TC57CIM/IEC61970/Base/Domain#Conductance>
                                        ] ,
                                        [ rdf:type owl:Restriction ;
                                          owl:onProperty :LinearShuntCompensator_gPerSection ;
                                          owl:maxQualifiedCardinality "1"^^xsd:nonNegativeInteger ;
                                          owl:onClass <https://w3id.org/netbeheer/IECCIM/TC57CIM/IEC61970/Base/Domain#Conductance>
                                        ] ;
                        rdfs:comment "A linear shunt compensator has banks or sections with equal admittance values." .


###  https://w3id.org/netbeheer/IECCIM/TC57CIM/IEC61970/Base/Wires#LinearShuntCompensatorPhase
:LinearShuntCompensatorPhase rdf:type owl:Class ;
                             rdfs:subClassOf :ShuntCompensatorPhase ,
                                             [ rdf:type owl:Restriction ;
                                               owl:onProperty :LinearShuntCompensatorPhase_bPerSection ;
                                               owl:minQualifiedCardinality "0"^^xsd:nonNegativeInteger ;
                                               owl:onClass <https://w3id.org/netbeheer/IECCIM/TC57CIM/IEC61970/Base/Domain#Susceptance>
                                             ] ,
                                             [ rdf:type owl:Restriction ;
                                               owl:onProperty :LinearShuntCompensatorPhase_gPerSection ;
                                               owl:minQualifiedCardinality "0"^^xsd:nonNegativeInteger ;
                                               owl:onClass <https://w3id.org/netbeheer/IECCIM/TC57CIM/IEC61970/Base/Domain#Conductance>
                                             ] ,
                                             [ rdf:type owl:Restriction ;
                                               owl:onProperty :LinearShuntCompensatorPhase_bPerSection ;
                                               owl:maxQualifiedCardinality "1"^^xsd:nonNegativeInteger ;
                                               owl:onClass <https://w3id.org/netbeheer/IECCIM/TC57CIM/IEC61970/Base/Domain#Susceptance>
                                             ] ,
                                             [ rdf:type owl:Restriction ;
                                               owl:onProperty :LinearShuntCompensatorPhase_gPerSection ;
                                               owl:maxQualifiedCardinality "1"^^xsd:nonNegativeInteger ;
                                               owl:onClass <https://w3id.org/netbeheer/IECCIM/TC57CIM/IEC61970/Base/Domain#Conductance>
                                             ] ;
                             rdfs:comment "A per phase linear shunt compensator has banks or sections with equal admittance values." .


###  https://w3id.org/netbeheer/IECCIM/TC57CIM/IEC61970/Base/Wires#LoadBreakSwitch
:LoadBreakSwitch rdf:type owl:Class ;
                 rdfs:subClassOf :ProtectedSwitch ;
                 rdfs:comment "A mechanical switching device capable of making, carrying, and breaking currents under normal operating conditions." .


###  https://w3id.org/netbeheer/IECCIM/TC57CIM/IEC61970/Base/Wires#MutualCoupling
:MutualCoupling rdf:type owl:Class ;
                rdfs:subClassOf <https://w3id.org/netbeheer/IECCIM/TC57CIM/IEC61970/Base/Core#IdentifiedObject> ,
                                [ rdf:type owl:Restriction ;
                                  owl:onProperty :MutualCoupling_b0ch ;
                                  owl:minQualifiedCardinality "0"^^xsd:nonNegativeInteger ;
                                  owl:onClass <https://w3id.org/netbeheer/IECCIM/TC57CIM/IEC61970/Base/Domain#Susceptance>
                                ] ,
                                [ rdf:type owl:Restriction ;
                                  owl:onProperty :MutualCoupling_distance11 ;
                                  owl:minQualifiedCardinality "0"^^xsd:nonNegativeInteger ;
                                  owl:onClass <https://w3id.org/netbeheer/IECCIM/TC57CIM/IEC61970/Base/Domain#Length>
                                ] ,
                                [ rdf:type owl:Restriction ;
                                  owl:onProperty :MutualCoupling_distance12 ;
                                  owl:minQualifiedCardinality "0"^^xsd:nonNegativeInteger ;
                                  owl:onClass <https://w3id.org/netbeheer/IECCIM/TC57CIM/IEC61970/Base/Domain#Length>
                                ] ,
                                [ rdf:type owl:Restriction ;
                                  owl:onProperty :MutualCoupling_distance21 ;
                                  owl:minQualifiedCardinality "0"^^xsd:nonNegativeInteger ;
                                  owl:onClass <https://w3id.org/netbeheer/IECCIM/TC57CIM/IEC61970/Base/Domain#Length>
                                ] ,
                                [ rdf:type owl:Restriction ;
                                  owl:onProperty :MutualCoupling_distance22 ;
                                  owl:minQualifiedCardinality "0"^^xsd:nonNegativeInteger ;
                                  owl:onClass <https://w3id.org/netbeheer/IECCIM/TC57CIM/IEC61970/Base/Domain#Length>
                                ] ,
                                [ rdf:type owl:Restriction ;
                                  owl:onProperty :MutualCoupling_g0ch ;
                                  owl:minQualifiedCardinality "0"^^xsd:nonNegativeInteger ;
                                  owl:onClass <https://w3id.org/netbeheer/IECCIM/TC57CIM/IEC61970/Base/Domain#Conductance>
                                ] ,
                                [ rdf:type owl:Restriction ;
                                  owl:onProperty :MutualCoupling_r0 ;
                                  owl:minQualifiedCardinality "0"^^xsd:nonNegativeInteger ;
                                  owl:onClass <https://w3id.org/netbeheer/IECCIM/TC57CIM/IEC61970/Base/Domain#Resistance>
                                ] ,
                                [ rdf:type owl:Restriction ;
                                  owl:onProperty :MutualCoupling_x0 ;
                                  owl:minQualifiedCardinality "0"^^xsd:nonNegativeInteger ;
                                  owl:onClass <https://w3id.org/netbeheer/IECCIM/TC57CIM/IEC61970/Base/Domain#Reactance>
                                ] ,
                                [ rdf:type owl:Restriction ;
                                  owl:onProperty :MutualCoupling_b0ch ;
                                  owl:maxQualifiedCardinality "1"^^xsd:nonNegativeInteger ;
                                  owl:onClass <https://w3id.org/netbeheer/IECCIM/TC57CIM/IEC61970/Base/Domain#Susceptance>
                                ] ,
                                [ rdf:type owl:Restriction ;
                                  owl:onProperty :MutualCoupling_distance11 ;
                                  owl:maxQualifiedCardinality "1"^^xsd:nonNegativeInteger ;
                                  owl:onClass <https://w3id.org/netbeheer/IECCIM/TC57CIM/IEC61970/Base/Domain#Length>
                                ] ,
                                [ rdf:type owl:Restriction ;
                                  owl:onProperty :MutualCoupling_distance12 ;
                                  owl:maxQualifiedCardinality "1"^^xsd:nonNegativeInteger ;
                                  owl:onClass <https://w3id.org/netbeheer/IECCIM/TC57CIM/IEC61970/Base/Domain#Length>
                                ] ,
                                [ rdf:type owl:Restriction ;
                                  owl:onProperty :MutualCoupling_distance21 ;
                                  owl:maxQualifiedCardinality "1"^^xsd:nonNegativeInteger ;
                                  owl:onClass <https://w3id.org/netbeheer/IECCIM/TC57CIM/IEC61970/Base/Domain#Length>
                                ] ,
                                [ rdf:type owl:Restriction ;
                                  owl:onProperty :MutualCoupling_distance22 ;
                                  owl:maxQualifiedCardinality "1"^^xsd:nonNegativeInteger ;
                                  owl:onClass <https://w3id.org/netbeheer/IECCIM/TC57CIM/IEC61970/Base/Domain#Length>
                                ] ,
                                [ rdf:type owl:Restriction ;
                                  owl:onProperty :MutualCoupling_g0ch ;
                                  owl:maxQualifiedCardinality "1"^^xsd:nonNegativeInteger ;
                                  owl:onClass <https://w3id.org/netbeheer/IECCIM/TC57CIM/IEC61970/Base/Domain#Conductance>
                                ] ,
                                [ rdf:type owl:Restriction ;
                                  owl:onProperty :MutualCoupling_r0 ;
                                  owl:maxQualifiedCardinality "1"^^xsd:nonNegativeInteger ;
                                  owl:onClass <https://w3id.org/netbeheer/IECCIM/TC57CIM/IEC61970/Base/Domain#Resistance>
                                ] ,
                                [ rdf:type owl:Restriction ;
                                  owl:onProperty :MutualCoupling_x0 ;
                                  owl:maxQualifiedCardinality "1"^^xsd:nonNegativeInteger ;
                                  owl:onClass <https://w3id.org/netbeheer/IECCIM/TC57CIM/IEC61970/Base/Domain#Reactance>
                                ] ;
                rdfs:comment """This class represents the zero sequence line mutual coupling.
""" .


###  https://w3id.org/netbeheer/IECCIM/TC57CIM/IEC61970/Base/Wires#NonlinearShuntCompensator
:NonlinearShuntCompensator rdf:type owl:Class ;
                           rdfs:subClassOf :ShuntCompensator ,
                                           [ rdf:type owl:Restriction ;
                                             owl:onProperty :NonlinearShuntCompensator_NonlinearShuntCompensatorPoints ;
                                             owl:qualifiedCardinality "1"^^xsd:nonNegativeInteger ;
                                             owl:onClass :NonlinearShuntCompensator
                                           ] ;
                           rdfs:comment "A non linear shunt compensator has bank or section admittance values that differs." .


###  https://w3id.org/netbeheer/IECCIM/TC57CIM/IEC61970/Base/Wires#NonlinearShuntCompensatorPhase
:NonlinearShuntCompensatorPhase rdf:type owl:Class ;
                                rdfs:subClassOf :ShuntCompensatorPhase ,
                                                [ rdf:type owl:Restriction ;
                                                  owl:onProperty :NonlinearShuntCompensatorPhase_NonlinearShuntCompensatorPhasePoints ;
                                                  owl:qualifiedCardinality "1"^^xsd:nonNegativeInteger ;
                                                  owl:onClass :NonlinearShuntCompensatorPhase
                                                ] ;
                                rdfs:comment "A per phase non linear shunt compensator has bank or section admittance values that differs." .


###  https://w3id.org/netbeheer/IECCIM/TC57CIM/IEC61970/Base/Wires#NonlinearShuntCompensatorPhasePoint
:NonlinearShuntCompensatorPhasePoint rdf:type owl:Class ;
                                     rdfs:subClassOf [ rdf:type owl:Restriction ;
                                                       owl:onProperty :NonlinearShuntCompensatorPhasePoint_NonlinearShuntCompensatorPhase ;
                                                       owl:minQualifiedCardinality "1"^^xsd:nonNegativeInteger ;
                                                       owl:onClass :NonlinearShuntCompensatorPhasePoint
                                                     ] ,
                                                     [ rdf:type owl:Restriction ;
                                                       owl:onProperty :NonlinearShuntCompensatorPhasePoint_b ;
                                                       owl:minQualifiedCardinality "0"^^xsd:nonNegativeInteger ;
                                                       owl:onClass <https://w3id.org/netbeheer/IECCIM/TC57CIM/IEC61970/Base/Domain#Susceptance>
                                                     ] ,
                                                     [ rdf:type owl:Restriction ;
                                                       owl:onProperty :NonlinearShuntCompensatorPhasePoint_g ;
                                                       owl:minQualifiedCardinality "0"^^xsd:nonNegativeInteger ;
                                                       owl:onClass <https://w3id.org/netbeheer/IECCIM/TC57CIM/IEC61970/Base/Domain#Conductance>
                                                     ] ,
                                                     [ rdf:type owl:Restriction ;
                                                       owl:onProperty :NonlinearShuntCompensatorPhasePoint_b ;
                                                       owl:maxQualifiedCardinality "1"^^xsd:nonNegativeInteger ;
                                                       owl:onClass <https://w3id.org/netbeheer/IECCIM/TC57CIM/IEC61970/Base/Domain#Susceptance>
                                                     ] ,
                                                     [ rdf:type owl:Restriction ;
                                                       owl:onProperty :NonlinearShuntCompensatorPhasePoint_g ;
                                                       owl:maxQualifiedCardinality "1"^^xsd:nonNegativeInteger ;
                                                       owl:onClass <https://w3id.org/netbeheer/IECCIM/TC57CIM/IEC61970/Base/Domain#Conductance>
                                                     ] ,
                                                     [ rdf:type owl:Restriction ;
                                                       owl:onProperty :NonlinearShuntCompensatorPhasePoint_sectionNumber ;
                                                       owl:minQualifiedCardinality "0"^^xsd:nonNegativeInteger ;
                                                       owl:onDataRange xsd:nonNegativeInteger
                                                     ] ,
                                                     [ rdf:type owl:Restriction ;
                                                       owl:onProperty :NonlinearShuntCompensatorPhasePoint_sectionNumber ;
                                                       owl:maxQualifiedCardinality "1"^^xsd:nonNegativeInteger ;
                                                       owl:onDataRange xsd:nonNegativeInteger
                                                     ] ;
                                     rdfs:comment "A per phase non linear shunt compensator bank or section admittance value." .


###  https://w3id.org/netbeheer/IECCIM/TC57CIM/IEC61970/Base/Wires#NonlinearShuntCompensatorPoint
:NonlinearShuntCompensatorPoint rdf:type owl:Class ;
                                rdfs:subClassOf [ rdf:type owl:Restriction ;
                                                  owl:onProperty :NonlinearShuntCompensatorPoint_NonlinearShuntCompensator ;
                                                  owl:minQualifiedCardinality "1"^^xsd:nonNegativeInteger ;
                                                  owl:onClass :NonlinearShuntCompensatorPoint
                                                ] ,
                                                [ rdf:type owl:Restriction ;
                                                  owl:onProperty :NonlinearShuntCompensatorPoint_b ;
                                                  owl:minQualifiedCardinality "0"^^xsd:nonNegativeInteger ;
                                                  owl:onClass <https://w3id.org/netbeheer/IECCIM/TC57CIM/IEC61970/Base/Domain#Susceptance>
                                                ] ,
                                                [ rdf:type owl:Restriction ;
                                                  owl:onProperty :NonlinearShuntCompensatorPoint_b0 ;
                                                  owl:minQualifiedCardinality "0"^^xsd:nonNegativeInteger ;
                                                  owl:onClass <https://w3id.org/netbeheer/IECCIM/TC57CIM/IEC61970/Base/Domain#Susceptance>
                                                ] ,
                                                [ rdf:type owl:Restriction ;
                                                  owl:onProperty :NonlinearShuntCompensatorPoint_g ;
                                                  owl:minQualifiedCardinality "0"^^xsd:nonNegativeInteger ;
                                                  owl:onClass <https://w3id.org/netbeheer/IECCIM/TC57CIM/IEC61970/Base/Domain#Conductance>
                                                ] ,
                                                [ rdf:type owl:Restriction ;
                                                  owl:onProperty :NonlinearShuntCompensatorPoint_g0 ;
                                                  owl:minQualifiedCardinality "0"^^xsd:nonNegativeInteger ;
                                                  owl:onClass <https://w3id.org/netbeheer/IECCIM/TC57CIM/IEC61970/Base/Domain#Conductance>
                                                ] ,
                                                [ rdf:type owl:Restriction ;
                                                  owl:onProperty :NonlinearShuntCompensatorPoint_b ;
                                                  owl:maxQualifiedCardinality "1"^^xsd:nonNegativeInteger ;
                                                  owl:onClass <https://w3id.org/netbeheer/IECCIM/TC57CIM/IEC61970/Base/Domain#Susceptance>
                                                ] ,
                                                [ rdf:type owl:Restriction ;
                                                  owl:onProperty :NonlinearShuntCompensatorPoint_b0 ;
                                                  owl:maxQualifiedCardinality "1"^^xsd:nonNegativeInteger ;
                                                  owl:onClass <https://w3id.org/netbeheer/IECCIM/TC57CIM/IEC61970/Base/Domain#Susceptance>
                                                ] ,
                                                [ rdf:type owl:Restriction ;
                                                  owl:onProperty :NonlinearShuntCompensatorPoint_g ;
                                                  owl:maxQualifiedCardinality "1"^^xsd:nonNegativeInteger ;
                                                  owl:onClass <https://w3id.org/netbeheer/IECCIM/TC57CIM/IEC61970/Base/Domain#Conductance>
                                                ] ,
                                                [ rdf:type owl:Restriction ;
                                                  owl:onProperty :NonlinearShuntCompensatorPoint_g0 ;
                                                  owl:maxQualifiedCardinality "1"^^xsd:nonNegativeInteger ;
                                                  owl:onClass <https://w3id.org/netbeheer/IECCIM/TC57CIM/IEC61970/Base/Domain#Conductance>
                                                ] ,
                                                [ rdf:type owl:Restriction ;
                                                  owl:onProperty :NonlinearShuntCompensatorPoint_sectionNumber ;
                                                  owl:minQualifiedCardinality "0"^^xsd:nonNegativeInteger ;
                                                  owl:onDataRange xsd:nonNegativeInteger
                                                ] ,
                                                [ rdf:type owl:Restriction ;
                                                  owl:onProperty :NonlinearShuntCompensatorPoint_sectionNumber ;
                                                  owl:maxQualifiedCardinality "1"^^xsd:nonNegativeInteger ;
                                                  owl:onDataRange xsd:nonNegativeInteger
                                                ] ;
                                rdfs:comment "A non linear shunt compensator bank or section admittance value." .


###  https://w3id.org/netbeheer/IECCIM/TC57CIM/IEC61970/Base/Wires#PerLengthImpedance
:PerLengthImpedance rdf:type owl:Class ;
                    rdfs:subClassOf :PerLengthLineParameter ,
                                    [ rdf:type owl:Restriction ;
                                      owl:onProperty :PerLengthImpedance_ACLineSegments ;
                                      owl:minQualifiedCardinality "0"^^xsd:nonNegativeInteger ;
                                      owl:onClass :PerLengthImpedance
                                    ] ,
                                    [ rdf:type owl:Restriction ;
                                      owl:onProperty :PerLengthImpedance_ACLineSegments ;
                                      owl:maxQualifiedCardinality "1"^^xsd:nonNegativeInteger ;
                                      owl:onClass :PerLengthImpedance
                                    ] ;
                    rdfs:comment """Common type for per-length impedance electrical catalogues.
""" .


###  https://w3id.org/netbeheer/IECCIM/TC57CIM/IEC61970/Base/Wires#PerLengthLineParameter
:PerLengthLineParameter rdf:type owl:Class ;
                        rdfs:subClassOf <https://w3id.org/netbeheer/IECCIM/TC57CIM/IEC61970/Base/Core#IdentifiedObject> ,
                                        [ rdf:type owl:Restriction ;
                                          owl:onProperty :PerLengthLineParameter_WireInfos ;
                                          owl:minQualifiedCardinality "0"^^xsd:nonNegativeInteger ;
                                          owl:onClass :PerLengthLineParameter
                                        ] ,
                                        [ rdf:type owl:Restriction ;
                                          owl:onProperty :PerLengthLineParameter_WireSpacingInfo ;
                                          owl:minQualifiedCardinality "0"^^xsd:nonNegativeInteger ;
                                          owl:onClass :PerLengthLineParameter
                                        ] ;
                        rdfs:comment "Common type for per-length electrical catalogues describing line parameters." .


###  https://w3id.org/netbeheer/IECCIM/TC57CIM/IEC61970/Base/Wires#PerLengthPhaseImpedance
:PerLengthPhaseImpedance rdf:type owl:Class ;
                         rdfs:subClassOf :PerLengthImpedance ,
                                         [ rdf:type owl:Restriction ;
                                           owl:onProperty :PerLengthPhaseImpedance_PhaseImpedanceData ;
                                           owl:qualifiedCardinality "1"^^xsd:nonNegativeInteger ;
                                           owl:onClass :PerLengthPhaseImpedance
                                         ] ,
                                         [ rdf:type owl:Restriction ;
                                           owl:onProperty :PerLengthPhaseImpedance_conductorCount ;
                                           owl:minQualifiedCardinality "0"^^xsd:nonNegativeInteger ;
                                           owl:onDataRange xsd:nonNegativeInteger
                                         ] ,
                                         [ rdf:type owl:Restriction ;
                                           owl:onProperty :PerLengthPhaseImpedance_conductorCount ;
                                           owl:maxQualifiedCardinality "1"^^xsd:nonNegativeInteger ;
                                           owl:onDataRange xsd:nonNegativeInteger
                                         ] ;
                         rdfs:comment "Impedance and admittance parameters per unit length for n-wire unbalanced lines, in matrix form." .


###  https://w3id.org/netbeheer/IECCIM/TC57CIM/IEC61970/Base/Wires#PerLengthSequenceImpedance
:PerLengthSequenceImpedance rdf:type owl:Class ;
                            rdfs:subClassOf :PerLengthImpedance ,
                                            [ rdf:type owl:Restriction ;
                                              owl:onProperty :PerLengthSequenceImpedance_b0ch ;
                                              owl:minQualifiedCardinality "0"^^xsd:nonNegativeInteger ;
                                              owl:onClass <https://w3id.org/netbeheer/IECCIM/TC57CIM/IEC61970/Base/Domain#SusceptancePerLength>
                                            ] ,
                                            [ rdf:type owl:Restriction ;
                                              owl:onProperty :PerLengthSequenceImpedance_bch ;
                                              owl:minQualifiedCardinality "0"^^xsd:nonNegativeInteger ;
                                              owl:onClass <https://w3id.org/netbeheer/IECCIM/TC57CIM/IEC61970/Base/Domain#SusceptancePerLength>
                                            ] ,
                                            [ rdf:type owl:Restriction ;
                                              owl:onProperty :PerLengthSequenceImpedance_g0ch ;
                                              owl:minQualifiedCardinality "0"^^xsd:nonNegativeInteger ;
                                              owl:onClass <https://w3id.org/netbeheer/IECCIM/TC57CIM/IEC61970/Base/Domain#ConductancePerLength>
                                            ] ,
                                            [ rdf:type owl:Restriction ;
                                              owl:onProperty :PerLengthSequenceImpedance_gch ;
                                              owl:minQualifiedCardinality "0"^^xsd:nonNegativeInteger ;
                                              owl:onClass <https://w3id.org/netbeheer/IECCIM/TC57CIM/IEC61970/Base/Domain#ConductancePerLength>
                                            ] ,
                                            [ rdf:type owl:Restriction ;
                                              owl:onProperty :PerLengthSequenceImpedance_r ;
                                              owl:minQualifiedCardinality "0"^^xsd:nonNegativeInteger ;
                                              owl:onClass <https://w3id.org/netbeheer/IECCIM/TC57CIM/IEC61970/Base/Domain#ResistancePerLength>
                                            ] ,
                                            [ rdf:type owl:Restriction ;
                                              owl:onProperty :PerLengthSequenceImpedance_r0 ;
                                              owl:minQualifiedCardinality "0"^^xsd:nonNegativeInteger ;
                                              owl:onClass <https://w3id.org/netbeheer/IECCIM/TC57CIM/IEC61970/Base/Domain#ResistancePerLength>
                                            ] ,
                                            [ rdf:type owl:Restriction ;
                                              owl:onProperty :PerLengthSequenceImpedance_x ;
                                              owl:minQualifiedCardinality "0"^^xsd:nonNegativeInteger ;
                                              owl:onClass <https://w3id.org/netbeheer/IECCIM/TC57CIM/IEC61970/Base/Domain#ReactancePerLength>
                                            ] ,
                                            [ rdf:type owl:Restriction ;
                                              owl:onProperty :PerLengthSequenceImpedance_x0 ;
                                              owl:minQualifiedCardinality "0"^^xsd:nonNegativeInteger ;
                                              owl:onClass <https://w3id.org/netbeheer/IECCIM/TC57CIM/IEC61970/Base/Domain#ReactancePerLength>
                                            ] ,
                                            [ rdf:type owl:Restriction ;
                                              owl:onProperty :PerLengthSequenceImpedance_b0ch ;
                                              owl:maxQualifiedCardinality "1"^^xsd:nonNegativeInteger ;
                                              owl:onClass <https://w3id.org/netbeheer/IECCIM/TC57CIM/IEC61970/Base/Domain#SusceptancePerLength>
                                            ] ,
                                            [ rdf:type owl:Restriction ;
                                              owl:onProperty :PerLengthSequenceImpedance_bch ;
                                              owl:maxQualifiedCardinality "1"^^xsd:nonNegativeInteger ;
                                              owl:onClass <https://w3id.org/netbeheer/IECCIM/TC57CIM/IEC61970/Base/Domain#SusceptancePerLength>
                                            ] ,
                                            [ rdf:type owl:Restriction ;
                                              owl:onProperty :PerLengthSequenceImpedance_g0ch ;
                                              owl:maxQualifiedCardinality "1"^^xsd:nonNegativeInteger ;
                                              owl:onClass <https://w3id.org/netbeheer/IECCIM/TC57CIM/IEC61970/Base/Domain#ConductancePerLength>
                                            ] ,
                                            [ rdf:type owl:Restriction ;
                                              owl:onProperty :PerLengthSequenceImpedance_gch ;
                                              owl:maxQualifiedCardinality "1"^^xsd:nonNegativeInteger ;
                                              owl:onClass <https://w3id.org/netbeheer/IECCIM/TC57CIM/IEC61970/Base/Domain#ConductancePerLength>
                                            ] ,
                                            [ rdf:type owl:Restriction ;
                                              owl:onProperty :PerLengthSequenceImpedance_r ;
                                              owl:maxQualifiedCardinality "1"^^xsd:nonNegativeInteger ;
                                              owl:onClass <https://w3id.org/netbeheer/IECCIM/TC57CIM/IEC61970/Base/Domain#ResistancePerLength>
                                            ] ,
                                            [ rdf:type owl:Restriction ;
                                              owl:onProperty :PerLengthSequenceImpedance_r0 ;
                                              owl:maxQualifiedCardinality "1"^^xsd:nonNegativeInteger ;
                                              owl:onClass <https://w3id.org/netbeheer/IECCIM/TC57CIM/IEC61970/Base/Domain#ResistancePerLength>
                                            ] ,
                                            [ rdf:type owl:Restriction ;
                                              owl:onProperty :PerLengthSequenceImpedance_x ;
                                              owl:maxQualifiedCardinality "1"^^xsd:nonNegativeInteger ;
                                              owl:onClass <https://w3id.org/netbeheer/IECCIM/TC57CIM/IEC61970/Base/Domain#ReactancePerLength>
                                            ] ,
                                            [ rdf:type owl:Restriction ;
                                              owl:onProperty :PerLengthSequenceImpedance_x0 ;
                                              owl:maxQualifiedCardinality "1"^^xsd:nonNegativeInteger ;
                                              owl:onClass <https://w3id.org/netbeheer/IECCIM/TC57CIM/IEC61970/Base/Domain#ReactancePerLength>
                                            ] ;
                            rdfs:comment "Sequence impedance and admittance parameters per unit length, for transposed lines of 1, 2, or 3 phases. For 1-phase lines, define x=x0=xself. For 2-phase lines, define x=xs-xm and x0=xs+xm." .


###  https://w3id.org/netbeheer/IECCIM/TC57CIM/IEC61970/Base/Wires#PetersenCoil
:PetersenCoil rdf:type owl:Class ;
              rdfs:subClassOf :EarthFaultCompensator ,
                              [ rdf:type owl:Restriction ;
                                owl:onProperty :PetersenCoil_nominalU ;
                                owl:minQualifiedCardinality "0"^^xsd:nonNegativeInteger ;
                                owl:onClass <https://w3id.org/netbeheer/IECCIM/TC57CIM/IEC61970/Base/Domain#Voltage>
                              ] ,
                              [ rdf:type owl:Restriction ;
                                owl:onProperty :PetersenCoil_offsetCurrent ;
                                owl:minQualifiedCardinality "0"^^xsd:nonNegativeInteger ;
                                owl:onClass <https://w3id.org/netbeheer/IECCIM/TC57CIM/IEC61970/Base/Domain#CurrentFlow>
                              ] ,
                              [ rdf:type owl:Restriction ;
                                owl:onProperty :PetersenCoil_positionCurrent ;
                                owl:minQualifiedCardinality "0"^^xsd:nonNegativeInteger ;
                                owl:onClass <https://w3id.org/netbeheer/IECCIM/TC57CIM/IEC61970/Base/Domain#CurrentFlow>
                              ] ,
                              [ rdf:type owl:Restriction ;
                                owl:onProperty :PetersenCoil_xGroundMax ;
                                owl:minQualifiedCardinality "0"^^xsd:nonNegativeInteger ;
                                owl:onClass <https://w3id.org/netbeheer/IECCIM/TC57CIM/IEC61970/Base/Domain#Reactance>
                              ] ,
                              [ rdf:type owl:Restriction ;
                                owl:onProperty :PetersenCoil_xGroundMin ;
                                owl:minQualifiedCardinality "0"^^xsd:nonNegativeInteger ;
                                owl:onClass <https://w3id.org/netbeheer/IECCIM/TC57CIM/IEC61970/Base/Domain#Reactance>
                              ] ,
                              [ rdf:type owl:Restriction ;
                                owl:onProperty :PetersenCoil_xGroundNominal ;
                                owl:minQualifiedCardinality "0"^^xsd:nonNegativeInteger ;
                                owl:onClass <https://w3id.org/netbeheer/IECCIM/TC57CIM/IEC61970/Base/Domain#Reactance>
                              ] ,
                              [ rdf:type owl:Restriction ;
                                owl:onProperty :PetersenCoil_nominalU ;
                                owl:maxQualifiedCardinality "1"^^xsd:nonNegativeInteger ;
                                owl:onClass <https://w3id.org/netbeheer/IECCIM/TC57CIM/IEC61970/Base/Domain#Voltage>
                              ] ,
                              [ rdf:type owl:Restriction ;
                                owl:onProperty :PetersenCoil_offsetCurrent ;
                                owl:maxQualifiedCardinality "1"^^xsd:nonNegativeInteger ;
                                owl:onClass <https://w3id.org/netbeheer/IECCIM/TC57CIM/IEC61970/Base/Domain#CurrentFlow>
                              ] ,
                              [ rdf:type owl:Restriction ;
                                owl:onProperty :PetersenCoil_positionCurrent ;
                                owl:maxQualifiedCardinality "1"^^xsd:nonNegativeInteger ;
                                owl:onClass <https://w3id.org/netbeheer/IECCIM/TC57CIM/IEC61970/Base/Domain#CurrentFlow>
                              ] ,
                              [ rdf:type owl:Restriction ;
                                owl:onProperty :PetersenCoil_xGroundMax ;
                                owl:maxQualifiedCardinality "1"^^xsd:nonNegativeInteger ;
                                owl:onClass <https://w3id.org/netbeheer/IECCIM/TC57CIM/IEC61970/Base/Domain#Reactance>
                              ] ,
                              [ rdf:type owl:Restriction ;
                                owl:onProperty :PetersenCoil_xGroundMin ;
                                owl:maxQualifiedCardinality "1"^^xsd:nonNegativeInteger ;
                                owl:onClass <https://w3id.org/netbeheer/IECCIM/TC57CIM/IEC61970/Base/Domain#Reactance>
                              ] ,
                              [ rdf:type owl:Restriction ;
                                owl:onProperty :PetersenCoil_xGroundNominal ;
                                owl:maxQualifiedCardinality "1"^^xsd:nonNegativeInteger ;
                                owl:onClass <https://w3id.org/netbeheer/IECCIM/TC57CIM/IEC61970/Base/Domain#Reactance>
                              ] ,
                              [ rdf:type owl:Restriction ;
                                owl:onProperty :PetersenCoil_mode ;
                                owl:minQualifiedCardinality "0"^^xsd:nonNegativeInteger ;
                                owl:onDataRange :PetersenCoilModeKind
                              ] ,
                              [ rdf:type owl:Restriction ;
                                owl:onProperty :PetersenCoil_mode ;
                                owl:maxQualifiedCardinality "1"^^xsd:nonNegativeInteger ;
                                owl:onDataRange :PetersenCoilModeKind
                              ] ;
              rdfs:comment "A tunable impedance device normally used to offset line charging during single line faults in an ungrounded section of network." .


###  https://w3id.org/netbeheer/IECCIM/TC57CIM/IEC61970/Base/Wires#PhaseImpedanceData
:PhaseImpedanceData rdf:type owl:Class ;
                    rdfs:subClassOf [ rdf:type owl:Restriction ;
                                      owl:onProperty :PhaseImpedanceData_PhaseImpedance ;
                                      owl:minQualifiedCardinality "1"^^xsd:nonNegativeInteger ;
                                      owl:onClass :PhaseImpedanceData
                                    ] ,
                                    [ rdf:type owl:Restriction ;
                                      owl:onProperty :PhaseImpedanceData_b ;
                                      owl:minQualifiedCardinality "0"^^xsd:nonNegativeInteger ;
                                      owl:onClass <https://w3id.org/netbeheer/IECCIM/TC57CIM/IEC61970/Base/Domain#SusceptancePerLength>
                                    ] ,
                                    [ rdf:type owl:Restriction ;
                                      owl:onProperty :PhaseImpedanceData_r ;
                                      owl:minQualifiedCardinality "0"^^xsd:nonNegativeInteger ;
                                      owl:onClass <https://w3id.org/netbeheer/IECCIM/TC57CIM/IEC61970/Base/Domain#ResistancePerLength>
                                    ] ,
                                    [ rdf:type owl:Restriction ;
                                      owl:onProperty :PhaseImpedanceData_x ;
                                      owl:minQualifiedCardinality "0"^^xsd:nonNegativeInteger ;
                                      owl:onClass <https://w3id.org/netbeheer/IECCIM/TC57CIM/IEC61970/Base/Domain#ReactancePerLength>
                                    ] ,
                                    [ rdf:type owl:Restriction ;
                                      owl:onProperty :PhaseImpedanceData_b ;
                                      owl:maxQualifiedCardinality "1"^^xsd:nonNegativeInteger ;
                                      owl:onClass <https://w3id.org/netbeheer/IECCIM/TC57CIM/IEC61970/Base/Domain#SusceptancePerLength>
                                    ] ,
                                    [ rdf:type owl:Restriction ;
                                      owl:onProperty :PhaseImpedanceData_r ;
                                      owl:maxQualifiedCardinality "1"^^xsd:nonNegativeInteger ;
                                      owl:onClass <https://w3id.org/netbeheer/IECCIM/TC57CIM/IEC61970/Base/Domain#ResistancePerLength>
                                    ] ,
                                    [ rdf:type owl:Restriction ;
                                      owl:onProperty :PhaseImpedanceData_x ;
                                      owl:maxQualifiedCardinality "1"^^xsd:nonNegativeInteger ;
                                      owl:onClass <https://w3id.org/netbeheer/IECCIM/TC57CIM/IEC61970/Base/Domain#ReactancePerLength>
                                    ] ,
                                    [ rdf:type owl:Restriction ;
                                      owl:onProperty :PhaseImpedanceData_sequenceNumber ;
                                      owl:minQualifiedCardinality "0"^^xsd:nonNegativeInteger ;
                                      owl:onDataRange xsd:nonNegativeInteger
                                    ] ,
                                    [ rdf:type owl:Restriction ;
                                      owl:onProperty :PhaseImpedanceData_sequenceNumber ;
                                      owl:maxQualifiedCardinality "1"^^xsd:nonNegativeInteger ;
                                      owl:onDataRange xsd:nonNegativeInteger
                                    ] ;
                    rdfs:comment "Triplet of resistance, reactance, and susceptance matrix element values." .


###  https://w3id.org/netbeheer/IECCIM/TC57CIM/IEC61970/Base/Wires#PhaseTapChanger
:PhaseTapChanger rdf:type owl:Class ;
                 rdfs:subClassOf :TapChanger ,
                                 [ rdf:type owl:Restriction ;
                                   owl:onProperty :PhaseTapChanger_TransformerEnd ;
                                   owl:minQualifiedCardinality "0"^^xsd:nonNegativeInteger ;
                                   owl:onClass :PhaseTapChanger
                                 ] ,
                                 [ rdf:type owl:Restriction ;
                                   owl:onProperty :PhaseTapChanger_TransformerEnd ;
                                   owl:maxQualifiedCardinality "1"^^xsd:nonNegativeInteger ;
                                   owl:onClass :PhaseTapChanger
                                 ] ;
                 rdfs:comment "A transformer phase shifting tap model that controls the phase angle difference across the power transformer and potentially the active power flow through the power transformer.  This phase tap model may also impact the voltage magnitude." .


###  https://w3id.org/netbeheer/IECCIM/TC57CIM/IEC61970/Base/Wires#PhaseTapChangerAsymmetrical
:PhaseTapChangerAsymmetrical rdf:type owl:Class ;
                             rdfs:subClassOf :PhaseTapChangerNonLinear ,
                                             [ rdf:type owl:Restriction ;
                                               owl:onProperty :PhaseTapChangerAsymmetrical_windingConnectionAngle ;
                                               owl:minQualifiedCardinality "0"^^xsd:nonNegativeInteger ;
                                               owl:onClass <https://w3id.org/netbeheer/IECCIM/TC57CIM/IEC61970/Base/Domain#AngleDegrees>
                                             ] ,
                                             [ rdf:type owl:Restriction ;
                                               owl:onProperty :PhaseTapChangerAsymmetrical_windingConnectionAngle ;
                                               owl:maxQualifiedCardinality "1"^^xsd:nonNegativeInteger ;
                                               owl:onClass <https://w3id.org/netbeheer/IECCIM/TC57CIM/IEC61970/Base/Domain#AngleDegrees>
                                             ] ;
                             rdfs:comment "Describes the tap model for an asymmetrical phase shifting transformer in which the difference voltage vector adds to the primary side voltage. The angle between the primary side voltage and the difference voltage is named the winding connection angle. The phase shift depends on both the difference voltage magnitude and the winding connection angle." .


###  https://w3id.org/netbeheer/IECCIM/TC57CIM/IEC61970/Base/Wires#PhaseTapChangerLinear
:PhaseTapChangerLinear rdf:type owl:Class ;
                       rdfs:subClassOf :PhaseTapChanger ,
                                       [ rdf:type owl:Restriction ;
                                         owl:onProperty :PhaseTapChangerLinear_stepPhaseShiftIncrement ;
                                         owl:minQualifiedCardinality "0"^^xsd:nonNegativeInteger ;
                                         owl:onClass <https://w3id.org/netbeheer/IECCIM/TC57CIM/IEC61970/Base/Domain#AngleDegrees>
                                       ] ,
                                       [ rdf:type owl:Restriction ;
                                         owl:onProperty :PhaseTapChangerLinear_xMax ;
                                         owl:minQualifiedCardinality "0"^^xsd:nonNegativeInteger ;
                                         owl:onClass <https://w3id.org/netbeheer/IECCIM/TC57CIM/IEC61970/Base/Domain#Reactance>
                                       ] ,
                                       [ rdf:type owl:Restriction ;
                                         owl:onProperty :PhaseTapChangerLinear_xMin ;
                                         owl:minQualifiedCardinality "0"^^xsd:nonNegativeInteger ;
                                         owl:onClass <https://w3id.org/netbeheer/IECCIM/TC57CIM/IEC61970/Base/Domain#Reactance>
                                       ] ,
                                       [ rdf:type owl:Restriction ;
                                         owl:onProperty :PhaseTapChangerLinear_stepPhaseShiftIncrement ;
                                         owl:maxQualifiedCardinality "1"^^xsd:nonNegativeInteger ;
                                         owl:onClass <https://w3id.org/netbeheer/IECCIM/TC57CIM/IEC61970/Base/Domain#AngleDegrees>
                                       ] ,
                                       [ rdf:type owl:Restriction ;
                                         owl:onProperty :PhaseTapChangerLinear_xMax ;
                                         owl:maxQualifiedCardinality "1"^^xsd:nonNegativeInteger ;
                                         owl:onClass <https://w3id.org/netbeheer/IECCIM/TC57CIM/IEC61970/Base/Domain#Reactance>
                                       ] ,
                                       [ rdf:type owl:Restriction ;
                                         owl:onProperty :PhaseTapChangerLinear_xMin ;
                                         owl:maxQualifiedCardinality "1"^^xsd:nonNegativeInteger ;
                                         owl:onClass <https://w3id.org/netbeheer/IECCIM/TC57CIM/IEC61970/Base/Domain#Reactance>
                                       ] ;
                       rdfs:comment """Describes a tap changer with a linear relation between the tap step and the phase angle difference across the transformer. This is a mathematical model that is an approximation of a real phase tap changer.
The phase angle is computed as stepPhaseShitfIncrement times the tap position.
The secondary side voltage magnitude is the same as at the primary side.""" .


###  https://w3id.org/netbeheer/IECCIM/TC57CIM/IEC61970/Base/Wires#PhaseTapChangerNonLinear
:PhaseTapChangerNonLinear rdf:type owl:Class ;
                          rdfs:subClassOf :PhaseTapChanger ,
                                          [ rdf:type owl:Restriction ;
                                            owl:onProperty :PhaseTapChangerNonLinear_voltageStepIncrement ;
                                            owl:minQualifiedCardinality "0"^^xsd:nonNegativeInteger ;
                                            owl:onClass <https://w3id.org/netbeheer/IECCIM/TC57CIM/IEC61970/Base/Domain#PerCent>
                                          ] ,
                                          [ rdf:type owl:Restriction ;
                                            owl:onProperty :PhaseTapChangerNonLinear_xMax ;
                                            owl:minQualifiedCardinality "0"^^xsd:nonNegativeInteger ;
                                            owl:onClass <https://w3id.org/netbeheer/IECCIM/TC57CIM/IEC61970/Base/Domain#Reactance>
                                          ] ,
                                          [ rdf:type owl:Restriction ;
                                            owl:onProperty :PhaseTapChangerNonLinear_xMin ;
                                            owl:minQualifiedCardinality "0"^^xsd:nonNegativeInteger ;
                                            owl:onClass <https://w3id.org/netbeheer/IECCIM/TC57CIM/IEC61970/Base/Domain#Reactance>
                                          ] ,
                                          [ rdf:type owl:Restriction ;
                                            owl:onProperty :PhaseTapChangerNonLinear_voltageStepIncrement ;
                                            owl:maxQualifiedCardinality "1"^^xsd:nonNegativeInteger ;
                                            owl:onClass <https://w3id.org/netbeheer/IECCIM/TC57CIM/IEC61970/Base/Domain#PerCent>
                                          ] ,
                                          [ rdf:type owl:Restriction ;
                                            owl:onProperty :PhaseTapChangerNonLinear_xMax ;
                                            owl:maxQualifiedCardinality "1"^^xsd:nonNegativeInteger ;
                                            owl:onClass <https://w3id.org/netbeheer/IECCIM/TC57CIM/IEC61970/Base/Domain#Reactance>
                                          ] ,
                                          [ rdf:type owl:Restriction ;
                                            owl:onProperty :PhaseTapChangerNonLinear_xMin ;
                                            owl:maxQualifiedCardinality "1"^^xsd:nonNegativeInteger ;
                                            owl:onClass <https://w3id.org/netbeheer/IECCIM/TC57CIM/IEC61970/Base/Domain#Reactance>
                                          ] ;
                          rdfs:comment "The non-linear phase tap changer describes the non-linear behavior of a phase tap changer. This is a base class for the symmetrical and asymmetrical phase tap changer models. The details of these models can be found in the IEC 61970-301 document." .


###  https://w3id.org/netbeheer/IECCIM/TC57CIM/IEC61970/Base/Wires#PhaseTapChangerSymmetrical
:PhaseTapChangerSymmetrical rdf:type owl:Class ;
                            rdfs:subClassOf :PhaseTapChangerNonLinear ;
                            rdfs:comment "Describes a symmetrical phase shifting transformer tap model in which the secondary side voltage magnitude is the same as at the primary side. The difference voltage magnitude is the base in an equal-sided triangle where the sides corresponds to the primary and secondary voltages. The phase angle difference corresponds to the top angle and can be expressed as twice the arctangent of half the total difference voltage." .


###  https://w3id.org/netbeheer/IECCIM/TC57CIM/IEC61970/Base/Wires#PhaseTapChangerTable
:PhaseTapChangerTable rdf:type owl:Class ;
                      rdfs:subClassOf <https://w3id.org/netbeheer/IECCIM/TC57CIM/IEC61970/Base/Core#IdentifiedObject> ,
                                      [ rdf:type owl:Restriction ;
                                        owl:onProperty :PhaseTapChangerTable_PhaseTapChangerTabular ;
                                        owl:minQualifiedCardinality "0"^^xsd:nonNegativeInteger ;
                                        owl:onClass :PhaseTapChangerTable
                                      ] ,
                                      [ rdf:type owl:Restriction ;
                                        owl:onProperty :PhaseTapChangerTable_PhaseTapChangerTablePoint ;
                                        owl:qualifiedCardinality "1"^^xsd:nonNegativeInteger ;
                                        owl:onClass :PhaseTapChangerTable
                                      ] ,
                                      [ rdf:type owl:Restriction ;
                                        owl:onProperty :PhaseTapChangerTable_PhaseTapChangerTabular ;
                                        owl:maxQualifiedCardinality "1"^^xsd:nonNegativeInteger ;
                                        owl:onClass :PhaseTapChangerTable
                                      ] ;
                      rdfs:comment "Describes a tabular curve for how the phase angle difference and impedance varies with the tap step." .


###  https://w3id.org/netbeheer/IECCIM/TC57CIM/IEC61970/Base/Wires#PhaseTapChangerTablePoint
:PhaseTapChangerTablePoint rdf:type owl:Class ;
                           rdfs:subClassOf :TapChangerTablePoint ,
                                           [ rdf:type owl:Restriction ;
                                             owl:onProperty :PhaseTapChangerTablePoint_PhaseTapChangerTable ;
                                             owl:minQualifiedCardinality "1"^^xsd:nonNegativeInteger ;
                                             owl:onClass :PhaseTapChangerTablePoint
                                           ] ,
                                           [ rdf:type owl:Restriction ;
                                             owl:onProperty :PhaseTapChangerTablePoint_angle ;
                                             owl:minQualifiedCardinality "0"^^xsd:nonNegativeInteger ;
                                             owl:onClass <https://w3id.org/netbeheer/IECCIM/TC57CIM/IEC61970/Base/Domain#AngleDegrees>
                                           ] ,
                                           [ rdf:type owl:Restriction ;
                                             owl:onProperty :PhaseTapChangerTablePoint_angle ;
                                             owl:maxQualifiedCardinality "1"^^xsd:nonNegativeInteger ;
                                             owl:onClass <https://w3id.org/netbeheer/IECCIM/TC57CIM/IEC61970/Base/Domain#AngleDegrees>
                                           ] ;
                           rdfs:comment """Describes each tap step in the phase tap changer tabular curve.
""" .


###  https://w3id.org/netbeheer/IECCIM/TC57CIM/IEC61970/Base/Wires#PhaseTapChangerTabular
:PhaseTapChangerTabular rdf:type owl:Class ;
                        rdfs:subClassOf :PhaseTapChanger ,
                                        [ rdf:type owl:Restriction ;
                                          owl:onProperty :PhaseTapChangerTabular_PhaseTapChangerTable ;
                                          owl:minQualifiedCardinality "0"^^xsd:nonNegativeInteger ;
                                          owl:onClass :PhaseTapChangerTabular
                                        ] .


###  https://w3id.org/netbeheer/IECCIM/TC57CIM/IEC61970/Base/Wires#Plant
:Plant rdf:type owl:Class ;
       rdfs:subClassOf <https://w3id.org/netbeheer/IECCIM/TC57CIM/IEC61970/Base/Core#EquipmentContainer> ;
       rdfs:comment "A Plant is a collection of equipment for purposes of generation." .


###  https://w3id.org/netbeheer/IECCIM/TC57CIM/IEC61970/Base/Wires#PowerTransformer
:PowerTransformer rdf:type owl:Class ;
                  rdfs:subClassOf <https://w3id.org/netbeheer/IECCIM/TC57CIM/IEC61970/Base/Core#ConductingEquipment> ,
                                  [ rdf:type owl:Restriction ;
                                    owl:onProperty :PowerTransformer_PowerTransformerEnd ;
                                    owl:minQualifiedCardinality "0"^^xsd:nonNegativeInteger ;
                                    owl:onClass :PowerTransformer
                                  ] ,
                                  [ rdf:type owl:Restriction ;
                                    owl:onProperty :PowerTransformer_TransformerTanks ;
                                    owl:minQualifiedCardinality "0"^^xsd:nonNegativeInteger ;
                                    owl:onClass :PowerTransformer
                                  ] ,
                                  [ rdf:type owl:Restriction ;
                                    owl:onProperty :PowerTransformer_beforeShCircuitHighestOperatingCurrent ;
                                    owl:minQualifiedCardinality "0"^^xsd:nonNegativeInteger ;
                                    owl:onClass <https://w3id.org/netbeheer/IECCIM/TC57CIM/IEC61970/Base/Domain#CurrentFlow>
                                  ] ,
                                  [ rdf:type owl:Restriction ;
                                    owl:onProperty :PowerTransformer_beforeShCircuitHighestOperatingVoltage ;
                                    owl:minQualifiedCardinality "0"^^xsd:nonNegativeInteger ;
                                    owl:onClass <https://w3id.org/netbeheer/IECCIM/TC57CIM/IEC61970/Base/Domain#Voltage>
                                  ] ,
                                  [ rdf:type owl:Restriction ;
                                    owl:onProperty :PowerTransformer_beforeShortCircuitAnglePf ;
                                    owl:minQualifiedCardinality "0"^^xsd:nonNegativeInteger ;
                                    owl:onClass <https://w3id.org/netbeheer/IECCIM/TC57CIM/IEC61970/Base/Domain#AngleDegrees>
                                  ] ,
                                  [ rdf:type owl:Restriction ;
                                    owl:onProperty :PowerTransformer_highSideMinOperatingU ;
                                    owl:minQualifiedCardinality "0"^^xsd:nonNegativeInteger ;
                                    owl:onClass <https://w3id.org/netbeheer/IECCIM/TC57CIM/IEC61970/Base/Domain#Voltage>
                                  ] ,
                                  [ rdf:type owl:Restriction ;
                                    owl:onProperty :PowerTransformer_PowerTransformerEnd ;
                                    owl:maxQualifiedCardinality "1"^^xsd:nonNegativeInteger ;
                                    owl:onClass :PowerTransformer
                                  ] ,
                                  [ rdf:type owl:Restriction ;
                                    owl:onProperty :PowerTransformer_TransformerTanks ;
                                    owl:maxQualifiedCardinality "1"^^xsd:nonNegativeInteger ;
                                    owl:onClass :PowerTransformer
                                  ] ,
                                  [ rdf:type owl:Restriction ;
                                    owl:onProperty :PowerTransformer_beforeShCircuitHighestOperatingCurrent ;
                                    owl:maxQualifiedCardinality "1"^^xsd:nonNegativeInteger ;
                                    owl:onClass <https://w3id.org/netbeheer/IECCIM/TC57CIM/IEC61970/Base/Domain#CurrentFlow>
                                  ] ,
                                  [ rdf:type owl:Restriction ;
                                    owl:onProperty :PowerTransformer_beforeShCircuitHighestOperatingVoltage ;
                                    owl:maxQualifiedCardinality "1"^^xsd:nonNegativeInteger ;
                                    owl:onClass <https://w3id.org/netbeheer/IECCIM/TC57CIM/IEC61970/Base/Domain#Voltage>
                                  ] ,
                                  [ rdf:type owl:Restriction ;
                                    owl:onProperty :PowerTransformer_beforeShortCircuitAnglePf ;
                                    owl:maxQualifiedCardinality "1"^^xsd:nonNegativeInteger ;
                                    owl:onClass <https://w3id.org/netbeheer/IECCIM/TC57CIM/IEC61970/Base/Domain#AngleDegrees>
                                  ] ,
                                  [ rdf:type owl:Restriction ;
                                    owl:onProperty :PowerTransformer_highSideMinOperatingU ;
                                    owl:maxQualifiedCardinality "1"^^xsd:nonNegativeInteger ;
                                    owl:onClass <https://w3id.org/netbeheer/IECCIM/TC57CIM/IEC61970/Base/Domain#Voltage>
                                  ] ,
                                  [ rdf:type owl:Restriction ;
                                    owl:onProperty :PowerTransformer_isPartOfGeneratorUnit ;
                                    owl:minQualifiedCardinality "0"^^xsd:nonNegativeInteger ;
                                    owl:onDataRange xsd:boolean
                                  ] ,
                                  [ rdf:type owl:Restriction ;
                                    owl:onProperty :PowerTransformer_operationalValuesConsidered ;
                                    owl:minQualifiedCardinality "0"^^xsd:nonNegativeInteger ;
                                    owl:onDataRange xsd:boolean
                                  ] ,
                                  [ rdf:type owl:Restriction ;
                                    owl:onProperty :PowerTransformer_vectorGroup ;
                                    owl:minQualifiedCardinality "0"^^xsd:nonNegativeInteger ;
                                    owl:onDataRange xsd:string
                                  ] ,
                                  [ rdf:type owl:Restriction ;
                                    owl:onProperty :PowerTransformer_isPartOfGeneratorUnit ;
                                    owl:maxQualifiedCardinality "1"^^xsd:nonNegativeInteger ;
                                    owl:onDataRange xsd:boolean
                                  ] ,
                                  [ rdf:type owl:Restriction ;
                                    owl:onProperty :PowerTransformer_operationalValuesConsidered ;
                                    owl:maxQualifiedCardinality "1"^^xsd:nonNegativeInteger ;
                                    owl:onDataRange xsd:boolean
                                  ] ,
                                  [ rdf:type owl:Restriction ;
                                    owl:onProperty :PowerTransformer_vectorGroup ;
                                    owl:maxQualifiedCardinality "1"^^xsd:nonNegativeInteger ;
                                    owl:onDataRange xsd:string
                                  ] ;
                  rdfs:comment """An electrical device consisting of  two or more coupled windings, with or without a magnetic core, for introducing mutual coupling between electric circuits. Transformers can be used to control voltage and phase shift (active power flow).
A power transformer may be composed of separate transformer tanks that need not be identical.
A power transformer can be modeled with or without tanks and is intended for use in both balanced and unbalanced representations.   A power transformer typically has two terminals, but may have one (grounding), three or more terminals.
The inherited association ConductingEquipment.BaseVoltage should not be used.  The association from TransformerEnd to BaseVoltage should be used instead.""" .


###  https://w3id.org/netbeheer/IECCIM/TC57CIM/IEC61970/Base/Wires#PowerTransformerEnd
:PowerTransformerEnd rdf:type owl:Class ;
                     rdfs:subClassOf :TransformerEnd ,
                                     [ rdf:type owl:Restriction ;
                                       owl:onProperty :PowerTransformerEnd_PowerTransformer ;
                                       owl:minQualifiedCardinality "0"^^xsd:nonNegativeInteger ;
                                       owl:onClass :PowerTransformerEnd
                                     ] ,
                                     [ rdf:type owl:Restriction ;
                                       owl:onProperty :PowerTransformerEnd_b ;
                                       owl:minQualifiedCardinality "0"^^xsd:nonNegativeInteger ;
                                       owl:onClass <https://w3id.org/netbeheer/IECCIM/TC57CIM/IEC61970/Base/Domain#Susceptance>
                                     ] ,
                                     [ rdf:type owl:Restriction ;
                                       owl:onProperty :PowerTransformerEnd_b0 ;
                                       owl:minQualifiedCardinality "0"^^xsd:nonNegativeInteger ;
                                       owl:onClass <https://w3id.org/netbeheer/IECCIM/TC57CIM/IEC61970/Base/Domain#Susceptance>
                                     ] ,
                                     [ rdf:type owl:Restriction ;
                                       owl:onProperty :PowerTransformerEnd_g ;
                                       owl:minQualifiedCardinality "0"^^xsd:nonNegativeInteger ;
                                       owl:onClass <https://w3id.org/netbeheer/IECCIM/TC57CIM/IEC61970/Base/Domain#Conductance>
                                     ] ,
                                     [ rdf:type owl:Restriction ;
                                       owl:onProperty :PowerTransformerEnd_g0 ;
                                       owl:minQualifiedCardinality "0"^^xsd:nonNegativeInteger ;
                                       owl:onClass <https://w3id.org/netbeheer/IECCIM/TC57CIM/IEC61970/Base/Domain#Conductance>
                                     ] ,
                                     [ rdf:type owl:Restriction ;
                                       owl:onProperty :PowerTransformerEnd_r ;
                                       owl:minQualifiedCardinality "0"^^xsd:nonNegativeInteger ;
                                       owl:onClass <https://w3id.org/netbeheer/IECCIM/TC57CIM/IEC61970/Base/Domain#Resistance>
                                     ] ,
                                     [ rdf:type owl:Restriction ;
                                       owl:onProperty :PowerTransformerEnd_r0 ;
                                       owl:minQualifiedCardinality "0"^^xsd:nonNegativeInteger ;
                                       owl:onClass <https://w3id.org/netbeheer/IECCIM/TC57CIM/IEC61970/Base/Domain#Resistance>
                                     ] ,
                                     [ rdf:type owl:Restriction ;
                                       owl:onProperty :PowerTransformerEnd_ratedS ;
                                       owl:minQualifiedCardinality "0"^^xsd:nonNegativeInteger ;
                                       owl:onClass <https://w3id.org/netbeheer/IECCIM/TC57CIM/IEC61970/Base/Domain#ApparentPower>
                                     ] ,
                                     [ rdf:type owl:Restriction ;
                                       owl:onProperty :PowerTransformerEnd_ratedU ;
                                       owl:minQualifiedCardinality "0"^^xsd:nonNegativeInteger ;
                                       owl:onClass <https://w3id.org/netbeheer/IECCIM/TC57CIM/IEC61970/Base/Domain#Voltage>
                                     ] ,
                                     [ rdf:type owl:Restriction ;
                                       owl:onProperty :PowerTransformerEnd_x ;
                                       owl:minQualifiedCardinality "0"^^xsd:nonNegativeInteger ;
                                       owl:onClass <https://w3id.org/netbeheer/IECCIM/TC57CIM/IEC61970/Base/Domain#Reactance>
                                     ] ,
                                     [ rdf:type owl:Restriction ;
                                       owl:onProperty :PowerTransformerEnd_x0 ;
                                       owl:minQualifiedCardinality "0"^^xsd:nonNegativeInteger ;
                                       owl:onClass <https://w3id.org/netbeheer/IECCIM/TC57CIM/IEC61970/Base/Domain#Reactance>
                                     ] ,
                                     [ rdf:type owl:Restriction ;
                                       owl:onProperty :PowerTransformerEnd_b ;
                                       owl:maxQualifiedCardinality "1"^^xsd:nonNegativeInteger ;
                                       owl:onClass <https://w3id.org/netbeheer/IECCIM/TC57CIM/IEC61970/Base/Domain#Susceptance>
                                     ] ,
                                     [ rdf:type owl:Restriction ;
                                       owl:onProperty :PowerTransformerEnd_b0 ;
                                       owl:maxQualifiedCardinality "1"^^xsd:nonNegativeInteger ;
                                       owl:onClass <https://w3id.org/netbeheer/IECCIM/TC57CIM/IEC61970/Base/Domain#Susceptance>
                                     ] ,
                                     [ rdf:type owl:Restriction ;
                                       owl:onProperty :PowerTransformerEnd_g ;
                                       owl:maxQualifiedCardinality "1"^^xsd:nonNegativeInteger ;
                                       owl:onClass <https://w3id.org/netbeheer/IECCIM/TC57CIM/IEC61970/Base/Domain#Conductance>
                                     ] ,
                                     [ rdf:type owl:Restriction ;
                                       owl:onProperty :PowerTransformerEnd_g0 ;
                                       owl:maxQualifiedCardinality "1"^^xsd:nonNegativeInteger ;
                                       owl:onClass <https://w3id.org/netbeheer/IECCIM/TC57CIM/IEC61970/Base/Domain#Conductance>
                                     ] ,
                                     [ rdf:type owl:Restriction ;
                                       owl:onProperty :PowerTransformerEnd_r ;
                                       owl:maxQualifiedCardinality "1"^^xsd:nonNegativeInteger ;
                                       owl:onClass <https://w3id.org/netbeheer/IECCIM/TC57CIM/IEC61970/Base/Domain#Resistance>
                                     ] ,
                                     [ rdf:type owl:Restriction ;
                                       owl:onProperty :PowerTransformerEnd_r0 ;
                                       owl:maxQualifiedCardinality "1"^^xsd:nonNegativeInteger ;
                                       owl:onClass <https://w3id.org/netbeheer/IECCIM/TC57CIM/IEC61970/Base/Domain#Resistance>
                                     ] ,
                                     [ rdf:type owl:Restriction ;
                                       owl:onProperty :PowerTransformerEnd_ratedS ;
                                       owl:maxQualifiedCardinality "1"^^xsd:nonNegativeInteger ;
                                       owl:onClass <https://w3id.org/netbeheer/IECCIM/TC57CIM/IEC61970/Base/Domain#ApparentPower>
                                     ] ,
                                     [ rdf:type owl:Restriction ;
                                       owl:onProperty :PowerTransformerEnd_ratedU ;
                                       owl:maxQualifiedCardinality "1"^^xsd:nonNegativeInteger ;
                                       owl:onClass <https://w3id.org/netbeheer/IECCIM/TC57CIM/IEC61970/Base/Domain#Voltage>
                                     ] ,
                                     [ rdf:type owl:Restriction ;
                                       owl:onProperty :PowerTransformerEnd_x ;
                                       owl:maxQualifiedCardinality "1"^^xsd:nonNegativeInteger ;
                                       owl:onClass <https://w3id.org/netbeheer/IECCIM/TC57CIM/IEC61970/Base/Domain#Reactance>
                                     ] ,
                                     [ rdf:type owl:Restriction ;
                                       owl:onProperty :PowerTransformerEnd_x0 ;
                                       owl:maxQualifiedCardinality "1"^^xsd:nonNegativeInteger ;
                                       owl:onClass <https://w3id.org/netbeheer/IECCIM/TC57CIM/IEC61970/Base/Domain#Reactance>
                                     ] ,
                                     [ rdf:type owl:Restriction ;
                                       owl:onProperty :PowerTransformerEnd_connectionKind ;
                                       owl:minQualifiedCardinality "0"^^xsd:nonNegativeInteger ;
                                       owl:onDataRange :WindingConnection
                                     ] ,
                                     [ rdf:type owl:Restriction ;
                                       owl:onProperty :PowerTransformerEnd_phaseAngleClock ;
                                       owl:minQualifiedCardinality "0"^^xsd:nonNegativeInteger ;
                                       owl:onDataRange xsd:nonNegativeInteger
                                     ] ,
                                     [ rdf:type owl:Restriction ;
                                       owl:onProperty :PowerTransformerEnd_connectionKind ;
                                       owl:maxQualifiedCardinality "1"^^xsd:nonNegativeInteger ;
                                       owl:onDataRange :WindingConnection
                                     ] ,
                                     [ rdf:type owl:Restriction ;
                                       owl:onProperty :PowerTransformerEnd_phaseAngleClock ;
                                       owl:maxQualifiedCardinality "1"^^xsd:nonNegativeInteger ;
                                       owl:onDataRange xsd:nonNegativeInteger
                                     ] ;
                     rdfs:comment """A PowerTransformerEnd is associated with each Terminal of a PowerTransformer.
The impedance values r, r0, x, and x0 of a PowerTransformerEnd represents a star equivalent as follows
1) for a two Terminal PowerTransformer the high voltage PowerTransformerEnd has non zero values on r, r0, x, and x0 while the low voltage PowerTransformerEnd has zero values for r, r0, x, and x0.
2) for a three Terminal PowerTransformer the three PowerTransformerEnds represents a star equivalent with each leg in the star represented by r, r0, x, and x0 values.
3) for a PowerTransformer with more than three Terminals the PowerTransformerEnd impedance values cannot be used. Instead use the TransformerMeshImpedance or split the transformer into multiple PowerTransformers.""" .


###  https://w3id.org/netbeheer/IECCIM/TC57CIM/IEC61970/Base/Wires#ProtectedSwitch
:ProtectedSwitch rdf:type owl:Class ;
                 rdfs:subClassOf :Switch ,
                                 [ rdf:type owl:Restriction ;
                                   owl:onProperty :ProtectedSwitch_OperatedByProtectionEquipment ;
                                   owl:minQualifiedCardinality "0"^^xsd:nonNegativeInteger ;
                                   owl:onClass :ProtectedSwitch
                                 ] ,
                                 [ rdf:type owl:Restriction ;
                                   owl:onProperty :ProtectedSwitch_breakingCapacity ;
                                   owl:minQualifiedCardinality "0"^^xsd:nonNegativeInteger ;
                                   owl:onClass <https://w3id.org/netbeheer/IECCIM/TC57CIM/IEC61970/Base/Domain#CurrentFlow>
                                 ] ,
                                 [ rdf:type owl:Restriction ;
                                   owl:onProperty :ProtectedSwitch_RecloseSequences ;
                                   owl:qualifiedCardinality "1"^^xsd:nonNegativeInteger ;
                                   owl:onClass :ProtectedSwitch
                                 ] ,
                                 [ rdf:type owl:Restriction ;
                                   owl:onProperty :ProtectedSwitch_breakingCapacity ;
                                   owl:maxQualifiedCardinality "1"^^xsd:nonNegativeInteger ;
                                   owl:onClass <https://w3id.org/netbeheer/IECCIM/TC57CIM/IEC61970/Base/Domain#CurrentFlow>
                                 ] ;
                 rdfs:comment "A ProtectedSwitch is a switching device that can be operated by ProtectionEquipment." .


###  https://w3id.org/netbeheer/IECCIM/TC57CIM/IEC61970/Base/Wires#RatioTapChanger
:RatioTapChanger rdf:type owl:Class ;
                 rdfs:subClassOf :TapChanger ,
                                 [ rdf:type owl:Restriction ;
                                   owl:onProperty :RatioTapChanger_RatioTapChangerTable ;
                                   owl:minQualifiedCardinality "0"^^xsd:nonNegativeInteger ;
                                   owl:onClass :RatioTapChanger
                                 ] ,
                                 [ rdf:type owl:Restriction ;
                                   owl:onProperty :RatioTapChanger_TransformerEnd ;
                                   owl:minQualifiedCardinality "0"^^xsd:nonNegativeInteger ;
                                   owl:onClass :RatioTapChanger
                                 ] ,
                                 [ rdf:type owl:Restriction ;
                                   owl:onProperty :RatioTapChanger_stepVoltageIncrement ;
                                   owl:minQualifiedCardinality "0"^^xsd:nonNegativeInteger ;
                                   owl:onClass <https://w3id.org/netbeheer/IECCIM/TC57CIM/IEC61970/Base/Domain#PerCent>
                                 ] ,
                                 [ rdf:type owl:Restriction ;
                                   owl:onProperty :RatioTapChanger_TransformerEnd ;
                                   owl:maxQualifiedCardinality "1"^^xsd:nonNegativeInteger ;
                                   owl:onClass :RatioTapChanger
                                 ] ,
                                 [ rdf:type owl:Restriction ;
                                   owl:onProperty :RatioTapChanger_stepVoltageIncrement ;
                                   owl:maxQualifiedCardinality "1"^^xsd:nonNegativeInteger ;
                                   owl:onClass <https://w3id.org/netbeheer/IECCIM/TC57CIM/IEC61970/Base/Domain#PerCent>
                                 ] ,
                                 [ rdf:type owl:Restriction ;
                                   owl:onProperty :RatioTapChanger_tculControlMode ;
                                   owl:minQualifiedCardinality "0"^^xsd:nonNegativeInteger ;
                                   owl:onDataRange :TransformerControlMode
                                 ] ,
                                 [ rdf:type owl:Restriction ;
                                   owl:onProperty :RatioTapChanger_tculControlMode ;
                                   owl:maxQualifiedCardinality "1"^^xsd:nonNegativeInteger ;
                                   owl:onDataRange :TransformerControlMode
                                 ] ;
                 rdfs:comment """A tap changer that changes the voltage ratio impacting the voltage magnitude but not the phase angle across the transformer.
""" .


###  https://w3id.org/netbeheer/IECCIM/TC57CIM/IEC61970/Base/Wires#RatioTapChangerTable
:RatioTapChangerTable rdf:type owl:Class ;
                      rdfs:subClassOf <https://w3id.org/netbeheer/IECCIM/TC57CIM/IEC61970/Base/Core#IdentifiedObject> ,
                                      [ rdf:type owl:Restriction ;
                                        owl:onProperty :RatioTapChangerTable_RatioTapChanger ;
                                        owl:minQualifiedCardinality "0"^^xsd:nonNegativeInteger ;
                                        owl:onClass :RatioTapChangerTable
                                      ] ,
                                      [ rdf:type owl:Restriction ;
                                        owl:onProperty :RatioTapChangerTable_RatioTapChangerTablePoint ;
                                        owl:qualifiedCardinality "1"^^xsd:nonNegativeInteger ;
                                        owl:onClass :RatioTapChangerTable
                                      ] ,
                                      [ rdf:type owl:Restriction ;
                                        owl:onProperty :RatioTapChangerTable_RatioTapChanger ;
                                        owl:maxQualifiedCardinality "1"^^xsd:nonNegativeInteger ;
                                        owl:onClass :RatioTapChangerTable
                                      ] ;
                      rdfs:comment "Describes a curve for how the voltage magnitude and impedance varies with the tap step. " .


###  https://w3id.org/netbeheer/IECCIM/TC57CIM/IEC61970/Base/Wires#RatioTapChangerTablePoint
:RatioTapChangerTablePoint rdf:type owl:Class ;
                           rdfs:subClassOf :TapChangerTablePoint ,
                                           [ rdf:type owl:Restriction ;
                                             owl:onProperty :RatioTapChangerTablePoint_RatioTapChangerTable ;
                                             owl:minQualifiedCardinality "1"^^xsd:nonNegativeInteger ;
                                             owl:onClass :RatioTapChangerTablePoint
                                           ] ;
                           rdfs:comment """Describes each tap step in the ratio tap changer tabular curve.
""" .


###  https://w3id.org/netbeheer/IECCIM/TC57CIM/IEC61970/Base/Wires#ReactiveCapabilityCurve
:ReactiveCapabilityCurve rdf:type owl:Class ;
                         rdfs:subClassOf <https://w3id.org/netbeheer/IECCIM/TC57CIM/IEC61970/Base/Core#Curve> ,
                                         [ rdf:type owl:Restriction ;
                                           owl:onProperty :ReactiveCapabilityCurve_EquivalentInjection ;
                                           owl:minQualifiedCardinality "0"^^xsd:nonNegativeInteger ;
                                           owl:onClass :ReactiveCapabilityCurve
                                         ] ,
                                         [ rdf:type owl:Restriction ;
                                           owl:onProperty :ReactiveCapabilityCurve_InitiallyUsedBySynchronousMachines ;
                                           owl:minQualifiedCardinality "0"^^xsd:nonNegativeInteger ;
                                           owl:onClass :ReactiveCapabilityCurve
                                         ] ,
                                         [ rdf:type owl:Restriction ;
                                           owl:onProperty :ReactiveCapabilityCurve_SynchronousMachines ;
                                           owl:minQualifiedCardinality "0"^^xsd:nonNegativeInteger ;
                                           owl:onClass :ReactiveCapabilityCurve
                                         ] ,
                                         [ rdf:type owl:Restriction ;
                                           owl:onProperty :ReactiveCapabilityCurve_coolantTemperature ;
                                           owl:minQualifiedCardinality "0"^^xsd:nonNegativeInteger ;
                                           owl:onClass <https://w3id.org/netbeheer/IECCIM/TC57CIM/IEC61970/Base/Domain#Temperature>
                                         ] ,
                                         [ rdf:type owl:Restriction ;
                                           owl:onProperty :ReactiveCapabilityCurve_hydrogenPressure ;
                                           owl:minQualifiedCardinality "0"^^xsd:nonNegativeInteger ;
                                           owl:onClass <https://w3id.org/netbeheer/IECCIM/TC57CIM/IEC61970/Base/Domain#Pressure>
                                         ] ,
                                         [ rdf:type owl:Restriction ;
                                           owl:onProperty :ReactiveCapabilityCurve_EquivalentInjection ;
                                           owl:maxQualifiedCardinality "1"^^xsd:nonNegativeInteger ;
                                           owl:onClass :ReactiveCapabilityCurve
                                         ] ,
                                         [ rdf:type owl:Restriction ;
                                           owl:onProperty :ReactiveCapabilityCurve_InitiallyUsedBySynchronousMachines ;
                                           owl:maxQualifiedCardinality "1"^^xsd:nonNegativeInteger ;
                                           owl:onClass :ReactiveCapabilityCurve
                                         ] ,
                                         [ rdf:type owl:Restriction ;
                                           owl:onProperty :ReactiveCapabilityCurve_coolantTemperature ;
                                           owl:maxQualifiedCardinality "1"^^xsd:nonNegativeInteger ;
                                           owl:onClass <https://w3id.org/netbeheer/IECCIM/TC57CIM/IEC61970/Base/Domain#Temperature>
                                         ] ,
                                         [ rdf:type owl:Restriction ;
                                           owl:onProperty :ReactiveCapabilityCurve_hydrogenPressure ;
                                           owl:maxQualifiedCardinality "1"^^xsd:nonNegativeInteger ;
                                           owl:onClass <https://w3id.org/netbeheer/IECCIM/TC57CIM/IEC61970/Base/Domain#Pressure>
                                         ] ;
                         rdfs:comment "Reactive power rating envelope versus the synchronous machine's active power, in both the generating and motoring modes. For each active power value there is a corresponding high and low reactive power limit  value. Typically there will be a separate curve for each coolant condition, such as hydrogen pressure.  The Y1 axis values represent reactive minimum and the Y2 axis values represent reactive maximum." .


###  https://w3id.org/netbeheer/IECCIM/TC57CIM/IEC61970/Base/Wires#Recloser
:Recloser rdf:type owl:Class ;
          rdfs:subClassOf :ProtectedSwitch ;
          rdfs:comment """Pole-mounted fault interrupter with built-in phase and ground relays, current transformer (CT), and supplemental controls.
""" .


###  https://w3id.org/netbeheer/IECCIM/TC57CIM/IEC61970/Base/Wires#RegulatingCondEq
:RegulatingCondEq rdf:type owl:Class ;
                  rdfs:subClassOf <https://w3id.org/netbeheer/IECCIM/TC57CIM/IEC61970/Base/Core#ConductingEquipment> ,
                                  [ rdf:type owl:Restriction ;
                                    owl:onProperty :RegulatingCondEq_RegulatingControl ;
                                    owl:minQualifiedCardinality "0"^^xsd:nonNegativeInteger ;
                                    owl:onClass :RegulatingCondEq
                                  ] ,
                                  [ rdf:type owl:Restriction ;
                                    owl:onProperty :RegulatingCondEq_controlEnabled ;
                                    owl:minQualifiedCardinality "0"^^xsd:nonNegativeInteger ;
                                    owl:onDataRange xsd:boolean
                                  ] ,
                                  [ rdf:type owl:Restriction ;
                                    owl:onProperty :RegulatingCondEq_controlEnabled ;
                                    owl:maxQualifiedCardinality "1"^^xsd:nonNegativeInteger ;
                                    owl:onDataRange xsd:boolean
                                  ] ;
                  rdfs:comment "A type of conducting equipment that can regulate a quantity (i.e. voltage or flow) at a specific point in the network. " .


###  https://w3id.org/netbeheer/IECCIM/TC57CIM/IEC61970/Base/Wires#RegulatingControl
:RegulatingControl rdf:type owl:Class ;
                   rdfs:subClassOf <https://w3id.org/netbeheer/IECCIM/TC57CIM/IEC61970/Base/Core#PowerSystemResource> ,
                                   [ rdf:type owl:Restriction ;
                                     owl:onProperty :RegulatingControl_RegulatingCondEq ;
                                     owl:minQualifiedCardinality "0"^^xsd:nonNegativeInteger ;
                                     owl:onClass :RegulatingControl
                                   ] ,
                                   [ rdf:type owl:Restriction ;
                                     owl:onProperty :RegulatingControl_ProtectiveActionRegulation ;
                                     owl:qualifiedCardinality "1"^^xsd:nonNegativeInteger ;
                                     owl:onClass :RegulatingControl
                                   ] ,
                                   [ rdf:type owl:Restriction ;
                                     owl:onProperty :RegulatingControl_RegulationSchedule ;
                                     owl:qualifiedCardinality "1"^^xsd:nonNegativeInteger ;
                                     owl:onClass :RegulatingControl
                                   ] ,
                                   [ rdf:type owl:Restriction ;
                                     owl:onProperty :RegulatingControl_RegulatingCondEq ;
                                     owl:maxQualifiedCardinality "1"^^xsd:nonNegativeInteger ;
                                     owl:onClass :RegulatingControl
                                   ] ,
                                   [ rdf:type owl:Restriction ;
                                     owl:onProperty :RegulatingControl_discrete ;
                                     owl:minQualifiedCardinality "0"^^xsd:nonNegativeInteger ;
                                     owl:onDataRange xsd:boolean
                                   ] ,
                                   [ rdf:type owl:Restriction ;
                                     owl:onProperty :RegulatingControl_enabled ;
                                     owl:minQualifiedCardinality "0"^^xsd:nonNegativeInteger ;
                                     owl:onDataRange xsd:boolean
                                   ] ,
                                   [ rdf:type owl:Restriction ;
                                     owl:onProperty :RegulatingControl_mode ;
                                     owl:minQualifiedCardinality "0"^^xsd:nonNegativeInteger ;
                                     owl:onDataRange :RegulatingControlModeKind
                                   ] ,
                                   [ rdf:type owl:Restriction ;
                                     owl:onProperty :RegulatingControl_monitoredPhase ;
                                     owl:minQualifiedCardinality "0"^^xsd:nonNegativeInteger ;
                                     owl:onDataRange <https://w3id.org/netbeheer/IECCIM/TC57CIM/IEC61970/Base/Core#PhaseCode>
                                   ] ,
                                   [ rdf:type owl:Restriction ;
                                     owl:onProperty :RegulatingControl_targetDeadband ;
                                     owl:minQualifiedCardinality "0"^^xsd:nonNegativeInteger ;
                                     owl:onDataRange xsd:float
                                   ] ,
                                   [ rdf:type owl:Restriction ;
                                     owl:onProperty :RegulatingControl_targetValue ;
                                     owl:minQualifiedCardinality "0"^^xsd:nonNegativeInteger ;
                                     owl:onDataRange xsd:float
                                   ] ,
                                   [ rdf:type owl:Restriction ;
                                     owl:onProperty :RegulatingControl_targetValueUnitMultiplier ;
                                     owl:minQualifiedCardinality "0"^^xsd:nonNegativeInteger ;
                                     owl:onDataRange <https://w3id.org/netbeheer/IECCIM/TC57CIM/IEC61970/Base/Domain#UnitMultiplier>
                                   ] ,
                                   [ rdf:type owl:Restriction ;
                                     owl:onProperty :RegulatingControl_discrete ;
                                     owl:maxQualifiedCardinality "1"^^xsd:nonNegativeInteger ;
                                     owl:onDataRange xsd:boolean
                                   ] ,
                                   [ rdf:type owl:Restriction ;
                                     owl:onProperty :RegulatingControl_enabled ;
                                     owl:maxQualifiedCardinality "1"^^xsd:nonNegativeInteger ;
                                     owl:onDataRange xsd:boolean
                                   ] ,
                                   [ rdf:type owl:Restriction ;
                                     owl:onProperty :RegulatingControl_mode ;
                                     owl:maxQualifiedCardinality "1"^^xsd:nonNegativeInteger ;
                                     owl:onDataRange :RegulatingControlModeKind
                                   ] ,
                                   [ rdf:type owl:Restriction ;
                                     owl:onProperty :RegulatingControl_monitoredPhase ;
                                     owl:maxQualifiedCardinality "1"^^xsd:nonNegativeInteger ;
                                     owl:onDataRange <https://w3id.org/netbeheer/IECCIM/TC57CIM/IEC61970/Base/Core#PhaseCode>
                                   ] ,
                                   [ rdf:type owl:Restriction ;
                                     owl:onProperty :RegulatingControl_targetDeadband ;
                                     owl:maxQualifiedCardinality "1"^^xsd:nonNegativeInteger ;
                                     owl:onDataRange xsd:float
                                   ] ,
                                   [ rdf:type owl:Restriction ;
                                     owl:onProperty :RegulatingControl_targetValue ;
                                     owl:maxQualifiedCardinality "1"^^xsd:nonNegativeInteger ;
                                     owl:onDataRange xsd:float
                                   ] ,
                                   [ rdf:type owl:Restriction ;
                                     owl:onProperty :RegulatingControl_targetValueUnitMultiplier ;
                                     owl:maxQualifiedCardinality "1"^^xsd:nonNegativeInteger ;
                                     owl:onDataRange <https://w3id.org/netbeheer/IECCIM/TC57CIM/IEC61970/Base/Domain#UnitMultiplier>
                                   ] ;
                   rdfs:comment """Specifies a set of equipment that works together to control a power system quantity such as voltage or flow. 
Remote bus voltage control is possible by specifying the controlled terminal located at some place remote from the controlling equipment.
In case multiple equipment, possibly of different types, control same terminal there must be only one RegulatingControl at that terminal. The most specific subtype of RegulatingControl shall be used in case such equipment participate in the control, e.g. TapChangerControl for tap changers.
For flow control  load sign convention is used, i.e. positive sign means flow out from a TopologicalNode (bus) into the conducting equipment.""" .


###  https://w3id.org/netbeheer/IECCIM/TC57CIM/IEC61970/Base/Wires#RegulationSchedule
:RegulationSchedule rdf:type owl:Class ;
                    rdfs:subClassOf <https://w3id.org/netbeheer/IECCIM/TC57CIM/IEC61970/Base/LoadModel#SeasonDayTypeSchedule> ,
                                    [ rdf:type owl:Restriction ;
                                      owl:onProperty :RegulationSchedule_RegulatingControl ;
                                      owl:minQualifiedCardinality "0"^^xsd:nonNegativeInteger ;
                                      owl:onClass :RegulationSchedule
                                    ] ,
                                    [ rdf:type owl:Restriction ;
                                      owl:onProperty :RegulationSchedule_VoltageControlZones ;
                                      owl:minQualifiedCardinality "0"^^xsd:nonNegativeInteger ;
                                      owl:onClass :RegulationSchedule
                                    ] ,
                                    [ rdf:type owl:Restriction ;
                                      owl:onProperty :RegulationSchedule_VoltageControlZones ;
                                      owl:maxQualifiedCardinality "1"^^xsd:nonNegativeInteger ;
                                      owl:onClass :RegulationSchedule
                                    ] ;
                    rdfs:comment "A pre-established pattern over time for a controlled variable, e.g., busbar voltage." .


###  https://w3id.org/netbeheer/IECCIM/TC57CIM/IEC61970/Base/Wires#RotatingMachine
:RotatingMachine rdf:type owl:Class ;
                 rdfs:subClassOf :RegulatingCondEq ,
                                 [ rdf:type owl:Restriction ;
                                   owl:onProperty :RotatingMachine_GeneratingUnit ;
                                   owl:minQualifiedCardinality "1"^^xsd:nonNegativeInteger ;
                                   owl:onClass :RotatingMachine
                                 ] ,
                                 [ rdf:type owl:Restriction ;
                                   owl:onProperty :RotatingMachine_p ;
                                   owl:minQualifiedCardinality "0"^^xsd:nonNegativeInteger ;
                                   owl:onClass <https://w3id.org/netbeheer/IECCIM/TC57CIM/IEC61970/Base/Domain#ActivePower>
                                 ] ,
                                 [ rdf:type owl:Restriction ;
                                   owl:onProperty :RotatingMachine_q ;
                                   owl:minQualifiedCardinality "0"^^xsd:nonNegativeInteger ;
                                   owl:onClass <https://w3id.org/netbeheer/IECCIM/TC57CIM/IEC61970/Base/Domain#ReactivePower>
                                 ] ,
                                 [ rdf:type owl:Restriction ;
                                   owl:onProperty :RotatingMachine_ratedS ;
                                   owl:minQualifiedCardinality "0"^^xsd:nonNegativeInteger ;
                                   owl:onClass <https://w3id.org/netbeheer/IECCIM/TC57CIM/IEC61970/Base/Domain#ApparentPower>
                                 ] ,
                                 [ rdf:type owl:Restriction ;
                                   owl:onProperty :RotatingMachine_ratedU ;
                                   owl:minQualifiedCardinality "0"^^xsd:nonNegativeInteger ;
                                   owl:onClass <https://w3id.org/netbeheer/IECCIM/TC57CIM/IEC61970/Base/Domain#Voltage>
                                 ] ,
                                 [ rdf:type owl:Restriction ;
                                   owl:onProperty :RotatingMachine_HydroPump ;
                                   owl:qualifiedCardinality "1"^^xsd:nonNegativeInteger ;
                                   owl:onClass :RotatingMachine
                                 ] ,
                                 [ rdf:type owl:Restriction ;
                                   owl:onProperty :RotatingMachine_p ;
                                   owl:maxQualifiedCardinality "1"^^xsd:nonNegativeInteger ;
                                   owl:onClass <https://w3id.org/netbeheer/IECCIM/TC57CIM/IEC61970/Base/Domain#ActivePower>
                                 ] ,
                                 [ rdf:type owl:Restriction ;
                                   owl:onProperty :RotatingMachine_q ;
                                   owl:maxQualifiedCardinality "1"^^xsd:nonNegativeInteger ;
                                   owl:onClass <https://w3id.org/netbeheer/IECCIM/TC57CIM/IEC61970/Base/Domain#ReactivePower>
                                 ] ,
                                 [ rdf:type owl:Restriction ;
                                   owl:onProperty :RotatingMachine_ratedS ;
                                   owl:maxQualifiedCardinality "1"^^xsd:nonNegativeInteger ;
                                   owl:onClass <https://w3id.org/netbeheer/IECCIM/TC57CIM/IEC61970/Base/Domain#ApparentPower>
                                 ] ,
                                 [ rdf:type owl:Restriction ;
                                   owl:onProperty :RotatingMachine_ratedU ;
                                   owl:maxQualifiedCardinality "1"^^xsd:nonNegativeInteger ;
                                   owl:onClass <https://w3id.org/netbeheer/IECCIM/TC57CIM/IEC61970/Base/Domain#Voltage>
                                 ] ,
                                 [ rdf:type owl:Restriction ;
                                   owl:onProperty :RotatingMachine_ratedPowerFactor ;
                                   owl:minQualifiedCardinality "0"^^xsd:nonNegativeInteger ;
                                   owl:onDataRange xsd:float
                                 ] ,
                                 [ rdf:type owl:Restriction ;
                                   owl:onProperty :RotatingMachine_ratedPowerFactor ;
                                   owl:maxQualifiedCardinality "1"^^xsd:nonNegativeInteger ;
                                   owl:onDataRange xsd:float
                                 ] ;
                 rdfs:comment "A rotating machine which may be used as a generator or motor." .


###  https://w3id.org/netbeheer/IECCIM/TC57CIM/IEC61970/Base/Wires#Sectionaliser
:Sectionaliser rdf:type owl:Class ;
               rdfs:subClassOf :Switch ;
               rdfs:comment """Automatic switch that will lock open to isolate a faulted section. It may, or may not, have load breaking capability. Its primary purpose is to provide fault sectionalising at locations where the fault current is either too high, or too low, for proper coordination of fuses.
""" .


###  https://w3id.org/netbeheer/IECCIM/TC57CIM/IEC61970/Base/Wires#SeriesCompensator
:SeriesCompensator rdf:type owl:Class ;
                   rdfs:subClassOf <https://w3id.org/netbeheer/IECCIM/TC57CIM/IEC61970/Base/Core#ConductingEquipment> ,
                                   [ rdf:type owl:Restriction ;
                                     owl:onProperty :SeriesCompensator_r ;
                                     owl:minQualifiedCardinality "0"^^xsd:nonNegativeInteger ;
                                     owl:onClass <https://w3id.org/netbeheer/IECCIM/TC57CIM/IEC61970/Base/Domain#Resistance>
                                   ] ,
                                   [ rdf:type owl:Restriction ;
                                     owl:onProperty :SeriesCompensator_r0 ;
                                     owl:minQualifiedCardinality "0"^^xsd:nonNegativeInteger ;
                                     owl:onClass <https://w3id.org/netbeheer/IECCIM/TC57CIM/IEC61970/Base/Domain#Resistance>
                                   ] ,
                                   [ rdf:type owl:Restriction ;
                                     owl:onProperty :SeriesCompensator_varistorRatedCurrent ;
                                     owl:minQualifiedCardinality "0"^^xsd:nonNegativeInteger ;
                                     owl:onClass <https://w3id.org/netbeheer/IECCIM/TC57CIM/IEC61970/Base/Domain#CurrentFlow>
                                   ] ,
                                   [ rdf:type owl:Restriction ;
                                     owl:onProperty :SeriesCompensator_varistorVoltageThreshold ;
                                     owl:minQualifiedCardinality "0"^^xsd:nonNegativeInteger ;
                                     owl:onClass <https://w3id.org/netbeheer/IECCIM/TC57CIM/IEC61970/Base/Domain#Voltage>
                                   ] ,
                                   [ rdf:type owl:Restriction ;
                                     owl:onProperty :SeriesCompensator_x ;
                                     owl:minQualifiedCardinality "0"^^xsd:nonNegativeInteger ;
                                     owl:onClass <https://w3id.org/netbeheer/IECCIM/TC57CIM/IEC61970/Base/Domain#Reactance>
                                   ] ,
                                   [ rdf:type owl:Restriction ;
                                     owl:onProperty :SeriesCompensator_x0 ;
                                     owl:minQualifiedCardinality "0"^^xsd:nonNegativeInteger ;
                                     owl:onClass <https://w3id.org/netbeheer/IECCIM/TC57CIM/IEC61970/Base/Domain#Reactance>
                                   ] ,
                                   [ rdf:type owl:Restriction ;
                                     owl:onProperty :SeriesCompensator_r ;
                                     owl:maxQualifiedCardinality "1"^^xsd:nonNegativeInteger ;
                                     owl:onClass <https://w3id.org/netbeheer/IECCIM/TC57CIM/IEC61970/Base/Domain#Resistance>
                                   ] ,
                                   [ rdf:type owl:Restriction ;
                                     owl:onProperty :SeriesCompensator_r0 ;
                                     owl:maxQualifiedCardinality "1"^^xsd:nonNegativeInteger ;
                                     owl:onClass <https://w3id.org/netbeheer/IECCIM/TC57CIM/IEC61970/Base/Domain#Resistance>
                                   ] ,
                                   [ rdf:type owl:Restriction ;
                                     owl:onProperty :SeriesCompensator_varistorRatedCurrent ;
                                     owl:maxQualifiedCardinality "1"^^xsd:nonNegativeInteger ;
                                     owl:onClass <https://w3id.org/netbeheer/IECCIM/TC57CIM/IEC61970/Base/Domain#CurrentFlow>
                                   ] ,
                                   [ rdf:type owl:Restriction ;
                                     owl:onProperty :SeriesCompensator_varistorVoltageThreshold ;
                                     owl:maxQualifiedCardinality "1"^^xsd:nonNegativeInteger ;
                                     owl:onClass <https://w3id.org/netbeheer/IECCIM/TC57CIM/IEC61970/Base/Domain#Voltage>
                                   ] ,
                                   [ rdf:type owl:Restriction ;
                                     owl:onProperty :SeriesCompensator_x ;
                                     owl:maxQualifiedCardinality "1"^^xsd:nonNegativeInteger ;
                                     owl:onClass <https://w3id.org/netbeheer/IECCIM/TC57CIM/IEC61970/Base/Domain#Reactance>
                                   ] ,
                                   [ rdf:type owl:Restriction ;
                                     owl:onProperty :SeriesCompensator_x0 ;
                                     owl:maxQualifiedCardinality "1"^^xsd:nonNegativeInteger ;
                                     owl:onClass <https://w3id.org/netbeheer/IECCIM/TC57CIM/IEC61970/Base/Domain#Reactance>
                                   ] ,
                                   [ rdf:type owl:Restriction ;
                                     owl:onProperty :SeriesCompensator_varistorPresent ;
                                     owl:minQualifiedCardinality "0"^^xsd:nonNegativeInteger ;
                                     owl:onDataRange xsd:boolean
                                   ] ,
                                   [ rdf:type owl:Restriction ;
                                     owl:onProperty :SeriesCompensator_varistorPresent ;
                                     owl:maxQualifiedCardinality "1"^^xsd:nonNegativeInteger ;
                                     owl:onDataRange xsd:boolean
                                   ] ;
                   rdfs:comment """A Series Compensator is a series capacitor or reactor or an AC transmission line without charging susceptance.  It is a two terminal device.
""" .


###  https://w3id.org/netbeheer/IECCIM/TC57CIM/IEC61970/Base/Wires#ShuntCompensator
:ShuntCompensator rdf:type owl:Class ;
                  rdfs:subClassOf :RegulatingCondEq ,
                                  [ rdf:type owl:Restriction ;
                                    owl:onProperty :ShuntCompensator_aVRDelay ;
                                    owl:minQualifiedCardinality "0"^^xsd:nonNegativeInteger ;
                                    owl:onClass <https://w3id.org/netbeheer/IECCIM/TC57CIM/IEC61970/Base/Domain#Seconds>
                                  ] ,
                                  [ rdf:type owl:Restriction ;
                                    owl:onProperty :ShuntCompensator_nomU ;
                                    owl:minQualifiedCardinality "0"^^xsd:nonNegativeInteger ;
                                    owl:onClass <https://w3id.org/netbeheer/IECCIM/TC57CIM/IEC61970/Base/Domain#Voltage>
                                  ] ,
                                  [ rdf:type owl:Restriction ;
                                    owl:onProperty :ShuntCompensator_voltageSensitivity ;
                                    owl:minQualifiedCardinality "0"^^xsd:nonNegativeInteger ;
                                    owl:onClass <https://w3id.org/netbeheer/IECCIM/TC57CIM/IEC61970/Base/Domain#VoltagePerReactivePower>
                                  ] ,
                                  [ rdf:type owl:Restriction ;
                                    owl:onProperty :ShuntCompensator_ShuntCompensatorPhase ;
                                    owl:qualifiedCardinality "1"^^xsd:nonNegativeInteger ;
                                    owl:onClass :ShuntCompensator
                                  ] ,
                                  [ rdf:type owl:Restriction ;
                                    owl:onProperty :ShuntCompensator_SvShuntCompensatorSections ;
                                    owl:qualifiedCardinality "1"^^xsd:nonNegativeInteger ;
                                    owl:onClass :ShuntCompensator
                                  ] ,
                                  [ rdf:type owl:Restriction ;
                                    owl:onProperty :ShuntCompensator_aVRDelay ;
                                    owl:maxQualifiedCardinality "1"^^xsd:nonNegativeInteger ;
                                    owl:onClass <https://w3id.org/netbeheer/IECCIM/TC57CIM/IEC61970/Base/Domain#Seconds>
                                  ] ,
                                  [ rdf:type owl:Restriction ;
                                    owl:onProperty :ShuntCompensator_nomU ;
                                    owl:maxQualifiedCardinality "1"^^xsd:nonNegativeInteger ;
                                    owl:onClass <https://w3id.org/netbeheer/IECCIM/TC57CIM/IEC61970/Base/Domain#Voltage>
                                  ] ,
                                  [ rdf:type owl:Restriction ;
                                    owl:onProperty :ShuntCompensator_voltageSensitivity ;
                                    owl:maxQualifiedCardinality "1"^^xsd:nonNegativeInteger ;
                                    owl:onClass <https://w3id.org/netbeheer/IECCIM/TC57CIM/IEC61970/Base/Domain#VoltagePerReactivePower>
                                  ] ,
                                  [ rdf:type owl:Restriction ;
                                    owl:onProperty :ShuntCompensator_grounded ;
                                    owl:minQualifiedCardinality "0"^^xsd:nonNegativeInteger ;
                                    owl:onDataRange xsd:boolean
                                  ] ,
                                  [ rdf:type owl:Restriction ;
                                    owl:onProperty :ShuntCompensator_maximumSections ;
                                    owl:minQualifiedCardinality "0"^^xsd:nonNegativeInteger ;
                                    owl:onDataRange xsd:nonNegativeInteger
                                  ] ,
                                  [ rdf:type owl:Restriction ;
                                    owl:onProperty :ShuntCompensator_normalSections ;
                                    owl:minQualifiedCardinality "0"^^xsd:nonNegativeInteger ;
                                    owl:onDataRange xsd:nonNegativeInteger
                                  ] ,
                                  [ rdf:type owl:Restriction ;
                                    owl:onProperty :ShuntCompensator_phaseConnection ;
                                    owl:minQualifiedCardinality "0"^^xsd:nonNegativeInteger ;
                                    owl:onDataRange :PhaseShuntConnectionKind
                                  ] ,
                                  [ rdf:type owl:Restriction ;
                                    owl:onProperty :ShuntCompensator_sections ;
                                    owl:minQualifiedCardinality "0"^^xsd:nonNegativeInteger ;
                                    owl:onDataRange xsd:float
                                  ] ,
                                  [ rdf:type owl:Restriction ;
                                    owl:onProperty :ShuntCompensator_switchOnCount ;
                                    owl:minQualifiedCardinality "0"^^xsd:nonNegativeInteger ;
                                    owl:onDataRange xsd:nonNegativeInteger
                                  ] ,
                                  [ rdf:type owl:Restriction ;
                                    owl:onProperty :ShuntCompensator_switchOnDate ;
                                    owl:minQualifiedCardinality "0"^^xsd:nonNegativeInteger ;
                                    owl:onDataRange xsd:dateTime
                                  ] ,
                                  [ rdf:type owl:Restriction ;
                                    owl:onProperty :ShuntCompensator_grounded ;
                                    owl:maxQualifiedCardinality "1"^^xsd:nonNegativeInteger ;
                                    owl:onDataRange xsd:boolean
                                  ] ,
                                  [ rdf:type owl:Restriction ;
                                    owl:onProperty :ShuntCompensator_maximumSections ;
                                    owl:maxQualifiedCardinality "1"^^xsd:nonNegativeInteger ;
                                    owl:onDataRange xsd:nonNegativeInteger
                                  ] ,
                                  [ rdf:type owl:Restriction ;
                                    owl:onProperty :ShuntCompensator_normalSections ;
                                    owl:maxQualifiedCardinality "1"^^xsd:nonNegativeInteger ;
                                    owl:onDataRange xsd:nonNegativeInteger
                                  ] ,
                                  [ rdf:type owl:Restriction ;
                                    owl:onProperty :ShuntCompensator_phaseConnection ;
                                    owl:maxQualifiedCardinality "1"^^xsd:nonNegativeInteger ;
                                    owl:onDataRange :PhaseShuntConnectionKind
                                  ] ,
                                  [ rdf:type owl:Restriction ;
                                    owl:onProperty :ShuntCompensator_sections ;
                                    owl:maxQualifiedCardinality "1"^^xsd:nonNegativeInteger ;
                                    owl:onDataRange xsd:float
                                  ] ,
                                  [ rdf:type owl:Restriction ;
                                    owl:onProperty :ShuntCompensator_switchOnCount ;
                                    owl:maxQualifiedCardinality "1"^^xsd:nonNegativeInteger ;
                                    owl:onDataRange xsd:nonNegativeInteger
                                  ] ,
                                  [ rdf:type owl:Restriction ;
                                    owl:onProperty :ShuntCompensator_switchOnDate ;
                                    owl:maxQualifiedCardinality "1"^^xsd:nonNegativeInteger ;
                                    owl:onDataRange xsd:dateTime
                                  ] ;
                  rdfs:comment "A shunt capacitor or reactor or switchable bank of shunt capacitors or reactors. A section of a shunt compensator is an individual capacitor or reactor.  A negative value for reactivePerSection indicates that the compensator is a reactor. ShuntCompensator is a single terminal device.  Ground is implied." .


###  https://w3id.org/netbeheer/IECCIM/TC57CIM/IEC61970/Base/Wires#ShuntCompensatorPhase
:ShuntCompensatorPhase rdf:type owl:Class ;
                       rdfs:subClassOf <https://w3id.org/netbeheer/IECCIM/TC57CIM/IEC61970/Base/Core#PowerSystemResource> ,
                                       [ rdf:type owl:Restriction ;
                                         owl:onProperty :ShuntCompensatorPhase_ShuntCompensator ;
                                         owl:minQualifiedCardinality "0"^^xsd:nonNegativeInteger ;
                                         owl:onClass :ShuntCompensatorPhase
                                       ] ,
                                       [ rdf:type owl:Restriction ;
                                         owl:onProperty :ShuntCompensatorPhase_maximumSections ;
                                         owl:minQualifiedCardinality "0"^^xsd:nonNegativeInteger ;
                                         owl:onDataRange xsd:nonNegativeInteger
                                       ] ,
                                       [ rdf:type owl:Restriction ;
                                         owl:onProperty :ShuntCompensatorPhase_normalSections ;
                                         owl:minQualifiedCardinality "0"^^xsd:nonNegativeInteger ;
                                         owl:onDataRange xsd:nonNegativeInteger
                                       ] ,
                                       [ rdf:type owl:Restriction ;
                                         owl:onProperty :ShuntCompensatorPhase_phase ;
                                         owl:minQualifiedCardinality "0"^^xsd:nonNegativeInteger ;
                                         owl:onDataRange :SinglePhaseKind
                                       ] ,
                                       [ rdf:type owl:Restriction ;
                                         owl:onProperty :ShuntCompensatorPhase_maximumSections ;
                                         owl:maxQualifiedCardinality "1"^^xsd:nonNegativeInteger ;
                                         owl:onDataRange xsd:nonNegativeInteger
                                       ] ,
                                       [ rdf:type owl:Restriction ;
                                         owl:onProperty :ShuntCompensatorPhase_normalSections ;
                                         owl:maxQualifiedCardinality "1"^^xsd:nonNegativeInteger ;
                                         owl:onDataRange xsd:nonNegativeInteger
                                       ] ,
                                       [ rdf:type owl:Restriction ;
                                         owl:onProperty :ShuntCompensatorPhase_phase ;
                                         owl:maxQualifiedCardinality "1"^^xsd:nonNegativeInteger ;
                                         owl:onDataRange :SinglePhaseKind
                                       ] ;
                       rdfs:comment "Single phase of a multi-phase shunt compensator when its attributes might be different per phase." .


###  https://w3id.org/netbeheer/IECCIM/TC57CIM/IEC61970/Base/Wires#StaticVarCompensator
:StaticVarCompensator rdf:type owl:Class ;
                      rdfs:subClassOf :RegulatingCondEq ,
                                      [ rdf:type owl:Restriction ;
                                        owl:onProperty :StaticVarCompensator_capacitiveRating ;
                                        owl:minQualifiedCardinality "0"^^xsd:nonNegativeInteger ;
                                        owl:onClass <https://w3id.org/netbeheer/IECCIM/TC57CIM/IEC61970/Base/Domain#Reactance>
                                      ] ,
                                      [ rdf:type owl:Restriction ;
                                        owl:onProperty :StaticVarCompensator_inductiveRating ;
                                        owl:minQualifiedCardinality "0"^^xsd:nonNegativeInteger ;
                                        owl:onClass <https://w3id.org/netbeheer/IECCIM/TC57CIM/IEC61970/Base/Domain#Reactance>
                                      ] ,
                                      [ rdf:type owl:Restriction ;
                                        owl:onProperty :StaticVarCompensator_q ;
                                        owl:minQualifiedCardinality "0"^^xsd:nonNegativeInteger ;
                                        owl:onClass <https://w3id.org/netbeheer/IECCIM/TC57CIM/IEC61970/Base/Domain#ReactivePower>
                                      ] ,
                                      [ rdf:type owl:Restriction ;
                                        owl:onProperty :StaticVarCompensator_slope ;
                                        owl:minQualifiedCardinality "0"^^xsd:nonNegativeInteger ;
                                        owl:onClass <https://w3id.org/netbeheer/IECCIM/TC57CIM/IEC61970/Base/Domain#VoltagePerReactivePower>
                                      ] ,
                                      [ rdf:type owl:Restriction ;
                                        owl:onProperty :StaticVarCompensator_voltageSetPoint ;
                                        owl:minQualifiedCardinality "0"^^xsd:nonNegativeInteger ;
                                        owl:onClass <https://w3id.org/netbeheer/IECCIM/TC57CIM/IEC61970/Base/Domain#Voltage>
                                      ] ,
                                      [ rdf:type owl:Restriction ;
                                        owl:onProperty :StaticVarCompensator_capacitiveRating ;
                                        owl:maxQualifiedCardinality "1"^^xsd:nonNegativeInteger ;
                                        owl:onClass <https://w3id.org/netbeheer/IECCIM/TC57CIM/IEC61970/Base/Domain#Reactance>
                                      ] ,
                                      [ rdf:type owl:Restriction ;
                                        owl:onProperty :StaticVarCompensator_inductiveRating ;
                                        owl:maxQualifiedCardinality "1"^^xsd:nonNegativeInteger ;
                                        owl:onClass <https://w3id.org/netbeheer/IECCIM/TC57CIM/IEC61970/Base/Domain#Reactance>
                                      ] ,
                                      [ rdf:type owl:Restriction ;
                                        owl:onProperty :StaticVarCompensator_q ;
                                        owl:maxQualifiedCardinality "1"^^xsd:nonNegativeInteger ;
                                        owl:onClass <https://w3id.org/netbeheer/IECCIM/TC57CIM/IEC61970/Base/Domain#ReactivePower>
                                      ] ,
                                      [ rdf:type owl:Restriction ;
                                        owl:onProperty :StaticVarCompensator_slope ;
                                        owl:maxQualifiedCardinality "1"^^xsd:nonNegativeInteger ;
                                        owl:onClass <https://w3id.org/netbeheer/IECCIM/TC57CIM/IEC61970/Base/Domain#VoltagePerReactivePower>
                                      ] ,
                                      [ rdf:type owl:Restriction ;
                                        owl:onProperty :StaticVarCompensator_voltageSetPoint ;
                                        owl:maxQualifiedCardinality "1"^^xsd:nonNegativeInteger ;
                                        owl:onClass <https://w3id.org/netbeheer/IECCIM/TC57CIM/IEC61970/Base/Domain#Voltage>
                                      ] ,
                                      [ rdf:type owl:Restriction ;
                                        owl:onProperty :StaticVarCompensator_sVCControlMode ;
                                        owl:minQualifiedCardinality "0"^^xsd:nonNegativeInteger ;
                                        owl:onDataRange :SVCControlMode
                                      ] ,
                                      [ rdf:type owl:Restriction ;
                                        owl:onProperty :StaticVarCompensator_sVCControlMode ;
                                        owl:maxQualifiedCardinality "1"^^xsd:nonNegativeInteger ;
                                        owl:onDataRange :SVCControlMode
                                      ] ;
                      rdfs:comment """A facility for providing variable and controllable shunt reactive power. The SVC typically consists of a stepdown transformer, filter, thyristor-controlled reactor, and thyristor-switched capacitor arms.

The SVC may operate in fixed MVar output mode or in voltage control mode. When in voltage control mode, the output of the SVC will be proportional to the deviation of voltage at the controlled bus from the voltage setpoint.  The SVC characteristic slope defines the proportion.  If the voltage at the controlled bus is equal to the voltage setpoint, the SVC MVar output is zero.""" .


###  https://w3id.org/netbeheer/IECCIM/TC57CIM/IEC61970/Base/Wires#Switch
:Switch rdf:type owl:Class ;
        rdfs:subClassOf <https://w3id.org/netbeheer/IECCIM/TC57CIM/IEC61970/Base/Core#ConductingEquipment> ,
                        [ rdf:type owl:Restriction ;
                          owl:onProperty :Switch_CompositeSwitch ;
                          owl:minQualifiedCardinality "0"^^xsd:nonNegativeInteger ;
                          owl:onClass :Switch
                        ] ,
                        [ rdf:type owl:Restriction ;
                          owl:onProperty :Switch_ConnectDisconnectFunctions ;
                          owl:minQualifiedCardinality "0"^^xsd:nonNegativeInteger ;
                          owl:onClass :Switch
                        ] ,
                        [ rdf:type owl:Restriction ;
                          owl:onProperty :Switch_Outage ;
                          owl:minQualifiedCardinality "0"^^xsd:nonNegativeInteger ;
                          owl:onClass :Switch
                        ] ,
                        [ rdf:type owl:Restriction ;
                          owl:onProperty :Switch_SwitchAction ;
                          owl:minQualifiedCardinality "0"^^xsd:nonNegativeInteger ;
                          owl:onClass :Switch
                        ] ,
                        [ rdf:type owl:Restriction ;
                          owl:onProperty :Switch_ratedCurrent ;
                          owl:minQualifiedCardinality "0"^^xsd:nonNegativeInteger ;
                          owl:onClass <https://w3id.org/netbeheer/IECCIM/TC57CIM/IEC61970/Base/Domain#CurrentFlow>
                        ] ,
                        [ rdf:type owl:Restriction ;
                          owl:onProperty :Switch_SwitchPhase ;
                          owl:qualifiedCardinality "1"^^xsd:nonNegativeInteger ;
                          owl:onClass :Switch
                        ] ,
                        [ rdf:type owl:Restriction ;
                          owl:onProperty :Switch_SwitchSchedules ;
                          owl:qualifiedCardinality "1"^^xsd:nonNegativeInteger ;
                          owl:onClass :Switch
                        ] ,
                        [ rdf:type owl:Restriction ;
                          owl:onProperty :Switch_SwitchAction ;
                          owl:maxQualifiedCardinality "1"^^xsd:nonNegativeInteger ;
                          owl:onClass :Switch
                        ] ,
                        [ rdf:type owl:Restriction ;
                          owl:onProperty :Switch_ratedCurrent ;
                          owl:maxQualifiedCardinality "1"^^xsd:nonNegativeInteger ;
                          owl:onClass <https://w3id.org/netbeheer/IECCIM/TC57CIM/IEC61970/Base/Domain#CurrentFlow>
                        ] ,
                        [ rdf:type owl:Restriction ;
                          owl:onProperty :Switch_normalOpen ;
                          owl:minQualifiedCardinality "0"^^xsd:nonNegativeInteger ;
                          owl:onDataRange xsd:boolean
                        ] ,
                        [ rdf:type owl:Restriction ;
                          owl:onProperty :Switch_open ;
                          owl:minQualifiedCardinality "0"^^xsd:nonNegativeInteger ;
                          owl:onDataRange xsd:boolean
                        ] ,
                        [ rdf:type owl:Restriction ;
                          owl:onProperty :Switch_retained ;
                          owl:minQualifiedCardinality "0"^^xsd:nonNegativeInteger ;
                          owl:onDataRange xsd:boolean
                        ] ,
                        [ rdf:type owl:Restriction ;
                          owl:onProperty :Switch_switchOnCount ;
                          owl:minQualifiedCardinality "0"^^xsd:nonNegativeInteger ;
                          owl:onDataRange xsd:nonNegativeInteger
                        ] ,
                        [ rdf:type owl:Restriction ;
                          owl:onProperty :Switch_switchOnDate ;
                          owl:minQualifiedCardinality "0"^^xsd:nonNegativeInteger ;
                          owl:onDataRange xsd:dateTime
                        ] ,
                        [ rdf:type owl:Restriction ;
                          owl:onProperty :Switch_normalOpen ;
                          owl:maxQualifiedCardinality "1"^^xsd:nonNegativeInteger ;
                          owl:onDataRange xsd:boolean
                        ] ,
                        [ rdf:type owl:Restriction ;
                          owl:onProperty :Switch_open ;
                          owl:maxQualifiedCardinality "1"^^xsd:nonNegativeInteger ;
                          owl:onDataRange xsd:boolean
                        ] ,
                        [ rdf:type owl:Restriction ;
                          owl:onProperty :Switch_retained ;
                          owl:maxQualifiedCardinality "1"^^xsd:nonNegativeInteger ;
                          owl:onDataRange xsd:boolean
                        ] ,
                        [ rdf:type owl:Restriction ;
                          owl:onProperty :Switch_switchOnCount ;
                          owl:maxQualifiedCardinality "1"^^xsd:nonNegativeInteger ;
                          owl:onDataRange xsd:nonNegativeInteger
                        ] ,
                        [ rdf:type owl:Restriction ;
                          owl:onProperty :Switch_switchOnDate ;
                          owl:maxQualifiedCardinality "1"^^xsd:nonNegativeInteger ;
                          owl:onDataRange xsd:dateTime
                        ] ;
        rdfs:comment "A generic device designed to close, or open, or both, one or more electric circuits.  All switches are two terminal devices including grounding switches." .


###  https://w3id.org/netbeheer/IECCIM/TC57CIM/IEC61970/Base/Wires#SwitchPhase
:SwitchPhase rdf:type owl:Class ;
             rdfs:subClassOf <https://w3id.org/netbeheer/IECCIM/TC57CIM/IEC61970/Base/Core#PowerSystemResource> ,
                             [ rdf:type owl:Restriction ;
                               owl:onProperty :SwitchPhase_Switch ;
                               owl:minQualifiedCardinality "0"^^xsd:nonNegativeInteger ;
                               owl:onClass :SwitchPhase
                             ] ,
                             [ rdf:type owl:Restriction ;
                               owl:onProperty :SwitchPhase_closed ;
                               owl:minQualifiedCardinality "0"^^xsd:nonNegativeInteger ;
                               owl:onDataRange xsd:boolean
                             ] ,
                             [ rdf:type owl:Restriction ;
                               owl:onProperty :SwitchPhase_normalOpen ;
                               owl:minQualifiedCardinality "0"^^xsd:nonNegativeInteger ;
                               owl:onDataRange xsd:boolean
                             ] ,
                             [ rdf:type owl:Restriction ;
                               owl:onProperty :SwitchPhase_phaseSide1 ;
                               owl:minQualifiedCardinality "0"^^xsd:nonNegativeInteger ;
                               owl:onDataRange :SinglePhaseKind
                             ] ,
                             [ rdf:type owl:Restriction ;
                               owl:onProperty :SwitchPhase_phaseSide2 ;
                               owl:minQualifiedCardinality "0"^^xsd:nonNegativeInteger ;
                               owl:onDataRange :SinglePhaseKind
                             ] ,
                             [ rdf:type owl:Restriction ;
                               owl:onProperty :SwitchPhase_closed ;
                               owl:maxQualifiedCardinality "1"^^xsd:nonNegativeInteger ;
                               owl:onDataRange xsd:boolean
                             ] ,
                             [ rdf:type owl:Restriction ;
                               owl:onProperty :SwitchPhase_normalOpen ;
                               owl:maxQualifiedCardinality "1"^^xsd:nonNegativeInteger ;
                               owl:onDataRange xsd:boolean
                             ] ,
                             [ rdf:type owl:Restriction ;
                               owl:onProperty :SwitchPhase_phaseSide1 ;
                               owl:maxQualifiedCardinality "1"^^xsd:nonNegativeInteger ;
                               owl:onDataRange :SinglePhaseKind
                             ] ,
                             [ rdf:type owl:Restriction ;
                               owl:onProperty :SwitchPhase_phaseSide2 ;
                               owl:maxQualifiedCardinality "1"^^xsd:nonNegativeInteger ;
                               owl:onDataRange :SinglePhaseKind
                             ] ;
             rdfs:comment """Single phase of a multi-phase switch when its attributes might be different per phase.
""" .


###  https://w3id.org/netbeheer/IECCIM/TC57CIM/IEC61970/Base/Wires#SwitchSchedule
:SwitchSchedule rdf:type owl:Class ;
                rdfs:subClassOf <https://w3id.org/netbeheer/IECCIM/TC57CIM/IEC61970/Base/LoadModel#SeasonDayTypeSchedule> ,
                                [ rdf:type owl:Restriction ;
                                  owl:onProperty :SwitchSchedule_Switch ;
                                  owl:minQualifiedCardinality "0"^^xsd:nonNegativeInteger ;
                                  owl:onClass :SwitchSchedule
                                ] ;
                rdfs:comment "A schedule of switch positions.  If RegularTimePoint.value1 is 0, the switch is open.  If 1, the switch is closed.  " .


###  https://w3id.org/netbeheer/IECCIM/TC57CIM/IEC61970/Base/Wires#SynchronousMachine
:SynchronousMachine rdf:type owl:Class ;
                    rdfs:subClassOf :RotatingMachine ,
                                    [ rdf:type owl:Restriction ;
                                      owl:onProperty :SynchronousMachine_InitialReactiveCapabilityCurve ;
                                      owl:minQualifiedCardinality "1"^^xsd:nonNegativeInteger ;
                                      owl:onClass :SynchronousMachine
                                    ] ,
                                    [ rdf:type owl:Restriction ;
                                      owl:onProperty :SynchronousMachine_PrimeMovers ;
                                      owl:minQualifiedCardinality "0"^^xsd:nonNegativeInteger ;
                                      owl:onClass :SynchronousMachine
                                    ] ,
                                    [ rdf:type owl:Restriction ;
                                      owl:onProperty :SynchronousMachine_ReactiveCapabilityCurves ;
                                      owl:minQualifiedCardinality "1"^^xsd:nonNegativeInteger ;
                                      owl:onClass :SynchronousMachine
                                    ] ,
                                    [ rdf:type owl:Restriction ;
                                      owl:onProperty :SynchronousMachine_aVRToManualLag ;
                                      owl:minQualifiedCardinality "0"^^xsd:nonNegativeInteger ;
                                      owl:onClass <https://w3id.org/netbeheer/IECCIM/TC57CIM/IEC61970/Base/Domain#Seconds>
                                    ] ,
                                    [ rdf:type owl:Restriction ;
                                      owl:onProperty :SynchronousMachine_aVRToManualLead ;
                                      owl:minQualifiedCardinality "0"^^xsd:nonNegativeInteger ;
                                      owl:onClass <https://w3id.org/netbeheer/IECCIM/TC57CIM/IEC61970/Base/Domain#Seconds>
                                    ] ,
                                    [ rdf:type owl:Restriction ;
                                      owl:onProperty :SynchronousMachine_baseQ ;
                                      owl:minQualifiedCardinality "0"^^xsd:nonNegativeInteger ;
                                      owl:onClass <https://w3id.org/netbeheer/IECCIM/TC57CIM/IEC61970/Base/Domain#ReactivePower>
                                    ] ,
                                    [ rdf:type owl:Restriction ;
                                      owl:onProperty :SynchronousMachine_condenserP ;
                                      owl:minQualifiedCardinality "0"^^xsd:nonNegativeInteger ;
                                      owl:onClass <https://w3id.org/netbeheer/IECCIM/TC57CIM/IEC61970/Base/Domain#ActivePower>
                                    ] ,
                                    [ rdf:type owl:Restriction ;
                                      owl:onProperty :SynchronousMachine_earthingStarPointR ;
                                      owl:minQualifiedCardinality "0"^^xsd:nonNegativeInteger ;
                                      owl:onClass <https://w3id.org/netbeheer/IECCIM/TC57CIM/IEC61970/Base/Domain#Resistance>
                                    ] ,
                                    [ rdf:type owl:Restriction ;
                                      owl:onProperty :SynchronousMachine_earthingStarPointX ;
                                      owl:minQualifiedCardinality "0"^^xsd:nonNegativeInteger ;
                                      owl:onClass <https://w3id.org/netbeheer/IECCIM/TC57CIM/IEC61970/Base/Domain#Reactance>
                                    ] ,
                                    [ rdf:type owl:Restriction ;
                                      owl:onProperty :SynchronousMachine_ikk ;
                                      owl:minQualifiedCardinality "0"^^xsd:nonNegativeInteger ;
                                      owl:onClass <https://w3id.org/netbeheer/IECCIM/TC57CIM/IEC61970/Base/Domain#CurrentFlow>
                                    ] ,
                                    [ rdf:type owl:Restriction ;
                                      owl:onProperty :SynchronousMachine_manualToAVR ;
                                      owl:minQualifiedCardinality "0"^^xsd:nonNegativeInteger ;
                                      owl:onClass <https://w3id.org/netbeheer/IECCIM/TC57CIM/IEC61970/Base/Domain#Seconds>
                                    ] ,
                                    [ rdf:type owl:Restriction ;
                                      owl:onProperty :SynchronousMachine_maxQ ;
                                      owl:minQualifiedCardinality "0"^^xsd:nonNegativeInteger ;
                                      owl:onClass <https://w3id.org/netbeheer/IECCIM/TC57CIM/IEC61970/Base/Domain#ReactivePower>
                                    ] ,
                                    [ rdf:type owl:Restriction ;
                                      owl:onProperty :SynchronousMachine_maxU ;
                                      owl:minQualifiedCardinality "0"^^xsd:nonNegativeInteger ;
                                      owl:onClass <https://w3id.org/netbeheer/IECCIM/TC57CIM/IEC61970/Base/Domain#Voltage>
                                    ] ,
                                    [ rdf:type owl:Restriction ;
                                      owl:onProperty :SynchronousMachine_minQ ;
                                      owl:minQualifiedCardinality "0"^^xsd:nonNegativeInteger ;
                                      owl:onClass <https://w3id.org/netbeheer/IECCIM/TC57CIM/IEC61970/Base/Domain#ReactivePower>
                                    ] ,
                                    [ rdf:type owl:Restriction ;
                                      owl:onProperty :SynchronousMachine_minU ;
                                      owl:minQualifiedCardinality "0"^^xsd:nonNegativeInteger ;
                                      owl:onClass <https://w3id.org/netbeheer/IECCIM/TC57CIM/IEC61970/Base/Domain#Voltage>
                                    ] ,
                                    [ rdf:type owl:Restriction ;
                                      owl:onProperty :SynchronousMachine_qPercent ;
                                      owl:minQualifiedCardinality "0"^^xsd:nonNegativeInteger ;
                                      owl:onClass <https://w3id.org/netbeheer/IECCIM/TC57CIM/IEC61970/Base/Domain#PerCent>
                                    ] ,
                                    [ rdf:type owl:Restriction ;
                                      owl:onProperty :SynchronousMachine_r ;
                                      owl:minQualifiedCardinality "0"^^xsd:nonNegativeInteger ;
                                      owl:onClass <https://w3id.org/netbeheer/IECCIM/TC57CIM/IEC61970/Base/Domain#Resistance>
                                    ] ,
                                    [ rdf:type owl:Restriction ;
                                      owl:onProperty :SynchronousMachine_r0 ;
                                      owl:minQualifiedCardinality "0"^^xsd:nonNegativeInteger ;
                                      owl:onClass <https://w3id.org/netbeheer/IECCIM/TC57CIM/IEC61970/Base/Domain#Resistance>
                                    ] ,
                                    [ rdf:type owl:Restriction ;
                                      owl:onProperty :SynchronousMachine_r2 ;
                                      owl:minQualifiedCardinality "0"^^xsd:nonNegativeInteger ;
                                      owl:onClass <https://w3id.org/netbeheer/IECCIM/TC57CIM/IEC61970/Base/Domain#Resistance>
                                    ] ,
                                    [ rdf:type owl:Restriction ;
                                      owl:onProperty :SynchronousMachine_satDirectSubtransX ;
                                      owl:minQualifiedCardinality "0"^^xsd:nonNegativeInteger ;
                                      owl:onClass <https://w3id.org/netbeheer/IECCIM/TC57CIM/IEC61970/Base/Domain#PU>
                                    ] ,
                                    [ rdf:type owl:Restriction ;
                                      owl:onProperty :SynchronousMachine_satDirectSyncX ;
                                      owl:minQualifiedCardinality "0"^^xsd:nonNegativeInteger ;
                                      owl:onClass <https://w3id.org/netbeheer/IECCIM/TC57CIM/IEC61970/Base/Domain#PU>
                                    ] ,
                                    [ rdf:type owl:Restriction ;
                                      owl:onProperty :SynchronousMachine_satDirectTransX ;
                                      owl:minQualifiedCardinality "0"^^xsd:nonNegativeInteger ;
                                      owl:onClass <https://w3id.org/netbeheer/IECCIM/TC57CIM/IEC61970/Base/Domain#PU>
                                    ] ,
                                    [ rdf:type owl:Restriction ;
                                      owl:onProperty :SynchronousMachine_voltageRegulationRange ;
                                      owl:minQualifiedCardinality "0"^^xsd:nonNegativeInteger ;
                                      owl:onClass <https://w3id.org/netbeheer/IECCIM/TC57CIM/IEC61970/Base/Domain#PerCent>
                                    ] ,
                                    [ rdf:type owl:Restriction ;
                                      owl:onProperty :SynchronousMachine_x0 ;
                                      owl:minQualifiedCardinality "0"^^xsd:nonNegativeInteger ;
                                      owl:onClass <https://w3id.org/netbeheer/IECCIM/TC57CIM/IEC61970/Base/Domain#Reactance>
                                    ] ,
                                    [ rdf:type owl:Restriction ;
                                      owl:onProperty :SynchronousMachine_x2 ;
                                      owl:minQualifiedCardinality "0"^^xsd:nonNegativeInteger ;
                                      owl:onClass <https://w3id.org/netbeheer/IECCIM/TC57CIM/IEC61970/Base/Domain#Reactance>
                                    ] ,
                                    [ rdf:type owl:Restriction ;
                                      owl:onProperty :SynchronousMachine_SynchronousMachineDynamics ;
                                      owl:qualifiedCardinality "1"^^xsd:nonNegativeInteger ;
                                      owl:onClass :SynchronousMachine
                                    ] ,
                                    [ rdf:type owl:Restriction ;
                                      owl:onProperty :SynchronousMachine_aVRToManualLag ;
                                      owl:maxQualifiedCardinality "1"^^xsd:nonNegativeInteger ;
                                      owl:onClass <https://w3id.org/netbeheer/IECCIM/TC57CIM/IEC61970/Base/Domain#Seconds>
                                    ] ,
                                    [ rdf:type owl:Restriction ;
                                      owl:onProperty :SynchronousMachine_aVRToManualLead ;
                                      owl:maxQualifiedCardinality "1"^^xsd:nonNegativeInteger ;
                                      owl:onClass <https://w3id.org/netbeheer/IECCIM/TC57CIM/IEC61970/Base/Domain#Seconds>
                                    ] ,
                                    [ rdf:type owl:Restriction ;
                                      owl:onProperty :SynchronousMachine_baseQ ;
                                      owl:maxQualifiedCardinality "1"^^xsd:nonNegativeInteger ;
                                      owl:onClass <https://w3id.org/netbeheer/IECCIM/TC57CIM/IEC61970/Base/Domain#ReactivePower>
                                    ] ,
                                    [ rdf:type owl:Restriction ;
                                      owl:onProperty :SynchronousMachine_condenserP ;
                                      owl:maxQualifiedCardinality "1"^^xsd:nonNegativeInteger ;
                                      owl:onClass <https://w3id.org/netbeheer/IECCIM/TC57CIM/IEC61970/Base/Domain#ActivePower>
                                    ] ,
                                    [ rdf:type owl:Restriction ;
                                      owl:onProperty :SynchronousMachine_earthingStarPointR ;
                                      owl:maxQualifiedCardinality "1"^^xsd:nonNegativeInteger ;
                                      owl:onClass <https://w3id.org/netbeheer/IECCIM/TC57CIM/IEC61970/Base/Domain#Resistance>
                                    ] ,
                                    [ rdf:type owl:Restriction ;
                                      owl:onProperty :SynchronousMachine_earthingStarPointX ;
                                      owl:maxQualifiedCardinality "1"^^xsd:nonNegativeInteger ;
                                      owl:onClass <https://w3id.org/netbeheer/IECCIM/TC57CIM/IEC61970/Base/Domain#Reactance>
                                    ] ,
                                    [ rdf:type owl:Restriction ;
                                      owl:onProperty :SynchronousMachine_ikk ;
                                      owl:maxQualifiedCardinality "1"^^xsd:nonNegativeInteger ;
                                      owl:onClass <https://w3id.org/netbeheer/IECCIM/TC57CIM/IEC61970/Base/Domain#CurrentFlow>
                                    ] ,
                                    [ rdf:type owl:Restriction ;
                                      owl:onProperty :SynchronousMachine_manualToAVR ;
                                      owl:maxQualifiedCardinality "1"^^xsd:nonNegativeInteger ;
                                      owl:onClass <https://w3id.org/netbeheer/IECCIM/TC57CIM/IEC61970/Base/Domain#Seconds>
                                    ] ,
                                    [ rdf:type owl:Restriction ;
                                      owl:onProperty :SynchronousMachine_maxQ ;
                                      owl:maxQualifiedCardinality "1"^^xsd:nonNegativeInteger ;
                                      owl:onClass <https://w3id.org/netbeheer/IECCIM/TC57CIM/IEC61970/Base/Domain#ReactivePower>
                                    ] ,
                                    [ rdf:type owl:Restriction ;
                                      owl:onProperty :SynchronousMachine_maxU ;
                                      owl:maxQualifiedCardinality "1"^^xsd:nonNegativeInteger ;
                                      owl:onClass <https://w3id.org/netbeheer/IECCIM/TC57CIM/IEC61970/Base/Domain#Voltage>
                                    ] ,
                                    [ rdf:type owl:Restriction ;
                                      owl:onProperty :SynchronousMachine_minQ ;
                                      owl:maxQualifiedCardinality "1"^^xsd:nonNegativeInteger ;
                                      owl:onClass <https://w3id.org/netbeheer/IECCIM/TC57CIM/IEC61970/Base/Domain#ReactivePower>
                                    ] ,
                                    [ rdf:type owl:Restriction ;
                                      owl:onProperty :SynchronousMachine_minU ;
                                      owl:maxQualifiedCardinality "1"^^xsd:nonNegativeInteger ;
                                      owl:onClass <https://w3id.org/netbeheer/IECCIM/TC57CIM/IEC61970/Base/Domain#Voltage>
                                    ] ,
                                    [ rdf:type owl:Restriction ;
                                      owl:onProperty :SynchronousMachine_qPercent ;
                                      owl:maxQualifiedCardinality "1"^^xsd:nonNegativeInteger ;
                                      owl:onClass <https://w3id.org/netbeheer/IECCIM/TC57CIM/IEC61970/Base/Domain#PerCent>
                                    ] ,
                                    [ rdf:type owl:Restriction ;
                                      owl:onProperty :SynchronousMachine_r ;
                                      owl:maxQualifiedCardinality "1"^^xsd:nonNegativeInteger ;
                                      owl:onClass <https://w3id.org/netbeheer/IECCIM/TC57CIM/IEC61970/Base/Domain#Resistance>
                                    ] ,
                                    [ rdf:type owl:Restriction ;
                                      owl:onProperty :SynchronousMachine_r0 ;
                                      owl:maxQualifiedCardinality "1"^^xsd:nonNegativeInteger ;
                                      owl:onClass <https://w3id.org/netbeheer/IECCIM/TC57CIM/IEC61970/Base/Domain#Resistance>
                                    ] ,
                                    [ rdf:type owl:Restriction ;
                                      owl:onProperty :SynchronousMachine_r2 ;
                                      owl:maxQualifiedCardinality "1"^^xsd:nonNegativeInteger ;
                                      owl:onClass <https://w3id.org/netbeheer/IECCIM/TC57CIM/IEC61970/Base/Domain#Resistance>
                                    ] ,
                                    [ rdf:type owl:Restriction ;
                                      owl:onProperty :SynchronousMachine_satDirectSubtransX ;
                                      owl:maxQualifiedCardinality "1"^^xsd:nonNegativeInteger ;
                                      owl:onClass <https://w3id.org/netbeheer/IECCIM/TC57CIM/IEC61970/Base/Domain#PU>
                                    ] ,
                                    [ rdf:type owl:Restriction ;
                                      owl:onProperty :SynchronousMachine_satDirectSyncX ;
                                      owl:maxQualifiedCardinality "1"^^xsd:nonNegativeInteger ;
                                      owl:onClass <https://w3id.org/netbeheer/IECCIM/TC57CIM/IEC61970/Base/Domain#PU>
                                    ] ,
                                    [ rdf:type owl:Restriction ;
                                      owl:onProperty :SynchronousMachine_satDirectTransX ;
                                      owl:maxQualifiedCardinality "1"^^xsd:nonNegativeInteger ;
                                      owl:onClass <https://w3id.org/netbeheer/IECCIM/TC57CIM/IEC61970/Base/Domain#PU>
                                    ] ,
                                    [ rdf:type owl:Restriction ;
                                      owl:onProperty :SynchronousMachine_voltageRegulationRange ;
                                      owl:maxQualifiedCardinality "1"^^xsd:nonNegativeInteger ;
                                      owl:onClass <https://w3id.org/netbeheer/IECCIM/TC57CIM/IEC61970/Base/Domain#PerCent>
                                    ] ,
                                    [ rdf:type owl:Restriction ;
                                      owl:onProperty :SynchronousMachine_x0 ;
                                      owl:maxQualifiedCardinality "1"^^xsd:nonNegativeInteger ;
                                      owl:onClass <https://w3id.org/netbeheer/IECCIM/TC57CIM/IEC61970/Base/Domain#Reactance>
                                    ] ,
                                    [ rdf:type owl:Restriction ;
                                      owl:onProperty :SynchronousMachine_x2 ;
                                      owl:maxQualifiedCardinality "1"^^xsd:nonNegativeInteger ;
                                      owl:onClass <https://w3id.org/netbeheer/IECCIM/TC57CIM/IEC61970/Base/Domain#Reactance>
                                    ] ,
                                    [ rdf:type owl:Restriction ;
                                      owl:onProperty :SynchronousMachine_coolantCondition ;
                                      owl:minQualifiedCardinality "0"^^xsd:nonNegativeInteger ;
                                      owl:onDataRange xsd:float
                                    ] ,
                                    [ rdf:type owl:Restriction ;
                                      owl:onProperty :SynchronousMachine_coolantType ;
                                      owl:minQualifiedCardinality "0"^^xsd:nonNegativeInteger ;
                                      owl:onDataRange :CoolantType
                                    ] ,
                                    [ rdf:type owl:Restriction ;
                                      owl:onProperty :SynchronousMachine_earthing ;
                                      owl:minQualifiedCardinality "0"^^xsd:nonNegativeInteger ;
                                      owl:onDataRange xsd:boolean
                                    ] ,
                                    [ rdf:type owl:Restriction ;
                                      owl:onProperty :SynchronousMachine_mu ;
                                      owl:minQualifiedCardinality "0"^^xsd:nonNegativeInteger ;
                                      owl:onDataRange xsd:float
                                    ] ,
                                    [ rdf:type owl:Restriction ;
                                      owl:onProperty :SynchronousMachine_operatingMode ;
                                      owl:minQualifiedCardinality "0"^^xsd:nonNegativeInteger ;
                                      owl:onDataRange :SynchronousMachineOperatingMode
                                    ] ,
                                    [ rdf:type owl:Restriction ;
                                      owl:onProperty :SynchronousMachine_referencePriority ;
                                      owl:minQualifiedCardinality "0"^^xsd:nonNegativeInteger ;
                                      owl:onDataRange xsd:nonNegativeInteger
                                    ] ,
                                    [ rdf:type owl:Restriction ;
                                      owl:onProperty :SynchronousMachine_shortCircuitRotorType ;
                                      owl:minQualifiedCardinality "0"^^xsd:nonNegativeInteger ;
                                      owl:onDataRange :ShortCircuitRotorKind
                                    ] ,
                                    [ rdf:type owl:Restriction ;
                                      owl:onProperty :SynchronousMachine_type ;
                                      owl:minQualifiedCardinality "0"^^xsd:nonNegativeInteger ;
                                      owl:onDataRange :SynchronousMachineKind
                                    ] ,
                                    [ rdf:type owl:Restriction ;
                                      owl:onProperty :SynchronousMachine_coolantCondition ;
                                      owl:maxQualifiedCardinality "1"^^xsd:nonNegativeInteger ;
                                      owl:onDataRange xsd:float
                                    ] ,
                                    [ rdf:type owl:Restriction ;
                                      owl:onProperty :SynchronousMachine_coolantType ;
                                      owl:maxQualifiedCardinality "1"^^xsd:nonNegativeInteger ;
                                      owl:onDataRange :CoolantType
                                    ] ,
                                    [ rdf:type owl:Restriction ;
                                      owl:onProperty :SynchronousMachine_earthing ;
                                      owl:maxQualifiedCardinality "1"^^xsd:nonNegativeInteger ;
                                      owl:onDataRange xsd:boolean
                                    ] ,
                                    [ rdf:type owl:Restriction ;
                                      owl:onProperty :SynchronousMachine_mu ;
                                      owl:maxQualifiedCardinality "1"^^xsd:nonNegativeInteger ;
                                      owl:onDataRange xsd:float
                                    ] ,
                                    [ rdf:type owl:Restriction ;
                                      owl:onProperty :SynchronousMachine_operatingMode ;
                                      owl:maxQualifiedCardinality "1"^^xsd:nonNegativeInteger ;
                                      owl:onDataRange :SynchronousMachineOperatingMode
                                    ] ,
                                    [ rdf:type owl:Restriction ;
                                      owl:onProperty :SynchronousMachine_referencePriority ;
                                      owl:maxQualifiedCardinality "1"^^xsd:nonNegativeInteger ;
                                      owl:onDataRange xsd:nonNegativeInteger
                                    ] ,
                                    [ rdf:type owl:Restriction ;
                                      owl:onProperty :SynchronousMachine_shortCircuitRotorType ;
                                      owl:maxQualifiedCardinality "1"^^xsd:nonNegativeInteger ;
                                      owl:onDataRange :ShortCircuitRotorKind
                                    ] ,
                                    [ rdf:type owl:Restriction ;
                                      owl:onProperty :SynchronousMachine_type ;
                                      owl:maxQualifiedCardinality "1"^^xsd:nonNegativeInteger ;
                                      owl:onDataRange :SynchronousMachineKind
                                    ] ;
                    rdfs:comment "An electromechanical device that operates with shaft rotating synchronously with the network. It is a single machine operating either as a generator or synchronous condenser or pump." .


###  https://w3id.org/netbeheer/IECCIM/TC57CIM/IEC61970/Base/Wires#TapChanger
:TapChanger rdf:type owl:Class ;
            rdfs:subClassOf <https://w3id.org/netbeheer/IECCIM/TC57CIM/IEC61970/Base/Core#PowerSystemResource> ,
                            [ rdf:type owl:Restriction ;
                              owl:onProperty :TapChanger_TapChangerControl ;
                              owl:minQualifiedCardinality "0"^^xsd:nonNegativeInteger ;
                              owl:onClass :TapChanger
                            ] ,
                            [ rdf:type owl:Restriction ;
                              owl:onProperty :TapChanger_initialDelay ;
                              owl:minQualifiedCardinality "0"^^xsd:nonNegativeInteger ;
                              owl:onClass <https://w3id.org/netbeheer/IECCIM/TC57CIM/IEC61970/Base/Domain#Seconds>
                            ] ,
                            [ rdf:type owl:Restriction ;
                              owl:onProperty :TapChanger_neutralU ;
                              owl:minQualifiedCardinality "0"^^xsd:nonNegativeInteger ;
                              owl:onClass <https://w3id.org/netbeheer/IECCIM/TC57CIM/IEC61970/Base/Domain#Voltage>
                            ] ,
                            [ rdf:type owl:Restriction ;
                              owl:onProperty :TapChanger_subsequentDelay ;
                              owl:minQualifiedCardinality "0"^^xsd:nonNegativeInteger ;
                              owl:onClass <https://w3id.org/netbeheer/IECCIM/TC57CIM/IEC61970/Base/Domain#Seconds>
                            ] ,
                            [ rdf:type owl:Restriction ;
                              owl:onProperty :TapChanger_SvTapStep ;
                              owl:qualifiedCardinality "1"^^xsd:nonNegativeInteger ;
                              owl:onClass :TapChanger
                            ] ,
                            [ rdf:type owl:Restriction ;
                              owl:onProperty :TapChanger_TapSchedules ;
                              owl:qualifiedCardinality "1"^^xsd:nonNegativeInteger ;
                              owl:onClass :TapChanger
                            ] ,
                            [ rdf:type owl:Restriction ;
                              owl:onProperty :TapChanger_initialDelay ;
                              owl:maxQualifiedCardinality "1"^^xsd:nonNegativeInteger ;
                              owl:onClass <https://w3id.org/netbeheer/IECCIM/TC57CIM/IEC61970/Base/Domain#Seconds>
                            ] ,
                            [ rdf:type owl:Restriction ;
                              owl:onProperty :TapChanger_neutralU ;
                              owl:maxQualifiedCardinality "1"^^xsd:nonNegativeInteger ;
                              owl:onClass <https://w3id.org/netbeheer/IECCIM/TC57CIM/IEC61970/Base/Domain#Voltage>
                            ] ,
                            [ rdf:type owl:Restriction ;
                              owl:onProperty :TapChanger_subsequentDelay ;
                              owl:maxQualifiedCardinality "1"^^xsd:nonNegativeInteger ;
                              owl:onClass <https://w3id.org/netbeheer/IECCIM/TC57CIM/IEC61970/Base/Domain#Seconds>
                            ] ,
                            [ rdf:type owl:Restriction ;
                              owl:onProperty :TapChanger_controlEnabled ;
                              owl:minQualifiedCardinality "0"^^xsd:nonNegativeInteger ;
                              owl:onDataRange xsd:boolean
                            ] ,
                            [ rdf:type owl:Restriction ;
                              owl:onProperty :TapChanger_highStep ;
                              owl:minQualifiedCardinality "0"^^xsd:nonNegativeInteger ;
                              owl:onDataRange xsd:nonNegativeInteger
                            ] ,
                            [ rdf:type owl:Restriction ;
                              owl:onProperty :TapChanger_lowStep ;
                              owl:minQualifiedCardinality "0"^^xsd:nonNegativeInteger ;
                              owl:onDataRange xsd:nonNegativeInteger
                            ] ,
                            [ rdf:type owl:Restriction ;
                              owl:onProperty :TapChanger_ltcFlag ;
                              owl:minQualifiedCardinality "0"^^xsd:nonNegativeInteger ;
                              owl:onDataRange xsd:boolean
                            ] ,
                            [ rdf:type owl:Restriction ;
                              owl:onProperty :TapChanger_neutralStep ;
                              owl:minQualifiedCardinality "0"^^xsd:nonNegativeInteger ;
                              owl:onDataRange xsd:nonNegativeInteger
                            ] ,
                            [ rdf:type owl:Restriction ;
                              owl:onProperty :TapChanger_normalStep ;
                              owl:minQualifiedCardinality "0"^^xsd:nonNegativeInteger ;
                              owl:onDataRange xsd:nonNegativeInteger
                            ] ,
                            [ rdf:type owl:Restriction ;
                              owl:onProperty :TapChanger_step ;
                              owl:minQualifiedCardinality "0"^^xsd:nonNegativeInteger ;
                              owl:onDataRange xsd:float
                            ] ,
                            [ rdf:type owl:Restriction ;
                              owl:onProperty :TapChanger_controlEnabled ;
                              owl:maxQualifiedCardinality "1"^^xsd:nonNegativeInteger ;
                              owl:onDataRange xsd:boolean
                            ] ,
                            [ rdf:type owl:Restriction ;
                              owl:onProperty :TapChanger_highStep ;
                              owl:maxQualifiedCardinality "1"^^xsd:nonNegativeInteger ;
                              owl:onDataRange xsd:nonNegativeInteger
                            ] ,
                            [ rdf:type owl:Restriction ;
                              owl:onProperty :TapChanger_lowStep ;
                              owl:maxQualifiedCardinality "1"^^xsd:nonNegativeInteger ;
                              owl:onDataRange xsd:nonNegativeInteger
                            ] ,
                            [ rdf:type owl:Restriction ;
                              owl:onProperty :TapChanger_ltcFlag ;
                              owl:maxQualifiedCardinality "1"^^xsd:nonNegativeInteger ;
                              owl:onDataRange xsd:boolean
                            ] ,
                            [ rdf:type owl:Restriction ;
                              owl:onProperty :TapChanger_neutralStep ;
                              owl:maxQualifiedCardinality "1"^^xsd:nonNegativeInteger ;
                              owl:onDataRange xsd:nonNegativeInteger
                            ] ,
                            [ rdf:type owl:Restriction ;
                              owl:onProperty :TapChanger_normalStep ;
                              owl:maxQualifiedCardinality "1"^^xsd:nonNegativeInteger ;
                              owl:onDataRange xsd:nonNegativeInteger
                            ] ,
                            [ rdf:type owl:Restriction ;
                              owl:onProperty :TapChanger_step ;
                              owl:maxQualifiedCardinality "1"^^xsd:nonNegativeInteger ;
                              owl:onDataRange xsd:float
                            ] ;
            rdfs:comment "Mechanism for changing transformer winding tap positions." .


###  https://w3id.org/netbeheer/IECCIM/TC57CIM/IEC61970/Base/Wires#TapChangerControl
:TapChangerControl rdf:type owl:Class ;
                   rdfs:subClassOf :RegulatingControl ,
                                   [ rdf:type owl:Restriction ;
                                     owl:onProperty :TapChangerControl_TapChanger ;
                                     owl:minQualifiedCardinality "0"^^xsd:nonNegativeInteger ;
                                     owl:onClass :TapChangerControl
                                   ] ,
                                   [ rdf:type owl:Restriction ;
                                     owl:onProperty :TapChangerControl_limitVoltage ;
                                     owl:minQualifiedCardinality "0"^^xsd:nonNegativeInteger ;
                                     owl:onClass <https://w3id.org/netbeheer/IECCIM/TC57CIM/IEC61970/Base/Domain#Voltage>
                                   ] ,
                                   [ rdf:type owl:Restriction ;
                                     owl:onProperty :TapChangerControl_lineDropR ;
                                     owl:minQualifiedCardinality "0"^^xsd:nonNegativeInteger ;
                                     owl:onClass <https://w3id.org/netbeheer/IECCIM/TC57CIM/IEC61970/Base/Domain#Resistance>
                                   ] ,
                                   [ rdf:type owl:Restriction ;
                                     owl:onProperty :TapChangerControl_lineDropX ;
                                     owl:minQualifiedCardinality "0"^^xsd:nonNegativeInteger ;
                                     owl:onClass <https://w3id.org/netbeheer/IECCIM/TC57CIM/IEC61970/Base/Domain#Reactance>
                                   ] ,
                                   [ rdf:type owl:Restriction ;
                                     owl:onProperty :TapChangerControl_reverseLineDropR ;
                                     owl:minQualifiedCardinality "0"^^xsd:nonNegativeInteger ;
                                     owl:onClass <https://w3id.org/netbeheer/IECCIM/TC57CIM/IEC61970/Base/Domain#Resistance>
                                   ] ,
                                   [ rdf:type owl:Restriction ;
                                     owl:onProperty :TapChangerControl_reverseLineDropX ;
                                     owl:minQualifiedCardinality "0"^^xsd:nonNegativeInteger ;
                                     owl:onClass <https://w3id.org/netbeheer/IECCIM/TC57CIM/IEC61970/Base/Domain#Reactance>
                                   ] ,
                                   [ rdf:type owl:Restriction ;
                                     owl:onProperty :TapChangerControl_TapChanger ;
                                     owl:maxQualifiedCardinality "1"^^xsd:nonNegativeInteger ;
                                     owl:onClass :TapChangerControl
                                   ] ,
                                   [ rdf:type owl:Restriction ;
                                     owl:onProperty :TapChangerControl_limitVoltage ;
                                     owl:maxQualifiedCardinality "1"^^xsd:nonNegativeInteger ;
                                     owl:onClass <https://w3id.org/netbeheer/IECCIM/TC57CIM/IEC61970/Base/Domain#Voltage>
                                   ] ,
                                   [ rdf:type owl:Restriction ;
                                     owl:onProperty :TapChangerControl_lineDropR ;
                                     owl:maxQualifiedCardinality "1"^^xsd:nonNegativeInteger ;
                                     owl:onClass <https://w3id.org/netbeheer/IECCIM/TC57CIM/IEC61970/Base/Domain#Resistance>
                                   ] ,
                                   [ rdf:type owl:Restriction ;
                                     owl:onProperty :TapChangerControl_lineDropX ;
                                     owl:maxQualifiedCardinality "1"^^xsd:nonNegativeInteger ;
                                     owl:onClass <https://w3id.org/netbeheer/IECCIM/TC57CIM/IEC61970/Base/Domain#Reactance>
                                   ] ,
                                   [ rdf:type owl:Restriction ;
                                     owl:onProperty :TapChangerControl_reverseLineDropR ;
                                     owl:maxQualifiedCardinality "1"^^xsd:nonNegativeInteger ;
                                     owl:onClass <https://w3id.org/netbeheer/IECCIM/TC57CIM/IEC61970/Base/Domain#Resistance>
                                   ] ,
                                   [ rdf:type owl:Restriction ;
                                     owl:onProperty :TapChangerControl_reverseLineDropX ;
                                     owl:maxQualifiedCardinality "1"^^xsd:nonNegativeInteger ;
                                     owl:onClass <https://w3id.org/netbeheer/IECCIM/TC57CIM/IEC61970/Base/Domain#Reactance>
                                   ] ,
                                   [ rdf:type owl:Restriction ;
                                     owl:onProperty :TapChangerControl_lineDropCompensation ;
                                     owl:minQualifiedCardinality "0"^^xsd:nonNegativeInteger ;
                                     owl:onDataRange xsd:boolean
                                   ] ,
                                   [ rdf:type owl:Restriction ;
                                     owl:onProperty :TapChangerControl_lineDropCompensation ;
                                     owl:maxQualifiedCardinality "1"^^xsd:nonNegativeInteger ;
                                     owl:onDataRange xsd:boolean
                                   ] ;
                   rdfs:comment "Describes behavior specific to tap changers, e.g. how the voltage at the end of a line varies with the load level and compensation of the voltage drop by tap adjustment." .


###  https://w3id.org/netbeheer/IECCIM/TC57CIM/IEC61970/Base/Wires#TapChangerTablePoint
:TapChangerTablePoint rdf:type owl:Class ;
                      rdfs:subClassOf [ rdf:type owl:Restriction ;
                                        owl:onProperty :TapChangerTablePoint_b ;
                                        owl:minQualifiedCardinality "0"^^xsd:nonNegativeInteger ;
                                        owl:onClass <https://w3id.org/netbeheer/IECCIM/TC57CIM/IEC61970/Base/Domain#PerCent>
                                      ] ,
                                      [ rdf:type owl:Restriction ;
                                        owl:onProperty :TapChangerTablePoint_g ;
                                        owl:minQualifiedCardinality "0"^^xsd:nonNegativeInteger ;
                                        owl:onClass <https://w3id.org/netbeheer/IECCIM/TC57CIM/IEC61970/Base/Domain#PerCent>
                                      ] ,
                                      [ rdf:type owl:Restriction ;
                                        owl:onProperty :TapChangerTablePoint_r ;
                                        owl:minQualifiedCardinality "0"^^xsd:nonNegativeInteger ;
                                        owl:onClass <https://w3id.org/netbeheer/IECCIM/TC57CIM/IEC61970/Base/Domain#PerCent>
                                      ] ,
                                      [ rdf:type owl:Restriction ;
                                        owl:onProperty :TapChangerTablePoint_x ;
                                        owl:minQualifiedCardinality "0"^^xsd:nonNegativeInteger ;
                                        owl:onClass <https://w3id.org/netbeheer/IECCIM/TC57CIM/IEC61970/Base/Domain#PerCent>
                                      ] ,
                                      [ rdf:type owl:Restriction ;
                                        owl:onProperty :TapChangerTablePoint_b ;
                                        owl:maxQualifiedCardinality "1"^^xsd:nonNegativeInteger ;
                                        owl:onClass <https://w3id.org/netbeheer/IECCIM/TC57CIM/IEC61970/Base/Domain#PerCent>
                                      ] ,
                                      [ rdf:type owl:Restriction ;
                                        owl:onProperty :TapChangerTablePoint_g ;
                                        owl:maxQualifiedCardinality "1"^^xsd:nonNegativeInteger ;
                                        owl:onClass <https://w3id.org/netbeheer/IECCIM/TC57CIM/IEC61970/Base/Domain#PerCent>
                                      ] ,
                                      [ rdf:type owl:Restriction ;
                                        owl:onProperty :TapChangerTablePoint_r ;
                                        owl:maxQualifiedCardinality "1"^^xsd:nonNegativeInteger ;
                                        owl:onClass <https://w3id.org/netbeheer/IECCIM/TC57CIM/IEC61970/Base/Domain#PerCent>
                                      ] ,
                                      [ rdf:type owl:Restriction ;
                                        owl:onProperty :TapChangerTablePoint_x ;
                                        owl:maxQualifiedCardinality "1"^^xsd:nonNegativeInteger ;
                                        owl:onClass <https://w3id.org/netbeheer/IECCIM/TC57CIM/IEC61970/Base/Domain#PerCent>
                                      ] ,
                                      [ rdf:type owl:Restriction ;
                                        owl:onProperty :TapChangerTablePoint_ratio ;
                                        owl:minQualifiedCardinality "0"^^xsd:nonNegativeInteger ;
                                        owl:onDataRange xsd:float
                                      ] ,
                                      [ rdf:type owl:Restriction ;
                                        owl:onProperty :TapChangerTablePoint_step ;
                                        owl:minQualifiedCardinality "0"^^xsd:nonNegativeInteger ;
                                        owl:onDataRange xsd:nonNegativeInteger
                                      ] ,
                                      [ rdf:type owl:Restriction ;
                                        owl:onProperty :TapChangerTablePoint_ratio ;
                                        owl:maxQualifiedCardinality "1"^^xsd:nonNegativeInteger ;
                                        owl:onDataRange xsd:float
                                      ] ,
                                      [ rdf:type owl:Restriction ;
                                        owl:onProperty :TapChangerTablePoint_step ;
                                        owl:maxQualifiedCardinality "1"^^xsd:nonNegativeInteger ;
                                        owl:onDataRange xsd:nonNegativeInteger
                                      ] .


###  https://w3id.org/netbeheer/IECCIM/TC57CIM/IEC61970/Base/Wires#TapSchedule
:TapSchedule rdf:type owl:Class ;
             rdfs:subClassOf <https://w3id.org/netbeheer/IECCIM/TC57CIM/IEC61970/Base/LoadModel#SeasonDayTypeSchedule> ,
                             [ rdf:type owl:Restriction ;
                               owl:onProperty :TapSchedule_TapChanger ;
                               owl:minQualifiedCardinality "0"^^xsd:nonNegativeInteger ;
                               owl:onClass :TapSchedule
                             ] ;
             rdfs:comment "A pre-established pattern over time for a tap step." .


###  https://w3id.org/netbeheer/IECCIM/TC57CIM/IEC61970/Base/Wires#TransformerCoreAdmittance
:TransformerCoreAdmittance rdf:type owl:Class ;
                           rdfs:subClassOf <https://w3id.org/netbeheer/IECCIM/TC57CIM/IEC61970/Base/Core#IdentifiedObject> ,
                                           [ rdf:type owl:Restriction ;
                                             owl:onProperty :TransformerCoreAdmittance_TransformerEnd ;
                                             owl:minQualifiedCardinality "0"^^xsd:nonNegativeInteger ;
                                             owl:onClass :TransformerCoreAdmittance
                                           ] ,
                                           [ rdf:type owl:Restriction ;
                                             owl:onProperty :TransformerCoreAdmittance_TransformerEndInfo ;
                                             owl:minQualifiedCardinality "0"^^xsd:nonNegativeInteger ;
                                             owl:onClass :TransformerCoreAdmittance
                                           ] ,
                                           [ rdf:type owl:Restriction ;
                                             owl:onProperty :TransformerCoreAdmittance_b ;
                                             owl:minQualifiedCardinality "0"^^xsd:nonNegativeInteger ;
                                             owl:onClass <https://w3id.org/netbeheer/IECCIM/TC57CIM/IEC61970/Base/Domain#Susceptance>
                                           ] ,
                                           [ rdf:type owl:Restriction ;
                                             owl:onProperty :TransformerCoreAdmittance_b0 ;
                                             owl:minQualifiedCardinality "0"^^xsd:nonNegativeInteger ;
                                             owl:onClass <https://w3id.org/netbeheer/IECCIM/TC57CIM/IEC61970/Base/Domain#Susceptance>
                                           ] ,
                                           [ rdf:type owl:Restriction ;
                                             owl:onProperty :TransformerCoreAdmittance_g ;
                                             owl:minQualifiedCardinality "0"^^xsd:nonNegativeInteger ;
                                             owl:onClass <https://w3id.org/netbeheer/IECCIM/TC57CIM/IEC61970/Base/Domain#Conductance>
                                           ] ,
                                           [ rdf:type owl:Restriction ;
                                             owl:onProperty :TransformerCoreAdmittance_g0 ;
                                             owl:minQualifiedCardinality "0"^^xsd:nonNegativeInteger ;
                                             owl:onClass <https://w3id.org/netbeheer/IECCIM/TC57CIM/IEC61970/Base/Domain#Conductance>
                                           ] ,
                                           [ rdf:type owl:Restriction ;
                                             owl:onProperty :TransformerCoreAdmittance_TransformerEnd ;
                                             owl:maxQualifiedCardinality "1"^^xsd:nonNegativeInteger ;
                                             owl:onClass :TransformerCoreAdmittance
                                           ] ,
                                           [ rdf:type owl:Restriction ;
                                             owl:onProperty :TransformerCoreAdmittance_TransformerEndInfo ;
                                             owl:maxQualifiedCardinality "1"^^xsd:nonNegativeInteger ;
                                             owl:onClass :TransformerCoreAdmittance
                                           ] ,
                                           [ rdf:type owl:Restriction ;
                                             owl:onProperty :TransformerCoreAdmittance_b ;
                                             owl:maxQualifiedCardinality "1"^^xsd:nonNegativeInteger ;
                                             owl:onClass <https://w3id.org/netbeheer/IECCIM/TC57CIM/IEC61970/Base/Domain#Susceptance>
                                           ] ,
                                           [ rdf:type owl:Restriction ;
                                             owl:onProperty :TransformerCoreAdmittance_b0 ;
                                             owl:maxQualifiedCardinality "1"^^xsd:nonNegativeInteger ;
                                             owl:onClass <https://w3id.org/netbeheer/IECCIM/TC57CIM/IEC61970/Base/Domain#Susceptance>
                                           ] ,
                                           [ rdf:type owl:Restriction ;
                                             owl:onProperty :TransformerCoreAdmittance_g ;
                                             owl:maxQualifiedCardinality "1"^^xsd:nonNegativeInteger ;
                                             owl:onClass <https://w3id.org/netbeheer/IECCIM/TC57CIM/IEC61970/Base/Domain#Conductance>
                                           ] ,
                                           [ rdf:type owl:Restriction ;
                                             owl:onProperty :TransformerCoreAdmittance_g0 ;
                                             owl:maxQualifiedCardinality "1"^^xsd:nonNegativeInteger ;
                                             owl:onClass <https://w3id.org/netbeheer/IECCIM/TC57CIM/IEC61970/Base/Domain#Conductance>
                                           ] ;
                           rdfs:comment """The transformer core admittance.  Used to specify the core admittance of a transformer in a manner that can be shared among power transformers.
""" .


###  https://w3id.org/netbeheer/IECCIM/TC57CIM/IEC61970/Base/Wires#TransformerEnd
:TransformerEnd rdf:type owl:Class ;
                rdfs:subClassOf <https://w3id.org/netbeheer/IECCIM/TC57CIM/IEC61970/Base/Core#IdentifiedObject> ,
                                [ rdf:type owl:Restriction ;
                                  owl:onProperty :TransformerEnd_CoreAdmittance ;
                                  owl:minQualifiedCardinality "0"^^xsd:nonNegativeInteger ;
                                  owl:onClass :TransformerEnd
                                ] ,
                                [ rdf:type owl:Restriction ;
                                  owl:onProperty :TransformerEnd_StarImpedance ;
                                  owl:minQualifiedCardinality "0"^^xsd:nonNegativeInteger ;
                                  owl:onClass :TransformerEnd
                                ] ,
                                [ rdf:type owl:Restriction ;
                                  owl:onProperty :TransformerEnd_ToMeshImpedance ;
                                  owl:minQualifiedCardinality "1"^^xsd:nonNegativeInteger ;
                                  owl:onClass :TransformerEnd
                                ] ,
                                [ rdf:type owl:Restriction ;
                                  owl:onProperty :TransformerEnd_bmagSat ;
                                  owl:minQualifiedCardinality "0"^^xsd:nonNegativeInteger ;
                                  owl:onClass <https://w3id.org/netbeheer/IECCIM/TC57CIM/IEC61970/Base/Domain#PerCent>
                                ] ,
                                [ rdf:type owl:Restriction ;
                                  owl:onProperty :TransformerEnd_magBaseU ;
                                  owl:minQualifiedCardinality "0"^^xsd:nonNegativeInteger ;
                                  owl:onClass <https://w3id.org/netbeheer/IECCIM/TC57CIM/IEC61970/Base/Domain#Voltage>
                                ] ,
                                [ rdf:type owl:Restriction ;
                                  owl:onProperty :TransformerEnd_magSatFlux ;
                                  owl:minQualifiedCardinality "0"^^xsd:nonNegativeInteger ;
                                  owl:onClass <https://w3id.org/netbeheer/IECCIM/TC57CIM/IEC61970/Base/Domain#PerCent>
                                ] ,
                                [ rdf:type owl:Restriction ;
                                  owl:onProperty :TransformerEnd_rground ;
                                  owl:minQualifiedCardinality "0"^^xsd:nonNegativeInteger ;
                                  owl:onClass <https://w3id.org/netbeheer/IECCIM/TC57CIM/IEC61970/Base/Domain#Resistance>
                                ] ,
                                [ rdf:type owl:Restriction ;
                                  owl:onProperty :TransformerEnd_xground ;
                                  owl:minQualifiedCardinality "0"^^xsd:nonNegativeInteger ;
                                  owl:onClass <https://w3id.org/netbeheer/IECCIM/TC57CIM/IEC61970/Base/Domain#Reactance>
                                ] ,
                                [ rdf:type owl:Restriction ;
                                  owl:onProperty :TransformerEnd_FromMeshImpedance ;
                                  owl:qualifiedCardinality "1"^^xsd:nonNegativeInteger ;
                                  owl:onClass :TransformerEnd
                                ] ,
                                [ rdf:type owl:Restriction ;
                                  owl:onProperty :TransformerEnd_FromWindingInsulations ;
                                  owl:qualifiedCardinality "1"^^xsd:nonNegativeInteger ;
                                  owl:onClass :TransformerEnd
                                ] ,
                                [ rdf:type owl:Restriction ;
                                  owl:onProperty :TransformerEnd_PhaseTapChanger ;
                                  owl:qualifiedCardinality "1"^^xsd:nonNegativeInteger ;
                                  owl:onClass :TransformerEnd
                                ] ,
                                [ rdf:type owl:Restriction ;
                                  owl:onProperty :TransformerEnd_RatioTapChanger ;
                                  owl:qualifiedCardinality "1"^^xsd:nonNegativeInteger ;
                                  owl:onClass :TransformerEnd
                                ] ,
                                [ rdf:type owl:Restriction ;
                                  owl:onProperty :TransformerEnd_ToWindingInsulations ;
                                  owl:qualifiedCardinality "1"^^xsd:nonNegativeInteger ;
                                  owl:onClass :TransformerEnd
                                ] ,
                                [ rdf:type owl:Restriction ;
                                  owl:onProperty :TransformerEnd_bmagSat ;
                                  owl:maxQualifiedCardinality "1"^^xsd:nonNegativeInteger ;
                                  owl:onClass <https://w3id.org/netbeheer/IECCIM/TC57CIM/IEC61970/Base/Domain#PerCent>
                                ] ,
                                [ rdf:type owl:Restriction ;
                                  owl:onProperty :TransformerEnd_magBaseU ;
                                  owl:maxQualifiedCardinality "1"^^xsd:nonNegativeInteger ;
                                  owl:onClass <https://w3id.org/netbeheer/IECCIM/TC57CIM/IEC61970/Base/Domain#Voltage>
                                ] ,
                                [ rdf:type owl:Restriction ;
                                  owl:onProperty :TransformerEnd_magSatFlux ;
                                  owl:maxQualifiedCardinality "1"^^xsd:nonNegativeInteger ;
                                  owl:onClass <https://w3id.org/netbeheer/IECCIM/TC57CIM/IEC61970/Base/Domain#PerCent>
                                ] ,
                                [ rdf:type owl:Restriction ;
                                  owl:onProperty :TransformerEnd_rground ;
                                  owl:maxQualifiedCardinality "1"^^xsd:nonNegativeInteger ;
                                  owl:onClass <https://w3id.org/netbeheer/IECCIM/TC57CIM/IEC61970/Base/Domain#Resistance>
                                ] ,
                                [ rdf:type owl:Restriction ;
                                  owl:onProperty :TransformerEnd_xground ;
                                  owl:maxQualifiedCardinality "1"^^xsd:nonNegativeInteger ;
                                  owl:onClass <https://w3id.org/netbeheer/IECCIM/TC57CIM/IEC61970/Base/Domain#Reactance>
                                ] ,
                                [ rdf:type owl:Restriction ;
                                  owl:onProperty :TransformerEnd_endNumber ;
                                  owl:minQualifiedCardinality "0"^^xsd:nonNegativeInteger ;
                                  owl:onDataRange xsd:nonNegativeInteger
                                ] ,
                                [ rdf:type owl:Restriction ;
                                  owl:onProperty :TransformerEnd_grounded ;
                                  owl:minQualifiedCardinality "0"^^xsd:nonNegativeInteger ;
                                  owl:onDataRange xsd:boolean
                                ] ,
                                [ rdf:type owl:Restriction ;
                                  owl:onProperty :TransformerEnd_endNumber ;
                                  owl:maxQualifiedCardinality "1"^^xsd:nonNegativeInteger ;
                                  owl:onDataRange xsd:nonNegativeInteger
                                ] ,
                                [ rdf:type owl:Restriction ;
                                  owl:onProperty :TransformerEnd_grounded ;
                                  owl:maxQualifiedCardinality "1"^^xsd:nonNegativeInteger ;
                                  owl:onDataRange xsd:boolean
                                ] ;
                rdfs:comment "A conducting connection point of a power transformer. It corresponds to a physical transformer winding terminal.  In earlier CIM versions, the TransformerWinding class served a similar purpose, but this class is more flexible because it associates to terminal but is not a specialization of ConductingEquipment." .


###  https://w3id.org/netbeheer/IECCIM/TC57CIM/IEC61970/Base/Wires#TransformerMeshImpedance
:TransformerMeshImpedance rdf:type owl:Class ;
                          rdfs:subClassOf <https://w3id.org/netbeheer/IECCIM/TC57CIM/IEC61970/Base/Core#IdentifiedObject> ,
                                          [ rdf:type owl:Restriction ;
                                            owl:onProperty :TransformerMeshImpedance_FromTransformerEnd ;
                                            owl:minQualifiedCardinality "0"^^xsd:nonNegativeInteger ;
                                            owl:onClass :TransformerMeshImpedance
                                          ] ,
                                          [ rdf:type owl:Restriction ;
                                            owl:onProperty :TransformerMeshImpedance_FromTransformerEndInfo ;
                                            owl:minQualifiedCardinality "0"^^xsd:nonNegativeInteger ;
                                            owl:onClass :TransformerMeshImpedance
                                          ] ,
                                          [ rdf:type owl:Restriction ;
                                            owl:onProperty :TransformerMeshImpedance_ToTransformerEnd ;
                                            owl:minQualifiedCardinality "0"^^xsd:nonNegativeInteger ;
                                            owl:onClass :TransformerMeshImpedance
                                          ] ,
                                          [ rdf:type owl:Restriction ;
                                            owl:onProperty :TransformerMeshImpedance_ToTransformerEndInfos ;
                                            owl:minQualifiedCardinality "0"^^xsd:nonNegativeInteger ;
                                            owl:onClass :TransformerMeshImpedance
                                          ] ,
                                          [ rdf:type owl:Restriction ;
                                            owl:onProperty :TransformerMeshImpedance_r ;
                                            owl:minQualifiedCardinality "0"^^xsd:nonNegativeInteger ;
                                            owl:onClass <https://w3id.org/netbeheer/IECCIM/TC57CIM/IEC61970/Base/Domain#Resistance>
                                          ] ,
                                          [ rdf:type owl:Restriction ;
                                            owl:onProperty :TransformerMeshImpedance_r0 ;
                                            owl:minQualifiedCardinality "0"^^xsd:nonNegativeInteger ;
                                            owl:onClass <https://w3id.org/netbeheer/IECCIM/TC57CIM/IEC61970/Base/Domain#Resistance>
                                          ] ,
                                          [ rdf:type owl:Restriction ;
                                            owl:onProperty :TransformerMeshImpedance_x ;
                                            owl:minQualifiedCardinality "0"^^xsd:nonNegativeInteger ;
                                            owl:onClass <https://w3id.org/netbeheer/IECCIM/TC57CIM/IEC61970/Base/Domain#Reactance>
                                          ] ,
                                          [ rdf:type owl:Restriction ;
                                            owl:onProperty :TransformerMeshImpedance_x0 ;
                                            owl:minQualifiedCardinality "0"^^xsd:nonNegativeInteger ;
                                            owl:onClass <https://w3id.org/netbeheer/IECCIM/TC57CIM/IEC61970/Base/Domain#Reactance>
                                          ] ,
                                          [ rdf:type owl:Restriction ;
                                            owl:onProperty :TransformerMeshImpedance_r ;
                                            owl:maxQualifiedCardinality "1"^^xsd:nonNegativeInteger ;
                                            owl:onClass <https://w3id.org/netbeheer/IECCIM/TC57CIM/IEC61970/Base/Domain#Resistance>
                                          ] ,
                                          [ rdf:type owl:Restriction ;
                                            owl:onProperty :TransformerMeshImpedance_r0 ;
                                            owl:maxQualifiedCardinality "1"^^xsd:nonNegativeInteger ;
                                            owl:onClass <https://w3id.org/netbeheer/IECCIM/TC57CIM/IEC61970/Base/Domain#Resistance>
                                          ] ,
                                          [ rdf:type owl:Restriction ;
                                            owl:onProperty :TransformerMeshImpedance_x ;
                                            owl:maxQualifiedCardinality "1"^^xsd:nonNegativeInteger ;
                                            owl:onClass <https://w3id.org/netbeheer/IECCIM/TC57CIM/IEC61970/Base/Domain#Reactance>
                                          ] ,
                                          [ rdf:type owl:Restriction ;
                                            owl:onProperty :TransformerMeshImpedance_x0 ;
                                            owl:maxQualifiedCardinality "1"^^xsd:nonNegativeInteger ;
                                            owl:onClass <https://w3id.org/netbeheer/IECCIM/TC57CIM/IEC61970/Base/Domain#Reactance>
                                          ] ;
                          rdfs:comment """Transformer mesh impedance (Delta-model) between transformer ends.
The typical case is that this class describes the impedance between two transformer ends pair-wise, i.e. the cardinalities at both tranformer end associations are 1. But in cases where two or more transformer ends are modeled the cardinalities are larger than 1.
""" .


###  https://w3id.org/netbeheer/IECCIM/TC57CIM/IEC61970/Base/Wires#TransformerStarImpedance
:TransformerStarImpedance rdf:type owl:Class ;
                          rdfs:subClassOf <https://w3id.org/netbeheer/IECCIM/TC57CIM/IEC61970/Base/Core#IdentifiedObject> ,
                                          [ rdf:type owl:Restriction ;
                                            owl:onProperty :TransformerStarImpedance_TransformerEnd ;
                                            owl:minQualifiedCardinality "0"^^xsd:nonNegativeInteger ;
                                            owl:onClass :TransformerStarImpedance
                                          ] ,
                                          [ rdf:type owl:Restriction ;
                                            owl:onProperty :TransformerStarImpedance_TransformerEndInfo ;
                                            owl:minQualifiedCardinality "0"^^xsd:nonNegativeInteger ;
                                            owl:onClass :TransformerStarImpedance
                                          ] ,
                                          [ rdf:type owl:Restriction ;
                                            owl:onProperty :TransformerStarImpedance_r ;
                                            owl:minQualifiedCardinality "0"^^xsd:nonNegativeInteger ;
                                            owl:onClass <https://w3id.org/netbeheer/IECCIM/TC57CIM/IEC61970/Base/Domain#Resistance>
                                          ] ,
                                          [ rdf:type owl:Restriction ;
                                            owl:onProperty :TransformerStarImpedance_r0 ;
                                            owl:minQualifiedCardinality "0"^^xsd:nonNegativeInteger ;
                                            owl:onClass <https://w3id.org/netbeheer/IECCIM/TC57CIM/IEC61970/Base/Domain#Resistance>
                                          ] ,
                                          [ rdf:type owl:Restriction ;
                                            owl:onProperty :TransformerStarImpedance_x ;
                                            owl:minQualifiedCardinality "0"^^xsd:nonNegativeInteger ;
                                            owl:onClass <https://w3id.org/netbeheer/IECCIM/TC57CIM/IEC61970/Base/Domain#Reactance>
                                          ] ,
                                          [ rdf:type owl:Restriction ;
                                            owl:onProperty :TransformerStarImpedance_x0 ;
                                            owl:minQualifiedCardinality "0"^^xsd:nonNegativeInteger ;
                                            owl:onClass <https://w3id.org/netbeheer/IECCIM/TC57CIM/IEC61970/Base/Domain#Reactance>
                                          ] ,
                                          [ rdf:type owl:Restriction ;
                                            owl:onProperty :TransformerStarImpedance_TransformerEnd ;
                                            owl:maxQualifiedCardinality "1"^^xsd:nonNegativeInteger ;
                                            owl:onClass :TransformerStarImpedance
                                          ] ,
                                          [ rdf:type owl:Restriction ;
                                            owl:onProperty :TransformerStarImpedance_TransformerEndInfo ;
                                            owl:maxQualifiedCardinality "1"^^xsd:nonNegativeInteger ;
                                            owl:onClass :TransformerStarImpedance
                                          ] ,
                                          [ rdf:type owl:Restriction ;
                                            owl:onProperty :TransformerStarImpedance_r ;
                                            owl:maxQualifiedCardinality "1"^^xsd:nonNegativeInteger ;
                                            owl:onClass <https://w3id.org/netbeheer/IECCIM/TC57CIM/IEC61970/Base/Domain#Resistance>
                                          ] ,
                                          [ rdf:type owl:Restriction ;
                                            owl:onProperty :TransformerStarImpedance_r0 ;
                                            owl:maxQualifiedCardinality "1"^^xsd:nonNegativeInteger ;
                                            owl:onClass <https://w3id.org/netbeheer/IECCIM/TC57CIM/IEC61970/Base/Domain#Resistance>
                                          ] ,
                                          [ rdf:type owl:Restriction ;
                                            owl:onProperty :TransformerStarImpedance_x ;
                                            owl:maxQualifiedCardinality "1"^^xsd:nonNegativeInteger ;
                                            owl:onClass <https://w3id.org/netbeheer/IECCIM/TC57CIM/IEC61970/Base/Domain#Reactance>
                                          ] ,
                                          [ rdf:type owl:Restriction ;
                                            owl:onProperty :TransformerStarImpedance_x0 ;
                                            owl:maxQualifiedCardinality "1"^^xsd:nonNegativeInteger ;
                                            owl:onClass <https://w3id.org/netbeheer/IECCIM/TC57CIM/IEC61970/Base/Domain#Reactance>
                                          ] ;
                          rdfs:comment """Transformer star impedance (Pi-model) that accurately reflects impedance for transformers with 2 or 3 windings. For transformers with 4 or more windings, you must use TransformerMeshImpedance class.
For transmission networks use PowerTransformerEnd impedances (r, r0, x, x0, b, b0, g and g0).
""" .


###  https://w3id.org/netbeheer/IECCIM/TC57CIM/IEC61970/Base/Wires#TransformerTank
:TransformerTank rdf:type owl:Class ;
                 rdfs:subClassOf <https://w3id.org/netbeheer/IECCIM/TC57CIM/IEC61970/Base/Core#Equipment> ,
                                 [ rdf:type owl:Restriction ;
                                   owl:onProperty :TransformerTank_PowerTransformer ;
                                   owl:minQualifiedCardinality "0"^^xsd:nonNegativeInteger ;
                                   owl:onClass :TransformerTank
                                 ] ,
                                 [ rdf:type owl:Restriction ;
                                   owl:onProperty :TransformerTank_TransformerObservations ;
                                   owl:minQualifiedCardinality "0"^^xsd:nonNegativeInteger ;
                                   owl:onClass :TransformerTank
                                 ] ,
                                 [ rdf:type owl:Restriction ;
                                   owl:onProperty :TransformerTank_TransformerTankEnds ;
                                   owl:minQualifiedCardinality "0"^^xsd:nonNegativeInteger ;
                                   owl:onClass :TransformerTank
                                 ] ,
                                 [ rdf:type owl:Restriction ;
                                   owl:onProperty :TransformerTank_TransformerObservations ;
                                   owl:maxQualifiedCardinality "1"^^xsd:nonNegativeInteger ;
                                   owl:onClass :TransformerTank
                                 ] ,
                                 [ rdf:type owl:Restriction ;
                                   owl:onProperty :TransformerTank_TransformerTankEnds ;
                                   owl:maxQualifiedCardinality "1"^^xsd:nonNegativeInteger ;
                                   owl:onClass :TransformerTank
                                 ] ;
                 rdfs:comment """An assembly of two or more coupled windings that transform electrical power between voltage levels. These windings are bound on a common core and place in the same tank. Transformer tank can be used to model both single-phase and 3-phase transformers.
""" .


###  https://w3id.org/netbeheer/IECCIM/TC57CIM/IEC61970/Base/Wires#TransformerTankEnd
:TransformerTankEnd rdf:type owl:Class ;
                    rdfs:subClassOf :TransformerEnd ,
                                    [ rdf:type owl:Restriction ;
                                      owl:onProperty :TransformerTankEnd_TransformerTank ;
                                      owl:minQualifiedCardinality "1"^^xsd:nonNegativeInteger ;
                                      owl:onClass :TransformerTankEnd
                                    ] ,
                                    [ rdf:type owl:Restriction ;
                                      owl:onProperty :TransformerTankEnd_phases ;
                                      owl:minQualifiedCardinality "0"^^xsd:nonNegativeInteger ;
                                      owl:onDataRange <https://w3id.org/netbeheer/IECCIM/TC57CIM/IEC61970/Base/Core#PhaseCode>
                                    ] ,
                                    [ rdf:type owl:Restriction ;
                                      owl:onProperty :TransformerTankEnd_phases ;
                                      owl:maxQualifiedCardinality "1"^^xsd:nonNegativeInteger ;
                                      owl:onDataRange <https://w3id.org/netbeheer/IECCIM/TC57CIM/IEC61970/Base/Core#PhaseCode>
                                    ] ;
                    rdfs:comment """Transformer tank end represents an individual winding for unbalanced models or for transformer tanks connected into a bank (and bank is modelled with the PowerTransformer).
""" .


###  https://w3id.org/netbeheer/IECCIM/TC57CIM/IEC61970/Base/Wires#VoltageControlZone
:VoltageControlZone rdf:type owl:Class ;
                    rdfs:subClassOf <https://w3id.org/netbeheer/IECCIM/TC57CIM/IEC61970/Base/Core#PowerSystemResource> ,
                                    [ rdf:type owl:Restriction ;
                                      owl:onProperty :VoltageControlZone_BusbarSection ;
                                      owl:minQualifiedCardinality "0"^^xsd:nonNegativeInteger ;
                                      owl:onClass :VoltageControlZone
                                    ] ,
                                    [ rdf:type owl:Restriction ;
                                      owl:onProperty :VoltageControlZone_RegulationSchedule ;
                                      owl:minQualifiedCardinality "0"^^xsd:nonNegativeInteger ;
                                      owl:onClass :VoltageControlZone
                                    ] ,
                                    [ rdf:type owl:Restriction ;
                                      owl:onProperty :VoltageControlZone_BusbarSection ;
                                      owl:maxQualifiedCardinality "1"^^xsd:nonNegativeInteger ;
                                      owl:onClass :VoltageControlZone
                                    ] ;
                    rdfs:comment "An area of the power system network which is defined for secondary voltage control purposes. A voltage control zone consists of a collection of substations with a designated bus bar section whose voltage will be controlled." .


###  https://w3id.org/netbeheer/IECCIM/TC57CIM/IEC61970/Dynamics/StandardModels/AsynchronousMachineDynamics#AsynchronousMachineDynamics
<https://w3id.org/netbeheer/IECCIM/TC57CIM/IEC61970/Dynamics/StandardModels/AsynchronousMachineDynamics#AsynchronousMachineDynamics> rdf:type owl:Class ;
                                                                                                                                     rdfs:subClassOf [ rdf:type owl:Restriction ;
                                                                                                                                                       owl:onProperty :AsynchronousMachineDynamics_AsynchronousMachine ;
                                                                                                                                                       owl:minQualifiedCardinality "0"^^xsd:nonNegativeInteger ;
                                                                                                                                                       owl:onClass <https://w3id.org/netbeheer/IECCIM/TC57CIM/IEC61970/Dynamics/StandardModels/AsynchronousMachineDynamics#AsynchronousMachineDynamics>
                                                                                                                                                     ] ,
                                                                                                                                                     [ rdf:type owl:Restriction ;
                                                                                                                                                       owl:onProperty :AsynchronousMachineDynamics_AsynchronousMachine ;
                                                                                                                                                       owl:maxQualifiedCardinality "1"^^xsd:nonNegativeInteger ;
                                                                                                                                                       owl:onClass <https://w3id.org/netbeheer/IECCIM/TC57CIM/IEC61970/Dynamics/StandardModels/AsynchronousMachineDynamics#AsynchronousMachineDynamics>
                                                                                                                                                     ] .


###  https://w3id.org/netbeheer/IECCIM/TC57CIM/IEC61970/Dynamics/StandardModels/LoadDynamics#LoadDynamics
<https://w3id.org/netbeheer/IECCIM/TC57CIM/IEC61970/Dynamics/StandardModels/LoadDynamics#LoadDynamics> rdf:type owl:Class ;
                                                                                                       rdfs:subClassOf [ rdf:type owl:Restriction ;
                                                                                                                         owl:onProperty :LoadDynamics_EnergyConsumer ;
                                                                                                                         owl:minQualifiedCardinality "0"^^xsd:nonNegativeInteger ;
                                                                                                                         owl:onClass <https://w3id.org/netbeheer/IECCIM/TC57CIM/IEC61970/Dynamics/StandardModels/LoadDynamics#LoadDynamics>
                                                                                                                       ] ,
                                                                                                                       [ rdf:type owl:Restriction ;
                                                                                                                         owl:onProperty :LoadDynamics_EnergyConsumer ;
                                                                                                                         owl:maxQualifiedCardinality "1"^^xsd:nonNegativeInteger ;
                                                                                                                         owl:onClass <https://w3id.org/netbeheer/IECCIM/TC57CIM/IEC61970/Dynamics/StandardModels/LoadDynamics#LoadDynamics>
                                                                                                                       ] .


###  https://w3id.org/netbeheer/IECCIM/TC57CIM/IEC61970/Dynamics/StandardModels/SynchronousMachineDynamics#SynchronousMachineDynamics
<https://w3id.org/netbeheer/IECCIM/TC57CIM/IEC61970/Dynamics/StandardModels/SynchronousMachineDynamics#SynchronousMachineDynamics> rdf:type owl:Class ;
                                                                                                                                   rdfs:subClassOf [ rdf:type owl:Restriction ;
                                                                                                                                                     owl:onProperty :SynchronousMachineDynamics_SynchronousMachine ;
                                                                                                                                                     owl:minQualifiedCardinality "0"^^xsd:nonNegativeInteger ;
                                                                                                                                                     owl:onClass <https://w3id.org/netbeheer/IECCIM/TC57CIM/IEC61970/Dynamics/StandardModels/SynchronousMachineDynamics#SynchronousMachineDynamics>
                                                                                                                                                   ] ,
                                                                                                                                                   [ rdf:type owl:Restriction ;
                                                                                                                                                     owl:onProperty :SynchronousMachineDynamics_SynchronousMachine ;
                                                                                                                                                     owl:maxQualifiedCardinality "1"^^xsd:nonNegativeInteger ;
                                                                                                                                                     owl:onClass <https://w3id.org/netbeheer/IECCIM/TC57CIM/IEC61970/Dynamics/StandardModels/SynchronousMachineDynamics#SynchronousMachineDynamics>
                                                                                                                                                   ] .


###  https://w3id.org/netbeheer/IECCIM/TC57CIM/IEC61970/Dynamics/StandardModels/WindDynamics#WindTurbineType3or4Dynamics
<https://w3id.org/netbeheer/IECCIM/TC57CIM/IEC61970/Dynamics/StandardModels/WindDynamics#WindTurbineType3or4Dynamics> rdf:type owl:Class ;
                                                                                                                      rdfs:subClassOf [ rdf:type owl:Restriction ;
                                                                                                                                        owl:onProperty :WindTurbineType3or4Dynamics_EnergySource ;
                                                                                                                                        owl:minQualifiedCardinality "0"^^xsd:nonNegativeInteger ;
                                                                                                                                        owl:onClass <https://w3id.org/netbeheer/IECCIM/TC57CIM/IEC61970/Dynamics/StandardModels/WindDynamics#WindTurbineType3or4Dynamics>
                                                                                                                                      ] ,
                                                                                                                                      [ rdf:type owl:Restriction ;
                                                                                                                                        owl:onProperty :WindTurbineType3or4Dynamics_EnergySource ;
                                                                                                                                        owl:maxQualifiedCardinality "1"^^xsd:nonNegativeInteger ;
                                                                                                                                        owl:onClass <https://w3id.org/netbeheer/IECCIM/TC57CIM/IEC61970/Dynamics/StandardModels/WindDynamics#WindTurbineType3or4Dynamics>
                                                                                                                                      ] .


###  https://w3id.org/netbeheer/IECCIM/TC57CIM/IEC61970/InfIEC61970/InfEnergySource#EnergySchedulingType
<https://w3id.org/netbeheer/IECCIM/TC57CIM/IEC61970/InfIEC61970/InfEnergySource#EnergySchedulingType> rdf:type owl:Class ;
                                                                                                      rdfs:subClassOf [ rdf:type owl:Restriction ;
                                                                                                                        owl:onProperty :EnergySchedulingType_EnergySource ;
                                                                                                                        owl:minQualifiedCardinality "0"^^xsd:nonNegativeInteger ;
                                                                                                                        owl:onClass <https://w3id.org/netbeheer/IECCIM/TC57CIM/IEC61970/InfIEC61970/InfEnergySource#EnergySchedulingType>
                                                                                                                      ] ,
                                                                                                                      [ rdf:type owl:Restriction ;
                                                                                                                        owl:onProperty :EnergySchedulingType_EnergySource ;
                                                                                                                        owl:maxQualifiedCardinality "1"^^xsd:nonNegativeInteger ;
                                                                                                                        owl:onClass <https://w3id.org/netbeheer/IECCIM/TC57CIM/IEC61970/InfIEC61970/InfEnergySource#EnergySchedulingType>
                                                                                                                      ] .


###  https://w3id.org/netbeheer/IECCIM/TC57CIM/IEC61970/InfIEC61970/InfSIPS#ProtectiveActionRegulation
<https://w3id.org/netbeheer/IECCIM/TC57CIM/IEC61970/InfIEC61970/InfSIPS#ProtectiveActionRegulation> rdf:type owl:Class ;
                                                                                                    rdfs:subClassOf [ rdf:type owl:Restriction ;
                                                                                                                      owl:onProperty :ProtectiveActionRegulation_RegulatingControl ;
                                                                                                                      owl:minQualifiedCardinality "0"^^xsd:nonNegativeInteger ;
                                                                                                                      owl:onClass <https://w3id.org/netbeheer/IECCIM/TC57CIM/IEC61970/InfIEC61970/InfSIPS#ProtectiveActionRegulation>
                                                                                                                    ] .


###  Generated by the OWL API (version 5.1.10.2019-03-12T22:31:15Z) https://github.com/owlcs/owlapi/
