<?xml version="1.0"?>
<rdf:RDF xmlns="https://w3id.org/netbeheer/referentiemodellen/IECCIM/TC57CIM/IEC61970/Base/Wires#"
     xml:base="https://w3id.org/netbeheer/referentiemodellen/IECCIM/TC57CIM/IEC61970/Base/Wires"
     xmlns:owl="http://www.w3.org/2002/07/owl#"
     xmlns:rdf="http://www.w3.org/1999/02/22-rdf-syntax-ns#"
     xmlns:xml="http://www.w3.org/XML/1998/namespace"
     xmlns:xsd="http://www.w3.org/2001/XMLSchema#"
     xmlns:rdfs="http://www.w3.org/2000/01/rdf-schema#">
    <owl:Ontology rdf:about="https://w3id.org/netbeheer/referentiemodellen/IECCIM/TC57CIM/IEC61970/Base/Wires#"/>
    


    <!-- 
    ///////////////////////////////////////////////////////////////////////////////////////
    //
    // Datatypes
    //
    ///////////////////////////////////////////////////////////////////////////////////////
     -->


    


    <!-- https://w3id.org/netbeheer/referentiemodellen/IECCIM/TC57CIM/IEC61970/Base/Core#PhaseCode -->


    <rdfs:Datatype rdf:about="https://w3id.org/netbeheer/referentiemodellen/IECCIM/TC57CIM/IEC61970/Base/Core#PhaseCode"/>
    


    <!-- https://w3id.org/netbeheer/referentiemodellen/IECCIM/TC57CIM/IEC61970/Base/Domain#UnitMultiplier -->


    <rdfs:Datatype rdf:about="https://w3id.org/netbeheer/referentiemodellen/IECCIM/TC57CIM/IEC61970/Base/Domain#UnitMultiplier"/>
    


    <!-- https://w3id.org/netbeheer/referentiemodellen/IECCIM/TC57CIM/IEC61970/Base/Wires#AsynchronousMachineKind -->


    <rdfs:Datatype rdf:about="https://w3id.org/netbeheer/referentiemodellen/IECCIM/TC57CIM/IEC61970/Base/Wires#AsynchronousMachineKind">
        <owl:equivalentClass>
            <rdfs:Datatype>
                <owl:oneOf>
                    <rdf:Description>
                        <rdf:type rdf:resource="http://www.w3.org/1999/02/22-rdf-syntax-ns#List"/>
                        <rdf:first>generator</rdf:first>
                        <rdf:rest>
                            <rdf:Description>
                                <rdf:type rdf:resource="http://www.w3.org/1999/02/22-rdf-syntax-ns#List"/>
                                <rdf:first>motor</rdf:first>
                                <rdf:rest rdf:resource="http://www.w3.org/1999/02/22-rdf-syntax-ns#nil"/>
                            </rdf:Description>
                        </rdf:rest>
                    </rdf:Description>
                </owl:oneOf>
            </rdfs:Datatype>
        </owl:equivalentClass>
    </rdfs:Datatype>
    


    <!-- https://w3id.org/netbeheer/referentiemodellen/IECCIM/TC57CIM/IEC61970/Base/Wires#CoolantType -->


    <rdfs:Datatype rdf:about="https://w3id.org/netbeheer/referentiemodellen/IECCIM/TC57CIM/IEC61970/Base/Wires#CoolantType">
        <owl:equivalentClass>
            <rdfs:Datatype>
                <owl:oneOf>
                    <rdf:Description>
                        <rdf:type rdf:resource="http://www.w3.org/1999/02/22-rdf-syntax-ns#List"/>
                        <rdf:first>air</rdf:first>
                        <rdf:rest>
                            <rdf:Description>
                                <rdf:type rdf:resource="http://www.w3.org/1999/02/22-rdf-syntax-ns#List"/>
                                <rdf:first>hydrogenGas</rdf:first>
                                <rdf:rest>
                                    <rdf:Description>
                                        <rdf:type rdf:resource="http://www.w3.org/1999/02/22-rdf-syntax-ns#List"/>
                                        <rdf:first>water</rdf:first>
                                        <rdf:rest rdf:resource="http://www.w3.org/1999/02/22-rdf-syntax-ns#nil"/>
                                    </rdf:Description>
                                </rdf:rest>
                            </rdf:Description>
                        </rdf:rest>
                    </rdf:Description>
                </owl:oneOf>
            </rdfs:Datatype>
        </owl:equivalentClass>
    </rdfs:Datatype>
    


    <!-- https://w3id.org/netbeheer/referentiemodellen/IECCIM/TC57CIM/IEC61970/Base/Wires#PetersenCoilModeKind -->


    <rdfs:Datatype rdf:about="https://w3id.org/netbeheer/referentiemodellen/IECCIM/TC57CIM/IEC61970/Base/Wires#PetersenCoilModeKind">
        <owl:equivalentClass>
            <rdfs:Datatype>
                <owl:oneOf>
                    <rdf:Description>
                        <rdf:type rdf:resource="http://www.w3.org/1999/02/22-rdf-syntax-ns#List"/>
                        <rdf:first>automaticPositioning</rdf:first>
                        <rdf:rest>
                            <rdf:Description>
                                <rdf:type rdf:resource="http://www.w3.org/1999/02/22-rdf-syntax-ns#List"/>
                                <rdf:first>fixed</rdf:first>
                                <rdf:rest>
                                    <rdf:Description>
                                        <rdf:type rdf:resource="http://www.w3.org/1999/02/22-rdf-syntax-ns#List"/>
                                        <rdf:first>manual</rdf:first>
                                        <rdf:rest rdf:resource="http://www.w3.org/1999/02/22-rdf-syntax-ns#nil"/>
                                    </rdf:Description>
                                </rdf:rest>
                            </rdf:Description>
                        </rdf:rest>
                    </rdf:Description>
                </owl:oneOf>
            </rdfs:Datatype>
        </owl:equivalentClass>
    </rdfs:Datatype>
    


    <!-- https://w3id.org/netbeheer/referentiemodellen/IECCIM/TC57CIM/IEC61970/Base/Wires#PhaseShuntConnectionKind -->


    <rdfs:Datatype rdf:about="https://w3id.org/netbeheer/referentiemodellen/IECCIM/TC57CIM/IEC61970/Base/Wires#PhaseShuntConnectionKind">
        <owl:equivalentClass>
            <rdfs:Datatype>
                <owl:oneOf>
                    <rdf:Description>
                        <rdf:type rdf:resource="http://www.w3.org/1999/02/22-rdf-syntax-ns#List"/>
                        <rdf:first>D</rdf:first>
                        <rdf:rest>
                            <rdf:Description>
                                <rdf:type rdf:resource="http://www.w3.org/1999/02/22-rdf-syntax-ns#List"/>
                                <rdf:first>G</rdf:first>
                                <rdf:rest>
                                    <rdf:Description>
                                        <rdf:type rdf:resource="http://www.w3.org/1999/02/22-rdf-syntax-ns#List"/>
                                        <rdf:first>I</rdf:first>
                                        <rdf:rest>
                                            <rdf:Description>
                                                <rdf:type rdf:resource="http://www.w3.org/1999/02/22-rdf-syntax-ns#List"/>
                                                <rdf:first>Y</rdf:first>
                                                <rdf:rest>
                                                    <rdf:Description>
                                                        <rdf:type rdf:resource="http://www.w3.org/1999/02/22-rdf-syntax-ns#List"/>
                                                        <rdf:first>Yn</rdf:first>
                                                        <rdf:rest rdf:resource="http://www.w3.org/1999/02/22-rdf-syntax-ns#nil"/>
                                                    </rdf:Description>
                                                </rdf:rest>
                                            </rdf:Description>
                                        </rdf:rest>
                                    </rdf:Description>
                                </rdf:rest>
                            </rdf:Description>
                        </rdf:rest>
                    </rdf:Description>
                </owl:oneOf>
            </rdfs:Datatype>
        </owl:equivalentClass>
    </rdfs:Datatype>
    


    <!-- https://w3id.org/netbeheer/referentiemodellen/IECCIM/TC57CIM/IEC61970/Base/Wires#RegulatingControlModeKind -->


    <rdfs:Datatype rdf:about="https://w3id.org/netbeheer/referentiemodellen/IECCIM/TC57CIM/IEC61970/Base/Wires#RegulatingControlModeKind">
        <owl:equivalentClass>
            <rdfs:Datatype>
                <owl:oneOf>
                    <rdf:Description>
                        <rdf:type rdf:resource="http://www.w3.org/1999/02/22-rdf-syntax-ns#List"/>
                        <rdf:first>activePower</rdf:first>
                        <rdf:rest>
                            <rdf:Description>
                                <rdf:type rdf:resource="http://www.w3.org/1999/02/22-rdf-syntax-ns#List"/>
                                <rdf:first>admittance</rdf:first>
                                <rdf:rest>
                                    <rdf:Description>
                                        <rdf:type rdf:resource="http://www.w3.org/1999/02/22-rdf-syntax-ns#List"/>
                                        <rdf:first>currentFlow</rdf:first>
                                        <rdf:rest>
                                            <rdf:Description>
                                                <rdf:type rdf:resource="http://www.w3.org/1999/02/22-rdf-syntax-ns#List"/>
                                                <rdf:first>powerFactor</rdf:first>
                                                <rdf:rest>
                                                    <rdf:Description>
                                                        <rdf:type rdf:resource="http://www.w3.org/1999/02/22-rdf-syntax-ns#List"/>
                                                        <rdf:first>reactivePower</rdf:first>
                                                        <rdf:rest>
                                                            <rdf:Description>
                                                                <rdf:type rdf:resource="http://www.w3.org/1999/02/22-rdf-syntax-ns#List"/>
                                                                <rdf:first>temperature</rdf:first>
                                                                <rdf:rest>
                                                                    <rdf:Description>
                                                                        <rdf:type rdf:resource="http://www.w3.org/1999/02/22-rdf-syntax-ns#List"/>
                                                                        <rdf:first>timeScheduled</rdf:first>
                                                                        <rdf:rest>
                                                                            <rdf:Description>
                                                                                <rdf:type rdf:resource="http://www.w3.org/1999/02/22-rdf-syntax-ns#List"/>
                                                                                <rdf:first>voltage</rdf:first>
                                                                                <rdf:rest rdf:resource="http://www.w3.org/1999/02/22-rdf-syntax-ns#nil"/>
                                                                            </rdf:Description>
                                                                        </rdf:rest>
                                                                    </rdf:Description>
                                                                </rdf:rest>
                                                            </rdf:Description>
                                                        </rdf:rest>
                                                    </rdf:Description>
                                                </rdf:rest>
                                            </rdf:Description>
                                        </rdf:rest>
                                    </rdf:Description>
                                </rdf:rest>
                            </rdf:Description>
                        </rdf:rest>
                    </rdf:Description>
                </owl:oneOf>
            </rdfs:Datatype>
        </owl:equivalentClass>
    </rdfs:Datatype>
    


    <!-- https://w3id.org/netbeheer/referentiemodellen/IECCIM/TC57CIM/IEC61970/Base/Wires#SVCControlMode -->


    <rdfs:Datatype rdf:about="https://w3id.org/netbeheer/referentiemodellen/IECCIM/TC57CIM/IEC61970/Base/Wires#SVCControlMode">
        <owl:equivalentClass>
            <rdfs:Datatype>
                <owl:oneOf>
                    <rdf:Description>
                        <rdf:type rdf:resource="http://www.w3.org/1999/02/22-rdf-syntax-ns#List"/>
                        <rdf:first>reactivePower</rdf:first>
                        <rdf:rest>
                            <rdf:Description>
                                <rdf:type rdf:resource="http://www.w3.org/1999/02/22-rdf-syntax-ns#List"/>
                                <rdf:first>voltage</rdf:first>
                                <rdf:rest rdf:resource="http://www.w3.org/1999/02/22-rdf-syntax-ns#nil"/>
                            </rdf:Description>
                        </rdf:rest>
                    </rdf:Description>
                </owl:oneOf>
            </rdfs:Datatype>
        </owl:equivalentClass>
    </rdfs:Datatype>
    


    <!-- https://w3id.org/netbeheer/referentiemodellen/IECCIM/TC57CIM/IEC61970/Base/Wires#ShortCircuitRotorKind -->


    <rdfs:Datatype rdf:about="https://w3id.org/netbeheer/referentiemodellen/IECCIM/TC57CIM/IEC61970/Base/Wires#ShortCircuitRotorKind">
        <owl:equivalentClass>
            <rdfs:Datatype>
                <owl:oneOf>
                    <rdf:Description>
                        <rdf:type rdf:resource="http://www.w3.org/1999/02/22-rdf-syntax-ns#List"/>
                        <rdf:first>salientPole1</rdf:first>
                        <rdf:rest>
                            <rdf:Description>
                                <rdf:type rdf:resource="http://www.w3.org/1999/02/22-rdf-syntax-ns#List"/>
                                <rdf:first>salientPole2</rdf:first>
                                <rdf:rest>
                                    <rdf:Description>
                                        <rdf:type rdf:resource="http://www.w3.org/1999/02/22-rdf-syntax-ns#List"/>
                                        <rdf:first>turboSeries1</rdf:first>
                                        <rdf:rest>
                                            <rdf:Description>
                                                <rdf:type rdf:resource="http://www.w3.org/1999/02/22-rdf-syntax-ns#List"/>
                                                <rdf:first>turboSeries2</rdf:first>
                                                <rdf:rest rdf:resource="http://www.w3.org/1999/02/22-rdf-syntax-ns#nil"/>
                                            </rdf:Description>
                                        </rdf:rest>
                                    </rdf:Description>
                                </rdf:rest>
                            </rdf:Description>
                        </rdf:rest>
                    </rdf:Description>
                </owl:oneOf>
            </rdfs:Datatype>
        </owl:equivalentClass>
    </rdfs:Datatype>
    


    <!-- https://w3id.org/netbeheer/referentiemodellen/IECCIM/TC57CIM/IEC61970/Base/Wires#SinglePhaseKind -->


    <rdfs:Datatype rdf:about="https://w3id.org/netbeheer/referentiemodellen/IECCIM/TC57CIM/IEC61970/Base/Wires#SinglePhaseKind">
        <owl:equivalentClass>
            <rdfs:Datatype>
                <owl:oneOf>
                    <rdf:Description>
                        <rdf:type rdf:resource="http://www.w3.org/1999/02/22-rdf-syntax-ns#List"/>
                        <rdf:first>A</rdf:first>
                        <rdf:rest>
                            <rdf:Description>
                                <rdf:type rdf:resource="http://www.w3.org/1999/02/22-rdf-syntax-ns#List"/>
                                <rdf:first>B</rdf:first>
                                <rdf:rest>
                                    <rdf:Description>
                                        <rdf:type rdf:resource="http://www.w3.org/1999/02/22-rdf-syntax-ns#List"/>
                                        <rdf:first>C</rdf:first>
                                        <rdf:rest>
                                            <rdf:Description>
                                                <rdf:type rdf:resource="http://www.w3.org/1999/02/22-rdf-syntax-ns#List"/>
                                                <rdf:first>N</rdf:first>
                                                <rdf:rest>
                                                    <rdf:Description>
                                                        <rdf:type rdf:resource="http://www.w3.org/1999/02/22-rdf-syntax-ns#List"/>
                                                        <rdf:first>s1</rdf:first>
                                                        <rdf:rest>
                                                            <rdf:Description>
                                                                <rdf:type rdf:resource="http://www.w3.org/1999/02/22-rdf-syntax-ns#List"/>
                                                                <rdf:first>s2</rdf:first>
                                                                <rdf:rest rdf:resource="http://www.w3.org/1999/02/22-rdf-syntax-ns#nil"/>
                                                            </rdf:Description>
                                                        </rdf:rest>
                                                    </rdf:Description>
                                                </rdf:rest>
                                            </rdf:Description>
                                        </rdf:rest>
                                    </rdf:Description>
                                </rdf:rest>
                            </rdf:Description>
                        </rdf:rest>
                    </rdf:Description>
                </owl:oneOf>
            </rdfs:Datatype>
        </owl:equivalentClass>
    </rdfs:Datatype>
    


    <!-- https://w3id.org/netbeheer/referentiemodellen/IECCIM/TC57CIM/IEC61970/Base/Wires#SynchronousMachineKind -->


    <rdfs:Datatype rdf:about="https://w3id.org/netbeheer/referentiemodellen/IECCIM/TC57CIM/IEC61970/Base/Wires#SynchronousMachineKind">
        <owl:equivalentClass>
            <rdfs:Datatype>
                <owl:oneOf>
                    <rdf:Description>
                        <rdf:type rdf:resource="http://www.w3.org/1999/02/22-rdf-syntax-ns#List"/>
                        <rdf:first>condenser</rdf:first>
                        <rdf:rest>
                            <rdf:Description>
                                <rdf:type rdf:resource="http://www.w3.org/1999/02/22-rdf-syntax-ns#List"/>
                                <rdf:first>generator</rdf:first>
                                <rdf:rest>
                                    <rdf:Description>
                                        <rdf:type rdf:resource="http://www.w3.org/1999/02/22-rdf-syntax-ns#List"/>
                                        <rdf:first>generatorOrCondenser</rdf:first>
                                        <rdf:rest>
                                            <rdf:Description>
                                                <rdf:type rdf:resource="http://www.w3.org/1999/02/22-rdf-syntax-ns#List"/>
                                                <rdf:first>generatorOrCondenserOrMotor</rdf:first>
                                                <rdf:rest>
                                                    <rdf:Description>
                                                        <rdf:type rdf:resource="http://www.w3.org/1999/02/22-rdf-syntax-ns#List"/>
                                                        <rdf:first>generatorOrMotor</rdf:first>
                                                        <rdf:rest>
                                                            <rdf:Description>
                                                                <rdf:type rdf:resource="http://www.w3.org/1999/02/22-rdf-syntax-ns#List"/>
                                                                <rdf:first>motor</rdf:first>
                                                                <rdf:rest>
                                                                    <rdf:Description>
                                                                        <rdf:type rdf:resource="http://www.w3.org/1999/02/22-rdf-syntax-ns#List"/>
                                                                        <rdf:first>motorOrCondenser</rdf:first>
                                                                        <rdf:rest rdf:resource="http://www.w3.org/1999/02/22-rdf-syntax-ns#nil"/>
                                                                    </rdf:Description>
                                                                </rdf:rest>
                                                            </rdf:Description>
                                                        </rdf:rest>
                                                    </rdf:Description>
                                                </rdf:rest>
                                            </rdf:Description>
                                        </rdf:rest>
                                    </rdf:Description>
                                </rdf:rest>
                            </rdf:Description>
                        </rdf:rest>
                    </rdf:Description>
                </owl:oneOf>
            </rdfs:Datatype>
        </owl:equivalentClass>
    </rdfs:Datatype>
    


    <!-- https://w3id.org/netbeheer/referentiemodellen/IECCIM/TC57CIM/IEC61970/Base/Wires#SynchronousMachineOperatingMode -->


    <rdfs:Datatype rdf:about="https://w3id.org/netbeheer/referentiemodellen/IECCIM/TC57CIM/IEC61970/Base/Wires#SynchronousMachineOperatingMode">
        <owl:equivalentClass>
            <rdfs:Datatype>
                <owl:oneOf>
                    <rdf:Description>
                        <rdf:type rdf:resource="http://www.w3.org/1999/02/22-rdf-syntax-ns#List"/>
                        <rdf:first>condenser</rdf:first>
                        <rdf:rest>
                            <rdf:Description>
                                <rdf:type rdf:resource="http://www.w3.org/1999/02/22-rdf-syntax-ns#List"/>
                                <rdf:first>generator</rdf:first>
                                <rdf:rest>
                                    <rdf:Description>
                                        <rdf:type rdf:resource="http://www.w3.org/1999/02/22-rdf-syntax-ns#List"/>
                                        <rdf:first>motor</rdf:first>
                                        <rdf:rest rdf:resource="http://www.w3.org/1999/02/22-rdf-syntax-ns#nil"/>
                                    </rdf:Description>
                                </rdf:rest>
                            </rdf:Description>
                        </rdf:rest>
                    </rdf:Description>
                </owl:oneOf>
            </rdfs:Datatype>
        </owl:equivalentClass>
    </rdfs:Datatype>
    


    <!-- https://w3id.org/netbeheer/referentiemodellen/IECCIM/TC57CIM/IEC61970/Base/Wires#TransformerControlMode -->


    <rdfs:Datatype rdf:about="https://w3id.org/netbeheer/referentiemodellen/IECCIM/TC57CIM/IEC61970/Base/Wires#TransformerControlMode">
        <owl:equivalentClass>
            <rdfs:Datatype>
                <owl:oneOf>
                    <rdf:Description>
                        <rdf:type rdf:resource="http://www.w3.org/1999/02/22-rdf-syntax-ns#List"/>
                        <rdf:first>reactive</rdf:first>
                        <rdf:rest>
                            <rdf:Description>
                                <rdf:type rdf:resource="http://www.w3.org/1999/02/22-rdf-syntax-ns#List"/>
                                <rdf:first>volt</rdf:first>
                                <rdf:rest rdf:resource="http://www.w3.org/1999/02/22-rdf-syntax-ns#nil"/>
                            </rdf:Description>
                        </rdf:rest>
                    </rdf:Description>
                </owl:oneOf>
            </rdfs:Datatype>
        </owl:equivalentClass>
    </rdfs:Datatype>
    


    <!-- https://w3id.org/netbeheer/referentiemodellen/IECCIM/TC57CIM/IEC61970/Base/Wires#WindingConnection -->


    <rdfs:Datatype rdf:about="https://w3id.org/netbeheer/referentiemodellen/IECCIM/TC57CIM/IEC61970/Base/Wires#WindingConnection">
        <owl:equivalentClass>
            <rdfs:Datatype>
                <owl:oneOf>
                    <rdf:Description>
                        <rdf:type rdf:resource="http://www.w3.org/1999/02/22-rdf-syntax-ns#List"/>
                        <rdf:first>A</rdf:first>
                        <rdf:rest>
                            <rdf:Description>
                                <rdf:type rdf:resource="http://www.w3.org/1999/02/22-rdf-syntax-ns#List"/>
                                <rdf:first>D</rdf:first>
                                <rdf:rest>
                                    <rdf:Description>
                                        <rdf:type rdf:resource="http://www.w3.org/1999/02/22-rdf-syntax-ns#List"/>
                                        <rdf:first>I</rdf:first>
                                        <rdf:rest>
                                            <rdf:Description>
                                                <rdf:type rdf:resource="http://www.w3.org/1999/02/22-rdf-syntax-ns#List"/>
                                                <rdf:first>Y</rdf:first>
                                                <rdf:rest>
                                                    <rdf:Description>
                                                        <rdf:type rdf:resource="http://www.w3.org/1999/02/22-rdf-syntax-ns#List"/>
                                                        <rdf:first>Yn</rdf:first>
                                                        <rdf:rest>
                                                            <rdf:Description>
                                                                <rdf:type rdf:resource="http://www.w3.org/1999/02/22-rdf-syntax-ns#List"/>
                                                                <rdf:first>Z</rdf:first>
                                                                <rdf:rest>
                                                                    <rdf:Description>
                                                                        <rdf:type rdf:resource="http://www.w3.org/1999/02/22-rdf-syntax-ns#List"/>
                                                                        <rdf:first>Zn</rdf:first>
                                                                        <rdf:rest rdf:resource="http://www.w3.org/1999/02/22-rdf-syntax-ns#nil"/>
                                                                    </rdf:Description>
                                                                </rdf:rest>
                                                            </rdf:Description>
                                                        </rdf:rest>
                                                    </rdf:Description>
                                                </rdf:rest>
                                            </rdf:Description>
                                        </rdf:rest>
                                    </rdf:Description>
                                </rdf:rest>
                            </rdf:Description>
                        </rdf:rest>
                    </rdf:Description>
                </owl:oneOf>
            </rdfs:Datatype>
        </owl:equivalentClass>
    </rdfs:Datatype>
    


    <!-- 
    ///////////////////////////////////////////////////////////////////////////////////////
    //
    // Object Properties
    //
    ///////////////////////////////////////////////////////////////////////////////////////
     -->


    


    <!-- https://w3id.org/netbeheer/referentiemodellen/IECCIM/TC57CIM/IEC61970/Base/Wires#ACLineSegmentPhase_ACLineSegment -->


    <owl:ObjectProperty rdf:about="https://w3id.org/netbeheer/referentiemodellen/IECCIM/TC57CIM/IEC61970/Base/Wires#ACLineSegmentPhase_ACLineSegment">
        <rdfs:domain rdf:resource="https://w3id.org/netbeheer/referentiemodellen/IECCIM/TC57CIM/IEC61970/Base/Wires#ACLineSegmentPhase"/>
        <rdfs:range rdf:resource="https://w3id.org/netbeheer/referentiemodellen/IECCIM/TC57CIM/IEC61970/Base/Wires#ACLineSegment"/>
        <rdfs:comment>The line segment phases which belong to the line segment.The line segment to which the phase belongs.</rdfs:comment>
    </owl:ObjectProperty>
    


    <!-- https://w3id.org/netbeheer/referentiemodellen/IECCIM/TC57CIM/IEC61970/Base/Wires#ACLineSegment_ACLineSegmentPhases -->


    <owl:ObjectProperty rdf:about="https://w3id.org/netbeheer/referentiemodellen/IECCIM/TC57CIM/IEC61970/Base/Wires#ACLineSegment_ACLineSegmentPhases">
        <owl:inverseOf rdf:resource="https://w3id.org/netbeheer/referentiemodellen/IECCIM/TC57CIM/IEC61970/Base/Wires#ACLineSegmentPhase_ACLineSegment"/>
        <rdf:type rdf:resource="http://www.w3.org/2002/07/owl#FunctionalProperty"/>
        <rdfs:domain rdf:resource="https://w3id.org/netbeheer/referentiemodellen/IECCIM/TC57CIM/IEC61970/Base/Wires#ACLineSegment"/>
        <rdfs:range rdf:resource="https://w3id.org/netbeheer/referentiemodellen/IECCIM/TC57CIM/IEC61970/Base/Wires#ACLineSegmentPhase"/>
        <rdfs:comment>The line segment phases which belong to the line segment.The line segment to which the phase belongs.</rdfs:comment>
    </owl:ObjectProperty>
    


    <!-- https://w3id.org/netbeheer/referentiemodellen/IECCIM/TC57CIM/IEC61970/Base/Wires#ACLineSegment_Clamp -->


    <owl:ObjectProperty rdf:about="https://w3id.org/netbeheer/referentiemodellen/IECCIM/TC57CIM/IEC61970/Base/Wires#ACLineSegment_Clamp">
        <rdf:type rdf:resource="http://www.w3.org/2002/07/owl#FunctionalProperty"/>
        <rdfs:domain rdf:resource="https://w3id.org/netbeheer/referentiemodellen/IECCIM/TC57CIM/IEC61970/Base/Wires#ACLineSegment"/>
        <rdfs:range rdf:resource="https://w3id.org/netbeheer/referentiemodellen/IECCIM/TC57CIM/IEC61970/Base/Wires#Clamp"/>
        <rdfs:comment>The line segment to which the clamp is connected.The clamps connected to the line segment.</rdfs:comment>
    </owl:ObjectProperty>
    


    <!-- https://w3id.org/netbeheer/referentiemodellen/IECCIM/TC57CIM/IEC61970/Base/Wires#ACLineSegment_Cut -->


    <owl:ObjectProperty rdf:about="https://w3id.org/netbeheer/referentiemodellen/IECCIM/TC57CIM/IEC61970/Base/Wires#ACLineSegment_Cut">
        <owl:inverseOf rdf:resource="https://w3id.org/netbeheer/referentiemodellen/IECCIM/TC57CIM/IEC61970/Base/Wires#Cut_ACLineSegment"/>
        <rdf:type rdf:resource="http://www.w3.org/2002/07/owl#FunctionalProperty"/>
        <rdfs:domain rdf:resource="https://w3id.org/netbeheer/referentiemodellen/IECCIM/TC57CIM/IEC61970/Base/Wires#ACLineSegment"/>
        <rdfs:range rdf:resource="https://w3id.org/netbeheer/referentiemodellen/IECCIM/TC57CIM/IEC61970/Base/Wires#Cut"/>
        <rdfs:comment>Cuts applied to the line segment.The line segment to which the cut is applied.</rdfs:comment>
    </owl:ObjectProperty>
    


    <!-- https://w3id.org/netbeheer/referentiemodellen/IECCIM/TC57CIM/IEC61970/Base/Wires#ACLineSegment_LineGroundingAction -->


    <owl:ObjectProperty rdf:about="https://w3id.org/netbeheer/referentiemodellen/IECCIM/TC57CIM/IEC61970/Base/Wires#ACLineSegment_LineGroundingAction">
        <owl:inverseOf rdf:resource="https://w3id.org/netbeheer/referentiemodellen/IECCIM/TC57CIM/IEC61970/Base/Wires#GroundAction_AlongACLineSegment"/>
        <rdfs:domain rdf:resource="https://w3id.org/netbeheer/referentiemodellen/IECCIM/TC57CIM/IEC61970/Base/Wires#ACLineSegment"/>
        <rdfs:range rdf:resource="https://w3id.org/netbeheer/referentiemodellen/IECCIM/TC57CIM/IEC61968/Operations#GroundAction"/>
        <rdfs:comment>Ground action involving clamp usage (for the case when the ground is applied along the line segment instead of at its terminals).The line segment that this ground action will affect. This is the only way to access relationship to clamp in case the ground needs to be placed along the line segment.</rdfs:comment>
    </owl:ObjectProperty>
    


    <!-- https://w3id.org/netbeheer/referentiemodellen/IECCIM/TC57CIM/IEC61970/Base/Wires#ACLineSegment_LineJumpingAction -->


    <owl:ObjectProperty rdf:about="https://w3id.org/netbeheer/referentiemodellen/IECCIM/TC57CIM/IEC61970/Base/Wires#ACLineSegment_LineJumpingAction">
        <owl:inverseOf rdf:resource="https://w3id.org/netbeheer/referentiemodellen/IECCIM/TC57CIM/IEC61970/Base/Wires#JumperAction_AlongACLineSegments"/>
        <rdfs:domain rdf:resource="https://w3id.org/netbeheer/referentiemodellen/IECCIM/TC57CIM/IEC61970/Base/Wires#ACLineSegment"/>
        <rdfs:range rdf:resource="https://w3id.org/netbeheer/referentiemodellen/IECCIM/TC57CIM/IEC61968/Operations#JumperAction"/>
        <rdfs:comment>Jumper action involving clamp usage (for the case when the jumper is applied along the line segment instead of at its terminals).The line segment that this jumper action will affect. This is the only way to access relationship to clamp in case the jumper needs to connect along the line segment.</rdfs:comment>
    </owl:ObjectProperty>
    


    <!-- https://w3id.org/netbeheer/referentiemodellen/IECCIM/TC57CIM/IEC61970/Base/Wires#ACLineSegment_PerLengthImpedance -->


    <owl:ObjectProperty rdf:about="https://w3id.org/netbeheer/referentiemodellen/IECCIM/TC57CIM/IEC61970/Base/Wires#ACLineSegment_PerLengthImpedance">
        <owl:inverseOf rdf:resource="https://w3id.org/netbeheer/referentiemodellen/IECCIM/TC57CIM/IEC61970/Base/Wires#PerLengthImpedance_ACLineSegments"/>
        <rdfs:domain rdf:resource="https://w3id.org/netbeheer/referentiemodellen/IECCIM/TC57CIM/IEC61970/Base/Wires#ACLineSegment"/>
        <rdfs:range rdf:resource="https://w3id.org/netbeheer/referentiemodellen/IECCIM/TC57CIM/IEC61970/Base/Wires#PerLengthImpedance"/>
        <rdfs:comment>Per-length impedance of this line segment.All line segments described by this per-length impedance.</rdfs:comment>
    </owl:ObjectProperty>
    


    <!-- https://w3id.org/netbeheer/referentiemodellen/IECCIM/TC57CIM/IEC61970/Base/Wires#ACLineSegment_WireSpacing -->


    <owl:ObjectProperty rdf:about="https://w3id.org/netbeheer/referentiemodellen/IECCIM/TC57CIM/IEC61970/Base/Wires#ACLineSegment_WireSpacing">
        <owl:inverseOf rdf:resource="https://w3id.org/netbeheer/referentiemodellen/IECCIM/TC57CIM/IEC61970/Base/Wires#WireSpacing_ACLineSegments"/>
        <rdfs:domain rdf:resource="https://w3id.org/netbeheer/referentiemodellen/IECCIM/TC57CIM/IEC61970/Base/Wires#ACLineSegment"/>
        <rdfs:range rdf:resource="https://w3id.org/netbeheer/referentiemodellen/IECCIM/TC57CIM/IEC61968/AssetInfo#WireSpacing"/>
        <rdfs:comment>Wire spacing configuration for this line segment.All line segments described with this wire spacing configuration.</rdfs:comment>
    </owl:ObjectProperty>
    


    <!-- https://w3id.org/netbeheer/referentiemodellen/IECCIM/TC57CIM/IEC61970/Base/Wires#ACLineSegment_b0ch -->


    <owl:ObjectProperty rdf:about="https://w3id.org/netbeheer/referentiemodellen/IECCIM/TC57CIM/IEC61970/Base/Wires#ACLineSegment_b0ch">
        <rdfs:domain rdf:resource="https://w3id.org/netbeheer/referentiemodellen/IECCIM/TC57CIM/IEC61970/Base/Wires#ACLineSegment"/>
        <rdfs:range rdf:resource="https://w3id.org/netbeheer/referentiemodellen/IECCIM/TC57CIM/IEC61970/Base/Domain#Susceptance"/>
        <rdfs:comment>Zero sequence shunt (charging) susceptance, uniformly distributed, of the entire line section.</rdfs:comment>
    </owl:ObjectProperty>
    


    <!-- https://w3id.org/netbeheer/referentiemodellen/IECCIM/TC57CIM/IEC61970/Base/Wires#ACLineSegment_bch -->


    <owl:ObjectProperty rdf:about="https://w3id.org/netbeheer/referentiemodellen/IECCIM/TC57CIM/IEC61970/Base/Wires#ACLineSegment_bch">
        <rdfs:domain rdf:resource="https://w3id.org/netbeheer/referentiemodellen/IECCIM/TC57CIM/IEC61970/Base/Wires#ACLineSegment"/>
        <rdfs:range rdf:resource="https://w3id.org/netbeheer/referentiemodellen/IECCIM/TC57CIM/IEC61970/Base/Domain#Susceptance"/>
        <rdfs:comment>Positive sequence shunt (charging) susceptance, uniformly distributed, of the entire line section.  This value represents the full charging over the full length of the line.</rdfs:comment>
    </owl:ObjectProperty>
    


    <!-- https://w3id.org/netbeheer/referentiemodellen/IECCIM/TC57CIM/IEC61970/Base/Wires#ACLineSegment_g0ch -->


    <owl:ObjectProperty rdf:about="https://w3id.org/netbeheer/referentiemodellen/IECCIM/TC57CIM/IEC61970/Base/Wires#ACLineSegment_g0ch">
        <rdfs:domain rdf:resource="https://w3id.org/netbeheer/referentiemodellen/IECCIM/TC57CIM/IEC61970/Base/Wires#ACLineSegment"/>
        <rdfs:range rdf:resource="https://w3id.org/netbeheer/referentiemodellen/IECCIM/TC57CIM/IEC61970/Base/Domain#Conductance"/>
        <rdfs:comment>Zero sequence shunt (charging) conductance, uniformly distributed, of the entire line section.</rdfs:comment>
    </owl:ObjectProperty>
    


    <!-- https://w3id.org/netbeheer/referentiemodellen/IECCIM/TC57CIM/IEC61970/Base/Wires#ACLineSegment_gch -->


    <owl:ObjectProperty rdf:about="https://w3id.org/netbeheer/referentiemodellen/IECCIM/TC57CIM/IEC61970/Base/Wires#ACLineSegment_gch">
        <rdfs:domain rdf:resource="https://w3id.org/netbeheer/referentiemodellen/IECCIM/TC57CIM/IEC61970/Base/Wires#ACLineSegment"/>
        <rdfs:range rdf:resource="https://w3id.org/netbeheer/referentiemodellen/IECCIM/TC57CIM/IEC61970/Base/Domain#Conductance"/>
        <rdfs:comment>Positive sequence shunt (charging) conductance, uniformly distributed, of the entire line section.</rdfs:comment>
    </owl:ObjectProperty>
    


    <!-- https://w3id.org/netbeheer/referentiemodellen/IECCIM/TC57CIM/IEC61970/Base/Wires#ACLineSegment_r -->


    <owl:ObjectProperty rdf:about="https://w3id.org/netbeheer/referentiemodellen/IECCIM/TC57CIM/IEC61970/Base/Wires#ACLineSegment_r">
        <rdfs:domain rdf:resource="https://w3id.org/netbeheer/referentiemodellen/IECCIM/TC57CIM/IEC61970/Base/Wires#ACLineSegment"/>
        <rdfs:range rdf:resource="https://w3id.org/netbeheer/referentiemodellen/IECCIM/TC57CIM/IEC61970/Base/Domain#Resistance"/>
        <rdfs:comment>Positive sequence series resistance of the entire line section.</rdfs:comment>
    </owl:ObjectProperty>
    


    <!-- https://w3id.org/netbeheer/referentiemodellen/IECCIM/TC57CIM/IEC61970/Base/Wires#ACLineSegment_r0 -->


    <owl:ObjectProperty rdf:about="https://w3id.org/netbeheer/referentiemodellen/IECCIM/TC57CIM/IEC61970/Base/Wires#ACLineSegment_r0">
        <rdfs:domain rdf:resource="https://w3id.org/netbeheer/referentiemodellen/IECCIM/TC57CIM/IEC61970/Base/Wires#ACLineSegment"/>
        <rdfs:range rdf:resource="https://w3id.org/netbeheer/referentiemodellen/IECCIM/TC57CIM/IEC61970/Base/Domain#Resistance"/>
        <rdfs:comment>Zero sequence series resistance of the entire line section.</rdfs:comment>
    </owl:ObjectProperty>
    


    <!-- https://w3id.org/netbeheer/referentiemodellen/IECCIM/TC57CIM/IEC61970/Base/Wires#ACLineSegment_shortCircuitEndTemperature -->


    <owl:ObjectProperty rdf:about="https://w3id.org/netbeheer/referentiemodellen/IECCIM/TC57CIM/IEC61970/Base/Wires#ACLineSegment_shortCircuitEndTemperature">
        <rdfs:domain rdf:resource="https://w3id.org/netbeheer/referentiemodellen/IECCIM/TC57CIM/IEC61970/Base/Wires#ACLineSegment"/>
        <rdfs:range rdf:resource="https://w3id.org/netbeheer/referentiemodellen/IECCIM/TC57CIM/IEC61970/Base/Domain#Temperature"/>
        <rdfs:comment>Maximum permitted temperature at the end of SC for the calculation of minimum short-circuit currents. Used for short circuit data exchange according to IEC 60909</rdfs:comment>
    </owl:ObjectProperty>
    


    <!-- https://w3id.org/netbeheer/referentiemodellen/IECCIM/TC57CIM/IEC61970/Base/Wires#ACLineSegment_x -->


    <owl:ObjectProperty rdf:about="https://w3id.org/netbeheer/referentiemodellen/IECCIM/TC57CIM/IEC61970/Base/Wires#ACLineSegment_x">
        <rdfs:domain rdf:resource="https://w3id.org/netbeheer/referentiemodellen/IECCIM/TC57CIM/IEC61970/Base/Wires#ACLineSegment"/>
        <rdfs:range rdf:resource="https://w3id.org/netbeheer/referentiemodellen/IECCIM/TC57CIM/IEC61970/Base/Domain#Reactance"/>
        <rdfs:comment>Positive sequence series reactance of the entire line section.</rdfs:comment>
    </owl:ObjectProperty>
    


    <!-- https://w3id.org/netbeheer/referentiemodellen/IECCIM/TC57CIM/IEC61970/Base/Wires#ACLineSegment_x0 -->


    <owl:ObjectProperty rdf:about="https://w3id.org/netbeheer/referentiemodellen/IECCIM/TC57CIM/IEC61970/Base/Wires#ACLineSegment_x0">
        <rdfs:domain rdf:resource="https://w3id.org/netbeheer/referentiemodellen/IECCIM/TC57CIM/IEC61970/Base/Wires#ACLineSegment"/>
        <rdfs:range rdf:resource="https://w3id.org/netbeheer/referentiemodellen/IECCIM/TC57CIM/IEC61970/Base/Domain#Reactance"/>
        <rdfs:comment>Zero sequence series reactance of the entire line section.</rdfs:comment>
    </owl:ObjectProperty>
    


    <!-- https://w3id.org/netbeheer/referentiemodellen/IECCIM/TC57CIM/IEC61970/Base/Wires#AsynchronousMachineDynamics_AsynchronousMachine -->


    <owl:ObjectProperty rdf:about="https://w3id.org/netbeheer/referentiemodellen/IECCIM/TC57CIM/IEC61970/Base/Wires#AsynchronousMachineDynamics_AsynchronousMachine">
        <rdfs:domain rdf:resource="https://w3id.org/netbeheer/referentiemodellen/IECCIM/TC57CIM/IEC61970/Dynamics/StandardModels/AsynchronousMachineDynamics#AsynchronousMachineDynamics"/>
        <rdfs:range rdf:resource="https://w3id.org/netbeheer/referentiemodellen/IECCIM/TC57CIM/IEC61970/Base/Wires#AsynchronousMachine"/>
        <rdfs:comment>Asynchronous machine dynamics model used to describe dynamic behavior of this asynchronous machine.Asynchronous machine to which this asynchronous machine dynamics model applies.</rdfs:comment>
    </owl:ObjectProperty>
    


    <!-- https://w3id.org/netbeheer/referentiemodellen/IECCIM/TC57CIM/IEC61970/Base/Wires#AsynchronousMachine_AsynchronousMachineDynamics -->


    <owl:ObjectProperty rdf:about="https://w3id.org/netbeheer/referentiemodellen/IECCIM/TC57CIM/IEC61970/Base/Wires#AsynchronousMachine_AsynchronousMachineDynamics">
        <owl:inverseOf rdf:resource="https://w3id.org/netbeheer/referentiemodellen/IECCIM/TC57CIM/IEC61970/Base/Wires#AsynchronousMachineDynamics_AsynchronousMachine"/>
        <rdf:type rdf:resource="http://www.w3.org/2002/07/owl#FunctionalProperty"/>
        <rdfs:domain rdf:resource="https://w3id.org/netbeheer/referentiemodellen/IECCIM/TC57CIM/IEC61970/Base/Wires#AsynchronousMachine"/>
        <rdfs:range rdf:resource="https://w3id.org/netbeheer/referentiemodellen/IECCIM/TC57CIM/IEC61970/Dynamics/StandardModels/AsynchronousMachineDynamics#AsynchronousMachineDynamics"/>
        <rdfs:comment>Asynchronous machine dynamics model used to describe dynamic behavior of this asynchronous machine.Asynchronous machine to which this asynchronous machine dynamics model applies.</rdfs:comment>
    </owl:ObjectProperty>
    


    <!-- https://w3id.org/netbeheer/referentiemodellen/IECCIM/TC57CIM/IEC61970/Base/Wires#AsynchronousMachine_efficiency -->


    <owl:ObjectProperty rdf:about="https://w3id.org/netbeheer/referentiemodellen/IECCIM/TC57CIM/IEC61970/Base/Wires#AsynchronousMachine_efficiency">
        <rdfs:domain rdf:resource="https://w3id.org/netbeheer/referentiemodellen/IECCIM/TC57CIM/IEC61970/Base/Wires#AsynchronousMachine"/>
        <rdfs:range rdf:resource="https://w3id.org/netbeheer/referentiemodellen/IECCIM/TC57CIM/IEC61970/Base/Domain#PerCent"/>
        <rdfs:comment>Efficiency of the asynchronous machine at nominal operation in percent. Indicator for converter drive motors. Used for short circuit data exchange according to IEC 60909</rdfs:comment>
    </owl:ObjectProperty>
    


    <!-- https://w3id.org/netbeheer/referentiemodellen/IECCIM/TC57CIM/IEC61970/Base/Wires#AsynchronousMachine_nominalFrequency -->


    <owl:ObjectProperty rdf:about="https://w3id.org/netbeheer/referentiemodellen/IECCIM/TC57CIM/IEC61970/Base/Wires#AsynchronousMachine_nominalFrequency">
        <rdfs:domain rdf:resource="https://w3id.org/netbeheer/referentiemodellen/IECCIM/TC57CIM/IEC61970/Base/Wires#AsynchronousMachine"/>
        <rdfs:range rdf:resource="https://w3id.org/netbeheer/referentiemodellen/IECCIM/TC57CIM/IEC61970/Base/Domain#Frequency"/>
        <rdfs:comment>Nameplate data indicates if the machine is 50 or 60 Hz.</rdfs:comment>
    </owl:ObjectProperty>
    


    <!-- https://w3id.org/netbeheer/referentiemodellen/IECCIM/TC57CIM/IEC61970/Base/Wires#AsynchronousMachine_nominalSpeed -->


    <owl:ObjectProperty rdf:about="https://w3id.org/netbeheer/referentiemodellen/IECCIM/TC57CIM/IEC61970/Base/Wires#AsynchronousMachine_nominalSpeed">
        <rdfs:domain rdf:resource="https://w3id.org/netbeheer/referentiemodellen/IECCIM/TC57CIM/IEC61970/Base/Wires#AsynchronousMachine"/>
        <rdfs:range rdf:resource="https://w3id.org/netbeheer/referentiemodellen/IECCIM/TC57CIM/IEC61970/Base/Domain#RotationSpeed"/>
        <rdfs:comment>Nameplate data.  Depends on the slip and number of pole pairs.</rdfs:comment>
    </owl:ObjectProperty>
    


    <!-- https://w3id.org/netbeheer/referentiemodellen/IECCIM/TC57CIM/IEC61970/Base/Wires#AsynchronousMachine_ratedMechanicalPower -->


    <owl:ObjectProperty rdf:about="https://w3id.org/netbeheer/referentiemodellen/IECCIM/TC57CIM/IEC61970/Base/Wires#AsynchronousMachine_ratedMechanicalPower">
        <rdfs:domain rdf:resource="https://w3id.org/netbeheer/referentiemodellen/IECCIM/TC57CIM/IEC61970/Base/Wires#AsynchronousMachine"/>
        <rdfs:range rdf:resource="https://w3id.org/netbeheer/referentiemodellen/IECCIM/TC57CIM/IEC61970/Base/Domain#ActivePower"/>
        <rdfs:comment>Rated mechanical power (Pr in the IEC 60909-0). Used for short circuit data exchange according to IEC 60909.</rdfs:comment>
    </owl:ObjectProperty>
    


    <!-- https://w3id.org/netbeheer/referentiemodellen/IECCIM/TC57CIM/IEC61970/Base/Wires#AsynchronousMachine_rr1 -->


    <owl:ObjectProperty rdf:about="https://w3id.org/netbeheer/referentiemodellen/IECCIM/TC57CIM/IEC61970/Base/Wires#AsynchronousMachine_rr1">
        <rdfs:domain rdf:resource="https://w3id.org/netbeheer/referentiemodellen/IECCIM/TC57CIM/IEC61970/Base/Wires#AsynchronousMachine"/>
        <rdfs:range rdf:resource="https://w3id.org/netbeheer/referentiemodellen/IECCIM/TC57CIM/IEC61970/Base/Domain#Resistance"/>
        <rdfs:comment>Damper 1 winding resistance.
</rdfs:comment>
    </owl:ObjectProperty>
    


    <!-- https://w3id.org/netbeheer/referentiemodellen/IECCIM/TC57CIM/IEC61970/Base/Wires#AsynchronousMachine_rr2 -->


    <owl:ObjectProperty rdf:about="https://w3id.org/netbeheer/referentiemodellen/IECCIM/TC57CIM/IEC61970/Base/Wires#AsynchronousMachine_rr2">
        <rdfs:domain rdf:resource="https://w3id.org/netbeheer/referentiemodellen/IECCIM/TC57CIM/IEC61970/Base/Wires#AsynchronousMachine"/>
        <rdfs:range rdf:resource="https://w3id.org/netbeheer/referentiemodellen/IECCIM/TC57CIM/IEC61970/Base/Domain#Resistance"/>
        <rdfs:comment>Damper 2 winding resistance.
</rdfs:comment>
    </owl:ObjectProperty>
    


    <!-- https://w3id.org/netbeheer/referentiemodellen/IECCIM/TC57CIM/IEC61970/Base/Wires#AsynchronousMachine_tpo -->


    <owl:ObjectProperty rdf:about="https://w3id.org/netbeheer/referentiemodellen/IECCIM/TC57CIM/IEC61970/Base/Wires#AsynchronousMachine_tpo">
        <rdfs:domain rdf:resource="https://w3id.org/netbeheer/referentiemodellen/IECCIM/TC57CIM/IEC61970/Base/Wires#AsynchronousMachine"/>
        <rdfs:range rdf:resource="https://w3id.org/netbeheer/referentiemodellen/IECCIM/TC57CIM/IEC61970/Base/Domain#Seconds"/>
        <rdfs:comment>Transient rotor time constant (greater than tppo).</rdfs:comment>
    </owl:ObjectProperty>
    


    <!-- https://w3id.org/netbeheer/referentiemodellen/IECCIM/TC57CIM/IEC61970/Base/Wires#AsynchronousMachine_tppo -->


    <owl:ObjectProperty rdf:about="https://w3id.org/netbeheer/referentiemodellen/IECCIM/TC57CIM/IEC61970/Base/Wires#AsynchronousMachine_tppo">
        <rdfs:domain rdf:resource="https://w3id.org/netbeheer/referentiemodellen/IECCIM/TC57CIM/IEC61970/Base/Wires#AsynchronousMachine"/>
        <rdfs:range rdf:resource="https://w3id.org/netbeheer/referentiemodellen/IECCIM/TC57CIM/IEC61970/Base/Domain#Seconds"/>
        <rdfs:comment>Sub-transient rotor time constant (greater than 0).
</rdfs:comment>
    </owl:ObjectProperty>
    


    <!-- https://w3id.org/netbeheer/referentiemodellen/IECCIM/TC57CIM/IEC61970/Base/Wires#AsynchronousMachine_xlr1 -->


    <owl:ObjectProperty rdf:about="https://w3id.org/netbeheer/referentiemodellen/IECCIM/TC57CIM/IEC61970/Base/Wires#AsynchronousMachine_xlr1">
        <rdfs:domain rdf:resource="https://w3id.org/netbeheer/referentiemodellen/IECCIM/TC57CIM/IEC61970/Base/Wires#AsynchronousMachine"/>
        <rdfs:range rdf:resource="https://w3id.org/netbeheer/referentiemodellen/IECCIM/TC57CIM/IEC61970/Base/Domain#Reactance"/>
        <rdfs:comment>Damper 1 winding leakage reactance.
</rdfs:comment>
    </owl:ObjectProperty>
    


    <!-- https://w3id.org/netbeheer/referentiemodellen/IECCIM/TC57CIM/IEC61970/Base/Wires#AsynchronousMachine_xlr2 -->


    <owl:ObjectProperty rdf:about="https://w3id.org/netbeheer/referentiemodellen/IECCIM/TC57CIM/IEC61970/Base/Wires#AsynchronousMachine_xlr2">
        <rdfs:domain rdf:resource="https://w3id.org/netbeheer/referentiemodellen/IECCIM/TC57CIM/IEC61970/Base/Wires#AsynchronousMachine"/>
        <rdfs:range rdf:resource="https://w3id.org/netbeheer/referentiemodellen/IECCIM/TC57CIM/IEC61970/Base/Domain#Reactance"/>
        <rdfs:comment>Damper 2 winding leakage reactance.
</rdfs:comment>
    </owl:ObjectProperty>
    


    <!-- https://w3id.org/netbeheer/referentiemodellen/IECCIM/TC57CIM/IEC61970/Base/Wires#AsynchronousMachine_xm -->


    <owl:ObjectProperty rdf:about="https://w3id.org/netbeheer/referentiemodellen/IECCIM/TC57CIM/IEC61970/Base/Wires#AsynchronousMachine_xm">
        <rdfs:domain rdf:resource="https://w3id.org/netbeheer/referentiemodellen/IECCIM/TC57CIM/IEC61970/Base/Wires#AsynchronousMachine"/>
        <rdfs:range rdf:resource="https://w3id.org/netbeheer/referentiemodellen/IECCIM/TC57CIM/IEC61970/Base/Domain#Reactance"/>
        <rdfs:comment>Magnetizing reactance.
</rdfs:comment>
    </owl:ObjectProperty>
    


    <!-- https://w3id.org/netbeheer/referentiemodellen/IECCIM/TC57CIM/IEC61970/Base/Wires#AsynchronousMachine_xp -->


    <owl:ObjectProperty rdf:about="https://w3id.org/netbeheer/referentiemodellen/IECCIM/TC57CIM/IEC61970/Base/Wires#AsynchronousMachine_xp">
        <rdfs:domain rdf:resource="https://w3id.org/netbeheer/referentiemodellen/IECCIM/TC57CIM/IEC61970/Base/Wires#AsynchronousMachine"/>
        <rdfs:range rdf:resource="https://w3id.org/netbeheer/referentiemodellen/IECCIM/TC57CIM/IEC61970/Base/Domain#Reactance"/>
        <rdfs:comment>Transient reactance (unsaturated) (greater than or equal to xpp).
</rdfs:comment>
    </owl:ObjectProperty>
    


    <!-- https://w3id.org/netbeheer/referentiemodellen/IECCIM/TC57CIM/IEC61970/Base/Wires#AsynchronousMachine_xpp -->


    <owl:ObjectProperty rdf:about="https://w3id.org/netbeheer/referentiemodellen/IECCIM/TC57CIM/IEC61970/Base/Wires#AsynchronousMachine_xpp">
        <rdfs:domain rdf:resource="https://w3id.org/netbeheer/referentiemodellen/IECCIM/TC57CIM/IEC61970/Base/Wires#AsynchronousMachine"/>
        <rdfs:range rdf:resource="https://w3id.org/netbeheer/referentiemodellen/IECCIM/TC57CIM/IEC61970/Base/Domain#Reactance"/>
        <rdfs:comment>Sub-transient reactance (unsaturated) (greather than Xl).
</rdfs:comment>
    </owl:ObjectProperty>
    


    <!-- https://w3id.org/netbeheer/referentiemodellen/IECCIM/TC57CIM/IEC61970/Base/Wires#AsynchronousMachine_xs -->


    <owl:ObjectProperty rdf:about="https://w3id.org/netbeheer/referentiemodellen/IECCIM/TC57CIM/IEC61970/Base/Wires#AsynchronousMachine_xs">
        <rdfs:domain rdf:resource="https://w3id.org/netbeheer/referentiemodellen/IECCIM/TC57CIM/IEC61970/Base/Wires#AsynchronousMachine"/>
        <rdfs:range rdf:resource="https://w3id.org/netbeheer/referentiemodellen/IECCIM/TC57CIM/IEC61970/Base/Domain#Reactance"/>
        <rdfs:comment>Synchronous reactance (greather than xp).
</rdfs:comment>
    </owl:ObjectProperty>
    


    <!-- https://w3id.org/netbeheer/referentiemodellen/IECCIM/TC57CIM/IEC61970/Base/Wires#Breaker_inTransitTime -->


    <owl:ObjectProperty rdf:about="https://w3id.org/netbeheer/referentiemodellen/IECCIM/TC57CIM/IEC61970/Base/Wires#Breaker_inTransitTime">
        <rdfs:domain rdf:resource="https://w3id.org/netbeheer/referentiemodellen/IECCIM/TC57CIM/IEC61970/Base/Wires#Breaker"/>
        <rdfs:range rdf:resource="https://w3id.org/netbeheer/referentiemodellen/IECCIM/TC57CIM/IEC61970/Base/Domain#Seconds"/>
        <rdfs:comment>The transition time from open to close.
</rdfs:comment>
    </owl:ObjectProperty>
    


    <!-- https://w3id.org/netbeheer/referentiemodellen/IECCIM/TC57CIM/IEC61970/Base/Wires#BusbarSection_VoltageControlZone -->


    <owl:ObjectProperty rdf:about="https://w3id.org/netbeheer/referentiemodellen/IECCIM/TC57CIM/IEC61970/Base/Wires#BusbarSection_VoltageControlZone">
        <rdf:type rdf:resource="http://www.w3.org/2002/07/owl#FunctionalProperty"/>
        <rdfs:domain rdf:resource="https://w3id.org/netbeheer/referentiemodellen/IECCIM/TC57CIM/IEC61970/Base/Wires#BusbarSection"/>
        <rdfs:range rdf:resource="https://w3id.org/netbeheer/referentiemodellen/IECCIM/TC57CIM/IEC61970/Base/Wires#VoltageControlZone"/>
        <rdfs:comment>A VoltageControlZone is controlled by a designated BusbarSection.A VoltageControlZone is controlled by a designated BusbarSection.</rdfs:comment>
    </owl:ObjectProperty>
    


    <!-- https://w3id.org/netbeheer/referentiemodellen/IECCIM/TC57CIM/IEC61970/Base/Wires#BusbarSection_ipMax -->


    <owl:ObjectProperty rdf:about="https://w3id.org/netbeheer/referentiemodellen/IECCIM/TC57CIM/IEC61970/Base/Wires#BusbarSection_ipMax">
        <rdfs:domain rdf:resource="https://w3id.org/netbeheer/referentiemodellen/IECCIM/TC57CIM/IEC61970/Base/Wires#BusbarSection"/>
        <rdfs:range rdf:resource="https://w3id.org/netbeheer/referentiemodellen/IECCIM/TC57CIM/IEC61970/Base/Domain#CurrentFlow"/>
        <rdfs:comment>Maximum allowable peak short-circuit current of busbar (Ipmax in the IEC 60909-0). 
Mechanical limit of the busbar in the substation itself. Used for short circuit data exchange according to IEC 60909</rdfs:comment>
    </owl:ObjectProperty>
    


    <!-- https://w3id.org/netbeheer/referentiemodellen/IECCIM/TC57CIM/IEC61970/Base/Wires#Clamp_ACLineSegment -->


    <owl:ObjectProperty rdf:about="https://w3id.org/netbeheer/referentiemodellen/IECCIM/TC57CIM/IEC61970/Base/Wires#Clamp_ACLineSegment">
        <owl:inverseOf rdf:resource="https://w3id.org/netbeheer/referentiemodellen/IECCIM/TC57CIM/IEC61970/Base/Wires#ACLineSegment_Clamp"/>
        <rdfs:domain rdf:resource="https://w3id.org/netbeheer/referentiemodellen/IECCIM/TC57CIM/IEC61970/Base/Wires#Clamp"/>
        <rdfs:range rdf:resource="https://w3id.org/netbeheer/referentiemodellen/IECCIM/TC57CIM/IEC61970/Base/Wires#ACLineSegment"/>
        <rdfs:comment>The line segment to which the clamp is connected.The clamps connected to the line segment.</rdfs:comment>
    </owl:ObjectProperty>
    


    <!-- https://w3id.org/netbeheer/referentiemodellen/IECCIM/TC57CIM/IEC61970/Base/Wires#Clamp_lengthFromTerminal1 -->


    <owl:ObjectProperty rdf:about="https://w3id.org/netbeheer/referentiemodellen/IECCIM/TC57CIM/IEC61970/Base/Wires#Clamp_lengthFromTerminal1">
        <rdfs:domain rdf:resource="https://w3id.org/netbeheer/referentiemodellen/IECCIM/TC57CIM/IEC61970/Base/Wires#Clamp"/>
        <rdfs:range rdf:resource="https://w3id.org/netbeheer/referentiemodellen/IECCIM/TC57CIM/IEC61970/Base/Domain#Length"/>
        <rdfs:comment>The length to the place where the clamp is located starting from side one of the line segment, i.e. the line segment terminal with sequence number equal to 1.
</rdfs:comment>
    </owl:ObjectProperty>
    


    <!-- https://w3id.org/netbeheer/referentiemodellen/IECCIM/TC57CIM/IEC61970/Base/Wires#CompositeSwitch_Switches -->


    <owl:ObjectProperty rdf:about="https://w3id.org/netbeheer/referentiemodellen/IECCIM/TC57CIM/IEC61970/Base/Wires#CompositeSwitch_Switches">
        <rdfs:domain rdf:resource="https://w3id.org/netbeheer/referentiemodellen/IECCIM/TC57CIM/IEC61970/Base/Wires#CompositeSwitch"/>
        <rdfs:range rdf:resource="https://w3id.org/netbeheer/referentiemodellen/IECCIM/TC57CIM/IEC61970/Base/Wires#Switch"/>
        <rdfs:comment>Composite switch to which this Switch belongs.Switches contained in this Composite switch.</rdfs:comment>
    </owl:ObjectProperty>
    


    <!-- https://w3id.org/netbeheer/referentiemodellen/IECCIM/TC57CIM/IEC61970/Base/Wires#Conductor_length -->


    <owl:ObjectProperty rdf:about="https://w3id.org/netbeheer/referentiemodellen/IECCIM/TC57CIM/IEC61970/Base/Wires#Conductor_length">
        <rdfs:domain rdf:resource="https://w3id.org/netbeheer/referentiemodellen/IECCIM/TC57CIM/IEC61970/Base/Wires#Conductor"/>
        <rdfs:range rdf:resource="https://w3id.org/netbeheer/referentiemodellen/IECCIM/TC57CIM/IEC61970/Base/Domain#Length"/>
        <rdfs:comment>Segment length for calculating line section capabilities</rdfs:comment>
    </owl:ObjectProperty>
    


    <!-- https://w3id.org/netbeheer/referentiemodellen/IECCIM/TC57CIM/IEC61970/Base/Wires#ConnectDisconnectFunction_Switches -->


    <owl:ObjectProperty rdf:about="https://w3id.org/netbeheer/referentiemodellen/IECCIM/TC57CIM/IEC61970/Base/Wires#ConnectDisconnectFunction_Switches">
        <rdfs:domain rdf:resource="https://w3id.org/netbeheer/referentiemodellen/IECCIM/TC57CIM/IEC61968/LoadControl#ConnectDisconnectFunction"/>
        <rdfs:range rdf:resource="https://w3id.org/netbeheer/referentiemodellen/IECCIM/TC57CIM/IEC61970/Base/Wires#Switch"/>
        <rdfs:comment></rdfs:comment>
    </owl:ObjectProperty>
    


    <!-- https://w3id.org/netbeheer/referentiemodellen/IECCIM/TC57CIM/IEC61970/Base/Wires#CutAction_Cut -->


    <owl:ObjectProperty rdf:about="https://w3id.org/netbeheer/referentiemodellen/IECCIM/TC57CIM/IEC61970/Base/Wires#CutAction_Cut">
        <rdfs:domain rdf:resource="https://w3id.org/netbeheer/referentiemodellen/IECCIM/TC57CIM/IEC61968/Operations#CutAction"/>
        <rdfs:range rdf:resource="https://w3id.org/netbeheer/referentiemodellen/IECCIM/TC57CIM/IEC61970/Base/Wires#Cut"/>
        <rdfs:comment>Action taken with this cut.Cut on which this action is taken.</rdfs:comment>
    </owl:ObjectProperty>
    


    <!-- https://w3id.org/netbeheer/referentiemodellen/IECCIM/TC57CIM/IEC61970/Base/Wires#Cut_ACLineSegment -->


    <owl:ObjectProperty rdf:about="https://w3id.org/netbeheer/referentiemodellen/IECCIM/TC57CIM/IEC61970/Base/Wires#Cut_ACLineSegment">
        <rdfs:domain rdf:resource="https://w3id.org/netbeheer/referentiemodellen/IECCIM/TC57CIM/IEC61970/Base/Wires#Cut"/>
        <rdfs:range rdf:resource="https://w3id.org/netbeheer/referentiemodellen/IECCIM/TC57CIM/IEC61970/Base/Wires#ACLineSegment"/>
        <rdfs:comment>Cuts applied to the line segment.The line segment to which the cut is applied.</rdfs:comment>
    </owl:ObjectProperty>
    


    <!-- https://w3id.org/netbeheer/referentiemodellen/IECCIM/TC57CIM/IEC61970/Base/Wires#Cut_CutAction -->


    <owl:ObjectProperty rdf:about="https://w3id.org/netbeheer/referentiemodellen/IECCIM/TC57CIM/IEC61970/Base/Wires#Cut_CutAction">
        <owl:inverseOf rdf:resource="https://w3id.org/netbeheer/referentiemodellen/IECCIM/TC57CIM/IEC61970/Base/Wires#CutAction_Cut"/>
        <rdfs:domain rdf:resource="https://w3id.org/netbeheer/referentiemodellen/IECCIM/TC57CIM/IEC61970/Base/Wires#Cut"/>
        <rdfs:range rdf:resource="https://w3id.org/netbeheer/referentiemodellen/IECCIM/TC57CIM/IEC61968/Operations#CutAction"/>
        <rdfs:comment>Action taken with this cut.Cut on which this action is taken.</rdfs:comment>
    </owl:ObjectProperty>
    


    <!-- https://w3id.org/netbeheer/referentiemodellen/IECCIM/TC57CIM/IEC61970/Base/Wires#Cut_lengthFromTerminal1 -->


    <owl:ObjectProperty rdf:about="https://w3id.org/netbeheer/referentiemodellen/IECCIM/TC57CIM/IEC61970/Base/Wires#Cut_lengthFromTerminal1">
        <rdfs:domain rdf:resource="https://w3id.org/netbeheer/referentiemodellen/IECCIM/TC57CIM/IEC61970/Base/Wires#Cut"/>
        <rdfs:range rdf:resource="https://w3id.org/netbeheer/referentiemodellen/IECCIM/TC57CIM/IEC61970/Base/Domain#Length"/>
        <rdfs:comment>The length to the place where the cut is located starting from side one of the cut line segment, i.e. the line segment Terminal with sequenceNumber equal to 1.
</rdfs:comment>
    </owl:ObjectProperty>
    


    <!-- https://w3id.org/netbeheer/referentiemodellen/IECCIM/TC57CIM/IEC61970/Base/Wires#EarthFaultCompensator_r -->


    <owl:ObjectProperty rdf:about="https://w3id.org/netbeheer/referentiemodellen/IECCIM/TC57CIM/IEC61970/Base/Wires#EarthFaultCompensator_r">
        <rdfs:domain rdf:resource="https://w3id.org/netbeheer/referentiemodellen/IECCIM/TC57CIM/IEC61970/Base/Wires#EarthFaultCompensator"/>
        <rdfs:range rdf:resource="https://w3id.org/netbeheer/referentiemodellen/IECCIM/TC57CIM/IEC61970/Base/Domain#Resistance"/>
        <rdfs:comment>Nominal resistance of device.</rdfs:comment>
    </owl:ObjectProperty>
    


    <!-- https://w3id.org/netbeheer/referentiemodellen/IECCIM/TC57CIM/IEC61970/Base/Wires#EnergyConsumerPhase_EnergyConsumer -->


    <owl:ObjectProperty rdf:about="https://w3id.org/netbeheer/referentiemodellen/IECCIM/TC57CIM/IEC61970/Base/Wires#EnergyConsumerPhase_EnergyConsumer">
        <owl:inverseOf rdf:resource="https://w3id.org/netbeheer/referentiemodellen/IECCIM/TC57CIM/IEC61970/Base/Wires#EnergyConsumer_EnergyConsumerPhase"/>
        <rdfs:domain rdf:resource="https://w3id.org/netbeheer/referentiemodellen/IECCIM/TC57CIM/IEC61970/Base/Wires#EnergyConsumerPhase"/>
        <rdfs:range rdf:resource="https://w3id.org/netbeheer/referentiemodellen/IECCIM/TC57CIM/IEC61970/Base/Wires#EnergyConsumer"/>
        <rdfs:comment>The energy consumer to which this phase belongs.The individual phase models for this energy consumer.</rdfs:comment>
    </owl:ObjectProperty>
    


    <!-- https://w3id.org/netbeheer/referentiemodellen/IECCIM/TC57CIM/IEC61970/Base/Wires#EnergyConsumerPhase_pfixed -->


    <owl:ObjectProperty rdf:about="https://w3id.org/netbeheer/referentiemodellen/IECCIM/TC57CIM/IEC61970/Base/Wires#EnergyConsumerPhase_pfixed">
        <rdfs:domain rdf:resource="https://w3id.org/netbeheer/referentiemodellen/IECCIM/TC57CIM/IEC61970/Base/Wires#EnergyConsumerPhase"/>
        <rdfs:range rdf:resource="https://w3id.org/netbeheer/referentiemodellen/IECCIM/TC57CIM/IEC61970/Base/Domain#ActivePower"/>
        <rdfs:comment>Active power of the load that is a fixed quantity. Load sign convention is used, i.e. positive sign means flow out from a node.
</rdfs:comment>
    </owl:ObjectProperty>
    


    <!-- https://w3id.org/netbeheer/referentiemodellen/IECCIM/TC57CIM/IEC61970/Base/Wires#EnergyConsumerPhase_pfixedPct -->


    <owl:ObjectProperty rdf:about="https://w3id.org/netbeheer/referentiemodellen/IECCIM/TC57CIM/IEC61970/Base/Wires#EnergyConsumerPhase_pfixedPct">
        <rdfs:domain rdf:resource="https://w3id.org/netbeheer/referentiemodellen/IECCIM/TC57CIM/IEC61970/Base/Wires#EnergyConsumerPhase"/>
        <rdfs:range rdf:resource="https://w3id.org/netbeheer/referentiemodellen/IECCIM/TC57CIM/IEC61970/Base/Domain#PerCent"/>
        <rdfs:comment>Fixed active power as per cent of load group fixed active power. Load sign convention is used, i.e. positive sign means flow out from a node.
</rdfs:comment>
    </owl:ObjectProperty>
    


    <!-- https://w3id.org/netbeheer/referentiemodellen/IECCIM/TC57CIM/IEC61970/Base/Wires#EnergyConsumerPhase_qfixed -->


    <owl:ObjectProperty rdf:about="https://w3id.org/netbeheer/referentiemodellen/IECCIM/TC57CIM/IEC61970/Base/Wires#EnergyConsumerPhase_qfixed">
        <rdfs:domain rdf:resource="https://w3id.org/netbeheer/referentiemodellen/IECCIM/TC57CIM/IEC61970/Base/Wires#EnergyConsumerPhase"/>
        <rdfs:range rdf:resource="https://w3id.org/netbeheer/referentiemodellen/IECCIM/TC57CIM/IEC61970/Base/Domain#ReactivePower"/>
        <rdfs:comment>Reactive power of the load that is a fixed quantity. Load sign convention is used, i.e. positive sign means flow out from a node.
</rdfs:comment>
    </owl:ObjectProperty>
    


    <!-- https://w3id.org/netbeheer/referentiemodellen/IECCIM/TC57CIM/IEC61970/Base/Wires#EnergyConsumerPhase_qfixedPct -->


    <owl:ObjectProperty rdf:about="https://w3id.org/netbeheer/referentiemodellen/IECCIM/TC57CIM/IEC61970/Base/Wires#EnergyConsumerPhase_qfixedPct">
        <rdfs:domain rdf:resource="https://w3id.org/netbeheer/referentiemodellen/IECCIM/TC57CIM/IEC61970/Base/Wires#EnergyConsumerPhase"/>
        <rdfs:range rdf:resource="https://w3id.org/netbeheer/referentiemodellen/IECCIM/TC57CIM/IEC61970/Base/Domain#PerCent"/>
        <rdfs:comment>Fixed reactive power as per cent of load group fixed reactive power. Load sign convention is used, i.e. positive sign means flow out from a node.
</rdfs:comment>
    </owl:ObjectProperty>
    


    <!-- https://w3id.org/netbeheer/referentiemodellen/IECCIM/TC57CIM/IEC61970/Base/Wires#EnergyConsumer_EnergyConsumerPhase -->


    <owl:ObjectProperty rdf:about="https://w3id.org/netbeheer/referentiemodellen/IECCIM/TC57CIM/IEC61970/Base/Wires#EnergyConsumer_EnergyConsumerPhase">
        <rdf:type rdf:resource="http://www.w3.org/2002/07/owl#FunctionalProperty"/>
        <rdfs:domain rdf:resource="https://w3id.org/netbeheer/referentiemodellen/IECCIM/TC57CIM/IEC61970/Base/Wires#EnergyConsumer"/>
        <rdfs:range rdf:resource="https://w3id.org/netbeheer/referentiemodellen/IECCIM/TC57CIM/IEC61970/Base/Wires#EnergyConsumerPhase"/>
        <rdfs:comment>The energy consumer to which this phase belongs.The individual phase models for this energy consumer.</rdfs:comment>
    </owl:ObjectProperty>
    


    <!-- https://w3id.org/netbeheer/referentiemodellen/IECCIM/TC57CIM/IEC61970/Base/Wires#EnergyConsumer_LoadDynamics -->


    <owl:ObjectProperty rdf:about="https://w3id.org/netbeheer/referentiemodellen/IECCIM/TC57CIM/IEC61970/Base/Wires#EnergyConsumer_LoadDynamics">
        <owl:inverseOf rdf:resource="https://w3id.org/netbeheer/referentiemodellen/IECCIM/TC57CIM/IEC61970/Base/Wires#LoadDynamics_EnergyConsumer"/>
        <rdfs:domain rdf:resource="https://w3id.org/netbeheer/referentiemodellen/IECCIM/TC57CIM/IEC61970/Base/Wires#EnergyConsumer"/>
        <rdfs:range rdf:resource="https://w3id.org/netbeheer/referentiemodellen/IECCIM/TC57CIM/IEC61970/Dynamics/StandardModels/LoadDynamics#LoadDynamics"/>
        <rdfs:comment>Load dynamics model used to describe dynamic behavior of this energy consumer.Energy consumer to which this dynamics load model applies.</rdfs:comment>
    </owl:ObjectProperty>
    


    <!-- https://w3id.org/netbeheer/referentiemodellen/IECCIM/TC57CIM/IEC61970/Base/Wires#EnergyConsumer_LoadResponse -->


    <owl:ObjectProperty rdf:about="https://w3id.org/netbeheer/referentiemodellen/IECCIM/TC57CIM/IEC61970/Base/Wires#EnergyConsumer_LoadResponse">
        <rdfs:domain rdf:resource="https://w3id.org/netbeheer/referentiemodellen/IECCIM/TC57CIM/IEC61970/Base/Wires#EnergyConsumer"/>
        <rdfs:range rdf:resource="https://w3id.org/netbeheer/referentiemodellen/IECCIM/TC57CIM/IEC61970/Base/LoadModel#LoadResponseCharacteristic"/>
        <rdfs:comment>The set of loads that have the response characteristics.The load response characteristic of this load.  If missing, this load is assumed to be constant power.</rdfs:comment>
    </owl:ObjectProperty>
    


    <!-- https://w3id.org/netbeheer/referentiemodellen/IECCIM/TC57CIM/IEC61970/Base/Wires#EnergyConsumer_PowerCutZone -->


    <owl:ObjectProperty rdf:about="https://w3id.org/netbeheer/referentiemodellen/IECCIM/TC57CIM/IEC61970/Base/Wires#EnergyConsumer_PowerCutZone">
        <owl:inverseOf rdf:resource="https://w3id.org/netbeheer/referentiemodellen/IECCIM/TC57CIM/IEC61970/Base/Wires#PowerCutZone_EnergyConsumers"/>
        <rdfs:domain rdf:resource="https://w3id.org/netbeheer/referentiemodellen/IECCIM/TC57CIM/IEC61970/Base/Wires#EnergyConsumer"/>
        <rdfs:range rdf:resource="https://w3id.org/netbeheer/referentiemodellen/IECCIM/TC57CIM/IEC61970/Base/LoadModel#PowerCutZone"/>
        <rdfs:comment>The  energy consumer is assigned to this power cut zone.Energy consumer is assigned to the power cut zone.</rdfs:comment>
    </owl:ObjectProperty>
    


    <!-- https://w3id.org/netbeheer/referentiemodellen/IECCIM/TC57CIM/IEC61970/Base/Wires#EnergyConsumer_p -->


    <owl:ObjectProperty rdf:about="https://w3id.org/netbeheer/referentiemodellen/IECCIM/TC57CIM/IEC61970/Base/Wires#EnergyConsumer_p">
        <rdfs:domain rdf:resource="https://w3id.org/netbeheer/referentiemodellen/IECCIM/TC57CIM/IEC61970/Base/Wires#EnergyConsumer"/>
        <rdfs:range rdf:resource="https://w3id.org/netbeheer/referentiemodellen/IECCIM/TC57CIM/IEC61970/Base/Domain#ActivePower"/>
        <rdfs:comment>Active power of the load. Load sign convention is used, i.e. positive sign means flow out from a node.
For voltage dependent loads the value is at rated voltage.
Starting value for a steady state solution.</rdfs:comment>
    </owl:ObjectProperty>
    


    <!-- https://w3id.org/netbeheer/referentiemodellen/IECCIM/TC57CIM/IEC61970/Base/Wires#EnergyConsumer_pfixed -->


    <owl:ObjectProperty rdf:about="https://w3id.org/netbeheer/referentiemodellen/IECCIM/TC57CIM/IEC61970/Base/Wires#EnergyConsumer_pfixed">
        <rdfs:domain rdf:resource="https://w3id.org/netbeheer/referentiemodellen/IECCIM/TC57CIM/IEC61970/Base/Wires#EnergyConsumer"/>
        <rdfs:range rdf:resource="https://w3id.org/netbeheer/referentiemodellen/IECCIM/TC57CIM/IEC61970/Base/Domain#ActivePower"/>
        <rdfs:comment>Active power of the load that is a fixed quantity. Load sign convention is used, i.e. positive sign means flow out from a node.
</rdfs:comment>
    </owl:ObjectProperty>
    


    <!-- https://w3id.org/netbeheer/referentiemodellen/IECCIM/TC57CIM/IEC61970/Base/Wires#EnergyConsumer_pfixedPct -->


    <owl:ObjectProperty rdf:about="https://w3id.org/netbeheer/referentiemodellen/IECCIM/TC57CIM/IEC61970/Base/Wires#EnergyConsumer_pfixedPct">
        <rdfs:domain rdf:resource="https://w3id.org/netbeheer/referentiemodellen/IECCIM/TC57CIM/IEC61970/Base/Wires#EnergyConsumer"/>
        <rdfs:range rdf:resource="https://w3id.org/netbeheer/referentiemodellen/IECCIM/TC57CIM/IEC61970/Base/Domain#PerCent"/>
        <rdfs:comment>Fixed active power as per cent of load group fixed active power. Load sign convention is used, i.e. positive sign means flow out from a node.
</rdfs:comment>
    </owl:ObjectProperty>
    


    <!-- https://w3id.org/netbeheer/referentiemodellen/IECCIM/TC57CIM/IEC61970/Base/Wires#EnergyConsumer_q -->


    <owl:ObjectProperty rdf:about="https://w3id.org/netbeheer/referentiemodellen/IECCIM/TC57CIM/IEC61970/Base/Wires#EnergyConsumer_q">
        <rdfs:domain rdf:resource="https://w3id.org/netbeheer/referentiemodellen/IECCIM/TC57CIM/IEC61970/Base/Wires#EnergyConsumer"/>
        <rdfs:range rdf:resource="https://w3id.org/netbeheer/referentiemodellen/IECCIM/TC57CIM/IEC61970/Base/Domain#ReactivePower"/>
        <rdfs:comment>Reactive power of the load. Load sign convention is used, i.e. positive sign means flow out from a node.
For voltage dependent loads the value is at rated voltage.
Starting value for a steady state solution.</rdfs:comment>
    </owl:ObjectProperty>
    


    <!-- https://w3id.org/netbeheer/referentiemodellen/IECCIM/TC57CIM/IEC61970/Base/Wires#EnergyConsumer_qfixed -->


    <owl:ObjectProperty rdf:about="https://w3id.org/netbeheer/referentiemodellen/IECCIM/TC57CIM/IEC61970/Base/Wires#EnergyConsumer_qfixed">
        <rdfs:domain rdf:resource="https://w3id.org/netbeheer/referentiemodellen/IECCIM/TC57CIM/IEC61970/Base/Wires#EnergyConsumer"/>
        <rdfs:range rdf:resource="https://w3id.org/netbeheer/referentiemodellen/IECCIM/TC57CIM/IEC61970/Base/Domain#ReactivePower"/>
        <rdfs:comment>Reactive power of the load that is a fixed quantity. Load sign convention is used, i.e. positive sign means flow out from a node.
</rdfs:comment>
    </owl:ObjectProperty>
    


    <!-- https://w3id.org/netbeheer/referentiemodellen/IECCIM/TC57CIM/IEC61970/Base/Wires#EnergyConsumer_qfixedPct -->


    <owl:ObjectProperty rdf:about="https://w3id.org/netbeheer/referentiemodellen/IECCIM/TC57CIM/IEC61970/Base/Wires#EnergyConsumer_qfixedPct">
        <rdfs:domain rdf:resource="https://w3id.org/netbeheer/referentiemodellen/IECCIM/TC57CIM/IEC61970/Base/Wires#EnergyConsumer"/>
        <rdfs:range rdf:resource="https://w3id.org/netbeheer/referentiemodellen/IECCIM/TC57CIM/IEC61970/Base/Domain#PerCent"/>
        <rdfs:comment>Fixed reactive power as per cent of load group fixed reactive power. Load sign convention is used, i.e. positive sign means flow out from a node.
</rdfs:comment>
    </owl:ObjectProperty>
    


    <!-- https://w3id.org/netbeheer/referentiemodellen/IECCIM/TC57CIM/IEC61970/Base/Wires#EnergySchedulingType_EnergySource -->


    <owl:ObjectProperty rdf:about="https://w3id.org/netbeheer/referentiemodellen/IECCIM/TC57CIM/IEC61970/Base/Wires#EnergySchedulingType_EnergySource">
        <owl:inverseOf rdf:resource="https://w3id.org/netbeheer/referentiemodellen/IECCIM/TC57CIM/IEC61970/Base/Wires#EnergySource_EnergySchedulingType"/>
        <rdfs:domain rdf:resource="https://w3id.org/netbeheer/referentiemodellen/IECCIM/TC57CIM/IEC61970/InfIEC61970/InfEnergySource#EnergySchedulingType"/>
        <rdfs:range rdf:resource="https://w3id.org/netbeheer/referentiemodellen/IECCIM/TC57CIM/IEC61970/Base/Wires#EnergySource"/>
        <rdfs:comment>Energy Source of a particular Energy Scheduling TypeEnergy Scheduling Type of an Energy Source</rdfs:comment>
    </owl:ObjectProperty>
    


    <!-- https://w3id.org/netbeheer/referentiemodellen/IECCIM/TC57CIM/IEC61970/Base/Wires#EnergySourceAction_EnergySource -->


    <owl:ObjectProperty rdf:about="https://w3id.org/netbeheer/referentiemodellen/IECCIM/TC57CIM/IEC61970/Base/Wires#EnergySourceAction_EnergySource">
        <rdfs:domain rdf:resource="https://w3id.org/netbeheer/referentiemodellen/IECCIM/TC57CIM/IEC61968/Operations#EnergySourceAction"/>
        <rdfs:range rdf:resource="https://w3id.org/netbeheer/referentiemodellen/IECCIM/TC57CIM/IEC61970/Base/Wires#EnergySource"/>
        <rdfs:comment>Action taken with this energy source.Energy source on which this action is taken.</rdfs:comment>
    </owl:ObjectProperty>
    


    <!-- https://w3id.org/netbeheer/referentiemodellen/IECCIM/TC57CIM/IEC61970/Base/Wires#EnergySourcePhase_EnergySource -->


    <owl:ObjectProperty rdf:about="https://w3id.org/netbeheer/referentiemodellen/IECCIM/TC57CIM/IEC61970/Base/Wires#EnergySourcePhase_EnergySource">
        <rdfs:domain rdf:resource="https://w3id.org/netbeheer/referentiemodellen/IECCIM/TC57CIM/IEC61970/Base/Wires#EnergySourcePhase"/>
        <rdfs:range rdf:resource="https://w3id.org/netbeheer/referentiemodellen/IECCIM/TC57CIM/IEC61970/Base/Wires#EnergySource"/>
        <rdfs:comment>The individual phase information of the energy source.The energy sourceto which the phase belongs.</rdfs:comment>
    </owl:ObjectProperty>
    


    <!-- https://w3id.org/netbeheer/referentiemodellen/IECCIM/TC57CIM/IEC61970/Base/Wires#EnergySource_EnergySchedulingType -->


    <owl:ObjectProperty rdf:about="https://w3id.org/netbeheer/referentiemodellen/IECCIM/TC57CIM/IEC61970/Base/Wires#EnergySource_EnergySchedulingType">
        <rdfs:domain rdf:resource="https://w3id.org/netbeheer/referentiemodellen/IECCIM/TC57CIM/IEC61970/Base/Wires#EnergySource"/>
        <rdfs:range rdf:resource="https://w3id.org/netbeheer/referentiemodellen/IECCIM/TC57CIM/IEC61970/InfIEC61970/InfEnergySource#EnergySchedulingType"/>
        <rdfs:comment>Energy Source of a particular Energy Scheduling TypeEnergy Scheduling Type of an Energy Source</rdfs:comment>
    </owl:ObjectProperty>
    


    <!-- https://w3id.org/netbeheer/referentiemodellen/IECCIM/TC57CIM/IEC61970/Base/Wires#EnergySource_EnergySourceAction -->


    <owl:ObjectProperty rdf:about="https://w3id.org/netbeheer/referentiemodellen/IECCIM/TC57CIM/IEC61970/Base/Wires#EnergySource_EnergySourceAction">
        <owl:inverseOf rdf:resource="https://w3id.org/netbeheer/referentiemodellen/IECCIM/TC57CIM/IEC61970/Base/Wires#EnergySourceAction_EnergySource"/>
        <rdfs:domain rdf:resource="https://w3id.org/netbeheer/referentiemodellen/IECCIM/TC57CIM/IEC61970/Base/Wires#EnergySource"/>
        <rdfs:range rdf:resource="https://w3id.org/netbeheer/referentiemodellen/IECCIM/TC57CIM/IEC61968/Operations#EnergySourceAction"/>
        <rdfs:comment>Action taken with this energy source.Energy source on which this action is taken.</rdfs:comment>
    </owl:ObjectProperty>
    


    <!-- https://w3id.org/netbeheer/referentiemodellen/IECCIM/TC57CIM/IEC61970/Base/Wires#EnergySource_EnergySourcePhase -->


    <owl:ObjectProperty rdf:about="https://w3id.org/netbeheer/referentiemodellen/IECCIM/TC57CIM/IEC61970/Base/Wires#EnergySource_EnergySourcePhase">
        <owl:inverseOf rdf:resource="https://w3id.org/netbeheer/referentiemodellen/IECCIM/TC57CIM/IEC61970/Base/Wires#EnergySourcePhase_EnergySource"/>
        <rdf:type rdf:resource="http://www.w3.org/2002/07/owl#FunctionalProperty"/>
        <rdfs:domain rdf:resource="https://w3id.org/netbeheer/referentiemodellen/IECCIM/TC57CIM/IEC61970/Base/Wires#EnergySource"/>
        <rdfs:range rdf:resource="https://w3id.org/netbeheer/referentiemodellen/IECCIM/TC57CIM/IEC61970/Base/Wires#EnergySourcePhase"/>
        <rdfs:comment>The individual phase information of the energy source.The energy sourceto which the phase belongs.</rdfs:comment>
    </owl:ObjectProperty>
    


    <!-- https://w3id.org/netbeheer/referentiemodellen/IECCIM/TC57CIM/IEC61970/Base/Wires#EnergySource_WindTurbineType3or4Dynamics -->


    <owl:ObjectProperty rdf:about="https://w3id.org/netbeheer/referentiemodellen/IECCIM/TC57CIM/IEC61970/Base/Wires#EnergySource_WindTurbineType3or4Dynamics">
        <owl:inverseOf rdf:resource="https://w3id.org/netbeheer/referentiemodellen/IECCIM/TC57CIM/IEC61970/Base/Wires#WindTurbineType3or4Dynamics_EnergySource"/>
        <rdf:type rdf:resource="http://www.w3.org/2002/07/owl#FunctionalProperty"/>
        <rdfs:domain rdf:resource="https://w3id.org/netbeheer/referentiemodellen/IECCIM/TC57CIM/IEC61970/Base/Wires#EnergySource"/>
        <rdfs:range rdf:resource="https://w3id.org/netbeheer/referentiemodellen/IECCIM/TC57CIM/IEC61970/Dynamics/StandardModels/WindDynamics#WindTurbineType3or4Dynamics"/>
        <rdfs:comment>Wind generator Type 3 or 4 dynamics model associated with this energy source.Energy Source (current source) with which this wind Type 3 or 4 dynamics model is asoociated.</rdfs:comment>
    </owl:ObjectProperty>
    


    <!-- https://w3id.org/netbeheer/referentiemodellen/IECCIM/TC57CIM/IEC61970/Base/Wires#EnergySource_activePower -->


    <owl:ObjectProperty rdf:about="https://w3id.org/netbeheer/referentiemodellen/IECCIM/TC57CIM/IEC61970/Base/Wires#EnergySource_activePower">
        <rdfs:domain rdf:resource="https://w3id.org/netbeheer/referentiemodellen/IECCIM/TC57CIM/IEC61970/Base/Wires#EnergySource"/>
        <rdfs:range rdf:resource="https://w3id.org/netbeheer/referentiemodellen/IECCIM/TC57CIM/IEC61970/Base/Domain#ActivePower"/>
        <rdfs:comment>High voltage source active injection. Load sign convention is used, i.e. positive sign means flow out from a node.
Starting value for steady state solutions.</rdfs:comment>
    </owl:ObjectProperty>
    


    <!-- https://w3id.org/netbeheer/referentiemodellen/IECCIM/TC57CIM/IEC61970/Base/Wires#EnergySource_nominalVoltage -->


    <owl:ObjectProperty rdf:about="https://w3id.org/netbeheer/referentiemodellen/IECCIM/TC57CIM/IEC61970/Base/Wires#EnergySource_nominalVoltage">
        <rdfs:domain rdf:resource="https://w3id.org/netbeheer/referentiemodellen/IECCIM/TC57CIM/IEC61970/Base/Wires#EnergySource"/>
        <rdfs:range rdf:resource="https://w3id.org/netbeheer/referentiemodellen/IECCIM/TC57CIM/IEC61970/Base/Domain#Voltage"/>
        <rdfs:comment>Phase-to-phase nominal voltage.</rdfs:comment>
    </owl:ObjectProperty>
    


    <!-- https://w3id.org/netbeheer/referentiemodellen/IECCIM/TC57CIM/IEC61970/Base/Wires#EnergySource_r -->


    <owl:ObjectProperty rdf:about="https://w3id.org/netbeheer/referentiemodellen/IECCIM/TC57CIM/IEC61970/Base/Wires#EnergySource_r">
        <rdfs:domain rdf:resource="https://w3id.org/netbeheer/referentiemodellen/IECCIM/TC57CIM/IEC61970/Base/Wires#EnergySource"/>
        <rdfs:range rdf:resource="https://w3id.org/netbeheer/referentiemodellen/IECCIM/TC57CIM/IEC61970/Base/Domain#Resistance"/>
        <rdfs:comment>Positive sequence Thevenin resistance.</rdfs:comment>
    </owl:ObjectProperty>
    


    <!-- https://w3id.org/netbeheer/referentiemodellen/IECCIM/TC57CIM/IEC61970/Base/Wires#EnergySource_r0 -->


    <owl:ObjectProperty rdf:about="https://w3id.org/netbeheer/referentiemodellen/IECCIM/TC57CIM/IEC61970/Base/Wires#EnergySource_r0">
        <rdfs:domain rdf:resource="https://w3id.org/netbeheer/referentiemodellen/IECCIM/TC57CIM/IEC61970/Base/Wires#EnergySource"/>
        <rdfs:range rdf:resource="https://w3id.org/netbeheer/referentiemodellen/IECCIM/TC57CIM/IEC61970/Base/Domain#Resistance"/>
        <rdfs:comment>Zero sequence Thevenin resistance.</rdfs:comment>
    </owl:ObjectProperty>
    


    <!-- https://w3id.org/netbeheer/referentiemodellen/IECCIM/TC57CIM/IEC61970/Base/Wires#EnergySource_reactivePower -->


    <owl:ObjectProperty rdf:about="https://w3id.org/netbeheer/referentiemodellen/IECCIM/TC57CIM/IEC61970/Base/Wires#EnergySource_reactivePower">
        <rdfs:domain rdf:resource="https://w3id.org/netbeheer/referentiemodellen/IECCIM/TC57CIM/IEC61970/Base/Wires#EnergySource"/>
        <rdfs:range rdf:resource="https://w3id.org/netbeheer/referentiemodellen/IECCIM/TC57CIM/IEC61970/Base/Domain#ReactivePower"/>
        <rdfs:comment>High voltage source reactive injection. Load sign convention is used, i.e. positive sign means flow out from a node.
Starting value for steady state solutions.</rdfs:comment>
    </owl:ObjectProperty>
    


    <!-- https://w3id.org/netbeheer/referentiemodellen/IECCIM/TC57CIM/IEC61970/Base/Wires#EnergySource_rn -->


    <owl:ObjectProperty rdf:about="https://w3id.org/netbeheer/referentiemodellen/IECCIM/TC57CIM/IEC61970/Base/Wires#EnergySource_rn">
        <rdfs:domain rdf:resource="https://w3id.org/netbeheer/referentiemodellen/IECCIM/TC57CIM/IEC61970/Base/Wires#EnergySource"/>
        <rdfs:range rdf:resource="https://w3id.org/netbeheer/referentiemodellen/IECCIM/TC57CIM/IEC61970/Base/Domain#Resistance"/>
        <rdfs:comment>Negative sequence Thevenin resistance.</rdfs:comment>
    </owl:ObjectProperty>
    


    <!-- https://w3id.org/netbeheer/referentiemodellen/IECCIM/TC57CIM/IEC61970/Base/Wires#EnergySource_voltageAngle -->


    <owl:ObjectProperty rdf:about="https://w3id.org/netbeheer/referentiemodellen/IECCIM/TC57CIM/IEC61970/Base/Wires#EnergySource_voltageAngle">
        <rdfs:domain rdf:resource="https://w3id.org/netbeheer/referentiemodellen/IECCIM/TC57CIM/IEC61970/Base/Wires#EnergySource"/>
        <rdfs:range rdf:resource="https://w3id.org/netbeheer/referentiemodellen/IECCIM/TC57CIM/IEC61970/Base/Domain#AngleRadians"/>
        <rdfs:comment>Phase angle of a-phase open circuit.</rdfs:comment>
    </owl:ObjectProperty>
    


    <!-- https://w3id.org/netbeheer/referentiemodellen/IECCIM/TC57CIM/IEC61970/Base/Wires#EnergySource_voltageMagnitude -->


    <owl:ObjectProperty rdf:about="https://w3id.org/netbeheer/referentiemodellen/IECCIM/TC57CIM/IEC61970/Base/Wires#EnergySource_voltageMagnitude">
        <rdfs:domain rdf:resource="https://w3id.org/netbeheer/referentiemodellen/IECCIM/TC57CIM/IEC61970/Base/Wires#EnergySource"/>
        <rdfs:range rdf:resource="https://w3id.org/netbeheer/referentiemodellen/IECCIM/TC57CIM/IEC61970/Base/Domain#Voltage"/>
        <rdfs:comment>Phase-to-phase open circuit voltage magnitude.</rdfs:comment>
    </owl:ObjectProperty>
    


    <!-- https://w3id.org/netbeheer/referentiemodellen/IECCIM/TC57CIM/IEC61970/Base/Wires#EnergySource_x -->


    <owl:ObjectProperty rdf:about="https://w3id.org/netbeheer/referentiemodellen/IECCIM/TC57CIM/IEC61970/Base/Wires#EnergySource_x">
        <rdfs:domain rdf:resource="https://w3id.org/netbeheer/referentiemodellen/IECCIM/TC57CIM/IEC61970/Base/Wires#EnergySource"/>
        <rdfs:range rdf:resource="https://w3id.org/netbeheer/referentiemodellen/IECCIM/TC57CIM/IEC61970/Base/Domain#Reactance"/>
        <rdfs:comment>Positive sequence Thevenin reactance.</rdfs:comment>
    </owl:ObjectProperty>
    


    <!-- https://w3id.org/netbeheer/referentiemodellen/IECCIM/TC57CIM/IEC61970/Base/Wires#EnergySource_x0 -->


    <owl:ObjectProperty rdf:about="https://w3id.org/netbeheer/referentiemodellen/IECCIM/TC57CIM/IEC61970/Base/Wires#EnergySource_x0">
        <rdfs:domain rdf:resource="https://w3id.org/netbeheer/referentiemodellen/IECCIM/TC57CIM/IEC61970/Base/Wires#EnergySource"/>
        <rdfs:range rdf:resource="https://w3id.org/netbeheer/referentiemodellen/IECCIM/TC57CIM/IEC61970/Base/Domain#Reactance"/>
        <rdfs:comment>Zero sequence Thevenin reactance.</rdfs:comment>
    </owl:ObjectProperty>
    


    <!-- https://w3id.org/netbeheer/referentiemodellen/IECCIM/TC57CIM/IEC61970/Base/Wires#EnergySource_xn -->


    <owl:ObjectProperty rdf:about="https://w3id.org/netbeheer/referentiemodellen/IECCIM/TC57CIM/IEC61970/Base/Wires#EnergySource_xn">
        <rdfs:domain rdf:resource="https://w3id.org/netbeheer/referentiemodellen/IECCIM/TC57CIM/IEC61970/Base/Wires#EnergySource"/>
        <rdfs:range rdf:resource="https://w3id.org/netbeheer/referentiemodellen/IECCIM/TC57CIM/IEC61970/Base/Domain#Reactance"/>
        <rdfs:comment>Negative sequence Thevenin reactance.</rdfs:comment>
    </owl:ObjectProperty>
    


    <!-- https://w3id.org/netbeheer/referentiemodellen/IECCIM/TC57CIM/IEC61970/Base/Wires#EquivalentInjection_ReactiveCapabilityCurve -->


    <owl:ObjectProperty rdf:about="https://w3id.org/netbeheer/referentiemodellen/IECCIM/TC57CIM/IEC61970/Base/Wires#EquivalentInjection_ReactiveCapabilityCurve">
        <owl:inverseOf rdf:resource="https://w3id.org/netbeheer/referentiemodellen/IECCIM/TC57CIM/IEC61970/Base/Wires#ReactiveCapabilityCurve_EquivalentInjection"/>
        <rdfs:domain rdf:resource="https://w3id.org/netbeheer/referentiemodellen/IECCIM/TC57CIM/IEC61970/Base/Equivalents#EquivalentInjection"/>
        <rdfs:range rdf:resource="https://w3id.org/netbeheer/referentiemodellen/IECCIM/TC57CIM/IEC61970/Base/Wires#ReactiveCapabilityCurve"/>
        <rdfs:comment>The reactive capability curve used by this equivalent injection.The equivalent injection using this reactive capability curve.</rdfs:comment>
    </owl:ObjectProperty>
    


    <!-- https://w3id.org/netbeheer/referentiemodellen/IECCIM/TC57CIM/IEC61970/Base/Wires#ExternalNetworkInjection_governorSCD -->


    <owl:ObjectProperty rdf:about="https://w3id.org/netbeheer/referentiemodellen/IECCIM/TC57CIM/IEC61970/Base/Wires#ExternalNetworkInjection_governorSCD">
        <rdfs:domain rdf:resource="https://w3id.org/netbeheer/referentiemodellen/IECCIM/TC57CIM/IEC61970/Base/Wires#ExternalNetworkInjection"/>
        <rdfs:range rdf:resource="https://w3id.org/netbeheer/referentiemodellen/IECCIM/TC57CIM/IEC61970/Base/Domain#ActivePowerPerFrequency"/>
        <rdfs:comment>Power Frequency Bias. This is the change in power injection divided by the change in frequency and negated.  A positive value of the power frequency bias provides additional power injection upon a drop in frequency.</rdfs:comment>
    </owl:ObjectProperty>
    


    <!-- https://w3id.org/netbeheer/referentiemodellen/IECCIM/TC57CIM/IEC61970/Base/Wires#ExternalNetworkInjection_maxInitialSymShCCurrent -->


    <owl:ObjectProperty rdf:about="https://w3id.org/netbeheer/referentiemodellen/IECCIM/TC57CIM/IEC61970/Base/Wires#ExternalNetworkInjection_maxInitialSymShCCurrent">
        <rdfs:domain rdf:resource="https://w3id.org/netbeheer/referentiemodellen/IECCIM/TC57CIM/IEC61970/Base/Wires#ExternalNetworkInjection"/>
        <rdfs:range rdf:resource="https://w3id.org/netbeheer/referentiemodellen/IECCIM/TC57CIM/IEC61970/Base/Domain#CurrentFlow"/>
        <rdfs:comment>  Maximum initial symmetrical short-circuit currents (Ik&quot; max) in A (Ik&quot; = Sk&quot;/(SQRT(3) Un)). Used for short circuit data exchange according to IEC 60909
</rdfs:comment>
    </owl:ObjectProperty>
    


    <!-- https://w3id.org/netbeheer/referentiemodellen/IECCIM/TC57CIM/IEC61970/Base/Wires#ExternalNetworkInjection_maxP -->


    <owl:ObjectProperty rdf:about="https://w3id.org/netbeheer/referentiemodellen/IECCIM/TC57CIM/IEC61970/Base/Wires#ExternalNetworkInjection_maxP">
        <rdfs:domain rdf:resource="https://w3id.org/netbeheer/referentiemodellen/IECCIM/TC57CIM/IEC61970/Base/Wires#ExternalNetworkInjection"/>
        <rdfs:range rdf:resource="https://w3id.org/netbeheer/referentiemodellen/IECCIM/TC57CIM/IEC61970/Base/Domain#ActivePower"/>
        <rdfs:comment>Maximum active power of the injection.</rdfs:comment>
    </owl:ObjectProperty>
    


    <!-- https://w3id.org/netbeheer/referentiemodellen/IECCIM/TC57CIM/IEC61970/Base/Wires#ExternalNetworkInjection_maxQ -->


    <owl:ObjectProperty rdf:about="https://w3id.org/netbeheer/referentiemodellen/IECCIM/TC57CIM/IEC61970/Base/Wires#ExternalNetworkInjection_maxQ">
        <rdfs:domain rdf:resource="https://w3id.org/netbeheer/referentiemodellen/IECCIM/TC57CIM/IEC61970/Base/Wires#ExternalNetworkInjection"/>
        <rdfs:range rdf:resource="https://w3id.org/netbeheer/referentiemodellen/IECCIM/TC57CIM/IEC61970/Base/Domain#ReactivePower"/>
        <rdfs:comment>Not for short circuit modelling; It is used for modelling of infeed for load flow exchange. If maxQ and minQ are not used ReactiveCapabilityCurve can be used 
</rdfs:comment>
    </owl:ObjectProperty>
    


    <!-- https://w3id.org/netbeheer/referentiemodellen/IECCIM/TC57CIM/IEC61970/Base/Wires#ExternalNetworkInjection_minInitialSymShCCurrent -->


    <owl:ObjectProperty rdf:about="https://w3id.org/netbeheer/referentiemodellen/IECCIM/TC57CIM/IEC61970/Base/Wires#ExternalNetworkInjection_minInitialSymShCCurrent">
        <rdfs:domain rdf:resource="https://w3id.org/netbeheer/referentiemodellen/IECCIM/TC57CIM/IEC61970/Base/Wires#ExternalNetworkInjection"/>
        <rdfs:range rdf:resource="https://w3id.org/netbeheer/referentiemodellen/IECCIM/TC57CIM/IEC61970/Base/Domain#CurrentFlow"/>
        <rdfs:comment>Minimum initial symmetrical short-circuit currents (Ik&quot; min) in A (Ik&quot; = Sk&quot;/(SQRT(3) Un)). Used for short circuit data exchange according to IEC 60909
</rdfs:comment>
    </owl:ObjectProperty>
    


    <!-- https://w3id.org/netbeheer/referentiemodellen/IECCIM/TC57CIM/IEC61970/Base/Wires#ExternalNetworkInjection_minP -->


    <owl:ObjectProperty rdf:about="https://w3id.org/netbeheer/referentiemodellen/IECCIM/TC57CIM/IEC61970/Base/Wires#ExternalNetworkInjection_minP">
        <rdfs:domain rdf:resource="https://w3id.org/netbeheer/referentiemodellen/IECCIM/TC57CIM/IEC61970/Base/Wires#ExternalNetworkInjection"/>
        <rdfs:range rdf:resource="https://w3id.org/netbeheer/referentiemodellen/IECCIM/TC57CIM/IEC61970/Base/Domain#ActivePower"/>
        <rdfs:comment>Minimum active power of the injection.</rdfs:comment>
    </owl:ObjectProperty>
    


    <!-- https://w3id.org/netbeheer/referentiemodellen/IECCIM/TC57CIM/IEC61970/Base/Wires#ExternalNetworkInjection_minQ -->


    <owl:ObjectProperty rdf:about="https://w3id.org/netbeheer/referentiemodellen/IECCIM/TC57CIM/IEC61970/Base/Wires#ExternalNetworkInjection_minQ">
        <rdfs:domain rdf:resource="https://w3id.org/netbeheer/referentiemodellen/IECCIM/TC57CIM/IEC61970/Base/Wires#ExternalNetworkInjection"/>
        <rdfs:range rdf:resource="https://w3id.org/netbeheer/referentiemodellen/IECCIM/TC57CIM/IEC61970/Base/Domain#ReactivePower"/>
        <rdfs:comment>Not for short circuit modelling; It is used for modelling of infeed for load flow exchange. If maxQ and minQ are not used ReactiveCapabilityCurve can be used
</rdfs:comment>
    </owl:ObjectProperty>
    


    <!-- https://w3id.org/netbeheer/referentiemodellen/IECCIM/TC57CIM/IEC61970/Base/Wires#ExternalNetworkInjection_p -->


    <owl:ObjectProperty rdf:about="https://w3id.org/netbeheer/referentiemodellen/IECCIM/TC57CIM/IEC61970/Base/Wires#ExternalNetworkInjection_p">
        <rdfs:domain rdf:resource="https://w3id.org/netbeheer/referentiemodellen/IECCIM/TC57CIM/IEC61970/Base/Wires#ExternalNetworkInjection"/>
        <rdfs:range rdf:resource="https://w3id.org/netbeheer/referentiemodellen/IECCIM/TC57CIM/IEC61970/Base/Domain#ActivePower"/>
        <rdfs:comment>Active power injection. Load sign convention is used, i.e. positive sign means flow out from a node.
Starting value for steady state solutions.</rdfs:comment>
    </owl:ObjectProperty>
    


    <!-- https://w3id.org/netbeheer/referentiemodellen/IECCIM/TC57CIM/IEC61970/Base/Wires#ExternalNetworkInjection_q -->


    <owl:ObjectProperty rdf:about="https://w3id.org/netbeheer/referentiemodellen/IECCIM/TC57CIM/IEC61970/Base/Wires#ExternalNetworkInjection_q">
        <rdfs:domain rdf:resource="https://w3id.org/netbeheer/referentiemodellen/IECCIM/TC57CIM/IEC61970/Base/Wires#ExternalNetworkInjection"/>
        <rdfs:range rdf:resource="https://w3id.org/netbeheer/referentiemodellen/IECCIM/TC57CIM/IEC61970/Base/Domain#ReactivePower"/>
        <rdfs:comment>Reactive power injection. Load sign convention is used, i.e. positive sign means flow out from a node.
Starting value for steady state solutions.</rdfs:comment>
    </owl:ObjectProperty>
    


    <!-- https://w3id.org/netbeheer/referentiemodellen/IECCIM/TC57CIM/IEC61970/Base/Wires#ExternalNetworkInjection_voltageFactor -->


    <owl:ObjectProperty rdf:about="https://w3id.org/netbeheer/referentiemodellen/IECCIM/TC57CIM/IEC61970/Base/Wires#ExternalNetworkInjection_voltageFactor">
        <rdfs:domain rdf:resource="https://w3id.org/netbeheer/referentiemodellen/IECCIM/TC57CIM/IEC61970/Base/Wires#ExternalNetworkInjection"/>
        <rdfs:range rdf:resource="https://w3id.org/netbeheer/referentiemodellen/IECCIM/TC57CIM/IEC61970/Base/Domain#PU"/>
        <rdfs:comment>Voltage factor in pu, which was used to calculate short-circuit current Ik&quot; and power Sk&quot;.
</rdfs:comment>
    </owl:ObjectProperty>
    


    <!-- https://w3id.org/netbeheer/referentiemodellen/IECCIM/TC57CIM/IEC61970/Base/Wires#FrequencyConverter_frequency -->


    <owl:ObjectProperty rdf:about="https://w3id.org/netbeheer/referentiemodellen/IECCIM/TC57CIM/IEC61970/Base/Wires#FrequencyConverter_frequency">
        <rdfs:domain rdf:resource="https://w3id.org/netbeheer/referentiemodellen/IECCIM/TC57CIM/IEC61970/Base/Wires#FrequencyConverter"/>
        <rdfs:range rdf:resource="https://w3id.org/netbeheer/referentiemodellen/IECCIM/TC57CIM/IEC61970/Base/Domain#Frequency"/>
        <rdfs:comment>Frequency on the AC side.</rdfs:comment>
    </owl:ObjectProperty>
    


    <!-- https://w3id.org/netbeheer/referentiemodellen/IECCIM/TC57CIM/IEC61970/Base/Wires#FrequencyConverter_maxP -->


    <owl:ObjectProperty rdf:about="https://w3id.org/netbeheer/referentiemodellen/IECCIM/TC57CIM/IEC61970/Base/Wires#FrequencyConverter_maxP">
        <rdfs:domain rdf:resource="https://w3id.org/netbeheer/referentiemodellen/IECCIM/TC57CIM/IEC61970/Base/Wires#FrequencyConverter"/>
        <rdfs:range rdf:resource="https://w3id.org/netbeheer/referentiemodellen/IECCIM/TC57CIM/IEC61970/Base/Domain#ActivePower"/>
        <rdfs:comment>The maximum active power on the DC side at which the frequence converter should operate.</rdfs:comment>
    </owl:ObjectProperty>
    


    <!-- https://w3id.org/netbeheer/referentiemodellen/IECCIM/TC57CIM/IEC61970/Base/Wires#FrequencyConverter_maxU -->


    <owl:ObjectProperty rdf:about="https://w3id.org/netbeheer/referentiemodellen/IECCIM/TC57CIM/IEC61970/Base/Wires#FrequencyConverter_maxU">
        <rdfs:domain rdf:resource="https://w3id.org/netbeheer/referentiemodellen/IECCIM/TC57CIM/IEC61970/Base/Wires#FrequencyConverter"/>
        <rdfs:range rdf:resource="https://w3id.org/netbeheer/referentiemodellen/IECCIM/TC57CIM/IEC61970/Base/Domain#Voltage"/>
        <rdfs:comment>The maximum voltage on the DC side at which the frequency converter should operate.</rdfs:comment>
    </owl:ObjectProperty>
    


    <!-- https://w3id.org/netbeheer/referentiemodellen/IECCIM/TC57CIM/IEC61970/Base/Wires#FrequencyConverter_minP -->


    <owl:ObjectProperty rdf:about="https://w3id.org/netbeheer/referentiemodellen/IECCIM/TC57CIM/IEC61970/Base/Wires#FrequencyConverter_minP">
        <rdfs:domain rdf:resource="https://w3id.org/netbeheer/referentiemodellen/IECCIM/TC57CIM/IEC61970/Base/Wires#FrequencyConverter"/>
        <rdfs:range rdf:resource="https://w3id.org/netbeheer/referentiemodellen/IECCIM/TC57CIM/IEC61970/Base/Domain#ActivePower"/>
        <rdfs:comment>The minimum active power on the DC side at which the frequence converter should operate.</rdfs:comment>
    </owl:ObjectProperty>
    


    <!-- https://w3id.org/netbeheer/referentiemodellen/IECCIM/TC57CIM/IEC61970/Base/Wires#FrequencyConverter_minU -->


    <owl:ObjectProperty rdf:about="https://w3id.org/netbeheer/referentiemodellen/IECCIM/TC57CIM/IEC61970/Base/Wires#FrequencyConverter_minU">
        <rdfs:domain rdf:resource="https://w3id.org/netbeheer/referentiemodellen/IECCIM/TC57CIM/IEC61970/Base/Wires#FrequencyConverter"/>
        <rdfs:range rdf:resource="https://w3id.org/netbeheer/referentiemodellen/IECCIM/TC57CIM/IEC61970/Base/Domain#Voltage"/>
        <rdfs:comment>The minimum voltage on the DC side at which the frequency converter should operate.</rdfs:comment>
    </owl:ObjectProperty>
    


    <!-- https://w3id.org/netbeheer/referentiemodellen/IECCIM/TC57CIM/IEC61970/Base/Wires#GeneratingUnit_RotatingMachine -->


    <owl:ObjectProperty rdf:about="https://w3id.org/netbeheer/referentiemodellen/IECCIM/TC57CIM/IEC61970/Base/Wires#GeneratingUnit_RotatingMachine">
        <rdfs:domain rdf:resource="https://w3id.org/netbeheer/referentiemodellen/IECCIM/TC57CIM/IEC61970/Base/Generation/Production#GeneratingUnit"/>
        <rdfs:range rdf:resource="https://w3id.org/netbeheer/referentiemodellen/IECCIM/TC57CIM/IEC61970/Base/Wires#RotatingMachine"/>
        <rdfs:comment>A synchronous machine may operate as a generator and as such becomes a member of a generating unit.A synchronous machine may operate as a generator and as such becomes a member of a generating unit.</rdfs:comment>
    </owl:ObjectProperty>
    


    <!-- https://w3id.org/netbeheer/referentiemodellen/IECCIM/TC57CIM/IEC61970/Base/Wires#GroundAction_AlongACLineSegment -->


    <owl:ObjectProperty rdf:about="https://w3id.org/netbeheer/referentiemodellen/IECCIM/TC57CIM/IEC61970/Base/Wires#GroundAction_AlongACLineSegment">
        <rdfs:domain rdf:resource="https://w3id.org/netbeheer/referentiemodellen/IECCIM/TC57CIM/IEC61968/Operations#GroundAction"/>
        <rdfs:range rdf:resource="https://w3id.org/netbeheer/referentiemodellen/IECCIM/TC57CIM/IEC61970/Base/Wires#ACLineSegment"/>
        <rdfs:comment>Ground action involving clamp usage (for the case when the ground is applied along the line segment instead of at its terminals).The line segment that this ground action will affect. This is the only way to access relationship to clamp in case the ground needs to be placed along the line segment.</rdfs:comment>
    </owl:ObjectProperty>
    


    <!-- https://w3id.org/netbeheer/referentiemodellen/IECCIM/TC57CIM/IEC61970/Base/Wires#GroundAction_Ground -->


    <owl:ObjectProperty rdf:about="https://w3id.org/netbeheer/referentiemodellen/IECCIM/TC57CIM/IEC61970/Base/Wires#GroundAction_Ground">
        <rdfs:domain rdf:resource="https://w3id.org/netbeheer/referentiemodellen/IECCIM/TC57CIM/IEC61968/Operations#GroundAction"/>
        <rdfs:range rdf:resource="https://w3id.org/netbeheer/referentiemodellen/IECCIM/TC57CIM/IEC61970/Base/Wires#Ground"/>
        <rdfs:comment>Action taken with this ground.Ground on which this action is taken.</rdfs:comment>
    </owl:ObjectProperty>
    


    <!-- https://w3id.org/netbeheer/referentiemodellen/IECCIM/TC57CIM/IEC61970/Base/Wires#Ground_GroundAction -->


    <owl:ObjectProperty rdf:about="https://w3id.org/netbeheer/referentiemodellen/IECCIM/TC57CIM/IEC61970/Base/Wires#Ground_GroundAction">
        <owl:inverseOf rdf:resource="https://w3id.org/netbeheer/referentiemodellen/IECCIM/TC57CIM/IEC61970/Base/Wires#GroundAction_Ground"/>
        <rdfs:domain rdf:resource="https://w3id.org/netbeheer/referentiemodellen/IECCIM/TC57CIM/IEC61970/Base/Wires#Ground"/>
        <rdfs:range rdf:resource="https://w3id.org/netbeheer/referentiemodellen/IECCIM/TC57CIM/IEC61968/Operations#GroundAction"/>
        <rdfs:comment>Action taken with this ground.Ground on which this action is taken.</rdfs:comment>
    </owl:ObjectProperty>
    


    <!-- https://w3id.org/netbeheer/referentiemodellen/IECCIM/TC57CIM/IEC61970/Base/Wires#GroundingImpedance_x -->


    <owl:ObjectProperty rdf:about="https://w3id.org/netbeheer/referentiemodellen/IECCIM/TC57CIM/IEC61970/Base/Wires#GroundingImpedance_x">
        <rdfs:domain rdf:resource="https://w3id.org/netbeheer/referentiemodellen/IECCIM/TC57CIM/IEC61970/Base/Wires#GroundingImpedance"/>
        <rdfs:range rdf:resource="https://w3id.org/netbeheer/referentiemodellen/IECCIM/TC57CIM/IEC61970/Base/Domain#Reactance"/>
        <rdfs:comment>Reactance of device.</rdfs:comment>
    </owl:ObjectProperty>
    


    <!-- https://w3id.org/netbeheer/referentiemodellen/IECCIM/TC57CIM/IEC61970/Base/Wires#HydroPump_RotatingMachine -->


    <owl:ObjectProperty rdf:about="https://w3id.org/netbeheer/referentiemodellen/IECCIM/TC57CIM/IEC61970/Base/Wires#HydroPump_RotatingMachine">
        <owl:inverseOf rdf:resource="https://w3id.org/netbeheer/referentiemodellen/IECCIM/TC57CIM/IEC61970/Base/Wires#RotatingMachine_HydroPump"/>
        <rdfs:domain rdf:resource="https://w3id.org/netbeheer/referentiemodellen/IECCIM/TC57CIM/IEC61970/Base/Generation/Production#HydroPump"/>
        <rdfs:range rdf:resource="https://w3id.org/netbeheer/referentiemodellen/IECCIM/TC57CIM/IEC61970/Base/Wires#RotatingMachine"/>
        <rdfs:comment>The synchronous machine drives the turbine which moves the water from a low elevation to a higher elevation. The direction of machine rotation for pumping may or may not be the same as for generating.The synchronous machine drives the turbine which moves the water from a low elevation to a higher elevation. The direction of machine rotation for pumping may or may not be the same as for generating.</rdfs:comment>
    </owl:ObjectProperty>
    


    <!-- https://w3id.org/netbeheer/referentiemodellen/IECCIM/TC57CIM/IEC61970/Base/Wires#JumperAction_AlongACLineSegments -->


    <owl:ObjectProperty rdf:about="https://w3id.org/netbeheer/referentiemodellen/IECCIM/TC57CIM/IEC61970/Base/Wires#JumperAction_AlongACLineSegments">
        <rdfs:domain rdf:resource="https://w3id.org/netbeheer/referentiemodellen/IECCIM/TC57CIM/IEC61968/Operations#JumperAction"/>
        <rdfs:range rdf:resource="https://w3id.org/netbeheer/referentiemodellen/IECCIM/TC57CIM/IEC61970/Base/Wires#ACLineSegment"/>
        <rdfs:comment>Jumper action involving clamp usage (for the case when the jumper is applied along the line segment instead of at its terminals).The line segment that this jumper action will affect. This is the only way to access relationship to clamp in case the jumper needs to connect along the line segment.</rdfs:comment>
    </owl:ObjectProperty>
    


    <!-- https://w3id.org/netbeheer/referentiemodellen/IECCIM/TC57CIM/IEC61970/Base/Wires#JumperAction_Jumper -->


    <owl:ObjectProperty rdf:about="https://w3id.org/netbeheer/referentiemodellen/IECCIM/TC57CIM/IEC61970/Base/Wires#JumperAction_Jumper">
        <rdfs:domain rdf:resource="https://w3id.org/netbeheer/referentiemodellen/IECCIM/TC57CIM/IEC61968/Operations#JumperAction"/>
        <rdfs:range rdf:resource="https://w3id.org/netbeheer/referentiemodellen/IECCIM/TC57CIM/IEC61970/Base/Wires#Jumper"/>
        <rdfs:comment>Action taken with this jumper.Jumper on which this action is taken.</rdfs:comment>
    </owl:ObjectProperty>
    


    <!-- https://w3id.org/netbeheer/referentiemodellen/IECCIM/TC57CIM/IEC61970/Base/Wires#Jumper_JumperAction -->


    <owl:ObjectProperty rdf:about="https://w3id.org/netbeheer/referentiemodellen/IECCIM/TC57CIM/IEC61970/Base/Wires#Jumper_JumperAction">
        <owl:inverseOf rdf:resource="https://w3id.org/netbeheer/referentiemodellen/IECCIM/TC57CIM/IEC61970/Base/Wires#JumperAction_Jumper"/>
        <rdfs:domain rdf:resource="https://w3id.org/netbeheer/referentiemodellen/IECCIM/TC57CIM/IEC61970/Base/Wires#Jumper"/>
        <rdfs:range rdf:resource="https://w3id.org/netbeheer/referentiemodellen/IECCIM/TC57CIM/IEC61968/Operations#JumperAction"/>
        <rdfs:comment>Action taken with this jumper.Jumper on which this action is taken.</rdfs:comment>
    </owl:ObjectProperty>
    


    <!-- https://w3id.org/netbeheer/referentiemodellen/IECCIM/TC57CIM/IEC61970/Base/Wires#LinearShuntCompensatorPhase_bPerSection -->


    <owl:ObjectProperty rdf:about="https://w3id.org/netbeheer/referentiemodellen/IECCIM/TC57CIM/IEC61970/Base/Wires#LinearShuntCompensatorPhase_bPerSection">
        <rdfs:domain rdf:resource="https://w3id.org/netbeheer/referentiemodellen/IECCIM/TC57CIM/IEC61970/Base/Wires#LinearShuntCompensatorPhase"/>
        <rdfs:range rdf:resource="https://w3id.org/netbeheer/referentiemodellen/IECCIM/TC57CIM/IEC61970/Base/Domain#Susceptance"/>
        <rdfs:comment>Susceptance per section of the phase if shunt compensator is wye connected.   Susceptance per section phase to phase if shunt compensator is delta connected.
</rdfs:comment>
    </owl:ObjectProperty>
    


    <!-- https://w3id.org/netbeheer/referentiemodellen/IECCIM/TC57CIM/IEC61970/Base/Wires#LinearShuntCompensatorPhase_gPerSection -->


    <owl:ObjectProperty rdf:about="https://w3id.org/netbeheer/referentiemodellen/IECCIM/TC57CIM/IEC61970/Base/Wires#LinearShuntCompensatorPhase_gPerSection">
        <rdfs:domain rdf:resource="https://w3id.org/netbeheer/referentiemodellen/IECCIM/TC57CIM/IEC61970/Base/Wires#LinearShuntCompensatorPhase"/>
        <rdfs:range rdf:resource="https://w3id.org/netbeheer/referentiemodellen/IECCIM/TC57CIM/IEC61970/Base/Domain#Conductance"/>
        <rdfs:comment>Conductance per section for this phase if shunt compensator is wye connected.  Conductance per section phase to phase if shunt compensator is delta connected.
</rdfs:comment>
    </owl:ObjectProperty>
    


    <!-- https://w3id.org/netbeheer/referentiemodellen/IECCIM/TC57CIM/IEC61970/Base/Wires#LinearShuntCompensator_b0PerSection -->


    <owl:ObjectProperty rdf:about="https://w3id.org/netbeheer/referentiemodellen/IECCIM/TC57CIM/IEC61970/Base/Wires#LinearShuntCompensator_b0PerSection">
        <rdfs:domain rdf:resource="https://w3id.org/netbeheer/referentiemodellen/IECCIM/TC57CIM/IEC61970/Base/Wires#LinearShuntCompensator"/>
        <rdfs:range rdf:resource="https://w3id.org/netbeheer/referentiemodellen/IECCIM/TC57CIM/IEC61970/Base/Domain#Susceptance"/>
        <rdfs:comment>Zero sequence shunt (charging) susceptance per section</rdfs:comment>
    </owl:ObjectProperty>
    


    <!-- https://w3id.org/netbeheer/referentiemodellen/IECCIM/TC57CIM/IEC61970/Base/Wires#LinearShuntCompensator_bPerSection -->


    <owl:ObjectProperty rdf:about="https://w3id.org/netbeheer/referentiemodellen/IECCIM/TC57CIM/IEC61970/Base/Wires#LinearShuntCompensator_bPerSection">
        <rdfs:domain rdf:resource="https://w3id.org/netbeheer/referentiemodellen/IECCIM/TC57CIM/IEC61970/Base/Wires#LinearShuntCompensator"/>
        <rdfs:range rdf:resource="https://w3id.org/netbeheer/referentiemodellen/IECCIM/TC57CIM/IEC61970/Base/Domain#Susceptance"/>
        <rdfs:comment>Positive sequence shunt (charging) susceptance per section</rdfs:comment>
    </owl:ObjectProperty>
    


    <!-- https://w3id.org/netbeheer/referentiemodellen/IECCIM/TC57CIM/IEC61970/Base/Wires#LinearShuntCompensator_g0PerSection -->


    <owl:ObjectProperty rdf:about="https://w3id.org/netbeheer/referentiemodellen/IECCIM/TC57CIM/IEC61970/Base/Wires#LinearShuntCompensator_g0PerSection">
        <rdfs:domain rdf:resource="https://w3id.org/netbeheer/referentiemodellen/IECCIM/TC57CIM/IEC61970/Base/Wires#LinearShuntCompensator"/>
        <rdfs:range rdf:resource="https://w3id.org/netbeheer/referentiemodellen/IECCIM/TC57CIM/IEC61970/Base/Domain#Conductance"/>
        <rdfs:comment>Zero sequence shunt (charging) conductance per section</rdfs:comment>
    </owl:ObjectProperty>
    


    <!-- https://w3id.org/netbeheer/referentiemodellen/IECCIM/TC57CIM/IEC61970/Base/Wires#LinearShuntCompensator_gPerSection -->


    <owl:ObjectProperty rdf:about="https://w3id.org/netbeheer/referentiemodellen/IECCIM/TC57CIM/IEC61970/Base/Wires#LinearShuntCompensator_gPerSection">
        <rdfs:domain rdf:resource="https://w3id.org/netbeheer/referentiemodellen/IECCIM/TC57CIM/IEC61970/Base/Wires#LinearShuntCompensator"/>
        <rdfs:range rdf:resource="https://w3id.org/netbeheer/referentiemodellen/IECCIM/TC57CIM/IEC61970/Base/Domain#Conductance"/>
        <rdfs:comment>Positive sequence shunt (charging) conductance per section</rdfs:comment>
    </owl:ObjectProperty>
    


    <!-- https://w3id.org/netbeheer/referentiemodellen/IECCIM/TC57CIM/IEC61970/Base/Wires#LoadDynamics_EnergyConsumer -->


    <owl:ObjectProperty rdf:about="https://w3id.org/netbeheer/referentiemodellen/IECCIM/TC57CIM/IEC61970/Base/Wires#LoadDynamics_EnergyConsumer">
        <rdfs:domain rdf:resource="https://w3id.org/netbeheer/referentiemodellen/IECCIM/TC57CIM/IEC61970/Dynamics/StandardModels/LoadDynamics#LoadDynamics"/>
        <rdfs:range rdf:resource="https://w3id.org/netbeheer/referentiemodellen/IECCIM/TC57CIM/IEC61970/Base/Wires#EnergyConsumer"/>
        <rdfs:comment>Load dynamics model used to describe dynamic behavior of this energy consumer.Energy consumer to which this dynamics load model applies.</rdfs:comment>
    </owl:ObjectProperty>
    


    <!-- https://w3id.org/netbeheer/referentiemodellen/IECCIM/TC57CIM/IEC61970/Base/Wires#LoadResponseCharacteristic_EnergyConsumer -->


    <owl:ObjectProperty rdf:about="https://w3id.org/netbeheer/referentiemodellen/IECCIM/TC57CIM/IEC61970/Base/Wires#LoadResponseCharacteristic_EnergyConsumer">
        <owl:inverseOf rdf:resource="https://w3id.org/netbeheer/referentiemodellen/IECCIM/TC57CIM/IEC61970/Base/Wires#EnergyConsumer_LoadResponse"/>
        <rdfs:domain rdf:resource="https://w3id.org/netbeheer/referentiemodellen/IECCIM/TC57CIM/IEC61970/Base/LoadModel#LoadResponseCharacteristic"/>
        <rdfs:range rdf:resource="https://w3id.org/netbeheer/referentiemodellen/IECCIM/TC57CIM/IEC61970/Base/Wires#EnergyConsumer"/>
        <rdfs:comment>The set of loads that have the response characteristics.The load response characteristic of this load.  If missing, this load is assumed to be constant power.</rdfs:comment>
    </owl:ObjectProperty>
    


    <!-- https://w3id.org/netbeheer/referentiemodellen/IECCIM/TC57CIM/IEC61970/Base/Wires#MutualCoupling_b0ch -->


    <owl:ObjectProperty rdf:about="https://w3id.org/netbeheer/referentiemodellen/IECCIM/TC57CIM/IEC61970/Base/Wires#MutualCoupling_b0ch">
        <rdfs:domain rdf:resource="https://w3id.org/netbeheer/referentiemodellen/IECCIM/TC57CIM/IEC61970/Base/Wires#MutualCoupling"/>
        <rdfs:range rdf:resource="https://w3id.org/netbeheer/referentiemodellen/IECCIM/TC57CIM/IEC61970/Base/Domain#Susceptance"/>
        <rdfs:comment>Zero sequence mutual coupling shunt (charging) susceptance, uniformly distributed, of the entire line section.</rdfs:comment>
    </owl:ObjectProperty>
    


    <!-- https://w3id.org/netbeheer/referentiemodellen/IECCIM/TC57CIM/IEC61970/Base/Wires#MutualCoupling_distance11 -->


    <owl:ObjectProperty rdf:about="https://w3id.org/netbeheer/referentiemodellen/IECCIM/TC57CIM/IEC61970/Base/Wires#MutualCoupling_distance11">
        <rdfs:domain rdf:resource="https://w3id.org/netbeheer/referentiemodellen/IECCIM/TC57CIM/IEC61970/Base/Wires#MutualCoupling"/>
        <rdfs:range rdf:resource="https://w3id.org/netbeheer/referentiemodellen/IECCIM/TC57CIM/IEC61970/Base/Domain#Length"/>
        <rdfs:comment>Distance to the start of the coupled region from the first line&apos;s terminal having sequence number equal to 1.
</rdfs:comment>
    </owl:ObjectProperty>
    


    <!-- https://w3id.org/netbeheer/referentiemodellen/IECCIM/TC57CIM/IEC61970/Base/Wires#MutualCoupling_distance12 -->


    <owl:ObjectProperty rdf:about="https://w3id.org/netbeheer/referentiemodellen/IECCIM/TC57CIM/IEC61970/Base/Wires#MutualCoupling_distance12">
        <rdfs:domain rdf:resource="https://w3id.org/netbeheer/referentiemodellen/IECCIM/TC57CIM/IEC61970/Base/Wires#MutualCoupling"/>
        <rdfs:range rdf:resource="https://w3id.org/netbeheer/referentiemodellen/IECCIM/TC57CIM/IEC61970/Base/Domain#Length"/>
        <rdfs:comment>Distance to the end of the coupled region from the first line&apos;s terminal with sequence number equal to 1.
</rdfs:comment>
    </owl:ObjectProperty>
    


    <!-- https://w3id.org/netbeheer/referentiemodellen/IECCIM/TC57CIM/IEC61970/Base/Wires#MutualCoupling_distance21 -->


    <owl:ObjectProperty rdf:about="https://w3id.org/netbeheer/referentiemodellen/IECCIM/TC57CIM/IEC61970/Base/Wires#MutualCoupling_distance21">
        <rdfs:domain rdf:resource="https://w3id.org/netbeheer/referentiemodellen/IECCIM/TC57CIM/IEC61970/Base/Wires#MutualCoupling"/>
        <rdfs:range rdf:resource="https://w3id.org/netbeheer/referentiemodellen/IECCIM/TC57CIM/IEC61970/Base/Domain#Length"/>
        <rdfs:comment>Distance to the start of coupled region from the second line&apos;s terminal with sequence number equal to 1.
</rdfs:comment>
    </owl:ObjectProperty>
    


    <!-- https://w3id.org/netbeheer/referentiemodellen/IECCIM/TC57CIM/IEC61970/Base/Wires#MutualCoupling_distance22 -->


    <owl:ObjectProperty rdf:about="https://w3id.org/netbeheer/referentiemodellen/IECCIM/TC57CIM/IEC61970/Base/Wires#MutualCoupling_distance22">
        <rdfs:domain rdf:resource="https://w3id.org/netbeheer/referentiemodellen/IECCIM/TC57CIM/IEC61970/Base/Wires#MutualCoupling"/>
        <rdfs:range rdf:resource="https://w3id.org/netbeheer/referentiemodellen/IECCIM/TC57CIM/IEC61970/Base/Domain#Length"/>
        <rdfs:comment>Distance to the end of coupled region from the second line&apos;s terminal with sequence number equal to 1.</rdfs:comment>
    </owl:ObjectProperty>
    


    <!-- https://w3id.org/netbeheer/referentiemodellen/IECCIM/TC57CIM/IEC61970/Base/Wires#MutualCoupling_g0ch -->


    <owl:ObjectProperty rdf:about="https://w3id.org/netbeheer/referentiemodellen/IECCIM/TC57CIM/IEC61970/Base/Wires#MutualCoupling_g0ch">
        <rdfs:domain rdf:resource="https://w3id.org/netbeheer/referentiemodellen/IECCIM/TC57CIM/IEC61970/Base/Wires#MutualCoupling"/>
        <rdfs:range rdf:resource="https://w3id.org/netbeheer/referentiemodellen/IECCIM/TC57CIM/IEC61970/Base/Domain#Conductance"/>
        <rdfs:comment>Zero sequence mutual coupling shunt (charging) conductance, uniformly distributed, of the entire line section.</rdfs:comment>
    </owl:ObjectProperty>
    


    <!-- https://w3id.org/netbeheer/referentiemodellen/IECCIM/TC57CIM/IEC61970/Base/Wires#MutualCoupling_r0 -->


    <owl:ObjectProperty rdf:about="https://w3id.org/netbeheer/referentiemodellen/IECCIM/TC57CIM/IEC61970/Base/Wires#MutualCoupling_r0">
        <rdfs:domain rdf:resource="https://w3id.org/netbeheer/referentiemodellen/IECCIM/TC57CIM/IEC61970/Base/Wires#MutualCoupling"/>
        <rdfs:range rdf:resource="https://w3id.org/netbeheer/referentiemodellen/IECCIM/TC57CIM/IEC61970/Base/Domain#Resistance"/>
        <rdfs:comment>Zero sequence branch-to-branch mutual impedance coupling, resistance.
</rdfs:comment>
    </owl:ObjectProperty>
    


    <!-- https://w3id.org/netbeheer/referentiemodellen/IECCIM/TC57CIM/IEC61970/Base/Wires#MutualCoupling_x0 -->


    <owl:ObjectProperty rdf:about="https://w3id.org/netbeheer/referentiemodellen/IECCIM/TC57CIM/IEC61970/Base/Wires#MutualCoupling_x0">
        <rdfs:domain rdf:resource="https://w3id.org/netbeheer/referentiemodellen/IECCIM/TC57CIM/IEC61970/Base/Wires#MutualCoupling"/>
        <rdfs:range rdf:resource="https://w3id.org/netbeheer/referentiemodellen/IECCIM/TC57CIM/IEC61970/Base/Domain#Reactance"/>
        <rdfs:comment>Zero sequence branch-to-branch mutual impedance coupling, reactance.
</rdfs:comment>
    </owl:ObjectProperty>
    


    <!-- https://w3id.org/netbeheer/referentiemodellen/IECCIM/TC57CIM/IEC61970/Base/Wires#NonlinearShuntCompensatorPhasePoint_NonlinearShuntCompensatorPhase -->


    <owl:ObjectProperty rdf:about="https://w3id.org/netbeheer/referentiemodellen/IECCIM/TC57CIM/IEC61970/Base/Wires#NonlinearShuntCompensatorPhasePoint_NonlinearShuntCompensatorPhase">
        <rdfs:domain rdf:resource="https://w3id.org/netbeheer/referentiemodellen/IECCIM/TC57CIM/IEC61970/Base/Wires#NonlinearShuntCompensatorPhasePoint"/>
        <rdfs:range rdf:resource="https://w3id.org/netbeheer/referentiemodellen/IECCIM/TC57CIM/IEC61970/Base/Wires#NonlinearShuntCompensatorPhase"/>
        <rdfs:comment>All points of the non-linear shunt compensator phase.Non-linear shunt compensator phase owning this point.</rdfs:comment>
    </owl:ObjectProperty>
    


    <!-- https://w3id.org/netbeheer/referentiemodellen/IECCIM/TC57CIM/IEC61970/Base/Wires#NonlinearShuntCompensatorPhasePoint_b -->


    <owl:ObjectProperty rdf:about="https://w3id.org/netbeheer/referentiemodellen/IECCIM/TC57CIM/IEC61970/Base/Wires#NonlinearShuntCompensatorPhasePoint_b">
        <rdfs:domain rdf:resource="https://w3id.org/netbeheer/referentiemodellen/IECCIM/TC57CIM/IEC61970/Base/Wires#NonlinearShuntCompensatorPhasePoint"/>
        <rdfs:range rdf:resource="https://w3id.org/netbeheer/referentiemodellen/IECCIM/TC57CIM/IEC61970/Base/Domain#Susceptance"/>
        <rdfs:comment>Positive sequence shunt (charging) susceptance per section</rdfs:comment>
    </owl:ObjectProperty>
    


    <!-- https://w3id.org/netbeheer/referentiemodellen/IECCIM/TC57CIM/IEC61970/Base/Wires#NonlinearShuntCompensatorPhasePoint_g -->


    <owl:ObjectProperty rdf:about="https://w3id.org/netbeheer/referentiemodellen/IECCIM/TC57CIM/IEC61970/Base/Wires#NonlinearShuntCompensatorPhasePoint_g">
        <rdfs:domain rdf:resource="https://w3id.org/netbeheer/referentiemodellen/IECCIM/TC57CIM/IEC61970/Base/Wires#NonlinearShuntCompensatorPhasePoint"/>
        <rdfs:range rdf:resource="https://w3id.org/netbeheer/referentiemodellen/IECCIM/TC57CIM/IEC61970/Base/Domain#Conductance"/>
        <rdfs:comment>Positive sequence shunt (charging) conductance per section</rdfs:comment>
    </owl:ObjectProperty>
    


    <!-- https://w3id.org/netbeheer/referentiemodellen/IECCIM/TC57CIM/IEC61970/Base/Wires#NonlinearShuntCompensatorPhase_NonlinearShuntCompensatorPhasePoints -->


    <owl:ObjectProperty rdf:about="https://w3id.org/netbeheer/referentiemodellen/IECCIM/TC57CIM/IEC61970/Base/Wires#NonlinearShuntCompensatorPhase_NonlinearShuntCompensatorPhasePoints">
        <owl:inverseOf rdf:resource="https://w3id.org/netbeheer/referentiemodellen/IECCIM/TC57CIM/IEC61970/Base/Wires#NonlinearShuntCompensatorPhasePoint_NonlinearShuntCompensatorPhase"/>
        <rdf:type rdf:resource="http://www.w3.org/2002/07/owl#FunctionalProperty"/>
        <rdfs:domain rdf:resource="https://w3id.org/netbeheer/referentiemodellen/IECCIM/TC57CIM/IEC61970/Base/Wires#NonlinearShuntCompensatorPhase"/>
        <rdfs:range rdf:resource="https://w3id.org/netbeheer/referentiemodellen/IECCIM/TC57CIM/IEC61970/Base/Wires#NonlinearShuntCompensatorPhasePoint"/>
        <rdfs:comment>All points of the non-linear shunt compensator phase.Non-linear shunt compensator phase owning this point.</rdfs:comment>
    </owl:ObjectProperty>
    


    <!-- https://w3id.org/netbeheer/referentiemodellen/IECCIM/TC57CIM/IEC61970/Base/Wires#NonlinearShuntCompensatorPoint_NonlinearShuntCompensator -->


    <owl:ObjectProperty rdf:about="https://w3id.org/netbeheer/referentiemodellen/IECCIM/TC57CIM/IEC61970/Base/Wires#NonlinearShuntCompensatorPoint_NonlinearShuntCompensator">
        <rdfs:domain rdf:resource="https://w3id.org/netbeheer/referentiemodellen/IECCIM/TC57CIM/IEC61970/Base/Wires#NonlinearShuntCompensatorPoint"/>
        <rdfs:range rdf:resource="https://w3id.org/netbeheer/referentiemodellen/IECCIM/TC57CIM/IEC61970/Base/Wires#NonlinearShuntCompensator"/>
        <rdfs:comment>All points of the non-linear shunt compensator.Non-linear shunt compensator owning this point.</rdfs:comment>
    </owl:ObjectProperty>
    


    <!-- https://w3id.org/netbeheer/referentiemodellen/IECCIM/TC57CIM/IEC61970/Base/Wires#NonlinearShuntCompensatorPoint_b -->


    <owl:ObjectProperty rdf:about="https://w3id.org/netbeheer/referentiemodellen/IECCIM/TC57CIM/IEC61970/Base/Wires#NonlinearShuntCompensatorPoint_b">
        <rdfs:domain rdf:resource="https://w3id.org/netbeheer/referentiemodellen/IECCIM/TC57CIM/IEC61970/Base/Wires#NonlinearShuntCompensatorPoint"/>
        <rdfs:range rdf:resource="https://w3id.org/netbeheer/referentiemodellen/IECCIM/TC57CIM/IEC61970/Base/Domain#Susceptance"/>
        <rdfs:comment>Positive sequence shunt (charging) susceptance per section</rdfs:comment>
    </owl:ObjectProperty>
    


    <!-- https://w3id.org/netbeheer/referentiemodellen/IECCIM/TC57CIM/IEC61970/Base/Wires#NonlinearShuntCompensatorPoint_b0 -->


    <owl:ObjectProperty rdf:about="https://w3id.org/netbeheer/referentiemodellen/IECCIM/TC57CIM/IEC61970/Base/Wires#NonlinearShuntCompensatorPoint_b0">
        <rdfs:domain rdf:resource="https://w3id.org/netbeheer/referentiemodellen/IECCIM/TC57CIM/IEC61970/Base/Wires#NonlinearShuntCompensatorPoint"/>
        <rdfs:range rdf:resource="https://w3id.org/netbeheer/referentiemodellen/IECCIM/TC57CIM/IEC61970/Base/Domain#Susceptance"/>
        <rdfs:comment>Zero sequence shunt (charging) susceptance per section</rdfs:comment>
    </owl:ObjectProperty>
    


    <!-- https://w3id.org/netbeheer/referentiemodellen/IECCIM/TC57CIM/IEC61970/Base/Wires#NonlinearShuntCompensatorPoint_g -->


    <owl:ObjectProperty rdf:about="https://w3id.org/netbeheer/referentiemodellen/IECCIM/TC57CIM/IEC61970/Base/Wires#NonlinearShuntCompensatorPoint_g">
        <rdfs:domain rdf:resource="https://w3id.org/netbeheer/referentiemodellen/IECCIM/TC57CIM/IEC61970/Base/Wires#NonlinearShuntCompensatorPoint"/>
        <rdfs:range rdf:resource="https://w3id.org/netbeheer/referentiemodellen/IECCIM/TC57CIM/IEC61970/Base/Domain#Conductance"/>
        <rdfs:comment>Positive sequence shunt (charging) conductance per section</rdfs:comment>
    </owl:ObjectProperty>
    


    <!-- https://w3id.org/netbeheer/referentiemodellen/IECCIM/TC57CIM/IEC61970/Base/Wires#NonlinearShuntCompensatorPoint_g0 -->


    <owl:ObjectProperty rdf:about="https://w3id.org/netbeheer/referentiemodellen/IECCIM/TC57CIM/IEC61970/Base/Wires#NonlinearShuntCompensatorPoint_g0">
        <rdfs:domain rdf:resource="https://w3id.org/netbeheer/referentiemodellen/IECCIM/TC57CIM/IEC61970/Base/Wires#NonlinearShuntCompensatorPoint"/>
        <rdfs:range rdf:resource="https://w3id.org/netbeheer/referentiemodellen/IECCIM/TC57CIM/IEC61970/Base/Domain#Conductance"/>
        <rdfs:comment>Zero sequence shunt (charging) conductance per section</rdfs:comment>
    </owl:ObjectProperty>
    


    <!-- https://w3id.org/netbeheer/referentiemodellen/IECCIM/TC57CIM/IEC61970/Base/Wires#NonlinearShuntCompensator_NonlinearShuntCompensatorPoints -->


    <owl:ObjectProperty rdf:about="https://w3id.org/netbeheer/referentiemodellen/IECCIM/TC57CIM/IEC61970/Base/Wires#NonlinearShuntCompensator_NonlinearShuntCompensatorPoints">
        <owl:inverseOf rdf:resource="https://w3id.org/netbeheer/referentiemodellen/IECCIM/TC57CIM/IEC61970/Base/Wires#NonlinearShuntCompensatorPoint_NonlinearShuntCompensator"/>
        <rdf:type rdf:resource="http://www.w3.org/2002/07/owl#FunctionalProperty"/>
        <rdfs:domain rdf:resource="https://w3id.org/netbeheer/referentiemodellen/IECCIM/TC57CIM/IEC61970/Base/Wires#NonlinearShuntCompensator"/>
        <rdfs:range rdf:resource="https://w3id.org/netbeheer/referentiemodellen/IECCIM/TC57CIM/IEC61970/Base/Wires#NonlinearShuntCompensatorPoint"/>
        <rdfs:comment>All points of the non-linear shunt compensator.Non-linear shunt compensator owning this point.</rdfs:comment>
    </owl:ObjectProperty>
    


    <!-- https://w3id.org/netbeheer/referentiemodellen/IECCIM/TC57CIM/IEC61970/Base/Wires#Outage_OpenedSwitches -->


    <owl:ObjectProperty rdf:about="https://w3id.org/netbeheer/referentiemodellen/IECCIM/TC57CIM/IEC61970/Base/Wires#Outage_OpenedSwitches">
        <rdfs:domain rdf:resource="https://w3id.org/netbeheer/referentiemodellen/IECCIM/TC57CIM/IEC61968/Operations#Outage"/>
        <rdfs:range rdf:resource="https://w3id.org/netbeheer/referentiemodellen/IECCIM/TC57CIM/IEC61970/Base/Wires#Switch"/>
        <rdfs:comment>Current outage of this protective device.All potentially open switches causing this outage. This realationship is meant to be used as &quot;indication&quot; for initiation of outage-related business processes, whereas for actual actions of switches, SwitchAction-Switch relationship should be used.</rdfs:comment>
    </owl:ObjectProperty>
    


    <!-- https://w3id.org/netbeheer/referentiemodellen/IECCIM/TC57CIM/IEC61970/Base/Wires#PerLengthImpedance_ACLineSegments -->


    <owl:ObjectProperty rdf:about="https://w3id.org/netbeheer/referentiemodellen/IECCIM/TC57CIM/IEC61970/Base/Wires#PerLengthImpedance_ACLineSegments">
        <rdfs:domain rdf:resource="https://w3id.org/netbeheer/referentiemodellen/IECCIM/TC57CIM/IEC61970/Base/Wires#PerLengthImpedance"/>
        <rdfs:range rdf:resource="https://w3id.org/netbeheer/referentiemodellen/IECCIM/TC57CIM/IEC61970/Base/Wires#ACLineSegment"/>
        <rdfs:comment>Per-length impedance of this line segment.All line segments described by this per-length impedance.</rdfs:comment>
    </owl:ObjectProperty>
    


    <!-- https://w3id.org/netbeheer/referentiemodellen/IECCIM/TC57CIM/IEC61970/Base/Wires#PerLengthLineParameter_WireInfos -->


    <owl:ObjectProperty rdf:about="https://w3id.org/netbeheer/referentiemodellen/IECCIM/TC57CIM/IEC61970/Base/Wires#PerLengthLineParameter_WireInfos">
        <owl:inverseOf rdf:resource="https://w3id.org/netbeheer/referentiemodellen/IECCIM/TC57CIM/IEC61970/Base/Wires#WireInfo_PerLengthParameters"/>
        <rdfs:domain rdf:resource="https://w3id.org/netbeheer/referentiemodellen/IECCIM/TC57CIM/IEC61970/Base/Wires#PerLengthLineParameter"/>
        <rdfs:range rdf:resource="https://w3id.org/netbeheer/referentiemodellen/IECCIM/TC57CIM/IEC61968/AssetInfo#WireInfo"/>
        <rdfs:comment>All wire datasheets used to calculate this per-length parameter.All per-length parameters calculated from this wire datasheet.</rdfs:comment>
    </owl:ObjectProperty>
    


    <!-- https://w3id.org/netbeheer/referentiemodellen/IECCIM/TC57CIM/IEC61970/Base/Wires#PerLengthLineParameter_WireSpacingInfo -->


    <owl:ObjectProperty rdf:about="https://w3id.org/netbeheer/referentiemodellen/IECCIM/TC57CIM/IEC61970/Base/Wires#PerLengthLineParameter_WireSpacingInfo">
        <owl:inverseOf rdf:resource="https://w3id.org/netbeheer/referentiemodellen/IECCIM/TC57CIM/IEC61970/Base/Wires#WireSpacing_PerLengthParameters"/>
        <rdfs:domain rdf:resource="https://w3id.org/netbeheer/referentiemodellen/IECCIM/TC57CIM/IEC61970/Base/Wires#PerLengthLineParameter"/>
        <rdfs:range rdf:resource="https://w3id.org/netbeheer/referentiemodellen/IECCIM/TC57CIM/IEC61968/AssetInfo#WireSpacing"/>
        <rdfs:comment>Wire spacing datasheet used to calculate this per-length parameter.All per-length parameters calculated from this wire spacing datasheet.</rdfs:comment>
    </owl:ObjectProperty>
    


    <!-- https://w3id.org/netbeheer/referentiemodellen/IECCIM/TC57CIM/IEC61970/Base/Wires#PerLengthPhaseImpedance_PhaseImpedanceData -->


    <owl:ObjectProperty rdf:about="https://w3id.org/netbeheer/referentiemodellen/IECCIM/TC57CIM/IEC61970/Base/Wires#PerLengthPhaseImpedance_PhaseImpedanceData">
        <rdf:type rdf:resource="http://www.w3.org/2002/07/owl#FunctionalProperty"/>
        <rdfs:domain rdf:resource="https://w3id.org/netbeheer/referentiemodellen/IECCIM/TC57CIM/IEC61970/Base/Wires#PerLengthPhaseImpedance"/>
        <rdfs:range rdf:resource="https://w3id.org/netbeheer/referentiemodellen/IECCIM/TC57CIM/IEC61970/Base/Wires#PhaseImpedanceData"/>
        <rdfs:comment>Conductor phase impedance to which this data belongs.All data that belong to this conductor phase impedance.</rdfs:comment>
    </owl:ObjectProperty>
    


    <!-- https://w3id.org/netbeheer/referentiemodellen/IECCIM/TC57CIM/IEC61970/Base/Wires#PerLengthSequenceImpedance_b0ch -->


    <owl:ObjectProperty rdf:about="https://w3id.org/netbeheer/referentiemodellen/IECCIM/TC57CIM/IEC61970/Base/Wires#PerLengthSequenceImpedance_b0ch">
        <rdfs:domain rdf:resource="https://w3id.org/netbeheer/referentiemodellen/IECCIM/TC57CIM/IEC61970/Base/Wires#PerLengthSequenceImpedance"/>
        <rdfs:range rdf:resource="https://w3id.org/netbeheer/referentiemodellen/IECCIM/TC57CIM/IEC61970/Base/Domain#SusceptancePerLength"/>
        <rdfs:comment>Zero sequence shunt (charging) susceptance, per unit of length.
</rdfs:comment>
    </owl:ObjectProperty>
    


    <!-- https://w3id.org/netbeheer/referentiemodellen/IECCIM/TC57CIM/IEC61970/Base/Wires#PerLengthSequenceImpedance_bch -->


    <owl:ObjectProperty rdf:about="https://w3id.org/netbeheer/referentiemodellen/IECCIM/TC57CIM/IEC61970/Base/Wires#PerLengthSequenceImpedance_bch">
        <rdfs:domain rdf:resource="https://w3id.org/netbeheer/referentiemodellen/IECCIM/TC57CIM/IEC61970/Base/Wires#PerLengthSequenceImpedance"/>
        <rdfs:range rdf:resource="https://w3id.org/netbeheer/referentiemodellen/IECCIM/TC57CIM/IEC61970/Base/Domain#SusceptancePerLength"/>
        <rdfs:comment>Positive sequence shunt (charging) susceptance, per unit of length.
</rdfs:comment>
    </owl:ObjectProperty>
    


    <!-- https://w3id.org/netbeheer/referentiemodellen/IECCIM/TC57CIM/IEC61970/Base/Wires#PerLengthSequenceImpedance_g0ch -->


    <owl:ObjectProperty rdf:about="https://w3id.org/netbeheer/referentiemodellen/IECCIM/TC57CIM/IEC61970/Base/Wires#PerLengthSequenceImpedance_g0ch">
        <rdfs:domain rdf:resource="https://w3id.org/netbeheer/referentiemodellen/IECCIM/TC57CIM/IEC61970/Base/Wires#PerLengthSequenceImpedance"/>
        <rdfs:range rdf:resource="https://w3id.org/netbeheer/referentiemodellen/IECCIM/TC57CIM/IEC61970/Base/Domain#ConductancePerLength"/>
        <rdfs:comment>Zero sequence shunt (charging) conductance, per unit of length.
</rdfs:comment>
    </owl:ObjectProperty>
    


    <!-- https://w3id.org/netbeheer/referentiemodellen/IECCIM/TC57CIM/IEC61970/Base/Wires#PerLengthSequenceImpedance_gch -->


    <owl:ObjectProperty rdf:about="https://w3id.org/netbeheer/referentiemodellen/IECCIM/TC57CIM/IEC61970/Base/Wires#PerLengthSequenceImpedance_gch">
        <rdfs:domain rdf:resource="https://w3id.org/netbeheer/referentiemodellen/IECCIM/TC57CIM/IEC61970/Base/Wires#PerLengthSequenceImpedance"/>
        <rdfs:range rdf:resource="https://w3id.org/netbeheer/referentiemodellen/IECCIM/TC57CIM/IEC61970/Base/Domain#ConductancePerLength"/>
        <rdfs:comment>Positive sequence shunt (charging) conductance, per unit of length.
</rdfs:comment>
    </owl:ObjectProperty>
    


    <!-- https://w3id.org/netbeheer/referentiemodellen/IECCIM/TC57CIM/IEC61970/Base/Wires#PerLengthSequenceImpedance_r -->


    <owl:ObjectProperty rdf:about="https://w3id.org/netbeheer/referentiemodellen/IECCIM/TC57CIM/IEC61970/Base/Wires#PerLengthSequenceImpedance_r">
        <rdfs:domain rdf:resource="https://w3id.org/netbeheer/referentiemodellen/IECCIM/TC57CIM/IEC61970/Base/Wires#PerLengthSequenceImpedance"/>
        <rdfs:range rdf:resource="https://w3id.org/netbeheer/referentiemodellen/IECCIM/TC57CIM/IEC61970/Base/Domain#ResistancePerLength"/>
        <rdfs:comment>Positive sequence series resistance, per unit of length.
</rdfs:comment>
    </owl:ObjectProperty>
    


    <!-- https://w3id.org/netbeheer/referentiemodellen/IECCIM/TC57CIM/IEC61970/Base/Wires#PerLengthSequenceImpedance_r0 -->


    <owl:ObjectProperty rdf:about="https://w3id.org/netbeheer/referentiemodellen/IECCIM/TC57CIM/IEC61970/Base/Wires#PerLengthSequenceImpedance_r0">
        <rdfs:domain rdf:resource="https://w3id.org/netbeheer/referentiemodellen/IECCIM/TC57CIM/IEC61970/Base/Wires#PerLengthSequenceImpedance"/>
        <rdfs:range rdf:resource="https://w3id.org/netbeheer/referentiemodellen/IECCIM/TC57CIM/IEC61970/Base/Domain#ResistancePerLength"/>
        <rdfs:comment>Zero sequence series resistance, per unit of length.
</rdfs:comment>
    </owl:ObjectProperty>
    


    <!-- https://w3id.org/netbeheer/referentiemodellen/IECCIM/TC57CIM/IEC61970/Base/Wires#PerLengthSequenceImpedance_x -->


    <owl:ObjectProperty rdf:about="https://w3id.org/netbeheer/referentiemodellen/IECCIM/TC57CIM/IEC61970/Base/Wires#PerLengthSequenceImpedance_x">
        <rdfs:domain rdf:resource="https://w3id.org/netbeheer/referentiemodellen/IECCIM/TC57CIM/IEC61970/Base/Wires#PerLengthSequenceImpedance"/>
        <rdfs:range rdf:resource="https://w3id.org/netbeheer/referentiemodellen/IECCIM/TC57CIM/IEC61970/Base/Domain#ReactancePerLength"/>
        <rdfs:comment>Positive sequence series reactance, per unit of length.
</rdfs:comment>
    </owl:ObjectProperty>
    


    <!-- https://w3id.org/netbeheer/referentiemodellen/IECCIM/TC57CIM/IEC61970/Base/Wires#PerLengthSequenceImpedance_x0 -->


    <owl:ObjectProperty rdf:about="https://w3id.org/netbeheer/referentiemodellen/IECCIM/TC57CIM/IEC61970/Base/Wires#PerLengthSequenceImpedance_x0">
        <rdfs:domain rdf:resource="https://w3id.org/netbeheer/referentiemodellen/IECCIM/TC57CIM/IEC61970/Base/Wires#PerLengthSequenceImpedance"/>
        <rdfs:range rdf:resource="https://w3id.org/netbeheer/referentiemodellen/IECCIM/TC57CIM/IEC61970/Base/Domain#ReactancePerLength"/>
        <rdfs:comment>Zero sequence series reactance, per unit of length.
</rdfs:comment>
    </owl:ObjectProperty>
    


    <!-- https://w3id.org/netbeheer/referentiemodellen/IECCIM/TC57CIM/IEC61970/Base/Wires#PetersenCoil_nominalU -->


    <owl:ObjectProperty rdf:about="https://w3id.org/netbeheer/referentiemodellen/IECCIM/TC57CIM/IEC61970/Base/Wires#PetersenCoil_nominalU">
        <rdfs:domain rdf:resource="https://w3id.org/netbeheer/referentiemodellen/IECCIM/TC57CIM/IEC61970/Base/Wires#PetersenCoil"/>
        <rdfs:range rdf:resource="https://w3id.org/netbeheer/referentiemodellen/IECCIM/TC57CIM/IEC61970/Base/Domain#Voltage"/>
        <rdfs:comment>The nominal voltage for which the coil is designed.</rdfs:comment>
    </owl:ObjectProperty>
    


    <!-- https://w3id.org/netbeheer/referentiemodellen/IECCIM/TC57CIM/IEC61970/Base/Wires#PetersenCoil_offsetCurrent -->


    <owl:ObjectProperty rdf:about="https://w3id.org/netbeheer/referentiemodellen/IECCIM/TC57CIM/IEC61970/Base/Wires#PetersenCoil_offsetCurrent">
        <rdfs:domain rdf:resource="https://w3id.org/netbeheer/referentiemodellen/IECCIM/TC57CIM/IEC61970/Base/Wires#PetersenCoil"/>
        <rdfs:range rdf:resource="https://w3id.org/netbeheer/referentiemodellen/IECCIM/TC57CIM/IEC61970/Base/Domain#CurrentFlow"/>
        <rdfs:comment>The offset current that the Petersen coil controller is operating from the resonant point.  This is normally a fixed amount for which the controller is configured and could be positive or negative.  Typically 0 to 60 Amperes depending on voltage and resonance conditions.</rdfs:comment>
    </owl:ObjectProperty>
    


    <!-- https://w3id.org/netbeheer/referentiemodellen/IECCIM/TC57CIM/IEC61970/Base/Wires#PetersenCoil_positionCurrent -->


    <owl:ObjectProperty rdf:about="https://w3id.org/netbeheer/referentiemodellen/IECCIM/TC57CIM/IEC61970/Base/Wires#PetersenCoil_positionCurrent">
        <rdfs:domain rdf:resource="https://w3id.org/netbeheer/referentiemodellen/IECCIM/TC57CIM/IEC61970/Base/Wires#PetersenCoil"/>
        <rdfs:range rdf:resource="https://w3id.org/netbeheer/referentiemodellen/IECCIM/TC57CIM/IEC61970/Base/Domain#CurrentFlow"/>
        <rdfs:comment>The control current used to control the Petersen coil also known as the position current.  Typically in the range of 20-200mA.</rdfs:comment>
    </owl:ObjectProperty>
    


    <!-- https://w3id.org/netbeheer/referentiemodellen/IECCIM/TC57CIM/IEC61970/Base/Wires#PetersenCoil_xGroundMax -->


    <owl:ObjectProperty rdf:about="https://w3id.org/netbeheer/referentiemodellen/IECCIM/TC57CIM/IEC61970/Base/Wires#PetersenCoil_xGroundMax">
        <rdfs:domain rdf:resource="https://w3id.org/netbeheer/referentiemodellen/IECCIM/TC57CIM/IEC61970/Base/Wires#PetersenCoil"/>
        <rdfs:range rdf:resource="https://w3id.org/netbeheer/referentiemodellen/IECCIM/TC57CIM/IEC61970/Base/Domain#Reactance"/>
        <rdfs:comment>The maximum reactance. </rdfs:comment>
    </owl:ObjectProperty>
    


    <!-- https://w3id.org/netbeheer/referentiemodellen/IECCIM/TC57CIM/IEC61970/Base/Wires#PetersenCoil_xGroundMin -->


    <owl:ObjectProperty rdf:about="https://w3id.org/netbeheer/referentiemodellen/IECCIM/TC57CIM/IEC61970/Base/Wires#PetersenCoil_xGroundMin">
        <rdfs:domain rdf:resource="https://w3id.org/netbeheer/referentiemodellen/IECCIM/TC57CIM/IEC61970/Base/Wires#PetersenCoil"/>
        <rdfs:range rdf:resource="https://w3id.org/netbeheer/referentiemodellen/IECCIM/TC57CIM/IEC61970/Base/Domain#Reactance"/>
        <rdfs:comment>The minimum reactance.</rdfs:comment>
    </owl:ObjectProperty>
    


    <!-- https://w3id.org/netbeheer/referentiemodellen/IECCIM/TC57CIM/IEC61970/Base/Wires#PetersenCoil_xGroundNominal -->


    <owl:ObjectProperty rdf:about="https://w3id.org/netbeheer/referentiemodellen/IECCIM/TC57CIM/IEC61970/Base/Wires#PetersenCoil_xGroundNominal">
        <rdfs:domain rdf:resource="https://w3id.org/netbeheer/referentiemodellen/IECCIM/TC57CIM/IEC61970/Base/Wires#PetersenCoil"/>
        <rdfs:range rdf:resource="https://w3id.org/netbeheer/referentiemodellen/IECCIM/TC57CIM/IEC61970/Base/Domain#Reactance"/>
        <rdfs:comment>The nominal reactance.  This is the operating point (normally over compensation) that is defined based on the resonance point in the healthy network condition.  The impedance is calculated based on nominal voltage divided by position current.</rdfs:comment>
    </owl:ObjectProperty>
    


    <!-- https://w3id.org/netbeheer/referentiemodellen/IECCIM/TC57CIM/IEC61970/Base/Wires#PhaseImpedanceData_PhaseImpedance -->


    <owl:ObjectProperty rdf:about="https://w3id.org/netbeheer/referentiemodellen/IECCIM/TC57CIM/IEC61970/Base/Wires#PhaseImpedanceData_PhaseImpedance">
        <owl:inverseOf rdf:resource="https://w3id.org/netbeheer/referentiemodellen/IECCIM/TC57CIM/IEC61970/Base/Wires#PerLengthPhaseImpedance_PhaseImpedanceData"/>
        <rdfs:domain rdf:resource="https://w3id.org/netbeheer/referentiemodellen/IECCIM/TC57CIM/IEC61970/Base/Wires#PhaseImpedanceData"/>
        <rdfs:range rdf:resource="https://w3id.org/netbeheer/referentiemodellen/IECCIM/TC57CIM/IEC61970/Base/Wires#PerLengthPhaseImpedance"/>
        <rdfs:comment>Conductor phase impedance to which this data belongs.All data that belong to this conductor phase impedance.</rdfs:comment>
    </owl:ObjectProperty>
    


    <!-- https://w3id.org/netbeheer/referentiemodellen/IECCIM/TC57CIM/IEC61970/Base/Wires#PhaseImpedanceData_b -->


    <owl:ObjectProperty rdf:about="https://w3id.org/netbeheer/referentiemodellen/IECCIM/TC57CIM/IEC61970/Base/Wires#PhaseImpedanceData_b">
        <rdfs:domain rdf:resource="https://w3id.org/netbeheer/referentiemodellen/IECCIM/TC57CIM/IEC61970/Base/Wires#PhaseImpedanceData"/>
        <rdfs:range rdf:resource="https://w3id.org/netbeheer/referentiemodellen/IECCIM/TC57CIM/IEC61970/Base/Domain#SusceptancePerLength"/>
        <rdfs:comment>Susceptance matrix element value, per length of unit.
</rdfs:comment>
    </owl:ObjectProperty>
    


    <!-- https://w3id.org/netbeheer/referentiemodellen/IECCIM/TC57CIM/IEC61970/Base/Wires#PhaseImpedanceData_r -->


    <owl:ObjectProperty rdf:about="https://w3id.org/netbeheer/referentiemodellen/IECCIM/TC57CIM/IEC61970/Base/Wires#PhaseImpedanceData_r">
        <rdfs:domain rdf:resource="https://w3id.org/netbeheer/referentiemodellen/IECCIM/TC57CIM/IEC61970/Base/Wires#PhaseImpedanceData"/>
        <rdfs:range rdf:resource="https://w3id.org/netbeheer/referentiemodellen/IECCIM/TC57CIM/IEC61970/Base/Domain#ResistancePerLength"/>
        <rdfs:comment>Resistance matrix element value, per length of unit.
</rdfs:comment>
    </owl:ObjectProperty>
    


    <!-- https://w3id.org/netbeheer/referentiemodellen/IECCIM/TC57CIM/IEC61970/Base/Wires#PhaseImpedanceData_x -->


    <owl:ObjectProperty rdf:about="https://w3id.org/netbeheer/referentiemodellen/IECCIM/TC57CIM/IEC61970/Base/Wires#PhaseImpedanceData_x">
        <rdfs:domain rdf:resource="https://w3id.org/netbeheer/referentiemodellen/IECCIM/TC57CIM/IEC61970/Base/Wires#PhaseImpedanceData"/>
        <rdfs:range rdf:resource="https://w3id.org/netbeheer/referentiemodellen/IECCIM/TC57CIM/IEC61970/Base/Domain#ReactancePerLength"/>
        <rdfs:comment>Reactance matrix element value, per length of unit.
</rdfs:comment>
    </owl:ObjectProperty>
    


    <!-- https://w3id.org/netbeheer/referentiemodellen/IECCIM/TC57CIM/IEC61970/Base/Wires#PhaseTapChangerAsymmetrical_windingConnectionAngle -->


    <owl:ObjectProperty rdf:about="https://w3id.org/netbeheer/referentiemodellen/IECCIM/TC57CIM/IEC61970/Base/Wires#PhaseTapChangerAsymmetrical_windingConnectionAngle">
        <rdfs:domain rdf:resource="https://w3id.org/netbeheer/referentiemodellen/IECCIM/TC57CIM/IEC61970/Base/Wires#PhaseTapChangerAsymmetrical"/>
        <rdfs:range rdf:resource="https://w3id.org/netbeheer/referentiemodellen/IECCIM/TC57CIM/IEC61970/Base/Domain#AngleDegrees"/>
        <rdfs:comment>The phase angle between the in-phase winding and the out-of -phase winding used for creating phase shift. The out-of-phase winding produces what is known as the difference voltage.  Setting this angle to 90 degrees is not the same as a symmemtrical transformer.
</rdfs:comment>
    </owl:ObjectProperty>
    


    <!-- https://w3id.org/netbeheer/referentiemodellen/IECCIM/TC57CIM/IEC61970/Base/Wires#PhaseTapChangerLinear_stepPhaseShiftIncrement -->


    <owl:ObjectProperty rdf:about="https://w3id.org/netbeheer/referentiemodellen/IECCIM/TC57CIM/IEC61970/Base/Wires#PhaseTapChangerLinear_stepPhaseShiftIncrement">
        <rdfs:domain rdf:resource="https://w3id.org/netbeheer/referentiemodellen/IECCIM/TC57CIM/IEC61970/Base/Wires#PhaseTapChangerLinear"/>
        <rdfs:range rdf:resource="https://w3id.org/netbeheer/referentiemodellen/IECCIM/TC57CIM/IEC61970/Base/Domain#AngleDegrees"/>
        <rdfs:comment>Phase shift per step position. A positive value indicates a positive phase shift from the winding where the tap is located to the other winding (for a two-winding transformer).
The actual phase shift increment might be more accurately computed from the symmetrical or asymmetrical models or a tap step table lookup if those are available.</rdfs:comment>
    </owl:ObjectProperty>
    


    <!-- https://w3id.org/netbeheer/referentiemodellen/IECCIM/TC57CIM/IEC61970/Base/Wires#PhaseTapChangerLinear_xMax -->


    <owl:ObjectProperty rdf:about="https://w3id.org/netbeheer/referentiemodellen/IECCIM/TC57CIM/IEC61970/Base/Wires#PhaseTapChangerLinear_xMax">
        <rdfs:domain rdf:resource="https://w3id.org/netbeheer/referentiemodellen/IECCIM/TC57CIM/IEC61970/Base/Wires#PhaseTapChangerLinear"/>
        <rdfs:range rdf:resource="https://w3id.org/netbeheer/referentiemodellen/IECCIM/TC57CIM/IEC61970/Base/Domain#Reactance"/>
        <rdfs:comment>The reactance depend on the tap position according to a &quot;u&quot; shaped curve. The maximum reactance (xMax) appear at the low and high tap positions.</rdfs:comment>
    </owl:ObjectProperty>
    


    <!-- https://w3id.org/netbeheer/referentiemodellen/IECCIM/TC57CIM/IEC61970/Base/Wires#PhaseTapChangerLinear_xMin -->


    <owl:ObjectProperty rdf:about="https://w3id.org/netbeheer/referentiemodellen/IECCIM/TC57CIM/IEC61970/Base/Wires#PhaseTapChangerLinear_xMin">
        <rdfs:domain rdf:resource="https://w3id.org/netbeheer/referentiemodellen/IECCIM/TC57CIM/IEC61970/Base/Wires#PhaseTapChangerLinear"/>
        <rdfs:range rdf:resource="https://w3id.org/netbeheer/referentiemodellen/IECCIM/TC57CIM/IEC61970/Base/Domain#Reactance"/>
        <rdfs:comment>The reactance depend on the tap position according to a &quot;u&quot; shaped curve. The minimum reactance (xMin) appear at the mid tap position.</rdfs:comment>
    </owl:ObjectProperty>
    


    <!-- https://w3id.org/netbeheer/referentiemodellen/IECCIM/TC57CIM/IEC61970/Base/Wires#PhaseTapChangerNonLinear_voltageStepIncrement -->


    <owl:ObjectProperty rdf:about="https://w3id.org/netbeheer/referentiemodellen/IECCIM/TC57CIM/IEC61970/Base/Wires#PhaseTapChangerNonLinear_voltageStepIncrement">
        <rdfs:domain rdf:resource="https://w3id.org/netbeheer/referentiemodellen/IECCIM/TC57CIM/IEC61970/Base/Wires#PhaseTapChangerNonLinear"/>
        <rdfs:range rdf:resource="https://w3id.org/netbeheer/referentiemodellen/IECCIM/TC57CIM/IEC61970/Base/Domain#PerCent"/>
        <rdfs:comment>The voltage step increment on the out of phase winding specified in percent of nominal voltage of the transformer end.
</rdfs:comment>
    </owl:ObjectProperty>
    


    <!-- https://w3id.org/netbeheer/referentiemodellen/IECCIM/TC57CIM/IEC61970/Base/Wires#PhaseTapChangerNonLinear_xMax -->


    <owl:ObjectProperty rdf:about="https://w3id.org/netbeheer/referentiemodellen/IECCIM/TC57CIM/IEC61970/Base/Wires#PhaseTapChangerNonLinear_xMax">
        <rdfs:domain rdf:resource="https://w3id.org/netbeheer/referentiemodellen/IECCIM/TC57CIM/IEC61970/Base/Wires#PhaseTapChangerNonLinear"/>
        <rdfs:range rdf:resource="https://w3id.org/netbeheer/referentiemodellen/IECCIM/TC57CIM/IEC61970/Base/Domain#Reactance"/>
        <rdfs:comment>The reactance depend on the tap position according to a &quot;u&quot; shaped curve. The maximum reactance (xMax) appear at the low and high tap positions.</rdfs:comment>
    </owl:ObjectProperty>
    


    <!-- https://w3id.org/netbeheer/referentiemodellen/IECCIM/TC57CIM/IEC61970/Base/Wires#PhaseTapChangerNonLinear_xMin -->


    <owl:ObjectProperty rdf:about="https://w3id.org/netbeheer/referentiemodellen/IECCIM/TC57CIM/IEC61970/Base/Wires#PhaseTapChangerNonLinear_xMin">
        <rdfs:domain rdf:resource="https://w3id.org/netbeheer/referentiemodellen/IECCIM/TC57CIM/IEC61970/Base/Wires#PhaseTapChangerNonLinear"/>
        <rdfs:range rdf:resource="https://w3id.org/netbeheer/referentiemodellen/IECCIM/TC57CIM/IEC61970/Base/Domain#Reactance"/>
        <rdfs:comment>The reactance depend on the tap position according to a &quot;u&quot; shaped curve. The minimum reactance (xMin) appear at the mid tap position.</rdfs:comment>
    </owl:ObjectProperty>
    


    <!-- https://w3id.org/netbeheer/referentiemodellen/IECCIM/TC57CIM/IEC61970/Base/Wires#PhaseTapChangerTablePoint_PhaseTapChangerTable -->


    <owl:ObjectProperty rdf:about="https://w3id.org/netbeheer/referentiemodellen/IECCIM/TC57CIM/IEC61970/Base/Wires#PhaseTapChangerTablePoint_PhaseTapChangerTable">
        <rdfs:domain rdf:resource="https://w3id.org/netbeheer/referentiemodellen/IECCIM/TC57CIM/IEC61970/Base/Wires#PhaseTapChangerTablePoint"/>
        <rdfs:range rdf:resource="https://w3id.org/netbeheer/referentiemodellen/IECCIM/TC57CIM/IEC61970/Base/Wires#PhaseTapChangerTable"/>
        <rdfs:comment>The points of this table.The table of this point.</rdfs:comment>
    </owl:ObjectProperty>
    


    <!-- https://w3id.org/netbeheer/referentiemodellen/IECCIM/TC57CIM/IEC61970/Base/Wires#PhaseTapChangerTablePoint_angle -->


    <owl:ObjectProperty rdf:about="https://w3id.org/netbeheer/referentiemodellen/IECCIM/TC57CIM/IEC61970/Base/Wires#PhaseTapChangerTablePoint_angle">
        <rdfs:domain rdf:resource="https://w3id.org/netbeheer/referentiemodellen/IECCIM/TC57CIM/IEC61970/Base/Wires#PhaseTapChangerTablePoint"/>
        <rdfs:range rdf:resource="https://w3id.org/netbeheer/referentiemodellen/IECCIM/TC57CIM/IEC61970/Base/Domain#AngleDegrees"/>
        <rdfs:comment>The angle difference in degrees.
</rdfs:comment>
    </owl:ObjectProperty>
    


    <!-- https://w3id.org/netbeheer/referentiemodellen/IECCIM/TC57CIM/IEC61970/Base/Wires#PhaseTapChangerTable_PhaseTapChangerTablePoint -->


    <owl:ObjectProperty rdf:about="https://w3id.org/netbeheer/referentiemodellen/IECCIM/TC57CIM/IEC61970/Base/Wires#PhaseTapChangerTable_PhaseTapChangerTablePoint">
        <owl:inverseOf rdf:resource="https://w3id.org/netbeheer/referentiemodellen/IECCIM/TC57CIM/IEC61970/Base/Wires#PhaseTapChangerTablePoint_PhaseTapChangerTable"/>
        <rdf:type rdf:resource="http://www.w3.org/2002/07/owl#FunctionalProperty"/>
        <rdfs:domain rdf:resource="https://w3id.org/netbeheer/referentiemodellen/IECCIM/TC57CIM/IEC61970/Base/Wires#PhaseTapChangerTable"/>
        <rdfs:range rdf:resource="https://w3id.org/netbeheer/referentiemodellen/IECCIM/TC57CIM/IEC61970/Base/Wires#PhaseTapChangerTablePoint"/>
        <rdfs:comment>The points of this table.The table of this point.</rdfs:comment>
    </owl:ObjectProperty>
    


    <!-- https://w3id.org/netbeheer/referentiemodellen/IECCIM/TC57CIM/IEC61970/Base/Wires#PhaseTapChangerTable_PhaseTapChangerTabular -->


    <owl:ObjectProperty rdf:about="https://w3id.org/netbeheer/referentiemodellen/IECCIM/TC57CIM/IEC61970/Base/Wires#PhaseTapChangerTable_PhaseTapChangerTabular">
        <rdfs:domain rdf:resource="https://w3id.org/netbeheer/referentiemodellen/IECCIM/TC57CIM/IEC61970/Base/Wires#PhaseTapChangerTable"/>
        <rdfs:range rdf:resource="https://w3id.org/netbeheer/referentiemodellen/IECCIM/TC57CIM/IEC61970/Base/Wires#PhaseTapChangerTabular"/>
        <rdfs:comment>The phase tap changer table for this phase tap changer.The phase tap changers to which this phase tap table applies.</rdfs:comment>
    </owl:ObjectProperty>
    


    <!-- https://w3id.org/netbeheer/referentiemodellen/IECCIM/TC57CIM/IEC61970/Base/Wires#PhaseTapChangerTabular_PhaseTapChangerTable -->


    <owl:ObjectProperty rdf:about="https://w3id.org/netbeheer/referentiemodellen/IECCIM/TC57CIM/IEC61970/Base/Wires#PhaseTapChangerTabular_PhaseTapChangerTable">
        <owl:inverseOf rdf:resource="https://w3id.org/netbeheer/referentiemodellen/IECCIM/TC57CIM/IEC61970/Base/Wires#PhaseTapChangerTable_PhaseTapChangerTabular"/>
        <rdfs:domain rdf:resource="https://w3id.org/netbeheer/referentiemodellen/IECCIM/TC57CIM/IEC61970/Base/Wires#PhaseTapChangerTabular"/>
        <rdfs:range rdf:resource="https://w3id.org/netbeheer/referentiemodellen/IECCIM/TC57CIM/IEC61970/Base/Wires#PhaseTapChangerTable"/>
        <rdfs:comment>The phase tap changer table for this phase tap changer.The phase tap changers to which this phase tap table applies.</rdfs:comment>
    </owl:ObjectProperty>
    


    <!-- https://w3id.org/netbeheer/referentiemodellen/IECCIM/TC57CIM/IEC61970/Base/Wires#PhaseTapChanger_TransformerEnd -->


    <owl:ObjectProperty rdf:about="https://w3id.org/netbeheer/referentiemodellen/IECCIM/TC57CIM/IEC61970/Base/Wires#PhaseTapChanger_TransformerEnd">
        <owl:inverseOf rdf:resource="https://w3id.org/netbeheer/referentiemodellen/IECCIM/TC57CIM/IEC61970/Base/Wires#TransformerEnd_PhaseTapChanger"/>
        <rdfs:domain rdf:resource="https://w3id.org/netbeheer/referentiemodellen/IECCIM/TC57CIM/IEC61970/Base/Wires#PhaseTapChanger"/>
        <rdfs:range rdf:resource="https://w3id.org/netbeheer/referentiemodellen/IECCIM/TC57CIM/IEC61970/Base/Wires#TransformerEnd"/>
        <rdfs:comment>Transformer end to which this phase tap changer belongs.Phase tap changer associated with this transformer end.</rdfs:comment>
    </owl:ObjectProperty>
    


    <!-- https://w3id.org/netbeheer/referentiemodellen/IECCIM/TC57CIM/IEC61970/Base/Wires#PowerCutZone_EnergyConsumers -->


    <owl:ObjectProperty rdf:about="https://w3id.org/netbeheer/referentiemodellen/IECCIM/TC57CIM/IEC61970/Base/Wires#PowerCutZone_EnergyConsumers">
        <rdfs:domain rdf:resource="https://w3id.org/netbeheer/referentiemodellen/IECCIM/TC57CIM/IEC61970/Base/LoadModel#PowerCutZone"/>
        <rdfs:range rdf:resource="https://w3id.org/netbeheer/referentiemodellen/IECCIM/TC57CIM/IEC61970/Base/Wires#EnergyConsumer"/>
        <rdfs:comment>The  energy consumer is assigned to this power cut zone.Energy consumer is assigned to the power cut zone.</rdfs:comment>
    </owl:ObjectProperty>
    


    <!-- https://w3id.org/netbeheer/referentiemodellen/IECCIM/TC57CIM/IEC61970/Base/Wires#PowerTransformerEnd_PowerTransformer -->


    <owl:ObjectProperty rdf:about="https://w3id.org/netbeheer/referentiemodellen/IECCIM/TC57CIM/IEC61970/Base/Wires#PowerTransformerEnd_PowerTransformer">
        <owl:inverseOf rdf:resource="https://w3id.org/netbeheer/referentiemodellen/IECCIM/TC57CIM/IEC61970/Base/Wires#PowerTransformer_PowerTransformerEnd"/>
        <rdfs:domain rdf:resource="https://w3id.org/netbeheer/referentiemodellen/IECCIM/TC57CIM/IEC61970/Base/Wires#PowerTransformerEnd"/>
        <rdfs:range rdf:resource="https://w3id.org/netbeheer/referentiemodellen/IECCIM/TC57CIM/IEC61970/Base/Wires#PowerTransformer"/>
        <rdfs:comment>The power transformer of this power transformer end.The ends of this power transformer.</rdfs:comment>
    </owl:ObjectProperty>
    


    <!-- https://w3id.org/netbeheer/referentiemodellen/IECCIM/TC57CIM/IEC61970/Base/Wires#PowerTransformerEnd_b -->


    <owl:ObjectProperty rdf:about="https://w3id.org/netbeheer/referentiemodellen/IECCIM/TC57CIM/IEC61970/Base/Wires#PowerTransformerEnd_b">
        <rdfs:domain rdf:resource="https://w3id.org/netbeheer/referentiemodellen/IECCIM/TC57CIM/IEC61970/Base/Wires#PowerTransformerEnd"/>
        <rdfs:range rdf:resource="https://w3id.org/netbeheer/referentiemodellen/IECCIM/TC57CIM/IEC61970/Base/Domain#Susceptance"/>
        <rdfs:comment>Magnetizing branch susceptance (B mag).  The value can be positive or negative.
</rdfs:comment>
    </owl:ObjectProperty>
    


    <!-- https://w3id.org/netbeheer/referentiemodellen/IECCIM/TC57CIM/IEC61970/Base/Wires#PowerTransformerEnd_b0 -->


    <owl:ObjectProperty rdf:about="https://w3id.org/netbeheer/referentiemodellen/IECCIM/TC57CIM/IEC61970/Base/Wires#PowerTransformerEnd_b0">
        <rdfs:domain rdf:resource="https://w3id.org/netbeheer/referentiemodellen/IECCIM/TC57CIM/IEC61970/Base/Wires#PowerTransformerEnd"/>
        <rdfs:range rdf:resource="https://w3id.org/netbeheer/referentiemodellen/IECCIM/TC57CIM/IEC61970/Base/Domain#Susceptance"/>
        <rdfs:comment>Zero sequence magnetizing branch susceptance.
</rdfs:comment>
    </owl:ObjectProperty>
    


    <!-- https://w3id.org/netbeheer/referentiemodellen/IECCIM/TC57CIM/IEC61970/Base/Wires#PowerTransformerEnd_g -->


    <owl:ObjectProperty rdf:about="https://w3id.org/netbeheer/referentiemodellen/IECCIM/TC57CIM/IEC61970/Base/Wires#PowerTransformerEnd_g">
        <rdfs:domain rdf:resource="https://w3id.org/netbeheer/referentiemodellen/IECCIM/TC57CIM/IEC61970/Base/Wires#PowerTransformerEnd"/>
        <rdfs:range rdf:resource="https://w3id.org/netbeheer/referentiemodellen/IECCIM/TC57CIM/IEC61970/Base/Domain#Conductance"/>
        <rdfs:comment>Magnetizing branch conductance.
</rdfs:comment>
    </owl:ObjectProperty>
    


    <!-- https://w3id.org/netbeheer/referentiemodellen/IECCIM/TC57CIM/IEC61970/Base/Wires#PowerTransformerEnd_g0 -->


    <owl:ObjectProperty rdf:about="https://w3id.org/netbeheer/referentiemodellen/IECCIM/TC57CIM/IEC61970/Base/Wires#PowerTransformerEnd_g0">
        <rdfs:domain rdf:resource="https://w3id.org/netbeheer/referentiemodellen/IECCIM/TC57CIM/IEC61970/Base/Wires#PowerTransformerEnd"/>
        <rdfs:range rdf:resource="https://w3id.org/netbeheer/referentiemodellen/IECCIM/TC57CIM/IEC61970/Base/Domain#Conductance"/>
        <rdfs:comment>Zero sequence magnetizing branch conductance (star-model).
</rdfs:comment>
    </owl:ObjectProperty>
    


    <!-- https://w3id.org/netbeheer/referentiemodellen/IECCIM/TC57CIM/IEC61970/Base/Wires#PowerTransformerEnd_r -->


    <owl:ObjectProperty rdf:about="https://w3id.org/netbeheer/referentiemodellen/IECCIM/TC57CIM/IEC61970/Base/Wires#PowerTransformerEnd_r">
        <rdfs:domain rdf:resource="https://w3id.org/netbeheer/referentiemodellen/IECCIM/TC57CIM/IEC61970/Base/Wires#PowerTransformerEnd"/>
        <rdfs:range rdf:resource="https://w3id.org/netbeheer/referentiemodellen/IECCIM/TC57CIM/IEC61970/Base/Domain#Resistance"/>
        <rdfs:comment>Resistance (star-model) of the transformer end.
The attribute shall be equal or greater than zero for non-equivalent transformers.</rdfs:comment>
    </owl:ObjectProperty>
    


    <!-- https://w3id.org/netbeheer/referentiemodellen/IECCIM/TC57CIM/IEC61970/Base/Wires#PowerTransformerEnd_r0 -->


    <owl:ObjectProperty rdf:about="https://w3id.org/netbeheer/referentiemodellen/IECCIM/TC57CIM/IEC61970/Base/Wires#PowerTransformerEnd_r0">
        <rdfs:domain rdf:resource="https://w3id.org/netbeheer/referentiemodellen/IECCIM/TC57CIM/IEC61970/Base/Wires#PowerTransformerEnd"/>
        <rdfs:range rdf:resource="https://w3id.org/netbeheer/referentiemodellen/IECCIM/TC57CIM/IEC61970/Base/Domain#Resistance"/>
        <rdfs:comment>Zero sequence series resistance (star-model) of the transformer end.
</rdfs:comment>
    </owl:ObjectProperty>
    


    <!-- https://w3id.org/netbeheer/referentiemodellen/IECCIM/TC57CIM/IEC61970/Base/Wires#PowerTransformerEnd_ratedS -->


    <owl:ObjectProperty rdf:about="https://w3id.org/netbeheer/referentiemodellen/IECCIM/TC57CIM/IEC61970/Base/Wires#PowerTransformerEnd_ratedS">
        <rdfs:domain rdf:resource="https://w3id.org/netbeheer/referentiemodellen/IECCIM/TC57CIM/IEC61970/Base/Wires#PowerTransformerEnd"/>
        <rdfs:range rdf:resource="https://w3id.org/netbeheer/referentiemodellen/IECCIM/TC57CIM/IEC61970/Base/Domain#ApparentPower"/>
        <rdfs:comment>Normal apparent power rating.
The attribute shall be a positive value. For a two-winding transformer the values for the high and low voltage sides shall be identical. </rdfs:comment>
    </owl:ObjectProperty>
    


    <!-- https://w3id.org/netbeheer/referentiemodellen/IECCIM/TC57CIM/IEC61970/Base/Wires#PowerTransformerEnd_ratedU -->


    <owl:ObjectProperty rdf:about="https://w3id.org/netbeheer/referentiemodellen/IECCIM/TC57CIM/IEC61970/Base/Wires#PowerTransformerEnd_ratedU">
        <rdfs:domain rdf:resource="https://w3id.org/netbeheer/referentiemodellen/IECCIM/TC57CIM/IEC61970/Base/Wires#PowerTransformerEnd"/>
        <rdfs:range rdf:resource="https://w3id.org/netbeheer/referentiemodellen/IECCIM/TC57CIM/IEC61970/Base/Domain#Voltage"/>
        <rdfs:comment>Rated voltage: phase-phase for three-phase windings, and either phase-phase or phase-neutral for single-phase windings.
A high voltage side, as given by TransformerEnd.endNumber, shall have a ratedU that is greater or equal than ratedU for the lower voltage sides.</rdfs:comment>
    </owl:ObjectProperty>
    


    <!-- https://w3id.org/netbeheer/referentiemodellen/IECCIM/TC57CIM/IEC61970/Base/Wires#PowerTransformerEnd_x -->


    <owl:ObjectProperty rdf:about="https://w3id.org/netbeheer/referentiemodellen/IECCIM/TC57CIM/IEC61970/Base/Wires#PowerTransformerEnd_x">
        <rdfs:domain rdf:resource="https://w3id.org/netbeheer/referentiemodellen/IECCIM/TC57CIM/IEC61970/Base/Wires#PowerTransformerEnd"/>
        <rdfs:range rdf:resource="https://w3id.org/netbeheer/referentiemodellen/IECCIM/TC57CIM/IEC61970/Base/Domain#Reactance"/>
        <rdfs:comment>Positive sequence series reactance (star-model) of the transformer end.
</rdfs:comment>
    </owl:ObjectProperty>
    


    <!-- https://w3id.org/netbeheer/referentiemodellen/IECCIM/TC57CIM/IEC61970/Base/Wires#PowerTransformerEnd_x0 -->


    <owl:ObjectProperty rdf:about="https://w3id.org/netbeheer/referentiemodellen/IECCIM/TC57CIM/IEC61970/Base/Wires#PowerTransformerEnd_x0">
        <rdfs:domain rdf:resource="https://w3id.org/netbeheer/referentiemodellen/IECCIM/TC57CIM/IEC61970/Base/Wires#PowerTransformerEnd"/>
        <rdfs:range rdf:resource="https://w3id.org/netbeheer/referentiemodellen/IECCIM/TC57CIM/IEC61970/Base/Domain#Reactance"/>
        <rdfs:comment>Zero sequence series reactance of the transformer end.
</rdfs:comment>
    </owl:ObjectProperty>
    


    <!-- https://w3id.org/netbeheer/referentiemodellen/IECCIM/TC57CIM/IEC61970/Base/Wires#PowerTransformer_PowerTransformerEnd -->


    <owl:ObjectProperty rdf:about="https://w3id.org/netbeheer/referentiemodellen/IECCIM/TC57CIM/IEC61970/Base/Wires#PowerTransformer_PowerTransformerEnd">
        <rdfs:domain rdf:resource="https://w3id.org/netbeheer/referentiemodellen/IECCIM/TC57CIM/IEC61970/Base/Wires#PowerTransformer"/>
        <rdfs:range rdf:resource="https://w3id.org/netbeheer/referentiemodellen/IECCIM/TC57CIM/IEC61970/Base/Wires#PowerTransformerEnd"/>
        <rdfs:comment>The power transformer of this power transformer end.The ends of this power transformer.</rdfs:comment>
    </owl:ObjectProperty>
    


    <!-- https://w3id.org/netbeheer/referentiemodellen/IECCIM/TC57CIM/IEC61970/Base/Wires#PowerTransformer_TransformerTanks -->


    <owl:ObjectProperty rdf:about="https://w3id.org/netbeheer/referentiemodellen/IECCIM/TC57CIM/IEC61970/Base/Wires#PowerTransformer_TransformerTanks">
        <owl:inverseOf rdf:resource="https://w3id.org/netbeheer/referentiemodellen/IECCIM/TC57CIM/IEC61970/Base/Wires#TransformerTank_PowerTransformer"/>
        <rdfs:domain rdf:resource="https://w3id.org/netbeheer/referentiemodellen/IECCIM/TC57CIM/IEC61970/Base/Wires#PowerTransformer"/>
        <rdfs:range rdf:resource="https://w3id.org/netbeheer/referentiemodellen/IECCIM/TC57CIM/IEC61970/Base/Wires#TransformerTank"/>
        <rdfs:comment>All transformers that belong to this bank.Bank this transformer belongs to.</rdfs:comment>
    </owl:ObjectProperty>
    


    <!-- https://w3id.org/netbeheer/referentiemodellen/IECCIM/TC57CIM/IEC61970/Base/Wires#PowerTransformer_beforeShCircuitHighestOperatingCurrent -->


    <owl:ObjectProperty rdf:about="https://w3id.org/netbeheer/referentiemodellen/IECCIM/TC57CIM/IEC61970/Base/Wires#PowerTransformer_beforeShCircuitHighestOperatingCurrent">
        <rdfs:domain rdf:resource="https://w3id.org/netbeheer/referentiemodellen/IECCIM/TC57CIM/IEC61970/Base/Wires#PowerTransformer"/>
        <rdfs:range rdf:resource="https://w3id.org/netbeheer/referentiemodellen/IECCIM/TC57CIM/IEC61970/Base/Domain#CurrentFlow"/>
        <rdfs:comment>The highest operating current (Ib in the IEC 60909-0) before short circuit (depends on network configuration and relevant reliability philosophy). It is used for calculation of the impedance correction factor KT defined in IEC 60909-0.</rdfs:comment>
    </owl:ObjectProperty>
    


    <!-- https://w3id.org/netbeheer/referentiemodellen/IECCIM/TC57CIM/IEC61970/Base/Wires#PowerTransformer_beforeShCircuitHighestOperatingVoltage -->


    <owl:ObjectProperty rdf:about="https://w3id.org/netbeheer/referentiemodellen/IECCIM/TC57CIM/IEC61970/Base/Wires#PowerTransformer_beforeShCircuitHighestOperatingVoltage">
        <rdfs:domain rdf:resource="https://w3id.org/netbeheer/referentiemodellen/IECCIM/TC57CIM/IEC61970/Base/Wires#PowerTransformer"/>
        <rdfs:range rdf:resource="https://w3id.org/netbeheer/referentiemodellen/IECCIM/TC57CIM/IEC61970/Base/Domain#Voltage"/>
        <rdfs:comment>The highest operating voltage (Ub in the IEC 60909-0) before short circuit. It is used for calculation of the impedance correction factor KT defined in IEC 60909-0. This is worst case voltage on the low side winding (Section 3.7.1 in the standard). Used to define operating conditions.</rdfs:comment>
    </owl:ObjectProperty>
    


    <!-- https://w3id.org/netbeheer/referentiemodellen/IECCIM/TC57CIM/IEC61970/Base/Wires#PowerTransformer_beforeShortCircuitAnglePf -->


    <owl:ObjectProperty rdf:about="https://w3id.org/netbeheer/referentiemodellen/IECCIM/TC57CIM/IEC61970/Base/Wires#PowerTransformer_beforeShortCircuitAnglePf">
        <rdfs:domain rdf:resource="https://w3id.org/netbeheer/referentiemodellen/IECCIM/TC57CIM/IEC61970/Base/Wires#PowerTransformer"/>
        <rdfs:range rdf:resource="https://w3id.org/netbeheer/referentiemodellen/IECCIM/TC57CIM/IEC61970/Base/Domain#AngleDegrees"/>
        <rdfs:comment>The angle of power factor before short circuit (phib in the IEC 60909-0). It is used for calculation of the impedance correction factor KT defined in IEC 60909-0. This is the worst case power factor. Used to define operating conditions.</rdfs:comment>
    </owl:ObjectProperty>
    


    <!-- https://w3id.org/netbeheer/referentiemodellen/IECCIM/TC57CIM/IEC61970/Base/Wires#PowerTransformer_highSideMinOperatingU -->


    <owl:ObjectProperty rdf:about="https://w3id.org/netbeheer/referentiemodellen/IECCIM/TC57CIM/IEC61970/Base/Wires#PowerTransformer_highSideMinOperatingU">
        <rdfs:domain rdf:resource="https://w3id.org/netbeheer/referentiemodellen/IECCIM/TC57CIM/IEC61970/Base/Wires#PowerTransformer"/>
        <rdfs:range rdf:resource="https://w3id.org/netbeheer/referentiemodellen/IECCIM/TC57CIM/IEC61970/Base/Domain#Voltage"/>
        <rdfs:comment>The minimum operating voltage (uQmin in the IEC 60909-0) at the high voltage side (Q side) of the unit transformer of the power station unit. A value well established from long-term operating experience of the system. It is used for calculation of the impedance correction factor KG defined in IEC 60909-0</rdfs:comment>
    </owl:ObjectProperty>
    


    <!-- https://w3id.org/netbeheer/referentiemodellen/IECCIM/TC57CIM/IEC61970/Base/Wires#PrimeMover_SynchronousMachines -->


    <owl:ObjectProperty rdf:about="https://w3id.org/netbeheer/referentiemodellen/IECCIM/TC57CIM/IEC61970/Base/Wires#PrimeMover_SynchronousMachines">
        <rdfs:domain rdf:resource="https://w3id.org/netbeheer/referentiemodellen/IECCIM/TC57CIM/IEC61970/Base/Generation/GenerationTrainingSimulation#PrimeMover"/>
        <rdfs:range rdf:resource="https://w3id.org/netbeheer/referentiemodellen/IECCIM/TC57CIM/IEC61970/Base/Wires#SynchronousMachine"/>
        <rdfs:comment>Prime movers that drive this SynchronousMachine.Synchronous machines this Prime mover drives.</rdfs:comment>
    </owl:ObjectProperty>
    


    <!-- https://w3id.org/netbeheer/referentiemodellen/IECCIM/TC57CIM/IEC61970/Base/Wires#ProtectedSwitch_OperatedByProtectionEquipment -->


    <owl:ObjectProperty rdf:about="https://w3id.org/netbeheer/referentiemodellen/IECCIM/TC57CIM/IEC61970/Base/Wires#ProtectedSwitch_OperatedByProtectionEquipment">
        <owl:inverseOf rdf:resource="https://w3id.org/netbeheer/referentiemodellen/IECCIM/TC57CIM/IEC61970/Base/Wires#ProtectionEquipment_ProtectedSwitches"/>
        <rdfs:domain rdf:resource="https://w3id.org/netbeheer/referentiemodellen/IECCIM/TC57CIM/IEC61970/Base/Wires#ProtectedSwitch"/>
        <rdfs:range rdf:resource="https://w3id.org/netbeheer/referentiemodellen/IECCIM/TC57CIM/IEC61970/Base/Protection#ProtectionEquipment"/>
        <rdfs:comment>Protection equipments that operate this ProtectedSwitch.Protected switches operated by this ProtectionEquipment.</rdfs:comment>
    </owl:ObjectProperty>
    


    <!-- https://w3id.org/netbeheer/referentiemodellen/IECCIM/TC57CIM/IEC61970/Base/Wires#ProtectedSwitch_RecloseSequences -->


    <owl:ObjectProperty rdf:about="https://w3id.org/netbeheer/referentiemodellen/IECCIM/TC57CIM/IEC61970/Base/Wires#ProtectedSwitch_RecloseSequences">
        <owl:inverseOf rdf:resource="https://w3id.org/netbeheer/referentiemodellen/IECCIM/TC57CIM/IEC61970/Base/Wires#RecloseSequence_ProtectedSwitch"/>
        <rdf:type rdf:resource="http://www.w3.org/2002/07/owl#FunctionalProperty"/>
        <rdfs:domain rdf:resource="https://w3id.org/netbeheer/referentiemodellen/IECCIM/TC57CIM/IEC61970/Base/Wires#ProtectedSwitch"/>
        <rdfs:range rdf:resource="https://w3id.org/netbeheer/referentiemodellen/IECCIM/TC57CIM/IEC61970/Base/Protection#RecloseSequence"/>
        <rdfs:comment>A breaker may have zero or more automatic reclosures after a trip occurs.A breaker may have zero or more automatic reclosures after a trip occurs.</rdfs:comment>
    </owl:ObjectProperty>
    


    <!-- https://w3id.org/netbeheer/referentiemodellen/IECCIM/TC57CIM/IEC61970/Base/Wires#ProtectedSwitch_breakingCapacity -->


    <owl:ObjectProperty rdf:about="https://w3id.org/netbeheer/referentiemodellen/IECCIM/TC57CIM/IEC61970/Base/Wires#ProtectedSwitch_breakingCapacity">
        <rdfs:domain rdf:resource="https://w3id.org/netbeheer/referentiemodellen/IECCIM/TC57CIM/IEC61970/Base/Wires#ProtectedSwitch"/>
        <rdfs:range rdf:resource="https://w3id.org/netbeheer/referentiemodellen/IECCIM/TC57CIM/IEC61970/Base/Domain#CurrentFlow"/>
        <rdfs:comment>The maximum fault current a breaking device can break safely under prescribed conditions of use.
</rdfs:comment>
    </owl:ObjectProperty>
    


    <!-- https://w3id.org/netbeheer/referentiemodellen/IECCIM/TC57CIM/IEC61970/Base/Wires#ProtectionEquipment_ProtectedSwitches -->


    <owl:ObjectProperty rdf:about="https://w3id.org/netbeheer/referentiemodellen/IECCIM/TC57CIM/IEC61970/Base/Wires#ProtectionEquipment_ProtectedSwitches">
        <rdfs:domain rdf:resource="https://w3id.org/netbeheer/referentiemodellen/IECCIM/TC57CIM/IEC61970/Base/Protection#ProtectionEquipment"/>
        <rdfs:range rdf:resource="https://w3id.org/netbeheer/referentiemodellen/IECCIM/TC57CIM/IEC61970/Base/Wires#ProtectedSwitch"/>
        <rdfs:comment>Protection equipments that operate this ProtectedSwitch.Protected switches operated by this ProtectionEquipment.</rdfs:comment>
    </owl:ObjectProperty>
    


    <!-- https://w3id.org/netbeheer/referentiemodellen/IECCIM/TC57CIM/IEC61970/Base/Wires#ProtectiveActionRegulation_RegulatingControl -->


    <owl:ObjectProperty rdf:about="https://w3id.org/netbeheer/referentiemodellen/IECCIM/TC57CIM/IEC61970/Base/Wires#ProtectiveActionRegulation_RegulatingControl">
        <rdfs:domain rdf:resource="https://w3id.org/netbeheer/referentiemodellen/IECCIM/TC57CIM/IEC61970/InfIEC61970/InfSIPS#ProtectiveActionRegulation"/>
        <rdfs:range rdf:resource="https://w3id.org/netbeheer/referentiemodellen/IECCIM/TC57CIM/IEC61970/Base/Wires#RegulatingControl"/>
        <rdfs:comment></rdfs:comment>
    </owl:ObjectProperty>
    


    <!-- https://w3id.org/netbeheer/referentiemodellen/IECCIM/TC57CIM/IEC61970/Base/Wires#RatioTapChangerTablePoint_RatioTapChangerTable -->


    <owl:ObjectProperty rdf:about="https://w3id.org/netbeheer/referentiemodellen/IECCIM/TC57CIM/IEC61970/Base/Wires#RatioTapChangerTablePoint_RatioTapChangerTable">
        <rdfs:domain rdf:resource="https://w3id.org/netbeheer/referentiemodellen/IECCIM/TC57CIM/IEC61970/Base/Wires#RatioTapChangerTablePoint"/>
        <rdfs:range rdf:resource="https://w3id.org/netbeheer/referentiemodellen/IECCIM/TC57CIM/IEC61970/Base/Wires#RatioTapChangerTable"/>
        <rdfs:comment>Points of this table.Table of this point.</rdfs:comment>
    </owl:ObjectProperty>
    


    <!-- https://w3id.org/netbeheer/referentiemodellen/IECCIM/TC57CIM/IEC61970/Base/Wires#RatioTapChangerTable_RatioTapChanger -->


    <owl:ObjectProperty rdf:about="https://w3id.org/netbeheer/referentiemodellen/IECCIM/TC57CIM/IEC61970/Base/Wires#RatioTapChangerTable_RatioTapChanger">
        <owl:inverseOf rdf:resource="https://w3id.org/netbeheer/referentiemodellen/IECCIM/TC57CIM/IEC61970/Base/Wires#RatioTapChanger_RatioTapChangerTable"/>
        <rdfs:domain rdf:resource="https://w3id.org/netbeheer/referentiemodellen/IECCIM/TC57CIM/IEC61970/Base/Wires#RatioTapChangerTable"/>
        <rdfs:range rdf:resource="https://w3id.org/netbeheer/referentiemodellen/IECCIM/TC57CIM/IEC61970/Base/Wires#RatioTapChanger"/>
        <rdfs:comment>The ratio tap changer of this tap ratio table.The tap ratio table for this ratio  tap changer.</rdfs:comment>
    </owl:ObjectProperty>
    


    <!-- https://w3id.org/netbeheer/referentiemodellen/IECCIM/TC57CIM/IEC61970/Base/Wires#RatioTapChangerTable_RatioTapChangerTablePoint -->


    <owl:ObjectProperty rdf:about="https://w3id.org/netbeheer/referentiemodellen/IECCIM/TC57CIM/IEC61970/Base/Wires#RatioTapChangerTable_RatioTapChangerTablePoint">
        <owl:inverseOf rdf:resource="https://w3id.org/netbeheer/referentiemodellen/IECCIM/TC57CIM/IEC61970/Base/Wires#RatioTapChangerTablePoint_RatioTapChangerTable"/>
        <rdf:type rdf:resource="http://www.w3.org/2002/07/owl#FunctionalProperty"/>
        <rdfs:domain rdf:resource="https://w3id.org/netbeheer/referentiemodellen/IECCIM/TC57CIM/IEC61970/Base/Wires#RatioTapChangerTable"/>
        <rdfs:range rdf:resource="https://w3id.org/netbeheer/referentiemodellen/IECCIM/TC57CIM/IEC61970/Base/Wires#RatioTapChangerTablePoint"/>
        <rdfs:comment>Points of this table.Table of this point.</rdfs:comment>
    </owl:ObjectProperty>
    


    <!-- https://w3id.org/netbeheer/referentiemodellen/IECCIM/TC57CIM/IEC61970/Base/Wires#RatioTapChanger_RatioTapChangerTable -->


    <owl:ObjectProperty rdf:about="https://w3id.org/netbeheer/referentiemodellen/IECCIM/TC57CIM/IEC61970/Base/Wires#RatioTapChanger_RatioTapChangerTable">
        <rdfs:domain rdf:resource="https://w3id.org/netbeheer/referentiemodellen/IECCIM/TC57CIM/IEC61970/Base/Wires#RatioTapChanger"/>
        <rdfs:range rdf:resource="https://w3id.org/netbeheer/referentiemodellen/IECCIM/TC57CIM/IEC61970/Base/Wires#RatioTapChangerTable"/>
        <rdfs:comment>The ratio tap changer of this tap ratio table.The tap ratio table for this ratio  tap changer.</rdfs:comment>
    </owl:ObjectProperty>
    


    <!-- https://w3id.org/netbeheer/referentiemodellen/IECCIM/TC57CIM/IEC61970/Base/Wires#RatioTapChanger_TransformerEnd -->


    <owl:ObjectProperty rdf:about="https://w3id.org/netbeheer/referentiemodellen/IECCIM/TC57CIM/IEC61970/Base/Wires#RatioTapChanger_TransformerEnd">
        <owl:inverseOf rdf:resource="https://w3id.org/netbeheer/referentiemodellen/IECCIM/TC57CIM/IEC61970/Base/Wires#TransformerEnd_RatioTapChanger"/>
        <rdfs:domain rdf:resource="https://w3id.org/netbeheer/referentiemodellen/IECCIM/TC57CIM/IEC61970/Base/Wires#RatioTapChanger"/>
        <rdfs:range rdf:resource="https://w3id.org/netbeheer/referentiemodellen/IECCIM/TC57CIM/IEC61970/Base/Wires#TransformerEnd"/>
        <rdfs:comment>Transformer end to which this ratio tap changer belongs.Ratio tap changer associated with this transformer end.</rdfs:comment>
    </owl:ObjectProperty>
    


    <!-- https://w3id.org/netbeheer/referentiemodellen/IECCIM/TC57CIM/IEC61970/Base/Wires#RatioTapChanger_stepVoltageIncrement -->


    <owl:ObjectProperty rdf:about="https://w3id.org/netbeheer/referentiemodellen/IECCIM/TC57CIM/IEC61970/Base/Wires#RatioTapChanger_stepVoltageIncrement">
        <rdfs:domain rdf:resource="https://w3id.org/netbeheer/referentiemodellen/IECCIM/TC57CIM/IEC61970/Base/Wires#RatioTapChanger"/>
        <rdfs:range rdf:resource="https://w3id.org/netbeheer/referentiemodellen/IECCIM/TC57CIM/IEC61970/Base/Domain#PerCent"/>
        <rdfs:comment>Tap step increment, in per cent of nominal voltage, per step position.
</rdfs:comment>
    </owl:ObjectProperty>
    


    <!-- https://w3id.org/netbeheer/referentiemodellen/IECCIM/TC57CIM/IEC61970/Base/Wires#ReactiveCapabilityCurve_EquivalentInjection -->


    <owl:ObjectProperty rdf:about="https://w3id.org/netbeheer/referentiemodellen/IECCIM/TC57CIM/IEC61970/Base/Wires#ReactiveCapabilityCurve_EquivalentInjection">
        <rdfs:domain rdf:resource="https://w3id.org/netbeheer/referentiemodellen/IECCIM/TC57CIM/IEC61970/Base/Wires#ReactiveCapabilityCurve"/>
        <rdfs:range rdf:resource="https://w3id.org/netbeheer/referentiemodellen/IECCIM/TC57CIM/IEC61970/Base/Equivalents#EquivalentInjection"/>
        <rdfs:comment>The reactive capability curve used by this equivalent injection.The equivalent injection using this reactive capability curve.</rdfs:comment>
    </owl:ObjectProperty>
    


    <!-- https://w3id.org/netbeheer/referentiemodellen/IECCIM/TC57CIM/IEC61970/Base/Wires#ReactiveCapabilityCurve_InitiallyUsedBySynchronousMachines -->


    <owl:ObjectProperty rdf:about="https://w3id.org/netbeheer/referentiemodellen/IECCIM/TC57CIM/IEC61970/Base/Wires#ReactiveCapabilityCurve_InitiallyUsedBySynchronousMachines">
        <rdfs:domain rdf:resource="https://w3id.org/netbeheer/referentiemodellen/IECCIM/TC57CIM/IEC61970/Base/Wires#ReactiveCapabilityCurve"/>
        <rdfs:range rdf:resource="https://w3id.org/netbeheer/referentiemodellen/IECCIM/TC57CIM/IEC61970/Base/Wires#SynchronousMachine"/>
        <rdfs:comment>The default reactive capability curve for use by a synchronous machine.Synchronous machines using this curve as default.</rdfs:comment>
    </owl:ObjectProperty>
    


    <!-- https://w3id.org/netbeheer/referentiemodellen/IECCIM/TC57CIM/IEC61970/Base/Wires#ReactiveCapabilityCurve_SynchronousMachines -->


    <owl:ObjectProperty rdf:about="https://w3id.org/netbeheer/referentiemodellen/IECCIM/TC57CIM/IEC61970/Base/Wires#ReactiveCapabilityCurve_SynchronousMachines">
        <rdfs:domain rdf:resource="https://w3id.org/netbeheer/referentiemodellen/IECCIM/TC57CIM/IEC61970/Base/Wires#ReactiveCapabilityCurve"/>
        <rdfs:range rdf:resource="https://w3id.org/netbeheer/referentiemodellen/IECCIM/TC57CIM/IEC61970/Base/Wires#SynchronousMachine"/>
        <rdfs:comment>All available reactive capability curves for this synchronous machine.Synchronous machines using this curve.</rdfs:comment>
    </owl:ObjectProperty>
    


    <!-- https://w3id.org/netbeheer/referentiemodellen/IECCIM/TC57CIM/IEC61970/Base/Wires#ReactiveCapabilityCurve_coolantTemperature -->


    <owl:ObjectProperty rdf:about="https://w3id.org/netbeheer/referentiemodellen/IECCIM/TC57CIM/IEC61970/Base/Wires#ReactiveCapabilityCurve_coolantTemperature">
        <rdfs:domain rdf:resource="https://w3id.org/netbeheer/referentiemodellen/IECCIM/TC57CIM/IEC61970/Base/Wires#ReactiveCapabilityCurve"/>
        <rdfs:range rdf:resource="https://w3id.org/netbeheer/referentiemodellen/IECCIM/TC57CIM/IEC61970/Base/Domain#Temperature"/>
        <rdfs:comment>The machine&apos;s coolant temperature (e.g., ambient air or stator circulating water).</rdfs:comment>
    </owl:ObjectProperty>
    


    <!-- https://w3id.org/netbeheer/referentiemodellen/IECCIM/TC57CIM/IEC61970/Base/Wires#ReactiveCapabilityCurve_hydrogenPressure -->


    <owl:ObjectProperty rdf:about="https://w3id.org/netbeheer/referentiemodellen/IECCIM/TC57CIM/IEC61970/Base/Wires#ReactiveCapabilityCurve_hydrogenPressure">
        <rdfs:domain rdf:resource="https://w3id.org/netbeheer/referentiemodellen/IECCIM/TC57CIM/IEC61970/Base/Wires#ReactiveCapabilityCurve"/>
        <rdfs:range rdf:resource="https://w3id.org/netbeheer/referentiemodellen/IECCIM/TC57CIM/IEC61970/Base/Domain#Pressure"/>
        <rdfs:comment>The hydrogen coolant pressure</rdfs:comment>
    </owl:ObjectProperty>
    


    <!-- https://w3id.org/netbeheer/referentiemodellen/IECCIM/TC57CIM/IEC61970/Base/Wires#RecloseSequence_ProtectedSwitch -->


    <owl:ObjectProperty rdf:about="https://w3id.org/netbeheer/referentiemodellen/IECCIM/TC57CIM/IEC61970/Base/Wires#RecloseSequence_ProtectedSwitch">
        <rdfs:domain rdf:resource="https://w3id.org/netbeheer/referentiemodellen/IECCIM/TC57CIM/IEC61970/Base/Protection#RecloseSequence"/>
        <rdfs:range rdf:resource="https://w3id.org/netbeheer/referentiemodellen/IECCIM/TC57CIM/IEC61970/Base/Wires#ProtectedSwitch"/>
        <rdfs:comment>A breaker may have zero or more automatic reclosures after a trip occurs.A breaker may have zero or more automatic reclosures after a trip occurs.</rdfs:comment>
    </owl:ObjectProperty>
    


    <!-- https://w3id.org/netbeheer/referentiemodellen/IECCIM/TC57CIM/IEC61970/Base/Wires#RegulatingCondEq_RegulatingControl -->


    <owl:ObjectProperty rdf:about="https://w3id.org/netbeheer/referentiemodellen/IECCIM/TC57CIM/IEC61970/Base/Wires#RegulatingCondEq_RegulatingControl">
        <rdfs:domain rdf:resource="https://w3id.org/netbeheer/referentiemodellen/IECCIM/TC57CIM/IEC61970/Base/Wires#RegulatingCondEq"/>
        <rdfs:range rdf:resource="https://w3id.org/netbeheer/referentiemodellen/IECCIM/TC57CIM/IEC61970/Base/Wires#RegulatingControl"/>
        <rdfs:comment>The equipment that participates in this regulating control scheme.The regulating control scheme in which this equipment participates.</rdfs:comment>
    </owl:ObjectProperty>
    


    <!-- https://w3id.org/netbeheer/referentiemodellen/IECCIM/TC57CIM/IEC61970/Base/Wires#RegulatingControl_ProtectiveActionRegulation -->


    <owl:ObjectProperty rdf:about="https://w3id.org/netbeheer/referentiemodellen/IECCIM/TC57CIM/IEC61970/Base/Wires#RegulatingControl_ProtectiveActionRegulation">
        <owl:inverseOf rdf:resource="https://w3id.org/netbeheer/referentiemodellen/IECCIM/TC57CIM/IEC61970/Base/Wires#ProtectiveActionRegulation_RegulatingControl"/>
        <rdf:type rdf:resource="http://www.w3.org/2002/07/owl#FunctionalProperty"/>
        <rdfs:domain rdf:resource="https://w3id.org/netbeheer/referentiemodellen/IECCIM/TC57CIM/IEC61970/Base/Wires#RegulatingControl"/>
        <rdfs:range rdf:resource="https://w3id.org/netbeheer/referentiemodellen/IECCIM/TC57CIM/IEC61970/InfIEC61970/InfSIPS#ProtectiveActionRegulation"/>
        <rdfs:comment></rdfs:comment>
    </owl:ObjectProperty>
    


    <!-- https://w3id.org/netbeheer/referentiemodellen/IECCIM/TC57CIM/IEC61970/Base/Wires#RegulatingControl_RegulatingCondEq -->


    <owl:ObjectProperty rdf:about="https://w3id.org/netbeheer/referentiemodellen/IECCIM/TC57CIM/IEC61970/Base/Wires#RegulatingControl_RegulatingCondEq">
        <owl:inverseOf rdf:resource="https://w3id.org/netbeheer/referentiemodellen/IECCIM/TC57CIM/IEC61970/Base/Wires#RegulatingCondEq_RegulatingControl"/>
        <rdfs:domain rdf:resource="https://w3id.org/netbeheer/referentiemodellen/IECCIM/TC57CIM/IEC61970/Base/Wires#RegulatingControl"/>
        <rdfs:range rdf:resource="https://w3id.org/netbeheer/referentiemodellen/IECCIM/TC57CIM/IEC61970/Base/Wires#RegulatingCondEq"/>
        <rdfs:comment>The equipment that participates in this regulating control scheme.The regulating control scheme in which this equipment participates.</rdfs:comment>
    </owl:ObjectProperty>
    


    <!-- https://w3id.org/netbeheer/referentiemodellen/IECCIM/TC57CIM/IEC61970/Base/Wires#RegulatingControl_RegulationSchedule -->


    <owl:ObjectProperty rdf:about="https://w3id.org/netbeheer/referentiemodellen/IECCIM/TC57CIM/IEC61970/Base/Wires#RegulatingControl_RegulationSchedule">
        <owl:inverseOf rdf:resource="https://w3id.org/netbeheer/referentiemodellen/IECCIM/TC57CIM/IEC61970/Base/Wires#RegulationSchedule_RegulatingControl"/>
        <rdf:type rdf:resource="http://www.w3.org/2002/07/owl#FunctionalProperty"/>
        <rdfs:domain rdf:resource="https://w3id.org/netbeheer/referentiemodellen/IECCIM/TC57CIM/IEC61970/Base/Wires#RegulatingControl"/>
        <rdfs:range rdf:resource="https://w3id.org/netbeheer/referentiemodellen/IECCIM/TC57CIM/IEC61970/Base/Wires#RegulationSchedule"/>
        <rdfs:comment>Schedule for this Regulating regulating control.Regulating controls that have this Schedule.</rdfs:comment>
    </owl:ObjectProperty>
    


    <!-- https://w3id.org/netbeheer/referentiemodellen/IECCIM/TC57CIM/IEC61970/Base/Wires#RegulationSchedule_RegulatingControl -->


    <owl:ObjectProperty rdf:about="https://w3id.org/netbeheer/referentiemodellen/IECCIM/TC57CIM/IEC61970/Base/Wires#RegulationSchedule_RegulatingControl">
        <rdfs:domain rdf:resource="https://w3id.org/netbeheer/referentiemodellen/IECCIM/TC57CIM/IEC61970/Base/Wires#RegulationSchedule"/>
        <rdfs:range rdf:resource="https://w3id.org/netbeheer/referentiemodellen/IECCIM/TC57CIM/IEC61970/Base/Wires#RegulatingControl"/>
        <rdfs:comment>Schedule for this Regulating regulating control.Regulating controls that have this Schedule.</rdfs:comment>
    </owl:ObjectProperty>
    


    <!-- https://w3id.org/netbeheer/referentiemodellen/IECCIM/TC57CIM/IEC61970/Base/Wires#RegulationSchedule_VoltageControlZones -->


    <owl:ObjectProperty rdf:about="https://w3id.org/netbeheer/referentiemodellen/IECCIM/TC57CIM/IEC61970/Base/Wires#RegulationSchedule_VoltageControlZones">
        <rdfs:domain rdf:resource="https://w3id.org/netbeheer/referentiemodellen/IECCIM/TC57CIM/IEC61970/Base/Wires#RegulationSchedule"/>
        <rdfs:range rdf:resource="https://w3id.org/netbeheer/referentiemodellen/IECCIM/TC57CIM/IEC61970/Base/Wires#VoltageControlZone"/>
        <rdfs:comment>A VoltageControlZone may have a  voltage regulation schedule.A VoltageControlZone may have a  voltage regulation schedule.</rdfs:comment>
    </owl:ObjectProperty>
    


    <!-- https://w3id.org/netbeheer/referentiemodellen/IECCIM/TC57CIM/IEC61970/Base/Wires#RotatingMachine_GeneratingUnit -->


    <owl:ObjectProperty rdf:about="https://w3id.org/netbeheer/referentiemodellen/IECCIM/TC57CIM/IEC61970/Base/Wires#RotatingMachine_GeneratingUnit">
        <owl:inverseOf rdf:resource="https://w3id.org/netbeheer/referentiemodellen/IECCIM/TC57CIM/IEC61970/Base/Wires#GeneratingUnit_RotatingMachine"/>
        <rdfs:domain rdf:resource="https://w3id.org/netbeheer/referentiemodellen/IECCIM/TC57CIM/IEC61970/Base/Wires#RotatingMachine"/>
        <rdfs:range rdf:resource="https://w3id.org/netbeheer/referentiemodellen/IECCIM/TC57CIM/IEC61970/Base/Generation/Production#GeneratingUnit"/>
        <rdfs:comment>A synchronous machine may operate as a generator and as such becomes a member of a generating unit.A synchronous machine may operate as a generator and as such becomes a member of a generating unit.</rdfs:comment>
    </owl:ObjectProperty>
    


    <!-- https://w3id.org/netbeheer/referentiemodellen/IECCIM/TC57CIM/IEC61970/Base/Wires#RotatingMachine_HydroPump -->


    <owl:ObjectProperty rdf:about="https://w3id.org/netbeheer/referentiemodellen/IECCIM/TC57CIM/IEC61970/Base/Wires#RotatingMachine_HydroPump">
        <rdf:type rdf:resource="http://www.w3.org/2002/07/owl#FunctionalProperty"/>
        <rdfs:domain rdf:resource="https://w3id.org/netbeheer/referentiemodellen/IECCIM/TC57CIM/IEC61970/Base/Wires#RotatingMachine"/>
        <rdfs:range rdf:resource="https://w3id.org/netbeheer/referentiemodellen/IECCIM/TC57CIM/IEC61970/Base/Generation/Production#HydroPump"/>
        <rdfs:comment>The synchronous machine drives the turbine which moves the water from a low elevation to a higher elevation. The direction of machine rotation for pumping may or may not be the same as for generating.The synchronous machine drives the turbine which moves the water from a low elevation to a higher elevation. The direction of machine rotation for pumping may or may not be the same as for generating.</rdfs:comment>
    </owl:ObjectProperty>
    


    <!-- https://w3id.org/netbeheer/referentiemodellen/IECCIM/TC57CIM/IEC61970/Base/Wires#RotatingMachine_p -->


    <owl:ObjectProperty rdf:about="https://w3id.org/netbeheer/referentiemodellen/IECCIM/TC57CIM/IEC61970/Base/Wires#RotatingMachine_p">
        <rdfs:domain rdf:resource="https://w3id.org/netbeheer/referentiemodellen/IECCIM/TC57CIM/IEC61970/Base/Wires#RotatingMachine"/>
        <rdfs:range rdf:resource="https://w3id.org/netbeheer/referentiemodellen/IECCIM/TC57CIM/IEC61970/Base/Domain#ActivePower"/>
        <rdfs:comment>Active power injection. Load sign convention is used, i.e. positive sign means flow out from a node.
Starting value for a steady state solution.</rdfs:comment>
    </owl:ObjectProperty>
    


    <!-- https://w3id.org/netbeheer/referentiemodellen/IECCIM/TC57CIM/IEC61970/Base/Wires#RotatingMachine_q -->


    <owl:ObjectProperty rdf:about="https://w3id.org/netbeheer/referentiemodellen/IECCIM/TC57CIM/IEC61970/Base/Wires#RotatingMachine_q">
        <rdfs:domain rdf:resource="https://w3id.org/netbeheer/referentiemodellen/IECCIM/TC57CIM/IEC61970/Base/Wires#RotatingMachine"/>
        <rdfs:range rdf:resource="https://w3id.org/netbeheer/referentiemodellen/IECCIM/TC57CIM/IEC61970/Base/Domain#ReactivePower"/>
        <rdfs:comment>Reactive power injection. Load sign convention is used, i.e. positive sign means flow out from a node.
Starting value for a steady state solution.</rdfs:comment>
    </owl:ObjectProperty>
    


    <!-- https://w3id.org/netbeheer/referentiemodellen/IECCIM/TC57CIM/IEC61970/Base/Wires#RotatingMachine_ratedS -->


    <owl:ObjectProperty rdf:about="https://w3id.org/netbeheer/referentiemodellen/IECCIM/TC57CIM/IEC61970/Base/Wires#RotatingMachine_ratedS">
        <rdfs:domain rdf:resource="https://w3id.org/netbeheer/referentiemodellen/IECCIM/TC57CIM/IEC61970/Base/Wires#RotatingMachine"/>
        <rdfs:range rdf:resource="https://w3id.org/netbeheer/referentiemodellen/IECCIM/TC57CIM/IEC61970/Base/Domain#ApparentPower"/>
        <rdfs:comment>Nameplate apparent power rating for the unit.
The attribute shall have a positive value.</rdfs:comment>
    </owl:ObjectProperty>
    


    <!-- https://w3id.org/netbeheer/referentiemodellen/IECCIM/TC57CIM/IEC61970/Base/Wires#RotatingMachine_ratedU -->


    <owl:ObjectProperty rdf:about="https://w3id.org/netbeheer/referentiemodellen/IECCIM/TC57CIM/IEC61970/Base/Wires#RotatingMachine_ratedU">
        <rdfs:domain rdf:resource="https://w3id.org/netbeheer/referentiemodellen/IECCIM/TC57CIM/IEC61970/Base/Wires#RotatingMachine"/>
        <rdfs:range rdf:resource="https://w3id.org/netbeheer/referentiemodellen/IECCIM/TC57CIM/IEC61970/Base/Domain#Voltage"/>
        <rdfs:comment>Rated voltage (nameplate data, Ur in IEC 60909-0). It is primarily used for short circuit data exchange according to IEC 60909.</rdfs:comment>
    </owl:ObjectProperty>
    


    <!-- https://w3id.org/netbeheer/referentiemodellen/IECCIM/TC57CIM/IEC61970/Base/Wires#SeriesCompensator_r -->


    <owl:ObjectProperty rdf:about="https://w3id.org/netbeheer/referentiemodellen/IECCIM/TC57CIM/IEC61970/Base/Wires#SeriesCompensator_r">
        <rdfs:domain rdf:resource="https://w3id.org/netbeheer/referentiemodellen/IECCIM/TC57CIM/IEC61970/Base/Wires#SeriesCompensator"/>
        <rdfs:range rdf:resource="https://w3id.org/netbeheer/referentiemodellen/IECCIM/TC57CIM/IEC61970/Base/Domain#Resistance"/>
        <rdfs:comment>Positive sequence resistance.</rdfs:comment>
    </owl:ObjectProperty>
    


    <!-- https://w3id.org/netbeheer/referentiemodellen/IECCIM/TC57CIM/IEC61970/Base/Wires#SeriesCompensator_r0 -->


    <owl:ObjectProperty rdf:about="https://w3id.org/netbeheer/referentiemodellen/IECCIM/TC57CIM/IEC61970/Base/Wires#SeriesCompensator_r0">
        <rdfs:domain rdf:resource="https://w3id.org/netbeheer/referentiemodellen/IECCIM/TC57CIM/IEC61970/Base/Wires#SeriesCompensator"/>
        <rdfs:range rdf:resource="https://w3id.org/netbeheer/referentiemodellen/IECCIM/TC57CIM/IEC61970/Base/Domain#Resistance"/>
        <rdfs:comment>Zero sequence resistance.
</rdfs:comment>
    </owl:ObjectProperty>
    


    <!-- https://w3id.org/netbeheer/referentiemodellen/IECCIM/TC57CIM/IEC61970/Base/Wires#SeriesCompensator_varistorRatedCurrent -->


    <owl:ObjectProperty rdf:about="https://w3id.org/netbeheer/referentiemodellen/IECCIM/TC57CIM/IEC61970/Base/Wires#SeriesCompensator_varistorRatedCurrent">
        <rdfs:domain rdf:resource="https://w3id.org/netbeheer/referentiemodellen/IECCIM/TC57CIM/IEC61970/Base/Wires#SeriesCompensator"/>
        <rdfs:range rdf:resource="https://w3id.org/netbeheer/referentiemodellen/IECCIM/TC57CIM/IEC61970/Base/Domain#CurrentFlow"/>
        <rdfs:comment>The maximum current the varistor is designed to handle at specified duration.</rdfs:comment>
    </owl:ObjectProperty>
    


    <!-- https://w3id.org/netbeheer/referentiemodellen/IECCIM/TC57CIM/IEC61970/Base/Wires#SeriesCompensator_varistorVoltageThreshold -->


    <owl:ObjectProperty rdf:about="https://w3id.org/netbeheer/referentiemodellen/IECCIM/TC57CIM/IEC61970/Base/Wires#SeriesCompensator_varistorVoltageThreshold">
        <rdfs:domain rdf:resource="https://w3id.org/netbeheer/referentiemodellen/IECCIM/TC57CIM/IEC61970/Base/Wires#SeriesCompensator"/>
        <rdfs:range rdf:resource="https://w3id.org/netbeheer/referentiemodellen/IECCIM/TC57CIM/IEC61970/Base/Domain#Voltage"/>
        <rdfs:comment>The dc voltage at which the varistor start conducting.</rdfs:comment>
    </owl:ObjectProperty>
    


    <!-- https://w3id.org/netbeheer/referentiemodellen/IECCIM/TC57CIM/IEC61970/Base/Wires#SeriesCompensator_x -->


    <owl:ObjectProperty rdf:about="https://w3id.org/netbeheer/referentiemodellen/IECCIM/TC57CIM/IEC61970/Base/Wires#SeriesCompensator_x">
        <rdfs:domain rdf:resource="https://w3id.org/netbeheer/referentiemodellen/IECCIM/TC57CIM/IEC61970/Base/Wires#SeriesCompensator"/>
        <rdfs:range rdf:resource="https://w3id.org/netbeheer/referentiemodellen/IECCIM/TC57CIM/IEC61970/Base/Domain#Reactance"/>
        <rdfs:comment>Positive sequence reactance.</rdfs:comment>
    </owl:ObjectProperty>
    


    <!-- https://w3id.org/netbeheer/referentiemodellen/IECCIM/TC57CIM/IEC61970/Base/Wires#SeriesCompensator_x0 -->


    <owl:ObjectProperty rdf:about="https://w3id.org/netbeheer/referentiemodellen/IECCIM/TC57CIM/IEC61970/Base/Wires#SeriesCompensator_x0">
        <rdfs:domain rdf:resource="https://w3id.org/netbeheer/referentiemodellen/IECCIM/TC57CIM/IEC61970/Base/Wires#SeriesCompensator"/>
        <rdfs:range rdf:resource="https://w3id.org/netbeheer/referentiemodellen/IECCIM/TC57CIM/IEC61970/Base/Domain#Reactance"/>
        <rdfs:comment>Zero sequence reactance.
</rdfs:comment>
    </owl:ObjectProperty>
    


    <!-- https://w3id.org/netbeheer/referentiemodellen/IECCIM/TC57CIM/IEC61970/Base/Wires#ShuntCompensatorPhase_ShuntCompensator -->


    <owl:ObjectProperty rdf:about="https://w3id.org/netbeheer/referentiemodellen/IECCIM/TC57CIM/IEC61970/Base/Wires#ShuntCompensatorPhase_ShuntCompensator">
        <owl:inverseOf rdf:resource="https://w3id.org/netbeheer/referentiemodellen/IECCIM/TC57CIM/IEC61970/Base/Wires#ShuntCompensator_ShuntCompensatorPhase"/>
        <rdfs:domain rdf:resource="https://w3id.org/netbeheer/referentiemodellen/IECCIM/TC57CIM/IEC61970/Base/Wires#ShuntCompensatorPhase"/>
        <rdfs:range rdf:resource="https://w3id.org/netbeheer/referentiemodellen/IECCIM/TC57CIM/IEC61970/Base/Wires#ShuntCompensator"/>
        <rdfs:comment>Shunt compensator of this shunt compensator phase.The individual phases models for the shunt compensator.</rdfs:comment>
    </owl:ObjectProperty>
    


    <!-- https://w3id.org/netbeheer/referentiemodellen/IECCIM/TC57CIM/IEC61970/Base/Wires#ShuntCompensator_ShuntCompensatorPhase -->


    <owl:ObjectProperty rdf:about="https://w3id.org/netbeheer/referentiemodellen/IECCIM/TC57CIM/IEC61970/Base/Wires#ShuntCompensator_ShuntCompensatorPhase">
        <rdf:type rdf:resource="http://www.w3.org/2002/07/owl#FunctionalProperty"/>
        <rdfs:domain rdf:resource="https://w3id.org/netbeheer/referentiemodellen/IECCIM/TC57CIM/IEC61970/Base/Wires#ShuntCompensator"/>
        <rdfs:range rdf:resource="https://w3id.org/netbeheer/referentiemodellen/IECCIM/TC57CIM/IEC61970/Base/Wires#ShuntCompensatorPhase"/>
        <rdfs:comment>Shunt compensator of this shunt compensator phase.The individual phases models for the shunt compensator.</rdfs:comment>
    </owl:ObjectProperty>
    


    <!-- https://w3id.org/netbeheer/referentiemodellen/IECCIM/TC57CIM/IEC61970/Base/Wires#ShuntCompensator_SvShuntCompensatorSections -->


    <owl:ObjectProperty rdf:about="https://w3id.org/netbeheer/referentiemodellen/IECCIM/TC57CIM/IEC61970/Base/Wires#ShuntCompensator_SvShuntCompensatorSections">
        <owl:inverseOf rdf:resource="https://w3id.org/netbeheer/referentiemodellen/IECCIM/TC57CIM/IEC61970/Base/Wires#SvShuntCompensatorSections_ShuntCompensator"/>
        <rdf:type rdf:resource="http://www.w3.org/2002/07/owl#FunctionalProperty"/>
        <rdfs:domain rdf:resource="https://w3id.org/netbeheer/referentiemodellen/IECCIM/TC57CIM/IEC61970/Base/Wires#ShuntCompensator"/>
        <rdfs:range rdf:resource="https://w3id.org/netbeheer/referentiemodellen/IECCIM/TC57CIM/IEC61970/Base/StateVariables#SvShuntCompensatorSections"/>
        <rdfs:comment>The state for the number of shunt compensator sections in service.The shunt compensator for which the state applies.</rdfs:comment>
    </owl:ObjectProperty>
    


    <!-- https://w3id.org/netbeheer/referentiemodellen/IECCIM/TC57CIM/IEC61970/Base/Wires#ShuntCompensator_aVRDelay -->


    <owl:ObjectProperty rdf:about="https://w3id.org/netbeheer/referentiemodellen/IECCIM/TC57CIM/IEC61970/Base/Wires#ShuntCompensator_aVRDelay">
        <rdfs:domain rdf:resource="https://w3id.org/netbeheer/referentiemodellen/IECCIM/TC57CIM/IEC61970/Base/Wires#ShuntCompensator"/>
        <rdfs:range rdf:resource="https://w3id.org/netbeheer/referentiemodellen/IECCIM/TC57CIM/IEC61970/Base/Domain#Seconds"/>
        <rdfs:comment>Time delay required for the device to be connected or disconnected by automatic voltage regulation (AVR).</rdfs:comment>
    </owl:ObjectProperty>
    


    <!-- https://w3id.org/netbeheer/referentiemodellen/IECCIM/TC57CIM/IEC61970/Base/Wires#ShuntCompensator_nomU -->


    <owl:ObjectProperty rdf:about="https://w3id.org/netbeheer/referentiemodellen/IECCIM/TC57CIM/IEC61970/Base/Wires#ShuntCompensator_nomU">
        <rdfs:domain rdf:resource="https://w3id.org/netbeheer/referentiemodellen/IECCIM/TC57CIM/IEC61970/Base/Wires#ShuntCompensator"/>
        <rdfs:range rdf:resource="https://w3id.org/netbeheer/referentiemodellen/IECCIM/TC57CIM/IEC61970/Base/Domain#Voltage"/>
        <rdfs:comment>The voltage at which the nominal reactive power may be calculated. This should normally be within 10% of the voltage at which the capacitor is connected to the network.
</rdfs:comment>
    </owl:ObjectProperty>
    


    <!-- https://w3id.org/netbeheer/referentiemodellen/IECCIM/TC57CIM/IEC61970/Base/Wires#ShuntCompensator_voltageSensitivity -->


    <owl:ObjectProperty rdf:about="https://w3id.org/netbeheer/referentiemodellen/IECCIM/TC57CIM/IEC61970/Base/Wires#ShuntCompensator_voltageSensitivity">
        <rdfs:domain rdf:resource="https://w3id.org/netbeheer/referentiemodellen/IECCIM/TC57CIM/IEC61970/Base/Wires#ShuntCompensator"/>
        <rdfs:range rdf:resource="https://w3id.org/netbeheer/referentiemodellen/IECCIM/TC57CIM/IEC61970/Base/Domain#VoltagePerReactivePower"/>
        <rdfs:comment>Voltage sensitivity required for the device to regulate the bus voltage, in voltage/reactive power.</rdfs:comment>
    </owl:ObjectProperty>
    


    <!-- https://w3id.org/netbeheer/referentiemodellen/IECCIM/TC57CIM/IEC61970/Base/Wires#StaticVarCompensator_capacitiveRating -->


    <owl:ObjectProperty rdf:about="https://w3id.org/netbeheer/referentiemodellen/IECCIM/TC57CIM/IEC61970/Base/Wires#StaticVarCompensator_capacitiveRating">
        <rdfs:domain rdf:resource="https://w3id.org/netbeheer/referentiemodellen/IECCIM/TC57CIM/IEC61970/Base/Wires#StaticVarCompensator"/>
        <rdfs:range rdf:resource="https://w3id.org/netbeheer/referentiemodellen/IECCIM/TC57CIM/IEC61970/Base/Domain#Reactance"/>
        <rdfs:comment>Maximum available capacitive reactance.
</rdfs:comment>
    </owl:ObjectProperty>
    


    <!-- https://w3id.org/netbeheer/referentiemodellen/IECCIM/TC57CIM/IEC61970/Base/Wires#StaticVarCompensator_inductiveRating -->


    <owl:ObjectProperty rdf:about="https://w3id.org/netbeheer/referentiemodellen/IECCIM/TC57CIM/IEC61970/Base/Wires#StaticVarCompensator_inductiveRating">
        <rdfs:domain rdf:resource="https://w3id.org/netbeheer/referentiemodellen/IECCIM/TC57CIM/IEC61970/Base/Wires#StaticVarCompensator"/>
        <rdfs:range rdf:resource="https://w3id.org/netbeheer/referentiemodellen/IECCIM/TC57CIM/IEC61970/Base/Domain#Reactance"/>
        <rdfs:comment>Maximum available inductive reactance.
</rdfs:comment>
    </owl:ObjectProperty>
    


    <!-- https://w3id.org/netbeheer/referentiemodellen/IECCIM/TC57CIM/IEC61970/Base/Wires#StaticVarCompensator_q -->


    <owl:ObjectProperty rdf:about="https://w3id.org/netbeheer/referentiemodellen/IECCIM/TC57CIM/IEC61970/Base/Wires#StaticVarCompensator_q">
        <rdfs:domain rdf:resource="https://w3id.org/netbeheer/referentiemodellen/IECCIM/TC57CIM/IEC61970/Base/Wires#StaticVarCompensator"/>
        <rdfs:range rdf:resource="https://w3id.org/netbeheer/referentiemodellen/IECCIM/TC57CIM/IEC61970/Base/Domain#ReactivePower"/>
        <rdfs:comment>Reactive power injection. Load sign convention is used, i.e. positive sign means flow out from a node.
Starting value for a steady state solution.</rdfs:comment>
    </owl:ObjectProperty>
    


    <!-- https://w3id.org/netbeheer/referentiemodellen/IECCIM/TC57CIM/IEC61970/Base/Wires#StaticVarCompensator_slope -->


    <owl:ObjectProperty rdf:about="https://w3id.org/netbeheer/referentiemodellen/IECCIM/TC57CIM/IEC61970/Base/Wires#StaticVarCompensator_slope">
        <rdfs:domain rdf:resource="https://w3id.org/netbeheer/referentiemodellen/IECCIM/TC57CIM/IEC61970/Base/Wires#StaticVarCompensator"/>
        <rdfs:range rdf:resource="https://w3id.org/netbeheer/referentiemodellen/IECCIM/TC57CIM/IEC61970/Base/Domain#VoltagePerReactivePower"/>
        <rdfs:comment>The characteristics slope of an SVC defines how the reactive power output changes in proportion to the difference between the regulated bus voltage and the voltage setpoint.</rdfs:comment>
    </owl:ObjectProperty>
    


    <!-- https://w3id.org/netbeheer/referentiemodellen/IECCIM/TC57CIM/IEC61970/Base/Wires#StaticVarCompensator_voltageSetPoint -->


    <owl:ObjectProperty rdf:about="https://w3id.org/netbeheer/referentiemodellen/IECCIM/TC57CIM/IEC61970/Base/Wires#StaticVarCompensator_voltageSetPoint">
        <rdfs:domain rdf:resource="https://w3id.org/netbeheer/referentiemodellen/IECCIM/TC57CIM/IEC61970/Base/Wires#StaticVarCompensator"/>
        <rdfs:range rdf:resource="https://w3id.org/netbeheer/referentiemodellen/IECCIM/TC57CIM/IEC61970/Base/Domain#Voltage"/>
        <rdfs:comment>The reactive power output of the SVC is proportional to the difference between the voltage at the regulated bus and the voltage setpoint.  When the regulated bus voltage is equal to the voltage setpoint, the reactive power output is zero.</rdfs:comment>
    </owl:ObjectProperty>
    


    <!-- https://w3id.org/netbeheer/referentiemodellen/IECCIM/TC57CIM/IEC61970/Base/Wires#SvShuntCompensatorSections_ShuntCompensator -->


    <owl:ObjectProperty rdf:about="https://w3id.org/netbeheer/referentiemodellen/IECCIM/TC57CIM/IEC61970/Base/Wires#SvShuntCompensatorSections_ShuntCompensator">
        <rdfs:domain rdf:resource="https://w3id.org/netbeheer/referentiemodellen/IECCIM/TC57CIM/IEC61970/Base/StateVariables#SvShuntCompensatorSections"/>
        <rdfs:range rdf:resource="https://w3id.org/netbeheer/referentiemodellen/IECCIM/TC57CIM/IEC61970/Base/Wires#ShuntCompensator"/>
        <rdfs:comment>The state for the number of shunt compensator sections in service.The shunt compensator for which the state applies.</rdfs:comment>
    </owl:ObjectProperty>
    


    <!-- https://w3id.org/netbeheer/referentiemodellen/IECCIM/TC57CIM/IEC61970/Base/Wires#SvTapStep_TapChanger -->


    <owl:ObjectProperty rdf:about="https://w3id.org/netbeheer/referentiemodellen/IECCIM/TC57CIM/IEC61970/Base/Wires#SvTapStep_TapChanger">
        <rdfs:domain rdf:resource="https://w3id.org/netbeheer/referentiemodellen/IECCIM/TC57CIM/IEC61970/Base/StateVariables#SvTapStep"/>
        <rdfs:range rdf:resource="https://w3id.org/netbeheer/referentiemodellen/IECCIM/TC57CIM/IEC61970/Base/Wires#TapChanger"/>
        <rdfs:comment>The tap step state associated with the tap changer.The tap changer associated with the tap step state.</rdfs:comment>
    </owl:ObjectProperty>
    


    <!-- https://w3id.org/netbeheer/referentiemodellen/IECCIM/TC57CIM/IEC61970/Base/Wires#SwitchAction_OperatedSwitch -->


    <owl:ObjectProperty rdf:about="https://w3id.org/netbeheer/referentiemodellen/IECCIM/TC57CIM/IEC61970/Base/Wires#SwitchAction_OperatedSwitch">
        <rdfs:domain rdf:resource="https://w3id.org/netbeheer/referentiemodellen/IECCIM/TC57CIM/IEC61968/Operations#SwitchAction"/>
        <rdfs:range rdf:resource="https://w3id.org/netbeheer/referentiemodellen/IECCIM/TC57CIM/IEC61970/Base/Wires#Switch"/>
        <rdfs:comment>Action changing status of this switch.Switch that is the object of this switch action.</rdfs:comment>
    </owl:ObjectProperty>
    


    <!-- https://w3id.org/netbeheer/referentiemodellen/IECCIM/TC57CIM/IEC61970/Base/Wires#SwitchPhase_Switch -->


    <owl:ObjectProperty rdf:about="https://w3id.org/netbeheer/referentiemodellen/IECCIM/TC57CIM/IEC61970/Base/Wires#SwitchPhase_Switch">
        <owl:inverseOf rdf:resource="https://w3id.org/netbeheer/referentiemodellen/IECCIM/TC57CIM/IEC61970/Base/Wires#Switch_SwitchPhase"/>
        <rdfs:domain rdf:resource="https://w3id.org/netbeheer/referentiemodellen/IECCIM/TC57CIM/IEC61970/Base/Wires#SwitchPhase"/>
        <rdfs:range rdf:resource="https://w3id.org/netbeheer/referentiemodellen/IECCIM/TC57CIM/IEC61970/Base/Wires#Switch"/>
        <rdfs:comment>The switch of the switch phase.The individual switch phases for the switch.</rdfs:comment>
    </owl:ObjectProperty>
    


    <!-- https://w3id.org/netbeheer/referentiemodellen/IECCIM/TC57CIM/IEC61970/Base/Wires#SwitchSchedule_Switch -->


    <owl:ObjectProperty rdf:about="https://w3id.org/netbeheer/referentiemodellen/IECCIM/TC57CIM/IEC61970/Base/Wires#SwitchSchedule_Switch">
        <owl:inverseOf rdf:resource="https://w3id.org/netbeheer/referentiemodellen/IECCIM/TC57CIM/IEC61970/Base/Wires#Switch_SwitchSchedules"/>
        <rdfs:domain rdf:resource="https://w3id.org/netbeheer/referentiemodellen/IECCIM/TC57CIM/IEC61970/Base/Wires#SwitchSchedule"/>
        <rdfs:range rdf:resource="https://w3id.org/netbeheer/referentiemodellen/IECCIM/TC57CIM/IEC61970/Base/Wires#Switch"/>
        <rdfs:comment>A SwitchSchedule is associated with a Switch.A Switch can be associated with SwitchSchedules.</rdfs:comment>
    </owl:ObjectProperty>
    


    <!-- https://w3id.org/netbeheer/referentiemodellen/IECCIM/TC57CIM/IEC61970/Base/Wires#Switch_CompositeSwitch -->


    <owl:ObjectProperty rdf:about="https://w3id.org/netbeheer/referentiemodellen/IECCIM/TC57CIM/IEC61970/Base/Wires#Switch_CompositeSwitch">
        <owl:inverseOf rdf:resource="https://w3id.org/netbeheer/referentiemodellen/IECCIM/TC57CIM/IEC61970/Base/Wires#CompositeSwitch_Switches"/>
        <rdfs:domain rdf:resource="https://w3id.org/netbeheer/referentiemodellen/IECCIM/TC57CIM/IEC61970/Base/Wires#Switch"/>
        <rdfs:range rdf:resource="https://w3id.org/netbeheer/referentiemodellen/IECCIM/TC57CIM/IEC61970/Base/Wires#CompositeSwitch"/>
        <rdfs:comment>Composite switch to which this Switch belongs.Switches contained in this Composite switch.</rdfs:comment>
    </owl:ObjectProperty>
    


    <!-- https://w3id.org/netbeheer/referentiemodellen/IECCIM/TC57CIM/IEC61970/Base/Wires#Switch_ConnectDisconnectFunctions -->


    <owl:ObjectProperty rdf:about="https://w3id.org/netbeheer/referentiemodellen/IECCIM/TC57CIM/IEC61970/Base/Wires#Switch_ConnectDisconnectFunctions">
        <owl:inverseOf rdf:resource="https://w3id.org/netbeheer/referentiemodellen/IECCIM/TC57CIM/IEC61970/Base/Wires#ConnectDisconnectFunction_Switches"/>
        <rdfs:domain rdf:resource="https://w3id.org/netbeheer/referentiemodellen/IECCIM/TC57CIM/IEC61970/Base/Wires#Switch"/>
        <rdfs:range rdf:resource="https://w3id.org/netbeheer/referentiemodellen/IECCIM/TC57CIM/IEC61968/LoadControl#ConnectDisconnectFunction"/>
        <rdfs:comment></rdfs:comment>
    </owl:ObjectProperty>
    


    <!-- https://w3id.org/netbeheer/referentiemodellen/IECCIM/TC57CIM/IEC61970/Base/Wires#Switch_Outage -->


    <owl:ObjectProperty rdf:about="https://w3id.org/netbeheer/referentiemodellen/IECCIM/TC57CIM/IEC61970/Base/Wires#Switch_Outage">
        <owl:inverseOf rdf:resource="https://w3id.org/netbeheer/referentiemodellen/IECCIM/TC57CIM/IEC61970/Base/Wires#Outage_OpenedSwitches"/>
        <rdfs:domain rdf:resource="https://w3id.org/netbeheer/referentiemodellen/IECCIM/TC57CIM/IEC61970/Base/Wires#Switch"/>
        <rdfs:range rdf:resource="https://w3id.org/netbeheer/referentiemodellen/IECCIM/TC57CIM/IEC61968/Operations#Outage"/>
        <rdfs:comment>Current outage of this protective device.All potentially open switches causing this outage. This realationship is meant to be used as &quot;indication&quot; for initiation of outage-related business processes, whereas for actual actions of switches, SwitchAction-Switch relationship should be used.</rdfs:comment>
    </owl:ObjectProperty>
    


    <!-- https://w3id.org/netbeheer/referentiemodellen/IECCIM/TC57CIM/IEC61970/Base/Wires#Switch_SwitchAction -->


    <owl:ObjectProperty rdf:about="https://w3id.org/netbeheer/referentiemodellen/IECCIM/TC57CIM/IEC61970/Base/Wires#Switch_SwitchAction">
        <owl:inverseOf rdf:resource="https://w3id.org/netbeheer/referentiemodellen/IECCIM/TC57CIM/IEC61970/Base/Wires#SwitchAction_OperatedSwitch"/>
        <rdfs:domain rdf:resource="https://w3id.org/netbeheer/referentiemodellen/IECCIM/TC57CIM/IEC61970/Base/Wires#Switch"/>
        <rdfs:range rdf:resource="https://w3id.org/netbeheer/referentiemodellen/IECCIM/TC57CIM/IEC61968/Operations#SwitchAction"/>
        <rdfs:comment>Action changing status of this switch.Switch that is the object of this switch action.</rdfs:comment>
    </owl:ObjectProperty>
    


    <!-- https://w3id.org/netbeheer/referentiemodellen/IECCIM/TC57CIM/IEC61970/Base/Wires#Switch_SwitchPhase -->


    <owl:ObjectProperty rdf:about="https://w3id.org/netbeheer/referentiemodellen/IECCIM/TC57CIM/IEC61970/Base/Wires#Switch_SwitchPhase">
        <rdf:type rdf:resource="http://www.w3.org/2002/07/owl#FunctionalProperty"/>
        <rdfs:domain rdf:resource="https://w3id.org/netbeheer/referentiemodellen/IECCIM/TC57CIM/IEC61970/Base/Wires#Switch"/>
        <rdfs:range rdf:resource="https://w3id.org/netbeheer/referentiemodellen/IECCIM/TC57CIM/IEC61970/Base/Wires#SwitchPhase"/>
        <rdfs:comment>The switch of the switch phase.The individual switch phases for the switch.</rdfs:comment>
    </owl:ObjectProperty>
    


    <!-- https://w3id.org/netbeheer/referentiemodellen/IECCIM/TC57CIM/IEC61970/Base/Wires#Switch_SwitchSchedules -->


    <owl:ObjectProperty rdf:about="https://w3id.org/netbeheer/referentiemodellen/IECCIM/TC57CIM/IEC61970/Base/Wires#Switch_SwitchSchedules">
        <rdf:type rdf:resource="http://www.w3.org/2002/07/owl#FunctionalProperty"/>
        <rdfs:domain rdf:resource="https://w3id.org/netbeheer/referentiemodellen/IECCIM/TC57CIM/IEC61970/Base/Wires#Switch"/>
        <rdfs:range rdf:resource="https://w3id.org/netbeheer/referentiemodellen/IECCIM/TC57CIM/IEC61970/Base/Wires#SwitchSchedule"/>
        <rdfs:comment>A SwitchSchedule is associated with a Switch.A Switch can be associated with SwitchSchedules.</rdfs:comment>
    </owl:ObjectProperty>
    


    <!-- https://w3id.org/netbeheer/referentiemodellen/IECCIM/TC57CIM/IEC61970/Base/Wires#Switch_ratedCurrent -->


    <owl:ObjectProperty rdf:about="https://w3id.org/netbeheer/referentiemodellen/IECCIM/TC57CIM/IEC61970/Base/Wires#Switch_ratedCurrent">
        <rdfs:domain rdf:resource="https://w3id.org/netbeheer/referentiemodellen/IECCIM/TC57CIM/IEC61970/Base/Wires#Switch"/>
        <rdfs:range rdf:resource="https://w3id.org/netbeheer/referentiemodellen/IECCIM/TC57CIM/IEC61970/Base/Domain#CurrentFlow"/>
        <rdfs:comment>The maximum continuous current carrying capacity in amps governed by the device material and construction.
</rdfs:comment>
    </owl:ObjectProperty>
    


    <!-- https://w3id.org/netbeheer/referentiemodellen/IECCIM/TC57CIM/IEC61970/Base/Wires#SynchronousMachineDynamics_SynchronousMachine -->


    <owl:ObjectProperty rdf:about="https://w3id.org/netbeheer/referentiemodellen/IECCIM/TC57CIM/IEC61970/Base/Wires#SynchronousMachineDynamics_SynchronousMachine">
        <rdfs:domain rdf:resource="https://w3id.org/netbeheer/referentiemodellen/IECCIM/TC57CIM/IEC61970/Dynamics/StandardModels/SynchronousMachineDynamics#SynchronousMachineDynamics"/>
        <rdfs:range rdf:resource="https://w3id.org/netbeheer/referentiemodellen/IECCIM/TC57CIM/IEC61970/Base/Wires#SynchronousMachine"/>
        <rdfs:comment>Synchronous machine dynamics model used to describe dynamic behavior of this synchronous machine.Synchronous machine to which synchronous machine dynamics model applies.</rdfs:comment>
    </owl:ObjectProperty>
    


    <!-- https://w3id.org/netbeheer/referentiemodellen/IECCIM/TC57CIM/IEC61970/Base/Wires#SynchronousMachine_InitialReactiveCapabilityCurve -->


    <owl:ObjectProperty rdf:about="https://w3id.org/netbeheer/referentiemodellen/IECCIM/TC57CIM/IEC61970/Base/Wires#SynchronousMachine_InitialReactiveCapabilityCurve">
        <owl:inverseOf rdf:resource="https://w3id.org/netbeheer/referentiemodellen/IECCIM/TC57CIM/IEC61970/Base/Wires#ReactiveCapabilityCurve_InitiallyUsedBySynchronousMachines"/>
        <rdfs:domain rdf:resource="https://w3id.org/netbeheer/referentiemodellen/IECCIM/TC57CIM/IEC61970/Base/Wires#SynchronousMachine"/>
        <rdfs:range rdf:resource="https://w3id.org/netbeheer/referentiemodellen/IECCIM/TC57CIM/IEC61970/Base/Wires#ReactiveCapabilityCurve"/>
        <rdfs:comment>The default reactive capability curve for use by a synchronous machine.Synchronous machines using this curve as default.</rdfs:comment>
    </owl:ObjectProperty>
    


    <!-- https://w3id.org/netbeheer/referentiemodellen/IECCIM/TC57CIM/IEC61970/Base/Wires#SynchronousMachine_PrimeMovers -->


    <owl:ObjectProperty rdf:about="https://w3id.org/netbeheer/referentiemodellen/IECCIM/TC57CIM/IEC61970/Base/Wires#SynchronousMachine_PrimeMovers">
        <owl:inverseOf rdf:resource="https://w3id.org/netbeheer/referentiemodellen/IECCIM/TC57CIM/IEC61970/Base/Wires#PrimeMover_SynchronousMachines"/>
        <rdfs:domain rdf:resource="https://w3id.org/netbeheer/referentiemodellen/IECCIM/TC57CIM/IEC61970/Base/Wires#SynchronousMachine"/>
        <rdfs:range rdf:resource="https://w3id.org/netbeheer/referentiemodellen/IECCIM/TC57CIM/IEC61970/Base/Generation/GenerationTrainingSimulation#PrimeMover"/>
        <rdfs:comment>Prime movers that drive this SynchronousMachine.Synchronous machines this Prime mover drives.</rdfs:comment>
    </owl:ObjectProperty>
    


    <!-- https://w3id.org/netbeheer/referentiemodellen/IECCIM/TC57CIM/IEC61970/Base/Wires#SynchronousMachine_ReactiveCapabilityCurves -->


    <owl:ObjectProperty rdf:about="https://w3id.org/netbeheer/referentiemodellen/IECCIM/TC57CIM/IEC61970/Base/Wires#SynchronousMachine_ReactiveCapabilityCurves">
        <owl:inverseOf rdf:resource="https://w3id.org/netbeheer/referentiemodellen/IECCIM/TC57CIM/IEC61970/Base/Wires#ReactiveCapabilityCurve_SynchronousMachines"/>
        <rdfs:domain rdf:resource="https://w3id.org/netbeheer/referentiemodellen/IECCIM/TC57CIM/IEC61970/Base/Wires#SynchronousMachine"/>
        <rdfs:range rdf:resource="https://w3id.org/netbeheer/referentiemodellen/IECCIM/TC57CIM/IEC61970/Base/Wires#ReactiveCapabilityCurve"/>
        <rdfs:comment>All available reactive capability curves for this synchronous machine.Synchronous machines using this curve.</rdfs:comment>
    </owl:ObjectProperty>
    


    <!-- https://w3id.org/netbeheer/referentiemodellen/IECCIM/TC57CIM/IEC61970/Base/Wires#SynchronousMachine_SynchronousMachineDynamics -->


    <owl:ObjectProperty rdf:about="https://w3id.org/netbeheer/referentiemodellen/IECCIM/TC57CIM/IEC61970/Base/Wires#SynchronousMachine_SynchronousMachineDynamics">
        <owl:inverseOf rdf:resource="https://w3id.org/netbeheer/referentiemodellen/IECCIM/TC57CIM/IEC61970/Base/Wires#SynchronousMachineDynamics_SynchronousMachine"/>
        <rdf:type rdf:resource="http://www.w3.org/2002/07/owl#FunctionalProperty"/>
        <rdfs:domain rdf:resource="https://w3id.org/netbeheer/referentiemodellen/IECCIM/TC57CIM/IEC61970/Base/Wires#SynchronousMachine"/>
        <rdfs:range rdf:resource="https://w3id.org/netbeheer/referentiemodellen/IECCIM/TC57CIM/IEC61970/Dynamics/StandardModels/SynchronousMachineDynamics#SynchronousMachineDynamics"/>
        <rdfs:comment>Synchronous machine dynamics model used to describe dynamic behavior of this synchronous machine.Synchronous machine to which synchronous machine dynamics model applies.</rdfs:comment>
    </owl:ObjectProperty>
    


    <!-- https://w3id.org/netbeheer/referentiemodellen/IECCIM/TC57CIM/IEC61970/Base/Wires#SynchronousMachine_aVRToManualLag -->


    <owl:ObjectProperty rdf:about="https://w3id.org/netbeheer/referentiemodellen/IECCIM/TC57CIM/IEC61970/Base/Wires#SynchronousMachine_aVRToManualLag">
        <rdfs:domain rdf:resource="https://w3id.org/netbeheer/referentiemodellen/IECCIM/TC57CIM/IEC61970/Base/Wires#SynchronousMachine"/>
        <rdfs:range rdf:resource="https://w3id.org/netbeheer/referentiemodellen/IECCIM/TC57CIM/IEC61970/Base/Domain#Seconds"/>
        <rdfs:comment>Time delay required when switching from Automatic Voltage Regulation (AVR) to Manual for a lagging MVAr violation.</rdfs:comment>
    </owl:ObjectProperty>
    


    <!-- https://w3id.org/netbeheer/referentiemodellen/IECCIM/TC57CIM/IEC61970/Base/Wires#SynchronousMachine_aVRToManualLead -->


    <owl:ObjectProperty rdf:about="https://w3id.org/netbeheer/referentiemodellen/IECCIM/TC57CIM/IEC61970/Base/Wires#SynchronousMachine_aVRToManualLead">
        <rdfs:domain rdf:resource="https://w3id.org/netbeheer/referentiemodellen/IECCIM/TC57CIM/IEC61970/Base/Wires#SynchronousMachine"/>
        <rdfs:range rdf:resource="https://w3id.org/netbeheer/referentiemodellen/IECCIM/TC57CIM/IEC61970/Base/Domain#Seconds"/>
        <rdfs:comment>Time delay required when switching from Automatic Voltage Regulation (AVR) to Manual for a leading MVAr violation.</rdfs:comment>
    </owl:ObjectProperty>
    


    <!-- https://w3id.org/netbeheer/referentiemodellen/IECCIM/TC57CIM/IEC61970/Base/Wires#SynchronousMachine_baseQ -->


    <owl:ObjectProperty rdf:about="https://w3id.org/netbeheer/referentiemodellen/IECCIM/TC57CIM/IEC61970/Base/Wires#SynchronousMachine_baseQ">
        <rdfs:domain rdf:resource="https://w3id.org/netbeheer/referentiemodellen/IECCIM/TC57CIM/IEC61970/Base/Wires#SynchronousMachine"/>
        <rdfs:range rdf:resource="https://w3id.org/netbeheer/referentiemodellen/IECCIM/TC57CIM/IEC61970/Base/Domain#ReactivePower"/>
        <rdfs:comment>Default base reactive power value. This value represents the initial reactive power that can be used by any application function.</rdfs:comment>
    </owl:ObjectProperty>
    


    <!-- https://w3id.org/netbeheer/referentiemodellen/IECCIM/TC57CIM/IEC61970/Base/Wires#SynchronousMachine_condenserP -->


    <owl:ObjectProperty rdf:about="https://w3id.org/netbeheer/referentiemodellen/IECCIM/TC57CIM/IEC61970/Base/Wires#SynchronousMachine_condenserP">
        <rdfs:domain rdf:resource="https://w3id.org/netbeheer/referentiemodellen/IECCIM/TC57CIM/IEC61970/Base/Wires#SynchronousMachine"/>
        <rdfs:range rdf:resource="https://w3id.org/netbeheer/referentiemodellen/IECCIM/TC57CIM/IEC61970/Base/Domain#ActivePower"/>
        <rdfs:comment>Active power consumed when in condenser mode operation.</rdfs:comment>
    </owl:ObjectProperty>
    


    <!-- https://w3id.org/netbeheer/referentiemodellen/IECCIM/TC57CIM/IEC61970/Base/Wires#SynchronousMachine_earthingStarPointR -->


    <owl:ObjectProperty rdf:about="https://w3id.org/netbeheer/referentiemodellen/IECCIM/TC57CIM/IEC61970/Base/Wires#SynchronousMachine_earthingStarPointR">
        <rdfs:domain rdf:resource="https://w3id.org/netbeheer/referentiemodellen/IECCIM/TC57CIM/IEC61970/Base/Wires#SynchronousMachine"/>
        <rdfs:range rdf:resource="https://w3id.org/netbeheer/referentiemodellen/IECCIM/TC57CIM/IEC61970/Base/Domain#Resistance"/>
        <rdfs:comment>Generator star point earthing resistance (Re). Used for short circuit data exchange according to IEC 60909</rdfs:comment>
    </owl:ObjectProperty>
    


    <!-- https://w3id.org/netbeheer/referentiemodellen/IECCIM/TC57CIM/IEC61970/Base/Wires#SynchronousMachine_earthingStarPointX -->


    <owl:ObjectProperty rdf:about="https://w3id.org/netbeheer/referentiemodellen/IECCIM/TC57CIM/IEC61970/Base/Wires#SynchronousMachine_earthingStarPointX">
        <rdfs:domain rdf:resource="https://w3id.org/netbeheer/referentiemodellen/IECCIM/TC57CIM/IEC61970/Base/Wires#SynchronousMachine"/>
        <rdfs:range rdf:resource="https://w3id.org/netbeheer/referentiemodellen/IECCIM/TC57CIM/IEC61970/Base/Domain#Reactance"/>
        <rdfs:comment>Generator star point earthing reactance (Xe). Used for short circuit data exchange according to IEC 60909</rdfs:comment>
    </owl:ObjectProperty>
    


    <!-- https://w3id.org/netbeheer/referentiemodellen/IECCIM/TC57CIM/IEC61970/Base/Wires#SynchronousMachine_ikk -->


    <owl:ObjectProperty rdf:about="https://w3id.org/netbeheer/referentiemodellen/IECCIM/TC57CIM/IEC61970/Base/Wires#SynchronousMachine_ikk">
        <rdfs:domain rdf:resource="https://w3id.org/netbeheer/referentiemodellen/IECCIM/TC57CIM/IEC61970/Base/Wires#SynchronousMachine"/>
        <rdfs:range rdf:resource="https://w3id.org/netbeheer/referentiemodellen/IECCIM/TC57CIM/IEC61970/Base/Domain#CurrentFlow"/>
        <rdfs:comment>Steady-state short-circuit current (in A for the profile) of generator with compound excitation during 3-phase short circuit.
- Ikk=0: Generator with no compound excitation.
- Ikk?0: Generator with compound excitation.
Ikk is used to calculate the minimum steady-state short-circuit current for generators with compound excitation
(Section 4.6.1.2 in the IEC 60909-0)
Used only for single fed short circuit on a generator. (Section 4.3.4.2. in the IEC 60909-0)</rdfs:comment>
    </owl:ObjectProperty>
    


    <!-- https://w3id.org/netbeheer/referentiemodellen/IECCIM/TC57CIM/IEC61970/Base/Wires#SynchronousMachine_manualToAVR -->


    <owl:ObjectProperty rdf:about="https://w3id.org/netbeheer/referentiemodellen/IECCIM/TC57CIM/IEC61970/Base/Wires#SynchronousMachine_manualToAVR">
        <rdfs:domain rdf:resource="https://w3id.org/netbeheer/referentiemodellen/IECCIM/TC57CIM/IEC61970/Base/Wires#SynchronousMachine"/>
        <rdfs:range rdf:resource="https://w3id.org/netbeheer/referentiemodellen/IECCIM/TC57CIM/IEC61970/Base/Domain#Seconds"/>
        <rdfs:comment>Time delay required when switching from Manual to Automatic Voltage Regulation. This value is used in the accelerating power reference frame for powerflow solutions</rdfs:comment>
    </owl:ObjectProperty>
    


    <!-- https://w3id.org/netbeheer/referentiemodellen/IECCIM/TC57CIM/IEC61970/Base/Wires#SynchronousMachine_maxQ -->


    <owl:ObjectProperty rdf:about="https://w3id.org/netbeheer/referentiemodellen/IECCIM/TC57CIM/IEC61970/Base/Wires#SynchronousMachine_maxQ">
        <rdfs:domain rdf:resource="https://w3id.org/netbeheer/referentiemodellen/IECCIM/TC57CIM/IEC61970/Base/Wires#SynchronousMachine"/>
        <rdfs:range rdf:resource="https://w3id.org/netbeheer/referentiemodellen/IECCIM/TC57CIM/IEC61970/Base/Domain#ReactivePower"/>
        <rdfs:comment>Maximum reactive power limit. This is the maximum (nameplate) limit for the unit.</rdfs:comment>
    </owl:ObjectProperty>
    


    <!-- https://w3id.org/netbeheer/referentiemodellen/IECCIM/TC57CIM/IEC61970/Base/Wires#SynchronousMachine_maxU -->


    <owl:ObjectProperty rdf:about="https://w3id.org/netbeheer/referentiemodellen/IECCIM/TC57CIM/IEC61970/Base/Wires#SynchronousMachine_maxU">
        <rdfs:domain rdf:resource="https://w3id.org/netbeheer/referentiemodellen/IECCIM/TC57CIM/IEC61970/Base/Wires#SynchronousMachine"/>
        <rdfs:range rdf:resource="https://w3id.org/netbeheer/referentiemodellen/IECCIM/TC57CIM/IEC61970/Base/Domain#Voltage"/>
        <rdfs:comment>Maximum voltage limit for the unit.</rdfs:comment>
    </owl:ObjectProperty>
    


    <!-- https://w3id.org/netbeheer/referentiemodellen/IECCIM/TC57CIM/IEC61970/Base/Wires#SynchronousMachine_minQ -->


    <owl:ObjectProperty rdf:about="https://w3id.org/netbeheer/referentiemodellen/IECCIM/TC57CIM/IEC61970/Base/Wires#SynchronousMachine_minQ">
        <rdfs:domain rdf:resource="https://w3id.org/netbeheer/referentiemodellen/IECCIM/TC57CIM/IEC61970/Base/Wires#SynchronousMachine"/>
        <rdfs:range rdf:resource="https://w3id.org/netbeheer/referentiemodellen/IECCIM/TC57CIM/IEC61970/Base/Domain#ReactivePower"/>
        <rdfs:comment>Minimum reactive power limit for the unit.</rdfs:comment>
    </owl:ObjectProperty>
    


    <!-- https://w3id.org/netbeheer/referentiemodellen/IECCIM/TC57CIM/IEC61970/Base/Wires#SynchronousMachine_minU -->


    <owl:ObjectProperty rdf:about="https://w3id.org/netbeheer/referentiemodellen/IECCIM/TC57CIM/IEC61970/Base/Wires#SynchronousMachine_minU">
        <rdfs:domain rdf:resource="https://w3id.org/netbeheer/referentiemodellen/IECCIM/TC57CIM/IEC61970/Base/Wires#SynchronousMachine"/>
        <rdfs:range rdf:resource="https://w3id.org/netbeheer/referentiemodellen/IECCIM/TC57CIM/IEC61970/Base/Domain#Voltage"/>
        <rdfs:comment>Minimum voltage  limit for the unit.</rdfs:comment>
    </owl:ObjectProperty>
    


    <!-- https://w3id.org/netbeheer/referentiemodellen/IECCIM/TC57CIM/IEC61970/Base/Wires#SynchronousMachine_qPercent -->


    <owl:ObjectProperty rdf:about="https://w3id.org/netbeheer/referentiemodellen/IECCIM/TC57CIM/IEC61970/Base/Wires#SynchronousMachine_qPercent">
        <rdfs:domain rdf:resource="https://w3id.org/netbeheer/referentiemodellen/IECCIM/TC57CIM/IEC61970/Base/Wires#SynchronousMachine"/>
        <rdfs:range rdf:resource="https://w3id.org/netbeheer/referentiemodellen/IECCIM/TC57CIM/IEC61970/Base/Domain#PerCent"/>
        <rdfs:comment>Percent of the coordinated reactive control that comes from this machine.</rdfs:comment>
    </owl:ObjectProperty>
    


    <!-- https://w3id.org/netbeheer/referentiemodellen/IECCIM/TC57CIM/IEC61970/Base/Wires#SynchronousMachine_r -->


    <owl:ObjectProperty rdf:about="https://w3id.org/netbeheer/referentiemodellen/IECCIM/TC57CIM/IEC61970/Base/Wires#SynchronousMachine_r">
        <rdfs:domain rdf:resource="https://w3id.org/netbeheer/referentiemodellen/IECCIM/TC57CIM/IEC61970/Base/Wires#SynchronousMachine"/>
        <rdfs:range rdf:resource="https://w3id.org/netbeheer/referentiemodellen/IECCIM/TC57CIM/IEC61970/Base/Domain#Resistance"/>
        <rdfs:comment>Equivalent resistance (RG) of generator. RG is considered for the calculation of all currents, except for the calculation of the peak current ip. Used for short circuit data exchange according to IEC 60909</rdfs:comment>
    </owl:ObjectProperty>
    


    <!-- https://w3id.org/netbeheer/referentiemodellen/IECCIM/TC57CIM/IEC61970/Base/Wires#SynchronousMachine_r0 -->


    <owl:ObjectProperty rdf:about="https://w3id.org/netbeheer/referentiemodellen/IECCIM/TC57CIM/IEC61970/Base/Wires#SynchronousMachine_r0">
        <rdfs:domain rdf:resource="https://w3id.org/netbeheer/referentiemodellen/IECCIM/TC57CIM/IEC61970/Base/Wires#SynchronousMachine"/>
        <rdfs:range rdf:resource="https://w3id.org/netbeheer/referentiemodellen/IECCIM/TC57CIM/IEC61970/Base/Domain#Resistance"/>
        <rdfs:comment>Zero sequence resistance of the synchronous machine.</rdfs:comment>
    </owl:ObjectProperty>
    


    <!-- https://w3id.org/netbeheer/referentiemodellen/IECCIM/TC57CIM/IEC61970/Base/Wires#SynchronousMachine_r2 -->


    <owl:ObjectProperty rdf:about="https://w3id.org/netbeheer/referentiemodellen/IECCIM/TC57CIM/IEC61970/Base/Wires#SynchronousMachine_r2">
        <rdfs:domain rdf:resource="https://w3id.org/netbeheer/referentiemodellen/IECCIM/TC57CIM/IEC61970/Base/Wires#SynchronousMachine"/>
        <rdfs:range rdf:resource="https://w3id.org/netbeheer/referentiemodellen/IECCIM/TC57CIM/IEC61970/Base/Domain#Resistance"/>
        <rdfs:comment>Negative sequence resistance.</rdfs:comment>
    </owl:ObjectProperty>
    


    <!-- https://w3id.org/netbeheer/referentiemodellen/IECCIM/TC57CIM/IEC61970/Base/Wires#SynchronousMachine_satDirectSubtransX -->


    <owl:ObjectProperty rdf:about="https://w3id.org/netbeheer/referentiemodellen/IECCIM/TC57CIM/IEC61970/Base/Wires#SynchronousMachine_satDirectSubtransX">
        <rdfs:domain rdf:resource="https://w3id.org/netbeheer/referentiemodellen/IECCIM/TC57CIM/IEC61970/Base/Wires#SynchronousMachine"/>
        <rdfs:range rdf:resource="https://w3id.org/netbeheer/referentiemodellen/IECCIM/TC57CIM/IEC61970/Base/Domain#PU"/>
        <rdfs:comment>Direct-axis subtransient reactance saturated, also known as Xd&quot;sat.</rdfs:comment>
    </owl:ObjectProperty>
    


    <!-- https://w3id.org/netbeheer/referentiemodellen/IECCIM/TC57CIM/IEC61970/Base/Wires#SynchronousMachine_satDirectSyncX -->


    <owl:ObjectProperty rdf:about="https://w3id.org/netbeheer/referentiemodellen/IECCIM/TC57CIM/IEC61970/Base/Wires#SynchronousMachine_satDirectSyncX">
        <rdfs:domain rdf:resource="https://w3id.org/netbeheer/referentiemodellen/IECCIM/TC57CIM/IEC61970/Base/Wires#SynchronousMachine"/>
        <rdfs:range rdf:resource="https://w3id.org/netbeheer/referentiemodellen/IECCIM/TC57CIM/IEC61970/Base/Domain#PU"/>
        <rdfs:comment>Direct-axes saturated synchronous reactance (xdsat); reciprocal of short-circuit ration. Used for short circuit data exchange, only for single fed short circuit on a generator. (Section 4.3.4.2. in the IEC 60909-0).</rdfs:comment>
    </owl:ObjectProperty>
    


    <!-- https://w3id.org/netbeheer/referentiemodellen/IECCIM/TC57CIM/IEC61970/Base/Wires#SynchronousMachine_satDirectTransX -->


    <owl:ObjectProperty rdf:about="https://w3id.org/netbeheer/referentiemodellen/IECCIM/TC57CIM/IEC61970/Base/Wires#SynchronousMachine_satDirectTransX">
        <rdfs:domain rdf:resource="https://w3id.org/netbeheer/referentiemodellen/IECCIM/TC57CIM/IEC61970/Base/Wires#SynchronousMachine"/>
        <rdfs:range rdf:resource="https://w3id.org/netbeheer/referentiemodellen/IECCIM/TC57CIM/IEC61970/Base/Domain#PU"/>
        <rdfs:comment>Saturated Direct-axis transient reactance. The attribute is primarily used for short circuit calculations according to ANSI.</rdfs:comment>
    </owl:ObjectProperty>
    


    <!-- https://w3id.org/netbeheer/referentiemodellen/IECCIM/TC57CIM/IEC61970/Base/Wires#SynchronousMachine_voltageRegulationRange -->


    <owl:ObjectProperty rdf:about="https://w3id.org/netbeheer/referentiemodellen/IECCIM/TC57CIM/IEC61970/Base/Wires#SynchronousMachine_voltageRegulationRange">
        <rdfs:domain rdf:resource="https://w3id.org/netbeheer/referentiemodellen/IECCIM/TC57CIM/IEC61970/Base/Wires#SynchronousMachine"/>
        <rdfs:range rdf:resource="https://w3id.org/netbeheer/referentiemodellen/IECCIM/TC57CIM/IEC61970/Base/Domain#PerCent"/>
        <rdfs:comment>Range of generator voltage regulation (PG in the IEC 60909-0) used for calculation of the impedance correction factor KG defined in IEC 60909-0
This attribute is used to describe the operating voltage of the generating unit.</rdfs:comment>
    </owl:ObjectProperty>
    


    <!-- https://w3id.org/netbeheer/referentiemodellen/IECCIM/TC57CIM/IEC61970/Base/Wires#SynchronousMachine_x0 -->


    <owl:ObjectProperty rdf:about="https://w3id.org/netbeheer/referentiemodellen/IECCIM/TC57CIM/IEC61970/Base/Wires#SynchronousMachine_x0">
        <rdfs:domain rdf:resource="https://w3id.org/netbeheer/referentiemodellen/IECCIM/TC57CIM/IEC61970/Base/Wires#SynchronousMachine"/>
        <rdfs:range rdf:resource="https://w3id.org/netbeheer/referentiemodellen/IECCIM/TC57CIM/IEC61970/Base/Domain#Reactance"/>
        <rdfs:comment>Zero sequence reactance of the synchronous machine.</rdfs:comment>
    </owl:ObjectProperty>
    


    <!-- https://w3id.org/netbeheer/referentiemodellen/IECCIM/TC57CIM/IEC61970/Base/Wires#SynchronousMachine_x2 -->


    <owl:ObjectProperty rdf:about="https://w3id.org/netbeheer/referentiemodellen/IECCIM/TC57CIM/IEC61970/Base/Wires#SynchronousMachine_x2">
        <rdfs:domain rdf:resource="https://w3id.org/netbeheer/referentiemodellen/IECCIM/TC57CIM/IEC61970/Base/Wires#SynchronousMachine"/>
        <rdfs:range rdf:resource="https://w3id.org/netbeheer/referentiemodellen/IECCIM/TC57CIM/IEC61970/Base/Domain#Reactance"/>
        <rdfs:comment>Negative sequence reactance.</rdfs:comment>
    </owl:ObjectProperty>
    


    <!-- https://w3id.org/netbeheer/referentiemodellen/IECCIM/TC57CIM/IEC61970/Base/Wires#TapChangerControl_TapChanger -->


    <owl:ObjectProperty rdf:about="https://w3id.org/netbeheer/referentiemodellen/IECCIM/TC57CIM/IEC61970/Base/Wires#TapChangerControl_TapChanger">
        <owl:inverseOf rdf:resource="https://w3id.org/netbeheer/referentiemodellen/IECCIM/TC57CIM/IEC61970/Base/Wires#TapChanger_TapChangerControl"/>
        <rdfs:domain rdf:resource="https://w3id.org/netbeheer/referentiemodellen/IECCIM/TC57CIM/IEC61970/Base/Wires#TapChangerControl"/>
        <rdfs:range rdf:resource="https://w3id.org/netbeheer/referentiemodellen/IECCIM/TC57CIM/IEC61970/Base/Wires#TapChanger"/>
        <rdfs:comment>The tap changers that participates in this regulating tap control scheme.The regulating control scheme in which this tap changer participates.</rdfs:comment>
    </owl:ObjectProperty>
    


    <!-- https://w3id.org/netbeheer/referentiemodellen/IECCIM/TC57CIM/IEC61970/Base/Wires#TapChangerControl_limitVoltage -->


    <owl:ObjectProperty rdf:about="https://w3id.org/netbeheer/referentiemodellen/IECCIM/TC57CIM/IEC61970/Base/Wires#TapChangerControl_limitVoltage">
        <rdfs:domain rdf:resource="https://w3id.org/netbeheer/referentiemodellen/IECCIM/TC57CIM/IEC61970/Base/Wires#TapChangerControl"/>
        <rdfs:range rdf:resource="https://w3id.org/netbeheer/referentiemodellen/IECCIM/TC57CIM/IEC61970/Base/Domain#Voltage"/>
        <rdfs:comment>Maximum allowed regulated voltage on the PT secondary, regardless of line drop compensation. Sometimes referred to as first-house protection.
</rdfs:comment>
    </owl:ObjectProperty>
    


    <!-- https://w3id.org/netbeheer/referentiemodellen/IECCIM/TC57CIM/IEC61970/Base/Wires#TapChangerControl_lineDropR -->


    <owl:ObjectProperty rdf:about="https://w3id.org/netbeheer/referentiemodellen/IECCIM/TC57CIM/IEC61970/Base/Wires#TapChangerControl_lineDropR">
        <rdfs:domain rdf:resource="https://w3id.org/netbeheer/referentiemodellen/IECCIM/TC57CIM/IEC61970/Base/Wires#TapChangerControl"/>
        <rdfs:range rdf:resource="https://w3id.org/netbeheer/referentiemodellen/IECCIM/TC57CIM/IEC61970/Base/Domain#Resistance"/>
        <rdfs:comment>Line drop compensator resistance setting for normal (forward) power flow.</rdfs:comment>
    </owl:ObjectProperty>
    


    <!-- https://w3id.org/netbeheer/referentiemodellen/IECCIM/TC57CIM/IEC61970/Base/Wires#TapChangerControl_lineDropX -->


    <owl:ObjectProperty rdf:about="https://w3id.org/netbeheer/referentiemodellen/IECCIM/TC57CIM/IEC61970/Base/Wires#TapChangerControl_lineDropX">
        <rdfs:domain rdf:resource="https://w3id.org/netbeheer/referentiemodellen/IECCIM/TC57CIM/IEC61970/Base/Wires#TapChangerControl"/>
        <rdfs:range rdf:resource="https://w3id.org/netbeheer/referentiemodellen/IECCIM/TC57CIM/IEC61970/Base/Domain#Reactance"/>
        <rdfs:comment>Line drop compensator reactance setting for normal (forward) power flow.</rdfs:comment>
    </owl:ObjectProperty>
    


    <!-- https://w3id.org/netbeheer/referentiemodellen/IECCIM/TC57CIM/IEC61970/Base/Wires#TapChangerControl_reverseLineDropR -->


    <owl:ObjectProperty rdf:about="https://w3id.org/netbeheer/referentiemodellen/IECCIM/TC57CIM/IEC61970/Base/Wires#TapChangerControl_reverseLineDropR">
        <rdfs:domain rdf:resource="https://w3id.org/netbeheer/referentiemodellen/IECCIM/TC57CIM/IEC61970/Base/Wires#TapChangerControl"/>
        <rdfs:range rdf:resource="https://w3id.org/netbeheer/referentiemodellen/IECCIM/TC57CIM/IEC61970/Base/Domain#Resistance"/>
        <rdfs:comment>Line drop compensator resistance setting for reverse power flow.</rdfs:comment>
    </owl:ObjectProperty>
    


    <!-- https://w3id.org/netbeheer/referentiemodellen/IECCIM/TC57CIM/IEC61970/Base/Wires#TapChangerControl_reverseLineDropX -->


    <owl:ObjectProperty rdf:about="https://w3id.org/netbeheer/referentiemodellen/IECCIM/TC57CIM/IEC61970/Base/Wires#TapChangerControl_reverseLineDropX">
        <rdfs:domain rdf:resource="https://w3id.org/netbeheer/referentiemodellen/IECCIM/TC57CIM/IEC61970/Base/Wires#TapChangerControl"/>
        <rdfs:range rdf:resource="https://w3id.org/netbeheer/referentiemodellen/IECCIM/TC57CIM/IEC61970/Base/Domain#Reactance"/>
        <rdfs:comment>Line drop compensator reactance setting for reverse power flow.</rdfs:comment>
    </owl:ObjectProperty>
    


    <!-- https://w3id.org/netbeheer/referentiemodellen/IECCIM/TC57CIM/IEC61970/Base/Wires#TapChangerTablePoint_b -->


    <owl:ObjectProperty rdf:about="https://w3id.org/netbeheer/referentiemodellen/IECCIM/TC57CIM/IEC61970/Base/Wires#TapChangerTablePoint_b">
        <rdfs:domain rdf:resource="https://w3id.org/netbeheer/referentiemodellen/IECCIM/TC57CIM/IEC61970/Base/Wires#TapChangerTablePoint"/>
        <rdfs:range rdf:resource="https://w3id.org/netbeheer/referentiemodellen/IECCIM/TC57CIM/IEC61970/Base/Domain#PerCent"/>
        <rdfs:comment>The magnetizing branch susceptance deviation in percent of nominal value. The actual susceptance is calculated as follows:
calculated magnetizing susceptance = b(nominal) * (1 + b(from this class)/100).   The b(nominal) is defined as the static magnetizing susceptance on the associated power transformer end or ends.  This model assumes the star impedance (pi model) form.
</rdfs:comment>
    </owl:ObjectProperty>
    


    <!-- https://w3id.org/netbeheer/referentiemodellen/IECCIM/TC57CIM/IEC61970/Base/Wires#TapChangerTablePoint_g -->


    <owl:ObjectProperty rdf:about="https://w3id.org/netbeheer/referentiemodellen/IECCIM/TC57CIM/IEC61970/Base/Wires#TapChangerTablePoint_g">
        <rdfs:domain rdf:resource="https://w3id.org/netbeheer/referentiemodellen/IECCIM/TC57CIM/IEC61970/Base/Wires#TapChangerTablePoint"/>
        <rdfs:range rdf:resource="https://w3id.org/netbeheer/referentiemodellen/IECCIM/TC57CIM/IEC61970/Base/Domain#PerCent"/>
        <rdfs:comment>The magnetizing branch conductance deviation in percent of nominal value. The actual conductance is calculated as follows:
calculated magnetizing conductance = g(nominal) * (1 + g(from this class)/100).   The g(nominal) is defined as the static magnetizing conductance on the associated power transformer end or ends.  This model assumes the star impedance (pi model) form.
</rdfs:comment>
    </owl:ObjectProperty>
    


    <!-- https://w3id.org/netbeheer/referentiemodellen/IECCIM/TC57CIM/IEC61970/Base/Wires#TapChangerTablePoint_r -->


    <owl:ObjectProperty rdf:about="https://w3id.org/netbeheer/referentiemodellen/IECCIM/TC57CIM/IEC61970/Base/Wires#TapChangerTablePoint_r">
        <rdfs:domain rdf:resource="https://w3id.org/netbeheer/referentiemodellen/IECCIM/TC57CIM/IEC61970/Base/Wires#TapChangerTablePoint"/>
        <rdfs:range rdf:resource="https://w3id.org/netbeheer/referentiemodellen/IECCIM/TC57CIM/IEC61970/Base/Domain#PerCent"/>
        <rdfs:comment>The resistance deviation in percent of nominal value. The actual reactance is calculated as follows:
calculated resistance = r(nominal) * (1 + r(from this class)/100).   The r(nominal) is defined as the static resistance on the associated power transformer end or ends.  This model assumes the star impedance (pi model) form.
</rdfs:comment>
    </owl:ObjectProperty>
    


    <!-- https://w3id.org/netbeheer/referentiemodellen/IECCIM/TC57CIM/IEC61970/Base/Wires#TapChangerTablePoint_x -->


    <owl:ObjectProperty rdf:about="https://w3id.org/netbeheer/referentiemodellen/IECCIM/TC57CIM/IEC61970/Base/Wires#TapChangerTablePoint_x">
        <rdfs:domain rdf:resource="https://w3id.org/netbeheer/referentiemodellen/IECCIM/TC57CIM/IEC61970/Base/Wires#TapChangerTablePoint"/>
        <rdfs:range rdf:resource="https://w3id.org/netbeheer/referentiemodellen/IECCIM/TC57CIM/IEC61970/Base/Domain#PerCent"/>
        <rdfs:comment>The series reactance deviation in percent of nominal value. The actual reactance is calculated as follows:
calculated reactance = x(nominal) * (1 + x(from this class)/100).   The x(nominal) is defined as the static series reactance on the associated power transformer end or ends.  This model assumes the star impedance (pi model) form.
</rdfs:comment>
    </owl:ObjectProperty>
    


    <!-- https://w3id.org/netbeheer/referentiemodellen/IECCIM/TC57CIM/IEC61970/Base/Wires#TapChanger_SvTapStep -->


    <owl:ObjectProperty rdf:about="https://w3id.org/netbeheer/referentiemodellen/IECCIM/TC57CIM/IEC61970/Base/Wires#TapChanger_SvTapStep">
        <owl:inverseOf rdf:resource="https://w3id.org/netbeheer/referentiemodellen/IECCIM/TC57CIM/IEC61970/Base/Wires#SvTapStep_TapChanger"/>
        <rdf:type rdf:resource="http://www.w3.org/2002/07/owl#FunctionalProperty"/>
        <rdfs:domain rdf:resource="https://w3id.org/netbeheer/referentiemodellen/IECCIM/TC57CIM/IEC61970/Base/Wires#TapChanger"/>
        <rdfs:range rdf:resource="https://w3id.org/netbeheer/referentiemodellen/IECCIM/TC57CIM/IEC61970/Base/StateVariables#SvTapStep"/>
        <rdfs:comment>The tap step state associated with the tap changer.The tap changer associated with the tap step state.</rdfs:comment>
    </owl:ObjectProperty>
    


    <!-- https://w3id.org/netbeheer/referentiemodellen/IECCIM/TC57CIM/IEC61970/Base/Wires#TapChanger_TapChangerControl -->


    <owl:ObjectProperty rdf:about="https://w3id.org/netbeheer/referentiemodellen/IECCIM/TC57CIM/IEC61970/Base/Wires#TapChanger_TapChangerControl">
        <rdfs:domain rdf:resource="https://w3id.org/netbeheer/referentiemodellen/IECCIM/TC57CIM/IEC61970/Base/Wires#TapChanger"/>
        <rdfs:range rdf:resource="https://w3id.org/netbeheer/referentiemodellen/IECCIM/TC57CIM/IEC61970/Base/Wires#TapChangerControl"/>
        <rdfs:comment>The tap changers that participates in this regulating tap control scheme.The regulating control scheme in which this tap changer participates.</rdfs:comment>
    </owl:ObjectProperty>
    


    <!-- https://w3id.org/netbeheer/referentiemodellen/IECCIM/TC57CIM/IEC61970/Base/Wires#TapChanger_TapSchedules -->


    <owl:ObjectProperty rdf:about="https://w3id.org/netbeheer/referentiemodellen/IECCIM/TC57CIM/IEC61970/Base/Wires#TapChanger_TapSchedules">
        <owl:inverseOf rdf:resource="https://w3id.org/netbeheer/referentiemodellen/IECCIM/TC57CIM/IEC61970/Base/Wires#TapSchedule_TapChanger"/>
        <rdf:type rdf:resource="http://www.w3.org/2002/07/owl#FunctionalProperty"/>
        <rdfs:domain rdf:resource="https://w3id.org/netbeheer/referentiemodellen/IECCIM/TC57CIM/IEC61970/Base/Wires#TapChanger"/>
        <rdfs:range rdf:resource="https://w3id.org/netbeheer/referentiemodellen/IECCIM/TC57CIM/IEC61970/Base/Wires#TapSchedule"/>
        <rdfs:comment>A TapChanger can have TapSchedules.A TapSchedule is associated with a TapChanger.</rdfs:comment>
    </owl:ObjectProperty>
    


    <!-- https://w3id.org/netbeheer/referentiemodellen/IECCIM/TC57CIM/IEC61970/Base/Wires#TapChanger_initialDelay -->


    <owl:ObjectProperty rdf:about="https://w3id.org/netbeheer/referentiemodellen/IECCIM/TC57CIM/IEC61970/Base/Wires#TapChanger_initialDelay">
        <rdfs:domain rdf:resource="https://w3id.org/netbeheer/referentiemodellen/IECCIM/TC57CIM/IEC61970/Base/Wires#TapChanger"/>
        <rdfs:range rdf:resource="https://w3id.org/netbeheer/referentiemodellen/IECCIM/TC57CIM/IEC61970/Base/Domain#Seconds"/>
        <rdfs:comment>For an LTC, the delay for initial tap changer operation (first step change)</rdfs:comment>
    </owl:ObjectProperty>
    


    <!-- https://w3id.org/netbeheer/referentiemodellen/IECCIM/TC57CIM/IEC61970/Base/Wires#TapChanger_neutralU -->


    <owl:ObjectProperty rdf:about="https://w3id.org/netbeheer/referentiemodellen/IECCIM/TC57CIM/IEC61970/Base/Wires#TapChanger_neutralU">
        <rdfs:domain rdf:resource="https://w3id.org/netbeheer/referentiemodellen/IECCIM/TC57CIM/IEC61970/Base/Wires#TapChanger"/>
        <rdfs:range rdf:resource="https://w3id.org/netbeheer/referentiemodellen/IECCIM/TC57CIM/IEC61970/Base/Domain#Voltage"/>
        <rdfs:comment>Voltage at which the winding operates at the neutral tap setting.</rdfs:comment>
    </owl:ObjectProperty>
    


    <!-- https://w3id.org/netbeheer/referentiemodellen/IECCIM/TC57CIM/IEC61970/Base/Wires#TapChanger_subsequentDelay -->


    <owl:ObjectProperty rdf:about="https://w3id.org/netbeheer/referentiemodellen/IECCIM/TC57CIM/IEC61970/Base/Wires#TapChanger_subsequentDelay">
        <rdfs:domain rdf:resource="https://w3id.org/netbeheer/referentiemodellen/IECCIM/TC57CIM/IEC61970/Base/Wires#TapChanger"/>
        <rdfs:range rdf:resource="https://w3id.org/netbeheer/referentiemodellen/IECCIM/TC57CIM/IEC61970/Base/Domain#Seconds"/>
        <rdfs:comment>For an LTC, the delay for subsequent tap changer operation (second and later step changes)</rdfs:comment>
    </owl:ObjectProperty>
    


    <!-- https://w3id.org/netbeheer/referentiemodellen/IECCIM/TC57CIM/IEC61970/Base/Wires#TapSchedule_TapChanger -->


    <owl:ObjectProperty rdf:about="https://w3id.org/netbeheer/referentiemodellen/IECCIM/TC57CIM/IEC61970/Base/Wires#TapSchedule_TapChanger">
        <rdfs:domain rdf:resource="https://w3id.org/netbeheer/referentiemodellen/IECCIM/TC57CIM/IEC61970/Base/Wires#TapSchedule"/>
        <rdfs:range rdf:resource="https://w3id.org/netbeheer/referentiemodellen/IECCIM/TC57CIM/IEC61970/Base/Wires#TapChanger"/>
        <rdfs:comment>A TapChanger can have TapSchedules.A TapSchedule is associated with a TapChanger.</rdfs:comment>
    </owl:ObjectProperty>
    


    <!-- https://w3id.org/netbeheer/referentiemodellen/IECCIM/TC57CIM/IEC61970/Base/Wires#TransformerCoreAdmittance_TransformerEnd -->


    <owl:ObjectProperty rdf:about="https://w3id.org/netbeheer/referentiemodellen/IECCIM/TC57CIM/IEC61970/Base/Wires#TransformerCoreAdmittance_TransformerEnd">
        <rdfs:domain rdf:resource="https://w3id.org/netbeheer/referentiemodellen/IECCIM/TC57CIM/IEC61970/Base/Wires#TransformerCoreAdmittance"/>
        <rdfs:range rdf:resource="https://w3id.org/netbeheer/referentiemodellen/IECCIM/TC57CIM/IEC61970/Base/Wires#TransformerEnd"/>
        <rdfs:comment>Core admittance of this transformer end, representing magnetising current and core losses. The full values of the transformer should be supplied for one transformer end only.All transformer ends having this core admittance.</rdfs:comment>
    </owl:ObjectProperty>
    


    <!-- https://w3id.org/netbeheer/referentiemodellen/IECCIM/TC57CIM/IEC61970/Base/Wires#TransformerCoreAdmittance_TransformerEndInfo -->


    <owl:ObjectProperty rdf:about="https://w3id.org/netbeheer/referentiemodellen/IECCIM/TC57CIM/IEC61970/Base/Wires#TransformerCoreAdmittance_TransformerEndInfo">
        <owl:inverseOf rdf:resource="https://w3id.org/netbeheer/referentiemodellen/IECCIM/TC57CIM/IEC61970/Base/Wires#TransformerEndInfo_CoreAdmittance"/>
        <rdfs:domain rdf:resource="https://w3id.org/netbeheer/referentiemodellen/IECCIM/TC57CIM/IEC61970/Base/Wires#TransformerCoreAdmittance"/>
        <rdfs:range rdf:resource="https://w3id.org/netbeheer/referentiemodellen/IECCIM/TC57CIM/IEC61968/AssetInfo#TransformerEndInfo"/>
        <rdfs:comment>Transformer end datasheet used to calculate this core admittance.Core admittance calculated from this transformer end datasheet, representing magnetising current and core losses. The full values of the transformer should be supplied for one transformer end info only.</rdfs:comment>
    </owl:ObjectProperty>
    


    <!-- https://w3id.org/netbeheer/referentiemodellen/IECCIM/TC57CIM/IEC61970/Base/Wires#TransformerCoreAdmittance_b -->


    <owl:ObjectProperty rdf:about="https://w3id.org/netbeheer/referentiemodellen/IECCIM/TC57CIM/IEC61970/Base/Wires#TransformerCoreAdmittance_b">
        <rdfs:domain rdf:resource="https://w3id.org/netbeheer/referentiemodellen/IECCIM/TC57CIM/IEC61970/Base/Wires#TransformerCoreAdmittance"/>
        <rdfs:range rdf:resource="https://w3id.org/netbeheer/referentiemodellen/IECCIM/TC57CIM/IEC61970/Base/Domain#Susceptance"/>
        <rdfs:comment>Magnetizing branch susceptance (B mag).  The value can be positive or negative.
</rdfs:comment>
    </owl:ObjectProperty>
    


    <!-- https://w3id.org/netbeheer/referentiemodellen/IECCIM/TC57CIM/IEC61970/Base/Wires#TransformerCoreAdmittance_b0 -->


    <owl:ObjectProperty rdf:about="https://w3id.org/netbeheer/referentiemodellen/IECCIM/TC57CIM/IEC61970/Base/Wires#TransformerCoreAdmittance_b0">
        <rdfs:domain rdf:resource="https://w3id.org/netbeheer/referentiemodellen/IECCIM/TC57CIM/IEC61970/Base/Wires#TransformerCoreAdmittance"/>
        <rdfs:range rdf:resource="https://w3id.org/netbeheer/referentiemodellen/IECCIM/TC57CIM/IEC61970/Base/Domain#Susceptance"/>
        <rdfs:comment>Zero sequence magnetizing branch susceptance.
</rdfs:comment>
    </owl:ObjectProperty>
    


    <!-- https://w3id.org/netbeheer/referentiemodellen/IECCIM/TC57CIM/IEC61970/Base/Wires#TransformerCoreAdmittance_g -->


    <owl:ObjectProperty rdf:about="https://w3id.org/netbeheer/referentiemodellen/IECCIM/TC57CIM/IEC61970/Base/Wires#TransformerCoreAdmittance_g">
        <rdfs:domain rdf:resource="https://w3id.org/netbeheer/referentiemodellen/IECCIM/TC57CIM/IEC61970/Base/Wires#TransformerCoreAdmittance"/>
        <rdfs:range rdf:resource="https://w3id.org/netbeheer/referentiemodellen/IECCIM/TC57CIM/IEC61970/Base/Domain#Conductance"/>
        <rdfs:comment>Magnetizing branch conductance (G mag).
</rdfs:comment>
    </owl:ObjectProperty>
    


    <!-- https://w3id.org/netbeheer/referentiemodellen/IECCIM/TC57CIM/IEC61970/Base/Wires#TransformerCoreAdmittance_g0 -->


    <owl:ObjectProperty rdf:about="https://w3id.org/netbeheer/referentiemodellen/IECCIM/TC57CIM/IEC61970/Base/Wires#TransformerCoreAdmittance_g0">
        <rdfs:domain rdf:resource="https://w3id.org/netbeheer/referentiemodellen/IECCIM/TC57CIM/IEC61970/Base/Wires#TransformerCoreAdmittance"/>
        <rdfs:range rdf:resource="https://w3id.org/netbeheer/referentiemodellen/IECCIM/TC57CIM/IEC61970/Base/Domain#Conductance"/>
        <rdfs:comment>Zero sequence magnetizing branch conductance.
</rdfs:comment>
    </owl:ObjectProperty>
    


    <!-- https://w3id.org/netbeheer/referentiemodellen/IECCIM/TC57CIM/IEC61970/Base/Wires#TransformerEndInfo_CoreAdmittance -->


    <owl:ObjectProperty rdf:about="https://w3id.org/netbeheer/referentiemodellen/IECCIM/TC57CIM/IEC61970/Base/Wires#TransformerEndInfo_CoreAdmittance">
        <rdfs:domain rdf:resource="https://w3id.org/netbeheer/referentiemodellen/IECCIM/TC57CIM/IEC61968/AssetInfo#TransformerEndInfo"/>
        <rdfs:range rdf:resource="https://w3id.org/netbeheer/referentiemodellen/IECCIM/TC57CIM/IEC61970/Base/Wires#TransformerCoreAdmittance"/>
        <rdfs:comment>Transformer end datasheet used to calculate this core admittance.Core admittance calculated from this transformer end datasheet, representing magnetising current and core losses. The full values of the transformer should be supplied for one transformer end info only.</rdfs:comment>
    </owl:ObjectProperty>
    


    <!-- https://w3id.org/netbeheer/referentiemodellen/IECCIM/TC57CIM/IEC61970/Base/Wires#TransformerEndInfo_FromMeshImpedances -->


    <owl:ObjectProperty rdf:about="https://w3id.org/netbeheer/referentiemodellen/IECCIM/TC57CIM/IEC61970/Base/Wires#TransformerEndInfo_FromMeshImpedances">
        <rdfs:domain rdf:resource="https://w3id.org/netbeheer/referentiemodellen/IECCIM/TC57CIM/IEC61968/AssetInfo#TransformerEndInfo"/>
        <rdfs:range rdf:resource="https://w3id.org/netbeheer/referentiemodellen/IECCIM/TC57CIM/IEC61970/Base/Wires#TransformerMeshImpedance"/>
        <rdfs:comment>&apos;from&apos; transformer end datasheet this mesh impedance is calculated from. It determines the voltage reference.All mesh impedances between this &apos;to&apos; and other &apos;from&apos; transformer ends.</rdfs:comment>
    </owl:ObjectProperty>
    


    <!-- https://w3id.org/netbeheer/referentiemodellen/IECCIM/TC57CIM/IEC61970/Base/Wires#TransformerEndInfo_ToMeshImpedances -->


    <owl:ObjectProperty rdf:about="https://w3id.org/netbeheer/referentiemodellen/IECCIM/TC57CIM/IEC61970/Base/Wires#TransformerEndInfo_ToMeshImpedances">
        <rdfs:domain rdf:resource="https://w3id.org/netbeheer/referentiemodellen/IECCIM/TC57CIM/IEC61968/AssetInfo#TransformerEndInfo"/>
        <rdfs:range rdf:resource="https://w3id.org/netbeheer/referentiemodellen/IECCIM/TC57CIM/IEC61970/Base/Wires#TransformerMeshImpedance"/>
        <rdfs:comment>All &apos;to&apos; transformer end datasheets this mesh impedance for &apos;from&apos; transformer end is calculated from.All mesh impedances between this &apos;from&apos; and other &apos;to&apos; transformer ends.</rdfs:comment>
    </owl:ObjectProperty>
    


    <!-- https://w3id.org/netbeheer/referentiemodellen/IECCIM/TC57CIM/IEC61970/Base/Wires#TransformerEndInfo_TransformerStarImpedance -->


    <owl:ObjectProperty rdf:about="https://w3id.org/netbeheer/referentiemodellen/IECCIM/TC57CIM/IEC61970/Base/Wires#TransformerEndInfo_TransformerStarImpedance">
        <rdfs:domain rdf:resource="https://w3id.org/netbeheer/referentiemodellen/IECCIM/TC57CIM/IEC61968/AssetInfo#TransformerEndInfo"/>
        <rdfs:range rdf:resource="https://w3id.org/netbeheer/referentiemodellen/IECCIM/TC57CIM/IEC61970/Base/Wires#TransformerStarImpedance"/>
        <rdfs:comment>Transformer end datasheet used to calculate this transformer star impedance.Transformer star impedance calculated from this transformer end datasheet.</rdfs:comment>
    </owl:ObjectProperty>
    


    <!-- https://w3id.org/netbeheer/referentiemodellen/IECCIM/TC57CIM/IEC61970/Base/Wires#TransformerEnd_CoreAdmittance -->


    <owl:ObjectProperty rdf:about="https://w3id.org/netbeheer/referentiemodellen/IECCIM/TC57CIM/IEC61970/Base/Wires#TransformerEnd_CoreAdmittance">
        <owl:inverseOf rdf:resource="https://w3id.org/netbeheer/referentiemodellen/IECCIM/TC57CIM/IEC61970/Base/Wires#TransformerCoreAdmittance_TransformerEnd"/>
        <rdfs:domain rdf:resource="https://w3id.org/netbeheer/referentiemodellen/IECCIM/TC57CIM/IEC61970/Base/Wires#TransformerEnd"/>
        <rdfs:range rdf:resource="https://w3id.org/netbeheer/referentiemodellen/IECCIM/TC57CIM/IEC61970/Base/Wires#TransformerCoreAdmittance"/>
        <rdfs:comment>Core admittance of this transformer end, representing magnetising current and core losses. The full values of the transformer should be supplied for one transformer end only.All transformer ends having this core admittance.</rdfs:comment>
    </owl:ObjectProperty>
    


    <!-- https://w3id.org/netbeheer/referentiemodellen/IECCIM/TC57CIM/IEC61970/Base/Wires#TransformerEnd_FromMeshImpedance -->


    <owl:ObjectProperty rdf:about="https://w3id.org/netbeheer/referentiemodellen/IECCIM/TC57CIM/IEC61970/Base/Wires#TransformerEnd_FromMeshImpedance">
        <owl:inverseOf rdf:resource="https://w3id.org/netbeheer/referentiemodellen/IECCIM/TC57CIM/IEC61970/Base/Wires#TransformerMeshImpedance_FromTransformerEnd"/>
        <rdf:type rdf:resource="http://www.w3.org/2002/07/owl#FunctionalProperty"/>
        <rdfs:domain rdf:resource="https://w3id.org/netbeheer/referentiemodellen/IECCIM/TC57CIM/IEC61970/Base/Wires#TransformerEnd"/>
        <rdfs:range rdf:resource="https://w3id.org/netbeheer/referentiemodellen/IECCIM/TC57CIM/IEC61970/Base/Wires#TransformerMeshImpedance"/>
        <rdfs:comment>All mesh impedances between this &apos;to&apos; and other &apos;from&apos; transformer ends.From end this mesh impedance is connected to. It determines the voltage reference.</rdfs:comment>
    </owl:ObjectProperty>
    


    <!-- https://w3id.org/netbeheer/referentiemodellen/IECCIM/TC57CIM/IEC61970/Base/Wires#TransformerEnd_FromWindingInsulations -->


    <owl:ObjectProperty rdf:about="https://w3id.org/netbeheer/referentiemodellen/IECCIM/TC57CIM/IEC61970/Base/Wires#TransformerEnd_FromWindingInsulations">
        <owl:inverseOf rdf:resource="https://w3id.org/netbeheer/referentiemodellen/IECCIM/TC57CIM/IEC61970/Base/Wires#WindingInsulation_FromWinding"/>
        <rdf:type rdf:resource="http://www.w3.org/2002/07/owl#FunctionalProperty"/>
        <rdfs:domain rdf:resource="https://w3id.org/netbeheer/referentiemodellen/IECCIM/TC57CIM/IEC61970/Base/Wires#TransformerEnd"/>
        <rdfs:range rdf:resource="https://w3id.org/netbeheer/referentiemodellen/IECCIM/TC57CIM/IEC61968/InfIEC61968/InfAssets#WindingInsulation"/>
        <rdfs:comment></rdfs:comment>
    </owl:ObjectProperty>
    


    <!-- https://w3id.org/netbeheer/referentiemodellen/IECCIM/TC57CIM/IEC61970/Base/Wires#TransformerEnd_PhaseTapChanger -->


    <owl:ObjectProperty rdf:about="https://w3id.org/netbeheer/referentiemodellen/IECCIM/TC57CIM/IEC61970/Base/Wires#TransformerEnd_PhaseTapChanger">
        <rdf:type rdf:resource="http://www.w3.org/2002/07/owl#FunctionalProperty"/>
        <rdfs:domain rdf:resource="https://w3id.org/netbeheer/referentiemodellen/IECCIM/TC57CIM/IEC61970/Base/Wires#TransformerEnd"/>
        <rdfs:range rdf:resource="https://w3id.org/netbeheer/referentiemodellen/IECCIM/TC57CIM/IEC61970/Base/Wires#PhaseTapChanger"/>
        <rdfs:comment>Transformer end to which this phase tap changer belongs.Phase tap changer associated with this transformer end.</rdfs:comment>
    </owl:ObjectProperty>
    


    <!-- https://w3id.org/netbeheer/referentiemodellen/IECCIM/TC57CIM/IEC61970/Base/Wires#TransformerEnd_RatioTapChanger -->


    <owl:ObjectProperty rdf:about="https://w3id.org/netbeheer/referentiemodellen/IECCIM/TC57CIM/IEC61970/Base/Wires#TransformerEnd_RatioTapChanger">
        <rdf:type rdf:resource="http://www.w3.org/2002/07/owl#FunctionalProperty"/>
        <rdfs:domain rdf:resource="https://w3id.org/netbeheer/referentiemodellen/IECCIM/TC57CIM/IEC61970/Base/Wires#TransformerEnd"/>
        <rdfs:range rdf:resource="https://w3id.org/netbeheer/referentiemodellen/IECCIM/TC57CIM/IEC61970/Base/Wires#RatioTapChanger"/>
        <rdfs:comment>Transformer end to which this ratio tap changer belongs.Ratio tap changer associated with this transformer end.</rdfs:comment>
    </owl:ObjectProperty>
    


    <!-- https://w3id.org/netbeheer/referentiemodellen/IECCIM/TC57CIM/IEC61970/Base/Wires#TransformerEnd_StarImpedance -->


    <owl:ObjectProperty rdf:about="https://w3id.org/netbeheer/referentiemodellen/IECCIM/TC57CIM/IEC61970/Base/Wires#TransformerEnd_StarImpedance">
        <rdfs:domain rdf:resource="https://w3id.org/netbeheer/referentiemodellen/IECCIM/TC57CIM/IEC61970/Base/Wires#TransformerEnd"/>
        <rdfs:range rdf:resource="https://w3id.org/netbeheer/referentiemodellen/IECCIM/TC57CIM/IEC61970/Base/Wires#TransformerStarImpedance"/>
        <rdfs:comment>All transformer ends having this star impedance.(accurate for 2- or 3-winding transformers only) Pi-model impedances of this transformer end. By convention, for a two winding transformer, the full values of the transformer should be entered on the high voltage end (endNumber=1).</rdfs:comment>
    </owl:ObjectProperty>
    


    <!-- https://w3id.org/netbeheer/referentiemodellen/IECCIM/TC57CIM/IEC61970/Base/Wires#TransformerEnd_ToMeshImpedance -->


    <owl:ObjectProperty rdf:about="https://w3id.org/netbeheer/referentiemodellen/IECCIM/TC57CIM/IEC61970/Base/Wires#TransformerEnd_ToMeshImpedance">
        <owl:inverseOf rdf:resource="https://w3id.org/netbeheer/referentiemodellen/IECCIM/TC57CIM/IEC61970/Base/Wires#TransformerMeshImpedance_ToTransformerEnd"/>
        <rdfs:domain rdf:resource="https://w3id.org/netbeheer/referentiemodellen/IECCIM/TC57CIM/IEC61970/Base/Wires#TransformerEnd"/>
        <rdfs:range rdf:resource="https://w3id.org/netbeheer/referentiemodellen/IECCIM/TC57CIM/IEC61970/Base/Wires#TransformerMeshImpedance"/>
        <rdfs:comment>All mesh impedances between this &apos;from&apos; and other &apos;to&apos; transformer ends.All transformer ends this mesh impedance is connected to.</rdfs:comment>
    </owl:ObjectProperty>
    


    <!-- https://w3id.org/netbeheer/referentiemodellen/IECCIM/TC57CIM/IEC61970/Base/Wires#TransformerEnd_ToWindingInsulations -->


    <owl:ObjectProperty rdf:about="https://w3id.org/netbeheer/referentiemodellen/IECCIM/TC57CIM/IEC61970/Base/Wires#TransformerEnd_ToWindingInsulations">
        <owl:inverseOf rdf:resource="https://w3id.org/netbeheer/referentiemodellen/IECCIM/TC57CIM/IEC61970/Base/Wires#WindingInsulation_ToWinding"/>
        <rdf:type rdf:resource="http://www.w3.org/2002/07/owl#FunctionalProperty"/>
        <rdfs:domain rdf:resource="https://w3id.org/netbeheer/referentiemodellen/IECCIM/TC57CIM/IEC61970/Base/Wires#TransformerEnd"/>
        <rdfs:range rdf:resource="https://w3id.org/netbeheer/referentiemodellen/IECCIM/TC57CIM/IEC61968/InfIEC61968/InfAssets#WindingInsulation"/>
        <rdfs:comment></rdfs:comment>
    </owl:ObjectProperty>
    


    <!-- https://w3id.org/netbeheer/referentiemodellen/IECCIM/TC57CIM/IEC61970/Base/Wires#TransformerEnd_bmagSat -->


    <owl:ObjectProperty rdf:about="https://w3id.org/netbeheer/referentiemodellen/IECCIM/TC57CIM/IEC61970/Base/Wires#TransformerEnd_bmagSat">
        <rdfs:domain rdf:resource="https://w3id.org/netbeheer/referentiemodellen/IECCIM/TC57CIM/IEC61970/Base/Wires#TransformerEnd"/>
        <rdfs:range rdf:resource="https://w3id.org/netbeheer/referentiemodellen/IECCIM/TC57CIM/IEC61970/Base/Domain#PerCent"/>
        <rdfs:comment>Core shunt magnetizing susceptance in the saturation region.
</rdfs:comment>
    </owl:ObjectProperty>
    


    <!-- https://w3id.org/netbeheer/referentiemodellen/IECCIM/TC57CIM/IEC61970/Base/Wires#TransformerEnd_magBaseU -->


    <owl:ObjectProperty rdf:about="https://w3id.org/netbeheer/referentiemodellen/IECCIM/TC57CIM/IEC61970/Base/Wires#TransformerEnd_magBaseU">
        <rdfs:domain rdf:resource="https://w3id.org/netbeheer/referentiemodellen/IECCIM/TC57CIM/IEC61970/Base/Wires#TransformerEnd"/>
        <rdfs:range rdf:resource="https://w3id.org/netbeheer/referentiemodellen/IECCIM/TC57CIM/IEC61970/Base/Domain#Voltage"/>
        <rdfs:comment>The reference voltage at which the magnetizing saturation measurements were made
</rdfs:comment>
    </owl:ObjectProperty>
    


    <!-- https://w3id.org/netbeheer/referentiemodellen/IECCIM/TC57CIM/IEC61970/Base/Wires#TransformerEnd_magSatFlux -->


    <owl:ObjectProperty rdf:about="https://w3id.org/netbeheer/referentiemodellen/IECCIM/TC57CIM/IEC61970/Base/Wires#TransformerEnd_magSatFlux">
        <rdfs:domain rdf:resource="https://w3id.org/netbeheer/referentiemodellen/IECCIM/TC57CIM/IEC61970/Base/Wires#TransformerEnd"/>
        <rdfs:range rdf:resource="https://w3id.org/netbeheer/referentiemodellen/IECCIM/TC57CIM/IEC61970/Base/Domain#PerCent"/>
        <rdfs:comment>Core magnetizing saturation curve knee flux level.
</rdfs:comment>
    </owl:ObjectProperty>
    


    <!-- https://w3id.org/netbeheer/referentiemodellen/IECCIM/TC57CIM/IEC61970/Base/Wires#TransformerEnd_rground -->


    <owl:ObjectProperty rdf:about="https://w3id.org/netbeheer/referentiemodellen/IECCIM/TC57CIM/IEC61970/Base/Wires#TransformerEnd_rground">
        <rdfs:domain rdf:resource="https://w3id.org/netbeheer/referentiemodellen/IECCIM/TC57CIM/IEC61970/Base/Wires#TransformerEnd"/>
        <rdfs:range rdf:resource="https://w3id.org/netbeheer/referentiemodellen/IECCIM/TC57CIM/IEC61970/Base/Domain#Resistance"/>
        <rdfs:comment>(for Yn and Zn connections) Resistance part of neutral impedance where &apos;grounded&apos; is true.</rdfs:comment>
    </owl:ObjectProperty>
    


    <!-- https://w3id.org/netbeheer/referentiemodellen/IECCIM/TC57CIM/IEC61970/Base/Wires#TransformerEnd_xground -->


    <owl:ObjectProperty rdf:about="https://w3id.org/netbeheer/referentiemodellen/IECCIM/TC57CIM/IEC61970/Base/Wires#TransformerEnd_xground">
        <rdfs:domain rdf:resource="https://w3id.org/netbeheer/referentiemodellen/IECCIM/TC57CIM/IEC61970/Base/Wires#TransformerEnd"/>
        <rdfs:range rdf:resource="https://w3id.org/netbeheer/referentiemodellen/IECCIM/TC57CIM/IEC61970/Base/Domain#Reactance"/>
        <rdfs:comment>(for Yn and Zn connections) Reactive part of neutral impedance where &apos;grounded&apos; is true.</rdfs:comment>
    </owl:ObjectProperty>
    


    <!-- https://w3id.org/netbeheer/referentiemodellen/IECCIM/TC57CIM/IEC61970/Base/Wires#TransformerMeshImpedance_FromTransformerEnd -->


    <owl:ObjectProperty rdf:about="https://w3id.org/netbeheer/referentiemodellen/IECCIM/TC57CIM/IEC61970/Base/Wires#TransformerMeshImpedance_FromTransformerEnd">
        <rdfs:domain rdf:resource="https://w3id.org/netbeheer/referentiemodellen/IECCIM/TC57CIM/IEC61970/Base/Wires#TransformerMeshImpedance"/>
        <rdfs:range rdf:resource="https://w3id.org/netbeheer/referentiemodellen/IECCIM/TC57CIM/IEC61970/Base/Wires#TransformerEnd"/>
        <rdfs:comment>All mesh impedances between this &apos;to&apos; and other &apos;from&apos; transformer ends.From end this mesh impedance is connected to. It determines the voltage reference.</rdfs:comment>
    </owl:ObjectProperty>
    


    <!-- https://w3id.org/netbeheer/referentiemodellen/IECCIM/TC57CIM/IEC61970/Base/Wires#TransformerMeshImpedance_FromTransformerEndInfo -->


    <owl:ObjectProperty rdf:about="https://w3id.org/netbeheer/referentiemodellen/IECCIM/TC57CIM/IEC61970/Base/Wires#TransformerMeshImpedance_FromTransformerEndInfo">
        <owl:inverseOf rdf:resource="https://w3id.org/netbeheer/referentiemodellen/IECCIM/TC57CIM/IEC61970/Base/Wires#TransformerEndInfo_FromMeshImpedances"/>
        <rdfs:domain rdf:resource="https://w3id.org/netbeheer/referentiemodellen/IECCIM/TC57CIM/IEC61970/Base/Wires#TransformerMeshImpedance"/>
        <rdfs:range rdf:resource="https://w3id.org/netbeheer/referentiemodellen/IECCIM/TC57CIM/IEC61968/AssetInfo#TransformerEndInfo"/>
        <rdfs:comment>&apos;from&apos; transformer end datasheet this mesh impedance is calculated from. It determines the voltage reference.All mesh impedances between this &apos;to&apos; and other &apos;from&apos; transformer ends.</rdfs:comment>
    </owl:ObjectProperty>
    


    <!-- https://w3id.org/netbeheer/referentiemodellen/IECCIM/TC57CIM/IEC61970/Base/Wires#TransformerMeshImpedance_ToTransformerEnd -->


    <owl:ObjectProperty rdf:about="https://w3id.org/netbeheer/referentiemodellen/IECCIM/TC57CIM/IEC61970/Base/Wires#TransformerMeshImpedance_ToTransformerEnd">
        <rdfs:domain rdf:resource="https://w3id.org/netbeheer/referentiemodellen/IECCIM/TC57CIM/IEC61970/Base/Wires#TransformerMeshImpedance"/>
        <rdfs:range rdf:resource="https://w3id.org/netbeheer/referentiemodellen/IECCIM/TC57CIM/IEC61970/Base/Wires#TransformerEnd"/>
        <rdfs:comment>All mesh impedances between this &apos;from&apos; and other &apos;to&apos; transformer ends.All transformer ends this mesh impedance is connected to.</rdfs:comment>
    </owl:ObjectProperty>
    


    <!-- https://w3id.org/netbeheer/referentiemodellen/IECCIM/TC57CIM/IEC61970/Base/Wires#TransformerMeshImpedance_ToTransformerEndInfos -->


    <owl:ObjectProperty rdf:about="https://w3id.org/netbeheer/referentiemodellen/IECCIM/TC57CIM/IEC61970/Base/Wires#TransformerMeshImpedance_ToTransformerEndInfos">
        <owl:inverseOf rdf:resource="https://w3id.org/netbeheer/referentiemodellen/IECCIM/TC57CIM/IEC61970/Base/Wires#TransformerEndInfo_ToMeshImpedances"/>
        <rdfs:domain rdf:resource="https://w3id.org/netbeheer/referentiemodellen/IECCIM/TC57CIM/IEC61970/Base/Wires#TransformerMeshImpedance"/>
        <rdfs:range rdf:resource="https://w3id.org/netbeheer/referentiemodellen/IECCIM/TC57CIM/IEC61968/AssetInfo#TransformerEndInfo"/>
        <rdfs:comment>All &apos;to&apos; transformer end datasheets this mesh impedance for &apos;from&apos; transformer end is calculated from.All mesh impedances between this &apos;from&apos; and other &apos;to&apos; transformer ends.</rdfs:comment>
    </owl:ObjectProperty>
    


    <!-- https://w3id.org/netbeheer/referentiemodellen/IECCIM/TC57CIM/IEC61970/Base/Wires#TransformerMeshImpedance_r -->


    <owl:ObjectProperty rdf:about="https://w3id.org/netbeheer/referentiemodellen/IECCIM/TC57CIM/IEC61970/Base/Wires#TransformerMeshImpedance_r">
        <rdfs:domain rdf:resource="https://w3id.org/netbeheer/referentiemodellen/IECCIM/TC57CIM/IEC61970/Base/Wires#TransformerMeshImpedance"/>
        <rdfs:range rdf:resource="https://w3id.org/netbeheer/referentiemodellen/IECCIM/TC57CIM/IEC61970/Base/Domain#Resistance"/>
        <rdfs:comment>Resistance between the &apos;from&apos; and the &apos;to&apos; end, seen from the &apos;from&apos; end.
</rdfs:comment>
    </owl:ObjectProperty>
    


    <!-- https://w3id.org/netbeheer/referentiemodellen/IECCIM/TC57CIM/IEC61970/Base/Wires#TransformerMeshImpedance_r0 -->


    <owl:ObjectProperty rdf:about="https://w3id.org/netbeheer/referentiemodellen/IECCIM/TC57CIM/IEC61970/Base/Wires#TransformerMeshImpedance_r0">
        <rdfs:domain rdf:resource="https://w3id.org/netbeheer/referentiemodellen/IECCIM/TC57CIM/IEC61970/Base/Wires#TransformerMeshImpedance"/>
        <rdfs:range rdf:resource="https://w3id.org/netbeheer/referentiemodellen/IECCIM/TC57CIM/IEC61970/Base/Domain#Resistance"/>
        <rdfs:comment>Zero-sequence resistance between the &apos;from&apos; and the &apos;to&apos; end, seen from the &apos;from&apos; end.
</rdfs:comment>
    </owl:ObjectProperty>
    


    <!-- https://w3id.org/netbeheer/referentiemodellen/IECCIM/TC57CIM/IEC61970/Base/Wires#TransformerMeshImpedance_x -->


    <owl:ObjectProperty rdf:about="https://w3id.org/netbeheer/referentiemodellen/IECCIM/TC57CIM/IEC61970/Base/Wires#TransformerMeshImpedance_x">
        <rdfs:domain rdf:resource="https://w3id.org/netbeheer/referentiemodellen/IECCIM/TC57CIM/IEC61970/Base/Wires#TransformerMeshImpedance"/>
        <rdfs:range rdf:resource="https://w3id.org/netbeheer/referentiemodellen/IECCIM/TC57CIM/IEC61970/Base/Domain#Reactance"/>
        <rdfs:comment>Reactance between the &apos;from&apos; and the &apos;to&apos; end, seen from the &apos;from&apos; end.
</rdfs:comment>
    </owl:ObjectProperty>
    


    <!-- https://w3id.org/netbeheer/referentiemodellen/IECCIM/TC57CIM/IEC61970/Base/Wires#TransformerMeshImpedance_x0 -->


    <owl:ObjectProperty rdf:about="https://w3id.org/netbeheer/referentiemodellen/IECCIM/TC57CIM/IEC61970/Base/Wires#TransformerMeshImpedance_x0">
        <rdfs:domain rdf:resource="https://w3id.org/netbeheer/referentiemodellen/IECCIM/TC57CIM/IEC61970/Base/Wires#TransformerMeshImpedance"/>
        <rdfs:range rdf:resource="https://w3id.org/netbeheer/referentiemodellen/IECCIM/TC57CIM/IEC61970/Base/Domain#Reactance"/>
        <rdfs:comment>Zero-sequence reactance between the &apos;from&apos; and the &apos;to&apos; end, seen from the &apos;from&apos; end.
</rdfs:comment>
    </owl:ObjectProperty>
    


    <!-- https://w3id.org/netbeheer/referentiemodellen/IECCIM/TC57CIM/IEC61970/Base/Wires#TransformerObservation_Transformer -->


    <owl:ObjectProperty rdf:about="https://w3id.org/netbeheer/referentiemodellen/IECCIM/TC57CIM/IEC61970/Base/Wires#TransformerObservation_Transformer">
        <rdfs:domain rdf:resource="https://w3id.org/netbeheer/referentiemodellen/IECCIM/TC57CIM/IEC61968/InfIEC61968/InfAssets#TransformerObservation"/>
        <rdfs:range rdf:resource="https://w3id.org/netbeheer/referentiemodellen/IECCIM/TC57CIM/IEC61970/Base/Wires#TransformerTank"/>
        <rdfs:comment></rdfs:comment>
    </owl:ObjectProperty>
    


    <!-- https://w3id.org/netbeheer/referentiemodellen/IECCIM/TC57CIM/IEC61970/Base/Wires#TransformerStarImpedance_TransformerEnd -->


    <owl:ObjectProperty rdf:about="https://w3id.org/netbeheer/referentiemodellen/IECCIM/TC57CIM/IEC61970/Base/Wires#TransformerStarImpedance_TransformerEnd">
        <owl:inverseOf rdf:resource="https://w3id.org/netbeheer/referentiemodellen/IECCIM/TC57CIM/IEC61970/Base/Wires#TransformerEnd_StarImpedance"/>
        <rdfs:domain rdf:resource="https://w3id.org/netbeheer/referentiemodellen/IECCIM/TC57CIM/IEC61970/Base/Wires#TransformerStarImpedance"/>
        <rdfs:range rdf:resource="https://w3id.org/netbeheer/referentiemodellen/IECCIM/TC57CIM/IEC61970/Base/Wires#TransformerEnd"/>
        <rdfs:comment>All transformer ends having this star impedance.(accurate for 2- or 3-winding transformers only) Pi-model impedances of this transformer end. By convention, for a two winding transformer, the full values of the transformer should be entered on the high voltage end (endNumber=1).</rdfs:comment>
    </owl:ObjectProperty>
    


    <!-- https://w3id.org/netbeheer/referentiemodellen/IECCIM/TC57CIM/IEC61970/Base/Wires#TransformerStarImpedance_TransformerEndInfo -->


    <owl:ObjectProperty rdf:about="https://w3id.org/netbeheer/referentiemodellen/IECCIM/TC57CIM/IEC61970/Base/Wires#TransformerStarImpedance_TransformerEndInfo">
        <owl:inverseOf rdf:resource="https://w3id.org/netbeheer/referentiemodellen/IECCIM/TC57CIM/IEC61970/Base/Wires#TransformerEndInfo_TransformerStarImpedance"/>
        <rdfs:domain rdf:resource="https://w3id.org/netbeheer/referentiemodellen/IECCIM/TC57CIM/IEC61970/Base/Wires#TransformerStarImpedance"/>
        <rdfs:range rdf:resource="https://w3id.org/netbeheer/referentiemodellen/IECCIM/TC57CIM/IEC61968/AssetInfo#TransformerEndInfo"/>
        <rdfs:comment>Transformer end datasheet used to calculate this transformer star impedance.Transformer star impedance calculated from this transformer end datasheet.</rdfs:comment>
    </owl:ObjectProperty>
    


    <!-- https://w3id.org/netbeheer/referentiemodellen/IECCIM/TC57CIM/IEC61970/Base/Wires#TransformerStarImpedance_r -->


    <owl:ObjectProperty rdf:about="https://w3id.org/netbeheer/referentiemodellen/IECCIM/TC57CIM/IEC61970/Base/Wires#TransformerStarImpedance_r">
        <rdfs:domain rdf:resource="https://w3id.org/netbeheer/referentiemodellen/IECCIM/TC57CIM/IEC61970/Base/Wires#TransformerStarImpedance"/>
        <rdfs:range rdf:resource="https://w3id.org/netbeheer/referentiemodellen/IECCIM/TC57CIM/IEC61970/Base/Domain#Resistance"/>
        <rdfs:comment>Resistance of the transformer end.
</rdfs:comment>
    </owl:ObjectProperty>
    


    <!-- https://w3id.org/netbeheer/referentiemodellen/IECCIM/TC57CIM/IEC61970/Base/Wires#TransformerStarImpedance_r0 -->


    <owl:ObjectProperty rdf:about="https://w3id.org/netbeheer/referentiemodellen/IECCIM/TC57CIM/IEC61970/Base/Wires#TransformerStarImpedance_r0">
        <rdfs:domain rdf:resource="https://w3id.org/netbeheer/referentiemodellen/IECCIM/TC57CIM/IEC61970/Base/Wires#TransformerStarImpedance"/>
        <rdfs:range rdf:resource="https://w3id.org/netbeheer/referentiemodellen/IECCIM/TC57CIM/IEC61970/Base/Domain#Resistance"/>
        <rdfs:comment>Zero sequence series resistance of the transformer end.
</rdfs:comment>
    </owl:ObjectProperty>
    


    <!-- https://w3id.org/netbeheer/referentiemodellen/IECCIM/TC57CIM/IEC61970/Base/Wires#TransformerStarImpedance_x -->


    <owl:ObjectProperty rdf:about="https://w3id.org/netbeheer/referentiemodellen/IECCIM/TC57CIM/IEC61970/Base/Wires#TransformerStarImpedance_x">
        <rdfs:domain rdf:resource="https://w3id.org/netbeheer/referentiemodellen/IECCIM/TC57CIM/IEC61970/Base/Wires#TransformerStarImpedance"/>
        <rdfs:range rdf:resource="https://w3id.org/netbeheer/referentiemodellen/IECCIM/TC57CIM/IEC61970/Base/Domain#Reactance"/>
        <rdfs:comment>Positive sequence series reactance of the transformer end.
</rdfs:comment>
    </owl:ObjectProperty>
    


    <!-- https://w3id.org/netbeheer/referentiemodellen/IECCIM/TC57CIM/IEC61970/Base/Wires#TransformerStarImpedance_x0 -->


    <owl:ObjectProperty rdf:about="https://w3id.org/netbeheer/referentiemodellen/IECCIM/TC57CIM/IEC61970/Base/Wires#TransformerStarImpedance_x0">
        <rdfs:domain rdf:resource="https://w3id.org/netbeheer/referentiemodellen/IECCIM/TC57CIM/IEC61970/Base/Wires#TransformerStarImpedance"/>
        <rdfs:range rdf:resource="https://w3id.org/netbeheer/referentiemodellen/IECCIM/TC57CIM/IEC61970/Base/Domain#Reactance"/>
        <rdfs:comment>Zero sequence series reactance of the transformer end.
</rdfs:comment>
    </owl:ObjectProperty>
    


    <!-- https://w3id.org/netbeheer/referentiemodellen/IECCIM/TC57CIM/IEC61970/Base/Wires#TransformerTankEnd_TransformerTank -->


    <owl:ObjectProperty rdf:about="https://w3id.org/netbeheer/referentiemodellen/IECCIM/TC57CIM/IEC61970/Base/Wires#TransformerTankEnd_TransformerTank">
        <rdfs:domain rdf:resource="https://w3id.org/netbeheer/referentiemodellen/IECCIM/TC57CIM/IEC61970/Base/Wires#TransformerTankEnd"/>
        <rdfs:range rdf:resource="https://w3id.org/netbeheer/referentiemodellen/IECCIM/TC57CIM/IEC61970/Base/Wires#TransformerTank"/>
        <rdfs:comment>All windings of this transformer.Transformer this winding belongs to.</rdfs:comment>
    </owl:ObjectProperty>
    


    <!-- https://w3id.org/netbeheer/referentiemodellen/IECCIM/TC57CIM/IEC61970/Base/Wires#TransformerTank_PowerTransformer -->


    <owl:ObjectProperty rdf:about="https://w3id.org/netbeheer/referentiemodellen/IECCIM/TC57CIM/IEC61970/Base/Wires#TransformerTank_PowerTransformer">
        <rdfs:domain rdf:resource="https://w3id.org/netbeheer/referentiemodellen/IECCIM/TC57CIM/IEC61970/Base/Wires#TransformerTank"/>
        <rdfs:range rdf:resource="https://w3id.org/netbeheer/referentiemodellen/IECCIM/TC57CIM/IEC61970/Base/Wires#PowerTransformer"/>
        <rdfs:comment>All transformers that belong to this bank.Bank this transformer belongs to.</rdfs:comment>
    </owl:ObjectProperty>
    


    <!-- https://w3id.org/netbeheer/referentiemodellen/IECCIM/TC57CIM/IEC61970/Base/Wires#TransformerTank_TransformerObservations -->


    <owl:ObjectProperty rdf:about="https://w3id.org/netbeheer/referentiemodellen/IECCIM/TC57CIM/IEC61970/Base/Wires#TransformerTank_TransformerObservations">
        <owl:inverseOf rdf:resource="https://w3id.org/netbeheer/referentiemodellen/IECCIM/TC57CIM/IEC61970/Base/Wires#TransformerObservation_Transformer"/>
        <rdfs:domain rdf:resource="https://w3id.org/netbeheer/referentiemodellen/IECCIM/TC57CIM/IEC61970/Base/Wires#TransformerTank"/>
        <rdfs:range rdf:resource="https://w3id.org/netbeheer/referentiemodellen/IECCIM/TC57CIM/IEC61968/InfIEC61968/InfAssets#TransformerObservation"/>
        <rdfs:comment></rdfs:comment>
    </owl:ObjectProperty>
    


    <!-- https://w3id.org/netbeheer/referentiemodellen/IECCIM/TC57CIM/IEC61970/Base/Wires#TransformerTank_TransformerTankEnds -->


    <owl:ObjectProperty rdf:about="https://w3id.org/netbeheer/referentiemodellen/IECCIM/TC57CIM/IEC61970/Base/Wires#TransformerTank_TransformerTankEnds">
        <owl:inverseOf rdf:resource="https://w3id.org/netbeheer/referentiemodellen/IECCIM/TC57CIM/IEC61970/Base/Wires#TransformerTankEnd_TransformerTank"/>
        <rdfs:domain rdf:resource="https://w3id.org/netbeheer/referentiemodellen/IECCIM/TC57CIM/IEC61970/Base/Wires#TransformerTank"/>
        <rdfs:range rdf:resource="https://w3id.org/netbeheer/referentiemodellen/IECCIM/TC57CIM/IEC61970/Base/Wires#TransformerTankEnd"/>
        <rdfs:comment>All windings of this transformer.Transformer this winding belongs to.</rdfs:comment>
    </owl:ObjectProperty>
    


    <!-- https://w3id.org/netbeheer/referentiemodellen/IECCIM/TC57CIM/IEC61970/Base/Wires#VoltageControlZone_BusbarSection -->


    <owl:ObjectProperty rdf:about="https://w3id.org/netbeheer/referentiemodellen/IECCIM/TC57CIM/IEC61970/Base/Wires#VoltageControlZone_BusbarSection">
        <owl:inverseOf rdf:resource="https://w3id.org/netbeheer/referentiemodellen/IECCIM/TC57CIM/IEC61970/Base/Wires#BusbarSection_VoltageControlZone"/>
        <rdfs:domain rdf:resource="https://w3id.org/netbeheer/referentiemodellen/IECCIM/TC57CIM/IEC61970/Base/Wires#VoltageControlZone"/>
        <rdfs:range rdf:resource="https://w3id.org/netbeheer/referentiemodellen/IECCIM/TC57CIM/IEC61970/Base/Wires#BusbarSection"/>
        <rdfs:comment>A VoltageControlZone is controlled by a designated BusbarSection.A VoltageControlZone is controlled by a designated BusbarSection.</rdfs:comment>
    </owl:ObjectProperty>
    


    <!-- https://w3id.org/netbeheer/referentiemodellen/IECCIM/TC57CIM/IEC61970/Base/Wires#VoltageControlZone_RegulationSchedule -->


    <owl:ObjectProperty rdf:about="https://w3id.org/netbeheer/referentiemodellen/IECCIM/TC57CIM/IEC61970/Base/Wires#VoltageControlZone_RegulationSchedule">
        <owl:inverseOf rdf:resource="https://w3id.org/netbeheer/referentiemodellen/IECCIM/TC57CIM/IEC61970/Base/Wires#RegulationSchedule_VoltageControlZones"/>
        <rdfs:domain rdf:resource="https://w3id.org/netbeheer/referentiemodellen/IECCIM/TC57CIM/IEC61970/Base/Wires#VoltageControlZone"/>
        <rdfs:range rdf:resource="https://w3id.org/netbeheer/referentiemodellen/IECCIM/TC57CIM/IEC61970/Base/Wires#RegulationSchedule"/>
        <rdfs:comment>A VoltageControlZone may have a  voltage regulation schedule.A VoltageControlZone may have a  voltage regulation schedule.</rdfs:comment>
    </owl:ObjectProperty>
    


    <!-- https://w3id.org/netbeheer/referentiemodellen/IECCIM/TC57CIM/IEC61970/Base/Wires#WindTurbineType3or4Dynamics_EnergySource -->


    <owl:ObjectProperty rdf:about="https://w3id.org/netbeheer/referentiemodellen/IECCIM/TC57CIM/IEC61970/Base/Wires#WindTurbineType3or4Dynamics_EnergySource">
        <rdfs:domain rdf:resource="https://w3id.org/netbeheer/referentiemodellen/IECCIM/TC57CIM/IEC61970/Dynamics/StandardModels/WindDynamics#WindTurbineType3or4Dynamics"/>
        <rdfs:range rdf:resource="https://w3id.org/netbeheer/referentiemodellen/IECCIM/TC57CIM/IEC61970/Base/Wires#EnergySource"/>
        <rdfs:comment>Wind generator Type 3 or 4 dynamics model associated with this energy source.Energy Source (current source) with which this wind Type 3 or 4 dynamics model is asoociated.</rdfs:comment>
    </owl:ObjectProperty>
    


    <!-- https://w3id.org/netbeheer/referentiemodellen/IECCIM/TC57CIM/IEC61970/Base/Wires#WindingInsulation_FromWinding -->


    <owl:ObjectProperty rdf:about="https://w3id.org/netbeheer/referentiemodellen/IECCIM/TC57CIM/IEC61970/Base/Wires#WindingInsulation_FromWinding">
        <rdfs:domain rdf:resource="https://w3id.org/netbeheer/referentiemodellen/IECCIM/TC57CIM/IEC61968/InfIEC61968/InfAssets#WindingInsulation"/>
        <rdfs:range rdf:resource="https://w3id.org/netbeheer/referentiemodellen/IECCIM/TC57CIM/IEC61970/Base/Wires#TransformerEnd"/>
        <rdfs:comment></rdfs:comment>
    </owl:ObjectProperty>
    


    <!-- https://w3id.org/netbeheer/referentiemodellen/IECCIM/TC57CIM/IEC61970/Base/Wires#WindingInsulation_ToWinding -->


    <owl:ObjectProperty rdf:about="https://w3id.org/netbeheer/referentiemodellen/IECCIM/TC57CIM/IEC61970/Base/Wires#WindingInsulation_ToWinding">
        <rdfs:domain rdf:resource="https://w3id.org/netbeheer/referentiemodellen/IECCIM/TC57CIM/IEC61968/InfIEC61968/InfAssets#WindingInsulation"/>
        <rdfs:range rdf:resource="https://w3id.org/netbeheer/referentiemodellen/IECCIM/TC57CIM/IEC61970/Base/Wires#TransformerEnd"/>
        <rdfs:comment></rdfs:comment>
    </owl:ObjectProperty>
    


    <!-- https://w3id.org/netbeheer/referentiemodellen/IECCIM/TC57CIM/IEC61970/Base/Wires#WireInfo_PerLengthParameters -->


    <owl:ObjectProperty rdf:about="https://w3id.org/netbeheer/referentiemodellen/IECCIM/TC57CIM/IEC61970/Base/Wires#WireInfo_PerLengthParameters">
        <rdfs:domain rdf:resource="https://w3id.org/netbeheer/referentiemodellen/IECCIM/TC57CIM/IEC61968/AssetInfo#WireInfo"/>
        <rdfs:range rdf:resource="https://w3id.org/netbeheer/referentiemodellen/IECCIM/TC57CIM/IEC61970/Base/Wires#PerLengthLineParameter"/>
        <rdfs:comment>All wire datasheets used to calculate this per-length parameter.All per-length parameters calculated from this wire datasheet.</rdfs:comment>
    </owl:ObjectProperty>
    


    <!-- https://w3id.org/netbeheer/referentiemodellen/IECCIM/TC57CIM/IEC61970/Base/Wires#WireSpacing_ACLineSegments -->


    <owl:ObjectProperty rdf:about="https://w3id.org/netbeheer/referentiemodellen/IECCIM/TC57CIM/IEC61970/Base/Wires#WireSpacing_ACLineSegments">
        <rdfs:domain rdf:resource="https://w3id.org/netbeheer/referentiemodellen/IECCIM/TC57CIM/IEC61968/AssetInfo#WireSpacing"/>
        <rdfs:range rdf:resource="https://w3id.org/netbeheer/referentiemodellen/IECCIM/TC57CIM/IEC61970/Base/Wires#ACLineSegment"/>
        <rdfs:comment>Wire spacing configuration for this line segment.All line segments described with this wire spacing configuration.</rdfs:comment>
    </owl:ObjectProperty>
    


    <!-- https://w3id.org/netbeheer/referentiemodellen/IECCIM/TC57CIM/IEC61970/Base/Wires#WireSpacing_PerLengthParameters -->


    <owl:ObjectProperty rdf:about="https://w3id.org/netbeheer/referentiemodellen/IECCIM/TC57CIM/IEC61970/Base/Wires#WireSpacing_PerLengthParameters">
        <rdfs:domain rdf:resource="https://w3id.org/netbeheer/referentiemodellen/IECCIM/TC57CIM/IEC61968/AssetInfo#WireSpacing"/>
        <rdfs:range rdf:resource="https://w3id.org/netbeheer/referentiemodellen/IECCIM/TC57CIM/IEC61970/Base/Wires#PerLengthLineParameter"/>
        <rdfs:comment>Wire spacing datasheet used to calculate this per-length parameter.All per-length parameters calculated from this wire spacing datasheet.</rdfs:comment>
    </owl:ObjectProperty>
    


    <!-- 
    ///////////////////////////////////////////////////////////////////////////////////////
    //
    // Data properties
    //
    ///////////////////////////////////////////////////////////////////////////////////////
     -->


    


    <!-- https://w3id.org/netbeheer/referentiemodellen/IECCIM/TC57CIM/IEC61970/Base/Wires#ACLineSegmentPhase_phase -->


    <owl:DatatypeProperty rdf:about="https://w3id.org/netbeheer/referentiemodellen/IECCIM/TC57CIM/IEC61970/Base/Wires#ACLineSegmentPhase_phase">
        <rdfs:domain rdf:resource="https://w3id.org/netbeheer/referentiemodellen/IECCIM/TC57CIM/IEC61970/Base/Wires#ACLineSegmentPhase"/>
        <rdfs:range rdf:resource="https://w3id.org/netbeheer/referentiemodellen/IECCIM/TC57CIM/IEC61970/Base/Wires#SinglePhaseKind"/>
        <rdfs:comment>The phase connection of the wire at both ends.
</rdfs:comment>
    </owl:DatatypeProperty>
    


    <!-- https://w3id.org/netbeheer/referentiemodellen/IECCIM/TC57CIM/IEC61970/Base/Wires#ACLineSegmentPhase_sequenceNumber -->


    <owl:DatatypeProperty rdf:about="https://w3id.org/netbeheer/referentiemodellen/IECCIM/TC57CIM/IEC61970/Base/Wires#ACLineSegmentPhase_sequenceNumber">
        <rdfs:domain rdf:resource="https://w3id.org/netbeheer/referentiemodellen/IECCIM/TC57CIM/IEC61970/Base/Wires#ACLineSegmentPhase"/>
        <rdfs:range rdf:resource="http://www.w3.org/2001/XMLSchema#nonNegativeInteger"/>
        <rdfs:comment>Number designation for this line segment phase. Each line segment phase within a line segment should have a unique sequence number. This is useful for unbalanced modeling to bind the mathematical model (PhaseImpedanceData of PerLengthPhaseImpedance) with the connectivity model (this class) and the physical model (WirePosition) without tight coupling.</rdfs:comment>
    </owl:DatatypeProperty>
    


    <!-- https://w3id.org/netbeheer/referentiemodellen/IECCIM/TC57CIM/IEC61970/Base/Wires#AsynchronousMachine_asynchronousMachineType -->


    <owl:DatatypeProperty rdf:about="https://w3id.org/netbeheer/referentiemodellen/IECCIM/TC57CIM/IEC61970/Base/Wires#AsynchronousMachine_asynchronousMachineType">
        <rdfs:domain rdf:resource="https://w3id.org/netbeheer/referentiemodellen/IECCIM/TC57CIM/IEC61970/Base/Wires#AsynchronousMachine"/>
        <rdfs:range rdf:resource="https://w3id.org/netbeheer/referentiemodellen/IECCIM/TC57CIM/IEC61970/Base/Wires#AsynchronousMachineKind"/>
        <rdfs:comment>Indicates the type of Asynchronous Machine (motor or generator).</rdfs:comment>
    </owl:DatatypeProperty>
    


    <!-- https://w3id.org/netbeheer/referentiemodellen/IECCIM/TC57CIM/IEC61970/Base/Wires#AsynchronousMachine_converterFedDrive -->


    <owl:DatatypeProperty rdf:about="https://w3id.org/netbeheer/referentiemodellen/IECCIM/TC57CIM/IEC61970/Base/Wires#AsynchronousMachine_converterFedDrive">
        <rdfs:domain rdf:resource="https://w3id.org/netbeheer/referentiemodellen/IECCIM/TC57CIM/IEC61970/Base/Wires#AsynchronousMachine"/>
        <rdfs:range rdf:resource="http://www.w3.org/2001/XMLSchema#boolean"/>
        <rdfs:comment>Indicates whether the machine is a converter fed drive. Used for short circuit data exchange according to IEC 60909</rdfs:comment>
    </owl:DatatypeProperty>
    


    <!-- https://w3id.org/netbeheer/referentiemodellen/IECCIM/TC57CIM/IEC61970/Base/Wires#AsynchronousMachine_iaIrRatio -->


    <owl:DatatypeProperty rdf:about="https://w3id.org/netbeheer/referentiemodellen/IECCIM/TC57CIM/IEC61970/Base/Wires#AsynchronousMachine_iaIrRatio">
        <rdfs:domain rdf:resource="https://w3id.org/netbeheer/referentiemodellen/IECCIM/TC57CIM/IEC61970/Base/Wires#AsynchronousMachine"/>
        <rdfs:range rdf:resource="http://www.w3.org/2001/XMLSchema#float"/>
        <rdfs:comment>Ratio of locked-rotor current to the rated current of the motor (Ia/Ir). Used for short circuit data exchange according to IEC 60909</rdfs:comment>
    </owl:DatatypeProperty>
    


    <!-- https://w3id.org/netbeheer/referentiemodellen/IECCIM/TC57CIM/IEC61970/Base/Wires#AsynchronousMachine_polePairNumber -->


    <owl:DatatypeProperty rdf:about="https://w3id.org/netbeheer/referentiemodellen/IECCIM/TC57CIM/IEC61970/Base/Wires#AsynchronousMachine_polePairNumber">
        <rdfs:domain rdf:resource="https://w3id.org/netbeheer/referentiemodellen/IECCIM/TC57CIM/IEC61970/Base/Wires#AsynchronousMachine"/>
        <rdfs:range rdf:resource="http://www.w3.org/2001/XMLSchema#nonNegativeInteger"/>
        <rdfs:comment>Number of pole pairs of stator. Used for short circuit data exchange according to IEC 60909</rdfs:comment>
    </owl:DatatypeProperty>
    


    <!-- https://w3id.org/netbeheer/referentiemodellen/IECCIM/TC57CIM/IEC61970/Base/Wires#AsynchronousMachine_reversible -->


    <owl:DatatypeProperty rdf:about="https://w3id.org/netbeheer/referentiemodellen/IECCIM/TC57CIM/IEC61970/Base/Wires#AsynchronousMachine_reversible">
        <rdfs:domain rdf:resource="https://w3id.org/netbeheer/referentiemodellen/IECCIM/TC57CIM/IEC61970/Base/Wires#AsynchronousMachine"/>
        <rdfs:range rdf:resource="http://www.w3.org/2001/XMLSchema#boolean"/>
        <rdfs:comment>Indicates for converter drive motors if the power can be reversible. Used for short circuit data exchange according to IEC 60909</rdfs:comment>
    </owl:DatatypeProperty>
    


    <!-- https://w3id.org/netbeheer/referentiemodellen/IECCIM/TC57CIM/IEC61970/Base/Wires#AsynchronousMachine_rxLockedRotorRatio -->


    <owl:DatatypeProperty rdf:about="https://w3id.org/netbeheer/referentiemodellen/IECCIM/TC57CIM/IEC61970/Base/Wires#AsynchronousMachine_rxLockedRotorRatio">
        <rdfs:domain rdf:resource="https://w3id.org/netbeheer/referentiemodellen/IECCIM/TC57CIM/IEC61970/Base/Wires#AsynchronousMachine"/>
        <rdfs:range rdf:resource="http://www.w3.org/2001/XMLSchema#float"/>
        <rdfs:comment>Locked rotor ratio (R/X). Used for short circuit data exchange according to IEC 60909</rdfs:comment>
    </owl:DatatypeProperty>
    


    <!-- https://w3id.org/netbeheer/referentiemodellen/IECCIM/TC57CIM/IEC61970/Base/Wires#CompositeSwitch_compositeSwitchType -->


    <owl:DatatypeProperty rdf:about="https://w3id.org/netbeheer/referentiemodellen/IECCIM/TC57CIM/IEC61970/Base/Wires#CompositeSwitch_compositeSwitchType">
        <rdfs:domain rdf:resource="https://w3id.org/netbeheer/referentiemodellen/IECCIM/TC57CIM/IEC61970/Base/Wires#CompositeSwitch"/>
        <rdfs:range rdf:resource="http://www.w3.org/2001/XMLSchema#string"/>
        <rdfs:comment>An alphanumeric code that can be used as a reference to extra information such as the description of the interlocking scheme if any.</rdfs:comment>
    </owl:DatatypeProperty>
    


    <!-- https://w3id.org/netbeheer/referentiemodellen/IECCIM/TC57CIM/IEC61970/Base/Wires#EnergyConsumerPhase_phase -->


    <owl:DatatypeProperty rdf:about="https://w3id.org/netbeheer/referentiemodellen/IECCIM/TC57CIM/IEC61970/Base/Wires#EnergyConsumerPhase_phase">
        <rdfs:domain rdf:resource="https://w3id.org/netbeheer/referentiemodellen/IECCIM/TC57CIM/IEC61970/Base/Wires#EnergyConsumerPhase"/>
        <rdfs:range rdf:resource="https://w3id.org/netbeheer/referentiemodellen/IECCIM/TC57CIM/IEC61970/Base/Wires#SinglePhaseKind"/>
        <rdfs:comment>Phase of this energy consumer component.   If the energy consumer is wye connected, the connection is from the indicated phase to the central ground or neutral point.  If the energy consumer is delta connected, the phase indicates an energy consumer connected from the indicated phase to the next logical non-neutral phase.
</rdfs:comment>
    </owl:DatatypeProperty>
    


    <!-- https://w3id.org/netbeheer/referentiemodellen/IECCIM/TC57CIM/IEC61970/Base/Wires#EnergyConsumer_customerCount -->


    <owl:DatatypeProperty rdf:about="https://w3id.org/netbeheer/referentiemodellen/IECCIM/TC57CIM/IEC61970/Base/Wires#EnergyConsumer_customerCount">
        <rdfs:domain rdf:resource="https://w3id.org/netbeheer/referentiemodellen/IECCIM/TC57CIM/IEC61970/Base/Wires#EnergyConsumer"/>
        <rdfs:range rdf:resource="http://www.w3.org/2001/XMLSchema#nonNegativeInteger"/>
        <rdfs:comment>Number of individual customers represented by this demand.
</rdfs:comment>
    </owl:DatatypeProperty>
    


    <!-- https://w3id.org/netbeheer/referentiemodellen/IECCIM/TC57CIM/IEC61970/Base/Wires#EnergyConsumer_grounded -->


    <owl:DatatypeProperty rdf:about="https://w3id.org/netbeheer/referentiemodellen/IECCIM/TC57CIM/IEC61970/Base/Wires#EnergyConsumer_grounded">
        <rdfs:domain rdf:resource="https://w3id.org/netbeheer/referentiemodellen/IECCIM/TC57CIM/IEC61970/Base/Wires#EnergyConsumer"/>
        <rdfs:range rdf:resource="http://www.w3.org/2001/XMLSchema#boolean"/>
        <rdfs:comment>Used for Yn and Zn connections. True if the neutral is solidly grounded.</rdfs:comment>
    </owl:DatatypeProperty>
    


    <!-- https://w3id.org/netbeheer/referentiemodellen/IECCIM/TC57CIM/IEC61970/Base/Wires#EnergyConsumer_phaseConnection -->


    <owl:DatatypeProperty rdf:about="https://w3id.org/netbeheer/referentiemodellen/IECCIM/TC57CIM/IEC61970/Base/Wires#EnergyConsumer_phaseConnection">
        <rdfs:domain rdf:resource="https://w3id.org/netbeheer/referentiemodellen/IECCIM/TC57CIM/IEC61970/Base/Wires#EnergyConsumer"/>
        <rdfs:range rdf:resource="https://w3id.org/netbeheer/referentiemodellen/IECCIM/TC57CIM/IEC61970/Base/Wires#PhaseShuntConnectionKind"/>
        <rdfs:comment>The type of phase connection, such as wye or delta.
</rdfs:comment>
    </owl:DatatypeProperty>
    


    <!-- https://w3id.org/netbeheer/referentiemodellen/IECCIM/TC57CIM/IEC61970/Base/Wires#EnergySourcePhase_phase -->


    <owl:DatatypeProperty rdf:about="https://w3id.org/netbeheer/referentiemodellen/IECCIM/TC57CIM/IEC61970/Base/Wires#EnergySourcePhase_phase">
        <rdfs:domain rdf:resource="https://w3id.org/netbeheer/referentiemodellen/IECCIM/TC57CIM/IEC61970/Base/Wires#EnergySourcePhase"/>
        <rdfs:range rdf:resource="https://w3id.org/netbeheer/referentiemodellen/IECCIM/TC57CIM/IEC61970/Base/Wires#SinglePhaseKind"/>
        <rdfs:comment>Phase of this energy source component.   If the energy source wye connected, the connection is from the indicated phase to the central ground or neutral point.  If the energy source is delta connected, the phase indicates an energy source connected from the indicated phase to the next logical non-neutral phase.</rdfs:comment>
    </owl:DatatypeProperty>
    


    <!-- https://w3id.org/netbeheer/referentiemodellen/IECCIM/TC57CIM/IEC61970/Base/Wires#ExternalNetworkInjection_ikSecond -->


    <owl:DatatypeProperty rdf:about="https://w3id.org/netbeheer/referentiemodellen/IECCIM/TC57CIM/IEC61970/Base/Wires#ExternalNetworkInjection_ikSecond">
        <rdfs:domain rdf:resource="https://w3id.org/netbeheer/referentiemodellen/IECCIM/TC57CIM/IEC61970/Base/Wires#ExternalNetworkInjection"/>
        <rdfs:range rdf:resource="http://www.w3.org/2001/XMLSchema#boolean"/>
        <rdfs:comment>Indicates whether initial symmetrical short-circuit current and power have been calculated according to IEC (Ik&quot;).
</rdfs:comment>
    </owl:DatatypeProperty>
    


    <!-- https://w3id.org/netbeheer/referentiemodellen/IECCIM/TC57CIM/IEC61970/Base/Wires#ExternalNetworkInjection_maxR0ToX0Ratio -->


    <owl:DatatypeProperty rdf:about="https://w3id.org/netbeheer/referentiemodellen/IECCIM/TC57CIM/IEC61970/Base/Wires#ExternalNetworkInjection_maxR0ToX0Ratio">
        <rdfs:domain rdf:resource="https://w3id.org/netbeheer/referentiemodellen/IECCIM/TC57CIM/IEC61970/Base/Wires#ExternalNetworkInjection"/>
        <rdfs:range rdf:resource="http://www.w3.org/2001/XMLSchema#float"/>
        <rdfs:comment>Maximum ratio of zero sequence resistance of Network Feeder to its zero sequence reactance (R(0)/X(0) max). Used for short circuit data exchange according to IEC 60909
</rdfs:comment>
    </owl:DatatypeProperty>
    


    <!-- https://w3id.org/netbeheer/referentiemodellen/IECCIM/TC57CIM/IEC61970/Base/Wires#ExternalNetworkInjection_maxR1ToX1Ratio -->


    <owl:DatatypeProperty rdf:about="https://w3id.org/netbeheer/referentiemodellen/IECCIM/TC57CIM/IEC61970/Base/Wires#ExternalNetworkInjection_maxR1ToX1Ratio">
        <rdfs:domain rdf:resource="https://w3id.org/netbeheer/referentiemodellen/IECCIM/TC57CIM/IEC61970/Base/Wires#ExternalNetworkInjection"/>
        <rdfs:range rdf:resource="http://www.w3.org/2001/XMLSchema#float"/>
        <rdfs:comment>Maximum ratio of positive sequence resistance of Network Feeder to its positive sequence reactance (R(1)/X(1) max). Used for short circuit data exchange according to IEC 60909
</rdfs:comment>
    </owl:DatatypeProperty>
    


    <!-- https://w3id.org/netbeheer/referentiemodellen/IECCIM/TC57CIM/IEC61970/Base/Wires#ExternalNetworkInjection_maxZ0ToZ1Ratio -->


    <owl:DatatypeProperty rdf:about="https://w3id.org/netbeheer/referentiemodellen/IECCIM/TC57CIM/IEC61970/Base/Wires#ExternalNetworkInjection_maxZ0ToZ1Ratio">
        <rdfs:domain rdf:resource="https://w3id.org/netbeheer/referentiemodellen/IECCIM/TC57CIM/IEC61970/Base/Wires#ExternalNetworkInjection"/>
        <rdfs:range rdf:resource="http://www.w3.org/2001/XMLSchema#float"/>
        <rdfs:comment>Maximum ratio of zero sequence impedance to its positive sequence impedance (Z(0)/Z(1) max). Used for short circuit data exchange according to IEC 60909
</rdfs:comment>
    </owl:DatatypeProperty>
    


    <!-- https://w3id.org/netbeheer/referentiemodellen/IECCIM/TC57CIM/IEC61970/Base/Wires#ExternalNetworkInjection_minR0ToX0Ratio -->


    <owl:DatatypeProperty rdf:about="https://w3id.org/netbeheer/referentiemodellen/IECCIM/TC57CIM/IEC61970/Base/Wires#ExternalNetworkInjection_minR0ToX0Ratio">
        <rdfs:domain rdf:resource="https://w3id.org/netbeheer/referentiemodellen/IECCIM/TC57CIM/IEC61970/Base/Wires#ExternalNetworkInjection"/>
        <rdfs:range rdf:resource="http://www.w3.org/2001/XMLSchema#float"/>
        <rdfs:comment>Indicates whether initial symmetrical short-circuit current and power have been calculated according to IEC (Ik&quot;). Used for short circuit data exchange according to IEC 6090
</rdfs:comment>
    </owl:DatatypeProperty>
    


    <!-- https://w3id.org/netbeheer/referentiemodellen/IECCIM/TC57CIM/IEC61970/Base/Wires#ExternalNetworkInjection_minR1ToX1Ratio -->


    <owl:DatatypeProperty rdf:about="https://w3id.org/netbeheer/referentiemodellen/IECCIM/TC57CIM/IEC61970/Base/Wires#ExternalNetworkInjection_minR1ToX1Ratio">
        <rdfs:domain rdf:resource="https://w3id.org/netbeheer/referentiemodellen/IECCIM/TC57CIM/IEC61970/Base/Wires#ExternalNetworkInjection"/>
        <rdfs:range rdf:resource="http://www.w3.org/2001/XMLSchema#float"/>
        <rdfs:comment>Minimum ratio of positive sequence resistance of Network Feeder to its positive sequence reactance (R(1)/X(1) min). Used for short circuit data exchange according to IEC 60909
</rdfs:comment>
    </owl:DatatypeProperty>
    


    <!-- https://w3id.org/netbeheer/referentiemodellen/IECCIM/TC57CIM/IEC61970/Base/Wires#ExternalNetworkInjection_minZ0ToZ1Ratio -->


    <owl:DatatypeProperty rdf:about="https://w3id.org/netbeheer/referentiemodellen/IECCIM/TC57CIM/IEC61970/Base/Wires#ExternalNetworkInjection_minZ0ToZ1Ratio">
        <rdfs:domain rdf:resource="https://w3id.org/netbeheer/referentiemodellen/IECCIM/TC57CIM/IEC61970/Base/Wires#ExternalNetworkInjection"/>
        <rdfs:range rdf:resource="http://www.w3.org/2001/XMLSchema#float"/>
        <rdfs:comment>Minimum ratio of zero sequence impedance to its positive sequence impedance (Z(0)/Z(1) min). Used for short circuit data exchange according to IEC 60909
</rdfs:comment>
    </owl:DatatypeProperty>
    


    <!-- https://w3id.org/netbeheer/referentiemodellen/IECCIM/TC57CIM/IEC61970/Base/Wires#ExternalNetworkInjection_referencePriority -->


    <owl:DatatypeProperty rdf:about="https://w3id.org/netbeheer/referentiemodellen/IECCIM/TC57CIM/IEC61970/Base/Wires#ExternalNetworkInjection_referencePriority">
        <rdfs:domain rdf:resource="https://w3id.org/netbeheer/referentiemodellen/IECCIM/TC57CIM/IEC61970/Base/Wires#ExternalNetworkInjection"/>
        <rdfs:range rdf:resource="http://www.w3.org/2001/XMLSchema#nonNegativeInteger"/>
        <rdfs:comment>Priority of unit for use as powerflow voltage phase angle reference bus selection. 0 = don t care (default) 1 = highest priority. 2 is less than 1 and so on.
</rdfs:comment>
    </owl:DatatypeProperty>
    


    <!-- https://w3id.org/netbeheer/referentiemodellen/IECCIM/TC57CIM/IEC61970/Base/Wires#NonlinearShuntCompensatorPhasePoint_sectionNumber -->


    <owl:DatatypeProperty rdf:about="https://w3id.org/netbeheer/referentiemodellen/IECCIM/TC57CIM/IEC61970/Base/Wires#NonlinearShuntCompensatorPhasePoint_sectionNumber">
        <rdfs:domain rdf:resource="https://w3id.org/netbeheer/referentiemodellen/IECCIM/TC57CIM/IEC61970/Base/Wires#NonlinearShuntCompensatorPhasePoint"/>
        <rdfs:range rdf:resource="http://www.w3.org/2001/XMLSchema#nonNegativeInteger"/>
        <rdfs:comment>The number of the section.</rdfs:comment>
    </owl:DatatypeProperty>
    


    <!-- https://w3id.org/netbeheer/referentiemodellen/IECCIM/TC57CIM/IEC61970/Base/Wires#NonlinearShuntCompensatorPoint_sectionNumber -->


    <owl:DatatypeProperty rdf:about="https://w3id.org/netbeheer/referentiemodellen/IECCIM/TC57CIM/IEC61970/Base/Wires#NonlinearShuntCompensatorPoint_sectionNumber">
        <rdfs:domain rdf:resource="https://w3id.org/netbeheer/referentiemodellen/IECCIM/TC57CIM/IEC61970/Base/Wires#NonlinearShuntCompensatorPoint"/>
        <rdfs:range rdf:resource="http://www.w3.org/2001/XMLSchema#nonNegativeInteger"/>
        <rdfs:comment>The number of the section.</rdfs:comment>
    </owl:DatatypeProperty>
    


    <!-- https://w3id.org/netbeheer/referentiemodellen/IECCIM/TC57CIM/IEC61970/Base/Wires#PerLengthPhaseImpedance_conductorCount -->


    <owl:DatatypeProperty rdf:about="https://w3id.org/netbeheer/referentiemodellen/IECCIM/TC57CIM/IEC61970/Base/Wires#PerLengthPhaseImpedance_conductorCount">
        <rdfs:domain rdf:resource="https://w3id.org/netbeheer/referentiemodellen/IECCIM/TC57CIM/IEC61970/Base/Wires#PerLengthPhaseImpedance"/>
        <rdfs:range rdf:resource="http://www.w3.org/2001/XMLSchema#nonNegativeInteger"/>
        <rdfs:comment>Number of phase, neutral, and other wires retained. Constrains the number of matrix elements and the phase codes that can be used with this matrix.</rdfs:comment>
    </owl:DatatypeProperty>
    


    <!-- https://w3id.org/netbeheer/referentiemodellen/IECCIM/TC57CIM/IEC61970/Base/Wires#PetersenCoil_mode -->


    <owl:DatatypeProperty rdf:about="https://w3id.org/netbeheer/referentiemodellen/IECCIM/TC57CIM/IEC61970/Base/Wires#PetersenCoil_mode">
        <rdfs:domain rdf:resource="https://w3id.org/netbeheer/referentiemodellen/IECCIM/TC57CIM/IEC61970/Base/Wires#PetersenCoil"/>
        <rdfs:range rdf:resource="https://w3id.org/netbeheer/referentiemodellen/IECCIM/TC57CIM/IEC61970/Base/Wires#PetersenCoilModeKind"/>
        <rdfs:comment>The mode of operation of the Petersen coil.</rdfs:comment>
    </owl:DatatypeProperty>
    


    <!-- https://w3id.org/netbeheer/referentiemodellen/IECCIM/TC57CIM/IEC61970/Base/Wires#PhaseImpedanceData_sequenceNumber -->


    <owl:DatatypeProperty rdf:about="https://w3id.org/netbeheer/referentiemodellen/IECCIM/TC57CIM/IEC61970/Base/Wires#PhaseImpedanceData_sequenceNumber">
        <rdfs:domain rdf:resource="https://w3id.org/netbeheer/referentiemodellen/IECCIM/TC57CIM/IEC61970/Base/Wires#PhaseImpedanceData"/>
        <rdfs:range rdf:resource="http://www.w3.org/2001/XMLSchema#nonNegativeInteger"/>
        <rdfs:comment>Column-wise element index, assuming a symmetrical matrix. Ranges from 1 to N + N*(N-1)/2, where N is the number of phases possibly including neutral.    For instance, with N=4, column 1 = [1 2 3 4 ], column 2 = [- 5 6 7 ], column 3 = [- - 8 9], column 4 = [- - - 10].</rdfs:comment>
    </owl:DatatypeProperty>
    


    <!-- https://w3id.org/netbeheer/referentiemodellen/IECCIM/TC57CIM/IEC61970/Base/Wires#PowerTransformerEnd_connectionKind -->


    <owl:DatatypeProperty rdf:about="https://w3id.org/netbeheer/referentiemodellen/IECCIM/TC57CIM/IEC61970/Base/Wires#PowerTransformerEnd_connectionKind">
        <rdfs:domain rdf:resource="https://w3id.org/netbeheer/referentiemodellen/IECCIM/TC57CIM/IEC61970/Base/Wires#PowerTransformerEnd"/>
        <rdfs:range rdf:resource="https://w3id.org/netbeheer/referentiemodellen/IECCIM/TC57CIM/IEC61970/Base/Wires#WindingConnection"/>
        <rdfs:comment>Kind of connection.
</rdfs:comment>
    </owl:DatatypeProperty>
    


    <!-- https://w3id.org/netbeheer/referentiemodellen/IECCIM/TC57CIM/IEC61970/Base/Wires#PowerTransformerEnd_phaseAngleClock -->


    <owl:DatatypeProperty rdf:about="https://w3id.org/netbeheer/referentiemodellen/IECCIM/TC57CIM/IEC61970/Base/Wires#PowerTransformerEnd_phaseAngleClock">
        <rdfs:domain rdf:resource="https://w3id.org/netbeheer/referentiemodellen/IECCIM/TC57CIM/IEC61970/Base/Wires#PowerTransformerEnd"/>
        <rdfs:range rdf:resource="http://www.w3.org/2001/XMLSchema#nonNegativeInteger"/>
        <rdfs:comment>Terminal voltage phase angle displacement where 360 degrees are represented with clock hours. The valid values are 0 to 11. For example, for the secondary side end of a transformer with vector group code of &apos;Dyn11&apos;, specify the connection kind as wye with neutral and specify the phase angle of the clock as 11.  The clock value of the transformer end number specified as 1, is assumed to be zero.  Note the transformer end number is not assumed to be the same as the terminal sequence number.
</rdfs:comment>
    </owl:DatatypeProperty>
    


    <!-- https://w3id.org/netbeheer/referentiemodellen/IECCIM/TC57CIM/IEC61970/Base/Wires#PowerTransformer_isPartOfGeneratorUnit -->


    <owl:DatatypeProperty rdf:about="https://w3id.org/netbeheer/referentiemodellen/IECCIM/TC57CIM/IEC61970/Base/Wires#PowerTransformer_isPartOfGeneratorUnit">
        <rdfs:domain rdf:resource="https://w3id.org/netbeheer/referentiemodellen/IECCIM/TC57CIM/IEC61970/Base/Wires#PowerTransformer"/>
        <rdfs:range rdf:resource="http://www.w3.org/2001/XMLSchema#boolean"/>
        <rdfs:comment>Indicates whether the machine is part of a power station unit. Used for short circuit data exchange according to IEC 60909</rdfs:comment>
    </owl:DatatypeProperty>
    


    <!-- https://w3id.org/netbeheer/referentiemodellen/IECCIM/TC57CIM/IEC61970/Base/Wires#PowerTransformer_operationalValuesConsidered -->


    <owl:DatatypeProperty rdf:about="https://w3id.org/netbeheer/referentiemodellen/IECCIM/TC57CIM/IEC61970/Base/Wires#PowerTransformer_operationalValuesConsidered">
        <rdfs:domain rdf:resource="https://w3id.org/netbeheer/referentiemodellen/IECCIM/TC57CIM/IEC61970/Base/Wires#PowerTransformer"/>
        <rdfs:range rdf:resource="http://www.w3.org/2001/XMLSchema#boolean"/>
        <rdfs:comment>It is used to define if the data (other attributes related to short circuit data exchange) defines long term operational conditions or not. Used for short circuit data exchange according to IEC 60909.</rdfs:comment>
    </owl:DatatypeProperty>
    


    <!-- https://w3id.org/netbeheer/referentiemodellen/IECCIM/TC57CIM/IEC61970/Base/Wires#PowerTransformer_vectorGroup -->


    <owl:DatatypeProperty rdf:about="https://w3id.org/netbeheer/referentiemodellen/IECCIM/TC57CIM/IEC61970/Base/Wires#PowerTransformer_vectorGroup">
        <rdfs:domain rdf:resource="https://w3id.org/netbeheer/referentiemodellen/IECCIM/TC57CIM/IEC61970/Base/Wires#PowerTransformer"/>
        <rdfs:range rdf:resource="http://www.w3.org/2001/XMLSchema#string"/>
        <rdfs:comment>Vector group of the transformer for protective relaying, e.g., Dyn1. For unbalanced transformers, this may not be simply determined from the constituent winding connections and phase angle dispacements.

The vectorGroup string consists of the following components in the order listed: high voltage winding connection, mid voltage winding connection (for three winding transformers), phase displacement clock number from 0 to 11,  low voltage winding connection 
phase displacement clock number from 0 to 11.   The winding connections are D (delta), Y (wye), YN (wye with neutral), Z (zigzag), ZN (zigzag with neutral), A (auto transformer). Upper case means the high voltage, lower case mid or low. The high voltage winding always has clock postion 0 and is not included in the vector group string.  Some examples: YNy0 (two winding wye to wye with no phase displacement), YNd11 (two winding wye to delta with 330 degrees phase displacement), YNyn0d5 (three winding transformer wye with neutral high voltgage, wye with neutral mid voltgage and no phase displacement, delta low voltage with 150 degrees displacement).

Phase displacement is defined as the angular difference between the phasors representing the voltages between the neutral point (real or imaginary) and the corresponding terminals of two windings, a positive sequence voltage system being applied to the high-voltage terminals, following each other in alphabetical sequence if they are lettered, or in numerical sequence if they are numbered: the phasors are assumed to rotate in a counter-clockwise sense.
</rdfs:comment>
    </owl:DatatypeProperty>
    


    <!-- https://w3id.org/netbeheer/referentiemodellen/IECCIM/TC57CIM/IEC61970/Base/Wires#RatioTapChanger_tculControlMode -->


    <owl:DatatypeProperty rdf:about="https://w3id.org/netbeheer/referentiemodellen/IECCIM/TC57CIM/IEC61970/Base/Wires#RatioTapChanger_tculControlMode">
        <rdfs:domain rdf:resource="https://w3id.org/netbeheer/referentiemodellen/IECCIM/TC57CIM/IEC61970/Base/Wires#RatioTapChanger"/>
        <rdfs:range rdf:resource="https://w3id.org/netbeheer/referentiemodellen/IECCIM/TC57CIM/IEC61970/Base/Wires#TransformerControlMode"/>
        <rdfs:comment>Specifies the regulation control mode (voltage or reactive) of the RatioTapChanger.</rdfs:comment>
    </owl:DatatypeProperty>
    


    <!-- https://w3id.org/netbeheer/referentiemodellen/IECCIM/TC57CIM/IEC61970/Base/Wires#RegulatingCondEq_controlEnabled -->


    <owl:DatatypeProperty rdf:about="https://w3id.org/netbeheer/referentiemodellen/IECCIM/TC57CIM/IEC61970/Base/Wires#RegulatingCondEq_controlEnabled">
        <rdfs:domain rdf:resource="https://w3id.org/netbeheer/referentiemodellen/IECCIM/TC57CIM/IEC61970/Base/Wires#RegulatingCondEq"/>
        <rdfs:range rdf:resource="http://www.w3.org/2001/XMLSchema#boolean"/>
        <rdfs:comment>Specifies the regulation status of the equipment.  True is regulating, false is not regulating.</rdfs:comment>
    </owl:DatatypeProperty>
    


    <!-- https://w3id.org/netbeheer/referentiemodellen/IECCIM/TC57CIM/IEC61970/Base/Wires#RegulatingControl_discrete -->


    <owl:DatatypeProperty rdf:about="https://w3id.org/netbeheer/referentiemodellen/IECCIM/TC57CIM/IEC61970/Base/Wires#RegulatingControl_discrete">
        <rdfs:domain rdf:resource="https://w3id.org/netbeheer/referentiemodellen/IECCIM/TC57CIM/IEC61970/Base/Wires#RegulatingControl"/>
        <rdfs:range rdf:resource="http://www.w3.org/2001/XMLSchema#boolean"/>
        <rdfs:comment>The regulation is performed in a discrete mode. This applies to equipment with discrete controls, e.g. tap changers and shunt compensators.</rdfs:comment>
    </owl:DatatypeProperty>
    


    <!-- https://w3id.org/netbeheer/referentiemodellen/IECCIM/TC57CIM/IEC61970/Base/Wires#RegulatingControl_enabled -->


    <owl:DatatypeProperty rdf:about="https://w3id.org/netbeheer/referentiemodellen/IECCIM/TC57CIM/IEC61970/Base/Wires#RegulatingControl_enabled">
        <rdfs:domain rdf:resource="https://w3id.org/netbeheer/referentiemodellen/IECCIM/TC57CIM/IEC61970/Base/Wires#RegulatingControl"/>
        <rdfs:range rdf:resource="http://www.w3.org/2001/XMLSchema#boolean"/>
        <rdfs:comment>The flag tells if regulation is enabled.</rdfs:comment>
    </owl:DatatypeProperty>
    


    <!-- https://w3id.org/netbeheer/referentiemodellen/IECCIM/TC57CIM/IEC61970/Base/Wires#RegulatingControl_mode -->


    <owl:DatatypeProperty rdf:about="https://w3id.org/netbeheer/referentiemodellen/IECCIM/TC57CIM/IEC61970/Base/Wires#RegulatingControl_mode">
        <rdfs:domain rdf:resource="https://w3id.org/netbeheer/referentiemodellen/IECCIM/TC57CIM/IEC61970/Base/Wires#RegulatingControl"/>
        <rdfs:range rdf:resource="https://w3id.org/netbeheer/referentiemodellen/IECCIM/TC57CIM/IEC61970/Base/Wires#RegulatingControlModeKind"/>
        <rdfs:comment>The regulating control mode presently available.  This specification allows for determining the kind of regulation without need for obtaining the units from a schedule.</rdfs:comment>
    </owl:DatatypeProperty>
    


    <!-- https://w3id.org/netbeheer/referentiemodellen/IECCIM/TC57CIM/IEC61970/Base/Wires#RegulatingControl_monitoredPhase -->


    <owl:DatatypeProperty rdf:about="https://w3id.org/netbeheer/referentiemodellen/IECCIM/TC57CIM/IEC61970/Base/Wires#RegulatingControl_monitoredPhase">
        <rdfs:domain rdf:resource="https://w3id.org/netbeheer/referentiemodellen/IECCIM/TC57CIM/IEC61970/Base/Wires#RegulatingControl"/>
        <rdfs:range rdf:resource="https://w3id.org/netbeheer/referentiemodellen/IECCIM/TC57CIM/IEC61970/Base/Core#PhaseCode"/>
        <rdfs:comment>Phase voltage controlling this regulator, measured at regulator location.</rdfs:comment>
    </owl:DatatypeProperty>
    


    <!-- https://w3id.org/netbeheer/referentiemodellen/IECCIM/TC57CIM/IEC61970/Base/Wires#RegulatingControl_targetDeadband -->


    <owl:DatatypeProperty rdf:about="https://w3id.org/netbeheer/referentiemodellen/IECCIM/TC57CIM/IEC61970/Base/Wires#RegulatingControl_targetDeadband">
        <rdfs:domain rdf:resource="https://w3id.org/netbeheer/referentiemodellen/IECCIM/TC57CIM/IEC61970/Base/Wires#RegulatingControl"/>
        <rdfs:range rdf:resource="http://www.w3.org/2001/XMLSchema#float"/>
        <rdfs:comment>This is a deadband used with discrete control to avoid excessive update of controls like tap changers and shunt compensator banks while regulating.
The units of those appropriate for the mode.</rdfs:comment>
    </owl:DatatypeProperty>
    


    <!-- https://w3id.org/netbeheer/referentiemodellen/IECCIM/TC57CIM/IEC61970/Base/Wires#RegulatingControl_targetValue -->


    <owl:DatatypeProperty rdf:about="https://w3id.org/netbeheer/referentiemodellen/IECCIM/TC57CIM/IEC61970/Base/Wires#RegulatingControl_targetValue">
        <rdfs:domain rdf:resource="https://w3id.org/netbeheer/referentiemodellen/IECCIM/TC57CIM/IEC61970/Base/Wires#RegulatingControl"/>
        <rdfs:range rdf:resource="http://www.w3.org/2001/XMLSchema#float"/>
        <rdfs:comment>The target value specified for case input.   This value can be used for the target value without the use of schedules. The value has the units appropriate to the mode attribute.</rdfs:comment>
    </owl:DatatypeProperty>
    


    <!-- https://w3id.org/netbeheer/referentiemodellen/IECCIM/TC57CIM/IEC61970/Base/Wires#RegulatingControl_targetValueUnitMultiplier -->


    <owl:DatatypeProperty rdf:about="https://w3id.org/netbeheer/referentiemodellen/IECCIM/TC57CIM/IEC61970/Base/Wires#RegulatingControl_targetValueUnitMultiplier">
        <rdfs:domain rdf:resource="https://w3id.org/netbeheer/referentiemodellen/IECCIM/TC57CIM/IEC61970/Base/Wires#RegulatingControl"/>
        <rdfs:range rdf:resource="https://w3id.org/netbeheer/referentiemodellen/IECCIM/TC57CIM/IEC61970/Base/Domain#UnitMultiplier"/>
        <rdfs:comment>Specify the multiplier for used for the targetValue.</rdfs:comment>
    </owl:DatatypeProperty>
    


    <!-- https://w3id.org/netbeheer/referentiemodellen/IECCIM/TC57CIM/IEC61970/Base/Wires#RotatingMachine_ratedPowerFactor -->


    <owl:DatatypeProperty rdf:about="https://w3id.org/netbeheer/referentiemodellen/IECCIM/TC57CIM/IEC61970/Base/Wires#RotatingMachine_ratedPowerFactor">
        <rdfs:domain rdf:resource="https://w3id.org/netbeheer/referentiemodellen/IECCIM/TC57CIM/IEC61970/Base/Wires#RotatingMachine"/>
        <rdfs:range rdf:resource="http://www.w3.org/2001/XMLSchema#float"/>
        <rdfs:comment>Power factor (nameplate data). It is primarily used for short circuit data exchange according to IEC 60909.</rdfs:comment>
    </owl:DatatypeProperty>
    


    <!-- https://w3id.org/netbeheer/referentiemodellen/IECCIM/TC57CIM/IEC61970/Base/Wires#SeriesCompensator_varistorPresent -->


    <owl:DatatypeProperty rdf:about="https://w3id.org/netbeheer/referentiemodellen/IECCIM/TC57CIM/IEC61970/Base/Wires#SeriesCompensator_varistorPresent">
        <rdfs:domain rdf:resource="https://w3id.org/netbeheer/referentiemodellen/IECCIM/TC57CIM/IEC61970/Base/Wires#SeriesCompensator"/>
        <rdfs:range rdf:resource="http://www.w3.org/2001/XMLSchema#boolean"/>
        <rdfs:comment>Describe if a metal oxide varistor (mov) for over voltage protection is configured at the series compensator.</rdfs:comment>
    </owl:DatatypeProperty>
    


    <!-- https://w3id.org/netbeheer/referentiemodellen/IECCIM/TC57CIM/IEC61970/Base/Wires#ShuntCompensatorPhase_maximumSections -->


    <owl:DatatypeProperty rdf:about="https://w3id.org/netbeheer/referentiemodellen/IECCIM/TC57CIM/IEC61970/Base/Wires#ShuntCompensatorPhase_maximumSections">
        <rdfs:domain rdf:resource="https://w3id.org/netbeheer/referentiemodellen/IECCIM/TC57CIM/IEC61970/Base/Wires#ShuntCompensatorPhase"/>
        <rdfs:range rdf:resource="http://www.w3.org/2001/XMLSchema#nonNegativeInteger"/>
        <rdfs:comment>The maximum number of sections that may be switched in for this phase. 
</rdfs:comment>
    </owl:DatatypeProperty>
    


    <!-- https://w3id.org/netbeheer/referentiemodellen/IECCIM/TC57CIM/IEC61970/Base/Wires#ShuntCompensatorPhase_normalSections -->


    <owl:DatatypeProperty rdf:about="https://w3id.org/netbeheer/referentiemodellen/IECCIM/TC57CIM/IEC61970/Base/Wires#ShuntCompensatorPhase_normalSections">
        <rdfs:domain rdf:resource="https://w3id.org/netbeheer/referentiemodellen/IECCIM/TC57CIM/IEC61970/Base/Wires#ShuntCompensatorPhase"/>
        <rdfs:range rdf:resource="http://www.w3.org/2001/XMLSchema#nonNegativeInteger"/>
        <rdfs:comment>For the capacitor phase, the normal number of sections switched in.
</rdfs:comment>
    </owl:DatatypeProperty>
    


    <!-- https://w3id.org/netbeheer/referentiemodellen/IECCIM/TC57CIM/IEC61970/Base/Wires#ShuntCompensatorPhase_phase -->


    <owl:DatatypeProperty rdf:about="https://w3id.org/netbeheer/referentiemodellen/IECCIM/TC57CIM/IEC61970/Base/Wires#ShuntCompensatorPhase_phase">
        <rdfs:domain rdf:resource="https://w3id.org/netbeheer/referentiemodellen/IECCIM/TC57CIM/IEC61970/Base/Wires#ShuntCompensatorPhase"/>
        <rdfs:range rdf:resource="https://w3id.org/netbeheer/referentiemodellen/IECCIM/TC57CIM/IEC61970/Base/Wires#SinglePhaseKind"/>
        <rdfs:comment>Phase of this shunt compensator component.   If the shunt compensator is wye connected, the connection is from the indicated phase to the central ground or neutral point.  If the shunt compensator is delta connected, the phase indicates a shunt compensator connected from the indicated phase to the next logical non-neutral phase.
</rdfs:comment>
    </owl:DatatypeProperty>
    


    <!-- https://w3id.org/netbeheer/referentiemodellen/IECCIM/TC57CIM/IEC61970/Base/Wires#ShuntCompensator_grounded -->


    <owl:DatatypeProperty rdf:about="https://w3id.org/netbeheer/referentiemodellen/IECCIM/TC57CIM/IEC61970/Base/Wires#ShuntCompensator_grounded">
        <rdfs:domain rdf:resource="https://w3id.org/netbeheer/referentiemodellen/IECCIM/TC57CIM/IEC61970/Base/Wires#ShuntCompensator"/>
        <rdfs:range rdf:resource="http://www.w3.org/2001/XMLSchema#boolean"/>
        <rdfs:comment>Used for Yn and Zn connections. True if the neutral is solidly grounded.</rdfs:comment>
    </owl:DatatypeProperty>
    


    <!-- https://w3id.org/netbeheer/referentiemodellen/IECCIM/TC57CIM/IEC61970/Base/Wires#ShuntCompensator_maximumSections -->


    <owl:DatatypeProperty rdf:about="https://w3id.org/netbeheer/referentiemodellen/IECCIM/TC57CIM/IEC61970/Base/Wires#ShuntCompensator_maximumSections">
        <rdfs:domain rdf:resource="https://w3id.org/netbeheer/referentiemodellen/IECCIM/TC57CIM/IEC61970/Base/Wires#ShuntCompensator"/>
        <rdfs:range rdf:resource="http://www.w3.org/2001/XMLSchema#nonNegativeInteger"/>
        <rdfs:comment>The maximum number of sections that may be switched in. 
</rdfs:comment>
    </owl:DatatypeProperty>
    


    <!-- https://w3id.org/netbeheer/referentiemodellen/IECCIM/TC57CIM/IEC61970/Base/Wires#ShuntCompensator_normalSections -->


    <owl:DatatypeProperty rdf:about="https://w3id.org/netbeheer/referentiemodellen/IECCIM/TC57CIM/IEC61970/Base/Wires#ShuntCompensator_normalSections">
        <rdfs:domain rdf:resource="https://w3id.org/netbeheer/referentiemodellen/IECCIM/TC57CIM/IEC61970/Base/Wires#ShuntCompensator"/>
        <rdfs:range rdf:resource="http://www.w3.org/2001/XMLSchema#nonNegativeInteger"/>
        <rdfs:comment>The normal number of sections switched in.
</rdfs:comment>
    </owl:DatatypeProperty>
    


    <!-- https://w3id.org/netbeheer/referentiemodellen/IECCIM/TC57CIM/IEC61970/Base/Wires#ShuntCompensator_phaseConnection -->


    <owl:DatatypeProperty rdf:about="https://w3id.org/netbeheer/referentiemodellen/IECCIM/TC57CIM/IEC61970/Base/Wires#ShuntCompensator_phaseConnection">
        <rdfs:domain rdf:resource="https://w3id.org/netbeheer/referentiemodellen/IECCIM/TC57CIM/IEC61970/Base/Wires#ShuntCompensator"/>
        <rdfs:range rdf:resource="https://w3id.org/netbeheer/referentiemodellen/IECCIM/TC57CIM/IEC61970/Base/Wires#PhaseShuntConnectionKind"/>
        <rdfs:comment>The type of phase connection, such as wye or delta.
</rdfs:comment>
    </owl:DatatypeProperty>
    


    <!-- https://w3id.org/netbeheer/referentiemodellen/IECCIM/TC57CIM/IEC61970/Base/Wires#ShuntCompensator_sections -->


    <owl:DatatypeProperty rdf:about="https://w3id.org/netbeheer/referentiemodellen/IECCIM/TC57CIM/IEC61970/Base/Wires#ShuntCompensator_sections">
        <rdfs:domain rdf:resource="https://w3id.org/netbeheer/referentiemodellen/IECCIM/TC57CIM/IEC61970/Base/Wires#ShuntCompensator"/>
        <rdfs:range rdf:resource="http://www.w3.org/2001/XMLSchema#float"/>
        <rdfs:comment>Shunt compensator sections in use.
Starting value for steady state solution. Non integer values are allowed to support continuous variables. The reasons for continuous value are to support study cases where no discrete shunt compensators has yet been designed, a solutions where a narrow voltage band force the sections to oscillate or accommodate for a continuous solution as input.</rdfs:comment>
    </owl:DatatypeProperty>
    


    <!-- https://w3id.org/netbeheer/referentiemodellen/IECCIM/TC57CIM/IEC61970/Base/Wires#ShuntCompensator_switchOnCount -->


    <owl:DatatypeProperty rdf:about="https://w3id.org/netbeheer/referentiemodellen/IECCIM/TC57CIM/IEC61970/Base/Wires#ShuntCompensator_switchOnCount">
        <rdfs:domain rdf:resource="https://w3id.org/netbeheer/referentiemodellen/IECCIM/TC57CIM/IEC61970/Base/Wires#ShuntCompensator"/>
        <rdfs:range rdf:resource="http://www.w3.org/2001/XMLSchema#nonNegativeInteger"/>
        <rdfs:comment>The switch on count since the capacitor count was last reset or initialized.</rdfs:comment>
    </owl:DatatypeProperty>
    


    <!-- https://w3id.org/netbeheer/referentiemodellen/IECCIM/TC57CIM/IEC61970/Base/Wires#ShuntCompensator_switchOnDate -->


    <owl:DatatypeProperty rdf:about="https://w3id.org/netbeheer/referentiemodellen/IECCIM/TC57CIM/IEC61970/Base/Wires#ShuntCompensator_switchOnDate">
        <rdfs:domain rdf:resource="https://w3id.org/netbeheer/referentiemodellen/IECCIM/TC57CIM/IEC61970/Base/Wires#ShuntCompensator"/>
        <rdfs:range rdf:resource="http://www.w3.org/2001/XMLSchema#dateTime"/>
        <rdfs:comment>The date and time when the capacitor bank was last switched on.</rdfs:comment>
    </owl:DatatypeProperty>
    


    <!-- https://w3id.org/netbeheer/referentiemodellen/IECCIM/TC57CIM/IEC61970/Base/Wires#StaticVarCompensator_sVCControlMode -->


    <owl:DatatypeProperty rdf:about="https://w3id.org/netbeheer/referentiemodellen/IECCIM/TC57CIM/IEC61970/Base/Wires#StaticVarCompensator_sVCControlMode">
        <rdfs:domain rdf:resource="https://w3id.org/netbeheer/referentiemodellen/IECCIM/TC57CIM/IEC61970/Base/Wires#StaticVarCompensator"/>
        <rdfs:range rdf:resource="https://w3id.org/netbeheer/referentiemodellen/IECCIM/TC57CIM/IEC61970/Base/Wires#SVCControlMode"/>
        <rdfs:comment>SVC control mode.</rdfs:comment>
    </owl:DatatypeProperty>
    


    <!-- https://w3id.org/netbeheer/referentiemodellen/IECCIM/TC57CIM/IEC61970/Base/Wires#SwitchPhase_closed -->


    <owl:DatatypeProperty rdf:about="https://w3id.org/netbeheer/referentiemodellen/IECCIM/TC57CIM/IEC61970/Base/Wires#SwitchPhase_closed">
        <rdfs:domain rdf:resource="https://w3id.org/netbeheer/referentiemodellen/IECCIM/TC57CIM/IEC61970/Base/Wires#SwitchPhase"/>
        <rdfs:range rdf:resource="http://www.w3.org/2001/XMLSchema#boolean"/>
        <rdfs:comment>The attribute tells if the switch is considered closed when used as input to topology processing.</rdfs:comment>
    </owl:DatatypeProperty>
    


    <!-- https://w3id.org/netbeheer/referentiemodellen/IECCIM/TC57CIM/IEC61970/Base/Wires#SwitchPhase_normalOpen -->


    <owl:DatatypeProperty rdf:about="https://w3id.org/netbeheer/referentiemodellen/IECCIM/TC57CIM/IEC61970/Base/Wires#SwitchPhase_normalOpen">
        <rdfs:domain rdf:resource="https://w3id.org/netbeheer/referentiemodellen/IECCIM/TC57CIM/IEC61970/Base/Wires#SwitchPhase"/>
        <rdfs:range rdf:resource="http://www.w3.org/2001/XMLSchema#boolean"/>
        <rdfs:comment>Used in cases when no Measurement for the status value is present. If the SwitchPhase has a status measurement the Discrete.normalValue is expected to match with this value.
</rdfs:comment>
    </owl:DatatypeProperty>
    


    <!-- https://w3id.org/netbeheer/referentiemodellen/IECCIM/TC57CIM/IEC61970/Base/Wires#SwitchPhase_phaseSide1 -->


    <owl:DatatypeProperty rdf:about="https://w3id.org/netbeheer/referentiemodellen/IECCIM/TC57CIM/IEC61970/Base/Wires#SwitchPhase_phaseSide1">
        <rdfs:domain rdf:resource="https://w3id.org/netbeheer/referentiemodellen/IECCIM/TC57CIM/IEC61970/Base/Wires#SwitchPhase"/>
        <rdfs:range rdf:resource="https://w3id.org/netbeheer/referentiemodellen/IECCIM/TC57CIM/IEC61970/Base/Wires#SinglePhaseKind"/>
        <rdfs:comment>Phase of this SwitchPhase on the side with terminal sequence number equal 1. Should be a phase contained in that terminal&amp;rsquo;s phases attribute.
</rdfs:comment>
    </owl:DatatypeProperty>
    


    <!-- https://w3id.org/netbeheer/referentiemodellen/IECCIM/TC57CIM/IEC61970/Base/Wires#SwitchPhase_phaseSide2 -->


    <owl:DatatypeProperty rdf:about="https://w3id.org/netbeheer/referentiemodellen/IECCIM/TC57CIM/IEC61970/Base/Wires#SwitchPhase_phaseSide2">
        <rdfs:domain rdf:resource="https://w3id.org/netbeheer/referentiemodellen/IECCIM/TC57CIM/IEC61970/Base/Wires#SwitchPhase"/>
        <rdfs:range rdf:resource="https://w3id.org/netbeheer/referentiemodellen/IECCIM/TC57CIM/IEC61970/Base/Wires#SinglePhaseKind"/>
        <rdfs:comment>Phase of this SwitchPhase on the side with terminal sequence number equal 2.  Should be a phase contained in that terminal&amp;rsquo;s Terminal.phases attribute.
</rdfs:comment>
    </owl:DatatypeProperty>
    


    <!-- https://w3id.org/netbeheer/referentiemodellen/IECCIM/TC57CIM/IEC61970/Base/Wires#Switch_normalOpen -->


    <owl:DatatypeProperty rdf:about="https://w3id.org/netbeheer/referentiemodellen/IECCIM/TC57CIM/IEC61970/Base/Wires#Switch_normalOpen">
        <rdfs:domain rdf:resource="https://w3id.org/netbeheer/referentiemodellen/IECCIM/TC57CIM/IEC61970/Base/Wires#Switch"/>
        <rdfs:range rdf:resource="http://www.w3.org/2001/XMLSchema#boolean"/>
        <rdfs:comment>The attribute is used in cases when no Measurement for the status value is present. If the Switch has a status measurement the Discrete.normalValue is expected to match with the Switch.normalOpen.</rdfs:comment>
    </owl:DatatypeProperty>
    


    <!-- https://w3id.org/netbeheer/referentiemodellen/IECCIM/TC57CIM/IEC61970/Base/Wires#Switch_open -->


    <owl:DatatypeProperty rdf:about="https://w3id.org/netbeheer/referentiemodellen/IECCIM/TC57CIM/IEC61970/Base/Wires#Switch_open">
        <rdfs:domain rdf:resource="https://w3id.org/netbeheer/referentiemodellen/IECCIM/TC57CIM/IEC61970/Base/Wires#Switch"/>
        <rdfs:range rdf:resource="http://www.w3.org/2001/XMLSchema#boolean"/>
        <rdfs:comment>The attribute tells if the switch is considered open when used as input to topology processing.</rdfs:comment>
    </owl:DatatypeProperty>
    


    <!-- https://w3id.org/netbeheer/referentiemodellen/IECCIM/TC57CIM/IEC61970/Base/Wires#Switch_retained -->


    <owl:DatatypeProperty rdf:about="https://w3id.org/netbeheer/referentiemodellen/IECCIM/TC57CIM/IEC61970/Base/Wires#Switch_retained">
        <rdfs:domain rdf:resource="https://w3id.org/netbeheer/referentiemodellen/IECCIM/TC57CIM/IEC61970/Base/Wires#Switch"/>
        <rdfs:range rdf:resource="http://www.w3.org/2001/XMLSchema#boolean"/>
        <rdfs:comment>Branch is retained in a bus branch model.  The flow through retained switches will normally be calculated in power flow.</rdfs:comment>
    </owl:DatatypeProperty>
    


    <!-- https://w3id.org/netbeheer/referentiemodellen/IECCIM/TC57CIM/IEC61970/Base/Wires#Switch_switchOnCount -->


    <owl:DatatypeProperty rdf:about="https://w3id.org/netbeheer/referentiemodellen/IECCIM/TC57CIM/IEC61970/Base/Wires#Switch_switchOnCount">
        <rdfs:domain rdf:resource="https://w3id.org/netbeheer/referentiemodellen/IECCIM/TC57CIM/IEC61970/Base/Wires#Switch"/>
        <rdfs:range rdf:resource="http://www.w3.org/2001/XMLSchema#nonNegativeInteger"/>
        <rdfs:comment>The switch on count since the switch was last reset or initialized.</rdfs:comment>
    </owl:DatatypeProperty>
    


    <!-- https://w3id.org/netbeheer/referentiemodellen/IECCIM/TC57CIM/IEC61970/Base/Wires#Switch_switchOnDate -->


    <owl:DatatypeProperty rdf:about="https://w3id.org/netbeheer/referentiemodellen/IECCIM/TC57CIM/IEC61970/Base/Wires#Switch_switchOnDate">
        <rdfs:domain rdf:resource="https://w3id.org/netbeheer/referentiemodellen/IECCIM/TC57CIM/IEC61970/Base/Wires#Switch"/>
        <rdfs:range rdf:resource="http://www.w3.org/2001/XMLSchema#dateTime"/>
        <rdfs:comment>The date and time when the switch was last switched on.</rdfs:comment>
    </owl:DatatypeProperty>
    


    <!-- https://w3id.org/netbeheer/referentiemodellen/IECCIM/TC57CIM/IEC61970/Base/Wires#SynchronousMachine_coolantCondition -->


    <owl:DatatypeProperty rdf:about="https://w3id.org/netbeheer/referentiemodellen/IECCIM/TC57CIM/IEC61970/Base/Wires#SynchronousMachine_coolantCondition">
        <rdfs:domain rdf:resource="https://w3id.org/netbeheer/referentiemodellen/IECCIM/TC57CIM/IEC61970/Base/Wires#SynchronousMachine"/>
        <rdfs:range rdf:resource="http://www.w3.org/2001/XMLSchema#float"/>
        <rdfs:comment>Temperature or pressure of coolant medium</rdfs:comment>
    </owl:DatatypeProperty>
    


    <!-- https://w3id.org/netbeheer/referentiemodellen/IECCIM/TC57CIM/IEC61970/Base/Wires#SynchronousMachine_coolantType -->


    <owl:DatatypeProperty rdf:about="https://w3id.org/netbeheer/referentiemodellen/IECCIM/TC57CIM/IEC61970/Base/Wires#SynchronousMachine_coolantType">
        <rdfs:domain rdf:resource="https://w3id.org/netbeheer/referentiemodellen/IECCIM/TC57CIM/IEC61970/Base/Wires#SynchronousMachine"/>
        <rdfs:range rdf:resource="https://w3id.org/netbeheer/referentiemodellen/IECCIM/TC57CIM/IEC61970/Base/Wires#CoolantType"/>
        <rdfs:comment>Method of cooling the machine.</rdfs:comment>
    </owl:DatatypeProperty>
    


    <!-- https://w3id.org/netbeheer/referentiemodellen/IECCIM/TC57CIM/IEC61970/Base/Wires#SynchronousMachine_earthing -->


    <owl:DatatypeProperty rdf:about="https://w3id.org/netbeheer/referentiemodellen/IECCIM/TC57CIM/IEC61970/Base/Wires#SynchronousMachine_earthing">
        <rdfs:domain rdf:resource="https://w3id.org/netbeheer/referentiemodellen/IECCIM/TC57CIM/IEC61970/Base/Wires#SynchronousMachine"/>
        <rdfs:range rdf:resource="http://www.w3.org/2001/XMLSchema#boolean"/>
        <rdfs:comment>Indicates whether or not the generator is earthed. Used for short circuit data exchange according to IEC 60909</rdfs:comment>
    </owl:DatatypeProperty>
    


    <!-- https://w3id.org/netbeheer/referentiemodellen/IECCIM/TC57CIM/IEC61970/Base/Wires#SynchronousMachine_mu -->


    <owl:DatatypeProperty rdf:about="https://w3id.org/netbeheer/referentiemodellen/IECCIM/TC57CIM/IEC61970/Base/Wires#SynchronousMachine_mu">
        <rdfs:domain rdf:resource="https://w3id.org/netbeheer/referentiemodellen/IECCIM/TC57CIM/IEC61970/Base/Wires#SynchronousMachine"/>
        <rdfs:range rdf:resource="http://www.w3.org/2001/XMLSchema#float"/>
        <rdfs:comment>Factor to calculate the breaking current (Section 4.5.2.1 in the IEC 60909-0).
Used only for single fed short circuit on a generator (Section 4.3.4.2. in the IEC 60909-0).</rdfs:comment>
    </owl:DatatypeProperty>
    


    <!-- https://w3id.org/netbeheer/referentiemodellen/IECCIM/TC57CIM/IEC61970/Base/Wires#SynchronousMachine_operatingMode -->


    <owl:DatatypeProperty rdf:about="https://w3id.org/netbeheer/referentiemodellen/IECCIM/TC57CIM/IEC61970/Base/Wires#SynchronousMachine_operatingMode">
        <rdfs:domain rdf:resource="https://w3id.org/netbeheer/referentiemodellen/IECCIM/TC57CIM/IEC61970/Base/Wires#SynchronousMachine"/>
        <rdfs:range rdf:resource="https://w3id.org/netbeheer/referentiemodellen/IECCIM/TC57CIM/IEC61970/Base/Wires#SynchronousMachineOperatingMode"/>
        <rdfs:comment>Current mode of operation.</rdfs:comment>
    </owl:DatatypeProperty>
    


    <!-- https://w3id.org/netbeheer/referentiemodellen/IECCIM/TC57CIM/IEC61970/Base/Wires#SynchronousMachine_referencePriority -->


    <owl:DatatypeProperty rdf:about="https://w3id.org/netbeheer/referentiemodellen/IECCIM/TC57CIM/IEC61970/Base/Wires#SynchronousMachine_referencePriority">
        <rdfs:domain rdf:resource="https://w3id.org/netbeheer/referentiemodellen/IECCIM/TC57CIM/IEC61970/Base/Wires#SynchronousMachine"/>
        <rdfs:range rdf:resource="http://www.w3.org/2001/XMLSchema#nonNegativeInteger"/>
        <rdfs:comment>Priority of unit for use as powerflow voltage phase angle reference bus selection. 0 = don t care (default) 1 = highest priority. 2 is less than 1 and so on.
</rdfs:comment>
    </owl:DatatypeProperty>
    


    <!-- https://w3id.org/netbeheer/referentiemodellen/IECCIM/TC57CIM/IEC61970/Base/Wires#SynchronousMachine_shortCircuitRotorType -->


    <owl:DatatypeProperty rdf:about="https://w3id.org/netbeheer/referentiemodellen/IECCIM/TC57CIM/IEC61970/Base/Wires#SynchronousMachine_shortCircuitRotorType">
        <rdfs:domain rdf:resource="https://w3id.org/netbeheer/referentiemodellen/IECCIM/TC57CIM/IEC61970/Base/Wires#SynchronousMachine"/>
        <rdfs:range rdf:resource="https://w3id.org/netbeheer/referentiemodellen/IECCIM/TC57CIM/IEC61970/Base/Wires#ShortCircuitRotorKind"/>
        <rdfs:comment>Type of rotor, used by short circuit applications, only for single fed short circuit according to IEC 60909.</rdfs:comment>
    </owl:DatatypeProperty>
    


    <!-- https://w3id.org/netbeheer/referentiemodellen/IECCIM/TC57CIM/IEC61970/Base/Wires#SynchronousMachine_type -->


    <owl:DatatypeProperty rdf:about="https://w3id.org/netbeheer/referentiemodellen/IECCIM/TC57CIM/IEC61970/Base/Wires#SynchronousMachine_type">
        <rdfs:domain rdf:resource="https://w3id.org/netbeheer/referentiemodellen/IECCIM/TC57CIM/IEC61970/Base/Wires#SynchronousMachine"/>
        <rdfs:range rdf:resource="https://w3id.org/netbeheer/referentiemodellen/IECCIM/TC57CIM/IEC61970/Base/Wires#SynchronousMachineKind"/>
        <rdfs:comment>Modes that this synchronous machine can operate in.</rdfs:comment>
    </owl:DatatypeProperty>
    


    <!-- https://w3id.org/netbeheer/referentiemodellen/IECCIM/TC57CIM/IEC61970/Base/Wires#TapChangerControl_lineDropCompensation -->


    <owl:DatatypeProperty rdf:about="https://w3id.org/netbeheer/referentiemodellen/IECCIM/TC57CIM/IEC61970/Base/Wires#TapChangerControl_lineDropCompensation">
        <rdfs:domain rdf:resource="https://w3id.org/netbeheer/referentiemodellen/IECCIM/TC57CIM/IEC61970/Base/Wires#TapChangerControl"/>
        <rdfs:range rdf:resource="http://www.w3.org/2001/XMLSchema#boolean"/>
        <rdfs:comment>If true, the line drop compensation is to be applied.</rdfs:comment>
    </owl:DatatypeProperty>
    


    <!-- https://w3id.org/netbeheer/referentiemodellen/IECCIM/TC57CIM/IEC61970/Base/Wires#TapChangerTablePoint_ratio -->


    <owl:DatatypeProperty rdf:about="https://w3id.org/netbeheer/referentiemodellen/IECCIM/TC57CIM/IEC61970/Base/Wires#TapChangerTablePoint_ratio">
        <rdfs:domain rdf:resource="https://w3id.org/netbeheer/referentiemodellen/IECCIM/TC57CIM/IEC61970/Base/Wires#TapChangerTablePoint"/>
        <rdfs:range rdf:resource="http://www.w3.org/2001/XMLSchema#float"/>
        <rdfs:comment>The voltage ratio in per unit. Hence this is a value close to one.
</rdfs:comment>
    </owl:DatatypeProperty>
    


    <!-- https://w3id.org/netbeheer/referentiemodellen/IECCIM/TC57CIM/IEC61970/Base/Wires#TapChangerTablePoint_step -->


    <owl:DatatypeProperty rdf:about="https://w3id.org/netbeheer/referentiemodellen/IECCIM/TC57CIM/IEC61970/Base/Wires#TapChangerTablePoint_step">
        <rdfs:domain rdf:resource="https://w3id.org/netbeheer/referentiemodellen/IECCIM/TC57CIM/IEC61970/Base/Wires#TapChangerTablePoint"/>
        <rdfs:range rdf:resource="http://www.w3.org/2001/XMLSchema#nonNegativeInteger"/>
        <rdfs:comment>The tap step.
</rdfs:comment>
    </owl:DatatypeProperty>
    


    <!-- https://w3id.org/netbeheer/referentiemodellen/IECCIM/TC57CIM/IEC61970/Base/Wires#TapChanger_controlEnabled -->


    <owl:DatatypeProperty rdf:about="https://w3id.org/netbeheer/referentiemodellen/IECCIM/TC57CIM/IEC61970/Base/Wires#TapChanger_controlEnabled">
        <rdfs:domain rdf:resource="https://w3id.org/netbeheer/referentiemodellen/IECCIM/TC57CIM/IEC61970/Base/Wires#TapChanger"/>
        <rdfs:range rdf:resource="http://www.w3.org/2001/XMLSchema#boolean"/>
        <rdfs:comment>Specifies the regulation status of the equipment.  True is regulating, false is not regulating.</rdfs:comment>
    </owl:DatatypeProperty>
    


    <!-- https://w3id.org/netbeheer/referentiemodellen/IECCIM/TC57CIM/IEC61970/Base/Wires#TapChanger_highStep -->


    <owl:DatatypeProperty rdf:about="https://w3id.org/netbeheer/referentiemodellen/IECCIM/TC57CIM/IEC61970/Base/Wires#TapChanger_highStep">
        <rdfs:domain rdf:resource="https://w3id.org/netbeheer/referentiemodellen/IECCIM/TC57CIM/IEC61970/Base/Wires#TapChanger"/>
        <rdfs:range rdf:resource="http://www.w3.org/2001/XMLSchema#nonNegativeInteger"/>
        <rdfs:comment>Highest possible tap step position, advance from neutral.
The attribute shall be greater than lowStep.</rdfs:comment>
    </owl:DatatypeProperty>
    


    <!-- https://w3id.org/netbeheer/referentiemodellen/IECCIM/TC57CIM/IEC61970/Base/Wires#TapChanger_lowStep -->


    <owl:DatatypeProperty rdf:about="https://w3id.org/netbeheer/referentiemodellen/IECCIM/TC57CIM/IEC61970/Base/Wires#TapChanger_lowStep">
        <rdfs:domain rdf:resource="https://w3id.org/netbeheer/referentiemodellen/IECCIM/TC57CIM/IEC61970/Base/Wires#TapChanger"/>
        <rdfs:range rdf:resource="http://www.w3.org/2001/XMLSchema#nonNegativeInteger"/>
        <rdfs:comment>Lowest possible tap step position, retard from neutral</rdfs:comment>
    </owl:DatatypeProperty>
    


    <!-- https://w3id.org/netbeheer/referentiemodellen/IECCIM/TC57CIM/IEC61970/Base/Wires#TapChanger_ltcFlag -->


    <owl:DatatypeProperty rdf:about="https://w3id.org/netbeheer/referentiemodellen/IECCIM/TC57CIM/IEC61970/Base/Wires#TapChanger_ltcFlag">
        <rdfs:domain rdf:resource="https://w3id.org/netbeheer/referentiemodellen/IECCIM/TC57CIM/IEC61970/Base/Wires#TapChanger"/>
        <rdfs:range rdf:resource="http://www.w3.org/2001/XMLSchema#boolean"/>
        <rdfs:comment>Specifies whether or not a TapChanger has load tap changing capabilities.</rdfs:comment>
    </owl:DatatypeProperty>
    


    <!-- https://w3id.org/netbeheer/referentiemodellen/IECCIM/TC57CIM/IEC61970/Base/Wires#TapChanger_neutralStep -->


    <owl:DatatypeProperty rdf:about="https://w3id.org/netbeheer/referentiemodellen/IECCIM/TC57CIM/IEC61970/Base/Wires#TapChanger_neutralStep">
        <rdfs:domain rdf:resource="https://w3id.org/netbeheer/referentiemodellen/IECCIM/TC57CIM/IEC61970/Base/Wires#TapChanger"/>
        <rdfs:range rdf:resource="http://www.w3.org/2001/XMLSchema#nonNegativeInteger"/>
        <rdfs:comment>The neutral tap step position for this winding.
The attribute shall be equal or greater than lowStep and equal or less than highStep.</rdfs:comment>
    </owl:DatatypeProperty>
    


    <!-- https://w3id.org/netbeheer/referentiemodellen/IECCIM/TC57CIM/IEC61970/Base/Wires#TapChanger_normalStep -->


    <owl:DatatypeProperty rdf:about="https://w3id.org/netbeheer/referentiemodellen/IECCIM/TC57CIM/IEC61970/Base/Wires#TapChanger_normalStep">
        <rdfs:domain rdf:resource="https://w3id.org/netbeheer/referentiemodellen/IECCIM/TC57CIM/IEC61970/Base/Wires#TapChanger"/>
        <rdfs:range rdf:resource="http://www.w3.org/2001/XMLSchema#nonNegativeInteger"/>
        <rdfs:comment>The tap step position used in &quot;normal&quot; network operation for this winding. For a &quot;Fixed&quot; tap changer indicates the current physical tap setting.
The attribute shall be equal or greater than lowStep and equal or less than highStep.</rdfs:comment>
    </owl:DatatypeProperty>
    


    <!-- https://w3id.org/netbeheer/referentiemodellen/IECCIM/TC57CIM/IEC61970/Base/Wires#TapChanger_step -->


    <owl:DatatypeProperty rdf:about="https://w3id.org/netbeheer/referentiemodellen/IECCIM/TC57CIM/IEC61970/Base/Wires#TapChanger_step">
        <rdfs:domain rdf:resource="https://w3id.org/netbeheer/referentiemodellen/IECCIM/TC57CIM/IEC61970/Base/Wires#TapChanger"/>
        <rdfs:range rdf:resource="http://www.w3.org/2001/XMLSchema#float"/>
        <rdfs:comment>Tap changer position.
Starting step for a steady state solution. Non integer values are allowed to support continuous tap variables. The reasons for continuous value are to support study cases where no discrete tap changers has yet been designed, a solutions where a narrow voltage band force the tap step to oscillate or accommodate for a continuous solution as input.
The attribute shall be equal or greater than lowStep and equal or less than highStep.</rdfs:comment>
    </owl:DatatypeProperty>
    


    <!-- https://w3id.org/netbeheer/referentiemodellen/IECCIM/TC57CIM/IEC61970/Base/Wires#TransformerEnd_endNumber -->


    <owl:DatatypeProperty rdf:about="https://w3id.org/netbeheer/referentiemodellen/IECCIM/TC57CIM/IEC61970/Base/Wires#TransformerEnd_endNumber">
        <rdfs:domain rdf:resource="https://w3id.org/netbeheer/referentiemodellen/IECCIM/TC57CIM/IEC61970/Base/Wires#TransformerEnd"/>
        <rdfs:range rdf:resource="http://www.w3.org/2001/XMLSchema#nonNegativeInteger"/>
        <rdfs:comment>Number for this transformer end, corresponding to the end&apos;s order in the power transformer vector group or phase angle clock number.  Highest voltage winding should be 1.  Each end within a power transformer should have a unique subsequent end number.   Note the transformer end number need not match the terminal sequence number.
</rdfs:comment>
    </owl:DatatypeProperty>
    


    <!-- https://w3id.org/netbeheer/referentiemodellen/IECCIM/TC57CIM/IEC61970/Base/Wires#TransformerEnd_grounded -->


    <owl:DatatypeProperty rdf:about="https://w3id.org/netbeheer/referentiemodellen/IECCIM/TC57CIM/IEC61970/Base/Wires#TransformerEnd_grounded">
        <rdfs:domain rdf:resource="https://w3id.org/netbeheer/referentiemodellen/IECCIM/TC57CIM/IEC61970/Base/Wires#TransformerEnd"/>
        <rdfs:range rdf:resource="http://www.w3.org/2001/XMLSchema#boolean"/>
        <rdfs:comment>(for Yn and Zn connections) True if the neutral is solidly grounded.</rdfs:comment>
    </owl:DatatypeProperty>
    


    <!-- https://w3id.org/netbeheer/referentiemodellen/IECCIM/TC57CIM/IEC61970/Base/Wires#TransformerTankEnd_phases -->


    <owl:DatatypeProperty rdf:about="https://w3id.org/netbeheer/referentiemodellen/IECCIM/TC57CIM/IEC61970/Base/Wires#TransformerTankEnd_phases">
        <rdfs:domain rdf:resource="https://w3id.org/netbeheer/referentiemodellen/IECCIM/TC57CIM/IEC61970/Base/Wires#TransformerTankEnd"/>
        <rdfs:range rdf:resource="https://w3id.org/netbeheer/referentiemodellen/IECCIM/TC57CIM/IEC61970/Base/Core#PhaseCode"/>
        <rdfs:comment>Describes the phases carried by a conducting equipment.</rdfs:comment>
    </owl:DatatypeProperty>
    


    <!-- 
    ///////////////////////////////////////////////////////////////////////////////////////
    //
    // Classes
    //
    ///////////////////////////////////////////////////////////////////////////////////////
     -->


    


    <!-- https://w3id.org/netbeheer/referentiemodellen/IECCIM/TC57CIM/IEC61968/AssetInfo#TransformerEndInfo -->


    <owl:Class rdf:about="https://w3id.org/netbeheer/referentiemodellen/IECCIM/TC57CIM/IEC61968/AssetInfo#TransformerEndInfo">
        <rdfs:subClassOf>
            <owl:Restriction>
                <owl:onProperty rdf:resource="https://w3id.org/netbeheer/referentiemodellen/IECCIM/TC57CIM/IEC61970/Base/Wires#TransformerEndInfo_CoreAdmittance"/>
                <owl:minQualifiedCardinality rdf:datatype="http://www.w3.org/2001/XMLSchema#nonNegativeInteger">0</owl:minQualifiedCardinality>
                <owl:onClass rdf:resource="https://w3id.org/netbeheer/referentiemodellen/IECCIM/TC57CIM/IEC61968/AssetInfo#TransformerEndInfo"/>
            </owl:Restriction>
        </rdfs:subClassOf>
        <rdfs:subClassOf>
            <owl:Restriction>
                <owl:onProperty rdf:resource="https://w3id.org/netbeheer/referentiemodellen/IECCIM/TC57CIM/IEC61970/Base/Wires#TransformerEndInfo_FromMeshImpedances"/>
                <owl:minQualifiedCardinality rdf:datatype="http://www.w3.org/2001/XMLSchema#nonNegativeInteger">0</owl:minQualifiedCardinality>
                <owl:onClass rdf:resource="https://w3id.org/netbeheer/referentiemodellen/IECCIM/TC57CIM/IEC61968/AssetInfo#TransformerEndInfo"/>
            </owl:Restriction>
        </rdfs:subClassOf>
        <rdfs:subClassOf>
            <owl:Restriction>
                <owl:onProperty rdf:resource="https://w3id.org/netbeheer/referentiemodellen/IECCIM/TC57CIM/IEC61970/Base/Wires#TransformerEndInfo_ToMeshImpedances"/>
                <owl:minQualifiedCardinality rdf:datatype="http://www.w3.org/2001/XMLSchema#nonNegativeInteger">0</owl:minQualifiedCardinality>
                <owl:onClass rdf:resource="https://w3id.org/netbeheer/referentiemodellen/IECCIM/TC57CIM/IEC61968/AssetInfo#TransformerEndInfo"/>
            </owl:Restriction>
        </rdfs:subClassOf>
        <rdfs:subClassOf>
            <owl:Restriction>
                <owl:onProperty rdf:resource="https://w3id.org/netbeheer/referentiemodellen/IECCIM/TC57CIM/IEC61970/Base/Wires#TransformerEndInfo_TransformerStarImpedance"/>
                <owl:minQualifiedCardinality rdf:datatype="http://www.w3.org/2001/XMLSchema#nonNegativeInteger">0</owl:minQualifiedCardinality>
                <owl:onClass rdf:resource="https://w3id.org/netbeheer/referentiemodellen/IECCIM/TC57CIM/IEC61968/AssetInfo#TransformerEndInfo"/>
            </owl:Restriction>
        </rdfs:subClassOf>
        <rdfs:subClassOf>
            <owl:Restriction>
                <owl:onProperty rdf:resource="https://w3id.org/netbeheer/referentiemodellen/IECCIM/TC57CIM/IEC61970/Base/Wires#TransformerEndInfo_CoreAdmittance"/>
                <owl:maxQualifiedCardinality rdf:datatype="http://www.w3.org/2001/XMLSchema#nonNegativeInteger">1</owl:maxQualifiedCardinality>
                <owl:onClass rdf:resource="https://w3id.org/netbeheer/referentiemodellen/IECCIM/TC57CIM/IEC61968/AssetInfo#TransformerEndInfo"/>
            </owl:Restriction>
        </rdfs:subClassOf>
        <rdfs:subClassOf>
            <owl:Restriction>
                <owl:onProperty rdf:resource="https://w3id.org/netbeheer/referentiemodellen/IECCIM/TC57CIM/IEC61970/Base/Wires#TransformerEndInfo_FromMeshImpedances"/>
                <owl:maxQualifiedCardinality rdf:datatype="http://www.w3.org/2001/XMLSchema#nonNegativeInteger">1</owl:maxQualifiedCardinality>
                <owl:onClass rdf:resource="https://w3id.org/netbeheer/referentiemodellen/IECCIM/TC57CIM/IEC61968/AssetInfo#TransformerEndInfo"/>
            </owl:Restriction>
        </rdfs:subClassOf>
        <rdfs:subClassOf>
            <owl:Restriction>
                <owl:onProperty rdf:resource="https://w3id.org/netbeheer/referentiemodellen/IECCIM/TC57CIM/IEC61970/Base/Wires#TransformerEndInfo_TransformerStarImpedance"/>
                <owl:maxQualifiedCardinality rdf:datatype="http://www.w3.org/2001/XMLSchema#nonNegativeInteger">1</owl:maxQualifiedCardinality>
                <owl:onClass rdf:resource="https://w3id.org/netbeheer/referentiemodellen/IECCIM/TC57CIM/IEC61968/AssetInfo#TransformerEndInfo"/>
            </owl:Restriction>
        </rdfs:subClassOf>
    </owl:Class>
    


    <!-- https://w3id.org/netbeheer/referentiemodellen/IECCIM/TC57CIM/IEC61968/AssetInfo#WireInfo -->


    <owl:Class rdf:about="https://w3id.org/netbeheer/referentiemodellen/IECCIM/TC57CIM/IEC61968/AssetInfo#WireInfo">
        <rdfs:subClassOf>
            <owl:Restriction>
                <owl:onProperty rdf:resource="https://w3id.org/netbeheer/referentiemodellen/IECCIM/TC57CIM/IEC61970/Base/Wires#WireInfo_PerLengthParameters"/>
                <owl:minQualifiedCardinality rdf:datatype="http://www.w3.org/2001/XMLSchema#nonNegativeInteger">0</owl:minQualifiedCardinality>
                <owl:onClass rdf:resource="https://w3id.org/netbeheer/referentiemodellen/IECCIM/TC57CIM/IEC61968/AssetInfo#WireInfo"/>
            </owl:Restriction>
        </rdfs:subClassOf>
    </owl:Class>
    


    <!-- https://w3id.org/netbeheer/referentiemodellen/IECCIM/TC57CIM/IEC61968/AssetInfo#WireSpacing -->


    <owl:Class rdf:about="https://w3id.org/netbeheer/referentiemodellen/IECCIM/TC57CIM/IEC61968/AssetInfo#WireSpacing">
        <rdfs:subClassOf>
            <owl:Restriction>
                <owl:onProperty rdf:resource="https://w3id.org/netbeheer/referentiemodellen/IECCIM/TC57CIM/IEC61970/Base/Wires#WireSpacing_ACLineSegments"/>
                <owl:minQualifiedCardinality rdf:datatype="http://www.w3.org/2001/XMLSchema#nonNegativeInteger">0</owl:minQualifiedCardinality>
                <owl:onClass rdf:resource="https://w3id.org/netbeheer/referentiemodellen/IECCIM/TC57CIM/IEC61968/AssetInfo#WireSpacing"/>
            </owl:Restriction>
        </rdfs:subClassOf>
        <rdfs:subClassOf>
            <owl:Restriction>
                <owl:onProperty rdf:resource="https://w3id.org/netbeheer/referentiemodellen/IECCIM/TC57CIM/IEC61970/Base/Wires#WireSpacing_PerLengthParameters"/>
                <owl:minQualifiedCardinality rdf:datatype="http://www.w3.org/2001/XMLSchema#nonNegativeInteger">0</owl:minQualifiedCardinality>
                <owl:onClass rdf:resource="https://w3id.org/netbeheer/referentiemodellen/IECCIM/TC57CIM/IEC61968/AssetInfo#WireSpacing"/>
            </owl:Restriction>
        </rdfs:subClassOf>
        <rdfs:subClassOf>
            <owl:Restriction>
                <owl:onProperty rdf:resource="https://w3id.org/netbeheer/referentiemodellen/IECCIM/TC57CIM/IEC61970/Base/Wires#WireSpacing_ACLineSegments"/>
                <owl:maxQualifiedCardinality rdf:datatype="http://www.w3.org/2001/XMLSchema#nonNegativeInteger">1</owl:maxQualifiedCardinality>
                <owl:onClass rdf:resource="https://w3id.org/netbeheer/referentiemodellen/IECCIM/TC57CIM/IEC61968/AssetInfo#WireSpacing"/>
            </owl:Restriction>
        </rdfs:subClassOf>
        <rdfs:subClassOf>
            <owl:Restriction>
                <owl:onProperty rdf:resource="https://w3id.org/netbeheer/referentiemodellen/IECCIM/TC57CIM/IEC61970/Base/Wires#WireSpacing_PerLengthParameters"/>
                <owl:maxQualifiedCardinality rdf:datatype="http://www.w3.org/2001/XMLSchema#nonNegativeInteger">1</owl:maxQualifiedCardinality>
                <owl:onClass rdf:resource="https://w3id.org/netbeheer/referentiemodellen/IECCIM/TC57CIM/IEC61968/AssetInfo#WireSpacing"/>
            </owl:Restriction>
        </rdfs:subClassOf>
    </owl:Class>
    


    <!-- https://w3id.org/netbeheer/referentiemodellen/IECCIM/TC57CIM/IEC61968/InfIEC61968/InfAssets#TransformerObservation -->


    <owl:Class rdf:about="https://w3id.org/netbeheer/referentiemodellen/IECCIM/TC57CIM/IEC61968/InfIEC61968/InfAssets#TransformerObservation">
        <rdfs:subClassOf>
            <owl:Restriction>
                <owl:onProperty rdf:resource="https://w3id.org/netbeheer/referentiemodellen/IECCIM/TC57CIM/IEC61970/Base/Wires#TransformerObservation_Transformer"/>
                <owl:minQualifiedCardinality rdf:datatype="http://www.w3.org/2001/XMLSchema#nonNegativeInteger">0</owl:minQualifiedCardinality>
                <owl:onClass rdf:resource="https://w3id.org/netbeheer/referentiemodellen/IECCIM/TC57CIM/IEC61968/InfIEC61968/InfAssets#TransformerObservation"/>
            </owl:Restriction>
        </rdfs:subClassOf>
    </owl:Class>
    


    <!-- https://w3id.org/netbeheer/referentiemodellen/IECCIM/TC57CIM/IEC61968/InfIEC61968/InfAssets#WindingInsulation -->


    <owl:Class rdf:about="https://w3id.org/netbeheer/referentiemodellen/IECCIM/TC57CIM/IEC61968/InfIEC61968/InfAssets#WindingInsulation">
        <rdfs:subClassOf>
            <owl:Restriction>
                <owl:onProperty rdf:resource="https://w3id.org/netbeheer/referentiemodellen/IECCIM/TC57CIM/IEC61970/Base/Wires#WindingInsulation_FromWinding"/>
                <owl:minQualifiedCardinality rdf:datatype="http://www.w3.org/2001/XMLSchema#nonNegativeInteger">0</owl:minQualifiedCardinality>
                <owl:onClass rdf:resource="https://w3id.org/netbeheer/referentiemodellen/IECCIM/TC57CIM/IEC61968/InfIEC61968/InfAssets#WindingInsulation"/>
            </owl:Restriction>
        </rdfs:subClassOf>
        <rdfs:subClassOf>
            <owl:Restriction>
                <owl:onProperty rdf:resource="https://w3id.org/netbeheer/referentiemodellen/IECCIM/TC57CIM/IEC61970/Base/Wires#WindingInsulation_ToWinding"/>
                <owl:minQualifiedCardinality rdf:datatype="http://www.w3.org/2001/XMLSchema#nonNegativeInteger">0</owl:minQualifiedCardinality>
                <owl:onClass rdf:resource="https://w3id.org/netbeheer/referentiemodellen/IECCIM/TC57CIM/IEC61968/InfIEC61968/InfAssets#WindingInsulation"/>
            </owl:Restriction>
        </rdfs:subClassOf>
    </owl:Class>
    


    <!-- https://w3id.org/netbeheer/referentiemodellen/IECCIM/TC57CIM/IEC61968/LoadControl#ConnectDisconnectFunction -->


    <owl:Class rdf:about="https://w3id.org/netbeheer/referentiemodellen/IECCIM/TC57CIM/IEC61968/LoadControl#ConnectDisconnectFunction">
        <rdfs:subClassOf>
            <owl:Restriction>
                <owl:onProperty rdf:resource="https://w3id.org/netbeheer/referentiemodellen/IECCIM/TC57CIM/IEC61970/Base/Wires#ConnectDisconnectFunction_Switches"/>
                <owl:minQualifiedCardinality rdf:datatype="http://www.w3.org/2001/XMLSchema#nonNegativeInteger">0</owl:minQualifiedCardinality>
                <owl:onClass rdf:resource="https://w3id.org/netbeheer/referentiemodellen/IECCIM/TC57CIM/IEC61968/LoadControl#ConnectDisconnectFunction"/>
            </owl:Restriction>
        </rdfs:subClassOf>
    </owl:Class>
    


    <!-- https://w3id.org/netbeheer/referentiemodellen/IECCIM/TC57CIM/IEC61968/Operations#CutAction -->


    <owl:Class rdf:about="https://w3id.org/netbeheer/referentiemodellen/IECCIM/TC57CIM/IEC61968/Operations#CutAction">
        <rdfs:subClassOf>
            <owl:Restriction>
                <owl:onProperty rdf:resource="https://w3id.org/netbeheer/referentiemodellen/IECCIM/TC57CIM/IEC61970/Base/Wires#CutAction_Cut"/>
                <owl:minQualifiedCardinality rdf:datatype="http://www.w3.org/2001/XMLSchema#nonNegativeInteger">0</owl:minQualifiedCardinality>
                <owl:onClass rdf:resource="https://w3id.org/netbeheer/referentiemodellen/IECCIM/TC57CIM/IEC61968/Operations#CutAction"/>
            </owl:Restriction>
        </rdfs:subClassOf>
        <rdfs:subClassOf>
            <owl:Restriction>
                <owl:onProperty rdf:resource="https://w3id.org/netbeheer/referentiemodellen/IECCIM/TC57CIM/IEC61970/Base/Wires#CutAction_Cut"/>
                <owl:maxQualifiedCardinality rdf:datatype="http://www.w3.org/2001/XMLSchema#nonNegativeInteger">1</owl:maxQualifiedCardinality>
                <owl:onClass rdf:resource="https://w3id.org/netbeheer/referentiemodellen/IECCIM/TC57CIM/IEC61968/Operations#CutAction"/>
            </owl:Restriction>
        </rdfs:subClassOf>
    </owl:Class>
    


    <!-- https://w3id.org/netbeheer/referentiemodellen/IECCIM/TC57CIM/IEC61968/Operations#EnergySourceAction -->


    <owl:Class rdf:about="https://w3id.org/netbeheer/referentiemodellen/IECCIM/TC57CIM/IEC61968/Operations#EnergySourceAction">
        <rdfs:subClassOf>
            <owl:Restriction>
                <owl:onProperty rdf:resource="https://w3id.org/netbeheer/referentiemodellen/IECCIM/TC57CIM/IEC61970/Base/Wires#EnergySourceAction_EnergySource"/>
                <owl:minQualifiedCardinality rdf:datatype="http://www.w3.org/2001/XMLSchema#nonNegativeInteger">0</owl:minQualifiedCardinality>
                <owl:onClass rdf:resource="https://w3id.org/netbeheer/referentiemodellen/IECCIM/TC57CIM/IEC61968/Operations#EnergySourceAction"/>
            </owl:Restriction>
        </rdfs:subClassOf>
        <rdfs:subClassOf>
            <owl:Restriction>
                <owl:onProperty rdf:resource="https://w3id.org/netbeheer/referentiemodellen/IECCIM/TC57CIM/IEC61970/Base/Wires#EnergySourceAction_EnergySource"/>
                <owl:maxQualifiedCardinality rdf:datatype="http://www.w3.org/2001/XMLSchema#nonNegativeInteger">1</owl:maxQualifiedCardinality>
                <owl:onClass rdf:resource="https://w3id.org/netbeheer/referentiemodellen/IECCIM/TC57CIM/IEC61968/Operations#EnergySourceAction"/>
            </owl:Restriction>
        </rdfs:subClassOf>
    </owl:Class>
    


    <!-- https://w3id.org/netbeheer/referentiemodellen/IECCIM/TC57CIM/IEC61968/Operations#GroundAction -->


    <owl:Class rdf:about="https://w3id.org/netbeheer/referentiemodellen/IECCIM/TC57CIM/IEC61968/Operations#GroundAction">
        <rdfs:subClassOf>
            <owl:Restriction>
                <owl:onProperty rdf:resource="https://w3id.org/netbeheer/referentiemodellen/IECCIM/TC57CIM/IEC61970/Base/Wires#GroundAction_AlongACLineSegment"/>
                <owl:minQualifiedCardinality rdf:datatype="http://www.w3.org/2001/XMLSchema#nonNegativeInteger">0</owl:minQualifiedCardinality>
                <owl:onClass rdf:resource="https://w3id.org/netbeheer/referentiemodellen/IECCIM/TC57CIM/IEC61968/Operations#GroundAction"/>
            </owl:Restriction>
        </rdfs:subClassOf>
        <rdfs:subClassOf>
            <owl:Restriction>
                <owl:onProperty rdf:resource="https://w3id.org/netbeheer/referentiemodellen/IECCIM/TC57CIM/IEC61970/Base/Wires#GroundAction_Ground"/>
                <owl:minQualifiedCardinality rdf:datatype="http://www.w3.org/2001/XMLSchema#nonNegativeInteger">0</owl:minQualifiedCardinality>
                <owl:onClass rdf:resource="https://w3id.org/netbeheer/referentiemodellen/IECCIM/TC57CIM/IEC61968/Operations#GroundAction"/>
            </owl:Restriction>
        </rdfs:subClassOf>
        <rdfs:subClassOf>
            <owl:Restriction>
                <owl:onProperty rdf:resource="https://w3id.org/netbeheer/referentiemodellen/IECCIM/TC57CIM/IEC61970/Base/Wires#GroundAction_AlongACLineSegment"/>
                <owl:maxQualifiedCardinality rdf:datatype="http://www.w3.org/2001/XMLSchema#nonNegativeInteger">1</owl:maxQualifiedCardinality>
                <owl:onClass rdf:resource="https://w3id.org/netbeheer/referentiemodellen/IECCIM/TC57CIM/IEC61968/Operations#GroundAction"/>
            </owl:Restriction>
        </rdfs:subClassOf>
        <rdfs:subClassOf>
            <owl:Restriction>
                <owl:onProperty rdf:resource="https://w3id.org/netbeheer/referentiemodellen/IECCIM/TC57CIM/IEC61970/Base/Wires#GroundAction_Ground"/>
                <owl:maxQualifiedCardinality rdf:datatype="http://www.w3.org/2001/XMLSchema#nonNegativeInteger">1</owl:maxQualifiedCardinality>
                <owl:onClass rdf:resource="https://w3id.org/netbeheer/referentiemodellen/IECCIM/TC57CIM/IEC61968/Operations#GroundAction"/>
            </owl:Restriction>
        </rdfs:subClassOf>
    </owl:Class>
    


    <!-- https://w3id.org/netbeheer/referentiemodellen/IECCIM/TC57CIM/IEC61968/Operations#JumperAction -->


    <owl:Class rdf:about="https://w3id.org/netbeheer/referentiemodellen/IECCIM/TC57CIM/IEC61968/Operations#JumperAction">
        <rdfs:subClassOf>
            <owl:Restriction>
                <owl:onProperty rdf:resource="https://w3id.org/netbeheer/referentiemodellen/IECCIM/TC57CIM/IEC61970/Base/Wires#JumperAction_AlongACLineSegments"/>
                <owl:minQualifiedCardinality rdf:datatype="http://www.w3.org/2001/XMLSchema#nonNegativeInteger">0</owl:minQualifiedCardinality>
                <owl:onClass rdf:resource="https://w3id.org/netbeheer/referentiemodellen/IECCIM/TC57CIM/IEC61968/Operations#JumperAction"/>
            </owl:Restriction>
        </rdfs:subClassOf>
        <rdfs:subClassOf>
            <owl:Restriction>
                <owl:onProperty rdf:resource="https://w3id.org/netbeheer/referentiemodellen/IECCIM/TC57CIM/IEC61970/Base/Wires#JumperAction_Jumper"/>
                <owl:minQualifiedCardinality rdf:datatype="http://www.w3.org/2001/XMLSchema#nonNegativeInteger">0</owl:minQualifiedCardinality>
                <owl:onClass rdf:resource="https://w3id.org/netbeheer/referentiemodellen/IECCIM/TC57CIM/IEC61968/Operations#JumperAction"/>
            </owl:Restriction>
        </rdfs:subClassOf>
        <rdfs:subClassOf>
            <owl:Restriction>
                <owl:onProperty rdf:resource="https://w3id.org/netbeheer/referentiemodellen/IECCIM/TC57CIM/IEC61970/Base/Wires#JumperAction_AlongACLineSegments"/>
                <owl:maxQualifiedCardinality rdf:datatype="http://www.w3.org/2001/XMLSchema#nonNegativeInteger">1</owl:maxQualifiedCardinality>
                <owl:onClass rdf:resource="https://w3id.org/netbeheer/referentiemodellen/IECCIM/TC57CIM/IEC61968/Operations#JumperAction"/>
            </owl:Restriction>
        </rdfs:subClassOf>
        <rdfs:subClassOf>
            <owl:Restriction>
                <owl:onProperty rdf:resource="https://w3id.org/netbeheer/referentiemodellen/IECCIM/TC57CIM/IEC61970/Base/Wires#JumperAction_Jumper"/>
                <owl:maxQualifiedCardinality rdf:datatype="http://www.w3.org/2001/XMLSchema#nonNegativeInteger">1</owl:maxQualifiedCardinality>
                <owl:onClass rdf:resource="https://w3id.org/netbeheer/referentiemodellen/IECCIM/TC57CIM/IEC61968/Operations#JumperAction"/>
            </owl:Restriction>
        </rdfs:subClassOf>
    </owl:Class>
    


    <!-- https://w3id.org/netbeheer/referentiemodellen/IECCIM/TC57CIM/IEC61968/Operations#Outage -->


    <owl:Class rdf:about="https://w3id.org/netbeheer/referentiemodellen/IECCIM/TC57CIM/IEC61968/Operations#Outage">
        <rdfs:subClassOf>
            <owl:Restriction>
                <owl:onProperty rdf:resource="https://w3id.org/netbeheer/referentiemodellen/IECCIM/TC57CIM/IEC61970/Base/Wires#Outage_OpenedSwitches"/>
                <owl:minQualifiedCardinality rdf:datatype="http://www.w3.org/2001/XMLSchema#nonNegativeInteger">0</owl:minQualifiedCardinality>
                <owl:onClass rdf:resource="https://w3id.org/netbeheer/referentiemodellen/IECCIM/TC57CIM/IEC61968/Operations#Outage"/>
            </owl:Restriction>
        </rdfs:subClassOf>
        <rdfs:subClassOf>
            <owl:Restriction>
                <owl:onProperty rdf:resource="https://w3id.org/netbeheer/referentiemodellen/IECCIM/TC57CIM/IEC61970/Base/Wires#Outage_OpenedSwitches"/>
                <owl:maxQualifiedCardinality rdf:datatype="http://www.w3.org/2001/XMLSchema#nonNegativeInteger">1</owl:maxQualifiedCardinality>
                <owl:onClass rdf:resource="https://w3id.org/netbeheer/referentiemodellen/IECCIM/TC57CIM/IEC61968/Operations#Outage"/>
            </owl:Restriction>
        </rdfs:subClassOf>
    </owl:Class>
    


    <!-- https://w3id.org/netbeheer/referentiemodellen/IECCIM/TC57CIM/IEC61968/Operations#SwitchAction -->


    <owl:Class rdf:about="https://w3id.org/netbeheer/referentiemodellen/IECCIM/TC57CIM/IEC61968/Operations#SwitchAction">
        <rdfs:subClassOf>
            <owl:Restriction>
                <owl:onProperty rdf:resource="https://w3id.org/netbeheer/referentiemodellen/IECCIM/TC57CIM/IEC61970/Base/Wires#SwitchAction_OperatedSwitch"/>
                <owl:minQualifiedCardinality rdf:datatype="http://www.w3.org/2001/XMLSchema#nonNegativeInteger">0</owl:minQualifiedCardinality>
                <owl:onClass rdf:resource="https://w3id.org/netbeheer/referentiemodellen/IECCIM/TC57CIM/IEC61968/Operations#SwitchAction"/>
            </owl:Restriction>
        </rdfs:subClassOf>
        <rdfs:subClassOf>
            <owl:Restriction>
                <owl:onProperty rdf:resource="https://w3id.org/netbeheer/referentiemodellen/IECCIM/TC57CIM/IEC61970/Base/Wires#SwitchAction_OperatedSwitch"/>
                <owl:maxQualifiedCardinality rdf:datatype="http://www.w3.org/2001/XMLSchema#nonNegativeInteger">1</owl:maxQualifiedCardinality>
                <owl:onClass rdf:resource="https://w3id.org/netbeheer/referentiemodellen/IECCIM/TC57CIM/IEC61968/Operations#SwitchAction"/>
            </owl:Restriction>
        </rdfs:subClassOf>
    </owl:Class>
    


    <!-- https://w3id.org/netbeheer/referentiemodellen/IECCIM/TC57CIM/IEC61970/Base/Core#ConductingEquipment -->


    <owl:Class rdf:about="https://w3id.org/netbeheer/referentiemodellen/IECCIM/TC57CIM/IEC61970/Base/Core#ConductingEquipment"/>
    


    <!-- https://w3id.org/netbeheer/referentiemodellen/IECCIM/TC57CIM/IEC61970/Base/Core#Curve -->


    <owl:Class rdf:about="https://w3id.org/netbeheer/referentiemodellen/IECCIM/TC57CIM/IEC61970/Base/Core#Curve"/>
    


    <!-- https://w3id.org/netbeheer/referentiemodellen/IECCIM/TC57CIM/IEC61970/Base/Core#Equipment -->


    <owl:Class rdf:about="https://w3id.org/netbeheer/referentiemodellen/IECCIM/TC57CIM/IEC61970/Base/Core#Equipment"/>
    


    <!-- https://w3id.org/netbeheer/referentiemodellen/IECCIM/TC57CIM/IEC61970/Base/Core#EquipmentContainer -->


    <owl:Class rdf:about="https://w3id.org/netbeheer/referentiemodellen/IECCIM/TC57CIM/IEC61970/Base/Core#EquipmentContainer"/>
    


    <!-- https://w3id.org/netbeheer/referentiemodellen/IECCIM/TC57CIM/IEC61970/Base/Core#IdentifiedObject -->


    <owl:Class rdf:about="https://w3id.org/netbeheer/referentiemodellen/IECCIM/TC57CIM/IEC61970/Base/Core#IdentifiedObject"/>
    


    <!-- https://w3id.org/netbeheer/referentiemodellen/IECCIM/TC57CIM/IEC61970/Base/Core#PowerSystemResource -->


    <owl:Class rdf:about="https://w3id.org/netbeheer/referentiemodellen/IECCIM/TC57CIM/IEC61970/Base/Core#PowerSystemResource"/>
    


    <!-- https://w3id.org/netbeheer/referentiemodellen/IECCIM/TC57CIM/IEC61970/Base/Domain#ActivePower -->


    <owl:Class rdf:about="https://w3id.org/netbeheer/referentiemodellen/IECCIM/TC57CIM/IEC61970/Base/Domain#ActivePower"/>
    


    <!-- https://w3id.org/netbeheer/referentiemodellen/IECCIM/TC57CIM/IEC61970/Base/Domain#ActivePowerPerFrequency -->


    <owl:Class rdf:about="https://w3id.org/netbeheer/referentiemodellen/IECCIM/TC57CIM/IEC61970/Base/Domain#ActivePowerPerFrequency"/>
    


    <!-- https://w3id.org/netbeheer/referentiemodellen/IECCIM/TC57CIM/IEC61970/Base/Domain#AngleDegrees -->


    <owl:Class rdf:about="https://w3id.org/netbeheer/referentiemodellen/IECCIM/TC57CIM/IEC61970/Base/Domain#AngleDegrees"/>
    


    <!-- https://w3id.org/netbeheer/referentiemodellen/IECCIM/TC57CIM/IEC61970/Base/Domain#AngleRadians -->


    <owl:Class rdf:about="https://w3id.org/netbeheer/referentiemodellen/IECCIM/TC57CIM/IEC61970/Base/Domain#AngleRadians"/>
    


    <!-- https://w3id.org/netbeheer/referentiemodellen/IECCIM/TC57CIM/IEC61970/Base/Domain#ApparentPower -->


    <owl:Class rdf:about="https://w3id.org/netbeheer/referentiemodellen/IECCIM/TC57CIM/IEC61970/Base/Domain#ApparentPower"/>
    


    <!-- https://w3id.org/netbeheer/referentiemodellen/IECCIM/TC57CIM/IEC61970/Base/Domain#Conductance -->


    <owl:Class rdf:about="https://w3id.org/netbeheer/referentiemodellen/IECCIM/TC57CIM/IEC61970/Base/Domain#Conductance"/>
    


    <!-- https://w3id.org/netbeheer/referentiemodellen/IECCIM/TC57CIM/IEC61970/Base/Domain#ConductancePerLength -->


    <owl:Class rdf:about="https://w3id.org/netbeheer/referentiemodellen/IECCIM/TC57CIM/IEC61970/Base/Domain#ConductancePerLength"/>
    


    <!-- https://w3id.org/netbeheer/referentiemodellen/IECCIM/TC57CIM/IEC61970/Base/Domain#CurrentFlow -->


    <owl:Class rdf:about="https://w3id.org/netbeheer/referentiemodellen/IECCIM/TC57CIM/IEC61970/Base/Domain#CurrentFlow"/>
    


    <!-- https://w3id.org/netbeheer/referentiemodellen/IECCIM/TC57CIM/IEC61970/Base/Domain#Frequency -->


    <owl:Class rdf:about="https://w3id.org/netbeheer/referentiemodellen/IECCIM/TC57CIM/IEC61970/Base/Domain#Frequency"/>
    


    <!-- https://w3id.org/netbeheer/referentiemodellen/IECCIM/TC57CIM/IEC61970/Base/Domain#Length -->


    <owl:Class rdf:about="https://w3id.org/netbeheer/referentiemodellen/IECCIM/TC57CIM/IEC61970/Base/Domain#Length"/>
    


    <!-- https://w3id.org/netbeheer/referentiemodellen/IECCIM/TC57CIM/IEC61970/Base/Domain#PU -->


    <owl:Class rdf:about="https://w3id.org/netbeheer/referentiemodellen/IECCIM/TC57CIM/IEC61970/Base/Domain#PU"/>
    


    <!-- https://w3id.org/netbeheer/referentiemodellen/IECCIM/TC57CIM/IEC61970/Base/Domain#PerCent -->


    <owl:Class rdf:about="https://w3id.org/netbeheer/referentiemodellen/IECCIM/TC57CIM/IEC61970/Base/Domain#PerCent"/>
    


    <!-- https://w3id.org/netbeheer/referentiemodellen/IECCIM/TC57CIM/IEC61970/Base/Domain#Pressure -->


    <owl:Class rdf:about="https://w3id.org/netbeheer/referentiemodellen/IECCIM/TC57CIM/IEC61970/Base/Domain#Pressure"/>
    


    <!-- https://w3id.org/netbeheer/referentiemodellen/IECCIM/TC57CIM/IEC61970/Base/Domain#Reactance -->


    <owl:Class rdf:about="https://w3id.org/netbeheer/referentiemodellen/IECCIM/TC57CIM/IEC61970/Base/Domain#Reactance"/>
    


    <!-- https://w3id.org/netbeheer/referentiemodellen/IECCIM/TC57CIM/IEC61970/Base/Domain#ReactancePerLength -->


    <owl:Class rdf:about="https://w3id.org/netbeheer/referentiemodellen/IECCIM/TC57CIM/IEC61970/Base/Domain#ReactancePerLength"/>
    


    <!-- https://w3id.org/netbeheer/referentiemodellen/IECCIM/TC57CIM/IEC61970/Base/Domain#ReactivePower -->


    <owl:Class rdf:about="https://w3id.org/netbeheer/referentiemodellen/IECCIM/TC57CIM/IEC61970/Base/Domain#ReactivePower"/>
    


    <!-- https://w3id.org/netbeheer/referentiemodellen/IECCIM/TC57CIM/IEC61970/Base/Domain#Resistance -->


    <owl:Class rdf:about="https://w3id.org/netbeheer/referentiemodellen/IECCIM/TC57CIM/IEC61970/Base/Domain#Resistance"/>
    


    <!-- https://w3id.org/netbeheer/referentiemodellen/IECCIM/TC57CIM/IEC61970/Base/Domain#ResistancePerLength -->


    <owl:Class rdf:about="https://w3id.org/netbeheer/referentiemodellen/IECCIM/TC57CIM/IEC61970/Base/Domain#ResistancePerLength"/>
    


    <!-- https://w3id.org/netbeheer/referentiemodellen/IECCIM/TC57CIM/IEC61970/Base/Domain#RotationSpeed -->


    <owl:Class rdf:about="https://w3id.org/netbeheer/referentiemodellen/IECCIM/TC57CIM/IEC61970/Base/Domain#RotationSpeed"/>
    


    <!-- https://w3id.org/netbeheer/referentiemodellen/IECCIM/TC57CIM/IEC61970/Base/Domain#Seconds -->


    <owl:Class rdf:about="https://w3id.org/netbeheer/referentiemodellen/IECCIM/TC57CIM/IEC61970/Base/Domain#Seconds"/>
    


    <!-- https://w3id.org/netbeheer/referentiemodellen/IECCIM/TC57CIM/IEC61970/Base/Domain#Susceptance -->


    <owl:Class rdf:about="https://w3id.org/netbeheer/referentiemodellen/IECCIM/TC57CIM/IEC61970/Base/Domain#Susceptance"/>
    


    <!-- https://w3id.org/netbeheer/referentiemodellen/IECCIM/TC57CIM/IEC61970/Base/Domain#SusceptancePerLength -->


    <owl:Class rdf:about="https://w3id.org/netbeheer/referentiemodellen/IECCIM/TC57CIM/IEC61970/Base/Domain#SusceptancePerLength"/>
    


    <!-- https://w3id.org/netbeheer/referentiemodellen/IECCIM/TC57CIM/IEC61970/Base/Domain#Temperature -->


    <owl:Class rdf:about="https://w3id.org/netbeheer/referentiemodellen/IECCIM/TC57CIM/IEC61970/Base/Domain#Temperature"/>
    


    <!-- https://w3id.org/netbeheer/referentiemodellen/IECCIM/TC57CIM/IEC61970/Base/Domain#Voltage -->


    <owl:Class rdf:about="https://w3id.org/netbeheer/referentiemodellen/IECCIM/TC57CIM/IEC61970/Base/Domain#Voltage"/>
    


    <!-- https://w3id.org/netbeheer/referentiemodellen/IECCIM/TC57CIM/IEC61970/Base/Domain#VoltagePerReactivePower -->


    <owl:Class rdf:about="https://w3id.org/netbeheer/referentiemodellen/IECCIM/TC57CIM/IEC61970/Base/Domain#VoltagePerReactivePower"/>
    


    <!-- https://w3id.org/netbeheer/referentiemodellen/IECCIM/TC57CIM/IEC61970/Base/Equivalents#EquivalentInjection -->


    <owl:Class rdf:about="https://w3id.org/netbeheer/referentiemodellen/IECCIM/TC57CIM/IEC61970/Base/Equivalents#EquivalentInjection">
        <rdfs:subClassOf>
            <owl:Restriction>
                <owl:onProperty rdf:resource="https://w3id.org/netbeheer/referentiemodellen/IECCIM/TC57CIM/IEC61970/Base/Wires#EquivalentInjection_ReactiveCapabilityCurve"/>
                <owl:minQualifiedCardinality rdf:datatype="http://www.w3.org/2001/XMLSchema#nonNegativeInteger">0</owl:minQualifiedCardinality>
                <owl:onClass rdf:resource="https://w3id.org/netbeheer/referentiemodellen/IECCIM/TC57CIM/IEC61970/Base/Equivalents#EquivalentInjection"/>
            </owl:Restriction>
        </rdfs:subClassOf>
    </owl:Class>
    


    <!-- https://w3id.org/netbeheer/referentiemodellen/IECCIM/TC57CIM/IEC61970/Base/Generation/GenerationTrainingSimulation#PrimeMover -->


    <owl:Class rdf:about="https://w3id.org/netbeheer/referentiemodellen/IECCIM/TC57CIM/IEC61970/Base/Generation/GenerationTrainingSimulation#PrimeMover">
        <rdfs:subClassOf>
            <owl:Restriction>
                <owl:onProperty rdf:resource="https://w3id.org/netbeheer/referentiemodellen/IECCIM/TC57CIM/IEC61970/Base/Wires#PrimeMover_SynchronousMachines"/>
                <owl:minQualifiedCardinality rdf:datatype="http://www.w3.org/2001/XMLSchema#nonNegativeInteger">0</owl:minQualifiedCardinality>
                <owl:onClass rdf:resource="https://w3id.org/netbeheer/referentiemodellen/IECCIM/TC57CIM/IEC61970/Base/Generation/GenerationTrainingSimulation#PrimeMover"/>
            </owl:Restriction>
        </rdfs:subClassOf>
    </owl:Class>
    


    <!-- https://w3id.org/netbeheer/referentiemodellen/IECCIM/TC57CIM/IEC61970/Base/Generation/Production#GeneratingUnit -->


    <owl:Class rdf:about="https://w3id.org/netbeheer/referentiemodellen/IECCIM/TC57CIM/IEC61970/Base/Generation/Production#GeneratingUnit">
        <rdfs:subClassOf>
            <owl:Restriction>
                <owl:onProperty rdf:resource="https://w3id.org/netbeheer/referentiemodellen/IECCIM/TC57CIM/IEC61970/Base/Wires#GeneratingUnit_RotatingMachine"/>
                <owl:minQualifiedCardinality rdf:datatype="http://www.w3.org/2001/XMLSchema#nonNegativeInteger">0</owl:minQualifiedCardinality>
                <owl:onClass rdf:resource="https://w3id.org/netbeheer/referentiemodellen/IECCIM/TC57CIM/IEC61970/Base/Generation/Production#GeneratingUnit"/>
            </owl:Restriction>
        </rdfs:subClassOf>
        <rdfs:subClassOf>
            <owl:Restriction>
                <owl:onProperty rdf:resource="https://w3id.org/netbeheer/referentiemodellen/IECCIM/TC57CIM/IEC61970/Base/Wires#GeneratingUnit_RotatingMachine"/>
                <owl:maxQualifiedCardinality rdf:datatype="http://www.w3.org/2001/XMLSchema#nonNegativeInteger">1</owl:maxQualifiedCardinality>
                <owl:onClass rdf:resource="https://w3id.org/netbeheer/referentiemodellen/IECCIM/TC57CIM/IEC61970/Base/Generation/Production#GeneratingUnit"/>
            </owl:Restriction>
        </rdfs:subClassOf>
    </owl:Class>
    


    <!-- https://w3id.org/netbeheer/referentiemodellen/IECCIM/TC57CIM/IEC61970/Base/Generation/Production#HydroPump -->


    <owl:Class rdf:about="https://w3id.org/netbeheer/referentiemodellen/IECCIM/TC57CIM/IEC61970/Base/Generation/Production#HydroPump">
        <rdfs:subClassOf>
            <owl:Restriction>
                <owl:onProperty rdf:resource="https://w3id.org/netbeheer/referentiemodellen/IECCIM/TC57CIM/IEC61970/Base/Wires#HydroPump_RotatingMachine"/>
                <owl:minQualifiedCardinality rdf:datatype="http://www.w3.org/2001/XMLSchema#nonNegativeInteger">0</owl:minQualifiedCardinality>
                <owl:onClass rdf:resource="https://w3id.org/netbeheer/referentiemodellen/IECCIM/TC57CIM/IEC61970/Base/Generation/Production#HydroPump"/>
            </owl:Restriction>
        </rdfs:subClassOf>
        <rdfs:subClassOf>
            <owl:Restriction>
                <owl:onProperty rdf:resource="https://w3id.org/netbeheer/referentiemodellen/IECCIM/TC57CIM/IEC61970/Base/Wires#HydroPump_RotatingMachine"/>
                <owl:maxQualifiedCardinality rdf:datatype="http://www.w3.org/2001/XMLSchema#nonNegativeInteger">1</owl:maxQualifiedCardinality>
                <owl:onClass rdf:resource="https://w3id.org/netbeheer/referentiemodellen/IECCIM/TC57CIM/IEC61970/Base/Generation/Production#HydroPump"/>
            </owl:Restriction>
        </rdfs:subClassOf>
    </owl:Class>
    


    <!-- https://w3id.org/netbeheer/referentiemodellen/IECCIM/TC57CIM/IEC61970/Base/LoadModel#LoadResponseCharacteristic -->


    <owl:Class rdf:about="https://w3id.org/netbeheer/referentiemodellen/IECCIM/TC57CIM/IEC61970/Base/LoadModel#LoadResponseCharacteristic">
        <rdfs:subClassOf>
            <owl:Restriction>
                <owl:onProperty rdf:resource="https://w3id.org/netbeheer/referentiemodellen/IECCIM/TC57CIM/IEC61970/Base/Wires#LoadResponseCharacteristic_EnergyConsumer"/>
                <owl:minQualifiedCardinality rdf:datatype="http://www.w3.org/2001/XMLSchema#nonNegativeInteger">0</owl:minQualifiedCardinality>
                <owl:onClass rdf:resource="https://w3id.org/netbeheer/referentiemodellen/IECCIM/TC57CIM/IEC61970/Base/LoadModel#LoadResponseCharacteristic"/>
            </owl:Restriction>
        </rdfs:subClassOf>
        <rdfs:subClassOf>
            <owl:Restriction>
                <owl:onProperty rdf:resource="https://w3id.org/netbeheer/referentiemodellen/IECCIM/TC57CIM/IEC61970/Base/Wires#LoadResponseCharacteristic_EnergyConsumer"/>
                <owl:maxQualifiedCardinality rdf:datatype="http://www.w3.org/2001/XMLSchema#nonNegativeInteger">1</owl:maxQualifiedCardinality>
                <owl:onClass rdf:resource="https://w3id.org/netbeheer/referentiemodellen/IECCIM/TC57CIM/IEC61970/Base/LoadModel#LoadResponseCharacteristic"/>
            </owl:Restriction>
        </rdfs:subClassOf>
    </owl:Class>
    


    <!-- https://w3id.org/netbeheer/referentiemodellen/IECCIM/TC57CIM/IEC61970/Base/LoadModel#PowerCutZone -->


    <owl:Class rdf:about="https://w3id.org/netbeheer/referentiemodellen/IECCIM/TC57CIM/IEC61970/Base/LoadModel#PowerCutZone">
        <rdfs:subClassOf>
            <owl:Restriction>
                <owl:onProperty rdf:resource="https://w3id.org/netbeheer/referentiemodellen/IECCIM/TC57CIM/IEC61970/Base/Wires#PowerCutZone_EnergyConsumers"/>
                <owl:minQualifiedCardinality rdf:datatype="http://www.w3.org/2001/XMLSchema#nonNegativeInteger">0</owl:minQualifiedCardinality>
                <owl:onClass rdf:resource="https://w3id.org/netbeheer/referentiemodellen/IECCIM/TC57CIM/IEC61970/Base/LoadModel#PowerCutZone"/>
            </owl:Restriction>
        </rdfs:subClassOf>
        <rdfs:subClassOf>
            <owl:Restriction>
                <owl:onProperty rdf:resource="https://w3id.org/netbeheer/referentiemodellen/IECCIM/TC57CIM/IEC61970/Base/Wires#PowerCutZone_EnergyConsumers"/>
                <owl:maxQualifiedCardinality rdf:datatype="http://www.w3.org/2001/XMLSchema#nonNegativeInteger">1</owl:maxQualifiedCardinality>
                <owl:onClass rdf:resource="https://w3id.org/netbeheer/referentiemodellen/IECCIM/TC57CIM/IEC61970/Base/LoadModel#PowerCutZone"/>
            </owl:Restriction>
        </rdfs:subClassOf>
    </owl:Class>
    


    <!-- https://w3id.org/netbeheer/referentiemodellen/IECCIM/TC57CIM/IEC61970/Base/LoadModel#SeasonDayTypeSchedule -->


    <owl:Class rdf:about="https://w3id.org/netbeheer/referentiemodellen/IECCIM/TC57CIM/IEC61970/Base/LoadModel#SeasonDayTypeSchedule"/>
    


    <!-- https://w3id.org/netbeheer/referentiemodellen/IECCIM/TC57CIM/IEC61970/Base/Protection#ProtectionEquipment -->


    <owl:Class rdf:about="https://w3id.org/netbeheer/referentiemodellen/IECCIM/TC57CIM/IEC61970/Base/Protection#ProtectionEquipment">
        <rdfs:subClassOf>
            <owl:Restriction>
                <owl:onProperty rdf:resource="https://w3id.org/netbeheer/referentiemodellen/IECCIM/TC57CIM/IEC61970/Base/Wires#ProtectionEquipment_ProtectedSwitches"/>
                <owl:minQualifiedCardinality rdf:datatype="http://www.w3.org/2001/XMLSchema#nonNegativeInteger">0</owl:minQualifiedCardinality>
                <owl:onClass rdf:resource="https://w3id.org/netbeheer/referentiemodellen/IECCIM/TC57CIM/IEC61970/Base/Protection#ProtectionEquipment"/>
            </owl:Restriction>
        </rdfs:subClassOf>
    </owl:Class>
    


    <!-- https://w3id.org/netbeheer/referentiemodellen/IECCIM/TC57CIM/IEC61970/Base/Protection#RecloseSequence -->


    <owl:Class rdf:about="https://w3id.org/netbeheer/referentiemodellen/IECCIM/TC57CIM/IEC61970/Base/Protection#RecloseSequence">
        <rdfs:subClassOf>
            <owl:Restriction>
                <owl:onProperty rdf:resource="https://w3id.org/netbeheer/referentiemodellen/IECCIM/TC57CIM/IEC61970/Base/Wires#RecloseSequence_ProtectedSwitch"/>
                <owl:minQualifiedCardinality rdf:datatype="http://www.w3.org/2001/XMLSchema#nonNegativeInteger">0</owl:minQualifiedCardinality>
                <owl:onClass rdf:resource="https://w3id.org/netbeheer/referentiemodellen/IECCIM/TC57CIM/IEC61970/Base/Protection#RecloseSequence"/>
            </owl:Restriction>
        </rdfs:subClassOf>
    </owl:Class>
    


    <!-- https://w3id.org/netbeheer/referentiemodellen/IECCIM/TC57CIM/IEC61970/Base/StateVariables#SvShuntCompensatorSections -->


    <owl:Class rdf:about="https://w3id.org/netbeheer/referentiemodellen/IECCIM/TC57CIM/IEC61970/Base/StateVariables#SvShuntCompensatorSections">
        <rdfs:subClassOf>
            <owl:Restriction>
                <owl:onProperty rdf:resource="https://w3id.org/netbeheer/referentiemodellen/IECCIM/TC57CIM/IEC61970/Base/Wires#SvShuntCompensatorSections_ShuntCompensator"/>
                <owl:minQualifiedCardinality rdf:datatype="http://www.w3.org/2001/XMLSchema#nonNegativeInteger">0</owl:minQualifiedCardinality>
                <owl:onClass rdf:resource="https://w3id.org/netbeheer/referentiemodellen/IECCIM/TC57CIM/IEC61970/Base/StateVariables#SvShuntCompensatorSections"/>
            </owl:Restriction>
        </rdfs:subClassOf>
        <rdfs:subClassOf>
            <owl:Restriction>
                <owl:onProperty rdf:resource="https://w3id.org/netbeheer/referentiemodellen/IECCIM/TC57CIM/IEC61970/Base/Wires#SvShuntCompensatorSections_ShuntCompensator"/>
                <owl:maxQualifiedCardinality rdf:datatype="http://www.w3.org/2001/XMLSchema#nonNegativeInteger">1</owl:maxQualifiedCardinality>
                <owl:onClass rdf:resource="https://w3id.org/netbeheer/referentiemodellen/IECCIM/TC57CIM/IEC61970/Base/StateVariables#SvShuntCompensatorSections"/>
            </owl:Restriction>
        </rdfs:subClassOf>
    </owl:Class>
    


    <!-- https://w3id.org/netbeheer/referentiemodellen/IECCIM/TC57CIM/IEC61970/Base/StateVariables#SvTapStep -->


    <owl:Class rdf:about="https://w3id.org/netbeheer/referentiemodellen/IECCIM/TC57CIM/IEC61970/Base/StateVariables#SvTapStep">
        <rdfs:subClassOf>
            <owl:Restriction>
                <owl:onProperty rdf:resource="https://w3id.org/netbeheer/referentiemodellen/IECCIM/TC57CIM/IEC61970/Base/Wires#SvTapStep_TapChanger"/>
                <owl:minQualifiedCardinality rdf:datatype="http://www.w3.org/2001/XMLSchema#nonNegativeInteger">0</owl:minQualifiedCardinality>
                <owl:onClass rdf:resource="https://w3id.org/netbeheer/referentiemodellen/IECCIM/TC57CIM/IEC61970/Base/StateVariables#SvTapStep"/>
            </owl:Restriction>
        </rdfs:subClassOf>
        <rdfs:subClassOf>
            <owl:Restriction>
                <owl:onProperty rdf:resource="https://w3id.org/netbeheer/referentiemodellen/IECCIM/TC57CIM/IEC61970/Base/Wires#SvTapStep_TapChanger"/>
                <owl:maxQualifiedCardinality rdf:datatype="http://www.w3.org/2001/XMLSchema#nonNegativeInteger">1</owl:maxQualifiedCardinality>
                <owl:onClass rdf:resource="https://w3id.org/netbeheer/referentiemodellen/IECCIM/TC57CIM/IEC61970/Base/StateVariables#SvTapStep"/>
            </owl:Restriction>
        </rdfs:subClassOf>
    </owl:Class>
    


    <!-- https://w3id.org/netbeheer/referentiemodellen/IECCIM/TC57CIM/IEC61970/Base/Wires#ACLineSegment -->


    <owl:Class rdf:about="https://w3id.org/netbeheer/referentiemodellen/IECCIM/TC57CIM/IEC61970/Base/Wires#ACLineSegment">
        <rdfs:subClassOf rdf:resource="https://w3id.org/netbeheer/referentiemodellen/IECCIM/TC57CIM/IEC61970/Base/Wires#Conductor"/>
        <rdfs:subClassOf>
            <owl:Restriction>
                <owl:onProperty rdf:resource="https://w3id.org/netbeheer/referentiemodellen/IECCIM/TC57CIM/IEC61970/Base/Wires#ACLineSegment_LineGroundingAction"/>
                <owl:minQualifiedCardinality rdf:datatype="http://www.w3.org/2001/XMLSchema#nonNegativeInteger">0</owl:minQualifiedCardinality>
                <owl:onClass rdf:resource="https://w3id.org/netbeheer/referentiemodellen/IECCIM/TC57CIM/IEC61970/Base/Wires#ACLineSegment"/>
            </owl:Restriction>
        </rdfs:subClassOf>
        <rdfs:subClassOf>
            <owl:Restriction>
                <owl:onProperty rdf:resource="https://w3id.org/netbeheer/referentiemodellen/IECCIM/TC57CIM/IEC61970/Base/Wires#ACLineSegment_LineJumpingAction"/>
                <owl:minQualifiedCardinality rdf:datatype="http://www.w3.org/2001/XMLSchema#nonNegativeInteger">0</owl:minQualifiedCardinality>
                <owl:onClass rdf:resource="https://w3id.org/netbeheer/referentiemodellen/IECCIM/TC57CIM/IEC61970/Base/Wires#ACLineSegment"/>
            </owl:Restriction>
        </rdfs:subClassOf>
        <rdfs:subClassOf>
            <owl:Restriction>
                <owl:onProperty rdf:resource="https://w3id.org/netbeheer/referentiemodellen/IECCIM/TC57CIM/IEC61970/Base/Wires#ACLineSegment_PerLengthImpedance"/>
                <owl:minQualifiedCardinality rdf:datatype="http://www.w3.org/2001/XMLSchema#nonNegativeInteger">0</owl:minQualifiedCardinality>
                <owl:onClass rdf:resource="https://w3id.org/netbeheer/referentiemodellen/IECCIM/TC57CIM/IEC61970/Base/Wires#ACLineSegment"/>
            </owl:Restriction>
        </rdfs:subClassOf>
        <rdfs:subClassOf>
            <owl:Restriction>
                <owl:onProperty rdf:resource="https://w3id.org/netbeheer/referentiemodellen/IECCIM/TC57CIM/IEC61970/Base/Wires#ACLineSegment_WireSpacing"/>
                <owl:minQualifiedCardinality rdf:datatype="http://www.w3.org/2001/XMLSchema#nonNegativeInteger">0</owl:minQualifiedCardinality>
                <owl:onClass rdf:resource="https://w3id.org/netbeheer/referentiemodellen/IECCIM/TC57CIM/IEC61970/Base/Wires#ACLineSegment"/>
            </owl:Restriction>
        </rdfs:subClassOf>
        <rdfs:subClassOf>
            <owl:Restriction>
                <owl:onProperty rdf:resource="https://w3id.org/netbeheer/referentiemodellen/IECCIM/TC57CIM/IEC61970/Base/Wires#ACLineSegment_b0ch"/>
                <owl:minQualifiedCardinality rdf:datatype="http://www.w3.org/2001/XMLSchema#nonNegativeInteger">0</owl:minQualifiedCardinality>
                <owl:onClass rdf:resource="https://w3id.org/netbeheer/referentiemodellen/IECCIM/TC57CIM/IEC61970/Base/Domain#Susceptance"/>
            </owl:Restriction>
        </rdfs:subClassOf>
        <rdfs:subClassOf>
            <owl:Restriction>
                <owl:onProperty rdf:resource="https://w3id.org/netbeheer/referentiemodellen/IECCIM/TC57CIM/IEC61970/Base/Wires#ACLineSegment_bch"/>
                <owl:minQualifiedCardinality rdf:datatype="http://www.w3.org/2001/XMLSchema#nonNegativeInteger">0</owl:minQualifiedCardinality>
                <owl:onClass rdf:resource="https://w3id.org/netbeheer/referentiemodellen/IECCIM/TC57CIM/IEC61970/Base/Domain#Susceptance"/>
            </owl:Restriction>
        </rdfs:subClassOf>
        <rdfs:subClassOf>
            <owl:Restriction>
                <owl:onProperty rdf:resource="https://w3id.org/netbeheer/referentiemodellen/IECCIM/TC57CIM/IEC61970/Base/Wires#ACLineSegment_g0ch"/>
                <owl:minQualifiedCardinality rdf:datatype="http://www.w3.org/2001/XMLSchema#nonNegativeInteger">0</owl:minQualifiedCardinality>
                <owl:onClass rdf:resource="https://w3id.org/netbeheer/referentiemodellen/IECCIM/TC57CIM/IEC61970/Base/Domain#Conductance"/>
            </owl:Restriction>
        </rdfs:subClassOf>
        <rdfs:subClassOf>
            <owl:Restriction>
                <owl:onProperty rdf:resource="https://w3id.org/netbeheer/referentiemodellen/IECCIM/TC57CIM/IEC61970/Base/Wires#ACLineSegment_gch"/>
                <owl:minQualifiedCardinality rdf:datatype="http://www.w3.org/2001/XMLSchema#nonNegativeInteger">0</owl:minQualifiedCardinality>
                <owl:onClass rdf:resource="https://w3id.org/netbeheer/referentiemodellen/IECCIM/TC57CIM/IEC61970/Base/Domain#Conductance"/>
            </owl:Restriction>
        </rdfs:subClassOf>
        <rdfs:subClassOf>
            <owl:Restriction>
                <owl:onProperty rdf:resource="https://w3id.org/netbeheer/referentiemodellen/IECCIM/TC57CIM/IEC61970/Base/Wires#ACLineSegment_r"/>
                <owl:minQualifiedCardinality rdf:datatype="http://www.w3.org/2001/XMLSchema#nonNegativeInteger">0</owl:minQualifiedCardinality>
                <owl:onClass rdf:resource="https://w3id.org/netbeheer/referentiemodellen/IECCIM/TC57CIM/IEC61970/Base/Domain#Resistance"/>
            </owl:Restriction>
        </rdfs:subClassOf>
        <rdfs:subClassOf>
            <owl:Restriction>
                <owl:onProperty rdf:resource="https://w3id.org/netbeheer/referentiemodellen/IECCIM/TC57CIM/IEC61970/Base/Wires#ACLineSegment_r0"/>
                <owl:minQualifiedCardinality rdf:datatype="http://www.w3.org/2001/XMLSchema#nonNegativeInteger">0</owl:minQualifiedCardinality>
                <owl:onClass rdf:resource="https://w3id.org/netbeheer/referentiemodellen/IECCIM/TC57CIM/IEC61970/Base/Domain#Resistance"/>
            </owl:Restriction>
        </rdfs:subClassOf>
        <rdfs:subClassOf>
            <owl:Restriction>
                <owl:onProperty rdf:resource="https://w3id.org/netbeheer/referentiemodellen/IECCIM/TC57CIM/IEC61970/Base/Wires#ACLineSegment_shortCircuitEndTemperature"/>
                <owl:minQualifiedCardinality rdf:datatype="http://www.w3.org/2001/XMLSchema#nonNegativeInteger">0</owl:minQualifiedCardinality>
                <owl:onClass rdf:resource="https://w3id.org/netbeheer/referentiemodellen/IECCIM/TC57CIM/IEC61970/Base/Domain#Temperature"/>
            </owl:Restriction>
        </rdfs:subClassOf>
        <rdfs:subClassOf>
            <owl:Restriction>
                <owl:onProperty rdf:resource="https://w3id.org/netbeheer/referentiemodellen/IECCIM/TC57CIM/IEC61970/Base/Wires#ACLineSegment_x"/>
                <owl:minQualifiedCardinality rdf:datatype="http://www.w3.org/2001/XMLSchema#nonNegativeInteger">0</owl:minQualifiedCardinality>
                <owl:onClass rdf:resource="https://w3id.org/netbeheer/referentiemodellen/IECCIM/TC57CIM/IEC61970/Base/Domain#Reactance"/>
            </owl:Restriction>
        </rdfs:subClassOf>
        <rdfs:subClassOf>
            <owl:Restriction>
                <owl:onProperty rdf:resource="https://w3id.org/netbeheer/referentiemodellen/IECCIM/TC57CIM/IEC61970/Base/Wires#ACLineSegment_x0"/>
                <owl:minQualifiedCardinality rdf:datatype="http://www.w3.org/2001/XMLSchema#nonNegativeInteger">0</owl:minQualifiedCardinality>
                <owl:onClass rdf:resource="https://w3id.org/netbeheer/referentiemodellen/IECCIM/TC57CIM/IEC61970/Base/Domain#Reactance"/>
            </owl:Restriction>
        </rdfs:subClassOf>
        <rdfs:subClassOf>
            <owl:Restriction>
                <owl:onProperty rdf:resource="https://w3id.org/netbeheer/referentiemodellen/IECCIM/TC57CIM/IEC61970/Base/Wires#ACLineSegment_ACLineSegmentPhases"/>
                <owl:qualifiedCardinality rdf:datatype="http://www.w3.org/2001/XMLSchema#nonNegativeInteger">1</owl:qualifiedCardinality>
                <owl:onClass rdf:resource="https://w3id.org/netbeheer/referentiemodellen/IECCIM/TC57CIM/IEC61970/Base/Wires#ACLineSegment"/>
            </owl:Restriction>
        </rdfs:subClassOf>
        <rdfs:subClassOf>
            <owl:Restriction>
                <owl:onProperty rdf:resource="https://w3id.org/netbeheer/referentiemodellen/IECCIM/TC57CIM/IEC61970/Base/Wires#ACLineSegment_Clamp"/>
                <owl:qualifiedCardinality rdf:datatype="http://www.w3.org/2001/XMLSchema#nonNegativeInteger">1</owl:qualifiedCardinality>
                <owl:onClass rdf:resource="https://w3id.org/netbeheer/referentiemodellen/IECCIM/TC57CIM/IEC61970/Base/Wires#ACLineSegment"/>
            </owl:Restriction>
        </rdfs:subClassOf>
        <rdfs:subClassOf>
            <owl:Restriction>
                <owl:onProperty rdf:resource="https://w3id.org/netbeheer/referentiemodellen/IECCIM/TC57CIM/IEC61970/Base/Wires#ACLineSegment_Cut"/>
                <owl:qualifiedCardinality rdf:datatype="http://www.w3.org/2001/XMLSchema#nonNegativeInteger">1</owl:qualifiedCardinality>
                <owl:onClass rdf:resource="https://w3id.org/netbeheer/referentiemodellen/IECCIM/TC57CIM/IEC61970/Base/Wires#ACLineSegment"/>
            </owl:Restriction>
        </rdfs:subClassOf>
        <rdfs:subClassOf>
            <owl:Restriction>
                <owl:onProperty rdf:resource="https://w3id.org/netbeheer/referentiemodellen/IECCIM/TC57CIM/IEC61970/Base/Wires#ACLineSegment_LineGroundingAction"/>
                <owl:maxQualifiedCardinality rdf:datatype="http://www.w3.org/2001/XMLSchema#nonNegativeInteger">1</owl:maxQualifiedCardinality>
                <owl:onClass rdf:resource="https://w3id.org/netbeheer/referentiemodellen/IECCIM/TC57CIM/IEC61970/Base/Wires#ACLineSegment"/>
            </owl:Restriction>
        </rdfs:subClassOf>
        <rdfs:subClassOf>
            <owl:Restriction>
                <owl:onProperty rdf:resource="https://w3id.org/netbeheer/referentiemodellen/IECCIM/TC57CIM/IEC61970/Base/Wires#ACLineSegment_b0ch"/>
                <owl:maxQualifiedCardinality rdf:datatype="http://www.w3.org/2001/XMLSchema#nonNegativeInteger">1</owl:maxQualifiedCardinality>
                <owl:onClass rdf:resource="https://w3id.org/netbeheer/referentiemodellen/IECCIM/TC57CIM/IEC61970/Base/Domain#Susceptance"/>
            </owl:Restriction>
        </rdfs:subClassOf>
        <rdfs:subClassOf>
            <owl:Restriction>
                <owl:onProperty rdf:resource="https://w3id.org/netbeheer/referentiemodellen/IECCIM/TC57CIM/IEC61970/Base/Wires#ACLineSegment_bch"/>
                <owl:maxQualifiedCardinality rdf:datatype="http://www.w3.org/2001/XMLSchema#nonNegativeInteger">1</owl:maxQualifiedCardinality>
                <owl:onClass rdf:resource="https://w3id.org/netbeheer/referentiemodellen/IECCIM/TC57CIM/IEC61970/Base/Domain#Susceptance"/>
            </owl:Restriction>
        </rdfs:subClassOf>
        <rdfs:subClassOf>
            <owl:Restriction>
                <owl:onProperty rdf:resource="https://w3id.org/netbeheer/referentiemodellen/IECCIM/TC57CIM/IEC61970/Base/Wires#ACLineSegment_g0ch"/>
                <owl:maxQualifiedCardinality rdf:datatype="http://www.w3.org/2001/XMLSchema#nonNegativeInteger">1</owl:maxQualifiedCardinality>
                <owl:onClass rdf:resource="https://w3id.org/netbeheer/referentiemodellen/IECCIM/TC57CIM/IEC61970/Base/Domain#Conductance"/>
            </owl:Restriction>
        </rdfs:subClassOf>
        <rdfs:subClassOf>
            <owl:Restriction>
                <owl:onProperty rdf:resource="https://w3id.org/netbeheer/referentiemodellen/IECCIM/TC57CIM/IEC61970/Base/Wires#ACLineSegment_gch"/>
                <owl:maxQualifiedCardinality rdf:datatype="http://www.w3.org/2001/XMLSchema#nonNegativeInteger">1</owl:maxQualifiedCardinality>
                <owl:onClass rdf:resource="https://w3id.org/netbeheer/referentiemodellen/IECCIM/TC57CIM/IEC61970/Base/Domain#Conductance"/>
            </owl:Restriction>
        </rdfs:subClassOf>
        <rdfs:subClassOf>
            <owl:Restriction>
                <owl:onProperty rdf:resource="https://w3id.org/netbeheer/referentiemodellen/IECCIM/TC57CIM/IEC61970/Base/Wires#ACLineSegment_r"/>
                <owl:maxQualifiedCardinality rdf:datatype="http://www.w3.org/2001/XMLSchema#nonNegativeInteger">1</owl:maxQualifiedCardinality>
                <owl:onClass rdf:resource="https://w3id.org/netbeheer/referentiemodellen/IECCIM/TC57CIM/IEC61970/Base/Domain#Resistance"/>
            </owl:Restriction>
        </rdfs:subClassOf>
        <rdfs:subClassOf>
            <owl:Restriction>
                <owl:onProperty rdf:resource="https://w3id.org/netbeheer/referentiemodellen/IECCIM/TC57CIM/IEC61970/Base/Wires#ACLineSegment_r0"/>
                <owl:maxQualifiedCardinality rdf:datatype="http://www.w3.org/2001/XMLSchema#nonNegativeInteger">1</owl:maxQualifiedCardinality>
                <owl:onClass rdf:resource="https://w3id.org/netbeheer/referentiemodellen/IECCIM/TC57CIM/IEC61970/Base/Domain#Resistance"/>
            </owl:Restriction>
        </rdfs:subClassOf>
        <rdfs:subClassOf>
            <owl:Restriction>
                <owl:onProperty rdf:resource="https://w3id.org/netbeheer/referentiemodellen/IECCIM/TC57CIM/IEC61970/Base/Wires#ACLineSegment_shortCircuitEndTemperature"/>
                <owl:maxQualifiedCardinality rdf:datatype="http://www.w3.org/2001/XMLSchema#nonNegativeInteger">1</owl:maxQualifiedCardinality>
                <owl:onClass rdf:resource="https://w3id.org/netbeheer/referentiemodellen/IECCIM/TC57CIM/IEC61970/Base/Domain#Temperature"/>
            </owl:Restriction>
        </rdfs:subClassOf>
        <rdfs:subClassOf>
            <owl:Restriction>
                <owl:onProperty rdf:resource="https://w3id.org/netbeheer/referentiemodellen/IECCIM/TC57CIM/IEC61970/Base/Wires#ACLineSegment_x"/>
                <owl:maxQualifiedCardinality rdf:datatype="http://www.w3.org/2001/XMLSchema#nonNegativeInteger">1</owl:maxQualifiedCardinality>
                <owl:onClass rdf:resource="https://w3id.org/netbeheer/referentiemodellen/IECCIM/TC57CIM/IEC61970/Base/Domain#Reactance"/>
            </owl:Restriction>
        </rdfs:subClassOf>
        <rdfs:subClassOf>
            <owl:Restriction>
                <owl:onProperty rdf:resource="https://w3id.org/netbeheer/referentiemodellen/IECCIM/TC57CIM/IEC61970/Base/Wires#ACLineSegment_x0"/>
                <owl:maxQualifiedCardinality rdf:datatype="http://www.w3.org/2001/XMLSchema#nonNegativeInteger">1</owl:maxQualifiedCardinality>
                <owl:onClass rdf:resource="https://w3id.org/netbeheer/referentiemodellen/IECCIM/TC57CIM/IEC61970/Base/Domain#Reactance"/>
            </owl:Restriction>
        </rdfs:subClassOf>
        <rdfs:comment>A wire or combination of wires, with consistent electrical characteristics, building a single electrical system, used to carry alternating current between points in the power system.
For symmetrical, transposed 3ph lines, it is sufficient to use  attributes of the line segment, which describe impedances and admittances for the entire length of the segment.  Additionally impedances can be computed by using length and associated per length impedances.
The BaseVoltage at the two ends of ACLineSegments in a Line shall have the same BaseVoltage.nominalVoltage. However, boundary lines  may have slightly different BaseVoltage.nominalVoltages and  variation is allowed. Larger voltage difference in general requires use of an equivalent branch.</rdfs:comment>
    </owl:Class>
    


    <!-- https://w3id.org/netbeheer/referentiemodellen/IECCIM/TC57CIM/IEC61970/Base/Wires#ACLineSegmentPhase -->


    <owl:Class rdf:about="https://w3id.org/netbeheer/referentiemodellen/IECCIM/TC57CIM/IEC61970/Base/Wires#ACLineSegmentPhase">
        <rdfs:subClassOf rdf:resource="https://w3id.org/netbeheer/referentiemodellen/IECCIM/TC57CIM/IEC61970/Base/Core#PowerSystemResource"/>
        <rdfs:subClassOf>
            <owl:Restriction>
                <owl:onProperty rdf:resource="https://w3id.org/netbeheer/referentiemodellen/IECCIM/TC57CIM/IEC61970/Base/Wires#ACLineSegmentPhase_ACLineSegment"/>
                <owl:minQualifiedCardinality rdf:datatype="http://www.w3.org/2001/XMLSchema#nonNegativeInteger">0</owl:minQualifiedCardinality>
                <owl:onClass rdf:resource="https://w3id.org/netbeheer/referentiemodellen/IECCIM/TC57CIM/IEC61970/Base/Wires#ACLineSegmentPhase"/>
            </owl:Restriction>
        </rdfs:subClassOf>
        <rdfs:subClassOf>
            <owl:Restriction>
                <owl:onProperty rdf:resource="https://w3id.org/netbeheer/referentiemodellen/IECCIM/TC57CIM/IEC61970/Base/Wires#ACLineSegmentPhase_phase"/>
                <owl:minQualifiedCardinality rdf:datatype="http://www.w3.org/2001/XMLSchema#nonNegativeInteger">0</owl:minQualifiedCardinality>
                <owl:onDataRange rdf:resource="https://w3id.org/netbeheer/referentiemodellen/IECCIM/TC57CIM/IEC61970/Base/Wires#SinglePhaseKind"/>
            </owl:Restriction>
        </rdfs:subClassOf>
        <rdfs:subClassOf>
            <owl:Restriction>
                <owl:onProperty rdf:resource="https://w3id.org/netbeheer/referentiemodellen/IECCIM/TC57CIM/IEC61970/Base/Wires#ACLineSegmentPhase_sequenceNumber"/>
                <owl:minQualifiedCardinality rdf:datatype="http://www.w3.org/2001/XMLSchema#nonNegativeInteger">0</owl:minQualifiedCardinality>
                <owl:onDataRange rdf:resource="http://www.w3.org/2001/XMLSchema#nonNegativeInteger"/>
            </owl:Restriction>
        </rdfs:subClassOf>
        <rdfs:subClassOf>
            <owl:Restriction>
                <owl:onProperty rdf:resource="https://w3id.org/netbeheer/referentiemodellen/IECCIM/TC57CIM/IEC61970/Base/Wires#ACLineSegmentPhase_phase"/>
                <owl:maxQualifiedCardinality rdf:datatype="http://www.w3.org/2001/XMLSchema#nonNegativeInteger">1</owl:maxQualifiedCardinality>
                <owl:onDataRange rdf:resource="https://w3id.org/netbeheer/referentiemodellen/IECCIM/TC57CIM/IEC61970/Base/Wires#SinglePhaseKind"/>
            </owl:Restriction>
        </rdfs:subClassOf>
        <rdfs:subClassOf>
            <owl:Restriction>
                <owl:onProperty rdf:resource="https://w3id.org/netbeheer/referentiemodellen/IECCIM/TC57CIM/IEC61970/Base/Wires#ACLineSegmentPhase_sequenceNumber"/>
                <owl:maxQualifiedCardinality rdf:datatype="http://www.w3.org/2001/XMLSchema#nonNegativeInteger">1</owl:maxQualifiedCardinality>
                <owl:onDataRange rdf:resource="http://www.w3.org/2001/XMLSchema#nonNegativeInteger"/>
            </owl:Restriction>
        </rdfs:subClassOf>
        <rdfs:comment>Represents a single wire of an alternating current line segment.
</rdfs:comment>
    </owl:Class>
    


    <!-- https://w3id.org/netbeheer/referentiemodellen/IECCIM/TC57CIM/IEC61970/Base/Wires#AsynchronousMachine -->


    <owl:Class rdf:about="https://w3id.org/netbeheer/referentiemodellen/IECCIM/TC57CIM/IEC61970/Base/Wires#AsynchronousMachine">
        <rdfs:subClassOf rdf:resource="https://w3id.org/netbeheer/referentiemodellen/IECCIM/TC57CIM/IEC61970/Base/Wires#RotatingMachine"/>
        <rdfs:subClassOf>
            <owl:Restriction>
                <owl:onProperty rdf:resource="https://w3id.org/netbeheer/referentiemodellen/IECCIM/TC57CIM/IEC61970/Base/Wires#AsynchronousMachine_efficiency"/>
                <owl:minQualifiedCardinality rdf:datatype="http://www.w3.org/2001/XMLSchema#nonNegativeInteger">0</owl:minQualifiedCardinality>
                <owl:onClass rdf:resource="https://w3id.org/netbeheer/referentiemodellen/IECCIM/TC57CIM/IEC61970/Base/Domain#PerCent"/>
            </owl:Restriction>
        </rdfs:subClassOf>
        <rdfs:subClassOf>
            <owl:Restriction>
                <owl:onProperty rdf:resource="https://w3id.org/netbeheer/referentiemodellen/IECCIM/TC57CIM/IEC61970/Base/Wires#AsynchronousMachine_nominalFrequency"/>
                <owl:minQualifiedCardinality rdf:datatype="http://www.w3.org/2001/XMLSchema#nonNegativeInteger">0</owl:minQualifiedCardinality>
                <owl:onClass rdf:resource="https://w3id.org/netbeheer/referentiemodellen/IECCIM/TC57CIM/IEC61970/Base/Domain#Frequency"/>
            </owl:Restriction>
        </rdfs:subClassOf>
        <rdfs:subClassOf>
            <owl:Restriction>
                <owl:onProperty rdf:resource="https://w3id.org/netbeheer/referentiemodellen/IECCIM/TC57CIM/IEC61970/Base/Wires#AsynchronousMachine_nominalSpeed"/>
                <owl:minQualifiedCardinality rdf:datatype="http://www.w3.org/2001/XMLSchema#nonNegativeInteger">0</owl:minQualifiedCardinality>
                <owl:onClass rdf:resource="https://w3id.org/netbeheer/referentiemodellen/IECCIM/TC57CIM/IEC61970/Base/Domain#RotationSpeed"/>
            </owl:Restriction>
        </rdfs:subClassOf>
        <rdfs:subClassOf>
            <owl:Restriction>
                <owl:onProperty rdf:resource="https://w3id.org/netbeheer/referentiemodellen/IECCIM/TC57CIM/IEC61970/Base/Wires#AsynchronousMachine_ratedMechanicalPower"/>
                <owl:minQualifiedCardinality rdf:datatype="http://www.w3.org/2001/XMLSchema#nonNegativeInteger">0</owl:minQualifiedCardinality>
                <owl:onClass rdf:resource="https://w3id.org/netbeheer/referentiemodellen/IECCIM/TC57CIM/IEC61970/Base/Domain#ActivePower"/>
            </owl:Restriction>
        </rdfs:subClassOf>
        <rdfs:subClassOf>
            <owl:Restriction>
                <owl:onProperty rdf:resource="https://w3id.org/netbeheer/referentiemodellen/IECCIM/TC57CIM/IEC61970/Base/Wires#AsynchronousMachine_rr1"/>
                <owl:minQualifiedCardinality rdf:datatype="http://www.w3.org/2001/XMLSchema#nonNegativeInteger">0</owl:minQualifiedCardinality>
                <owl:onClass rdf:resource="https://w3id.org/netbeheer/referentiemodellen/IECCIM/TC57CIM/IEC61970/Base/Domain#Resistance"/>
            </owl:Restriction>
        </rdfs:subClassOf>
        <rdfs:subClassOf>
            <owl:Restriction>
                <owl:onProperty rdf:resource="https://w3id.org/netbeheer/referentiemodellen/IECCIM/TC57CIM/IEC61970/Base/Wires#AsynchronousMachine_rr2"/>
                <owl:minQualifiedCardinality rdf:datatype="http://www.w3.org/2001/XMLSchema#nonNegativeInteger">0</owl:minQualifiedCardinality>
                <owl:onClass rdf:resource="https://w3id.org/netbeheer/referentiemodellen/IECCIM/TC57CIM/IEC61970/Base/Domain#Resistance"/>
            </owl:Restriction>
        </rdfs:subClassOf>
        <rdfs:subClassOf>
            <owl:Restriction>
                <owl:onProperty rdf:resource="https://w3id.org/netbeheer/referentiemodellen/IECCIM/TC57CIM/IEC61970/Base/Wires#AsynchronousMachine_tpo"/>
                <owl:minQualifiedCardinality rdf:datatype="http://www.w3.org/2001/XMLSchema#nonNegativeInteger">0</owl:minQualifiedCardinality>
                <owl:onClass rdf:resource="https://w3id.org/netbeheer/referentiemodellen/IECCIM/TC57CIM/IEC61970/Base/Domain#Seconds"/>
            </owl:Restriction>
        </rdfs:subClassOf>
        <rdfs:subClassOf>
            <owl:Restriction>
                <owl:onProperty rdf:resource="https://w3id.org/netbeheer/referentiemodellen/IECCIM/TC57CIM/IEC61970/Base/Wires#AsynchronousMachine_tppo"/>
                <owl:minQualifiedCardinality rdf:datatype="http://www.w3.org/2001/XMLSchema#nonNegativeInteger">0</owl:minQualifiedCardinality>
                <owl:onClass rdf:resource="https://w3id.org/netbeheer/referentiemodellen/IECCIM/TC57CIM/IEC61970/Base/Domain#Seconds"/>
            </owl:Restriction>
        </rdfs:subClassOf>
        <rdfs:subClassOf>
            <owl:Restriction>
                <owl:onProperty rdf:resource="https://w3id.org/netbeheer/referentiemodellen/IECCIM/TC57CIM/IEC61970/Base/Wires#AsynchronousMachine_xlr1"/>
                <owl:minQualifiedCardinality rdf:datatype="http://www.w3.org/2001/XMLSchema#nonNegativeInteger">0</owl:minQualifiedCardinality>
                <owl:onClass rdf:resource="https://w3id.org/netbeheer/referentiemodellen/IECCIM/TC57CIM/IEC61970/Base/Domain#Reactance"/>
            </owl:Restriction>
        </rdfs:subClassOf>
        <rdfs:subClassOf>
            <owl:Restriction>
                <owl:onProperty rdf:resource="https://w3id.org/netbeheer/referentiemodellen/IECCIM/TC57CIM/IEC61970/Base/Wires#AsynchronousMachine_xlr2"/>
                <owl:minQualifiedCardinality rdf:datatype="http://www.w3.org/2001/XMLSchema#nonNegativeInteger">0</owl:minQualifiedCardinality>
                <owl:onClass rdf:resource="https://w3id.org/netbeheer/referentiemodellen/IECCIM/TC57CIM/IEC61970/Base/Domain#Reactance"/>
            </owl:Restriction>
        </rdfs:subClassOf>
        <rdfs:subClassOf>
            <owl:Restriction>
                <owl:onProperty rdf:resource="https://w3id.org/netbeheer/referentiemodellen/IECCIM/TC57CIM/IEC61970/Base/Wires#AsynchronousMachine_xm"/>
                <owl:minQualifiedCardinality rdf:datatype="http://www.w3.org/2001/XMLSchema#nonNegativeInteger">0</owl:minQualifiedCardinality>
                <owl:onClass rdf:resource="https://w3id.org/netbeheer/referentiemodellen/IECCIM/TC57CIM/IEC61970/Base/Domain#Reactance"/>
            </owl:Restriction>
        </rdfs:subClassOf>
        <rdfs:subClassOf>
            <owl:Restriction>
                <owl:onProperty rdf:resource="https://w3id.org/netbeheer/referentiemodellen/IECCIM/TC57CIM/IEC61970/Base/Wires#AsynchronousMachine_xp"/>
                <owl:minQualifiedCardinality rdf:datatype="http://www.w3.org/2001/XMLSchema#nonNegativeInteger">0</owl:minQualifiedCardinality>
                <owl:onClass rdf:resource="https://w3id.org/netbeheer/referentiemodellen/IECCIM/TC57CIM/IEC61970/Base/Domain#Reactance"/>
            </owl:Restriction>
        </rdfs:subClassOf>
        <rdfs:subClassOf>
            <owl:Restriction>
                <owl:onProperty rdf:resource="https://w3id.org/netbeheer/referentiemodellen/IECCIM/TC57CIM/IEC61970/Base/Wires#AsynchronousMachine_xpp"/>
                <owl:minQualifiedCardinality rdf:datatype="http://www.w3.org/2001/XMLSchema#nonNegativeInteger">0</owl:minQualifiedCardinality>
                <owl:onClass rdf:resource="https://w3id.org/netbeheer/referentiemodellen/IECCIM/TC57CIM/IEC61970/Base/Domain#Reactance"/>
            </owl:Restriction>
        </rdfs:subClassOf>
        <rdfs:subClassOf>
            <owl:Restriction>
                <owl:onProperty rdf:resource="https://w3id.org/netbeheer/referentiemodellen/IECCIM/TC57CIM/IEC61970/Base/Wires#AsynchronousMachine_xs"/>
                <owl:minQualifiedCardinality rdf:datatype="http://www.w3.org/2001/XMLSchema#nonNegativeInteger">0</owl:minQualifiedCardinality>
                <owl:onClass rdf:resource="https://w3id.org/netbeheer/referentiemodellen/IECCIM/TC57CIM/IEC61970/Base/Domain#Reactance"/>
            </owl:Restriction>
        </rdfs:subClassOf>
        <rdfs:subClassOf>
            <owl:Restriction>
                <owl:onProperty rdf:resource="https://w3id.org/netbeheer/referentiemodellen/IECCIM/TC57CIM/IEC61970/Base/Wires#AsynchronousMachine_AsynchronousMachineDynamics"/>
                <owl:qualifiedCardinality rdf:datatype="http://www.w3.org/2001/XMLSchema#nonNegativeInteger">1</owl:qualifiedCardinality>
                <owl:onClass rdf:resource="https://w3id.org/netbeheer/referentiemodellen/IECCIM/TC57CIM/IEC61970/Base/Wires#AsynchronousMachine"/>
            </owl:Restriction>
        </rdfs:subClassOf>
        <rdfs:subClassOf>
            <owl:Restriction>
                <owl:onProperty rdf:resource="https://w3id.org/netbeheer/referentiemodellen/IECCIM/TC57CIM/IEC61970/Base/Wires#AsynchronousMachine_efficiency"/>
                <owl:maxQualifiedCardinality rdf:datatype="http://www.w3.org/2001/XMLSchema#nonNegativeInteger">1</owl:maxQualifiedCardinality>
                <owl:onClass rdf:resource="https://w3id.org/netbeheer/referentiemodellen/IECCIM/TC57CIM/IEC61970/Base/Domain#PerCent"/>
            </owl:Restriction>
        </rdfs:subClassOf>
        <rdfs:subClassOf>
            <owl:Restriction>
                <owl:onProperty rdf:resource="https://w3id.org/netbeheer/referentiemodellen/IECCIM/TC57CIM/IEC61970/Base/Wires#AsynchronousMachine_nominalFrequency"/>
                <owl:maxQualifiedCardinality rdf:datatype="http://www.w3.org/2001/XMLSchema#nonNegativeInteger">1</owl:maxQualifiedCardinality>
                <owl:onClass rdf:resource="https://w3id.org/netbeheer/referentiemodellen/IECCIM/TC57CIM/IEC61970/Base/Domain#Frequency"/>
            </owl:Restriction>
        </rdfs:subClassOf>
        <rdfs:subClassOf>
            <owl:Restriction>
                <owl:onProperty rdf:resource="https://w3id.org/netbeheer/referentiemodellen/IECCIM/TC57CIM/IEC61970/Base/Wires#AsynchronousMachine_nominalSpeed"/>
                <owl:maxQualifiedCardinality rdf:datatype="http://www.w3.org/2001/XMLSchema#nonNegativeInteger">1</owl:maxQualifiedCardinality>
                <owl:onClass rdf:resource="https://w3id.org/netbeheer/referentiemodellen/IECCIM/TC57CIM/IEC61970/Base/Domain#RotationSpeed"/>
            </owl:Restriction>
        </rdfs:subClassOf>
        <rdfs:subClassOf>
            <owl:Restriction>
                <owl:onProperty rdf:resource="https://w3id.org/netbeheer/referentiemodellen/IECCIM/TC57CIM/IEC61970/Base/Wires#AsynchronousMachine_ratedMechanicalPower"/>
                <owl:maxQualifiedCardinality rdf:datatype="http://www.w3.org/2001/XMLSchema#nonNegativeInteger">1</owl:maxQualifiedCardinality>
                <owl:onClass rdf:resource="https://w3id.org/netbeheer/referentiemodellen/IECCIM/TC57CIM/IEC61970/Base/Domain#ActivePower"/>
            </owl:Restriction>
        </rdfs:subClassOf>
        <rdfs:subClassOf>
            <owl:Restriction>
                <owl:onProperty rdf:resource="https://w3id.org/netbeheer/referentiemodellen/IECCIM/TC57CIM/IEC61970/Base/Wires#AsynchronousMachine_rr1"/>
                <owl:maxQualifiedCardinality rdf:datatype="http://www.w3.org/2001/XMLSchema#nonNegativeInteger">1</owl:maxQualifiedCardinality>
                <owl:onClass rdf:resource="https://w3id.org/netbeheer/referentiemodellen/IECCIM/TC57CIM/IEC61970/Base/Domain#Resistance"/>
            </owl:Restriction>
        </rdfs:subClassOf>
        <rdfs:subClassOf>
            <owl:Restriction>
                <owl:onProperty rdf:resource="https://w3id.org/netbeheer/referentiemodellen/IECCIM/TC57CIM/IEC61970/Base/Wires#AsynchronousMachine_rr2"/>
                <owl:maxQualifiedCardinality rdf:datatype="http://www.w3.org/2001/XMLSchema#nonNegativeInteger">1</owl:maxQualifiedCardinality>
                <owl:onClass rdf:resource="https://w3id.org/netbeheer/referentiemodellen/IECCIM/TC57CIM/IEC61970/Base/Domain#Resistance"/>
            </owl:Restriction>
        </rdfs:subClassOf>
        <rdfs:subClassOf>
            <owl:Restriction>
                <owl:onProperty rdf:resource="https://w3id.org/netbeheer/referentiemodellen/IECCIM/TC57CIM/IEC61970/Base/Wires#AsynchronousMachine_tpo"/>
                <owl:maxQualifiedCardinality rdf:datatype="http://www.w3.org/2001/XMLSchema#nonNegativeInteger">1</owl:maxQualifiedCardinality>
                <owl:onClass rdf:resource="https://w3id.org/netbeheer/referentiemodellen/IECCIM/TC57CIM/IEC61970/Base/Domain#Seconds"/>
            </owl:Restriction>
        </rdfs:subClassOf>
        <rdfs:subClassOf>
            <owl:Restriction>
                <owl:onProperty rdf:resource="https://w3id.org/netbeheer/referentiemodellen/IECCIM/TC57CIM/IEC61970/Base/Wires#AsynchronousMachine_tppo"/>
                <owl:maxQualifiedCardinality rdf:datatype="http://www.w3.org/2001/XMLSchema#nonNegativeInteger">1</owl:maxQualifiedCardinality>
                <owl:onClass rdf:resource="https://w3id.org/netbeheer/referentiemodellen/IECCIM/TC57CIM/IEC61970/Base/Domain#Seconds"/>
            </owl:Restriction>
        </rdfs:subClassOf>
        <rdfs:subClassOf>
            <owl:Restriction>
                <owl:onProperty rdf:resource="https://w3id.org/netbeheer/referentiemodellen/IECCIM/TC57CIM/IEC61970/Base/Wires#AsynchronousMachine_xlr1"/>
                <owl:maxQualifiedCardinality rdf:datatype="http://www.w3.org/2001/XMLSchema#nonNegativeInteger">1</owl:maxQualifiedCardinality>
                <owl:onClass rdf:resource="https://w3id.org/netbeheer/referentiemodellen/IECCIM/TC57CIM/IEC61970/Base/Domain#Reactance"/>
            </owl:Restriction>
        </rdfs:subClassOf>
        <rdfs:subClassOf>
            <owl:Restriction>
                <owl:onProperty rdf:resource="https://w3id.org/netbeheer/referentiemodellen/IECCIM/TC57CIM/IEC61970/Base/Wires#AsynchronousMachine_xlr2"/>
                <owl:maxQualifiedCardinality rdf:datatype="http://www.w3.org/2001/XMLSchema#nonNegativeInteger">1</owl:maxQualifiedCardinality>
                <owl:onClass rdf:resource="https://w3id.org/netbeheer/referentiemodellen/IECCIM/TC57CIM/IEC61970/Base/Domain#Reactance"/>
            </owl:Restriction>
        </rdfs:subClassOf>
        <rdfs:subClassOf>
            <owl:Restriction>
                <owl:onProperty rdf:resource="https://w3id.org/netbeheer/referentiemodellen/IECCIM/TC57CIM/IEC61970/Base/Wires#AsynchronousMachine_xm"/>
                <owl:maxQualifiedCardinality rdf:datatype="http://www.w3.org/2001/XMLSchema#nonNegativeInteger">1</owl:maxQualifiedCardinality>
                <owl:onClass rdf:resource="https://w3id.org/netbeheer/referentiemodellen/IECCIM/TC57CIM/IEC61970/Base/Domain#Reactance"/>
            </owl:Restriction>
        </rdfs:subClassOf>
        <rdfs:subClassOf>
            <owl:Restriction>
                <owl:onProperty rdf:resource="https://w3id.org/netbeheer/referentiemodellen/IECCIM/TC57CIM/IEC61970/Base/Wires#AsynchronousMachine_xp"/>
                <owl:maxQualifiedCardinality rdf:datatype="http://www.w3.org/2001/XMLSchema#nonNegativeInteger">1</owl:maxQualifiedCardinality>
                <owl:onClass rdf:resource="https://w3id.org/netbeheer/referentiemodellen/IECCIM/TC57CIM/IEC61970/Base/Domain#Reactance"/>
            </owl:Restriction>
        </rdfs:subClassOf>
        <rdfs:subClassOf>
            <owl:Restriction>
                <owl:onProperty rdf:resource="https://w3id.org/netbeheer/referentiemodellen/IECCIM/TC57CIM/IEC61970/Base/Wires#AsynchronousMachine_xpp"/>
                <owl:maxQualifiedCardinality rdf:datatype="http://www.w3.org/2001/XMLSchema#nonNegativeInteger">1</owl:maxQualifiedCardinality>
                <owl:onClass rdf:resource="https://w3id.org/netbeheer/referentiemodellen/IECCIM/TC57CIM/IEC61970/Base/Domain#Reactance"/>
            </owl:Restriction>
        </rdfs:subClassOf>
        <rdfs:subClassOf>
            <owl:Restriction>
                <owl:onProperty rdf:resource="https://w3id.org/netbeheer/referentiemodellen/IECCIM/TC57CIM/IEC61970/Base/Wires#AsynchronousMachine_xs"/>
                <owl:maxQualifiedCardinality rdf:datatype="http://www.w3.org/2001/XMLSchema#nonNegativeInteger">1</owl:maxQualifiedCardinality>
                <owl:onClass rdf:resource="https://w3id.org/netbeheer/referentiemodellen/IECCIM/TC57CIM/IEC61970/Base/Domain#Reactance"/>
            </owl:Restriction>
        </rdfs:subClassOf>
        <rdfs:subClassOf>
            <owl:Restriction>
                <owl:onProperty rdf:resource="https://w3id.org/netbeheer/referentiemodellen/IECCIM/TC57CIM/IEC61970/Base/Wires#AsynchronousMachine_asynchronousMachineType"/>
                <owl:minQualifiedCardinality rdf:datatype="http://www.w3.org/2001/XMLSchema#nonNegativeInteger">0</owl:minQualifiedCardinality>
                <owl:onDataRange rdf:resource="https://w3id.org/netbeheer/referentiemodellen/IECCIM/TC57CIM/IEC61970/Base/Wires#AsynchronousMachineKind"/>
            </owl:Restriction>
        </rdfs:subClassOf>
        <rdfs:subClassOf>
            <owl:Restriction>
                <owl:onProperty rdf:resource="https://w3id.org/netbeheer/referentiemodellen/IECCIM/TC57CIM/IEC61970/Base/Wires#AsynchronousMachine_converterFedDrive"/>
                <owl:minQualifiedCardinality rdf:datatype="http://www.w3.org/2001/XMLSchema#nonNegativeInteger">0</owl:minQualifiedCardinality>
                <owl:onDataRange rdf:resource="http://www.w3.org/2001/XMLSchema#boolean"/>
            </owl:Restriction>
        </rdfs:subClassOf>
        <rdfs:subClassOf>
            <owl:Restriction>
                <owl:onProperty rdf:resource="https://w3id.org/netbeheer/referentiemodellen/IECCIM/TC57CIM/IEC61970/Base/Wires#AsynchronousMachine_iaIrRatio"/>
                <owl:minQualifiedCardinality rdf:datatype="http://www.w3.org/2001/XMLSchema#nonNegativeInteger">0</owl:minQualifiedCardinality>
                <owl:onDataRange rdf:resource="http://www.w3.org/2001/XMLSchema#float"/>
            </owl:Restriction>
        </rdfs:subClassOf>
        <rdfs:subClassOf>
            <owl:Restriction>
                <owl:onProperty rdf:resource="https://w3id.org/netbeheer/referentiemodellen/IECCIM/TC57CIM/IEC61970/Base/Wires#AsynchronousMachine_polePairNumber"/>
                <owl:minQualifiedCardinality rdf:datatype="http://www.w3.org/2001/XMLSchema#nonNegativeInteger">0</owl:minQualifiedCardinality>
                <owl:onDataRange rdf:resource="http://www.w3.org/2001/XMLSchema#nonNegativeInteger"/>
            </owl:Restriction>
        </rdfs:subClassOf>
        <rdfs:subClassOf>
            <owl:Restriction>
                <owl:onProperty rdf:resource="https://w3id.org/netbeheer/referentiemodellen/IECCIM/TC57CIM/IEC61970/Base/Wires#AsynchronousMachine_reversible"/>
                <owl:minQualifiedCardinality rdf:datatype="http://www.w3.org/2001/XMLSchema#nonNegativeInteger">0</owl:minQualifiedCardinality>
                <owl:onDataRange rdf:resource="http://www.w3.org/2001/XMLSchema#boolean"/>
            </owl:Restriction>
        </rdfs:subClassOf>
        <rdfs:subClassOf>
            <owl:Restriction>
                <owl:onProperty rdf:resource="https://w3id.org/netbeheer/referentiemodellen/IECCIM/TC57CIM/IEC61970/Base/Wires#AsynchronousMachine_rxLockedRotorRatio"/>
                <owl:minQualifiedCardinality rdf:datatype="http://www.w3.org/2001/XMLSchema#nonNegativeInteger">0</owl:minQualifiedCardinality>
                <owl:onDataRange rdf:resource="http://www.w3.org/2001/XMLSchema#float"/>
            </owl:Restriction>
        </rdfs:subClassOf>
        <rdfs:subClassOf>
            <owl:Restriction>
                <owl:onProperty rdf:resource="https://w3id.org/netbeheer/referentiemodellen/IECCIM/TC57CIM/IEC61970/Base/Wires#AsynchronousMachine_asynchronousMachineType"/>
                <owl:maxQualifiedCardinality rdf:datatype="http://www.w3.org/2001/XMLSchema#nonNegativeInteger">1</owl:maxQualifiedCardinality>
                <owl:onDataRange rdf:resource="https://w3id.org/netbeheer/referentiemodellen/IECCIM/TC57CIM/IEC61970/Base/Wires#AsynchronousMachineKind"/>
            </owl:Restriction>
        </rdfs:subClassOf>
        <rdfs:subClassOf>
            <owl:Restriction>
                <owl:onProperty rdf:resource="https://w3id.org/netbeheer/referentiemodellen/IECCIM/TC57CIM/IEC61970/Base/Wires#AsynchronousMachine_converterFedDrive"/>
                <owl:maxQualifiedCardinality rdf:datatype="http://www.w3.org/2001/XMLSchema#nonNegativeInteger">1</owl:maxQualifiedCardinality>
                <owl:onDataRange rdf:resource="http://www.w3.org/2001/XMLSchema#boolean"/>
            </owl:Restriction>
        </rdfs:subClassOf>
        <rdfs:subClassOf>
            <owl:Restriction>
                <owl:onProperty rdf:resource="https://w3id.org/netbeheer/referentiemodellen/IECCIM/TC57CIM/IEC61970/Base/Wires#AsynchronousMachine_iaIrRatio"/>
                <owl:maxQualifiedCardinality rdf:datatype="http://www.w3.org/2001/XMLSchema#nonNegativeInteger">1</owl:maxQualifiedCardinality>
                <owl:onDataRange rdf:resource="http://www.w3.org/2001/XMLSchema#float"/>
            </owl:Restriction>
        </rdfs:subClassOf>
        <rdfs:subClassOf>
            <owl:Restriction>
                <owl:onProperty rdf:resource="https://w3id.org/netbeheer/referentiemodellen/IECCIM/TC57CIM/IEC61970/Base/Wires#AsynchronousMachine_polePairNumber"/>
                <owl:maxQualifiedCardinality rdf:datatype="http://www.w3.org/2001/XMLSchema#nonNegativeInteger">1</owl:maxQualifiedCardinality>
                <owl:onDataRange rdf:resource="http://www.w3.org/2001/XMLSchema#nonNegativeInteger"/>
            </owl:Restriction>
        </rdfs:subClassOf>
        <rdfs:subClassOf>
            <owl:Restriction>
                <owl:onProperty rdf:resource="https://w3id.org/netbeheer/referentiemodellen/IECCIM/TC57CIM/IEC61970/Base/Wires#AsynchronousMachine_reversible"/>
                <owl:maxQualifiedCardinality rdf:datatype="http://www.w3.org/2001/XMLSchema#nonNegativeInteger">1</owl:maxQualifiedCardinality>
                <owl:onDataRange rdf:resource="http://www.w3.org/2001/XMLSchema#boolean"/>
            </owl:Restriction>
        </rdfs:subClassOf>
        <rdfs:subClassOf>
            <owl:Restriction>
                <owl:onProperty rdf:resource="https://w3id.org/netbeheer/referentiemodellen/IECCIM/TC57CIM/IEC61970/Base/Wires#AsynchronousMachine_rxLockedRotorRatio"/>
                <owl:maxQualifiedCardinality rdf:datatype="http://www.w3.org/2001/XMLSchema#nonNegativeInteger">1</owl:maxQualifiedCardinality>
                <owl:onDataRange rdf:resource="http://www.w3.org/2001/XMLSchema#float"/>
            </owl:Restriction>
        </rdfs:subClassOf>
        <rdfs:comment>A rotating machine whose shaft rotates asynchronously with the electrical field.  Also known as an induction machine with no external connection to the rotor windings, e.g squirrel-cage induction machine.</rdfs:comment>
    </owl:Class>
    


    <!-- https://w3id.org/netbeheer/referentiemodellen/IECCIM/TC57CIM/IEC61970/Base/Wires#Breaker -->


    <owl:Class rdf:about="https://w3id.org/netbeheer/referentiemodellen/IECCIM/TC57CIM/IEC61970/Base/Wires#Breaker">
        <rdfs:subClassOf rdf:resource="https://w3id.org/netbeheer/referentiemodellen/IECCIM/TC57CIM/IEC61970/Base/Wires#ProtectedSwitch"/>
        <rdfs:subClassOf>
            <owl:Restriction>
                <owl:onProperty rdf:resource="https://w3id.org/netbeheer/referentiemodellen/IECCIM/TC57CIM/IEC61970/Base/Wires#Breaker_inTransitTime"/>
                <owl:minQualifiedCardinality rdf:datatype="http://www.w3.org/2001/XMLSchema#nonNegativeInteger">0</owl:minQualifiedCardinality>
                <owl:onClass rdf:resource="https://w3id.org/netbeheer/referentiemodellen/IECCIM/TC57CIM/IEC61970/Base/Domain#Seconds"/>
            </owl:Restriction>
        </rdfs:subClassOf>
        <rdfs:subClassOf>
            <owl:Restriction>
                <owl:onProperty rdf:resource="https://w3id.org/netbeheer/referentiemodellen/IECCIM/TC57CIM/IEC61970/Base/Wires#Breaker_inTransitTime"/>
                <owl:maxQualifiedCardinality rdf:datatype="http://www.w3.org/2001/XMLSchema#nonNegativeInteger">1</owl:maxQualifiedCardinality>
                <owl:onClass rdf:resource="https://w3id.org/netbeheer/referentiemodellen/IECCIM/TC57CIM/IEC61970/Base/Domain#Seconds"/>
            </owl:Restriction>
        </rdfs:subClassOf>
        <rdfs:comment>A mechanical switching device capable of making, carrying, and breaking currents under normal circuit conditions and also making, carrying for a specified time, and breaking currents under specified abnormal circuit conditions e.g.  those of short circuit.</rdfs:comment>
    </owl:Class>
    


    <!-- https://w3id.org/netbeheer/referentiemodellen/IECCIM/TC57CIM/IEC61970/Base/Wires#BusbarSection -->


    <owl:Class rdf:about="https://w3id.org/netbeheer/referentiemodellen/IECCIM/TC57CIM/IEC61970/Base/Wires#BusbarSection">
        <rdfs:subClassOf rdf:resource="https://w3id.org/netbeheer/referentiemodellen/IECCIM/TC57CIM/IEC61970/Base/Wires#Connector"/>
        <rdfs:subClassOf>
            <owl:Restriction>
                <owl:onProperty rdf:resource="https://w3id.org/netbeheer/referentiemodellen/IECCIM/TC57CIM/IEC61970/Base/Wires#BusbarSection_ipMax"/>
                <owl:minQualifiedCardinality rdf:datatype="http://www.w3.org/2001/XMLSchema#nonNegativeInteger">0</owl:minQualifiedCardinality>
                <owl:onClass rdf:resource="https://w3id.org/netbeheer/referentiemodellen/IECCIM/TC57CIM/IEC61970/Base/Domain#CurrentFlow"/>
            </owl:Restriction>
        </rdfs:subClassOf>
        <rdfs:subClassOf>
            <owl:Restriction>
                <owl:onProperty rdf:resource="https://w3id.org/netbeheer/referentiemodellen/IECCIM/TC57CIM/IEC61970/Base/Wires#BusbarSection_VoltageControlZone"/>
                <owl:qualifiedCardinality rdf:datatype="http://www.w3.org/2001/XMLSchema#nonNegativeInteger">1</owl:qualifiedCardinality>
                <owl:onClass rdf:resource="https://w3id.org/netbeheer/referentiemodellen/IECCIM/TC57CIM/IEC61970/Base/Wires#BusbarSection"/>
            </owl:Restriction>
        </rdfs:subClassOf>
        <rdfs:subClassOf>
            <owl:Restriction>
                <owl:onProperty rdf:resource="https://w3id.org/netbeheer/referentiemodellen/IECCIM/TC57CIM/IEC61970/Base/Wires#BusbarSection_ipMax"/>
                <owl:maxQualifiedCardinality rdf:datatype="http://www.w3.org/2001/XMLSchema#nonNegativeInteger">1</owl:maxQualifiedCardinality>
                <owl:onClass rdf:resource="https://w3id.org/netbeheer/referentiemodellen/IECCIM/TC57CIM/IEC61970/Base/Domain#CurrentFlow"/>
            </owl:Restriction>
        </rdfs:subClassOf>
        <rdfs:comment>A conductor, or group of conductors, with negligible impedance, that serve to connect other conducting equipment within a single substation. 
Voltage measurements are typically obtained from VoltageTransformers that are connected to busbar sections. A bus bar section may have many physical terminals but for analysis is modelled with exactly one logical terminal.</rdfs:comment>
    </owl:Class>
    


    <!-- https://w3id.org/netbeheer/referentiemodellen/IECCIM/TC57CIM/IEC61970/Base/Wires#Clamp -->


    <owl:Class rdf:about="https://w3id.org/netbeheer/referentiemodellen/IECCIM/TC57CIM/IEC61970/Base/Wires#Clamp">
        <rdfs:subClassOf rdf:resource="https://w3id.org/netbeheer/referentiemodellen/IECCIM/TC57CIM/IEC61970/Base/Core#ConductingEquipment"/>
        <rdfs:subClassOf>
            <owl:Restriction>
                <owl:onProperty rdf:resource="https://w3id.org/netbeheer/referentiemodellen/IECCIM/TC57CIM/IEC61970/Base/Wires#Clamp_ACLineSegment"/>
                <owl:minQualifiedCardinality rdf:datatype="http://www.w3.org/2001/XMLSchema#nonNegativeInteger">0</owl:minQualifiedCardinality>
                <owl:onClass rdf:resource="https://w3id.org/netbeheer/referentiemodellen/IECCIM/TC57CIM/IEC61970/Base/Wires#Clamp"/>
            </owl:Restriction>
        </rdfs:subClassOf>
        <rdfs:subClassOf>
            <owl:Restriction>
                <owl:onProperty rdf:resource="https://w3id.org/netbeheer/referentiemodellen/IECCIM/TC57CIM/IEC61970/Base/Wires#Clamp_lengthFromTerminal1"/>
                <owl:minQualifiedCardinality rdf:datatype="http://www.w3.org/2001/XMLSchema#nonNegativeInteger">0</owl:minQualifiedCardinality>
                <owl:onClass rdf:resource="https://w3id.org/netbeheer/referentiemodellen/IECCIM/TC57CIM/IEC61970/Base/Domain#Length"/>
            </owl:Restriction>
        </rdfs:subClassOf>
        <rdfs:subClassOf>
            <owl:Restriction>
                <owl:onProperty rdf:resource="https://w3id.org/netbeheer/referentiemodellen/IECCIM/TC57CIM/IEC61970/Base/Wires#Clamp_lengthFromTerminal1"/>
                <owl:maxQualifiedCardinality rdf:datatype="http://www.w3.org/2001/XMLSchema#nonNegativeInteger">1</owl:maxQualifiedCardinality>
                <owl:onClass rdf:resource="https://w3id.org/netbeheer/referentiemodellen/IECCIM/TC57CIM/IEC61970/Base/Domain#Length"/>
            </owl:Restriction>
        </rdfs:subClassOf>
        <rdfs:comment>A Clamp is a galvanic connection at a line segment where other equipment is connected. A Clamp does not cut the line segment. 
A Clamp is ConductingEquipment and has one Terminal with an associated ConnectivityNode. Any other ConductingEquipment can be connected to the Clamp ConnectivityNode.
</rdfs:comment>
    </owl:Class>
    


    <!-- https://w3id.org/netbeheer/referentiemodellen/IECCIM/TC57CIM/IEC61970/Base/Wires#CompositeSwitch -->


    <owl:Class rdf:about="https://w3id.org/netbeheer/referentiemodellen/IECCIM/TC57CIM/IEC61970/Base/Wires#CompositeSwitch">
        <rdfs:subClassOf rdf:resource="https://w3id.org/netbeheer/referentiemodellen/IECCIM/TC57CIM/IEC61970/Base/Core#Equipment"/>
        <rdfs:subClassOf>
            <owl:Restriction>
                <owl:onProperty rdf:resource="https://w3id.org/netbeheer/referentiemodellen/IECCIM/TC57CIM/IEC61970/Base/Wires#CompositeSwitch_Switches"/>
                <owl:minQualifiedCardinality rdf:datatype="http://www.w3.org/2001/XMLSchema#nonNegativeInteger">0</owl:minQualifiedCardinality>
                <owl:onClass rdf:resource="https://w3id.org/netbeheer/referentiemodellen/IECCIM/TC57CIM/IEC61970/Base/Wires#CompositeSwitch"/>
            </owl:Restriction>
        </rdfs:subClassOf>
        <rdfs:subClassOf>
            <owl:Restriction>
                <owl:onProperty rdf:resource="https://w3id.org/netbeheer/referentiemodellen/IECCIM/TC57CIM/IEC61970/Base/Wires#CompositeSwitch_Switches"/>
                <owl:maxQualifiedCardinality rdf:datatype="http://www.w3.org/2001/XMLSchema#nonNegativeInteger">1</owl:maxQualifiedCardinality>
                <owl:onClass rdf:resource="https://w3id.org/netbeheer/referentiemodellen/IECCIM/TC57CIM/IEC61970/Base/Wires#CompositeSwitch"/>
            </owl:Restriction>
        </rdfs:subClassOf>
        <rdfs:subClassOf>
            <owl:Restriction>
                <owl:onProperty rdf:resource="https://w3id.org/netbeheer/referentiemodellen/IECCIM/TC57CIM/IEC61970/Base/Wires#CompositeSwitch_compositeSwitchType"/>
                <owl:minQualifiedCardinality rdf:datatype="http://www.w3.org/2001/XMLSchema#nonNegativeInteger">0</owl:minQualifiedCardinality>
                <owl:onDataRange rdf:resource="http://www.w3.org/2001/XMLSchema#string"/>
            </owl:Restriction>
        </rdfs:subClassOf>
        <rdfs:subClassOf>
            <owl:Restriction>
                <owl:onProperty rdf:resource="https://w3id.org/netbeheer/referentiemodellen/IECCIM/TC57CIM/IEC61970/Base/Wires#CompositeSwitch_compositeSwitchType"/>
                <owl:maxQualifiedCardinality rdf:datatype="http://www.w3.org/2001/XMLSchema#nonNegativeInteger">1</owl:maxQualifiedCardinality>
                <owl:onDataRange rdf:resource="http://www.w3.org/2001/XMLSchema#string"/>
            </owl:Restriction>
        </rdfs:subClassOf>
        <rdfs:comment>A model of a set of individual Switches normally enclosed within the same cabinet and possibly with interlocks that restrict the combination of switch positions. These are typically found in medium voltage distribution networks. 
A CompositeSwitch could represent a Ring-Main-Unit (RMU), or pad-mounted switchgear, with primitive internal devices such as an internal bus-bar plus 3 or 4 internal switches each of which may individually be open or closed. A CompositeSwitch and a set of contained Switches can also be used to represent a multi-position switch e.g. a switch that can connect a circuit to Ground, Open or Busbar.</rdfs:comment>
    </owl:Class>
    


    <!-- https://w3id.org/netbeheer/referentiemodellen/IECCIM/TC57CIM/IEC61970/Base/Wires#Conductor -->


    <owl:Class rdf:about="https://w3id.org/netbeheer/referentiemodellen/IECCIM/TC57CIM/IEC61970/Base/Wires#Conductor">
        <rdfs:subClassOf rdf:resource="https://w3id.org/netbeheer/referentiemodellen/IECCIM/TC57CIM/IEC61970/Base/Core#ConductingEquipment"/>
        <rdfs:subClassOf>
            <owl:Restriction>
                <owl:onProperty rdf:resource="https://w3id.org/netbeheer/referentiemodellen/IECCIM/TC57CIM/IEC61970/Base/Wires#Conductor_length"/>
                <owl:minQualifiedCardinality rdf:datatype="http://www.w3.org/2001/XMLSchema#nonNegativeInteger">0</owl:minQualifiedCardinality>
                <owl:onClass rdf:resource="https://w3id.org/netbeheer/referentiemodellen/IECCIM/TC57CIM/IEC61970/Base/Domain#Length"/>
            </owl:Restriction>
        </rdfs:subClassOf>
        <rdfs:subClassOf>
            <owl:Restriction>
                <owl:onProperty rdf:resource="https://w3id.org/netbeheer/referentiemodellen/IECCIM/TC57CIM/IEC61970/Base/Wires#Conductor_length"/>
                <owl:maxQualifiedCardinality rdf:datatype="http://www.w3.org/2001/XMLSchema#nonNegativeInteger">1</owl:maxQualifiedCardinality>
                <owl:onClass rdf:resource="https://w3id.org/netbeheer/referentiemodellen/IECCIM/TC57CIM/IEC61970/Base/Domain#Length"/>
            </owl:Restriction>
        </rdfs:subClassOf>
        <rdfs:comment>Combination of conducting material with consistent electrical characteristics, building a single electrical system, used to carry current between points in the power system.  </rdfs:comment>
    </owl:Class>
    


    <!-- https://w3id.org/netbeheer/referentiemodellen/IECCIM/TC57CIM/IEC61970/Base/Wires#Connector -->


    <owl:Class rdf:about="https://w3id.org/netbeheer/referentiemodellen/IECCIM/TC57CIM/IEC61970/Base/Wires#Connector">
        <rdfs:subClassOf rdf:resource="https://w3id.org/netbeheer/referentiemodellen/IECCIM/TC57CIM/IEC61970/Base/Core#ConductingEquipment"/>
        <rdfs:comment>A conductor, or group of conductors, with negligible impedance, that serve to connect other conducting equipment within a single substation and are modelled with a single logical terminal.</rdfs:comment>
    </owl:Class>
    


    <!-- https://w3id.org/netbeheer/referentiemodellen/IECCIM/TC57CIM/IEC61970/Base/Wires#Cut -->


    <owl:Class rdf:about="https://w3id.org/netbeheer/referentiemodellen/IECCIM/TC57CIM/IEC61970/Base/Wires#Cut">
        <rdfs:subClassOf rdf:resource="https://w3id.org/netbeheer/referentiemodellen/IECCIM/TC57CIM/IEC61970/Base/Wires#Switch"/>
        <rdfs:subClassOf>
            <owl:Restriction>
                <owl:onProperty rdf:resource="https://w3id.org/netbeheer/referentiemodellen/IECCIM/TC57CIM/IEC61970/Base/Wires#Cut_ACLineSegment"/>
                <owl:minQualifiedCardinality rdf:datatype="http://www.w3.org/2001/XMLSchema#nonNegativeInteger">0</owl:minQualifiedCardinality>
                <owl:onClass rdf:resource="https://w3id.org/netbeheer/referentiemodellen/IECCIM/TC57CIM/IEC61970/Base/Wires#Cut"/>
            </owl:Restriction>
        </rdfs:subClassOf>
        <rdfs:subClassOf>
            <owl:Restriction>
                <owl:onProperty rdf:resource="https://w3id.org/netbeheer/referentiemodellen/IECCIM/TC57CIM/IEC61970/Base/Wires#Cut_CutAction"/>
                <owl:minQualifiedCardinality rdf:datatype="http://www.w3.org/2001/XMLSchema#nonNegativeInteger">0</owl:minQualifiedCardinality>
                <owl:onClass rdf:resource="https://w3id.org/netbeheer/referentiemodellen/IECCIM/TC57CIM/IEC61970/Base/Wires#Cut"/>
            </owl:Restriction>
        </rdfs:subClassOf>
        <rdfs:subClassOf>
            <owl:Restriction>
                <owl:onProperty rdf:resource="https://w3id.org/netbeheer/referentiemodellen/IECCIM/TC57CIM/IEC61970/Base/Wires#Cut_lengthFromTerminal1"/>
                <owl:minQualifiedCardinality rdf:datatype="http://www.w3.org/2001/XMLSchema#nonNegativeInteger">0</owl:minQualifiedCardinality>
                <owl:onClass rdf:resource="https://w3id.org/netbeheer/referentiemodellen/IECCIM/TC57CIM/IEC61970/Base/Domain#Length"/>
            </owl:Restriction>
        </rdfs:subClassOf>
        <rdfs:subClassOf>
            <owl:Restriction>
                <owl:onProperty rdf:resource="https://w3id.org/netbeheer/referentiemodellen/IECCIM/TC57CIM/IEC61970/Base/Wires#Cut_CutAction"/>
                <owl:maxQualifiedCardinality rdf:datatype="http://www.w3.org/2001/XMLSchema#nonNegativeInteger">1</owl:maxQualifiedCardinality>
                <owl:onClass rdf:resource="https://w3id.org/netbeheer/referentiemodellen/IECCIM/TC57CIM/IEC61970/Base/Wires#Cut"/>
            </owl:Restriction>
        </rdfs:subClassOf>
        <rdfs:subClassOf>
            <owl:Restriction>
                <owl:onProperty rdf:resource="https://w3id.org/netbeheer/referentiemodellen/IECCIM/TC57CIM/IEC61970/Base/Wires#Cut_lengthFromTerminal1"/>
                <owl:maxQualifiedCardinality rdf:datatype="http://www.w3.org/2001/XMLSchema#nonNegativeInteger">1</owl:maxQualifiedCardinality>
                <owl:onClass rdf:resource="https://w3id.org/netbeheer/referentiemodellen/IECCIM/TC57CIM/IEC61970/Base/Domain#Length"/>
            </owl:Restriction>
        </rdfs:subClassOf>
        <rdfs:comment>A cut separates a line segment into two parts. The cut appears as a switch inserted between these two parts and connects them together. As the cut is normally open there is no galvanic connection between the two line segment parts. But it is possible to close the cut to get galvanic connection.
The cut terminals are oriented towards the line segment terminals with the same sequence number. Hence the cut terminal with sequence number equal to 1 is oriented to the line segment&apos;s terminal with sequence number equal to 1.
The cut terminals also act as connection points for jumpers and other equipment, e.g. a mobile generator. To enable this, connectivity nodes are placed at the cut terminals. Once the connectivity nodes are in place any conducting equipment can be connected at them.
</rdfs:comment>
    </owl:Class>
    


    <!-- https://w3id.org/netbeheer/referentiemodellen/IECCIM/TC57CIM/IEC61970/Base/Wires#Disconnector -->


    <owl:Class rdf:about="https://w3id.org/netbeheer/referentiemodellen/IECCIM/TC57CIM/IEC61970/Base/Wires#Disconnector">
        <rdfs:subClassOf rdf:resource="https://w3id.org/netbeheer/referentiemodellen/IECCIM/TC57CIM/IEC61970/Base/Wires#Switch"/>
        <rdfs:comment>A manually operated or motor operated mechanical switching device used for changing the connections in a circuit, or for isolating a circuit or equipment from a source of power. It is required to open or close circuits when negligible current is broken or made. </rdfs:comment>
    </owl:Class>
    


    <!-- https://w3id.org/netbeheer/referentiemodellen/IECCIM/TC57CIM/IEC61970/Base/Wires#EarthFaultCompensator -->


    <owl:Class rdf:about="https://w3id.org/netbeheer/referentiemodellen/IECCIM/TC57CIM/IEC61970/Base/Wires#EarthFaultCompensator">
        <rdfs:subClassOf rdf:resource="https://w3id.org/netbeheer/referentiemodellen/IECCIM/TC57CIM/IEC61970/Base/Core#ConductingEquipment"/>
        <rdfs:subClassOf>
            <owl:Restriction>
                <owl:onProperty rdf:resource="https://w3id.org/netbeheer/referentiemodellen/IECCIM/TC57CIM/IEC61970/Base/Wires#EarthFaultCompensator_r"/>
                <owl:minQualifiedCardinality rdf:datatype="http://www.w3.org/2001/XMLSchema#nonNegativeInteger">0</owl:minQualifiedCardinality>
                <owl:onClass rdf:resource="https://w3id.org/netbeheer/referentiemodellen/IECCIM/TC57CIM/IEC61970/Base/Domain#Resistance"/>
            </owl:Restriction>
        </rdfs:subClassOf>
        <rdfs:subClassOf>
            <owl:Restriction>
                <owl:onProperty rdf:resource="https://w3id.org/netbeheer/referentiemodellen/IECCIM/TC57CIM/IEC61970/Base/Wires#EarthFaultCompensator_r"/>
                <owl:maxQualifiedCardinality rdf:datatype="http://www.w3.org/2001/XMLSchema#nonNegativeInteger">1</owl:maxQualifiedCardinality>
                <owl:onClass rdf:resource="https://w3id.org/netbeheer/referentiemodellen/IECCIM/TC57CIM/IEC61970/Base/Domain#Resistance"/>
            </owl:Restriction>
        </rdfs:subClassOf>
        <rdfs:comment>A conducting equipment used to represent a connection to ground which is typically used to compensate earth faults..   An earth fault compensator device modeled with a single terminal implies a second terminal solidly connected to ground.  If two terminals are modeled, the ground is not assumed and normal connection rules apply.</rdfs:comment>
    </owl:Class>
    


    <!-- https://w3id.org/netbeheer/referentiemodellen/IECCIM/TC57CIM/IEC61970/Base/Wires#EnergyConsumer -->


    <owl:Class rdf:about="https://w3id.org/netbeheer/referentiemodellen/IECCIM/TC57CIM/IEC61970/Base/Wires#EnergyConsumer">
        <rdfs:subClassOf rdf:resource="https://w3id.org/netbeheer/referentiemodellen/IECCIM/TC57CIM/IEC61970/Base/Core#ConductingEquipment"/>
        <rdfs:subClassOf>
            <owl:Restriction>
                <owl:onProperty rdf:resource="https://w3id.org/netbeheer/referentiemodellen/IECCIM/TC57CIM/IEC61970/Base/Wires#EnergyConsumer_LoadDynamics"/>
                <owl:minQualifiedCardinality rdf:datatype="http://www.w3.org/2001/XMLSchema#nonNegativeInteger">0</owl:minQualifiedCardinality>
                <owl:onClass rdf:resource="https://w3id.org/netbeheer/referentiemodellen/IECCIM/TC57CIM/IEC61970/Base/Wires#EnergyConsumer"/>
            </owl:Restriction>
        </rdfs:subClassOf>
        <rdfs:subClassOf>
            <owl:Restriction>
                <owl:onProperty rdf:resource="https://w3id.org/netbeheer/referentiemodellen/IECCIM/TC57CIM/IEC61970/Base/Wires#EnergyConsumer_LoadResponse"/>
                <owl:minQualifiedCardinality rdf:datatype="http://www.w3.org/2001/XMLSchema#nonNegativeInteger">0</owl:minQualifiedCardinality>
                <owl:onClass rdf:resource="https://w3id.org/netbeheer/referentiemodellen/IECCIM/TC57CIM/IEC61970/Base/Wires#EnergyConsumer"/>
            </owl:Restriction>
        </rdfs:subClassOf>
        <rdfs:subClassOf>
            <owl:Restriction>
                <owl:onProperty rdf:resource="https://w3id.org/netbeheer/referentiemodellen/IECCIM/TC57CIM/IEC61970/Base/Wires#EnergyConsumer_PowerCutZone"/>
                <owl:minQualifiedCardinality rdf:datatype="http://www.w3.org/2001/XMLSchema#nonNegativeInteger">1</owl:minQualifiedCardinality>
                <owl:onClass rdf:resource="https://w3id.org/netbeheer/referentiemodellen/IECCIM/TC57CIM/IEC61970/Base/Wires#EnergyConsumer"/>
            </owl:Restriction>
        </rdfs:subClassOf>
        <rdfs:subClassOf>
            <owl:Restriction>
                <owl:onProperty rdf:resource="https://w3id.org/netbeheer/referentiemodellen/IECCIM/TC57CIM/IEC61970/Base/Wires#EnergyConsumer_p"/>
                <owl:minQualifiedCardinality rdf:datatype="http://www.w3.org/2001/XMLSchema#nonNegativeInteger">0</owl:minQualifiedCardinality>
                <owl:onClass rdf:resource="https://w3id.org/netbeheer/referentiemodellen/IECCIM/TC57CIM/IEC61970/Base/Domain#ActivePower"/>
            </owl:Restriction>
        </rdfs:subClassOf>
        <rdfs:subClassOf>
            <owl:Restriction>
                <owl:onProperty rdf:resource="https://w3id.org/netbeheer/referentiemodellen/IECCIM/TC57CIM/IEC61970/Base/Wires#EnergyConsumer_pfixed"/>
                <owl:minQualifiedCardinality rdf:datatype="http://www.w3.org/2001/XMLSchema#nonNegativeInteger">0</owl:minQualifiedCardinality>
                <owl:onClass rdf:resource="https://w3id.org/netbeheer/referentiemodellen/IECCIM/TC57CIM/IEC61970/Base/Domain#ActivePower"/>
            </owl:Restriction>
        </rdfs:subClassOf>
        <rdfs:subClassOf>
            <owl:Restriction>
                <owl:onProperty rdf:resource="https://w3id.org/netbeheer/referentiemodellen/IECCIM/TC57CIM/IEC61970/Base/Wires#EnergyConsumer_pfixedPct"/>
                <owl:minQualifiedCardinality rdf:datatype="http://www.w3.org/2001/XMLSchema#nonNegativeInteger">0</owl:minQualifiedCardinality>
                <owl:onClass rdf:resource="https://w3id.org/netbeheer/referentiemodellen/IECCIM/TC57CIM/IEC61970/Base/Domain#PerCent"/>
            </owl:Restriction>
        </rdfs:subClassOf>
        <rdfs:subClassOf>
            <owl:Restriction>
                <owl:onProperty rdf:resource="https://w3id.org/netbeheer/referentiemodellen/IECCIM/TC57CIM/IEC61970/Base/Wires#EnergyConsumer_q"/>
                <owl:minQualifiedCardinality rdf:datatype="http://www.w3.org/2001/XMLSchema#nonNegativeInteger">0</owl:minQualifiedCardinality>
                <owl:onClass rdf:resource="https://w3id.org/netbeheer/referentiemodellen/IECCIM/TC57CIM/IEC61970/Base/Domain#ReactivePower"/>
            </owl:Restriction>
        </rdfs:subClassOf>
        <rdfs:subClassOf>
            <owl:Restriction>
                <owl:onProperty rdf:resource="https://w3id.org/netbeheer/referentiemodellen/IECCIM/TC57CIM/IEC61970/Base/Wires#EnergyConsumer_qfixed"/>
                <owl:minQualifiedCardinality rdf:datatype="http://www.w3.org/2001/XMLSchema#nonNegativeInteger">0</owl:minQualifiedCardinality>
                <owl:onClass rdf:resource="https://w3id.org/netbeheer/referentiemodellen/IECCIM/TC57CIM/IEC61970/Base/Domain#ReactivePower"/>
            </owl:Restriction>
        </rdfs:subClassOf>
        <rdfs:subClassOf>
            <owl:Restriction>
                <owl:onProperty rdf:resource="https://w3id.org/netbeheer/referentiemodellen/IECCIM/TC57CIM/IEC61970/Base/Wires#EnergyConsumer_qfixedPct"/>
                <owl:minQualifiedCardinality rdf:datatype="http://www.w3.org/2001/XMLSchema#nonNegativeInteger">0</owl:minQualifiedCardinality>
                <owl:onClass rdf:resource="https://w3id.org/netbeheer/referentiemodellen/IECCIM/TC57CIM/IEC61970/Base/Domain#PerCent"/>
            </owl:Restriction>
        </rdfs:subClassOf>
        <rdfs:subClassOf>
            <owl:Restriction>
                <owl:onProperty rdf:resource="https://w3id.org/netbeheer/referentiemodellen/IECCIM/TC57CIM/IEC61970/Base/Wires#EnergyConsumer_EnergyConsumerPhase"/>
                <owl:qualifiedCardinality rdf:datatype="http://www.w3.org/2001/XMLSchema#nonNegativeInteger">1</owl:qualifiedCardinality>
                <owl:onClass rdf:resource="https://w3id.org/netbeheer/referentiemodellen/IECCIM/TC57CIM/IEC61970/Base/Wires#EnergyConsumer"/>
            </owl:Restriction>
        </rdfs:subClassOf>
        <rdfs:subClassOf>
            <owl:Restriction>
                <owl:onProperty rdf:resource="https://w3id.org/netbeheer/referentiemodellen/IECCIM/TC57CIM/IEC61970/Base/Wires#EnergyConsumer_p"/>
                <owl:maxQualifiedCardinality rdf:datatype="http://www.w3.org/2001/XMLSchema#nonNegativeInteger">1</owl:maxQualifiedCardinality>
                <owl:onClass rdf:resource="https://w3id.org/netbeheer/referentiemodellen/IECCIM/TC57CIM/IEC61970/Base/Domain#ActivePower"/>
            </owl:Restriction>
        </rdfs:subClassOf>
        <rdfs:subClassOf>
            <owl:Restriction>
                <owl:onProperty rdf:resource="https://w3id.org/netbeheer/referentiemodellen/IECCIM/TC57CIM/IEC61970/Base/Wires#EnergyConsumer_pfixed"/>
                <owl:maxQualifiedCardinality rdf:datatype="http://www.w3.org/2001/XMLSchema#nonNegativeInteger">1</owl:maxQualifiedCardinality>
                <owl:onClass rdf:resource="https://w3id.org/netbeheer/referentiemodellen/IECCIM/TC57CIM/IEC61970/Base/Domain#ActivePower"/>
            </owl:Restriction>
        </rdfs:subClassOf>
        <rdfs:subClassOf>
            <owl:Restriction>
                <owl:onProperty rdf:resource="https://w3id.org/netbeheer/referentiemodellen/IECCIM/TC57CIM/IEC61970/Base/Wires#EnergyConsumer_pfixedPct"/>
                <owl:maxQualifiedCardinality rdf:datatype="http://www.w3.org/2001/XMLSchema#nonNegativeInteger">1</owl:maxQualifiedCardinality>
                <owl:onClass rdf:resource="https://w3id.org/netbeheer/referentiemodellen/IECCIM/TC57CIM/IEC61970/Base/Domain#PerCent"/>
            </owl:Restriction>
        </rdfs:subClassOf>
        <rdfs:subClassOf>
            <owl:Restriction>
                <owl:onProperty rdf:resource="https://w3id.org/netbeheer/referentiemodellen/IECCIM/TC57CIM/IEC61970/Base/Wires#EnergyConsumer_q"/>
                <owl:maxQualifiedCardinality rdf:datatype="http://www.w3.org/2001/XMLSchema#nonNegativeInteger">1</owl:maxQualifiedCardinality>
                <owl:onClass rdf:resource="https://w3id.org/netbeheer/referentiemodellen/IECCIM/TC57CIM/IEC61970/Base/Domain#ReactivePower"/>
            </owl:Restriction>
        </rdfs:subClassOf>
        <rdfs:subClassOf>
            <owl:Restriction>
                <owl:onProperty rdf:resource="https://w3id.org/netbeheer/referentiemodellen/IECCIM/TC57CIM/IEC61970/Base/Wires#EnergyConsumer_qfixed"/>
                <owl:maxQualifiedCardinality rdf:datatype="http://www.w3.org/2001/XMLSchema#nonNegativeInteger">1</owl:maxQualifiedCardinality>
                <owl:onClass rdf:resource="https://w3id.org/netbeheer/referentiemodellen/IECCIM/TC57CIM/IEC61970/Base/Domain#ReactivePower"/>
            </owl:Restriction>
        </rdfs:subClassOf>
        <rdfs:subClassOf>
            <owl:Restriction>
                <owl:onProperty rdf:resource="https://w3id.org/netbeheer/referentiemodellen/IECCIM/TC57CIM/IEC61970/Base/Wires#EnergyConsumer_qfixedPct"/>
                <owl:maxQualifiedCardinality rdf:datatype="http://www.w3.org/2001/XMLSchema#nonNegativeInteger">1</owl:maxQualifiedCardinality>
                <owl:onClass rdf:resource="https://w3id.org/netbeheer/referentiemodellen/IECCIM/TC57CIM/IEC61970/Base/Domain#PerCent"/>
            </owl:Restriction>
        </rdfs:subClassOf>
        <rdfs:subClassOf>
            <owl:Restriction>
                <owl:onProperty rdf:resource="https://w3id.org/netbeheer/referentiemodellen/IECCIM/TC57CIM/IEC61970/Base/Wires#EnergyConsumer_customerCount"/>
                <owl:minQualifiedCardinality rdf:datatype="http://www.w3.org/2001/XMLSchema#nonNegativeInteger">0</owl:minQualifiedCardinality>
                <owl:onDataRange rdf:resource="http://www.w3.org/2001/XMLSchema#nonNegativeInteger"/>
            </owl:Restriction>
        </rdfs:subClassOf>
        <rdfs:subClassOf>
            <owl:Restriction>
                <owl:onProperty rdf:resource="https://w3id.org/netbeheer/referentiemodellen/IECCIM/TC57CIM/IEC61970/Base/Wires#EnergyConsumer_grounded"/>
                <owl:minQualifiedCardinality rdf:datatype="http://www.w3.org/2001/XMLSchema#nonNegativeInteger">0</owl:minQualifiedCardinality>
                <owl:onDataRange rdf:resource="http://www.w3.org/2001/XMLSchema#boolean"/>
            </owl:Restriction>
        </rdfs:subClassOf>
        <rdfs:subClassOf>
            <owl:Restriction>
                <owl:onProperty rdf:resource="https://w3id.org/netbeheer/referentiemodellen/IECCIM/TC57CIM/IEC61970/Base/Wires#EnergyConsumer_phaseConnection"/>
                <owl:minQualifiedCardinality rdf:datatype="http://www.w3.org/2001/XMLSchema#nonNegativeInteger">0</owl:minQualifiedCardinality>
                <owl:onDataRange rdf:resource="https://w3id.org/netbeheer/referentiemodellen/IECCIM/TC57CIM/IEC61970/Base/Wires#PhaseShuntConnectionKind"/>
            </owl:Restriction>
        </rdfs:subClassOf>
        <rdfs:subClassOf>
            <owl:Restriction>
                <owl:onProperty rdf:resource="https://w3id.org/netbeheer/referentiemodellen/IECCIM/TC57CIM/IEC61970/Base/Wires#EnergyConsumer_customerCount"/>
                <owl:maxQualifiedCardinality rdf:datatype="http://www.w3.org/2001/XMLSchema#nonNegativeInteger">1</owl:maxQualifiedCardinality>
                <owl:onDataRange rdf:resource="http://www.w3.org/2001/XMLSchema#nonNegativeInteger"/>
            </owl:Restriction>
        </rdfs:subClassOf>
        <rdfs:subClassOf>
            <owl:Restriction>
                <owl:onProperty rdf:resource="https://w3id.org/netbeheer/referentiemodellen/IECCIM/TC57CIM/IEC61970/Base/Wires#EnergyConsumer_grounded"/>
                <owl:maxQualifiedCardinality rdf:datatype="http://www.w3.org/2001/XMLSchema#nonNegativeInteger">1</owl:maxQualifiedCardinality>
                <owl:onDataRange rdf:resource="http://www.w3.org/2001/XMLSchema#boolean"/>
            </owl:Restriction>
        </rdfs:subClassOf>
        <rdfs:subClassOf>
            <owl:Restriction>
                <owl:onProperty rdf:resource="https://w3id.org/netbeheer/referentiemodellen/IECCIM/TC57CIM/IEC61970/Base/Wires#EnergyConsumer_phaseConnection"/>
                <owl:maxQualifiedCardinality rdf:datatype="http://www.w3.org/2001/XMLSchema#nonNegativeInteger">1</owl:maxQualifiedCardinality>
                <owl:onDataRange rdf:resource="https://w3id.org/netbeheer/referentiemodellen/IECCIM/TC57CIM/IEC61970/Base/Wires#PhaseShuntConnectionKind"/>
            </owl:Restriction>
        </rdfs:subClassOf>
        <rdfs:comment>Generic user of energy - a  point of consumption on the power system model.</rdfs:comment>
    </owl:Class>
    


    <!-- https://w3id.org/netbeheer/referentiemodellen/IECCIM/TC57CIM/IEC61970/Base/Wires#EnergyConsumerPhase -->


    <owl:Class rdf:about="https://w3id.org/netbeheer/referentiemodellen/IECCIM/TC57CIM/IEC61970/Base/Wires#EnergyConsumerPhase">
        <rdfs:subClassOf rdf:resource="https://w3id.org/netbeheer/referentiemodellen/IECCIM/TC57CIM/IEC61970/Base/Core#PowerSystemResource"/>
        <rdfs:subClassOf>
            <owl:Restriction>
                <owl:onProperty rdf:resource="https://w3id.org/netbeheer/referentiemodellen/IECCIM/TC57CIM/IEC61970/Base/Wires#EnergyConsumerPhase_EnergyConsumer"/>
                <owl:minQualifiedCardinality rdf:datatype="http://www.w3.org/2001/XMLSchema#nonNegativeInteger">0</owl:minQualifiedCardinality>
                <owl:onClass rdf:resource="https://w3id.org/netbeheer/referentiemodellen/IECCIM/TC57CIM/IEC61970/Base/Wires#EnergyConsumerPhase"/>
            </owl:Restriction>
        </rdfs:subClassOf>
        <rdfs:subClassOf>
            <owl:Restriction>
                <owl:onProperty rdf:resource="https://w3id.org/netbeheer/referentiemodellen/IECCIM/TC57CIM/IEC61970/Base/Wires#EnergyConsumerPhase_pfixed"/>
                <owl:minQualifiedCardinality rdf:datatype="http://www.w3.org/2001/XMLSchema#nonNegativeInteger">0</owl:minQualifiedCardinality>
                <owl:onClass rdf:resource="https://w3id.org/netbeheer/referentiemodellen/IECCIM/TC57CIM/IEC61970/Base/Domain#ActivePower"/>
            </owl:Restriction>
        </rdfs:subClassOf>
        <rdfs:subClassOf>
            <owl:Restriction>
                <owl:onProperty rdf:resource="https://w3id.org/netbeheer/referentiemodellen/IECCIM/TC57CIM/IEC61970/Base/Wires#EnergyConsumerPhase_pfixedPct"/>
                <owl:minQualifiedCardinality rdf:datatype="http://www.w3.org/2001/XMLSchema#nonNegativeInteger">0</owl:minQualifiedCardinality>
                <owl:onClass rdf:resource="https://w3id.org/netbeheer/referentiemodellen/IECCIM/TC57CIM/IEC61970/Base/Domain#PerCent"/>
            </owl:Restriction>
        </rdfs:subClassOf>
        <rdfs:subClassOf>
            <owl:Restriction>
                <owl:onProperty rdf:resource="https://w3id.org/netbeheer/referentiemodellen/IECCIM/TC57CIM/IEC61970/Base/Wires#EnergyConsumerPhase_qfixed"/>
                <owl:minQualifiedCardinality rdf:datatype="http://www.w3.org/2001/XMLSchema#nonNegativeInteger">0</owl:minQualifiedCardinality>
                <owl:onClass rdf:resource="https://w3id.org/netbeheer/referentiemodellen/IECCIM/TC57CIM/IEC61970/Base/Domain#ReactivePower"/>
            </owl:Restriction>
        </rdfs:subClassOf>
        <rdfs:subClassOf>
            <owl:Restriction>
                <owl:onProperty rdf:resource="https://w3id.org/netbeheer/referentiemodellen/IECCIM/TC57CIM/IEC61970/Base/Wires#EnergyConsumerPhase_qfixedPct"/>
                <owl:minQualifiedCardinality rdf:datatype="http://www.w3.org/2001/XMLSchema#nonNegativeInteger">0</owl:minQualifiedCardinality>
                <owl:onClass rdf:resource="https://w3id.org/netbeheer/referentiemodellen/IECCIM/TC57CIM/IEC61970/Base/Domain#PerCent"/>
            </owl:Restriction>
        </rdfs:subClassOf>
        <rdfs:subClassOf>
            <owl:Restriction>
                <owl:onProperty rdf:resource="https://w3id.org/netbeheer/referentiemodellen/IECCIM/TC57CIM/IEC61970/Base/Wires#EnergyConsumerPhase_pfixed"/>
                <owl:maxQualifiedCardinality rdf:datatype="http://www.w3.org/2001/XMLSchema#nonNegativeInteger">1</owl:maxQualifiedCardinality>
                <owl:onClass rdf:resource="https://w3id.org/netbeheer/referentiemodellen/IECCIM/TC57CIM/IEC61970/Base/Domain#ActivePower"/>
            </owl:Restriction>
        </rdfs:subClassOf>
        <rdfs:subClassOf>
            <owl:Restriction>
                <owl:onProperty rdf:resource="https://w3id.org/netbeheer/referentiemodellen/IECCIM/TC57CIM/IEC61970/Base/Wires#EnergyConsumerPhase_pfixedPct"/>
                <owl:maxQualifiedCardinality rdf:datatype="http://www.w3.org/2001/XMLSchema#nonNegativeInteger">1</owl:maxQualifiedCardinality>
                <owl:onClass rdf:resource="https://w3id.org/netbeheer/referentiemodellen/IECCIM/TC57CIM/IEC61970/Base/Domain#PerCent"/>
            </owl:Restriction>
        </rdfs:subClassOf>
        <rdfs:subClassOf>
            <owl:Restriction>
                <owl:onProperty rdf:resource="https://w3id.org/netbeheer/referentiemodellen/IECCIM/TC57CIM/IEC61970/Base/Wires#EnergyConsumerPhase_qfixed"/>
                <owl:maxQualifiedCardinality rdf:datatype="http://www.w3.org/2001/XMLSchema#nonNegativeInteger">1</owl:maxQualifiedCardinality>
                <owl:onClass rdf:resource="https://w3id.org/netbeheer/referentiemodellen/IECCIM/TC57CIM/IEC61970/Base/Domain#ReactivePower"/>
            </owl:Restriction>
        </rdfs:subClassOf>
        <rdfs:subClassOf>
            <owl:Restriction>
                <owl:onProperty rdf:resource="https://w3id.org/netbeheer/referentiemodellen/IECCIM/TC57CIM/IEC61970/Base/Wires#EnergyConsumerPhase_qfixedPct"/>
                <owl:maxQualifiedCardinality rdf:datatype="http://www.w3.org/2001/XMLSchema#nonNegativeInteger">1</owl:maxQualifiedCardinality>
                <owl:onClass rdf:resource="https://w3id.org/netbeheer/referentiemodellen/IECCIM/TC57CIM/IEC61970/Base/Domain#PerCent"/>
            </owl:Restriction>
        </rdfs:subClassOf>
        <rdfs:subClassOf>
            <owl:Restriction>
                <owl:onProperty rdf:resource="https://w3id.org/netbeheer/referentiemodellen/IECCIM/TC57CIM/IEC61970/Base/Wires#EnergyConsumerPhase_phase"/>
                <owl:minQualifiedCardinality rdf:datatype="http://www.w3.org/2001/XMLSchema#nonNegativeInteger">0</owl:minQualifiedCardinality>
                <owl:onDataRange rdf:resource="https://w3id.org/netbeheer/referentiemodellen/IECCIM/TC57CIM/IEC61970/Base/Wires#SinglePhaseKind"/>
            </owl:Restriction>
        </rdfs:subClassOf>
        <rdfs:subClassOf>
            <owl:Restriction>
                <owl:onProperty rdf:resource="https://w3id.org/netbeheer/referentiemodellen/IECCIM/TC57CIM/IEC61970/Base/Wires#EnergyConsumerPhase_phase"/>
                <owl:maxQualifiedCardinality rdf:datatype="http://www.w3.org/2001/XMLSchema#nonNegativeInteger">1</owl:maxQualifiedCardinality>
                <owl:onDataRange rdf:resource="https://w3id.org/netbeheer/referentiemodellen/IECCIM/TC57CIM/IEC61970/Base/Wires#SinglePhaseKind"/>
            </owl:Restriction>
        </rdfs:subClassOf>
        <rdfs:comment>A single phase of an energy consumer.
</rdfs:comment>
    </owl:Class>
    


    <!-- https://w3id.org/netbeheer/referentiemodellen/IECCIM/TC57CIM/IEC61970/Base/Wires#EnergySource -->


    <owl:Class rdf:about="https://w3id.org/netbeheer/referentiemodellen/IECCIM/TC57CIM/IEC61970/Base/Wires#EnergySource">
        <rdfs:subClassOf rdf:resource="https://w3id.org/netbeheer/referentiemodellen/IECCIM/TC57CIM/IEC61970/Base/Core#ConductingEquipment"/>
        <rdfs:subClassOf>
            <owl:Restriction>
                <owl:onProperty rdf:resource="https://w3id.org/netbeheer/referentiemodellen/IECCIM/TC57CIM/IEC61970/Base/Wires#EnergySource_EnergySchedulingType"/>
                <owl:minQualifiedCardinality rdf:datatype="http://www.w3.org/2001/XMLSchema#nonNegativeInteger">0</owl:minQualifiedCardinality>
                <owl:onClass rdf:resource="https://w3id.org/netbeheer/referentiemodellen/IECCIM/TC57CIM/IEC61970/Base/Wires#EnergySource"/>
            </owl:Restriction>
        </rdfs:subClassOf>
        <rdfs:subClassOf>
            <owl:Restriction>
                <owl:onProperty rdf:resource="https://w3id.org/netbeheer/referentiemodellen/IECCIM/TC57CIM/IEC61970/Base/Wires#EnergySource_EnergySourceAction"/>
                <owl:minQualifiedCardinality rdf:datatype="http://www.w3.org/2001/XMLSchema#nonNegativeInteger">0</owl:minQualifiedCardinality>
                <owl:onClass rdf:resource="https://w3id.org/netbeheer/referentiemodellen/IECCIM/TC57CIM/IEC61970/Base/Wires#EnergySource"/>
            </owl:Restriction>
        </rdfs:subClassOf>
        <rdfs:subClassOf>
            <owl:Restriction>
                <owl:onProperty rdf:resource="https://w3id.org/netbeheer/referentiemodellen/IECCIM/TC57CIM/IEC61970/Base/Wires#EnergySource_activePower"/>
                <owl:minQualifiedCardinality rdf:datatype="http://www.w3.org/2001/XMLSchema#nonNegativeInteger">0</owl:minQualifiedCardinality>
                <owl:onClass rdf:resource="https://w3id.org/netbeheer/referentiemodellen/IECCIM/TC57CIM/IEC61970/Base/Domain#ActivePower"/>
            </owl:Restriction>
        </rdfs:subClassOf>
        <rdfs:subClassOf>
            <owl:Restriction>
                <owl:onProperty rdf:resource="https://w3id.org/netbeheer/referentiemodellen/IECCIM/TC57CIM/IEC61970/Base/Wires#EnergySource_nominalVoltage"/>
                <owl:minQualifiedCardinality rdf:datatype="http://www.w3.org/2001/XMLSchema#nonNegativeInteger">0</owl:minQualifiedCardinality>
                <owl:onClass rdf:resource="https://w3id.org/netbeheer/referentiemodellen/IECCIM/TC57CIM/IEC61970/Base/Domain#Voltage"/>
            </owl:Restriction>
        </rdfs:subClassOf>
        <rdfs:subClassOf>
            <owl:Restriction>
                <owl:onProperty rdf:resource="https://w3id.org/netbeheer/referentiemodellen/IECCIM/TC57CIM/IEC61970/Base/Wires#EnergySource_r"/>
                <owl:minQualifiedCardinality rdf:datatype="http://www.w3.org/2001/XMLSchema#nonNegativeInteger">0</owl:minQualifiedCardinality>
                <owl:onClass rdf:resource="https://w3id.org/netbeheer/referentiemodellen/IECCIM/TC57CIM/IEC61970/Base/Domain#Resistance"/>
            </owl:Restriction>
        </rdfs:subClassOf>
        <rdfs:subClassOf>
            <owl:Restriction>
                <owl:onProperty rdf:resource="https://w3id.org/netbeheer/referentiemodellen/IECCIM/TC57CIM/IEC61970/Base/Wires#EnergySource_r0"/>
                <owl:minQualifiedCardinality rdf:datatype="http://www.w3.org/2001/XMLSchema#nonNegativeInteger">0</owl:minQualifiedCardinality>
                <owl:onClass rdf:resource="https://w3id.org/netbeheer/referentiemodellen/IECCIM/TC57CIM/IEC61970/Base/Domain#Resistance"/>
            </owl:Restriction>
        </rdfs:subClassOf>
        <rdfs:subClassOf>
            <owl:Restriction>
                <owl:onProperty rdf:resource="https://w3id.org/netbeheer/referentiemodellen/IECCIM/TC57CIM/IEC61970/Base/Wires#EnergySource_reactivePower"/>
                <owl:minQualifiedCardinality rdf:datatype="http://www.w3.org/2001/XMLSchema#nonNegativeInteger">0</owl:minQualifiedCardinality>
                <owl:onClass rdf:resource="https://w3id.org/netbeheer/referentiemodellen/IECCIM/TC57CIM/IEC61970/Base/Domain#ReactivePower"/>
            </owl:Restriction>
        </rdfs:subClassOf>
        <rdfs:subClassOf>
            <owl:Restriction>
                <owl:onProperty rdf:resource="https://w3id.org/netbeheer/referentiemodellen/IECCIM/TC57CIM/IEC61970/Base/Wires#EnergySource_rn"/>
                <owl:minQualifiedCardinality rdf:datatype="http://www.w3.org/2001/XMLSchema#nonNegativeInteger">0</owl:minQualifiedCardinality>
                <owl:onClass rdf:resource="https://w3id.org/netbeheer/referentiemodellen/IECCIM/TC57CIM/IEC61970/Base/Domain#Resistance"/>
            </owl:Restriction>
        </rdfs:subClassOf>
        <rdfs:subClassOf>
            <owl:Restriction>
                <owl:onProperty rdf:resource="https://w3id.org/netbeheer/referentiemodellen/IECCIM/TC57CIM/IEC61970/Base/Wires#EnergySource_voltageAngle"/>
                <owl:minQualifiedCardinality rdf:datatype="http://www.w3.org/2001/XMLSchema#nonNegativeInteger">0</owl:minQualifiedCardinality>
                <owl:onClass rdf:resource="https://w3id.org/netbeheer/referentiemodellen/IECCIM/TC57CIM/IEC61970/Base/Domain#AngleRadians"/>
            </owl:Restriction>
        </rdfs:subClassOf>
        <rdfs:subClassOf>
            <owl:Restriction>
                <owl:onProperty rdf:resource="https://w3id.org/netbeheer/referentiemodellen/IECCIM/TC57CIM/IEC61970/Base/Wires#EnergySource_voltageMagnitude"/>
                <owl:minQualifiedCardinality rdf:datatype="http://www.w3.org/2001/XMLSchema#nonNegativeInteger">0</owl:minQualifiedCardinality>
                <owl:onClass rdf:resource="https://w3id.org/netbeheer/referentiemodellen/IECCIM/TC57CIM/IEC61970/Base/Domain#Voltage"/>
            </owl:Restriction>
        </rdfs:subClassOf>
        <rdfs:subClassOf>
            <owl:Restriction>
                <owl:onProperty rdf:resource="https://w3id.org/netbeheer/referentiemodellen/IECCIM/TC57CIM/IEC61970/Base/Wires#EnergySource_x"/>
                <owl:minQualifiedCardinality rdf:datatype="http://www.w3.org/2001/XMLSchema#nonNegativeInteger">0</owl:minQualifiedCardinality>
                <owl:onClass rdf:resource="https://w3id.org/netbeheer/referentiemodellen/IECCIM/TC57CIM/IEC61970/Base/Domain#Reactance"/>
            </owl:Restriction>
        </rdfs:subClassOf>
        <rdfs:subClassOf>
            <owl:Restriction>
                <owl:onProperty rdf:resource="https://w3id.org/netbeheer/referentiemodellen/IECCIM/TC57CIM/IEC61970/Base/Wires#EnergySource_x0"/>
                <owl:minQualifiedCardinality rdf:datatype="http://www.w3.org/2001/XMLSchema#nonNegativeInteger">0</owl:minQualifiedCardinality>
                <owl:onClass rdf:resource="https://w3id.org/netbeheer/referentiemodellen/IECCIM/TC57CIM/IEC61970/Base/Domain#Reactance"/>
            </owl:Restriction>
        </rdfs:subClassOf>
        <rdfs:subClassOf>
            <owl:Restriction>
                <owl:onProperty rdf:resource="https://w3id.org/netbeheer/referentiemodellen/IECCIM/TC57CIM/IEC61970/Base/Wires#EnergySource_xn"/>
                <owl:minQualifiedCardinality rdf:datatype="http://www.w3.org/2001/XMLSchema#nonNegativeInteger">0</owl:minQualifiedCardinality>
                <owl:onClass rdf:resource="https://w3id.org/netbeheer/referentiemodellen/IECCIM/TC57CIM/IEC61970/Base/Domain#Reactance"/>
            </owl:Restriction>
        </rdfs:subClassOf>
        <rdfs:subClassOf>
            <owl:Restriction>
                <owl:onProperty rdf:resource="https://w3id.org/netbeheer/referentiemodellen/IECCIM/TC57CIM/IEC61970/Base/Wires#EnergySource_EnergySourcePhase"/>
                <owl:qualifiedCardinality rdf:datatype="http://www.w3.org/2001/XMLSchema#nonNegativeInteger">1</owl:qualifiedCardinality>
                <owl:onClass rdf:resource="https://w3id.org/netbeheer/referentiemodellen/IECCIM/TC57CIM/IEC61970/Base/Wires#EnergySource"/>
            </owl:Restriction>
        </rdfs:subClassOf>
        <rdfs:subClassOf>
            <owl:Restriction>
                <owl:onProperty rdf:resource="https://w3id.org/netbeheer/referentiemodellen/IECCIM/TC57CIM/IEC61970/Base/Wires#EnergySource_WindTurbineType3or4Dynamics"/>
                <owl:qualifiedCardinality rdf:datatype="http://www.w3.org/2001/XMLSchema#nonNegativeInteger">1</owl:qualifiedCardinality>
                <owl:onClass rdf:resource="https://w3id.org/netbeheer/referentiemodellen/IECCIM/TC57CIM/IEC61970/Base/Wires#EnergySource"/>
            </owl:Restriction>
        </rdfs:subClassOf>
        <rdfs:subClassOf>
            <owl:Restriction>
                <owl:onProperty rdf:resource="https://w3id.org/netbeheer/referentiemodellen/IECCIM/TC57CIM/IEC61970/Base/Wires#EnergySource_EnergySourceAction"/>
                <owl:maxQualifiedCardinality rdf:datatype="http://www.w3.org/2001/XMLSchema#nonNegativeInteger">1</owl:maxQualifiedCardinality>
                <owl:onClass rdf:resource="https://w3id.org/netbeheer/referentiemodellen/IECCIM/TC57CIM/IEC61970/Base/Wires#EnergySource"/>
            </owl:Restriction>
        </rdfs:subClassOf>
        <rdfs:subClassOf>
            <owl:Restriction>
                <owl:onProperty rdf:resource="https://w3id.org/netbeheer/referentiemodellen/IECCIM/TC57CIM/IEC61970/Base/Wires#EnergySource_activePower"/>
                <owl:maxQualifiedCardinality rdf:datatype="http://www.w3.org/2001/XMLSchema#nonNegativeInteger">1</owl:maxQualifiedCardinality>
                <owl:onClass rdf:resource="https://w3id.org/netbeheer/referentiemodellen/IECCIM/TC57CIM/IEC61970/Base/Domain#ActivePower"/>
            </owl:Restriction>
        </rdfs:subClassOf>
        <rdfs:subClassOf>
            <owl:Restriction>
                <owl:onProperty rdf:resource="https://w3id.org/netbeheer/referentiemodellen/IECCIM/TC57CIM/IEC61970/Base/Wires#EnergySource_nominalVoltage"/>
                <owl:maxQualifiedCardinality rdf:datatype="http://www.w3.org/2001/XMLSchema#nonNegativeInteger">1</owl:maxQualifiedCardinality>
                <owl:onClass rdf:resource="https://w3id.org/netbeheer/referentiemodellen/IECCIM/TC57CIM/IEC61970/Base/Domain#Voltage"/>
            </owl:Restriction>
        </rdfs:subClassOf>
        <rdfs:subClassOf>
            <owl:Restriction>
                <owl:onProperty rdf:resource="https://w3id.org/netbeheer/referentiemodellen/IECCIM/TC57CIM/IEC61970/Base/Wires#EnergySource_r"/>
                <owl:maxQualifiedCardinality rdf:datatype="http://www.w3.org/2001/XMLSchema#nonNegativeInteger">1</owl:maxQualifiedCardinality>
                <owl:onClass rdf:resource="https://w3id.org/netbeheer/referentiemodellen/IECCIM/TC57CIM/IEC61970/Base/Domain#Resistance"/>
            </owl:Restriction>
        </rdfs:subClassOf>
        <rdfs:subClassOf>
            <owl:Restriction>
                <owl:onProperty rdf:resource="https://w3id.org/netbeheer/referentiemodellen/IECCIM/TC57CIM/IEC61970/Base/Wires#EnergySource_r0"/>
                <owl:maxQualifiedCardinality rdf:datatype="http://www.w3.org/2001/XMLSchema#nonNegativeInteger">1</owl:maxQualifiedCardinality>
                <owl:onClass rdf:resource="https://w3id.org/netbeheer/referentiemodellen/IECCIM/TC57CIM/IEC61970/Base/Domain#Resistance"/>
            </owl:Restriction>
        </rdfs:subClassOf>
        <rdfs:subClassOf>
            <owl:Restriction>
                <owl:onProperty rdf:resource="https://w3id.org/netbeheer/referentiemodellen/IECCIM/TC57CIM/IEC61970/Base/Wires#EnergySource_reactivePower"/>
                <owl:maxQualifiedCardinality rdf:datatype="http://www.w3.org/2001/XMLSchema#nonNegativeInteger">1</owl:maxQualifiedCardinality>
                <owl:onClass rdf:resource="https://w3id.org/netbeheer/referentiemodellen/IECCIM/TC57CIM/IEC61970/Base/Domain#ReactivePower"/>
            </owl:Restriction>
        </rdfs:subClassOf>
        <rdfs:subClassOf>
            <owl:Restriction>
                <owl:onProperty rdf:resource="https://w3id.org/netbeheer/referentiemodellen/IECCIM/TC57CIM/IEC61970/Base/Wires#EnergySource_rn"/>
                <owl:maxQualifiedCardinality rdf:datatype="http://www.w3.org/2001/XMLSchema#nonNegativeInteger">1</owl:maxQualifiedCardinality>
                <owl:onClass rdf:resource="https://w3id.org/netbeheer/referentiemodellen/IECCIM/TC57CIM/IEC61970/Base/Domain#Resistance"/>
            </owl:Restriction>
        </rdfs:subClassOf>
        <rdfs:subClassOf>
            <owl:Restriction>
                <owl:onProperty rdf:resource="https://w3id.org/netbeheer/referentiemodellen/IECCIM/TC57CIM/IEC61970/Base/Wires#EnergySource_voltageAngle"/>
                <owl:maxQualifiedCardinality rdf:datatype="http://www.w3.org/2001/XMLSchema#nonNegativeInteger">1</owl:maxQualifiedCardinality>
                <owl:onClass rdf:resource="https://w3id.org/netbeheer/referentiemodellen/IECCIM/TC57CIM/IEC61970/Base/Domain#AngleRadians"/>
            </owl:Restriction>
        </rdfs:subClassOf>
        <rdfs:subClassOf>
            <owl:Restriction>
                <owl:onProperty rdf:resource="https://w3id.org/netbeheer/referentiemodellen/IECCIM/TC57CIM/IEC61970/Base/Wires#EnergySource_voltageMagnitude"/>
                <owl:maxQualifiedCardinality rdf:datatype="http://www.w3.org/2001/XMLSchema#nonNegativeInteger">1</owl:maxQualifiedCardinality>
                <owl:onClass rdf:resource="https://w3id.org/netbeheer/referentiemodellen/IECCIM/TC57CIM/IEC61970/Base/Domain#Voltage"/>
            </owl:Restriction>
        </rdfs:subClassOf>
        <rdfs:subClassOf>
            <owl:Restriction>
                <owl:onProperty rdf:resource="https://w3id.org/netbeheer/referentiemodellen/IECCIM/TC57CIM/IEC61970/Base/Wires#EnergySource_x"/>
                <owl:maxQualifiedCardinality rdf:datatype="http://www.w3.org/2001/XMLSchema#nonNegativeInteger">1</owl:maxQualifiedCardinality>
                <owl:onClass rdf:resource="https://w3id.org/netbeheer/referentiemodellen/IECCIM/TC57CIM/IEC61970/Base/Domain#Reactance"/>
            </owl:Restriction>
        </rdfs:subClassOf>
        <rdfs:subClassOf>
            <owl:Restriction>
                <owl:onProperty rdf:resource="https://w3id.org/netbeheer/referentiemodellen/IECCIM/TC57CIM/IEC61970/Base/Wires#EnergySource_x0"/>
                <owl:maxQualifiedCardinality rdf:datatype="http://www.w3.org/2001/XMLSchema#nonNegativeInteger">1</owl:maxQualifiedCardinality>
                <owl:onClass rdf:resource="https://w3id.org/netbeheer/referentiemodellen/IECCIM/TC57CIM/IEC61970/Base/Domain#Reactance"/>
            </owl:Restriction>
        </rdfs:subClassOf>
        <rdfs:subClassOf>
            <owl:Restriction>
                <owl:onProperty rdf:resource="https://w3id.org/netbeheer/referentiemodellen/IECCIM/TC57CIM/IEC61970/Base/Wires#EnergySource_xn"/>
                <owl:maxQualifiedCardinality rdf:datatype="http://www.w3.org/2001/XMLSchema#nonNegativeInteger">1</owl:maxQualifiedCardinality>
                <owl:onClass rdf:resource="https://w3id.org/netbeheer/referentiemodellen/IECCIM/TC57CIM/IEC61970/Base/Domain#Reactance"/>
            </owl:Restriction>
        </rdfs:subClassOf>
        <rdfs:comment>A generic equivalent for an energy supplier on a transmission or distribution voltage level.</rdfs:comment>
    </owl:Class>
    


    <!-- https://w3id.org/netbeheer/referentiemodellen/IECCIM/TC57CIM/IEC61970/Base/Wires#EnergySourcePhase -->


    <owl:Class rdf:about="https://w3id.org/netbeheer/referentiemodellen/IECCIM/TC57CIM/IEC61970/Base/Wires#EnergySourcePhase">
        <rdfs:subClassOf rdf:resource="https://w3id.org/netbeheer/referentiemodellen/IECCIM/TC57CIM/IEC61970/Base/Core#PowerSystemResource"/>
        <rdfs:subClassOf>
            <owl:Restriction>
                <owl:onProperty rdf:resource="https://w3id.org/netbeheer/referentiemodellen/IECCIM/TC57CIM/IEC61970/Base/Wires#EnergySourcePhase_EnergySource"/>
                <owl:minQualifiedCardinality rdf:datatype="http://www.w3.org/2001/XMLSchema#nonNegativeInteger">0</owl:minQualifiedCardinality>
                <owl:onClass rdf:resource="https://w3id.org/netbeheer/referentiemodellen/IECCIM/TC57CIM/IEC61970/Base/Wires#EnergySourcePhase"/>
            </owl:Restriction>
        </rdfs:subClassOf>
        <rdfs:subClassOf>
            <owl:Restriction>
                <owl:onProperty rdf:resource="https://w3id.org/netbeheer/referentiemodellen/IECCIM/TC57CIM/IEC61970/Base/Wires#EnergySourcePhase_phase"/>
                <owl:minQualifiedCardinality rdf:datatype="http://www.w3.org/2001/XMLSchema#nonNegativeInteger">0</owl:minQualifiedCardinality>
                <owl:onDataRange rdf:resource="https://w3id.org/netbeheer/referentiemodellen/IECCIM/TC57CIM/IEC61970/Base/Wires#SinglePhaseKind"/>
            </owl:Restriction>
        </rdfs:subClassOf>
        <rdfs:subClassOf>
            <owl:Restriction>
                <owl:onProperty rdf:resource="https://w3id.org/netbeheer/referentiemodellen/IECCIM/TC57CIM/IEC61970/Base/Wires#EnergySourcePhase_phase"/>
                <owl:maxQualifiedCardinality rdf:datatype="http://www.w3.org/2001/XMLSchema#nonNegativeInteger">1</owl:maxQualifiedCardinality>
                <owl:onDataRange rdf:resource="https://w3id.org/netbeheer/referentiemodellen/IECCIM/TC57CIM/IEC61970/Base/Wires#SinglePhaseKind"/>
            </owl:Restriction>
        </rdfs:subClassOf>
        <rdfs:comment>Represents the single phase information of an unbalanced energy source.</rdfs:comment>
    </owl:Class>
    


    <!-- https://w3id.org/netbeheer/referentiemodellen/IECCIM/TC57CIM/IEC61970/Base/Wires#ExternalNetworkInjection -->


    <owl:Class rdf:about="https://w3id.org/netbeheer/referentiemodellen/IECCIM/TC57CIM/IEC61970/Base/Wires#ExternalNetworkInjection">
        <rdfs:subClassOf rdf:resource="https://w3id.org/netbeheer/referentiemodellen/IECCIM/TC57CIM/IEC61970/Base/Wires#RegulatingCondEq"/>
        <rdfs:subClassOf>
            <owl:Restriction>
                <owl:onProperty rdf:resource="https://w3id.org/netbeheer/referentiemodellen/IECCIM/TC57CIM/IEC61970/Base/Wires#ExternalNetworkInjection_governorSCD"/>
                <owl:minQualifiedCardinality rdf:datatype="http://www.w3.org/2001/XMLSchema#nonNegativeInteger">0</owl:minQualifiedCardinality>
                <owl:onClass rdf:resource="https://w3id.org/netbeheer/referentiemodellen/IECCIM/TC57CIM/IEC61970/Base/Domain#ActivePowerPerFrequency"/>
            </owl:Restriction>
        </rdfs:subClassOf>
        <rdfs:subClassOf>
            <owl:Restriction>
                <owl:onProperty rdf:resource="https://w3id.org/netbeheer/referentiemodellen/IECCIM/TC57CIM/IEC61970/Base/Wires#ExternalNetworkInjection_maxInitialSymShCCurrent"/>
                <owl:minQualifiedCardinality rdf:datatype="http://www.w3.org/2001/XMLSchema#nonNegativeInteger">0</owl:minQualifiedCardinality>
                <owl:onClass rdf:resource="https://w3id.org/netbeheer/referentiemodellen/IECCIM/TC57CIM/IEC61970/Base/Domain#CurrentFlow"/>
            </owl:Restriction>
        </rdfs:subClassOf>
        <rdfs:subClassOf>
            <owl:Restriction>
                <owl:onProperty rdf:resource="https://w3id.org/netbeheer/referentiemodellen/IECCIM/TC57CIM/IEC61970/Base/Wires#ExternalNetworkInjection_maxP"/>
                <owl:minQualifiedCardinality rdf:datatype="http://www.w3.org/2001/XMLSchema#nonNegativeInteger">0</owl:minQualifiedCardinality>
                <owl:onClass rdf:resource="https://w3id.org/netbeheer/referentiemodellen/IECCIM/TC57CIM/IEC61970/Base/Domain#ActivePower"/>
            </owl:Restriction>
        </rdfs:subClassOf>
        <rdfs:subClassOf>
            <owl:Restriction>
                <owl:onProperty rdf:resource="https://w3id.org/netbeheer/referentiemodellen/IECCIM/TC57CIM/IEC61970/Base/Wires#ExternalNetworkInjection_maxQ"/>
                <owl:minQualifiedCardinality rdf:datatype="http://www.w3.org/2001/XMLSchema#nonNegativeInteger">0</owl:minQualifiedCardinality>
                <owl:onClass rdf:resource="https://w3id.org/netbeheer/referentiemodellen/IECCIM/TC57CIM/IEC61970/Base/Domain#ReactivePower"/>
            </owl:Restriction>
        </rdfs:subClassOf>
        <rdfs:subClassOf>
            <owl:Restriction>
                <owl:onProperty rdf:resource="https://w3id.org/netbeheer/referentiemodellen/IECCIM/TC57CIM/IEC61970/Base/Wires#ExternalNetworkInjection_minInitialSymShCCurrent"/>
                <owl:minQualifiedCardinality rdf:datatype="http://www.w3.org/2001/XMLSchema#nonNegativeInteger">0</owl:minQualifiedCardinality>
                <owl:onClass rdf:resource="https://w3id.org/netbeheer/referentiemodellen/IECCIM/TC57CIM/IEC61970/Base/Domain#CurrentFlow"/>
            </owl:Restriction>
        </rdfs:subClassOf>
        <rdfs:subClassOf>
            <owl:Restriction>
                <owl:onProperty rdf:resource="https://w3id.org/netbeheer/referentiemodellen/IECCIM/TC57CIM/IEC61970/Base/Wires#ExternalNetworkInjection_minP"/>
                <owl:minQualifiedCardinality rdf:datatype="http://www.w3.org/2001/XMLSchema#nonNegativeInteger">0</owl:minQualifiedCardinality>
                <owl:onClass rdf:resource="https://w3id.org/netbeheer/referentiemodellen/IECCIM/TC57CIM/IEC61970/Base/Domain#ActivePower"/>
            </owl:Restriction>
        </rdfs:subClassOf>
        <rdfs:subClassOf>
            <owl:Restriction>
                <owl:onProperty rdf:resource="https://w3id.org/netbeheer/referentiemodellen/IECCIM/TC57CIM/IEC61970/Base/Wires#ExternalNetworkInjection_minQ"/>
                <owl:minQualifiedCardinality rdf:datatype="http://www.w3.org/2001/XMLSchema#nonNegativeInteger">0</owl:minQualifiedCardinality>
                <owl:onClass rdf:resource="https://w3id.org/netbeheer/referentiemodellen/IECCIM/TC57CIM/IEC61970/Base/Domain#ReactivePower"/>
            </owl:Restriction>
        </rdfs:subClassOf>
        <rdfs:subClassOf>
            <owl:Restriction>
                <owl:onProperty rdf:resource="https://w3id.org/netbeheer/referentiemodellen/IECCIM/TC57CIM/IEC61970/Base/Wires#ExternalNetworkInjection_p"/>
                <owl:minQualifiedCardinality rdf:datatype="http://www.w3.org/2001/XMLSchema#nonNegativeInteger">0</owl:minQualifiedCardinality>
                <owl:onClass rdf:resource="https://w3id.org/netbeheer/referentiemodellen/IECCIM/TC57CIM/IEC61970/Base/Domain#ActivePower"/>
            </owl:Restriction>
        </rdfs:subClassOf>
        <rdfs:subClassOf>
            <owl:Restriction>
                <owl:onProperty rdf:resource="https://w3id.org/netbeheer/referentiemodellen/IECCIM/TC57CIM/IEC61970/Base/Wires#ExternalNetworkInjection_q"/>
                <owl:minQualifiedCardinality rdf:datatype="http://www.w3.org/2001/XMLSchema#nonNegativeInteger">0</owl:minQualifiedCardinality>
                <owl:onClass rdf:resource="https://w3id.org/netbeheer/referentiemodellen/IECCIM/TC57CIM/IEC61970/Base/Domain#ReactivePower"/>
            </owl:Restriction>
        </rdfs:subClassOf>
        <rdfs:subClassOf>
            <owl:Restriction>
                <owl:onProperty rdf:resource="https://w3id.org/netbeheer/referentiemodellen/IECCIM/TC57CIM/IEC61970/Base/Wires#ExternalNetworkInjection_voltageFactor"/>
                <owl:minQualifiedCardinality rdf:datatype="http://www.w3.org/2001/XMLSchema#nonNegativeInteger">0</owl:minQualifiedCardinality>
                <owl:onClass rdf:resource="https://w3id.org/netbeheer/referentiemodellen/IECCIM/TC57CIM/IEC61970/Base/Domain#PU"/>
            </owl:Restriction>
        </rdfs:subClassOf>
        <rdfs:subClassOf>
            <owl:Restriction>
                <owl:onProperty rdf:resource="https://w3id.org/netbeheer/referentiemodellen/IECCIM/TC57CIM/IEC61970/Base/Wires#ExternalNetworkInjection_governorSCD"/>
                <owl:maxQualifiedCardinality rdf:datatype="http://www.w3.org/2001/XMLSchema#nonNegativeInteger">1</owl:maxQualifiedCardinality>
                <owl:onClass rdf:resource="https://w3id.org/netbeheer/referentiemodellen/IECCIM/TC57CIM/IEC61970/Base/Domain#ActivePowerPerFrequency"/>
            </owl:Restriction>
        </rdfs:subClassOf>
        <rdfs:subClassOf>
            <owl:Restriction>
                <owl:onProperty rdf:resource="https://w3id.org/netbeheer/referentiemodellen/IECCIM/TC57CIM/IEC61970/Base/Wires#ExternalNetworkInjection_maxInitialSymShCCurrent"/>
                <owl:maxQualifiedCardinality rdf:datatype="http://www.w3.org/2001/XMLSchema#nonNegativeInteger">1</owl:maxQualifiedCardinality>
                <owl:onClass rdf:resource="https://w3id.org/netbeheer/referentiemodellen/IECCIM/TC57CIM/IEC61970/Base/Domain#CurrentFlow"/>
            </owl:Restriction>
        </rdfs:subClassOf>
        <rdfs:subClassOf>
            <owl:Restriction>
                <owl:onProperty rdf:resource="https://w3id.org/netbeheer/referentiemodellen/IECCIM/TC57CIM/IEC61970/Base/Wires#ExternalNetworkInjection_maxP"/>
                <owl:maxQualifiedCardinality rdf:datatype="http://www.w3.org/2001/XMLSchema#nonNegativeInteger">1</owl:maxQualifiedCardinality>
                <owl:onClass rdf:resource="https://w3id.org/netbeheer/referentiemodellen/IECCIM/TC57CIM/IEC61970/Base/Domain#ActivePower"/>
            </owl:Restriction>
        </rdfs:subClassOf>
        <rdfs:subClassOf>
            <owl:Restriction>
                <owl:onProperty rdf:resource="https://w3id.org/netbeheer/referentiemodellen/IECCIM/TC57CIM/IEC61970/Base/Wires#ExternalNetworkInjection_maxQ"/>
                <owl:maxQualifiedCardinality rdf:datatype="http://www.w3.org/2001/XMLSchema#nonNegativeInteger">1</owl:maxQualifiedCardinality>
                <owl:onClass rdf:resource="https://w3id.org/netbeheer/referentiemodellen/IECCIM/TC57CIM/IEC61970/Base/Domain#ReactivePower"/>
            </owl:Restriction>
        </rdfs:subClassOf>
        <rdfs:subClassOf>
            <owl:Restriction>
                <owl:onProperty rdf:resource="https://w3id.org/netbeheer/referentiemodellen/IECCIM/TC57CIM/IEC61970/Base/Wires#ExternalNetworkInjection_minInitialSymShCCurrent"/>
                <owl:maxQualifiedCardinality rdf:datatype="http://www.w3.org/2001/XMLSchema#nonNegativeInteger">1</owl:maxQualifiedCardinality>
                <owl:onClass rdf:resource="https://w3id.org/netbeheer/referentiemodellen/IECCIM/TC57CIM/IEC61970/Base/Domain#CurrentFlow"/>
            </owl:Restriction>
        </rdfs:subClassOf>
        <rdfs:subClassOf>
            <owl:Restriction>
                <owl:onProperty rdf:resource="https://w3id.org/netbeheer/referentiemodellen/IECCIM/TC57CIM/IEC61970/Base/Wires#ExternalNetworkInjection_minP"/>
                <owl:maxQualifiedCardinality rdf:datatype="http://www.w3.org/2001/XMLSchema#nonNegativeInteger">1</owl:maxQualifiedCardinality>
                <owl:onClass rdf:resource="https://w3id.org/netbeheer/referentiemodellen/IECCIM/TC57CIM/IEC61970/Base/Domain#ActivePower"/>
            </owl:Restriction>
        </rdfs:subClassOf>
        <rdfs:subClassOf>
            <owl:Restriction>
                <owl:onProperty rdf:resource="https://w3id.org/netbeheer/referentiemodellen/IECCIM/TC57CIM/IEC61970/Base/Wires#ExternalNetworkInjection_minQ"/>
                <owl:maxQualifiedCardinality rdf:datatype="http://www.w3.org/2001/XMLSchema#nonNegativeInteger">1</owl:maxQualifiedCardinality>
                <owl:onClass rdf:resource="https://w3id.org/netbeheer/referentiemodellen/IECCIM/TC57CIM/IEC61970/Base/Domain#ReactivePower"/>
            </owl:Restriction>
        </rdfs:subClassOf>
        <rdfs:subClassOf>
            <owl:Restriction>
                <owl:onProperty rdf:resource="https://w3id.org/netbeheer/referentiemodellen/IECCIM/TC57CIM/IEC61970/Base/Wires#ExternalNetworkInjection_p"/>
                <owl:maxQualifiedCardinality rdf:datatype="http://www.w3.org/2001/XMLSchema#nonNegativeInteger">1</owl:maxQualifiedCardinality>
                <owl:onClass rdf:resource="https://w3id.org/netbeheer/referentiemodellen/IECCIM/TC57CIM/IEC61970/Base/Domain#ActivePower"/>
            </owl:Restriction>
        </rdfs:subClassOf>
        <rdfs:subClassOf>
            <owl:Restriction>
                <owl:onProperty rdf:resource="https://w3id.org/netbeheer/referentiemodellen/IECCIM/TC57CIM/IEC61970/Base/Wires#ExternalNetworkInjection_q"/>
                <owl:maxQualifiedCardinality rdf:datatype="http://www.w3.org/2001/XMLSchema#nonNegativeInteger">1</owl:maxQualifiedCardinality>
                <owl:onClass rdf:resource="https://w3id.org/netbeheer/referentiemodellen/IECCIM/TC57CIM/IEC61970/Base/Domain#ReactivePower"/>
            </owl:Restriction>
        </rdfs:subClassOf>
        <rdfs:subClassOf>
            <owl:Restriction>
                <owl:onProperty rdf:resource="https://w3id.org/netbeheer/referentiemodellen/IECCIM/TC57CIM/IEC61970/Base/Wires#ExternalNetworkInjection_voltageFactor"/>
                <owl:maxQualifiedCardinality rdf:datatype="http://www.w3.org/2001/XMLSchema#nonNegativeInteger">1</owl:maxQualifiedCardinality>
                <owl:onClass rdf:resource="https://w3id.org/netbeheer/referentiemodellen/IECCIM/TC57CIM/IEC61970/Base/Domain#PU"/>
            </owl:Restriction>
        </rdfs:subClassOf>
        <rdfs:subClassOf>
            <owl:Restriction>
                <owl:onProperty rdf:resource="https://w3id.org/netbeheer/referentiemodellen/IECCIM/TC57CIM/IEC61970/Base/Wires#ExternalNetworkInjection_ikSecond"/>
                <owl:minQualifiedCardinality rdf:datatype="http://www.w3.org/2001/XMLSchema#nonNegativeInteger">0</owl:minQualifiedCardinality>
                <owl:onDataRange rdf:resource="http://www.w3.org/2001/XMLSchema#boolean"/>
            </owl:Restriction>
        </rdfs:subClassOf>
        <rdfs:subClassOf>
            <owl:Restriction>
                <owl:onProperty rdf:resource="https://w3id.org/netbeheer/referentiemodellen/IECCIM/TC57CIM/IEC61970/Base/Wires#ExternalNetworkInjection_maxR0ToX0Ratio"/>
                <owl:minQualifiedCardinality rdf:datatype="http://www.w3.org/2001/XMLSchema#nonNegativeInteger">0</owl:minQualifiedCardinality>
                <owl:onDataRange rdf:resource="http://www.w3.org/2001/XMLSchema#float"/>
            </owl:Restriction>
        </rdfs:subClassOf>
        <rdfs:subClassOf>
            <owl:Restriction>
                <owl:onProperty rdf:resource="https://w3id.org/netbeheer/referentiemodellen/IECCIM/TC57CIM/IEC61970/Base/Wires#ExternalNetworkInjection_maxR1ToX1Ratio"/>
                <owl:minQualifiedCardinality rdf:datatype="http://www.w3.org/2001/XMLSchema#nonNegativeInteger">0</owl:minQualifiedCardinality>
                <owl:onDataRange rdf:resource="http://www.w3.org/2001/XMLSchema#float"/>
            </owl:Restriction>
        </rdfs:subClassOf>
        <rdfs:subClassOf>
            <owl:Restriction>
                <owl:onProperty rdf:resource="https://w3id.org/netbeheer/referentiemodellen/IECCIM/TC57CIM/IEC61970/Base/Wires#ExternalNetworkInjection_maxZ0ToZ1Ratio"/>
                <owl:minQualifiedCardinality rdf:datatype="http://www.w3.org/2001/XMLSchema#nonNegativeInteger">0</owl:minQualifiedCardinality>
                <owl:onDataRange rdf:resource="http://www.w3.org/2001/XMLSchema#float"/>
            </owl:Restriction>
        </rdfs:subClassOf>
        <rdfs:subClassOf>
            <owl:Restriction>
                <owl:onProperty rdf:resource="https://w3id.org/netbeheer/referentiemodellen/IECCIM/TC57CIM/IEC61970/Base/Wires#ExternalNetworkInjection_minR0ToX0Ratio"/>
                <owl:minQualifiedCardinality rdf:datatype="http://www.w3.org/2001/XMLSchema#nonNegativeInteger">0</owl:minQualifiedCardinality>
                <owl:onDataRange rdf:resource="http://www.w3.org/2001/XMLSchema#float"/>
            </owl:Restriction>
        </rdfs:subClassOf>
        <rdfs:subClassOf>
            <owl:Restriction>
                <owl:onProperty rdf:resource="https://w3id.org/netbeheer/referentiemodellen/IECCIM/TC57CIM/IEC61970/Base/Wires#ExternalNetworkInjection_minR1ToX1Ratio"/>
                <owl:minQualifiedCardinality rdf:datatype="http://www.w3.org/2001/XMLSchema#nonNegativeInteger">0</owl:minQualifiedCardinality>
                <owl:onDataRange rdf:resource="http://www.w3.org/2001/XMLSchema#float"/>
            </owl:Restriction>
        </rdfs:subClassOf>
        <rdfs:subClassOf>
            <owl:Restriction>
                <owl:onProperty rdf:resource="https://w3id.org/netbeheer/referentiemodellen/IECCIM/TC57CIM/IEC61970/Base/Wires#ExternalNetworkInjection_minZ0ToZ1Ratio"/>
                <owl:minQualifiedCardinality rdf:datatype="http://www.w3.org/2001/XMLSchema#nonNegativeInteger">0</owl:minQualifiedCardinality>
                <owl:onDataRange rdf:resource="http://www.w3.org/2001/XMLSchema#float"/>
            </owl:Restriction>
        </rdfs:subClassOf>
        <rdfs:subClassOf>
            <owl:Restriction>
                <owl:onProperty rdf:resource="https://w3id.org/netbeheer/referentiemodellen/IECCIM/TC57CIM/IEC61970/Base/Wires#ExternalNetworkInjection_referencePriority"/>
                <owl:minQualifiedCardinality rdf:datatype="http://www.w3.org/2001/XMLSchema#nonNegativeInteger">0</owl:minQualifiedCardinality>
                <owl:onDataRange rdf:resource="http://www.w3.org/2001/XMLSchema#nonNegativeInteger"/>
            </owl:Restriction>
        </rdfs:subClassOf>
        <rdfs:subClassOf>
            <owl:Restriction>
                <owl:onProperty rdf:resource="https://w3id.org/netbeheer/referentiemodellen/IECCIM/TC57CIM/IEC61970/Base/Wires#ExternalNetworkInjection_ikSecond"/>
                <owl:maxQualifiedCardinality rdf:datatype="http://www.w3.org/2001/XMLSchema#nonNegativeInteger">1</owl:maxQualifiedCardinality>
                <owl:onDataRange rdf:resource="http://www.w3.org/2001/XMLSchema#boolean"/>
            </owl:Restriction>
        </rdfs:subClassOf>
        <rdfs:subClassOf>
            <owl:Restriction>
                <owl:onProperty rdf:resource="https://w3id.org/netbeheer/referentiemodellen/IECCIM/TC57CIM/IEC61970/Base/Wires#ExternalNetworkInjection_maxR0ToX0Ratio"/>
                <owl:maxQualifiedCardinality rdf:datatype="http://www.w3.org/2001/XMLSchema#nonNegativeInteger">1</owl:maxQualifiedCardinality>
                <owl:onDataRange rdf:resource="http://www.w3.org/2001/XMLSchema#float"/>
            </owl:Restriction>
        </rdfs:subClassOf>
        <rdfs:subClassOf>
            <owl:Restriction>
                <owl:onProperty rdf:resource="https://w3id.org/netbeheer/referentiemodellen/IECCIM/TC57CIM/IEC61970/Base/Wires#ExternalNetworkInjection_maxR1ToX1Ratio"/>
                <owl:maxQualifiedCardinality rdf:datatype="http://www.w3.org/2001/XMLSchema#nonNegativeInteger">1</owl:maxQualifiedCardinality>
                <owl:onDataRange rdf:resource="http://www.w3.org/2001/XMLSchema#float"/>
            </owl:Restriction>
        </rdfs:subClassOf>
        <rdfs:subClassOf>
            <owl:Restriction>
                <owl:onProperty rdf:resource="https://w3id.org/netbeheer/referentiemodellen/IECCIM/TC57CIM/IEC61970/Base/Wires#ExternalNetworkInjection_maxZ0ToZ1Ratio"/>
                <owl:maxQualifiedCardinality rdf:datatype="http://www.w3.org/2001/XMLSchema#nonNegativeInteger">1</owl:maxQualifiedCardinality>
                <owl:onDataRange rdf:resource="http://www.w3.org/2001/XMLSchema#float"/>
            </owl:Restriction>
        </rdfs:subClassOf>
        <rdfs:subClassOf>
            <owl:Restriction>
                <owl:onProperty rdf:resource="https://w3id.org/netbeheer/referentiemodellen/IECCIM/TC57CIM/IEC61970/Base/Wires#ExternalNetworkInjection_minR0ToX0Ratio"/>
                <owl:maxQualifiedCardinality rdf:datatype="http://www.w3.org/2001/XMLSchema#nonNegativeInteger">1</owl:maxQualifiedCardinality>
                <owl:onDataRange rdf:resource="http://www.w3.org/2001/XMLSchema#float"/>
            </owl:Restriction>
        </rdfs:subClassOf>
        <rdfs:subClassOf>
            <owl:Restriction>
                <owl:onProperty rdf:resource="https://w3id.org/netbeheer/referentiemodellen/IECCIM/TC57CIM/IEC61970/Base/Wires#ExternalNetworkInjection_minR1ToX1Ratio"/>
                <owl:maxQualifiedCardinality rdf:datatype="http://www.w3.org/2001/XMLSchema#nonNegativeInteger">1</owl:maxQualifiedCardinality>
                <owl:onDataRange rdf:resource="http://www.w3.org/2001/XMLSchema#float"/>
            </owl:Restriction>
        </rdfs:subClassOf>
        <rdfs:subClassOf>
            <owl:Restriction>
                <owl:onProperty rdf:resource="https://w3id.org/netbeheer/referentiemodellen/IECCIM/TC57CIM/IEC61970/Base/Wires#ExternalNetworkInjection_minZ0ToZ1Ratio"/>
                <owl:maxQualifiedCardinality rdf:datatype="http://www.w3.org/2001/XMLSchema#nonNegativeInteger">1</owl:maxQualifiedCardinality>
                <owl:onDataRange rdf:resource="http://www.w3.org/2001/XMLSchema#float"/>
            </owl:Restriction>
        </rdfs:subClassOf>
        <rdfs:subClassOf>
            <owl:Restriction>
                <owl:onProperty rdf:resource="https://w3id.org/netbeheer/referentiemodellen/IECCIM/TC57CIM/IEC61970/Base/Wires#ExternalNetworkInjection_referencePriority"/>
                <owl:maxQualifiedCardinality rdf:datatype="http://www.w3.org/2001/XMLSchema#nonNegativeInteger">1</owl:maxQualifiedCardinality>
                <owl:onDataRange rdf:resource="http://www.w3.org/2001/XMLSchema#nonNegativeInteger"/>
            </owl:Restriction>
        </rdfs:subClassOf>
        <rdfs:comment>This class represents external network and it is used for IEC 60909 calculations.</rdfs:comment>
    </owl:Class>
    


    <!-- https://w3id.org/netbeheer/referentiemodellen/IECCIM/TC57CIM/IEC61970/Base/Wires#FrequencyConverter -->


    <owl:Class rdf:about="https://w3id.org/netbeheer/referentiemodellen/IECCIM/TC57CIM/IEC61970/Base/Wires#FrequencyConverter">
        <rdfs:subClassOf rdf:resource="https://w3id.org/netbeheer/referentiemodellen/IECCIM/TC57CIM/IEC61970/Base/Wires#RegulatingCondEq"/>
        <rdfs:subClassOf>
            <owl:Restriction>
                <owl:onProperty rdf:resource="https://w3id.org/netbeheer/referentiemodellen/IECCIM/TC57CIM/IEC61970/Base/Wires#FrequencyConverter_frequency"/>
                <owl:minQualifiedCardinality rdf:datatype="http://www.w3.org/2001/XMLSchema#nonNegativeInteger">0</owl:minQualifiedCardinality>
                <owl:onClass rdf:resource="https://w3id.org/netbeheer/referentiemodellen/IECCIM/TC57CIM/IEC61970/Base/Domain#Frequency"/>
            </owl:Restriction>
        </rdfs:subClassOf>
        <rdfs:subClassOf>
            <owl:Restriction>
                <owl:onProperty rdf:resource="https://w3id.org/netbeheer/referentiemodellen/IECCIM/TC57CIM/IEC61970/Base/Wires#FrequencyConverter_maxP"/>
                <owl:minQualifiedCardinality rdf:datatype="http://www.w3.org/2001/XMLSchema#nonNegativeInteger">0</owl:minQualifiedCardinality>
                <owl:onClass rdf:resource="https://w3id.org/netbeheer/referentiemodellen/IECCIM/TC57CIM/IEC61970/Base/Domain#ActivePower"/>
            </owl:Restriction>
        </rdfs:subClassOf>
        <rdfs:subClassOf>
            <owl:Restriction>
                <owl:onProperty rdf:resource="https://w3id.org/netbeheer/referentiemodellen/IECCIM/TC57CIM/IEC61970/Base/Wires#FrequencyConverter_maxU"/>
                <owl:minQualifiedCardinality rdf:datatype="http://www.w3.org/2001/XMLSchema#nonNegativeInteger">0</owl:minQualifiedCardinality>
                <owl:onClass rdf:resource="https://w3id.org/netbeheer/referentiemodellen/IECCIM/TC57CIM/IEC61970/Base/Domain#Voltage"/>
            </owl:Restriction>
        </rdfs:subClassOf>
        <rdfs:subClassOf>
            <owl:Restriction>
                <owl:onProperty rdf:resource="https://w3id.org/netbeheer/referentiemodellen/IECCIM/TC57CIM/IEC61970/Base/Wires#FrequencyConverter_minP"/>
                <owl:minQualifiedCardinality rdf:datatype="http://www.w3.org/2001/XMLSchema#nonNegativeInteger">0</owl:minQualifiedCardinality>
                <owl:onClass rdf:resource="https://w3id.org/netbeheer/referentiemodellen/IECCIM/TC57CIM/IEC61970/Base/Domain#ActivePower"/>
            </owl:Restriction>
        </rdfs:subClassOf>
        <rdfs:subClassOf>
            <owl:Restriction>
                <owl:onProperty rdf:resource="https://w3id.org/netbeheer/referentiemodellen/IECCIM/TC57CIM/IEC61970/Base/Wires#FrequencyConverter_minU"/>
                <owl:minQualifiedCardinality rdf:datatype="http://www.w3.org/2001/XMLSchema#nonNegativeInteger">0</owl:minQualifiedCardinality>
                <owl:onClass rdf:resource="https://w3id.org/netbeheer/referentiemodellen/IECCIM/TC57CIM/IEC61970/Base/Domain#Voltage"/>
            </owl:Restriction>
        </rdfs:subClassOf>
        <rdfs:subClassOf>
            <owl:Restriction>
                <owl:onProperty rdf:resource="https://w3id.org/netbeheer/referentiemodellen/IECCIM/TC57CIM/IEC61970/Base/Wires#FrequencyConverter_frequency"/>
                <owl:maxQualifiedCardinality rdf:datatype="http://www.w3.org/2001/XMLSchema#nonNegativeInteger">1</owl:maxQualifiedCardinality>
                <owl:onClass rdf:resource="https://w3id.org/netbeheer/referentiemodellen/IECCIM/TC57CIM/IEC61970/Base/Domain#Frequency"/>
            </owl:Restriction>
        </rdfs:subClassOf>
        <rdfs:subClassOf>
            <owl:Restriction>
                <owl:onProperty rdf:resource="https://w3id.org/netbeheer/referentiemodellen/IECCIM/TC57CIM/IEC61970/Base/Wires#FrequencyConverter_maxP"/>
                <owl:maxQualifiedCardinality rdf:datatype="http://www.w3.org/2001/XMLSchema#nonNegativeInteger">1</owl:maxQualifiedCardinality>
                <owl:onClass rdf:resource="https://w3id.org/netbeheer/referentiemodellen/IECCIM/TC57CIM/IEC61970/Base/Domain#ActivePower"/>
            </owl:Restriction>
        </rdfs:subClassOf>
        <rdfs:subClassOf>
            <owl:Restriction>
                <owl:onProperty rdf:resource="https://w3id.org/netbeheer/referentiemodellen/IECCIM/TC57CIM/IEC61970/Base/Wires#FrequencyConverter_maxU"/>
                <owl:maxQualifiedCardinality rdf:datatype="http://www.w3.org/2001/XMLSchema#nonNegativeInteger">1</owl:maxQualifiedCardinality>
                <owl:onClass rdf:resource="https://w3id.org/netbeheer/referentiemodellen/IECCIM/TC57CIM/IEC61970/Base/Domain#Voltage"/>
            </owl:Restriction>
        </rdfs:subClassOf>
        <rdfs:subClassOf>
            <owl:Restriction>
                <owl:onProperty rdf:resource="https://w3id.org/netbeheer/referentiemodellen/IECCIM/TC57CIM/IEC61970/Base/Wires#FrequencyConverter_minP"/>
                <owl:maxQualifiedCardinality rdf:datatype="http://www.w3.org/2001/XMLSchema#nonNegativeInteger">1</owl:maxQualifiedCardinality>
                <owl:onClass rdf:resource="https://w3id.org/netbeheer/referentiemodellen/IECCIM/TC57CIM/IEC61970/Base/Domain#ActivePower"/>
            </owl:Restriction>
        </rdfs:subClassOf>
        <rdfs:subClassOf>
            <owl:Restriction>
                <owl:onProperty rdf:resource="https://w3id.org/netbeheer/referentiemodellen/IECCIM/TC57CIM/IEC61970/Base/Wires#FrequencyConverter_minU"/>
                <owl:maxQualifiedCardinality rdf:datatype="http://www.w3.org/2001/XMLSchema#nonNegativeInteger">1</owl:maxQualifiedCardinality>
                <owl:onClass rdf:resource="https://w3id.org/netbeheer/referentiemodellen/IECCIM/TC57CIM/IEC61970/Base/Domain#Voltage"/>
            </owl:Restriction>
        </rdfs:subClassOf>
        <rdfs:comment>A device to convert from one frequency to another (e.g., frequency F1 to F2) comprises a pair of FrequencyConverter instances. One converts from F1 to DC, the other converts the DC to F2.</rdfs:comment>
    </owl:Class>
    


    <!-- https://w3id.org/netbeheer/referentiemodellen/IECCIM/TC57CIM/IEC61970/Base/Wires#Fuse -->


    <owl:Class rdf:about="https://w3id.org/netbeheer/referentiemodellen/IECCIM/TC57CIM/IEC61970/Base/Wires#Fuse">
        <rdfs:subClassOf rdf:resource="https://w3id.org/netbeheer/referentiemodellen/IECCIM/TC57CIM/IEC61970/Base/Wires#Switch"/>
        <rdfs:comment>An overcurrent protective device with a circuit opening fusible part that is heated and severed by the passage of overcurrent through it. A fuse is considered a switching device because it breaks current.</rdfs:comment>
    </owl:Class>
    


    <!-- https://w3id.org/netbeheer/referentiemodellen/IECCIM/TC57CIM/IEC61970/Base/Wires#Ground -->


    <owl:Class rdf:about="https://w3id.org/netbeheer/referentiemodellen/IECCIM/TC57CIM/IEC61970/Base/Wires#Ground">
        <rdfs:subClassOf rdf:resource="https://w3id.org/netbeheer/referentiemodellen/IECCIM/TC57CIM/IEC61970/Base/Core#ConductingEquipment"/>
        <rdfs:subClassOf>
            <owl:Restriction>
                <owl:onProperty rdf:resource="https://w3id.org/netbeheer/referentiemodellen/IECCIM/TC57CIM/IEC61970/Base/Wires#Ground_GroundAction"/>
                <owl:minQualifiedCardinality rdf:datatype="http://www.w3.org/2001/XMLSchema#nonNegativeInteger">0</owl:minQualifiedCardinality>
                <owl:onClass rdf:resource="https://w3id.org/netbeheer/referentiemodellen/IECCIM/TC57CIM/IEC61970/Base/Wires#Ground"/>
            </owl:Restriction>
        </rdfs:subClassOf>
        <rdfs:subClassOf>
            <owl:Restriction>
                <owl:onProperty rdf:resource="https://w3id.org/netbeheer/referentiemodellen/IECCIM/TC57CIM/IEC61970/Base/Wires#Ground_GroundAction"/>
                <owl:maxQualifiedCardinality rdf:datatype="http://www.w3.org/2001/XMLSchema#nonNegativeInteger">1</owl:maxQualifiedCardinality>
                <owl:onClass rdf:resource="https://w3id.org/netbeheer/referentiemodellen/IECCIM/TC57CIM/IEC61970/Base/Wires#Ground"/>
            </owl:Restriction>
        </rdfs:subClassOf>
        <rdfs:comment>A point where the system is grounded used for connecting conducting equipment to ground. The power system model can have any number of grounds.</rdfs:comment>
    </owl:Class>
    


    <!-- https://w3id.org/netbeheer/referentiemodellen/IECCIM/TC57CIM/IEC61970/Base/Wires#GroundDisconnector -->


    <owl:Class rdf:about="https://w3id.org/netbeheer/referentiemodellen/IECCIM/TC57CIM/IEC61970/Base/Wires#GroundDisconnector">
        <rdfs:subClassOf rdf:resource="https://w3id.org/netbeheer/referentiemodellen/IECCIM/TC57CIM/IEC61970/Base/Wires#Switch"/>
        <rdfs:comment>A manually operated or motor operated mechanical switching device used for isolating a circuit or equipment from ground.</rdfs:comment>
    </owl:Class>
    


    <!-- https://w3id.org/netbeheer/referentiemodellen/IECCIM/TC57CIM/IEC61970/Base/Wires#GroundingImpedance -->


    <owl:Class rdf:about="https://w3id.org/netbeheer/referentiemodellen/IECCIM/TC57CIM/IEC61970/Base/Wires#GroundingImpedance">
        <rdfs:subClassOf rdf:resource="https://w3id.org/netbeheer/referentiemodellen/IECCIM/TC57CIM/IEC61970/Base/Wires#EarthFaultCompensator"/>
        <rdfs:subClassOf>
            <owl:Restriction>
                <owl:onProperty rdf:resource="https://w3id.org/netbeheer/referentiemodellen/IECCIM/TC57CIM/IEC61970/Base/Wires#GroundingImpedance_x"/>
                <owl:minQualifiedCardinality rdf:datatype="http://www.w3.org/2001/XMLSchema#nonNegativeInteger">0</owl:minQualifiedCardinality>
                <owl:onClass rdf:resource="https://w3id.org/netbeheer/referentiemodellen/IECCIM/TC57CIM/IEC61970/Base/Domain#Reactance"/>
            </owl:Restriction>
        </rdfs:subClassOf>
        <rdfs:subClassOf>
            <owl:Restriction>
                <owl:onProperty rdf:resource="https://w3id.org/netbeheer/referentiemodellen/IECCIM/TC57CIM/IEC61970/Base/Wires#GroundingImpedance_x"/>
                <owl:maxQualifiedCardinality rdf:datatype="http://www.w3.org/2001/XMLSchema#nonNegativeInteger">1</owl:maxQualifiedCardinality>
                <owl:onClass rdf:resource="https://w3id.org/netbeheer/referentiemodellen/IECCIM/TC57CIM/IEC61970/Base/Domain#Reactance"/>
            </owl:Restriction>
        </rdfs:subClassOf>
        <rdfs:comment>A fixed impedance device used for grounding.</rdfs:comment>
    </owl:Class>
    


    <!-- https://w3id.org/netbeheer/referentiemodellen/IECCIM/TC57CIM/IEC61970/Base/Wires#Jumper -->


    <owl:Class rdf:about="https://w3id.org/netbeheer/referentiemodellen/IECCIM/TC57CIM/IEC61970/Base/Wires#Jumper">
        <rdfs:subClassOf rdf:resource="https://w3id.org/netbeheer/referentiemodellen/IECCIM/TC57CIM/IEC61970/Base/Wires#Switch"/>
        <rdfs:subClassOf>
            <owl:Restriction>
                <owl:onProperty rdf:resource="https://w3id.org/netbeheer/referentiemodellen/IECCIM/TC57CIM/IEC61970/Base/Wires#Jumper_JumperAction"/>
                <owl:minQualifiedCardinality rdf:datatype="http://www.w3.org/2001/XMLSchema#nonNegativeInteger">0</owl:minQualifiedCardinality>
                <owl:onClass rdf:resource="https://w3id.org/netbeheer/referentiemodellen/IECCIM/TC57CIM/IEC61970/Base/Wires#Jumper"/>
            </owl:Restriction>
        </rdfs:subClassOf>
        <rdfs:subClassOf>
            <owl:Restriction>
                <owl:onProperty rdf:resource="https://w3id.org/netbeheer/referentiemodellen/IECCIM/TC57CIM/IEC61970/Base/Wires#Jumper_JumperAction"/>
                <owl:maxQualifiedCardinality rdf:datatype="http://www.w3.org/2001/XMLSchema#nonNegativeInteger">1</owl:maxQualifiedCardinality>
                <owl:onClass rdf:resource="https://w3id.org/netbeheer/referentiemodellen/IECCIM/TC57CIM/IEC61970/Base/Wires#Jumper"/>
            </owl:Restriction>
        </rdfs:subClassOf>
        <rdfs:comment>A short section of conductor with negligible impedance which can be manually removed and replaced if the circuit is de-energized. Note that zero-impedance branches can potentially be modeled by other equipment types.
</rdfs:comment>
    </owl:Class>
    


    <!-- https://w3id.org/netbeheer/referentiemodellen/IECCIM/TC57CIM/IEC61970/Base/Wires#Junction -->


    <owl:Class rdf:about="https://w3id.org/netbeheer/referentiemodellen/IECCIM/TC57CIM/IEC61970/Base/Wires#Junction">
        <rdfs:subClassOf rdf:resource="https://w3id.org/netbeheer/referentiemodellen/IECCIM/TC57CIM/IEC61970/Base/Wires#Connector"/>
        <rdfs:comment>A point where one or more conducting equipments are connected with zero resistance.</rdfs:comment>
    </owl:Class>
    


    <!-- https://w3id.org/netbeheer/referentiemodellen/IECCIM/TC57CIM/IEC61970/Base/Wires#Line -->


    <owl:Class rdf:about="https://w3id.org/netbeheer/referentiemodellen/IECCIM/TC57CIM/IEC61970/Base/Wires#Line">
        <rdfs:subClassOf rdf:resource="https://w3id.org/netbeheer/referentiemodellen/IECCIM/TC57CIM/IEC61970/Base/Core#EquipmentContainer"/>
        <rdfs:comment>Contains equipment beyond a substation belonging to a power transmission line. </rdfs:comment>
    </owl:Class>
    


    <!-- https://w3id.org/netbeheer/referentiemodellen/IECCIM/TC57CIM/IEC61970/Base/Wires#LinearShuntCompensator -->


    <owl:Class rdf:about="https://w3id.org/netbeheer/referentiemodellen/IECCIM/TC57CIM/IEC61970/Base/Wires#LinearShuntCompensator">
        <rdfs:subClassOf rdf:resource="https://w3id.org/netbeheer/referentiemodellen/IECCIM/TC57CIM/IEC61970/Base/Wires#ShuntCompensator"/>
        <rdfs:subClassOf>
            <owl:Restriction>
                <owl:onProperty rdf:resource="https://w3id.org/netbeheer/referentiemodellen/IECCIM/TC57CIM/IEC61970/Base/Wires#LinearShuntCompensator_b0PerSection"/>
                <owl:minQualifiedCardinality rdf:datatype="http://www.w3.org/2001/XMLSchema#nonNegativeInteger">0</owl:minQualifiedCardinality>
                <owl:onClass rdf:resource="https://w3id.org/netbeheer/referentiemodellen/IECCIM/TC57CIM/IEC61970/Base/Domain#Susceptance"/>
            </owl:Restriction>
        </rdfs:subClassOf>
        <rdfs:subClassOf>
            <owl:Restriction>
                <owl:onProperty rdf:resource="https://w3id.org/netbeheer/referentiemodellen/IECCIM/TC57CIM/IEC61970/Base/Wires#LinearShuntCompensator_bPerSection"/>
                <owl:minQualifiedCardinality rdf:datatype="http://www.w3.org/2001/XMLSchema#nonNegativeInteger">0</owl:minQualifiedCardinality>
                <owl:onClass rdf:resource="https://w3id.org/netbeheer/referentiemodellen/IECCIM/TC57CIM/IEC61970/Base/Domain#Susceptance"/>
            </owl:Restriction>
        </rdfs:subClassOf>
        <rdfs:subClassOf>
            <owl:Restriction>
                <owl:onProperty rdf:resource="https://w3id.org/netbeheer/referentiemodellen/IECCIM/TC57CIM/IEC61970/Base/Wires#LinearShuntCompensator_g0PerSection"/>
                <owl:minQualifiedCardinality rdf:datatype="http://www.w3.org/2001/XMLSchema#nonNegativeInteger">0</owl:minQualifiedCardinality>
                <owl:onClass rdf:resource="https://w3id.org/netbeheer/referentiemodellen/IECCIM/TC57CIM/IEC61970/Base/Domain#Conductance"/>
            </owl:Restriction>
        </rdfs:subClassOf>
        <rdfs:subClassOf>
            <owl:Restriction>
                <owl:onProperty rdf:resource="https://w3id.org/netbeheer/referentiemodellen/IECCIM/TC57CIM/IEC61970/Base/Wires#LinearShuntCompensator_gPerSection"/>
                <owl:minQualifiedCardinality rdf:datatype="http://www.w3.org/2001/XMLSchema#nonNegativeInteger">0</owl:minQualifiedCardinality>
                <owl:onClass rdf:resource="https://w3id.org/netbeheer/referentiemodellen/IECCIM/TC57CIM/IEC61970/Base/Domain#Conductance"/>
            </owl:Restriction>
        </rdfs:subClassOf>
        <rdfs:subClassOf>
            <owl:Restriction>
                <owl:onProperty rdf:resource="https://w3id.org/netbeheer/referentiemodellen/IECCIM/TC57CIM/IEC61970/Base/Wires#LinearShuntCompensator_b0PerSection"/>
                <owl:maxQualifiedCardinality rdf:datatype="http://www.w3.org/2001/XMLSchema#nonNegativeInteger">1</owl:maxQualifiedCardinality>
                <owl:onClass rdf:resource="https://w3id.org/netbeheer/referentiemodellen/IECCIM/TC57CIM/IEC61970/Base/Domain#Susceptance"/>
            </owl:Restriction>
        </rdfs:subClassOf>
        <rdfs:subClassOf>
            <owl:Restriction>
                <owl:onProperty rdf:resource="https://w3id.org/netbeheer/referentiemodellen/IECCIM/TC57CIM/IEC61970/Base/Wires#LinearShuntCompensator_bPerSection"/>
                <owl:maxQualifiedCardinality rdf:datatype="http://www.w3.org/2001/XMLSchema#nonNegativeInteger">1</owl:maxQualifiedCardinality>
                <owl:onClass rdf:resource="https://w3id.org/netbeheer/referentiemodellen/IECCIM/TC57CIM/IEC61970/Base/Domain#Susceptance"/>
            </owl:Restriction>
        </rdfs:subClassOf>
        <rdfs:subClassOf>
            <owl:Restriction>
                <owl:onProperty rdf:resource="https://w3id.org/netbeheer/referentiemodellen/IECCIM/TC57CIM/IEC61970/Base/Wires#LinearShuntCompensator_g0PerSection"/>
                <owl:maxQualifiedCardinality rdf:datatype="http://www.w3.org/2001/XMLSchema#nonNegativeInteger">1</owl:maxQualifiedCardinality>
                <owl:onClass rdf:resource="https://w3id.org/netbeheer/referentiemodellen/IECCIM/TC57CIM/IEC61970/Base/Domain#Conductance"/>
            </owl:Restriction>
        </rdfs:subClassOf>
        <rdfs:subClassOf>
            <owl:Restriction>
                <owl:onProperty rdf:resource="https://w3id.org/netbeheer/referentiemodellen/IECCIM/TC57CIM/IEC61970/Base/Wires#LinearShuntCompensator_gPerSection"/>
                <owl:maxQualifiedCardinality rdf:datatype="http://www.w3.org/2001/XMLSchema#nonNegativeInteger">1</owl:maxQualifiedCardinality>
                <owl:onClass rdf:resource="https://w3id.org/netbeheer/referentiemodellen/IECCIM/TC57CIM/IEC61970/Base/Domain#Conductance"/>
            </owl:Restriction>
        </rdfs:subClassOf>
        <rdfs:comment>A linear shunt compensator has banks or sections with equal admittance values.</rdfs:comment>
    </owl:Class>
    


    <!-- https://w3id.org/netbeheer/referentiemodellen/IECCIM/TC57CIM/IEC61970/Base/Wires#LinearShuntCompensatorPhase -->


    <owl:Class rdf:about="https://w3id.org/netbeheer/referentiemodellen/IECCIM/TC57CIM/IEC61970/Base/Wires#LinearShuntCompensatorPhase">
        <rdfs:subClassOf rdf:resource="https://w3id.org/netbeheer/referentiemodellen/IECCIM/TC57CIM/IEC61970/Base/Wires#ShuntCompensatorPhase"/>
        <rdfs:subClassOf>
            <owl:Restriction>
                <owl:onProperty rdf:resource="https://w3id.org/netbeheer/referentiemodellen/IECCIM/TC57CIM/IEC61970/Base/Wires#LinearShuntCompensatorPhase_bPerSection"/>
                <owl:minQualifiedCardinality rdf:datatype="http://www.w3.org/2001/XMLSchema#nonNegativeInteger">0</owl:minQualifiedCardinality>
                <owl:onClass rdf:resource="https://w3id.org/netbeheer/referentiemodellen/IECCIM/TC57CIM/IEC61970/Base/Domain#Susceptance"/>
            </owl:Restriction>
        </rdfs:subClassOf>
        <rdfs:subClassOf>
            <owl:Restriction>
                <owl:onProperty rdf:resource="https://w3id.org/netbeheer/referentiemodellen/IECCIM/TC57CIM/IEC61970/Base/Wires#LinearShuntCompensatorPhase_gPerSection"/>
                <owl:minQualifiedCardinality rdf:datatype="http://www.w3.org/2001/XMLSchema#nonNegativeInteger">0</owl:minQualifiedCardinality>
                <owl:onClass rdf:resource="https://w3id.org/netbeheer/referentiemodellen/IECCIM/TC57CIM/IEC61970/Base/Domain#Conductance"/>
            </owl:Restriction>
        </rdfs:subClassOf>
        <rdfs:subClassOf>
            <owl:Restriction>
                <owl:onProperty rdf:resource="https://w3id.org/netbeheer/referentiemodellen/IECCIM/TC57CIM/IEC61970/Base/Wires#LinearShuntCompensatorPhase_bPerSection"/>
                <owl:maxQualifiedCardinality rdf:datatype="http://www.w3.org/2001/XMLSchema#nonNegativeInteger">1</owl:maxQualifiedCardinality>
                <owl:onClass rdf:resource="https://w3id.org/netbeheer/referentiemodellen/IECCIM/TC57CIM/IEC61970/Base/Domain#Susceptance"/>
            </owl:Restriction>
        </rdfs:subClassOf>
        <rdfs:subClassOf>
            <owl:Restriction>
                <owl:onProperty rdf:resource="https://w3id.org/netbeheer/referentiemodellen/IECCIM/TC57CIM/IEC61970/Base/Wires#LinearShuntCompensatorPhase_gPerSection"/>
                <owl:maxQualifiedCardinality rdf:datatype="http://www.w3.org/2001/XMLSchema#nonNegativeInteger">1</owl:maxQualifiedCardinality>
                <owl:onClass rdf:resource="https://w3id.org/netbeheer/referentiemodellen/IECCIM/TC57CIM/IEC61970/Base/Domain#Conductance"/>
            </owl:Restriction>
        </rdfs:subClassOf>
        <rdfs:comment>A per phase linear shunt compensator has banks or sections with equal admittance values.</rdfs:comment>
    </owl:Class>
    


    <!-- https://w3id.org/netbeheer/referentiemodellen/IECCIM/TC57CIM/IEC61970/Base/Wires#LoadBreakSwitch -->


    <owl:Class rdf:about="https://w3id.org/netbeheer/referentiemodellen/IECCIM/TC57CIM/IEC61970/Base/Wires#LoadBreakSwitch">
        <rdfs:subClassOf rdf:resource="https://w3id.org/netbeheer/referentiemodellen/IECCIM/TC57CIM/IEC61970/Base/Wires#ProtectedSwitch"/>
        <rdfs:comment>A mechanical switching device capable of making, carrying, and breaking currents under normal operating conditions.</rdfs:comment>
    </owl:Class>
    


    <!-- https://w3id.org/netbeheer/referentiemodellen/IECCIM/TC57CIM/IEC61970/Base/Wires#MutualCoupling -->


    <owl:Class rdf:about="https://w3id.org/netbeheer/referentiemodellen/IECCIM/TC57CIM/IEC61970/Base/Wires#MutualCoupling">
        <rdfs:subClassOf rdf:resource="https://w3id.org/netbeheer/referentiemodellen/IECCIM/TC57CIM/IEC61970/Base/Core#IdentifiedObject"/>
        <rdfs:subClassOf>
            <owl:Restriction>
                <owl:onProperty rdf:resource="https://w3id.org/netbeheer/referentiemodellen/IECCIM/TC57CIM/IEC61970/Base/Wires#MutualCoupling_b0ch"/>
                <owl:minQualifiedCardinality rdf:datatype="http://www.w3.org/2001/XMLSchema#nonNegativeInteger">0</owl:minQualifiedCardinality>
                <owl:onClass rdf:resource="https://w3id.org/netbeheer/referentiemodellen/IECCIM/TC57CIM/IEC61970/Base/Domain#Susceptance"/>
            </owl:Restriction>
        </rdfs:subClassOf>
        <rdfs:subClassOf>
            <owl:Restriction>
                <owl:onProperty rdf:resource="https://w3id.org/netbeheer/referentiemodellen/IECCIM/TC57CIM/IEC61970/Base/Wires#MutualCoupling_distance11"/>
                <owl:minQualifiedCardinality rdf:datatype="http://www.w3.org/2001/XMLSchema#nonNegativeInteger">0</owl:minQualifiedCardinality>
                <owl:onClass rdf:resource="https://w3id.org/netbeheer/referentiemodellen/IECCIM/TC57CIM/IEC61970/Base/Domain#Length"/>
            </owl:Restriction>
        </rdfs:subClassOf>
        <rdfs:subClassOf>
            <owl:Restriction>
                <owl:onProperty rdf:resource="https://w3id.org/netbeheer/referentiemodellen/IECCIM/TC57CIM/IEC61970/Base/Wires#MutualCoupling_distance12"/>
                <owl:minQualifiedCardinality rdf:datatype="http://www.w3.org/2001/XMLSchema#nonNegativeInteger">0</owl:minQualifiedCardinality>
                <owl:onClass rdf:resource="https://w3id.org/netbeheer/referentiemodellen/IECCIM/TC57CIM/IEC61970/Base/Domain#Length"/>
            </owl:Restriction>
        </rdfs:subClassOf>
        <rdfs:subClassOf>
            <owl:Restriction>
                <owl:onProperty rdf:resource="https://w3id.org/netbeheer/referentiemodellen/IECCIM/TC57CIM/IEC61970/Base/Wires#MutualCoupling_distance21"/>
                <owl:minQualifiedCardinality rdf:datatype="http://www.w3.org/2001/XMLSchema#nonNegativeInteger">0</owl:minQualifiedCardinality>
                <owl:onClass rdf:resource="https://w3id.org/netbeheer/referentiemodellen/IECCIM/TC57CIM/IEC61970/Base/Domain#Length"/>
            </owl:Restriction>
        </rdfs:subClassOf>
        <rdfs:subClassOf>
            <owl:Restriction>
                <owl:onProperty rdf:resource="https://w3id.org/netbeheer/referentiemodellen/IECCIM/TC57CIM/IEC61970/Base/Wires#MutualCoupling_distance22"/>
                <owl:minQualifiedCardinality rdf:datatype="http://www.w3.org/2001/XMLSchema#nonNegativeInteger">0</owl:minQualifiedCardinality>
                <owl:onClass rdf:resource="https://w3id.org/netbeheer/referentiemodellen/IECCIM/TC57CIM/IEC61970/Base/Domain#Length"/>
            </owl:Restriction>
        </rdfs:subClassOf>
        <rdfs:subClassOf>
            <owl:Restriction>
                <owl:onProperty rdf:resource="https://w3id.org/netbeheer/referentiemodellen/IECCIM/TC57CIM/IEC61970/Base/Wires#MutualCoupling_g0ch"/>
                <owl:minQualifiedCardinality rdf:datatype="http://www.w3.org/2001/XMLSchema#nonNegativeInteger">0</owl:minQualifiedCardinality>
                <owl:onClass rdf:resource="https://w3id.org/netbeheer/referentiemodellen/IECCIM/TC57CIM/IEC61970/Base/Domain#Conductance"/>
            </owl:Restriction>
        </rdfs:subClassOf>
        <rdfs:subClassOf>
            <owl:Restriction>
                <owl:onProperty rdf:resource="https://w3id.org/netbeheer/referentiemodellen/IECCIM/TC57CIM/IEC61970/Base/Wires#MutualCoupling_r0"/>
                <owl:minQualifiedCardinality rdf:datatype="http://www.w3.org/2001/XMLSchema#nonNegativeInteger">0</owl:minQualifiedCardinality>
                <owl:onClass rdf:resource="https://w3id.org/netbeheer/referentiemodellen/IECCIM/TC57CIM/IEC61970/Base/Domain#Resistance"/>
            </owl:Restriction>
        </rdfs:subClassOf>
        <rdfs:subClassOf>
            <owl:Restriction>
                <owl:onProperty rdf:resource="https://w3id.org/netbeheer/referentiemodellen/IECCIM/TC57CIM/IEC61970/Base/Wires#MutualCoupling_x0"/>
                <owl:minQualifiedCardinality rdf:datatype="http://www.w3.org/2001/XMLSchema#nonNegativeInteger">0</owl:minQualifiedCardinality>
                <owl:onClass rdf:resource="https://w3id.org/netbeheer/referentiemodellen/IECCIM/TC57CIM/IEC61970/Base/Domain#Reactance"/>
            </owl:Restriction>
        </rdfs:subClassOf>
        <rdfs:subClassOf>
            <owl:Restriction>
                <owl:onProperty rdf:resource="https://w3id.org/netbeheer/referentiemodellen/IECCIM/TC57CIM/IEC61970/Base/Wires#MutualCoupling_b0ch"/>
                <owl:maxQualifiedCardinality rdf:datatype="http://www.w3.org/2001/XMLSchema#nonNegativeInteger">1</owl:maxQualifiedCardinality>
                <owl:onClass rdf:resource="https://w3id.org/netbeheer/referentiemodellen/IECCIM/TC57CIM/IEC61970/Base/Domain#Susceptance"/>
            </owl:Restriction>
        </rdfs:subClassOf>
        <rdfs:subClassOf>
            <owl:Restriction>
                <owl:onProperty rdf:resource="https://w3id.org/netbeheer/referentiemodellen/IECCIM/TC57CIM/IEC61970/Base/Wires#MutualCoupling_distance11"/>
                <owl:maxQualifiedCardinality rdf:datatype="http://www.w3.org/2001/XMLSchema#nonNegativeInteger">1</owl:maxQualifiedCardinality>
                <owl:onClass rdf:resource="https://w3id.org/netbeheer/referentiemodellen/IECCIM/TC57CIM/IEC61970/Base/Domain#Length"/>
            </owl:Restriction>
        </rdfs:subClassOf>
        <rdfs:subClassOf>
            <owl:Restriction>
                <owl:onProperty rdf:resource="https://w3id.org/netbeheer/referentiemodellen/IECCIM/TC57CIM/IEC61970/Base/Wires#MutualCoupling_distance12"/>
                <owl:maxQualifiedCardinality rdf:datatype="http://www.w3.org/2001/XMLSchema#nonNegativeInteger">1</owl:maxQualifiedCardinality>
                <owl:onClass rdf:resource="https://w3id.org/netbeheer/referentiemodellen/IECCIM/TC57CIM/IEC61970/Base/Domain#Length"/>
            </owl:Restriction>
        </rdfs:subClassOf>
        <rdfs:subClassOf>
            <owl:Restriction>
                <owl:onProperty rdf:resource="https://w3id.org/netbeheer/referentiemodellen/IECCIM/TC57CIM/IEC61970/Base/Wires#MutualCoupling_distance21"/>
                <owl:maxQualifiedCardinality rdf:datatype="http://www.w3.org/2001/XMLSchema#nonNegativeInteger">1</owl:maxQualifiedCardinality>
                <owl:onClass rdf:resource="https://w3id.org/netbeheer/referentiemodellen/IECCIM/TC57CIM/IEC61970/Base/Domain#Length"/>
            </owl:Restriction>
        </rdfs:subClassOf>
        <rdfs:subClassOf>
            <owl:Restriction>
                <owl:onProperty rdf:resource="https://w3id.org/netbeheer/referentiemodellen/IECCIM/TC57CIM/IEC61970/Base/Wires#MutualCoupling_distance22"/>
                <owl:maxQualifiedCardinality rdf:datatype="http://www.w3.org/2001/XMLSchema#nonNegativeInteger">1</owl:maxQualifiedCardinality>
                <owl:onClass rdf:resource="https://w3id.org/netbeheer/referentiemodellen/IECCIM/TC57CIM/IEC61970/Base/Domain#Length"/>
            </owl:Restriction>
        </rdfs:subClassOf>
        <rdfs:subClassOf>
            <owl:Restriction>
                <owl:onProperty rdf:resource="https://w3id.org/netbeheer/referentiemodellen/IECCIM/TC57CIM/IEC61970/Base/Wires#MutualCoupling_g0ch"/>
                <owl:maxQualifiedCardinality rdf:datatype="http://www.w3.org/2001/XMLSchema#nonNegativeInteger">1</owl:maxQualifiedCardinality>
                <owl:onClass rdf:resource="https://w3id.org/netbeheer/referentiemodellen/IECCIM/TC57CIM/IEC61970/Base/Domain#Conductance"/>
            </owl:Restriction>
        </rdfs:subClassOf>
        <rdfs:subClassOf>
            <owl:Restriction>
                <owl:onProperty rdf:resource="https://w3id.org/netbeheer/referentiemodellen/IECCIM/TC57CIM/IEC61970/Base/Wires#MutualCoupling_r0"/>
                <owl:maxQualifiedCardinality rdf:datatype="http://www.w3.org/2001/XMLSchema#nonNegativeInteger">1</owl:maxQualifiedCardinality>
                <owl:onClass rdf:resource="https://w3id.org/netbeheer/referentiemodellen/IECCIM/TC57CIM/IEC61970/Base/Domain#Resistance"/>
            </owl:Restriction>
        </rdfs:subClassOf>
        <rdfs:subClassOf>
            <owl:Restriction>
                <owl:onProperty rdf:resource="https://w3id.org/netbeheer/referentiemodellen/IECCIM/TC57CIM/IEC61970/Base/Wires#MutualCoupling_x0"/>
                <owl:maxQualifiedCardinality rdf:datatype="http://www.w3.org/2001/XMLSchema#nonNegativeInteger">1</owl:maxQualifiedCardinality>
                <owl:onClass rdf:resource="https://w3id.org/netbeheer/referentiemodellen/IECCIM/TC57CIM/IEC61970/Base/Domain#Reactance"/>
            </owl:Restriction>
        </rdfs:subClassOf>
        <rdfs:comment>This class represents the zero sequence line mutual coupling.
</rdfs:comment>
    </owl:Class>
    


    <!-- https://w3id.org/netbeheer/referentiemodellen/IECCIM/TC57CIM/IEC61970/Base/Wires#NonlinearShuntCompensator -->


    <owl:Class rdf:about="https://w3id.org/netbeheer/referentiemodellen/IECCIM/TC57CIM/IEC61970/Base/Wires#NonlinearShuntCompensator">
        <rdfs:subClassOf rdf:resource="https://w3id.org/netbeheer/referentiemodellen/IECCIM/TC57CIM/IEC61970/Base/Wires#ShuntCompensator"/>
        <rdfs:subClassOf>
            <owl:Restriction>
                <owl:onProperty rdf:resource="https://w3id.org/netbeheer/referentiemodellen/IECCIM/TC57CIM/IEC61970/Base/Wires#NonlinearShuntCompensator_NonlinearShuntCompensatorPoints"/>
                <owl:qualifiedCardinality rdf:datatype="http://www.w3.org/2001/XMLSchema#nonNegativeInteger">1</owl:qualifiedCardinality>
                <owl:onClass rdf:resource="https://w3id.org/netbeheer/referentiemodellen/IECCIM/TC57CIM/IEC61970/Base/Wires#NonlinearShuntCompensator"/>
            </owl:Restriction>
        </rdfs:subClassOf>
        <rdfs:comment>A non linear shunt compensator has bank or section admittance values that differs.</rdfs:comment>
    </owl:Class>
    


    <!-- https://w3id.org/netbeheer/referentiemodellen/IECCIM/TC57CIM/IEC61970/Base/Wires#NonlinearShuntCompensatorPhase -->


    <owl:Class rdf:about="https://w3id.org/netbeheer/referentiemodellen/IECCIM/TC57CIM/IEC61970/Base/Wires#NonlinearShuntCompensatorPhase">
        <rdfs:subClassOf rdf:resource="https://w3id.org/netbeheer/referentiemodellen/IECCIM/TC57CIM/IEC61970/Base/Wires#ShuntCompensatorPhase"/>
        <rdfs:subClassOf>
            <owl:Restriction>
                <owl:onProperty rdf:resource="https://w3id.org/netbeheer/referentiemodellen/IECCIM/TC57CIM/IEC61970/Base/Wires#NonlinearShuntCompensatorPhase_NonlinearShuntCompensatorPhasePoints"/>
                <owl:qualifiedCardinality rdf:datatype="http://www.w3.org/2001/XMLSchema#nonNegativeInteger">1</owl:qualifiedCardinality>
                <owl:onClass rdf:resource="https://w3id.org/netbeheer/referentiemodellen/IECCIM/TC57CIM/IEC61970/Base/Wires#NonlinearShuntCompensatorPhase"/>
            </owl:Restriction>
        </rdfs:subClassOf>
        <rdfs:comment>A per phase non linear shunt compensator has bank or section admittance values that differs.</rdfs:comment>
    </owl:Class>
    


    <!-- https://w3id.org/netbeheer/referentiemodellen/IECCIM/TC57CIM/IEC61970/Base/Wires#NonlinearShuntCompensatorPhasePoint -->


    <owl:Class rdf:about="https://w3id.org/netbeheer/referentiemodellen/IECCIM/TC57CIM/IEC61970/Base/Wires#NonlinearShuntCompensatorPhasePoint">
        <rdfs:subClassOf>
            <owl:Restriction>
                <owl:onProperty rdf:resource="https://w3id.org/netbeheer/referentiemodellen/IECCIM/TC57CIM/IEC61970/Base/Wires#NonlinearShuntCompensatorPhasePoint_NonlinearShuntCompensatorPhase"/>
                <owl:minQualifiedCardinality rdf:datatype="http://www.w3.org/2001/XMLSchema#nonNegativeInteger">1</owl:minQualifiedCardinality>
                <owl:onClass rdf:resource="https://w3id.org/netbeheer/referentiemodellen/IECCIM/TC57CIM/IEC61970/Base/Wires#NonlinearShuntCompensatorPhasePoint"/>
            </owl:Restriction>
        </rdfs:subClassOf>
        <rdfs:subClassOf>
            <owl:Restriction>
                <owl:onProperty rdf:resource="https://w3id.org/netbeheer/referentiemodellen/IECCIM/TC57CIM/IEC61970/Base/Wires#NonlinearShuntCompensatorPhasePoint_b"/>
                <owl:minQualifiedCardinality rdf:datatype="http://www.w3.org/2001/XMLSchema#nonNegativeInteger">0</owl:minQualifiedCardinality>
                <owl:onClass rdf:resource="https://w3id.org/netbeheer/referentiemodellen/IECCIM/TC57CIM/IEC61970/Base/Domain#Susceptance"/>
            </owl:Restriction>
        </rdfs:subClassOf>
        <rdfs:subClassOf>
            <owl:Restriction>
                <owl:onProperty rdf:resource="https://w3id.org/netbeheer/referentiemodellen/IECCIM/TC57CIM/IEC61970/Base/Wires#NonlinearShuntCompensatorPhasePoint_g"/>
                <owl:minQualifiedCardinality rdf:datatype="http://www.w3.org/2001/XMLSchema#nonNegativeInteger">0</owl:minQualifiedCardinality>
                <owl:onClass rdf:resource="https://w3id.org/netbeheer/referentiemodellen/IECCIM/TC57CIM/IEC61970/Base/Domain#Conductance"/>
            </owl:Restriction>
        </rdfs:subClassOf>
        <rdfs:subClassOf>
            <owl:Restriction>
                <owl:onProperty rdf:resource="https://w3id.org/netbeheer/referentiemodellen/IECCIM/TC57CIM/IEC61970/Base/Wires#NonlinearShuntCompensatorPhasePoint_b"/>
                <owl:maxQualifiedCardinality rdf:datatype="http://www.w3.org/2001/XMLSchema#nonNegativeInteger">1</owl:maxQualifiedCardinality>
                <owl:onClass rdf:resource="https://w3id.org/netbeheer/referentiemodellen/IECCIM/TC57CIM/IEC61970/Base/Domain#Susceptance"/>
            </owl:Restriction>
        </rdfs:subClassOf>
        <rdfs:subClassOf>
            <owl:Restriction>
                <owl:onProperty rdf:resource="https://w3id.org/netbeheer/referentiemodellen/IECCIM/TC57CIM/IEC61970/Base/Wires#NonlinearShuntCompensatorPhasePoint_g"/>
                <owl:maxQualifiedCardinality rdf:datatype="http://www.w3.org/2001/XMLSchema#nonNegativeInteger">1</owl:maxQualifiedCardinality>
                <owl:onClass rdf:resource="https://w3id.org/netbeheer/referentiemodellen/IECCIM/TC57CIM/IEC61970/Base/Domain#Conductance"/>
            </owl:Restriction>
        </rdfs:subClassOf>
        <rdfs:subClassOf>
            <owl:Restriction>
                <owl:onProperty rdf:resource="https://w3id.org/netbeheer/referentiemodellen/IECCIM/TC57CIM/IEC61970/Base/Wires#NonlinearShuntCompensatorPhasePoint_sectionNumber"/>
                <owl:minQualifiedCardinality rdf:datatype="http://www.w3.org/2001/XMLSchema#nonNegativeInteger">0</owl:minQualifiedCardinality>
                <owl:onDataRange rdf:resource="http://www.w3.org/2001/XMLSchema#nonNegativeInteger"/>
            </owl:Restriction>
        </rdfs:subClassOf>
        <rdfs:subClassOf>
            <owl:Restriction>
                <owl:onProperty rdf:resource="https://w3id.org/netbeheer/referentiemodellen/IECCIM/TC57CIM/IEC61970/Base/Wires#NonlinearShuntCompensatorPhasePoint_sectionNumber"/>
                <owl:maxQualifiedCardinality rdf:datatype="http://www.w3.org/2001/XMLSchema#nonNegativeInteger">1</owl:maxQualifiedCardinality>
                <owl:onDataRange rdf:resource="http://www.w3.org/2001/XMLSchema#nonNegativeInteger"/>
            </owl:Restriction>
        </rdfs:subClassOf>
        <rdfs:comment>A per phase non linear shunt compensator bank or section admittance value.</rdfs:comment>
    </owl:Class>
    


    <!-- https://w3id.org/netbeheer/referentiemodellen/IECCIM/TC57CIM/IEC61970/Base/Wires#NonlinearShuntCompensatorPoint -->


    <owl:Class rdf:about="https://w3id.org/netbeheer/referentiemodellen/IECCIM/TC57CIM/IEC61970/Base/Wires#NonlinearShuntCompensatorPoint">
        <rdfs:subClassOf>
            <owl:Restriction>
                <owl:onProperty rdf:resource="https://w3id.org/netbeheer/referentiemodellen/IECCIM/TC57CIM/IEC61970/Base/Wires#NonlinearShuntCompensatorPoint_NonlinearShuntCompensator"/>
                <owl:minQualifiedCardinality rdf:datatype="http://www.w3.org/2001/XMLSchema#nonNegativeInteger">1</owl:minQualifiedCardinality>
                <owl:onClass rdf:resource="https://w3id.org/netbeheer/referentiemodellen/IECCIM/TC57CIM/IEC61970/Base/Wires#NonlinearShuntCompensatorPoint"/>
            </owl:Restriction>
        </rdfs:subClassOf>
        <rdfs:subClassOf>
            <owl:Restriction>
                <owl:onProperty rdf:resource="https://w3id.org/netbeheer/referentiemodellen/IECCIM/TC57CIM/IEC61970/Base/Wires#NonlinearShuntCompensatorPoint_b"/>
                <owl:minQualifiedCardinality rdf:datatype="http://www.w3.org/2001/XMLSchema#nonNegativeInteger">0</owl:minQualifiedCardinality>
                <owl:onClass rdf:resource="https://w3id.org/netbeheer/referentiemodellen/IECCIM/TC57CIM/IEC61970/Base/Domain#Susceptance"/>
            </owl:Restriction>
        </rdfs:subClassOf>
        <rdfs:subClassOf>
            <owl:Restriction>
                <owl:onProperty rdf:resource="https://w3id.org/netbeheer/referentiemodellen/IECCIM/TC57CIM/IEC61970/Base/Wires#NonlinearShuntCompensatorPoint_b0"/>
                <owl:minQualifiedCardinality rdf:datatype="http://www.w3.org/2001/XMLSchema#nonNegativeInteger">0</owl:minQualifiedCardinality>
                <owl:onClass rdf:resource="https://w3id.org/netbeheer/referentiemodellen/IECCIM/TC57CIM/IEC61970/Base/Domain#Susceptance"/>
            </owl:Restriction>
        </rdfs:subClassOf>
        <rdfs:subClassOf>
            <owl:Restriction>
                <owl:onProperty rdf:resource="https://w3id.org/netbeheer/referentiemodellen/IECCIM/TC57CIM/IEC61970/Base/Wires#NonlinearShuntCompensatorPoint_g"/>
                <owl:minQualifiedCardinality rdf:datatype="http://www.w3.org/2001/XMLSchema#nonNegativeInteger">0</owl:minQualifiedCardinality>
                <owl:onClass rdf:resource="https://w3id.org/netbeheer/referentiemodellen/IECCIM/TC57CIM/IEC61970/Base/Domain#Conductance"/>
            </owl:Restriction>
        </rdfs:subClassOf>
        <rdfs:subClassOf>
            <owl:Restriction>
                <owl:onProperty rdf:resource="https://w3id.org/netbeheer/referentiemodellen/IECCIM/TC57CIM/IEC61970/Base/Wires#NonlinearShuntCompensatorPoint_g0"/>
                <owl:minQualifiedCardinality rdf:datatype="http://www.w3.org/2001/XMLSchema#nonNegativeInteger">0</owl:minQualifiedCardinality>
                <owl:onClass rdf:resource="https://w3id.org/netbeheer/referentiemodellen/IECCIM/TC57CIM/IEC61970/Base/Domain#Conductance"/>
            </owl:Restriction>
        </rdfs:subClassOf>
        <rdfs:subClassOf>
            <owl:Restriction>
                <owl:onProperty rdf:resource="https://w3id.org/netbeheer/referentiemodellen/IECCIM/TC57CIM/IEC61970/Base/Wires#NonlinearShuntCompensatorPoint_b"/>
                <owl:maxQualifiedCardinality rdf:datatype="http://www.w3.org/2001/XMLSchema#nonNegativeInteger">1</owl:maxQualifiedCardinality>
                <owl:onClass rdf:resource="https://w3id.org/netbeheer/referentiemodellen/IECCIM/TC57CIM/IEC61970/Base/Domain#Susceptance"/>
            </owl:Restriction>
        </rdfs:subClassOf>
        <rdfs:subClassOf>
            <owl:Restriction>
                <owl:onProperty rdf:resource="https://w3id.org/netbeheer/referentiemodellen/IECCIM/TC57CIM/IEC61970/Base/Wires#NonlinearShuntCompensatorPoint_b0"/>
                <owl:maxQualifiedCardinality rdf:datatype="http://www.w3.org/2001/XMLSchema#nonNegativeInteger">1</owl:maxQualifiedCardinality>
                <owl:onClass rdf:resource="https://w3id.org/netbeheer/referentiemodellen/IECCIM/TC57CIM/IEC61970/Base/Domain#Susceptance"/>
            </owl:Restriction>
        </rdfs:subClassOf>
        <rdfs:subClassOf>
            <owl:Restriction>
                <owl:onProperty rdf:resource="https://w3id.org/netbeheer/referentiemodellen/IECCIM/TC57CIM/IEC61970/Base/Wires#NonlinearShuntCompensatorPoint_g"/>
                <owl:maxQualifiedCardinality rdf:datatype="http://www.w3.org/2001/XMLSchema#nonNegativeInteger">1</owl:maxQualifiedCardinality>
                <owl:onClass rdf:resource="https://w3id.org/netbeheer/referentiemodellen/IECCIM/TC57CIM/IEC61970/Base/Domain#Conductance"/>
            </owl:Restriction>
        </rdfs:subClassOf>
        <rdfs:subClassOf>
            <owl:Restriction>
                <owl:onProperty rdf:resource="https://w3id.org/netbeheer/referentiemodellen/IECCIM/TC57CIM/IEC61970/Base/Wires#NonlinearShuntCompensatorPoint_g0"/>
                <owl:maxQualifiedCardinality rdf:datatype="http://www.w3.org/2001/XMLSchema#nonNegativeInteger">1</owl:maxQualifiedCardinality>
                <owl:onClass rdf:resource="https://w3id.org/netbeheer/referentiemodellen/IECCIM/TC57CIM/IEC61970/Base/Domain#Conductance"/>
            </owl:Restriction>
        </rdfs:subClassOf>
        <rdfs:subClassOf>
            <owl:Restriction>
                <owl:onProperty rdf:resource="https://w3id.org/netbeheer/referentiemodellen/IECCIM/TC57CIM/IEC61970/Base/Wires#NonlinearShuntCompensatorPoint_sectionNumber"/>
                <owl:minQualifiedCardinality rdf:datatype="http://www.w3.org/2001/XMLSchema#nonNegativeInteger">0</owl:minQualifiedCardinality>
                <owl:onDataRange rdf:resource="http://www.w3.org/2001/XMLSchema#nonNegativeInteger"/>
            </owl:Restriction>
        </rdfs:subClassOf>
        <rdfs:subClassOf>
            <owl:Restriction>
                <owl:onProperty rdf:resource="https://w3id.org/netbeheer/referentiemodellen/IECCIM/TC57CIM/IEC61970/Base/Wires#NonlinearShuntCompensatorPoint_sectionNumber"/>
                <owl:maxQualifiedCardinality rdf:datatype="http://www.w3.org/2001/XMLSchema#nonNegativeInteger">1</owl:maxQualifiedCardinality>
                <owl:onDataRange rdf:resource="http://www.w3.org/2001/XMLSchema#nonNegativeInteger"/>
            </owl:Restriction>
        </rdfs:subClassOf>
        <rdfs:comment>A non linear shunt compensator bank or section admittance value.</rdfs:comment>
    </owl:Class>
    


    <!-- https://w3id.org/netbeheer/referentiemodellen/IECCIM/TC57CIM/IEC61970/Base/Wires#PerLengthImpedance -->


    <owl:Class rdf:about="https://w3id.org/netbeheer/referentiemodellen/IECCIM/TC57CIM/IEC61970/Base/Wires#PerLengthImpedance">
        <rdfs:subClassOf rdf:resource="https://w3id.org/netbeheer/referentiemodellen/IECCIM/TC57CIM/IEC61970/Base/Wires#PerLengthLineParameter"/>
        <rdfs:subClassOf>
            <owl:Restriction>
                <owl:onProperty rdf:resource="https://w3id.org/netbeheer/referentiemodellen/IECCIM/TC57CIM/IEC61970/Base/Wires#PerLengthImpedance_ACLineSegments"/>
                <owl:minQualifiedCardinality rdf:datatype="http://www.w3.org/2001/XMLSchema#nonNegativeInteger">0</owl:minQualifiedCardinality>
                <owl:onClass rdf:resource="https://w3id.org/netbeheer/referentiemodellen/IECCIM/TC57CIM/IEC61970/Base/Wires#PerLengthImpedance"/>
            </owl:Restriction>
        </rdfs:subClassOf>
        <rdfs:subClassOf>
            <owl:Restriction>
                <owl:onProperty rdf:resource="https://w3id.org/netbeheer/referentiemodellen/IECCIM/TC57CIM/IEC61970/Base/Wires#PerLengthImpedance_ACLineSegments"/>
                <owl:maxQualifiedCardinality rdf:datatype="http://www.w3.org/2001/XMLSchema#nonNegativeInteger">1</owl:maxQualifiedCardinality>
                <owl:onClass rdf:resource="https://w3id.org/netbeheer/referentiemodellen/IECCIM/TC57CIM/IEC61970/Base/Wires#PerLengthImpedance"/>
            </owl:Restriction>
        </rdfs:subClassOf>
        <rdfs:comment>Common type for per-length impedance electrical catalogues.
</rdfs:comment>
    </owl:Class>
    


    <!-- https://w3id.org/netbeheer/referentiemodellen/IECCIM/TC57CIM/IEC61970/Base/Wires#PerLengthLineParameter -->


    <owl:Class rdf:about="https://w3id.org/netbeheer/referentiemodellen/IECCIM/TC57CIM/IEC61970/Base/Wires#PerLengthLineParameter">
        <rdfs:subClassOf rdf:resource="https://w3id.org/netbeheer/referentiemodellen/IECCIM/TC57CIM/IEC61970/Base/Core#IdentifiedObject"/>
        <rdfs:subClassOf>
            <owl:Restriction>
                <owl:onProperty rdf:resource="https://w3id.org/netbeheer/referentiemodellen/IECCIM/TC57CIM/IEC61970/Base/Wires#PerLengthLineParameter_WireInfos"/>
                <owl:minQualifiedCardinality rdf:datatype="http://www.w3.org/2001/XMLSchema#nonNegativeInteger">0</owl:minQualifiedCardinality>
                <owl:onClass rdf:resource="https://w3id.org/netbeheer/referentiemodellen/IECCIM/TC57CIM/IEC61970/Base/Wires#PerLengthLineParameter"/>
            </owl:Restriction>
        </rdfs:subClassOf>
        <rdfs:subClassOf>
            <owl:Restriction>
                <owl:onProperty rdf:resource="https://w3id.org/netbeheer/referentiemodellen/IECCIM/TC57CIM/IEC61970/Base/Wires#PerLengthLineParameter_WireSpacingInfo"/>
                <owl:minQualifiedCardinality rdf:datatype="http://www.w3.org/2001/XMLSchema#nonNegativeInteger">0</owl:minQualifiedCardinality>
                <owl:onClass rdf:resource="https://w3id.org/netbeheer/referentiemodellen/IECCIM/TC57CIM/IEC61970/Base/Wires#PerLengthLineParameter"/>
            </owl:Restriction>
        </rdfs:subClassOf>
        <rdfs:comment>Common type for per-length electrical catalogues describing line parameters.</rdfs:comment>
    </owl:Class>
    


    <!-- https://w3id.org/netbeheer/referentiemodellen/IECCIM/TC57CIM/IEC61970/Base/Wires#PerLengthPhaseImpedance -->


    <owl:Class rdf:about="https://w3id.org/netbeheer/referentiemodellen/IECCIM/TC57CIM/IEC61970/Base/Wires#PerLengthPhaseImpedance">
        <rdfs:subClassOf rdf:resource="https://w3id.org/netbeheer/referentiemodellen/IECCIM/TC57CIM/IEC61970/Base/Wires#PerLengthImpedance"/>
        <rdfs:subClassOf>
            <owl:Restriction>
                <owl:onProperty rdf:resource="https://w3id.org/netbeheer/referentiemodellen/IECCIM/TC57CIM/IEC61970/Base/Wires#PerLengthPhaseImpedance_PhaseImpedanceData"/>
                <owl:qualifiedCardinality rdf:datatype="http://www.w3.org/2001/XMLSchema#nonNegativeInteger">1</owl:qualifiedCardinality>
                <owl:onClass rdf:resource="https://w3id.org/netbeheer/referentiemodellen/IECCIM/TC57CIM/IEC61970/Base/Wires#PerLengthPhaseImpedance"/>
            </owl:Restriction>
        </rdfs:subClassOf>
        <rdfs:subClassOf>
            <owl:Restriction>
                <owl:onProperty rdf:resource="https://w3id.org/netbeheer/referentiemodellen/IECCIM/TC57CIM/IEC61970/Base/Wires#PerLengthPhaseImpedance_conductorCount"/>
                <owl:minQualifiedCardinality rdf:datatype="http://www.w3.org/2001/XMLSchema#nonNegativeInteger">0</owl:minQualifiedCardinality>
                <owl:onDataRange rdf:resource="http://www.w3.org/2001/XMLSchema#nonNegativeInteger"/>
            </owl:Restriction>
        </rdfs:subClassOf>
        <rdfs:subClassOf>
            <owl:Restriction>
                <owl:onProperty rdf:resource="https://w3id.org/netbeheer/referentiemodellen/IECCIM/TC57CIM/IEC61970/Base/Wires#PerLengthPhaseImpedance_conductorCount"/>
                <owl:maxQualifiedCardinality rdf:datatype="http://www.w3.org/2001/XMLSchema#nonNegativeInteger">1</owl:maxQualifiedCardinality>
                <owl:onDataRange rdf:resource="http://www.w3.org/2001/XMLSchema#nonNegativeInteger"/>
            </owl:Restriction>
        </rdfs:subClassOf>
        <rdfs:comment>Impedance and admittance parameters per unit length for n-wire unbalanced lines, in matrix form.</rdfs:comment>
    </owl:Class>
    


    <!-- https://w3id.org/netbeheer/referentiemodellen/IECCIM/TC57CIM/IEC61970/Base/Wires#PerLengthSequenceImpedance -->


    <owl:Class rdf:about="https://w3id.org/netbeheer/referentiemodellen/IECCIM/TC57CIM/IEC61970/Base/Wires#PerLengthSequenceImpedance">
        <rdfs:subClassOf rdf:resource="https://w3id.org/netbeheer/referentiemodellen/IECCIM/TC57CIM/IEC61970/Base/Wires#PerLengthImpedance"/>
        <rdfs:subClassOf>
            <owl:Restriction>
                <owl:onProperty rdf:resource="https://w3id.org/netbeheer/referentiemodellen/IECCIM/TC57CIM/IEC61970/Base/Wires#PerLengthSequenceImpedance_b0ch"/>
                <owl:minQualifiedCardinality rdf:datatype="http://www.w3.org/2001/XMLSchema#nonNegativeInteger">0</owl:minQualifiedCardinality>
                <owl:onClass rdf:resource="https://w3id.org/netbeheer/referentiemodellen/IECCIM/TC57CIM/IEC61970/Base/Domain#SusceptancePerLength"/>
            </owl:Restriction>
        </rdfs:subClassOf>
        <rdfs:subClassOf>
            <owl:Restriction>
                <owl:onProperty rdf:resource="https://w3id.org/netbeheer/referentiemodellen/IECCIM/TC57CIM/IEC61970/Base/Wires#PerLengthSequenceImpedance_bch"/>
                <owl:minQualifiedCardinality rdf:datatype="http://www.w3.org/2001/XMLSchema#nonNegativeInteger">0</owl:minQualifiedCardinality>
                <owl:onClass rdf:resource="https://w3id.org/netbeheer/referentiemodellen/IECCIM/TC57CIM/IEC61970/Base/Domain#SusceptancePerLength"/>
            </owl:Restriction>
        </rdfs:subClassOf>
        <rdfs:subClassOf>
            <owl:Restriction>
                <owl:onProperty rdf:resource="https://w3id.org/netbeheer/referentiemodellen/IECCIM/TC57CIM/IEC61970/Base/Wires#PerLengthSequenceImpedance_g0ch"/>
                <owl:minQualifiedCardinality rdf:datatype="http://www.w3.org/2001/XMLSchema#nonNegativeInteger">0</owl:minQualifiedCardinality>
                <owl:onClass rdf:resource="https://w3id.org/netbeheer/referentiemodellen/IECCIM/TC57CIM/IEC61970/Base/Domain#ConductancePerLength"/>
            </owl:Restriction>
        </rdfs:subClassOf>
        <rdfs:subClassOf>
            <owl:Restriction>
                <owl:onProperty rdf:resource="https://w3id.org/netbeheer/referentiemodellen/IECCIM/TC57CIM/IEC61970/Base/Wires#PerLengthSequenceImpedance_gch"/>
                <owl:minQualifiedCardinality rdf:datatype="http://www.w3.org/2001/XMLSchema#nonNegativeInteger">0</owl:minQualifiedCardinality>
                <owl:onClass rdf:resource="https://w3id.org/netbeheer/referentiemodellen/IECCIM/TC57CIM/IEC61970/Base/Domain#ConductancePerLength"/>
            </owl:Restriction>
        </rdfs:subClassOf>
        <rdfs:subClassOf>
            <owl:Restriction>
                <owl:onProperty rdf:resource="https://w3id.org/netbeheer/referentiemodellen/IECCIM/TC57CIM/IEC61970/Base/Wires#PerLengthSequenceImpedance_r"/>
                <owl:minQualifiedCardinality rdf:datatype="http://www.w3.org/2001/XMLSchema#nonNegativeInteger">0</owl:minQualifiedCardinality>
                <owl:onClass rdf:resource="https://w3id.org/netbeheer/referentiemodellen/IECCIM/TC57CIM/IEC61970/Base/Domain#ResistancePerLength"/>
            </owl:Restriction>
        </rdfs:subClassOf>
        <rdfs:subClassOf>
            <owl:Restriction>
                <owl:onProperty rdf:resource="https://w3id.org/netbeheer/referentiemodellen/IECCIM/TC57CIM/IEC61970/Base/Wires#PerLengthSequenceImpedance_r0"/>
                <owl:minQualifiedCardinality rdf:datatype="http://www.w3.org/2001/XMLSchema#nonNegativeInteger">0</owl:minQualifiedCardinality>
                <owl:onClass rdf:resource="https://w3id.org/netbeheer/referentiemodellen/IECCIM/TC57CIM/IEC61970/Base/Domain#ResistancePerLength"/>
            </owl:Restriction>
        </rdfs:subClassOf>
        <rdfs:subClassOf>
            <owl:Restriction>
                <owl:onProperty rdf:resource="https://w3id.org/netbeheer/referentiemodellen/IECCIM/TC57CIM/IEC61970/Base/Wires#PerLengthSequenceImpedance_x"/>
                <owl:minQualifiedCardinality rdf:datatype="http://www.w3.org/2001/XMLSchema#nonNegativeInteger">0</owl:minQualifiedCardinality>
                <owl:onClass rdf:resource="https://w3id.org/netbeheer/referentiemodellen/IECCIM/TC57CIM/IEC61970/Base/Domain#ReactancePerLength"/>
            </owl:Restriction>
        </rdfs:subClassOf>
        <rdfs:subClassOf>
            <owl:Restriction>
                <owl:onProperty rdf:resource="https://w3id.org/netbeheer/referentiemodellen/IECCIM/TC57CIM/IEC61970/Base/Wires#PerLengthSequenceImpedance_x0"/>
                <owl:minQualifiedCardinality rdf:datatype="http://www.w3.org/2001/XMLSchema#nonNegativeInteger">0</owl:minQualifiedCardinality>
                <owl:onClass rdf:resource="https://w3id.org/netbeheer/referentiemodellen/IECCIM/TC57CIM/IEC61970/Base/Domain#ReactancePerLength"/>
            </owl:Restriction>
        </rdfs:subClassOf>
        <rdfs:subClassOf>
            <owl:Restriction>
                <owl:onProperty rdf:resource="https://w3id.org/netbeheer/referentiemodellen/IECCIM/TC57CIM/IEC61970/Base/Wires#PerLengthSequenceImpedance_b0ch"/>
                <owl:maxQualifiedCardinality rdf:datatype="http://www.w3.org/2001/XMLSchema#nonNegativeInteger">1</owl:maxQualifiedCardinality>
                <owl:onClass rdf:resource="https://w3id.org/netbeheer/referentiemodellen/IECCIM/TC57CIM/IEC61970/Base/Domain#SusceptancePerLength"/>
            </owl:Restriction>
        </rdfs:subClassOf>
        <rdfs:subClassOf>
            <owl:Restriction>
                <owl:onProperty rdf:resource="https://w3id.org/netbeheer/referentiemodellen/IECCIM/TC57CIM/IEC61970/Base/Wires#PerLengthSequenceImpedance_bch"/>
                <owl:maxQualifiedCardinality rdf:datatype="http://www.w3.org/2001/XMLSchema#nonNegativeInteger">1</owl:maxQualifiedCardinality>
                <owl:onClass rdf:resource="https://w3id.org/netbeheer/referentiemodellen/IECCIM/TC57CIM/IEC61970/Base/Domain#SusceptancePerLength"/>
            </owl:Restriction>
        </rdfs:subClassOf>
        <rdfs:subClassOf>
            <owl:Restriction>
                <owl:onProperty rdf:resource="https://w3id.org/netbeheer/referentiemodellen/IECCIM/TC57CIM/IEC61970/Base/Wires#PerLengthSequenceImpedance_g0ch"/>
                <owl:maxQualifiedCardinality rdf:datatype="http://www.w3.org/2001/XMLSchema#nonNegativeInteger">1</owl:maxQualifiedCardinality>
                <owl:onClass rdf:resource="https://w3id.org/netbeheer/referentiemodellen/IECCIM/TC57CIM/IEC61970/Base/Domain#ConductancePerLength"/>
            </owl:Restriction>
        </rdfs:subClassOf>
        <rdfs:subClassOf>
            <owl:Restriction>
                <owl:onProperty rdf:resource="https://w3id.org/netbeheer/referentiemodellen/IECCIM/TC57CIM/IEC61970/Base/Wires#PerLengthSequenceImpedance_gch"/>
                <owl:maxQualifiedCardinality rdf:datatype="http://www.w3.org/2001/XMLSchema#nonNegativeInteger">1</owl:maxQualifiedCardinality>
                <owl:onClass rdf:resource="https://w3id.org/netbeheer/referentiemodellen/IECCIM/TC57CIM/IEC61970/Base/Domain#ConductancePerLength"/>
            </owl:Restriction>
        </rdfs:subClassOf>
        <rdfs:subClassOf>
            <owl:Restriction>
                <owl:onProperty rdf:resource="https://w3id.org/netbeheer/referentiemodellen/IECCIM/TC57CIM/IEC61970/Base/Wires#PerLengthSequenceImpedance_r"/>
                <owl:maxQualifiedCardinality rdf:datatype="http://www.w3.org/2001/XMLSchema#nonNegativeInteger">1</owl:maxQualifiedCardinality>
                <owl:onClass rdf:resource="https://w3id.org/netbeheer/referentiemodellen/IECCIM/TC57CIM/IEC61970/Base/Domain#ResistancePerLength"/>
            </owl:Restriction>
        </rdfs:subClassOf>
        <rdfs:subClassOf>
            <owl:Restriction>
                <owl:onProperty rdf:resource="https://w3id.org/netbeheer/referentiemodellen/IECCIM/TC57CIM/IEC61970/Base/Wires#PerLengthSequenceImpedance_r0"/>
                <owl:maxQualifiedCardinality rdf:datatype="http://www.w3.org/2001/XMLSchema#nonNegativeInteger">1</owl:maxQualifiedCardinality>
                <owl:onClass rdf:resource="https://w3id.org/netbeheer/referentiemodellen/IECCIM/TC57CIM/IEC61970/Base/Domain#ResistancePerLength"/>
            </owl:Restriction>
        </rdfs:subClassOf>
        <rdfs:subClassOf>
            <owl:Restriction>
                <owl:onProperty rdf:resource="https://w3id.org/netbeheer/referentiemodellen/IECCIM/TC57CIM/IEC61970/Base/Wires#PerLengthSequenceImpedance_x"/>
                <owl:maxQualifiedCardinality rdf:datatype="http://www.w3.org/2001/XMLSchema#nonNegativeInteger">1</owl:maxQualifiedCardinality>
                <owl:onClass rdf:resource="https://w3id.org/netbeheer/referentiemodellen/IECCIM/TC57CIM/IEC61970/Base/Domain#ReactancePerLength"/>
            </owl:Restriction>
        </rdfs:subClassOf>
        <rdfs:subClassOf>
            <owl:Restriction>
                <owl:onProperty rdf:resource="https://w3id.org/netbeheer/referentiemodellen/IECCIM/TC57CIM/IEC61970/Base/Wires#PerLengthSequenceImpedance_x0"/>
                <owl:maxQualifiedCardinality rdf:datatype="http://www.w3.org/2001/XMLSchema#nonNegativeInteger">1</owl:maxQualifiedCardinality>
                <owl:onClass rdf:resource="https://w3id.org/netbeheer/referentiemodellen/IECCIM/TC57CIM/IEC61970/Base/Domain#ReactancePerLength"/>
            </owl:Restriction>
        </rdfs:subClassOf>
        <rdfs:comment>Sequence impedance and admittance parameters per unit length, for transposed lines of 1, 2, or 3 phases. For 1-phase lines, define x=x0=xself. For 2-phase lines, define x=xs-xm and x0=xs+xm.</rdfs:comment>
    </owl:Class>
    


    <!-- https://w3id.org/netbeheer/referentiemodellen/IECCIM/TC57CIM/IEC61970/Base/Wires#PetersenCoil -->


    <owl:Class rdf:about="https://w3id.org/netbeheer/referentiemodellen/IECCIM/TC57CIM/IEC61970/Base/Wires#PetersenCoil">
        <rdfs:subClassOf rdf:resource="https://w3id.org/netbeheer/referentiemodellen/IECCIM/TC57CIM/IEC61970/Base/Wires#EarthFaultCompensator"/>
        <rdfs:subClassOf>
            <owl:Restriction>
                <owl:onProperty rdf:resource="https://w3id.org/netbeheer/referentiemodellen/IECCIM/TC57CIM/IEC61970/Base/Wires#PetersenCoil_nominalU"/>
                <owl:minQualifiedCardinality rdf:datatype="http://www.w3.org/2001/XMLSchema#nonNegativeInteger">0</owl:minQualifiedCardinality>
                <owl:onClass rdf:resource="https://w3id.org/netbeheer/referentiemodellen/IECCIM/TC57CIM/IEC61970/Base/Domain#Voltage"/>
            </owl:Restriction>
        </rdfs:subClassOf>
        <rdfs:subClassOf>
            <owl:Restriction>
                <owl:onProperty rdf:resource="https://w3id.org/netbeheer/referentiemodellen/IECCIM/TC57CIM/IEC61970/Base/Wires#PetersenCoil_offsetCurrent"/>
                <owl:minQualifiedCardinality rdf:datatype="http://www.w3.org/2001/XMLSchema#nonNegativeInteger">0</owl:minQualifiedCardinality>
                <owl:onClass rdf:resource="https://w3id.org/netbeheer/referentiemodellen/IECCIM/TC57CIM/IEC61970/Base/Domain#CurrentFlow"/>
            </owl:Restriction>
        </rdfs:subClassOf>
        <rdfs:subClassOf>
            <owl:Restriction>
                <owl:onProperty rdf:resource="https://w3id.org/netbeheer/referentiemodellen/IECCIM/TC57CIM/IEC61970/Base/Wires#PetersenCoil_positionCurrent"/>
                <owl:minQualifiedCardinality rdf:datatype="http://www.w3.org/2001/XMLSchema#nonNegativeInteger">0</owl:minQualifiedCardinality>
                <owl:onClass rdf:resource="https://w3id.org/netbeheer/referentiemodellen/IECCIM/TC57CIM/IEC61970/Base/Domain#CurrentFlow"/>
            </owl:Restriction>
        </rdfs:subClassOf>
        <rdfs:subClassOf>
            <owl:Restriction>
                <owl:onProperty rdf:resource="https://w3id.org/netbeheer/referentiemodellen/IECCIM/TC57CIM/IEC61970/Base/Wires#PetersenCoil_xGroundMax"/>
                <owl:minQualifiedCardinality rdf:datatype="http://www.w3.org/2001/XMLSchema#nonNegativeInteger">0</owl:minQualifiedCardinality>
                <owl:onClass rdf:resource="https://w3id.org/netbeheer/referentiemodellen/IECCIM/TC57CIM/IEC61970/Base/Domain#Reactance"/>
            </owl:Restriction>
        </rdfs:subClassOf>
        <rdfs:subClassOf>
            <owl:Restriction>
                <owl:onProperty rdf:resource="https://w3id.org/netbeheer/referentiemodellen/IECCIM/TC57CIM/IEC61970/Base/Wires#PetersenCoil_xGroundMin"/>
                <owl:minQualifiedCardinality rdf:datatype="http://www.w3.org/2001/XMLSchema#nonNegativeInteger">0</owl:minQualifiedCardinality>
                <owl:onClass rdf:resource="https://w3id.org/netbeheer/referentiemodellen/IECCIM/TC57CIM/IEC61970/Base/Domain#Reactance"/>
            </owl:Restriction>
        </rdfs:subClassOf>
        <rdfs:subClassOf>
            <owl:Restriction>
                <owl:onProperty rdf:resource="https://w3id.org/netbeheer/referentiemodellen/IECCIM/TC57CIM/IEC61970/Base/Wires#PetersenCoil_xGroundNominal"/>
                <owl:minQualifiedCardinality rdf:datatype="http://www.w3.org/2001/XMLSchema#nonNegativeInteger">0</owl:minQualifiedCardinality>
                <owl:onClass rdf:resource="https://w3id.org/netbeheer/referentiemodellen/IECCIM/TC57CIM/IEC61970/Base/Domain#Reactance"/>
            </owl:Restriction>
        </rdfs:subClassOf>
        <rdfs:subClassOf>
            <owl:Restriction>
                <owl:onProperty rdf:resource="https://w3id.org/netbeheer/referentiemodellen/IECCIM/TC57CIM/IEC61970/Base/Wires#PetersenCoil_nominalU"/>
                <owl:maxQualifiedCardinality rdf:datatype="http://www.w3.org/2001/XMLSchema#nonNegativeInteger">1</owl:maxQualifiedCardinality>
                <owl:onClass rdf:resource="https://w3id.org/netbeheer/referentiemodellen/IECCIM/TC57CIM/IEC61970/Base/Domain#Voltage"/>
            </owl:Restriction>
        </rdfs:subClassOf>
        <rdfs:subClassOf>
            <owl:Restriction>
                <owl:onProperty rdf:resource="https://w3id.org/netbeheer/referentiemodellen/IECCIM/TC57CIM/IEC61970/Base/Wires#PetersenCoil_offsetCurrent"/>
                <owl:maxQualifiedCardinality rdf:datatype="http://www.w3.org/2001/XMLSchema#nonNegativeInteger">1</owl:maxQualifiedCardinality>
                <owl:onClass rdf:resource="https://w3id.org/netbeheer/referentiemodellen/IECCIM/TC57CIM/IEC61970/Base/Domain#CurrentFlow"/>
            </owl:Restriction>
        </rdfs:subClassOf>
        <rdfs:subClassOf>
            <owl:Restriction>
                <owl:onProperty rdf:resource="https://w3id.org/netbeheer/referentiemodellen/IECCIM/TC57CIM/IEC61970/Base/Wires#PetersenCoil_positionCurrent"/>
                <owl:maxQualifiedCardinality rdf:datatype="http://www.w3.org/2001/XMLSchema#nonNegativeInteger">1</owl:maxQualifiedCardinality>
                <owl:onClass rdf:resource="https://w3id.org/netbeheer/referentiemodellen/IECCIM/TC57CIM/IEC61970/Base/Domain#CurrentFlow"/>
            </owl:Restriction>
        </rdfs:subClassOf>
        <rdfs:subClassOf>
            <owl:Restriction>
                <owl:onProperty rdf:resource="https://w3id.org/netbeheer/referentiemodellen/IECCIM/TC57CIM/IEC61970/Base/Wires#PetersenCoil_xGroundMax"/>
                <owl:maxQualifiedCardinality rdf:datatype="http://www.w3.org/2001/XMLSchema#nonNegativeInteger">1</owl:maxQualifiedCardinality>
                <owl:onClass rdf:resource="https://w3id.org/netbeheer/referentiemodellen/IECCIM/TC57CIM/IEC61970/Base/Domain#Reactance"/>
            </owl:Restriction>
        </rdfs:subClassOf>
        <rdfs:subClassOf>
            <owl:Restriction>
                <owl:onProperty rdf:resource="https://w3id.org/netbeheer/referentiemodellen/IECCIM/TC57CIM/IEC61970/Base/Wires#PetersenCoil_xGroundMin"/>
                <owl:maxQualifiedCardinality rdf:datatype="http://www.w3.org/2001/XMLSchema#nonNegativeInteger">1</owl:maxQualifiedCardinality>
                <owl:onClass rdf:resource="https://w3id.org/netbeheer/referentiemodellen/IECCIM/TC57CIM/IEC61970/Base/Domain#Reactance"/>
            </owl:Restriction>
        </rdfs:subClassOf>
        <rdfs:subClassOf>
            <owl:Restriction>
                <owl:onProperty rdf:resource="https://w3id.org/netbeheer/referentiemodellen/IECCIM/TC57CIM/IEC61970/Base/Wires#PetersenCoil_xGroundNominal"/>
                <owl:maxQualifiedCardinality rdf:datatype="http://www.w3.org/2001/XMLSchema#nonNegativeInteger">1</owl:maxQualifiedCardinality>
                <owl:onClass rdf:resource="https://w3id.org/netbeheer/referentiemodellen/IECCIM/TC57CIM/IEC61970/Base/Domain#Reactance"/>
            </owl:Restriction>
        </rdfs:subClassOf>
        <rdfs:subClassOf>
            <owl:Restriction>
                <owl:onProperty rdf:resource="https://w3id.org/netbeheer/referentiemodellen/IECCIM/TC57CIM/IEC61970/Base/Wires#PetersenCoil_mode"/>
                <owl:minQualifiedCardinality rdf:datatype="http://www.w3.org/2001/XMLSchema#nonNegativeInteger">0</owl:minQualifiedCardinality>
                <owl:onDataRange rdf:resource="https://w3id.org/netbeheer/referentiemodellen/IECCIM/TC57CIM/IEC61970/Base/Wires#PetersenCoilModeKind"/>
            </owl:Restriction>
        </rdfs:subClassOf>
        <rdfs:subClassOf>
            <owl:Restriction>
                <owl:onProperty rdf:resource="https://w3id.org/netbeheer/referentiemodellen/IECCIM/TC57CIM/IEC61970/Base/Wires#PetersenCoil_mode"/>
                <owl:maxQualifiedCardinality rdf:datatype="http://www.w3.org/2001/XMLSchema#nonNegativeInteger">1</owl:maxQualifiedCardinality>
                <owl:onDataRange rdf:resource="https://w3id.org/netbeheer/referentiemodellen/IECCIM/TC57CIM/IEC61970/Base/Wires#PetersenCoilModeKind"/>
            </owl:Restriction>
        </rdfs:subClassOf>
        <rdfs:comment>A tunable impedance device normally used to offset line charging during single line faults in an ungrounded section of network.</rdfs:comment>
    </owl:Class>
    


    <!-- https://w3id.org/netbeheer/referentiemodellen/IECCIM/TC57CIM/IEC61970/Base/Wires#PhaseImpedanceData -->


    <owl:Class rdf:about="https://w3id.org/netbeheer/referentiemodellen/IECCIM/TC57CIM/IEC61970/Base/Wires#PhaseImpedanceData">
        <rdfs:subClassOf>
            <owl:Restriction>
                <owl:onProperty rdf:resource="https://w3id.org/netbeheer/referentiemodellen/IECCIM/TC57CIM/IEC61970/Base/Wires#PhaseImpedanceData_PhaseImpedance"/>
                <owl:minQualifiedCardinality rdf:datatype="http://www.w3.org/2001/XMLSchema#nonNegativeInteger">1</owl:minQualifiedCardinality>
                <owl:onClass rdf:resource="https://w3id.org/netbeheer/referentiemodellen/IECCIM/TC57CIM/IEC61970/Base/Wires#PhaseImpedanceData"/>
            </owl:Restriction>
        </rdfs:subClassOf>
        <rdfs:subClassOf>
            <owl:Restriction>
                <owl:onProperty rdf:resource="https://w3id.org/netbeheer/referentiemodellen/IECCIM/TC57CIM/IEC61970/Base/Wires#PhaseImpedanceData_b"/>
                <owl:minQualifiedCardinality rdf:datatype="http://www.w3.org/2001/XMLSchema#nonNegativeInteger">0</owl:minQualifiedCardinality>
                <owl:onClass rdf:resource="https://w3id.org/netbeheer/referentiemodellen/IECCIM/TC57CIM/IEC61970/Base/Domain#SusceptancePerLength"/>
            </owl:Restriction>
        </rdfs:subClassOf>
        <rdfs:subClassOf>
            <owl:Restriction>
                <owl:onProperty rdf:resource="https://w3id.org/netbeheer/referentiemodellen/IECCIM/TC57CIM/IEC61970/Base/Wires#PhaseImpedanceData_r"/>
                <owl:minQualifiedCardinality rdf:datatype="http://www.w3.org/2001/XMLSchema#nonNegativeInteger">0</owl:minQualifiedCardinality>
                <owl:onClass rdf:resource="https://w3id.org/netbeheer/referentiemodellen/IECCIM/TC57CIM/IEC61970/Base/Domain#ResistancePerLength"/>
            </owl:Restriction>
        </rdfs:subClassOf>
        <rdfs:subClassOf>
            <owl:Restriction>
                <owl:onProperty rdf:resource="https://w3id.org/netbeheer/referentiemodellen/IECCIM/TC57CIM/IEC61970/Base/Wires#PhaseImpedanceData_x"/>
                <owl:minQualifiedCardinality rdf:datatype="http://www.w3.org/2001/XMLSchema#nonNegativeInteger">0</owl:minQualifiedCardinality>
                <owl:onClass rdf:resource="https://w3id.org/netbeheer/referentiemodellen/IECCIM/TC57CIM/IEC61970/Base/Domain#ReactancePerLength"/>
            </owl:Restriction>
        </rdfs:subClassOf>
        <rdfs:subClassOf>
            <owl:Restriction>
                <owl:onProperty rdf:resource="https://w3id.org/netbeheer/referentiemodellen/IECCIM/TC57CIM/IEC61970/Base/Wires#PhaseImpedanceData_b"/>
                <owl:maxQualifiedCardinality rdf:datatype="http://www.w3.org/2001/XMLSchema#nonNegativeInteger">1</owl:maxQualifiedCardinality>
                <owl:onClass rdf:resource="https://w3id.org/netbeheer/referentiemodellen/IECCIM/TC57CIM/IEC61970/Base/Domain#SusceptancePerLength"/>
            </owl:Restriction>
        </rdfs:subClassOf>
        <rdfs:subClassOf>
            <owl:Restriction>
                <owl:onProperty rdf:resource="https://w3id.org/netbeheer/referentiemodellen/IECCIM/TC57CIM/IEC61970/Base/Wires#PhaseImpedanceData_r"/>
                <owl:maxQualifiedCardinality rdf:datatype="http://www.w3.org/2001/XMLSchema#nonNegativeInteger">1</owl:maxQualifiedCardinality>
                <owl:onClass rdf:resource="https://w3id.org/netbeheer/referentiemodellen/IECCIM/TC57CIM/IEC61970/Base/Domain#ResistancePerLength"/>
            </owl:Restriction>
        </rdfs:subClassOf>
        <rdfs:subClassOf>
            <owl:Restriction>
                <owl:onProperty rdf:resource="https://w3id.org/netbeheer/referentiemodellen/IECCIM/TC57CIM/IEC61970/Base/Wires#PhaseImpedanceData_x"/>
                <owl:maxQualifiedCardinality rdf:datatype="http://www.w3.org/2001/XMLSchema#nonNegativeInteger">1</owl:maxQualifiedCardinality>
                <owl:onClass rdf:resource="https://w3id.org/netbeheer/referentiemodellen/IECCIM/TC57CIM/IEC61970/Base/Domain#ReactancePerLength"/>
            </owl:Restriction>
        </rdfs:subClassOf>
        <rdfs:subClassOf>
            <owl:Restriction>
                <owl:onProperty rdf:resource="https://w3id.org/netbeheer/referentiemodellen/IECCIM/TC57CIM/IEC61970/Base/Wires#PhaseImpedanceData_sequenceNumber"/>
                <owl:minQualifiedCardinality rdf:datatype="http://www.w3.org/2001/XMLSchema#nonNegativeInteger">0</owl:minQualifiedCardinality>
                <owl:onDataRange rdf:resource="http://www.w3.org/2001/XMLSchema#nonNegativeInteger"/>
            </owl:Restriction>
        </rdfs:subClassOf>
        <rdfs:subClassOf>
            <owl:Restriction>
                <owl:onProperty rdf:resource="https://w3id.org/netbeheer/referentiemodellen/IECCIM/TC57CIM/IEC61970/Base/Wires#PhaseImpedanceData_sequenceNumber"/>
                <owl:maxQualifiedCardinality rdf:datatype="http://www.w3.org/2001/XMLSchema#nonNegativeInteger">1</owl:maxQualifiedCardinality>
                <owl:onDataRange rdf:resource="http://www.w3.org/2001/XMLSchema#nonNegativeInteger"/>
            </owl:Restriction>
        </rdfs:subClassOf>
        <rdfs:comment>Triplet of resistance, reactance, and susceptance matrix element values.</rdfs:comment>
    </owl:Class>
    


    <!-- https://w3id.org/netbeheer/referentiemodellen/IECCIM/TC57CIM/IEC61970/Base/Wires#PhaseTapChanger -->


    <owl:Class rdf:about="https://w3id.org/netbeheer/referentiemodellen/IECCIM/TC57CIM/IEC61970/Base/Wires#PhaseTapChanger">
        <rdfs:subClassOf rdf:resource="https://w3id.org/netbeheer/referentiemodellen/IECCIM/TC57CIM/IEC61970/Base/Wires#TapChanger"/>
        <rdfs:subClassOf>
            <owl:Restriction>
                <owl:onProperty rdf:resource="https://w3id.org/netbeheer/referentiemodellen/IECCIM/TC57CIM/IEC61970/Base/Wires#PhaseTapChanger_TransformerEnd"/>
                <owl:minQualifiedCardinality rdf:datatype="http://www.w3.org/2001/XMLSchema#nonNegativeInteger">0</owl:minQualifiedCardinality>
                <owl:onClass rdf:resource="https://w3id.org/netbeheer/referentiemodellen/IECCIM/TC57CIM/IEC61970/Base/Wires#PhaseTapChanger"/>
            </owl:Restriction>
        </rdfs:subClassOf>
        <rdfs:subClassOf>
            <owl:Restriction>
                <owl:onProperty rdf:resource="https://w3id.org/netbeheer/referentiemodellen/IECCIM/TC57CIM/IEC61970/Base/Wires#PhaseTapChanger_TransformerEnd"/>
                <owl:maxQualifiedCardinality rdf:datatype="http://www.w3.org/2001/XMLSchema#nonNegativeInteger">1</owl:maxQualifiedCardinality>
                <owl:onClass rdf:resource="https://w3id.org/netbeheer/referentiemodellen/IECCIM/TC57CIM/IEC61970/Base/Wires#PhaseTapChanger"/>
            </owl:Restriction>
        </rdfs:subClassOf>
        <rdfs:comment>A transformer phase shifting tap model that controls the phase angle difference across the power transformer and potentially the active power flow through the power transformer.  This phase tap model may also impact the voltage magnitude.</rdfs:comment>
    </owl:Class>
    


    <!-- https://w3id.org/netbeheer/referentiemodellen/IECCIM/TC57CIM/IEC61970/Base/Wires#PhaseTapChangerAsymmetrical -->


    <owl:Class rdf:about="https://w3id.org/netbeheer/referentiemodellen/IECCIM/TC57CIM/IEC61970/Base/Wires#PhaseTapChangerAsymmetrical">
        <rdfs:subClassOf rdf:resource="https://w3id.org/netbeheer/referentiemodellen/IECCIM/TC57CIM/IEC61970/Base/Wires#PhaseTapChangerNonLinear"/>
        <rdfs:subClassOf>
            <owl:Restriction>
                <owl:onProperty rdf:resource="https://w3id.org/netbeheer/referentiemodellen/IECCIM/TC57CIM/IEC61970/Base/Wires#PhaseTapChangerAsymmetrical_windingConnectionAngle"/>
                <owl:minQualifiedCardinality rdf:datatype="http://www.w3.org/2001/XMLSchema#nonNegativeInteger">0</owl:minQualifiedCardinality>
                <owl:onClass rdf:resource="https://w3id.org/netbeheer/referentiemodellen/IECCIM/TC57CIM/IEC61970/Base/Domain#AngleDegrees"/>
            </owl:Restriction>
        </rdfs:subClassOf>
        <rdfs:subClassOf>
            <owl:Restriction>
                <owl:onProperty rdf:resource="https://w3id.org/netbeheer/referentiemodellen/IECCIM/TC57CIM/IEC61970/Base/Wires#PhaseTapChangerAsymmetrical_windingConnectionAngle"/>
                <owl:maxQualifiedCardinality rdf:datatype="http://www.w3.org/2001/XMLSchema#nonNegativeInteger">1</owl:maxQualifiedCardinality>
                <owl:onClass rdf:resource="https://w3id.org/netbeheer/referentiemodellen/IECCIM/TC57CIM/IEC61970/Base/Domain#AngleDegrees"/>
            </owl:Restriction>
        </rdfs:subClassOf>
        <rdfs:comment>Describes the tap model for an asymmetrical phase shifting transformer in which the difference voltage vector adds to the primary side voltage. The angle between the primary side voltage and the difference voltage is named the winding connection angle. The phase shift depends on both the difference voltage magnitude and the winding connection angle.</rdfs:comment>
    </owl:Class>
    


    <!-- https://w3id.org/netbeheer/referentiemodellen/IECCIM/TC57CIM/IEC61970/Base/Wires#PhaseTapChangerLinear -->


    <owl:Class rdf:about="https://w3id.org/netbeheer/referentiemodellen/IECCIM/TC57CIM/IEC61970/Base/Wires#PhaseTapChangerLinear">
        <rdfs:subClassOf rdf:resource="https://w3id.org/netbeheer/referentiemodellen/IECCIM/TC57CIM/IEC61970/Base/Wires#PhaseTapChanger"/>
        <rdfs:subClassOf>
            <owl:Restriction>
                <owl:onProperty rdf:resource="https://w3id.org/netbeheer/referentiemodellen/IECCIM/TC57CIM/IEC61970/Base/Wires#PhaseTapChangerLinear_stepPhaseShiftIncrement"/>
                <owl:minQualifiedCardinality rdf:datatype="http://www.w3.org/2001/XMLSchema#nonNegativeInteger">0</owl:minQualifiedCardinality>
                <owl:onClass rdf:resource="https://w3id.org/netbeheer/referentiemodellen/IECCIM/TC57CIM/IEC61970/Base/Domain#AngleDegrees"/>
            </owl:Restriction>
        </rdfs:subClassOf>
        <rdfs:subClassOf>
            <owl:Restriction>
                <owl:onProperty rdf:resource="https://w3id.org/netbeheer/referentiemodellen/IECCIM/TC57CIM/IEC61970/Base/Wires#PhaseTapChangerLinear_xMax"/>
                <owl:minQualifiedCardinality rdf:datatype="http://www.w3.org/2001/XMLSchema#nonNegativeInteger">0</owl:minQualifiedCardinality>
                <owl:onClass rdf:resource="https://w3id.org/netbeheer/referentiemodellen/IECCIM/TC57CIM/IEC61970/Base/Domain#Reactance"/>
            </owl:Restriction>
        </rdfs:subClassOf>
        <rdfs:subClassOf>
            <owl:Restriction>
                <owl:onProperty rdf:resource="https://w3id.org/netbeheer/referentiemodellen/IECCIM/TC57CIM/IEC61970/Base/Wires#PhaseTapChangerLinear_xMin"/>
                <owl:minQualifiedCardinality rdf:datatype="http://www.w3.org/2001/XMLSchema#nonNegativeInteger">0</owl:minQualifiedCardinality>
                <owl:onClass rdf:resource="https://w3id.org/netbeheer/referentiemodellen/IECCIM/TC57CIM/IEC61970/Base/Domain#Reactance"/>
            </owl:Restriction>
        </rdfs:subClassOf>
        <rdfs:subClassOf>
            <owl:Restriction>
                <owl:onProperty rdf:resource="https://w3id.org/netbeheer/referentiemodellen/IECCIM/TC57CIM/IEC61970/Base/Wires#PhaseTapChangerLinear_stepPhaseShiftIncrement"/>
                <owl:maxQualifiedCardinality rdf:datatype="http://www.w3.org/2001/XMLSchema#nonNegativeInteger">1</owl:maxQualifiedCardinality>
                <owl:onClass rdf:resource="https://w3id.org/netbeheer/referentiemodellen/IECCIM/TC57CIM/IEC61970/Base/Domain#AngleDegrees"/>
            </owl:Restriction>
        </rdfs:subClassOf>
        <rdfs:subClassOf>
            <owl:Restriction>
                <owl:onProperty rdf:resource="https://w3id.org/netbeheer/referentiemodellen/IECCIM/TC57CIM/IEC61970/Base/Wires#PhaseTapChangerLinear_xMax"/>
                <owl:maxQualifiedCardinality rdf:datatype="http://www.w3.org/2001/XMLSchema#nonNegativeInteger">1</owl:maxQualifiedCardinality>
                <owl:onClass rdf:resource="https://w3id.org/netbeheer/referentiemodellen/IECCIM/TC57CIM/IEC61970/Base/Domain#Reactance"/>
            </owl:Restriction>
        </rdfs:subClassOf>
        <rdfs:subClassOf>
            <owl:Restriction>
                <owl:onProperty rdf:resource="https://w3id.org/netbeheer/referentiemodellen/IECCIM/TC57CIM/IEC61970/Base/Wires#PhaseTapChangerLinear_xMin"/>
                <owl:maxQualifiedCardinality rdf:datatype="http://www.w3.org/2001/XMLSchema#nonNegativeInteger">1</owl:maxQualifiedCardinality>
                <owl:onClass rdf:resource="https://w3id.org/netbeheer/referentiemodellen/IECCIM/TC57CIM/IEC61970/Base/Domain#Reactance"/>
            </owl:Restriction>
        </rdfs:subClassOf>
        <rdfs:comment>Describes a tap changer with a linear relation between the tap step and the phase angle difference across the transformer. This is a mathematical model that is an approximation of a real phase tap changer.
The phase angle is computed as stepPhaseShitfIncrement times the tap position.
The secondary side voltage magnitude is the same as at the primary side.</rdfs:comment>
    </owl:Class>
    


    <!-- https://w3id.org/netbeheer/referentiemodellen/IECCIM/TC57CIM/IEC61970/Base/Wires#PhaseTapChangerNonLinear -->


    <owl:Class rdf:about="https://w3id.org/netbeheer/referentiemodellen/IECCIM/TC57CIM/IEC61970/Base/Wires#PhaseTapChangerNonLinear">
        <rdfs:subClassOf rdf:resource="https://w3id.org/netbeheer/referentiemodellen/IECCIM/TC57CIM/IEC61970/Base/Wires#PhaseTapChanger"/>
        <rdfs:subClassOf>
            <owl:Restriction>
                <owl:onProperty rdf:resource="https://w3id.org/netbeheer/referentiemodellen/IECCIM/TC57CIM/IEC61970/Base/Wires#PhaseTapChangerNonLinear_voltageStepIncrement"/>
                <owl:minQualifiedCardinality rdf:datatype="http://www.w3.org/2001/XMLSchema#nonNegativeInteger">0</owl:minQualifiedCardinality>
                <owl:onClass rdf:resource="https://w3id.org/netbeheer/referentiemodellen/IECCIM/TC57CIM/IEC61970/Base/Domain#PerCent"/>
            </owl:Restriction>
        </rdfs:subClassOf>
        <rdfs:subClassOf>
            <owl:Restriction>
                <owl:onProperty rdf:resource="https://w3id.org/netbeheer/referentiemodellen/IECCIM/TC57CIM/IEC61970/Base/Wires#PhaseTapChangerNonLinear_xMax"/>
                <owl:minQualifiedCardinality rdf:datatype="http://www.w3.org/2001/XMLSchema#nonNegativeInteger">0</owl:minQualifiedCardinality>
                <owl:onClass rdf:resource="https://w3id.org/netbeheer/referentiemodellen/IECCIM/TC57CIM/IEC61970/Base/Domain#Reactance"/>
            </owl:Restriction>
        </rdfs:subClassOf>
        <rdfs:subClassOf>
            <owl:Restriction>
                <owl:onProperty rdf:resource="https://w3id.org/netbeheer/referentiemodellen/IECCIM/TC57CIM/IEC61970/Base/Wires#PhaseTapChangerNonLinear_xMin"/>
                <owl:minQualifiedCardinality rdf:datatype="http://www.w3.org/2001/XMLSchema#nonNegativeInteger">0</owl:minQualifiedCardinality>
                <owl:onClass rdf:resource="https://w3id.org/netbeheer/referentiemodellen/IECCIM/TC57CIM/IEC61970/Base/Domain#Reactance"/>
            </owl:Restriction>
        </rdfs:subClassOf>
        <rdfs:subClassOf>
            <owl:Restriction>
                <owl:onProperty rdf:resource="https://w3id.org/netbeheer/referentiemodellen/IECCIM/TC57CIM/IEC61970/Base/Wires#PhaseTapChangerNonLinear_voltageStepIncrement"/>
                <owl:maxQualifiedCardinality rdf:datatype="http://www.w3.org/2001/XMLSchema#nonNegativeInteger">1</owl:maxQualifiedCardinality>
                <owl:onClass rdf:resource="https://w3id.org/netbeheer/referentiemodellen/IECCIM/TC57CIM/IEC61970/Base/Domain#PerCent"/>
            </owl:Restriction>
        </rdfs:subClassOf>
        <rdfs:subClassOf>
            <owl:Restriction>
                <owl:onProperty rdf:resource="https://w3id.org/netbeheer/referentiemodellen/IECCIM/TC57CIM/IEC61970/Base/Wires#PhaseTapChangerNonLinear_xMax"/>
                <owl:maxQualifiedCardinality rdf:datatype="http://www.w3.org/2001/XMLSchema#nonNegativeInteger">1</owl:maxQualifiedCardinality>
                <owl:onClass rdf:resource="https://w3id.org/netbeheer/referentiemodellen/IECCIM/TC57CIM/IEC61970/Base/Domain#Reactance"/>
            </owl:Restriction>
        </rdfs:subClassOf>
        <rdfs:subClassOf>
            <owl:Restriction>
                <owl:onProperty rdf:resource="https://w3id.org/netbeheer/referentiemodellen/IECCIM/TC57CIM/IEC61970/Base/Wires#PhaseTapChangerNonLinear_xMin"/>
                <owl:maxQualifiedCardinality rdf:datatype="http://www.w3.org/2001/XMLSchema#nonNegativeInteger">1</owl:maxQualifiedCardinality>
                <owl:onClass rdf:resource="https://w3id.org/netbeheer/referentiemodellen/IECCIM/TC57CIM/IEC61970/Base/Domain#Reactance"/>
            </owl:Restriction>
        </rdfs:subClassOf>
        <rdfs:comment>The non-linear phase tap changer describes the non-linear behavior of a phase tap changer. This is a base class for the symmetrical and asymmetrical phase tap changer models. The details of these models can be found in the IEC 61970-301 document.</rdfs:comment>
    </owl:Class>
    


    <!-- https://w3id.org/netbeheer/referentiemodellen/IECCIM/TC57CIM/IEC61970/Base/Wires#PhaseTapChangerSymmetrical -->


    <owl:Class rdf:about="https://w3id.org/netbeheer/referentiemodellen/IECCIM/TC57CIM/IEC61970/Base/Wires#PhaseTapChangerSymmetrical">
        <rdfs:subClassOf rdf:resource="https://w3id.org/netbeheer/referentiemodellen/IECCIM/TC57CIM/IEC61970/Base/Wires#PhaseTapChangerNonLinear"/>
        <rdfs:comment>Describes a symmetrical phase shifting transformer tap model in which the secondary side voltage magnitude is the same as at the primary side. The difference voltage magnitude is the base in an equal-sided triangle where the sides corresponds to the primary and secondary voltages. The phase angle difference corresponds to the top angle and can be expressed as twice the arctangent of half the total difference voltage.</rdfs:comment>
    </owl:Class>
    


    <!-- https://w3id.org/netbeheer/referentiemodellen/IECCIM/TC57CIM/IEC61970/Base/Wires#PhaseTapChangerTable -->


    <owl:Class rdf:about="https://w3id.org/netbeheer/referentiemodellen/IECCIM/TC57CIM/IEC61970/Base/Wires#PhaseTapChangerTable">
        <rdfs:subClassOf rdf:resource="https://w3id.org/netbeheer/referentiemodellen/IECCIM/TC57CIM/IEC61970/Base/Core#IdentifiedObject"/>
        <rdfs:subClassOf>
            <owl:Restriction>
                <owl:onProperty rdf:resource="https://w3id.org/netbeheer/referentiemodellen/IECCIM/TC57CIM/IEC61970/Base/Wires#PhaseTapChangerTable_PhaseTapChangerTabular"/>
                <owl:minQualifiedCardinality rdf:datatype="http://www.w3.org/2001/XMLSchema#nonNegativeInteger">0</owl:minQualifiedCardinality>
                <owl:onClass rdf:resource="https://w3id.org/netbeheer/referentiemodellen/IECCIM/TC57CIM/IEC61970/Base/Wires#PhaseTapChangerTable"/>
            </owl:Restriction>
        </rdfs:subClassOf>
        <rdfs:subClassOf>
            <owl:Restriction>
                <owl:onProperty rdf:resource="https://w3id.org/netbeheer/referentiemodellen/IECCIM/TC57CIM/IEC61970/Base/Wires#PhaseTapChangerTable_PhaseTapChangerTablePoint"/>
                <owl:qualifiedCardinality rdf:datatype="http://www.w3.org/2001/XMLSchema#nonNegativeInteger">1</owl:qualifiedCardinality>
                <owl:onClass rdf:resource="https://w3id.org/netbeheer/referentiemodellen/IECCIM/TC57CIM/IEC61970/Base/Wires#PhaseTapChangerTable"/>
            </owl:Restriction>
        </rdfs:subClassOf>
        <rdfs:subClassOf>
            <owl:Restriction>
                <owl:onProperty rdf:resource="https://w3id.org/netbeheer/referentiemodellen/IECCIM/TC57CIM/IEC61970/Base/Wires#PhaseTapChangerTable_PhaseTapChangerTabular"/>
                <owl:maxQualifiedCardinality rdf:datatype="http://www.w3.org/2001/XMLSchema#nonNegativeInteger">1</owl:maxQualifiedCardinality>
                <owl:onClass rdf:resource="https://w3id.org/netbeheer/referentiemodellen/IECCIM/TC57CIM/IEC61970/Base/Wires#PhaseTapChangerTable"/>
            </owl:Restriction>
        </rdfs:subClassOf>
        <rdfs:comment>Describes a tabular curve for how the phase angle difference and impedance varies with the tap step.</rdfs:comment>
    </owl:Class>
    


    <!-- https://w3id.org/netbeheer/referentiemodellen/IECCIM/TC57CIM/IEC61970/Base/Wires#PhaseTapChangerTablePoint -->


    <owl:Class rdf:about="https://w3id.org/netbeheer/referentiemodellen/IECCIM/TC57CIM/IEC61970/Base/Wires#PhaseTapChangerTablePoint">
        <rdfs:subClassOf rdf:resource="https://w3id.org/netbeheer/referentiemodellen/IECCIM/TC57CIM/IEC61970/Base/Wires#TapChangerTablePoint"/>
        <rdfs:subClassOf>
            <owl:Restriction>
                <owl:onProperty rdf:resource="https://w3id.org/netbeheer/referentiemodellen/IECCIM/TC57CIM/IEC61970/Base/Wires#PhaseTapChangerTablePoint_PhaseTapChangerTable"/>
                <owl:minQualifiedCardinality rdf:datatype="http://www.w3.org/2001/XMLSchema#nonNegativeInteger">1</owl:minQualifiedCardinality>
                <owl:onClass rdf:resource="https://w3id.org/netbeheer/referentiemodellen/IECCIM/TC57CIM/IEC61970/Base/Wires#PhaseTapChangerTablePoint"/>
            </owl:Restriction>
        </rdfs:subClassOf>
        <rdfs:subClassOf>
            <owl:Restriction>
                <owl:onProperty rdf:resource="https://w3id.org/netbeheer/referentiemodellen/IECCIM/TC57CIM/IEC61970/Base/Wires#PhaseTapChangerTablePoint_angle"/>
                <owl:minQualifiedCardinality rdf:datatype="http://www.w3.org/2001/XMLSchema#nonNegativeInteger">0</owl:minQualifiedCardinality>
                <owl:onClass rdf:resource="https://w3id.org/netbeheer/referentiemodellen/IECCIM/TC57CIM/IEC61970/Base/Domain#AngleDegrees"/>
            </owl:Restriction>
        </rdfs:subClassOf>
        <rdfs:subClassOf>
            <owl:Restriction>
                <owl:onProperty rdf:resource="https://w3id.org/netbeheer/referentiemodellen/IECCIM/TC57CIM/IEC61970/Base/Wires#PhaseTapChangerTablePoint_angle"/>
                <owl:maxQualifiedCardinality rdf:datatype="http://www.w3.org/2001/XMLSchema#nonNegativeInteger">1</owl:maxQualifiedCardinality>
                <owl:onClass rdf:resource="https://w3id.org/netbeheer/referentiemodellen/IECCIM/TC57CIM/IEC61970/Base/Domain#AngleDegrees"/>
            </owl:Restriction>
        </rdfs:subClassOf>
        <rdfs:comment>Describes each tap step in the phase tap changer tabular curve.
</rdfs:comment>
    </owl:Class>
    


    <!-- https://w3id.org/netbeheer/referentiemodellen/IECCIM/TC57CIM/IEC61970/Base/Wires#PhaseTapChangerTabular -->


    <owl:Class rdf:about="https://w3id.org/netbeheer/referentiemodellen/IECCIM/TC57CIM/IEC61970/Base/Wires#PhaseTapChangerTabular">
        <rdfs:subClassOf rdf:resource="https://w3id.org/netbeheer/referentiemodellen/IECCIM/TC57CIM/IEC61970/Base/Wires#PhaseTapChanger"/>
        <rdfs:subClassOf>
            <owl:Restriction>
                <owl:onProperty rdf:resource="https://w3id.org/netbeheer/referentiemodellen/IECCIM/TC57CIM/IEC61970/Base/Wires#PhaseTapChangerTabular_PhaseTapChangerTable"/>
                <owl:minQualifiedCardinality rdf:datatype="http://www.w3.org/2001/XMLSchema#nonNegativeInteger">0</owl:minQualifiedCardinality>
                <owl:onClass rdf:resource="https://w3id.org/netbeheer/referentiemodellen/IECCIM/TC57CIM/IEC61970/Base/Wires#PhaseTapChangerTabular"/>
            </owl:Restriction>
        </rdfs:subClassOf>
    </owl:Class>
    


    <!-- https://w3id.org/netbeheer/referentiemodellen/IECCIM/TC57CIM/IEC61970/Base/Wires#Plant -->


    <owl:Class rdf:about="https://w3id.org/netbeheer/referentiemodellen/IECCIM/TC57CIM/IEC61970/Base/Wires#Plant">
        <rdfs:subClassOf rdf:resource="https://w3id.org/netbeheer/referentiemodellen/IECCIM/TC57CIM/IEC61970/Base/Core#EquipmentContainer"/>
        <rdfs:comment>A Plant is a collection of equipment for purposes of generation.</rdfs:comment>
    </owl:Class>
    


    <!-- https://w3id.org/netbeheer/referentiemodellen/IECCIM/TC57CIM/IEC61970/Base/Wires#PowerTransformer -->


    <owl:Class rdf:about="https://w3id.org/netbeheer/referentiemodellen/IECCIM/TC57CIM/IEC61970/Base/Wires#PowerTransformer">
        <rdfs:subClassOf rdf:resource="https://w3id.org/netbeheer/referentiemodellen/IECCIM/TC57CIM/IEC61970/Base/Core#ConductingEquipment"/>
        <rdfs:subClassOf>
            <owl:Restriction>
                <owl:onProperty rdf:resource="https://w3id.org/netbeheer/referentiemodellen/IECCIM/TC57CIM/IEC61970/Base/Wires#PowerTransformer_PowerTransformerEnd"/>
                <owl:minQualifiedCardinality rdf:datatype="http://www.w3.org/2001/XMLSchema#nonNegativeInteger">0</owl:minQualifiedCardinality>
                <owl:onClass rdf:resource="https://w3id.org/netbeheer/referentiemodellen/IECCIM/TC57CIM/IEC61970/Base/Wires#PowerTransformer"/>
            </owl:Restriction>
        </rdfs:subClassOf>
        <rdfs:subClassOf>
            <owl:Restriction>
                <owl:onProperty rdf:resource="https://w3id.org/netbeheer/referentiemodellen/IECCIM/TC57CIM/IEC61970/Base/Wires#PowerTransformer_TransformerTanks"/>
                <owl:minQualifiedCardinality rdf:datatype="http://www.w3.org/2001/XMLSchema#nonNegativeInteger">0</owl:minQualifiedCardinality>
                <owl:onClass rdf:resource="https://w3id.org/netbeheer/referentiemodellen/IECCIM/TC57CIM/IEC61970/Base/Wires#PowerTransformer"/>
            </owl:Restriction>
        </rdfs:subClassOf>
        <rdfs:subClassOf>
            <owl:Restriction>
                <owl:onProperty rdf:resource="https://w3id.org/netbeheer/referentiemodellen/IECCIM/TC57CIM/IEC61970/Base/Wires#PowerTransformer_beforeShCircuitHighestOperatingCurrent"/>
                <owl:minQualifiedCardinality rdf:datatype="http://www.w3.org/2001/XMLSchema#nonNegativeInteger">0</owl:minQualifiedCardinality>
                <owl:onClass rdf:resource="https://w3id.org/netbeheer/referentiemodellen/IECCIM/TC57CIM/IEC61970/Base/Domain#CurrentFlow"/>
            </owl:Restriction>
        </rdfs:subClassOf>
        <rdfs:subClassOf>
            <owl:Restriction>
                <owl:onProperty rdf:resource="https://w3id.org/netbeheer/referentiemodellen/IECCIM/TC57CIM/IEC61970/Base/Wires#PowerTransformer_beforeShCircuitHighestOperatingVoltage"/>
                <owl:minQualifiedCardinality rdf:datatype="http://www.w3.org/2001/XMLSchema#nonNegativeInteger">0</owl:minQualifiedCardinality>
                <owl:onClass rdf:resource="https://w3id.org/netbeheer/referentiemodellen/IECCIM/TC57CIM/IEC61970/Base/Domain#Voltage"/>
            </owl:Restriction>
        </rdfs:subClassOf>
        <rdfs:subClassOf>
            <owl:Restriction>
                <owl:onProperty rdf:resource="https://w3id.org/netbeheer/referentiemodellen/IECCIM/TC57CIM/IEC61970/Base/Wires#PowerTransformer_beforeShortCircuitAnglePf"/>
                <owl:minQualifiedCardinality rdf:datatype="http://www.w3.org/2001/XMLSchema#nonNegativeInteger">0</owl:minQualifiedCardinality>
                <owl:onClass rdf:resource="https://w3id.org/netbeheer/referentiemodellen/IECCIM/TC57CIM/IEC61970/Base/Domain#AngleDegrees"/>
            </owl:Restriction>
        </rdfs:subClassOf>
        <rdfs:subClassOf>
            <owl:Restriction>
                <owl:onProperty rdf:resource="https://w3id.org/netbeheer/referentiemodellen/IECCIM/TC57CIM/IEC61970/Base/Wires#PowerTransformer_highSideMinOperatingU"/>
                <owl:minQualifiedCardinality rdf:datatype="http://www.w3.org/2001/XMLSchema#nonNegativeInteger">0</owl:minQualifiedCardinality>
                <owl:onClass rdf:resource="https://w3id.org/netbeheer/referentiemodellen/IECCIM/TC57CIM/IEC61970/Base/Domain#Voltage"/>
            </owl:Restriction>
        </rdfs:subClassOf>
        <rdfs:subClassOf>
            <owl:Restriction>
                <owl:onProperty rdf:resource="https://w3id.org/netbeheer/referentiemodellen/IECCIM/TC57CIM/IEC61970/Base/Wires#PowerTransformer_PowerTransformerEnd"/>
                <owl:maxQualifiedCardinality rdf:datatype="http://www.w3.org/2001/XMLSchema#nonNegativeInteger">1</owl:maxQualifiedCardinality>
                <owl:onClass rdf:resource="https://w3id.org/netbeheer/referentiemodellen/IECCIM/TC57CIM/IEC61970/Base/Wires#PowerTransformer"/>
            </owl:Restriction>
        </rdfs:subClassOf>
        <rdfs:subClassOf>
            <owl:Restriction>
                <owl:onProperty rdf:resource="https://w3id.org/netbeheer/referentiemodellen/IECCIM/TC57CIM/IEC61970/Base/Wires#PowerTransformer_TransformerTanks"/>
                <owl:maxQualifiedCardinality rdf:datatype="http://www.w3.org/2001/XMLSchema#nonNegativeInteger">1</owl:maxQualifiedCardinality>
                <owl:onClass rdf:resource="https://w3id.org/netbeheer/referentiemodellen/IECCIM/TC57CIM/IEC61970/Base/Wires#PowerTransformer"/>
            </owl:Restriction>
        </rdfs:subClassOf>
        <rdfs:subClassOf>
            <owl:Restriction>
                <owl:onProperty rdf:resource="https://w3id.org/netbeheer/referentiemodellen/IECCIM/TC57CIM/IEC61970/Base/Wires#PowerTransformer_beforeShCircuitHighestOperatingCurrent"/>
                <owl:maxQualifiedCardinality rdf:datatype="http://www.w3.org/2001/XMLSchema#nonNegativeInteger">1</owl:maxQualifiedCardinality>
                <owl:onClass rdf:resource="https://w3id.org/netbeheer/referentiemodellen/IECCIM/TC57CIM/IEC61970/Base/Domain#CurrentFlow"/>
            </owl:Restriction>
        </rdfs:subClassOf>
        <rdfs:subClassOf>
            <owl:Restriction>
                <owl:onProperty rdf:resource="https://w3id.org/netbeheer/referentiemodellen/IECCIM/TC57CIM/IEC61970/Base/Wires#PowerTransformer_beforeShCircuitHighestOperatingVoltage"/>
                <owl:maxQualifiedCardinality rdf:datatype="http://www.w3.org/2001/XMLSchema#nonNegativeInteger">1</owl:maxQualifiedCardinality>
                <owl:onClass rdf:resource="https://w3id.org/netbeheer/referentiemodellen/IECCIM/TC57CIM/IEC61970/Base/Domain#Voltage"/>
            </owl:Restriction>
        </rdfs:subClassOf>
        <rdfs:subClassOf>
            <owl:Restriction>
                <owl:onProperty rdf:resource="https://w3id.org/netbeheer/referentiemodellen/IECCIM/TC57CIM/IEC61970/Base/Wires#PowerTransformer_beforeShortCircuitAnglePf"/>
                <owl:maxQualifiedCardinality rdf:datatype="http://www.w3.org/2001/XMLSchema#nonNegativeInteger">1</owl:maxQualifiedCardinality>
                <owl:onClass rdf:resource="https://w3id.org/netbeheer/referentiemodellen/IECCIM/TC57CIM/IEC61970/Base/Domain#AngleDegrees"/>
            </owl:Restriction>
        </rdfs:subClassOf>
        <rdfs:subClassOf>
            <owl:Restriction>
                <owl:onProperty rdf:resource="https://w3id.org/netbeheer/referentiemodellen/IECCIM/TC57CIM/IEC61970/Base/Wires#PowerTransformer_highSideMinOperatingU"/>
                <owl:maxQualifiedCardinality rdf:datatype="http://www.w3.org/2001/XMLSchema#nonNegativeInteger">1</owl:maxQualifiedCardinality>
                <owl:onClass rdf:resource="https://w3id.org/netbeheer/referentiemodellen/IECCIM/TC57CIM/IEC61970/Base/Domain#Voltage"/>
            </owl:Restriction>
        </rdfs:subClassOf>
        <rdfs:subClassOf>
            <owl:Restriction>
                <owl:onProperty rdf:resource="https://w3id.org/netbeheer/referentiemodellen/IECCIM/TC57CIM/IEC61970/Base/Wires#PowerTransformer_isPartOfGeneratorUnit"/>
                <owl:minQualifiedCardinality rdf:datatype="http://www.w3.org/2001/XMLSchema#nonNegativeInteger">0</owl:minQualifiedCardinality>
                <owl:onDataRange rdf:resource="http://www.w3.org/2001/XMLSchema#boolean"/>
            </owl:Restriction>
        </rdfs:subClassOf>
        <rdfs:subClassOf>
            <owl:Restriction>
                <owl:onProperty rdf:resource="https://w3id.org/netbeheer/referentiemodellen/IECCIM/TC57CIM/IEC61970/Base/Wires#PowerTransformer_operationalValuesConsidered"/>
                <owl:minQualifiedCardinality rdf:datatype="http://www.w3.org/2001/XMLSchema#nonNegativeInteger">0</owl:minQualifiedCardinality>
                <owl:onDataRange rdf:resource="http://www.w3.org/2001/XMLSchema#boolean"/>
            </owl:Restriction>
        </rdfs:subClassOf>
        <rdfs:subClassOf>
            <owl:Restriction>
                <owl:onProperty rdf:resource="https://w3id.org/netbeheer/referentiemodellen/IECCIM/TC57CIM/IEC61970/Base/Wires#PowerTransformer_vectorGroup"/>
                <owl:minQualifiedCardinality rdf:datatype="http://www.w3.org/2001/XMLSchema#nonNegativeInteger">0</owl:minQualifiedCardinality>
                <owl:onDataRange rdf:resource="http://www.w3.org/2001/XMLSchema#string"/>
            </owl:Restriction>
        </rdfs:subClassOf>
        <rdfs:subClassOf>
            <owl:Restriction>
                <owl:onProperty rdf:resource="https://w3id.org/netbeheer/referentiemodellen/IECCIM/TC57CIM/IEC61970/Base/Wires#PowerTransformer_isPartOfGeneratorUnit"/>
                <owl:maxQualifiedCardinality rdf:datatype="http://www.w3.org/2001/XMLSchema#nonNegativeInteger">1</owl:maxQualifiedCardinality>
                <owl:onDataRange rdf:resource="http://www.w3.org/2001/XMLSchema#boolean"/>
            </owl:Restriction>
        </rdfs:subClassOf>
        <rdfs:subClassOf>
            <owl:Restriction>
                <owl:onProperty rdf:resource="https://w3id.org/netbeheer/referentiemodellen/IECCIM/TC57CIM/IEC61970/Base/Wires#PowerTransformer_operationalValuesConsidered"/>
                <owl:maxQualifiedCardinality rdf:datatype="http://www.w3.org/2001/XMLSchema#nonNegativeInteger">1</owl:maxQualifiedCardinality>
                <owl:onDataRange rdf:resource="http://www.w3.org/2001/XMLSchema#boolean"/>
            </owl:Restriction>
        </rdfs:subClassOf>
        <rdfs:subClassOf>
            <owl:Restriction>
                <owl:onProperty rdf:resource="https://w3id.org/netbeheer/referentiemodellen/IECCIM/TC57CIM/IEC61970/Base/Wires#PowerTransformer_vectorGroup"/>
                <owl:maxQualifiedCardinality rdf:datatype="http://www.w3.org/2001/XMLSchema#nonNegativeInteger">1</owl:maxQualifiedCardinality>
                <owl:onDataRange rdf:resource="http://www.w3.org/2001/XMLSchema#string"/>
            </owl:Restriction>
        </rdfs:subClassOf>
        <rdfs:comment>An electrical device consisting of  two or more coupled windings, with or without a magnetic core, for introducing mutual coupling between electric circuits. Transformers can be used to control voltage and phase shift (active power flow).
A power transformer may be composed of separate transformer tanks that need not be identical.
A power transformer can be modeled with or without tanks and is intended for use in both balanced and unbalanced representations.   A power transformer typically has two terminals, but may have one (grounding), three or more terminals.
The inherited association ConductingEquipment.BaseVoltage should not be used.  The association from TransformerEnd to BaseVoltage should be used instead.</rdfs:comment>
    </owl:Class>
    


    <!-- https://w3id.org/netbeheer/referentiemodellen/IECCIM/TC57CIM/IEC61970/Base/Wires#PowerTransformerEnd -->


    <owl:Class rdf:about="https://w3id.org/netbeheer/referentiemodellen/IECCIM/TC57CIM/IEC61970/Base/Wires#PowerTransformerEnd">
        <rdfs:subClassOf rdf:resource="https://w3id.org/netbeheer/referentiemodellen/IECCIM/TC57CIM/IEC61970/Base/Wires#TransformerEnd"/>
        <rdfs:subClassOf>
            <owl:Restriction>
                <owl:onProperty rdf:resource="https://w3id.org/netbeheer/referentiemodellen/IECCIM/TC57CIM/IEC61970/Base/Wires#PowerTransformerEnd_PowerTransformer"/>
                <owl:minQualifiedCardinality rdf:datatype="http://www.w3.org/2001/XMLSchema#nonNegativeInteger">0</owl:minQualifiedCardinality>
                <owl:onClass rdf:resource="https://w3id.org/netbeheer/referentiemodellen/IECCIM/TC57CIM/IEC61970/Base/Wires#PowerTransformerEnd"/>
            </owl:Restriction>
        </rdfs:subClassOf>
        <rdfs:subClassOf>
            <owl:Restriction>
                <owl:onProperty rdf:resource="https://w3id.org/netbeheer/referentiemodellen/IECCIM/TC57CIM/IEC61970/Base/Wires#PowerTransformerEnd_b"/>
                <owl:minQualifiedCardinality rdf:datatype="http://www.w3.org/2001/XMLSchema#nonNegativeInteger">0</owl:minQualifiedCardinality>
                <owl:onClass rdf:resource="https://w3id.org/netbeheer/referentiemodellen/IECCIM/TC57CIM/IEC61970/Base/Domain#Susceptance"/>
            </owl:Restriction>
        </rdfs:subClassOf>
        <rdfs:subClassOf>
            <owl:Restriction>
                <owl:onProperty rdf:resource="https://w3id.org/netbeheer/referentiemodellen/IECCIM/TC57CIM/IEC61970/Base/Wires#PowerTransformerEnd_b0"/>
                <owl:minQualifiedCardinality rdf:datatype="http://www.w3.org/2001/XMLSchema#nonNegativeInteger">0</owl:minQualifiedCardinality>
                <owl:onClass rdf:resource="https://w3id.org/netbeheer/referentiemodellen/IECCIM/TC57CIM/IEC61970/Base/Domain#Susceptance"/>
            </owl:Restriction>
        </rdfs:subClassOf>
        <rdfs:subClassOf>
            <owl:Restriction>
                <owl:onProperty rdf:resource="https://w3id.org/netbeheer/referentiemodellen/IECCIM/TC57CIM/IEC61970/Base/Wires#PowerTransformerEnd_g"/>
                <owl:minQualifiedCardinality rdf:datatype="http://www.w3.org/2001/XMLSchema#nonNegativeInteger">0</owl:minQualifiedCardinality>
                <owl:onClass rdf:resource="https://w3id.org/netbeheer/referentiemodellen/IECCIM/TC57CIM/IEC61970/Base/Domain#Conductance"/>
            </owl:Restriction>
        </rdfs:subClassOf>
        <rdfs:subClassOf>
            <owl:Restriction>
                <owl:onProperty rdf:resource="https://w3id.org/netbeheer/referentiemodellen/IECCIM/TC57CIM/IEC61970/Base/Wires#PowerTransformerEnd_g0"/>
                <owl:minQualifiedCardinality rdf:datatype="http://www.w3.org/2001/XMLSchema#nonNegativeInteger">0</owl:minQualifiedCardinality>
                <owl:onClass rdf:resource="https://w3id.org/netbeheer/referentiemodellen/IECCIM/TC57CIM/IEC61970/Base/Domain#Conductance"/>
            </owl:Restriction>
        </rdfs:subClassOf>
        <rdfs:subClassOf>
            <owl:Restriction>
                <owl:onProperty rdf:resource="https://w3id.org/netbeheer/referentiemodellen/IECCIM/TC57CIM/IEC61970/Base/Wires#PowerTransformerEnd_r"/>
                <owl:minQualifiedCardinality rdf:datatype="http://www.w3.org/2001/XMLSchema#nonNegativeInteger">0</owl:minQualifiedCardinality>
                <owl:onClass rdf:resource="https://w3id.org/netbeheer/referentiemodellen/IECCIM/TC57CIM/IEC61970/Base/Domain#Resistance"/>
            </owl:Restriction>
        </rdfs:subClassOf>
        <rdfs:subClassOf>
            <owl:Restriction>
                <owl:onProperty rdf:resource="https://w3id.org/netbeheer/referentiemodellen/IECCIM/TC57CIM/IEC61970/Base/Wires#PowerTransformerEnd_r0"/>
                <owl:minQualifiedCardinality rdf:datatype="http://www.w3.org/2001/XMLSchema#nonNegativeInteger">0</owl:minQualifiedCardinality>
                <owl:onClass rdf:resource="https://w3id.org/netbeheer/referentiemodellen/IECCIM/TC57CIM/IEC61970/Base/Domain#Resistance"/>
            </owl:Restriction>
        </rdfs:subClassOf>
        <rdfs:subClassOf>
            <owl:Restriction>
                <owl:onProperty rdf:resource="https://w3id.org/netbeheer/referentiemodellen/IECCIM/TC57CIM/IEC61970/Base/Wires#PowerTransformerEnd_ratedS"/>
                <owl:minQualifiedCardinality rdf:datatype="http://www.w3.org/2001/XMLSchema#nonNegativeInteger">0</owl:minQualifiedCardinality>
                <owl:onClass rdf:resource="https://w3id.org/netbeheer/referentiemodellen/IECCIM/TC57CIM/IEC61970/Base/Domain#ApparentPower"/>
            </owl:Restriction>
        </rdfs:subClassOf>
        <rdfs:subClassOf>
            <owl:Restriction>
                <owl:onProperty rdf:resource="https://w3id.org/netbeheer/referentiemodellen/IECCIM/TC57CIM/IEC61970/Base/Wires#PowerTransformerEnd_ratedU"/>
                <owl:minQualifiedCardinality rdf:datatype="http://www.w3.org/2001/XMLSchema#nonNegativeInteger">0</owl:minQualifiedCardinality>
                <owl:onClass rdf:resource="https://w3id.org/netbeheer/referentiemodellen/IECCIM/TC57CIM/IEC61970/Base/Domain#Voltage"/>
            </owl:Restriction>
        </rdfs:subClassOf>
        <rdfs:subClassOf>
            <owl:Restriction>
                <owl:onProperty rdf:resource="https://w3id.org/netbeheer/referentiemodellen/IECCIM/TC57CIM/IEC61970/Base/Wires#PowerTransformerEnd_x"/>
                <owl:minQualifiedCardinality rdf:datatype="http://www.w3.org/2001/XMLSchema#nonNegativeInteger">0</owl:minQualifiedCardinality>
                <owl:onClass rdf:resource="https://w3id.org/netbeheer/referentiemodellen/IECCIM/TC57CIM/IEC61970/Base/Domain#Reactance"/>
            </owl:Restriction>
        </rdfs:subClassOf>
        <rdfs:subClassOf>
            <owl:Restriction>
                <owl:onProperty rdf:resource="https://w3id.org/netbeheer/referentiemodellen/IECCIM/TC57CIM/IEC61970/Base/Wires#PowerTransformerEnd_x0"/>
                <owl:minQualifiedCardinality rdf:datatype="http://www.w3.org/2001/XMLSchema#nonNegativeInteger">0</owl:minQualifiedCardinality>
                <owl:onClass rdf:resource="https://w3id.org/netbeheer/referentiemodellen/IECCIM/TC57CIM/IEC61970/Base/Domain#Reactance"/>
            </owl:Restriction>
        </rdfs:subClassOf>
        <rdfs:subClassOf>
            <owl:Restriction>
                <owl:onProperty rdf:resource="https://w3id.org/netbeheer/referentiemodellen/IECCIM/TC57CIM/IEC61970/Base/Wires#PowerTransformerEnd_b"/>
                <owl:maxQualifiedCardinality rdf:datatype="http://www.w3.org/2001/XMLSchema#nonNegativeInteger">1</owl:maxQualifiedCardinality>
                <owl:onClass rdf:resource="https://w3id.org/netbeheer/referentiemodellen/IECCIM/TC57CIM/IEC61970/Base/Domain#Susceptance"/>
            </owl:Restriction>
        </rdfs:subClassOf>
        <rdfs:subClassOf>
            <owl:Restriction>
                <owl:onProperty rdf:resource="https://w3id.org/netbeheer/referentiemodellen/IECCIM/TC57CIM/IEC61970/Base/Wires#PowerTransformerEnd_b0"/>
                <owl:maxQualifiedCardinality rdf:datatype="http://www.w3.org/2001/XMLSchema#nonNegativeInteger">1</owl:maxQualifiedCardinality>
                <owl:onClass rdf:resource="https://w3id.org/netbeheer/referentiemodellen/IECCIM/TC57CIM/IEC61970/Base/Domain#Susceptance"/>
            </owl:Restriction>
        </rdfs:subClassOf>
        <rdfs:subClassOf>
            <owl:Restriction>
                <owl:onProperty rdf:resource="https://w3id.org/netbeheer/referentiemodellen/IECCIM/TC57CIM/IEC61970/Base/Wires#PowerTransformerEnd_g"/>
                <owl:maxQualifiedCardinality rdf:datatype="http://www.w3.org/2001/XMLSchema#nonNegativeInteger">1</owl:maxQualifiedCardinality>
                <owl:onClass rdf:resource="https://w3id.org/netbeheer/referentiemodellen/IECCIM/TC57CIM/IEC61970/Base/Domain#Conductance"/>
            </owl:Restriction>
        </rdfs:subClassOf>
        <rdfs:subClassOf>
            <owl:Restriction>
                <owl:onProperty rdf:resource="https://w3id.org/netbeheer/referentiemodellen/IECCIM/TC57CIM/IEC61970/Base/Wires#PowerTransformerEnd_g0"/>
                <owl:maxQualifiedCardinality rdf:datatype="http://www.w3.org/2001/XMLSchema#nonNegativeInteger">1</owl:maxQualifiedCardinality>
                <owl:onClass rdf:resource="https://w3id.org/netbeheer/referentiemodellen/IECCIM/TC57CIM/IEC61970/Base/Domain#Conductance"/>
            </owl:Restriction>
        </rdfs:subClassOf>
        <rdfs:subClassOf>
            <owl:Restriction>
                <owl:onProperty rdf:resource="https://w3id.org/netbeheer/referentiemodellen/IECCIM/TC57CIM/IEC61970/Base/Wires#PowerTransformerEnd_r"/>
                <owl:maxQualifiedCardinality rdf:datatype="http://www.w3.org/2001/XMLSchema#nonNegativeInteger">1</owl:maxQualifiedCardinality>
                <owl:onClass rdf:resource="https://w3id.org/netbeheer/referentiemodellen/IECCIM/TC57CIM/IEC61970/Base/Domain#Resistance"/>
            </owl:Restriction>
        </rdfs:subClassOf>
        <rdfs:subClassOf>
            <owl:Restriction>
                <owl:onProperty rdf:resource="https://w3id.org/netbeheer/referentiemodellen/IECCIM/TC57CIM/IEC61970/Base/Wires#PowerTransformerEnd_r0"/>
                <owl:maxQualifiedCardinality rdf:datatype="http://www.w3.org/2001/XMLSchema#nonNegativeInteger">1</owl:maxQualifiedCardinality>
                <owl:onClass rdf:resource="https://w3id.org/netbeheer/referentiemodellen/IECCIM/TC57CIM/IEC61970/Base/Domain#Resistance"/>
            </owl:Restriction>
        </rdfs:subClassOf>
        <rdfs:subClassOf>
            <owl:Restriction>
                <owl:onProperty rdf:resource="https://w3id.org/netbeheer/referentiemodellen/IECCIM/TC57CIM/IEC61970/Base/Wires#PowerTransformerEnd_ratedS"/>
                <owl:maxQualifiedCardinality rdf:datatype="http://www.w3.org/2001/XMLSchema#nonNegativeInteger">1</owl:maxQualifiedCardinality>
                <owl:onClass rdf:resource="https://w3id.org/netbeheer/referentiemodellen/IECCIM/TC57CIM/IEC61970/Base/Domain#ApparentPower"/>
            </owl:Restriction>
        </rdfs:subClassOf>
        <rdfs:subClassOf>
            <owl:Restriction>
                <owl:onProperty rdf:resource="https://w3id.org/netbeheer/referentiemodellen/IECCIM/TC57CIM/IEC61970/Base/Wires#PowerTransformerEnd_ratedU"/>
                <owl:maxQualifiedCardinality rdf:datatype="http://www.w3.org/2001/XMLSchema#nonNegativeInteger">1</owl:maxQualifiedCardinality>
                <owl:onClass rdf:resource="https://w3id.org/netbeheer/referentiemodellen/IECCIM/TC57CIM/IEC61970/Base/Domain#Voltage"/>
            </owl:Restriction>
        </rdfs:subClassOf>
        <rdfs:subClassOf>
            <owl:Restriction>
                <owl:onProperty rdf:resource="https://w3id.org/netbeheer/referentiemodellen/IECCIM/TC57CIM/IEC61970/Base/Wires#PowerTransformerEnd_x"/>
                <owl:maxQualifiedCardinality rdf:datatype="http://www.w3.org/2001/XMLSchema#nonNegativeInteger">1</owl:maxQualifiedCardinality>
                <owl:onClass rdf:resource="https://w3id.org/netbeheer/referentiemodellen/IECCIM/TC57CIM/IEC61970/Base/Domain#Reactance"/>
            </owl:Restriction>
        </rdfs:subClassOf>
        <rdfs:subClassOf>
            <owl:Restriction>
                <owl:onProperty rdf:resource="https://w3id.org/netbeheer/referentiemodellen/IECCIM/TC57CIM/IEC61970/Base/Wires#PowerTransformerEnd_x0"/>
                <owl:maxQualifiedCardinality rdf:datatype="http://www.w3.org/2001/XMLSchema#nonNegativeInteger">1</owl:maxQualifiedCardinality>
                <owl:onClass rdf:resource="https://w3id.org/netbeheer/referentiemodellen/IECCIM/TC57CIM/IEC61970/Base/Domain#Reactance"/>
            </owl:Restriction>
        </rdfs:subClassOf>
        <rdfs:subClassOf>
            <owl:Restriction>
                <owl:onProperty rdf:resource="https://w3id.org/netbeheer/referentiemodellen/IECCIM/TC57CIM/IEC61970/Base/Wires#PowerTransformerEnd_connectionKind"/>
                <owl:minQualifiedCardinality rdf:datatype="http://www.w3.org/2001/XMLSchema#nonNegativeInteger">0</owl:minQualifiedCardinality>
                <owl:onDataRange rdf:resource="https://w3id.org/netbeheer/referentiemodellen/IECCIM/TC57CIM/IEC61970/Base/Wires#WindingConnection"/>
            </owl:Restriction>
        </rdfs:subClassOf>
        <rdfs:subClassOf>
            <owl:Restriction>
                <owl:onProperty rdf:resource="https://w3id.org/netbeheer/referentiemodellen/IECCIM/TC57CIM/IEC61970/Base/Wires#PowerTransformerEnd_phaseAngleClock"/>
                <owl:minQualifiedCardinality rdf:datatype="http://www.w3.org/2001/XMLSchema#nonNegativeInteger">0</owl:minQualifiedCardinality>
                <owl:onDataRange rdf:resource="http://www.w3.org/2001/XMLSchema#nonNegativeInteger"/>
            </owl:Restriction>
        </rdfs:subClassOf>
        <rdfs:subClassOf>
            <owl:Restriction>
                <owl:onProperty rdf:resource="https://w3id.org/netbeheer/referentiemodellen/IECCIM/TC57CIM/IEC61970/Base/Wires#PowerTransformerEnd_connectionKind"/>
                <owl:maxQualifiedCardinality rdf:datatype="http://www.w3.org/2001/XMLSchema#nonNegativeInteger">1</owl:maxQualifiedCardinality>
                <owl:onDataRange rdf:resource="https://w3id.org/netbeheer/referentiemodellen/IECCIM/TC57CIM/IEC61970/Base/Wires#WindingConnection"/>
            </owl:Restriction>
        </rdfs:subClassOf>
        <rdfs:subClassOf>
            <owl:Restriction>
                <owl:onProperty rdf:resource="https://w3id.org/netbeheer/referentiemodellen/IECCIM/TC57CIM/IEC61970/Base/Wires#PowerTransformerEnd_phaseAngleClock"/>
                <owl:maxQualifiedCardinality rdf:datatype="http://www.w3.org/2001/XMLSchema#nonNegativeInteger">1</owl:maxQualifiedCardinality>
                <owl:onDataRange rdf:resource="http://www.w3.org/2001/XMLSchema#nonNegativeInteger"/>
            </owl:Restriction>
        </rdfs:subClassOf>
        <rdfs:comment>A PowerTransformerEnd is associated with each Terminal of a PowerTransformer.
The impedance values r, r0, x, and x0 of a PowerTransformerEnd represents a star equivalent as follows
1) for a two Terminal PowerTransformer the high voltage PowerTransformerEnd has non zero values on r, r0, x, and x0 while the low voltage PowerTransformerEnd has zero values for r, r0, x, and x0.
2) for a three Terminal PowerTransformer the three PowerTransformerEnds represents a star equivalent with each leg in the star represented by r, r0, x, and x0 values.
3) for a PowerTransformer with more than three Terminals the PowerTransformerEnd impedance values cannot be used. Instead use the TransformerMeshImpedance or split the transformer into multiple PowerTransformers.</rdfs:comment>
    </owl:Class>
    


    <!-- https://w3id.org/netbeheer/referentiemodellen/IECCIM/TC57CIM/IEC61970/Base/Wires#ProtectedSwitch -->


    <owl:Class rdf:about="https://w3id.org/netbeheer/referentiemodellen/IECCIM/TC57CIM/IEC61970/Base/Wires#ProtectedSwitch">
        <rdfs:subClassOf rdf:resource="https://w3id.org/netbeheer/referentiemodellen/IECCIM/TC57CIM/IEC61970/Base/Wires#Switch"/>
        <rdfs:subClassOf>
            <owl:Restriction>
                <owl:onProperty rdf:resource="https://w3id.org/netbeheer/referentiemodellen/IECCIM/TC57CIM/IEC61970/Base/Wires#ProtectedSwitch_OperatedByProtectionEquipment"/>
                <owl:minQualifiedCardinality rdf:datatype="http://www.w3.org/2001/XMLSchema#nonNegativeInteger">0</owl:minQualifiedCardinality>
                <owl:onClass rdf:resource="https://w3id.org/netbeheer/referentiemodellen/IECCIM/TC57CIM/IEC61970/Base/Wires#ProtectedSwitch"/>
            </owl:Restriction>
        </rdfs:subClassOf>
        <rdfs:subClassOf>
            <owl:Restriction>
                <owl:onProperty rdf:resource="https://w3id.org/netbeheer/referentiemodellen/IECCIM/TC57CIM/IEC61970/Base/Wires#ProtectedSwitch_breakingCapacity"/>
                <owl:minQualifiedCardinality rdf:datatype="http://www.w3.org/2001/XMLSchema#nonNegativeInteger">0</owl:minQualifiedCardinality>
                <owl:onClass rdf:resource="https://w3id.org/netbeheer/referentiemodellen/IECCIM/TC57CIM/IEC61970/Base/Domain#CurrentFlow"/>
            </owl:Restriction>
        </rdfs:subClassOf>
        <rdfs:subClassOf>
            <owl:Restriction>
                <owl:onProperty rdf:resource="https://w3id.org/netbeheer/referentiemodellen/IECCIM/TC57CIM/IEC61970/Base/Wires#ProtectedSwitch_RecloseSequences"/>
                <owl:qualifiedCardinality rdf:datatype="http://www.w3.org/2001/XMLSchema#nonNegativeInteger">1</owl:qualifiedCardinality>
                <owl:onClass rdf:resource="https://w3id.org/netbeheer/referentiemodellen/IECCIM/TC57CIM/IEC61970/Base/Wires#ProtectedSwitch"/>
            </owl:Restriction>
        </rdfs:subClassOf>
        <rdfs:subClassOf>
            <owl:Restriction>
                <owl:onProperty rdf:resource="https://w3id.org/netbeheer/referentiemodellen/IECCIM/TC57CIM/IEC61970/Base/Wires#ProtectedSwitch_breakingCapacity"/>
                <owl:maxQualifiedCardinality rdf:datatype="http://www.w3.org/2001/XMLSchema#nonNegativeInteger">1</owl:maxQualifiedCardinality>
                <owl:onClass rdf:resource="https://w3id.org/netbeheer/referentiemodellen/IECCIM/TC57CIM/IEC61970/Base/Domain#CurrentFlow"/>
            </owl:Restriction>
        </rdfs:subClassOf>
        <rdfs:comment>A ProtectedSwitch is a switching device that can be operated by ProtectionEquipment.</rdfs:comment>
    </owl:Class>
    


    <!-- https://w3id.org/netbeheer/referentiemodellen/IECCIM/TC57CIM/IEC61970/Base/Wires#RatioTapChanger -->


    <owl:Class rdf:about="https://w3id.org/netbeheer/referentiemodellen/IECCIM/TC57CIM/IEC61970/Base/Wires#RatioTapChanger">
        <rdfs:subClassOf rdf:resource="https://w3id.org/netbeheer/referentiemodellen/IECCIM/TC57CIM/IEC61970/Base/Wires#TapChanger"/>
        <rdfs:subClassOf>
            <owl:Restriction>
                <owl:onProperty rdf:resource="https://w3id.org/netbeheer/referentiemodellen/IECCIM/TC57CIM/IEC61970/Base/Wires#RatioTapChanger_RatioTapChangerTable"/>
                <owl:minQualifiedCardinality rdf:datatype="http://www.w3.org/2001/XMLSchema#nonNegativeInteger">0</owl:minQualifiedCardinality>
                <owl:onClass rdf:resource="https://w3id.org/netbeheer/referentiemodellen/IECCIM/TC57CIM/IEC61970/Base/Wires#RatioTapChanger"/>
            </owl:Restriction>
        </rdfs:subClassOf>
        <rdfs:subClassOf>
            <owl:Restriction>
                <owl:onProperty rdf:resource="https://w3id.org/netbeheer/referentiemodellen/IECCIM/TC57CIM/IEC61970/Base/Wires#RatioTapChanger_TransformerEnd"/>
                <owl:minQualifiedCardinality rdf:datatype="http://www.w3.org/2001/XMLSchema#nonNegativeInteger">0</owl:minQualifiedCardinality>
                <owl:onClass rdf:resource="https://w3id.org/netbeheer/referentiemodellen/IECCIM/TC57CIM/IEC61970/Base/Wires#RatioTapChanger"/>
            </owl:Restriction>
        </rdfs:subClassOf>
        <rdfs:subClassOf>
            <owl:Restriction>
                <owl:onProperty rdf:resource="https://w3id.org/netbeheer/referentiemodellen/IECCIM/TC57CIM/IEC61970/Base/Wires#RatioTapChanger_stepVoltageIncrement"/>
                <owl:minQualifiedCardinality rdf:datatype="http://www.w3.org/2001/XMLSchema#nonNegativeInteger">0</owl:minQualifiedCardinality>
                <owl:onClass rdf:resource="https://w3id.org/netbeheer/referentiemodellen/IECCIM/TC57CIM/IEC61970/Base/Domain#PerCent"/>
            </owl:Restriction>
        </rdfs:subClassOf>
        <rdfs:subClassOf>
            <owl:Restriction>
                <owl:onProperty rdf:resource="https://w3id.org/netbeheer/referentiemodellen/IECCIM/TC57CIM/IEC61970/Base/Wires#RatioTapChanger_TransformerEnd"/>
                <owl:maxQualifiedCardinality rdf:datatype="http://www.w3.org/2001/XMLSchema#nonNegativeInteger">1</owl:maxQualifiedCardinality>
                <owl:onClass rdf:resource="https://w3id.org/netbeheer/referentiemodellen/IECCIM/TC57CIM/IEC61970/Base/Wires#RatioTapChanger"/>
            </owl:Restriction>
        </rdfs:subClassOf>
        <rdfs:subClassOf>
            <owl:Restriction>
                <owl:onProperty rdf:resource="https://w3id.org/netbeheer/referentiemodellen/IECCIM/TC57CIM/IEC61970/Base/Wires#RatioTapChanger_stepVoltageIncrement"/>
                <owl:maxQualifiedCardinality rdf:datatype="http://www.w3.org/2001/XMLSchema#nonNegativeInteger">1</owl:maxQualifiedCardinality>
                <owl:onClass rdf:resource="https://w3id.org/netbeheer/referentiemodellen/IECCIM/TC57CIM/IEC61970/Base/Domain#PerCent"/>
            </owl:Restriction>
        </rdfs:subClassOf>
        <rdfs:subClassOf>
            <owl:Restriction>
                <owl:onProperty rdf:resource="https://w3id.org/netbeheer/referentiemodellen/IECCIM/TC57CIM/IEC61970/Base/Wires#RatioTapChanger_tculControlMode"/>
                <owl:minQualifiedCardinality rdf:datatype="http://www.w3.org/2001/XMLSchema#nonNegativeInteger">0</owl:minQualifiedCardinality>
                <owl:onDataRange rdf:resource="https://w3id.org/netbeheer/referentiemodellen/IECCIM/TC57CIM/IEC61970/Base/Wires#TransformerControlMode"/>
            </owl:Restriction>
        </rdfs:subClassOf>
        <rdfs:subClassOf>
            <owl:Restriction>
                <owl:onProperty rdf:resource="https://w3id.org/netbeheer/referentiemodellen/IECCIM/TC57CIM/IEC61970/Base/Wires#RatioTapChanger_tculControlMode"/>
                <owl:maxQualifiedCardinality rdf:datatype="http://www.w3.org/2001/XMLSchema#nonNegativeInteger">1</owl:maxQualifiedCardinality>
                <owl:onDataRange rdf:resource="https://w3id.org/netbeheer/referentiemodellen/IECCIM/TC57CIM/IEC61970/Base/Wires#TransformerControlMode"/>
            </owl:Restriction>
        </rdfs:subClassOf>
        <rdfs:comment>A tap changer that changes the voltage ratio impacting the voltage magnitude but not the phase angle across the transformer.
</rdfs:comment>
    </owl:Class>
    


    <!-- https://w3id.org/netbeheer/referentiemodellen/IECCIM/TC57CIM/IEC61970/Base/Wires#RatioTapChangerTable -->


    <owl:Class rdf:about="https://w3id.org/netbeheer/referentiemodellen/IECCIM/TC57CIM/IEC61970/Base/Wires#RatioTapChangerTable">
        <rdfs:subClassOf rdf:resource="https://w3id.org/netbeheer/referentiemodellen/IECCIM/TC57CIM/IEC61970/Base/Core#IdentifiedObject"/>
        <rdfs:subClassOf>
            <owl:Restriction>
                <owl:onProperty rdf:resource="https://w3id.org/netbeheer/referentiemodellen/IECCIM/TC57CIM/IEC61970/Base/Wires#RatioTapChangerTable_RatioTapChanger"/>
                <owl:minQualifiedCardinality rdf:datatype="http://www.w3.org/2001/XMLSchema#nonNegativeInteger">0</owl:minQualifiedCardinality>
                <owl:onClass rdf:resource="https://w3id.org/netbeheer/referentiemodellen/IECCIM/TC57CIM/IEC61970/Base/Wires#RatioTapChangerTable"/>
            </owl:Restriction>
        </rdfs:subClassOf>
        <rdfs:subClassOf>
            <owl:Restriction>
                <owl:onProperty rdf:resource="https://w3id.org/netbeheer/referentiemodellen/IECCIM/TC57CIM/IEC61970/Base/Wires#RatioTapChangerTable_RatioTapChangerTablePoint"/>
                <owl:qualifiedCardinality rdf:datatype="http://www.w3.org/2001/XMLSchema#nonNegativeInteger">1</owl:qualifiedCardinality>
                <owl:onClass rdf:resource="https://w3id.org/netbeheer/referentiemodellen/IECCIM/TC57CIM/IEC61970/Base/Wires#RatioTapChangerTable"/>
            </owl:Restriction>
        </rdfs:subClassOf>
        <rdfs:subClassOf>
            <owl:Restriction>
                <owl:onProperty rdf:resource="https://w3id.org/netbeheer/referentiemodellen/IECCIM/TC57CIM/IEC61970/Base/Wires#RatioTapChangerTable_RatioTapChanger"/>
                <owl:maxQualifiedCardinality rdf:datatype="http://www.w3.org/2001/XMLSchema#nonNegativeInteger">1</owl:maxQualifiedCardinality>
                <owl:onClass rdf:resource="https://w3id.org/netbeheer/referentiemodellen/IECCIM/TC57CIM/IEC61970/Base/Wires#RatioTapChangerTable"/>
            </owl:Restriction>
        </rdfs:subClassOf>
        <rdfs:comment>Describes a curve for how the voltage magnitude and impedance varies with the tap step. </rdfs:comment>
    </owl:Class>
    


    <!-- https://w3id.org/netbeheer/referentiemodellen/IECCIM/TC57CIM/IEC61970/Base/Wires#RatioTapChangerTablePoint -->


    <owl:Class rdf:about="https://w3id.org/netbeheer/referentiemodellen/IECCIM/TC57CIM/IEC61970/Base/Wires#RatioTapChangerTablePoint">
        <rdfs:subClassOf rdf:resource="https://w3id.org/netbeheer/referentiemodellen/IECCIM/TC57CIM/IEC61970/Base/Wires#TapChangerTablePoint"/>
        <rdfs:subClassOf>
            <owl:Restriction>
                <owl:onProperty rdf:resource="https://w3id.org/netbeheer/referentiemodellen/IECCIM/TC57CIM/IEC61970/Base/Wires#RatioTapChangerTablePoint_RatioTapChangerTable"/>
                <owl:minQualifiedCardinality rdf:datatype="http://www.w3.org/2001/XMLSchema#nonNegativeInteger">1</owl:minQualifiedCardinality>
                <owl:onClass rdf:resource="https://w3id.org/netbeheer/referentiemodellen/IECCIM/TC57CIM/IEC61970/Base/Wires#RatioTapChangerTablePoint"/>
            </owl:Restriction>
        </rdfs:subClassOf>
        <rdfs:comment>Describes each tap step in the ratio tap changer tabular curve.
</rdfs:comment>
    </owl:Class>
    


    <!-- https://w3id.org/netbeheer/referentiemodellen/IECCIM/TC57CIM/IEC61970/Base/Wires#ReactiveCapabilityCurve -->


    <owl:Class rdf:about="https://w3id.org/netbeheer/referentiemodellen/IECCIM/TC57CIM/IEC61970/Base/Wires#ReactiveCapabilityCurve">
        <rdfs:subClassOf rdf:resource="https://w3id.org/netbeheer/referentiemodellen/IECCIM/TC57CIM/IEC61970/Base/Core#Curve"/>
        <rdfs:subClassOf>
            <owl:Restriction>
                <owl:onProperty rdf:resource="https://w3id.org/netbeheer/referentiemodellen/IECCIM/TC57CIM/IEC61970/Base/Wires#ReactiveCapabilityCurve_EquivalentInjection"/>
                <owl:minQualifiedCardinality rdf:datatype="http://www.w3.org/2001/XMLSchema#nonNegativeInteger">0</owl:minQualifiedCardinality>
                <owl:onClass rdf:resource="https://w3id.org/netbeheer/referentiemodellen/IECCIM/TC57CIM/IEC61970/Base/Wires#ReactiveCapabilityCurve"/>
            </owl:Restriction>
        </rdfs:subClassOf>
        <rdfs:subClassOf>
            <owl:Restriction>
                <owl:onProperty rdf:resource="https://w3id.org/netbeheer/referentiemodellen/IECCIM/TC57CIM/IEC61970/Base/Wires#ReactiveCapabilityCurve_InitiallyUsedBySynchronousMachines"/>
                <owl:minQualifiedCardinality rdf:datatype="http://www.w3.org/2001/XMLSchema#nonNegativeInteger">0</owl:minQualifiedCardinality>
                <owl:onClass rdf:resource="https://w3id.org/netbeheer/referentiemodellen/IECCIM/TC57CIM/IEC61970/Base/Wires#ReactiveCapabilityCurve"/>
            </owl:Restriction>
        </rdfs:subClassOf>
        <rdfs:subClassOf>
            <owl:Restriction>
                <owl:onProperty rdf:resource="https://w3id.org/netbeheer/referentiemodellen/IECCIM/TC57CIM/IEC61970/Base/Wires#ReactiveCapabilityCurve_SynchronousMachines"/>
                <owl:minQualifiedCardinality rdf:datatype="http://www.w3.org/2001/XMLSchema#nonNegativeInteger">0</owl:minQualifiedCardinality>
                <owl:onClass rdf:resource="https://w3id.org/netbeheer/referentiemodellen/IECCIM/TC57CIM/IEC61970/Base/Wires#ReactiveCapabilityCurve"/>
            </owl:Restriction>
        </rdfs:subClassOf>
        <rdfs:subClassOf>
            <owl:Restriction>
                <owl:onProperty rdf:resource="https://w3id.org/netbeheer/referentiemodellen/IECCIM/TC57CIM/IEC61970/Base/Wires#ReactiveCapabilityCurve_coolantTemperature"/>
                <owl:minQualifiedCardinality rdf:datatype="http://www.w3.org/2001/XMLSchema#nonNegativeInteger">0</owl:minQualifiedCardinality>
                <owl:onClass rdf:resource="https://w3id.org/netbeheer/referentiemodellen/IECCIM/TC57CIM/IEC61970/Base/Domain#Temperature"/>
            </owl:Restriction>
        </rdfs:subClassOf>
        <rdfs:subClassOf>
            <owl:Restriction>
                <owl:onProperty rdf:resource="https://w3id.org/netbeheer/referentiemodellen/IECCIM/TC57CIM/IEC61970/Base/Wires#ReactiveCapabilityCurve_hydrogenPressure"/>
                <owl:minQualifiedCardinality rdf:datatype="http://www.w3.org/2001/XMLSchema#nonNegativeInteger">0</owl:minQualifiedCardinality>
                <owl:onClass rdf:resource="https://w3id.org/netbeheer/referentiemodellen/IECCIM/TC57CIM/IEC61970/Base/Domain#Pressure"/>
            </owl:Restriction>
        </rdfs:subClassOf>
        <rdfs:subClassOf>
            <owl:Restriction>
                <owl:onProperty rdf:resource="https://w3id.org/netbeheer/referentiemodellen/IECCIM/TC57CIM/IEC61970/Base/Wires#ReactiveCapabilityCurve_EquivalentInjection"/>
                <owl:maxQualifiedCardinality rdf:datatype="http://www.w3.org/2001/XMLSchema#nonNegativeInteger">1</owl:maxQualifiedCardinality>
                <owl:onClass rdf:resource="https://w3id.org/netbeheer/referentiemodellen/IECCIM/TC57CIM/IEC61970/Base/Wires#ReactiveCapabilityCurve"/>
            </owl:Restriction>
        </rdfs:subClassOf>
        <rdfs:subClassOf>
            <owl:Restriction>
                <owl:onProperty rdf:resource="https://w3id.org/netbeheer/referentiemodellen/IECCIM/TC57CIM/IEC61970/Base/Wires#ReactiveCapabilityCurve_InitiallyUsedBySynchronousMachines"/>
                <owl:maxQualifiedCardinality rdf:datatype="http://www.w3.org/2001/XMLSchema#nonNegativeInteger">1</owl:maxQualifiedCardinality>
                <owl:onClass rdf:resource="https://w3id.org/netbeheer/referentiemodellen/IECCIM/TC57CIM/IEC61970/Base/Wires#ReactiveCapabilityCurve"/>
            </owl:Restriction>
        </rdfs:subClassOf>
        <rdfs:subClassOf>
            <owl:Restriction>
                <owl:onProperty rdf:resource="https://w3id.org/netbeheer/referentiemodellen/IECCIM/TC57CIM/IEC61970/Base/Wires#ReactiveCapabilityCurve_coolantTemperature"/>
                <owl:maxQualifiedCardinality rdf:datatype="http://www.w3.org/2001/XMLSchema#nonNegativeInteger">1</owl:maxQualifiedCardinality>
                <owl:onClass rdf:resource="https://w3id.org/netbeheer/referentiemodellen/IECCIM/TC57CIM/IEC61970/Base/Domain#Temperature"/>
            </owl:Restriction>
        </rdfs:subClassOf>
        <rdfs:subClassOf>
            <owl:Restriction>
                <owl:onProperty rdf:resource="https://w3id.org/netbeheer/referentiemodellen/IECCIM/TC57CIM/IEC61970/Base/Wires#ReactiveCapabilityCurve_hydrogenPressure"/>
                <owl:maxQualifiedCardinality rdf:datatype="http://www.w3.org/2001/XMLSchema#nonNegativeInteger">1</owl:maxQualifiedCardinality>
                <owl:onClass rdf:resource="https://w3id.org/netbeheer/referentiemodellen/IECCIM/TC57CIM/IEC61970/Base/Domain#Pressure"/>
            </owl:Restriction>
        </rdfs:subClassOf>
        <rdfs:comment>Reactive power rating envelope versus the synchronous machine&apos;s active power, in both the generating and motoring modes. For each active power value there is a corresponding high and low reactive power limit  value. Typically there will be a separate curve for each coolant condition, such as hydrogen pressure.  The Y1 axis values represent reactive minimum and the Y2 axis values represent reactive maximum.</rdfs:comment>
    </owl:Class>
    


    <!-- https://w3id.org/netbeheer/referentiemodellen/IECCIM/TC57CIM/IEC61970/Base/Wires#Recloser -->


    <owl:Class rdf:about="https://w3id.org/netbeheer/referentiemodellen/IECCIM/TC57CIM/IEC61970/Base/Wires#Recloser">
        <rdfs:subClassOf rdf:resource="https://w3id.org/netbeheer/referentiemodellen/IECCIM/TC57CIM/IEC61970/Base/Wires#ProtectedSwitch"/>
        <rdfs:comment>Pole-mounted fault interrupter with built-in phase and ground relays, current transformer (CT), and supplemental controls.
</rdfs:comment>
    </owl:Class>
    


    <!-- https://w3id.org/netbeheer/referentiemodellen/IECCIM/TC57CIM/IEC61970/Base/Wires#RegulatingCondEq -->


    <owl:Class rdf:about="https://w3id.org/netbeheer/referentiemodellen/IECCIM/TC57CIM/IEC61970/Base/Wires#RegulatingCondEq">
        <rdfs:subClassOf rdf:resource="https://w3id.org/netbeheer/referentiemodellen/IECCIM/TC57CIM/IEC61970/Base/Core#ConductingEquipment"/>
        <rdfs:subClassOf>
            <owl:Restriction>
                <owl:onProperty rdf:resource="https://w3id.org/netbeheer/referentiemodellen/IECCIM/TC57CIM/IEC61970/Base/Wires#RegulatingCondEq_RegulatingControl"/>
                <owl:minQualifiedCardinality rdf:datatype="http://www.w3.org/2001/XMLSchema#nonNegativeInteger">0</owl:minQualifiedCardinality>
                <owl:onClass rdf:resource="https://w3id.org/netbeheer/referentiemodellen/IECCIM/TC57CIM/IEC61970/Base/Wires#RegulatingCondEq"/>
            </owl:Restriction>
        </rdfs:subClassOf>
        <rdfs:subClassOf>
            <owl:Restriction>
                <owl:onProperty rdf:resource="https://w3id.org/netbeheer/referentiemodellen/IECCIM/TC57CIM/IEC61970/Base/Wires#RegulatingCondEq_controlEnabled"/>
                <owl:minQualifiedCardinality rdf:datatype="http://www.w3.org/2001/XMLSchema#nonNegativeInteger">0</owl:minQualifiedCardinality>
                <owl:onDataRange rdf:resource="http://www.w3.org/2001/XMLSchema#boolean"/>
            </owl:Restriction>
        </rdfs:subClassOf>
        <rdfs:subClassOf>
            <owl:Restriction>
                <owl:onProperty rdf:resource="https://w3id.org/netbeheer/referentiemodellen/IECCIM/TC57CIM/IEC61970/Base/Wires#RegulatingCondEq_controlEnabled"/>
                <owl:maxQualifiedCardinality rdf:datatype="http://www.w3.org/2001/XMLSchema#nonNegativeInteger">1</owl:maxQualifiedCardinality>
                <owl:onDataRange rdf:resource="http://www.w3.org/2001/XMLSchema#boolean"/>
            </owl:Restriction>
        </rdfs:subClassOf>
        <rdfs:comment>A type of conducting equipment that can regulate a quantity (i.e. voltage or flow) at a specific point in the network. </rdfs:comment>
    </owl:Class>
    


    <!-- https://w3id.org/netbeheer/referentiemodellen/IECCIM/TC57CIM/IEC61970/Base/Wires#RegulatingControl -->


    <owl:Class rdf:about="https://w3id.org/netbeheer/referentiemodellen/IECCIM/TC57CIM/IEC61970/Base/Wires#RegulatingControl">
        <rdfs:subClassOf rdf:resource="https://w3id.org/netbeheer/referentiemodellen/IECCIM/TC57CIM/IEC61970/Base/Core#PowerSystemResource"/>
        <rdfs:subClassOf>
            <owl:Restriction>
                <owl:onProperty rdf:resource="https://w3id.org/netbeheer/referentiemodellen/IECCIM/TC57CIM/IEC61970/Base/Wires#RegulatingControl_RegulatingCondEq"/>
                <owl:minQualifiedCardinality rdf:datatype="http://www.w3.org/2001/XMLSchema#nonNegativeInteger">0</owl:minQualifiedCardinality>
                <owl:onClass rdf:resource="https://w3id.org/netbeheer/referentiemodellen/IECCIM/TC57CIM/IEC61970/Base/Wires#RegulatingControl"/>
            </owl:Restriction>
        </rdfs:subClassOf>
        <rdfs:subClassOf>
            <owl:Restriction>
                <owl:onProperty rdf:resource="https://w3id.org/netbeheer/referentiemodellen/IECCIM/TC57CIM/IEC61970/Base/Wires#RegulatingControl_ProtectiveActionRegulation"/>
                <owl:qualifiedCardinality rdf:datatype="http://www.w3.org/2001/XMLSchema#nonNegativeInteger">1</owl:qualifiedCardinality>
                <owl:onClass rdf:resource="https://w3id.org/netbeheer/referentiemodellen/IECCIM/TC57CIM/IEC61970/Base/Wires#RegulatingControl"/>
            </owl:Restriction>
        </rdfs:subClassOf>
        <rdfs:subClassOf>
            <owl:Restriction>
                <owl:onProperty rdf:resource="https://w3id.org/netbeheer/referentiemodellen/IECCIM/TC57CIM/IEC61970/Base/Wires#RegulatingControl_RegulationSchedule"/>
                <owl:qualifiedCardinality rdf:datatype="http://www.w3.org/2001/XMLSchema#nonNegativeInteger">1</owl:qualifiedCardinality>
                <owl:onClass rdf:resource="https://w3id.org/netbeheer/referentiemodellen/IECCIM/TC57CIM/IEC61970/Base/Wires#RegulatingControl"/>
            </owl:Restriction>
        </rdfs:subClassOf>
        <rdfs:subClassOf>
            <owl:Restriction>
                <owl:onProperty rdf:resource="https://w3id.org/netbeheer/referentiemodellen/IECCIM/TC57CIM/IEC61970/Base/Wires#RegulatingControl_RegulatingCondEq"/>
                <owl:maxQualifiedCardinality rdf:datatype="http://www.w3.org/2001/XMLSchema#nonNegativeInteger">1</owl:maxQualifiedCardinality>
                <owl:onClass rdf:resource="https://w3id.org/netbeheer/referentiemodellen/IECCIM/TC57CIM/IEC61970/Base/Wires#RegulatingControl"/>
            </owl:Restriction>
        </rdfs:subClassOf>
        <rdfs:subClassOf>
            <owl:Restriction>
                <owl:onProperty rdf:resource="https://w3id.org/netbeheer/referentiemodellen/IECCIM/TC57CIM/IEC61970/Base/Wires#RegulatingControl_discrete"/>
                <owl:minQualifiedCardinality rdf:datatype="http://www.w3.org/2001/XMLSchema#nonNegativeInteger">0</owl:minQualifiedCardinality>
                <owl:onDataRange rdf:resource="http://www.w3.org/2001/XMLSchema#boolean"/>
            </owl:Restriction>
        </rdfs:subClassOf>
        <rdfs:subClassOf>
            <owl:Restriction>
                <owl:onProperty rdf:resource="https://w3id.org/netbeheer/referentiemodellen/IECCIM/TC57CIM/IEC61970/Base/Wires#RegulatingControl_enabled"/>
                <owl:minQualifiedCardinality rdf:datatype="http://www.w3.org/2001/XMLSchema#nonNegativeInteger">0</owl:minQualifiedCardinality>
                <owl:onDataRange rdf:resource="http://www.w3.org/2001/XMLSchema#boolean"/>
            </owl:Restriction>
        </rdfs:subClassOf>
        <rdfs:subClassOf>
            <owl:Restriction>
                <owl:onProperty rdf:resource="https://w3id.org/netbeheer/referentiemodellen/IECCIM/TC57CIM/IEC61970/Base/Wires#RegulatingControl_mode"/>
                <owl:minQualifiedCardinality rdf:datatype="http://www.w3.org/2001/XMLSchema#nonNegativeInteger">0</owl:minQualifiedCardinality>
                <owl:onDataRange rdf:resource="https://w3id.org/netbeheer/referentiemodellen/IECCIM/TC57CIM/IEC61970/Base/Wires#RegulatingControlModeKind"/>
            </owl:Restriction>
        </rdfs:subClassOf>
        <rdfs:subClassOf>
            <owl:Restriction>
                <owl:onProperty rdf:resource="https://w3id.org/netbeheer/referentiemodellen/IECCIM/TC57CIM/IEC61970/Base/Wires#RegulatingControl_monitoredPhase"/>
                <owl:minQualifiedCardinality rdf:datatype="http://www.w3.org/2001/XMLSchema#nonNegativeInteger">0</owl:minQualifiedCardinality>
                <owl:onDataRange rdf:resource="https://w3id.org/netbeheer/referentiemodellen/IECCIM/TC57CIM/IEC61970/Base/Core#PhaseCode"/>
            </owl:Restriction>
        </rdfs:subClassOf>
        <rdfs:subClassOf>
            <owl:Restriction>
                <owl:onProperty rdf:resource="https://w3id.org/netbeheer/referentiemodellen/IECCIM/TC57CIM/IEC61970/Base/Wires#RegulatingControl_targetDeadband"/>
                <owl:minQualifiedCardinality rdf:datatype="http://www.w3.org/2001/XMLSchema#nonNegativeInteger">0</owl:minQualifiedCardinality>
                <owl:onDataRange rdf:resource="http://www.w3.org/2001/XMLSchema#float"/>
            </owl:Restriction>
        </rdfs:subClassOf>
        <rdfs:subClassOf>
            <owl:Restriction>
                <owl:onProperty rdf:resource="https://w3id.org/netbeheer/referentiemodellen/IECCIM/TC57CIM/IEC61970/Base/Wires#RegulatingControl_targetValue"/>
                <owl:minQualifiedCardinality rdf:datatype="http://www.w3.org/2001/XMLSchema#nonNegativeInteger">0</owl:minQualifiedCardinality>
                <owl:onDataRange rdf:resource="http://www.w3.org/2001/XMLSchema#float"/>
            </owl:Restriction>
        </rdfs:subClassOf>
        <rdfs:subClassOf>
            <owl:Restriction>
                <owl:onProperty rdf:resource="https://w3id.org/netbeheer/referentiemodellen/IECCIM/TC57CIM/IEC61970/Base/Wires#RegulatingControl_targetValueUnitMultiplier"/>
                <owl:minQualifiedCardinality rdf:datatype="http://www.w3.org/2001/XMLSchema#nonNegativeInteger">0</owl:minQualifiedCardinality>
                <owl:onDataRange rdf:resource="https://w3id.org/netbeheer/referentiemodellen/IECCIM/TC57CIM/IEC61970/Base/Domain#UnitMultiplier"/>
            </owl:Restriction>
        </rdfs:subClassOf>
        <rdfs:subClassOf>
            <owl:Restriction>
                <owl:onProperty rdf:resource="https://w3id.org/netbeheer/referentiemodellen/IECCIM/TC57CIM/IEC61970/Base/Wires#RegulatingControl_discrete"/>
                <owl:maxQualifiedCardinality rdf:datatype="http://www.w3.org/2001/XMLSchema#nonNegativeInteger">1</owl:maxQualifiedCardinality>
                <owl:onDataRange rdf:resource="http://www.w3.org/2001/XMLSchema#boolean"/>
            </owl:Restriction>
        </rdfs:subClassOf>
        <rdfs:subClassOf>
            <owl:Restriction>
                <owl:onProperty rdf:resource="https://w3id.org/netbeheer/referentiemodellen/IECCIM/TC57CIM/IEC61970/Base/Wires#RegulatingControl_enabled"/>
                <owl:maxQualifiedCardinality rdf:datatype="http://www.w3.org/2001/XMLSchema#nonNegativeInteger">1</owl:maxQualifiedCardinality>
                <owl:onDataRange rdf:resource="http://www.w3.org/2001/XMLSchema#boolean"/>
            </owl:Restriction>
        </rdfs:subClassOf>
        <rdfs:subClassOf>
            <owl:Restriction>
                <owl:onProperty rdf:resource="https://w3id.org/netbeheer/referentiemodellen/IECCIM/TC57CIM/IEC61970/Base/Wires#RegulatingControl_mode"/>
                <owl:maxQualifiedCardinality rdf:datatype="http://www.w3.org/2001/XMLSchema#nonNegativeInteger">1</owl:maxQualifiedCardinality>
                <owl:onDataRange rdf:resource="https://w3id.org/netbeheer/referentiemodellen/IECCIM/TC57CIM/IEC61970/Base/Wires#RegulatingControlModeKind"/>
            </owl:Restriction>
        </rdfs:subClassOf>
        <rdfs:subClassOf>
            <owl:Restriction>
                <owl:onProperty rdf:resource="https://w3id.org/netbeheer/referentiemodellen/IECCIM/TC57CIM/IEC61970/Base/Wires#RegulatingControl_monitoredPhase"/>
                <owl:maxQualifiedCardinality rdf:datatype="http://www.w3.org/2001/XMLSchema#nonNegativeInteger">1</owl:maxQualifiedCardinality>
                <owl:onDataRange rdf:resource="https://w3id.org/netbeheer/referentiemodellen/IECCIM/TC57CIM/IEC61970/Base/Core#PhaseCode"/>
            </owl:Restriction>
        </rdfs:subClassOf>
        <rdfs:subClassOf>
            <owl:Restriction>
                <owl:onProperty rdf:resource="https://w3id.org/netbeheer/referentiemodellen/IECCIM/TC57CIM/IEC61970/Base/Wires#RegulatingControl_targetDeadband"/>
                <owl:maxQualifiedCardinality rdf:datatype="http://www.w3.org/2001/XMLSchema#nonNegativeInteger">1</owl:maxQualifiedCardinality>
                <owl:onDataRange rdf:resource="http://www.w3.org/2001/XMLSchema#float"/>
            </owl:Restriction>
        </rdfs:subClassOf>
        <rdfs:subClassOf>
            <owl:Restriction>
                <owl:onProperty rdf:resource="https://w3id.org/netbeheer/referentiemodellen/IECCIM/TC57CIM/IEC61970/Base/Wires#RegulatingControl_targetValue"/>
                <owl:maxQualifiedCardinality rdf:datatype="http://www.w3.org/2001/XMLSchema#nonNegativeInteger">1</owl:maxQualifiedCardinality>
                <owl:onDataRange rdf:resource="http://www.w3.org/2001/XMLSchema#float"/>
            </owl:Restriction>
        </rdfs:subClassOf>
        <rdfs:subClassOf>
            <owl:Restriction>
                <owl:onProperty rdf:resource="https://w3id.org/netbeheer/referentiemodellen/IECCIM/TC57CIM/IEC61970/Base/Wires#RegulatingControl_targetValueUnitMultiplier"/>
                <owl:maxQualifiedCardinality rdf:datatype="http://www.w3.org/2001/XMLSchema#nonNegativeInteger">1</owl:maxQualifiedCardinality>
                <owl:onDataRange rdf:resource="https://w3id.org/netbeheer/referentiemodellen/IECCIM/TC57CIM/IEC61970/Base/Domain#UnitMultiplier"/>
            </owl:Restriction>
        </rdfs:subClassOf>
        <rdfs:comment>Specifies a set of equipment that works together to control a power system quantity such as voltage or flow. 
Remote bus voltage control is possible by specifying the controlled terminal located at some place remote from the controlling equipment.
In case multiple equipment, possibly of different types, control same terminal there must be only one RegulatingControl at that terminal. The most specific subtype of RegulatingControl shall be used in case such equipment participate in the control, e.g. TapChangerControl for tap changers.
For flow control  load sign convention is used, i.e. positive sign means flow out from a TopologicalNode (bus) into the conducting equipment.</rdfs:comment>
    </owl:Class>
    


    <!-- https://w3id.org/netbeheer/referentiemodellen/IECCIM/TC57CIM/IEC61970/Base/Wires#RegulationSchedule -->


    <owl:Class rdf:about="https://w3id.org/netbeheer/referentiemodellen/IECCIM/TC57CIM/IEC61970/Base/Wires#RegulationSchedule">
        <rdfs:subClassOf rdf:resource="https://w3id.org/netbeheer/referentiemodellen/IECCIM/TC57CIM/IEC61970/Base/LoadModel#SeasonDayTypeSchedule"/>
        <rdfs:subClassOf>
            <owl:Restriction>
                <owl:onProperty rdf:resource="https://w3id.org/netbeheer/referentiemodellen/IECCIM/TC57CIM/IEC61970/Base/Wires#RegulationSchedule_RegulatingControl"/>
                <owl:minQualifiedCardinality rdf:datatype="http://www.w3.org/2001/XMLSchema#nonNegativeInteger">0</owl:minQualifiedCardinality>
                <owl:onClass rdf:resource="https://w3id.org/netbeheer/referentiemodellen/IECCIM/TC57CIM/IEC61970/Base/Wires#RegulationSchedule"/>
            </owl:Restriction>
        </rdfs:subClassOf>
        <rdfs:subClassOf>
            <owl:Restriction>
                <owl:onProperty rdf:resource="https://w3id.org/netbeheer/referentiemodellen/IECCIM/TC57CIM/IEC61970/Base/Wires#RegulationSchedule_VoltageControlZones"/>
                <owl:minQualifiedCardinality rdf:datatype="http://www.w3.org/2001/XMLSchema#nonNegativeInteger">0</owl:minQualifiedCardinality>
                <owl:onClass rdf:resource="https://w3id.org/netbeheer/referentiemodellen/IECCIM/TC57CIM/IEC61970/Base/Wires#RegulationSchedule"/>
            </owl:Restriction>
        </rdfs:subClassOf>
        <rdfs:subClassOf>
            <owl:Restriction>
                <owl:onProperty rdf:resource="https://w3id.org/netbeheer/referentiemodellen/IECCIM/TC57CIM/IEC61970/Base/Wires#RegulationSchedule_VoltageControlZones"/>
                <owl:maxQualifiedCardinality rdf:datatype="http://www.w3.org/2001/XMLSchema#nonNegativeInteger">1</owl:maxQualifiedCardinality>
                <owl:onClass rdf:resource="https://w3id.org/netbeheer/referentiemodellen/IECCIM/TC57CIM/IEC61970/Base/Wires#RegulationSchedule"/>
            </owl:Restriction>
        </rdfs:subClassOf>
        <rdfs:comment>A pre-established pattern over time for a controlled variable, e.g., busbar voltage.</rdfs:comment>
    </owl:Class>
    


    <!-- https://w3id.org/netbeheer/referentiemodellen/IECCIM/TC57CIM/IEC61970/Base/Wires#RotatingMachine -->


    <owl:Class rdf:about="https://w3id.org/netbeheer/referentiemodellen/IECCIM/TC57CIM/IEC61970/Base/Wires#RotatingMachine">
        <rdfs:subClassOf rdf:resource="https://w3id.org/netbeheer/referentiemodellen/IECCIM/TC57CIM/IEC61970/Base/Wires#RegulatingCondEq"/>
        <rdfs:subClassOf>
            <owl:Restriction>
                <owl:onProperty rdf:resource="https://w3id.org/netbeheer/referentiemodellen/IECCIM/TC57CIM/IEC61970/Base/Wires#RotatingMachine_GeneratingUnit"/>
                <owl:minQualifiedCardinality rdf:datatype="http://www.w3.org/2001/XMLSchema#nonNegativeInteger">1</owl:minQualifiedCardinality>
                <owl:onClass rdf:resource="https://w3id.org/netbeheer/referentiemodellen/IECCIM/TC57CIM/IEC61970/Base/Wires#RotatingMachine"/>
            </owl:Restriction>
        </rdfs:subClassOf>
        <rdfs:subClassOf>
            <owl:Restriction>
                <owl:onProperty rdf:resource="https://w3id.org/netbeheer/referentiemodellen/IECCIM/TC57CIM/IEC61970/Base/Wires#RotatingMachine_p"/>
                <owl:minQualifiedCardinality rdf:datatype="http://www.w3.org/2001/XMLSchema#nonNegativeInteger">0</owl:minQualifiedCardinality>
                <owl:onClass rdf:resource="https://w3id.org/netbeheer/referentiemodellen/IECCIM/TC57CIM/IEC61970/Base/Domain#ActivePower"/>
            </owl:Restriction>
        </rdfs:subClassOf>
        <rdfs:subClassOf>
            <owl:Restriction>
                <owl:onProperty rdf:resource="https://w3id.org/netbeheer/referentiemodellen/IECCIM/TC57CIM/IEC61970/Base/Wires#RotatingMachine_q"/>
                <owl:minQualifiedCardinality rdf:datatype="http://www.w3.org/2001/XMLSchema#nonNegativeInteger">0</owl:minQualifiedCardinality>
                <owl:onClass rdf:resource="https://w3id.org/netbeheer/referentiemodellen/IECCIM/TC57CIM/IEC61970/Base/Domain#ReactivePower"/>
            </owl:Restriction>
        </rdfs:subClassOf>
        <rdfs:subClassOf>
            <owl:Restriction>
                <owl:onProperty rdf:resource="https://w3id.org/netbeheer/referentiemodellen/IECCIM/TC57CIM/IEC61970/Base/Wires#RotatingMachine_ratedS"/>
                <owl:minQualifiedCardinality rdf:datatype="http://www.w3.org/2001/XMLSchema#nonNegativeInteger">0</owl:minQualifiedCardinality>
                <owl:onClass rdf:resource="https://w3id.org/netbeheer/referentiemodellen/IECCIM/TC57CIM/IEC61970/Base/Domain#ApparentPower"/>
            </owl:Restriction>
        </rdfs:subClassOf>
        <rdfs:subClassOf>
            <owl:Restriction>
                <owl:onProperty rdf:resource="https://w3id.org/netbeheer/referentiemodellen/IECCIM/TC57CIM/IEC61970/Base/Wires#RotatingMachine_ratedU"/>
                <owl:minQualifiedCardinality rdf:datatype="http://www.w3.org/2001/XMLSchema#nonNegativeInteger">0</owl:minQualifiedCardinality>
                <owl:onClass rdf:resource="https://w3id.org/netbeheer/referentiemodellen/IECCIM/TC57CIM/IEC61970/Base/Domain#Voltage"/>
            </owl:Restriction>
        </rdfs:subClassOf>
        <rdfs:subClassOf>
            <owl:Restriction>
                <owl:onProperty rdf:resource="https://w3id.org/netbeheer/referentiemodellen/IECCIM/TC57CIM/IEC61970/Base/Wires#RotatingMachine_HydroPump"/>
                <owl:qualifiedCardinality rdf:datatype="http://www.w3.org/2001/XMLSchema#nonNegativeInteger">1</owl:qualifiedCardinality>
                <owl:onClass rdf:resource="https://w3id.org/netbeheer/referentiemodellen/IECCIM/TC57CIM/IEC61970/Base/Wires#RotatingMachine"/>
            </owl:Restriction>
        </rdfs:subClassOf>
        <rdfs:subClassOf>
            <owl:Restriction>
                <owl:onProperty rdf:resource="https://w3id.org/netbeheer/referentiemodellen/IECCIM/TC57CIM/IEC61970/Base/Wires#RotatingMachine_p"/>
                <owl:maxQualifiedCardinality rdf:datatype="http://www.w3.org/2001/XMLSchema#nonNegativeInteger">1</owl:maxQualifiedCardinality>
                <owl:onClass rdf:resource="https://w3id.org/netbeheer/referentiemodellen/IECCIM/TC57CIM/IEC61970/Base/Domain#ActivePower"/>
            </owl:Restriction>
        </rdfs:subClassOf>
        <rdfs:subClassOf>
            <owl:Restriction>
                <owl:onProperty rdf:resource="https://w3id.org/netbeheer/referentiemodellen/IECCIM/TC57CIM/IEC61970/Base/Wires#RotatingMachine_q"/>
                <owl:maxQualifiedCardinality rdf:datatype="http://www.w3.org/2001/XMLSchema#nonNegativeInteger">1</owl:maxQualifiedCardinality>
                <owl:onClass rdf:resource="https://w3id.org/netbeheer/referentiemodellen/IECCIM/TC57CIM/IEC61970/Base/Domain#ReactivePower"/>
            </owl:Restriction>
        </rdfs:subClassOf>
        <rdfs:subClassOf>
            <owl:Restriction>
                <owl:onProperty rdf:resource="https://w3id.org/netbeheer/referentiemodellen/IECCIM/TC57CIM/IEC61970/Base/Wires#RotatingMachine_ratedS"/>
                <owl:maxQualifiedCardinality rdf:datatype="http://www.w3.org/2001/XMLSchema#nonNegativeInteger">1</owl:maxQualifiedCardinality>
                <owl:onClass rdf:resource="https://w3id.org/netbeheer/referentiemodellen/IECCIM/TC57CIM/IEC61970/Base/Domain#ApparentPower"/>
            </owl:Restriction>
        </rdfs:subClassOf>
        <rdfs:subClassOf>
            <owl:Restriction>
                <owl:onProperty rdf:resource="https://w3id.org/netbeheer/referentiemodellen/IECCIM/TC57CIM/IEC61970/Base/Wires#RotatingMachine_ratedU"/>
                <owl:maxQualifiedCardinality rdf:datatype="http://www.w3.org/2001/XMLSchema#nonNegativeInteger">1</owl:maxQualifiedCardinality>
                <owl:onClass rdf:resource="https://w3id.org/netbeheer/referentiemodellen/IECCIM/TC57CIM/IEC61970/Base/Domain#Voltage"/>
            </owl:Restriction>
        </rdfs:subClassOf>
        <rdfs:subClassOf>
            <owl:Restriction>
                <owl:onProperty rdf:resource="https://w3id.org/netbeheer/referentiemodellen/IECCIM/TC57CIM/IEC61970/Base/Wires#RotatingMachine_ratedPowerFactor"/>
                <owl:minQualifiedCardinality rdf:datatype="http://www.w3.org/2001/XMLSchema#nonNegativeInteger">0</owl:minQualifiedCardinality>
                <owl:onDataRange rdf:resource="http://www.w3.org/2001/XMLSchema#float"/>
            </owl:Restriction>
        </rdfs:subClassOf>
        <rdfs:subClassOf>
            <owl:Restriction>
                <owl:onProperty rdf:resource="https://w3id.org/netbeheer/referentiemodellen/IECCIM/TC57CIM/IEC61970/Base/Wires#RotatingMachine_ratedPowerFactor"/>
                <owl:maxQualifiedCardinality rdf:datatype="http://www.w3.org/2001/XMLSchema#nonNegativeInteger">1</owl:maxQualifiedCardinality>
                <owl:onDataRange rdf:resource="http://www.w3.org/2001/XMLSchema#float"/>
            </owl:Restriction>
        </rdfs:subClassOf>
        <rdfs:comment>A rotating machine which may be used as a generator or motor.</rdfs:comment>
    </owl:Class>
    


    <!-- https://w3id.org/netbeheer/referentiemodellen/IECCIM/TC57CIM/IEC61970/Base/Wires#Sectionaliser -->


    <owl:Class rdf:about="https://w3id.org/netbeheer/referentiemodellen/IECCIM/TC57CIM/IEC61970/Base/Wires#Sectionaliser">
        <rdfs:subClassOf rdf:resource="https://w3id.org/netbeheer/referentiemodellen/IECCIM/TC57CIM/IEC61970/Base/Wires#Switch"/>
        <rdfs:comment>Automatic switch that will lock open to isolate a faulted section. It may, or may not, have load breaking capability. Its primary purpose is to provide fault sectionalising at locations where the fault current is either too high, or too low, for proper coordination of fuses.
</rdfs:comment>
    </owl:Class>
    


    <!-- https://w3id.org/netbeheer/referentiemodellen/IECCIM/TC57CIM/IEC61970/Base/Wires#SeriesCompensator -->


    <owl:Class rdf:about="https://w3id.org/netbeheer/referentiemodellen/IECCIM/TC57CIM/IEC61970/Base/Wires#SeriesCompensator">
        <rdfs:subClassOf rdf:resource="https://w3id.org/netbeheer/referentiemodellen/IECCIM/TC57CIM/IEC61970/Base/Core#ConductingEquipment"/>
        <rdfs:subClassOf>
            <owl:Restriction>
                <owl:onProperty rdf:resource="https://w3id.org/netbeheer/referentiemodellen/IECCIM/TC57CIM/IEC61970/Base/Wires#SeriesCompensator_r"/>
                <owl:minQualifiedCardinality rdf:datatype="http://www.w3.org/2001/XMLSchema#nonNegativeInteger">0</owl:minQualifiedCardinality>
                <owl:onClass rdf:resource="https://w3id.org/netbeheer/referentiemodellen/IECCIM/TC57CIM/IEC61970/Base/Domain#Resistance"/>
            </owl:Restriction>
        </rdfs:subClassOf>
        <rdfs:subClassOf>
            <owl:Restriction>
                <owl:onProperty rdf:resource="https://w3id.org/netbeheer/referentiemodellen/IECCIM/TC57CIM/IEC61970/Base/Wires#SeriesCompensator_r0"/>
                <owl:minQualifiedCardinality rdf:datatype="http://www.w3.org/2001/XMLSchema#nonNegativeInteger">0</owl:minQualifiedCardinality>
                <owl:onClass rdf:resource="https://w3id.org/netbeheer/referentiemodellen/IECCIM/TC57CIM/IEC61970/Base/Domain#Resistance"/>
            </owl:Restriction>
        </rdfs:subClassOf>
        <rdfs:subClassOf>
            <owl:Restriction>
                <owl:onProperty rdf:resource="https://w3id.org/netbeheer/referentiemodellen/IECCIM/TC57CIM/IEC61970/Base/Wires#SeriesCompensator_varistorRatedCurrent"/>
                <owl:minQualifiedCardinality rdf:datatype="http://www.w3.org/2001/XMLSchema#nonNegativeInteger">0</owl:minQualifiedCardinality>
                <owl:onClass rdf:resource="https://w3id.org/netbeheer/referentiemodellen/IECCIM/TC57CIM/IEC61970/Base/Domain#CurrentFlow"/>
            </owl:Restriction>
        </rdfs:subClassOf>
        <rdfs:subClassOf>
            <owl:Restriction>
                <owl:onProperty rdf:resource="https://w3id.org/netbeheer/referentiemodellen/IECCIM/TC57CIM/IEC61970/Base/Wires#SeriesCompensator_varistorVoltageThreshold"/>
                <owl:minQualifiedCardinality rdf:datatype="http://www.w3.org/2001/XMLSchema#nonNegativeInteger">0</owl:minQualifiedCardinality>
                <owl:onClass rdf:resource="https://w3id.org/netbeheer/referentiemodellen/IECCIM/TC57CIM/IEC61970/Base/Domain#Voltage"/>
            </owl:Restriction>
        </rdfs:subClassOf>
        <rdfs:subClassOf>
            <owl:Restriction>
                <owl:onProperty rdf:resource="https://w3id.org/netbeheer/referentiemodellen/IECCIM/TC57CIM/IEC61970/Base/Wires#SeriesCompensator_x"/>
                <owl:minQualifiedCardinality rdf:datatype="http://www.w3.org/2001/XMLSchema#nonNegativeInteger">0</owl:minQualifiedCardinality>
                <owl:onClass rdf:resource="https://w3id.org/netbeheer/referentiemodellen/IECCIM/TC57CIM/IEC61970/Base/Domain#Reactance"/>
            </owl:Restriction>
        </rdfs:subClassOf>
        <rdfs:subClassOf>
            <owl:Restriction>
                <owl:onProperty rdf:resource="https://w3id.org/netbeheer/referentiemodellen/IECCIM/TC57CIM/IEC61970/Base/Wires#SeriesCompensator_x0"/>
                <owl:minQualifiedCardinality rdf:datatype="http://www.w3.org/2001/XMLSchema#nonNegativeInteger">0</owl:minQualifiedCardinality>
                <owl:onClass rdf:resource="https://w3id.org/netbeheer/referentiemodellen/IECCIM/TC57CIM/IEC61970/Base/Domain#Reactance"/>
            </owl:Restriction>
        </rdfs:subClassOf>
        <rdfs:subClassOf>
            <owl:Restriction>
                <owl:onProperty rdf:resource="https://w3id.org/netbeheer/referentiemodellen/IECCIM/TC57CIM/IEC61970/Base/Wires#SeriesCompensator_r"/>
                <owl:maxQualifiedCardinality rdf:datatype="http://www.w3.org/2001/XMLSchema#nonNegativeInteger">1</owl:maxQualifiedCardinality>
                <owl:onClass rdf:resource="https://w3id.org/netbeheer/referentiemodellen/IECCIM/TC57CIM/IEC61970/Base/Domain#Resistance"/>
            </owl:Restriction>
        </rdfs:subClassOf>
        <rdfs:subClassOf>
            <owl:Restriction>
                <owl:onProperty rdf:resource="https://w3id.org/netbeheer/referentiemodellen/IECCIM/TC57CIM/IEC61970/Base/Wires#SeriesCompensator_r0"/>
                <owl:maxQualifiedCardinality rdf:datatype="http://www.w3.org/2001/XMLSchema#nonNegativeInteger">1</owl:maxQualifiedCardinality>
                <owl:onClass rdf:resource="https://w3id.org/netbeheer/referentiemodellen/IECCIM/TC57CIM/IEC61970/Base/Domain#Resistance"/>
            </owl:Restriction>
        </rdfs:subClassOf>
        <rdfs:subClassOf>
            <owl:Restriction>
                <owl:onProperty rdf:resource="https://w3id.org/netbeheer/referentiemodellen/IECCIM/TC57CIM/IEC61970/Base/Wires#SeriesCompensator_varistorRatedCurrent"/>
                <owl:maxQualifiedCardinality rdf:datatype="http://www.w3.org/2001/XMLSchema#nonNegativeInteger">1</owl:maxQualifiedCardinality>
                <owl:onClass rdf:resource="https://w3id.org/netbeheer/referentiemodellen/IECCIM/TC57CIM/IEC61970/Base/Domain#CurrentFlow"/>
            </owl:Restriction>
        </rdfs:subClassOf>
        <rdfs:subClassOf>
            <owl:Restriction>
                <owl:onProperty rdf:resource="https://w3id.org/netbeheer/referentiemodellen/IECCIM/TC57CIM/IEC61970/Base/Wires#SeriesCompensator_varistorVoltageThreshold"/>
                <owl:maxQualifiedCardinality rdf:datatype="http://www.w3.org/2001/XMLSchema#nonNegativeInteger">1</owl:maxQualifiedCardinality>
                <owl:onClass rdf:resource="https://w3id.org/netbeheer/referentiemodellen/IECCIM/TC57CIM/IEC61970/Base/Domain#Voltage"/>
            </owl:Restriction>
        </rdfs:subClassOf>
        <rdfs:subClassOf>
            <owl:Restriction>
                <owl:onProperty rdf:resource="https://w3id.org/netbeheer/referentiemodellen/IECCIM/TC57CIM/IEC61970/Base/Wires#SeriesCompensator_x"/>
                <owl:maxQualifiedCardinality rdf:datatype="http://www.w3.org/2001/XMLSchema#nonNegativeInteger">1</owl:maxQualifiedCardinality>
                <owl:onClass rdf:resource="https://w3id.org/netbeheer/referentiemodellen/IECCIM/TC57CIM/IEC61970/Base/Domain#Reactance"/>
            </owl:Restriction>
        </rdfs:subClassOf>
        <rdfs:subClassOf>
            <owl:Restriction>
                <owl:onProperty rdf:resource="https://w3id.org/netbeheer/referentiemodellen/IECCIM/TC57CIM/IEC61970/Base/Wires#SeriesCompensator_x0"/>
                <owl:maxQualifiedCardinality rdf:datatype="http://www.w3.org/2001/XMLSchema#nonNegativeInteger">1</owl:maxQualifiedCardinality>
                <owl:onClass rdf:resource="https://w3id.org/netbeheer/referentiemodellen/IECCIM/TC57CIM/IEC61970/Base/Domain#Reactance"/>
            </owl:Restriction>
        </rdfs:subClassOf>
        <rdfs:subClassOf>
            <owl:Restriction>
                <owl:onProperty rdf:resource="https://w3id.org/netbeheer/referentiemodellen/IECCIM/TC57CIM/IEC61970/Base/Wires#SeriesCompensator_varistorPresent"/>
                <owl:minQualifiedCardinality rdf:datatype="http://www.w3.org/2001/XMLSchema#nonNegativeInteger">0</owl:minQualifiedCardinality>
                <owl:onDataRange rdf:resource="http://www.w3.org/2001/XMLSchema#boolean"/>
            </owl:Restriction>
        </rdfs:subClassOf>
        <rdfs:subClassOf>
            <owl:Restriction>
                <owl:onProperty rdf:resource="https://w3id.org/netbeheer/referentiemodellen/IECCIM/TC57CIM/IEC61970/Base/Wires#SeriesCompensator_varistorPresent"/>
                <owl:maxQualifiedCardinality rdf:datatype="http://www.w3.org/2001/XMLSchema#nonNegativeInteger">1</owl:maxQualifiedCardinality>
                <owl:onDataRange rdf:resource="http://www.w3.org/2001/XMLSchema#boolean"/>
            </owl:Restriction>
        </rdfs:subClassOf>
        <rdfs:comment>A Series Compensator is a series capacitor or reactor or an AC transmission line without charging susceptance.  It is a two terminal device.
</rdfs:comment>
    </owl:Class>
    


    <!-- https://w3id.org/netbeheer/referentiemodellen/IECCIM/TC57CIM/IEC61970/Base/Wires#ShuntCompensator -->


    <owl:Class rdf:about="https://w3id.org/netbeheer/referentiemodellen/IECCIM/TC57CIM/IEC61970/Base/Wires#ShuntCompensator">
        <rdfs:subClassOf rdf:resource="https://w3id.org/netbeheer/referentiemodellen/IECCIM/TC57CIM/IEC61970/Base/Wires#RegulatingCondEq"/>
        <rdfs:subClassOf>
            <owl:Restriction>
                <owl:onProperty rdf:resource="https://w3id.org/netbeheer/referentiemodellen/IECCIM/TC57CIM/IEC61970/Base/Wires#ShuntCompensator_aVRDelay"/>
                <owl:minQualifiedCardinality rdf:datatype="http://www.w3.org/2001/XMLSchema#nonNegativeInteger">0</owl:minQualifiedCardinality>
                <owl:onClass rdf:resource="https://w3id.org/netbeheer/referentiemodellen/IECCIM/TC57CIM/IEC61970/Base/Domain#Seconds"/>
            </owl:Restriction>
        </rdfs:subClassOf>
        <rdfs:subClassOf>
            <owl:Restriction>
                <owl:onProperty rdf:resource="https://w3id.org/netbeheer/referentiemodellen/IECCIM/TC57CIM/IEC61970/Base/Wires#ShuntCompensator_nomU"/>
                <owl:minQualifiedCardinality rdf:datatype="http://www.w3.org/2001/XMLSchema#nonNegativeInteger">0</owl:minQualifiedCardinality>
                <owl:onClass rdf:resource="https://w3id.org/netbeheer/referentiemodellen/IECCIM/TC57CIM/IEC61970/Base/Domain#Voltage"/>
            </owl:Restriction>
        </rdfs:subClassOf>
        <rdfs:subClassOf>
            <owl:Restriction>
                <owl:onProperty rdf:resource="https://w3id.org/netbeheer/referentiemodellen/IECCIM/TC57CIM/IEC61970/Base/Wires#ShuntCompensator_voltageSensitivity"/>
                <owl:minQualifiedCardinality rdf:datatype="http://www.w3.org/2001/XMLSchema#nonNegativeInteger">0</owl:minQualifiedCardinality>
                <owl:onClass rdf:resource="https://w3id.org/netbeheer/referentiemodellen/IECCIM/TC57CIM/IEC61970/Base/Domain#VoltagePerReactivePower"/>
            </owl:Restriction>
        </rdfs:subClassOf>
        <rdfs:subClassOf>
            <owl:Restriction>
                <owl:onProperty rdf:resource="https://w3id.org/netbeheer/referentiemodellen/IECCIM/TC57CIM/IEC61970/Base/Wires#ShuntCompensator_ShuntCompensatorPhase"/>
                <owl:qualifiedCardinality rdf:datatype="http://www.w3.org/2001/XMLSchema#nonNegativeInteger">1</owl:qualifiedCardinality>
                <owl:onClass rdf:resource="https://w3id.org/netbeheer/referentiemodellen/IECCIM/TC57CIM/IEC61970/Base/Wires#ShuntCompensator"/>
            </owl:Restriction>
        </rdfs:subClassOf>
        <rdfs:subClassOf>
            <owl:Restriction>
                <owl:onProperty rdf:resource="https://w3id.org/netbeheer/referentiemodellen/IECCIM/TC57CIM/IEC61970/Base/Wires#ShuntCompensator_SvShuntCompensatorSections"/>
                <owl:qualifiedCardinality rdf:datatype="http://www.w3.org/2001/XMLSchema#nonNegativeInteger">1</owl:qualifiedCardinality>
                <owl:onClass rdf:resource="https://w3id.org/netbeheer/referentiemodellen/IECCIM/TC57CIM/IEC61970/Base/Wires#ShuntCompensator"/>
            </owl:Restriction>
        </rdfs:subClassOf>
        <rdfs:subClassOf>
            <owl:Restriction>
                <owl:onProperty rdf:resource="https://w3id.org/netbeheer/referentiemodellen/IECCIM/TC57CIM/IEC61970/Base/Wires#ShuntCompensator_aVRDelay"/>
                <owl:maxQualifiedCardinality rdf:datatype="http://www.w3.org/2001/XMLSchema#nonNegativeInteger">1</owl:maxQualifiedCardinality>
                <owl:onClass rdf:resource="https://w3id.org/netbeheer/referentiemodellen/IECCIM/TC57CIM/IEC61970/Base/Domain#Seconds"/>
            </owl:Restriction>
        </rdfs:subClassOf>
        <rdfs:subClassOf>
            <owl:Restriction>
                <owl:onProperty rdf:resource="https://w3id.org/netbeheer/referentiemodellen/IECCIM/TC57CIM/IEC61970/Base/Wires#ShuntCompensator_nomU"/>
                <owl:maxQualifiedCardinality rdf:datatype="http://www.w3.org/2001/XMLSchema#nonNegativeInteger">1</owl:maxQualifiedCardinality>
                <owl:onClass rdf:resource="https://w3id.org/netbeheer/referentiemodellen/IECCIM/TC57CIM/IEC61970/Base/Domain#Voltage"/>
            </owl:Restriction>
        </rdfs:subClassOf>
        <rdfs:subClassOf>
            <owl:Restriction>
                <owl:onProperty rdf:resource="https://w3id.org/netbeheer/referentiemodellen/IECCIM/TC57CIM/IEC61970/Base/Wires#ShuntCompensator_voltageSensitivity"/>
                <owl:maxQualifiedCardinality rdf:datatype="http://www.w3.org/2001/XMLSchema#nonNegativeInteger">1</owl:maxQualifiedCardinality>
                <owl:onClass rdf:resource="https://w3id.org/netbeheer/referentiemodellen/IECCIM/TC57CIM/IEC61970/Base/Domain#VoltagePerReactivePower"/>
            </owl:Restriction>
        </rdfs:subClassOf>
        <rdfs:subClassOf>
            <owl:Restriction>
                <owl:onProperty rdf:resource="https://w3id.org/netbeheer/referentiemodellen/IECCIM/TC57CIM/IEC61970/Base/Wires#ShuntCompensator_grounded"/>
                <owl:minQualifiedCardinality rdf:datatype="http://www.w3.org/2001/XMLSchema#nonNegativeInteger">0</owl:minQualifiedCardinality>
                <owl:onDataRange rdf:resource="http://www.w3.org/2001/XMLSchema#boolean"/>
            </owl:Restriction>
        </rdfs:subClassOf>
        <rdfs:subClassOf>
            <owl:Restriction>
                <owl:onProperty rdf:resource="https://w3id.org/netbeheer/referentiemodellen/IECCIM/TC57CIM/IEC61970/Base/Wires#ShuntCompensator_maximumSections"/>
                <owl:minQualifiedCardinality rdf:datatype="http://www.w3.org/2001/XMLSchema#nonNegativeInteger">0</owl:minQualifiedCardinality>
                <owl:onDataRange rdf:resource="http://www.w3.org/2001/XMLSchema#nonNegativeInteger"/>
            </owl:Restriction>
        </rdfs:subClassOf>
        <rdfs:subClassOf>
            <owl:Restriction>
                <owl:onProperty rdf:resource="https://w3id.org/netbeheer/referentiemodellen/IECCIM/TC57CIM/IEC61970/Base/Wires#ShuntCompensator_normalSections"/>
                <owl:minQualifiedCardinality rdf:datatype="http://www.w3.org/2001/XMLSchema#nonNegativeInteger">0</owl:minQualifiedCardinality>
                <owl:onDataRange rdf:resource="http://www.w3.org/2001/XMLSchema#nonNegativeInteger"/>
            </owl:Restriction>
        </rdfs:subClassOf>
        <rdfs:subClassOf>
            <owl:Restriction>
                <owl:onProperty rdf:resource="https://w3id.org/netbeheer/referentiemodellen/IECCIM/TC57CIM/IEC61970/Base/Wires#ShuntCompensator_phaseConnection"/>
                <owl:minQualifiedCardinality rdf:datatype="http://www.w3.org/2001/XMLSchema#nonNegativeInteger">0</owl:minQualifiedCardinality>
                <owl:onDataRange rdf:resource="https://w3id.org/netbeheer/referentiemodellen/IECCIM/TC57CIM/IEC61970/Base/Wires#PhaseShuntConnectionKind"/>
            </owl:Restriction>
        </rdfs:subClassOf>
        <rdfs:subClassOf>
            <owl:Restriction>
                <owl:onProperty rdf:resource="https://w3id.org/netbeheer/referentiemodellen/IECCIM/TC57CIM/IEC61970/Base/Wires#ShuntCompensator_sections"/>
                <owl:minQualifiedCardinality rdf:datatype="http://www.w3.org/2001/XMLSchema#nonNegativeInteger">0</owl:minQualifiedCardinality>
                <owl:onDataRange rdf:resource="http://www.w3.org/2001/XMLSchema#float"/>
            </owl:Restriction>
        </rdfs:subClassOf>
        <rdfs:subClassOf>
            <owl:Restriction>
                <owl:onProperty rdf:resource="https://w3id.org/netbeheer/referentiemodellen/IECCIM/TC57CIM/IEC61970/Base/Wires#ShuntCompensator_switchOnCount"/>
                <owl:minQualifiedCardinality rdf:datatype="http://www.w3.org/2001/XMLSchema#nonNegativeInteger">0</owl:minQualifiedCardinality>
                <owl:onDataRange rdf:resource="http://www.w3.org/2001/XMLSchema#nonNegativeInteger"/>
            </owl:Restriction>
        </rdfs:subClassOf>
        <rdfs:subClassOf>
            <owl:Restriction>
                <owl:onProperty rdf:resource="https://w3id.org/netbeheer/referentiemodellen/IECCIM/TC57CIM/IEC61970/Base/Wires#ShuntCompensator_switchOnDate"/>
                <owl:minQualifiedCardinality rdf:datatype="http://www.w3.org/2001/XMLSchema#nonNegativeInteger">0</owl:minQualifiedCardinality>
                <owl:onDataRange rdf:resource="http://www.w3.org/2001/XMLSchema#dateTime"/>
            </owl:Restriction>
        </rdfs:subClassOf>
        <rdfs:subClassOf>
            <owl:Restriction>
                <owl:onProperty rdf:resource="https://w3id.org/netbeheer/referentiemodellen/IECCIM/TC57CIM/IEC61970/Base/Wires#ShuntCompensator_grounded"/>
                <owl:maxQualifiedCardinality rdf:datatype="http://www.w3.org/2001/XMLSchema#nonNegativeInteger">1</owl:maxQualifiedCardinality>
                <owl:onDataRange rdf:resource="http://www.w3.org/2001/XMLSchema#boolean"/>
            </owl:Restriction>
        </rdfs:subClassOf>
        <rdfs:subClassOf>
            <owl:Restriction>
                <owl:onProperty rdf:resource="https://w3id.org/netbeheer/referentiemodellen/IECCIM/TC57CIM/IEC61970/Base/Wires#ShuntCompensator_maximumSections"/>
                <owl:maxQualifiedCardinality rdf:datatype="http://www.w3.org/2001/XMLSchema#nonNegativeInteger">1</owl:maxQualifiedCardinality>
                <owl:onDataRange rdf:resource="http://www.w3.org/2001/XMLSchema#nonNegativeInteger"/>
            </owl:Restriction>
        </rdfs:subClassOf>
        <rdfs:subClassOf>
            <owl:Restriction>
                <owl:onProperty rdf:resource="https://w3id.org/netbeheer/referentiemodellen/IECCIM/TC57CIM/IEC61970/Base/Wires#ShuntCompensator_normalSections"/>
                <owl:maxQualifiedCardinality rdf:datatype="http://www.w3.org/2001/XMLSchema#nonNegativeInteger">1</owl:maxQualifiedCardinality>
                <owl:onDataRange rdf:resource="http://www.w3.org/2001/XMLSchema#nonNegativeInteger"/>
            </owl:Restriction>
        </rdfs:subClassOf>
        <rdfs:subClassOf>
            <owl:Restriction>
                <owl:onProperty rdf:resource="https://w3id.org/netbeheer/referentiemodellen/IECCIM/TC57CIM/IEC61970/Base/Wires#ShuntCompensator_phaseConnection"/>
                <owl:maxQualifiedCardinality rdf:datatype="http://www.w3.org/2001/XMLSchema#nonNegativeInteger">1</owl:maxQualifiedCardinality>
                <owl:onDataRange rdf:resource="https://w3id.org/netbeheer/referentiemodellen/IECCIM/TC57CIM/IEC61970/Base/Wires#PhaseShuntConnectionKind"/>
            </owl:Restriction>
        </rdfs:subClassOf>
        <rdfs:subClassOf>
            <owl:Restriction>
                <owl:onProperty rdf:resource="https://w3id.org/netbeheer/referentiemodellen/IECCIM/TC57CIM/IEC61970/Base/Wires#ShuntCompensator_sections"/>
                <owl:maxQualifiedCardinality rdf:datatype="http://www.w3.org/2001/XMLSchema#nonNegativeInteger">1</owl:maxQualifiedCardinality>
                <owl:onDataRange rdf:resource="http://www.w3.org/2001/XMLSchema#float"/>
            </owl:Restriction>
        </rdfs:subClassOf>
        <rdfs:subClassOf>
            <owl:Restriction>
                <owl:onProperty rdf:resource="https://w3id.org/netbeheer/referentiemodellen/IECCIM/TC57CIM/IEC61970/Base/Wires#ShuntCompensator_switchOnCount"/>
                <owl:maxQualifiedCardinality rdf:datatype="http://www.w3.org/2001/XMLSchema#nonNegativeInteger">1</owl:maxQualifiedCardinality>
                <owl:onDataRange rdf:resource="http://www.w3.org/2001/XMLSchema#nonNegativeInteger"/>
            </owl:Restriction>
        </rdfs:subClassOf>
        <rdfs:subClassOf>
            <owl:Restriction>
                <owl:onProperty rdf:resource="https://w3id.org/netbeheer/referentiemodellen/IECCIM/TC57CIM/IEC61970/Base/Wires#ShuntCompensator_switchOnDate"/>
                <owl:maxQualifiedCardinality rdf:datatype="http://www.w3.org/2001/XMLSchema#nonNegativeInteger">1</owl:maxQualifiedCardinality>
                <owl:onDataRange rdf:resource="http://www.w3.org/2001/XMLSchema#dateTime"/>
            </owl:Restriction>
        </rdfs:subClassOf>
        <rdfs:comment>A shunt capacitor or reactor or switchable bank of shunt capacitors or reactors. A section of a shunt compensator is an individual capacitor or reactor.  A negative value for reactivePerSection indicates that the compensator is a reactor. ShuntCompensator is a single terminal device.  Ground is implied.</rdfs:comment>
    </owl:Class>
    


    <!-- https://w3id.org/netbeheer/referentiemodellen/IECCIM/TC57CIM/IEC61970/Base/Wires#ShuntCompensatorPhase -->


    <owl:Class rdf:about="https://w3id.org/netbeheer/referentiemodellen/IECCIM/TC57CIM/IEC61970/Base/Wires#ShuntCompensatorPhase">
        <rdfs:subClassOf rdf:resource="https://w3id.org/netbeheer/referentiemodellen/IECCIM/TC57CIM/IEC61970/Base/Core#PowerSystemResource"/>
        <rdfs:subClassOf>
            <owl:Restriction>
                <owl:onProperty rdf:resource="https://w3id.org/netbeheer/referentiemodellen/IECCIM/TC57CIM/IEC61970/Base/Wires#ShuntCompensatorPhase_ShuntCompensator"/>
                <owl:minQualifiedCardinality rdf:datatype="http://www.w3.org/2001/XMLSchema#nonNegativeInteger">0</owl:minQualifiedCardinality>
                <owl:onClass rdf:resource="https://w3id.org/netbeheer/referentiemodellen/IECCIM/TC57CIM/IEC61970/Base/Wires#ShuntCompensatorPhase"/>
            </owl:Restriction>
        </rdfs:subClassOf>
        <rdfs:subClassOf>
            <owl:Restriction>
                <owl:onProperty rdf:resource="https://w3id.org/netbeheer/referentiemodellen/IECCIM/TC57CIM/IEC61970/Base/Wires#ShuntCompensatorPhase_maximumSections"/>
                <owl:minQualifiedCardinality rdf:datatype="http://www.w3.org/2001/XMLSchema#nonNegativeInteger">0</owl:minQualifiedCardinality>
                <owl:onDataRange rdf:resource="http://www.w3.org/2001/XMLSchema#nonNegativeInteger"/>
            </owl:Restriction>
        </rdfs:subClassOf>
        <rdfs:subClassOf>
            <owl:Restriction>
                <owl:onProperty rdf:resource="https://w3id.org/netbeheer/referentiemodellen/IECCIM/TC57CIM/IEC61970/Base/Wires#ShuntCompensatorPhase_normalSections"/>
                <owl:minQualifiedCardinality rdf:datatype="http://www.w3.org/2001/XMLSchema#nonNegativeInteger">0</owl:minQualifiedCardinality>
                <owl:onDataRange rdf:resource="http://www.w3.org/2001/XMLSchema#nonNegativeInteger"/>
            </owl:Restriction>
        </rdfs:subClassOf>
        <rdfs:subClassOf>
            <owl:Restriction>
                <owl:onProperty rdf:resource="https://w3id.org/netbeheer/referentiemodellen/IECCIM/TC57CIM/IEC61970/Base/Wires#ShuntCompensatorPhase_phase"/>
                <owl:minQualifiedCardinality rdf:datatype="http://www.w3.org/2001/XMLSchema#nonNegativeInteger">0</owl:minQualifiedCardinality>
                <owl:onDataRange rdf:resource="https://w3id.org/netbeheer/referentiemodellen/IECCIM/TC57CIM/IEC61970/Base/Wires#SinglePhaseKind"/>
            </owl:Restriction>
        </rdfs:subClassOf>
        <rdfs:subClassOf>
            <owl:Restriction>
                <owl:onProperty rdf:resource="https://w3id.org/netbeheer/referentiemodellen/IECCIM/TC57CIM/IEC61970/Base/Wires#ShuntCompensatorPhase_maximumSections"/>
                <owl:maxQualifiedCardinality rdf:datatype="http://www.w3.org/2001/XMLSchema#nonNegativeInteger">1</owl:maxQualifiedCardinality>
                <owl:onDataRange rdf:resource="http://www.w3.org/2001/XMLSchema#nonNegativeInteger"/>
            </owl:Restriction>
        </rdfs:subClassOf>
        <rdfs:subClassOf>
            <owl:Restriction>
                <owl:onProperty rdf:resource="https://w3id.org/netbeheer/referentiemodellen/IECCIM/TC57CIM/IEC61970/Base/Wires#ShuntCompensatorPhase_normalSections"/>
                <owl:maxQualifiedCardinality rdf:datatype="http://www.w3.org/2001/XMLSchema#nonNegativeInteger">1</owl:maxQualifiedCardinality>
                <owl:onDataRange rdf:resource="http://www.w3.org/2001/XMLSchema#nonNegativeInteger"/>
            </owl:Restriction>
        </rdfs:subClassOf>
        <rdfs:subClassOf>
            <owl:Restriction>
                <owl:onProperty rdf:resource="https://w3id.org/netbeheer/referentiemodellen/IECCIM/TC57CIM/IEC61970/Base/Wires#ShuntCompensatorPhase_phase"/>
                <owl:maxQualifiedCardinality rdf:datatype="http://www.w3.org/2001/XMLSchema#nonNegativeInteger">1</owl:maxQualifiedCardinality>
                <owl:onDataRange rdf:resource="https://w3id.org/netbeheer/referentiemodellen/IECCIM/TC57CIM/IEC61970/Base/Wires#SinglePhaseKind"/>
            </owl:Restriction>
        </rdfs:subClassOf>
        <rdfs:comment>Single phase of a multi-phase shunt compensator when its attributes might be different per phase.</rdfs:comment>
    </owl:Class>
    


    <!-- https://w3id.org/netbeheer/referentiemodellen/IECCIM/TC57CIM/IEC61970/Base/Wires#StaticVarCompensator -->


    <owl:Class rdf:about="https://w3id.org/netbeheer/referentiemodellen/IECCIM/TC57CIM/IEC61970/Base/Wires#StaticVarCompensator">
        <rdfs:subClassOf rdf:resource="https://w3id.org/netbeheer/referentiemodellen/IECCIM/TC57CIM/IEC61970/Base/Wires#RegulatingCondEq"/>
        <rdfs:subClassOf>
            <owl:Restriction>
                <owl:onProperty rdf:resource="https://w3id.org/netbeheer/referentiemodellen/IECCIM/TC57CIM/IEC61970/Base/Wires#StaticVarCompensator_capacitiveRating"/>
                <owl:minQualifiedCardinality rdf:datatype="http://www.w3.org/2001/XMLSchema#nonNegativeInteger">0</owl:minQualifiedCardinality>
                <owl:onClass rdf:resource="https://w3id.org/netbeheer/referentiemodellen/IECCIM/TC57CIM/IEC61970/Base/Domain#Reactance"/>
            </owl:Restriction>
        </rdfs:subClassOf>
        <rdfs:subClassOf>
            <owl:Restriction>
                <owl:onProperty rdf:resource="https://w3id.org/netbeheer/referentiemodellen/IECCIM/TC57CIM/IEC61970/Base/Wires#StaticVarCompensator_inductiveRating"/>
                <owl:minQualifiedCardinality rdf:datatype="http://www.w3.org/2001/XMLSchema#nonNegativeInteger">0</owl:minQualifiedCardinality>
                <owl:onClass rdf:resource="https://w3id.org/netbeheer/referentiemodellen/IECCIM/TC57CIM/IEC61970/Base/Domain#Reactance"/>
            </owl:Restriction>
        </rdfs:subClassOf>
        <rdfs:subClassOf>
            <owl:Restriction>
                <owl:onProperty rdf:resource="https://w3id.org/netbeheer/referentiemodellen/IECCIM/TC57CIM/IEC61970/Base/Wires#StaticVarCompensator_q"/>
                <owl:minQualifiedCardinality rdf:datatype="http://www.w3.org/2001/XMLSchema#nonNegativeInteger">0</owl:minQualifiedCardinality>
                <owl:onClass rdf:resource="https://w3id.org/netbeheer/referentiemodellen/IECCIM/TC57CIM/IEC61970/Base/Domain#ReactivePower"/>
            </owl:Restriction>
        </rdfs:subClassOf>
        <rdfs:subClassOf>
            <owl:Restriction>
                <owl:onProperty rdf:resource="https://w3id.org/netbeheer/referentiemodellen/IECCIM/TC57CIM/IEC61970/Base/Wires#StaticVarCompensator_slope"/>
                <owl:minQualifiedCardinality rdf:datatype="http://www.w3.org/2001/XMLSchema#nonNegativeInteger">0</owl:minQualifiedCardinality>
                <owl:onClass rdf:resource="https://w3id.org/netbeheer/referentiemodellen/IECCIM/TC57CIM/IEC61970/Base/Domain#VoltagePerReactivePower"/>
            </owl:Restriction>
        </rdfs:subClassOf>
        <rdfs:subClassOf>
            <owl:Restriction>
                <owl:onProperty rdf:resource="https://w3id.org/netbeheer/referentiemodellen/IECCIM/TC57CIM/IEC61970/Base/Wires#StaticVarCompensator_voltageSetPoint"/>
                <owl:minQualifiedCardinality rdf:datatype="http://www.w3.org/2001/XMLSchema#nonNegativeInteger">0</owl:minQualifiedCardinality>
                <owl:onClass rdf:resource="https://w3id.org/netbeheer/referentiemodellen/IECCIM/TC57CIM/IEC61970/Base/Domain#Voltage"/>
            </owl:Restriction>
        </rdfs:subClassOf>
        <rdfs:subClassOf>
            <owl:Restriction>
                <owl:onProperty rdf:resource="https://w3id.org/netbeheer/referentiemodellen/IECCIM/TC57CIM/IEC61970/Base/Wires#StaticVarCompensator_capacitiveRating"/>
                <owl:maxQualifiedCardinality rdf:datatype="http://www.w3.org/2001/XMLSchema#nonNegativeInteger">1</owl:maxQualifiedCardinality>
                <owl:onClass rdf:resource="https://w3id.org/netbeheer/referentiemodellen/IECCIM/TC57CIM/IEC61970/Base/Domain#Reactance"/>
            </owl:Restriction>
        </rdfs:subClassOf>
        <rdfs:subClassOf>
            <owl:Restriction>
                <owl:onProperty rdf:resource="https://w3id.org/netbeheer/referentiemodellen/IECCIM/TC57CIM/IEC61970/Base/Wires#StaticVarCompensator_inductiveRating"/>
                <owl:maxQualifiedCardinality rdf:datatype="http://www.w3.org/2001/XMLSchema#nonNegativeInteger">1</owl:maxQualifiedCardinality>
                <owl:onClass rdf:resource="https://w3id.org/netbeheer/referentiemodellen/IECCIM/TC57CIM/IEC61970/Base/Domain#Reactance"/>
            </owl:Restriction>
        </rdfs:subClassOf>
        <rdfs:subClassOf>
            <owl:Restriction>
                <owl:onProperty rdf:resource="https://w3id.org/netbeheer/referentiemodellen/IECCIM/TC57CIM/IEC61970/Base/Wires#StaticVarCompensator_q"/>
                <owl:maxQualifiedCardinality rdf:datatype="http://www.w3.org/2001/XMLSchema#nonNegativeInteger">1</owl:maxQualifiedCardinality>
                <owl:onClass rdf:resource="https://w3id.org/netbeheer/referentiemodellen/IECCIM/TC57CIM/IEC61970/Base/Domain#ReactivePower"/>
            </owl:Restriction>
        </rdfs:subClassOf>
        <rdfs:subClassOf>
            <owl:Restriction>
                <owl:onProperty rdf:resource="https://w3id.org/netbeheer/referentiemodellen/IECCIM/TC57CIM/IEC61970/Base/Wires#StaticVarCompensator_slope"/>
                <owl:maxQualifiedCardinality rdf:datatype="http://www.w3.org/2001/XMLSchema#nonNegativeInteger">1</owl:maxQualifiedCardinality>
                <owl:onClass rdf:resource="https://w3id.org/netbeheer/referentiemodellen/IECCIM/TC57CIM/IEC61970/Base/Domain#VoltagePerReactivePower"/>
            </owl:Restriction>
        </rdfs:subClassOf>
        <rdfs:subClassOf>
            <owl:Restriction>
                <owl:onProperty rdf:resource="https://w3id.org/netbeheer/referentiemodellen/IECCIM/TC57CIM/IEC61970/Base/Wires#StaticVarCompensator_voltageSetPoint"/>
                <owl:maxQualifiedCardinality rdf:datatype="http://www.w3.org/2001/XMLSchema#nonNegativeInteger">1</owl:maxQualifiedCardinality>
                <owl:onClass rdf:resource="https://w3id.org/netbeheer/referentiemodellen/IECCIM/TC57CIM/IEC61970/Base/Domain#Voltage"/>
            </owl:Restriction>
        </rdfs:subClassOf>
        <rdfs:subClassOf>
            <owl:Restriction>
                <owl:onProperty rdf:resource="https://w3id.org/netbeheer/referentiemodellen/IECCIM/TC57CIM/IEC61970/Base/Wires#StaticVarCompensator_sVCControlMode"/>
                <owl:minQualifiedCardinality rdf:datatype="http://www.w3.org/2001/XMLSchema#nonNegativeInteger">0</owl:minQualifiedCardinality>
                <owl:onDataRange rdf:resource="https://w3id.org/netbeheer/referentiemodellen/IECCIM/TC57CIM/IEC61970/Base/Wires#SVCControlMode"/>
            </owl:Restriction>
        </rdfs:subClassOf>
        <rdfs:subClassOf>
            <owl:Restriction>
                <owl:onProperty rdf:resource="https://w3id.org/netbeheer/referentiemodellen/IECCIM/TC57CIM/IEC61970/Base/Wires#StaticVarCompensator_sVCControlMode"/>
                <owl:maxQualifiedCardinality rdf:datatype="http://www.w3.org/2001/XMLSchema#nonNegativeInteger">1</owl:maxQualifiedCardinality>
                <owl:onDataRange rdf:resource="https://w3id.org/netbeheer/referentiemodellen/IECCIM/TC57CIM/IEC61970/Base/Wires#SVCControlMode"/>
            </owl:Restriction>
        </rdfs:subClassOf>
        <rdfs:comment>A facility for providing variable and controllable shunt reactive power. The SVC typically consists of a stepdown transformer, filter, thyristor-controlled reactor, and thyristor-switched capacitor arms.

The SVC may operate in fixed MVar output mode or in voltage control mode. When in voltage control mode, the output of the SVC will be proportional to the deviation of voltage at the controlled bus from the voltage setpoint.  The SVC characteristic slope defines the proportion.  If the voltage at the controlled bus is equal to the voltage setpoint, the SVC MVar output is zero.</rdfs:comment>
    </owl:Class>
    


    <!-- https://w3id.org/netbeheer/referentiemodellen/IECCIM/TC57CIM/IEC61970/Base/Wires#Switch -->


    <owl:Class rdf:about="https://w3id.org/netbeheer/referentiemodellen/IECCIM/TC57CIM/IEC61970/Base/Wires#Switch">
        <rdfs:subClassOf rdf:resource="https://w3id.org/netbeheer/referentiemodellen/IECCIM/TC57CIM/IEC61970/Base/Core#ConductingEquipment"/>
        <rdfs:subClassOf>
            <owl:Restriction>
                <owl:onProperty rdf:resource="https://w3id.org/netbeheer/referentiemodellen/IECCIM/TC57CIM/IEC61970/Base/Wires#Switch_CompositeSwitch"/>
                <owl:minQualifiedCardinality rdf:datatype="http://www.w3.org/2001/XMLSchema#nonNegativeInteger">0</owl:minQualifiedCardinality>
                <owl:onClass rdf:resource="https://w3id.org/netbeheer/referentiemodellen/IECCIM/TC57CIM/IEC61970/Base/Wires#Switch"/>
            </owl:Restriction>
        </rdfs:subClassOf>
        <rdfs:subClassOf>
            <owl:Restriction>
                <owl:onProperty rdf:resource="https://w3id.org/netbeheer/referentiemodellen/IECCIM/TC57CIM/IEC61970/Base/Wires#Switch_ConnectDisconnectFunctions"/>
                <owl:minQualifiedCardinality rdf:datatype="http://www.w3.org/2001/XMLSchema#nonNegativeInteger">0</owl:minQualifiedCardinality>
                <owl:onClass rdf:resource="https://w3id.org/netbeheer/referentiemodellen/IECCIM/TC57CIM/IEC61970/Base/Wires#Switch"/>
            </owl:Restriction>
        </rdfs:subClassOf>
        <rdfs:subClassOf>
            <owl:Restriction>
                <owl:onProperty rdf:resource="https://w3id.org/netbeheer/referentiemodellen/IECCIM/TC57CIM/IEC61970/Base/Wires#Switch_Outage"/>
                <owl:minQualifiedCardinality rdf:datatype="http://www.w3.org/2001/XMLSchema#nonNegativeInteger">0</owl:minQualifiedCardinality>
                <owl:onClass rdf:resource="https://w3id.org/netbeheer/referentiemodellen/IECCIM/TC57CIM/IEC61970/Base/Wires#Switch"/>
            </owl:Restriction>
        </rdfs:subClassOf>
        <rdfs:subClassOf>
            <owl:Restriction>
                <owl:onProperty rdf:resource="https://w3id.org/netbeheer/referentiemodellen/IECCIM/TC57CIM/IEC61970/Base/Wires#Switch_SwitchAction"/>
                <owl:minQualifiedCardinality rdf:datatype="http://www.w3.org/2001/XMLSchema#nonNegativeInteger">0</owl:minQualifiedCardinality>
                <owl:onClass rdf:resource="https://w3id.org/netbeheer/referentiemodellen/IECCIM/TC57CIM/IEC61970/Base/Wires#Switch"/>
            </owl:Restriction>
        </rdfs:subClassOf>
        <rdfs:subClassOf>
            <owl:Restriction>
                <owl:onProperty rdf:resource="https://w3id.org/netbeheer/referentiemodellen/IECCIM/TC57CIM/IEC61970/Base/Wires#Switch_ratedCurrent"/>
                <owl:minQualifiedCardinality rdf:datatype="http://www.w3.org/2001/XMLSchema#nonNegativeInteger">0</owl:minQualifiedCardinality>
                <owl:onClass rdf:resource="https://w3id.org/netbeheer/referentiemodellen/IECCIM/TC57CIM/IEC61970/Base/Domain#CurrentFlow"/>
            </owl:Restriction>
        </rdfs:subClassOf>
        <rdfs:subClassOf>
            <owl:Restriction>
                <owl:onProperty rdf:resource="https://w3id.org/netbeheer/referentiemodellen/IECCIM/TC57CIM/IEC61970/Base/Wires#Switch_SwitchPhase"/>
                <owl:qualifiedCardinality rdf:datatype="http://www.w3.org/2001/XMLSchema#nonNegativeInteger">1</owl:qualifiedCardinality>
                <owl:onClass rdf:resource="https://w3id.org/netbeheer/referentiemodellen/IECCIM/TC57CIM/IEC61970/Base/Wires#Switch"/>
            </owl:Restriction>
        </rdfs:subClassOf>
        <rdfs:subClassOf>
            <owl:Restriction>
                <owl:onProperty rdf:resource="https://w3id.org/netbeheer/referentiemodellen/IECCIM/TC57CIM/IEC61970/Base/Wires#Switch_SwitchSchedules"/>
                <owl:qualifiedCardinality rdf:datatype="http://www.w3.org/2001/XMLSchema#nonNegativeInteger">1</owl:qualifiedCardinality>
                <owl:onClass rdf:resource="https://w3id.org/netbeheer/referentiemodellen/IECCIM/TC57CIM/IEC61970/Base/Wires#Switch"/>
            </owl:Restriction>
        </rdfs:subClassOf>
        <rdfs:subClassOf>
            <owl:Restriction>
                <owl:onProperty rdf:resource="https://w3id.org/netbeheer/referentiemodellen/IECCIM/TC57CIM/IEC61970/Base/Wires#Switch_SwitchAction"/>
                <owl:maxQualifiedCardinality rdf:datatype="http://www.w3.org/2001/XMLSchema#nonNegativeInteger">1</owl:maxQualifiedCardinality>
                <owl:onClass rdf:resource="https://w3id.org/netbeheer/referentiemodellen/IECCIM/TC57CIM/IEC61970/Base/Wires#Switch"/>
            </owl:Restriction>
        </rdfs:subClassOf>
        <rdfs:subClassOf>
            <owl:Restriction>
                <owl:onProperty rdf:resource="https://w3id.org/netbeheer/referentiemodellen/IECCIM/TC57CIM/IEC61970/Base/Wires#Switch_ratedCurrent"/>
                <owl:maxQualifiedCardinality rdf:datatype="http://www.w3.org/2001/XMLSchema#nonNegativeInteger">1</owl:maxQualifiedCardinality>
                <owl:onClass rdf:resource="https://w3id.org/netbeheer/referentiemodellen/IECCIM/TC57CIM/IEC61970/Base/Domain#CurrentFlow"/>
            </owl:Restriction>
        </rdfs:subClassOf>
        <rdfs:subClassOf>
            <owl:Restriction>
                <owl:onProperty rdf:resource="https://w3id.org/netbeheer/referentiemodellen/IECCIM/TC57CIM/IEC61970/Base/Wires#Switch_normalOpen"/>
                <owl:minQualifiedCardinality rdf:datatype="http://www.w3.org/2001/XMLSchema#nonNegativeInteger">0</owl:minQualifiedCardinality>
                <owl:onDataRange rdf:resource="http://www.w3.org/2001/XMLSchema#boolean"/>
            </owl:Restriction>
        </rdfs:subClassOf>
        <rdfs:subClassOf>
            <owl:Restriction>
                <owl:onProperty rdf:resource="https://w3id.org/netbeheer/referentiemodellen/IECCIM/TC57CIM/IEC61970/Base/Wires#Switch_open"/>
                <owl:minQualifiedCardinality rdf:datatype="http://www.w3.org/2001/XMLSchema#nonNegativeInteger">0</owl:minQualifiedCardinality>
                <owl:onDataRange rdf:resource="http://www.w3.org/2001/XMLSchema#boolean"/>
            </owl:Restriction>
        </rdfs:subClassOf>
        <rdfs:subClassOf>
            <owl:Restriction>
                <owl:onProperty rdf:resource="https://w3id.org/netbeheer/referentiemodellen/IECCIM/TC57CIM/IEC61970/Base/Wires#Switch_retained"/>
                <owl:minQualifiedCardinality rdf:datatype="http://www.w3.org/2001/XMLSchema#nonNegativeInteger">0</owl:minQualifiedCardinality>
                <owl:onDataRange rdf:resource="http://www.w3.org/2001/XMLSchema#boolean"/>
            </owl:Restriction>
        </rdfs:subClassOf>
        <rdfs:subClassOf>
            <owl:Restriction>
                <owl:onProperty rdf:resource="https://w3id.org/netbeheer/referentiemodellen/IECCIM/TC57CIM/IEC61970/Base/Wires#Switch_switchOnCount"/>
                <owl:minQualifiedCardinality rdf:datatype="http://www.w3.org/2001/XMLSchema#nonNegativeInteger">0</owl:minQualifiedCardinality>
                <owl:onDataRange rdf:resource="http://www.w3.org/2001/XMLSchema#nonNegativeInteger"/>
            </owl:Restriction>
        </rdfs:subClassOf>
        <rdfs:subClassOf>
            <owl:Restriction>
                <owl:onProperty rdf:resource="https://w3id.org/netbeheer/referentiemodellen/IECCIM/TC57CIM/IEC61970/Base/Wires#Switch_switchOnDate"/>
                <owl:minQualifiedCardinality rdf:datatype="http://www.w3.org/2001/XMLSchema#nonNegativeInteger">0</owl:minQualifiedCardinality>
                <owl:onDataRange rdf:resource="http://www.w3.org/2001/XMLSchema#dateTime"/>
            </owl:Restriction>
        </rdfs:subClassOf>
        <rdfs:subClassOf>
            <owl:Restriction>
                <owl:onProperty rdf:resource="https://w3id.org/netbeheer/referentiemodellen/IECCIM/TC57CIM/IEC61970/Base/Wires#Switch_normalOpen"/>
                <owl:maxQualifiedCardinality rdf:datatype="http://www.w3.org/2001/XMLSchema#nonNegativeInteger">1</owl:maxQualifiedCardinality>
                <owl:onDataRange rdf:resource="http://www.w3.org/2001/XMLSchema#boolean"/>
            </owl:Restriction>
        </rdfs:subClassOf>
        <rdfs:subClassOf>
            <owl:Restriction>
                <owl:onProperty rdf:resource="https://w3id.org/netbeheer/referentiemodellen/IECCIM/TC57CIM/IEC61970/Base/Wires#Switch_open"/>
                <owl:maxQualifiedCardinality rdf:datatype="http://www.w3.org/2001/XMLSchema#nonNegativeInteger">1</owl:maxQualifiedCardinality>
                <owl:onDataRange rdf:resource="http://www.w3.org/2001/XMLSchema#boolean"/>
            </owl:Restriction>
        </rdfs:subClassOf>
        <rdfs:subClassOf>
            <owl:Restriction>
                <owl:onProperty rdf:resource="https://w3id.org/netbeheer/referentiemodellen/IECCIM/TC57CIM/IEC61970/Base/Wires#Switch_retained"/>
                <owl:maxQualifiedCardinality rdf:datatype="http://www.w3.org/2001/XMLSchema#nonNegativeInteger">1</owl:maxQualifiedCardinality>
                <owl:onDataRange rdf:resource="http://www.w3.org/2001/XMLSchema#boolean"/>
            </owl:Restriction>
        </rdfs:subClassOf>
        <rdfs:subClassOf>
            <owl:Restriction>
                <owl:onProperty rdf:resource="https://w3id.org/netbeheer/referentiemodellen/IECCIM/TC57CIM/IEC61970/Base/Wires#Switch_switchOnCount"/>
                <owl:maxQualifiedCardinality rdf:datatype="http://www.w3.org/2001/XMLSchema#nonNegativeInteger">1</owl:maxQualifiedCardinality>
                <owl:onDataRange rdf:resource="http://www.w3.org/2001/XMLSchema#nonNegativeInteger"/>
            </owl:Restriction>
        </rdfs:subClassOf>
        <rdfs:subClassOf>
            <owl:Restriction>
                <owl:onProperty rdf:resource="https://w3id.org/netbeheer/referentiemodellen/IECCIM/TC57CIM/IEC61970/Base/Wires#Switch_switchOnDate"/>
                <owl:maxQualifiedCardinality rdf:datatype="http://www.w3.org/2001/XMLSchema#nonNegativeInteger">1</owl:maxQualifiedCardinality>
                <owl:onDataRange rdf:resource="http://www.w3.org/2001/XMLSchema#dateTime"/>
            </owl:Restriction>
        </rdfs:subClassOf>
        <rdfs:comment>A generic device designed to close, or open, or both, one or more electric circuits.  All switches are two terminal devices including grounding switches.</rdfs:comment>
    </owl:Class>
    


    <!-- https://w3id.org/netbeheer/referentiemodellen/IECCIM/TC57CIM/IEC61970/Base/Wires#SwitchPhase -->


    <owl:Class rdf:about="https://w3id.org/netbeheer/referentiemodellen/IECCIM/TC57CIM/IEC61970/Base/Wires#SwitchPhase">
        <rdfs:subClassOf rdf:resource="https://w3id.org/netbeheer/referentiemodellen/IECCIM/TC57CIM/IEC61970/Base/Core#PowerSystemResource"/>
        <rdfs:subClassOf>
            <owl:Restriction>
                <owl:onProperty rdf:resource="https://w3id.org/netbeheer/referentiemodellen/IECCIM/TC57CIM/IEC61970/Base/Wires#SwitchPhase_Switch"/>
                <owl:minQualifiedCardinality rdf:datatype="http://www.w3.org/2001/XMLSchema#nonNegativeInteger">0</owl:minQualifiedCardinality>
                <owl:onClass rdf:resource="https://w3id.org/netbeheer/referentiemodellen/IECCIM/TC57CIM/IEC61970/Base/Wires#SwitchPhase"/>
            </owl:Restriction>
        </rdfs:subClassOf>
        <rdfs:subClassOf>
            <owl:Restriction>
                <owl:onProperty rdf:resource="https://w3id.org/netbeheer/referentiemodellen/IECCIM/TC57CIM/IEC61970/Base/Wires#SwitchPhase_closed"/>
                <owl:minQualifiedCardinality rdf:datatype="http://www.w3.org/2001/XMLSchema#nonNegativeInteger">0</owl:minQualifiedCardinality>
                <owl:onDataRange rdf:resource="http://www.w3.org/2001/XMLSchema#boolean"/>
            </owl:Restriction>
        </rdfs:subClassOf>
        <rdfs:subClassOf>
            <owl:Restriction>
                <owl:onProperty rdf:resource="https://w3id.org/netbeheer/referentiemodellen/IECCIM/TC57CIM/IEC61970/Base/Wires#SwitchPhase_normalOpen"/>
                <owl:minQualifiedCardinality rdf:datatype="http://www.w3.org/2001/XMLSchema#nonNegativeInteger">0</owl:minQualifiedCardinality>
                <owl:onDataRange rdf:resource="http://www.w3.org/2001/XMLSchema#boolean"/>
            </owl:Restriction>
        </rdfs:subClassOf>
        <rdfs:subClassOf>
            <owl:Restriction>
                <owl:onProperty rdf:resource="https://w3id.org/netbeheer/referentiemodellen/IECCIM/TC57CIM/IEC61970/Base/Wires#SwitchPhase_phaseSide1"/>
                <owl:minQualifiedCardinality rdf:datatype="http://www.w3.org/2001/XMLSchema#nonNegativeInteger">0</owl:minQualifiedCardinality>
                <owl:onDataRange rdf:resource="https://w3id.org/netbeheer/referentiemodellen/IECCIM/TC57CIM/IEC61970/Base/Wires#SinglePhaseKind"/>
            </owl:Restriction>
        </rdfs:subClassOf>
        <rdfs:subClassOf>
            <owl:Restriction>
                <owl:onProperty rdf:resource="https://w3id.org/netbeheer/referentiemodellen/IECCIM/TC57CIM/IEC61970/Base/Wires#SwitchPhase_phaseSide2"/>
                <owl:minQualifiedCardinality rdf:datatype="http://www.w3.org/2001/XMLSchema#nonNegativeInteger">0</owl:minQualifiedCardinality>
                <owl:onDataRange rdf:resource="https://w3id.org/netbeheer/referentiemodellen/IECCIM/TC57CIM/IEC61970/Base/Wires#SinglePhaseKind"/>
            </owl:Restriction>
        </rdfs:subClassOf>
        <rdfs:subClassOf>
            <owl:Restriction>
                <owl:onProperty rdf:resource="https://w3id.org/netbeheer/referentiemodellen/IECCIM/TC57CIM/IEC61970/Base/Wires#SwitchPhase_closed"/>
                <owl:maxQualifiedCardinality rdf:datatype="http://www.w3.org/2001/XMLSchema#nonNegativeInteger">1</owl:maxQualifiedCardinality>
                <owl:onDataRange rdf:resource="http://www.w3.org/2001/XMLSchema#boolean"/>
            </owl:Restriction>
        </rdfs:subClassOf>
        <rdfs:subClassOf>
            <owl:Restriction>
                <owl:onProperty rdf:resource="https://w3id.org/netbeheer/referentiemodellen/IECCIM/TC57CIM/IEC61970/Base/Wires#SwitchPhase_normalOpen"/>
                <owl:maxQualifiedCardinality rdf:datatype="http://www.w3.org/2001/XMLSchema#nonNegativeInteger">1</owl:maxQualifiedCardinality>
                <owl:onDataRange rdf:resource="http://www.w3.org/2001/XMLSchema#boolean"/>
            </owl:Restriction>
        </rdfs:subClassOf>
        <rdfs:subClassOf>
            <owl:Restriction>
                <owl:onProperty rdf:resource="https://w3id.org/netbeheer/referentiemodellen/IECCIM/TC57CIM/IEC61970/Base/Wires#SwitchPhase_phaseSide1"/>
                <owl:maxQualifiedCardinality rdf:datatype="http://www.w3.org/2001/XMLSchema#nonNegativeInteger">1</owl:maxQualifiedCardinality>
                <owl:onDataRange rdf:resource="https://w3id.org/netbeheer/referentiemodellen/IECCIM/TC57CIM/IEC61970/Base/Wires#SinglePhaseKind"/>
            </owl:Restriction>
        </rdfs:subClassOf>
        <rdfs:subClassOf>
            <owl:Restriction>
                <owl:onProperty rdf:resource="https://w3id.org/netbeheer/referentiemodellen/IECCIM/TC57CIM/IEC61970/Base/Wires#SwitchPhase_phaseSide2"/>
                <owl:maxQualifiedCardinality rdf:datatype="http://www.w3.org/2001/XMLSchema#nonNegativeInteger">1</owl:maxQualifiedCardinality>
                <owl:onDataRange rdf:resource="https://w3id.org/netbeheer/referentiemodellen/IECCIM/TC57CIM/IEC61970/Base/Wires#SinglePhaseKind"/>
            </owl:Restriction>
        </rdfs:subClassOf>
        <rdfs:comment>Single phase of a multi-phase switch when its attributes might be different per phase.
</rdfs:comment>
    </owl:Class>
    


    <!-- https://w3id.org/netbeheer/referentiemodellen/IECCIM/TC57CIM/IEC61970/Base/Wires#SwitchSchedule -->


    <owl:Class rdf:about="https://w3id.org/netbeheer/referentiemodellen/IECCIM/TC57CIM/IEC61970/Base/Wires#SwitchSchedule">
        <rdfs:subClassOf rdf:resource="https://w3id.org/netbeheer/referentiemodellen/IECCIM/TC57CIM/IEC61970/Base/LoadModel#SeasonDayTypeSchedule"/>
        <rdfs:subClassOf>
            <owl:Restriction>
                <owl:onProperty rdf:resource="https://w3id.org/netbeheer/referentiemodellen/IECCIM/TC57CIM/IEC61970/Base/Wires#SwitchSchedule_Switch"/>
                <owl:minQualifiedCardinality rdf:datatype="http://www.w3.org/2001/XMLSchema#nonNegativeInteger">0</owl:minQualifiedCardinality>
                <owl:onClass rdf:resource="https://w3id.org/netbeheer/referentiemodellen/IECCIM/TC57CIM/IEC61970/Base/Wires#SwitchSchedule"/>
            </owl:Restriction>
        </rdfs:subClassOf>
        <rdfs:comment>A schedule of switch positions.  If RegularTimePoint.value1 is 0, the switch is open.  If 1, the switch is closed.  </rdfs:comment>
    </owl:Class>
    


    <!-- https://w3id.org/netbeheer/referentiemodellen/IECCIM/TC57CIM/IEC61970/Base/Wires#SynchronousMachine -->


    <owl:Class rdf:about="https://w3id.org/netbeheer/referentiemodellen/IECCIM/TC57CIM/IEC61970/Base/Wires#SynchronousMachine">
        <rdfs:subClassOf rdf:resource="https://w3id.org/netbeheer/referentiemodellen/IECCIM/TC57CIM/IEC61970/Base/Wires#RotatingMachine"/>
        <rdfs:subClassOf>
            <owl:Restriction>
                <owl:onProperty rdf:resource="https://w3id.org/netbeheer/referentiemodellen/IECCIM/TC57CIM/IEC61970/Base/Wires#SynchronousMachine_InitialReactiveCapabilityCurve"/>
                <owl:minQualifiedCardinality rdf:datatype="http://www.w3.org/2001/XMLSchema#nonNegativeInteger">1</owl:minQualifiedCardinality>
                <owl:onClass rdf:resource="https://w3id.org/netbeheer/referentiemodellen/IECCIM/TC57CIM/IEC61970/Base/Wires#SynchronousMachine"/>
            </owl:Restriction>
        </rdfs:subClassOf>
        <rdfs:subClassOf>
            <owl:Restriction>
                <owl:onProperty rdf:resource="https://w3id.org/netbeheer/referentiemodellen/IECCIM/TC57CIM/IEC61970/Base/Wires#SynchronousMachine_PrimeMovers"/>
                <owl:minQualifiedCardinality rdf:datatype="http://www.w3.org/2001/XMLSchema#nonNegativeInteger">0</owl:minQualifiedCardinality>
                <owl:onClass rdf:resource="https://w3id.org/netbeheer/referentiemodellen/IECCIM/TC57CIM/IEC61970/Base/Wires#SynchronousMachine"/>
            </owl:Restriction>
        </rdfs:subClassOf>
        <rdfs:subClassOf>
            <owl:Restriction>
                <owl:onProperty rdf:resource="https://w3id.org/netbeheer/referentiemodellen/IECCIM/TC57CIM/IEC61970/Base/Wires#SynchronousMachine_ReactiveCapabilityCurves"/>
                <owl:minQualifiedCardinality rdf:datatype="http://www.w3.org/2001/XMLSchema#nonNegativeInteger">1</owl:minQualifiedCardinality>
                <owl:onClass rdf:resource="https://w3id.org/netbeheer/referentiemodellen/IECCIM/TC57CIM/IEC61970/Base/Wires#SynchronousMachine"/>
            </owl:Restriction>
        </rdfs:subClassOf>
        <rdfs:subClassOf>
            <owl:Restriction>
                <owl:onProperty rdf:resource="https://w3id.org/netbeheer/referentiemodellen/IECCIM/TC57CIM/IEC61970/Base/Wires#SynchronousMachine_aVRToManualLag"/>
                <owl:minQualifiedCardinality rdf:datatype="http://www.w3.org/2001/XMLSchema#nonNegativeInteger">0</owl:minQualifiedCardinality>
                <owl:onClass rdf:resource="https://w3id.org/netbeheer/referentiemodellen/IECCIM/TC57CIM/IEC61970/Base/Domain#Seconds"/>
            </owl:Restriction>
        </rdfs:subClassOf>
        <rdfs:subClassOf>
            <owl:Restriction>
                <owl:onProperty rdf:resource="https://w3id.org/netbeheer/referentiemodellen/IECCIM/TC57CIM/IEC61970/Base/Wires#SynchronousMachine_aVRToManualLead"/>
                <owl:minQualifiedCardinality rdf:datatype="http://www.w3.org/2001/XMLSchema#nonNegativeInteger">0</owl:minQualifiedCardinality>
                <owl:onClass rdf:resource="https://w3id.org/netbeheer/referentiemodellen/IECCIM/TC57CIM/IEC61970/Base/Domain#Seconds"/>
            </owl:Restriction>
        </rdfs:subClassOf>
        <rdfs:subClassOf>
            <owl:Restriction>
                <owl:onProperty rdf:resource="https://w3id.org/netbeheer/referentiemodellen/IECCIM/TC57CIM/IEC61970/Base/Wires#SynchronousMachine_baseQ"/>
                <owl:minQualifiedCardinality rdf:datatype="http://www.w3.org/2001/XMLSchema#nonNegativeInteger">0</owl:minQualifiedCardinality>
                <owl:onClass rdf:resource="https://w3id.org/netbeheer/referentiemodellen/IECCIM/TC57CIM/IEC61970/Base/Domain#ReactivePower"/>
            </owl:Restriction>
        </rdfs:subClassOf>
        <rdfs:subClassOf>
            <owl:Restriction>
                <owl:onProperty rdf:resource="https://w3id.org/netbeheer/referentiemodellen/IECCIM/TC57CIM/IEC61970/Base/Wires#SynchronousMachine_condenserP"/>
                <owl:minQualifiedCardinality rdf:datatype="http://www.w3.org/2001/XMLSchema#nonNegativeInteger">0</owl:minQualifiedCardinality>
                <owl:onClass rdf:resource="https://w3id.org/netbeheer/referentiemodellen/IECCIM/TC57CIM/IEC61970/Base/Domain#ActivePower"/>
            </owl:Restriction>
        </rdfs:subClassOf>
        <rdfs:subClassOf>
            <owl:Restriction>
                <owl:onProperty rdf:resource="https://w3id.org/netbeheer/referentiemodellen/IECCIM/TC57CIM/IEC61970/Base/Wires#SynchronousMachine_earthingStarPointR"/>
                <owl:minQualifiedCardinality rdf:datatype="http://www.w3.org/2001/XMLSchema#nonNegativeInteger">0</owl:minQualifiedCardinality>
                <owl:onClass rdf:resource="https://w3id.org/netbeheer/referentiemodellen/IECCIM/TC57CIM/IEC61970/Base/Domain#Resistance"/>
            </owl:Restriction>
        </rdfs:subClassOf>
        <rdfs:subClassOf>
            <owl:Restriction>
                <owl:onProperty rdf:resource="https://w3id.org/netbeheer/referentiemodellen/IECCIM/TC57CIM/IEC61970/Base/Wires#SynchronousMachine_earthingStarPointX"/>
                <owl:minQualifiedCardinality rdf:datatype="http://www.w3.org/2001/XMLSchema#nonNegativeInteger">0</owl:minQualifiedCardinality>
                <owl:onClass rdf:resource="https://w3id.org/netbeheer/referentiemodellen/IECCIM/TC57CIM/IEC61970/Base/Domain#Reactance"/>
            </owl:Restriction>
        </rdfs:subClassOf>
        <rdfs:subClassOf>
            <owl:Restriction>
                <owl:onProperty rdf:resource="https://w3id.org/netbeheer/referentiemodellen/IECCIM/TC57CIM/IEC61970/Base/Wires#SynchronousMachine_ikk"/>
                <owl:minQualifiedCardinality rdf:datatype="http://www.w3.org/2001/XMLSchema#nonNegativeInteger">0</owl:minQualifiedCardinality>
                <owl:onClass rdf:resource="https://w3id.org/netbeheer/referentiemodellen/IECCIM/TC57CIM/IEC61970/Base/Domain#CurrentFlow"/>
            </owl:Restriction>
        </rdfs:subClassOf>
        <rdfs:subClassOf>
            <owl:Restriction>
                <owl:onProperty rdf:resource="https://w3id.org/netbeheer/referentiemodellen/IECCIM/TC57CIM/IEC61970/Base/Wires#SynchronousMachine_manualToAVR"/>
                <owl:minQualifiedCardinality rdf:datatype="http://www.w3.org/2001/XMLSchema#nonNegativeInteger">0</owl:minQualifiedCardinality>
                <owl:onClass rdf:resource="https://w3id.org/netbeheer/referentiemodellen/IECCIM/TC57CIM/IEC61970/Base/Domain#Seconds"/>
            </owl:Restriction>
        </rdfs:subClassOf>
        <rdfs:subClassOf>
            <owl:Restriction>
                <owl:onProperty rdf:resource="https://w3id.org/netbeheer/referentiemodellen/IECCIM/TC57CIM/IEC61970/Base/Wires#SynchronousMachine_maxQ"/>
                <owl:minQualifiedCardinality rdf:datatype="http://www.w3.org/2001/XMLSchema#nonNegativeInteger">0</owl:minQualifiedCardinality>
                <owl:onClass rdf:resource="https://w3id.org/netbeheer/referentiemodellen/IECCIM/TC57CIM/IEC61970/Base/Domain#ReactivePower"/>
            </owl:Restriction>
        </rdfs:subClassOf>
        <rdfs:subClassOf>
            <owl:Restriction>
                <owl:onProperty rdf:resource="https://w3id.org/netbeheer/referentiemodellen/IECCIM/TC57CIM/IEC61970/Base/Wires#SynchronousMachine_maxU"/>
                <owl:minQualifiedCardinality rdf:datatype="http://www.w3.org/2001/XMLSchema#nonNegativeInteger">0</owl:minQualifiedCardinality>
                <owl:onClass rdf:resource="https://w3id.org/netbeheer/referentiemodellen/IECCIM/TC57CIM/IEC61970/Base/Domain#Voltage"/>
            </owl:Restriction>
        </rdfs:subClassOf>
        <rdfs:subClassOf>
            <owl:Restriction>
                <owl:onProperty rdf:resource="https://w3id.org/netbeheer/referentiemodellen/IECCIM/TC57CIM/IEC61970/Base/Wires#SynchronousMachine_minQ"/>
                <owl:minQualifiedCardinality rdf:datatype="http://www.w3.org/2001/XMLSchema#nonNegativeInteger">0</owl:minQualifiedCardinality>
                <owl:onClass rdf:resource="https://w3id.org/netbeheer/referentiemodellen/IECCIM/TC57CIM/IEC61970/Base/Domain#ReactivePower"/>
            </owl:Restriction>
        </rdfs:subClassOf>
        <rdfs:subClassOf>
            <owl:Restriction>
                <owl:onProperty rdf:resource="https://w3id.org/netbeheer/referentiemodellen/IECCIM/TC57CIM/IEC61970/Base/Wires#SynchronousMachine_minU"/>
                <owl:minQualifiedCardinality rdf:datatype="http://www.w3.org/2001/XMLSchema#nonNegativeInteger">0</owl:minQualifiedCardinality>
                <owl:onClass rdf:resource="https://w3id.org/netbeheer/referentiemodellen/IECCIM/TC57CIM/IEC61970/Base/Domain#Voltage"/>
            </owl:Restriction>
        </rdfs:subClassOf>
        <rdfs:subClassOf>
            <owl:Restriction>
                <owl:onProperty rdf:resource="https://w3id.org/netbeheer/referentiemodellen/IECCIM/TC57CIM/IEC61970/Base/Wires#SynchronousMachine_qPercent"/>
                <owl:minQualifiedCardinality rdf:datatype="http://www.w3.org/2001/XMLSchema#nonNegativeInteger">0</owl:minQualifiedCardinality>
                <owl:onClass rdf:resource="https://w3id.org/netbeheer/referentiemodellen/IECCIM/TC57CIM/IEC61970/Base/Domain#PerCent"/>
            </owl:Restriction>
        </rdfs:subClassOf>
        <rdfs:subClassOf>
            <owl:Restriction>
                <owl:onProperty rdf:resource="https://w3id.org/netbeheer/referentiemodellen/IECCIM/TC57CIM/IEC61970/Base/Wires#SynchronousMachine_r"/>
                <owl:minQualifiedCardinality rdf:datatype="http://www.w3.org/2001/XMLSchema#nonNegativeInteger">0</owl:minQualifiedCardinality>
                <owl:onClass rdf:resource="https://w3id.org/netbeheer/referentiemodellen/IECCIM/TC57CIM/IEC61970/Base/Domain#Resistance"/>
            </owl:Restriction>
        </rdfs:subClassOf>
        <rdfs:subClassOf>
            <owl:Restriction>
                <owl:onProperty rdf:resource="https://w3id.org/netbeheer/referentiemodellen/IECCIM/TC57CIM/IEC61970/Base/Wires#SynchronousMachine_r0"/>
                <owl:minQualifiedCardinality rdf:datatype="http://www.w3.org/2001/XMLSchema#nonNegativeInteger">0</owl:minQualifiedCardinality>
                <owl:onClass rdf:resource="https://w3id.org/netbeheer/referentiemodellen/IECCIM/TC57CIM/IEC61970/Base/Domain#Resistance"/>
            </owl:Restriction>
        </rdfs:subClassOf>
        <rdfs:subClassOf>
            <owl:Restriction>
                <owl:onProperty rdf:resource="https://w3id.org/netbeheer/referentiemodellen/IECCIM/TC57CIM/IEC61970/Base/Wires#SynchronousMachine_r2"/>
                <owl:minQualifiedCardinality rdf:datatype="http://www.w3.org/2001/XMLSchema#nonNegativeInteger">0</owl:minQualifiedCardinality>
                <owl:onClass rdf:resource="https://w3id.org/netbeheer/referentiemodellen/IECCIM/TC57CIM/IEC61970/Base/Domain#Resistance"/>
            </owl:Restriction>
        </rdfs:subClassOf>
        <rdfs:subClassOf>
            <owl:Restriction>
                <owl:onProperty rdf:resource="https://w3id.org/netbeheer/referentiemodellen/IECCIM/TC57CIM/IEC61970/Base/Wires#SynchronousMachine_satDirectSubtransX"/>
                <owl:minQualifiedCardinality rdf:datatype="http://www.w3.org/2001/XMLSchema#nonNegativeInteger">0</owl:minQualifiedCardinality>
                <owl:onClass rdf:resource="https://w3id.org/netbeheer/referentiemodellen/IECCIM/TC57CIM/IEC61970/Base/Domain#PU"/>
            </owl:Restriction>
        </rdfs:subClassOf>
        <rdfs:subClassOf>
            <owl:Restriction>
                <owl:onProperty rdf:resource="https://w3id.org/netbeheer/referentiemodellen/IECCIM/TC57CIM/IEC61970/Base/Wires#SynchronousMachine_satDirectSyncX"/>
                <owl:minQualifiedCardinality rdf:datatype="http://www.w3.org/2001/XMLSchema#nonNegativeInteger">0</owl:minQualifiedCardinality>
                <owl:onClass rdf:resource="https://w3id.org/netbeheer/referentiemodellen/IECCIM/TC57CIM/IEC61970/Base/Domain#PU"/>
            </owl:Restriction>
        </rdfs:subClassOf>
        <rdfs:subClassOf>
            <owl:Restriction>
                <owl:onProperty rdf:resource="https://w3id.org/netbeheer/referentiemodellen/IECCIM/TC57CIM/IEC61970/Base/Wires#SynchronousMachine_satDirectTransX"/>
                <owl:minQualifiedCardinality rdf:datatype="http://www.w3.org/2001/XMLSchema#nonNegativeInteger">0</owl:minQualifiedCardinality>
                <owl:onClass rdf:resource="https://w3id.org/netbeheer/referentiemodellen/IECCIM/TC57CIM/IEC61970/Base/Domain#PU"/>
            </owl:Restriction>
        </rdfs:subClassOf>
        <rdfs:subClassOf>
            <owl:Restriction>
                <owl:onProperty rdf:resource="https://w3id.org/netbeheer/referentiemodellen/IECCIM/TC57CIM/IEC61970/Base/Wires#SynchronousMachine_voltageRegulationRange"/>
                <owl:minQualifiedCardinality rdf:datatype="http://www.w3.org/2001/XMLSchema#nonNegativeInteger">0</owl:minQualifiedCardinality>
                <owl:onClass rdf:resource="https://w3id.org/netbeheer/referentiemodellen/IECCIM/TC57CIM/IEC61970/Base/Domain#PerCent"/>
            </owl:Restriction>
        </rdfs:subClassOf>
        <rdfs:subClassOf>
            <owl:Restriction>
                <owl:onProperty rdf:resource="https://w3id.org/netbeheer/referentiemodellen/IECCIM/TC57CIM/IEC61970/Base/Wires#SynchronousMachine_x0"/>
                <owl:minQualifiedCardinality rdf:datatype="http://www.w3.org/2001/XMLSchema#nonNegativeInteger">0</owl:minQualifiedCardinality>
                <owl:onClass rdf:resource="https://w3id.org/netbeheer/referentiemodellen/IECCIM/TC57CIM/IEC61970/Base/Domain#Reactance"/>
            </owl:Restriction>
        </rdfs:subClassOf>
        <rdfs:subClassOf>
            <owl:Restriction>
                <owl:onProperty rdf:resource="https://w3id.org/netbeheer/referentiemodellen/IECCIM/TC57CIM/IEC61970/Base/Wires#SynchronousMachine_x2"/>
                <owl:minQualifiedCardinality rdf:datatype="http://www.w3.org/2001/XMLSchema#nonNegativeInteger">0</owl:minQualifiedCardinality>
                <owl:onClass rdf:resource="https://w3id.org/netbeheer/referentiemodellen/IECCIM/TC57CIM/IEC61970/Base/Domain#Reactance"/>
            </owl:Restriction>
        </rdfs:subClassOf>
        <rdfs:subClassOf>
            <owl:Restriction>
                <owl:onProperty rdf:resource="https://w3id.org/netbeheer/referentiemodellen/IECCIM/TC57CIM/IEC61970/Base/Wires#SynchronousMachine_SynchronousMachineDynamics"/>
                <owl:qualifiedCardinality rdf:datatype="http://www.w3.org/2001/XMLSchema#nonNegativeInteger">1</owl:qualifiedCardinality>
                <owl:onClass rdf:resource="https://w3id.org/netbeheer/referentiemodellen/IECCIM/TC57CIM/IEC61970/Base/Wires#SynchronousMachine"/>
            </owl:Restriction>
        </rdfs:subClassOf>
        <rdfs:subClassOf>
            <owl:Restriction>
                <owl:onProperty rdf:resource="https://w3id.org/netbeheer/referentiemodellen/IECCIM/TC57CIM/IEC61970/Base/Wires#SynchronousMachine_aVRToManualLag"/>
                <owl:maxQualifiedCardinality rdf:datatype="http://www.w3.org/2001/XMLSchema#nonNegativeInteger">1</owl:maxQualifiedCardinality>
                <owl:onClass rdf:resource="https://w3id.org/netbeheer/referentiemodellen/IECCIM/TC57CIM/IEC61970/Base/Domain#Seconds"/>
            </owl:Restriction>
        </rdfs:subClassOf>
        <rdfs:subClassOf>
            <owl:Restriction>
                <owl:onProperty rdf:resource="https://w3id.org/netbeheer/referentiemodellen/IECCIM/TC57CIM/IEC61970/Base/Wires#SynchronousMachine_aVRToManualLead"/>
                <owl:maxQualifiedCardinality rdf:datatype="http://www.w3.org/2001/XMLSchema#nonNegativeInteger">1</owl:maxQualifiedCardinality>
                <owl:onClass rdf:resource="https://w3id.org/netbeheer/referentiemodellen/IECCIM/TC57CIM/IEC61970/Base/Domain#Seconds"/>
            </owl:Restriction>
        </rdfs:subClassOf>
        <rdfs:subClassOf>
            <owl:Restriction>
                <owl:onProperty rdf:resource="https://w3id.org/netbeheer/referentiemodellen/IECCIM/TC57CIM/IEC61970/Base/Wires#SynchronousMachine_baseQ"/>
                <owl:maxQualifiedCardinality rdf:datatype="http://www.w3.org/2001/XMLSchema#nonNegativeInteger">1</owl:maxQualifiedCardinality>
                <owl:onClass rdf:resource="https://w3id.org/netbeheer/referentiemodellen/IECCIM/TC57CIM/IEC61970/Base/Domain#ReactivePower"/>
            </owl:Restriction>
        </rdfs:subClassOf>
        <rdfs:subClassOf>
            <owl:Restriction>
                <owl:onProperty rdf:resource="https://w3id.org/netbeheer/referentiemodellen/IECCIM/TC57CIM/IEC61970/Base/Wires#SynchronousMachine_condenserP"/>
                <owl:maxQualifiedCardinality rdf:datatype="http://www.w3.org/2001/XMLSchema#nonNegativeInteger">1</owl:maxQualifiedCardinality>
                <owl:onClass rdf:resource="https://w3id.org/netbeheer/referentiemodellen/IECCIM/TC57CIM/IEC61970/Base/Domain#ActivePower"/>
            </owl:Restriction>
        </rdfs:subClassOf>
        <rdfs:subClassOf>
            <owl:Restriction>
                <owl:onProperty rdf:resource="https://w3id.org/netbeheer/referentiemodellen/IECCIM/TC57CIM/IEC61970/Base/Wires#SynchronousMachine_earthingStarPointR"/>
                <owl:maxQualifiedCardinality rdf:datatype="http://www.w3.org/2001/XMLSchema#nonNegativeInteger">1</owl:maxQualifiedCardinality>
                <owl:onClass rdf:resource="https://w3id.org/netbeheer/referentiemodellen/IECCIM/TC57CIM/IEC61970/Base/Domain#Resistance"/>
            </owl:Restriction>
        </rdfs:subClassOf>
        <rdfs:subClassOf>
            <owl:Restriction>
                <owl:onProperty rdf:resource="https://w3id.org/netbeheer/referentiemodellen/IECCIM/TC57CIM/IEC61970/Base/Wires#SynchronousMachine_earthingStarPointX"/>
                <owl:maxQualifiedCardinality rdf:datatype="http://www.w3.org/2001/XMLSchema#nonNegativeInteger">1</owl:maxQualifiedCardinality>
                <owl:onClass rdf:resource="https://w3id.org/netbeheer/referentiemodellen/IECCIM/TC57CIM/IEC61970/Base/Domain#Reactance"/>
            </owl:Restriction>
        </rdfs:subClassOf>
        <rdfs:subClassOf>
            <owl:Restriction>
                <owl:onProperty rdf:resource="https://w3id.org/netbeheer/referentiemodellen/IECCIM/TC57CIM/IEC61970/Base/Wires#SynchronousMachine_ikk"/>
                <owl:maxQualifiedCardinality rdf:datatype="http://www.w3.org/2001/XMLSchema#nonNegativeInteger">1</owl:maxQualifiedCardinality>
                <owl:onClass rdf:resource="https://w3id.org/netbeheer/referentiemodellen/IECCIM/TC57CIM/IEC61970/Base/Domain#CurrentFlow"/>
            </owl:Restriction>
        </rdfs:subClassOf>
        <rdfs:subClassOf>
            <owl:Restriction>
                <owl:onProperty rdf:resource="https://w3id.org/netbeheer/referentiemodellen/IECCIM/TC57CIM/IEC61970/Base/Wires#SynchronousMachine_manualToAVR"/>
                <owl:maxQualifiedCardinality rdf:datatype="http://www.w3.org/2001/XMLSchema#nonNegativeInteger">1</owl:maxQualifiedCardinality>
                <owl:onClass rdf:resource="https://w3id.org/netbeheer/referentiemodellen/IECCIM/TC57CIM/IEC61970/Base/Domain#Seconds"/>
            </owl:Restriction>
        </rdfs:subClassOf>
        <rdfs:subClassOf>
            <owl:Restriction>
                <owl:onProperty rdf:resource="https://w3id.org/netbeheer/referentiemodellen/IECCIM/TC57CIM/IEC61970/Base/Wires#SynchronousMachine_maxQ"/>
                <owl:maxQualifiedCardinality rdf:datatype="http://www.w3.org/2001/XMLSchema#nonNegativeInteger">1</owl:maxQualifiedCardinality>
                <owl:onClass rdf:resource="https://w3id.org/netbeheer/referentiemodellen/IECCIM/TC57CIM/IEC61970/Base/Domain#ReactivePower"/>
            </owl:Restriction>
        </rdfs:subClassOf>
        <rdfs:subClassOf>
            <owl:Restriction>
                <owl:onProperty rdf:resource="https://w3id.org/netbeheer/referentiemodellen/IECCIM/TC57CIM/IEC61970/Base/Wires#SynchronousMachine_maxU"/>
                <owl:maxQualifiedCardinality rdf:datatype="http://www.w3.org/2001/XMLSchema#nonNegativeInteger">1</owl:maxQualifiedCardinality>
                <owl:onClass rdf:resource="https://w3id.org/netbeheer/referentiemodellen/IECCIM/TC57CIM/IEC61970/Base/Domain#Voltage"/>
            </owl:Restriction>
        </rdfs:subClassOf>
        <rdfs:subClassOf>
            <owl:Restriction>
                <owl:onProperty rdf:resource="https://w3id.org/netbeheer/referentiemodellen/IECCIM/TC57CIM/IEC61970/Base/Wires#SynchronousMachine_minQ"/>
                <owl:maxQualifiedCardinality rdf:datatype="http://www.w3.org/2001/XMLSchema#nonNegativeInteger">1</owl:maxQualifiedCardinality>
                <owl:onClass rdf:resource="https://w3id.org/netbeheer/referentiemodellen/IECCIM/TC57CIM/IEC61970/Base/Domain#ReactivePower"/>
            </owl:Restriction>
        </rdfs:subClassOf>
        <rdfs:subClassOf>
            <owl:Restriction>
                <owl:onProperty rdf:resource="https://w3id.org/netbeheer/referentiemodellen/IECCIM/TC57CIM/IEC61970/Base/Wires#SynchronousMachine_minU"/>
                <owl:maxQualifiedCardinality rdf:datatype="http://www.w3.org/2001/XMLSchema#nonNegativeInteger">1</owl:maxQualifiedCardinality>
                <owl:onClass rdf:resource="https://w3id.org/netbeheer/referentiemodellen/IECCIM/TC57CIM/IEC61970/Base/Domain#Voltage"/>
            </owl:Restriction>
        </rdfs:subClassOf>
        <rdfs:subClassOf>
            <owl:Restriction>
                <owl:onProperty rdf:resource="https://w3id.org/netbeheer/referentiemodellen/IECCIM/TC57CIM/IEC61970/Base/Wires#SynchronousMachine_qPercent"/>
                <owl:maxQualifiedCardinality rdf:datatype="http://www.w3.org/2001/XMLSchema#nonNegativeInteger">1</owl:maxQualifiedCardinality>
                <owl:onClass rdf:resource="https://w3id.org/netbeheer/referentiemodellen/IECCIM/TC57CIM/IEC61970/Base/Domain#PerCent"/>
            </owl:Restriction>
        </rdfs:subClassOf>
        <rdfs:subClassOf>
            <owl:Restriction>
                <owl:onProperty rdf:resource="https://w3id.org/netbeheer/referentiemodellen/IECCIM/TC57CIM/IEC61970/Base/Wires#SynchronousMachine_r"/>
                <owl:maxQualifiedCardinality rdf:datatype="http://www.w3.org/2001/XMLSchema#nonNegativeInteger">1</owl:maxQualifiedCardinality>
                <owl:onClass rdf:resource="https://w3id.org/netbeheer/referentiemodellen/IECCIM/TC57CIM/IEC61970/Base/Domain#Resistance"/>
            </owl:Restriction>
        </rdfs:subClassOf>
        <rdfs:subClassOf>
            <owl:Restriction>
                <owl:onProperty rdf:resource="https://w3id.org/netbeheer/referentiemodellen/IECCIM/TC57CIM/IEC61970/Base/Wires#SynchronousMachine_r0"/>
                <owl:maxQualifiedCardinality rdf:datatype="http://www.w3.org/2001/XMLSchema#nonNegativeInteger">1</owl:maxQualifiedCardinality>
                <owl:onClass rdf:resource="https://w3id.org/netbeheer/referentiemodellen/IECCIM/TC57CIM/IEC61970/Base/Domain#Resistance"/>
            </owl:Restriction>
        </rdfs:subClassOf>
        <rdfs:subClassOf>
            <owl:Restriction>
                <owl:onProperty rdf:resource="https://w3id.org/netbeheer/referentiemodellen/IECCIM/TC57CIM/IEC61970/Base/Wires#SynchronousMachine_r2"/>
                <owl:maxQualifiedCardinality rdf:datatype="http://www.w3.org/2001/XMLSchema#nonNegativeInteger">1</owl:maxQualifiedCardinality>
                <owl:onClass rdf:resource="https://w3id.org/netbeheer/referentiemodellen/IECCIM/TC57CIM/IEC61970/Base/Domain#Resistance"/>
            </owl:Restriction>
        </rdfs:subClassOf>
        <rdfs:subClassOf>
            <owl:Restriction>
                <owl:onProperty rdf:resource="https://w3id.org/netbeheer/referentiemodellen/IECCIM/TC57CIM/IEC61970/Base/Wires#SynchronousMachine_satDirectSubtransX"/>
                <owl:maxQualifiedCardinality rdf:datatype="http://www.w3.org/2001/XMLSchema#nonNegativeInteger">1</owl:maxQualifiedCardinality>
                <owl:onClass rdf:resource="https://w3id.org/netbeheer/referentiemodellen/IECCIM/TC57CIM/IEC61970/Base/Domain#PU"/>
            </owl:Restriction>
        </rdfs:subClassOf>
        <rdfs:subClassOf>
            <owl:Restriction>
                <owl:onProperty rdf:resource="https://w3id.org/netbeheer/referentiemodellen/IECCIM/TC57CIM/IEC61970/Base/Wires#SynchronousMachine_satDirectSyncX"/>
                <owl:maxQualifiedCardinality rdf:datatype="http://www.w3.org/2001/XMLSchema#nonNegativeInteger">1</owl:maxQualifiedCardinality>
                <owl:onClass rdf:resource="https://w3id.org/netbeheer/referentiemodellen/IECCIM/TC57CIM/IEC61970/Base/Domain#PU"/>
            </owl:Restriction>
        </rdfs:subClassOf>
        <rdfs:subClassOf>
            <owl:Restriction>
                <owl:onProperty rdf:resource="https://w3id.org/netbeheer/referentiemodellen/IECCIM/TC57CIM/IEC61970/Base/Wires#SynchronousMachine_satDirectTransX"/>
                <owl:maxQualifiedCardinality rdf:datatype="http://www.w3.org/2001/XMLSchema#nonNegativeInteger">1</owl:maxQualifiedCardinality>
                <owl:onClass rdf:resource="https://w3id.org/netbeheer/referentiemodellen/IECCIM/TC57CIM/IEC61970/Base/Domain#PU"/>
            </owl:Restriction>
        </rdfs:subClassOf>
        <rdfs:subClassOf>
            <owl:Restriction>
                <owl:onProperty rdf:resource="https://w3id.org/netbeheer/referentiemodellen/IECCIM/TC57CIM/IEC61970/Base/Wires#SynchronousMachine_voltageRegulationRange"/>
                <owl:maxQualifiedCardinality rdf:datatype="http://www.w3.org/2001/XMLSchema#nonNegativeInteger">1</owl:maxQualifiedCardinality>
                <owl:onClass rdf:resource="https://w3id.org/netbeheer/referentiemodellen/IECCIM/TC57CIM/IEC61970/Base/Domain#PerCent"/>
            </owl:Restriction>
        </rdfs:subClassOf>
        <rdfs:subClassOf>
            <owl:Restriction>
                <owl:onProperty rdf:resource="https://w3id.org/netbeheer/referentiemodellen/IECCIM/TC57CIM/IEC61970/Base/Wires#SynchronousMachine_x0"/>
                <owl:maxQualifiedCardinality rdf:datatype="http://www.w3.org/2001/XMLSchema#nonNegativeInteger">1</owl:maxQualifiedCardinality>
                <owl:onClass rdf:resource="https://w3id.org/netbeheer/referentiemodellen/IECCIM/TC57CIM/IEC61970/Base/Domain#Reactance"/>
            </owl:Restriction>
        </rdfs:subClassOf>
        <rdfs:subClassOf>
            <owl:Restriction>
                <owl:onProperty rdf:resource="https://w3id.org/netbeheer/referentiemodellen/IECCIM/TC57CIM/IEC61970/Base/Wires#SynchronousMachine_x2"/>
                <owl:maxQualifiedCardinality rdf:datatype="http://www.w3.org/2001/XMLSchema#nonNegativeInteger">1</owl:maxQualifiedCardinality>
                <owl:onClass rdf:resource="https://w3id.org/netbeheer/referentiemodellen/IECCIM/TC57CIM/IEC61970/Base/Domain#Reactance"/>
            </owl:Restriction>
        </rdfs:subClassOf>
        <rdfs:subClassOf>
            <owl:Restriction>
                <owl:onProperty rdf:resource="https://w3id.org/netbeheer/referentiemodellen/IECCIM/TC57CIM/IEC61970/Base/Wires#SynchronousMachine_coolantCondition"/>
                <owl:minQualifiedCardinality rdf:datatype="http://www.w3.org/2001/XMLSchema#nonNegativeInteger">0</owl:minQualifiedCardinality>
                <owl:onDataRange rdf:resource="http://www.w3.org/2001/XMLSchema#float"/>
            </owl:Restriction>
        </rdfs:subClassOf>
        <rdfs:subClassOf>
            <owl:Restriction>
                <owl:onProperty rdf:resource="https://w3id.org/netbeheer/referentiemodellen/IECCIM/TC57CIM/IEC61970/Base/Wires#SynchronousMachine_coolantType"/>
                <owl:minQualifiedCardinality rdf:datatype="http://www.w3.org/2001/XMLSchema#nonNegativeInteger">0</owl:minQualifiedCardinality>
                <owl:onDataRange rdf:resource="https://w3id.org/netbeheer/referentiemodellen/IECCIM/TC57CIM/IEC61970/Base/Wires#CoolantType"/>
            </owl:Restriction>
        </rdfs:subClassOf>
        <rdfs:subClassOf>
            <owl:Restriction>
                <owl:onProperty rdf:resource="https://w3id.org/netbeheer/referentiemodellen/IECCIM/TC57CIM/IEC61970/Base/Wires#SynchronousMachine_earthing"/>
                <owl:minQualifiedCardinality rdf:datatype="http://www.w3.org/2001/XMLSchema#nonNegativeInteger">0</owl:minQualifiedCardinality>
                <owl:onDataRange rdf:resource="http://www.w3.org/2001/XMLSchema#boolean"/>
            </owl:Restriction>
        </rdfs:subClassOf>
        <rdfs:subClassOf>
            <owl:Restriction>
                <owl:onProperty rdf:resource="https://w3id.org/netbeheer/referentiemodellen/IECCIM/TC57CIM/IEC61970/Base/Wires#SynchronousMachine_mu"/>
                <owl:minQualifiedCardinality rdf:datatype="http://www.w3.org/2001/XMLSchema#nonNegativeInteger">0</owl:minQualifiedCardinality>
                <owl:onDataRange rdf:resource="http://www.w3.org/2001/XMLSchema#float"/>
            </owl:Restriction>
        </rdfs:subClassOf>
        <rdfs:subClassOf>
            <owl:Restriction>
                <owl:onProperty rdf:resource="https://w3id.org/netbeheer/referentiemodellen/IECCIM/TC57CIM/IEC61970/Base/Wires#SynchronousMachine_operatingMode"/>
                <owl:minQualifiedCardinality rdf:datatype="http://www.w3.org/2001/XMLSchema#nonNegativeInteger">0</owl:minQualifiedCardinality>
                <owl:onDataRange rdf:resource="https://w3id.org/netbeheer/referentiemodellen/IECCIM/TC57CIM/IEC61970/Base/Wires#SynchronousMachineOperatingMode"/>
            </owl:Restriction>
        </rdfs:subClassOf>
        <rdfs:subClassOf>
            <owl:Restriction>
                <owl:onProperty rdf:resource="https://w3id.org/netbeheer/referentiemodellen/IECCIM/TC57CIM/IEC61970/Base/Wires#SynchronousMachine_referencePriority"/>
                <owl:minQualifiedCardinality rdf:datatype="http://www.w3.org/2001/XMLSchema#nonNegativeInteger">0</owl:minQualifiedCardinality>
                <owl:onDataRange rdf:resource="http://www.w3.org/2001/XMLSchema#nonNegativeInteger"/>
            </owl:Restriction>
        </rdfs:subClassOf>
        <rdfs:subClassOf>
            <owl:Restriction>
                <owl:onProperty rdf:resource="https://w3id.org/netbeheer/referentiemodellen/IECCIM/TC57CIM/IEC61970/Base/Wires#SynchronousMachine_shortCircuitRotorType"/>
                <owl:minQualifiedCardinality rdf:datatype="http://www.w3.org/2001/XMLSchema#nonNegativeInteger">0</owl:minQualifiedCardinality>
                <owl:onDataRange rdf:resource="https://w3id.org/netbeheer/referentiemodellen/IECCIM/TC57CIM/IEC61970/Base/Wires#ShortCircuitRotorKind"/>
            </owl:Restriction>
        </rdfs:subClassOf>
        <rdfs:subClassOf>
            <owl:Restriction>
                <owl:onProperty rdf:resource="https://w3id.org/netbeheer/referentiemodellen/IECCIM/TC57CIM/IEC61970/Base/Wires#SynchronousMachine_type"/>
                <owl:minQualifiedCardinality rdf:datatype="http://www.w3.org/2001/XMLSchema#nonNegativeInteger">0</owl:minQualifiedCardinality>
                <owl:onDataRange rdf:resource="https://w3id.org/netbeheer/referentiemodellen/IECCIM/TC57CIM/IEC61970/Base/Wires#SynchronousMachineKind"/>
            </owl:Restriction>
        </rdfs:subClassOf>
        <rdfs:subClassOf>
            <owl:Restriction>
                <owl:onProperty rdf:resource="https://w3id.org/netbeheer/referentiemodellen/IECCIM/TC57CIM/IEC61970/Base/Wires#SynchronousMachine_coolantCondition"/>
                <owl:maxQualifiedCardinality rdf:datatype="http://www.w3.org/2001/XMLSchema#nonNegativeInteger">1</owl:maxQualifiedCardinality>
                <owl:onDataRange rdf:resource="http://www.w3.org/2001/XMLSchema#float"/>
            </owl:Restriction>
        </rdfs:subClassOf>
        <rdfs:subClassOf>
            <owl:Restriction>
                <owl:onProperty rdf:resource="https://w3id.org/netbeheer/referentiemodellen/IECCIM/TC57CIM/IEC61970/Base/Wires#SynchronousMachine_coolantType"/>
                <owl:maxQualifiedCardinality rdf:datatype="http://www.w3.org/2001/XMLSchema#nonNegativeInteger">1</owl:maxQualifiedCardinality>
                <owl:onDataRange rdf:resource="https://w3id.org/netbeheer/referentiemodellen/IECCIM/TC57CIM/IEC61970/Base/Wires#CoolantType"/>
            </owl:Restriction>
        </rdfs:subClassOf>
        <rdfs:subClassOf>
            <owl:Restriction>
                <owl:onProperty rdf:resource="https://w3id.org/netbeheer/referentiemodellen/IECCIM/TC57CIM/IEC61970/Base/Wires#SynchronousMachine_earthing"/>
                <owl:maxQualifiedCardinality rdf:datatype="http://www.w3.org/2001/XMLSchema#nonNegativeInteger">1</owl:maxQualifiedCardinality>
                <owl:onDataRange rdf:resource="http://www.w3.org/2001/XMLSchema#boolean"/>
            </owl:Restriction>
        </rdfs:subClassOf>
        <rdfs:subClassOf>
            <owl:Restriction>
                <owl:onProperty rdf:resource="https://w3id.org/netbeheer/referentiemodellen/IECCIM/TC57CIM/IEC61970/Base/Wires#SynchronousMachine_mu"/>
                <owl:maxQualifiedCardinality rdf:datatype="http://www.w3.org/2001/XMLSchema#nonNegativeInteger">1</owl:maxQualifiedCardinality>
                <owl:onDataRange rdf:resource="http://www.w3.org/2001/XMLSchema#float"/>
            </owl:Restriction>
        </rdfs:subClassOf>
        <rdfs:subClassOf>
            <owl:Restriction>
                <owl:onProperty rdf:resource="https://w3id.org/netbeheer/referentiemodellen/IECCIM/TC57CIM/IEC61970/Base/Wires#SynchronousMachine_operatingMode"/>
                <owl:maxQualifiedCardinality rdf:datatype="http://www.w3.org/2001/XMLSchema#nonNegativeInteger">1</owl:maxQualifiedCardinality>
                <owl:onDataRange rdf:resource="https://w3id.org/netbeheer/referentiemodellen/IECCIM/TC57CIM/IEC61970/Base/Wires#SynchronousMachineOperatingMode"/>
            </owl:Restriction>
        </rdfs:subClassOf>
        <rdfs:subClassOf>
            <owl:Restriction>
                <owl:onProperty rdf:resource="https://w3id.org/netbeheer/referentiemodellen/IECCIM/TC57CIM/IEC61970/Base/Wires#SynchronousMachine_referencePriority"/>
                <owl:maxQualifiedCardinality rdf:datatype="http://www.w3.org/2001/XMLSchema#nonNegativeInteger">1</owl:maxQualifiedCardinality>
                <owl:onDataRange rdf:resource="http://www.w3.org/2001/XMLSchema#nonNegativeInteger"/>
            </owl:Restriction>
        </rdfs:subClassOf>
        <rdfs:subClassOf>
            <owl:Restriction>
                <owl:onProperty rdf:resource="https://w3id.org/netbeheer/referentiemodellen/IECCIM/TC57CIM/IEC61970/Base/Wires#SynchronousMachine_shortCircuitRotorType"/>
                <owl:maxQualifiedCardinality rdf:datatype="http://www.w3.org/2001/XMLSchema#nonNegativeInteger">1</owl:maxQualifiedCardinality>
                <owl:onDataRange rdf:resource="https://w3id.org/netbeheer/referentiemodellen/IECCIM/TC57CIM/IEC61970/Base/Wires#ShortCircuitRotorKind"/>
            </owl:Restriction>
        </rdfs:subClassOf>
        <rdfs:subClassOf>
            <owl:Restriction>
                <owl:onProperty rdf:resource="https://w3id.org/netbeheer/referentiemodellen/IECCIM/TC57CIM/IEC61970/Base/Wires#SynchronousMachine_type"/>
                <owl:maxQualifiedCardinality rdf:datatype="http://www.w3.org/2001/XMLSchema#nonNegativeInteger">1</owl:maxQualifiedCardinality>
                <owl:onDataRange rdf:resource="https://w3id.org/netbeheer/referentiemodellen/IECCIM/TC57CIM/IEC61970/Base/Wires#SynchronousMachineKind"/>
            </owl:Restriction>
        </rdfs:subClassOf>
        <rdfs:comment>An electromechanical device that operates with shaft rotating synchronously with the network. It is a single machine operating either as a generator or synchronous condenser or pump.</rdfs:comment>
    </owl:Class>
    


    <!-- https://w3id.org/netbeheer/referentiemodellen/IECCIM/TC57CIM/IEC61970/Base/Wires#TapChanger -->


    <owl:Class rdf:about="https://w3id.org/netbeheer/referentiemodellen/IECCIM/TC57CIM/IEC61970/Base/Wires#TapChanger">
        <rdfs:subClassOf rdf:resource="https://w3id.org/netbeheer/referentiemodellen/IECCIM/TC57CIM/IEC61970/Base/Core#PowerSystemResource"/>
        <rdfs:subClassOf>
            <owl:Restriction>
                <owl:onProperty rdf:resource="https://w3id.org/netbeheer/referentiemodellen/IECCIM/TC57CIM/IEC61970/Base/Wires#TapChanger_TapChangerControl"/>
                <owl:minQualifiedCardinality rdf:datatype="http://www.w3.org/2001/XMLSchema#nonNegativeInteger">0</owl:minQualifiedCardinality>
                <owl:onClass rdf:resource="https://w3id.org/netbeheer/referentiemodellen/IECCIM/TC57CIM/IEC61970/Base/Wires#TapChanger"/>
            </owl:Restriction>
        </rdfs:subClassOf>
        <rdfs:subClassOf>
            <owl:Restriction>
                <owl:onProperty rdf:resource="https://w3id.org/netbeheer/referentiemodellen/IECCIM/TC57CIM/IEC61970/Base/Wires#TapChanger_initialDelay"/>
                <owl:minQualifiedCardinality rdf:datatype="http://www.w3.org/2001/XMLSchema#nonNegativeInteger">0</owl:minQualifiedCardinality>
                <owl:onClass rdf:resource="https://w3id.org/netbeheer/referentiemodellen/IECCIM/TC57CIM/IEC61970/Base/Domain#Seconds"/>
            </owl:Restriction>
        </rdfs:subClassOf>
        <rdfs:subClassOf>
            <owl:Restriction>
                <owl:onProperty rdf:resource="https://w3id.org/netbeheer/referentiemodellen/IECCIM/TC57CIM/IEC61970/Base/Wires#TapChanger_neutralU"/>
                <owl:minQualifiedCardinality rdf:datatype="http://www.w3.org/2001/XMLSchema#nonNegativeInteger">0</owl:minQualifiedCardinality>
                <owl:onClass rdf:resource="https://w3id.org/netbeheer/referentiemodellen/IECCIM/TC57CIM/IEC61970/Base/Domain#Voltage"/>
            </owl:Restriction>
        </rdfs:subClassOf>
        <rdfs:subClassOf>
            <owl:Restriction>
                <owl:onProperty rdf:resource="https://w3id.org/netbeheer/referentiemodellen/IECCIM/TC57CIM/IEC61970/Base/Wires#TapChanger_subsequentDelay"/>
                <owl:minQualifiedCardinality rdf:datatype="http://www.w3.org/2001/XMLSchema#nonNegativeInteger">0</owl:minQualifiedCardinality>
                <owl:onClass rdf:resource="https://w3id.org/netbeheer/referentiemodellen/IECCIM/TC57CIM/IEC61970/Base/Domain#Seconds"/>
            </owl:Restriction>
        </rdfs:subClassOf>
        <rdfs:subClassOf>
            <owl:Restriction>
                <owl:onProperty rdf:resource="https://w3id.org/netbeheer/referentiemodellen/IECCIM/TC57CIM/IEC61970/Base/Wires#TapChanger_SvTapStep"/>
                <owl:qualifiedCardinality rdf:datatype="http://www.w3.org/2001/XMLSchema#nonNegativeInteger">1</owl:qualifiedCardinality>
                <owl:onClass rdf:resource="https://w3id.org/netbeheer/referentiemodellen/IECCIM/TC57CIM/IEC61970/Base/Wires#TapChanger"/>
            </owl:Restriction>
        </rdfs:subClassOf>
        <rdfs:subClassOf>
            <owl:Restriction>
                <owl:onProperty rdf:resource="https://w3id.org/netbeheer/referentiemodellen/IECCIM/TC57CIM/IEC61970/Base/Wires#TapChanger_TapSchedules"/>
                <owl:qualifiedCardinality rdf:datatype="http://www.w3.org/2001/XMLSchema#nonNegativeInteger">1</owl:qualifiedCardinality>
                <owl:onClass rdf:resource="https://w3id.org/netbeheer/referentiemodellen/IECCIM/TC57CIM/IEC61970/Base/Wires#TapChanger"/>
            </owl:Restriction>
        </rdfs:subClassOf>
        <rdfs:subClassOf>
            <owl:Restriction>
                <owl:onProperty rdf:resource="https://w3id.org/netbeheer/referentiemodellen/IECCIM/TC57CIM/IEC61970/Base/Wires#TapChanger_initialDelay"/>
                <owl:maxQualifiedCardinality rdf:datatype="http://www.w3.org/2001/XMLSchema#nonNegativeInteger">1</owl:maxQualifiedCardinality>
                <owl:onClass rdf:resource="https://w3id.org/netbeheer/referentiemodellen/IECCIM/TC57CIM/IEC61970/Base/Domain#Seconds"/>
            </owl:Restriction>
        </rdfs:subClassOf>
        <rdfs:subClassOf>
            <owl:Restriction>
                <owl:onProperty rdf:resource="https://w3id.org/netbeheer/referentiemodellen/IECCIM/TC57CIM/IEC61970/Base/Wires#TapChanger_neutralU"/>
                <owl:maxQualifiedCardinality rdf:datatype="http://www.w3.org/2001/XMLSchema#nonNegativeInteger">1</owl:maxQualifiedCardinality>
                <owl:onClass rdf:resource="https://w3id.org/netbeheer/referentiemodellen/IECCIM/TC57CIM/IEC61970/Base/Domain#Voltage"/>
            </owl:Restriction>
        </rdfs:subClassOf>
        <rdfs:subClassOf>
            <owl:Restriction>
                <owl:onProperty rdf:resource="https://w3id.org/netbeheer/referentiemodellen/IECCIM/TC57CIM/IEC61970/Base/Wires#TapChanger_subsequentDelay"/>
                <owl:maxQualifiedCardinality rdf:datatype="http://www.w3.org/2001/XMLSchema#nonNegativeInteger">1</owl:maxQualifiedCardinality>
                <owl:onClass rdf:resource="https://w3id.org/netbeheer/referentiemodellen/IECCIM/TC57CIM/IEC61970/Base/Domain#Seconds"/>
            </owl:Restriction>
        </rdfs:subClassOf>
        <rdfs:subClassOf>
            <owl:Restriction>
                <owl:onProperty rdf:resource="https://w3id.org/netbeheer/referentiemodellen/IECCIM/TC57CIM/IEC61970/Base/Wires#TapChanger_controlEnabled"/>
                <owl:minQualifiedCardinality rdf:datatype="http://www.w3.org/2001/XMLSchema#nonNegativeInteger">0</owl:minQualifiedCardinality>
                <owl:onDataRange rdf:resource="http://www.w3.org/2001/XMLSchema#boolean"/>
            </owl:Restriction>
        </rdfs:subClassOf>
        <rdfs:subClassOf>
            <owl:Restriction>
                <owl:onProperty rdf:resource="https://w3id.org/netbeheer/referentiemodellen/IECCIM/TC57CIM/IEC61970/Base/Wires#TapChanger_highStep"/>
                <owl:minQualifiedCardinality rdf:datatype="http://www.w3.org/2001/XMLSchema#nonNegativeInteger">0</owl:minQualifiedCardinality>
                <owl:onDataRange rdf:resource="http://www.w3.org/2001/XMLSchema#nonNegativeInteger"/>
            </owl:Restriction>
        </rdfs:subClassOf>
        <rdfs:subClassOf>
            <owl:Restriction>
                <owl:onProperty rdf:resource="https://w3id.org/netbeheer/referentiemodellen/IECCIM/TC57CIM/IEC61970/Base/Wires#TapChanger_lowStep"/>
                <owl:minQualifiedCardinality rdf:datatype="http://www.w3.org/2001/XMLSchema#nonNegativeInteger">0</owl:minQualifiedCardinality>
                <owl:onDataRange rdf:resource="http://www.w3.org/2001/XMLSchema#nonNegativeInteger"/>
            </owl:Restriction>
        </rdfs:subClassOf>
        <rdfs:subClassOf>
            <owl:Restriction>
                <owl:onProperty rdf:resource="https://w3id.org/netbeheer/referentiemodellen/IECCIM/TC57CIM/IEC61970/Base/Wires#TapChanger_ltcFlag"/>
                <owl:minQualifiedCardinality rdf:datatype="http://www.w3.org/2001/XMLSchema#nonNegativeInteger">0</owl:minQualifiedCardinality>
                <owl:onDataRange rdf:resource="http://www.w3.org/2001/XMLSchema#boolean"/>
            </owl:Restriction>
        </rdfs:subClassOf>
        <rdfs:subClassOf>
            <owl:Restriction>
                <owl:onProperty rdf:resource="https://w3id.org/netbeheer/referentiemodellen/IECCIM/TC57CIM/IEC61970/Base/Wires#TapChanger_neutralStep"/>
                <owl:minQualifiedCardinality rdf:datatype="http://www.w3.org/2001/XMLSchema#nonNegativeInteger">0</owl:minQualifiedCardinality>
                <owl:onDataRange rdf:resource="http://www.w3.org/2001/XMLSchema#nonNegativeInteger"/>
            </owl:Restriction>
        </rdfs:subClassOf>
        <rdfs:subClassOf>
            <owl:Restriction>
                <owl:onProperty rdf:resource="https://w3id.org/netbeheer/referentiemodellen/IECCIM/TC57CIM/IEC61970/Base/Wires#TapChanger_normalStep"/>
                <owl:minQualifiedCardinality rdf:datatype="http://www.w3.org/2001/XMLSchema#nonNegativeInteger">0</owl:minQualifiedCardinality>
                <owl:onDataRange rdf:resource="http://www.w3.org/2001/XMLSchema#nonNegativeInteger"/>
            </owl:Restriction>
        </rdfs:subClassOf>
        <rdfs:subClassOf>
            <owl:Restriction>
                <owl:onProperty rdf:resource="https://w3id.org/netbeheer/referentiemodellen/IECCIM/TC57CIM/IEC61970/Base/Wires#TapChanger_step"/>
                <owl:minQualifiedCardinality rdf:datatype="http://www.w3.org/2001/XMLSchema#nonNegativeInteger">0</owl:minQualifiedCardinality>
                <owl:onDataRange rdf:resource="http://www.w3.org/2001/XMLSchema#float"/>
            </owl:Restriction>
        </rdfs:subClassOf>
        <rdfs:subClassOf>
            <owl:Restriction>
                <owl:onProperty rdf:resource="https://w3id.org/netbeheer/referentiemodellen/IECCIM/TC57CIM/IEC61970/Base/Wires#TapChanger_controlEnabled"/>
                <owl:maxQualifiedCardinality rdf:datatype="http://www.w3.org/2001/XMLSchema#nonNegativeInteger">1</owl:maxQualifiedCardinality>
                <owl:onDataRange rdf:resource="http://www.w3.org/2001/XMLSchema#boolean"/>
            </owl:Restriction>
        </rdfs:subClassOf>
        <rdfs:subClassOf>
            <owl:Restriction>
                <owl:onProperty rdf:resource="https://w3id.org/netbeheer/referentiemodellen/IECCIM/TC57CIM/IEC61970/Base/Wires#TapChanger_highStep"/>
                <owl:maxQualifiedCardinality rdf:datatype="http://www.w3.org/2001/XMLSchema#nonNegativeInteger">1</owl:maxQualifiedCardinality>
                <owl:onDataRange rdf:resource="http://www.w3.org/2001/XMLSchema#nonNegativeInteger"/>
            </owl:Restriction>
        </rdfs:subClassOf>
        <rdfs:subClassOf>
            <owl:Restriction>
                <owl:onProperty rdf:resource="https://w3id.org/netbeheer/referentiemodellen/IECCIM/TC57CIM/IEC61970/Base/Wires#TapChanger_lowStep"/>
                <owl:maxQualifiedCardinality rdf:datatype="http://www.w3.org/2001/XMLSchema#nonNegativeInteger">1</owl:maxQualifiedCardinality>
                <owl:onDataRange rdf:resource="http://www.w3.org/2001/XMLSchema#nonNegativeInteger"/>
            </owl:Restriction>
        </rdfs:subClassOf>
        <rdfs:subClassOf>
            <owl:Restriction>
                <owl:onProperty rdf:resource="https://w3id.org/netbeheer/referentiemodellen/IECCIM/TC57CIM/IEC61970/Base/Wires#TapChanger_ltcFlag"/>
                <owl:maxQualifiedCardinality rdf:datatype="http://www.w3.org/2001/XMLSchema#nonNegativeInteger">1</owl:maxQualifiedCardinality>
                <owl:onDataRange rdf:resource="http://www.w3.org/2001/XMLSchema#boolean"/>
            </owl:Restriction>
        </rdfs:subClassOf>
        <rdfs:subClassOf>
            <owl:Restriction>
                <owl:onProperty rdf:resource="https://w3id.org/netbeheer/referentiemodellen/IECCIM/TC57CIM/IEC61970/Base/Wires#TapChanger_neutralStep"/>
                <owl:maxQualifiedCardinality rdf:datatype="http://www.w3.org/2001/XMLSchema#nonNegativeInteger">1</owl:maxQualifiedCardinality>
                <owl:onDataRange rdf:resource="http://www.w3.org/2001/XMLSchema#nonNegativeInteger"/>
            </owl:Restriction>
        </rdfs:subClassOf>
        <rdfs:subClassOf>
            <owl:Restriction>
                <owl:onProperty rdf:resource="https://w3id.org/netbeheer/referentiemodellen/IECCIM/TC57CIM/IEC61970/Base/Wires#TapChanger_normalStep"/>
                <owl:maxQualifiedCardinality rdf:datatype="http://www.w3.org/2001/XMLSchema#nonNegativeInteger">1</owl:maxQualifiedCardinality>
                <owl:onDataRange rdf:resource="http://www.w3.org/2001/XMLSchema#nonNegativeInteger"/>
            </owl:Restriction>
        </rdfs:subClassOf>
        <rdfs:subClassOf>
            <owl:Restriction>
                <owl:onProperty rdf:resource="https://w3id.org/netbeheer/referentiemodellen/IECCIM/TC57CIM/IEC61970/Base/Wires#TapChanger_step"/>
                <owl:maxQualifiedCardinality rdf:datatype="http://www.w3.org/2001/XMLSchema#nonNegativeInteger">1</owl:maxQualifiedCardinality>
                <owl:onDataRange rdf:resource="http://www.w3.org/2001/XMLSchema#float"/>
            </owl:Restriction>
        </rdfs:subClassOf>
        <rdfs:comment>Mechanism for changing transformer winding tap positions.</rdfs:comment>
    </owl:Class>
    


    <!-- https://w3id.org/netbeheer/referentiemodellen/IECCIM/TC57CIM/IEC61970/Base/Wires#TapChangerControl -->


    <owl:Class rdf:about="https://w3id.org/netbeheer/referentiemodellen/IECCIM/TC57CIM/IEC61970/Base/Wires#TapChangerControl">
        <rdfs:subClassOf rdf:resource="https://w3id.org/netbeheer/referentiemodellen/IECCIM/TC57CIM/IEC61970/Base/Wires#RegulatingControl"/>
        <rdfs:subClassOf>
            <owl:Restriction>
                <owl:onProperty rdf:resource="https://w3id.org/netbeheer/referentiemodellen/IECCIM/TC57CIM/IEC61970/Base/Wires#TapChangerControl_TapChanger"/>
                <owl:minQualifiedCardinality rdf:datatype="http://www.w3.org/2001/XMLSchema#nonNegativeInteger">0</owl:minQualifiedCardinality>
                <owl:onClass rdf:resource="https://w3id.org/netbeheer/referentiemodellen/IECCIM/TC57CIM/IEC61970/Base/Wires#TapChangerControl"/>
            </owl:Restriction>
        </rdfs:subClassOf>
        <rdfs:subClassOf>
            <owl:Restriction>
                <owl:onProperty rdf:resource="https://w3id.org/netbeheer/referentiemodellen/IECCIM/TC57CIM/IEC61970/Base/Wires#TapChangerControl_limitVoltage"/>
                <owl:minQualifiedCardinality rdf:datatype="http://www.w3.org/2001/XMLSchema#nonNegativeInteger">0</owl:minQualifiedCardinality>
                <owl:onClass rdf:resource="https://w3id.org/netbeheer/referentiemodellen/IECCIM/TC57CIM/IEC61970/Base/Domain#Voltage"/>
            </owl:Restriction>
        </rdfs:subClassOf>
        <rdfs:subClassOf>
            <owl:Restriction>
                <owl:onProperty rdf:resource="https://w3id.org/netbeheer/referentiemodellen/IECCIM/TC57CIM/IEC61970/Base/Wires#TapChangerControl_lineDropR"/>
                <owl:minQualifiedCardinality rdf:datatype="http://www.w3.org/2001/XMLSchema#nonNegativeInteger">0</owl:minQualifiedCardinality>
                <owl:onClass rdf:resource="https://w3id.org/netbeheer/referentiemodellen/IECCIM/TC57CIM/IEC61970/Base/Domain#Resistance"/>
            </owl:Restriction>
        </rdfs:subClassOf>
        <rdfs:subClassOf>
            <owl:Restriction>
                <owl:onProperty rdf:resource="https://w3id.org/netbeheer/referentiemodellen/IECCIM/TC57CIM/IEC61970/Base/Wires#TapChangerControl_lineDropX"/>
                <owl:minQualifiedCardinality rdf:datatype="http://www.w3.org/2001/XMLSchema#nonNegativeInteger">0</owl:minQualifiedCardinality>
                <owl:onClass rdf:resource="https://w3id.org/netbeheer/referentiemodellen/IECCIM/TC57CIM/IEC61970/Base/Domain#Reactance"/>
            </owl:Restriction>
        </rdfs:subClassOf>
        <rdfs:subClassOf>
            <owl:Restriction>
                <owl:onProperty rdf:resource="https://w3id.org/netbeheer/referentiemodellen/IECCIM/TC57CIM/IEC61970/Base/Wires#TapChangerControl_reverseLineDropR"/>
                <owl:minQualifiedCardinality rdf:datatype="http://www.w3.org/2001/XMLSchema#nonNegativeInteger">0</owl:minQualifiedCardinality>
                <owl:onClass rdf:resource="https://w3id.org/netbeheer/referentiemodellen/IECCIM/TC57CIM/IEC61970/Base/Domain#Resistance"/>
            </owl:Restriction>
        </rdfs:subClassOf>
        <rdfs:subClassOf>
            <owl:Restriction>
                <owl:onProperty rdf:resource="https://w3id.org/netbeheer/referentiemodellen/IECCIM/TC57CIM/IEC61970/Base/Wires#TapChangerControl_reverseLineDropX"/>
                <owl:minQualifiedCardinality rdf:datatype="http://www.w3.org/2001/XMLSchema#nonNegativeInteger">0</owl:minQualifiedCardinality>
                <owl:onClass rdf:resource="https://w3id.org/netbeheer/referentiemodellen/IECCIM/TC57CIM/IEC61970/Base/Domain#Reactance"/>
            </owl:Restriction>
        </rdfs:subClassOf>
        <rdfs:subClassOf>
            <owl:Restriction>
                <owl:onProperty rdf:resource="https://w3id.org/netbeheer/referentiemodellen/IECCIM/TC57CIM/IEC61970/Base/Wires#TapChangerControl_TapChanger"/>
                <owl:maxQualifiedCardinality rdf:datatype="http://www.w3.org/2001/XMLSchema#nonNegativeInteger">1</owl:maxQualifiedCardinality>
                <owl:onClass rdf:resource="https://w3id.org/netbeheer/referentiemodellen/IECCIM/TC57CIM/IEC61970/Base/Wires#TapChangerControl"/>
            </owl:Restriction>
        </rdfs:subClassOf>
        <rdfs:subClassOf>
            <owl:Restriction>
                <owl:onProperty rdf:resource="https://w3id.org/netbeheer/referentiemodellen/IECCIM/TC57CIM/IEC61970/Base/Wires#TapChangerControl_limitVoltage"/>
                <owl:maxQualifiedCardinality rdf:datatype="http://www.w3.org/2001/XMLSchema#nonNegativeInteger">1</owl:maxQualifiedCardinality>
                <owl:onClass rdf:resource="https://w3id.org/netbeheer/referentiemodellen/IECCIM/TC57CIM/IEC61970/Base/Domain#Voltage"/>
            </owl:Restriction>
        </rdfs:subClassOf>
        <rdfs:subClassOf>
            <owl:Restriction>
                <owl:onProperty rdf:resource="https://w3id.org/netbeheer/referentiemodellen/IECCIM/TC57CIM/IEC61970/Base/Wires#TapChangerControl_lineDropR"/>
                <owl:maxQualifiedCardinality rdf:datatype="http://www.w3.org/2001/XMLSchema#nonNegativeInteger">1</owl:maxQualifiedCardinality>
                <owl:onClass rdf:resource="https://w3id.org/netbeheer/referentiemodellen/IECCIM/TC57CIM/IEC61970/Base/Domain#Resistance"/>
            </owl:Restriction>
        </rdfs:subClassOf>
        <rdfs:subClassOf>
            <owl:Restriction>
                <owl:onProperty rdf:resource="https://w3id.org/netbeheer/referentiemodellen/IECCIM/TC57CIM/IEC61970/Base/Wires#TapChangerControl_lineDropX"/>
                <owl:maxQualifiedCardinality rdf:datatype="http://www.w3.org/2001/XMLSchema#nonNegativeInteger">1</owl:maxQualifiedCardinality>
                <owl:onClass rdf:resource="https://w3id.org/netbeheer/referentiemodellen/IECCIM/TC57CIM/IEC61970/Base/Domain#Reactance"/>
            </owl:Restriction>
        </rdfs:subClassOf>
        <rdfs:subClassOf>
            <owl:Restriction>
                <owl:onProperty rdf:resource="https://w3id.org/netbeheer/referentiemodellen/IECCIM/TC57CIM/IEC61970/Base/Wires#TapChangerControl_reverseLineDropR"/>
                <owl:maxQualifiedCardinality rdf:datatype="http://www.w3.org/2001/XMLSchema#nonNegativeInteger">1</owl:maxQualifiedCardinality>
                <owl:onClass rdf:resource="https://w3id.org/netbeheer/referentiemodellen/IECCIM/TC57CIM/IEC61970/Base/Domain#Resistance"/>
            </owl:Restriction>
        </rdfs:subClassOf>
        <rdfs:subClassOf>
            <owl:Restriction>
                <owl:onProperty rdf:resource="https://w3id.org/netbeheer/referentiemodellen/IECCIM/TC57CIM/IEC61970/Base/Wires#TapChangerControl_reverseLineDropX"/>
                <owl:maxQualifiedCardinality rdf:datatype="http://www.w3.org/2001/XMLSchema#nonNegativeInteger">1</owl:maxQualifiedCardinality>
                <owl:onClass rdf:resource="https://w3id.org/netbeheer/referentiemodellen/IECCIM/TC57CIM/IEC61970/Base/Domain#Reactance"/>
            </owl:Restriction>
        </rdfs:subClassOf>
        <rdfs:subClassOf>
            <owl:Restriction>
                <owl:onProperty rdf:resource="https://w3id.org/netbeheer/referentiemodellen/IECCIM/TC57CIM/IEC61970/Base/Wires#TapChangerControl_lineDropCompensation"/>
                <owl:minQualifiedCardinality rdf:datatype="http://www.w3.org/2001/XMLSchema#nonNegativeInteger">0</owl:minQualifiedCardinality>
                <owl:onDataRange rdf:resource="http://www.w3.org/2001/XMLSchema#boolean"/>
            </owl:Restriction>
        </rdfs:subClassOf>
        <rdfs:subClassOf>
            <owl:Restriction>
                <owl:onProperty rdf:resource="https://w3id.org/netbeheer/referentiemodellen/IECCIM/TC57CIM/IEC61970/Base/Wires#TapChangerControl_lineDropCompensation"/>
                <owl:maxQualifiedCardinality rdf:datatype="http://www.w3.org/2001/XMLSchema#nonNegativeInteger">1</owl:maxQualifiedCardinality>
                <owl:onDataRange rdf:resource="http://www.w3.org/2001/XMLSchema#boolean"/>
            </owl:Restriction>
        </rdfs:subClassOf>
        <rdfs:comment>Describes behavior specific to tap changers, e.g. how the voltage at the end of a line varies with the load level and compensation of the voltage drop by tap adjustment.</rdfs:comment>
    </owl:Class>
    


    <!-- https://w3id.org/netbeheer/referentiemodellen/IECCIM/TC57CIM/IEC61970/Base/Wires#TapChangerTablePoint -->


    <owl:Class rdf:about="https://w3id.org/netbeheer/referentiemodellen/IECCIM/TC57CIM/IEC61970/Base/Wires#TapChangerTablePoint">
        <rdfs:subClassOf>
            <owl:Restriction>
                <owl:onProperty rdf:resource="https://w3id.org/netbeheer/referentiemodellen/IECCIM/TC57CIM/IEC61970/Base/Wires#TapChangerTablePoint_b"/>
                <owl:minQualifiedCardinality rdf:datatype="http://www.w3.org/2001/XMLSchema#nonNegativeInteger">0</owl:minQualifiedCardinality>
                <owl:onClass rdf:resource="https://w3id.org/netbeheer/referentiemodellen/IECCIM/TC57CIM/IEC61970/Base/Domain#PerCent"/>
            </owl:Restriction>
        </rdfs:subClassOf>
        <rdfs:subClassOf>
            <owl:Restriction>
                <owl:onProperty rdf:resource="https://w3id.org/netbeheer/referentiemodellen/IECCIM/TC57CIM/IEC61970/Base/Wires#TapChangerTablePoint_g"/>
                <owl:minQualifiedCardinality rdf:datatype="http://www.w3.org/2001/XMLSchema#nonNegativeInteger">0</owl:minQualifiedCardinality>
                <owl:onClass rdf:resource="https://w3id.org/netbeheer/referentiemodellen/IECCIM/TC57CIM/IEC61970/Base/Domain#PerCent"/>
            </owl:Restriction>
        </rdfs:subClassOf>
        <rdfs:subClassOf>
            <owl:Restriction>
                <owl:onProperty rdf:resource="https://w3id.org/netbeheer/referentiemodellen/IECCIM/TC57CIM/IEC61970/Base/Wires#TapChangerTablePoint_r"/>
                <owl:minQualifiedCardinality rdf:datatype="http://www.w3.org/2001/XMLSchema#nonNegativeInteger">0</owl:minQualifiedCardinality>
                <owl:onClass rdf:resource="https://w3id.org/netbeheer/referentiemodellen/IECCIM/TC57CIM/IEC61970/Base/Domain#PerCent"/>
            </owl:Restriction>
        </rdfs:subClassOf>
        <rdfs:subClassOf>
            <owl:Restriction>
                <owl:onProperty rdf:resource="https://w3id.org/netbeheer/referentiemodellen/IECCIM/TC57CIM/IEC61970/Base/Wires#TapChangerTablePoint_x"/>
                <owl:minQualifiedCardinality rdf:datatype="http://www.w3.org/2001/XMLSchema#nonNegativeInteger">0</owl:minQualifiedCardinality>
                <owl:onClass rdf:resource="https://w3id.org/netbeheer/referentiemodellen/IECCIM/TC57CIM/IEC61970/Base/Domain#PerCent"/>
            </owl:Restriction>
        </rdfs:subClassOf>
        <rdfs:subClassOf>
            <owl:Restriction>
                <owl:onProperty rdf:resource="https://w3id.org/netbeheer/referentiemodellen/IECCIM/TC57CIM/IEC61970/Base/Wires#TapChangerTablePoint_b"/>
                <owl:maxQualifiedCardinality rdf:datatype="http://www.w3.org/2001/XMLSchema#nonNegativeInteger">1</owl:maxQualifiedCardinality>
                <owl:onClass rdf:resource="https://w3id.org/netbeheer/referentiemodellen/IECCIM/TC57CIM/IEC61970/Base/Domain#PerCent"/>
            </owl:Restriction>
        </rdfs:subClassOf>
        <rdfs:subClassOf>
            <owl:Restriction>
                <owl:onProperty rdf:resource="https://w3id.org/netbeheer/referentiemodellen/IECCIM/TC57CIM/IEC61970/Base/Wires#TapChangerTablePoint_g"/>
                <owl:maxQualifiedCardinality rdf:datatype="http://www.w3.org/2001/XMLSchema#nonNegativeInteger">1</owl:maxQualifiedCardinality>
                <owl:onClass rdf:resource="https://w3id.org/netbeheer/referentiemodellen/IECCIM/TC57CIM/IEC61970/Base/Domain#PerCent"/>
            </owl:Restriction>
        </rdfs:subClassOf>
        <rdfs:subClassOf>
            <owl:Restriction>
                <owl:onProperty rdf:resource="https://w3id.org/netbeheer/referentiemodellen/IECCIM/TC57CIM/IEC61970/Base/Wires#TapChangerTablePoint_r"/>
                <owl:maxQualifiedCardinality rdf:datatype="http://www.w3.org/2001/XMLSchema#nonNegativeInteger">1</owl:maxQualifiedCardinality>
                <owl:onClass rdf:resource="https://w3id.org/netbeheer/referentiemodellen/IECCIM/TC57CIM/IEC61970/Base/Domain#PerCent"/>
            </owl:Restriction>
        </rdfs:subClassOf>
        <rdfs:subClassOf>
            <owl:Restriction>
                <owl:onProperty rdf:resource="https://w3id.org/netbeheer/referentiemodellen/IECCIM/TC57CIM/IEC61970/Base/Wires#TapChangerTablePoint_x"/>
                <owl:maxQualifiedCardinality rdf:datatype="http://www.w3.org/2001/XMLSchema#nonNegativeInteger">1</owl:maxQualifiedCardinality>
                <owl:onClass rdf:resource="https://w3id.org/netbeheer/referentiemodellen/IECCIM/TC57CIM/IEC61970/Base/Domain#PerCent"/>
            </owl:Restriction>
        </rdfs:subClassOf>
        <rdfs:subClassOf>
            <owl:Restriction>
                <owl:onProperty rdf:resource="https://w3id.org/netbeheer/referentiemodellen/IECCIM/TC57CIM/IEC61970/Base/Wires#TapChangerTablePoint_ratio"/>
                <owl:minQualifiedCardinality rdf:datatype="http://www.w3.org/2001/XMLSchema#nonNegativeInteger">0</owl:minQualifiedCardinality>
                <owl:onDataRange rdf:resource="http://www.w3.org/2001/XMLSchema#float"/>
            </owl:Restriction>
        </rdfs:subClassOf>
        <rdfs:subClassOf>
            <owl:Restriction>
                <owl:onProperty rdf:resource="https://w3id.org/netbeheer/referentiemodellen/IECCIM/TC57CIM/IEC61970/Base/Wires#TapChangerTablePoint_step"/>
                <owl:minQualifiedCardinality rdf:datatype="http://www.w3.org/2001/XMLSchema#nonNegativeInteger">0</owl:minQualifiedCardinality>
                <owl:onDataRange rdf:resource="http://www.w3.org/2001/XMLSchema#nonNegativeInteger"/>
            </owl:Restriction>
        </rdfs:subClassOf>
        <rdfs:subClassOf>
            <owl:Restriction>
                <owl:onProperty rdf:resource="https://w3id.org/netbeheer/referentiemodellen/IECCIM/TC57CIM/IEC61970/Base/Wires#TapChangerTablePoint_ratio"/>
                <owl:maxQualifiedCardinality rdf:datatype="http://www.w3.org/2001/XMLSchema#nonNegativeInteger">1</owl:maxQualifiedCardinality>
                <owl:onDataRange rdf:resource="http://www.w3.org/2001/XMLSchema#float"/>
            </owl:Restriction>
        </rdfs:subClassOf>
        <rdfs:subClassOf>
            <owl:Restriction>
                <owl:onProperty rdf:resource="https://w3id.org/netbeheer/referentiemodellen/IECCIM/TC57CIM/IEC61970/Base/Wires#TapChangerTablePoint_step"/>
                <owl:maxQualifiedCardinality rdf:datatype="http://www.w3.org/2001/XMLSchema#nonNegativeInteger">1</owl:maxQualifiedCardinality>
                <owl:onDataRange rdf:resource="http://www.w3.org/2001/XMLSchema#nonNegativeInteger"/>
            </owl:Restriction>
        </rdfs:subClassOf>
    </owl:Class>
    


    <!-- https://w3id.org/netbeheer/referentiemodellen/IECCIM/TC57CIM/IEC61970/Base/Wires#TapSchedule -->


    <owl:Class rdf:about="https://w3id.org/netbeheer/referentiemodellen/IECCIM/TC57CIM/IEC61970/Base/Wires#TapSchedule">
        <rdfs:subClassOf rdf:resource="https://w3id.org/netbeheer/referentiemodellen/IECCIM/TC57CIM/IEC61970/Base/LoadModel#SeasonDayTypeSchedule"/>
        <rdfs:subClassOf>
            <owl:Restriction>
                <owl:onProperty rdf:resource="https://w3id.org/netbeheer/referentiemodellen/IECCIM/TC57CIM/IEC61970/Base/Wires#TapSchedule_TapChanger"/>
                <owl:minQualifiedCardinality rdf:datatype="http://www.w3.org/2001/XMLSchema#nonNegativeInteger">0</owl:minQualifiedCardinality>
                <owl:onClass rdf:resource="https://w3id.org/netbeheer/referentiemodellen/IECCIM/TC57CIM/IEC61970/Base/Wires#TapSchedule"/>
            </owl:Restriction>
        </rdfs:subClassOf>
        <rdfs:comment>A pre-established pattern over time for a tap step.</rdfs:comment>
    </owl:Class>
    


    <!-- https://w3id.org/netbeheer/referentiemodellen/IECCIM/TC57CIM/IEC61970/Base/Wires#TransformerCoreAdmittance -->


    <owl:Class rdf:about="https://w3id.org/netbeheer/referentiemodellen/IECCIM/TC57CIM/IEC61970/Base/Wires#TransformerCoreAdmittance">
        <rdfs:subClassOf rdf:resource="https://w3id.org/netbeheer/referentiemodellen/IECCIM/TC57CIM/IEC61970/Base/Core#IdentifiedObject"/>
        <rdfs:subClassOf>
            <owl:Restriction>
                <owl:onProperty rdf:resource="https://w3id.org/netbeheer/referentiemodellen/IECCIM/TC57CIM/IEC61970/Base/Wires#TransformerCoreAdmittance_TransformerEnd"/>
                <owl:minQualifiedCardinality rdf:datatype="http://www.w3.org/2001/XMLSchema#nonNegativeInteger">0</owl:minQualifiedCardinality>
                <owl:onClass rdf:resource="https://w3id.org/netbeheer/referentiemodellen/IECCIM/TC57CIM/IEC61970/Base/Wires#TransformerCoreAdmittance"/>
            </owl:Restriction>
        </rdfs:subClassOf>
        <rdfs:subClassOf>
            <owl:Restriction>
                <owl:onProperty rdf:resource="https://w3id.org/netbeheer/referentiemodellen/IECCIM/TC57CIM/IEC61970/Base/Wires#TransformerCoreAdmittance_TransformerEndInfo"/>
                <owl:minQualifiedCardinality rdf:datatype="http://www.w3.org/2001/XMLSchema#nonNegativeInteger">0</owl:minQualifiedCardinality>
                <owl:onClass rdf:resource="https://w3id.org/netbeheer/referentiemodellen/IECCIM/TC57CIM/IEC61970/Base/Wires#TransformerCoreAdmittance"/>
            </owl:Restriction>
        </rdfs:subClassOf>
        <rdfs:subClassOf>
            <owl:Restriction>
                <owl:onProperty rdf:resource="https://w3id.org/netbeheer/referentiemodellen/IECCIM/TC57CIM/IEC61970/Base/Wires#TransformerCoreAdmittance_b"/>
                <owl:minQualifiedCardinality rdf:datatype="http://www.w3.org/2001/XMLSchema#nonNegativeInteger">0</owl:minQualifiedCardinality>
                <owl:onClass rdf:resource="https://w3id.org/netbeheer/referentiemodellen/IECCIM/TC57CIM/IEC61970/Base/Domain#Susceptance"/>
            </owl:Restriction>
        </rdfs:subClassOf>
        <rdfs:subClassOf>
            <owl:Restriction>
                <owl:onProperty rdf:resource="https://w3id.org/netbeheer/referentiemodellen/IECCIM/TC57CIM/IEC61970/Base/Wires#TransformerCoreAdmittance_b0"/>
                <owl:minQualifiedCardinality rdf:datatype="http://www.w3.org/2001/XMLSchema#nonNegativeInteger">0</owl:minQualifiedCardinality>
                <owl:onClass rdf:resource="https://w3id.org/netbeheer/referentiemodellen/IECCIM/TC57CIM/IEC61970/Base/Domain#Susceptance"/>
            </owl:Restriction>
        </rdfs:subClassOf>
        <rdfs:subClassOf>
            <owl:Restriction>
                <owl:onProperty rdf:resource="https://w3id.org/netbeheer/referentiemodellen/IECCIM/TC57CIM/IEC61970/Base/Wires#TransformerCoreAdmittance_g"/>
                <owl:minQualifiedCardinality rdf:datatype="http://www.w3.org/2001/XMLSchema#nonNegativeInteger">0</owl:minQualifiedCardinality>
                <owl:onClass rdf:resource="https://w3id.org/netbeheer/referentiemodellen/IECCIM/TC57CIM/IEC61970/Base/Domain#Conductance"/>
            </owl:Restriction>
        </rdfs:subClassOf>
        <rdfs:subClassOf>
            <owl:Restriction>
                <owl:onProperty rdf:resource="https://w3id.org/netbeheer/referentiemodellen/IECCIM/TC57CIM/IEC61970/Base/Wires#TransformerCoreAdmittance_g0"/>
                <owl:minQualifiedCardinality rdf:datatype="http://www.w3.org/2001/XMLSchema#nonNegativeInteger">0</owl:minQualifiedCardinality>
                <owl:onClass rdf:resource="https://w3id.org/netbeheer/referentiemodellen/IECCIM/TC57CIM/IEC61970/Base/Domain#Conductance"/>
            </owl:Restriction>
        </rdfs:subClassOf>
        <rdfs:subClassOf>
            <owl:Restriction>
                <owl:onProperty rdf:resource="https://w3id.org/netbeheer/referentiemodellen/IECCIM/TC57CIM/IEC61970/Base/Wires#TransformerCoreAdmittance_TransformerEnd"/>
                <owl:maxQualifiedCardinality rdf:datatype="http://www.w3.org/2001/XMLSchema#nonNegativeInteger">1</owl:maxQualifiedCardinality>
                <owl:onClass rdf:resource="https://w3id.org/netbeheer/referentiemodellen/IECCIM/TC57CIM/IEC61970/Base/Wires#TransformerCoreAdmittance"/>
            </owl:Restriction>
        </rdfs:subClassOf>
        <rdfs:subClassOf>
            <owl:Restriction>
                <owl:onProperty rdf:resource="https://w3id.org/netbeheer/referentiemodellen/IECCIM/TC57CIM/IEC61970/Base/Wires#TransformerCoreAdmittance_TransformerEndInfo"/>
                <owl:maxQualifiedCardinality rdf:datatype="http://www.w3.org/2001/XMLSchema#nonNegativeInteger">1</owl:maxQualifiedCardinality>
                <owl:onClass rdf:resource="https://w3id.org/netbeheer/referentiemodellen/IECCIM/TC57CIM/IEC61970/Base/Wires#TransformerCoreAdmittance"/>
            </owl:Restriction>
        </rdfs:subClassOf>
        <rdfs:subClassOf>
            <owl:Restriction>
                <owl:onProperty rdf:resource="https://w3id.org/netbeheer/referentiemodellen/IECCIM/TC57CIM/IEC61970/Base/Wires#TransformerCoreAdmittance_b"/>
                <owl:maxQualifiedCardinality rdf:datatype="http://www.w3.org/2001/XMLSchema#nonNegativeInteger">1</owl:maxQualifiedCardinality>
                <owl:onClass rdf:resource="https://w3id.org/netbeheer/referentiemodellen/IECCIM/TC57CIM/IEC61970/Base/Domain#Susceptance"/>
            </owl:Restriction>
        </rdfs:subClassOf>
        <rdfs:subClassOf>
            <owl:Restriction>
                <owl:onProperty rdf:resource="https://w3id.org/netbeheer/referentiemodellen/IECCIM/TC57CIM/IEC61970/Base/Wires#TransformerCoreAdmittance_b0"/>
                <owl:maxQualifiedCardinality rdf:datatype="http://www.w3.org/2001/XMLSchema#nonNegativeInteger">1</owl:maxQualifiedCardinality>
                <owl:onClass rdf:resource="https://w3id.org/netbeheer/referentiemodellen/IECCIM/TC57CIM/IEC61970/Base/Domain#Susceptance"/>
            </owl:Restriction>
        </rdfs:subClassOf>
        <rdfs:subClassOf>
            <owl:Restriction>
                <owl:onProperty rdf:resource="https://w3id.org/netbeheer/referentiemodellen/IECCIM/TC57CIM/IEC61970/Base/Wires#TransformerCoreAdmittance_g"/>
                <owl:maxQualifiedCardinality rdf:datatype="http://www.w3.org/2001/XMLSchema#nonNegativeInteger">1</owl:maxQualifiedCardinality>
                <owl:onClass rdf:resource="https://w3id.org/netbeheer/referentiemodellen/IECCIM/TC57CIM/IEC61970/Base/Domain#Conductance"/>
            </owl:Restriction>
        </rdfs:subClassOf>
        <rdfs:subClassOf>
            <owl:Restriction>
                <owl:onProperty rdf:resource="https://w3id.org/netbeheer/referentiemodellen/IECCIM/TC57CIM/IEC61970/Base/Wires#TransformerCoreAdmittance_g0"/>
                <owl:maxQualifiedCardinality rdf:datatype="http://www.w3.org/2001/XMLSchema#nonNegativeInteger">1</owl:maxQualifiedCardinality>
                <owl:onClass rdf:resource="https://w3id.org/netbeheer/referentiemodellen/IECCIM/TC57CIM/IEC61970/Base/Domain#Conductance"/>
            </owl:Restriction>
        </rdfs:subClassOf>
        <rdfs:comment>The transformer core admittance.  Used to specify the core admittance of a transformer in a manner that can be shared among power transformers.
</rdfs:comment>
    </owl:Class>
    


    <!-- https://w3id.org/netbeheer/referentiemodellen/IECCIM/TC57CIM/IEC61970/Base/Wires#TransformerEnd -->


    <owl:Class rdf:about="https://w3id.org/netbeheer/referentiemodellen/IECCIM/TC57CIM/IEC61970/Base/Wires#TransformerEnd">
        <rdfs:subClassOf rdf:resource="https://w3id.org/netbeheer/referentiemodellen/IECCIM/TC57CIM/IEC61970/Base/Core#IdentifiedObject"/>
        <rdfs:subClassOf>
            <owl:Restriction>
                <owl:onProperty rdf:resource="https://w3id.org/netbeheer/referentiemodellen/IECCIM/TC57CIM/IEC61970/Base/Wires#TransformerEnd_CoreAdmittance"/>
                <owl:minQualifiedCardinality rdf:datatype="http://www.w3.org/2001/XMLSchema#nonNegativeInteger">0</owl:minQualifiedCardinality>
                <owl:onClass rdf:resource="https://w3id.org/netbeheer/referentiemodellen/IECCIM/TC57CIM/IEC61970/Base/Wires#TransformerEnd"/>
            </owl:Restriction>
        </rdfs:subClassOf>
        <rdfs:subClassOf>
            <owl:Restriction>
                <owl:onProperty rdf:resource="https://w3id.org/netbeheer/referentiemodellen/IECCIM/TC57CIM/IEC61970/Base/Wires#TransformerEnd_StarImpedance"/>
                <owl:minQualifiedCardinality rdf:datatype="http://www.w3.org/2001/XMLSchema#nonNegativeInteger">0</owl:minQualifiedCardinality>
                <owl:onClass rdf:resource="https://w3id.org/netbeheer/referentiemodellen/IECCIM/TC57CIM/IEC61970/Base/Wires#TransformerEnd"/>
            </owl:Restriction>
        </rdfs:subClassOf>
        <rdfs:subClassOf>
            <owl:Restriction>
                <owl:onProperty rdf:resource="https://w3id.org/netbeheer/referentiemodellen/IECCIM/TC57CIM/IEC61970/Base/Wires#TransformerEnd_ToMeshImpedance"/>
                <owl:minQualifiedCardinality rdf:datatype="http://www.w3.org/2001/XMLSchema#nonNegativeInteger">1</owl:minQualifiedCardinality>
                <owl:onClass rdf:resource="https://w3id.org/netbeheer/referentiemodellen/IECCIM/TC57CIM/IEC61970/Base/Wires#TransformerEnd"/>
            </owl:Restriction>
        </rdfs:subClassOf>
        <rdfs:subClassOf>
            <owl:Restriction>
                <owl:onProperty rdf:resource="https://w3id.org/netbeheer/referentiemodellen/IECCIM/TC57CIM/IEC61970/Base/Wires#TransformerEnd_bmagSat"/>
                <owl:minQualifiedCardinality rdf:datatype="http://www.w3.org/2001/XMLSchema#nonNegativeInteger">0</owl:minQualifiedCardinality>
                <owl:onClass rdf:resource="https://w3id.org/netbeheer/referentiemodellen/IECCIM/TC57CIM/IEC61970/Base/Domain#PerCent"/>
            </owl:Restriction>
        </rdfs:subClassOf>
        <rdfs:subClassOf>
            <owl:Restriction>
                <owl:onProperty rdf:resource="https://w3id.org/netbeheer/referentiemodellen/IECCIM/TC57CIM/IEC61970/Base/Wires#TransformerEnd_magBaseU"/>
                <owl:minQualifiedCardinality rdf:datatype="http://www.w3.org/2001/XMLSchema#nonNegativeInteger">0</owl:minQualifiedCardinality>
                <owl:onClass rdf:resource="https://w3id.org/netbeheer/referentiemodellen/IECCIM/TC57CIM/IEC61970/Base/Domain#Voltage"/>
            </owl:Restriction>
        </rdfs:subClassOf>
        <rdfs:subClassOf>
            <owl:Restriction>
                <owl:onProperty rdf:resource="https://w3id.org/netbeheer/referentiemodellen/IECCIM/TC57CIM/IEC61970/Base/Wires#TransformerEnd_magSatFlux"/>
                <owl:minQualifiedCardinality rdf:datatype="http://www.w3.org/2001/XMLSchema#nonNegativeInteger">0</owl:minQualifiedCardinality>
                <owl:onClass rdf:resource="https://w3id.org/netbeheer/referentiemodellen/IECCIM/TC57CIM/IEC61970/Base/Domain#PerCent"/>
            </owl:Restriction>
        </rdfs:subClassOf>
        <rdfs:subClassOf>
            <owl:Restriction>
                <owl:onProperty rdf:resource="https://w3id.org/netbeheer/referentiemodellen/IECCIM/TC57CIM/IEC61970/Base/Wires#TransformerEnd_rground"/>
                <owl:minQualifiedCardinality rdf:datatype="http://www.w3.org/2001/XMLSchema#nonNegativeInteger">0</owl:minQualifiedCardinality>
                <owl:onClass rdf:resource="https://w3id.org/netbeheer/referentiemodellen/IECCIM/TC57CIM/IEC61970/Base/Domain#Resistance"/>
            </owl:Restriction>
        </rdfs:subClassOf>
        <rdfs:subClassOf>
            <owl:Restriction>
                <owl:onProperty rdf:resource="https://w3id.org/netbeheer/referentiemodellen/IECCIM/TC57CIM/IEC61970/Base/Wires#TransformerEnd_xground"/>
                <owl:minQualifiedCardinality rdf:datatype="http://www.w3.org/2001/XMLSchema#nonNegativeInteger">0</owl:minQualifiedCardinality>
                <owl:onClass rdf:resource="https://w3id.org/netbeheer/referentiemodellen/IECCIM/TC57CIM/IEC61970/Base/Domain#Reactance"/>
            </owl:Restriction>
        </rdfs:subClassOf>
        <rdfs:subClassOf>
            <owl:Restriction>
                <owl:onProperty rdf:resource="https://w3id.org/netbeheer/referentiemodellen/IECCIM/TC57CIM/IEC61970/Base/Wires#TransformerEnd_FromMeshImpedance"/>
                <owl:qualifiedCardinality rdf:datatype="http://www.w3.org/2001/XMLSchema#nonNegativeInteger">1</owl:qualifiedCardinality>
                <owl:onClass rdf:resource="https://w3id.org/netbeheer/referentiemodellen/IECCIM/TC57CIM/IEC61970/Base/Wires#TransformerEnd"/>
            </owl:Restriction>
        </rdfs:subClassOf>
        <rdfs:subClassOf>
            <owl:Restriction>
                <owl:onProperty rdf:resource="https://w3id.org/netbeheer/referentiemodellen/IECCIM/TC57CIM/IEC61970/Base/Wires#TransformerEnd_FromWindingInsulations"/>
                <owl:qualifiedCardinality rdf:datatype="http://www.w3.org/2001/XMLSchema#nonNegativeInteger">1</owl:qualifiedCardinality>
                <owl:onClass rdf:resource="https://w3id.org/netbeheer/referentiemodellen/IECCIM/TC57CIM/IEC61970/Base/Wires#TransformerEnd"/>
            </owl:Restriction>
        </rdfs:subClassOf>
        <rdfs:subClassOf>
            <owl:Restriction>
                <owl:onProperty rdf:resource="https://w3id.org/netbeheer/referentiemodellen/IECCIM/TC57CIM/IEC61970/Base/Wires#TransformerEnd_PhaseTapChanger"/>
                <owl:qualifiedCardinality rdf:datatype="http://www.w3.org/2001/XMLSchema#nonNegativeInteger">1</owl:qualifiedCardinality>
                <owl:onClass rdf:resource="https://w3id.org/netbeheer/referentiemodellen/IECCIM/TC57CIM/IEC61970/Base/Wires#TransformerEnd"/>
            </owl:Restriction>
        </rdfs:subClassOf>
        <rdfs:subClassOf>
            <owl:Restriction>
                <owl:onProperty rdf:resource="https://w3id.org/netbeheer/referentiemodellen/IECCIM/TC57CIM/IEC61970/Base/Wires#TransformerEnd_RatioTapChanger"/>
                <owl:qualifiedCardinality rdf:datatype="http://www.w3.org/2001/XMLSchema#nonNegativeInteger">1</owl:qualifiedCardinality>
                <owl:onClass rdf:resource="https://w3id.org/netbeheer/referentiemodellen/IECCIM/TC57CIM/IEC61970/Base/Wires#TransformerEnd"/>
            </owl:Restriction>
        </rdfs:subClassOf>
        <rdfs:subClassOf>
            <owl:Restriction>
                <owl:onProperty rdf:resource="https://w3id.org/netbeheer/referentiemodellen/IECCIM/TC57CIM/IEC61970/Base/Wires#TransformerEnd_ToWindingInsulations"/>
                <owl:qualifiedCardinality rdf:datatype="http://www.w3.org/2001/XMLSchema#nonNegativeInteger">1</owl:qualifiedCardinality>
                <owl:onClass rdf:resource="https://w3id.org/netbeheer/referentiemodellen/IECCIM/TC57CIM/IEC61970/Base/Wires#TransformerEnd"/>
            </owl:Restriction>
        </rdfs:subClassOf>
        <rdfs:subClassOf>
            <owl:Restriction>
                <owl:onProperty rdf:resource="https://w3id.org/netbeheer/referentiemodellen/IECCIM/TC57CIM/IEC61970/Base/Wires#TransformerEnd_bmagSat"/>
                <owl:maxQualifiedCardinality rdf:datatype="http://www.w3.org/2001/XMLSchema#nonNegativeInteger">1</owl:maxQualifiedCardinality>
                <owl:onClass rdf:resource="https://w3id.org/netbeheer/referentiemodellen/IECCIM/TC57CIM/IEC61970/Base/Domain#PerCent"/>
            </owl:Restriction>
        </rdfs:subClassOf>
        <rdfs:subClassOf>
            <owl:Restriction>
                <owl:onProperty rdf:resource="https://w3id.org/netbeheer/referentiemodellen/IECCIM/TC57CIM/IEC61970/Base/Wires#TransformerEnd_magBaseU"/>
                <owl:maxQualifiedCardinality rdf:datatype="http://www.w3.org/2001/XMLSchema#nonNegativeInteger">1</owl:maxQualifiedCardinality>
                <owl:onClass rdf:resource="https://w3id.org/netbeheer/referentiemodellen/IECCIM/TC57CIM/IEC61970/Base/Domain#Voltage"/>
            </owl:Restriction>
        </rdfs:subClassOf>
        <rdfs:subClassOf>
            <owl:Restriction>
                <owl:onProperty rdf:resource="https://w3id.org/netbeheer/referentiemodellen/IECCIM/TC57CIM/IEC61970/Base/Wires#TransformerEnd_magSatFlux"/>
                <owl:maxQualifiedCardinality rdf:datatype="http://www.w3.org/2001/XMLSchema#nonNegativeInteger">1</owl:maxQualifiedCardinality>
                <owl:onClass rdf:resource="https://w3id.org/netbeheer/referentiemodellen/IECCIM/TC57CIM/IEC61970/Base/Domain#PerCent"/>
            </owl:Restriction>
        </rdfs:subClassOf>
        <rdfs:subClassOf>
            <owl:Restriction>
                <owl:onProperty rdf:resource="https://w3id.org/netbeheer/referentiemodellen/IECCIM/TC57CIM/IEC61970/Base/Wires#TransformerEnd_rground"/>
                <owl:maxQualifiedCardinality rdf:datatype="http://www.w3.org/2001/XMLSchema#nonNegativeInteger">1</owl:maxQualifiedCardinality>
                <owl:onClass rdf:resource="https://w3id.org/netbeheer/referentiemodellen/IECCIM/TC57CIM/IEC61970/Base/Domain#Resistance"/>
            </owl:Restriction>
        </rdfs:subClassOf>
        <rdfs:subClassOf>
            <owl:Restriction>
                <owl:onProperty rdf:resource="https://w3id.org/netbeheer/referentiemodellen/IECCIM/TC57CIM/IEC61970/Base/Wires#TransformerEnd_xground"/>
                <owl:maxQualifiedCardinality rdf:datatype="http://www.w3.org/2001/XMLSchema#nonNegativeInteger">1</owl:maxQualifiedCardinality>
                <owl:onClass rdf:resource="https://w3id.org/netbeheer/referentiemodellen/IECCIM/TC57CIM/IEC61970/Base/Domain#Reactance"/>
            </owl:Restriction>
        </rdfs:subClassOf>
        <rdfs:subClassOf>
            <owl:Restriction>
                <owl:onProperty rdf:resource="https://w3id.org/netbeheer/referentiemodellen/IECCIM/TC57CIM/IEC61970/Base/Wires#TransformerEnd_endNumber"/>
                <owl:minQualifiedCardinality rdf:datatype="http://www.w3.org/2001/XMLSchema#nonNegativeInteger">0</owl:minQualifiedCardinality>
                <owl:onDataRange rdf:resource="http://www.w3.org/2001/XMLSchema#nonNegativeInteger"/>
            </owl:Restriction>
        </rdfs:subClassOf>
        <rdfs:subClassOf>
            <owl:Restriction>
                <owl:onProperty rdf:resource="https://w3id.org/netbeheer/referentiemodellen/IECCIM/TC57CIM/IEC61970/Base/Wires#TransformerEnd_grounded"/>
                <owl:minQualifiedCardinality rdf:datatype="http://www.w3.org/2001/XMLSchema#nonNegativeInteger">0</owl:minQualifiedCardinality>
                <owl:onDataRange rdf:resource="http://www.w3.org/2001/XMLSchema#boolean"/>
            </owl:Restriction>
        </rdfs:subClassOf>
        <rdfs:subClassOf>
            <owl:Restriction>
                <owl:onProperty rdf:resource="https://w3id.org/netbeheer/referentiemodellen/IECCIM/TC57CIM/IEC61970/Base/Wires#TransformerEnd_endNumber"/>
                <owl:maxQualifiedCardinality rdf:datatype="http://www.w3.org/2001/XMLSchema#nonNegativeInteger">1</owl:maxQualifiedCardinality>
                <owl:onDataRange rdf:resource="http://www.w3.org/2001/XMLSchema#nonNegativeInteger"/>
            </owl:Restriction>
        </rdfs:subClassOf>
        <rdfs:subClassOf>
            <owl:Restriction>
                <owl:onProperty rdf:resource="https://w3id.org/netbeheer/referentiemodellen/IECCIM/TC57CIM/IEC61970/Base/Wires#TransformerEnd_grounded"/>
                <owl:maxQualifiedCardinality rdf:datatype="http://www.w3.org/2001/XMLSchema#nonNegativeInteger">1</owl:maxQualifiedCardinality>
                <owl:onDataRange rdf:resource="http://www.w3.org/2001/XMLSchema#boolean"/>
            </owl:Restriction>
        </rdfs:subClassOf>
        <rdfs:comment>A conducting connection point of a power transformer. It corresponds to a physical transformer winding terminal.  In earlier CIM versions, the TransformerWinding class served a similar purpose, but this class is more flexible because it associates to terminal but is not a specialization of ConductingEquipment.</rdfs:comment>
    </owl:Class>
    


    <!-- https://w3id.org/netbeheer/referentiemodellen/IECCIM/TC57CIM/IEC61970/Base/Wires#TransformerMeshImpedance -->


    <owl:Class rdf:about="https://w3id.org/netbeheer/referentiemodellen/IECCIM/TC57CIM/IEC61970/Base/Wires#TransformerMeshImpedance">
        <rdfs:subClassOf rdf:resource="https://w3id.org/netbeheer/referentiemodellen/IECCIM/TC57CIM/IEC61970/Base/Core#IdentifiedObject"/>
        <rdfs:subClassOf>
            <owl:Restriction>
                <owl:onProperty rdf:resource="https://w3id.org/netbeheer/referentiemodellen/IECCIM/TC57CIM/IEC61970/Base/Wires#TransformerMeshImpedance_FromTransformerEnd"/>
                <owl:minQualifiedCardinality rdf:datatype="http://www.w3.org/2001/XMLSchema#nonNegativeInteger">0</owl:minQualifiedCardinality>
                <owl:onClass rdf:resource="https://w3id.org/netbeheer/referentiemodellen/IECCIM/TC57CIM/IEC61970/Base/Wires#TransformerMeshImpedance"/>
            </owl:Restriction>
        </rdfs:subClassOf>
        <rdfs:subClassOf>
            <owl:Restriction>
                <owl:onProperty rdf:resource="https://w3id.org/netbeheer/referentiemodellen/IECCIM/TC57CIM/IEC61970/Base/Wires#TransformerMeshImpedance_FromTransformerEndInfo"/>
                <owl:minQualifiedCardinality rdf:datatype="http://www.w3.org/2001/XMLSchema#nonNegativeInteger">0</owl:minQualifiedCardinality>
                <owl:onClass rdf:resource="https://w3id.org/netbeheer/referentiemodellen/IECCIM/TC57CIM/IEC61970/Base/Wires#TransformerMeshImpedance"/>
            </owl:Restriction>
        </rdfs:subClassOf>
        <rdfs:subClassOf>
            <owl:Restriction>
                <owl:onProperty rdf:resource="https://w3id.org/netbeheer/referentiemodellen/IECCIM/TC57CIM/IEC61970/Base/Wires#TransformerMeshImpedance_ToTransformerEnd"/>
                <owl:minQualifiedCardinality rdf:datatype="http://www.w3.org/2001/XMLSchema#nonNegativeInteger">0</owl:minQualifiedCardinality>
                <owl:onClass rdf:resource="https://w3id.org/netbeheer/referentiemodellen/IECCIM/TC57CIM/IEC61970/Base/Wires#TransformerMeshImpedance"/>
            </owl:Restriction>
        </rdfs:subClassOf>
        <rdfs:subClassOf>
            <owl:Restriction>
                <owl:onProperty rdf:resource="https://w3id.org/netbeheer/referentiemodellen/IECCIM/TC57CIM/IEC61970/Base/Wires#TransformerMeshImpedance_ToTransformerEndInfos"/>
                <owl:minQualifiedCardinality rdf:datatype="http://www.w3.org/2001/XMLSchema#nonNegativeInteger">0</owl:minQualifiedCardinality>
                <owl:onClass rdf:resource="https://w3id.org/netbeheer/referentiemodellen/IECCIM/TC57CIM/IEC61970/Base/Wires#TransformerMeshImpedance"/>
            </owl:Restriction>
        </rdfs:subClassOf>
        <rdfs:subClassOf>
            <owl:Restriction>
                <owl:onProperty rdf:resource="https://w3id.org/netbeheer/referentiemodellen/IECCIM/TC57CIM/IEC61970/Base/Wires#TransformerMeshImpedance_r"/>
                <owl:minQualifiedCardinality rdf:datatype="http://www.w3.org/2001/XMLSchema#nonNegativeInteger">0</owl:minQualifiedCardinality>
                <owl:onClass rdf:resource="https://w3id.org/netbeheer/referentiemodellen/IECCIM/TC57CIM/IEC61970/Base/Domain#Resistance"/>
            </owl:Restriction>
        </rdfs:subClassOf>
        <rdfs:subClassOf>
            <owl:Restriction>
                <owl:onProperty rdf:resource="https://w3id.org/netbeheer/referentiemodellen/IECCIM/TC57CIM/IEC61970/Base/Wires#TransformerMeshImpedance_r0"/>
                <owl:minQualifiedCardinality rdf:datatype="http://www.w3.org/2001/XMLSchema#nonNegativeInteger">0</owl:minQualifiedCardinality>
                <owl:onClass rdf:resource="https://w3id.org/netbeheer/referentiemodellen/IECCIM/TC57CIM/IEC61970/Base/Domain#Resistance"/>
            </owl:Restriction>
        </rdfs:subClassOf>
        <rdfs:subClassOf>
            <owl:Restriction>
                <owl:onProperty rdf:resource="https://w3id.org/netbeheer/referentiemodellen/IECCIM/TC57CIM/IEC61970/Base/Wires#TransformerMeshImpedance_x"/>
                <owl:minQualifiedCardinality rdf:datatype="http://www.w3.org/2001/XMLSchema#nonNegativeInteger">0</owl:minQualifiedCardinality>
                <owl:onClass rdf:resource="https://w3id.org/netbeheer/referentiemodellen/IECCIM/TC57CIM/IEC61970/Base/Domain#Reactance"/>
            </owl:Restriction>
        </rdfs:subClassOf>
        <rdfs:subClassOf>
            <owl:Restriction>
                <owl:onProperty rdf:resource="https://w3id.org/netbeheer/referentiemodellen/IECCIM/TC57CIM/IEC61970/Base/Wires#TransformerMeshImpedance_x0"/>
                <owl:minQualifiedCardinality rdf:datatype="http://www.w3.org/2001/XMLSchema#nonNegativeInteger">0</owl:minQualifiedCardinality>
                <owl:onClass rdf:resource="https://w3id.org/netbeheer/referentiemodellen/IECCIM/TC57CIM/IEC61970/Base/Domain#Reactance"/>
            </owl:Restriction>
        </rdfs:subClassOf>
        <rdfs:subClassOf>
            <owl:Restriction>
                <owl:onProperty rdf:resource="https://w3id.org/netbeheer/referentiemodellen/IECCIM/TC57CIM/IEC61970/Base/Wires#TransformerMeshImpedance_r"/>
                <owl:maxQualifiedCardinality rdf:datatype="http://www.w3.org/2001/XMLSchema#nonNegativeInteger">1</owl:maxQualifiedCardinality>
                <owl:onClass rdf:resource="https://w3id.org/netbeheer/referentiemodellen/IECCIM/TC57CIM/IEC61970/Base/Domain#Resistance"/>
            </owl:Restriction>
        </rdfs:subClassOf>
        <rdfs:subClassOf>
            <owl:Restriction>
                <owl:onProperty rdf:resource="https://w3id.org/netbeheer/referentiemodellen/IECCIM/TC57CIM/IEC61970/Base/Wires#TransformerMeshImpedance_r0"/>
                <owl:maxQualifiedCardinality rdf:datatype="http://www.w3.org/2001/XMLSchema#nonNegativeInteger">1</owl:maxQualifiedCardinality>
                <owl:onClass rdf:resource="https://w3id.org/netbeheer/referentiemodellen/IECCIM/TC57CIM/IEC61970/Base/Domain#Resistance"/>
            </owl:Restriction>
        </rdfs:subClassOf>
        <rdfs:subClassOf>
            <owl:Restriction>
                <owl:onProperty rdf:resource="https://w3id.org/netbeheer/referentiemodellen/IECCIM/TC57CIM/IEC61970/Base/Wires#TransformerMeshImpedance_x"/>
                <owl:maxQualifiedCardinality rdf:datatype="http://www.w3.org/2001/XMLSchema#nonNegativeInteger">1</owl:maxQualifiedCardinality>
                <owl:onClass rdf:resource="https://w3id.org/netbeheer/referentiemodellen/IECCIM/TC57CIM/IEC61970/Base/Domain#Reactance"/>
            </owl:Restriction>
        </rdfs:subClassOf>
        <rdfs:subClassOf>
            <owl:Restriction>
                <owl:onProperty rdf:resource="https://w3id.org/netbeheer/referentiemodellen/IECCIM/TC57CIM/IEC61970/Base/Wires#TransformerMeshImpedance_x0"/>
                <owl:maxQualifiedCardinality rdf:datatype="http://www.w3.org/2001/XMLSchema#nonNegativeInteger">1</owl:maxQualifiedCardinality>
                <owl:onClass rdf:resource="https://w3id.org/netbeheer/referentiemodellen/IECCIM/TC57CIM/IEC61970/Base/Domain#Reactance"/>
            </owl:Restriction>
        </rdfs:subClassOf>
        <rdfs:comment>Transformer mesh impedance (Delta-model) between transformer ends.
The typical case is that this class describes the impedance between two transformer ends pair-wise, i.e. the cardinalities at both tranformer end associations are 1. But in cases where two or more transformer ends are modeled the cardinalities are larger than 1.
</rdfs:comment>
    </owl:Class>
    


    <!-- https://w3id.org/netbeheer/referentiemodellen/IECCIM/TC57CIM/IEC61970/Base/Wires#TransformerStarImpedance -->


    <owl:Class rdf:about="https://w3id.org/netbeheer/referentiemodellen/IECCIM/TC57CIM/IEC61970/Base/Wires#TransformerStarImpedance">
        <rdfs:subClassOf rdf:resource="https://w3id.org/netbeheer/referentiemodellen/IECCIM/TC57CIM/IEC61970/Base/Core#IdentifiedObject"/>
        <rdfs:subClassOf>
            <owl:Restriction>
                <owl:onProperty rdf:resource="https://w3id.org/netbeheer/referentiemodellen/IECCIM/TC57CIM/IEC61970/Base/Wires#TransformerStarImpedance_TransformerEnd"/>
                <owl:minQualifiedCardinality rdf:datatype="http://www.w3.org/2001/XMLSchema#nonNegativeInteger">0</owl:minQualifiedCardinality>
                <owl:onClass rdf:resource="https://w3id.org/netbeheer/referentiemodellen/IECCIM/TC57CIM/IEC61970/Base/Wires#TransformerStarImpedance"/>
            </owl:Restriction>
        </rdfs:subClassOf>
        <rdfs:subClassOf>
            <owl:Restriction>
                <owl:onProperty rdf:resource="https://w3id.org/netbeheer/referentiemodellen/IECCIM/TC57CIM/IEC61970/Base/Wires#TransformerStarImpedance_TransformerEndInfo"/>
                <owl:minQualifiedCardinality rdf:datatype="http://www.w3.org/2001/XMLSchema#nonNegativeInteger">0</owl:minQualifiedCardinality>
                <owl:onClass rdf:resource="https://w3id.org/netbeheer/referentiemodellen/IECCIM/TC57CIM/IEC61970/Base/Wires#TransformerStarImpedance"/>
            </owl:Restriction>
        </rdfs:subClassOf>
        <rdfs:subClassOf>
            <owl:Restriction>
                <owl:onProperty rdf:resource="https://w3id.org/netbeheer/referentiemodellen/IECCIM/TC57CIM/IEC61970/Base/Wires#TransformerStarImpedance_r"/>
                <owl:minQualifiedCardinality rdf:datatype="http://www.w3.org/2001/XMLSchema#nonNegativeInteger">0</owl:minQualifiedCardinality>
                <owl:onClass rdf:resource="https://w3id.org/netbeheer/referentiemodellen/IECCIM/TC57CIM/IEC61970/Base/Domain#Resistance"/>
            </owl:Restriction>
        </rdfs:subClassOf>
        <rdfs:subClassOf>
            <owl:Restriction>
                <owl:onProperty rdf:resource="https://w3id.org/netbeheer/referentiemodellen/IECCIM/TC57CIM/IEC61970/Base/Wires#TransformerStarImpedance_r0"/>
                <owl:minQualifiedCardinality rdf:datatype="http://www.w3.org/2001/XMLSchema#nonNegativeInteger">0</owl:minQualifiedCardinality>
                <owl:onClass rdf:resource="https://w3id.org/netbeheer/referentiemodellen/IECCIM/TC57CIM/IEC61970/Base/Domain#Resistance"/>
            </owl:Restriction>
        </rdfs:subClassOf>
        <rdfs:subClassOf>
            <owl:Restriction>
                <owl:onProperty rdf:resource="https://w3id.org/netbeheer/referentiemodellen/IECCIM/TC57CIM/IEC61970/Base/Wires#TransformerStarImpedance_x"/>
                <owl:minQualifiedCardinality rdf:datatype="http://www.w3.org/2001/XMLSchema#nonNegativeInteger">0</owl:minQualifiedCardinality>
                <owl:onClass rdf:resource="https://w3id.org/netbeheer/referentiemodellen/IECCIM/TC57CIM/IEC61970/Base/Domain#Reactance"/>
            </owl:Restriction>
        </rdfs:subClassOf>
        <rdfs:subClassOf>
            <owl:Restriction>
                <owl:onProperty rdf:resource="https://w3id.org/netbeheer/referentiemodellen/IECCIM/TC57CIM/IEC61970/Base/Wires#TransformerStarImpedance_x0"/>
                <owl:minQualifiedCardinality rdf:datatype="http://www.w3.org/2001/XMLSchema#nonNegativeInteger">0</owl:minQualifiedCardinality>
                <owl:onClass rdf:resource="https://w3id.org/netbeheer/referentiemodellen/IECCIM/TC57CIM/IEC61970/Base/Domain#Reactance"/>
            </owl:Restriction>
        </rdfs:subClassOf>
        <rdfs:subClassOf>
            <owl:Restriction>
                <owl:onProperty rdf:resource="https://w3id.org/netbeheer/referentiemodellen/IECCIM/TC57CIM/IEC61970/Base/Wires#TransformerStarImpedance_TransformerEnd"/>
                <owl:maxQualifiedCardinality rdf:datatype="http://www.w3.org/2001/XMLSchema#nonNegativeInteger">1</owl:maxQualifiedCardinality>
                <owl:onClass rdf:resource="https://w3id.org/netbeheer/referentiemodellen/IECCIM/TC57CIM/IEC61970/Base/Wires#TransformerStarImpedance"/>
            </owl:Restriction>
        </rdfs:subClassOf>
        <rdfs:subClassOf>
            <owl:Restriction>
                <owl:onProperty rdf:resource="https://w3id.org/netbeheer/referentiemodellen/IECCIM/TC57CIM/IEC61970/Base/Wires#TransformerStarImpedance_TransformerEndInfo"/>
                <owl:maxQualifiedCardinality rdf:datatype="http://www.w3.org/2001/XMLSchema#nonNegativeInteger">1</owl:maxQualifiedCardinality>
                <owl:onClass rdf:resource="https://w3id.org/netbeheer/referentiemodellen/IECCIM/TC57CIM/IEC61970/Base/Wires#TransformerStarImpedance"/>
            </owl:Restriction>
        </rdfs:subClassOf>
        <rdfs:subClassOf>
            <owl:Restriction>
                <owl:onProperty rdf:resource="https://w3id.org/netbeheer/referentiemodellen/IECCIM/TC57CIM/IEC61970/Base/Wires#TransformerStarImpedance_r"/>
                <owl:maxQualifiedCardinality rdf:datatype="http://www.w3.org/2001/XMLSchema#nonNegativeInteger">1</owl:maxQualifiedCardinality>
                <owl:onClass rdf:resource="https://w3id.org/netbeheer/referentiemodellen/IECCIM/TC57CIM/IEC61970/Base/Domain#Resistance"/>
            </owl:Restriction>
        </rdfs:subClassOf>
        <rdfs:subClassOf>
            <owl:Restriction>
                <owl:onProperty rdf:resource="https://w3id.org/netbeheer/referentiemodellen/IECCIM/TC57CIM/IEC61970/Base/Wires#TransformerStarImpedance_r0"/>
                <owl:maxQualifiedCardinality rdf:datatype="http://www.w3.org/2001/XMLSchema#nonNegativeInteger">1</owl:maxQualifiedCardinality>
                <owl:onClass rdf:resource="https://w3id.org/netbeheer/referentiemodellen/IECCIM/TC57CIM/IEC61970/Base/Domain#Resistance"/>
            </owl:Restriction>
        </rdfs:subClassOf>
        <rdfs:subClassOf>
            <owl:Restriction>
                <owl:onProperty rdf:resource="https://w3id.org/netbeheer/referentiemodellen/IECCIM/TC57CIM/IEC61970/Base/Wires#TransformerStarImpedance_x"/>
                <owl:maxQualifiedCardinality rdf:datatype="http://www.w3.org/2001/XMLSchema#nonNegativeInteger">1</owl:maxQualifiedCardinality>
                <owl:onClass rdf:resource="https://w3id.org/netbeheer/referentiemodellen/IECCIM/TC57CIM/IEC61970/Base/Domain#Reactance"/>
            </owl:Restriction>
        </rdfs:subClassOf>
        <rdfs:subClassOf>
            <owl:Restriction>
                <owl:onProperty rdf:resource="https://w3id.org/netbeheer/referentiemodellen/IECCIM/TC57CIM/IEC61970/Base/Wires#TransformerStarImpedance_x0"/>
                <owl:maxQualifiedCardinality rdf:datatype="http://www.w3.org/2001/XMLSchema#nonNegativeInteger">1</owl:maxQualifiedCardinality>
                <owl:onClass rdf:resource="https://w3id.org/netbeheer/referentiemodellen/IECCIM/TC57CIM/IEC61970/Base/Domain#Reactance"/>
            </owl:Restriction>
        </rdfs:subClassOf>
        <rdfs:comment>Transformer star impedance (Pi-model) that accurately reflects impedance for transformers with 2 or 3 windings. For transformers with 4 or more windings, you must use TransformerMeshImpedance class.
For transmission networks use PowerTransformerEnd impedances (r, r0, x, x0, b, b0, g and g0).
</rdfs:comment>
    </owl:Class>
    


    <!-- https://w3id.org/netbeheer/referentiemodellen/IECCIM/TC57CIM/IEC61970/Base/Wires#TransformerTank -->


    <owl:Class rdf:about="https://w3id.org/netbeheer/referentiemodellen/IECCIM/TC57CIM/IEC61970/Base/Wires#TransformerTank">
        <rdfs:subClassOf rdf:resource="https://w3id.org/netbeheer/referentiemodellen/IECCIM/TC57CIM/IEC61970/Base/Core#Equipment"/>
        <rdfs:subClassOf>
            <owl:Restriction>
                <owl:onProperty rdf:resource="https://w3id.org/netbeheer/referentiemodellen/IECCIM/TC57CIM/IEC61970/Base/Wires#TransformerTank_PowerTransformer"/>
                <owl:minQualifiedCardinality rdf:datatype="http://www.w3.org/2001/XMLSchema#nonNegativeInteger">0</owl:minQualifiedCardinality>
                <owl:onClass rdf:resource="https://w3id.org/netbeheer/referentiemodellen/IECCIM/TC57CIM/IEC61970/Base/Wires#TransformerTank"/>
            </owl:Restriction>
        </rdfs:subClassOf>
        <rdfs:subClassOf>
            <owl:Restriction>
                <owl:onProperty rdf:resource="https://w3id.org/netbeheer/referentiemodellen/IECCIM/TC57CIM/IEC61970/Base/Wires#TransformerTank_TransformerObservations"/>
                <owl:minQualifiedCardinality rdf:datatype="http://www.w3.org/2001/XMLSchema#nonNegativeInteger">0</owl:minQualifiedCardinality>
                <owl:onClass rdf:resource="https://w3id.org/netbeheer/referentiemodellen/IECCIM/TC57CIM/IEC61970/Base/Wires#TransformerTank"/>
            </owl:Restriction>
        </rdfs:subClassOf>
        <rdfs:subClassOf>
            <owl:Restriction>
                <owl:onProperty rdf:resource="https://w3id.org/netbeheer/referentiemodellen/IECCIM/TC57CIM/IEC61970/Base/Wires#TransformerTank_TransformerTankEnds"/>
                <owl:minQualifiedCardinality rdf:datatype="http://www.w3.org/2001/XMLSchema#nonNegativeInteger">0</owl:minQualifiedCardinality>
                <owl:onClass rdf:resource="https://w3id.org/netbeheer/referentiemodellen/IECCIM/TC57CIM/IEC61970/Base/Wires#TransformerTank"/>
            </owl:Restriction>
        </rdfs:subClassOf>
        <rdfs:subClassOf>
            <owl:Restriction>
                <owl:onProperty rdf:resource="https://w3id.org/netbeheer/referentiemodellen/IECCIM/TC57CIM/IEC61970/Base/Wires#TransformerTank_TransformerObservations"/>
                <owl:maxQualifiedCardinality rdf:datatype="http://www.w3.org/2001/XMLSchema#nonNegativeInteger">1</owl:maxQualifiedCardinality>
                <owl:onClass rdf:resource="https://w3id.org/netbeheer/referentiemodellen/IECCIM/TC57CIM/IEC61970/Base/Wires#TransformerTank"/>
            </owl:Restriction>
        </rdfs:subClassOf>
        <rdfs:subClassOf>
            <owl:Restriction>
                <owl:onProperty rdf:resource="https://w3id.org/netbeheer/referentiemodellen/IECCIM/TC57CIM/IEC61970/Base/Wires#TransformerTank_TransformerTankEnds"/>
                <owl:maxQualifiedCardinality rdf:datatype="http://www.w3.org/2001/XMLSchema#nonNegativeInteger">1</owl:maxQualifiedCardinality>
                <owl:onClass rdf:resource="https://w3id.org/netbeheer/referentiemodellen/IECCIM/TC57CIM/IEC61970/Base/Wires#TransformerTank"/>
            </owl:Restriction>
        </rdfs:subClassOf>
        <rdfs:comment>An assembly of two or more coupled windings that transform electrical power between voltage levels. These windings are bound on a common core and place in the same tank. Transformer tank can be used to model both single-phase and 3-phase transformers.
</rdfs:comment>
    </owl:Class>
    


    <!-- https://w3id.org/netbeheer/referentiemodellen/IECCIM/TC57CIM/IEC61970/Base/Wires#TransformerTankEnd -->


    <owl:Class rdf:about="https://w3id.org/netbeheer/referentiemodellen/IECCIM/TC57CIM/IEC61970/Base/Wires#TransformerTankEnd">
        <rdfs:subClassOf rdf:resource="https://w3id.org/netbeheer/referentiemodellen/IECCIM/TC57CIM/IEC61970/Base/Wires#TransformerEnd"/>
        <rdfs:subClassOf>
            <owl:Restriction>
                <owl:onProperty rdf:resource="https://w3id.org/netbeheer/referentiemodellen/IECCIM/TC57CIM/IEC61970/Base/Wires#TransformerTankEnd_TransformerTank"/>
                <owl:minQualifiedCardinality rdf:datatype="http://www.w3.org/2001/XMLSchema#nonNegativeInteger">1</owl:minQualifiedCardinality>
                <owl:onClass rdf:resource="https://w3id.org/netbeheer/referentiemodellen/IECCIM/TC57CIM/IEC61970/Base/Wires#TransformerTankEnd"/>
            </owl:Restriction>
        </rdfs:subClassOf>
        <rdfs:subClassOf>
            <owl:Restriction>
                <owl:onProperty rdf:resource="https://w3id.org/netbeheer/referentiemodellen/IECCIM/TC57CIM/IEC61970/Base/Wires#TransformerTankEnd_phases"/>
                <owl:minQualifiedCardinality rdf:datatype="http://www.w3.org/2001/XMLSchema#nonNegativeInteger">0</owl:minQualifiedCardinality>
                <owl:onDataRange rdf:resource="https://w3id.org/netbeheer/referentiemodellen/IECCIM/TC57CIM/IEC61970/Base/Core#PhaseCode"/>
            </owl:Restriction>
        </rdfs:subClassOf>
        <rdfs:subClassOf>
            <owl:Restriction>
                <owl:onProperty rdf:resource="https://w3id.org/netbeheer/referentiemodellen/IECCIM/TC57CIM/IEC61970/Base/Wires#TransformerTankEnd_phases"/>
                <owl:maxQualifiedCardinality rdf:datatype="http://www.w3.org/2001/XMLSchema#nonNegativeInteger">1</owl:maxQualifiedCardinality>
                <owl:onDataRange rdf:resource="https://w3id.org/netbeheer/referentiemodellen/IECCIM/TC57CIM/IEC61970/Base/Core#PhaseCode"/>
            </owl:Restriction>
        </rdfs:subClassOf>
        <rdfs:comment>Transformer tank end represents an individual winding for unbalanced models or for transformer tanks connected into a bank (and bank is modelled with the PowerTransformer).
</rdfs:comment>
    </owl:Class>
    


    <!-- https://w3id.org/netbeheer/referentiemodellen/IECCIM/TC57CIM/IEC61970/Base/Wires#VoltageControlZone -->


    <owl:Class rdf:about="https://w3id.org/netbeheer/referentiemodellen/IECCIM/TC57CIM/IEC61970/Base/Wires#VoltageControlZone">
        <rdfs:subClassOf rdf:resource="https://w3id.org/netbeheer/referentiemodellen/IECCIM/TC57CIM/IEC61970/Base/Core#PowerSystemResource"/>
        <rdfs:subClassOf>
            <owl:Restriction>
                <owl:onProperty rdf:resource="https://w3id.org/netbeheer/referentiemodellen/IECCIM/TC57CIM/IEC61970/Base/Wires#VoltageControlZone_BusbarSection"/>
                <owl:minQualifiedCardinality rdf:datatype="http://www.w3.org/2001/XMLSchema#nonNegativeInteger">0</owl:minQualifiedCardinality>
                <owl:onClass rdf:resource="https://w3id.org/netbeheer/referentiemodellen/IECCIM/TC57CIM/IEC61970/Base/Wires#VoltageControlZone"/>
            </owl:Restriction>
        </rdfs:subClassOf>
        <rdfs:subClassOf>
            <owl:Restriction>
                <owl:onProperty rdf:resource="https://w3id.org/netbeheer/referentiemodellen/IECCIM/TC57CIM/IEC61970/Base/Wires#VoltageControlZone_RegulationSchedule"/>
                <owl:minQualifiedCardinality rdf:datatype="http://www.w3.org/2001/XMLSchema#nonNegativeInteger">0</owl:minQualifiedCardinality>
                <owl:onClass rdf:resource="https://w3id.org/netbeheer/referentiemodellen/IECCIM/TC57CIM/IEC61970/Base/Wires#VoltageControlZone"/>
            </owl:Restriction>
        </rdfs:subClassOf>
        <rdfs:subClassOf>
            <owl:Restriction>
                <owl:onProperty rdf:resource="https://w3id.org/netbeheer/referentiemodellen/IECCIM/TC57CIM/IEC61970/Base/Wires#VoltageControlZone_BusbarSection"/>
                <owl:maxQualifiedCardinality rdf:datatype="http://www.w3.org/2001/XMLSchema#nonNegativeInteger">1</owl:maxQualifiedCardinality>
                <owl:onClass rdf:resource="https://w3id.org/netbeheer/referentiemodellen/IECCIM/TC57CIM/IEC61970/Base/Wires#VoltageControlZone"/>
            </owl:Restriction>
        </rdfs:subClassOf>
        <rdfs:comment>An area of the power system network which is defined for secondary voltage control purposes. A voltage control zone consists of a collection of substations with a designated bus bar section whose voltage will be controlled.</rdfs:comment>
    </owl:Class>
    


    <!-- https://w3id.org/netbeheer/referentiemodellen/IECCIM/TC57CIM/IEC61970/Dynamics/StandardModels/AsynchronousMachineDynamics#AsynchronousMachineDynamics -->


    <owl:Class rdf:about="https://w3id.org/netbeheer/referentiemodellen/IECCIM/TC57CIM/IEC61970/Dynamics/StandardModels/AsynchronousMachineDynamics#AsynchronousMachineDynamics">
        <rdfs:subClassOf>
            <owl:Restriction>
                <owl:onProperty rdf:resource="https://w3id.org/netbeheer/referentiemodellen/IECCIM/TC57CIM/IEC61970/Base/Wires#AsynchronousMachineDynamics_AsynchronousMachine"/>
                <owl:minQualifiedCardinality rdf:datatype="http://www.w3.org/2001/XMLSchema#nonNegativeInteger">0</owl:minQualifiedCardinality>
                <owl:onClass rdf:resource="https://w3id.org/netbeheer/referentiemodellen/IECCIM/TC57CIM/IEC61970/Dynamics/StandardModels/AsynchronousMachineDynamics#AsynchronousMachineDynamics"/>
            </owl:Restriction>
        </rdfs:subClassOf>
        <rdfs:subClassOf>
            <owl:Restriction>
                <owl:onProperty rdf:resource="https://w3id.org/netbeheer/referentiemodellen/IECCIM/TC57CIM/IEC61970/Base/Wires#AsynchronousMachineDynamics_AsynchronousMachine"/>
                <owl:maxQualifiedCardinality rdf:datatype="http://www.w3.org/2001/XMLSchema#nonNegativeInteger">1</owl:maxQualifiedCardinality>
                <owl:onClass rdf:resource="https://w3id.org/netbeheer/referentiemodellen/IECCIM/TC57CIM/IEC61970/Dynamics/StandardModels/AsynchronousMachineDynamics#AsynchronousMachineDynamics"/>
            </owl:Restriction>
        </rdfs:subClassOf>
    </owl:Class>
    


    <!-- https://w3id.org/netbeheer/referentiemodellen/IECCIM/TC57CIM/IEC61970/Dynamics/StandardModels/LoadDynamics#LoadDynamics -->


    <owl:Class rdf:about="https://w3id.org/netbeheer/referentiemodellen/IECCIM/TC57CIM/IEC61970/Dynamics/StandardModels/LoadDynamics#LoadDynamics">
        <rdfs:subClassOf>
            <owl:Restriction>
                <owl:onProperty rdf:resource="https://w3id.org/netbeheer/referentiemodellen/IECCIM/TC57CIM/IEC61970/Base/Wires#LoadDynamics_EnergyConsumer"/>
                <owl:minQualifiedCardinality rdf:datatype="http://www.w3.org/2001/XMLSchema#nonNegativeInteger">0</owl:minQualifiedCardinality>
                <owl:onClass rdf:resource="https://w3id.org/netbeheer/referentiemodellen/IECCIM/TC57CIM/IEC61970/Dynamics/StandardModels/LoadDynamics#LoadDynamics"/>
            </owl:Restriction>
        </rdfs:subClassOf>
        <rdfs:subClassOf>
            <owl:Restriction>
                <owl:onProperty rdf:resource="https://w3id.org/netbeheer/referentiemodellen/IECCIM/TC57CIM/IEC61970/Base/Wires#LoadDynamics_EnergyConsumer"/>
                <owl:maxQualifiedCardinality rdf:datatype="http://www.w3.org/2001/XMLSchema#nonNegativeInteger">1</owl:maxQualifiedCardinality>
                <owl:onClass rdf:resource="https://w3id.org/netbeheer/referentiemodellen/IECCIM/TC57CIM/IEC61970/Dynamics/StandardModels/LoadDynamics#LoadDynamics"/>
            </owl:Restriction>
        </rdfs:subClassOf>
    </owl:Class>
    


    <!-- https://w3id.org/netbeheer/referentiemodellen/IECCIM/TC57CIM/IEC61970/Dynamics/StandardModels/SynchronousMachineDynamics#SynchronousMachineDynamics -->


    <owl:Class rdf:about="https://w3id.org/netbeheer/referentiemodellen/IECCIM/TC57CIM/IEC61970/Dynamics/StandardModels/SynchronousMachineDynamics#SynchronousMachineDynamics">
        <rdfs:subClassOf>
            <owl:Restriction>
                <owl:onProperty rdf:resource="https://w3id.org/netbeheer/referentiemodellen/IECCIM/TC57CIM/IEC61970/Base/Wires#SynchronousMachineDynamics_SynchronousMachine"/>
                <owl:minQualifiedCardinality rdf:datatype="http://www.w3.org/2001/XMLSchema#nonNegativeInteger">0</owl:minQualifiedCardinality>
                <owl:onClass rdf:resource="https://w3id.org/netbeheer/referentiemodellen/IECCIM/TC57CIM/IEC61970/Dynamics/StandardModels/SynchronousMachineDynamics#SynchronousMachineDynamics"/>
            </owl:Restriction>
        </rdfs:subClassOf>
        <rdfs:subClassOf>
            <owl:Restriction>
                <owl:onProperty rdf:resource="https://w3id.org/netbeheer/referentiemodellen/IECCIM/TC57CIM/IEC61970/Base/Wires#SynchronousMachineDynamics_SynchronousMachine"/>
                <owl:maxQualifiedCardinality rdf:datatype="http://www.w3.org/2001/XMLSchema#nonNegativeInteger">1</owl:maxQualifiedCardinality>
                <owl:onClass rdf:resource="https://w3id.org/netbeheer/referentiemodellen/IECCIM/TC57CIM/IEC61970/Dynamics/StandardModels/SynchronousMachineDynamics#SynchronousMachineDynamics"/>
            </owl:Restriction>
        </rdfs:subClassOf>
    </owl:Class>
    


    <!-- https://w3id.org/netbeheer/referentiemodellen/IECCIM/TC57CIM/IEC61970/Dynamics/StandardModels/WindDynamics#WindTurbineType3or4Dynamics -->


    <owl:Class rdf:about="https://w3id.org/netbeheer/referentiemodellen/IECCIM/TC57CIM/IEC61970/Dynamics/StandardModels/WindDynamics#WindTurbineType3or4Dynamics">
        <rdfs:subClassOf>
            <owl:Restriction>
                <owl:onProperty rdf:resource="https://w3id.org/netbeheer/referentiemodellen/IECCIM/TC57CIM/IEC61970/Base/Wires#WindTurbineType3or4Dynamics_EnergySource"/>
                <owl:minQualifiedCardinality rdf:datatype="http://www.w3.org/2001/XMLSchema#nonNegativeInteger">0</owl:minQualifiedCardinality>
                <owl:onClass rdf:resource="https://w3id.org/netbeheer/referentiemodellen/IECCIM/TC57CIM/IEC61970/Dynamics/StandardModels/WindDynamics#WindTurbineType3or4Dynamics"/>
            </owl:Restriction>
        </rdfs:subClassOf>
        <rdfs:subClassOf>
            <owl:Restriction>
                <owl:onProperty rdf:resource="https://w3id.org/netbeheer/referentiemodellen/IECCIM/TC57CIM/IEC61970/Base/Wires#WindTurbineType3or4Dynamics_EnergySource"/>
                <owl:maxQualifiedCardinality rdf:datatype="http://www.w3.org/2001/XMLSchema#nonNegativeInteger">1</owl:maxQualifiedCardinality>
                <owl:onClass rdf:resource="https://w3id.org/netbeheer/referentiemodellen/IECCIM/TC57CIM/IEC61970/Dynamics/StandardModels/WindDynamics#WindTurbineType3or4Dynamics"/>
            </owl:Restriction>
        </rdfs:subClassOf>
    </owl:Class>
    


    <!-- https://w3id.org/netbeheer/referentiemodellen/IECCIM/TC57CIM/IEC61970/InfIEC61970/InfEnergySource#EnergySchedulingType -->


    <owl:Class rdf:about="https://w3id.org/netbeheer/referentiemodellen/IECCIM/TC57CIM/IEC61970/InfIEC61970/InfEnergySource#EnergySchedulingType">
        <rdfs:subClassOf>
            <owl:Restriction>
                <owl:onProperty rdf:resource="https://w3id.org/netbeheer/referentiemodellen/IECCIM/TC57CIM/IEC61970/Base/Wires#EnergySchedulingType_EnergySource"/>
                <owl:minQualifiedCardinality rdf:datatype="http://www.w3.org/2001/XMLSchema#nonNegativeInteger">0</owl:minQualifiedCardinality>
                <owl:onClass rdf:resource="https://w3id.org/netbeheer/referentiemodellen/IECCIM/TC57CIM/IEC61970/InfIEC61970/InfEnergySource#EnergySchedulingType"/>
            </owl:Restriction>
        </rdfs:subClassOf>
        <rdfs:subClassOf>
            <owl:Restriction>
                <owl:onProperty rdf:resource="https://w3id.org/netbeheer/referentiemodellen/IECCIM/TC57CIM/IEC61970/Base/Wires#EnergySchedulingType_EnergySource"/>
                <owl:maxQualifiedCardinality rdf:datatype="http://www.w3.org/2001/XMLSchema#nonNegativeInteger">1</owl:maxQualifiedCardinality>
                <owl:onClass rdf:resource="https://w3id.org/netbeheer/referentiemodellen/IECCIM/TC57CIM/IEC61970/InfIEC61970/InfEnergySource#EnergySchedulingType"/>
            </owl:Restriction>
        </rdfs:subClassOf>
    </owl:Class>
    


    <!-- https://w3id.org/netbeheer/referentiemodellen/IECCIM/TC57CIM/IEC61970/InfIEC61970/InfSIPS#ProtectiveActionRegulation -->


    <owl:Class rdf:about="https://w3id.org/netbeheer/referentiemodellen/IECCIM/TC57CIM/IEC61970/InfIEC61970/InfSIPS#ProtectiveActionRegulation">
        <rdfs:subClassOf>
            <owl:Restriction>
                <owl:onProperty rdf:resource="https://w3id.org/netbeheer/referentiemodellen/IECCIM/TC57CIM/IEC61970/Base/Wires#ProtectiveActionRegulation_RegulatingControl"/>
                <owl:minQualifiedCardinality rdf:datatype="http://www.w3.org/2001/XMLSchema#nonNegativeInteger">0</owl:minQualifiedCardinality>
                <owl:onClass rdf:resource="https://w3id.org/netbeheer/referentiemodellen/IECCIM/TC57CIM/IEC61970/InfIEC61970/InfSIPS#ProtectiveActionRegulation"/>
            </owl:Restriction>
        </rdfs:subClassOf>
    </owl:Class>
</rdf:RDF>



<!-- Generated by the OWL API (version 5.1.10.2019-03-12T22:31:15Z) https://github.com/owlcs/owlapi/ -->


