@prefix : <https://w3id.org/netbeheer/IECCIM/TC57CIM/IEC61970/Base/Generation/Production#> .
@prefix owl: <http://www.w3.org/2002/07/owl#> .
@prefix rdf: <http://www.w3.org/1999/02/22-rdf-syntax-ns#> .
@prefix xml: <http://www.w3.org/XML/1998/namespace> .
@prefix xsd: <http://www.w3.org/2001/XMLSchema#> .
@prefix rdfs: <http://www.w3.org/2000/01/rdf-schema#> .
@base <https://w3id.org/netbeheer/IECCIM/TC57CIM/IEC61970/Base/Generation/Production#> .

<https://w3id.org/netbeheer/IECCIM/TC57CIM/IEC61970/Base/Generation/Production#> rdf:type owl:Ontology .

#################################################################
#    Datatypes
#################################################################

###  https://w3id.org/netbeheer/IECCIM/TC57CIM/IEC61970/Base/Domain#Currency
<https://w3id.org/netbeheer/IECCIM/TC57CIM/IEC61970/Base/Domain#Currency> rdf:type rdfs:Datatype .


###  https://w3id.org/netbeheer/IECCIM/TC57CIM/IEC61970/Base/Domain#UnitMultiplier
<https://w3id.org/netbeheer/IECCIM/TC57CIM/IEC61970/Base/Domain#UnitMultiplier> rdf:type rdfs:Datatype .


###  https://w3id.org/netbeheer/IECCIM/TC57CIM/IEC61970/Base/Domain#UnitSymbol
<https://w3id.org/netbeheer/IECCIM/TC57CIM/IEC61970/Base/Domain#UnitSymbol> rdf:type rdfs:Datatype .


###  https://w3id.org/netbeheer/IECCIM/TC57CIM/IEC61970/Base/Generation/Production#EmissionType
:EmissionType rdf:type rdfs:Datatype ;
              owl:equivalentClass [ rdf:type rdfs:Datatype ;
                                    owl:oneOf [ rdf:type rdf:List ;
                                                rdf:first "carbonDioxide" ;
                                                rdf:rest [ rdf:type rdf:List ;
                                                           rdf:first "carbonDisulfide" ;
                                                           rdf:rest [ rdf:type rdf:List ;
                                                                      rdf:first "chlorine" ;
                                                                      rdf:rest [ rdf:type rdf:List ;
                                                                                 rdf:first "hydrogenSulfide" ;
                                                                                 rdf:rest [ rdf:type rdf:List ;
                                                                                            rdf:first "nitrogenOxide" ;
                                                                                            rdf:rest rdf:nil
                                                                                          ]
                                                                               ]
                                                                    ]
                                                         ]
                                              ]
                                  ] .


###  https://w3id.org/netbeheer/IECCIM/TC57CIM/IEC61970/Base/Generation/Production#EmissionValueSource
:EmissionValueSource rdf:type rdfs:Datatype ;
                     owl:equivalentClass [ rdf:type rdfs:Datatype ;
                                           owl:oneOf [ rdf:type rdf:List ;
                                                       rdf:first "calculated" ;
                                                       rdf:rest [ rdf:type rdf:List ;
                                                                  rdf:first "measured" ;
                                                                  rdf:rest rdf:nil
                                                                ]
                                                     ]
                                         ] .


###  https://w3id.org/netbeheer/IECCIM/TC57CIM/IEC61970/Base/Generation/Production#FuelType
:FuelType rdf:type rdfs:Datatype ;
          owl:equivalentClass [ rdf:type rdfs:Datatype ;
                                owl:oneOf [ rdf:type rdf:List ;
                                            rdf:first "coal" ;
                                            rdf:rest [ rdf:type rdf:List ;
                                                       rdf:first "gas" ;
                                                       rdf:rest [ rdf:type rdf:List ;
                                                                  rdf:first "hardCoal" ;
                                                                  rdf:rest [ rdf:type rdf:List ;
                                                                             rdf:first "lignite" ;
                                                                             rdf:rest [ rdf:type rdf:List ;
                                                                                        rdf:first "oil" ;
                                                                                        rdf:rest [ rdf:type rdf:List ;
                                                                                                   rdf:first "oilShale" ;
                                                                                                   rdf:rest rdf:nil
                                                                                                 ]
                                                                                      ]
                                                                           ]
                                                                ]
                                                     ]
                                          ]
                              ] .


###  https://w3id.org/netbeheer/IECCIM/TC57CIM/IEC61970/Base/Generation/Production#GeneratorControlMode
:GeneratorControlMode rdf:type rdfs:Datatype ;
                      owl:equivalentClass [ rdf:type rdfs:Datatype ;
                                            owl:oneOf [ rdf:type rdf:List ;
                                                        rdf:first "pulse" ;
                                                        rdf:rest [ rdf:type rdf:List ;
                                                                   rdf:first "setpoint" ;
                                                                   rdf:rest rdf:nil
                                                                 ]
                                                      ]
                                          ] .


###  https://w3id.org/netbeheer/IECCIM/TC57CIM/IEC61970/Base/Generation/Production#GeneratorControlSource
:GeneratorControlSource rdf:type rdfs:Datatype ;
                        owl:equivalentClass [ rdf:type rdfs:Datatype ;
                                              owl:oneOf [ rdf:type rdf:List ;
                                                          rdf:first "offAGC" ;
                                                          rdf:rest [ rdf:type rdf:List ;
                                                                     rdf:first "onAGC" ;
                                                                     rdf:rest [ rdf:type rdf:List ;
                                                                                rdf:first "plantControl" ;
                                                                                rdf:rest [ rdf:type rdf:List ;
                                                                                           rdf:first "unavailable" ;
                                                                                           rdf:rest rdf:nil
                                                                                         ]
                                                                              ]
                                                                   ]
                                                        ]
                                            ] .


###  https://w3id.org/netbeheer/IECCIM/TC57CIM/IEC61970/Base/Generation/Production#HydroEnergyConversionKind
:HydroEnergyConversionKind rdf:type rdfs:Datatype ;
                           owl:equivalentClass [ rdf:type rdfs:Datatype ;
                                                 owl:oneOf [ rdf:type rdf:List ;
                                                             rdf:first "generator" ;
                                                             rdf:rest [ rdf:type rdf:List ;
                                                                        rdf:first "pumpAndGenerator" ;
                                                                        rdf:rest rdf:nil
                                                                      ]
                                                           ]
                                               ] .


###  https://w3id.org/netbeheer/IECCIM/TC57CIM/IEC61970/Base/Generation/Production#HydroPlantStorageKind
:HydroPlantStorageKind rdf:type rdfs:Datatype ;
                       owl:equivalentClass [ rdf:type rdfs:Datatype ;
                                             owl:oneOf [ rdf:type rdf:List ;
                                                         rdf:first "pumpedStorage" ;
                                                         rdf:rest [ rdf:type rdf:List ;
                                                                    rdf:first "runOfRiver" ;
                                                                    rdf:rest [ rdf:type rdf:List ;
                                                                               rdf:first "storage" ;
                                                                               rdf:rest rdf:nil
                                                                             ]
                                                                  ]
                                                       ]
                                           ] .


###  https://w3id.org/netbeheer/IECCIM/TC57CIM/IEC61970/Base/Generation/Production#WindGenUnitKind
:WindGenUnitKind rdf:type rdfs:Datatype ;
                 owl:equivalentClass [ rdf:type rdfs:Datatype ;
                                       owl:oneOf [ rdf:type rdf:List ;
                                                   rdf:first "offshore" ;
                                                   rdf:rest [ rdf:type rdf:List ;
                                                              rdf:first "onshore" ;
                                                              rdf:rest rdf:nil
                                                            ]
                                                 ]
                                     ] .


#################################################################
#    Object Properties
#################################################################

###  https://w3id.org/netbeheer/IECCIM/TC57CIM/IEC61970/Base/Generation/Production#AirCompressor_CAESPlant
:AirCompressor_CAESPlant rdf:type owl:ObjectProperty ;
                         owl:inverseOf :CAESPlant_AirCompressor ;
                         rdf:type owl:FunctionalProperty ;
                         rdfs:domain :AirCompressor ;
                         rdfs:range :CAESPlant ;
                         rdfs:comment "An air compressor may be a member of a compressed air energy storage plant.An air compressor may be a member of a compressed air energy storage plant." .


###  https://w3id.org/netbeheer/IECCIM/TC57CIM/IEC61970/Base/Generation/Production#CAESPlant_AirCompressor
:CAESPlant_AirCompressor rdf:type owl:ObjectProperty ,
                                  owl:FunctionalProperty ;
                         rdfs:domain :CAESPlant ;
                         rdfs:range :AirCompressor ;
                         rdfs:comment "An air compressor may be a member of a compressed air energy storage plant.An air compressor may be a member of a compressed air energy storage plant." .


###  https://w3id.org/netbeheer/IECCIM/TC57CIM/IEC61970/Base/Generation/Production#CAESPlant_ThermalGeneratingUnit
:CAESPlant_ThermalGeneratingUnit rdf:type owl:ObjectProperty ;
                                 rdfs:domain :CAESPlant ;
                                 rdfs:range :ThermalGeneratingUnit ;
                                 rdfs:comment "A thermal generating unit may be a member of a compressed air energy storage plant.A thermal generating unit may be a member of a compressed air energy storage plant." .


###  https://w3id.org/netbeheer/IECCIM/TC57CIM/IEC61970/Base/Generation/Production#CAESPlant_energyStorageCapacity
:CAESPlant_energyStorageCapacity rdf:type owl:ObjectProperty ;
                                 rdfs:domain :CAESPlant ;
                                 rdfs:range <https://w3id.org/netbeheer/IECCIM/TC57CIM/IEC61970/Base/Domain#RealEnergy> ;
                                 rdfs:comment "The rated energy storage capacity." .


###  https://w3id.org/netbeheer/IECCIM/TC57CIM/IEC61970/Base/Generation/Production#CAESPlant_ratedCapacityP
:CAESPlant_ratedCapacityP rdf:type owl:ObjectProperty ;
                          rdfs:domain :CAESPlant ;
                          rdfs:range <https://w3id.org/netbeheer/IECCIM/TC57CIM/IEC61970/Base/Domain#ActivePower> ;
                          rdfs:comment """The CAES plant's gross rated generating capacity.
""" .


###  https://w3id.org/netbeheer/IECCIM/TC57CIM/IEC61970/Base/Generation/Production#CogenerationPlant_SteamSendoutSchedule
:CogenerationPlant_SteamSendoutSchedule rdf:type owl:ObjectProperty ;
                                        owl:inverseOf :SteamSendoutSchedule_CogenerationPlant ;
                                        rdf:type owl:FunctionalProperty ;
                                        rdfs:domain :CogenerationPlant ;
                                        rdfs:range :SteamSendoutSchedule ;
                                        rdfs:comment "A cogeneration plant has a steam sendout schedule.A cogeneration plant has a steam sendout schedule." .


###  https://w3id.org/netbeheer/IECCIM/TC57CIM/IEC61970/Base/Generation/Production#CogenerationPlant_ThermalGeneratingUnits
:CogenerationPlant_ThermalGeneratingUnits rdf:type owl:ObjectProperty ;
                                          rdfs:domain :CogenerationPlant ;
                                          rdfs:range :ThermalGeneratingUnit ;
                                          rdfs:comment "A thermal generating unit may be a member of a cogeneration plant.A thermal generating unit may be a member of a cogeneration plant." .


###  https://w3id.org/netbeheer/IECCIM/TC57CIM/IEC61970/Base/Generation/Production#CogenerationPlant_ratedP
:CogenerationPlant_ratedP rdf:type owl:ObjectProperty ;
                          rdfs:domain :CogenerationPlant ;
                          rdfs:range <https://w3id.org/netbeheer/IECCIM/TC57CIM/IEC61970/Base/Domain#ActivePower> ;
                          rdfs:comment """The rated output active power of the cogeneration plant.
""" .


###  https://w3id.org/netbeheer/IECCIM/TC57CIM/IEC61970/Base/Generation/Production#CombinedCyclePlant_ThermalGeneratingUnits
:CombinedCyclePlant_ThermalGeneratingUnits rdf:type owl:ObjectProperty ;
                                           rdfs:domain :CombinedCyclePlant ;
                                           rdfs:range :ThermalGeneratingUnit ;
                                           rdfs:comment "A thermal generating unit may be a member of a combined cycle plant.A thermal generating unit may be a member of a combined cycle plant." .


###  https://w3id.org/netbeheer/IECCIM/TC57CIM/IEC61970/Base/Generation/Production#CombinedCyclePlant_combCyclePlantRating
:CombinedCyclePlant_combCyclePlantRating rdf:type owl:ObjectProperty ;
                                         rdfs:domain :CombinedCyclePlant ;
                                         rdfs:range <https://w3id.org/netbeheer/IECCIM/TC57CIM/IEC61970/Base/Domain#ActivePower> ;
                                         rdfs:comment """The combined cycle plant's active power output rating.
""" .


###  https://w3id.org/netbeheer/IECCIM/TC57CIM/IEC61970/Base/Generation/Production#ControlAreaGeneratingUnit_GeneratingUnit
:ControlAreaGeneratingUnit_GeneratingUnit rdf:type owl:ObjectProperty ;
                                          rdfs:domain <https://w3id.org/netbeheer/IECCIM/TC57CIM/IEC61970/Base/ControlArea#ControlAreaGeneratingUnit> ;
                                          rdfs:range :GeneratingUnit ;
                                          rdfs:comment "ControlArea specifications for this generating unit.The generating unit specified for this control area.  Note that a control area should include a GeneratingUnit only once." .


###  https://w3id.org/netbeheer/IECCIM/TC57CIM/IEC61970/Base/Generation/Production#EmissionAccount_ThermalGeneratingUnit
:EmissionAccount_ThermalGeneratingUnit rdf:type owl:ObjectProperty ;
                                       rdfs:domain :EmissionAccount ;
                                       rdfs:range :ThermalGeneratingUnit ;
                                       rdfs:comment "A thermal generating unit may have one or more emission allowance accounts.A thermal generating unit may have one or more emission allowance accounts." .


###  https://w3id.org/netbeheer/IECCIM/TC57CIM/IEC61970/Base/Generation/Production#EmissionCurve_ThermalGeneratingUnit
:EmissionCurve_ThermalGeneratingUnit rdf:type owl:ObjectProperty ;
                                     rdfs:domain :EmissionCurve ;
                                     rdfs:range :ThermalGeneratingUnit ;
                                     rdfs:comment "A thermal generating unit may have  one or more emission curves.A thermal generating unit may have  one or more emission curves." .


###  https://w3id.org/netbeheer/IECCIM/TC57CIM/IEC61970/Base/Generation/Production#EmissionCurve_emissionContent
:EmissionCurve_emissionContent rdf:type owl:ObjectProperty ;
                               rdfs:domain :EmissionCurve ;
                               rdfs:range :Emission ;
                               rdfs:comment """The emission content per quantity of fuel burned.
""" .


###  https://w3id.org/netbeheer/IECCIM/TC57CIM/IEC61970/Base/Generation/Production#FossilFuel_FuelAllocationSchedules
:FossilFuel_FuelAllocationSchedules rdf:type owl:ObjectProperty ,
                                             owl:FunctionalProperty ;
                                    rdfs:domain :FossilFuel ;
                                    rdfs:range :FuelAllocationSchedule ;
                                    rdfs:comment "A fuel allocation schedule must have a fossil fuel.A fuel allocation schedule must have a fossil fuel." .


###  https://w3id.org/netbeheer/IECCIM/TC57CIM/IEC61970/Base/Generation/Production#FossilFuel_ThermalGeneratingUnit
:FossilFuel_ThermalGeneratingUnit rdf:type owl:ObjectProperty ;
                                  rdfs:domain :FossilFuel ;
                                  rdfs:range :ThermalGeneratingUnit ;
                                  rdfs:comment "A thermal generating unit may have one or more fossil fuels.A thermal generating unit may have one or more fossil fuels." .


###  https://w3id.org/netbeheer/IECCIM/TC57CIM/IEC61970/Base/Generation/Production#FossilFuel_fuelCost
:FossilFuel_fuelCost rdf:type owl:ObjectProperty ;
                     rdfs:domain :FossilFuel ;
                     rdfs:range :CostPerHeatUnit ;
                     rdfs:comment """The cost in terms of heat value for the given type of fuel.
""" .


###  https://w3id.org/netbeheer/IECCIM/TC57CIM/IEC61970/Base/Generation/Production#FossilFuel_fuelDispatchCost
:FossilFuel_fuelDispatchCost rdf:type owl:ObjectProperty ;
                             rdfs:domain :FossilFuel ;
                             rdfs:range :CostPerHeatUnit ;
                             rdfs:comment """The cost of fuel used for economic dispatching which includes: fuel cost, transportation cost,  and incremental maintenance cost.
""" .


###  https://w3id.org/netbeheer/IECCIM/TC57CIM/IEC61970/Base/Generation/Production#FossilFuel_fuelEffFactor
:FossilFuel_fuelEffFactor rdf:type owl:ObjectProperty ;
                          rdfs:domain :FossilFuel ;
                          rdfs:range <https://w3id.org/netbeheer/IECCIM/TC57CIM/IEC61970/Base/Domain#PU> ;
                          rdfs:comment """The efficiency factor for the fuel (per unit) in terms of the effective energy absorbed.
""" .


###  https://w3id.org/netbeheer/IECCIM/TC57CIM/IEC61970/Base/Generation/Production#FossilFuel_fuelHandlingCost
:FossilFuel_fuelHandlingCost rdf:type owl:ObjectProperty ;
                             rdfs:domain :FossilFuel ;
                             rdfs:range :CostPerHeatUnit ;
                             rdfs:comment """Handling and processing cost associated with this fuel.
""" .


###  https://w3id.org/netbeheer/IECCIM/TC57CIM/IEC61970/Base/Generation/Production#FossilFuel_fuelMixture
:FossilFuel_fuelMixture rdf:type owl:ObjectProperty ;
                        rdfs:domain :FossilFuel ;
                        rdfs:range <https://w3id.org/netbeheer/IECCIM/TC57CIM/IEC61970/Base/Domain#PerCent> ;
                        rdfs:comment "Relative amount of the given type of fuel, when multiple fuels are being consumed." .


###  https://w3id.org/netbeheer/IECCIM/TC57CIM/IEC61970/Base/Generation/Production#FossilFuel_fuelSulfur
:FossilFuel_fuelSulfur rdf:type owl:ObjectProperty ;
                       rdfs:domain :FossilFuel ;
                       rdfs:range <https://w3id.org/netbeheer/IECCIM/TC57CIM/IEC61970/Base/Domain#PU> ;
                       rdfs:comment """The fuel's fraction of pollution credit per unit of heat content.
""" .


###  https://w3id.org/netbeheer/IECCIM/TC57CIM/IEC61970/Base/Generation/Production#FossilFuel_highBreakpointP
:FossilFuel_highBreakpointP rdf:type owl:ObjectProperty ;
                            rdfs:domain :FossilFuel ;
                            rdfs:range <https://w3id.org/netbeheer/IECCIM/TC57CIM/IEC61970/Base/Domain#ActivePower> ;
                            rdfs:comment "The active power output level of the unit at which the given type of fuel is switched on. This fuel (e.g., oil) is sometimes used to supplement the base fuel (e.g., coal) at high active power output levels." .


###  https://w3id.org/netbeheer/IECCIM/TC57CIM/IEC61970/Base/Generation/Production#FossilFuel_lowBreakpointP
:FossilFuel_lowBreakpointP rdf:type owl:ObjectProperty ;
                           rdfs:domain :FossilFuel ;
                           rdfs:range <https://w3id.org/netbeheer/IECCIM/TC57CIM/IEC61970/Base/Domain#ActivePower> ;
                           rdfs:comment "The active power output level of the unit at which the given type of fuel is switched off. This fuel (e.g., oil) is sometimes used to stabilize the base fuel (e.g., coal) at low active power output levels." .


###  https://w3id.org/netbeheer/IECCIM/TC57CIM/IEC61970/Base/Generation/Production#FuelAllocationSchedule_FossilFuel
:FuelAllocationSchedule_FossilFuel rdf:type owl:ObjectProperty ;
                                   owl:inverseOf :FossilFuel_FuelAllocationSchedules ;
                                   rdfs:domain :FuelAllocationSchedule ;
                                   rdfs:range :FossilFuel ;
                                   rdfs:comment "A fuel allocation schedule must have a fossil fuel.A fuel allocation schedule must have a fossil fuel." .


###  https://w3id.org/netbeheer/IECCIM/TC57CIM/IEC61970/Base/Generation/Production#FuelAllocationSchedule_ThermalGeneratingUnit
:FuelAllocationSchedule_ThermalGeneratingUnit rdf:type owl:ObjectProperty ;
                                              rdfs:domain :FuelAllocationSchedule ;
                                              rdfs:range :ThermalGeneratingUnit ;
                                              rdfs:comment "A thermal generating unit may have one or more fuel allocation schedules.A thermal generating unit may have one or more fuel allocation schedules." .


###  https://w3id.org/netbeheer/IECCIM/TC57CIM/IEC61970/Base/Generation/Production#GenUnitOpCostCurve_GeneratingUnit
:GenUnitOpCostCurve_GeneratingUnit rdf:type owl:ObjectProperty ;
                                   rdfs:domain :GenUnitOpCostCurve ;
                                   rdfs:range :GeneratingUnit ;
                                   rdfs:comment "A generating unit may have one or more cost curves, depending upon fuel mixture and fuel cost.A generating unit may have one or more cost curves, depending upon fuel mixture and fuel cost." .


###  https://w3id.org/netbeheer/IECCIM/TC57CIM/IEC61970/Base/Generation/Production#GenUnitOpSchedule_GeneratingUnit
:GenUnitOpSchedule_GeneratingUnit rdf:type owl:ObjectProperty ;
                                  rdfs:domain :GenUnitOpSchedule ;
                                  rdfs:range :GeneratingUnit ;
                                  rdfs:comment "A generating unit may have an operating schedule, indicating the planned operation of the unit.A generating unit may have an operating schedule, indicating the planned operation of the unit." .


###  https://w3id.org/netbeheer/IECCIM/TC57CIM/IEC61970/Base/Generation/Production#GeneratingUnit_ControlAreaGeneratingUnit
:GeneratingUnit_ControlAreaGeneratingUnit rdf:type owl:ObjectProperty ;
                                          owl:inverseOf :ControlAreaGeneratingUnit_GeneratingUnit ;
                                          rdf:type owl:FunctionalProperty ;
                                          rdfs:domain :GeneratingUnit ;
                                          rdfs:range <https://w3id.org/netbeheer/IECCIM/TC57CIM/IEC61970/Base/ControlArea#ControlAreaGeneratingUnit> ;
                                          rdfs:comment "ControlArea specifications for this generating unit.The generating unit specified for this control area.  Note that a control area should include a GeneratingUnit only once." .


###  https://w3id.org/netbeheer/IECCIM/TC57CIM/IEC61970/Base/Generation/Production#GeneratingUnit_GenUnitOpCostCurves
:GeneratingUnit_GenUnitOpCostCurves rdf:type owl:ObjectProperty ;
                                    owl:inverseOf :GenUnitOpCostCurve_GeneratingUnit ;
                                    rdf:type owl:FunctionalProperty ;
                                    rdfs:domain :GeneratingUnit ;
                                    rdfs:range :GenUnitOpCostCurve ;
                                    rdfs:comment "A generating unit may have one or more cost curves, depending upon fuel mixture and fuel cost.A generating unit may have one or more cost curves, depending upon fuel mixture and fuel cost." .


###  https://w3id.org/netbeheer/IECCIM/TC57CIM/IEC61970/Base/Generation/Production#GeneratingUnit_GenUnitOpSchedule
:GeneratingUnit_GenUnitOpSchedule rdf:type owl:ObjectProperty ;
                                  owl:inverseOf :GenUnitOpSchedule_GeneratingUnit ;
                                  rdf:type owl:FunctionalProperty ;
                                  rdfs:domain :GeneratingUnit ;
                                  rdfs:range :GenUnitOpSchedule ;
                                  rdfs:comment "A generating unit may have an operating schedule, indicating the planned operation of the unit.A generating unit may have an operating schedule, indicating the planned operation of the unit." .


###  https://w3id.org/netbeheer/IECCIM/TC57CIM/IEC61970/Base/Generation/Production#GeneratingUnit_GrossToNetActivePowerCurves
:GeneratingUnit_GrossToNetActivePowerCurves rdf:type owl:ObjectProperty ;
                                            owl:inverseOf :GrossToNetActivePowerCurve_GeneratingUnit ;
                                            rdf:type owl:FunctionalProperty ;
                                            rdfs:domain :GeneratingUnit ;
                                            rdfs:range :GrossToNetActivePowerCurve ;
                                            rdfs:comment "A generating unit may have a gross active power to net active power curve, describing the losses and auxiliary power requirements of the unit.A generating unit may have a gross active power to net active power curve, describing the losses and auxiliary power requirements of the unit." .


###  https://w3id.org/netbeheer/IECCIM/TC57CIM/IEC61970/Base/Generation/Production#GeneratingUnit_allocSpinResP
:GeneratingUnit_allocSpinResP rdf:type owl:ObjectProperty ;
                              rdfs:domain :GeneratingUnit ;
                              rdfs:range <https://w3id.org/netbeheer/IECCIM/TC57CIM/IEC61970/Base/Domain#ActivePower> ;
                              rdfs:comment """The planned unused capacity (spinning reserve) which can be used to support emergency load.
""" .


###  https://w3id.org/netbeheer/IECCIM/TC57CIM/IEC61970/Base/Generation/Production#GeneratingUnit_autoCntrlMarginP
:GeneratingUnit_autoCntrlMarginP rdf:type owl:ObjectProperty ;
                                 rdfs:domain :GeneratingUnit ;
                                 rdfs:range <https://w3id.org/netbeheer/IECCIM/TC57CIM/IEC61970/Base/Domain#ActivePower> ;
                                 rdfs:comment "The planned unused capacity which can be used to support automatic control overruns." .


###  https://w3id.org/netbeheer/IECCIM/TC57CIM/IEC61970/Base/Generation/Production#GeneratingUnit_baseP
:GeneratingUnit_baseP rdf:type owl:ObjectProperty ;
                      rdfs:domain :GeneratingUnit ;
                      rdfs:range <https://w3id.org/netbeheer/IECCIM/TC57CIM/IEC61970/Base/Domain#ActivePower> ;
                      rdfs:comment "For dispatchable units, this value represents the economic active power basepoint, for units that are not dispatchable, this value represents the fixed generation value. The value must be between the operating low and high limits." .


###  https://w3id.org/netbeheer/IECCIM/TC57CIM/IEC61970/Base/Generation/Production#GeneratingUnit_controlDeadband
:GeneratingUnit_controlDeadband rdf:type owl:ObjectProperty ;
                                rdfs:domain :GeneratingUnit ;
                                rdfs:range <https://w3id.org/netbeheer/IECCIM/TC57CIM/IEC61970/Base/Domain#ActivePower> ;
                                rdfs:comment "Unit control error deadband. When a unit's desired active power change is less than this deadband, then no control pulses will be sent to the unit." .


###  https://w3id.org/netbeheer/IECCIM/TC57CIM/IEC61970/Base/Generation/Production#GeneratingUnit_controlPulseHigh
:GeneratingUnit_controlPulseHigh rdf:type owl:ObjectProperty ;
                                 rdfs:domain :GeneratingUnit ;
                                 rdfs:range <https://w3id.org/netbeheer/IECCIM/TC57CIM/IEC61970/Base/Domain#Seconds> ;
                                 rdfs:comment """Pulse high limit which is the largest control pulse that the unit can respond to.
""" .


###  https://w3id.org/netbeheer/IECCIM/TC57CIM/IEC61970/Base/Generation/Production#GeneratingUnit_controlPulseLow
:GeneratingUnit_controlPulseLow rdf:type owl:ObjectProperty ;
                                rdfs:domain :GeneratingUnit ;
                                rdfs:range <https://w3id.org/netbeheer/IECCIM/TC57CIM/IEC61970/Base/Domain#Seconds> ;
                                rdfs:comment """Pulse low limit which is the smallest control pulse that the unit can respond to.
""" .


###  https://w3id.org/netbeheer/IECCIM/TC57CIM/IEC61970/Base/Generation/Production#GeneratingUnit_controlResponseRate
:GeneratingUnit_controlResponseRate rdf:type owl:ObjectProperty ;
                                    rdfs:domain :GeneratingUnit ;
                                    rdfs:range <https://w3id.org/netbeheer/IECCIM/TC57CIM/IEC61970/Base/Domain#ActivePowerChangeRate> ;
                                    rdfs:comment "Unit response rate which specifies the active power change for a control pulse of one second in the most responsive loading level of the unit." .


###  https://w3id.org/netbeheer/IECCIM/TC57CIM/IEC61970/Base/Generation/Production#GeneratingUnit_efficiency
:GeneratingUnit_efficiency rdf:type owl:ObjectProperty ;
                           rdfs:domain :GeneratingUnit ;
                           rdfs:range <https://w3id.org/netbeheer/IECCIM/TC57CIM/IEC61970/Base/Domain#PerCent> ;
                           rdfs:comment "The efficiency of the unit in converting mechanical energy, from the prime mover, into electrical energy." .


###  https://w3id.org/netbeheer/IECCIM/TC57CIM/IEC61970/Base/Generation/Production#GeneratingUnit_governorMPL
:GeneratingUnit_governorMPL rdf:type owl:ObjectProperty ;
                            rdfs:domain :GeneratingUnit ;
                            rdfs:range <https://w3id.org/netbeheer/IECCIM/TC57CIM/IEC61970/Base/Domain#PU> ;
                            rdfs:comment """Governor motor position limit.
""" .


###  https://w3id.org/netbeheer/IECCIM/TC57CIM/IEC61970/Base/Generation/Production#GeneratingUnit_governorSCD
:GeneratingUnit_governorSCD rdf:type owl:ObjectProperty ;
                            rdfs:domain :GeneratingUnit ;
                            rdfs:range <https://w3id.org/netbeheer/IECCIM/TC57CIM/IEC61970/Base/Domain#PerCent> ;
                            rdfs:comment "Governor Speed Changer Droop.   This is the change in generator power output divided by the change in frequency normalized by the nominal power of the generator and the nominal frequency and expressed in percent and negated. A positive value of speed change droop provides additional generator output upon a drop in frequency." .


###  https://w3id.org/netbeheer/IECCIM/TC57CIM/IEC61970/Base/Generation/Production#GeneratingUnit_highControlLimit
:GeneratingUnit_highControlLimit rdf:type owl:ObjectProperty ;
                                 rdfs:domain :GeneratingUnit ;
                                 rdfs:range <https://w3id.org/netbeheer/IECCIM/TC57CIM/IEC61970/Base/Domain#ActivePower> ;
                                 rdfs:comment """High limit for secondary (AGC) control.
""" .


###  https://w3id.org/netbeheer/IECCIM/TC57CIM/IEC61970/Base/Generation/Production#GeneratingUnit_initialP
:GeneratingUnit_initialP rdf:type owl:ObjectProperty ;
                         rdfs:domain :GeneratingUnit ;
                         rdfs:range <https://w3id.org/netbeheer/IECCIM/TC57CIM/IEC61970/Base/Domain#ActivePower> ;
                         rdfs:comment """Default initial active power  which is used to store a powerflow result for the initial active power for this unit in this network configuration.
""" .


###  https://w3id.org/netbeheer/IECCIM/TC57CIM/IEC61970/Base/Generation/Production#GeneratingUnit_lowControlLimit
:GeneratingUnit_lowControlLimit rdf:type owl:ObjectProperty ;
                                rdfs:domain :GeneratingUnit ;
                                rdfs:range <https://w3id.org/netbeheer/IECCIM/TC57CIM/IEC61970/Base/Domain#ActivePower> ;
                                rdfs:comment """Low limit for secondary (AGC) control.
""" .


###  https://w3id.org/netbeheer/IECCIM/TC57CIM/IEC61970/Base/Generation/Production#GeneratingUnit_lowerRampRate
:GeneratingUnit_lowerRampRate rdf:type owl:ObjectProperty ;
                              rdfs:domain :GeneratingUnit ;
                              rdfs:range <https://w3id.org/netbeheer/IECCIM/TC57CIM/IEC61970/Base/Domain#ActivePowerChangeRate> ;
                              rdfs:comment """The normal maximum rate the generating unit active power output can be lowered by control actions.
""" .


###  https://w3id.org/netbeheer/IECCIM/TC57CIM/IEC61970/Base/Generation/Production#GeneratingUnit_maxEconomicP
:GeneratingUnit_maxEconomicP rdf:type owl:ObjectProperty ;
                             rdfs:domain :GeneratingUnit ;
                             rdfs:range <https://w3id.org/netbeheer/IECCIM/TC57CIM/IEC61970/Base/Domain#ActivePower> ;
                             rdfs:comment """Maximum high economic active power limit, that should not exceed the maximum operating active power limit.
""" .


###  https://w3id.org/netbeheer/IECCIM/TC57CIM/IEC61970/Base/Generation/Production#GeneratingUnit_maxOperatingP
:GeneratingUnit_maxOperatingP rdf:type owl:ObjectProperty ;
                              rdfs:domain :GeneratingUnit ;
                              rdfs:range <https://w3id.org/netbeheer/IECCIM/TC57CIM/IEC61970/Base/Domain#ActivePower> ;
                              rdfs:comment """This is the maximum operating active power limit the dispatcher can enter for this unit.
""" .


###  https://w3id.org/netbeheer/IECCIM/TC57CIM/IEC61970/Base/Generation/Production#GeneratingUnit_maximumAllowableSpinningReserve
:GeneratingUnit_maximumAllowableSpinningReserve rdf:type owl:ObjectProperty ;
                                                rdfs:domain :GeneratingUnit ;
                                                rdfs:range <https://w3id.org/netbeheer/IECCIM/TC57CIM/IEC61970/Base/Domain#ActivePower> ;
                                                rdfs:comment "Maximum allowable spinning reserve. Spinning reserve will never be considered greater than this value regardless of the current operating point." .


###  https://w3id.org/netbeheer/IECCIM/TC57CIM/IEC61970/Base/Generation/Production#GeneratingUnit_minEconomicP
:GeneratingUnit_minEconomicP rdf:type owl:ObjectProperty ;
                             rdfs:domain :GeneratingUnit ;
                             rdfs:range <https://w3id.org/netbeheer/IECCIM/TC57CIM/IEC61970/Base/Domain#ActivePower> ;
                             rdfs:comment """Low economic active power limit that must be greater than or equal to the minimum operating active power limit.
""" .


###  https://w3id.org/netbeheer/IECCIM/TC57CIM/IEC61970/Base/Generation/Production#GeneratingUnit_minOperatingP
:GeneratingUnit_minOperatingP rdf:type owl:ObjectProperty ;
                              rdfs:domain :GeneratingUnit ;
                              rdfs:range <https://w3id.org/netbeheer/IECCIM/TC57CIM/IEC61970/Base/Domain#ActivePower> ;
                              rdfs:comment "This is the minimum operating active power limit the dispatcher can enter for this unit." .


###  https://w3id.org/netbeheer/IECCIM/TC57CIM/IEC61970/Base/Generation/Production#GeneratingUnit_minimumOffTime
:GeneratingUnit_minimumOffTime rdf:type owl:ObjectProperty ;
                               rdfs:domain :GeneratingUnit ;
                               rdfs:range <https://w3id.org/netbeheer/IECCIM/TC57CIM/IEC61970/Base/Domain#Seconds> ;
                               rdfs:comment """Minimum time interval between unit shutdown and startup.
""" .


###  https://w3id.org/netbeheer/IECCIM/TC57CIM/IEC61970/Base/Generation/Production#GeneratingUnit_modelDetail
:GeneratingUnit_modelDetail rdf:type owl:ObjectProperty ;
                            rdfs:domain :GeneratingUnit ;
                            rdfs:range :Classification ;
                            rdfs:comment """Detail level of the generator model data.
""" .


###  https://w3id.org/netbeheer/IECCIM/TC57CIM/IEC61970/Base/Generation/Production#GeneratingUnit_nominalP
:GeneratingUnit_nominalP rdf:type owl:ObjectProperty ;
                         rdfs:domain :GeneratingUnit ;
                         rdfs:range <https://w3id.org/netbeheer/IECCIM/TC57CIM/IEC61970/Base/Domain#ActivePower> ;
                         rdfs:comment """The nominal power of the generating unit.  Used to give precise meaning to percentage based attributes such as the governor speed change droop (governorSCD attribute).
The attribute shall be a positive value equal or less than RotatingMachine.ratedS.""" .


###  https://w3id.org/netbeheer/IECCIM/TC57CIM/IEC61970/Base/Generation/Production#GeneratingUnit_raiseRampRate
:GeneratingUnit_raiseRampRate rdf:type owl:ObjectProperty ;
                              rdfs:domain :GeneratingUnit ;
                              rdfs:range <https://w3id.org/netbeheer/IECCIM/TC57CIM/IEC61970/Base/Domain#ActivePowerChangeRate> ;
                              rdfs:comment """The normal maximum rate the generating unit active power output can be raised by control actions.
""" .


###  https://w3id.org/netbeheer/IECCIM/TC57CIM/IEC61970/Base/Generation/Production#GeneratingUnit_ratedGrossMaxP
:GeneratingUnit_ratedGrossMaxP rdf:type owl:ObjectProperty ;
                               rdfs:domain :GeneratingUnit ;
                               rdfs:range <https://w3id.org/netbeheer/IECCIM/TC57CIM/IEC61970/Base/Domain#ActivePower> ;
                               rdfs:comment """The unit's gross rated maximum capacity (book value).
""" .


###  https://w3id.org/netbeheer/IECCIM/TC57CIM/IEC61970/Base/Generation/Production#GeneratingUnit_ratedGrossMinP
:GeneratingUnit_ratedGrossMinP rdf:type owl:ObjectProperty ;
                               rdfs:domain :GeneratingUnit ;
                               rdfs:range <https://w3id.org/netbeheer/IECCIM/TC57CIM/IEC61970/Base/Domain#ActivePower> ;
                               rdfs:comment """The gross rated minimum generation level which the unit can safely operate at while delivering power to the transmission grid.
""" .


###  https://w3id.org/netbeheer/IECCIM/TC57CIM/IEC61970/Base/Generation/Production#GeneratingUnit_ratedNetMaxP
:GeneratingUnit_ratedNetMaxP rdf:type owl:ObjectProperty ;
                             rdfs:domain :GeneratingUnit ;
                             rdfs:range <https://w3id.org/netbeheer/IECCIM/TC57CIM/IEC61970/Base/Domain#ActivePower> ;
                             rdfs:comment """The net rated maximum capacity determined by subtracting the auxiliary power used to operate the internal plant machinery from the rated gross maximum capacity.
""" .


###  https://w3id.org/netbeheer/IECCIM/TC57CIM/IEC61970/Base/Generation/Production#GeneratingUnit_startupCost
:GeneratingUnit_startupCost rdf:type owl:ObjectProperty ;
                            rdfs:domain :GeneratingUnit ;
                            rdfs:range <https://w3id.org/netbeheer/IECCIM/TC57CIM/IEC61970/Base/Domain#Money> ;
                            rdfs:comment "The initial startup cost incurred for each start of the GeneratingUnit." .


###  https://w3id.org/netbeheer/IECCIM/TC57CIM/IEC61970/Base/Generation/Production#GeneratingUnit_startupTime
:GeneratingUnit_startupTime rdf:type owl:ObjectProperty ;
                            rdfs:domain :GeneratingUnit ;
                            rdfs:range <https://w3id.org/netbeheer/IECCIM/TC57CIM/IEC61970/Base/Domain#Seconds> ;
                            rdfs:comment """Time it takes to get the unit on-line, from the time that the prime mover mechanical power is applied.
""" .


###  https://w3id.org/netbeheer/IECCIM/TC57CIM/IEC61970/Base/Generation/Production#GeneratingUnit_totalEfficiency
:GeneratingUnit_totalEfficiency rdf:type owl:ObjectProperty ;
                                rdfs:domain :GeneratingUnit ;
                                rdfs:range <https://w3id.org/netbeheer/IECCIM/TC57CIM/IEC61970/Base/Domain#PerCent> ;
                                rdfs:comment "The efficiency of the unit in converting the fuel into electrical energy." .


###  https://w3id.org/netbeheer/IECCIM/TC57CIM/IEC61970/Base/Generation/Production#GeneratingUnit_variableCost
:GeneratingUnit_variableCost rdf:type owl:ObjectProperty ;
                             rdfs:domain :GeneratingUnit ;
                             rdfs:range <https://w3id.org/netbeheer/IECCIM/TC57CIM/IEC61970/Base/Domain#Money> ;
                             rdfs:comment "The variable cost component of production per unit of ActivePower." .


###  https://w3id.org/netbeheer/IECCIM/TC57CIM/IEC61970/Base/Generation/Production#GrossToNetActivePowerCurve_GeneratingUnit
:GrossToNetActivePowerCurve_GeneratingUnit rdf:type owl:ObjectProperty ;
                                           rdfs:domain :GrossToNetActivePowerCurve ;
                                           rdfs:range :GeneratingUnit ;
                                           rdfs:comment "A generating unit may have a gross active power to net active power curve, describing the losses and auxiliary power requirements of the unit.A generating unit may have a gross active power to net active power curve, describing the losses and auxiliary power requirements of the unit." .


###  https://w3id.org/netbeheer/IECCIM/TC57CIM/IEC61970/Base/Generation/Production#HeatInputCurve_ThermalGeneratingUnit
:HeatInputCurve_ThermalGeneratingUnit rdf:type owl:ObjectProperty ;
                                      rdfs:domain :HeatInputCurve ;
                                      rdfs:range :ThermalGeneratingUnit ;
                                      rdfs:comment "A thermal generating unit may have a heat input curve.A thermal generating unit may have a heat input curve." .


###  https://w3id.org/netbeheer/IECCIM/TC57CIM/IEC61970/Base/Generation/Production#HeatInputCurve_auxPowerMult
:HeatInputCurve_auxPowerMult rdf:type owl:ObjectProperty ;
                             rdfs:domain :HeatInputCurve ;
                             rdfs:range <https://w3id.org/netbeheer/IECCIM/TC57CIM/IEC61970/Base/Domain#PU> ;
                             rdfs:comment "Power output - auxiliary power multiplier adjustment factor." .


###  https://w3id.org/netbeheer/IECCIM/TC57CIM/IEC61970/Base/Generation/Production#HeatInputCurve_auxPowerOffset
:HeatInputCurve_auxPowerOffset rdf:type owl:ObjectProperty ;
                               rdfs:domain :HeatInputCurve ;
                               rdfs:range <https://w3id.org/netbeheer/IECCIM/TC57CIM/IEC61970/Base/Domain#ActivePower> ;
                               rdfs:comment """Power output - auxiliary power offset adjustment factor.
""" .


###  https://w3id.org/netbeheer/IECCIM/TC57CIM/IEC61970/Base/Generation/Production#HeatInputCurve_heatInputEff
:HeatInputCurve_heatInputEff rdf:type owl:ObjectProperty ;
                             rdfs:domain :HeatInputCurve ;
                             rdfs:range <https://w3id.org/netbeheer/IECCIM/TC57CIM/IEC61970/Base/Domain#PU> ;
                             rdfs:comment "Heat input - efficiency multiplier adjustment factor." .


###  https://w3id.org/netbeheer/IECCIM/TC57CIM/IEC61970/Base/Generation/Production#HeatInputCurve_heatInputOffset
:HeatInputCurve_heatInputOffset rdf:type owl:ObjectProperty ;
                                rdfs:domain :HeatInputCurve ;
                                rdfs:range :HeatRate ;
                                rdfs:comment "Heat input - offset adjustment factor." .


###  https://w3id.org/netbeheer/IECCIM/TC57CIM/IEC61970/Base/Generation/Production#HeatRateCurve_ThermalGeneratingUnit
:HeatRateCurve_ThermalGeneratingUnit rdf:type owl:ObjectProperty ;
                                     rdfs:domain :HeatRateCurve ;
                                     rdfs:range :ThermalGeneratingUnit ;
                                     rdfs:comment "A thermal generating unit may have a heat rate curve.A thermal generating unit may have a heat rate curve." .


###  https://w3id.org/netbeheer/IECCIM/TC57CIM/IEC61970/Base/Generation/Production#HydroGeneratingEfficiencyCurve_HydroGeneratingUnit
:HydroGeneratingEfficiencyCurve_HydroGeneratingUnit rdf:type owl:ObjectProperty ;
                                                    rdfs:domain :HydroGeneratingEfficiencyCurve ;
                                                    rdfs:range :HydroGeneratingUnit ;
                                                    rdfs:comment "A hydro generating unit has an efficiency curve.A hydro generating unit has an efficiency curve." .


###  https://w3id.org/netbeheer/IECCIM/TC57CIM/IEC61970/Base/Generation/Production#HydroGeneratingUnit_HydroGeneratingEfficiencyCurves
:HydroGeneratingUnit_HydroGeneratingEfficiencyCurves rdf:type owl:ObjectProperty ;
                                                     owl:inverseOf :HydroGeneratingEfficiencyCurve_HydroGeneratingUnit ;
                                                     rdf:type owl:FunctionalProperty ;
                                                     rdfs:domain :HydroGeneratingUnit ;
                                                     rdfs:range :HydroGeneratingEfficiencyCurve ;
                                                     rdfs:comment "A hydro generating unit has an efficiency curve.A hydro generating unit has an efficiency curve." .


###  https://w3id.org/netbeheer/IECCIM/TC57CIM/IEC61970/Base/Generation/Production#HydroGeneratingUnit_HydroPowerPlant
:HydroGeneratingUnit_HydroPowerPlant rdf:type owl:ObjectProperty ;
                                     owl:inverseOf :HydroPowerPlant_HydroGeneratingUnits ;
                                     rdfs:domain :HydroGeneratingUnit ;
                                     rdfs:range :HydroPowerPlant ;
                                     rdfs:comment "The hydro generating unit belongs to a hydro power plant.The hydro generating unit belongs to a hydro power plant." .


###  https://w3id.org/netbeheer/IECCIM/TC57CIM/IEC61970/Base/Generation/Production#HydroGeneratingUnit_PenstockLossCurve
:HydroGeneratingUnit_PenstockLossCurve rdf:type owl:ObjectProperty ;
                                       owl:inverseOf :PenstockLossCurve_HydroGeneratingUnit ;
                                       rdf:type owl:FunctionalProperty ;
                                       rdfs:domain :HydroGeneratingUnit ;
                                       rdfs:range :PenstockLossCurve ;
                                       rdfs:comment "A hydro generating unit has a penstock loss curve.A hydro generating unit has a penstock loss curve." .


###  https://w3id.org/netbeheer/IECCIM/TC57CIM/IEC61970/Base/Generation/Production#HydroGeneratingUnit_TailbayLossCurve
:HydroGeneratingUnit_TailbayLossCurve rdf:type owl:ObjectProperty ;
                                      owl:inverseOf :TailbayLossCurve_HydroGeneratingUnit ;
                                      rdf:type owl:FunctionalProperty ;
                                      rdfs:domain :HydroGeneratingUnit ;
                                      rdfs:range :TailbayLossCurve ;
                                      rdfs:comment "A hydro generating unit has a tailbay loss curve.A hydro generating unit has a tailbay loss curve." .


###  https://w3id.org/netbeheer/IECCIM/TC57CIM/IEC61970/Base/Generation/Production#HydroGeneratingUnit_hydroUnitWaterCost
:HydroGeneratingUnit_hydroUnitWaterCost rdf:type owl:ObjectProperty ;
                                        rdfs:domain :HydroGeneratingUnit ;
                                        rdfs:range <https://w3id.org/netbeheer/IECCIM/TC57CIM/IEC61970/Base/Domain#CostPerVolume> ;
                                        rdfs:comment """The equivalent cost of water that drives the hydro turbine.
""" .


###  https://w3id.org/netbeheer/IECCIM/TC57CIM/IEC61970/Base/Generation/Production#HydroPowerPlant_GenSourcePumpDischargeReservoir
:HydroPowerPlant_GenSourcePumpDischargeReservoir rdf:type owl:ObjectProperty ;
                                                 rdfs:domain :HydroPowerPlant ;
                                                 rdfs:range :Reservoir ;
                                                 rdfs:comment "Generators are supplied water from or pumps discharge water to an upstream reservoir.Generators are supplied water from or pumps discharge water to an upstream reservoir." .


###  https://w3id.org/netbeheer/IECCIM/TC57CIM/IEC61970/Base/Generation/Production#HydroPowerPlant_HydroGeneratingUnits
:HydroPowerPlant_HydroGeneratingUnits rdf:type owl:ObjectProperty ;
                                      rdfs:domain :HydroPowerPlant ;
                                      rdfs:range :HydroGeneratingUnit ;
                                      rdfs:comment "The hydro generating unit belongs to a hydro power plant.The hydro generating unit belongs to a hydro power plant." .


###  https://w3id.org/netbeheer/IECCIM/TC57CIM/IEC61970/Base/Generation/Production#HydroPowerPlant_HydroPumps
:HydroPowerPlant_HydroPumps rdf:type owl:ObjectProperty ;
                            rdfs:domain :HydroPowerPlant ;
                            rdfs:range :HydroPump ;
                            rdfs:comment "The hydro pump may be a member of a pumped storage plant or a pump for distributing water.The hydro pump may be a member of a pumped storage plant or a pump for distributing water." .


###  https://w3id.org/netbeheer/IECCIM/TC57CIM/IEC61970/Base/Generation/Production#HydroPowerPlant_Reservoir
:HydroPowerPlant_Reservoir rdf:type owl:ObjectProperty ;
                           rdfs:domain :HydroPowerPlant ;
                           rdfs:range :Reservoir ;
                           rdfs:comment "Generators discharge water to or pumps are supplied water from a downstream reservoir.Generators discharge water to or pumps are supplied water from a downstream reservoir." .


###  https://w3id.org/netbeheer/IECCIM/TC57CIM/IEC61970/Base/Generation/Production#HydroPowerPlant_dischargeTravelDelay
:HydroPowerPlant_dischargeTravelDelay rdf:type owl:ObjectProperty ;
                                      rdfs:domain :HydroPowerPlant ;
                                      rdfs:range <https://w3id.org/netbeheer/IECCIM/TC57CIM/IEC61970/Base/Domain#Seconds> ;
                                      rdfs:comment """Water travel delay from tailbay to next downstream hydro power station.
""" .


###  https://w3id.org/netbeheer/IECCIM/TC57CIM/IEC61970/Base/Generation/Production#HydroPowerPlant_genRatedP
:HydroPowerPlant_genRatedP rdf:type owl:ObjectProperty ;
                           rdfs:domain :HydroPowerPlant ;
                           rdfs:range <https://w3id.org/netbeheer/IECCIM/TC57CIM/IEC61970/Base/Domain#ActivePower> ;
                           rdfs:comment """The hydro plant's generating rating active power for rated head conditions.
""" .


###  https://w3id.org/netbeheer/IECCIM/TC57CIM/IEC61970/Base/Generation/Production#HydroPowerPlant_plantDischargeCapacity
:HydroPowerPlant_plantDischargeCapacity rdf:type owl:ObjectProperty ;
                                        rdfs:domain :HydroPowerPlant ;
                                        rdfs:range <https://w3id.org/netbeheer/IECCIM/TC57CIM/IEC61970/Base/Domain#VolumeFlowRate> ;
                                        rdfs:comment """Total plant discharge capacity.
""" .


###  https://w3id.org/netbeheer/IECCIM/TC57CIM/IEC61970/Base/Generation/Production#HydroPowerPlant_plantRatedHead
:HydroPowerPlant_plantRatedHead rdf:type owl:ObjectProperty ;
                                rdfs:domain :HydroPowerPlant ;
                                rdfs:range <https://w3id.org/netbeheer/IECCIM/TC57CIM/IEC61970/Base/Domain#Length> ;
                                rdfs:comment """The plant's rated gross head.
""" .


###  https://w3id.org/netbeheer/IECCIM/TC57CIM/IEC61970/Base/Generation/Production#HydroPowerPlant_pumpRatedP
:HydroPowerPlant_pumpRatedP rdf:type owl:ObjectProperty ;
                            rdfs:domain :HydroPowerPlant ;
                            rdfs:range <https://w3id.org/netbeheer/IECCIM/TC57CIM/IEC61970/Base/Domain#ActivePower> ;
                            rdfs:comment """The hydro plant's pumping rating active power for rated head conditions.
""" .


###  https://w3id.org/netbeheer/IECCIM/TC57CIM/IEC61970/Base/Generation/Production#HydroPowerPlant_surgeTankCrestLevel
:HydroPowerPlant_surgeTankCrestLevel rdf:type owl:ObjectProperty ;
                                     rdfs:domain :HydroPowerPlant ;
                                     rdfs:range <https://w3id.org/netbeheer/IECCIM/TC57CIM/IEC61970/Base/Domain#WaterLevel> ;
                                     rdfs:comment """The level at which the surge tank spills.
""" .


###  https://w3id.org/netbeheer/IECCIM/TC57CIM/IEC61970/Base/Generation/Production#HydroPumpOpSchedule_HydroPump
:HydroPumpOpSchedule_HydroPump rdf:type owl:ObjectProperty ;
                               rdfs:domain :HydroPumpOpSchedule ;
                               rdfs:range :HydroPump ;
                               rdfs:comment "The hydro pump has a pumping schedule over time, indicating when pumping is to occur.The hydro pump has a pumping schedule over time, indicating when pumping is to occur." .


###  https://w3id.org/netbeheer/IECCIM/TC57CIM/IEC61970/Base/Generation/Production#HydroPump_HydroPowerPlant
:HydroPump_HydroPowerPlant rdf:type owl:ObjectProperty ;
                           owl:inverseOf :HydroPowerPlant_HydroPumps ;
                           rdfs:domain :HydroPump ;
                           rdfs:range :HydroPowerPlant ;
                           rdfs:comment "The hydro pump may be a member of a pumped storage plant or a pump for distributing water.The hydro pump may be a member of a pumped storage plant or a pump for distributing water." .


###  https://w3id.org/netbeheer/IECCIM/TC57CIM/IEC61970/Base/Generation/Production#HydroPump_HydroPumpOpSchedule
:HydroPump_HydroPumpOpSchedule rdf:type owl:ObjectProperty ;
                               owl:inverseOf :HydroPumpOpSchedule_HydroPump ;
                               rdf:type owl:FunctionalProperty ;
                               rdfs:domain :HydroPump ;
                               rdfs:range :HydroPumpOpSchedule ;
                               rdfs:comment "The hydro pump has a pumping schedule over time, indicating when pumping is to occur.The hydro pump has a pumping schedule over time, indicating when pumping is to occur." .


###  https://w3id.org/netbeheer/IECCIM/TC57CIM/IEC61970/Base/Generation/Production#HydroPump_pumpDischAtMaxHead
:HydroPump_pumpDischAtMaxHead rdf:type owl:ObjectProperty ;
                              rdfs:domain :HydroPump ;
                              rdfs:range <https://w3id.org/netbeheer/IECCIM/TC57CIM/IEC61970/Base/Domain#VolumeFlowRate> ;
                              rdfs:comment """The pumping discharge under maximum head conditions, usually at full gate.
""" .


###  https://w3id.org/netbeheer/IECCIM/TC57CIM/IEC61970/Base/Generation/Production#HydroPump_pumpDischAtMinHead
:HydroPump_pumpDischAtMinHead rdf:type owl:ObjectProperty ;
                              rdfs:domain :HydroPump ;
                              rdfs:range <https://w3id.org/netbeheer/IECCIM/TC57CIM/IEC61970/Base/Domain#VolumeFlowRate> ;
                              rdfs:comment """The pumping discharge under minimum head conditions, usually at full gate.
""" .


###  https://w3id.org/netbeheer/IECCIM/TC57CIM/IEC61970/Base/Generation/Production#HydroPump_pumpPowerAtMaxHead
:HydroPump_pumpPowerAtMaxHead rdf:type owl:ObjectProperty ;
                              rdfs:domain :HydroPump ;
                              rdfs:range <https://w3id.org/netbeheer/IECCIM/TC57CIM/IEC61970/Base/Domain#ActivePower> ;
                              rdfs:comment """The pumping power under maximum head conditions, usually at full gate.
""" .


###  https://w3id.org/netbeheer/IECCIM/TC57CIM/IEC61970/Base/Generation/Production#HydroPump_pumpPowerAtMinHead
:HydroPump_pumpPowerAtMinHead rdf:type owl:ObjectProperty ;
                              rdfs:domain :HydroPump ;
                              rdfs:range <https://w3id.org/netbeheer/IECCIM/TC57CIM/IEC61970/Base/Domain#ActivePower> ;
                              rdfs:comment "The pumping power under minimum head conditions, usually at full gate." .


###  https://w3id.org/netbeheer/IECCIM/TC57CIM/IEC61970/Base/Generation/Production#IncrementalHeatRateCurve_ThermalGeneratingUnit
:IncrementalHeatRateCurve_ThermalGeneratingUnit rdf:type owl:ObjectProperty ;
                                                rdfs:domain :IncrementalHeatRateCurve ;
                                                rdfs:range :ThermalGeneratingUnit ;
                                                rdfs:comment "A thermal generating unit may have an incremental heat rate curve.A thermal generating unit may have an incremental heat rate curve." .


###  https://w3id.org/netbeheer/IECCIM/TC57CIM/IEC61970/Base/Generation/Production#InflowForecast_Reservoir
:InflowForecast_Reservoir rdf:type owl:ObjectProperty ;
                          rdfs:domain :InflowForecast ;
                          rdfs:range :Reservoir ;
                          rdfs:comment "A reservoir may have a \"natural\" inflow forecast.A reservoir may have a \"natural\" inflow forecast." .


###  https://w3id.org/netbeheer/IECCIM/TC57CIM/IEC61970/Base/Generation/Production#LevelVsVolumeCurve_Reservoir
:LevelVsVolumeCurve_Reservoir rdf:type owl:ObjectProperty ;
                              rdfs:domain :LevelVsVolumeCurve ;
                              rdfs:range :Reservoir ;
                              rdfs:comment "A reservoir may have a level versus volume relationship.A reservoir may have a level versus volume relationship." .


###  https://w3id.org/netbeheer/IECCIM/TC57CIM/IEC61970/Base/Generation/Production#PenstockLossCurve_HydroGeneratingUnit
:PenstockLossCurve_HydroGeneratingUnit rdf:type owl:ObjectProperty ;
                                       rdfs:domain :PenstockLossCurve ;
                                       rdfs:range :HydroGeneratingUnit ;
                                       rdfs:comment "A hydro generating unit has a penstock loss curve.A hydro generating unit has a penstock loss curve." .


###  https://w3id.org/netbeheer/IECCIM/TC57CIM/IEC61970/Base/Generation/Production#Reservoir_HydroPowerPlants
:Reservoir_HydroPowerPlants rdf:type owl:ObjectProperty ;
                            owl:inverseOf :HydroPowerPlant_Reservoir ;
                            rdfs:domain :Reservoir ;
                            rdfs:range :HydroPowerPlant ;
                            rdfs:comment "Generators discharge water to or pumps are supplied water from a downstream reservoir.Generators discharge water to or pumps are supplied water from a downstream reservoir." .


###  https://w3id.org/netbeheer/IECCIM/TC57CIM/IEC61970/Base/Generation/Production#Reservoir_InflowForecasts
:Reservoir_InflowForecasts rdf:type owl:ObjectProperty ;
                           owl:inverseOf :InflowForecast_Reservoir ;
                           rdf:type owl:FunctionalProperty ;
                           rdfs:domain :Reservoir ;
                           rdfs:range :InflowForecast ;
                           rdfs:comment "A reservoir may have a \"natural\" inflow forecast.A reservoir may have a \"natural\" inflow forecast." .


###  https://w3id.org/netbeheer/IECCIM/TC57CIM/IEC61970/Base/Generation/Production#Reservoir_LevelVsVolumeCurves
:Reservoir_LevelVsVolumeCurves rdf:type owl:ObjectProperty ;
                               owl:inverseOf :LevelVsVolumeCurve_Reservoir ;
                               rdf:type owl:FunctionalProperty ;
                               rdfs:domain :Reservoir ;
                               rdfs:range :LevelVsVolumeCurve ;
                               rdfs:comment "A reservoir may have a level versus volume relationship.A reservoir may have a level versus volume relationship." .


###  https://w3id.org/netbeheer/IECCIM/TC57CIM/IEC61970/Base/Generation/Production#Reservoir_SpillsFromReservoir
:Reservoir_SpillsFromReservoir rdf:type owl:ObjectProperty ;
                               owl:inverseOf :Reservoir_SpillsIntoReservoirs ;
                               rdfs:domain :Reservoir ;
                               rdfs:range :Reservoir ;
                               rdfs:comment "A reservoir may spill into a downstream reservoir.A reservoir may spill into a downstream reservoir." .


###  https://w3id.org/netbeheer/IECCIM/TC57CIM/IEC61970/Base/Generation/Production#Reservoir_SpillsIntoReservoirs
:Reservoir_SpillsIntoReservoirs rdf:type owl:ObjectProperty ;
                                rdfs:domain :Reservoir ;
                                rdfs:range :Reservoir ;
                                rdfs:comment "A reservoir may spill into a downstream reservoir.A reservoir may spill into a downstream reservoir." .


###  https://w3id.org/netbeheer/IECCIM/TC57CIM/IEC61970/Base/Generation/Production#Reservoir_TargetLevelSchedule
:Reservoir_TargetLevelSchedule rdf:type owl:ObjectProperty ;
                               owl:inverseOf :TargetLevelSchedule_Reservoir ;
                               rdf:type owl:FunctionalProperty ;
                               rdfs:domain :Reservoir ;
                               rdfs:range :TargetLevelSchedule ;
                               rdfs:comment "A reservoir may have a water level target schedule.A reservoir may have a water level target schedule." .


###  https://w3id.org/netbeheer/IECCIM/TC57CIM/IEC61970/Base/Generation/Production#Reservoir_UpstreamFromHydroPowerPlants
:Reservoir_UpstreamFromHydroPowerPlants rdf:type owl:ObjectProperty ;
                                        owl:inverseOf :HydroPowerPlant_GenSourcePumpDischargeReservoir ;
                                        rdf:type owl:FunctionalProperty ;
                                        rdfs:domain :Reservoir ;
                                        rdfs:range :HydroPowerPlant ;
                                        rdfs:comment "Generators are supplied water from or pumps discharge water to an upstream reservoir.Generators are supplied water from or pumps discharge water to an upstream reservoir." .


###  https://w3id.org/netbeheer/IECCIM/TC57CIM/IEC61970/Base/Generation/Production#Reservoir_activeStorageCapacity
:Reservoir_activeStorageCapacity rdf:type owl:ObjectProperty ;
                                 rdfs:domain :Reservoir ;
                                 rdfs:range <https://w3id.org/netbeheer/IECCIM/TC57CIM/IEC61970/Base/Domain#Volume> ;
                                 rdfs:comment """Storage volume between the full supply level and the normal minimum operating level.
""" .


###  https://w3id.org/netbeheer/IECCIM/TC57CIM/IEC61970/Base/Generation/Production#Reservoir_fullSupplyLevel
:Reservoir_fullSupplyLevel rdf:type owl:ObjectProperty ;
                           rdfs:domain :Reservoir ;
                           rdfs:range <https://w3id.org/netbeheer/IECCIM/TC57CIM/IEC61970/Base/Domain#WaterLevel> ;
                           rdfs:comment "Full supply level, above which water will spill. This can be the spillway crest level or the top of closed gates." .


###  https://w3id.org/netbeheer/IECCIM/TC57CIM/IEC61970/Base/Generation/Production#Reservoir_grossCapacity
:Reservoir_grossCapacity rdf:type owl:ObjectProperty ;
                         rdfs:domain :Reservoir ;
                         rdfs:range <https://w3id.org/netbeheer/IECCIM/TC57CIM/IEC61970/Base/Domain#Volume> ;
                         rdfs:comment """Total capacity of reservoir.
""" .


###  https://w3id.org/netbeheer/IECCIM/TC57CIM/IEC61970/Base/Generation/Production#Reservoir_normalMinOperateLevel
:Reservoir_normalMinOperateLevel rdf:type owl:ObjectProperty ;
                                 rdfs:domain :Reservoir ;
                                 rdfs:range <https://w3id.org/netbeheer/IECCIM/TC57CIM/IEC61970/Base/Domain#WaterLevel> ;
                                 rdfs:comment """Normal minimum operating level below which the penstocks will draw air.
""" .


###  https://w3id.org/netbeheer/IECCIM/TC57CIM/IEC61970/Base/Generation/Production#Reservoir_spillTravelDelay
:Reservoir_spillTravelDelay rdf:type owl:ObjectProperty ;
                            rdfs:domain :Reservoir ;
                            rdfs:range <https://w3id.org/netbeheer/IECCIM/TC57CIM/IEC61970/Base/Domain#Seconds> ;
                            rdfs:comment """The spillway water travel delay to the next downstream reservoir.
""" .


###  https://w3id.org/netbeheer/IECCIM/TC57CIM/IEC61970/Base/Generation/Production#Reservoir_spillwayCrestLength
:Reservoir_spillwayCrestLength rdf:type owl:ObjectProperty ;
                               rdfs:domain :Reservoir ;
                               rdfs:range <https://w3id.org/netbeheer/IECCIM/TC57CIM/IEC61970/Base/Domain#Length> ;
                               rdfs:comment """The length of the spillway crest.
""" .


###  https://w3id.org/netbeheer/IECCIM/TC57CIM/IEC61970/Base/Generation/Production#Reservoir_spillwayCrestLevel
:Reservoir_spillwayCrestLevel rdf:type owl:ObjectProperty ;
                              rdfs:domain :Reservoir ;
                              rdfs:range <https://w3id.org/netbeheer/IECCIM/TC57CIM/IEC61970/Base/Domain#WaterLevel> ;
                              rdfs:comment """Spillway crest level above which water will spill.
""" .


###  https://w3id.org/netbeheer/IECCIM/TC57CIM/IEC61970/Base/Generation/Production#ShutdownCurve_ThermalGeneratingUnit
:ShutdownCurve_ThermalGeneratingUnit rdf:type owl:ObjectProperty ;
                                     rdfs:domain :ShutdownCurve ;
                                     rdfs:range :ThermalGeneratingUnit ;
                                     rdfs:comment "A thermal generating unit may have a shutdown curve.A thermal generating unit may have a shutdown curve." .


###  https://w3id.org/netbeheer/IECCIM/TC57CIM/IEC61970/Base/Generation/Production#ShutdownCurve_shutdownCost
:ShutdownCurve_shutdownCost rdf:type owl:ObjectProperty ;
                            rdfs:domain :ShutdownCurve ;
                            rdfs:range <https://w3id.org/netbeheer/IECCIM/TC57CIM/IEC61970/Base/Domain#Money> ;
                            rdfs:comment """Fixed shutdown cost.
""" .


###  https://w3id.org/netbeheer/IECCIM/TC57CIM/IEC61970/Base/Generation/Production#StartIgnFuelCurve_StartupModel
:StartIgnFuelCurve_StartupModel rdf:type owl:ObjectProperty ;
                                rdfs:domain :StartIgnFuelCurve ;
                                rdfs:range :StartupModel ;
                                rdfs:comment "The unit's startup model may have a startup ignition fuel curve.The unit's startup model may have a startup ignition fuel curve." .


###  https://w3id.org/netbeheer/IECCIM/TC57CIM/IEC61970/Base/Generation/Production#StartMainFuelCurve_StartupModel
:StartMainFuelCurve_StartupModel rdf:type owl:ObjectProperty ;
                                 rdfs:domain :StartMainFuelCurve ;
                                 rdfs:range :StartupModel ;
                                 rdfs:comment "The unit's startup model may have a startup main fuel curve.The unit's startup model may have a startup main fuel curve." .


###  https://w3id.org/netbeheer/IECCIM/TC57CIM/IEC61970/Base/Generation/Production#StartRampCurve_StartupModel
:StartRampCurve_StartupModel rdf:type owl:ObjectProperty ;
                             rdfs:domain :StartRampCurve ;
                             rdfs:range :StartupModel ;
                             rdfs:comment "The unit's startup model may have a startup ramp curve.The unit's startup model may have a startup ramp curve." .


###  https://w3id.org/netbeheer/IECCIM/TC57CIM/IEC61970/Base/Generation/Production#StartRampCurve_hotStandbyRamp
:StartRampCurve_hotStandbyRamp rdf:type owl:ObjectProperty ;
                               rdfs:domain :StartRampCurve ;
                               rdfs:range <https://w3id.org/netbeheer/IECCIM/TC57CIM/IEC61970/Base/Domain#ActivePowerChangeRate> ;
                               rdfs:comment """The startup ramp rate in gross for a unit that is on hot standby.
""" .


###  https://w3id.org/netbeheer/IECCIM/TC57CIM/IEC61970/Base/Generation/Production#StartupModel_StartIgnFuelCurve
:StartupModel_StartIgnFuelCurve rdf:type owl:ObjectProperty ;
                                owl:inverseOf :StartIgnFuelCurve_StartupModel ;
                                rdf:type owl:FunctionalProperty ;
                                rdfs:domain :StartupModel ;
                                rdfs:range :StartIgnFuelCurve ;
                                rdfs:comment "The unit's startup model may have a startup ignition fuel curve.The unit's startup model may have a startup ignition fuel curve." .


###  https://w3id.org/netbeheer/IECCIM/TC57CIM/IEC61970/Base/Generation/Production#StartupModel_StartMainFuelCurve
:StartupModel_StartMainFuelCurve rdf:type owl:ObjectProperty ;
                                 owl:inverseOf :StartMainFuelCurve_StartupModel ;
                                 rdf:type owl:FunctionalProperty ;
                                 rdfs:domain :StartupModel ;
                                 rdfs:range :StartMainFuelCurve ;
                                 rdfs:comment "The unit's startup model may have a startup main fuel curve.The unit's startup model may have a startup main fuel curve." .


###  https://w3id.org/netbeheer/IECCIM/TC57CIM/IEC61970/Base/Generation/Production#StartupModel_StartRampCurve
:StartupModel_StartRampCurve rdf:type owl:ObjectProperty ;
                             owl:inverseOf :StartRampCurve_StartupModel ;
                             rdf:type owl:FunctionalProperty ;
                             rdfs:domain :StartupModel ;
                             rdfs:range :StartRampCurve ;
                             rdfs:comment "The unit's startup model may have a startup ramp curve.The unit's startup model may have a startup ramp curve." .


###  https://w3id.org/netbeheer/IECCIM/TC57CIM/IEC61970/Base/Generation/Production#StartupModel_ThermalGeneratingUnit
:StartupModel_ThermalGeneratingUnit rdf:type owl:ObjectProperty ;
                                    rdfs:domain :StartupModel ;
                                    rdfs:range :ThermalGeneratingUnit ;
                                    rdfs:comment "A thermal generating unit may have a startup model.A thermal generating unit may have a startup model." .


###  https://w3id.org/netbeheer/IECCIM/TC57CIM/IEC61970/Base/Generation/Production#StartupModel_fixedMaintCost
:StartupModel_fixedMaintCost rdf:type owl:ObjectProperty ;
                             rdfs:domain :StartupModel ;
                             rdfs:range <https://w3id.org/netbeheer/IECCIM/TC57CIM/IEC61970/Base/Domain#CostRate> ;
                             rdfs:comment """Fixed maintenance cost.
""" .


###  https://w3id.org/netbeheer/IECCIM/TC57CIM/IEC61970/Base/Generation/Production#StartupModel_hotStandbyHeat
:StartupModel_hotStandbyHeat rdf:type owl:ObjectProperty ;
                             rdfs:domain :StartupModel ;
                             rdfs:range :HeatRate ;
                             rdfs:comment """The amount of heat input per time uint required for hot standby operation.
""" .


###  https://w3id.org/netbeheer/IECCIM/TC57CIM/IEC61970/Base/Generation/Production#StartupModel_incrementalMaintCost
:StartupModel_incrementalMaintCost rdf:type owl:ObjectProperty ;
                                   rdfs:domain :StartupModel ;
                                   rdfs:range <https://w3id.org/netbeheer/IECCIM/TC57CIM/IEC61970/Base/Domain#CostPerEnergyUnit> ;
                                   rdfs:comment """Incremental maintenance cost.
""" .


###  https://w3id.org/netbeheer/IECCIM/TC57CIM/IEC61970/Base/Generation/Production#StartupModel_minimumDownTime
:StartupModel_minimumDownTime rdf:type owl:ObjectProperty ;
                              rdfs:domain :StartupModel ;
                              rdfs:range <https://w3id.org/netbeheer/IECCIM/TC57CIM/IEC61970/Base/Domain#Hours> ;
                              rdfs:comment """The minimum number of hours the unit must be down before restart.
""" .


###  https://w3id.org/netbeheer/IECCIM/TC57CIM/IEC61970/Base/Generation/Production#StartupModel_minimumRunTime
:StartupModel_minimumRunTime rdf:type owl:ObjectProperty ;
                             rdfs:domain :StartupModel ;
                             rdfs:range <https://w3id.org/netbeheer/IECCIM/TC57CIM/IEC61970/Base/Domain#Hours> ;
                             rdfs:comment """The minimum number of hours the unit must be operating before being allowed to shut down.
""" .


###  https://w3id.org/netbeheer/IECCIM/TC57CIM/IEC61970/Base/Generation/Production#StartupModel_riskFactorCost
:StartupModel_riskFactorCost rdf:type owl:ObjectProperty ;
                             rdfs:domain :StartupModel ;
                             rdfs:range <https://w3id.org/netbeheer/IECCIM/TC57CIM/IEC61970/Base/Domain#Money> ;
                             rdfs:comment "The opportunity cost associated with the return in monetary unit. This represents the restart's \"share\" of the unit depreciation and risk of an event which would damage the unit." .


###  https://w3id.org/netbeheer/IECCIM/TC57CIM/IEC61970/Base/Generation/Production#StartupModel_startupCost
:StartupModel_startupCost rdf:type owl:ObjectProperty ;
                          rdfs:domain :StartupModel ;
                          rdfs:range <https://w3id.org/netbeheer/IECCIM/TC57CIM/IEC61970/Base/Domain#Money> ;
                          rdfs:comment """Total miscellaneous start up costs.
""" .


###  https://w3id.org/netbeheer/IECCIM/TC57CIM/IEC61970/Base/Generation/Production#StartupModel_stbyAuxP
:StartupModel_stbyAuxP rdf:type owl:ObjectProperty ;
                       rdfs:domain :StartupModel ;
                       rdfs:range <https://w3id.org/netbeheer/IECCIM/TC57CIM/IEC61970/Base/Domain#ActivePower> ;
                       rdfs:comment """The unit's auxiliary active power consumption to maintain standby mode.
""" .


###  https://w3id.org/netbeheer/IECCIM/TC57CIM/IEC61970/Base/Generation/Production#SteamSendoutSchedule_CogenerationPlant
:SteamSendoutSchedule_CogenerationPlant rdf:type owl:ObjectProperty ,
                                                 owl:FunctionalProperty ;
                                        rdfs:domain :SteamSendoutSchedule ;
                                        rdfs:range :CogenerationPlant ;
                                        rdfs:comment "A cogeneration plant has a steam sendout schedule.A cogeneration plant has a steam sendout schedule." .


###  https://w3id.org/netbeheer/IECCIM/TC57CIM/IEC61970/Base/Generation/Production#TailbayLossCurve_HydroGeneratingUnit
:TailbayLossCurve_HydroGeneratingUnit rdf:type owl:ObjectProperty ;
                                      rdfs:domain :TailbayLossCurve ;
                                      rdfs:range :HydroGeneratingUnit ;
                                      rdfs:comment "A hydro generating unit has a tailbay loss curve.A hydro generating unit has a tailbay loss curve." .


###  https://w3id.org/netbeheer/IECCIM/TC57CIM/IEC61970/Base/Generation/Production#TargetLevelSchedule_Reservoir
:TargetLevelSchedule_Reservoir rdf:type owl:ObjectProperty ;
                               rdfs:domain :TargetLevelSchedule ;
                               rdfs:range :Reservoir ;
                               rdfs:comment "A reservoir may have a water level target schedule.A reservoir may have a water level target schedule." .


###  https://w3id.org/netbeheer/IECCIM/TC57CIM/IEC61970/Base/Generation/Production#TargetLevelSchedule_highLevelLimit
:TargetLevelSchedule_highLevelLimit rdf:type owl:ObjectProperty ;
                                    rdfs:domain :TargetLevelSchedule ;
                                    rdfs:range <https://w3id.org/netbeheer/IECCIM/TC57CIM/IEC61970/Base/Domain#WaterLevel> ;
                                    rdfs:comment """High target level limit, above which the reservoir operation will be penalized.
""" .


###  https://w3id.org/netbeheer/IECCIM/TC57CIM/IEC61970/Base/Generation/Production#TargetLevelSchedule_lowLevelLimit
:TargetLevelSchedule_lowLevelLimit rdf:type owl:ObjectProperty ;
                                   rdfs:domain :TargetLevelSchedule ;
                                   rdfs:range <https://w3id.org/netbeheer/IECCIM/TC57CIM/IEC61970/Base/Domain#WaterLevel> ;
                                   rdfs:comment """Low target level limit, below which the reservoir operation will be penalized.
""" .


###  https://w3id.org/netbeheer/IECCIM/TC57CIM/IEC61970/Base/Generation/Production#ThermalGeneratingUnit_CAESPlant
:ThermalGeneratingUnit_CAESPlant rdf:type owl:ObjectProperty ;
                                 owl:inverseOf :CAESPlant_ThermalGeneratingUnit ;
                                 rdfs:domain :ThermalGeneratingUnit ;
                                 rdfs:range :CAESPlant ;
                                 rdfs:comment "A thermal generating unit may be a member of a compressed air energy storage plant.A thermal generating unit may be a member of a compressed air energy storage plant." .


###  https://w3id.org/netbeheer/IECCIM/TC57CIM/IEC61970/Base/Generation/Production#ThermalGeneratingUnit_CogenerationPlant
:ThermalGeneratingUnit_CogenerationPlant rdf:type owl:ObjectProperty ;
                                         owl:inverseOf :CogenerationPlant_ThermalGeneratingUnits ;
                                         rdfs:domain :ThermalGeneratingUnit ;
                                         rdfs:range :CogenerationPlant ;
                                         rdfs:comment "A thermal generating unit may be a member of a cogeneration plant.A thermal generating unit may be a member of a cogeneration plant." .


###  https://w3id.org/netbeheer/IECCIM/TC57CIM/IEC61970/Base/Generation/Production#ThermalGeneratingUnit_CombinedCyclePlant
:ThermalGeneratingUnit_CombinedCyclePlant rdf:type owl:ObjectProperty ;
                                          owl:inverseOf :CombinedCyclePlant_ThermalGeneratingUnits ;
                                          rdfs:domain :ThermalGeneratingUnit ;
                                          rdfs:range :CombinedCyclePlant ;
                                          rdfs:comment "A thermal generating unit may be a member of a combined cycle plant.A thermal generating unit may be a member of a combined cycle plant." .


###  https://w3id.org/netbeheer/IECCIM/TC57CIM/IEC61970/Base/Generation/Production#ThermalGeneratingUnit_EmissionCurves
:ThermalGeneratingUnit_EmissionCurves rdf:type owl:ObjectProperty ;
                                      owl:inverseOf :EmissionCurve_ThermalGeneratingUnit ;
                                      rdf:type owl:FunctionalProperty ;
                                      rdfs:domain :ThermalGeneratingUnit ;
                                      rdfs:range :EmissionCurve ;
                                      rdfs:comment "A thermal generating unit may have  one or more emission curves.A thermal generating unit may have  one or more emission curves." .


###  https://w3id.org/netbeheer/IECCIM/TC57CIM/IEC61970/Base/Generation/Production#ThermalGeneratingUnit_EmmissionAccounts
:ThermalGeneratingUnit_EmmissionAccounts rdf:type owl:ObjectProperty ;
                                         owl:inverseOf :EmissionAccount_ThermalGeneratingUnit ;
                                         rdf:type owl:FunctionalProperty ;
                                         rdfs:domain :ThermalGeneratingUnit ;
                                         rdfs:range :EmissionAccount ;
                                         rdfs:comment "A thermal generating unit may have one or more emission allowance accounts.A thermal generating unit may have one or more emission allowance accounts." .


###  https://w3id.org/netbeheer/IECCIM/TC57CIM/IEC61970/Base/Generation/Production#ThermalGeneratingUnit_FossilFuels
:ThermalGeneratingUnit_FossilFuels rdf:type owl:ObjectProperty ;
                                   owl:inverseOf :FossilFuel_ThermalGeneratingUnit ;
                                   rdf:type owl:FunctionalProperty ;
                                   rdfs:domain :ThermalGeneratingUnit ;
                                   rdfs:range :FossilFuel ;
                                   rdfs:comment "A thermal generating unit may have one or more fossil fuels.A thermal generating unit may have one or more fossil fuels." .


###  https://w3id.org/netbeheer/IECCIM/TC57CIM/IEC61970/Base/Generation/Production#ThermalGeneratingUnit_FuelAllocationSchedules
:ThermalGeneratingUnit_FuelAllocationSchedules rdf:type owl:ObjectProperty ;
                                               owl:inverseOf :FuelAllocationSchedule_ThermalGeneratingUnit ;
                                               rdf:type owl:FunctionalProperty ;
                                               rdfs:domain :ThermalGeneratingUnit ;
                                               rdfs:range :FuelAllocationSchedule ;
                                               rdfs:comment "A thermal generating unit may have one or more fuel allocation schedules.A thermal generating unit may have one or more fuel allocation schedules." .


###  https://w3id.org/netbeheer/IECCIM/TC57CIM/IEC61970/Base/Generation/Production#ThermalGeneratingUnit_HeatInputCurve
:ThermalGeneratingUnit_HeatInputCurve rdf:type owl:ObjectProperty ;
                                      owl:inverseOf :HeatInputCurve_ThermalGeneratingUnit ;
                                      rdf:type owl:FunctionalProperty ;
                                      rdfs:domain :ThermalGeneratingUnit ;
                                      rdfs:range :HeatInputCurve ;
                                      rdfs:comment "A thermal generating unit may have a heat input curve.A thermal generating unit may have a heat input curve." .


###  https://w3id.org/netbeheer/IECCIM/TC57CIM/IEC61970/Base/Generation/Production#ThermalGeneratingUnit_HeatRateCurve
:ThermalGeneratingUnit_HeatRateCurve rdf:type owl:ObjectProperty ;
                                     owl:inverseOf :HeatRateCurve_ThermalGeneratingUnit ;
                                     rdf:type owl:FunctionalProperty ;
                                     rdfs:domain :ThermalGeneratingUnit ;
                                     rdfs:range :HeatRateCurve ;
                                     rdfs:comment "A thermal generating unit may have a heat rate curve.A thermal generating unit may have a heat rate curve." .


###  https://w3id.org/netbeheer/IECCIM/TC57CIM/IEC61970/Base/Generation/Production#ThermalGeneratingUnit_IncrementalHeatRateCurve
:ThermalGeneratingUnit_IncrementalHeatRateCurve rdf:type owl:ObjectProperty ;
                                                owl:inverseOf :IncrementalHeatRateCurve_ThermalGeneratingUnit ;
                                                rdf:type owl:FunctionalProperty ;
                                                rdfs:domain :ThermalGeneratingUnit ;
                                                rdfs:range :IncrementalHeatRateCurve ;
                                                rdfs:comment "A thermal generating unit may have an incremental heat rate curve.A thermal generating unit may have an incremental heat rate curve." .


###  https://w3id.org/netbeheer/IECCIM/TC57CIM/IEC61970/Base/Generation/Production#ThermalGeneratingUnit_ShutdownCurve
:ThermalGeneratingUnit_ShutdownCurve rdf:type owl:ObjectProperty ;
                                     owl:inverseOf :ShutdownCurve_ThermalGeneratingUnit ;
                                     rdf:type owl:FunctionalProperty ;
                                     rdfs:domain :ThermalGeneratingUnit ;
                                     rdfs:range :ShutdownCurve ;
                                     rdfs:comment "A thermal generating unit may have a shutdown curve.A thermal generating unit may have a shutdown curve." .


###  https://w3id.org/netbeheer/IECCIM/TC57CIM/IEC61970/Base/Generation/Production#ThermalGeneratingUnit_StartupModel
:ThermalGeneratingUnit_StartupModel rdf:type owl:ObjectProperty ;
                                    owl:inverseOf :StartupModel_ThermalGeneratingUnit ;
                                    rdf:type owl:FunctionalProperty ;
                                    rdfs:domain :ThermalGeneratingUnit ;
                                    rdfs:range :StartupModel ;
                                    rdfs:comment "A thermal generating unit may have a startup model.A thermal generating unit may have a startup model." .


###  https://w3id.org/netbeheer/IECCIM/TC57CIM/IEC61970/Base/Generation/Production#ThermalGeneratingUnit_oMCost
:ThermalGeneratingUnit_oMCost rdf:type owl:ObjectProperty ;
                              rdfs:domain :ThermalGeneratingUnit ;
                              rdfs:range :CostPerHeatUnit ;
                              rdfs:comment """Operating and maintenance cost for the thermal unit.
""" .


#################################################################
#    Data properties
#################################################################

###  https://w3id.org/netbeheer/IECCIM/TC57CIM/IEC61970/Base/Generation/Production#AirCompressor_airCompressorRating
:AirCompressor_airCompressorRating rdf:type owl:DatatypeProperty ;
                                   rdfs:domain :AirCompressor ;
                                   rdfs:range xsd:float ;
                                   rdfs:comment """Rating of the CAES air compressor.
""" .


###  https://w3id.org/netbeheer/IECCIM/TC57CIM/IEC61970/Base/Generation/Production#Classification_multiplier
:Classification_multiplier rdf:type owl:DatatypeProperty ;
                           rdfs:domain :Classification ;
                           rdfs:range <https://w3id.org/netbeheer/IECCIM/TC57CIM/IEC61970/Base/Domain#UnitMultiplier> .


###  https://w3id.org/netbeheer/IECCIM/TC57CIM/IEC61970/Base/Generation/Production#Classification_unit
:Classification_unit rdf:type owl:DatatypeProperty ;
                     rdfs:domain :Classification ;
                     rdfs:range <https://w3id.org/netbeheer/IECCIM/TC57CIM/IEC61970/Base/Domain#UnitSymbol> .


###  https://w3id.org/netbeheer/IECCIM/TC57CIM/IEC61970/Base/Generation/Production#Classification_value
:Classification_value rdf:type owl:DatatypeProperty ;
                      rdfs:domain :Classification ;
                      rdfs:range xsd:nonNegativeInteger .


###  https://w3id.org/netbeheer/IECCIM/TC57CIM/IEC61970/Base/Generation/Production#CogenerationPlant_cogenHPSendoutRating
:CogenerationPlant_cogenHPSendoutRating rdf:type owl:DatatypeProperty ;
                                        rdfs:domain :CogenerationPlant ;
                                        rdfs:range xsd:float ;
                                        rdfs:comment """The high pressure steam sendout.
""" .


###  https://w3id.org/netbeheer/IECCIM/TC57CIM/IEC61970/Base/Generation/Production#CogenerationPlant_cogenHPSteamRating
:CogenerationPlant_cogenHPSteamRating rdf:type owl:DatatypeProperty ;
                                      rdfs:domain :CogenerationPlant ;
                                      rdfs:range xsd:float ;
                                      rdfs:comment """The high pressure steam rating.
""" .


###  https://w3id.org/netbeheer/IECCIM/TC57CIM/IEC61970/Base/Generation/Production#CogenerationPlant_cogenLPSendoutRating
:CogenerationPlant_cogenLPSendoutRating rdf:type owl:DatatypeProperty ;
                                        rdfs:domain :CogenerationPlant ;
                                        rdfs:range xsd:float ;
                                        rdfs:comment """The low pressure steam sendout.
""" .


###  https://w3id.org/netbeheer/IECCIM/TC57CIM/IEC61970/Base/Generation/Production#CogenerationPlant_cogenLPSteamRating
:CogenerationPlant_cogenLPSteamRating rdf:type owl:DatatypeProperty ;
                                      rdfs:domain :CogenerationPlant ;
                                      rdfs:range xsd:float ;
                                      rdfs:comment """The low pressure steam rating.
""" .


###  https://w3id.org/netbeheer/IECCIM/TC57CIM/IEC61970/Base/Generation/Production#CostPerHeatUnit_denominatorMultiplier
:CostPerHeatUnit_denominatorMultiplier rdf:type owl:DatatypeProperty ;
                                       rdfs:domain :CostPerHeatUnit ;
                                       rdfs:range <https://w3id.org/netbeheer/IECCIM/TC57CIM/IEC61970/Base/Domain#UnitMultiplier> .


###  https://w3id.org/netbeheer/IECCIM/TC57CIM/IEC61970/Base/Generation/Production#CostPerHeatUnit_denominatorUnit
:CostPerHeatUnit_denominatorUnit rdf:type owl:DatatypeProperty ;
                                 rdfs:domain :CostPerHeatUnit ;
                                 rdfs:range <https://w3id.org/netbeheer/IECCIM/TC57CIM/IEC61970/Base/Domain#UnitSymbol> .


###  https://w3id.org/netbeheer/IECCIM/TC57CIM/IEC61970/Base/Generation/Production#CostPerHeatUnit_multiplier
:CostPerHeatUnit_multiplier rdf:type owl:DatatypeProperty ;
                            rdfs:domain :CostPerHeatUnit ;
                            rdfs:range <https://w3id.org/netbeheer/IECCIM/TC57CIM/IEC61970/Base/Domain#UnitMultiplier> .


###  https://w3id.org/netbeheer/IECCIM/TC57CIM/IEC61970/Base/Generation/Production#CostPerHeatUnit_unit
:CostPerHeatUnit_unit rdf:type owl:DatatypeProperty ;
                      rdfs:domain :CostPerHeatUnit ;
                      rdfs:range <https://w3id.org/netbeheer/IECCIM/TC57CIM/IEC61970/Base/Domain#Currency> .


###  https://w3id.org/netbeheer/IECCIM/TC57CIM/IEC61970/Base/Generation/Production#CostPerHeatUnit_value
:CostPerHeatUnit_value rdf:type owl:DatatypeProperty ;
                       rdfs:domain :CostPerHeatUnit ;
                       rdfs:range xsd:float .


###  https://w3id.org/netbeheer/IECCIM/TC57CIM/IEC61970/Base/Generation/Production#EmissionAccount_emissionType
:EmissionAccount_emissionType rdf:type owl:DatatypeProperty ;
                              rdfs:domain :EmissionAccount ;
                              rdfs:range :EmissionType ;
                              rdfs:comment "The type of emission, for example sulfur dioxide (SO2). The y1AxisUnits of the curve contains the unit of measure (e.g. kg) and the emissionType is the type of emission (e.g. sulfer dioxide)." .


###  https://w3id.org/netbeheer/IECCIM/TC57CIM/IEC61970/Base/Generation/Production#EmissionAccount_emissionValueSource
:EmissionAccount_emissionValueSource rdf:type owl:DatatypeProperty ;
                                     rdfs:domain :EmissionAccount ;
                                     rdfs:range :EmissionValueSource ;
                                     rdfs:comment "The source of the emission value." .


###  https://w3id.org/netbeheer/IECCIM/TC57CIM/IEC61970/Base/Generation/Production#EmissionCurve_emissionType
:EmissionCurve_emissionType rdf:type owl:DatatypeProperty ;
                            rdfs:domain :EmissionCurve ;
                            rdfs:range :EmissionType ;
                            rdfs:comment "The type of emission, which also gives the production rate measurement unit. The y1AxisUnits of the curve contains the unit of measure (e.g. kg) and the emissionType is the type of emission (e.g. sulfer dioxide)." .


###  https://w3id.org/netbeheer/IECCIM/TC57CIM/IEC61970/Base/Generation/Production#EmissionCurve_isNetGrossP
:EmissionCurve_isNetGrossP rdf:type owl:DatatypeProperty ;
                           rdfs:domain :EmissionCurve ;
                           rdfs:range xsd:boolean ;
                           rdfs:comment """Flag is set to true when output is expressed in net active power.
""" .


###  https://w3id.org/netbeheer/IECCIM/TC57CIM/IEC61970/Base/Generation/Production#Emission_multiplier
:Emission_multiplier rdf:type owl:DatatypeProperty ;
                     rdfs:domain :Emission ;
                     rdfs:range <https://w3id.org/netbeheer/IECCIM/TC57CIM/IEC61970/Base/Domain#UnitMultiplier> .


###  https://w3id.org/netbeheer/IECCIM/TC57CIM/IEC61970/Base/Generation/Production#Emission_unit
:Emission_unit rdf:type owl:DatatypeProperty ;
               rdfs:domain :Emission ;
               rdfs:range <https://w3id.org/netbeheer/IECCIM/TC57CIM/IEC61970/Base/Domain#UnitSymbol> .


###  https://w3id.org/netbeheer/IECCIM/TC57CIM/IEC61970/Base/Generation/Production#Emission_value
:Emission_value rdf:type owl:DatatypeProperty ;
                rdfs:domain :Emission ;
                rdfs:range xsd:float .


###  https://w3id.org/netbeheer/IECCIM/TC57CIM/IEC61970/Base/Generation/Production#FossilFuel_fossilFuelType
:FossilFuel_fossilFuelType rdf:type owl:DatatypeProperty ;
                           rdfs:domain :FossilFuel ;
                           rdfs:range :FuelType ;
                           rdfs:comment "The type of fossil fuel, such as coal, oil, or gas." .


###  https://w3id.org/netbeheer/IECCIM/TC57CIM/IEC61970/Base/Generation/Production#FossilFuel_fuelHeatContent
:FossilFuel_fuelHeatContent rdf:type owl:DatatypeProperty ;
                            rdfs:domain :FossilFuel ;
                            rdfs:range xsd:float ;
                            rdfs:comment """The amount of heat per weight (or volume) of the given type of fuel.
""" .


###  https://w3id.org/netbeheer/IECCIM/TC57CIM/IEC61970/Base/Generation/Production#FuelAllocationSchedule_fuelAllocationEndDate
:FuelAllocationSchedule_fuelAllocationEndDate rdf:type owl:DatatypeProperty ;
                                              rdfs:domain :FuelAllocationSchedule ;
                                              rdfs:range xsd:dateTime ;
                                              rdfs:comment """The end time and date of the fuel allocation schedule.
""" .


###  https://w3id.org/netbeheer/IECCIM/TC57CIM/IEC61970/Base/Generation/Production#FuelAllocationSchedule_fuelAllocationStartDate
:FuelAllocationSchedule_fuelAllocationStartDate rdf:type owl:DatatypeProperty ;
                                                rdfs:domain :FuelAllocationSchedule ;
                                                rdfs:range xsd:dateTime ;
                                                rdfs:comment """The start time and date of the fuel allocation schedule.
""" .


###  https://w3id.org/netbeheer/IECCIM/TC57CIM/IEC61970/Base/Generation/Production#FuelAllocationSchedule_fuelType
:FuelAllocationSchedule_fuelType rdf:type owl:DatatypeProperty ;
                                 rdfs:domain :FuelAllocationSchedule ;
                                 rdfs:range :FuelType ;
                                 rdfs:comment """The type of fuel, which also indicates the corresponding measurement unit.
""" .


###  https://w3id.org/netbeheer/IECCIM/TC57CIM/IEC61970/Base/Generation/Production#FuelAllocationSchedule_maxFuelAllocation
:FuelAllocationSchedule_maxFuelAllocation rdf:type owl:DatatypeProperty ;
                                          rdfs:domain :FuelAllocationSchedule ;
                                          rdfs:range xsd:float ;
                                          rdfs:comment """The maximum amount fuel that is allocated for consumption for the scheduled time period.
""" .


###  https://w3id.org/netbeheer/IECCIM/TC57CIM/IEC61970/Base/Generation/Production#FuelAllocationSchedule_minFuelAllocation
:FuelAllocationSchedule_minFuelAllocation rdf:type owl:DatatypeProperty ;
                                          rdfs:domain :FuelAllocationSchedule ;
                                          rdfs:range xsd:float ;
                                          rdfs:comment """The minimum amount fuel that is allocated for consumption for the scheduled time period, e.g., based on a \"take-or-pay\" contract.
""" .


###  https://w3id.org/netbeheer/IECCIM/TC57CIM/IEC61970/Base/Generation/Production#GenUnitOpCostCurve_isNetGrossP
:GenUnitOpCostCurve_isNetGrossP rdf:type owl:DatatypeProperty ;
                                rdfs:domain :GenUnitOpCostCurve ;
                                rdfs:range xsd:boolean ;
                                rdfs:comment """Flag is set to true when output is expressed in net active power.
""" .


###  https://w3id.org/netbeheer/IECCIM/TC57CIM/IEC61970/Base/Generation/Production#GeneratingUnit_genControlMode
:GeneratingUnit_genControlMode rdf:type owl:DatatypeProperty ;
                               rdfs:domain :GeneratingUnit ;
                               rdfs:range :GeneratorControlMode ;
                               rdfs:comment "The unit control mode." .


###  https://w3id.org/netbeheer/IECCIM/TC57CIM/IEC61970/Base/Generation/Production#GeneratingUnit_genControlSource
:GeneratingUnit_genControlSource rdf:type owl:DatatypeProperty ;
                                 rdfs:domain :GeneratingUnit ;
                                 rdfs:range :GeneratorControlSource ;
                                 rdfs:comment "The source of controls for a generating unit." .


###  https://w3id.org/netbeheer/IECCIM/TC57CIM/IEC61970/Base/Generation/Production#GeneratingUnit_longPF
:GeneratingUnit_longPF rdf:type owl:DatatypeProperty ;
                       rdfs:domain :GeneratingUnit ;
                       rdfs:range xsd:float ;
                       rdfs:comment """Generating unit long term economic participation factor.
""" .


###  https://w3id.org/netbeheer/IECCIM/TC57CIM/IEC61970/Base/Generation/Production#GeneratingUnit_normalPF
:GeneratingUnit_normalPF rdf:type owl:DatatypeProperty ;
                         rdfs:domain :GeneratingUnit ;
                         rdfs:range xsd:float ;
                         rdfs:comment """Generating unit economic participation factor.
""" .


###  https://w3id.org/netbeheer/IECCIM/TC57CIM/IEC61970/Base/Generation/Production#GeneratingUnit_penaltyFactor
:GeneratingUnit_penaltyFactor rdf:type owl:DatatypeProperty ;
                              rdfs:domain :GeneratingUnit ;
                              rdfs:range xsd:float ;
                              rdfs:comment "Defined as: 1 / ( 1 - Incremental Transmission Loss); with the Incremental Transmission Loss expressed as a plus or minus value. The typical range of penalty factors is (0.9 to 1.1)." .


###  https://w3id.org/netbeheer/IECCIM/TC57CIM/IEC61970/Base/Generation/Production#GeneratingUnit_shortPF
:GeneratingUnit_shortPF rdf:type owl:DatatypeProperty ;
                        rdfs:domain :GeneratingUnit ;
                        rdfs:range xsd:float ;
                        rdfs:comment """Generating unit short term economic participation factor.
""" .


###  https://w3id.org/netbeheer/IECCIM/TC57CIM/IEC61970/Base/Generation/Production#GeneratingUnit_tieLinePF
:GeneratingUnit_tieLinePF rdf:type owl:DatatypeProperty ;
                          rdfs:domain :GeneratingUnit ;
                          rdfs:range xsd:float ;
                          rdfs:comment """Generating unit economic participation factor.
""" .


###  https://w3id.org/netbeheer/IECCIM/TC57CIM/IEC61970/Base/Generation/Production#HeatInputCurve_isNetGrossP
:HeatInputCurve_isNetGrossP rdf:type owl:DatatypeProperty ;
                            rdfs:domain :HeatInputCurve ;
                            rdfs:range xsd:boolean ;
                            rdfs:comment """Flag is set to true when output is expressed in net active power.
""" .


###  https://w3id.org/netbeheer/IECCIM/TC57CIM/IEC61970/Base/Generation/Production#HeatRateCurve_isNetGrossP
:HeatRateCurve_isNetGrossP rdf:type owl:DatatypeProperty ;
                           rdfs:domain :HeatRateCurve ;
                           rdfs:range xsd:boolean ;
                           rdfs:comment """Flag is set to true when output is expressed in net active power.
""" .


###  https://w3id.org/netbeheer/IECCIM/TC57CIM/IEC61970/Base/Generation/Production#HeatRate_multiplier
:HeatRate_multiplier rdf:type owl:DatatypeProperty ;
                     rdfs:domain :HeatRate ;
                     rdfs:range <https://w3id.org/netbeheer/IECCIM/TC57CIM/IEC61970/Base/Domain#UnitMultiplier> .


###  https://w3id.org/netbeheer/IECCIM/TC57CIM/IEC61970/Base/Generation/Production#HeatRate_unit
:HeatRate_unit rdf:type owl:DatatypeProperty ;
               rdfs:domain :HeatRate ;
               rdfs:range <https://w3id.org/netbeheer/IECCIM/TC57CIM/IEC61970/Base/Domain#UnitSymbol> .


###  https://w3id.org/netbeheer/IECCIM/TC57CIM/IEC61970/Base/Generation/Production#HeatRate_value
:HeatRate_value rdf:type owl:DatatypeProperty ;
                rdfs:domain :HeatRate ;
                rdfs:range xsd:float .


###  https://w3id.org/netbeheer/IECCIM/TC57CIM/IEC61970/Base/Generation/Production#HydroGeneratingUnit_energyConversionCapability
:HydroGeneratingUnit_energyConversionCapability rdf:type owl:DatatypeProperty ;
                                                rdfs:domain :HydroGeneratingUnit ;
                                                rdfs:range :HydroEnergyConversionKind ;
                                                rdfs:comment "Energy conversion capability for generating." .


###  https://w3id.org/netbeheer/IECCIM/TC57CIM/IEC61970/Base/Generation/Production#HydroPowerPlant_hydroPlantStorageType
:HydroPowerPlant_hydroPlantStorageType rdf:type owl:DatatypeProperty ;
                                       rdfs:domain :HydroPowerPlant ;
                                       rdfs:range :HydroPlantStorageKind ;
                                       rdfs:comment "The type of hydro power plant water storage." .


###  https://w3id.org/netbeheer/IECCIM/TC57CIM/IEC61970/Base/Generation/Production#HydroPowerPlant_penstockType
:HydroPowerPlant_penstockType rdf:type owl:DatatypeProperty ;
                              rdfs:domain :HydroPowerPlant ;
                              rdfs:range xsd:string ;
                              rdfs:comment "Type and configuration of hydro plant penstock(s)." .


###  https://w3id.org/netbeheer/IECCIM/TC57CIM/IEC61970/Base/Generation/Production#HydroPowerPlant_surgeTankCode
:HydroPowerPlant_surgeTankCode rdf:type owl:DatatypeProperty ;
                               rdfs:domain :HydroPowerPlant ;
                               rdfs:range xsd:string ;
                               rdfs:comment "A code describing the type (or absence) of surge tank that is associated with the hydro power plant." .


###  https://w3id.org/netbeheer/IECCIM/TC57CIM/IEC61970/Base/Generation/Production#IncrementalHeatRateCurve_isNetGrossP
:IncrementalHeatRateCurve_isNetGrossP rdf:type owl:DatatypeProperty ;
                                      rdfs:domain :IncrementalHeatRateCurve ;
                                      rdfs:range xsd:boolean ;
                                      rdfs:comment """Flag is set to true when output is expressed in net active power.
""" .


###  https://w3id.org/netbeheer/IECCIM/TC57CIM/IEC61970/Base/Generation/Production#Reservoir_energyStorageRating
:Reservoir_energyStorageRating rdf:type owl:DatatypeProperty ;
                               rdfs:domain :Reservoir ;
                               rdfs:range xsd:float ;
                               rdfs:comment """The reservoir's energy storage rating in energy for given head conditions.
""" .


###  https://w3id.org/netbeheer/IECCIM/TC57CIM/IEC61970/Base/Generation/Production#Reservoir_riverOutletWorks
:Reservoir_riverOutletWorks rdf:type owl:DatatypeProperty ;
                            rdfs:domain :Reservoir ;
                            rdfs:range xsd:string ;
                            rdfs:comment """River outlet works for riparian right releases or other purposes.
""" .


###  https://w3id.org/netbeheer/IECCIM/TC57CIM/IEC61970/Base/Generation/Production#Reservoir_spillWayGateType
:Reservoir_spillWayGateType rdf:type owl:DatatypeProperty ;
                            rdfs:domain :Reservoir ;
                            rdfs:range xsd:string ;
                            rdfs:comment "Type of spillway gate, including parameters." .


###  https://w3id.org/netbeheer/IECCIM/TC57CIM/IEC61970/Base/Generation/Production#Reservoir_spillwayCapacity
:Reservoir_spillwayCapacity rdf:type owl:DatatypeProperty ;
                            rdfs:domain :Reservoir ;
                            rdfs:range xsd:float ;
                            rdfs:comment """The flow capacity of the spillway in cubic meters per second.
""" .


###  https://w3id.org/netbeheer/IECCIM/TC57CIM/IEC61970/Base/Generation/Production#ShutdownCurve_shutdownDate
:ShutdownCurve_shutdownDate rdf:type owl:DatatypeProperty ;
                            rdfs:domain :ShutdownCurve ;
                            rdfs:range xsd:dateTime ;
                            rdfs:comment """The date and time of the most recent generating unit shutdown.
""" .


###  https://w3id.org/netbeheer/IECCIM/TC57CIM/IEC61970/Base/Generation/Production#StartIgnFuelCurve_ignitionFuelType
:StartIgnFuelCurve_ignitionFuelType rdf:type owl:DatatypeProperty ;
                                    rdfs:domain :StartIgnFuelCurve ;
                                    rdfs:range :FuelType ;
                                    rdfs:comment """Type of ignition fuel.
""" .


###  https://w3id.org/netbeheer/IECCIM/TC57CIM/IEC61970/Base/Generation/Production#StartMainFuelCurve_mainFuelType
:StartMainFuelCurve_mainFuelType rdf:type owl:DatatypeProperty ;
                                 rdfs:domain :StartMainFuelCurve ;
                                 rdfs:range :FuelType ;
                                 rdfs:comment """Type of main fuel.
""" .


###  https://w3id.org/netbeheer/IECCIM/TC57CIM/IEC61970/Base/Generation/Production#StartupModel_startupDate
:StartupModel_startupDate rdf:type owl:DatatypeProperty ;
                          rdfs:domain :StartupModel ;
                          rdfs:range xsd:dateTime ;
                          rdfs:comment """The date and time of the most recent generating unit startup.
""" .


###  https://w3id.org/netbeheer/IECCIM/TC57CIM/IEC61970/Base/Generation/Production#StartupModel_startupPriority
:StartupModel_startupPriority rdf:type owl:DatatypeProperty ;
                              rdfs:domain :StartupModel ;
                              rdfs:range xsd:nonNegativeInteger ;
                              rdfs:comment "Startup priority within control area where lower numbers indicate higher priorities.  More than one unit in an area may be assigned the same priority." .


###  https://w3id.org/netbeheer/IECCIM/TC57CIM/IEC61970/Base/Generation/Production#WindGeneratingUnit_windGenUnitType
:WindGeneratingUnit_windGenUnitType rdf:type owl:DatatypeProperty ;
                                    rdfs:domain :WindGeneratingUnit ;
                                    rdfs:range :WindGenUnitKind ;
                                    rdfs:comment "The kind of wind generating unit" .


#################################################################
#    Classes
#################################################################

###  https://w3id.org/netbeheer/IECCIM/TC57CIM/IEC61970/Base/ControlArea#ControlAreaGeneratingUnit
<https://w3id.org/netbeheer/IECCIM/TC57CIM/IEC61970/Base/ControlArea#ControlAreaGeneratingUnit> rdf:type owl:Class ;
                                                                                                rdfs:subClassOf [ rdf:type owl:Restriction ;
                                                                                                                  owl:onProperty :ControlAreaGeneratingUnit_GeneratingUnit ;
                                                                                                                  owl:minQualifiedCardinality "0"^^xsd:nonNegativeInteger ;
                                                                                                                  owl:onClass <https://w3id.org/netbeheer/IECCIM/TC57CIM/IEC61970/Base/ControlArea#ControlAreaGeneratingUnit>
                                                                                                                ] .


###  https://w3id.org/netbeheer/IECCIM/TC57CIM/IEC61970/Base/Core#Curve
<https://w3id.org/netbeheer/IECCIM/TC57CIM/IEC61970/Base/Core#Curve> rdf:type owl:Class .


###  https://w3id.org/netbeheer/IECCIM/TC57CIM/IEC61970/Base/Core#Equipment
<https://w3id.org/netbeheer/IECCIM/TC57CIM/IEC61970/Base/Core#Equipment> rdf:type owl:Class .


###  https://w3id.org/netbeheer/IECCIM/TC57CIM/IEC61970/Base/Core#IdentifiedObject
<https://w3id.org/netbeheer/IECCIM/TC57CIM/IEC61970/Base/Core#IdentifiedObject> rdf:type owl:Class .


###  https://w3id.org/netbeheer/IECCIM/TC57CIM/IEC61970/Base/Core#PowerSystemResource
<https://w3id.org/netbeheer/IECCIM/TC57CIM/IEC61970/Base/Core#PowerSystemResource> rdf:type owl:Class .


###  https://w3id.org/netbeheer/IECCIM/TC57CIM/IEC61970/Base/Core#RegularIntervalSchedule
<https://w3id.org/netbeheer/IECCIM/TC57CIM/IEC61970/Base/Core#RegularIntervalSchedule> rdf:type owl:Class .


###  https://w3id.org/netbeheer/IECCIM/TC57CIM/IEC61970/Base/Domain#ActivePower
<https://w3id.org/netbeheer/IECCIM/TC57CIM/IEC61970/Base/Domain#ActivePower> rdf:type owl:Class .


###  https://w3id.org/netbeheer/IECCIM/TC57CIM/IEC61970/Base/Domain#ActivePowerChangeRate
<https://w3id.org/netbeheer/IECCIM/TC57CIM/IEC61970/Base/Domain#ActivePowerChangeRate> rdf:type owl:Class .


###  https://w3id.org/netbeheer/IECCIM/TC57CIM/IEC61970/Base/Domain#CostPerEnergyUnit
<https://w3id.org/netbeheer/IECCIM/TC57CIM/IEC61970/Base/Domain#CostPerEnergyUnit> rdf:type owl:Class .


###  https://w3id.org/netbeheer/IECCIM/TC57CIM/IEC61970/Base/Domain#CostPerVolume
<https://w3id.org/netbeheer/IECCIM/TC57CIM/IEC61970/Base/Domain#CostPerVolume> rdf:type owl:Class .


###  https://w3id.org/netbeheer/IECCIM/TC57CIM/IEC61970/Base/Domain#CostRate
<https://w3id.org/netbeheer/IECCIM/TC57CIM/IEC61970/Base/Domain#CostRate> rdf:type owl:Class .


###  https://w3id.org/netbeheer/IECCIM/TC57CIM/IEC61970/Base/Domain#Hours
<https://w3id.org/netbeheer/IECCIM/TC57CIM/IEC61970/Base/Domain#Hours> rdf:type owl:Class .


###  https://w3id.org/netbeheer/IECCIM/TC57CIM/IEC61970/Base/Domain#Length
<https://w3id.org/netbeheer/IECCIM/TC57CIM/IEC61970/Base/Domain#Length> rdf:type owl:Class .


###  https://w3id.org/netbeheer/IECCIM/TC57CIM/IEC61970/Base/Domain#Money
<https://w3id.org/netbeheer/IECCIM/TC57CIM/IEC61970/Base/Domain#Money> rdf:type owl:Class .


###  https://w3id.org/netbeheer/IECCIM/TC57CIM/IEC61970/Base/Domain#PU
<https://w3id.org/netbeheer/IECCIM/TC57CIM/IEC61970/Base/Domain#PU> rdf:type owl:Class .


###  https://w3id.org/netbeheer/IECCIM/TC57CIM/IEC61970/Base/Domain#PerCent
<https://w3id.org/netbeheer/IECCIM/TC57CIM/IEC61970/Base/Domain#PerCent> rdf:type owl:Class .


###  https://w3id.org/netbeheer/IECCIM/TC57CIM/IEC61970/Base/Domain#RealEnergy
<https://w3id.org/netbeheer/IECCIM/TC57CIM/IEC61970/Base/Domain#RealEnergy> rdf:type owl:Class .


###  https://w3id.org/netbeheer/IECCIM/TC57CIM/IEC61970/Base/Domain#Seconds
<https://w3id.org/netbeheer/IECCIM/TC57CIM/IEC61970/Base/Domain#Seconds> rdf:type owl:Class .


###  https://w3id.org/netbeheer/IECCIM/TC57CIM/IEC61970/Base/Domain#Volume
<https://w3id.org/netbeheer/IECCIM/TC57CIM/IEC61970/Base/Domain#Volume> rdf:type owl:Class .


###  https://w3id.org/netbeheer/IECCIM/TC57CIM/IEC61970/Base/Domain#VolumeFlowRate
<https://w3id.org/netbeheer/IECCIM/TC57CIM/IEC61970/Base/Domain#VolumeFlowRate> rdf:type owl:Class .


###  https://w3id.org/netbeheer/IECCIM/TC57CIM/IEC61970/Base/Domain#WaterLevel
<https://w3id.org/netbeheer/IECCIM/TC57CIM/IEC61970/Base/Domain#WaterLevel> rdf:type owl:Class .


###  https://w3id.org/netbeheer/IECCIM/TC57CIM/IEC61970/Base/Generation/Production#AirCompressor
:AirCompressor rdf:type owl:Class ;
               rdfs:subClassOf <https://w3id.org/netbeheer/IECCIM/TC57CIM/IEC61970/Base/Core#PowerSystemResource> ,
                               [ rdf:type owl:Restriction ;
                                 owl:onProperty :AirCompressor_CAESPlant ;
                                 owl:qualifiedCardinality "1"^^xsd:nonNegativeInteger ;
                                 owl:onClass :AirCompressor
                               ] ,
                               [ rdf:type owl:Restriction ;
                                 owl:onProperty :AirCompressor_airCompressorRating ;
                                 owl:minQualifiedCardinality "0"^^xsd:nonNegativeInteger ;
                                 owl:onDataRange xsd:float
                               ] ,
                               [ rdf:type owl:Restriction ;
                                 owl:onProperty :AirCompressor_airCompressorRating ;
                                 owl:maxQualifiedCardinality "1"^^xsd:nonNegativeInteger ;
                                 owl:onDataRange xsd:float
                               ] ;
               rdfs:comment """Combustion turbine air compressor which is an integral part of a compressed air energy storage (CAES) plant.
""" .


###  https://w3id.org/netbeheer/IECCIM/TC57CIM/IEC61970/Base/Generation/Production#CAESPlant
:CAESPlant rdf:type owl:Class ;
           rdfs:subClassOf <https://w3id.org/netbeheer/IECCIM/TC57CIM/IEC61970/Base/Core#PowerSystemResource> ,
                           [ rdf:type owl:Restriction ;
                             owl:onProperty :CAESPlant_ThermalGeneratingUnit ;
                             owl:minQualifiedCardinality "0"^^xsd:nonNegativeInteger ;
                             owl:onClass :CAESPlant
                           ] ,
                           [ rdf:type owl:Restriction ;
                             owl:onProperty :CAESPlant_energyStorageCapacity ;
                             owl:minQualifiedCardinality "0"^^xsd:nonNegativeInteger ;
                             owl:onClass <https://w3id.org/netbeheer/IECCIM/TC57CIM/IEC61970/Base/Domain#RealEnergy>
                           ] ,
                           [ rdf:type owl:Restriction ;
                             owl:onProperty :CAESPlant_ratedCapacityP ;
                             owl:minQualifiedCardinality "0"^^xsd:nonNegativeInteger ;
                             owl:onClass <https://w3id.org/netbeheer/IECCIM/TC57CIM/IEC61970/Base/Domain#ActivePower>
                           ] ,
                           [ rdf:type owl:Restriction ;
                             owl:onProperty :CAESPlant_AirCompressor ;
                             owl:qualifiedCardinality "1"^^xsd:nonNegativeInteger ;
                             owl:onClass :CAESPlant
                           ] ,
                           [ rdf:type owl:Restriction ;
                             owl:onProperty :CAESPlant_ThermalGeneratingUnit ;
                             owl:maxQualifiedCardinality "1"^^xsd:nonNegativeInteger ;
                             owl:onClass :CAESPlant
                           ] ,
                           [ rdf:type owl:Restriction ;
                             owl:onProperty :CAESPlant_energyStorageCapacity ;
                             owl:maxQualifiedCardinality "1"^^xsd:nonNegativeInteger ;
                             owl:onClass <https://w3id.org/netbeheer/IECCIM/TC57CIM/IEC61970/Base/Domain#RealEnergy>
                           ] ,
                           [ rdf:type owl:Restriction ;
                             owl:onProperty :CAESPlant_ratedCapacityP ;
                             owl:maxQualifiedCardinality "1"^^xsd:nonNegativeInteger ;
                             owl:onClass <https://w3id.org/netbeheer/IECCIM/TC57CIM/IEC61970/Base/Domain#ActivePower>
                           ] ;
           rdfs:comment """Compressed air energy storage plant.
""" .


###  https://w3id.org/netbeheer/IECCIM/TC57CIM/IEC61970/Base/Generation/Production#Classification
:Classification rdf:type owl:Class ;
                rdfs:subClassOf [ rdf:type owl:Restriction ;
                                  owl:onProperty :Classification_multiplier ;
                                  owl:minQualifiedCardinality "0"^^xsd:nonNegativeInteger ;
                                  owl:onDataRange <https://w3id.org/netbeheer/IECCIM/TC57CIM/IEC61970/Base/Domain#UnitMultiplier>
                                ] ,
                                [ rdf:type owl:Restriction ;
                                  owl:onProperty :Classification_unit ;
                                  owl:minQualifiedCardinality "0"^^xsd:nonNegativeInteger ;
                                  owl:onDataRange <https://w3id.org/netbeheer/IECCIM/TC57CIM/IEC61970/Base/Domain#UnitSymbol>
                                ] ,
                                [ rdf:type owl:Restriction ;
                                  owl:onProperty :Classification_value ;
                                  owl:minQualifiedCardinality "0"^^xsd:nonNegativeInteger ;
                                  owl:onDataRange xsd:nonNegativeInteger
                                ] ,
                                [ rdf:type owl:Restriction ;
                                  owl:onProperty :Classification_multiplier ;
                                  owl:maxQualifiedCardinality "1"^^xsd:nonNegativeInteger ;
                                  owl:onDataRange <https://w3id.org/netbeheer/IECCIM/TC57CIM/IEC61970/Base/Domain#UnitMultiplier>
                                ] ,
                                [ rdf:type owl:Restriction ;
                                  owl:onProperty :Classification_unit ;
                                  owl:maxQualifiedCardinality "1"^^xsd:nonNegativeInteger ;
                                  owl:onDataRange <https://w3id.org/netbeheer/IECCIM/TC57CIM/IEC61970/Base/Domain#UnitSymbol>
                                ] ,
                                [ rdf:type owl:Restriction ;
                                  owl:onProperty :Classification_value ;
                                  owl:maxQualifiedCardinality "1"^^xsd:nonNegativeInteger ;
                                  owl:onDataRange xsd:nonNegativeInteger
                                ] ;
                rdfs:comment """Classification of level.  Specify as 1..n, with 1 being the most detailed, highest priority, etc as described on the attribue using this data type.
""" .


###  https://w3id.org/netbeheer/IECCIM/TC57CIM/IEC61970/Base/Generation/Production#CogenerationPlant
:CogenerationPlant rdf:type owl:Class ;
                   rdfs:subClassOf <https://w3id.org/netbeheer/IECCIM/TC57CIM/IEC61970/Base/Core#PowerSystemResource> ,
                                   [ rdf:type owl:Restriction ;
                                     owl:onProperty :CogenerationPlant_ThermalGeneratingUnits ;
                                     owl:minQualifiedCardinality "0"^^xsd:nonNegativeInteger ;
                                     owl:onClass :CogenerationPlant
                                   ] ,
                                   [ rdf:type owl:Restriction ;
                                     owl:onProperty :CogenerationPlant_ratedP ;
                                     owl:minQualifiedCardinality "0"^^xsd:nonNegativeInteger ;
                                     owl:onClass <https://w3id.org/netbeheer/IECCIM/TC57CIM/IEC61970/Base/Domain#ActivePower>
                                   ] ,
                                   [ rdf:type owl:Restriction ;
                                     owl:onProperty :CogenerationPlant_SteamSendoutSchedule ;
                                     owl:qualifiedCardinality "1"^^xsd:nonNegativeInteger ;
                                     owl:onClass :CogenerationPlant
                                   ] ,
                                   [ rdf:type owl:Restriction ;
                                     owl:onProperty :CogenerationPlant_ThermalGeneratingUnits ;
                                     owl:maxQualifiedCardinality "1"^^xsd:nonNegativeInteger ;
                                     owl:onClass :CogenerationPlant
                                   ] ,
                                   [ rdf:type owl:Restriction ;
                                     owl:onProperty :CogenerationPlant_ratedP ;
                                     owl:maxQualifiedCardinality "1"^^xsd:nonNegativeInteger ;
                                     owl:onClass <https://w3id.org/netbeheer/IECCIM/TC57CIM/IEC61970/Base/Domain#ActivePower>
                                   ] ,
                                   [ rdf:type owl:Restriction ;
                                     owl:onProperty :CogenerationPlant_cogenHPSendoutRating ;
                                     owl:minQualifiedCardinality "0"^^xsd:nonNegativeInteger ;
                                     owl:onDataRange xsd:float
                                   ] ,
                                   [ rdf:type owl:Restriction ;
                                     owl:onProperty :CogenerationPlant_cogenHPSteamRating ;
                                     owl:minQualifiedCardinality "0"^^xsd:nonNegativeInteger ;
                                     owl:onDataRange xsd:float
                                   ] ,
                                   [ rdf:type owl:Restriction ;
                                     owl:onProperty :CogenerationPlant_cogenLPSendoutRating ;
                                     owl:minQualifiedCardinality "0"^^xsd:nonNegativeInteger ;
                                     owl:onDataRange xsd:float
                                   ] ,
                                   [ rdf:type owl:Restriction ;
                                     owl:onProperty :CogenerationPlant_cogenLPSteamRating ;
                                     owl:minQualifiedCardinality "0"^^xsd:nonNegativeInteger ;
                                     owl:onDataRange xsd:float
                                   ] ,
                                   [ rdf:type owl:Restriction ;
                                     owl:onProperty :CogenerationPlant_cogenHPSendoutRating ;
                                     owl:maxQualifiedCardinality "1"^^xsd:nonNegativeInteger ;
                                     owl:onDataRange xsd:float
                                   ] ,
                                   [ rdf:type owl:Restriction ;
                                     owl:onProperty :CogenerationPlant_cogenHPSteamRating ;
                                     owl:maxQualifiedCardinality "1"^^xsd:nonNegativeInteger ;
                                     owl:onDataRange xsd:float
                                   ] ,
                                   [ rdf:type owl:Restriction ;
                                     owl:onProperty :CogenerationPlant_cogenLPSendoutRating ;
                                     owl:maxQualifiedCardinality "1"^^xsd:nonNegativeInteger ;
                                     owl:onDataRange xsd:float
                                   ] ,
                                   [ rdf:type owl:Restriction ;
                                     owl:onProperty :CogenerationPlant_cogenLPSteamRating ;
                                     owl:maxQualifiedCardinality "1"^^xsd:nonNegativeInteger ;
                                     owl:onDataRange xsd:float
                                   ] ;
                   rdfs:comment """A set of thermal generating units for the production of electrical energy and process steam (usually from the output of the steam turbines). The steam sendout is typically used for industrial purposes or for municipal heating and cooling.
""" .


###  https://w3id.org/netbeheer/IECCIM/TC57CIM/IEC61970/Base/Generation/Production#CombinedCyclePlant
:CombinedCyclePlant rdf:type owl:Class ;
                    rdfs:subClassOf <https://w3id.org/netbeheer/IECCIM/TC57CIM/IEC61970/Base/Core#PowerSystemResource> ,
                                    [ rdf:type owl:Restriction ;
                                      owl:onProperty :CombinedCyclePlant_ThermalGeneratingUnits ;
                                      owl:minQualifiedCardinality "0"^^xsd:nonNegativeInteger ;
                                      owl:onClass :CombinedCyclePlant
                                    ] ,
                                    [ rdf:type owl:Restriction ;
                                      owl:onProperty :CombinedCyclePlant_combCyclePlantRating ;
                                      owl:minQualifiedCardinality "0"^^xsd:nonNegativeInteger ;
                                      owl:onClass <https://w3id.org/netbeheer/IECCIM/TC57CIM/IEC61970/Base/Domain#ActivePower>
                                    ] ,
                                    [ rdf:type owl:Restriction ;
                                      owl:onProperty :CombinedCyclePlant_ThermalGeneratingUnits ;
                                      owl:maxQualifiedCardinality "1"^^xsd:nonNegativeInteger ;
                                      owl:onClass :CombinedCyclePlant
                                    ] ,
                                    [ rdf:type owl:Restriction ;
                                      owl:onProperty :CombinedCyclePlant_combCyclePlantRating ;
                                      owl:maxQualifiedCardinality "1"^^xsd:nonNegativeInteger ;
                                      owl:onClass <https://w3id.org/netbeheer/IECCIM/TC57CIM/IEC61970/Base/Domain#ActivePower>
                                    ] ;
                    rdfs:comment """A set of combustion turbines and steam turbines where the exhaust heat from the combustion turbines is recovered to make steam for the steam turbines, resulting in greater overall plant efficiency.
""" .


###  https://w3id.org/netbeheer/IECCIM/TC57CIM/IEC61970/Base/Generation/Production#CostPerHeatUnit
:CostPerHeatUnit rdf:type owl:Class ;
                 rdfs:subClassOf [ rdf:type owl:Restriction ;
                                   owl:onProperty :CostPerHeatUnit_denominatorMultiplier ;
                                   owl:minQualifiedCardinality "0"^^xsd:nonNegativeInteger ;
                                   owl:onDataRange <https://w3id.org/netbeheer/IECCIM/TC57CIM/IEC61970/Base/Domain#UnitMultiplier>
                                 ] ,
                                 [ rdf:type owl:Restriction ;
                                   owl:onProperty :CostPerHeatUnit_denominatorUnit ;
                                   owl:minQualifiedCardinality "0"^^xsd:nonNegativeInteger ;
                                   owl:onDataRange <https://w3id.org/netbeheer/IECCIM/TC57CIM/IEC61970/Base/Domain#UnitSymbol>
                                 ] ,
                                 [ rdf:type owl:Restriction ;
                                   owl:onProperty :CostPerHeatUnit_multiplier ;
                                   owl:minQualifiedCardinality "0"^^xsd:nonNegativeInteger ;
                                   owl:onDataRange <https://w3id.org/netbeheer/IECCIM/TC57CIM/IEC61970/Base/Domain#UnitMultiplier>
                                 ] ,
                                 [ rdf:type owl:Restriction ;
                                   owl:onProperty :CostPerHeatUnit_unit ;
                                   owl:minQualifiedCardinality "0"^^xsd:nonNegativeInteger ;
                                   owl:onDataRange <https://w3id.org/netbeheer/IECCIM/TC57CIM/IEC61970/Base/Domain#Currency>
                                 ] ,
                                 [ rdf:type owl:Restriction ;
                                   owl:onProperty :CostPerHeatUnit_value ;
                                   owl:minQualifiedCardinality "0"^^xsd:nonNegativeInteger ;
                                   owl:onDataRange xsd:float
                                 ] ,
                                 [ rdf:type owl:Restriction ;
                                   owl:onProperty :CostPerHeatUnit_denominatorMultiplier ;
                                   owl:maxQualifiedCardinality "1"^^xsd:nonNegativeInteger ;
                                   owl:onDataRange <https://w3id.org/netbeheer/IECCIM/TC57CIM/IEC61970/Base/Domain#UnitMultiplier>
                                 ] ,
                                 [ rdf:type owl:Restriction ;
                                   owl:onProperty :CostPerHeatUnit_denominatorUnit ;
                                   owl:maxQualifiedCardinality "1"^^xsd:nonNegativeInteger ;
                                   owl:onDataRange <https://w3id.org/netbeheer/IECCIM/TC57CIM/IEC61970/Base/Domain#UnitSymbol>
                                 ] ,
                                 [ rdf:type owl:Restriction ;
                                   owl:onProperty :CostPerHeatUnit_multiplier ;
                                   owl:maxQualifiedCardinality "1"^^xsd:nonNegativeInteger ;
                                   owl:onDataRange <https://w3id.org/netbeheer/IECCIM/TC57CIM/IEC61970/Base/Domain#UnitMultiplier>
                                 ] ,
                                 [ rdf:type owl:Restriction ;
                                   owl:onProperty :CostPerHeatUnit_unit ;
                                   owl:maxQualifiedCardinality "1"^^xsd:nonNegativeInteger ;
                                   owl:onDataRange <https://w3id.org/netbeheer/IECCIM/TC57CIM/IEC61970/Base/Domain#Currency>
                                 ] ,
                                 [ rdf:type owl:Restriction ;
                                   owl:onProperty :CostPerHeatUnit_value ;
                                   owl:maxQualifiedCardinality "1"^^xsd:nonNegativeInteger ;
                                   owl:onDataRange xsd:float
                                 ] ;
                 rdfs:comment """Cost, in units of currency, per quantity of heat generated.
""" .


###  https://w3id.org/netbeheer/IECCIM/TC57CIM/IEC61970/Base/Generation/Production#Emission
:Emission rdf:type owl:Class ;
          rdfs:subClassOf [ rdf:type owl:Restriction ;
                            owl:onProperty :Emission_multiplier ;
                            owl:minQualifiedCardinality "0"^^xsd:nonNegativeInteger ;
                            owl:onDataRange <https://w3id.org/netbeheer/IECCIM/TC57CIM/IEC61970/Base/Domain#UnitMultiplier>
                          ] ,
                          [ rdf:type owl:Restriction ;
                            owl:onProperty :Emission_unit ;
                            owl:minQualifiedCardinality "0"^^xsd:nonNegativeInteger ;
                            owl:onDataRange <https://w3id.org/netbeheer/IECCIM/TC57CIM/IEC61970/Base/Domain#UnitSymbol>
                          ] ,
                          [ rdf:type owl:Restriction ;
                            owl:onProperty :Emission_value ;
                            owl:minQualifiedCardinality "0"^^xsd:nonNegativeInteger ;
                            owl:onDataRange xsd:float
                          ] ,
                          [ rdf:type owl:Restriction ;
                            owl:onProperty :Emission_multiplier ;
                            owl:maxQualifiedCardinality "1"^^xsd:nonNegativeInteger ;
                            owl:onDataRange <https://w3id.org/netbeheer/IECCIM/TC57CIM/IEC61970/Base/Domain#UnitMultiplier>
                          ] ,
                          [ rdf:type owl:Restriction ;
                            owl:onProperty :Emission_unit ;
                            owl:maxQualifiedCardinality "1"^^xsd:nonNegativeInteger ;
                            owl:onDataRange <https://w3id.org/netbeheer/IECCIM/TC57CIM/IEC61970/Base/Domain#UnitSymbol>
                          ] ,
                          [ rdf:type owl:Restriction ;
                            owl:onProperty :Emission_value ;
                            owl:maxQualifiedCardinality "1"^^xsd:nonNegativeInteger ;
                            owl:onDataRange xsd:float
                          ] ;
          rdfs:comment """Quantity of emission per fuel heat content.
""" .


###  https://w3id.org/netbeheer/IECCIM/TC57CIM/IEC61970/Base/Generation/Production#EmissionAccount
:EmissionAccount rdf:type owl:Class ;
                 rdfs:subClassOf <https://w3id.org/netbeheer/IECCIM/TC57CIM/IEC61970/Base/Core#Curve> ,
                                 [ rdf:type owl:Restriction ;
                                   owl:onProperty :EmissionAccount_ThermalGeneratingUnit ;
                                   owl:minQualifiedCardinality "0"^^xsd:nonNegativeInteger ;
                                   owl:onClass :EmissionAccount
                                 ] ,
                                 [ rdf:type owl:Restriction ;
                                   owl:onProperty :EmissionAccount_emissionType ;
                                   owl:minQualifiedCardinality "0"^^xsd:nonNegativeInteger ;
                                   owl:onDataRange :EmissionType
                                 ] ,
                                 [ rdf:type owl:Restriction ;
                                   owl:onProperty :EmissionAccount_emissionValueSource ;
                                   owl:minQualifiedCardinality "0"^^xsd:nonNegativeInteger ;
                                   owl:onDataRange :EmissionValueSource
                                 ] ,
                                 [ rdf:type owl:Restriction ;
                                   owl:onProperty :EmissionAccount_emissionType ;
                                   owl:maxQualifiedCardinality "1"^^xsd:nonNegativeInteger ;
                                   owl:onDataRange :EmissionType
                                 ] ,
                                 [ rdf:type owl:Restriction ;
                                   owl:onProperty :EmissionAccount_emissionValueSource ;
                                   owl:maxQualifiedCardinality "1"^^xsd:nonNegativeInteger ;
                                   owl:onDataRange :EmissionValueSource
                                 ] ;
                 rdfs:comment """Accounts for tracking emissions usage and credits for thermal generating units. A unit may have zero or more emission accounts, and will typically have one for tracking usage and one for tracking credits.
""" .


###  https://w3id.org/netbeheer/IECCIM/TC57CIM/IEC61970/Base/Generation/Production#EmissionCurve
:EmissionCurve rdf:type owl:Class ;
               rdfs:subClassOf <https://w3id.org/netbeheer/IECCIM/TC57CIM/IEC61970/Base/Core#Curve> ,
                               [ rdf:type owl:Restriction ;
                                 owl:onProperty :EmissionCurve_ThermalGeneratingUnit ;
                                 owl:minQualifiedCardinality "0"^^xsd:nonNegativeInteger ;
                                 owl:onClass :EmissionCurve
                               ] ,
                               [ rdf:type owl:Restriction ;
                                 owl:onProperty :EmissionCurve_emissionContent ;
                                 owl:minQualifiedCardinality "0"^^xsd:nonNegativeInteger ;
                                 owl:onClass :Emission
                               ] ,
                               [ rdf:type owl:Restriction ;
                                 owl:onProperty :EmissionCurve_emissionContent ;
                                 owl:maxQualifiedCardinality "1"^^xsd:nonNegativeInteger ;
                                 owl:onClass :Emission
                               ] ,
                               [ rdf:type owl:Restriction ;
                                 owl:onProperty :EmissionCurve_emissionType ;
                                 owl:minQualifiedCardinality "0"^^xsd:nonNegativeInteger ;
                                 owl:onDataRange :EmissionType
                               ] ,
                               [ rdf:type owl:Restriction ;
                                 owl:onProperty :EmissionCurve_isNetGrossP ;
                                 owl:minQualifiedCardinality "0"^^xsd:nonNegativeInteger ;
                                 owl:onDataRange xsd:boolean
                               ] ,
                               [ rdf:type owl:Restriction ;
                                 owl:onProperty :EmissionCurve_emissionType ;
                                 owl:maxQualifiedCardinality "1"^^xsd:nonNegativeInteger ;
                                 owl:onDataRange :EmissionType
                               ] ,
                               [ rdf:type owl:Restriction ;
                                 owl:onProperty :EmissionCurve_isNetGrossP ;
                                 owl:maxQualifiedCardinality "1"^^xsd:nonNegativeInteger ;
                                 owl:onDataRange xsd:boolean
                               ] ;
               rdfs:comment """Relationship between the unit's emission rate in units of mass per hour (Y-axis) and output active power (X-axis) for a given type of emission. This curve applies when only one type of fuel is being burned.
""" .


###  https://w3id.org/netbeheer/IECCIM/TC57CIM/IEC61970/Base/Generation/Production#FossilFuel
:FossilFuel rdf:type owl:Class ;
            rdfs:subClassOf <https://w3id.org/netbeheer/IECCIM/TC57CIM/IEC61970/Base/Core#IdentifiedObject> ,
                            [ rdf:type owl:Restriction ;
                              owl:onProperty :FossilFuel_ThermalGeneratingUnit ;
                              owl:minQualifiedCardinality "0"^^xsd:nonNegativeInteger ;
                              owl:onClass :FossilFuel
                            ] ,
                            [ rdf:type owl:Restriction ;
                              owl:onProperty :FossilFuel_fuelCost ;
                              owl:minQualifiedCardinality "0"^^xsd:nonNegativeInteger ;
                              owl:onClass :CostPerHeatUnit
                            ] ,
                            [ rdf:type owl:Restriction ;
                              owl:onProperty :FossilFuel_fuelDispatchCost ;
                              owl:minQualifiedCardinality "0"^^xsd:nonNegativeInteger ;
                              owl:onClass :CostPerHeatUnit
                            ] ,
                            [ rdf:type owl:Restriction ;
                              owl:onProperty :FossilFuel_fuelEffFactor ;
                              owl:minQualifiedCardinality "0"^^xsd:nonNegativeInteger ;
                              owl:onClass <https://w3id.org/netbeheer/IECCIM/TC57CIM/IEC61970/Base/Domain#PU>
                            ] ,
                            [ rdf:type owl:Restriction ;
                              owl:onProperty :FossilFuel_fuelHandlingCost ;
                              owl:minQualifiedCardinality "0"^^xsd:nonNegativeInteger ;
                              owl:onClass :CostPerHeatUnit
                            ] ,
                            [ rdf:type owl:Restriction ;
                              owl:onProperty :FossilFuel_fuelMixture ;
                              owl:minQualifiedCardinality "0"^^xsd:nonNegativeInteger ;
                              owl:onClass <https://w3id.org/netbeheer/IECCIM/TC57CIM/IEC61970/Base/Domain#PerCent>
                            ] ,
                            [ rdf:type owl:Restriction ;
                              owl:onProperty :FossilFuel_fuelSulfur ;
                              owl:minQualifiedCardinality "0"^^xsd:nonNegativeInteger ;
                              owl:onClass <https://w3id.org/netbeheer/IECCIM/TC57CIM/IEC61970/Base/Domain#PU>
                            ] ,
                            [ rdf:type owl:Restriction ;
                              owl:onProperty :FossilFuel_highBreakpointP ;
                              owl:minQualifiedCardinality "0"^^xsd:nonNegativeInteger ;
                              owl:onClass <https://w3id.org/netbeheer/IECCIM/TC57CIM/IEC61970/Base/Domain#ActivePower>
                            ] ,
                            [ rdf:type owl:Restriction ;
                              owl:onProperty :FossilFuel_lowBreakpointP ;
                              owl:minQualifiedCardinality "0"^^xsd:nonNegativeInteger ;
                              owl:onClass <https://w3id.org/netbeheer/IECCIM/TC57CIM/IEC61970/Base/Domain#ActivePower>
                            ] ,
                            [ rdf:type owl:Restriction ;
                              owl:onProperty :FossilFuel_FuelAllocationSchedules ;
                              owl:qualifiedCardinality "1"^^xsd:nonNegativeInteger ;
                              owl:onClass :FossilFuel
                            ] ,
                            [ rdf:type owl:Restriction ;
                              owl:onProperty :FossilFuel_fuelCost ;
                              owl:maxQualifiedCardinality "1"^^xsd:nonNegativeInteger ;
                              owl:onClass :CostPerHeatUnit
                            ] ,
                            [ rdf:type owl:Restriction ;
                              owl:onProperty :FossilFuel_fuelDispatchCost ;
                              owl:maxQualifiedCardinality "1"^^xsd:nonNegativeInteger ;
                              owl:onClass :CostPerHeatUnit
                            ] ,
                            [ rdf:type owl:Restriction ;
                              owl:onProperty :FossilFuel_fuelEffFactor ;
                              owl:maxQualifiedCardinality "1"^^xsd:nonNegativeInteger ;
                              owl:onClass <https://w3id.org/netbeheer/IECCIM/TC57CIM/IEC61970/Base/Domain#PU>
                            ] ,
                            [ rdf:type owl:Restriction ;
                              owl:onProperty :FossilFuel_fuelHandlingCost ;
                              owl:maxQualifiedCardinality "1"^^xsd:nonNegativeInteger ;
                              owl:onClass :CostPerHeatUnit
                            ] ,
                            [ rdf:type owl:Restriction ;
                              owl:onProperty :FossilFuel_fuelMixture ;
                              owl:maxQualifiedCardinality "1"^^xsd:nonNegativeInteger ;
                              owl:onClass <https://w3id.org/netbeheer/IECCIM/TC57CIM/IEC61970/Base/Domain#PerCent>
                            ] ,
                            [ rdf:type owl:Restriction ;
                              owl:onProperty :FossilFuel_fuelSulfur ;
                              owl:maxQualifiedCardinality "1"^^xsd:nonNegativeInteger ;
                              owl:onClass <https://w3id.org/netbeheer/IECCIM/TC57CIM/IEC61970/Base/Domain#PU>
                            ] ,
                            [ rdf:type owl:Restriction ;
                              owl:onProperty :FossilFuel_highBreakpointP ;
                              owl:maxQualifiedCardinality "1"^^xsd:nonNegativeInteger ;
                              owl:onClass <https://w3id.org/netbeheer/IECCIM/TC57CIM/IEC61970/Base/Domain#ActivePower>
                            ] ,
                            [ rdf:type owl:Restriction ;
                              owl:onProperty :FossilFuel_lowBreakpointP ;
                              owl:maxQualifiedCardinality "1"^^xsd:nonNegativeInteger ;
                              owl:onClass <https://w3id.org/netbeheer/IECCIM/TC57CIM/IEC61970/Base/Domain#ActivePower>
                            ] ,
                            [ rdf:type owl:Restriction ;
                              owl:onProperty :FossilFuel_fossilFuelType ;
                              owl:minQualifiedCardinality "0"^^xsd:nonNegativeInteger ;
                              owl:onDataRange :FuelType
                            ] ,
                            [ rdf:type owl:Restriction ;
                              owl:onProperty :FossilFuel_fuelHeatContent ;
                              owl:minQualifiedCardinality "0"^^xsd:nonNegativeInteger ;
                              owl:onDataRange xsd:float
                            ] ,
                            [ rdf:type owl:Restriction ;
                              owl:onProperty :FossilFuel_fossilFuelType ;
                              owl:maxQualifiedCardinality "1"^^xsd:nonNegativeInteger ;
                              owl:onDataRange :FuelType
                            ] ,
                            [ rdf:type owl:Restriction ;
                              owl:onProperty :FossilFuel_fuelHeatContent ;
                              owl:maxQualifiedCardinality "1"^^xsd:nonNegativeInteger ;
                              owl:onDataRange xsd:float
                            ] ;
            rdfs:comment "The fossil fuel consumed by the non-nuclear thermal generating unit.   For example, coal, oil, gas, etc.   This a the specific fuels that the generating unit can consume." .


###  https://w3id.org/netbeheer/IECCIM/TC57CIM/IEC61970/Base/Generation/Production#FuelAllocationSchedule
:FuelAllocationSchedule rdf:type owl:Class ;
                        rdfs:subClassOf <https://w3id.org/netbeheer/IECCIM/TC57CIM/IEC61970/Base/Core#Curve> ,
                                        [ rdf:type owl:Restriction ;
                                          owl:onProperty :FuelAllocationSchedule_FossilFuel ;
                                          owl:minQualifiedCardinality "0"^^xsd:nonNegativeInteger ;
                                          owl:onClass :FuelAllocationSchedule
                                        ] ,
                                        [ rdf:type owl:Restriction ;
                                          owl:onProperty :FuelAllocationSchedule_ThermalGeneratingUnit ;
                                          owl:minQualifiedCardinality "0"^^xsd:nonNegativeInteger ;
                                          owl:onClass :FuelAllocationSchedule
                                        ] ,
                                        [ rdf:type owl:Restriction ;
                                          owl:onProperty :FuelAllocationSchedule_fuelAllocationEndDate ;
                                          owl:minQualifiedCardinality "0"^^xsd:nonNegativeInteger ;
                                          owl:onDataRange xsd:dateTime
                                        ] ,
                                        [ rdf:type owl:Restriction ;
                                          owl:onProperty :FuelAllocationSchedule_fuelAllocationStartDate ;
                                          owl:minQualifiedCardinality "0"^^xsd:nonNegativeInteger ;
                                          owl:onDataRange xsd:dateTime
                                        ] ,
                                        [ rdf:type owl:Restriction ;
                                          owl:onProperty :FuelAllocationSchedule_fuelType ;
                                          owl:minQualifiedCardinality "0"^^xsd:nonNegativeInteger ;
                                          owl:onDataRange :FuelType
                                        ] ,
                                        [ rdf:type owl:Restriction ;
                                          owl:onProperty :FuelAllocationSchedule_maxFuelAllocation ;
                                          owl:minQualifiedCardinality "0"^^xsd:nonNegativeInteger ;
                                          owl:onDataRange xsd:float
                                        ] ,
                                        [ rdf:type owl:Restriction ;
                                          owl:onProperty :FuelAllocationSchedule_minFuelAllocation ;
                                          owl:minQualifiedCardinality "0"^^xsd:nonNegativeInteger ;
                                          owl:onDataRange xsd:float
                                        ] ,
                                        [ rdf:type owl:Restriction ;
                                          owl:onProperty :FuelAllocationSchedule_fuelAllocationEndDate ;
                                          owl:maxQualifiedCardinality "1"^^xsd:nonNegativeInteger ;
                                          owl:onDataRange xsd:dateTime
                                        ] ,
                                        [ rdf:type owl:Restriction ;
                                          owl:onProperty :FuelAllocationSchedule_fuelAllocationStartDate ;
                                          owl:maxQualifiedCardinality "1"^^xsd:nonNegativeInteger ;
                                          owl:onDataRange xsd:dateTime
                                        ] ,
                                        [ rdf:type owl:Restriction ;
                                          owl:onProperty :FuelAllocationSchedule_fuelType ;
                                          owl:maxQualifiedCardinality "1"^^xsd:nonNegativeInteger ;
                                          owl:onDataRange :FuelType
                                        ] ,
                                        [ rdf:type owl:Restriction ;
                                          owl:onProperty :FuelAllocationSchedule_maxFuelAllocation ;
                                          owl:maxQualifiedCardinality "1"^^xsd:nonNegativeInteger ;
                                          owl:onDataRange xsd:float
                                        ] ,
                                        [ rdf:type owl:Restriction ;
                                          owl:onProperty :FuelAllocationSchedule_minFuelAllocation ;
                                          owl:maxQualifiedCardinality "1"^^xsd:nonNegativeInteger ;
                                          owl:onDataRange xsd:float
                                        ] ;
                        rdfs:comment """The amount of fuel of a given type which is allocated for consumption over a specified period of time.
""" .


###  https://w3id.org/netbeheer/IECCIM/TC57CIM/IEC61970/Base/Generation/Production#GenUnitOpCostCurve
:GenUnitOpCostCurve rdf:type owl:Class ;
                    rdfs:subClassOf <https://w3id.org/netbeheer/IECCIM/TC57CIM/IEC61970/Base/Core#Curve> ,
                                    [ rdf:type owl:Restriction ;
                                      owl:onProperty :GenUnitOpCostCurve_GeneratingUnit ;
                                      owl:minQualifiedCardinality "0"^^xsd:nonNegativeInteger ;
                                      owl:onClass :GenUnitOpCostCurve
                                    ] ,
                                    [ rdf:type owl:Restriction ;
                                      owl:onProperty :GenUnitOpCostCurve_isNetGrossP ;
                                      owl:minQualifiedCardinality "0"^^xsd:nonNegativeInteger ;
                                      owl:onDataRange xsd:boolean
                                    ] ,
                                    [ rdf:type owl:Restriction ;
                                      owl:onProperty :GenUnitOpCostCurve_isNetGrossP ;
                                      owl:maxQualifiedCardinality "1"^^xsd:nonNegativeInteger ;
                                      owl:onDataRange xsd:boolean
                                    ] ;
                    rdfs:comment "Relationship between unit operating cost (Y-axis) and unit output active power (X-axis). The operating cost curve for thermal units is derived from heat input and fuel costs. The operating cost curve for hydro units is derived from water flow rates and equivalent water costs." .


###  https://w3id.org/netbeheer/IECCIM/TC57CIM/IEC61970/Base/Generation/Production#GenUnitOpSchedule
:GenUnitOpSchedule rdf:type owl:Class ;
                   rdfs:subClassOf <https://w3id.org/netbeheer/IECCIM/TC57CIM/IEC61970/Base/Core#RegularIntervalSchedule> ,
                                   [ rdf:type owl:Restriction ;
                                     owl:onProperty :GenUnitOpSchedule_GeneratingUnit ;
                                     owl:minQualifiedCardinality "0"^^xsd:nonNegativeInteger ;
                                     owl:onClass :GenUnitOpSchedule
                                   ] ,
                                   [ rdf:type owl:Restriction ;
                                     owl:onProperty :GenUnitOpSchedule_GeneratingUnit ;
                                     owl:maxQualifiedCardinality "1"^^xsd:nonNegativeInteger ;
                                     owl:onClass :GenUnitOpSchedule
                                   ] ;
                   rdfs:comment """The generating unit's Operator-approved current operating schedule (or plan), typically produced with the aid of unit commitment type analyses. The X-axis represents absolute time. The Y1-axis represents the status (0=off-line and unavailable: 1=available: 2=must run: 3=must run at fixed power value: etc.). The Y2-axis represents the must run fixed power value where required.
""" .


###  https://w3id.org/netbeheer/IECCIM/TC57CIM/IEC61970/Base/Generation/Production#GeneratingUnit
:GeneratingUnit rdf:type owl:Class ;
                rdfs:subClassOf <https://w3id.org/netbeheer/IECCIM/TC57CIM/IEC61970/Base/Core#Equipment> ,
                                [ rdf:type owl:Restriction ;
                                  owl:onProperty :GeneratingUnit_allocSpinResP ;
                                  owl:minQualifiedCardinality "0"^^xsd:nonNegativeInteger ;
                                  owl:onClass <https://w3id.org/netbeheer/IECCIM/TC57CIM/IEC61970/Base/Domain#ActivePower>
                                ] ,
                                [ rdf:type owl:Restriction ;
                                  owl:onProperty :GeneratingUnit_autoCntrlMarginP ;
                                  owl:minQualifiedCardinality "0"^^xsd:nonNegativeInteger ;
                                  owl:onClass <https://w3id.org/netbeheer/IECCIM/TC57CIM/IEC61970/Base/Domain#ActivePower>
                                ] ,
                                [ rdf:type owl:Restriction ;
                                  owl:onProperty :GeneratingUnit_baseP ;
                                  owl:minQualifiedCardinality "0"^^xsd:nonNegativeInteger ;
                                  owl:onClass <https://w3id.org/netbeheer/IECCIM/TC57CIM/IEC61970/Base/Domain#ActivePower>
                                ] ,
                                [ rdf:type owl:Restriction ;
                                  owl:onProperty :GeneratingUnit_controlDeadband ;
                                  owl:minQualifiedCardinality "0"^^xsd:nonNegativeInteger ;
                                  owl:onClass <https://w3id.org/netbeheer/IECCIM/TC57CIM/IEC61970/Base/Domain#ActivePower>
                                ] ,
                                [ rdf:type owl:Restriction ;
                                  owl:onProperty :GeneratingUnit_controlPulseHigh ;
                                  owl:minQualifiedCardinality "0"^^xsd:nonNegativeInteger ;
                                  owl:onClass <https://w3id.org/netbeheer/IECCIM/TC57CIM/IEC61970/Base/Domain#Seconds>
                                ] ,
                                [ rdf:type owl:Restriction ;
                                  owl:onProperty :GeneratingUnit_controlPulseLow ;
                                  owl:minQualifiedCardinality "0"^^xsd:nonNegativeInteger ;
                                  owl:onClass <https://w3id.org/netbeheer/IECCIM/TC57CIM/IEC61970/Base/Domain#Seconds>
                                ] ,
                                [ rdf:type owl:Restriction ;
                                  owl:onProperty :GeneratingUnit_controlResponseRate ;
                                  owl:minQualifiedCardinality "0"^^xsd:nonNegativeInteger ;
                                  owl:onClass <https://w3id.org/netbeheer/IECCIM/TC57CIM/IEC61970/Base/Domain#ActivePowerChangeRate>
                                ] ,
                                [ rdf:type owl:Restriction ;
                                  owl:onProperty :GeneratingUnit_efficiency ;
                                  owl:minQualifiedCardinality "0"^^xsd:nonNegativeInteger ;
                                  owl:onClass <https://w3id.org/netbeheer/IECCIM/TC57CIM/IEC61970/Base/Domain#PerCent>
                                ] ,
                                [ rdf:type owl:Restriction ;
                                  owl:onProperty :GeneratingUnit_governorMPL ;
                                  owl:minQualifiedCardinality "0"^^xsd:nonNegativeInteger ;
                                  owl:onClass <https://w3id.org/netbeheer/IECCIM/TC57CIM/IEC61970/Base/Domain#PU>
                                ] ,
                                [ rdf:type owl:Restriction ;
                                  owl:onProperty :GeneratingUnit_governorSCD ;
                                  owl:minQualifiedCardinality "0"^^xsd:nonNegativeInteger ;
                                  owl:onClass <https://w3id.org/netbeheer/IECCIM/TC57CIM/IEC61970/Base/Domain#PerCent>
                                ] ,
                                [ rdf:type owl:Restriction ;
                                  owl:onProperty :GeneratingUnit_highControlLimit ;
                                  owl:minQualifiedCardinality "0"^^xsd:nonNegativeInteger ;
                                  owl:onClass <https://w3id.org/netbeheer/IECCIM/TC57CIM/IEC61970/Base/Domain#ActivePower>
                                ] ,
                                [ rdf:type owl:Restriction ;
                                  owl:onProperty :GeneratingUnit_initialP ;
                                  owl:minQualifiedCardinality "0"^^xsd:nonNegativeInteger ;
                                  owl:onClass <https://w3id.org/netbeheer/IECCIM/TC57CIM/IEC61970/Base/Domain#ActivePower>
                                ] ,
                                [ rdf:type owl:Restriction ;
                                  owl:onProperty :GeneratingUnit_lowControlLimit ;
                                  owl:minQualifiedCardinality "0"^^xsd:nonNegativeInteger ;
                                  owl:onClass <https://w3id.org/netbeheer/IECCIM/TC57CIM/IEC61970/Base/Domain#ActivePower>
                                ] ,
                                [ rdf:type owl:Restriction ;
                                  owl:onProperty :GeneratingUnit_lowerRampRate ;
                                  owl:minQualifiedCardinality "0"^^xsd:nonNegativeInteger ;
                                  owl:onClass <https://w3id.org/netbeheer/IECCIM/TC57CIM/IEC61970/Base/Domain#ActivePowerChangeRate>
                                ] ,
                                [ rdf:type owl:Restriction ;
                                  owl:onProperty :GeneratingUnit_maxEconomicP ;
                                  owl:minQualifiedCardinality "0"^^xsd:nonNegativeInteger ;
                                  owl:onClass <https://w3id.org/netbeheer/IECCIM/TC57CIM/IEC61970/Base/Domain#ActivePower>
                                ] ,
                                [ rdf:type owl:Restriction ;
                                  owl:onProperty :GeneratingUnit_maxOperatingP ;
                                  owl:minQualifiedCardinality "0"^^xsd:nonNegativeInteger ;
                                  owl:onClass <https://w3id.org/netbeheer/IECCIM/TC57CIM/IEC61970/Base/Domain#ActivePower>
                                ] ,
                                [ rdf:type owl:Restriction ;
                                  owl:onProperty :GeneratingUnit_maximumAllowableSpinningReserve ;
                                  owl:minQualifiedCardinality "0"^^xsd:nonNegativeInteger ;
                                  owl:onClass <https://w3id.org/netbeheer/IECCIM/TC57CIM/IEC61970/Base/Domain#ActivePower>
                                ] ,
                                [ rdf:type owl:Restriction ;
                                  owl:onProperty :GeneratingUnit_minEconomicP ;
                                  owl:minQualifiedCardinality "0"^^xsd:nonNegativeInteger ;
                                  owl:onClass <https://w3id.org/netbeheer/IECCIM/TC57CIM/IEC61970/Base/Domain#ActivePower>
                                ] ,
                                [ rdf:type owl:Restriction ;
                                  owl:onProperty :GeneratingUnit_minOperatingP ;
                                  owl:minQualifiedCardinality "0"^^xsd:nonNegativeInteger ;
                                  owl:onClass <https://w3id.org/netbeheer/IECCIM/TC57CIM/IEC61970/Base/Domain#ActivePower>
                                ] ,
                                [ rdf:type owl:Restriction ;
                                  owl:onProperty :GeneratingUnit_minimumOffTime ;
                                  owl:minQualifiedCardinality "0"^^xsd:nonNegativeInteger ;
                                  owl:onClass <https://w3id.org/netbeheer/IECCIM/TC57CIM/IEC61970/Base/Domain#Seconds>
                                ] ,
                                [ rdf:type owl:Restriction ;
                                  owl:onProperty :GeneratingUnit_modelDetail ;
                                  owl:minQualifiedCardinality "0"^^xsd:nonNegativeInteger ;
                                  owl:onClass :Classification
                                ] ,
                                [ rdf:type owl:Restriction ;
                                  owl:onProperty :GeneratingUnit_nominalP ;
                                  owl:minQualifiedCardinality "0"^^xsd:nonNegativeInteger ;
                                  owl:onClass <https://w3id.org/netbeheer/IECCIM/TC57CIM/IEC61970/Base/Domain#ActivePower>
                                ] ,
                                [ rdf:type owl:Restriction ;
                                  owl:onProperty :GeneratingUnit_raiseRampRate ;
                                  owl:minQualifiedCardinality "0"^^xsd:nonNegativeInteger ;
                                  owl:onClass <https://w3id.org/netbeheer/IECCIM/TC57CIM/IEC61970/Base/Domain#ActivePowerChangeRate>
                                ] ,
                                [ rdf:type owl:Restriction ;
                                  owl:onProperty :GeneratingUnit_ratedGrossMaxP ;
                                  owl:minQualifiedCardinality "0"^^xsd:nonNegativeInteger ;
                                  owl:onClass <https://w3id.org/netbeheer/IECCIM/TC57CIM/IEC61970/Base/Domain#ActivePower>
                                ] ,
                                [ rdf:type owl:Restriction ;
                                  owl:onProperty :GeneratingUnit_ratedGrossMinP ;
                                  owl:minQualifiedCardinality "0"^^xsd:nonNegativeInteger ;
                                  owl:onClass <https://w3id.org/netbeheer/IECCIM/TC57CIM/IEC61970/Base/Domain#ActivePower>
                                ] ,
                                [ rdf:type owl:Restriction ;
                                  owl:onProperty :GeneratingUnit_ratedNetMaxP ;
                                  owl:minQualifiedCardinality "0"^^xsd:nonNegativeInteger ;
                                  owl:onClass <https://w3id.org/netbeheer/IECCIM/TC57CIM/IEC61970/Base/Domain#ActivePower>
                                ] ,
                                [ rdf:type owl:Restriction ;
                                  owl:onProperty :GeneratingUnit_startupCost ;
                                  owl:minQualifiedCardinality "0"^^xsd:nonNegativeInteger ;
                                  owl:onClass <https://w3id.org/netbeheer/IECCIM/TC57CIM/IEC61970/Base/Domain#Money>
                                ] ,
                                [ rdf:type owl:Restriction ;
                                  owl:onProperty :GeneratingUnit_startupTime ;
                                  owl:minQualifiedCardinality "0"^^xsd:nonNegativeInteger ;
                                  owl:onClass <https://w3id.org/netbeheer/IECCIM/TC57CIM/IEC61970/Base/Domain#Seconds>
                                ] ,
                                [ rdf:type owl:Restriction ;
                                  owl:onProperty :GeneratingUnit_totalEfficiency ;
                                  owl:minQualifiedCardinality "0"^^xsd:nonNegativeInteger ;
                                  owl:onClass <https://w3id.org/netbeheer/IECCIM/TC57CIM/IEC61970/Base/Domain#PerCent>
                                ] ,
                                [ rdf:type owl:Restriction ;
                                  owl:onProperty :GeneratingUnit_variableCost ;
                                  owl:minQualifiedCardinality "0"^^xsd:nonNegativeInteger ;
                                  owl:onClass <https://w3id.org/netbeheer/IECCIM/TC57CIM/IEC61970/Base/Domain#Money>
                                ] ,
                                [ rdf:type owl:Restriction ;
                                  owl:onProperty :GeneratingUnit_ControlAreaGeneratingUnit ;
                                  owl:qualifiedCardinality "1"^^xsd:nonNegativeInteger ;
                                  owl:onClass :GeneratingUnit
                                ] ,
                                [ rdf:type owl:Restriction ;
                                  owl:onProperty :GeneratingUnit_GenUnitOpCostCurves ;
                                  owl:qualifiedCardinality "1"^^xsd:nonNegativeInteger ;
                                  owl:onClass :GeneratingUnit
                                ] ,
                                [ rdf:type owl:Restriction ;
                                  owl:onProperty :GeneratingUnit_GenUnitOpSchedule ;
                                  owl:qualifiedCardinality "1"^^xsd:nonNegativeInteger ;
                                  owl:onClass :GeneratingUnit
                                ] ,
                                [ rdf:type owl:Restriction ;
                                  owl:onProperty :GeneratingUnit_GrossToNetActivePowerCurves ;
                                  owl:qualifiedCardinality "1"^^xsd:nonNegativeInteger ;
                                  owl:onClass :GeneratingUnit
                                ] ,
                                [ rdf:type owl:Restriction ;
                                  owl:onProperty :GeneratingUnit_allocSpinResP ;
                                  owl:maxQualifiedCardinality "1"^^xsd:nonNegativeInteger ;
                                  owl:onClass <https://w3id.org/netbeheer/IECCIM/TC57CIM/IEC61970/Base/Domain#ActivePower>
                                ] ,
                                [ rdf:type owl:Restriction ;
                                  owl:onProperty :GeneratingUnit_autoCntrlMarginP ;
                                  owl:maxQualifiedCardinality "1"^^xsd:nonNegativeInteger ;
                                  owl:onClass <https://w3id.org/netbeheer/IECCIM/TC57CIM/IEC61970/Base/Domain#ActivePower>
                                ] ,
                                [ rdf:type owl:Restriction ;
                                  owl:onProperty :GeneratingUnit_baseP ;
                                  owl:maxQualifiedCardinality "1"^^xsd:nonNegativeInteger ;
                                  owl:onClass <https://w3id.org/netbeheer/IECCIM/TC57CIM/IEC61970/Base/Domain#ActivePower>
                                ] ,
                                [ rdf:type owl:Restriction ;
                                  owl:onProperty :GeneratingUnit_controlDeadband ;
                                  owl:maxQualifiedCardinality "1"^^xsd:nonNegativeInteger ;
                                  owl:onClass <https://w3id.org/netbeheer/IECCIM/TC57CIM/IEC61970/Base/Domain#ActivePower>
                                ] ,
                                [ rdf:type owl:Restriction ;
                                  owl:onProperty :GeneratingUnit_controlPulseHigh ;
                                  owl:maxQualifiedCardinality "1"^^xsd:nonNegativeInteger ;
                                  owl:onClass <https://w3id.org/netbeheer/IECCIM/TC57CIM/IEC61970/Base/Domain#Seconds>
                                ] ,
                                [ rdf:type owl:Restriction ;
                                  owl:onProperty :GeneratingUnit_controlPulseLow ;
                                  owl:maxQualifiedCardinality "1"^^xsd:nonNegativeInteger ;
                                  owl:onClass <https://w3id.org/netbeheer/IECCIM/TC57CIM/IEC61970/Base/Domain#Seconds>
                                ] ,
                                [ rdf:type owl:Restriction ;
                                  owl:onProperty :GeneratingUnit_controlResponseRate ;
                                  owl:maxQualifiedCardinality "1"^^xsd:nonNegativeInteger ;
                                  owl:onClass <https://w3id.org/netbeheer/IECCIM/TC57CIM/IEC61970/Base/Domain#ActivePowerChangeRate>
                                ] ,
                                [ rdf:type owl:Restriction ;
                                  owl:onProperty :GeneratingUnit_efficiency ;
                                  owl:maxQualifiedCardinality "1"^^xsd:nonNegativeInteger ;
                                  owl:onClass <https://w3id.org/netbeheer/IECCIM/TC57CIM/IEC61970/Base/Domain#PerCent>
                                ] ,
                                [ rdf:type owl:Restriction ;
                                  owl:onProperty :GeneratingUnit_governorMPL ;
                                  owl:maxQualifiedCardinality "1"^^xsd:nonNegativeInteger ;
                                  owl:onClass <https://w3id.org/netbeheer/IECCIM/TC57CIM/IEC61970/Base/Domain#PU>
                                ] ,
                                [ rdf:type owl:Restriction ;
                                  owl:onProperty :GeneratingUnit_governorSCD ;
                                  owl:maxQualifiedCardinality "1"^^xsd:nonNegativeInteger ;
                                  owl:onClass <https://w3id.org/netbeheer/IECCIM/TC57CIM/IEC61970/Base/Domain#PerCent>
                                ] ,
                                [ rdf:type owl:Restriction ;
                                  owl:onProperty :GeneratingUnit_highControlLimit ;
                                  owl:maxQualifiedCardinality "1"^^xsd:nonNegativeInteger ;
                                  owl:onClass <https://w3id.org/netbeheer/IECCIM/TC57CIM/IEC61970/Base/Domain#ActivePower>
                                ] ,
                                [ rdf:type owl:Restriction ;
                                  owl:onProperty :GeneratingUnit_initialP ;
                                  owl:maxQualifiedCardinality "1"^^xsd:nonNegativeInteger ;
                                  owl:onClass <https://w3id.org/netbeheer/IECCIM/TC57CIM/IEC61970/Base/Domain#ActivePower>
                                ] ,
                                [ rdf:type owl:Restriction ;
                                  owl:onProperty :GeneratingUnit_lowControlLimit ;
                                  owl:maxQualifiedCardinality "1"^^xsd:nonNegativeInteger ;
                                  owl:onClass <https://w3id.org/netbeheer/IECCIM/TC57CIM/IEC61970/Base/Domain#ActivePower>
                                ] ,
                                [ rdf:type owl:Restriction ;
                                  owl:onProperty :GeneratingUnit_lowerRampRate ;
                                  owl:maxQualifiedCardinality "1"^^xsd:nonNegativeInteger ;
                                  owl:onClass <https://w3id.org/netbeheer/IECCIM/TC57CIM/IEC61970/Base/Domain#ActivePowerChangeRate>
                                ] ,
                                [ rdf:type owl:Restriction ;
                                  owl:onProperty :GeneratingUnit_maxEconomicP ;
                                  owl:maxQualifiedCardinality "1"^^xsd:nonNegativeInteger ;
                                  owl:onClass <https://w3id.org/netbeheer/IECCIM/TC57CIM/IEC61970/Base/Domain#ActivePower>
                                ] ,
                                [ rdf:type owl:Restriction ;
                                  owl:onProperty :GeneratingUnit_maxOperatingP ;
                                  owl:maxQualifiedCardinality "1"^^xsd:nonNegativeInteger ;
                                  owl:onClass <https://w3id.org/netbeheer/IECCIM/TC57CIM/IEC61970/Base/Domain#ActivePower>
                                ] ,
                                [ rdf:type owl:Restriction ;
                                  owl:onProperty :GeneratingUnit_maximumAllowableSpinningReserve ;
                                  owl:maxQualifiedCardinality "1"^^xsd:nonNegativeInteger ;
                                  owl:onClass <https://w3id.org/netbeheer/IECCIM/TC57CIM/IEC61970/Base/Domain#ActivePower>
                                ] ,
                                [ rdf:type owl:Restriction ;
                                  owl:onProperty :GeneratingUnit_minEconomicP ;
                                  owl:maxQualifiedCardinality "1"^^xsd:nonNegativeInteger ;
                                  owl:onClass <https://w3id.org/netbeheer/IECCIM/TC57CIM/IEC61970/Base/Domain#ActivePower>
                                ] ,
                                [ rdf:type owl:Restriction ;
                                  owl:onProperty :GeneratingUnit_minOperatingP ;
                                  owl:maxQualifiedCardinality "1"^^xsd:nonNegativeInteger ;
                                  owl:onClass <https://w3id.org/netbeheer/IECCIM/TC57CIM/IEC61970/Base/Domain#ActivePower>
                                ] ,
                                [ rdf:type owl:Restriction ;
                                  owl:onProperty :GeneratingUnit_minimumOffTime ;
                                  owl:maxQualifiedCardinality "1"^^xsd:nonNegativeInteger ;
                                  owl:onClass <https://w3id.org/netbeheer/IECCIM/TC57CIM/IEC61970/Base/Domain#Seconds>
                                ] ,
                                [ rdf:type owl:Restriction ;
                                  owl:onProperty :GeneratingUnit_modelDetail ;
                                  owl:maxQualifiedCardinality "1"^^xsd:nonNegativeInteger ;
                                  owl:onClass :Classification
                                ] ,
                                [ rdf:type owl:Restriction ;
                                  owl:onProperty :GeneratingUnit_nominalP ;
                                  owl:maxQualifiedCardinality "1"^^xsd:nonNegativeInteger ;
                                  owl:onClass <https://w3id.org/netbeheer/IECCIM/TC57CIM/IEC61970/Base/Domain#ActivePower>
                                ] ,
                                [ rdf:type owl:Restriction ;
                                  owl:onProperty :GeneratingUnit_raiseRampRate ;
                                  owl:maxQualifiedCardinality "1"^^xsd:nonNegativeInteger ;
                                  owl:onClass <https://w3id.org/netbeheer/IECCIM/TC57CIM/IEC61970/Base/Domain#ActivePowerChangeRate>
                                ] ,
                                [ rdf:type owl:Restriction ;
                                  owl:onProperty :GeneratingUnit_ratedGrossMaxP ;
                                  owl:maxQualifiedCardinality "1"^^xsd:nonNegativeInteger ;
                                  owl:onClass <https://w3id.org/netbeheer/IECCIM/TC57CIM/IEC61970/Base/Domain#ActivePower>
                                ] ,
                                [ rdf:type owl:Restriction ;
                                  owl:onProperty :GeneratingUnit_ratedGrossMinP ;
                                  owl:maxQualifiedCardinality "1"^^xsd:nonNegativeInteger ;
                                  owl:onClass <https://w3id.org/netbeheer/IECCIM/TC57CIM/IEC61970/Base/Domain#ActivePower>
                                ] ,
                                [ rdf:type owl:Restriction ;
                                  owl:onProperty :GeneratingUnit_ratedNetMaxP ;
                                  owl:maxQualifiedCardinality "1"^^xsd:nonNegativeInteger ;
                                  owl:onClass <https://w3id.org/netbeheer/IECCIM/TC57CIM/IEC61970/Base/Domain#ActivePower>
                                ] ,
                                [ rdf:type owl:Restriction ;
                                  owl:onProperty :GeneratingUnit_startupCost ;
                                  owl:maxQualifiedCardinality "1"^^xsd:nonNegativeInteger ;
                                  owl:onClass <https://w3id.org/netbeheer/IECCIM/TC57CIM/IEC61970/Base/Domain#Money>
                                ] ,
                                [ rdf:type owl:Restriction ;
                                  owl:onProperty :GeneratingUnit_startupTime ;
                                  owl:maxQualifiedCardinality "1"^^xsd:nonNegativeInteger ;
                                  owl:onClass <https://w3id.org/netbeheer/IECCIM/TC57CIM/IEC61970/Base/Domain#Seconds>
                                ] ,
                                [ rdf:type owl:Restriction ;
                                  owl:onProperty :GeneratingUnit_totalEfficiency ;
                                  owl:maxQualifiedCardinality "1"^^xsd:nonNegativeInteger ;
                                  owl:onClass <https://w3id.org/netbeheer/IECCIM/TC57CIM/IEC61970/Base/Domain#PerCent>
                                ] ,
                                [ rdf:type owl:Restriction ;
                                  owl:onProperty :GeneratingUnit_variableCost ;
                                  owl:maxQualifiedCardinality "1"^^xsd:nonNegativeInteger ;
                                  owl:onClass <https://w3id.org/netbeheer/IECCIM/TC57CIM/IEC61970/Base/Domain#Money>
                                ] ,
                                [ rdf:type owl:Restriction ;
                                  owl:onProperty :GeneratingUnit_genControlMode ;
                                  owl:minQualifiedCardinality "0"^^xsd:nonNegativeInteger ;
                                  owl:onDataRange :GeneratorControlMode
                                ] ,
                                [ rdf:type owl:Restriction ;
                                  owl:onProperty :GeneratingUnit_genControlSource ;
                                  owl:minQualifiedCardinality "0"^^xsd:nonNegativeInteger ;
                                  owl:onDataRange :GeneratorControlSource
                                ] ,
                                [ rdf:type owl:Restriction ;
                                  owl:onProperty :GeneratingUnit_longPF ;
                                  owl:minQualifiedCardinality "0"^^xsd:nonNegativeInteger ;
                                  owl:onDataRange xsd:float
                                ] ,
                                [ rdf:type owl:Restriction ;
                                  owl:onProperty :GeneratingUnit_normalPF ;
                                  owl:minQualifiedCardinality "0"^^xsd:nonNegativeInteger ;
                                  owl:onDataRange xsd:float
                                ] ,
                                [ rdf:type owl:Restriction ;
                                  owl:onProperty :GeneratingUnit_penaltyFactor ;
                                  owl:minQualifiedCardinality "0"^^xsd:nonNegativeInteger ;
                                  owl:onDataRange xsd:float
                                ] ,
                                [ rdf:type owl:Restriction ;
                                  owl:onProperty :GeneratingUnit_shortPF ;
                                  owl:minQualifiedCardinality "0"^^xsd:nonNegativeInteger ;
                                  owl:onDataRange xsd:float
                                ] ,
                                [ rdf:type owl:Restriction ;
                                  owl:onProperty :GeneratingUnit_tieLinePF ;
                                  owl:minQualifiedCardinality "0"^^xsd:nonNegativeInteger ;
                                  owl:onDataRange xsd:float
                                ] ,
                                [ rdf:type owl:Restriction ;
                                  owl:onProperty :GeneratingUnit_genControlMode ;
                                  owl:maxQualifiedCardinality "1"^^xsd:nonNegativeInteger ;
                                  owl:onDataRange :GeneratorControlMode
                                ] ,
                                [ rdf:type owl:Restriction ;
                                  owl:onProperty :GeneratingUnit_genControlSource ;
                                  owl:maxQualifiedCardinality "1"^^xsd:nonNegativeInteger ;
                                  owl:onDataRange :GeneratorControlSource
                                ] ,
                                [ rdf:type owl:Restriction ;
                                  owl:onProperty :GeneratingUnit_longPF ;
                                  owl:maxQualifiedCardinality "1"^^xsd:nonNegativeInteger ;
                                  owl:onDataRange xsd:float
                                ] ,
                                [ rdf:type owl:Restriction ;
                                  owl:onProperty :GeneratingUnit_normalPF ;
                                  owl:maxQualifiedCardinality "1"^^xsd:nonNegativeInteger ;
                                  owl:onDataRange xsd:float
                                ] ,
                                [ rdf:type owl:Restriction ;
                                  owl:onProperty :GeneratingUnit_penaltyFactor ;
                                  owl:maxQualifiedCardinality "1"^^xsd:nonNegativeInteger ;
                                  owl:onDataRange xsd:float
                                ] ,
                                [ rdf:type owl:Restriction ;
                                  owl:onProperty :GeneratingUnit_shortPF ;
                                  owl:maxQualifiedCardinality "1"^^xsd:nonNegativeInteger ;
                                  owl:onDataRange xsd:float
                                ] ,
                                [ rdf:type owl:Restriction ;
                                  owl:onProperty :GeneratingUnit_tieLinePF ;
                                  owl:maxQualifiedCardinality "1"^^xsd:nonNegativeInteger ;
                                  owl:onDataRange xsd:float
                                ] ;
                rdfs:comment "A single or set of synchronous machines for converting mechanical power into alternating-current power. For example, individual machines within a set may be defined for scheduling purposes while a single control signal is derived for the set. In this case there would be a GeneratingUnit for each member of the set and an additional GeneratingUnit corresponding to the set." .


###  https://w3id.org/netbeheer/IECCIM/TC57CIM/IEC61970/Base/Generation/Production#GrossToNetActivePowerCurve
:GrossToNetActivePowerCurve rdf:type owl:Class ;
                            rdfs:subClassOf <https://w3id.org/netbeheer/IECCIM/TC57CIM/IEC61970/Base/Core#Curve> ,
                                            [ rdf:type owl:Restriction ;
                                              owl:onProperty :GrossToNetActivePowerCurve_GeneratingUnit ;
                                              owl:minQualifiedCardinality "0"^^xsd:nonNegativeInteger ;
                                              owl:onClass :GrossToNetActivePowerCurve
                                            ] ;
                            rdfs:comment """Relationship between the generating unit's gross active power output on the X-axis (measured at the terminals of the machine(s)) and the generating unit's net active power output on the Y-axis (based on utility-defined measurements at the power station). Station service loads, when modeled, should be treated as non-conforming bus loads. There may be more than one curve, depending on the auxiliary equipment that is in service.
""" .


###  https://w3id.org/netbeheer/IECCIM/TC57CIM/IEC61970/Base/Generation/Production#HeatInputCurve
:HeatInputCurve rdf:type owl:Class ;
                rdfs:subClassOf <https://w3id.org/netbeheer/IECCIM/TC57CIM/IEC61970/Base/Core#Curve> ,
                                [ rdf:type owl:Restriction ;
                                  owl:onProperty :HeatInputCurve_ThermalGeneratingUnit ;
                                  owl:minQualifiedCardinality "0"^^xsd:nonNegativeInteger ;
                                  owl:onClass :HeatInputCurve
                                ] ,
                                [ rdf:type owl:Restriction ;
                                  owl:onProperty :HeatInputCurve_auxPowerMult ;
                                  owl:minQualifiedCardinality "0"^^xsd:nonNegativeInteger ;
                                  owl:onClass <https://w3id.org/netbeheer/IECCIM/TC57CIM/IEC61970/Base/Domain#PU>
                                ] ,
                                [ rdf:type owl:Restriction ;
                                  owl:onProperty :HeatInputCurve_auxPowerOffset ;
                                  owl:minQualifiedCardinality "0"^^xsd:nonNegativeInteger ;
                                  owl:onClass <https://w3id.org/netbeheer/IECCIM/TC57CIM/IEC61970/Base/Domain#ActivePower>
                                ] ,
                                [ rdf:type owl:Restriction ;
                                  owl:onProperty :HeatInputCurve_heatInputEff ;
                                  owl:minQualifiedCardinality "0"^^xsd:nonNegativeInteger ;
                                  owl:onClass <https://w3id.org/netbeheer/IECCIM/TC57CIM/IEC61970/Base/Domain#PU>
                                ] ,
                                [ rdf:type owl:Restriction ;
                                  owl:onProperty :HeatInputCurve_heatInputOffset ;
                                  owl:minQualifiedCardinality "0"^^xsd:nonNegativeInteger ;
                                  owl:onClass :HeatRate
                                ] ,
                                [ rdf:type owl:Restriction ;
                                  owl:onProperty :HeatInputCurve_ThermalGeneratingUnit ;
                                  owl:maxQualifiedCardinality "1"^^xsd:nonNegativeInteger ;
                                  owl:onClass :HeatInputCurve
                                ] ,
                                [ rdf:type owl:Restriction ;
                                  owl:onProperty :HeatInputCurve_auxPowerMult ;
                                  owl:maxQualifiedCardinality "1"^^xsd:nonNegativeInteger ;
                                  owl:onClass <https://w3id.org/netbeheer/IECCIM/TC57CIM/IEC61970/Base/Domain#PU>
                                ] ,
                                [ rdf:type owl:Restriction ;
                                  owl:onProperty :HeatInputCurve_auxPowerOffset ;
                                  owl:maxQualifiedCardinality "1"^^xsd:nonNegativeInteger ;
                                  owl:onClass <https://w3id.org/netbeheer/IECCIM/TC57CIM/IEC61970/Base/Domain#ActivePower>
                                ] ,
                                [ rdf:type owl:Restriction ;
                                  owl:onProperty :HeatInputCurve_heatInputEff ;
                                  owl:maxQualifiedCardinality "1"^^xsd:nonNegativeInteger ;
                                  owl:onClass <https://w3id.org/netbeheer/IECCIM/TC57CIM/IEC61970/Base/Domain#PU>
                                ] ,
                                [ rdf:type owl:Restriction ;
                                  owl:onProperty :HeatInputCurve_heatInputOffset ;
                                  owl:maxQualifiedCardinality "1"^^xsd:nonNegativeInteger ;
                                  owl:onClass :HeatRate
                                ] ,
                                [ rdf:type owl:Restriction ;
                                  owl:onProperty :HeatInputCurve_isNetGrossP ;
                                  owl:minQualifiedCardinality "0"^^xsd:nonNegativeInteger ;
                                  owl:onDataRange xsd:boolean
                                ] ,
                                [ rdf:type owl:Restriction ;
                                  owl:onProperty :HeatInputCurve_isNetGrossP ;
                                  owl:maxQualifiedCardinality "1"^^xsd:nonNegativeInteger ;
                                  owl:onDataRange xsd:boolean
                                ] ;
                rdfs:comment """Relationship between unit heat input in energy per time for main fuel (Y1-axis) and supplemental fuel (Y2-axis) versus unit output in active power (X-axis). The quantity of main fuel used to sustain generation at this output level is prorated for throttling between definition points. The quantity of supplemental fuel used at this output level is fixed and not prorated.
""" .


###  https://w3id.org/netbeheer/IECCIM/TC57CIM/IEC61970/Base/Generation/Production#HeatRate
:HeatRate rdf:type owl:Class ;
          rdfs:subClassOf [ rdf:type owl:Restriction ;
                            owl:onProperty :HeatRate_multiplier ;
                            owl:minQualifiedCardinality "0"^^xsd:nonNegativeInteger ;
                            owl:onDataRange <https://w3id.org/netbeheer/IECCIM/TC57CIM/IEC61970/Base/Domain#UnitMultiplier>
                          ] ,
                          [ rdf:type owl:Restriction ;
                            owl:onProperty :HeatRate_unit ;
                            owl:minQualifiedCardinality "0"^^xsd:nonNegativeInteger ;
                            owl:onDataRange <https://w3id.org/netbeheer/IECCIM/TC57CIM/IEC61970/Base/Domain#UnitSymbol>
                          ] ,
                          [ rdf:type owl:Restriction ;
                            owl:onProperty :HeatRate_value ;
                            owl:minQualifiedCardinality "0"^^xsd:nonNegativeInteger ;
                            owl:onDataRange xsd:float
                          ] ,
                          [ rdf:type owl:Restriction ;
                            owl:onProperty :HeatRate_multiplier ;
                            owl:maxQualifiedCardinality "1"^^xsd:nonNegativeInteger ;
                            owl:onDataRange <https://w3id.org/netbeheer/IECCIM/TC57CIM/IEC61970/Base/Domain#UnitMultiplier>
                          ] ,
                          [ rdf:type owl:Restriction ;
                            owl:onProperty :HeatRate_unit ;
                            owl:maxQualifiedCardinality "1"^^xsd:nonNegativeInteger ;
                            owl:onDataRange <https://w3id.org/netbeheer/IECCIM/TC57CIM/IEC61970/Base/Domain#UnitSymbol>
                          ] ,
                          [ rdf:type owl:Restriction ;
                            owl:onProperty :HeatRate_value ;
                            owl:maxQualifiedCardinality "1"^^xsd:nonNegativeInteger ;
                            owl:onDataRange xsd:float
                          ] ;
          rdfs:comment """Heat generated, in energy pertime unit of elapsed time.
""" .


###  https://w3id.org/netbeheer/IECCIM/TC57CIM/IEC61970/Base/Generation/Production#HeatRateCurve
:HeatRateCurve rdf:type owl:Class ;
               rdfs:subClassOf <https://w3id.org/netbeheer/IECCIM/TC57CIM/IEC61970/Base/Core#Curve> ,
                               [ rdf:type owl:Restriction ;
                                 owl:onProperty :HeatRateCurve_ThermalGeneratingUnit ;
                                 owl:minQualifiedCardinality "0"^^xsd:nonNegativeInteger ;
                                 owl:onClass :HeatRateCurve
                               ] ,
                               [ rdf:type owl:Restriction ;
                                 owl:onProperty :HeatRateCurve_ThermalGeneratingUnit ;
                                 owl:maxQualifiedCardinality "1"^^xsd:nonNegativeInteger ;
                                 owl:onClass :HeatRateCurve
                               ] ,
                               [ rdf:type owl:Restriction ;
                                 owl:onProperty :HeatRateCurve_isNetGrossP ;
                                 owl:minQualifiedCardinality "0"^^xsd:nonNegativeInteger ;
                                 owl:onDataRange xsd:boolean
                               ] ,
                               [ rdf:type owl:Restriction ;
                                 owl:onProperty :HeatRateCurve_isNetGrossP ;
                                 owl:maxQualifiedCardinality "1"^^xsd:nonNegativeInteger ;
                                 owl:onDataRange xsd:boolean
                               ] ;
               rdfs:comment "Relationship between unit heat rate per active power (Y-axis) and  unit output (X-axis). The heat input is from all fuels." .


###  https://w3id.org/netbeheer/IECCIM/TC57CIM/IEC61970/Base/Generation/Production#HydroGeneratingEfficiencyCurve
:HydroGeneratingEfficiencyCurve rdf:type owl:Class ;
                                rdfs:subClassOf <https://w3id.org/netbeheer/IECCIM/TC57CIM/IEC61970/Base/Core#Curve> ,
                                                [ rdf:type owl:Restriction ;
                                                  owl:onProperty :HydroGeneratingEfficiencyCurve_HydroGeneratingUnit ;
                                                  owl:minQualifiedCardinality "0"^^xsd:nonNegativeInteger ;
                                                  owl:onClass :HydroGeneratingEfficiencyCurve
                                                ] ;
                                rdfs:comment """Relationship between unit efficiency in percent and unit output active power for a given net head in meters. The relationship between efficiency, discharge, head, and power output is expressed as follows:   E =KP/HQ
Where:  (E=percentage)  (P=active power)  (H=height)  (Q=volume/time unit)  (K=constant)
For example, a curve instance for a given net head could relate efficiency (Y-axis) versus active power output (X-axis) or versus discharge on the X-axis.
""" .


###  https://w3id.org/netbeheer/IECCIM/TC57CIM/IEC61970/Base/Generation/Production#HydroGeneratingUnit
:HydroGeneratingUnit rdf:type owl:Class ;
                     rdfs:subClassOf :GeneratingUnit ,
                                     [ rdf:type owl:Restriction ;
                                       owl:onProperty :HydroGeneratingUnit_HydroPowerPlant ;
                                       owl:minQualifiedCardinality "0"^^xsd:nonNegativeInteger ;
                                       owl:onClass :HydroGeneratingUnit
                                     ] ,
                                     [ rdf:type owl:Restriction ;
                                       owl:onProperty :HydroGeneratingUnit_hydroUnitWaterCost ;
                                       owl:minQualifiedCardinality "0"^^xsd:nonNegativeInteger ;
                                       owl:onClass <https://w3id.org/netbeheer/IECCIM/TC57CIM/IEC61970/Base/Domain#CostPerVolume>
                                     ] ,
                                     [ rdf:type owl:Restriction ;
                                       owl:onProperty :HydroGeneratingUnit_HydroGeneratingEfficiencyCurves ;
                                       owl:qualifiedCardinality "1"^^xsd:nonNegativeInteger ;
                                       owl:onClass :HydroGeneratingUnit
                                     ] ,
                                     [ rdf:type owl:Restriction ;
                                       owl:onProperty :HydroGeneratingUnit_PenstockLossCurve ;
                                       owl:qualifiedCardinality "1"^^xsd:nonNegativeInteger ;
                                       owl:onClass :HydroGeneratingUnit
                                     ] ,
                                     [ rdf:type owl:Restriction ;
                                       owl:onProperty :HydroGeneratingUnit_TailbayLossCurve ;
                                       owl:qualifiedCardinality "1"^^xsd:nonNegativeInteger ;
                                       owl:onClass :HydroGeneratingUnit
                                     ] ,
                                     [ rdf:type owl:Restriction ;
                                       owl:onProperty :HydroGeneratingUnit_hydroUnitWaterCost ;
                                       owl:maxQualifiedCardinality "1"^^xsd:nonNegativeInteger ;
                                       owl:onClass <https://w3id.org/netbeheer/IECCIM/TC57CIM/IEC61970/Base/Domain#CostPerVolume>
                                     ] ,
                                     [ rdf:type owl:Restriction ;
                                       owl:onProperty :HydroGeneratingUnit_energyConversionCapability ;
                                       owl:minQualifiedCardinality "0"^^xsd:nonNegativeInteger ;
                                       owl:onDataRange :HydroEnergyConversionKind
                                     ] ,
                                     [ rdf:type owl:Restriction ;
                                       owl:onProperty :HydroGeneratingUnit_energyConversionCapability ;
                                       owl:maxQualifiedCardinality "1"^^xsd:nonNegativeInteger ;
                                       owl:onDataRange :HydroEnergyConversionKind
                                     ] ;
                     rdfs:comment """A generating unit whose prime mover is a hydraulic turbine (e.g., Francis, Pelton, Kaplan).
""" .


###  https://w3id.org/netbeheer/IECCIM/TC57CIM/IEC61970/Base/Generation/Production#HydroPowerPlant
:HydroPowerPlant rdf:type owl:Class ;
                 rdfs:subClassOf <https://w3id.org/netbeheer/IECCIM/TC57CIM/IEC61970/Base/Core#PowerSystemResource> ,
                                 [ rdf:type owl:Restriction ;
                                   owl:onProperty :HydroPowerPlant_GenSourcePumpDischargeReservoir ;
                                   owl:minQualifiedCardinality "0"^^xsd:nonNegativeInteger ;
                                   owl:onClass :HydroPowerPlant
                                 ] ,
                                 [ rdf:type owl:Restriction ;
                                   owl:onProperty :HydroPowerPlant_HydroGeneratingUnits ;
                                   owl:minQualifiedCardinality "0"^^xsd:nonNegativeInteger ;
                                   owl:onClass :HydroPowerPlant
                                 ] ,
                                 [ rdf:type owl:Restriction ;
                                   owl:onProperty :HydroPowerPlant_HydroPumps ;
                                   owl:minQualifiedCardinality "0"^^xsd:nonNegativeInteger ;
                                   owl:onClass :HydroPowerPlant
                                 ] ,
                                 [ rdf:type owl:Restriction ;
                                   owl:onProperty :HydroPowerPlant_Reservoir ;
                                   owl:minQualifiedCardinality "0"^^xsd:nonNegativeInteger ;
                                   owl:onClass :HydroPowerPlant
                                 ] ,
                                 [ rdf:type owl:Restriction ;
                                   owl:onProperty :HydroPowerPlant_dischargeTravelDelay ;
                                   owl:minQualifiedCardinality "0"^^xsd:nonNegativeInteger ;
                                   owl:onClass <https://w3id.org/netbeheer/IECCIM/TC57CIM/IEC61970/Base/Domain#Seconds>
                                 ] ,
                                 [ rdf:type owl:Restriction ;
                                   owl:onProperty :HydroPowerPlant_genRatedP ;
                                   owl:minQualifiedCardinality "0"^^xsd:nonNegativeInteger ;
                                   owl:onClass <https://w3id.org/netbeheer/IECCIM/TC57CIM/IEC61970/Base/Domain#ActivePower>
                                 ] ,
                                 [ rdf:type owl:Restriction ;
                                   owl:onProperty :HydroPowerPlant_plantDischargeCapacity ;
                                   owl:minQualifiedCardinality "0"^^xsd:nonNegativeInteger ;
                                   owl:onClass <https://w3id.org/netbeheer/IECCIM/TC57CIM/IEC61970/Base/Domain#VolumeFlowRate>
                                 ] ,
                                 [ rdf:type owl:Restriction ;
                                   owl:onProperty :HydroPowerPlant_plantRatedHead ;
                                   owl:minQualifiedCardinality "0"^^xsd:nonNegativeInteger ;
                                   owl:onClass <https://w3id.org/netbeheer/IECCIM/TC57CIM/IEC61970/Base/Domain#Length>
                                 ] ,
                                 [ rdf:type owl:Restriction ;
                                   owl:onProperty :HydroPowerPlant_pumpRatedP ;
                                   owl:minQualifiedCardinality "0"^^xsd:nonNegativeInteger ;
                                   owl:onClass <https://w3id.org/netbeheer/IECCIM/TC57CIM/IEC61970/Base/Domain#ActivePower>
                                 ] ,
                                 [ rdf:type owl:Restriction ;
                                   owl:onProperty :HydroPowerPlant_surgeTankCrestLevel ;
                                   owl:minQualifiedCardinality "0"^^xsd:nonNegativeInteger ;
                                   owl:onClass <https://w3id.org/netbeheer/IECCIM/TC57CIM/IEC61970/Base/Domain#WaterLevel>
                                 ] ,
                                 [ rdf:type owl:Restriction ;
                                   owl:onProperty :HydroPowerPlant_HydroGeneratingUnits ;
                                   owl:maxQualifiedCardinality "1"^^xsd:nonNegativeInteger ;
                                   owl:onClass :HydroPowerPlant
                                 ] ,
                                 [ rdf:type owl:Restriction ;
                                   owl:onProperty :HydroPowerPlant_HydroPumps ;
                                   owl:maxQualifiedCardinality "1"^^xsd:nonNegativeInteger ;
                                   owl:onClass :HydroPowerPlant
                                 ] ,
                                 [ rdf:type owl:Restriction ;
                                   owl:onProperty :HydroPowerPlant_dischargeTravelDelay ;
                                   owl:maxQualifiedCardinality "1"^^xsd:nonNegativeInteger ;
                                   owl:onClass <https://w3id.org/netbeheer/IECCIM/TC57CIM/IEC61970/Base/Domain#Seconds>
                                 ] ,
                                 [ rdf:type owl:Restriction ;
                                   owl:onProperty :HydroPowerPlant_genRatedP ;
                                   owl:maxQualifiedCardinality "1"^^xsd:nonNegativeInteger ;
                                   owl:onClass <https://w3id.org/netbeheer/IECCIM/TC57CIM/IEC61970/Base/Domain#ActivePower>
                                 ] ,
                                 [ rdf:type owl:Restriction ;
                                   owl:onProperty :HydroPowerPlant_plantDischargeCapacity ;
                                   owl:maxQualifiedCardinality "1"^^xsd:nonNegativeInteger ;
                                   owl:onClass <https://w3id.org/netbeheer/IECCIM/TC57CIM/IEC61970/Base/Domain#VolumeFlowRate>
                                 ] ,
                                 [ rdf:type owl:Restriction ;
                                   owl:onProperty :HydroPowerPlant_plantRatedHead ;
                                   owl:maxQualifiedCardinality "1"^^xsd:nonNegativeInteger ;
                                   owl:onClass <https://w3id.org/netbeheer/IECCIM/TC57CIM/IEC61970/Base/Domain#Length>
                                 ] ,
                                 [ rdf:type owl:Restriction ;
                                   owl:onProperty :HydroPowerPlant_pumpRatedP ;
                                   owl:maxQualifiedCardinality "1"^^xsd:nonNegativeInteger ;
                                   owl:onClass <https://w3id.org/netbeheer/IECCIM/TC57CIM/IEC61970/Base/Domain#ActivePower>
                                 ] ,
                                 [ rdf:type owl:Restriction ;
                                   owl:onProperty :HydroPowerPlant_surgeTankCrestLevel ;
                                   owl:maxQualifiedCardinality "1"^^xsd:nonNegativeInteger ;
                                   owl:onClass <https://w3id.org/netbeheer/IECCIM/TC57CIM/IEC61970/Base/Domain#WaterLevel>
                                 ] ,
                                 [ rdf:type owl:Restriction ;
                                   owl:onProperty :HydroPowerPlant_hydroPlantStorageType ;
                                   owl:minQualifiedCardinality "0"^^xsd:nonNegativeInteger ;
                                   owl:onDataRange :HydroPlantStorageKind
                                 ] ,
                                 [ rdf:type owl:Restriction ;
                                   owl:onProperty :HydroPowerPlant_penstockType ;
                                   owl:minQualifiedCardinality "0"^^xsd:nonNegativeInteger ;
                                   owl:onDataRange xsd:string
                                 ] ,
                                 [ rdf:type owl:Restriction ;
                                   owl:onProperty :HydroPowerPlant_surgeTankCode ;
                                   owl:minQualifiedCardinality "0"^^xsd:nonNegativeInteger ;
                                   owl:onDataRange xsd:string
                                 ] ,
                                 [ rdf:type owl:Restriction ;
                                   owl:onProperty :HydroPowerPlant_hydroPlantStorageType ;
                                   owl:maxQualifiedCardinality "1"^^xsd:nonNegativeInteger ;
                                   owl:onDataRange :HydroPlantStorageKind
                                 ] ,
                                 [ rdf:type owl:Restriction ;
                                   owl:onProperty :HydroPowerPlant_penstockType ;
                                   owl:maxQualifiedCardinality "1"^^xsd:nonNegativeInteger ;
                                   owl:onDataRange xsd:string
                                 ] ,
                                 [ rdf:type owl:Restriction ;
                                   owl:onProperty :HydroPowerPlant_surgeTankCode ;
                                   owl:maxQualifiedCardinality "1"^^xsd:nonNegativeInteger ;
                                   owl:onDataRange xsd:string
                                 ] ;
                 rdfs:comment "A hydro power station which can generate or pump. When generating, the generator turbines receive water from an upper reservoir. When pumping, the pumps receive their water from a lower reservoir." .


###  https://w3id.org/netbeheer/IECCIM/TC57CIM/IEC61970/Base/Generation/Production#HydroPump
:HydroPump rdf:type owl:Class ;
           rdfs:subClassOf <https://w3id.org/netbeheer/IECCIM/TC57CIM/IEC61970/Base/Core#Equipment> ,
                           [ rdf:type owl:Restriction ;
                             owl:onProperty :HydroPump_HydroPowerPlant ;
                             owl:minQualifiedCardinality "0"^^xsd:nonNegativeInteger ;
                             owl:onClass :HydroPump
                           ] ,
                           [ rdf:type owl:Restriction ;
                             owl:onProperty :HydroPump_pumpDischAtMaxHead ;
                             owl:minQualifiedCardinality "0"^^xsd:nonNegativeInteger ;
                             owl:onClass <https://w3id.org/netbeheer/IECCIM/TC57CIM/IEC61970/Base/Domain#VolumeFlowRate>
                           ] ,
                           [ rdf:type owl:Restriction ;
                             owl:onProperty :HydroPump_pumpDischAtMinHead ;
                             owl:minQualifiedCardinality "0"^^xsd:nonNegativeInteger ;
                             owl:onClass <https://w3id.org/netbeheer/IECCIM/TC57CIM/IEC61970/Base/Domain#VolumeFlowRate>
                           ] ,
                           [ rdf:type owl:Restriction ;
                             owl:onProperty :HydroPump_pumpPowerAtMaxHead ;
                             owl:minQualifiedCardinality "0"^^xsd:nonNegativeInteger ;
                             owl:onClass <https://w3id.org/netbeheer/IECCIM/TC57CIM/IEC61970/Base/Domain#ActivePower>
                           ] ,
                           [ rdf:type owl:Restriction ;
                             owl:onProperty :HydroPump_pumpPowerAtMinHead ;
                             owl:minQualifiedCardinality "0"^^xsd:nonNegativeInteger ;
                             owl:onClass <https://w3id.org/netbeheer/IECCIM/TC57CIM/IEC61970/Base/Domain#ActivePower>
                           ] ,
                           [ rdf:type owl:Restriction ;
                             owl:onProperty :HydroPump_HydroPumpOpSchedule ;
                             owl:qualifiedCardinality "1"^^xsd:nonNegativeInteger ;
                             owl:onClass :HydroPump
                           ] ,
                           [ rdf:type owl:Restriction ;
                             owl:onProperty :HydroPump_pumpDischAtMaxHead ;
                             owl:maxQualifiedCardinality "1"^^xsd:nonNegativeInteger ;
                             owl:onClass <https://w3id.org/netbeheer/IECCIM/TC57CIM/IEC61970/Base/Domain#VolumeFlowRate>
                           ] ,
                           [ rdf:type owl:Restriction ;
                             owl:onProperty :HydroPump_pumpDischAtMinHead ;
                             owl:maxQualifiedCardinality "1"^^xsd:nonNegativeInteger ;
                             owl:onClass <https://w3id.org/netbeheer/IECCIM/TC57CIM/IEC61970/Base/Domain#VolumeFlowRate>
                           ] ,
                           [ rdf:type owl:Restriction ;
                             owl:onProperty :HydroPump_pumpPowerAtMaxHead ;
                             owl:maxQualifiedCardinality "1"^^xsd:nonNegativeInteger ;
                             owl:onClass <https://w3id.org/netbeheer/IECCIM/TC57CIM/IEC61970/Base/Domain#ActivePower>
                           ] ,
                           [ rdf:type owl:Restriction ;
                             owl:onProperty :HydroPump_pumpPowerAtMinHead ;
                             owl:maxQualifiedCardinality "1"^^xsd:nonNegativeInteger ;
                             owl:onClass <https://w3id.org/netbeheer/IECCIM/TC57CIM/IEC61970/Base/Domain#ActivePower>
                           ] ;
           rdfs:comment "A synchronous motor-driven pump, typically associated with a pumped storage plant." .


###  https://w3id.org/netbeheer/IECCIM/TC57CIM/IEC61970/Base/Generation/Production#HydroPumpOpSchedule
:HydroPumpOpSchedule rdf:type owl:Class ;
                     rdfs:subClassOf <https://w3id.org/netbeheer/IECCIM/TC57CIM/IEC61970/Base/Core#RegularIntervalSchedule> ,
                                     [ rdf:type owl:Restriction ;
                                       owl:onProperty :HydroPumpOpSchedule_HydroPump ;
                                       owl:minQualifiedCardinality "0"^^xsd:nonNegativeInteger ;
                                       owl:onClass :HydroPumpOpSchedule
                                     ] ,
                                     [ rdf:type owl:Restriction ;
                                       owl:onProperty :HydroPumpOpSchedule_HydroPump ;
                                       owl:maxQualifiedCardinality "1"^^xsd:nonNegativeInteger ;
                                       owl:onClass :HydroPumpOpSchedule
                                     ] ;
                     rdfs:comment """The hydro pump's Operator-approved current operating schedule (or plan), typically produced with the aid of unit commitment type analyses.The unit's operating schedule status is typically given as: (0=unavailable) (1=avilable to startup or shutdown)  (2=must pump).
""" .


###  https://w3id.org/netbeheer/IECCIM/TC57CIM/IEC61970/Base/Generation/Production#IncrementalHeatRateCurve
:IncrementalHeatRateCurve rdf:type owl:Class ;
                          rdfs:subClassOf <https://w3id.org/netbeheer/IECCIM/TC57CIM/IEC61970/Base/Core#Curve> ,
                                          [ rdf:type owl:Restriction ;
                                            owl:onProperty :IncrementalHeatRateCurve_ThermalGeneratingUnit ;
                                            owl:minQualifiedCardinality "0"^^xsd:nonNegativeInteger ;
                                            owl:onClass :IncrementalHeatRateCurve
                                          ] ,
                                          [ rdf:type owl:Restriction ;
                                            owl:onProperty :IncrementalHeatRateCurve_ThermalGeneratingUnit ;
                                            owl:maxQualifiedCardinality "1"^^xsd:nonNegativeInteger ;
                                            owl:onClass :IncrementalHeatRateCurve
                                          ] ,
                                          [ rdf:type owl:Restriction ;
                                            owl:onProperty :IncrementalHeatRateCurve_isNetGrossP ;
                                            owl:minQualifiedCardinality "0"^^xsd:nonNegativeInteger ;
                                            owl:onDataRange xsd:boolean
                                          ] ,
                                          [ rdf:type owl:Restriction ;
                                            owl:onProperty :IncrementalHeatRateCurve_isNetGrossP ;
                                            owl:maxQualifiedCardinality "1"^^xsd:nonNegativeInteger ;
                                            owl:onDataRange xsd:boolean
                                          ] ;
                          rdfs:comment "Relationship between unit incremental heat rate in (delta energy/time) per (delta active power) and unit output in active power. The IHR curve represents the slope of the HeatInputCurve. Note that the \"incremental heat rate\" and the \"heat rate\" have the same engineering units." .


###  https://w3id.org/netbeheer/IECCIM/TC57CIM/IEC61970/Base/Generation/Production#InflowForecast
:InflowForecast rdf:type owl:Class ;
                rdfs:subClassOf <https://w3id.org/netbeheer/IECCIM/TC57CIM/IEC61970/Base/Core#RegularIntervalSchedule> ,
                                [ rdf:type owl:Restriction ;
                                  owl:onProperty :InflowForecast_Reservoir ;
                                  owl:minQualifiedCardinality "0"^^xsd:nonNegativeInteger ;
                                  owl:onClass :InflowForecast
                                ] ;
                rdfs:comment "Natural water inflow to a reservoir, usually forecasted from predicted rain and snowmelt. Typically in one hour increments for up to 10 days. The forecast is given in average cubic meters per second over the time increment." .


###  https://w3id.org/netbeheer/IECCIM/TC57CIM/IEC61970/Base/Generation/Production#LevelVsVolumeCurve
:LevelVsVolumeCurve rdf:type owl:Class ;
                    rdfs:subClassOf <https://w3id.org/netbeheer/IECCIM/TC57CIM/IEC61970/Base/Core#Curve> ,
                                    [ rdf:type owl:Restriction ;
                                      owl:onProperty :LevelVsVolumeCurve_Reservoir ;
                                      owl:minQualifiedCardinality "0"^^xsd:nonNegativeInteger ;
                                      owl:onClass :LevelVsVolumeCurve
                                    ] ;
                    rdfs:comment "Relationship between reservoir volume and reservoir level. The  volume is at the y-axis and the reservoir level at the x-axis." .


###  https://w3id.org/netbeheer/IECCIM/TC57CIM/IEC61970/Base/Generation/Production#NuclearGeneratingUnit
:NuclearGeneratingUnit rdf:type owl:Class ;
                       rdfs:subClassOf :GeneratingUnit ;
                       rdfs:comment "A nuclear generating unit." .


###  https://w3id.org/netbeheer/IECCIM/TC57CIM/IEC61970/Base/Generation/Production#PenstockLossCurve
:PenstockLossCurve rdf:type owl:Class ;
                   rdfs:subClassOf <https://w3id.org/netbeheer/IECCIM/TC57CIM/IEC61970/Base/Core#Curve> ,
                                   [ rdf:type owl:Restriction ;
                                     owl:onProperty :PenstockLossCurve_HydroGeneratingUnit ;
                                     owl:minQualifiedCardinality "0"^^xsd:nonNegativeInteger ;
                                     owl:onClass :PenstockLossCurve
                                   ] ,
                                   [ rdf:type owl:Restriction ;
                                     owl:onProperty :PenstockLossCurve_HydroGeneratingUnit ;
                                     owl:maxQualifiedCardinality "1"^^xsd:nonNegativeInteger ;
                                     owl:onClass :PenstockLossCurve
                                   ] ;
                   rdfs:comment "Relationship between penstock head loss (in meters) and  total discharge through the penstock (in cubic meters per second). One or more turbines may be connected to the same penstock." .


###  https://w3id.org/netbeheer/IECCIM/TC57CIM/IEC61970/Base/Generation/Production#Reservoir
:Reservoir rdf:type owl:Class ;
           rdfs:subClassOf <https://w3id.org/netbeheer/IECCIM/TC57CIM/IEC61970/Base/Core#PowerSystemResource> ,
                           [ rdf:type owl:Restriction ;
                             owl:onProperty :Reservoir_HydroPowerPlants ;
                             owl:minQualifiedCardinality "0"^^xsd:nonNegativeInteger ;
                             owl:onClass :Reservoir
                           ] ,
                           [ rdf:type owl:Restriction ;
                             owl:onProperty :Reservoir_SpillsFromReservoir ;
                             owl:minQualifiedCardinality "0"^^xsd:nonNegativeInteger ;
                             owl:onClass :Reservoir
                           ] ,
                           [ rdf:type owl:Restriction ;
                             owl:onProperty :Reservoir_SpillsIntoReservoirs ;
                             owl:minQualifiedCardinality "0"^^xsd:nonNegativeInteger ;
                             owl:onClass :Reservoir
                           ] ,
                           [ rdf:type owl:Restriction ;
                             owl:onProperty :Reservoir_activeStorageCapacity ;
                             owl:minQualifiedCardinality "0"^^xsd:nonNegativeInteger ;
                             owl:onClass <https://w3id.org/netbeheer/IECCIM/TC57CIM/IEC61970/Base/Domain#Volume>
                           ] ,
                           [ rdf:type owl:Restriction ;
                             owl:onProperty :Reservoir_fullSupplyLevel ;
                             owl:minQualifiedCardinality "0"^^xsd:nonNegativeInteger ;
                             owl:onClass <https://w3id.org/netbeheer/IECCIM/TC57CIM/IEC61970/Base/Domain#WaterLevel>
                           ] ,
                           [ rdf:type owl:Restriction ;
                             owl:onProperty :Reservoir_grossCapacity ;
                             owl:minQualifiedCardinality "0"^^xsd:nonNegativeInteger ;
                             owl:onClass <https://w3id.org/netbeheer/IECCIM/TC57CIM/IEC61970/Base/Domain#Volume>
                           ] ,
                           [ rdf:type owl:Restriction ;
                             owl:onProperty :Reservoir_normalMinOperateLevel ;
                             owl:minQualifiedCardinality "0"^^xsd:nonNegativeInteger ;
                             owl:onClass <https://w3id.org/netbeheer/IECCIM/TC57CIM/IEC61970/Base/Domain#WaterLevel>
                           ] ,
                           [ rdf:type owl:Restriction ;
                             owl:onProperty :Reservoir_spillTravelDelay ;
                             owl:minQualifiedCardinality "0"^^xsd:nonNegativeInteger ;
                             owl:onClass <https://w3id.org/netbeheer/IECCIM/TC57CIM/IEC61970/Base/Domain#Seconds>
                           ] ,
                           [ rdf:type owl:Restriction ;
                             owl:onProperty :Reservoir_spillwayCrestLength ;
                             owl:minQualifiedCardinality "0"^^xsd:nonNegativeInteger ;
                             owl:onClass <https://w3id.org/netbeheer/IECCIM/TC57CIM/IEC61970/Base/Domain#Length>
                           ] ,
                           [ rdf:type owl:Restriction ;
                             owl:onProperty :Reservoir_spillwayCrestLevel ;
                             owl:minQualifiedCardinality "0"^^xsd:nonNegativeInteger ;
                             owl:onClass <https://w3id.org/netbeheer/IECCIM/TC57CIM/IEC61970/Base/Domain#WaterLevel>
                           ] ,
                           [ rdf:type owl:Restriction ;
                             owl:onProperty :Reservoir_InflowForecasts ;
                             owl:qualifiedCardinality "1"^^xsd:nonNegativeInteger ;
                             owl:onClass :Reservoir
                           ] ,
                           [ rdf:type owl:Restriction ;
                             owl:onProperty :Reservoir_LevelVsVolumeCurves ;
                             owl:qualifiedCardinality "1"^^xsd:nonNegativeInteger ;
                             owl:onClass :Reservoir
                           ] ,
                           [ rdf:type owl:Restriction ;
                             owl:onProperty :Reservoir_TargetLevelSchedule ;
                             owl:qualifiedCardinality "1"^^xsd:nonNegativeInteger ;
                             owl:onClass :Reservoir
                           ] ,
                           [ rdf:type owl:Restriction ;
                             owl:onProperty :Reservoir_UpstreamFromHydroPowerPlants ;
                             owl:qualifiedCardinality "1"^^xsd:nonNegativeInteger ;
                             owl:onClass :Reservoir
                           ] ,
                           [ rdf:type owl:Restriction ;
                             owl:onProperty :Reservoir_HydroPowerPlants ;
                             owl:maxQualifiedCardinality "1"^^xsd:nonNegativeInteger ;
                             owl:onClass :Reservoir
                           ] ,
                           [ rdf:type owl:Restriction ;
                             owl:onProperty :Reservoir_SpillsIntoReservoirs ;
                             owl:maxQualifiedCardinality "1"^^xsd:nonNegativeInteger ;
                             owl:onClass :Reservoir
                           ] ,
                           [ rdf:type owl:Restriction ;
                             owl:onProperty :Reservoir_activeStorageCapacity ;
                             owl:maxQualifiedCardinality "1"^^xsd:nonNegativeInteger ;
                             owl:onClass <https://w3id.org/netbeheer/IECCIM/TC57CIM/IEC61970/Base/Domain#Volume>
                           ] ,
                           [ rdf:type owl:Restriction ;
                             owl:onProperty :Reservoir_fullSupplyLevel ;
                             owl:maxQualifiedCardinality "1"^^xsd:nonNegativeInteger ;
                             owl:onClass <https://w3id.org/netbeheer/IECCIM/TC57CIM/IEC61970/Base/Domain#WaterLevel>
                           ] ,
                           [ rdf:type owl:Restriction ;
                             owl:onProperty :Reservoir_grossCapacity ;
                             owl:maxQualifiedCardinality "1"^^xsd:nonNegativeInteger ;
                             owl:onClass <https://w3id.org/netbeheer/IECCIM/TC57CIM/IEC61970/Base/Domain#Volume>
                           ] ,
                           [ rdf:type owl:Restriction ;
                             owl:onProperty :Reservoir_normalMinOperateLevel ;
                             owl:maxQualifiedCardinality "1"^^xsd:nonNegativeInteger ;
                             owl:onClass <https://w3id.org/netbeheer/IECCIM/TC57CIM/IEC61970/Base/Domain#WaterLevel>
                           ] ,
                           [ rdf:type owl:Restriction ;
                             owl:onProperty :Reservoir_spillTravelDelay ;
                             owl:maxQualifiedCardinality "1"^^xsd:nonNegativeInteger ;
                             owl:onClass <https://w3id.org/netbeheer/IECCIM/TC57CIM/IEC61970/Base/Domain#Seconds>
                           ] ,
                           [ rdf:type owl:Restriction ;
                             owl:onProperty :Reservoir_spillwayCrestLength ;
                             owl:maxQualifiedCardinality "1"^^xsd:nonNegativeInteger ;
                             owl:onClass <https://w3id.org/netbeheer/IECCIM/TC57CIM/IEC61970/Base/Domain#Length>
                           ] ,
                           [ rdf:type owl:Restriction ;
                             owl:onProperty :Reservoir_spillwayCrestLevel ;
                             owl:maxQualifiedCardinality "1"^^xsd:nonNegativeInteger ;
                             owl:onClass <https://w3id.org/netbeheer/IECCIM/TC57CIM/IEC61970/Base/Domain#WaterLevel>
                           ] ,
                           [ rdf:type owl:Restriction ;
                             owl:onProperty :Reservoir_energyStorageRating ;
                             owl:minQualifiedCardinality "0"^^xsd:nonNegativeInteger ;
                             owl:onDataRange xsd:float
                           ] ,
                           [ rdf:type owl:Restriction ;
                             owl:onProperty :Reservoir_riverOutletWorks ;
                             owl:minQualifiedCardinality "0"^^xsd:nonNegativeInteger ;
                             owl:onDataRange xsd:string
                           ] ,
                           [ rdf:type owl:Restriction ;
                             owl:onProperty :Reservoir_spillWayGateType ;
                             owl:minQualifiedCardinality "0"^^xsd:nonNegativeInteger ;
                             owl:onDataRange xsd:string
                           ] ,
                           [ rdf:type owl:Restriction ;
                             owl:onProperty :Reservoir_spillwayCapacity ;
                             owl:minQualifiedCardinality "0"^^xsd:nonNegativeInteger ;
                             owl:onDataRange xsd:float
                           ] ,
                           [ rdf:type owl:Restriction ;
                             owl:onProperty :Reservoir_energyStorageRating ;
                             owl:maxQualifiedCardinality "1"^^xsd:nonNegativeInteger ;
                             owl:onDataRange xsd:float
                           ] ,
                           [ rdf:type owl:Restriction ;
                             owl:onProperty :Reservoir_riverOutletWorks ;
                             owl:maxQualifiedCardinality "1"^^xsd:nonNegativeInteger ;
                             owl:onDataRange xsd:string
                           ] ,
                           [ rdf:type owl:Restriction ;
                             owl:onProperty :Reservoir_spillWayGateType ;
                             owl:maxQualifiedCardinality "1"^^xsd:nonNegativeInteger ;
                             owl:onDataRange xsd:string
                           ] ,
                           [ rdf:type owl:Restriction ;
                             owl:onProperty :Reservoir_spillwayCapacity ;
                             owl:maxQualifiedCardinality "1"^^xsd:nonNegativeInteger ;
                             owl:onDataRange xsd:float
                           ] ;
           rdfs:comment """A water storage facility within a hydro system, including: ponds, lakes, lagoons, and rivers. The storage is usually behind some type of dam.
""" .


###  https://w3id.org/netbeheer/IECCIM/TC57CIM/IEC61970/Base/Generation/Production#ShutdownCurve
:ShutdownCurve rdf:type owl:Class ;
               rdfs:subClassOf <https://w3id.org/netbeheer/IECCIM/TC57CIM/IEC61970/Base/Core#Curve> ,
                               [ rdf:type owl:Restriction ;
                                 owl:onProperty :ShutdownCurve_ThermalGeneratingUnit ;
                                 owl:minQualifiedCardinality "0"^^xsd:nonNegativeInteger ;
                                 owl:onClass :ShutdownCurve
                               ] ,
                               [ rdf:type owl:Restriction ;
                                 owl:onProperty :ShutdownCurve_shutdownCost ;
                                 owl:minQualifiedCardinality "0"^^xsd:nonNegativeInteger ;
                                 owl:onClass <https://w3id.org/netbeheer/IECCIM/TC57CIM/IEC61970/Base/Domain#Money>
                               ] ,
                               [ rdf:type owl:Restriction ;
                                 owl:onProperty :ShutdownCurve_ThermalGeneratingUnit ;
                                 owl:maxQualifiedCardinality "1"^^xsd:nonNegativeInteger ;
                                 owl:onClass :ShutdownCurve
                               ] ,
                               [ rdf:type owl:Restriction ;
                                 owl:onProperty :ShutdownCurve_shutdownCost ;
                                 owl:maxQualifiedCardinality "1"^^xsd:nonNegativeInteger ;
                                 owl:onClass <https://w3id.org/netbeheer/IECCIM/TC57CIM/IEC61970/Base/Domain#Money>
                               ] ,
                               [ rdf:type owl:Restriction ;
                                 owl:onProperty :ShutdownCurve_shutdownDate ;
                                 owl:minQualifiedCardinality "0"^^xsd:nonNegativeInteger ;
                                 owl:onDataRange xsd:dateTime
                               ] ,
                               [ rdf:type owl:Restriction ;
                                 owl:onProperty :ShutdownCurve_shutdownDate ;
                                 owl:maxQualifiedCardinality "1"^^xsd:nonNegativeInteger ;
                                 owl:onDataRange xsd:dateTime
                               ] ;
               rdfs:comment """Relationship between the rate in gross active power/minute (Y-axis) at which a unit should be shutdown and its present gross MW output (X-axis).
""" .


###  https://w3id.org/netbeheer/IECCIM/TC57CIM/IEC61970/Base/Generation/Production#SolarGeneratingUnit
:SolarGeneratingUnit rdf:type owl:Class ;
                     rdfs:subClassOf :GeneratingUnit ;
                     rdfs:comment "A solar thermal generating unit." .


###  https://w3id.org/netbeheer/IECCIM/TC57CIM/IEC61970/Base/Generation/Production#StartIgnFuelCurve
:StartIgnFuelCurve rdf:type owl:Class ;
                   rdfs:subClassOf <https://w3id.org/netbeheer/IECCIM/TC57CIM/IEC61970/Base/Core#Curve> ,
                                   [ rdf:type owl:Restriction ;
                                     owl:onProperty :StartIgnFuelCurve_StartupModel ;
                                     owl:minQualifiedCardinality "0"^^xsd:nonNegativeInteger ;
                                     owl:onClass :StartIgnFuelCurve
                                   ] ,
                                   [ rdf:type owl:Restriction ;
                                     owl:onProperty :StartIgnFuelCurve_StartupModel ;
                                     owl:maxQualifiedCardinality "1"^^xsd:nonNegativeInteger ;
                                     owl:onClass :StartIgnFuelCurve
                                   ] ,
                                   [ rdf:type owl:Restriction ;
                                     owl:onProperty :StartIgnFuelCurve_ignitionFuelType ;
                                     owl:minQualifiedCardinality "0"^^xsd:nonNegativeInteger ;
                                     owl:onDataRange :FuelType
                                   ] ,
                                   [ rdf:type owl:Restriction ;
                                     owl:onProperty :StartIgnFuelCurve_ignitionFuelType ;
                                     owl:maxQualifiedCardinality "1"^^xsd:nonNegativeInteger ;
                                     owl:onDataRange :FuelType
                                   ] ;
                   rdfs:comment """The quantity of ignition fuel (Y-axis) used to restart and repay the auxiliary power consumed versus the number of hours (X-axis) the unit was off line.
""" .


###  https://w3id.org/netbeheer/IECCIM/TC57CIM/IEC61970/Base/Generation/Production#StartMainFuelCurve
:StartMainFuelCurve rdf:type owl:Class ;
                    rdfs:subClassOf <https://w3id.org/netbeheer/IECCIM/TC57CIM/IEC61970/Base/Core#Curve> ,
                                    [ rdf:type owl:Restriction ;
                                      owl:onProperty :StartMainFuelCurve_StartupModel ;
                                      owl:minQualifiedCardinality "0"^^xsd:nonNegativeInteger ;
                                      owl:onClass :StartMainFuelCurve
                                    ] ,
                                    [ rdf:type owl:Restriction ;
                                      owl:onProperty :StartMainFuelCurve_StartupModel ;
                                      owl:maxQualifiedCardinality "1"^^xsd:nonNegativeInteger ;
                                      owl:onClass :StartMainFuelCurve
                                    ] ,
                                    [ rdf:type owl:Restriction ;
                                      owl:onProperty :StartMainFuelCurve_mainFuelType ;
                                      owl:minQualifiedCardinality "0"^^xsd:nonNegativeInteger ;
                                      owl:onDataRange :FuelType
                                    ] ,
                                    [ rdf:type owl:Restriction ;
                                      owl:onProperty :StartMainFuelCurve_mainFuelType ;
                                      owl:maxQualifiedCardinality "1"^^xsd:nonNegativeInteger ;
                                      owl:onDataRange :FuelType
                                    ] ;
                    rdfs:comment """The quantity of main fuel (Y-axis) used to restart and repay the auxiliary power consumed versus the number of hours (X-axis) the unit was off line.
""" .


###  https://w3id.org/netbeheer/IECCIM/TC57CIM/IEC61970/Base/Generation/Production#StartRampCurve
:StartRampCurve rdf:type owl:Class ;
                rdfs:subClassOf <https://w3id.org/netbeheer/IECCIM/TC57CIM/IEC61970/Base/Core#Curve> ,
                                [ rdf:type owl:Restriction ;
                                  owl:onProperty :StartRampCurve_StartupModel ;
                                  owl:minQualifiedCardinality "0"^^xsd:nonNegativeInteger ;
                                  owl:onClass :StartRampCurve
                                ] ,
                                [ rdf:type owl:Restriction ;
                                  owl:onProperty :StartRampCurve_hotStandbyRamp ;
                                  owl:minQualifiedCardinality "0"^^xsd:nonNegativeInteger ;
                                  owl:onClass <https://w3id.org/netbeheer/IECCIM/TC57CIM/IEC61970/Base/Domain#ActivePowerChangeRate>
                                ] ,
                                [ rdf:type owl:Restriction ;
                                  owl:onProperty :StartRampCurve_StartupModel ;
                                  owl:maxQualifiedCardinality "1"^^xsd:nonNegativeInteger ;
                                  owl:onClass :StartRampCurve
                                ] ,
                                [ rdf:type owl:Restriction ;
                                  owl:onProperty :StartRampCurve_hotStandbyRamp ;
                                  owl:maxQualifiedCardinality "1"^^xsd:nonNegativeInteger ;
                                  owl:onClass <https://w3id.org/netbeheer/IECCIM/TC57CIM/IEC61970/Base/Domain#ActivePowerChangeRate>
                                ] ;
                rdfs:comment """Rate in gross active power/minute (Y-axis) at which a unit can be loaded versus the number of hours (X-axis) the unit was off line.
""" .


###  https://w3id.org/netbeheer/IECCIM/TC57CIM/IEC61970/Base/Generation/Production#StartupModel
:StartupModel rdf:type owl:Class ;
              rdfs:subClassOf <https://w3id.org/netbeheer/IECCIM/TC57CIM/IEC61970/Base/Core#IdentifiedObject> ,
                              [ rdf:type owl:Restriction ;
                                owl:onProperty :StartupModel_ThermalGeneratingUnit ;
                                owl:minQualifiedCardinality "0"^^xsd:nonNegativeInteger ;
                                owl:onClass :StartupModel
                              ] ,
                              [ rdf:type owl:Restriction ;
                                owl:onProperty :StartupModel_fixedMaintCost ;
                                owl:minQualifiedCardinality "0"^^xsd:nonNegativeInteger ;
                                owl:onClass <https://w3id.org/netbeheer/IECCIM/TC57CIM/IEC61970/Base/Domain#CostRate>
                              ] ,
                              [ rdf:type owl:Restriction ;
                                owl:onProperty :StartupModel_hotStandbyHeat ;
                                owl:minQualifiedCardinality "0"^^xsd:nonNegativeInteger ;
                                owl:onClass :HeatRate
                              ] ,
                              [ rdf:type owl:Restriction ;
                                owl:onProperty :StartupModel_incrementalMaintCost ;
                                owl:minQualifiedCardinality "0"^^xsd:nonNegativeInteger ;
                                owl:onClass <https://w3id.org/netbeheer/IECCIM/TC57CIM/IEC61970/Base/Domain#CostPerEnergyUnit>
                              ] ,
                              [ rdf:type owl:Restriction ;
                                owl:onProperty :StartupModel_minimumDownTime ;
                                owl:minQualifiedCardinality "0"^^xsd:nonNegativeInteger ;
                                owl:onClass <https://w3id.org/netbeheer/IECCIM/TC57CIM/IEC61970/Base/Domain#Hours>
                              ] ,
                              [ rdf:type owl:Restriction ;
                                owl:onProperty :StartupModel_minimumRunTime ;
                                owl:minQualifiedCardinality "0"^^xsd:nonNegativeInteger ;
                                owl:onClass <https://w3id.org/netbeheer/IECCIM/TC57CIM/IEC61970/Base/Domain#Hours>
                              ] ,
                              [ rdf:type owl:Restriction ;
                                owl:onProperty :StartupModel_riskFactorCost ;
                                owl:minQualifiedCardinality "0"^^xsd:nonNegativeInteger ;
                                owl:onClass <https://w3id.org/netbeheer/IECCIM/TC57CIM/IEC61970/Base/Domain#Money>
                              ] ,
                              [ rdf:type owl:Restriction ;
                                owl:onProperty :StartupModel_startupCost ;
                                owl:minQualifiedCardinality "0"^^xsd:nonNegativeInteger ;
                                owl:onClass <https://w3id.org/netbeheer/IECCIM/TC57CIM/IEC61970/Base/Domain#Money>
                              ] ,
                              [ rdf:type owl:Restriction ;
                                owl:onProperty :StartupModel_stbyAuxP ;
                                owl:minQualifiedCardinality "0"^^xsd:nonNegativeInteger ;
                                owl:onClass <https://w3id.org/netbeheer/IECCIM/TC57CIM/IEC61970/Base/Domain#ActivePower>
                              ] ,
                              [ rdf:type owl:Restriction ;
                                owl:onProperty :StartupModel_StartIgnFuelCurve ;
                                owl:qualifiedCardinality "1"^^xsd:nonNegativeInteger ;
                                owl:onClass :StartupModel
                              ] ,
                              [ rdf:type owl:Restriction ;
                                owl:onProperty :StartupModel_StartMainFuelCurve ;
                                owl:qualifiedCardinality "1"^^xsd:nonNegativeInteger ;
                                owl:onClass :StartupModel
                              ] ,
                              [ rdf:type owl:Restriction ;
                                owl:onProperty :StartupModel_StartRampCurve ;
                                owl:qualifiedCardinality "1"^^xsd:nonNegativeInteger ;
                                owl:onClass :StartupModel
                              ] ,
                              [ rdf:type owl:Restriction ;
                                owl:onProperty :StartupModel_ThermalGeneratingUnit ;
                                owl:maxQualifiedCardinality "1"^^xsd:nonNegativeInteger ;
                                owl:onClass :StartupModel
                              ] ,
                              [ rdf:type owl:Restriction ;
                                owl:onProperty :StartupModel_fixedMaintCost ;
                                owl:maxQualifiedCardinality "1"^^xsd:nonNegativeInteger ;
                                owl:onClass <https://w3id.org/netbeheer/IECCIM/TC57CIM/IEC61970/Base/Domain#CostRate>
                              ] ,
                              [ rdf:type owl:Restriction ;
                                owl:onProperty :StartupModel_hotStandbyHeat ;
                                owl:maxQualifiedCardinality "1"^^xsd:nonNegativeInteger ;
                                owl:onClass :HeatRate
                              ] ,
                              [ rdf:type owl:Restriction ;
                                owl:onProperty :StartupModel_incrementalMaintCost ;
                                owl:maxQualifiedCardinality "1"^^xsd:nonNegativeInteger ;
                                owl:onClass <https://w3id.org/netbeheer/IECCIM/TC57CIM/IEC61970/Base/Domain#CostPerEnergyUnit>
                              ] ,
                              [ rdf:type owl:Restriction ;
                                owl:onProperty :StartupModel_minimumDownTime ;
                                owl:maxQualifiedCardinality "1"^^xsd:nonNegativeInteger ;
                                owl:onClass <https://w3id.org/netbeheer/IECCIM/TC57CIM/IEC61970/Base/Domain#Hours>
                              ] ,
                              [ rdf:type owl:Restriction ;
                                owl:onProperty :StartupModel_minimumRunTime ;
                                owl:maxQualifiedCardinality "1"^^xsd:nonNegativeInteger ;
                                owl:onClass <https://w3id.org/netbeheer/IECCIM/TC57CIM/IEC61970/Base/Domain#Hours>
                              ] ,
                              [ rdf:type owl:Restriction ;
                                owl:onProperty :StartupModel_riskFactorCost ;
                                owl:maxQualifiedCardinality "1"^^xsd:nonNegativeInteger ;
                                owl:onClass <https://w3id.org/netbeheer/IECCIM/TC57CIM/IEC61970/Base/Domain#Money>
                              ] ,
                              [ rdf:type owl:Restriction ;
                                owl:onProperty :StartupModel_startupCost ;
                                owl:maxQualifiedCardinality "1"^^xsd:nonNegativeInteger ;
                                owl:onClass <https://w3id.org/netbeheer/IECCIM/TC57CIM/IEC61970/Base/Domain#Money>
                              ] ,
                              [ rdf:type owl:Restriction ;
                                owl:onProperty :StartupModel_stbyAuxP ;
                                owl:maxQualifiedCardinality "1"^^xsd:nonNegativeInteger ;
                                owl:onClass <https://w3id.org/netbeheer/IECCIM/TC57CIM/IEC61970/Base/Domain#ActivePower>
                              ] ,
                              [ rdf:type owl:Restriction ;
                                owl:onProperty :StartupModel_startupDate ;
                                owl:minQualifiedCardinality "0"^^xsd:nonNegativeInteger ;
                                owl:onDataRange xsd:dateTime
                              ] ,
                              [ rdf:type owl:Restriction ;
                                owl:onProperty :StartupModel_startupPriority ;
                                owl:minQualifiedCardinality "0"^^xsd:nonNegativeInteger ;
                                owl:onDataRange xsd:nonNegativeInteger
                              ] ,
                              [ rdf:type owl:Restriction ;
                                owl:onProperty :StartupModel_startupDate ;
                                owl:maxQualifiedCardinality "1"^^xsd:nonNegativeInteger ;
                                owl:onDataRange xsd:dateTime
                              ] ,
                              [ rdf:type owl:Restriction ;
                                owl:onProperty :StartupModel_startupPriority ;
                                owl:maxQualifiedCardinality "1"^^xsd:nonNegativeInteger ;
                                owl:onDataRange xsd:nonNegativeInteger
                              ] ;
              rdfs:comment """Unit start up characteristics depending on how long the unit has been off line.
""" .


###  https://w3id.org/netbeheer/IECCIM/TC57CIM/IEC61970/Base/Generation/Production#SteamSendoutSchedule
:SteamSendoutSchedule rdf:type owl:Class ;
                      rdfs:subClassOf <https://w3id.org/netbeheer/IECCIM/TC57CIM/IEC61970/Base/Core#RegularIntervalSchedule> ,
                                      [ rdf:type owl:Restriction ;
                                        owl:onProperty :SteamSendoutSchedule_CogenerationPlant ;
                                        owl:qualifiedCardinality "1"^^xsd:nonNegativeInteger ;
                                        owl:onClass :SteamSendoutSchedule
                                      ] ;
                      rdfs:comment "The cogeneration plant's steam sendout schedule in volume per time unit." .


###  https://w3id.org/netbeheer/IECCIM/TC57CIM/IEC61970/Base/Generation/Production#TailbayLossCurve
:TailbayLossCurve rdf:type owl:Class ;
                  rdfs:subClassOf <https://w3id.org/netbeheer/IECCIM/TC57CIM/IEC61970/Base/Core#Curve> ,
                                  [ rdf:type owl:Restriction ;
                                    owl:onProperty :TailbayLossCurve_HydroGeneratingUnit ;
                                    owl:minQualifiedCardinality "0"^^xsd:nonNegativeInteger ;
                                    owl:onClass :TailbayLossCurve
                                  ] ;
                  rdfs:comment """Relationship between tailbay head loss hight (y-axis) and the total discharge into the power station's tailbay volume per time unit (x-axis) . There could be more than one curve depending on the level of the tailbay reservoir or river level.
""" .


###  https://w3id.org/netbeheer/IECCIM/TC57CIM/IEC61970/Base/Generation/Production#TargetLevelSchedule
:TargetLevelSchedule rdf:type owl:Class ;
                     rdfs:subClassOf <https://w3id.org/netbeheer/IECCIM/TC57CIM/IEC61970/Base/Core#Curve> ,
                                     [ rdf:type owl:Restriction ;
                                       owl:onProperty :TargetLevelSchedule_Reservoir ;
                                       owl:minQualifiedCardinality "0"^^xsd:nonNegativeInteger ;
                                       owl:onClass :TargetLevelSchedule
                                     ] ,
                                     [ rdf:type owl:Restriction ;
                                       owl:onProperty :TargetLevelSchedule_highLevelLimit ;
                                       owl:minQualifiedCardinality "0"^^xsd:nonNegativeInteger ;
                                       owl:onClass <https://w3id.org/netbeheer/IECCIM/TC57CIM/IEC61970/Base/Domain#WaterLevel>
                                     ] ,
                                     [ rdf:type owl:Restriction ;
                                       owl:onProperty :TargetLevelSchedule_lowLevelLimit ;
                                       owl:minQualifiedCardinality "0"^^xsd:nonNegativeInteger ;
                                       owl:onClass <https://w3id.org/netbeheer/IECCIM/TC57CIM/IEC61970/Base/Domain#WaterLevel>
                                     ] ,
                                     [ rdf:type owl:Restriction ;
                                       owl:onProperty :TargetLevelSchedule_Reservoir ;
                                       owl:maxQualifiedCardinality "1"^^xsd:nonNegativeInteger ;
                                       owl:onClass :TargetLevelSchedule
                                     ] ,
                                     [ rdf:type owl:Restriction ;
                                       owl:onProperty :TargetLevelSchedule_highLevelLimit ;
                                       owl:maxQualifiedCardinality "1"^^xsd:nonNegativeInteger ;
                                       owl:onClass <https://w3id.org/netbeheer/IECCIM/TC57CIM/IEC61970/Base/Domain#WaterLevel>
                                     ] ,
                                     [ rdf:type owl:Restriction ;
                                       owl:onProperty :TargetLevelSchedule_lowLevelLimit ;
                                       owl:maxQualifiedCardinality "1"^^xsd:nonNegativeInteger ;
                                       owl:onClass <https://w3id.org/netbeheer/IECCIM/TC57CIM/IEC61970/Base/Domain#WaterLevel>
                                     ] ;
                     rdfs:comment """Reservoir water level targets from advanced studies or \"rule curves\". Typically in one hour increments for up to 10 days.
""" .


###  https://w3id.org/netbeheer/IECCIM/TC57CIM/IEC61970/Base/Generation/Production#ThermalGeneratingUnit
:ThermalGeneratingUnit rdf:type owl:Class ;
                       rdfs:subClassOf :GeneratingUnit ,
                                       [ rdf:type owl:Restriction ;
                                         owl:onProperty :ThermalGeneratingUnit_CAESPlant ;
                                         owl:minQualifiedCardinality "0"^^xsd:nonNegativeInteger ;
                                         owl:onClass :ThermalGeneratingUnit
                                       ] ,
                                       [ rdf:type owl:Restriction ;
                                         owl:onProperty :ThermalGeneratingUnit_CogenerationPlant ;
                                         owl:minQualifiedCardinality "0"^^xsd:nonNegativeInteger ;
                                         owl:onClass :ThermalGeneratingUnit
                                       ] ,
                                       [ rdf:type owl:Restriction ;
                                         owl:onProperty :ThermalGeneratingUnit_CombinedCyclePlant ;
                                         owl:minQualifiedCardinality "0"^^xsd:nonNegativeInteger ;
                                         owl:onClass :ThermalGeneratingUnit
                                       ] ,
                                       [ rdf:type owl:Restriction ;
                                         owl:onProperty :ThermalGeneratingUnit_oMCost ;
                                         owl:minQualifiedCardinality "0"^^xsd:nonNegativeInteger ;
                                         owl:onClass :CostPerHeatUnit
                                       ] ,
                                       [ rdf:type owl:Restriction ;
                                         owl:onProperty :ThermalGeneratingUnit_EmissionCurves ;
                                         owl:qualifiedCardinality "1"^^xsd:nonNegativeInteger ;
                                         owl:onClass :ThermalGeneratingUnit
                                       ] ,
                                       [ rdf:type owl:Restriction ;
                                         owl:onProperty :ThermalGeneratingUnit_EmmissionAccounts ;
                                         owl:qualifiedCardinality "1"^^xsd:nonNegativeInteger ;
                                         owl:onClass :ThermalGeneratingUnit
                                       ] ,
                                       [ rdf:type owl:Restriction ;
                                         owl:onProperty :ThermalGeneratingUnit_FossilFuels ;
                                         owl:qualifiedCardinality "1"^^xsd:nonNegativeInteger ;
                                         owl:onClass :ThermalGeneratingUnit
                                       ] ,
                                       [ rdf:type owl:Restriction ;
                                         owl:onProperty :ThermalGeneratingUnit_FuelAllocationSchedules ;
                                         owl:qualifiedCardinality "1"^^xsd:nonNegativeInteger ;
                                         owl:onClass :ThermalGeneratingUnit
                                       ] ,
                                       [ rdf:type owl:Restriction ;
                                         owl:onProperty :ThermalGeneratingUnit_HeatInputCurve ;
                                         owl:qualifiedCardinality "1"^^xsd:nonNegativeInteger ;
                                         owl:onClass :ThermalGeneratingUnit
                                       ] ,
                                       [ rdf:type owl:Restriction ;
                                         owl:onProperty :ThermalGeneratingUnit_HeatRateCurve ;
                                         owl:qualifiedCardinality "1"^^xsd:nonNegativeInteger ;
                                         owl:onClass :ThermalGeneratingUnit
                                       ] ,
                                       [ rdf:type owl:Restriction ;
                                         owl:onProperty :ThermalGeneratingUnit_IncrementalHeatRateCurve ;
                                         owl:qualifiedCardinality "1"^^xsd:nonNegativeInteger ;
                                         owl:onClass :ThermalGeneratingUnit
                                       ] ,
                                       [ rdf:type owl:Restriction ;
                                         owl:onProperty :ThermalGeneratingUnit_ShutdownCurve ;
                                         owl:qualifiedCardinality "1"^^xsd:nonNegativeInteger ;
                                         owl:onClass :ThermalGeneratingUnit
                                       ] ,
                                       [ rdf:type owl:Restriction ;
                                         owl:onProperty :ThermalGeneratingUnit_StartupModel ;
                                         owl:qualifiedCardinality "1"^^xsd:nonNegativeInteger ;
                                         owl:onClass :ThermalGeneratingUnit
                                       ] ,
                                       [ rdf:type owl:Restriction ;
                                         owl:onProperty :ThermalGeneratingUnit_CAESPlant ;
                                         owl:maxQualifiedCardinality "1"^^xsd:nonNegativeInteger ;
                                         owl:onClass :ThermalGeneratingUnit
                                       ] ,
                                       [ rdf:type owl:Restriction ;
                                         owl:onProperty :ThermalGeneratingUnit_oMCost ;
                                         owl:maxQualifiedCardinality "1"^^xsd:nonNegativeInteger ;
                                         owl:onClass :CostPerHeatUnit
                                       ] ;
                       rdfs:comment """A generating unit whose prime mover could be a steam turbine, combustion turbine, or diesel engine.
""" .


###  https://w3id.org/netbeheer/IECCIM/TC57CIM/IEC61970/Base/Generation/Production#WindGeneratingUnit
:WindGeneratingUnit rdf:type owl:Class ;
                    rdfs:subClassOf :GeneratingUnit ,
                                    [ rdf:type owl:Restriction ;
                                      owl:onProperty :WindGeneratingUnit_windGenUnitType ;
                                      owl:minQualifiedCardinality "0"^^xsd:nonNegativeInteger ;
                                      owl:onDataRange :WindGenUnitKind
                                    ] ,
                                    [ rdf:type owl:Restriction ;
                                      owl:onProperty :WindGeneratingUnit_windGenUnitType ;
                                      owl:maxQualifiedCardinality "1"^^xsd:nonNegativeInteger ;
                                      owl:onDataRange :WindGenUnitKind
                                    ] ;
                    rdfs:comment "A wind driven generating unit.  May be used to represent a single turbine or an aggregation.  " .


###  Generated by the OWL API (version 5.1.10.2019-03-12T22:31:15Z) https://github.com/owlcs/owlapi/
